<?xml version="1.0"?>


<!DOCTYPE rdf:RDF [
    <!ENTITY void "http://rdfs.org/ns/void#" >
    <!ENTITY dcterms "http://purl.org/dc/terms/" >
    <!ENTITY owl "http://www.w3.org/2002/07/owl#" >
    <!ENTITY dce "http://purl.org/dc/elements/1.1/" >
    <!ENTITY xsd "http://www.w3.org/2001/XMLSchema#" >
    <!ENTITY glview "http://schema.geolink.org/dev/view#" >
    <!ENTITY grg "http://www.isotc211.org/schemas/grg/" >
    <!ENTITY skos "http://www.w3.org/2004/02/skos/core#" >
    <!ENTITY rdfs "http://www.w3.org/2000/01/rdf-schema#" >
    <!ENTITY glvoc_l05 "http://schema.geolink.org/dev/voc/nvs/L05#" >
    <!ENTITY rdf "http://www.w3.org/1999/02/22-rdf-syntax-ns#" >
]>


<rdf:RDF xmlns="http://schema.geolink.org/dev/voc/nvs/L05#"
     xml:base="http://schema.geolink.org/dev/voc/nvs/L05"
     xmlns:void="http://rdfs.org/ns/void#"
     xmlns:rdf="http://www.w3.org/1999/02/22-rdf-syntax-ns#"
     xmlns:owl="http://www.w3.org/2002/07/owl#"
     xmlns:glview="http://schema.geolink.org/dev/view#"
     xmlns:dce="http://purl.org/dc/elements/1.1/"
     xmlns:glvoc_l05="http://schema.geolink.org/dev/voc/nvs/L05#"
     xmlns:xsd="http://www.w3.org/2001/XMLSchema#"
     xmlns:dcterms="http://purl.org/dc/terms/"
     xmlns:skos="http://www.w3.org/2004/02/skos/core#"
     xmlns:rdfs="http://www.w3.org/2000/01/rdf-schema#"
     xmlns:grg="http://www.isotc211.org/schemas/grg/">
    <owl:Ontology rdf:about="http://schema.geolink.org/dev/voc/nvs/L05">
        <rdfs:label>SeaDataNet device categories</rdfs:label>
        <dcterms:date>2015-02-12 02:00:03.0</dcterms:date>
        <owl:versionInfo>49</owl:versionInfo>
        <rdfs:comment xml:lang="en">This ontology captures instrument types from SeaDataNet device categories as hosted in the NERC vocabulary server</rdfs:comment>
        <owl:imports rdf:resource="http://schema.geolink.org/dev/voc/nvs/L05hierarchy"/>
        <rdfs:seeAlso rdf:resource="http://vocab.nerc.ac.uk/collection/L05/"/>
    </owl:Ontology>
    


    <!-- 
    ///////////////////////////////////////////////////////////////////////////////////////
    //
    // Object Properties
    //
    ///////////////////////////////////////////////////////////////////////////////////////
     -->

    


    <!-- http://schema.geolink.org/dev/view#hasInstrumentType -->

    <owl:ObjectProperty rdf:about="&glview;hasInstrumentType"/>
    


    <!-- 
    ///////////////////////////////////////////////////////////////////////////////////////
    //
    // Classes
    //
    ///////////////////////////////////////////////////////////////////////////////////////
     -->

    


    <!-- http://schema.geolink.org/dev/view#Instrument -->

    <owl:Class rdf:about="&glview;Instrument"/>
    


    <!-- http://schema.geolink.org/dev/view#InstrumentType -->

    <owl:Class rdf:about="&glview;InstrumentType"/>
    


    <!-- http://schema.geolink.org/dev/voc/nvs/L05#AQPL -->

    <owl:Class rdf:about="&glvoc_l05;AQPL">
        <owl:equivalentClass>
            <owl:Restriction>
                <owl:onProperty rdf:resource="&glview;hasInstrumentType"/>
                <owl:hasValue rdf:resource="&glvoc_l05;AQPL"/>
            </owl:Restriction>
        </owl:equivalentClass>
        <rdfs:subClassOf rdf:resource="&glview;Instrument"/>
    </owl:Class>
    


    <!-- http://schema.geolink.org/dev/voc/nvs/L05#ARAG -->

    <owl:Class rdf:about="&glvoc_l05;ARAG">
        <owl:equivalentClass>
            <owl:Restriction>
                <owl:onProperty rdf:resource="&glview;hasInstrumentType"/>
                <owl:hasValue rdf:resource="&glvoc_l05;ARAG"/>
            </owl:Restriction>
        </owl:equivalentClass>
        <rdfs:subClassOf rdf:resource="&glview;Instrument"/>
    </owl:Class>
    


    <!-- http://schema.geolink.org/dev/voc/nvs/L05#ATRANS -->

    <owl:Class rdf:about="&glvoc_l05;ATRANS">
        <owl:equivalentClass>
            <owl:Restriction>
                <owl:onProperty rdf:resource="&glview;hasInstrumentType"/>
                <owl:hasValue rdf:resource="&glvoc_l05;ATRANS"/>
            </owl:Restriction>
        </owl:equivalentClass>
        <rdfs:subClassOf rdf:resource="&glview;Instrument"/>
    </owl:Class>
    


    <!-- http://schema.geolink.org/dev/voc/nvs/L05#BLUMS -->

    <owl:Class rdf:about="&glvoc_l05;BLUMS">
        <owl:equivalentClass>
            <owl:Restriction>
                <owl:onProperty rdf:resource="&glview;hasInstrumentType"/>
                <owl:hasValue rdf:resource="&glvoc_l05;BLUMS"/>
            </owl:Restriction>
        </owl:equivalentClass>
        <rdfs:subClassOf rdf:resource="&glview;Instrument"/>
    </owl:Class>
    


    <!-- http://schema.geolink.org/dev/voc/nvs/L05#BOMR -->

    <owl:Class rdf:about="&glvoc_l05;BOMR">
        <owl:equivalentClass>
            <owl:Restriction>
                <owl:onProperty rdf:resource="&glview;hasInstrumentType"/>
                <owl:hasValue rdf:resource="&glvoc_l05;BOMR"/>
            </owl:Restriction>
        </owl:equivalentClass>
        <rdfs:subClassOf rdf:resource="&glview;Instrument"/>
    </owl:Class>
    


    <!-- http://schema.geolink.org/dev/voc/nvs/L05#CCOV -->

    <owl:Class rdf:about="&glvoc_l05;CCOV">
        <owl:equivalentClass>
            <owl:Restriction>
                <owl:onProperty rdf:resource="&glview;hasInstrumentType"/>
                <owl:hasValue rdf:resource="&glvoc_l05;CCOV"/>
            </owl:Restriction>
        </owl:equivalentClass>
        <rdfs:subClassOf rdf:resource="&glview;Instrument"/>
    </owl:Class>
    


    <!-- http://schema.geolink.org/dev/voc/nvs/L05#CHRP -->

    <owl:Class rdf:about="&glvoc_l05;CHRP">
        <owl:equivalentClass>
            <owl:Restriction>
                <owl:onProperty rdf:resource="&glview;hasInstrumentType"/>
                <owl:hasValue rdf:resource="&glvoc_l05;CHRP"/>
            </owl:Restriction>
        </owl:equivalentClass>
        <rdfs:subClassOf rdf:resource="&glview;Instrument"/>
    </owl:Class>
    


    <!-- http://schema.geolink.org/dev/voc/nvs/L05#COLCMP -->

    <owl:Class rdf:about="&glvoc_l05;COLCMP">
        <owl:equivalentClass>
            <owl:Restriction>
                <owl:onProperty rdf:resource="&glview;hasInstrumentType"/>
                <owl:hasValue rdf:resource="&glvoc_l05;COLCMP"/>
            </owl:Restriction>
        </owl:equivalentClass>
        <rdfs:subClassOf rdf:resource="&glview;Instrument"/>
    </owl:Class>
    


    <!-- http://schema.geolink.org/dev/voc/nvs/L05#CSEM -->

    <owl:Class rdf:about="&glvoc_l05;CSEM">
        <owl:equivalentClass>
            <owl:Restriction>
                <owl:onProperty rdf:resource="&glview;hasInstrumentType"/>
                <owl:hasValue rdf:resource="&glvoc_l05;CSEM"/>
            </owl:Restriction>
        </owl:equivalentClass>
        <rdfs:subClassOf rdf:resource="&glview;Instrument"/>
    </owl:Class>
    


    <!-- http://schema.geolink.org/dev/voc/nvs/L05#EMSR -->

    <owl:Class rdf:about="&glvoc_l05;EMSR">
        <owl:equivalentClass>
            <owl:Restriction>
                <owl:onProperty rdf:resource="&glview;hasInstrumentType"/>
                <owl:hasValue rdf:resource="&glvoc_l05;EMSR"/>
            </owl:Restriction>
        </owl:equivalentClass>
        <rdfs:subClassOf rdf:resource="&glview;Instrument"/>
    </owl:Class>
    


    <!-- http://schema.geolink.org/dev/voc/nvs/L05#EQUIL -->

    <owl:Class rdf:about="&glvoc_l05;EQUIL">
        <owl:equivalentClass>
            <owl:Restriction>
                <owl:onProperty rdf:resource="&glview;hasInstrumentType"/>
                <owl:hasValue rdf:resource="&glvoc_l05;EQUIL"/>
            </owl:Restriction>
        </owl:equivalentClass>
        <rdfs:subClassOf rdf:resource="&glview;Instrument"/>
    </owl:Class>
    


    <!-- http://schema.geolink.org/dev/voc/nvs/L05#ERTQ -->

    <owl:Class rdf:about="&glvoc_l05;ERTQ">
        <owl:equivalentClass>
            <owl:Restriction>
                <owl:onProperty rdf:resource="&glview;hasInstrumentType"/>
                <owl:hasValue rdf:resource="&glvoc_l05;ERTQ"/>
            </owl:Restriction>
        </owl:equivalentClass>
        <rdfs:subClassOf rdf:resource="&glview;Instrument"/>
    </owl:Class>
    


    <!-- http://schema.geolink.org/dev/voc/nvs/L05#EXHL -->

    <owl:Class rdf:about="&glvoc_l05;EXHL">
        <owl:equivalentClass>
            <owl:Restriction>
                <owl:onProperty rdf:resource="&glview;hasInstrumentType"/>
                <owl:hasValue rdf:resource="&glvoc_l05;EXHL"/>
            </owl:Restriction>
        </owl:equivalentClass>
        <rdfs:subClassOf rdf:resource="&glview;Instrument"/>
    </owl:Class>
    


    <!-- http://schema.geolink.org/dev/voc/nvs/L05#EXLH -->

    <owl:Class rdf:about="&glvoc_l05;EXLH">
        <owl:equivalentClass>
            <owl:Restriction>
                <owl:onProperty rdf:resource="&glview;hasInstrumentType"/>
                <owl:hasValue rdf:resource="&glvoc_l05;EXLH"/>
            </owl:Restriction>
        </owl:equivalentClass>
        <rdfs:subClassOf rdf:resource="&glview;Instrument"/>
    </owl:Class>
    


    <!-- http://schema.geolink.org/dev/voc/nvs/L05#FFES -->

    <owl:Class rdf:about="&glvoc_l05;FFES">
        <owl:equivalentClass>
            <owl:Restriction>
                <owl:onProperty rdf:resource="&glview;hasInstrumentType"/>
                <owl:hasValue rdf:resource="&glvoc_l05;FFES"/>
            </owl:Restriction>
        </owl:equivalentClass>
        <rdfs:subClassOf rdf:resource="&glview;Instrument"/>
    </owl:Class>
    


    <!-- http://schema.geolink.org/dev/voc/nvs/L05#FLXS -->

    <owl:Class rdf:about="&glvoc_l05;FLXS">
        <owl:equivalentClass>
            <owl:Restriction>
                <owl:onProperty rdf:resource="&glview;hasInstrumentType"/>
                <owl:hasValue rdf:resource="&glvoc_l05;FLXS"/>
            </owl:Restriction>
        </owl:equivalentClass>
        <rdfs:subClassOf rdf:resource="&glview;Instrument"/>
    </owl:Class>
    


    <!-- http://schema.geolink.org/dev/voc/nvs/L05#FLXT -->

    <owl:Class rdf:about="&glvoc_l05;FLXT">
        <owl:equivalentClass>
            <owl:Restriction>
                <owl:onProperty rdf:resource="&glview;hasInstrumentType"/>
                <owl:hasValue rdf:resource="&glvoc_l05;FLXT"/>
            </owl:Restriction>
        </owl:equivalentClass>
        <rdfs:subClassOf rdf:resource="&glview;Instrument"/>
    </owl:Class>
    


    <!-- http://schema.geolink.org/dev/voc/nvs/L05#GIAG -->

    <owl:Class rdf:about="&glvoc_l05;GIAG">
        <owl:equivalentClass>
            <owl:Restriction>
                <owl:onProperty rdf:resource="&glview;hasInstrumentType"/>
                <owl:hasValue rdf:resource="&glvoc_l05;GIAG"/>
            </owl:Restriction>
        </owl:equivalentClass>
        <rdfs:subClassOf rdf:resource="&glview;Instrument"/>
    </owl:Class>
    


    <!-- http://schema.geolink.org/dev/voc/nvs/L05#ICEP -->

    <owl:Class rdf:about="&glvoc_l05;ICEP">
        <owl:equivalentClass>
            <owl:Restriction>
                <owl:onProperty rdf:resource="&glview;hasInstrumentType"/>
                <owl:hasValue rdf:resource="&glvoc_l05;ICEP"/>
            </owl:Restriction>
        </owl:equivalentClass>
        <rdfs:subClassOf rdf:resource="&glview;Instrument"/>
    </owl:Class>
    


    <!-- http://schema.geolink.org/dev/voc/nvs/L05#LAB01 -->

    <owl:Class rdf:about="&glvoc_l05;LAB01">
        <owl:equivalentClass>
            <owl:Restriction>
                <owl:onProperty rdf:resource="&glview;hasInstrumentType"/>
                <owl:hasValue rdf:resource="&glvoc_l05;LAB01"/>
            </owl:Restriction>
        </owl:equivalentClass>
        <rdfs:subClassOf rdf:resource="&glview;Instrument"/>
    </owl:Class>
    


    <!-- http://schema.geolink.org/dev/voc/nvs/L05#LAB02 -->

    <owl:Class rdf:about="&glvoc_l05;LAB02">
        <owl:equivalentClass>
            <owl:Restriction>
                <owl:onProperty rdf:resource="&glview;hasInstrumentType"/>
                <owl:hasValue rdf:resource="&glvoc_l05;LAB02"/>
            </owl:Restriction>
        </owl:equivalentClass>
        <rdfs:subClassOf rdf:resource="&glview;Instrument"/>
    </owl:Class>
    


    <!-- http://schema.geolink.org/dev/voc/nvs/L05#LAB03 -->

    <owl:Class rdf:about="&glvoc_l05;LAB03">
        <owl:equivalentClass>
            <owl:Restriction>
                <owl:onProperty rdf:resource="&glview;hasInstrumentType"/>
                <owl:hasValue rdf:resource="&glvoc_l05;LAB03"/>
            </owl:Restriction>
        </owl:equivalentClass>
        <rdfs:subClassOf rdf:resource="&glview;Instrument"/>
    </owl:Class>
    


    <!-- http://schema.geolink.org/dev/voc/nvs/L05#LAB04 -->

    <owl:Class rdf:about="&glvoc_l05;LAB04">
        <owl:equivalentClass>
            <owl:Restriction>
                <owl:onProperty rdf:resource="&glview;hasInstrumentType"/>
                <owl:hasValue rdf:resource="&glvoc_l05;LAB04"/>
            </owl:Restriction>
        </owl:equivalentClass>
        <rdfs:subClassOf rdf:resource="&glview;Instrument"/>
    </owl:Class>
    


    <!-- http://schema.geolink.org/dev/voc/nvs/L05#LAB05 -->

    <owl:Class rdf:about="&glvoc_l05;LAB05">
        <owl:equivalentClass>
            <owl:Restriction>
                <owl:onProperty rdf:resource="&glview;hasInstrumentType"/>
                <owl:hasValue rdf:resource="&glvoc_l05;LAB05"/>
            </owl:Restriction>
        </owl:equivalentClass>
        <rdfs:subClassOf rdf:resource="&glview;Instrument"/>
    </owl:Class>
    


    <!-- http://schema.geolink.org/dev/voc/nvs/L05#LAB06 -->

    <owl:Class rdf:about="&glvoc_l05;LAB06">
        <owl:equivalentClass>
            <owl:Restriction>
                <owl:onProperty rdf:resource="&glview;hasInstrumentType"/>
                <owl:hasValue rdf:resource="&glvoc_l05;LAB06"/>
            </owl:Restriction>
        </owl:equivalentClass>
        <rdfs:subClassOf rdf:resource="&glview;Instrument"/>
    </owl:Class>
    


    <!-- http://schema.geolink.org/dev/voc/nvs/L05#LAB07 -->

    <owl:Class rdf:about="&glvoc_l05;LAB07">
        <owl:equivalentClass>
            <owl:Restriction>
                <owl:onProperty rdf:resource="&glview;hasInstrumentType"/>
                <owl:hasValue rdf:resource="&glvoc_l05;LAB07"/>
            </owl:Restriction>
        </owl:equivalentClass>
        <rdfs:subClassOf rdf:resource="&glview;Instrument"/>
    </owl:Class>
    


    <!-- http://schema.geolink.org/dev/voc/nvs/L05#LAB08 -->

    <owl:Class rdf:about="&glvoc_l05;LAB08">
        <owl:equivalentClass>
            <owl:Restriction>
                <owl:onProperty rdf:resource="&glview;hasInstrumentType"/>
                <owl:hasValue rdf:resource="&glvoc_l05;LAB08"/>
            </owl:Restriction>
        </owl:equivalentClass>
        <rdfs:subClassOf rdf:resource="&glview;Instrument"/>
    </owl:Class>
    


    <!-- http://schema.geolink.org/dev/voc/nvs/L05#LAB09 -->

    <owl:Class rdf:about="&glvoc_l05;LAB09">
        <owl:equivalentClass>
            <owl:Restriction>
                <owl:onProperty rdf:resource="&glview;hasInstrumentType"/>
                <owl:hasValue rdf:resource="&glvoc_l05;LAB09"/>
            </owl:Restriction>
        </owl:equivalentClass>
        <rdfs:subClassOf rdf:resource="&glview;Instrument"/>
    </owl:Class>
    


    <!-- http://schema.geolink.org/dev/voc/nvs/L05#LAB10 -->

    <owl:Class rdf:about="&glvoc_l05;LAB10">
        <owl:equivalentClass>
            <owl:Restriction>
                <owl:onProperty rdf:resource="&glview;hasInstrumentType"/>
                <owl:hasValue rdf:resource="&glvoc_l05;LAB10"/>
            </owl:Restriction>
        </owl:equivalentClass>
        <rdfs:subClassOf rdf:resource="&glview;Instrument"/>
    </owl:Class>
    


    <!-- http://schema.geolink.org/dev/voc/nvs/L05#LAB11 -->

    <owl:Class rdf:about="&glvoc_l05;LAB11">
        <owl:equivalentClass>
            <owl:Restriction>
                <owl:onProperty rdf:resource="&glview;hasInstrumentType"/>
                <owl:hasValue rdf:resource="&glvoc_l05;LAB11"/>
            </owl:Restriction>
        </owl:equivalentClass>
        <rdfs:subClassOf rdf:resource="&glview;Instrument"/>
    </owl:Class>
    


    <!-- http://schema.geolink.org/dev/voc/nvs/L05#LAB12 -->

    <owl:Class rdf:about="&glvoc_l05;LAB12">
        <owl:equivalentClass>
            <owl:Restriction>
                <owl:onProperty rdf:resource="&glview;hasInstrumentType"/>
                <owl:hasValue rdf:resource="&glvoc_l05;LAB12"/>
            </owl:Restriction>
        </owl:equivalentClass>
        <rdfs:subClassOf rdf:resource="&glview;Instrument"/>
    </owl:Class>
    


    <!-- http://schema.geolink.org/dev/voc/nvs/L05#LAB13 -->

    <owl:Class rdf:about="&glvoc_l05;LAB13">
        <owl:equivalentClass>
            <owl:Restriction>
                <owl:onProperty rdf:resource="&glview;hasInstrumentType"/>
                <owl:hasValue rdf:resource="&glvoc_l05;LAB13"/>
            </owl:Restriction>
        </owl:equivalentClass>
        <rdfs:subClassOf rdf:resource="&glview;Instrument"/>
    </owl:Class>
    


    <!-- http://schema.geolink.org/dev/voc/nvs/L05#LAB14 -->

    <owl:Class rdf:about="&glvoc_l05;LAB14">
        <owl:equivalentClass>
            <owl:Restriction>
                <owl:onProperty rdf:resource="&glview;hasInstrumentType"/>
                <owl:hasValue rdf:resource="&glvoc_l05;LAB14"/>
            </owl:Restriction>
        </owl:equivalentClass>
        <rdfs:subClassOf rdf:resource="&glview;Instrument"/>
    </owl:Class>
    


    <!-- http://schema.geolink.org/dev/voc/nvs/L05#LAB15 -->

    <owl:Class rdf:about="&glvoc_l05;LAB15">
        <owl:equivalentClass>
            <owl:Restriction>
                <owl:onProperty rdf:resource="&glview;hasInstrumentType"/>
                <owl:hasValue rdf:resource="&glvoc_l05;LAB15"/>
            </owl:Restriction>
        </owl:equivalentClass>
        <rdfs:subClassOf rdf:resource="&glview;Instrument"/>
    </owl:Class>
    


    <!-- http://schema.geolink.org/dev/voc/nvs/L05#LAB16 -->

    <owl:Class rdf:about="&glvoc_l05;LAB16">
        <owl:equivalentClass>
            <owl:Restriction>
                <owl:onProperty rdf:resource="&glview;hasInstrumentType"/>
                <owl:hasValue rdf:resource="&glvoc_l05;LAB16"/>
            </owl:Restriction>
        </owl:equivalentClass>
        <rdfs:subClassOf rdf:resource="&glview;Instrument"/>
    </owl:Class>
    


    <!-- http://schema.geolink.org/dev/voc/nvs/L05#LAB17 -->

    <owl:Class rdf:about="&glvoc_l05;LAB17">
        <owl:equivalentClass>
            <owl:Restriction>
                <owl:onProperty rdf:resource="&glview;hasInstrumentType"/>
                <owl:hasValue rdf:resource="&glvoc_l05;LAB17"/>
            </owl:Restriction>
        </owl:equivalentClass>
        <rdfs:subClassOf rdf:resource="&glview;Instrument"/>
    </owl:Class>
    


    <!-- http://schema.geolink.org/dev/voc/nvs/L05#LAB18 -->

    <owl:Class rdf:about="&glvoc_l05;LAB18">
        <owl:equivalentClass>
            <owl:Restriction>
                <owl:onProperty rdf:resource="&glview;hasInstrumentType"/>
                <owl:hasValue rdf:resource="&glvoc_l05;LAB18"/>
            </owl:Restriction>
        </owl:equivalentClass>
        <rdfs:subClassOf rdf:resource="&glview;Instrument"/>
    </owl:Class>
    


    <!-- http://schema.geolink.org/dev/voc/nvs/L05#LAB19 -->

    <owl:Class rdf:about="&glvoc_l05;LAB19">
        <owl:equivalentClass>
            <owl:Restriction>
                <owl:onProperty rdf:resource="&glview;hasInstrumentType"/>
                <owl:hasValue rdf:resource="&glvoc_l05;LAB19"/>
            </owl:Restriction>
        </owl:equivalentClass>
        <rdfs:subClassOf rdf:resource="&glview;Instrument"/>
    </owl:Class>
    


    <!-- http://schema.geolink.org/dev/voc/nvs/L05#LAB20 -->

    <owl:Class rdf:about="&glvoc_l05;LAB20">
        <owl:equivalentClass>
            <owl:Restriction>
                <owl:onProperty rdf:resource="&glview;hasInstrumentType"/>
                <owl:hasValue rdf:resource="&glvoc_l05;LAB20"/>
            </owl:Restriction>
        </owl:equivalentClass>
        <rdfs:subClassOf rdf:resource="&glview;Instrument"/>
    </owl:Class>
    


    <!-- http://schema.geolink.org/dev/voc/nvs/L05#LAB21 -->

    <owl:Class rdf:about="&glvoc_l05;LAB21">
        <owl:equivalentClass>
            <owl:Restriction>
                <owl:onProperty rdf:resource="&glview;hasInstrumentType"/>
                <owl:hasValue rdf:resource="&glvoc_l05;LAB21"/>
            </owl:Restriction>
        </owl:equivalentClass>
        <rdfs:subClassOf rdf:resource="&glview;Instrument"/>
    </owl:Class>
    


    <!-- http://schema.geolink.org/dev/voc/nvs/L05#LAB22 -->

    <owl:Class rdf:about="&glvoc_l05;LAB22">
        <owl:equivalentClass>
            <owl:Restriction>
                <owl:onProperty rdf:resource="&glview;hasInstrumentType"/>
                <owl:hasValue rdf:resource="&glvoc_l05;LAB22"/>
            </owl:Restriction>
        </owl:equivalentClass>
        <rdfs:subClassOf rdf:resource="&glview;Instrument"/>
    </owl:Class>
    


    <!-- http://schema.geolink.org/dev/voc/nvs/L05#LAB23 -->

    <owl:Class rdf:about="&glvoc_l05;LAB23">
        <owl:equivalentClass>
            <owl:Restriction>
                <owl:onProperty rdf:resource="&glview;hasInstrumentType"/>
                <owl:hasValue rdf:resource="&glvoc_l05;LAB23"/>
            </owl:Restriction>
        </owl:equivalentClass>
        <rdfs:subClassOf rdf:resource="&glview;Instrument"/>
    </owl:Class>
    


    <!-- http://schema.geolink.org/dev/voc/nvs/L05#LAB24 -->

    <owl:Class rdf:about="&glvoc_l05;LAB24">
        <owl:equivalentClass>
            <owl:Restriction>
                <owl:onProperty rdf:resource="&glview;hasInstrumentType"/>
                <owl:hasValue rdf:resource="&glvoc_l05;LAB24"/>
            </owl:Restriction>
        </owl:equivalentClass>
        <rdfs:subClassOf rdf:resource="&glview;Instrument"/>
    </owl:Class>
    


    <!-- http://schema.geolink.org/dev/voc/nvs/L05#LAB25 -->

    <owl:Class rdf:about="&glvoc_l05;LAB25">
        <owl:equivalentClass>
            <owl:Restriction>
                <owl:onProperty rdf:resource="&glview;hasInstrumentType"/>
                <owl:hasValue rdf:resource="&glvoc_l05;LAB25"/>
            </owl:Restriction>
        </owl:equivalentClass>
        <rdfs:subClassOf rdf:resource="&glview;Instrument"/>
    </owl:Class>
    


    <!-- http://schema.geolink.org/dev/voc/nvs/L05#LAB26 -->

    <owl:Class rdf:about="&glvoc_l05;LAB26">
        <owl:equivalentClass>
            <owl:Restriction>
                <owl:onProperty rdf:resource="&glview;hasInstrumentType"/>
                <owl:hasValue rdf:resource="&glvoc_l05;LAB26"/>
            </owl:Restriction>
        </owl:equivalentClass>
        <rdfs:subClassOf rdf:resource="&glview;Instrument"/>
    </owl:Class>
    


    <!-- http://schema.geolink.org/dev/voc/nvs/L05#LAB27 -->

    <owl:Class rdf:about="&glvoc_l05;LAB27">
        <owl:equivalentClass>
            <owl:Restriction>
                <owl:onProperty rdf:resource="&glview;hasInstrumentType"/>
                <owl:hasValue rdf:resource="&glvoc_l05;LAB27"/>
            </owl:Restriction>
        </owl:equivalentClass>
        <rdfs:subClassOf rdf:resource="&glview;Instrument"/>
    </owl:Class>
    


    <!-- http://schema.geolink.org/dev/voc/nvs/L05#LAB28 -->

    <owl:Class rdf:about="&glvoc_l05;LAB28">
        <owl:equivalentClass>
            <owl:Restriction>
                <owl:onProperty rdf:resource="&glview;hasInstrumentType"/>
                <owl:hasValue rdf:resource="&glvoc_l05;LAB28"/>
            </owl:Restriction>
        </owl:equivalentClass>
        <rdfs:subClassOf rdf:resource="&glview;Instrument"/>
    </owl:Class>
    


    <!-- http://schema.geolink.org/dev/voc/nvs/L05#LAB29 -->

    <owl:Class rdf:about="&glvoc_l05;LAB29">
        <owl:equivalentClass>
            <owl:Restriction>
                <owl:onProperty rdf:resource="&glview;hasInstrumentType"/>
                <owl:hasValue rdf:resource="&glvoc_l05;LAB29"/>
            </owl:Restriction>
        </owl:equivalentClass>
        <rdfs:subClassOf rdf:resource="&glview;Instrument"/>
    </owl:Class>
    


    <!-- http://schema.geolink.org/dev/voc/nvs/L05#LAB30 -->

    <owl:Class rdf:about="&glvoc_l05;LAB30">
        <owl:equivalentClass>
            <owl:Restriction>
                <owl:onProperty rdf:resource="&glview;hasInstrumentType"/>
                <owl:hasValue rdf:resource="&glvoc_l05;LAB30"/>
            </owl:Restriction>
        </owl:equivalentClass>
        <rdfs:subClassOf rdf:resource="&glview;Instrument"/>
    </owl:Class>
    


    <!-- http://schema.geolink.org/dev/voc/nvs/L05#LAB31 -->

    <owl:Class rdf:about="&glvoc_l05;LAB31">
        <owl:equivalentClass>
            <owl:Restriction>
                <owl:onProperty rdf:resource="&glview;hasInstrumentType"/>
                <owl:hasValue rdf:resource="&glvoc_l05;LAB31"/>
            </owl:Restriction>
        </owl:equivalentClass>
        <rdfs:subClassOf rdf:resource="&glview;Instrument"/>
    </owl:Class>
    


    <!-- http://schema.geolink.org/dev/voc/nvs/L05#LAB32 -->

    <owl:Class rdf:about="&glvoc_l05;LAB32">
        <owl:equivalentClass>
            <owl:Restriction>
                <owl:onProperty rdf:resource="&glview;hasInstrumentType"/>
                <owl:hasValue rdf:resource="&glvoc_l05;LAB32"/>
            </owl:Restriction>
        </owl:equivalentClass>
        <rdfs:subClassOf rdf:resource="&glview;Instrument"/>
    </owl:Class>
    


    <!-- http://schema.geolink.org/dev/voc/nvs/L05#LAB33 -->

    <owl:Class rdf:about="&glvoc_l05;LAB33">
        <owl:equivalentClass>
            <owl:Restriction>
                <owl:onProperty rdf:resource="&glview;hasInstrumentType"/>
                <owl:hasValue rdf:resource="&glvoc_l05;LAB33"/>
            </owl:Restriction>
        </owl:equivalentClass>
        <rdfs:subClassOf rdf:resource="&glview;Instrument"/>
    </owl:Class>
    


    <!-- http://schema.geolink.org/dev/voc/nvs/L05#LAB34 -->

    <owl:Class rdf:about="&glvoc_l05;LAB34">
        <owl:equivalentClass>
            <owl:Restriction>
                <owl:onProperty rdf:resource="&glview;hasInstrumentType"/>
                <owl:hasValue rdf:resource="&glvoc_l05;LAB34"/>
            </owl:Restriction>
        </owl:equivalentClass>
        <rdfs:subClassOf rdf:resource="&glview;Instrument"/>
    </owl:Class>
    


    <!-- http://schema.geolink.org/dev/voc/nvs/L05#LAB35 -->

    <owl:Class rdf:about="&glvoc_l05;LAB35">
        <owl:equivalentClass>
            <owl:Restriction>
                <owl:onProperty rdf:resource="&glview;hasInstrumentType"/>
                <owl:hasValue rdf:resource="&glvoc_l05;LAB35"/>
            </owl:Restriction>
        </owl:equivalentClass>
        <rdfs:subClassOf rdf:resource="&glview;Instrument"/>
    </owl:Class>
    


    <!-- http://schema.geolink.org/dev/voc/nvs/L05#LAB36 -->

    <owl:Class rdf:about="&glvoc_l05;LAB36">
        <owl:equivalentClass>
            <owl:Restriction>
                <owl:onProperty rdf:resource="&glview;hasInstrumentType"/>
                <owl:hasValue rdf:resource="&glvoc_l05;LAB36"/>
            </owl:Restriction>
        </owl:equivalentClass>
        <rdfs:subClassOf rdf:resource="&glview;Instrument"/>
    </owl:Class>
    


    <!-- http://schema.geolink.org/dev/voc/nvs/L05#LAB37 -->

    <owl:Class rdf:about="&glvoc_l05;LAB37">
        <owl:equivalentClass>
            <owl:Restriction>
                <owl:onProperty rdf:resource="&glview;hasInstrumentType"/>
                <owl:hasValue rdf:resource="&glvoc_l05;LAB37"/>
            </owl:Restriction>
        </owl:equivalentClass>
        <rdfs:subClassOf rdf:resource="&glview;Instrument"/>
    </owl:Class>
    


    <!-- http://schema.geolink.org/dev/voc/nvs/L05#LAB38 -->

    <owl:Class rdf:about="&glvoc_l05;LAB38">
        <owl:equivalentClass>
            <owl:Restriction>
                <owl:onProperty rdf:resource="&glview;hasInstrumentType"/>
                <owl:hasValue rdf:resource="&glvoc_l05;LAB38"/>
            </owl:Restriction>
        </owl:equivalentClass>
        <rdfs:subClassOf rdf:resource="&glview;Instrument"/>
    </owl:Class>
    


    <!-- http://schema.geolink.org/dev/voc/nvs/L05#LAB39 -->

    <owl:Class rdf:about="&glvoc_l05;LAB39">
        <owl:equivalentClass>
            <owl:Restriction>
                <owl:onProperty rdf:resource="&glview;hasInstrumentType"/>
                <owl:hasValue rdf:resource="&glvoc_l05;LAB39"/>
            </owl:Restriction>
        </owl:equivalentClass>
        <rdfs:subClassOf rdf:resource="&glview;Instrument"/>
    </owl:Class>
    


    <!-- http://schema.geolink.org/dev/voc/nvs/L05#LAB40 -->

    <owl:Class rdf:about="&glvoc_l05;LAB40">
        <owl:equivalentClass>
            <owl:Restriction>
                <owl:onProperty rdf:resource="&glview;hasInstrumentType"/>
                <owl:hasValue rdf:resource="&glvoc_l05;LAB40"/>
            </owl:Restriction>
        </owl:equivalentClass>
        <rdfs:subClassOf rdf:resource="&glview;Instrument"/>
    </owl:Class>
    


    <!-- http://schema.geolink.org/dev/voc/nvs/L05#LAB41 -->

    <owl:Class rdf:about="&glvoc_l05;LAB41">
        <owl:equivalentClass>
            <owl:Restriction>
                <owl:onProperty rdf:resource="&glview;hasInstrumentType"/>
                <owl:hasValue rdf:resource="&glvoc_l05;LAB41"/>
            </owl:Restriction>
        </owl:equivalentClass>
        <rdfs:subClassOf rdf:resource="&glview;Instrument"/>
    </owl:Class>
    


    <!-- http://schema.geolink.org/dev/voc/nvs/L05#LAB42 -->

    <owl:Class rdf:about="&glvoc_l05;LAB42">
        <owl:equivalentClass>
            <owl:Restriction>
                <owl:onProperty rdf:resource="&glview;hasInstrumentType"/>
                <owl:hasValue rdf:resource="&glvoc_l05;LAB42"/>
            </owl:Restriction>
        </owl:equivalentClass>
        <rdfs:subClassOf rdf:resource="&glview;Instrument"/>
    </owl:Class>
    


    <!-- http://schema.geolink.org/dev/voc/nvs/L05#LAB43 -->

    <owl:Class rdf:about="&glvoc_l05;LAB43">
        <owl:equivalentClass>
            <owl:Restriction>
                <owl:onProperty rdf:resource="&glview;hasInstrumentType"/>
                <owl:hasValue rdf:resource="&glvoc_l05;LAB43"/>
            </owl:Restriction>
        </owl:equivalentClass>
        <rdfs:subClassOf rdf:resource="&glview;Instrument"/>
    </owl:Class>
    


    <!-- http://schema.geolink.org/dev/voc/nvs/L05#LAB44 -->

    <owl:Class rdf:about="&glvoc_l05;LAB44">
        <owl:equivalentClass>
            <owl:Restriction>
                <owl:onProperty rdf:resource="&glview;hasInstrumentType"/>
                <owl:hasValue rdf:resource="&glvoc_l05;LAB44"/>
            </owl:Restriction>
        </owl:equivalentClass>
        <rdfs:subClassOf rdf:resource="&glview;Instrument"/>
    </owl:Class>
    


    <!-- http://schema.geolink.org/dev/voc/nvs/L05#LBTG -->

    <owl:Class rdf:about="&glvoc_l05;LBTG">
        <owl:equivalentClass>
            <owl:Restriction>
                <owl:onProperty rdf:resource="&glview;hasInstrumentType"/>
                <owl:hasValue rdf:resource="&glvoc_l05;LBTG"/>
            </owl:Restriction>
        </owl:equivalentClass>
        <rdfs:subClassOf rdf:resource="&glview;Instrument"/>
    </owl:Class>
    


    <!-- http://schema.geolink.org/dev/voc/nvs/L05#MMIS -->

    <owl:Class rdf:about="&glvoc_l05;MMIS">
        <owl:equivalentClass>
            <owl:Restriction>
                <owl:onProperty rdf:resource="&glview;hasInstrumentType"/>
                <owl:hasValue rdf:resource="&glvoc_l05;MMIS"/>
            </owl:Restriction>
        </owl:equivalentClass>
        <rdfs:subClassOf rdf:resource="&glview;Instrument"/>
    </owl:Class>
    


    <!-- http://schema.geolink.org/dev/voc/nvs/L05#MOD01 -->

    <owl:Class rdf:about="&glvoc_l05;MOD01">
        <owl:equivalentClass>
            <owl:Restriction>
                <owl:onProperty rdf:resource="&glview;hasInstrumentType"/>
                <owl:hasValue rdf:resource="&glvoc_l05;MOD01"/>
            </owl:Restriction>
        </owl:equivalentClass>
        <rdfs:subClassOf rdf:resource="&glview;Instrument"/>
    </owl:Class>
    


    <!-- http://schema.geolink.org/dev/voc/nvs/L05#MOD02 -->

    <owl:Class rdf:about="&glvoc_l05;MOD02">
        <owl:equivalentClass>
            <owl:Restriction>
                <owl:onProperty rdf:resource="&glview;hasInstrumentType"/>
                <owl:hasValue rdf:resource="&glvoc_l05;MOD02"/>
            </owl:Restriction>
        </owl:equivalentClass>
        <rdfs:subClassOf rdf:resource="&glview;Instrument"/>
    </owl:Class>
    


    <!-- http://schema.geolink.org/dev/voc/nvs/L05#MOD03 -->

    <owl:Class rdf:about="&glvoc_l05;MOD03">
        <owl:equivalentClass>
            <owl:Restriction>
                <owl:onProperty rdf:resource="&glview;hasInstrumentType"/>
                <owl:hasValue rdf:resource="&glvoc_l05;MOD03"/>
            </owl:Restriction>
        </owl:equivalentClass>
        <rdfs:subClassOf rdf:resource="&glview;Instrument"/>
    </owl:Class>
    


    <!-- http://schema.geolink.org/dev/voc/nvs/L05#MOD04 -->

    <owl:Class rdf:about="&glvoc_l05;MOD04">
        <owl:equivalentClass>
            <owl:Restriction>
                <owl:onProperty rdf:resource="&glview;hasInstrumentType"/>
                <owl:hasValue rdf:resource="&glvoc_l05;MOD04"/>
            </owl:Restriction>
        </owl:equivalentClass>
        <rdfs:subClassOf rdf:resource="&glview;Instrument"/>
    </owl:Class>
    


    <!-- http://schema.geolink.org/dev/voc/nvs/L05#MOD05 -->

    <owl:Class rdf:about="&glvoc_l05;MOD05">
        <owl:equivalentClass>
            <owl:Restriction>
                <owl:onProperty rdf:resource="&glview;hasInstrumentType"/>
                <owl:hasValue rdf:resource="&glvoc_l05;MOD05"/>
            </owl:Restriction>
        </owl:equivalentClass>
        <rdfs:subClassOf rdf:resource="&glview;Instrument"/>
    </owl:Class>
    


    <!-- http://schema.geolink.org/dev/voc/nvs/L05#MOD06 -->

    <owl:Class rdf:about="&glvoc_l05;MOD06">
        <owl:equivalentClass>
            <owl:Restriction>
                <owl:onProperty rdf:resource="&glview;hasInstrumentType"/>
                <owl:hasValue rdf:resource="&glvoc_l05;MOD06"/>
            </owl:Restriction>
        </owl:equivalentClass>
        <rdfs:subClassOf rdf:resource="&glview;Instrument"/>
    </owl:Class>
    


    <!-- http://schema.geolink.org/dev/voc/nvs/L05#MOD07 -->

    <owl:Class rdf:about="&glvoc_l05;MOD07">
        <owl:equivalentClass>
            <owl:Restriction>
                <owl:onProperty rdf:resource="&glview;hasInstrumentType"/>
                <owl:hasValue rdf:resource="&glvoc_l05;MOD07"/>
            </owl:Restriction>
        </owl:equivalentClass>
        <rdfs:subClassOf rdf:resource="&glview;Instrument"/>
    </owl:Class>
    


    <!-- http://schema.geolink.org/dev/voc/nvs/L05#MOD08 -->

    <owl:Class rdf:about="&glvoc_l05;MOD08">
        <owl:equivalentClass>
            <owl:Restriction>
                <owl:onProperty rdf:resource="&glview;hasInstrumentType"/>
                <owl:hasValue rdf:resource="&glvoc_l05;MOD08"/>
            </owl:Restriction>
        </owl:equivalentClass>
        <rdfs:subClassOf rdf:resource="&glview;Instrument"/>
    </owl:Class>
    


    <!-- http://schema.geolink.org/dev/voc/nvs/L05#MVBR -->

    <owl:Class rdf:about="&glvoc_l05;MVBR">
        <owl:equivalentClass>
            <owl:Restriction>
                <owl:onProperty rdf:resource="&glview;hasInstrumentType"/>
                <owl:hasValue rdf:resource="&glvoc_l05;MVBR"/>
            </owl:Restriction>
        </owl:equivalentClass>
        <rdfs:subClassOf rdf:resource="&glview;Instrument"/>
    </owl:Class>
    


    <!-- http://schema.geolink.org/dev/voc/nvs/L05#NATS -->

    <owl:Class rdf:about="&glvoc_l05;NATS">
        <owl:equivalentClass>
            <owl:Restriction>
                <owl:onProperty rdf:resource="&glview;hasInstrumentType"/>
                <owl:hasValue rdf:resource="&glvoc_l05;NATS"/>
            </owl:Restriction>
        </owl:equivalentClass>
        <rdfs:subClassOf rdf:resource="&glview;Instrument"/>
    </owl:Class>
    


    <!-- http://schema.geolink.org/dev/voc/nvs/L05#PERMON -->

    <owl:Class rdf:about="&glvoc_l05;PERMON">
        <owl:equivalentClass>
            <owl:Restriction>
                <owl:onProperty rdf:resource="&glview;hasInstrumentType"/>
                <owl:hasValue rdf:resource="&glvoc_l05;PERMON"/>
            </owl:Restriction>
        </owl:equivalentClass>
        <rdfs:subClassOf rdf:resource="&glview;Instrument"/>
    </owl:Class>
    


    <!-- http://schema.geolink.org/dev/voc/nvs/L05#POS01 -->

    <owl:Class rdf:about="&glvoc_l05;POS01">
        <owl:equivalentClass>
            <owl:Restriction>
                <owl:onProperty rdf:resource="&glview;hasInstrumentType"/>
                <owl:hasValue rdf:resource="&glvoc_l05;POS01"/>
            </owl:Restriction>
        </owl:equivalentClass>
        <rdfs:subClassOf rdf:resource="&glview;Instrument"/>
    </owl:Class>
    


    <!-- http://schema.geolink.org/dev/voc/nvs/L05#POS02 -->

    <owl:Class rdf:about="&glvoc_l05;POS02">
        <owl:equivalentClass>
            <owl:Restriction>
                <owl:onProperty rdf:resource="&glview;hasInstrumentType"/>
                <owl:hasValue rdf:resource="&glvoc_l05;POS02"/>
            </owl:Restriction>
        </owl:equivalentClass>
        <rdfs:subClassOf rdf:resource="&glview;Instrument"/>
    </owl:Class>
    


    <!-- http://schema.geolink.org/dev/voc/nvs/L05#POS03 -->

    <owl:Class rdf:about="&glvoc_l05;POS03">
        <owl:equivalentClass>
            <owl:Restriction>
                <owl:onProperty rdf:resource="&glview;hasInstrumentType"/>
                <owl:hasValue rdf:resource="&glvoc_l05;POS03"/>
            </owl:Restriction>
        </owl:equivalentClass>
        <rdfs:subClassOf rdf:resource="&glview;Instrument"/>
    </owl:Class>
    


    <!-- http://schema.geolink.org/dev/voc/nvs/L05#POS04 -->

    <owl:Class rdf:about="&glvoc_l05;POS04">
        <owl:equivalentClass>
            <owl:Restriction>
                <owl:onProperty rdf:resource="&glview;hasInstrumentType"/>
                <owl:hasValue rdf:resource="&glvoc_l05;POS04"/>
            </owl:Restriction>
        </owl:equivalentClass>
        <rdfs:subClassOf rdf:resource="&glview;Instrument"/>
    </owl:Class>
    


    <!-- http://schema.geolink.org/dev/voc/nvs/L05#POS05 -->

    <owl:Class rdf:about="&glvoc_l05;POS05">
        <owl:equivalentClass>
            <owl:Restriction>
                <owl:onProperty rdf:resource="&glview;hasInstrumentType"/>
                <owl:hasValue rdf:resource="&glvoc_l05;POS05"/>
            </owl:Restriction>
        </owl:equivalentClass>
        <rdfs:subClassOf rdf:resource="&glview;Instrument"/>
    </owl:Class>
    


    <!-- http://schema.geolink.org/dev/voc/nvs/L05#POS06 -->

    <owl:Class rdf:about="&glvoc_l05;POS06">
        <owl:equivalentClass>
            <owl:Restriction>
                <owl:onProperty rdf:resource="&glview;hasInstrumentType"/>
                <owl:hasValue rdf:resource="&glvoc_l05;POS06"/>
            </owl:Restriction>
        </owl:equivalentClass>
        <rdfs:subClassOf rdf:resource="&glview;Instrument"/>
    </owl:Class>
    


    <!-- http://schema.geolink.org/dev/voc/nvs/L05#POS07 -->

    <owl:Class rdf:about="&glvoc_l05;POS07">
        <owl:equivalentClass>
            <owl:Restriction>
                <owl:onProperty rdf:resource="&glview;hasInstrumentType"/>
                <owl:hasValue rdf:resource="&glvoc_l05;POS07"/>
            </owl:Restriction>
        </owl:equivalentClass>
        <rdfs:subClassOf rdf:resource="&glview;Instrument"/>
    </owl:Class>
    


    <!-- http://schema.geolink.org/dev/voc/nvs/L05#POS08 -->

    <owl:Class rdf:about="&glvoc_l05;POS08">
        <owl:equivalentClass>
            <owl:Restriction>
                <owl:onProperty rdf:resource="&glview;hasInstrumentType"/>
                <owl:hasValue rdf:resource="&glvoc_l05;POS08"/>
            </owl:Restriction>
        </owl:equivalentClass>
        <rdfs:subClassOf rdf:resource="&glview;Instrument"/>
    </owl:Class>
    


    <!-- http://schema.geolink.org/dev/voc/nvs/L05#POS09 -->

    <owl:Class rdf:about="&glvoc_l05;POS09">
        <owl:equivalentClass>
            <owl:Restriction>
                <owl:onProperty rdf:resource="&glview;hasInstrumentType"/>
                <owl:hasValue rdf:resource="&glvoc_l05;POS09"/>
            </owl:Restriction>
        </owl:equivalentClass>
        <rdfs:subClassOf rdf:resource="&glview;Instrument"/>
    </owl:Class>
    


    <!-- http://schema.geolink.org/dev/voc/nvs/L05#POS10 -->

    <owl:Class rdf:about="&glvoc_l05;POS10">
        <owl:equivalentClass>
            <owl:Restriction>
                <owl:onProperty rdf:resource="&glview;hasInstrumentType"/>
                <owl:hasValue rdf:resource="&glvoc_l05;POS10"/>
            </owl:Restriction>
        </owl:equivalentClass>
        <rdfs:subClassOf rdf:resource="&glview;Instrument"/>
    </owl:Class>
    


    <!-- http://schema.geolink.org/dev/voc/nvs/L05#POS11 -->

    <owl:Class rdf:about="&glvoc_l05;POS11">
        <owl:equivalentClass>
            <owl:Restriction>
                <owl:onProperty rdf:resource="&glview;hasInstrumentType"/>
                <owl:hasValue rdf:resource="&glvoc_l05;POS11"/>
            </owl:Restriction>
        </owl:equivalentClass>
        <rdfs:subClassOf rdf:resource="&glview;Instrument"/>
    </owl:Class>
    


    <!-- http://schema.geolink.org/dev/voc/nvs/L05#POS12 -->

    <owl:Class rdf:about="&glvoc_l05;POS12">
        <owl:equivalentClass>
            <owl:Restriction>
                <owl:onProperty rdf:resource="&glview;hasInstrumentType"/>
                <owl:hasValue rdf:resource="&glvoc_l05;POS12"/>
            </owl:Restriction>
        </owl:equivalentClass>
        <rdfs:subClassOf rdf:resource="&glview;Instrument"/>
    </owl:Class>
    


    <!-- http://schema.geolink.org/dev/voc/nvs/L05#POS13 -->

    <owl:Class rdf:about="&glvoc_l05;POS13">
        <owl:equivalentClass>
            <owl:Restriction>
                <owl:onProperty rdf:resource="&glview;hasInstrumentType"/>
                <owl:hasValue rdf:resource="&glvoc_l05;POS13"/>
            </owl:Restriction>
        </owl:equivalentClass>
        <rdfs:subClassOf rdf:resource="&glview;Instrument"/>
    </owl:Class>
    


    <!-- http://schema.geolink.org/dev/voc/nvs/L05#POS14 -->

    <owl:Class rdf:about="&glvoc_l05;POS14">
        <owl:equivalentClass>
            <owl:Restriction>
                <owl:onProperty rdf:resource="&glview;hasInstrumentType"/>
                <owl:hasValue rdf:resource="&glvoc_l05;POS14"/>
            </owl:Restriction>
        </owl:equivalentClass>
        <rdfs:subClassOf rdf:resource="&glview;Instrument"/>
    </owl:Class>
    


    <!-- http://schema.geolink.org/dev/voc/nvs/L05#POS15 -->

    <owl:Class rdf:about="&glvoc_l05;POS15">
        <owl:equivalentClass>
            <owl:Restriction>
                <owl:onProperty rdf:resource="&glview;hasInstrumentType"/>
                <owl:hasValue rdf:resource="&glvoc_l05;POS15"/>
            </owl:Restriction>
        </owl:equivalentClass>
        <rdfs:subClassOf rdf:resource="&glview;Instrument"/>
    </owl:Class>
    


    <!-- http://schema.geolink.org/dev/voc/nvs/L05#POS16 -->

    <owl:Class rdf:about="&glvoc_l05;POS16">
        <owl:equivalentClass>
            <owl:Restriction>
                <owl:onProperty rdf:resource="&glview;hasInstrumentType"/>
                <owl:hasValue rdf:resource="&glvoc_l05;POS16"/>
            </owl:Restriction>
        </owl:equivalentClass>
        <rdfs:subClassOf rdf:resource="&glview;Instrument"/>
    </owl:Class>
    


    <!-- http://schema.geolink.org/dev/voc/nvs/L05#POS17 -->

    <owl:Class rdf:about="&glvoc_l05;POS17">
        <owl:equivalentClass>
            <owl:Restriction>
                <owl:onProperty rdf:resource="&glview;hasInstrumentType"/>
                <owl:hasValue rdf:resource="&glvoc_l05;POS17"/>
            </owl:Restriction>
        </owl:equivalentClass>
        <rdfs:subClassOf rdf:resource="&glview;Instrument"/>
    </owl:Class>
    


    <!-- http://schema.geolink.org/dev/voc/nvs/L05#POS18 -->

    <owl:Class rdf:about="&glvoc_l05;POS18">
        <owl:equivalentClass>
            <owl:Restriction>
                <owl:onProperty rdf:resource="&glview;hasInstrumentType"/>
                <owl:hasValue rdf:resource="&glvoc_l05;POS18"/>
            </owl:Restriction>
        </owl:equivalentClass>
        <rdfs:subClassOf rdf:resource="&glview;Instrument"/>
    </owl:Class>
    


    <!-- http://schema.geolink.org/dev/voc/nvs/L05#POS19 -->

    <owl:Class rdf:about="&glvoc_l05;POS19">
        <owl:equivalentClass>
            <owl:Restriction>
                <owl:onProperty rdf:resource="&glview;hasInstrumentType"/>
                <owl:hasValue rdf:resource="&glvoc_l05;POS19"/>
            </owl:Restriction>
        </owl:equivalentClass>
        <rdfs:subClassOf rdf:resource="&glview;Instrument"/>
    </owl:Class>
    


    <!-- http://schema.geolink.org/dev/voc/nvs/L05#POS20 -->

    <owl:Class rdf:about="&glvoc_l05;POS20">
        <owl:equivalentClass>
            <owl:Restriction>
                <owl:onProperty rdf:resource="&glview;hasInstrumentType"/>
                <owl:hasValue rdf:resource="&glvoc_l05;POS20"/>
            </owl:Restriction>
        </owl:equivalentClass>
        <rdfs:subClassOf rdf:resource="&glview;Instrument"/>
    </owl:Class>
    


    <!-- http://schema.geolink.org/dev/voc/nvs/L05#POS21 -->

    <owl:Class rdf:about="&glvoc_l05;POS21">
        <owl:equivalentClass>
            <owl:Restriction>
                <owl:onProperty rdf:resource="&glview;hasInstrumentType"/>
                <owl:hasValue rdf:resource="&glvoc_l05;POS21"/>
            </owl:Restriction>
        </owl:equivalentClass>
        <rdfs:subClassOf rdf:resource="&glview;Instrument"/>
    </owl:Class>
    


    <!-- http://schema.geolink.org/dev/voc/nvs/L05#POS22 -->

    <owl:Class rdf:about="&glvoc_l05;POS22">
        <owl:equivalentClass>
            <owl:Restriction>
                <owl:onProperty rdf:resource="&glview;hasInstrumentType"/>
                <owl:hasValue rdf:resource="&glvoc_l05;POS22"/>
            </owl:Restriction>
        </owl:equivalentClass>
        <rdfs:subClassOf rdf:resource="&glview;Instrument"/>
    </owl:Class>
    


    <!-- http://schema.geolink.org/dev/voc/nvs/L05#POS23 -->

    <owl:Class rdf:about="&glvoc_l05;POS23">
        <owl:equivalentClass>
            <owl:Restriction>
                <owl:onProperty rdf:resource="&glview;hasInstrumentType"/>
                <owl:hasValue rdf:resource="&glvoc_l05;POS23"/>
            </owl:Restriction>
        </owl:equivalentClass>
        <rdfs:subClassOf rdf:resource="&glview;Instrument"/>
    </owl:Class>
    


    <!-- http://schema.geolink.org/dev/voc/nvs/L05#POS24 -->

    <owl:Class rdf:about="&glvoc_l05;POS24">
        <owl:equivalentClass>
            <owl:Restriction>
                <owl:onProperty rdf:resource="&glview;hasInstrumentType"/>
                <owl:hasValue rdf:resource="&glvoc_l05;POS24"/>
            </owl:Restriction>
        </owl:equivalentClass>
        <rdfs:subClassOf rdf:resource="&glview;Instrument"/>
    </owl:Class>
    


    <!-- http://schema.geolink.org/dev/voc/nvs/L05#POS25 -->

    <owl:Class rdf:about="&glvoc_l05;POS25">
        <owl:equivalentClass>
            <owl:Restriction>
                <owl:onProperty rdf:resource="&glview;hasInstrumentType"/>
                <owl:hasValue rdf:resource="&glvoc_l05;POS25"/>
            </owl:Restriction>
        </owl:equivalentClass>
        <rdfs:subClassOf rdf:resource="&glview;Instrument"/>
    </owl:Class>
    


    <!-- http://schema.geolink.org/dev/voc/nvs/L05#POS26 -->

    <owl:Class rdf:about="&glvoc_l05;POS26">
        <owl:equivalentClass>
            <owl:Restriction>
                <owl:onProperty rdf:resource="&glview;hasInstrumentType"/>
                <owl:hasValue rdf:resource="&glvoc_l05;POS26"/>
            </owl:Restriction>
        </owl:equivalentClass>
        <rdfs:subClassOf rdf:resource="&glview;Instrument"/>
    </owl:Class>
    


    <!-- http://schema.geolink.org/dev/voc/nvs/L05#SBAG -->

    <owl:Class rdf:about="&glvoc_l05;SBAG">
        <owl:equivalentClass>
            <owl:Restriction>
                <owl:onProperty rdf:resource="&glview;hasInstrumentType"/>
                <owl:hasValue rdf:resource="&glvoc_l05;SBAG"/>
            </owl:Restriction>
        </owl:equivalentClass>
        <rdfs:subClassOf rdf:resource="&glview;Instrument"/>
    </owl:Class>
    


    <!-- http://schema.geolink.org/dev/voc/nvs/L05#SNAG -->

    <owl:Class rdf:about="&glvoc_l05;SNAG">
        <owl:equivalentClass>
            <owl:Restriction>
                <owl:onProperty rdf:resource="&glview;hasInstrumentType"/>
                <owl:hasValue rdf:resource="&glvoc_l05;SNAG"/>
            </owl:Restriction>
        </owl:equivalentClass>
        <rdfs:subClassOf rdf:resource="&glview;Instrument"/>
    </owl:Class>
    


    <!-- http://schema.geolink.org/dev/voc/nvs/L05#SNWG -->

    <owl:Class rdf:about="&glvoc_l05;SNWG">
        <owl:equivalentClass>
            <owl:Restriction>
                <owl:onProperty rdf:resource="&glview;hasInstrumentType"/>
                <owl:hasValue rdf:resource="&glvoc_l05;SNWG"/>
            </owl:Restriction>
        </owl:equivalentClass>
        <rdfs:subClassOf rdf:resource="&glview;Instrument"/>
    </owl:Class>
    


    <!-- http://schema.geolink.org/dev/voc/nvs/L05#SPRK -->

    <owl:Class rdf:about="&glvoc_l05;SPRK">
        <owl:equivalentClass>
            <owl:Restriction>
                <owl:onProperty rdf:resource="&glview;hasInstrumentType"/>
                <owl:hasValue rdf:resource="&glvoc_l05;SPRK"/>
            </owl:Restriction>
        </owl:equivalentClass>
        <rdfs:subClassOf rdf:resource="&glview;Instrument"/>
    </owl:Class>
    


    <!-- http://schema.geolink.org/dev/voc/nvs/L05#TFSAMP -->

    <owl:Class rdf:about="&glvoc_l05;TFSAMP">
        <owl:equivalentClass>
            <owl:Restriction>
                <owl:onProperty rdf:resource="&glview;hasInstrumentType"/>
                <owl:hasValue rdf:resource="&glvoc_l05;TFSAMP"/>
            </owl:Restriction>
        </owl:equivalentClass>
        <rdfs:subClassOf rdf:resource="&glview;Instrument"/>
    </owl:Class>
    


    <!-- http://schema.geolink.org/dev/voc/nvs/L05#TRTG -->

    <owl:Class rdf:about="&glvoc_l05;TRTG">
        <owl:equivalentClass>
            <owl:Restriction>
                <owl:onProperty rdf:resource="&glview;hasInstrumentType"/>
                <owl:hasValue rdf:resource="&glvoc_l05;TRTG"/>
            </owl:Restriction>
        </owl:equivalentClass>
        <rdfs:subClassOf rdf:resource="&glview;Instrument"/>
    </owl:Class>
    


    <!-- http://schema.geolink.org/dev/voc/nvs/L05#VSHC -->

    <owl:Class rdf:about="&glvoc_l05;VSHC">
        <owl:equivalentClass>
            <owl:Restriction>
                <owl:onProperty rdf:resource="&glview;hasInstrumentType"/>
                <owl:hasValue rdf:resource="&glvoc_l05;VSHC"/>
            </owl:Restriction>
        </owl:equivalentClass>
        <rdfs:subClassOf rdf:resource="&glview;Instrument"/>
    </owl:Class>
    


    <!-- http://schema.geolink.org/dev/voc/nvs/L05#WPS -->

    <owl:Class rdf:about="&glvoc_l05;WPS">
        <owl:equivalentClass>
            <owl:Restriction>
                <owl:onProperty rdf:resource="&glview;hasInstrumentType"/>
                <owl:hasValue rdf:resource="&glvoc_l05;WPS"/>
            </owl:Restriction>
        </owl:equivalentClass>
        <rdfs:subClassOf rdf:resource="&glview;Instrument"/>
    </owl:Class>
    


    <!-- http://schema.geolink.org/dev/voc/nvs/L05#101 -->

    <owl:Class rdf:about="&glvoc_l05;101">
        <owl:equivalentClass>
            <owl:Restriction>
                <owl:onProperty rdf:resource="&glview;hasInstrumentType"/>
                <owl:hasValue rdf:resource="&glvoc_l05;101"/>
            </owl:Restriction>
        </owl:equivalentClass>
        <rdfs:subClassOf rdf:resource="&glview;Instrument"/>
    </owl:Class>
    


    <!-- http://schema.geolink.org/dev/voc/nvs/L05#102 -->

    <owl:Class rdf:about="&glvoc_l05;102">
        <owl:equivalentClass>
            <owl:Restriction>
                <owl:onProperty rdf:resource="&glview;hasInstrumentType"/>
                <owl:hasValue rdf:resource="&glvoc_l05;102"/>
            </owl:Restriction>
        </owl:equivalentClass>
        <rdfs:subClassOf rdf:resource="&glview;Instrument"/>
    </owl:Class>
    


    <!-- http://schema.geolink.org/dev/voc/nvs/L05#103 -->

    <owl:Class rdf:about="&glvoc_l05;103">
        <owl:equivalentClass>
            <owl:Restriction>
                <owl:onProperty rdf:resource="&glview;hasInstrumentType"/>
                <owl:hasValue rdf:resource="&glvoc_l05;103"/>
            </owl:Restriction>
        </owl:equivalentClass>
        <rdfs:subClassOf rdf:resource="&glview;Instrument"/>
    </owl:Class>
    


    <!-- http://schema.geolink.org/dev/voc/nvs/L05#11 -->

    <owl:Class rdf:about="&glvoc_l05;11">
        <owl:equivalentClass>
            <owl:Restriction>
                <owl:onProperty rdf:resource="&glview;hasInstrumentType"/>
                <owl:hasValue rdf:resource="&glvoc_l05;11"/>
            </owl:Restriction>
        </owl:equivalentClass>
        <rdfs:subClassOf rdf:resource="&glview;Instrument"/>
    </owl:Class>
    


    <!-- http://schema.geolink.org/dev/voc/nvs/L05#110 -->

    <owl:Class rdf:about="&glvoc_l05;110">
        <owl:equivalentClass>
            <owl:Restriction>
                <owl:onProperty rdf:resource="&glview;hasInstrumentType"/>
                <owl:hasValue rdf:resource="&glvoc_l05;110"/>
            </owl:Restriction>
        </owl:equivalentClass>
        <rdfs:subClassOf rdf:resource="&glview;Instrument"/>
    </owl:Class>
    


    <!-- http://schema.geolink.org/dev/voc/nvs/L05#111 -->

    <owl:Class rdf:about="&glvoc_l05;111">
        <owl:equivalentClass>
            <owl:Restriction>
                <owl:onProperty rdf:resource="&glview;hasInstrumentType"/>
                <owl:hasValue rdf:resource="&glvoc_l05;111"/>
            </owl:Restriction>
        </owl:equivalentClass>
        <rdfs:subClassOf rdf:resource="&glview;Instrument"/>
    </owl:Class>
    


    <!-- http://schema.geolink.org/dev/voc/nvs/L05#112 -->

    <owl:Class rdf:about="&glvoc_l05;112">
        <owl:equivalentClass>
            <owl:Restriction>
                <owl:onProperty rdf:resource="&glview;hasInstrumentType"/>
                <owl:hasValue rdf:resource="&glvoc_l05;112"/>
            </owl:Restriction>
        </owl:equivalentClass>
        <rdfs:subClassOf rdf:resource="&glview;Instrument"/>
    </owl:Class>
    


    <!-- http://schema.geolink.org/dev/voc/nvs/L05#113 -->

    <owl:Class rdf:about="&glvoc_l05;113">
        <owl:equivalentClass>
            <owl:Restriction>
                <owl:onProperty rdf:resource="&glview;hasInstrumentType"/>
                <owl:hasValue rdf:resource="&glvoc_l05;113"/>
            </owl:Restriction>
        </owl:equivalentClass>
        <rdfs:subClassOf rdf:resource="&glview;Instrument"/>
    </owl:Class>
    


    <!-- http://schema.geolink.org/dev/voc/nvs/L05#114 -->

    <owl:Class rdf:about="&glvoc_l05;114">
        <owl:equivalentClass>
            <owl:Restriction>
                <owl:onProperty rdf:resource="&glview;hasInstrumentType"/>
                <owl:hasValue rdf:resource="&glvoc_l05;114"/>
            </owl:Restriction>
        </owl:equivalentClass>
        <rdfs:subClassOf rdf:resource="&glview;Instrument"/>
    </owl:Class>
    


    <!-- http://schema.geolink.org/dev/voc/nvs/L05#115 -->

    <owl:Class rdf:about="&glvoc_l05;115">
        <owl:equivalentClass>
            <owl:Restriction>
                <owl:onProperty rdf:resource="&glview;hasInstrumentType"/>
                <owl:hasValue rdf:resource="&glvoc_l05;115"/>
            </owl:Restriction>
        </owl:equivalentClass>
        <rdfs:subClassOf rdf:resource="&glview;Instrument"/>
    </owl:Class>
    


    <!-- http://schema.geolink.org/dev/voc/nvs/L05#116 -->

    <owl:Class rdf:about="&glvoc_l05;116">
        <owl:equivalentClass>
            <owl:Restriction>
                <owl:onProperty rdf:resource="&glview;hasInstrumentType"/>
                <owl:hasValue rdf:resource="&glvoc_l05;116"/>
            </owl:Restriction>
        </owl:equivalentClass>
        <rdfs:subClassOf rdf:resource="&glview;Instrument"/>
    </owl:Class>
    


    <!-- http://schema.geolink.org/dev/voc/nvs/L05#12 -->

    <owl:Class rdf:about="&glvoc_l05;12">
        <owl:equivalentClass>
            <owl:Restriction>
                <owl:onProperty rdf:resource="&glview;hasInstrumentType"/>
                <owl:hasValue rdf:resource="&glvoc_l05;12"/>
            </owl:Restriction>
        </owl:equivalentClass>
        <rdfs:subClassOf rdf:resource="&glview;Instrument"/>
    </owl:Class>
    


    <!-- http://schema.geolink.org/dev/voc/nvs/L05#121 -->

    <owl:Class rdf:about="&glvoc_l05;121">
        <owl:equivalentClass>
            <owl:Restriction>
                <owl:onProperty rdf:resource="&glview;hasInstrumentType"/>
                <owl:hasValue rdf:resource="&glvoc_l05;121"/>
            </owl:Restriction>
        </owl:equivalentClass>
        <rdfs:subClassOf rdf:resource="&glview;Instrument"/>
    </owl:Class>
    


    <!-- http://schema.geolink.org/dev/voc/nvs/L05#122 -->

    <owl:Class rdf:about="&glvoc_l05;122">
        <owl:equivalentClass>
            <owl:Restriction>
                <owl:onProperty rdf:resource="&glview;hasInstrumentType"/>
                <owl:hasValue rdf:resource="&glvoc_l05;122"/>
            </owl:Restriction>
        </owl:equivalentClass>
        <rdfs:subClassOf rdf:resource="&glview;Instrument"/>
    </owl:Class>
    


    <!-- http://schema.geolink.org/dev/voc/nvs/L05#123 -->

    <owl:Class rdf:about="&glvoc_l05;123">
        <owl:equivalentClass>
            <owl:Restriction>
                <owl:onProperty rdf:resource="&glview;hasInstrumentType"/>
                <owl:hasValue rdf:resource="&glvoc_l05;123"/>
            </owl:Restriction>
        </owl:equivalentClass>
        <rdfs:subClassOf rdf:resource="&glview;Instrument"/>
    </owl:Class>
    


    <!-- http://schema.geolink.org/dev/voc/nvs/L05#124 -->

    <owl:Class rdf:about="&glvoc_l05;124">
        <owl:equivalentClass>
            <owl:Restriction>
                <owl:onProperty rdf:resource="&glview;hasInstrumentType"/>
                <owl:hasValue rdf:resource="&glvoc_l05;124"/>
            </owl:Restriction>
        </owl:equivalentClass>
        <rdfs:subClassOf rdf:resource="&glview;Instrument"/>
    </owl:Class>
    


    <!-- http://schema.geolink.org/dev/voc/nvs/L05#13 -->

    <owl:Class rdf:about="&glvoc_l05;13">
        <owl:equivalentClass>
            <owl:Restriction>
                <owl:onProperty rdf:resource="&glview;hasInstrumentType"/>
                <owl:hasValue rdf:resource="&glvoc_l05;13"/>
            </owl:Restriction>
        </owl:equivalentClass>
        <rdfs:subClassOf rdf:resource="&glview;Instrument"/>
    </owl:Class>
    


    <!-- http://schema.geolink.org/dev/voc/nvs/L05#130 -->

    <owl:Class rdf:about="&glvoc_l05;130">
        <owl:equivalentClass>
            <owl:Restriction>
                <owl:onProperty rdf:resource="&glview;hasInstrumentType"/>
                <owl:hasValue rdf:resource="&glvoc_l05;130"/>
            </owl:Restriction>
        </owl:equivalentClass>
        <rdfs:subClassOf rdf:resource="&glview;Instrument"/>
    </owl:Class>
    


    <!-- http://schema.geolink.org/dev/voc/nvs/L05#131 -->

    <owl:Class rdf:about="&glvoc_l05;131">
        <owl:equivalentClass>
            <owl:Restriction>
                <owl:onProperty rdf:resource="&glview;hasInstrumentType"/>
                <owl:hasValue rdf:resource="&glvoc_l05;131"/>
            </owl:Restriction>
        </owl:equivalentClass>
        <rdfs:subClassOf rdf:resource="&glview;Instrument"/>
    </owl:Class>
    


    <!-- http://schema.geolink.org/dev/voc/nvs/L05#132 -->

    <owl:Class rdf:about="&glvoc_l05;132">
        <owl:equivalentClass>
            <owl:Restriction>
                <owl:onProperty rdf:resource="&glview;hasInstrumentType"/>
                <owl:hasValue rdf:resource="&glvoc_l05;132"/>
            </owl:Restriction>
        </owl:equivalentClass>
        <rdfs:subClassOf rdf:resource="&glview;Instrument"/>
    </owl:Class>
    


    <!-- http://schema.geolink.org/dev/voc/nvs/L05#133 -->

    <owl:Class rdf:about="&glvoc_l05;133">
        <owl:equivalentClass>
            <owl:Restriction>
                <owl:onProperty rdf:resource="&glview;hasInstrumentType"/>
                <owl:hasValue rdf:resource="&glvoc_l05;133"/>
            </owl:Restriction>
        </owl:equivalentClass>
        <rdfs:subClassOf rdf:resource="&glview;Instrument"/>
    </owl:Class>
    


    <!-- http://schema.geolink.org/dev/voc/nvs/L05#134 -->

    <owl:Class rdf:about="&glvoc_l05;134">
        <owl:equivalentClass>
            <owl:Restriction>
                <owl:onProperty rdf:resource="&glview;hasInstrumentType"/>
                <owl:hasValue rdf:resource="&glvoc_l05;134"/>
            </owl:Restriction>
        </owl:equivalentClass>
        <rdfs:subClassOf rdf:resource="&glview;Instrument"/>
    </owl:Class>
    


    <!-- http://schema.geolink.org/dev/voc/nvs/L05#135 -->

    <owl:Class rdf:about="&glvoc_l05;135">
        <owl:equivalentClass>
            <owl:Restriction>
                <owl:onProperty rdf:resource="&glview;hasInstrumentType"/>
                <owl:hasValue rdf:resource="&glvoc_l05;135"/>
            </owl:Restriction>
        </owl:equivalentClass>
        <rdfs:subClassOf rdf:resource="&glview;Instrument"/>
    </owl:Class>
    


    <!-- http://schema.geolink.org/dev/voc/nvs/L05#14 -->

    <owl:Class rdf:about="&glvoc_l05;14">
        <owl:equivalentClass>
            <owl:Restriction>
                <owl:onProperty rdf:resource="&glview;hasInstrumentType"/>
                <owl:hasValue rdf:resource="&glvoc_l05;14"/>
            </owl:Restriction>
        </owl:equivalentClass>
        <rdfs:subClassOf rdf:resource="&glview;Instrument"/>
    </owl:Class>
    


    <!-- http://schema.geolink.org/dev/voc/nvs/L05#150 -->

    <owl:Class rdf:about="&glvoc_l05;150">
        <owl:equivalentClass>
            <owl:Restriction>
                <owl:onProperty rdf:resource="&glview;hasInstrumentType"/>
                <owl:hasValue rdf:resource="&glvoc_l05;150"/>
            </owl:Restriction>
        </owl:equivalentClass>
        <rdfs:subClassOf rdf:resource="&glview;Instrument"/>
    </owl:Class>
    


    <!-- http://schema.geolink.org/dev/voc/nvs/L05#151 -->

    <owl:Class rdf:about="&glvoc_l05;151">
        <owl:equivalentClass>
            <owl:Restriction>
                <owl:onProperty rdf:resource="&glview;hasInstrumentType"/>
                <owl:hasValue rdf:resource="&glvoc_l05;151"/>
            </owl:Restriction>
        </owl:equivalentClass>
        <rdfs:subClassOf rdf:resource="&glview;Instrument"/>
    </owl:Class>
    


    <!-- http://schema.geolink.org/dev/voc/nvs/L05#152 -->

    <owl:Class rdf:about="&glvoc_l05;152">
        <owl:equivalentClass>
            <owl:Restriction>
                <owl:onProperty rdf:resource="&glview;hasInstrumentType"/>
                <owl:hasValue rdf:resource="&glvoc_l05;152"/>
            </owl:Restriction>
        </owl:equivalentClass>
        <rdfs:subClassOf rdf:resource="&glview;Instrument"/>
    </owl:Class>
    


    <!-- http://schema.geolink.org/dev/voc/nvs/L05#153 -->

    <owl:Class rdf:about="&glvoc_l05;153">
        <owl:equivalentClass>
            <owl:Restriction>
                <owl:onProperty rdf:resource="&glview;hasInstrumentType"/>
                <owl:hasValue rdf:resource="&glvoc_l05;153"/>
            </owl:Restriction>
        </owl:equivalentClass>
        <rdfs:subClassOf rdf:resource="&glview;Instrument"/>
    </owl:Class>
    


    <!-- http://schema.geolink.org/dev/voc/nvs/L05#154 -->

    <owl:Class rdf:about="&glvoc_l05;154">
        <owl:equivalentClass>
            <owl:Restriction>
                <owl:onProperty rdf:resource="&glview;hasInstrumentType"/>
                <owl:hasValue rdf:resource="&glvoc_l05;154"/>
            </owl:Restriction>
        </owl:equivalentClass>
        <rdfs:subClassOf rdf:resource="&glview;Instrument"/>
    </owl:Class>
    


    <!-- http://schema.geolink.org/dev/voc/nvs/L05#155 -->

    <owl:Class rdf:about="&glvoc_l05;155">
        <owl:equivalentClass>
            <owl:Restriction>
                <owl:onProperty rdf:resource="&glview;hasInstrumentType"/>
                <owl:hasValue rdf:resource="&glvoc_l05;155"/>
            </owl:Restriction>
        </owl:equivalentClass>
        <rdfs:subClassOf rdf:resource="&glview;Instrument"/>
    </owl:Class>
    


    <!-- http://schema.geolink.org/dev/voc/nvs/L05#156 -->

    <owl:Class rdf:about="&glvoc_l05;156">
        <owl:equivalentClass>
            <owl:Restriction>
                <owl:onProperty rdf:resource="&glview;hasInstrumentType"/>
                <owl:hasValue rdf:resource="&glvoc_l05;156"/>
            </owl:Restriction>
        </owl:equivalentClass>
        <rdfs:subClassOf rdf:resource="&glview;Instrument"/>
    </owl:Class>
    


    <!-- http://schema.geolink.org/dev/voc/nvs/L05#157 -->

    <owl:Class rdf:about="&glvoc_l05;157">
        <owl:equivalentClass>
            <owl:Restriction>
                <owl:onProperty rdf:resource="&glview;hasInstrumentType"/>
                <owl:hasValue rdf:resource="&glvoc_l05;157"/>
            </owl:Restriction>
        </owl:equivalentClass>
        <rdfs:subClassOf rdf:resource="&glview;Instrument"/>
    </owl:Class>
    


    <!-- http://schema.geolink.org/dev/voc/nvs/L05#158 -->

    <owl:Class rdf:about="&glvoc_l05;158">
        <owl:equivalentClass>
            <owl:Restriction>
                <owl:onProperty rdf:resource="&glview;hasInstrumentType"/>
                <owl:hasValue rdf:resource="&glvoc_l05;158"/>
            </owl:Restriction>
        </owl:equivalentClass>
        <rdfs:subClassOf rdf:resource="&glview;Instrument"/>
    </owl:Class>
    


    <!-- http://schema.geolink.org/dev/voc/nvs/L05#159 -->

    <owl:Class rdf:about="&glvoc_l05;159">
        <owl:equivalentClass>
            <owl:Restriction>
                <owl:onProperty rdf:resource="&glview;hasInstrumentType"/>
                <owl:hasValue rdf:resource="&glvoc_l05;159"/>
            </owl:Restriction>
        </owl:equivalentClass>
        <rdfs:subClassOf rdf:resource="&glview;Instrument"/>
    </owl:Class>
    


    <!-- http://schema.geolink.org/dev/voc/nvs/L05#180 -->

    <owl:Class rdf:about="&glvoc_l05;180">
        <owl:equivalentClass>
            <owl:Restriction>
                <owl:onProperty rdf:resource="&glview;hasInstrumentType"/>
                <owl:hasValue rdf:resource="&glvoc_l05;180"/>
            </owl:Restriction>
        </owl:equivalentClass>
        <rdfs:subClassOf rdf:resource="&glview;Instrument"/>
    </owl:Class>
    


    <!-- http://schema.geolink.org/dev/voc/nvs/L05#181 -->

    <owl:Class rdf:about="&glvoc_l05;181">
        <owl:equivalentClass>
            <owl:Restriction>
                <owl:onProperty rdf:resource="&glview;hasInstrumentType"/>
                <owl:hasValue rdf:resource="&glvoc_l05;181"/>
            </owl:Restriction>
        </owl:equivalentClass>
        <rdfs:subClassOf rdf:resource="&glview;Instrument"/>
    </owl:Class>
    


    <!-- http://schema.geolink.org/dev/voc/nvs/L05#182 -->

    <owl:Class rdf:about="&glvoc_l05;182">
        <owl:equivalentClass>
            <owl:Restriction>
                <owl:onProperty rdf:resource="&glview;hasInstrumentType"/>
                <owl:hasValue rdf:resource="&glvoc_l05;182"/>
            </owl:Restriction>
        </owl:equivalentClass>
        <rdfs:subClassOf rdf:resource="&glview;Instrument"/>
    </owl:Class>
    


    <!-- http://schema.geolink.org/dev/voc/nvs/L05#183 -->

    <owl:Class rdf:about="&glvoc_l05;183">
        <owl:equivalentClass>
            <owl:Restriction>
                <owl:onProperty rdf:resource="&glview;hasInstrumentType"/>
                <owl:hasValue rdf:resource="&glvoc_l05;183"/>
            </owl:Restriction>
        </owl:equivalentClass>
        <rdfs:subClassOf rdf:resource="&glview;Instrument"/>
    </owl:Class>
    


    <!-- http://schema.geolink.org/dev/voc/nvs/L05#184 -->

    <owl:Class rdf:about="&glvoc_l05;184">
        <owl:equivalentClass>
            <owl:Restriction>
                <owl:onProperty rdf:resource="&glview;hasInstrumentType"/>
                <owl:hasValue rdf:resource="&glvoc_l05;184"/>
            </owl:Restriction>
        </owl:equivalentClass>
        <rdfs:subClassOf rdf:resource="&glview;Instrument"/>
    </owl:Class>
    


    <!-- http://schema.geolink.org/dev/voc/nvs/L05#185 -->

    <owl:Class rdf:about="&glvoc_l05;185">
        <owl:equivalentClass>
            <owl:Restriction>
                <owl:onProperty rdf:resource="&glview;hasInstrumentType"/>
                <owl:hasValue rdf:resource="&glvoc_l05;185"/>
            </owl:Restriction>
        </owl:equivalentClass>
        <rdfs:subClassOf rdf:resource="&glview;Instrument"/>
    </owl:Class>
    


    <!-- http://schema.geolink.org/dev/voc/nvs/L05#186 -->

    <owl:Class rdf:about="&glvoc_l05;186">
        <owl:equivalentClass>
            <owl:Restriction>
                <owl:onProperty rdf:resource="&glview;hasInstrumentType"/>
                <owl:hasValue rdf:resource="&glvoc_l05;186"/>
            </owl:Restriction>
        </owl:equivalentClass>
        <rdfs:subClassOf rdf:resource="&glview;Instrument"/>
    </owl:Class>
    


    <!-- http://schema.geolink.org/dev/voc/nvs/L05#21 -->

    <owl:Class rdf:about="&glvoc_l05;21">
        <owl:equivalentClass>
            <owl:Restriction>
                <owl:onProperty rdf:resource="&glview;hasInstrumentType"/>
                <owl:hasValue rdf:resource="&glvoc_l05;21"/>
            </owl:Restriction>
        </owl:equivalentClass>
        <rdfs:subClassOf rdf:resource="&glview;Instrument"/>
    </owl:Class>
    


    <!-- http://schema.geolink.org/dev/voc/nvs/L05#22 -->

    <owl:Class rdf:about="&glvoc_l05;22">
        <owl:equivalentClass>
            <owl:Restriction>
                <owl:onProperty rdf:resource="&glview;hasInstrumentType"/>
                <owl:hasValue rdf:resource="&glvoc_l05;22"/>
            </owl:Restriction>
        </owl:equivalentClass>
        <rdfs:subClassOf rdf:resource="&glview;Instrument"/>
    </owl:Class>
    


    <!-- http://schema.geolink.org/dev/voc/nvs/L05#23 -->

    <owl:Class rdf:about="&glvoc_l05;23">
        <owl:equivalentClass>
            <owl:Restriction>
                <owl:onProperty rdf:resource="&glview;hasInstrumentType"/>
                <owl:hasValue rdf:resource="&glvoc_l05;23"/>
            </owl:Restriction>
        </owl:equivalentClass>
        <rdfs:subClassOf rdf:resource="&glview;Instrument"/>
    </owl:Class>
    


    <!-- http://schema.geolink.org/dev/voc/nvs/L05#24 -->

    <owl:Class rdf:about="&glvoc_l05;24">
        <owl:equivalentClass>
            <owl:Restriction>
                <owl:onProperty rdf:resource="&glview;hasInstrumentType"/>
                <owl:hasValue rdf:resource="&glvoc_l05;24"/>
            </owl:Restriction>
        </owl:equivalentClass>
        <rdfs:subClassOf rdf:resource="&glview;Instrument"/>
    </owl:Class>
    


    <!-- http://schema.geolink.org/dev/voc/nvs/L05#30 -->

    <owl:Class rdf:about="&glvoc_l05;30">
        <owl:equivalentClass>
            <owl:Restriction>
                <owl:onProperty rdf:resource="&glview;hasInstrumentType"/>
                <owl:hasValue rdf:resource="&glvoc_l05;30"/>
            </owl:Restriction>
        </owl:equivalentClass>
        <rdfs:subClassOf rdf:resource="&glview;Instrument"/>
    </owl:Class>
    


    <!-- http://schema.geolink.org/dev/voc/nvs/L05#301 -->

    <owl:Class rdf:about="&glvoc_l05;301">
        <owl:equivalentClass>
            <owl:Restriction>
                <owl:onProperty rdf:resource="&glview;hasInstrumentType"/>
                <owl:hasValue rdf:resource="&glvoc_l05;301"/>
            </owl:Restriction>
        </owl:equivalentClass>
        <rdfs:subClassOf rdf:resource="&glview;Instrument"/>
    </owl:Class>
    


    <!-- http://schema.geolink.org/dev/voc/nvs/L05#302 -->

    <owl:Class rdf:about="&glvoc_l05;302">
        <owl:equivalentClass>
            <owl:Restriction>
                <owl:onProperty rdf:resource="&glview;hasInstrumentType"/>
                <owl:hasValue rdf:resource="&glvoc_l05;302"/>
            </owl:Restriction>
        </owl:equivalentClass>
        <rdfs:subClassOf rdf:resource="&glview;Instrument"/>
    </owl:Class>
    


    <!-- http://schema.geolink.org/dev/voc/nvs/L05#303 -->

    <owl:Class rdf:about="&glvoc_l05;303">
        <owl:equivalentClass>
            <owl:Restriction>
                <owl:onProperty rdf:resource="&glview;hasInstrumentType"/>
                <owl:hasValue rdf:resource="&glvoc_l05;303"/>
            </owl:Restriction>
        </owl:equivalentClass>
        <rdfs:subClassOf rdf:resource="&glview;Instrument"/>
    </owl:Class>
    


    <!-- http://schema.geolink.org/dev/voc/nvs/L05#304 -->

    <owl:Class rdf:about="&glvoc_l05;304">
        <owl:equivalentClass>
            <owl:Restriction>
                <owl:onProperty rdf:resource="&glview;hasInstrumentType"/>
                <owl:hasValue rdf:resource="&glvoc_l05;304"/>
            </owl:Restriction>
        </owl:equivalentClass>
        <rdfs:subClassOf rdf:resource="&glview;Instrument"/>
    </owl:Class>
    


    <!-- http://schema.geolink.org/dev/voc/nvs/L05#305 -->

    <owl:Class rdf:about="&glvoc_l05;305">
        <owl:equivalentClass>
            <owl:Restriction>
                <owl:onProperty rdf:resource="&glview;hasInstrumentType"/>
                <owl:hasValue rdf:resource="&glvoc_l05;305"/>
            </owl:Restriction>
        </owl:equivalentClass>
        <rdfs:subClassOf rdf:resource="&glview;Instrument"/>
    </owl:Class>
    


    <!-- http://schema.geolink.org/dev/voc/nvs/L05#306 -->

    <owl:Class rdf:about="&glvoc_l05;306">
        <owl:equivalentClass>
            <owl:Restriction>
                <owl:onProperty rdf:resource="&glview;hasInstrumentType"/>
                <owl:hasValue rdf:resource="&glvoc_l05;306"/>
            </owl:Restriction>
        </owl:equivalentClass>
        <rdfs:subClassOf rdf:resource="&glview;Instrument"/>
    </owl:Class>
    


    <!-- http://schema.geolink.org/dev/voc/nvs/L05#307 -->

    <owl:Class rdf:about="&glvoc_l05;307">
        <owl:equivalentClass>
            <owl:Restriction>
                <owl:onProperty rdf:resource="&glview;hasInstrumentType"/>
                <owl:hasValue rdf:resource="&glvoc_l05;307"/>
            </owl:Restriction>
        </owl:equivalentClass>
        <rdfs:subClassOf rdf:resource="&glview;Instrument"/>
    </owl:Class>
    


    <!-- http://schema.geolink.org/dev/voc/nvs/L05#308 -->

    <owl:Class rdf:about="&glvoc_l05;308">
        <owl:equivalentClass>
            <owl:Restriction>
                <owl:onProperty rdf:resource="&glview;hasInstrumentType"/>
                <owl:hasValue rdf:resource="&glvoc_l05;308"/>
            </owl:Restriction>
        </owl:equivalentClass>
        <rdfs:subClassOf rdf:resource="&glview;Instrument"/>
    </owl:Class>
    


    <!-- http://schema.geolink.org/dev/voc/nvs/L05#309 -->

    <owl:Class rdf:about="&glvoc_l05;309">
        <owl:equivalentClass>
            <owl:Restriction>
                <owl:onProperty rdf:resource="&glview;hasInstrumentType"/>
                <owl:hasValue rdf:resource="&glvoc_l05;309"/>
            </owl:Restriction>
        </owl:equivalentClass>
        <rdfs:subClassOf rdf:resource="&glview;Instrument"/>
    </owl:Class>
    


    <!-- http://schema.geolink.org/dev/voc/nvs/L05#31 -->

    <owl:Class rdf:about="&glvoc_l05;31">
        <owl:equivalentClass>
            <owl:Restriction>
                <owl:onProperty rdf:resource="&glview;hasInstrumentType"/>
                <owl:hasValue rdf:resource="&glvoc_l05;31"/>
            </owl:Restriction>
        </owl:equivalentClass>
        <rdfs:subClassOf rdf:resource="&glview;Instrument"/>
    </owl:Class>
    


    <!-- http://schema.geolink.org/dev/voc/nvs/L05#310 -->

    <owl:Class rdf:about="&glvoc_l05;310">
        <owl:equivalentClass>
            <owl:Restriction>
                <owl:onProperty rdf:resource="&glview;hasInstrumentType"/>
                <owl:hasValue rdf:resource="&glvoc_l05;310"/>
            </owl:Restriction>
        </owl:equivalentClass>
        <rdfs:subClassOf rdf:resource="&glview;Instrument"/>
    </owl:Class>
    


    <!-- http://schema.geolink.org/dev/voc/nvs/L05#311 -->

    <owl:Class rdf:about="&glvoc_l05;311">
        <owl:equivalentClass>
            <owl:Restriction>
                <owl:onProperty rdf:resource="&glview;hasInstrumentType"/>
                <owl:hasValue rdf:resource="&glvoc_l05;311"/>
            </owl:Restriction>
        </owl:equivalentClass>
        <rdfs:subClassOf rdf:resource="&glview;Instrument"/>
    </owl:Class>
    


    <!-- http://schema.geolink.org/dev/voc/nvs/L05#312 -->

    <owl:Class rdf:about="&glvoc_l05;312">
        <owl:equivalentClass>
            <owl:Restriction>
                <owl:onProperty rdf:resource="&glview;hasInstrumentType"/>
                <owl:hasValue rdf:resource="&glvoc_l05;312"/>
            </owl:Restriction>
        </owl:equivalentClass>
        <rdfs:subClassOf rdf:resource="&glview;Instrument"/>
    </owl:Class>
    


    <!-- http://schema.geolink.org/dev/voc/nvs/L05#313 -->

    <owl:Class rdf:about="&glvoc_l05;313">
        <owl:equivalentClass>
            <owl:Restriction>
                <owl:onProperty rdf:resource="&glview;hasInstrumentType"/>
                <owl:hasValue rdf:resource="&glvoc_l05;313"/>
            </owl:Restriction>
        </owl:equivalentClass>
        <rdfs:subClassOf rdf:resource="&glview;Instrument"/>
    </owl:Class>
    


    <!-- http://schema.geolink.org/dev/voc/nvs/L05#32 -->

    <owl:Class rdf:about="&glvoc_l05;32">
        <owl:equivalentClass>
            <owl:Restriction>
                <owl:onProperty rdf:resource="&glview;hasInstrumentType"/>
                <owl:hasValue rdf:resource="&glvoc_l05;32"/>
            </owl:Restriction>
        </owl:equivalentClass>
        <rdfs:subClassOf rdf:resource="&glview;Instrument"/>
    </owl:Class>
    


    <!-- http://schema.geolink.org/dev/voc/nvs/L05#33 -->

    <owl:Class rdf:about="&glvoc_l05;33">
        <owl:equivalentClass>
            <owl:Restriction>
                <owl:onProperty rdf:resource="&glview;hasInstrumentType"/>
                <owl:hasValue rdf:resource="&glvoc_l05;33"/>
            </owl:Restriction>
        </owl:equivalentClass>
        <rdfs:subClassOf rdf:resource="&glview;Instrument"/>
    </owl:Class>
    


    <!-- http://schema.geolink.org/dev/voc/nvs/L05#350 -->

    <owl:Class rdf:about="&glvoc_l05;350">
        <owl:equivalentClass>
            <owl:Restriction>
                <owl:onProperty rdf:resource="&glview;hasInstrumentType"/>
                <owl:hasValue rdf:resource="&glvoc_l05;350"/>
            </owl:Restriction>
        </owl:equivalentClass>
        <rdfs:subClassOf rdf:resource="&glview;Instrument"/>
    </owl:Class>
    


    <!-- http://schema.geolink.org/dev/voc/nvs/L05#351 -->

    <owl:Class rdf:about="&glvoc_l05;351">
        <owl:equivalentClass>
            <owl:Restriction>
                <owl:onProperty rdf:resource="&glview;hasInstrumentType"/>
                <owl:hasValue rdf:resource="&glvoc_l05;351"/>
            </owl:Restriction>
        </owl:equivalentClass>
        <rdfs:subClassOf rdf:resource="&glview;Instrument"/>
    </owl:Class>
    


    <!-- http://schema.geolink.org/dev/voc/nvs/L05#352 -->

    <owl:Class rdf:about="&glvoc_l05;352">
        <owl:equivalentClass>
            <owl:Restriction>
                <owl:onProperty rdf:resource="&glview;hasInstrumentType"/>
                <owl:hasValue rdf:resource="&glvoc_l05;352"/>
            </owl:Restriction>
        </owl:equivalentClass>
        <rdfs:subClassOf rdf:resource="&glview;Instrument"/>
    </owl:Class>
    


    <!-- http://schema.geolink.org/dev/voc/nvs/L05#353 -->

    <owl:Class rdf:about="&glvoc_l05;353">
        <owl:equivalentClass>
            <owl:Restriction>
                <owl:onProperty rdf:resource="&glview;hasInstrumentType"/>
                <owl:hasValue rdf:resource="&glvoc_l05;353"/>
            </owl:Restriction>
        </owl:equivalentClass>
        <rdfs:subClassOf rdf:resource="&glview;Instrument"/>
    </owl:Class>
    


    <!-- http://schema.geolink.org/dev/voc/nvs/L05#354 -->

    <owl:Class rdf:about="&glvoc_l05;354">
        <owl:equivalentClass>
            <owl:Restriction>
                <owl:onProperty rdf:resource="&glview;hasInstrumentType"/>
                <owl:hasValue rdf:resource="&glvoc_l05;354"/>
            </owl:Restriction>
        </owl:equivalentClass>
        <rdfs:subClassOf rdf:resource="&glview;Instrument"/>
    </owl:Class>
    


    <!-- http://schema.geolink.org/dev/voc/nvs/L05#355 -->

    <owl:Class rdf:about="&glvoc_l05;355">
        <owl:equivalentClass>
            <owl:Restriction>
                <owl:onProperty rdf:resource="&glview;hasInstrumentType"/>
                <owl:hasValue rdf:resource="&glvoc_l05;355"/>
            </owl:Restriction>
        </owl:equivalentClass>
        <rdfs:subClassOf rdf:resource="&glview;Instrument"/>
    </owl:Class>
    


    <!-- http://schema.geolink.org/dev/voc/nvs/L05#356 -->

    <owl:Class rdf:about="&glvoc_l05;356">
        <owl:equivalentClass>
            <owl:Restriction>
                <owl:onProperty rdf:resource="&glview;hasInstrumentType"/>
                <owl:hasValue rdf:resource="&glvoc_l05;356"/>
            </owl:Restriction>
        </owl:equivalentClass>
        <rdfs:subClassOf rdf:resource="&glview;Instrument"/>
    </owl:Class>
    


    <!-- http://schema.geolink.org/dev/voc/nvs/L05#357 -->

    <owl:Class rdf:about="&glvoc_l05;357">
        <owl:equivalentClass>
            <owl:Restriction>
                <owl:onProperty rdf:resource="&glview;hasInstrumentType"/>
                <owl:hasValue rdf:resource="&glvoc_l05;357"/>
            </owl:Restriction>
        </owl:equivalentClass>
        <rdfs:subClassOf rdf:resource="&glview;Instrument"/>
    </owl:Class>
    


    <!-- http://schema.geolink.org/dev/voc/nvs/L05#358 -->

    <owl:Class rdf:about="&glvoc_l05;358">
        <owl:equivalentClass>
            <owl:Restriction>
                <owl:onProperty rdf:resource="&glview;hasInstrumentType"/>
                <owl:hasValue rdf:resource="&glvoc_l05;358"/>
            </owl:Restriction>
        </owl:equivalentClass>
        <rdfs:subClassOf rdf:resource="&glview;Instrument"/>
    </owl:Class>
    


    <!-- http://schema.geolink.org/dev/voc/nvs/L05#359 -->

    <owl:Class rdf:about="&glvoc_l05;359">
        <owl:equivalentClass>
            <owl:Restriction>
                <owl:onProperty rdf:resource="&glview;hasInstrumentType"/>
                <owl:hasValue rdf:resource="&glvoc_l05;359"/>
            </owl:Restriction>
        </owl:equivalentClass>
        <rdfs:subClassOf rdf:resource="&glview;Instrument"/>
    </owl:Class>
    


    <!-- http://schema.geolink.org/dev/voc/nvs/L05#360 -->

    <owl:Class rdf:about="&glvoc_l05;360">
        <owl:equivalentClass>
            <owl:Restriction>
                <owl:onProperty rdf:resource="&glview;hasInstrumentType"/>
                <owl:hasValue rdf:resource="&glvoc_l05;360"/>
            </owl:Restriction>
        </owl:equivalentClass>
        <rdfs:subClassOf rdf:resource="&glview;Instrument"/>
    </owl:Class>
    


    <!-- http://schema.geolink.org/dev/voc/nvs/L05#361 -->

    <owl:Class rdf:about="&glvoc_l05;361">
        <owl:equivalentClass>
            <owl:Restriction>
                <owl:onProperty rdf:resource="&glview;hasInstrumentType"/>
                <owl:hasValue rdf:resource="&glvoc_l05;361"/>
            </owl:Restriction>
        </owl:equivalentClass>
        <rdfs:subClassOf rdf:resource="&glview;Instrument"/>
    </owl:Class>
    


    <!-- http://schema.geolink.org/dev/voc/nvs/L05#362 -->

    <owl:Class rdf:about="&glvoc_l05;362">
        <owl:equivalentClass>
            <owl:Restriction>
                <owl:onProperty rdf:resource="&glview;hasInstrumentType"/>
                <owl:hasValue rdf:resource="&glvoc_l05;362"/>
            </owl:Restriction>
        </owl:equivalentClass>
        <rdfs:subClassOf rdf:resource="&glview;Instrument"/>
    </owl:Class>
    


    <!-- http://schema.geolink.org/dev/voc/nvs/L05#363 -->

    <owl:Class rdf:about="&glvoc_l05;363">
        <owl:equivalentClass>
            <owl:Restriction>
                <owl:onProperty rdf:resource="&glview;hasInstrumentType"/>
                <owl:hasValue rdf:resource="&glvoc_l05;363"/>
            </owl:Restriction>
        </owl:equivalentClass>
        <rdfs:subClassOf rdf:resource="&glview;Instrument"/>
    </owl:Class>
    


    <!-- http://schema.geolink.org/dev/voc/nvs/L05#364 -->

    <owl:Class rdf:about="&glvoc_l05;364">
        <owl:equivalentClass>
            <owl:Restriction>
                <owl:onProperty rdf:resource="&glview;hasInstrumentType"/>
                <owl:hasValue rdf:resource="&glvoc_l05;364"/>
            </owl:Restriction>
        </owl:equivalentClass>
        <rdfs:subClassOf rdf:resource="&glview;Instrument"/>
    </owl:Class>
    


    <!-- http://schema.geolink.org/dev/voc/nvs/L05#365 -->

    <owl:Class rdf:about="&glvoc_l05;365">
        <owl:equivalentClass>
            <owl:Restriction>
                <owl:onProperty rdf:resource="&glview;hasInstrumentType"/>
                <owl:hasValue rdf:resource="&glvoc_l05;365"/>
            </owl:Restriction>
        </owl:equivalentClass>
        <rdfs:subClassOf rdf:resource="&glview;Instrument"/>
    </owl:Class>
    


    <!-- http://schema.geolink.org/dev/voc/nvs/L05#366 -->

    <owl:Class rdf:about="&glvoc_l05;366">
        <owl:equivalentClass>
            <owl:Restriction>
                <owl:onProperty rdf:resource="&glview;hasInstrumentType"/>
                <owl:hasValue rdf:resource="&glvoc_l05;366"/>
            </owl:Restriction>
        </owl:equivalentClass>
        <rdfs:subClassOf rdf:resource="&glview;Instrument"/>
    </owl:Class>
    


    <!-- http://schema.geolink.org/dev/voc/nvs/L05#367 -->

    <owl:Class rdf:about="&glvoc_l05;367">
        <owl:equivalentClass>
            <owl:Restriction>
                <owl:onProperty rdf:resource="&glview;hasInstrumentType"/>
                <owl:hasValue rdf:resource="&glvoc_l05;367"/>
            </owl:Restriction>
        </owl:equivalentClass>
        <rdfs:subClassOf rdf:resource="&glview;Instrument"/>
    </owl:Class>
    


    <!-- http://schema.geolink.org/dev/voc/nvs/L05#368 -->

    <owl:Class rdf:about="&glvoc_l05;368">
        <owl:equivalentClass>
            <owl:Restriction>
                <owl:onProperty rdf:resource="&glview;hasInstrumentType"/>
                <owl:hasValue rdf:resource="&glvoc_l05;368"/>
            </owl:Restriction>
        </owl:equivalentClass>
        <rdfs:subClassOf rdf:resource="&glview;Instrument"/>
    </owl:Class>
    


    <!-- http://schema.geolink.org/dev/voc/nvs/L05#369 -->

    <owl:Class rdf:about="&glvoc_l05;369">
        <owl:equivalentClass>
            <owl:Restriction>
                <owl:onProperty rdf:resource="&glview;hasInstrumentType"/>
                <owl:hasValue rdf:resource="&glvoc_l05;369"/>
            </owl:Restriction>
        </owl:equivalentClass>
        <rdfs:subClassOf rdf:resource="&glview;Instrument"/>
    </owl:Class>
    


    <!-- http://schema.geolink.org/dev/voc/nvs/L05#370 -->

    <owl:Class rdf:about="&glvoc_l05;370">
        <owl:equivalentClass>
            <owl:Restriction>
                <owl:onProperty rdf:resource="&glview;hasInstrumentType"/>
                <owl:hasValue rdf:resource="&glvoc_l05;370"/>
            </owl:Restriction>
        </owl:equivalentClass>
        <rdfs:subClassOf rdf:resource="&glview;Instrument"/>
    </owl:Class>
    


    <!-- http://schema.geolink.org/dev/voc/nvs/L05#371 -->

    <owl:Class rdf:about="&glvoc_l05;371">
        <owl:equivalentClass>
            <owl:Restriction>
                <owl:onProperty rdf:resource="&glview;hasInstrumentType"/>
                <owl:hasValue rdf:resource="&glvoc_l05;371"/>
            </owl:Restriction>
        </owl:equivalentClass>
        <rdfs:subClassOf rdf:resource="&glview;Instrument"/>
    </owl:Class>
    


    <!-- http://schema.geolink.org/dev/voc/nvs/L05#372 -->

    <owl:Class rdf:about="&glvoc_l05;372">
        <owl:equivalentClass>
            <owl:Restriction>
                <owl:onProperty rdf:resource="&glview;hasInstrumentType"/>
                <owl:hasValue rdf:resource="&glvoc_l05;372"/>
            </owl:Restriction>
        </owl:equivalentClass>
        <rdfs:subClassOf rdf:resource="&glview;Instrument"/>
    </owl:Class>
    


    <!-- http://schema.geolink.org/dev/voc/nvs/L05#373 -->

    <owl:Class rdf:about="&glvoc_l05;373">
        <owl:equivalentClass>
            <owl:Restriction>
                <owl:onProperty rdf:resource="&glview;hasInstrumentType"/>
                <owl:hasValue rdf:resource="&glvoc_l05;373"/>
            </owl:Restriction>
        </owl:equivalentClass>
        <rdfs:subClassOf rdf:resource="&glview;Instrument"/>
    </owl:Class>
    


    <!-- http://schema.geolink.org/dev/voc/nvs/L05#374 -->

    <owl:Class rdf:about="&glvoc_l05;374">
        <owl:equivalentClass>
            <owl:Restriction>
                <owl:onProperty rdf:resource="&glview;hasInstrumentType"/>
                <owl:hasValue rdf:resource="&glvoc_l05;374"/>
            </owl:Restriction>
        </owl:equivalentClass>
        <rdfs:subClassOf rdf:resource="&glview;Instrument"/>
    </owl:Class>
    


    <!-- http://schema.geolink.org/dev/voc/nvs/L05#375 -->

    <owl:Class rdf:about="&glvoc_l05;375">
        <owl:equivalentClass>
            <owl:Restriction>
                <owl:onProperty rdf:resource="&glview;hasInstrumentType"/>
                <owl:hasValue rdf:resource="&glvoc_l05;375"/>
            </owl:Restriction>
        </owl:equivalentClass>
        <rdfs:subClassOf rdf:resource="&glview;Instrument"/>
    </owl:Class>
    


    <!-- http://schema.geolink.org/dev/voc/nvs/L05#376 -->

    <owl:Class rdf:about="&glvoc_l05;376">
        <owl:equivalentClass>
            <owl:Restriction>
                <owl:onProperty rdf:resource="&glview;hasInstrumentType"/>
                <owl:hasValue rdf:resource="&glvoc_l05;376"/>
            </owl:Restriction>
        </owl:equivalentClass>
        <rdfs:subClassOf rdf:resource="&glview;Instrument"/>
    </owl:Class>
    


    <!-- http://schema.geolink.org/dev/voc/nvs/L05#377 -->

    <owl:Class rdf:about="&glvoc_l05;377">
        <owl:equivalentClass>
            <owl:Restriction>
                <owl:onProperty rdf:resource="&glview;hasInstrumentType"/>
                <owl:hasValue rdf:resource="&glvoc_l05;377"/>
            </owl:Restriction>
        </owl:equivalentClass>
        <rdfs:subClassOf rdf:resource="&glview;Instrument"/>
    </owl:Class>
    


    <!-- http://schema.geolink.org/dev/voc/nvs/L05#378 -->

    <owl:Class rdf:about="&glvoc_l05;378">
        <owl:equivalentClass>
            <owl:Restriction>
                <owl:onProperty rdf:resource="&glview;hasInstrumentType"/>
                <owl:hasValue rdf:resource="&glvoc_l05;378"/>
            </owl:Restriction>
        </owl:equivalentClass>
        <rdfs:subClassOf rdf:resource="&glview;Instrument"/>
    </owl:Class>
    


    <!-- http://schema.geolink.org/dev/voc/nvs/L05#379 -->

    <owl:Class rdf:about="&glvoc_l05;379">
        <owl:equivalentClass>
            <owl:Restriction>
                <owl:onProperty rdf:resource="&glview;hasInstrumentType"/>
                <owl:hasValue rdf:resource="&glvoc_l05;379"/>
            </owl:Restriction>
        </owl:equivalentClass>
        <rdfs:subClassOf rdf:resource="&glview;Instrument"/>
    </owl:Class>
    


    <!-- http://schema.geolink.org/dev/voc/nvs/L05#380 -->

    <owl:Class rdf:about="&glvoc_l05;380">
        <owl:equivalentClass>
            <owl:Restriction>
                <owl:onProperty rdf:resource="&glview;hasInstrumentType"/>
                <owl:hasValue rdf:resource="&glvoc_l05;380"/>
            </owl:Restriction>
        </owl:equivalentClass>
        <rdfs:subClassOf rdf:resource="&glview;Instrument"/>
    </owl:Class>
    


    <!-- http://schema.geolink.org/dev/voc/nvs/L05#381 -->

    <owl:Class rdf:about="&glvoc_l05;381">
        <owl:equivalentClass>
            <owl:Restriction>
                <owl:onProperty rdf:resource="&glview;hasInstrumentType"/>
                <owl:hasValue rdf:resource="&glvoc_l05;381"/>
            </owl:Restriction>
        </owl:equivalentClass>
        <rdfs:subClassOf rdf:resource="&glview;Instrument"/>
    </owl:Class>
    


    <!-- http://schema.geolink.org/dev/voc/nvs/L05#382 -->

    <owl:Class rdf:about="&glvoc_l05;382">
        <owl:equivalentClass>
            <owl:Restriction>
                <owl:onProperty rdf:resource="&glview;hasInstrumentType"/>
                <owl:hasValue rdf:resource="&glvoc_l05;382"/>
            </owl:Restriction>
        </owl:equivalentClass>
        <rdfs:subClassOf rdf:resource="&glview;Instrument"/>
    </owl:Class>
    


    <!-- http://schema.geolink.org/dev/voc/nvs/L05#383 -->

    <owl:Class rdf:about="&glvoc_l05;383">
        <owl:equivalentClass>
            <owl:Restriction>
                <owl:onProperty rdf:resource="&glview;hasInstrumentType"/>
                <owl:hasValue rdf:resource="&glvoc_l05;383"/>
            </owl:Restriction>
        </owl:equivalentClass>
        <rdfs:subClassOf rdf:resource="&glview;Instrument"/>
    </owl:Class>
    


    <!-- http://schema.geolink.org/dev/voc/nvs/L05#384 -->

    <owl:Class rdf:about="&glvoc_l05;384">
        <owl:equivalentClass>
            <owl:Restriction>
                <owl:onProperty rdf:resource="&glview;hasInstrumentType"/>
                <owl:hasValue rdf:resource="&glvoc_l05;384"/>
            </owl:Restriction>
        </owl:equivalentClass>
        <rdfs:subClassOf rdf:resource="&glview;Instrument"/>
    </owl:Class>
    


    <!-- http://schema.geolink.org/dev/voc/nvs/L05#385 -->

    <owl:Class rdf:about="&glvoc_l05;385">
        <owl:equivalentClass>
            <owl:Restriction>
                <owl:onProperty rdf:resource="&glview;hasInstrumentType"/>
                <owl:hasValue rdf:resource="&glvoc_l05;385"/>
            </owl:Restriction>
        </owl:equivalentClass>
        <rdfs:subClassOf rdf:resource="&glview;Instrument"/>
    </owl:Class>
    


    <!-- http://schema.geolink.org/dev/voc/nvs/L05#386 -->

    <owl:Class rdf:about="&glvoc_l05;386">
        <owl:equivalentClass>
            <owl:Restriction>
                <owl:onProperty rdf:resource="&glview;hasInstrumentType"/>
                <owl:hasValue rdf:resource="&glvoc_l05;386"/>
            </owl:Restriction>
        </owl:equivalentClass>
        <rdfs:subClassOf rdf:resource="&glview;Instrument"/>
    </owl:Class>
    


    <!-- http://schema.geolink.org/dev/voc/nvs/L05#387 -->

    <owl:Class rdf:about="&glvoc_l05;387">
        <owl:equivalentClass>
            <owl:Restriction>
                <owl:onProperty rdf:resource="&glview;hasInstrumentType"/>
                <owl:hasValue rdf:resource="&glvoc_l05;387"/>
            </owl:Restriction>
        </owl:equivalentClass>
        <rdfs:subClassOf rdf:resource="&glview;Instrument"/>
    </owl:Class>
    


    <!-- http://schema.geolink.org/dev/voc/nvs/L05#388 -->

    <owl:Class rdf:about="&glvoc_l05;388">
        <owl:equivalentClass>
            <owl:Restriction>
                <owl:onProperty rdf:resource="&glview;hasInstrumentType"/>
                <owl:hasValue rdf:resource="&glvoc_l05;388"/>
            </owl:Restriction>
        </owl:equivalentClass>
        <rdfs:subClassOf rdf:resource="&glview;Instrument"/>
    </owl:Class>
    


    <!-- http://schema.geolink.org/dev/voc/nvs/L05#50 -->

    <owl:Class rdf:about="&glvoc_l05;50">
        <owl:equivalentClass>
            <owl:Restriction>
                <owl:onProperty rdf:resource="&glview;hasInstrumentType"/>
                <owl:hasValue rdf:resource="&glvoc_l05;50"/>
            </owl:Restriction>
        </owl:equivalentClass>
        <rdfs:subClassOf rdf:resource="&glview;Instrument"/>
    </owl:Class>
    


    <!-- http://schema.geolink.org/dev/voc/nvs/L05#51 -->

    <owl:Class rdf:about="&glvoc_l05;51">
        <owl:equivalentClass>
            <owl:Restriction>
                <owl:onProperty rdf:resource="&glview;hasInstrumentType"/>
                <owl:hasValue rdf:resource="&glvoc_l05;51"/>
            </owl:Restriction>
        </owl:equivalentClass>
        <rdfs:subClassOf rdf:resource="&glview;Instrument"/>
    </owl:Class>
    


    <!-- http://schema.geolink.org/dev/voc/nvs/L05#52 -->

    <owl:Class rdf:about="&glvoc_l05;52">
        <owl:equivalentClass>
            <owl:Restriction>
                <owl:onProperty rdf:resource="&glview;hasInstrumentType"/>
                <owl:hasValue rdf:resource="&glvoc_l05;52"/>
            </owl:Restriction>
        </owl:equivalentClass>
        <rdfs:subClassOf rdf:resource="&glview;Instrument"/>
    </owl:Class>
    


    <!-- http://schema.geolink.org/dev/voc/nvs/L05#53 -->

    <owl:Class rdf:about="&glvoc_l05;53">
        <owl:equivalentClass>
            <owl:Restriction>
                <owl:onProperty rdf:resource="&glview;hasInstrumentType"/>
                <owl:hasValue rdf:resource="&glvoc_l05;53"/>
            </owl:Restriction>
        </owl:equivalentClass>
        <rdfs:subClassOf rdf:resource="&glview;Instrument"/>
    </owl:Class>
    


    <!-- http://schema.geolink.org/dev/voc/nvs/L05#54 -->

    <owl:Class rdf:about="&glvoc_l05;54">
        <owl:equivalentClass>
            <owl:Restriction>
                <owl:onProperty rdf:resource="&glview;hasInstrumentType"/>
                <owl:hasValue rdf:resource="&glvoc_l05;54"/>
            </owl:Restriction>
        </owl:equivalentClass>
        <rdfs:subClassOf rdf:resource="&glview;Instrument"/>
    </owl:Class>
    


    <!-- http://schema.geolink.org/dev/voc/nvs/L05#55 -->

    <owl:Class rdf:about="&glvoc_l05;55">
        <owl:equivalentClass>
            <owl:Restriction>
                <owl:onProperty rdf:resource="&glview;hasInstrumentType"/>
                <owl:hasValue rdf:resource="&glvoc_l05;55"/>
            </owl:Restriction>
        </owl:equivalentClass>
        <rdfs:subClassOf rdf:resource="&glview;Instrument"/>
    </owl:Class>
    


    <!-- http://schema.geolink.org/dev/voc/nvs/L05#56 -->

    <owl:Class rdf:about="&glvoc_l05;56">
        <owl:equivalentClass>
            <owl:Restriction>
                <owl:onProperty rdf:resource="&glview;hasInstrumentType"/>
                <owl:hasValue rdf:resource="&glvoc_l05;56"/>
            </owl:Restriction>
        </owl:equivalentClass>
        <rdfs:subClassOf rdf:resource="&glview;Instrument"/>
    </owl:Class>
    


    <!-- http://schema.geolink.org/dev/voc/nvs/L05#57 -->

    <owl:Class rdf:about="&glvoc_l05;57">
        <owl:equivalentClass>
            <owl:Restriction>
                <owl:onProperty rdf:resource="&glview;hasInstrumentType"/>
                <owl:hasValue rdf:resource="&glvoc_l05;57"/>
            </owl:Restriction>
        </owl:equivalentClass>
        <rdfs:subClassOf rdf:resource="&glview;Instrument"/>
    </owl:Class>
    


    <!-- http://schema.geolink.org/dev/voc/nvs/L05#58 -->

    <owl:Class rdf:about="&glvoc_l05;58">
        <owl:equivalentClass>
            <owl:Restriction>
                <owl:onProperty rdf:resource="&glview;hasInstrumentType"/>
                <owl:hasValue rdf:resource="&glvoc_l05;58"/>
            </owl:Restriction>
        </owl:equivalentClass>
        <rdfs:subClassOf rdf:resource="&glview;Instrument"/>
    </owl:Class>
    


    <!-- http://schema.geolink.org/dev/voc/nvs/L05#59 -->

    <owl:Class rdf:about="&glvoc_l05;59">
        <owl:equivalentClass>
            <owl:Restriction>
                <owl:onProperty rdf:resource="&glview;hasInstrumentType"/>
                <owl:hasValue rdf:resource="&glvoc_l05;59"/>
            </owl:Restriction>
        </owl:equivalentClass>
        <rdfs:subClassOf rdf:resource="&glview;Instrument"/>
    </owl:Class>
    


    <!-- http://schema.geolink.org/dev/voc/nvs/L05#60 -->

    <owl:Class rdf:about="&glvoc_l05;60">
        <owl:equivalentClass>
            <owl:Restriction>
                <owl:onProperty rdf:resource="&glview;hasInstrumentType"/>
                <owl:hasValue rdf:resource="&glvoc_l05;60"/>
            </owl:Restriction>
        </owl:equivalentClass>
        <rdfs:subClassOf rdf:resource="&glview;Instrument"/>
    </owl:Class>
    


    <!-- http://schema.geolink.org/dev/voc/nvs/L05#61 -->

    <owl:Class rdf:about="&glvoc_l05;61">
        <owl:equivalentClass>
            <owl:Restriction>
                <owl:onProperty rdf:resource="&glview;hasInstrumentType"/>
                <owl:hasValue rdf:resource="&glvoc_l05;61"/>
            </owl:Restriction>
        </owl:equivalentClass>
        <rdfs:subClassOf rdf:resource="&glview;Instrument"/>
    </owl:Class>
    


    <!-- http://schema.geolink.org/dev/voc/nvs/L05#62 -->

    <owl:Class rdf:about="&glvoc_l05;62">
        <owl:equivalentClass>
            <owl:Restriction>
                <owl:onProperty rdf:resource="&glview;hasInstrumentType"/>
                <owl:hasValue rdf:resource="&glvoc_l05;62"/>
            </owl:Restriction>
        </owl:equivalentClass>
        <rdfs:subClassOf rdf:resource="&glview;Instrument"/>
    </owl:Class>
    


    <!-- http://schema.geolink.org/dev/voc/nvs/L05#63 -->

    <owl:Class rdf:about="&glvoc_l05;63">
        <owl:equivalentClass>
            <owl:Restriction>
                <owl:onProperty rdf:resource="&glview;hasInstrumentType"/>
                <owl:hasValue rdf:resource="&glvoc_l05;63"/>
            </owl:Restriction>
        </owl:equivalentClass>
        <rdfs:subClassOf rdf:resource="&glview;Instrument"/>
    </owl:Class>
    


    <!-- http://schema.geolink.org/dev/voc/nvs/L05#64 -->

    <owl:Class rdf:about="&glvoc_l05;64">
        <owl:equivalentClass>
            <owl:Restriction>
                <owl:onProperty rdf:resource="&glview;hasInstrumentType"/>
                <owl:hasValue rdf:resource="&glvoc_l05;64"/>
            </owl:Restriction>
        </owl:equivalentClass>
        <rdfs:subClassOf rdf:resource="&glview;Instrument"/>
    </owl:Class>
    


    <!-- http://schema.geolink.org/dev/voc/nvs/L05#65 -->

    <owl:Class rdf:about="&glvoc_l05;65">
        <owl:equivalentClass>
            <owl:Restriction>
                <owl:onProperty rdf:resource="&glview;hasInstrumentType"/>
                <owl:hasValue rdf:resource="&glvoc_l05;65"/>
            </owl:Restriction>
        </owl:equivalentClass>
        <rdfs:subClassOf rdf:resource="&glview;Instrument"/>
    </owl:Class>
    


    <!-- http://schema.geolink.org/dev/voc/nvs/L05#66 -->

    <owl:Class rdf:about="&glvoc_l05;66">
        <owl:equivalentClass>
            <owl:Restriction>
                <owl:onProperty rdf:resource="&glview;hasInstrumentType"/>
                <owl:hasValue rdf:resource="&glvoc_l05;66"/>
            </owl:Restriction>
        </owl:equivalentClass>
        <rdfs:subClassOf rdf:resource="&glview;Instrument"/>
    </owl:Class>
    


    <!-- http://schema.geolink.org/dev/voc/nvs/L05#67 -->

    <owl:Class rdf:about="&glvoc_l05;67">
        <owl:equivalentClass>
            <owl:Restriction>
                <owl:onProperty rdf:resource="&glview;hasInstrumentType"/>
                <owl:hasValue rdf:resource="&glvoc_l05;67"/>
            </owl:Restriction>
        </owl:equivalentClass>
        <rdfs:subClassOf rdf:resource="&glview;Instrument"/>
    </owl:Class>
    


    <!-- http://schema.geolink.org/dev/voc/nvs/L05#68 -->

    <owl:Class rdf:about="&glvoc_l05;68">
        <owl:equivalentClass>
            <owl:Restriction>
                <owl:onProperty rdf:resource="&glview;hasInstrumentType"/>
                <owl:hasValue rdf:resource="&glvoc_l05;68"/>
            </owl:Restriction>
        </owl:equivalentClass>
        <rdfs:subClassOf rdf:resource="&glview;Instrument"/>
    </owl:Class>
    


    <!-- http://schema.geolink.org/dev/voc/nvs/L05#69 -->

    <owl:Class rdf:about="&glvoc_l05;69">
        <owl:equivalentClass>
            <owl:Restriction>
                <owl:onProperty rdf:resource="&glview;hasInstrumentType"/>
                <owl:hasValue rdf:resource="&glvoc_l05;69"/>
            </owl:Restriction>
        </owl:equivalentClass>
        <rdfs:subClassOf rdf:resource="&glview;Instrument"/>
    </owl:Class>
    


    <!-- http://schema.geolink.org/dev/voc/nvs/L05#81 -->

    <owl:Class rdf:about="&glvoc_l05;81">
        <owl:equivalentClass>
            <owl:Restriction>
                <owl:onProperty rdf:resource="&glview;hasInstrumentType"/>
                <owl:hasValue rdf:resource="&glvoc_l05;81"/>
            </owl:Restriction>
        </owl:equivalentClass>
        <rdfs:subClassOf rdf:resource="&glview;Instrument"/>
    </owl:Class>
    


    <!-- http://schema.geolink.org/dev/voc/nvs/L05#82 -->

    <owl:Class rdf:about="&glvoc_l05;82">
        <owl:equivalentClass>
            <owl:Restriction>
                <owl:onProperty rdf:resource="&glview;hasInstrumentType"/>
                <owl:hasValue rdf:resource="&glvoc_l05;82"/>
            </owl:Restriction>
        </owl:equivalentClass>
        <rdfs:subClassOf rdf:resource="&glview;Instrument"/>
    </owl:Class>
    


    <!-- http://schema.geolink.org/dev/voc/nvs/L05#83 -->

    <owl:Class rdf:about="&glvoc_l05;83">
        <owl:equivalentClass>
            <owl:Restriction>
                <owl:onProperty rdf:resource="&glview;hasInstrumentType"/>
                <owl:hasValue rdf:resource="&glvoc_l05;83"/>
            </owl:Restriction>
        </owl:equivalentClass>
        <rdfs:subClassOf rdf:resource="&glview;Instrument"/>
    </owl:Class>
    


    <!-- http://schema.geolink.org/dev/voc/nvs/L05#84 -->

    <owl:Class rdf:about="&glvoc_l05;84">
        <owl:equivalentClass>
            <owl:Restriction>
                <owl:onProperty rdf:resource="&glview;hasInstrumentType"/>
                <owl:hasValue rdf:resource="&glvoc_l05;84"/>
            </owl:Restriction>
        </owl:equivalentClass>
        <rdfs:subClassOf rdf:resource="&glview;Instrument"/>
    </owl:Class>
    


    <!-- http://schema.geolink.org/dev/voc/nvs/L05#85 -->

    <owl:Class rdf:about="&glvoc_l05;85">
        <owl:equivalentClass>
            <owl:Restriction>
                <owl:onProperty rdf:resource="&glview;hasInstrumentType"/>
                <owl:hasValue rdf:resource="&glvoc_l05;85"/>
            </owl:Restriction>
        </owl:equivalentClass>
        <rdfs:subClassOf rdf:resource="&glview;Instrument"/>
    </owl:Class>
    


    <!-- http://schema.geolink.org/dev/voc/nvs/L05#90 -->

    <owl:Class rdf:about="&glvoc_l05;90">
        <owl:equivalentClass>
            <owl:Restriction>
                <owl:onProperty rdf:resource="&glview;hasInstrumentType"/>
                <owl:hasValue rdf:resource="&glvoc_l05;90"/>
            </owl:Restriction>
        </owl:equivalentClass>
        <rdfs:subClassOf rdf:resource="&glview;Instrument"/>
    </owl:Class>
    


    <!-- http://schema.geolink.org/dev/voc/nvs/L05#91 -->

    <owl:Class rdf:about="&glvoc_l05;91">
        <owl:equivalentClass>
            <owl:Restriction>
                <owl:onProperty rdf:resource="&glview;hasInstrumentType"/>
                <owl:hasValue rdf:resource="&glvoc_l05;91"/>
            </owl:Restriction>
        </owl:equivalentClass>
        <rdfs:subClassOf rdf:resource="&glview;Instrument"/>
    </owl:Class>
    


    <!-- http://schema.geolink.org/dev/voc/nvs/L05#999 -->

    <owl:Class rdf:about="&glvoc_l05;999">
        <owl:equivalentClass>
            <owl:Restriction>
                <owl:onProperty rdf:resource="&glview;hasInstrumentType"/>
                <owl:hasValue rdf:resource="&glvoc_l05;999"/>
            </owl:Restriction>
        </owl:equivalentClass>
        <rdfs:subClassOf rdf:resource="&glview;Instrument"/>
    </owl:Class>
    


    <!-- 
    ///////////////////////////////////////////////////////////////////////////////////////
    //
    // Individuals
    //
    ///////////////////////////////////////////////////////////////////////////////////////
     -->

    


    <!-- http://schema.geolink.org/dev/voc/nvs/L05#AQPL -->

    <owl:NamedIndividual rdf:about="&glvoc_l05;AQPL">
        <rdf:type rdf:resource="&glview;InstrumentType"/>
    </owl:NamedIndividual>
    


    <!-- http://schema.geolink.org/dev/voc/nvs/L05#ARAG -->

    <owl:NamedIndividual rdf:about="&glvoc_l05;ARAG">
        <rdf:type rdf:resource="&glview;InstrumentType"/>
    </owl:NamedIndividual>
    


    <!-- http://schema.geolink.org/dev/voc/nvs/L05#ATRANS -->

    <owl:NamedIndividual rdf:about="&glvoc_l05;ATRANS">
        <rdf:type rdf:resource="&glview;InstrumentType"/>
    </owl:NamedIndividual>
    


    <!-- http://schema.geolink.org/dev/voc/nvs/L05#BLUMS -->

    <owl:NamedIndividual rdf:about="&glvoc_l05;BLUMS">
        <rdf:type rdf:resource="&glview;InstrumentType"/>
    </owl:NamedIndividual>
    


    <!-- http://schema.geolink.org/dev/voc/nvs/L05#BOMR -->

    <owl:NamedIndividual rdf:about="&glvoc_l05;BOMR">
        <rdf:type rdf:resource="&glview;InstrumentType"/>
    </owl:NamedIndividual>
    


    <!-- http://schema.geolink.org/dev/voc/nvs/L05#CCOV -->

    <owl:NamedIndividual rdf:about="&glvoc_l05;CCOV">
        <rdf:type rdf:resource="&glview;InstrumentType"/>
    </owl:NamedIndividual>
    


    <!-- http://schema.geolink.org/dev/voc/nvs/L05#CHRP -->

    <owl:NamedIndividual rdf:about="&glvoc_l05;CHRP">
        <rdf:type rdf:resource="&glview;InstrumentType"/>
    </owl:NamedIndividual>
    


    <!-- http://schema.geolink.org/dev/voc/nvs/L05#COLCMP -->

    <owl:NamedIndividual rdf:about="&glvoc_l05;COLCMP">
        <rdf:type rdf:resource="&glview;InstrumentType"/>
    </owl:NamedIndividual>
    


    <!-- http://schema.geolink.org/dev/voc/nvs/L05#CSEM -->

    <owl:NamedIndividual rdf:about="&glvoc_l05;CSEM">
        <rdf:type rdf:resource="&glview;InstrumentType"/>
    </owl:NamedIndividual>
    


    <!-- http://schema.geolink.org/dev/voc/nvs/L05#EMSR -->

    <owl:NamedIndividual rdf:about="&glvoc_l05;EMSR">
        <rdf:type rdf:resource="&glview;InstrumentType"/>
    </owl:NamedIndividual>
    


    <!-- http://schema.geolink.org/dev/voc/nvs/L05#EQUIL -->

    <owl:NamedIndividual rdf:about="&glvoc_l05;EQUIL">
        <rdf:type rdf:resource="&glview;InstrumentType"/>
    </owl:NamedIndividual>
    


    <!-- http://schema.geolink.org/dev/voc/nvs/L05#ERTQ -->

    <owl:NamedIndividual rdf:about="&glvoc_l05;ERTQ">
        <rdf:type rdf:resource="&glview;InstrumentType"/>
    </owl:NamedIndividual>
    


    <!-- http://schema.geolink.org/dev/voc/nvs/L05#EXHL -->

    <owl:NamedIndividual rdf:about="&glvoc_l05;EXHL">
        <rdf:type rdf:resource="&glview;InstrumentType"/>
    </owl:NamedIndividual>
    


    <!-- http://schema.geolink.org/dev/voc/nvs/L05#EXLH -->

    <owl:NamedIndividual rdf:about="&glvoc_l05;EXLH">
        <rdf:type rdf:resource="&glview;InstrumentType"/>
    </owl:NamedIndividual>
    


    <!-- http://schema.geolink.org/dev/voc/nvs/L05#FFES -->

    <owl:NamedIndividual rdf:about="&glvoc_l05;FFES">
        <rdf:type rdf:resource="&glview;InstrumentType"/>
    </owl:NamedIndividual>
    


    <!-- http://schema.geolink.org/dev/voc/nvs/L05#FLXS -->

    <owl:NamedIndividual rdf:about="&glvoc_l05;FLXS">
        <rdf:type rdf:resource="&glview;InstrumentType"/>
    </owl:NamedIndividual>
    


    <!-- http://schema.geolink.org/dev/voc/nvs/L05#FLXT -->

    <owl:NamedIndividual rdf:about="&glvoc_l05;FLXT">
        <rdf:type rdf:resource="&glview;InstrumentType"/>
    </owl:NamedIndividual>
    


    <!-- http://schema.geolink.org/dev/voc/nvs/L05#GIAG -->

    <owl:NamedIndividual rdf:about="&glvoc_l05;GIAG">
        <rdf:type rdf:resource="&glview;InstrumentType"/>
    </owl:NamedIndividual>
    


    <!-- http://schema.geolink.org/dev/voc/nvs/L05#ICEP -->

    <owl:NamedIndividual rdf:about="&glvoc_l05;ICEP">
        <rdf:type rdf:resource="&glview;InstrumentType"/>
    </owl:NamedIndividual>
    


    <!-- http://schema.geolink.org/dev/voc/nvs/L05#LAB01 -->

    <owl:NamedIndividual rdf:about="&glvoc_l05;LAB01">
        <rdf:type rdf:resource="&glview;InstrumentType"/>
    </owl:NamedIndividual>
    


    <!-- http://schema.geolink.org/dev/voc/nvs/L05#LAB02 -->

    <owl:NamedIndividual rdf:about="&glvoc_l05;LAB02">
        <rdf:type rdf:resource="&glview;InstrumentType"/>
    </owl:NamedIndividual>
    


    <!-- http://schema.geolink.org/dev/voc/nvs/L05#LAB03 -->

    <owl:NamedIndividual rdf:about="&glvoc_l05;LAB03">
        <rdf:type rdf:resource="&glview;InstrumentType"/>
    </owl:NamedIndividual>
    


    <!-- http://schema.geolink.org/dev/voc/nvs/L05#LAB04 -->

    <owl:NamedIndividual rdf:about="&glvoc_l05;LAB04">
        <rdf:type rdf:resource="&glview;InstrumentType"/>
    </owl:NamedIndividual>
    


    <!-- http://schema.geolink.org/dev/voc/nvs/L05#LAB05 -->

    <owl:NamedIndividual rdf:about="&glvoc_l05;LAB05">
        <rdf:type rdf:resource="&glview;InstrumentType"/>
    </owl:NamedIndividual>
    


    <!-- http://schema.geolink.org/dev/voc/nvs/L05#LAB06 -->

    <owl:NamedIndividual rdf:about="&glvoc_l05;LAB06">
        <rdf:type rdf:resource="&glview;InstrumentType"/>
    </owl:NamedIndividual>
    


    <!-- http://schema.geolink.org/dev/voc/nvs/L05#LAB07 -->

    <owl:NamedIndividual rdf:about="&glvoc_l05;LAB07">
        <rdf:type rdf:resource="&glview;InstrumentType"/>
    </owl:NamedIndividual>
    


    <!-- http://schema.geolink.org/dev/voc/nvs/L05#LAB08 -->

    <owl:NamedIndividual rdf:about="&glvoc_l05;LAB08">
        <rdf:type rdf:resource="&glview;InstrumentType"/>
    </owl:NamedIndividual>
    


    <!-- http://schema.geolink.org/dev/voc/nvs/L05#LAB09 -->

    <owl:NamedIndividual rdf:about="&glvoc_l05;LAB09">
        <rdf:type rdf:resource="&glview;InstrumentType"/>
    </owl:NamedIndividual>
    


    <!-- http://schema.geolink.org/dev/voc/nvs/L05#LAB10 -->

    <owl:NamedIndividual rdf:about="&glvoc_l05;LAB10">
        <rdf:type rdf:resource="&glview;InstrumentType"/>
    </owl:NamedIndividual>
    


    <!-- http://schema.geolink.org/dev/voc/nvs/L05#LAB11 -->

    <owl:NamedIndividual rdf:about="&glvoc_l05;LAB11">
        <rdf:type rdf:resource="&glview;InstrumentType"/>
    </owl:NamedIndividual>
    


    <!-- http://schema.geolink.org/dev/voc/nvs/L05#LAB12 -->

    <owl:NamedIndividual rdf:about="&glvoc_l05;LAB12">
        <rdf:type rdf:resource="&glview;InstrumentType"/>
    </owl:NamedIndividual>
    


    <!-- http://schema.geolink.org/dev/voc/nvs/L05#LAB13 -->

    <owl:NamedIndividual rdf:about="&glvoc_l05;LAB13">
        <rdf:type rdf:resource="&glview;InstrumentType"/>
    </owl:NamedIndividual>
    


    <!-- http://schema.geolink.org/dev/voc/nvs/L05#LAB14 -->

    <owl:NamedIndividual rdf:about="&glvoc_l05;LAB14">
        <rdf:type rdf:resource="&glview;InstrumentType"/>
    </owl:NamedIndividual>
    


    <!-- http://schema.geolink.org/dev/voc/nvs/L05#LAB15 -->

    <owl:NamedIndividual rdf:about="&glvoc_l05;LAB15">
        <rdf:type rdf:resource="&glview;InstrumentType"/>
    </owl:NamedIndividual>
    


    <!-- http://schema.geolink.org/dev/voc/nvs/L05#LAB16 -->

    <owl:NamedIndividual rdf:about="&glvoc_l05;LAB16">
        <rdf:type rdf:resource="&glview;InstrumentType"/>
    </owl:NamedIndividual>
    


    <!-- http://schema.geolink.org/dev/voc/nvs/L05#LAB17 -->

    <owl:NamedIndividual rdf:about="&glvoc_l05;LAB17">
        <rdf:type rdf:resource="&glview;InstrumentType"/>
    </owl:NamedIndividual>
    


    <!-- http://schema.geolink.org/dev/voc/nvs/L05#LAB18 -->

    <owl:NamedIndividual rdf:about="&glvoc_l05;LAB18">
        <rdf:type rdf:resource="&glview;InstrumentType"/>
    </owl:NamedIndividual>
    


    <!-- http://schema.geolink.org/dev/voc/nvs/L05#LAB19 -->

    <owl:NamedIndividual rdf:about="&glvoc_l05;LAB19">
        <rdf:type rdf:resource="&glview;InstrumentType"/>
    </owl:NamedIndividual>
    


    <!-- http://schema.geolink.org/dev/voc/nvs/L05#LAB20 -->

    <owl:NamedIndividual rdf:about="&glvoc_l05;LAB20">
        <rdf:type rdf:resource="&glview;InstrumentType"/>
    </owl:NamedIndividual>
    


    <!-- http://schema.geolink.org/dev/voc/nvs/L05#LAB21 -->

    <owl:NamedIndividual rdf:about="&glvoc_l05;LAB21">
        <rdf:type rdf:resource="&glview;InstrumentType"/>
    </owl:NamedIndividual>
    


    <!-- http://schema.geolink.org/dev/voc/nvs/L05#LAB22 -->

    <owl:NamedIndividual rdf:about="&glvoc_l05;LAB22">
        <rdf:type rdf:resource="&glview;InstrumentType"/>
    </owl:NamedIndividual>
    


    <!-- http://schema.geolink.org/dev/voc/nvs/L05#LAB23 -->

    <owl:NamedIndividual rdf:about="&glvoc_l05;LAB23">
        <rdf:type rdf:resource="&glview;InstrumentType"/>
    </owl:NamedIndividual>
    


    <!-- http://schema.geolink.org/dev/voc/nvs/L05#LAB24 -->

    <owl:NamedIndividual rdf:about="&glvoc_l05;LAB24">
        <rdf:type rdf:resource="&glview;InstrumentType"/>
    </owl:NamedIndividual>
    


    <!-- http://schema.geolink.org/dev/voc/nvs/L05#LAB25 -->

    <owl:NamedIndividual rdf:about="&glvoc_l05;LAB25">
        <rdf:type rdf:resource="&glview;InstrumentType"/>
    </owl:NamedIndividual>
    


    <!-- http://schema.geolink.org/dev/voc/nvs/L05#LAB26 -->

    <owl:NamedIndividual rdf:about="&glvoc_l05;LAB26">
        <rdf:type rdf:resource="&glview;InstrumentType"/>
    </owl:NamedIndividual>
    


    <!-- http://schema.geolink.org/dev/voc/nvs/L05#LAB27 -->

    <owl:NamedIndividual rdf:about="&glvoc_l05;LAB27">
        <rdf:type rdf:resource="&glview;InstrumentType"/>
    </owl:NamedIndividual>
    


    <!-- http://schema.geolink.org/dev/voc/nvs/L05#LAB28 -->

    <owl:NamedIndividual rdf:about="&glvoc_l05;LAB28">
        <rdf:type rdf:resource="&glview;InstrumentType"/>
    </owl:NamedIndividual>
    


    <!-- http://schema.geolink.org/dev/voc/nvs/L05#LAB29 -->

    <owl:NamedIndividual rdf:about="&glvoc_l05;LAB29">
        <rdf:type rdf:resource="&glview;InstrumentType"/>
    </owl:NamedIndividual>
    


    <!-- http://schema.geolink.org/dev/voc/nvs/L05#LAB30 -->

    <owl:NamedIndividual rdf:about="&glvoc_l05;LAB30">
        <rdf:type rdf:resource="&glview;InstrumentType"/>
    </owl:NamedIndividual>
    


    <!-- http://schema.geolink.org/dev/voc/nvs/L05#LAB31 -->

    <owl:NamedIndividual rdf:about="&glvoc_l05;LAB31">
        <rdf:type rdf:resource="&glview;InstrumentType"/>
    </owl:NamedIndividual>
    


    <!-- http://schema.geolink.org/dev/voc/nvs/L05#LAB32 -->

    <owl:NamedIndividual rdf:about="&glvoc_l05;LAB32">
        <rdf:type rdf:resource="&glview;InstrumentType"/>
    </owl:NamedIndividual>
    


    <!-- http://schema.geolink.org/dev/voc/nvs/L05#LAB33 -->

    <owl:NamedIndividual rdf:about="&glvoc_l05;LAB33">
        <rdf:type rdf:resource="&glview;InstrumentType"/>
    </owl:NamedIndividual>
    


    <!-- http://schema.geolink.org/dev/voc/nvs/L05#LAB34 -->

    <owl:NamedIndividual rdf:about="&glvoc_l05;LAB34">
        <rdf:type rdf:resource="&glview;InstrumentType"/>
    </owl:NamedIndividual>
    


    <!-- http://schema.geolink.org/dev/voc/nvs/L05#LAB35 -->

    <owl:NamedIndividual rdf:about="&glvoc_l05;LAB35">
        <rdf:type rdf:resource="&glview;InstrumentType"/>
    </owl:NamedIndividual>
    


    <!-- http://schema.geolink.org/dev/voc/nvs/L05#LAB36 -->

    <owl:NamedIndividual rdf:about="&glvoc_l05;LAB36">
        <rdf:type rdf:resource="&glview;InstrumentType"/>
    </owl:NamedIndividual>
    


    <!-- http://schema.geolink.org/dev/voc/nvs/L05#LAB37 -->

    <owl:NamedIndividual rdf:about="&glvoc_l05;LAB37">
        <rdf:type rdf:resource="&glview;InstrumentType"/>
    </owl:NamedIndividual>
    


    <!-- http://schema.geolink.org/dev/voc/nvs/L05#LAB38 -->

    <owl:NamedIndividual rdf:about="&glvoc_l05;LAB38">
        <rdf:type rdf:resource="&glview;InstrumentType"/>
    </owl:NamedIndividual>
    


    <!-- http://schema.geolink.org/dev/voc/nvs/L05#LAB39 -->

    <owl:NamedIndividual rdf:about="&glvoc_l05;LAB39">
        <rdf:type rdf:resource="&glview;InstrumentType"/>
    </owl:NamedIndividual>
    


    <!-- http://schema.geolink.org/dev/voc/nvs/L05#LAB40 -->

    <owl:NamedIndividual rdf:about="&glvoc_l05;LAB40">
        <rdf:type rdf:resource="&glview;InstrumentType"/>
    </owl:NamedIndividual>
    


    <!-- http://schema.geolink.org/dev/voc/nvs/L05#LAB41 -->

    <owl:NamedIndividual rdf:about="&glvoc_l05;LAB41">
        <rdf:type rdf:resource="&glview;InstrumentType"/>
    </owl:NamedIndividual>
    


    <!-- http://schema.geolink.org/dev/voc/nvs/L05#LAB42 -->

    <owl:NamedIndividual rdf:about="&glvoc_l05;LAB42">
        <rdf:type rdf:resource="&glview;InstrumentType"/>
    </owl:NamedIndividual>
    


    <!-- http://schema.geolink.org/dev/voc/nvs/L05#LAB43 -->

    <owl:NamedIndividual rdf:about="&glvoc_l05;LAB43">
        <rdf:type rdf:resource="&glview;InstrumentType"/>
    </owl:NamedIndividual>
    


    <!-- http://schema.geolink.org/dev/voc/nvs/L05#LAB44 -->

    <owl:NamedIndividual rdf:about="&glvoc_l05;LAB44">
        <rdf:type rdf:resource="&glview;InstrumentType"/>
    </owl:NamedIndividual>
    


    <!-- http://schema.geolink.org/dev/voc/nvs/L05#LBTG -->

    <owl:NamedIndividual rdf:about="&glvoc_l05;LBTG">
        <rdf:type rdf:resource="&glview;InstrumentType"/>
    </owl:NamedIndividual>
    


    <!-- http://schema.geolink.org/dev/voc/nvs/L05#MMIS -->

    <owl:NamedIndividual rdf:about="&glvoc_l05;MMIS">
        <rdf:type rdf:resource="&glview;InstrumentType"/>
    </owl:NamedIndividual>
    


    <!-- http://schema.geolink.org/dev/voc/nvs/L05#MOD01 -->

    <owl:NamedIndividual rdf:about="&glvoc_l05;MOD01">
        <rdf:type rdf:resource="&glview;InstrumentType"/>
    </owl:NamedIndividual>
    


    <!-- http://schema.geolink.org/dev/voc/nvs/L05#MOD02 -->

    <owl:NamedIndividual rdf:about="&glvoc_l05;MOD02">
        <rdf:type rdf:resource="&glview;InstrumentType"/>
    </owl:NamedIndividual>
    


    <!-- http://schema.geolink.org/dev/voc/nvs/L05#MOD03 -->

    <owl:NamedIndividual rdf:about="&glvoc_l05;MOD03">
        <rdf:type rdf:resource="&glview;InstrumentType"/>
    </owl:NamedIndividual>
    


    <!-- http://schema.geolink.org/dev/voc/nvs/L05#MOD04 -->

    <owl:NamedIndividual rdf:about="&glvoc_l05;MOD04">
        <rdf:type rdf:resource="&glview;InstrumentType"/>
    </owl:NamedIndividual>
    


    <!-- http://schema.geolink.org/dev/voc/nvs/L05#MOD05 -->

    <owl:NamedIndividual rdf:about="&glvoc_l05;MOD05">
        <rdf:type rdf:resource="&glview;InstrumentType"/>
    </owl:NamedIndividual>
    


    <!-- http://schema.geolink.org/dev/voc/nvs/L05#MOD06 -->

    <owl:NamedIndividual rdf:about="&glvoc_l05;MOD06">
        <rdf:type rdf:resource="&glview;InstrumentType"/>
    </owl:NamedIndividual>
    


    <!-- http://schema.geolink.org/dev/voc/nvs/L05#MOD07 -->

    <owl:NamedIndividual rdf:about="&glvoc_l05;MOD07">
        <rdf:type rdf:resource="&glview;InstrumentType"/>
    </owl:NamedIndividual>
    


    <!-- http://schema.geolink.org/dev/voc/nvs/L05#MOD08 -->

    <owl:NamedIndividual rdf:about="&glvoc_l05;MOD08">
        <rdf:type rdf:resource="&glview;InstrumentType"/>
    </owl:NamedIndividual>
    


    <!-- http://schema.geolink.org/dev/voc/nvs/L05#MVBR -->

    <owl:NamedIndividual rdf:about="&glvoc_l05;MVBR">
        <rdf:type rdf:resource="&glview;InstrumentType"/>
    </owl:NamedIndividual>
    


    <!-- http://schema.geolink.org/dev/voc/nvs/L05#NATS -->

    <owl:NamedIndividual rdf:about="&glvoc_l05;NATS">
        <rdf:type rdf:resource="&glview;InstrumentType"/>
    </owl:NamedIndividual>
    


    <!-- http://schema.geolink.org/dev/voc/nvs/L05#PERMON -->

    <owl:NamedIndividual rdf:about="&glvoc_l05;PERMON">
        <rdf:type rdf:resource="&glview;InstrumentType"/>
    </owl:NamedIndividual>
    


    <!-- http://schema.geolink.org/dev/voc/nvs/L05#POS01 -->

    <owl:NamedIndividual rdf:about="&glvoc_l05;POS01">
        <rdf:type rdf:resource="&glview;InstrumentType"/>
    </owl:NamedIndividual>
    


    <!-- http://schema.geolink.org/dev/voc/nvs/L05#POS02 -->

    <owl:NamedIndividual rdf:about="&glvoc_l05;POS02">
        <rdf:type rdf:resource="&glview;InstrumentType"/>
    </owl:NamedIndividual>
    


    <!-- http://schema.geolink.org/dev/voc/nvs/L05#POS03 -->

    <owl:NamedIndividual rdf:about="&glvoc_l05;POS03">
        <rdf:type rdf:resource="&glview;InstrumentType"/>
    </owl:NamedIndividual>
    


    <!-- http://schema.geolink.org/dev/voc/nvs/L05#POS04 -->

    <owl:NamedIndividual rdf:about="&glvoc_l05;POS04">
        <rdf:type rdf:resource="&glview;InstrumentType"/>
    </owl:NamedIndividual>
    


    <!-- http://schema.geolink.org/dev/voc/nvs/L05#POS05 -->

    <owl:NamedIndividual rdf:about="&glvoc_l05;POS05">
        <rdf:type rdf:resource="&glview;InstrumentType"/>
    </owl:NamedIndividual>
    


    <!-- http://schema.geolink.org/dev/voc/nvs/L05#POS06 -->

    <owl:NamedIndividual rdf:about="&glvoc_l05;POS06">
        <rdf:type rdf:resource="&glview;InstrumentType"/>
    </owl:NamedIndividual>
    


    <!-- http://schema.geolink.org/dev/voc/nvs/L05#POS07 -->

    <owl:NamedIndividual rdf:about="&glvoc_l05;POS07">
        <rdf:type rdf:resource="&glview;InstrumentType"/>
    </owl:NamedIndividual>
    


    <!-- http://schema.geolink.org/dev/voc/nvs/L05#POS08 -->

    <owl:NamedIndividual rdf:about="&glvoc_l05;POS08">
        <rdf:type rdf:resource="&glview;InstrumentType"/>
    </owl:NamedIndividual>
    


    <!-- http://schema.geolink.org/dev/voc/nvs/L05#POS09 -->

    <owl:NamedIndividual rdf:about="&glvoc_l05;POS09">
        <rdf:type rdf:resource="&glview;InstrumentType"/>
    </owl:NamedIndividual>
    


    <!-- http://schema.geolink.org/dev/voc/nvs/L05#POS10 -->

    <owl:NamedIndividual rdf:about="&glvoc_l05;POS10">
        <rdf:type rdf:resource="&glview;InstrumentType"/>
    </owl:NamedIndividual>
    


    <!-- http://schema.geolink.org/dev/voc/nvs/L05#POS11 -->

    <owl:NamedIndividual rdf:about="&glvoc_l05;POS11">
        <rdf:type rdf:resource="&glview;InstrumentType"/>
    </owl:NamedIndividual>
    


    <!-- http://schema.geolink.org/dev/voc/nvs/L05#POS12 -->

    <owl:NamedIndividual rdf:about="&glvoc_l05;POS12">
        <rdf:type rdf:resource="&glview;InstrumentType"/>
    </owl:NamedIndividual>
    


    <!-- http://schema.geolink.org/dev/voc/nvs/L05#POS13 -->

    <owl:NamedIndividual rdf:about="&glvoc_l05;POS13">
        <rdf:type rdf:resource="&glview;InstrumentType"/>
    </owl:NamedIndividual>
    


    <!-- http://schema.geolink.org/dev/voc/nvs/L05#POS14 -->

    <owl:NamedIndividual rdf:about="&glvoc_l05;POS14">
        <rdf:type rdf:resource="&glview;InstrumentType"/>
    </owl:NamedIndividual>
    


    <!-- http://schema.geolink.org/dev/voc/nvs/L05#POS15 -->

    <owl:NamedIndividual rdf:about="&glvoc_l05;POS15">
        <rdf:type rdf:resource="&glview;InstrumentType"/>
    </owl:NamedIndividual>
    


    <!-- http://schema.geolink.org/dev/voc/nvs/L05#POS16 -->

    <owl:NamedIndividual rdf:about="&glvoc_l05;POS16">
        <rdf:type rdf:resource="&glview;InstrumentType"/>
    </owl:NamedIndividual>
    


    <!-- http://schema.geolink.org/dev/voc/nvs/L05#POS17 -->

    <owl:NamedIndividual rdf:about="&glvoc_l05;POS17">
        <rdf:type rdf:resource="&glview;InstrumentType"/>
    </owl:NamedIndividual>
    


    <!-- http://schema.geolink.org/dev/voc/nvs/L05#POS18 -->

    <owl:NamedIndividual rdf:about="&glvoc_l05;POS18">
        <rdf:type rdf:resource="&glview;InstrumentType"/>
    </owl:NamedIndividual>
    


    <!-- http://schema.geolink.org/dev/voc/nvs/L05#POS19 -->

    <owl:NamedIndividual rdf:about="&glvoc_l05;POS19">
        <rdf:type rdf:resource="&glview;InstrumentType"/>
    </owl:NamedIndividual>
    


    <!-- http://schema.geolink.org/dev/voc/nvs/L05#POS20 -->

    <owl:NamedIndividual rdf:about="&glvoc_l05;POS20">
        <rdf:type rdf:resource="&glview;InstrumentType"/>
    </owl:NamedIndividual>
    


    <!-- http://schema.geolink.org/dev/voc/nvs/L05#POS21 -->

    <owl:NamedIndividual rdf:about="&glvoc_l05;POS21">
        <rdf:type rdf:resource="&glview;InstrumentType"/>
    </owl:NamedIndividual>
    


    <!-- http://schema.geolink.org/dev/voc/nvs/L05#POS22 -->

    <owl:NamedIndividual rdf:about="&glvoc_l05;POS22">
        <rdf:type rdf:resource="&glview;InstrumentType"/>
    </owl:NamedIndividual>
    


    <!-- http://schema.geolink.org/dev/voc/nvs/L05#POS23 -->

    <owl:NamedIndividual rdf:about="&glvoc_l05;POS23">
        <rdf:type rdf:resource="&glview;InstrumentType"/>
    </owl:NamedIndividual>
    


    <!-- http://schema.geolink.org/dev/voc/nvs/L05#POS24 -->

    <owl:NamedIndividual rdf:about="&glvoc_l05;POS24">
        <rdf:type rdf:resource="&glview;InstrumentType"/>
    </owl:NamedIndividual>
    


    <!-- http://schema.geolink.org/dev/voc/nvs/L05#POS25 -->

    <owl:NamedIndividual rdf:about="&glvoc_l05;POS25">
        <rdf:type rdf:resource="&glview;InstrumentType"/>
    </owl:NamedIndividual>
    


    <!-- http://schema.geolink.org/dev/voc/nvs/L05#POS26 -->

    <owl:NamedIndividual rdf:about="&glvoc_l05;POS26">
        <rdf:type rdf:resource="&glview;InstrumentType"/>
    </owl:NamedIndividual>
    


    <!-- http://schema.geolink.org/dev/voc/nvs/L05#SBAG -->

    <owl:NamedIndividual rdf:about="&glvoc_l05;SBAG">
        <rdf:type rdf:resource="&glview;InstrumentType"/>
    </owl:NamedIndividual>
    


    <!-- http://schema.geolink.org/dev/voc/nvs/L05#SNAG -->

    <owl:NamedIndividual rdf:about="&glvoc_l05;SNAG">
        <rdf:type rdf:resource="&glview;InstrumentType"/>
    </owl:NamedIndividual>
    


    <!-- http://schema.geolink.org/dev/voc/nvs/L05#SNWG -->

    <owl:NamedIndividual rdf:about="&glvoc_l05;SNWG">
        <rdf:type rdf:resource="&glview;InstrumentType"/>
    </owl:NamedIndividual>
    


    <!-- http://schema.geolink.org/dev/voc/nvs/L05#SPRK -->

    <owl:NamedIndividual rdf:about="&glvoc_l05;SPRK">
        <rdf:type rdf:resource="&glview;InstrumentType"/>
    </owl:NamedIndividual>
    


    <!-- http://schema.geolink.org/dev/voc/nvs/L05#TFSAMP -->

    <owl:NamedIndividual rdf:about="&glvoc_l05;TFSAMP">
        <rdf:type rdf:resource="&glview;InstrumentType"/>
    </owl:NamedIndividual>
    


    <!-- http://schema.geolink.org/dev/voc/nvs/L05#TRTG -->

    <owl:NamedIndividual rdf:about="&glvoc_l05;TRTG">
        <rdf:type rdf:resource="&glview;InstrumentType"/>
    </owl:NamedIndividual>
    


    <!-- http://schema.geolink.org/dev/voc/nvs/L05#VSHC -->

    <owl:NamedIndividual rdf:about="&glvoc_l05;VSHC">
        <rdf:type rdf:resource="&glview;InstrumentType"/>
    </owl:NamedIndividual>
    


    <!-- http://schema.geolink.org/dev/voc/nvs/L05#WPS -->

    <owl:NamedIndividual rdf:about="&glvoc_l05;WPS">
        <rdf:type rdf:resource="&glview;InstrumentType"/>
    </owl:NamedIndividual>
    


    <!-- http://schema.geolink.org/dev/voc/nvs/L05#101 -->

    <owl:NamedIndividual rdf:about="&glvoc_l05;101">
        <rdf:type rdf:resource="&glview;InstrumentType"/>
    </owl:NamedIndividual>
    


    <!-- http://schema.geolink.org/dev/voc/nvs/L05#102 -->

    <owl:NamedIndividual rdf:about="&glvoc_l05;102">
        <rdf:type rdf:resource="&glview;InstrumentType"/>
    </owl:NamedIndividual>
    


    <!-- http://schema.geolink.org/dev/voc/nvs/L05#103 -->

    <owl:NamedIndividual rdf:about="&glvoc_l05;103">
        <rdf:type rdf:resource="&glview;InstrumentType"/>
    </owl:NamedIndividual>
    


    <!-- http://schema.geolink.org/dev/voc/nvs/L05#11 -->

    <owl:NamedIndividual rdf:about="&glvoc_l05;11">
        <rdf:type rdf:resource="&glview;InstrumentType"/>
    </owl:NamedIndividual>
    


    <!-- http://schema.geolink.org/dev/voc/nvs/L05#110 -->

    <owl:NamedIndividual rdf:about="&glvoc_l05;110">
        <rdf:type rdf:resource="&glview;InstrumentType"/>
    </owl:NamedIndividual>
    


    <!-- http://schema.geolink.org/dev/voc/nvs/L05#111 -->

    <owl:NamedIndividual rdf:about="&glvoc_l05;111">
        <rdf:type rdf:resource="&glview;InstrumentType"/>
    </owl:NamedIndividual>
    


    <!-- http://schema.geolink.org/dev/voc/nvs/L05#112 -->

    <owl:NamedIndividual rdf:about="&glvoc_l05;112">
        <rdf:type rdf:resource="&glview;InstrumentType"/>
    </owl:NamedIndividual>
    


    <!-- http://schema.geolink.org/dev/voc/nvs/L05#113 -->

    <owl:NamedIndividual rdf:about="&glvoc_l05;113">
        <rdf:type rdf:resource="&glview;InstrumentType"/>
    </owl:NamedIndividual>
    


    <!-- http://schema.geolink.org/dev/voc/nvs/L05#114 -->

    <owl:NamedIndividual rdf:about="&glvoc_l05;114">
        <rdf:type rdf:resource="&glview;InstrumentType"/>
    </owl:NamedIndividual>
    


    <!-- http://schema.geolink.org/dev/voc/nvs/L05#115 -->

    <owl:NamedIndividual rdf:about="&glvoc_l05;115">
        <rdf:type rdf:resource="&glview;InstrumentType"/>
    </owl:NamedIndividual>
    


    <!-- http://schema.geolink.org/dev/voc/nvs/L05#116 -->

    <owl:NamedIndividual rdf:about="&glvoc_l05;116">
        <rdf:type rdf:resource="&glview;InstrumentType"/>
    </owl:NamedIndividual>
    


    <!-- http://schema.geolink.org/dev/voc/nvs/L05#12 -->

    <owl:NamedIndividual rdf:about="&glvoc_l05;12">
        <rdf:type rdf:resource="&glview;InstrumentType"/>
    </owl:NamedIndividual>
    


    <!-- http://schema.geolink.org/dev/voc/nvs/L05#121 -->

    <owl:NamedIndividual rdf:about="&glvoc_l05;121">
        <rdf:type rdf:resource="&glview;InstrumentType"/>
    </owl:NamedIndividual>
    


    <!-- http://schema.geolink.org/dev/voc/nvs/L05#122 -->

    <owl:NamedIndividual rdf:about="&glvoc_l05;122">
        <rdf:type rdf:resource="&glview;InstrumentType"/>
    </owl:NamedIndividual>
    


    <!-- http://schema.geolink.org/dev/voc/nvs/L05#123 -->

    <owl:NamedIndividual rdf:about="&glvoc_l05;123">
        <rdf:type rdf:resource="&glview;InstrumentType"/>
    </owl:NamedIndividual>
    


    <!-- http://schema.geolink.org/dev/voc/nvs/L05#124 -->

    <owl:NamedIndividual rdf:about="&glvoc_l05;124">
        <rdf:type rdf:resource="&glview;InstrumentType"/>
    </owl:NamedIndividual>
    


    <!-- http://schema.geolink.org/dev/voc/nvs/L05#13 -->

    <owl:NamedIndividual rdf:about="&glvoc_l05;13">
        <rdf:type rdf:resource="&glview;InstrumentType"/>
    </owl:NamedIndividual>
    


    <!-- http://schema.geolink.org/dev/voc/nvs/L05#130 -->

    <owl:NamedIndividual rdf:about="&glvoc_l05;130">
        <rdf:type rdf:resource="&glview;InstrumentType"/>
    </owl:NamedIndividual>
    


    <!-- http://schema.geolink.org/dev/voc/nvs/L05#131 -->

    <owl:NamedIndividual rdf:about="&glvoc_l05;131">
        <rdf:type rdf:resource="&glview;InstrumentType"/>
    </owl:NamedIndividual>
    


    <!-- http://schema.geolink.org/dev/voc/nvs/L05#132 -->

    <owl:NamedIndividual rdf:about="&glvoc_l05;132">
        <rdf:type rdf:resource="&glview;InstrumentType"/>
    </owl:NamedIndividual>
    


    <!-- http://schema.geolink.org/dev/voc/nvs/L05#133 -->

    <owl:NamedIndividual rdf:about="&glvoc_l05;133">
        <rdf:type rdf:resource="&glview;InstrumentType"/>
    </owl:NamedIndividual>
    


    <!-- http://schema.geolink.org/dev/voc/nvs/L05#134 -->

    <owl:NamedIndividual rdf:about="&glvoc_l05;134">
        <rdf:type rdf:resource="&glview;InstrumentType"/>
    </owl:NamedIndividual>
    


    <!-- http://schema.geolink.org/dev/voc/nvs/L05#135 -->

    <owl:NamedIndividual rdf:about="&glvoc_l05;135">
        <rdf:type rdf:resource="&glview;InstrumentType"/>
    </owl:NamedIndividual>
    


    <!-- http://schema.geolink.org/dev/voc/nvs/L05#14 -->

    <owl:NamedIndividual rdf:about="&glvoc_l05;14">
        <rdf:type rdf:resource="&glview;InstrumentType"/>
    </owl:NamedIndividual>
    


    <!-- http://schema.geolink.org/dev/voc/nvs/L05#150 -->

    <owl:NamedIndividual rdf:about="&glvoc_l05;150">
        <rdf:type rdf:resource="&glview;InstrumentType"/>
    </owl:NamedIndividual>
    


    <!-- http://schema.geolink.org/dev/voc/nvs/L05#151 -->

    <owl:NamedIndividual rdf:about="&glvoc_l05;151">
        <rdf:type rdf:resource="&glview;InstrumentType"/>
    </owl:NamedIndividual>
    


    <!-- http://schema.geolink.org/dev/voc/nvs/L05#152 -->

    <owl:NamedIndividual rdf:about="&glvoc_l05;152">
        <rdf:type rdf:resource="&glview;InstrumentType"/>
    </owl:NamedIndividual>
    


    <!-- http://schema.geolink.org/dev/voc/nvs/L05#153 -->

    <owl:NamedIndividual rdf:about="&glvoc_l05;153">
        <rdf:type rdf:resource="&glview;InstrumentType"/>
    </owl:NamedIndividual>
    


    <!-- http://schema.geolink.org/dev/voc/nvs/L05#154 -->

    <owl:NamedIndividual rdf:about="&glvoc_l05;154">
        <rdf:type rdf:resource="&glview;InstrumentType"/>
    </owl:NamedIndividual>
    


    <!-- http://schema.geolink.org/dev/voc/nvs/L05#155 -->

    <owl:NamedIndividual rdf:about="&glvoc_l05;155">
        <rdf:type rdf:resource="&glview;InstrumentType"/>
    </owl:NamedIndividual>
    


    <!-- http://schema.geolink.org/dev/voc/nvs/L05#156 -->

    <owl:NamedIndividual rdf:about="&glvoc_l05;156">
        <rdf:type rdf:resource="&glview;InstrumentType"/>
    </owl:NamedIndividual>
    


    <!-- http://schema.geolink.org/dev/voc/nvs/L05#157 -->

    <owl:NamedIndividual rdf:about="&glvoc_l05;157">
        <rdf:type rdf:resource="&glview;InstrumentType"/>
    </owl:NamedIndividual>
    


    <!-- http://schema.geolink.org/dev/voc/nvs/L05#158 -->

    <owl:NamedIndividual rdf:about="&glvoc_l05;158">
        <rdf:type rdf:resource="&glview;InstrumentType"/>
    </owl:NamedIndividual>
    


    <!-- http://schema.geolink.org/dev/voc/nvs/L05#159 -->

    <owl:NamedIndividual rdf:about="&glvoc_l05;159">
        <rdf:type rdf:resource="&glview;InstrumentType"/>
    </owl:NamedIndividual>
    


    <!-- http://schema.geolink.org/dev/voc/nvs/L05#180 -->

    <owl:NamedIndividual rdf:about="&glvoc_l05;180">
        <rdf:type rdf:resource="&glview;InstrumentType"/>
    </owl:NamedIndividual>
    


    <!-- http://schema.geolink.org/dev/voc/nvs/L05#181 -->

    <owl:NamedIndividual rdf:about="&glvoc_l05;181">
        <rdf:type rdf:resource="&glview;InstrumentType"/>
    </owl:NamedIndividual>
    


    <!-- http://schema.geolink.org/dev/voc/nvs/L05#182 -->

    <owl:NamedIndividual rdf:about="&glvoc_l05;182">
        <rdf:type rdf:resource="&glview;InstrumentType"/>
    </owl:NamedIndividual>
    


    <!-- http://schema.geolink.org/dev/voc/nvs/L05#183 -->

    <owl:NamedIndividual rdf:about="&glvoc_l05;183">
        <rdf:type rdf:resource="&glview;InstrumentType"/>
    </owl:NamedIndividual>
    


    <!-- http://schema.geolink.org/dev/voc/nvs/L05#184 -->

    <owl:NamedIndividual rdf:about="&glvoc_l05;184">
        <rdf:type rdf:resource="&glview;InstrumentType"/>
    </owl:NamedIndividual>
    


    <!-- http://schema.geolink.org/dev/voc/nvs/L05#185 -->

    <owl:NamedIndividual rdf:about="&glvoc_l05;185">
        <rdf:type rdf:resource="&glview;InstrumentType"/>
    </owl:NamedIndividual>
    


    <!-- http://schema.geolink.org/dev/voc/nvs/L05#186 -->

    <owl:NamedIndividual rdf:about="&glvoc_l05;186">
        <rdf:type rdf:resource="&glview;InstrumentType"/>
    </owl:NamedIndividual>
    


    <!-- http://schema.geolink.org/dev/voc/nvs/L05#21 -->

    <owl:NamedIndividual rdf:about="&glvoc_l05;21">
        <rdf:type rdf:resource="&glview;InstrumentType"/>
    </owl:NamedIndividual>
    


    <!-- http://schema.geolink.org/dev/voc/nvs/L05#22 -->

    <owl:NamedIndividual rdf:about="&glvoc_l05;22">
        <rdf:type rdf:resource="&glview;InstrumentType"/>
    </owl:NamedIndividual>
    


    <!-- http://schema.geolink.org/dev/voc/nvs/L05#23 -->

    <owl:NamedIndividual rdf:about="&glvoc_l05;23">
        <rdf:type rdf:resource="&glview;InstrumentType"/>
    </owl:NamedIndividual>
    


    <!-- http://schema.geolink.org/dev/voc/nvs/L05#24 -->

    <owl:NamedIndividual rdf:about="&glvoc_l05;24">
        <rdf:type rdf:resource="&glview;InstrumentType"/>
    </owl:NamedIndividual>
    


    <!-- http://schema.geolink.org/dev/voc/nvs/L05#30 -->

    <owl:NamedIndividual rdf:about="&glvoc_l05;30">
        <rdf:type rdf:resource="&glview;InstrumentType"/>
    </owl:NamedIndividual>
    


    <!-- http://schema.geolink.org/dev/voc/nvs/L05#301 -->

    <owl:NamedIndividual rdf:about="&glvoc_l05;301">
        <rdf:type rdf:resource="&glview;InstrumentType"/>
    </owl:NamedIndividual>
    


    <!-- http://schema.geolink.org/dev/voc/nvs/L05#302 -->

    <owl:NamedIndividual rdf:about="&glvoc_l05;302">
        <rdf:type rdf:resource="&glview;InstrumentType"/>
    </owl:NamedIndividual>
    


    <!-- http://schema.geolink.org/dev/voc/nvs/L05#303 -->

    <owl:NamedIndividual rdf:about="&glvoc_l05;303">
        <rdf:type rdf:resource="&glview;InstrumentType"/>
    </owl:NamedIndividual>
    


    <!-- http://schema.geolink.org/dev/voc/nvs/L05#304 -->

    <owl:NamedIndividual rdf:about="&glvoc_l05;304">
        <rdf:type rdf:resource="&glview;InstrumentType"/>
    </owl:NamedIndividual>
    


    <!-- http://schema.geolink.org/dev/voc/nvs/L05#305 -->

    <owl:NamedIndividual rdf:about="&glvoc_l05;305">
        <rdf:type rdf:resource="&glview;InstrumentType"/>
    </owl:NamedIndividual>
    


    <!-- http://schema.geolink.org/dev/voc/nvs/L05#306 -->

    <owl:NamedIndividual rdf:about="&glvoc_l05;306">
        <rdf:type rdf:resource="&glview;InstrumentType"/>
    </owl:NamedIndividual>
    


    <!-- http://schema.geolink.org/dev/voc/nvs/L05#307 -->

    <owl:NamedIndividual rdf:about="&glvoc_l05;307">
        <rdf:type rdf:resource="&glview;InstrumentType"/>
    </owl:NamedIndividual>
    


    <!-- http://schema.geolink.org/dev/voc/nvs/L05#308 -->

    <owl:NamedIndividual rdf:about="&glvoc_l05;308">
        <rdf:type rdf:resource="&glview;InstrumentType"/>
    </owl:NamedIndividual>
    


    <!-- http://schema.geolink.org/dev/voc/nvs/L05#309 -->

    <owl:NamedIndividual rdf:about="&glvoc_l05;309">
        <rdf:type rdf:resource="&glview;InstrumentType"/>
    </owl:NamedIndividual>
    


    <!-- http://schema.geolink.org/dev/voc/nvs/L05#31 -->

    <owl:NamedIndividual rdf:about="&glvoc_l05;31">
        <rdf:type rdf:resource="&glview;InstrumentType"/>
    </owl:NamedIndividual>
    


    <!-- http://schema.geolink.org/dev/voc/nvs/L05#310 -->

    <owl:NamedIndividual rdf:about="&glvoc_l05;310">
        <rdf:type rdf:resource="&glview;InstrumentType"/>
    </owl:NamedIndividual>
    


    <!-- http://schema.geolink.org/dev/voc/nvs/L05#311 -->

    <owl:NamedIndividual rdf:about="&glvoc_l05;311">
        <rdf:type rdf:resource="&glview;InstrumentType"/>
    </owl:NamedIndividual>
    


    <!-- http://schema.geolink.org/dev/voc/nvs/L05#312 -->

    <owl:NamedIndividual rdf:about="&glvoc_l05;312">
        <rdf:type rdf:resource="&glview;InstrumentType"/>
    </owl:NamedIndividual>
    


    <!-- http://schema.geolink.org/dev/voc/nvs/L05#313 -->

    <owl:NamedIndividual rdf:about="&glvoc_l05;313">
        <rdf:type rdf:resource="&glview;InstrumentType"/>
    </owl:NamedIndividual>
    


    <!-- http://schema.geolink.org/dev/voc/nvs/L05#32 -->

    <owl:NamedIndividual rdf:about="&glvoc_l05;32">
        <rdf:type rdf:resource="&glview;InstrumentType"/>
    </owl:NamedIndividual>
    


    <!-- http://schema.geolink.org/dev/voc/nvs/L05#33 -->

    <owl:NamedIndividual rdf:about="&glvoc_l05;33">
        <rdf:type rdf:resource="&glview;InstrumentType"/>
    </owl:NamedIndividual>
    


    <!-- http://schema.geolink.org/dev/voc/nvs/L05#350 -->

    <owl:NamedIndividual rdf:about="&glvoc_l05;350">
        <rdf:type rdf:resource="&glview;InstrumentType"/>
    </owl:NamedIndividual>
    


    <!-- http://schema.geolink.org/dev/voc/nvs/L05#351 -->

    <owl:NamedIndividual rdf:about="&glvoc_l05;351">
        <rdf:type rdf:resource="&glview;InstrumentType"/>
    </owl:NamedIndividual>
    


    <!-- http://schema.geolink.org/dev/voc/nvs/L05#352 -->

    <owl:NamedIndividual rdf:about="&glvoc_l05;352">
        <rdf:type rdf:resource="&glview;InstrumentType"/>
    </owl:NamedIndividual>
    


    <!-- http://schema.geolink.org/dev/voc/nvs/L05#353 -->

    <owl:NamedIndividual rdf:about="&glvoc_l05;353">
        <rdf:type rdf:resource="&glview;InstrumentType"/>
    </owl:NamedIndividual>
    


    <!-- http://schema.geolink.org/dev/voc/nvs/L05#354 -->

    <owl:NamedIndividual rdf:about="&glvoc_l05;354">
        <rdf:type rdf:resource="&glview;InstrumentType"/>
    </owl:NamedIndividual>
    


    <!-- http://schema.geolink.org/dev/voc/nvs/L05#355 -->

    <owl:NamedIndividual rdf:about="&glvoc_l05;355">
        <rdf:type rdf:resource="&glview;InstrumentType"/>
    </owl:NamedIndividual>
    


    <!-- http://schema.geolink.org/dev/voc/nvs/L05#356 -->

    <owl:NamedIndividual rdf:about="&glvoc_l05;356">
        <rdf:type rdf:resource="&glview;InstrumentType"/>
    </owl:NamedIndividual>
    


    <!-- http://schema.geolink.org/dev/voc/nvs/L05#357 -->

    <owl:NamedIndividual rdf:about="&glvoc_l05;357">
        <rdf:type rdf:resource="&glview;InstrumentType"/>
    </owl:NamedIndividual>
    


    <!-- http://schema.geolink.org/dev/voc/nvs/L05#358 -->

    <owl:NamedIndividual rdf:about="&glvoc_l05;358">
        <rdf:type rdf:resource="&glview;InstrumentType"/>
    </owl:NamedIndividual>
    


    <!-- http://schema.geolink.org/dev/voc/nvs/L05#359 -->

    <owl:NamedIndividual rdf:about="&glvoc_l05;359">
        <rdf:type rdf:resource="&glview;InstrumentType"/>
    </owl:NamedIndividual>
    


    <!-- http://schema.geolink.org/dev/voc/nvs/L05#360 -->

    <owl:NamedIndividual rdf:about="&glvoc_l05;360">
        <rdf:type rdf:resource="&glview;InstrumentType"/>
    </owl:NamedIndividual>
    


    <!-- http://schema.geolink.org/dev/voc/nvs/L05#361 -->

    <owl:NamedIndividual rdf:about="&glvoc_l05;361">
        <rdf:type rdf:resource="&glview;InstrumentType"/>
    </owl:NamedIndividual>
    


    <!-- http://schema.geolink.org/dev/voc/nvs/L05#362 -->

    <owl:NamedIndividual rdf:about="&glvoc_l05;362">
        <rdf:type rdf:resource="&glview;InstrumentType"/>
    </owl:NamedIndividual>
    


    <!-- http://schema.geolink.org/dev/voc/nvs/L05#363 -->

    <owl:NamedIndividual rdf:about="&glvoc_l05;363">
        <rdf:type rdf:resource="&glview;InstrumentType"/>
    </owl:NamedIndividual>
    


    <!-- http://schema.geolink.org/dev/voc/nvs/L05#364 -->

    <owl:NamedIndividual rdf:about="&glvoc_l05;364">
        <rdf:type rdf:resource="&glview;InstrumentType"/>
    </owl:NamedIndividual>
    


    <!-- http://schema.geolink.org/dev/voc/nvs/L05#365 -->

    <owl:NamedIndividual rdf:about="&glvoc_l05;365">
        <rdf:type rdf:resource="&glview;InstrumentType"/>
    </owl:NamedIndividual>
    


    <!-- http://schema.geolink.org/dev/voc/nvs/L05#366 -->

    <owl:NamedIndividual rdf:about="&glvoc_l05;366">
        <rdf:type rdf:resource="&glview;InstrumentType"/>
    </owl:NamedIndividual>
    


    <!-- http://schema.geolink.org/dev/voc/nvs/L05#367 -->

    <owl:NamedIndividual rdf:about="&glvoc_l05;367">
        <rdf:type rdf:resource="&glview;InstrumentType"/>
    </owl:NamedIndividual>
    


    <!-- http://schema.geolink.org/dev/voc/nvs/L05#368 -->

    <owl:NamedIndividual rdf:about="&glvoc_l05;368">
        <rdf:type rdf:resource="&glview;InstrumentType"/>
    </owl:NamedIndividual>
    


    <!-- http://schema.geolink.org/dev/voc/nvs/L05#369 -->

    <owl:NamedIndividual rdf:about="&glvoc_l05;369">
        <rdf:type rdf:resource="&glview;InstrumentType"/>
    </owl:NamedIndividual>
    


    <!-- http://schema.geolink.org/dev/voc/nvs/L05#370 -->

    <owl:NamedIndividual rdf:about="&glvoc_l05;370">
        <rdf:type rdf:resource="&glview;InstrumentType"/>
    </owl:NamedIndividual>
    


    <!-- http://schema.geolink.org/dev/voc/nvs/L05#371 -->

    <owl:NamedIndividual rdf:about="&glvoc_l05;371">
        <rdf:type rdf:resource="&glview;InstrumentType"/>
    </owl:NamedIndividual>
    


    <!-- http://schema.geolink.org/dev/voc/nvs/L05#372 -->

    <owl:NamedIndividual rdf:about="&glvoc_l05;372">
        <rdf:type rdf:resource="&glview;InstrumentType"/>
    </owl:NamedIndividual>
    


    <!-- http://schema.geolink.org/dev/voc/nvs/L05#373 -->

    <owl:NamedIndividual rdf:about="&glvoc_l05;373">
        <rdf:type rdf:resource="&glview;InstrumentType"/>
    </owl:NamedIndividual>
    


    <!-- http://schema.geolink.org/dev/voc/nvs/L05#374 -->

    <owl:NamedIndividual rdf:about="&glvoc_l05;374">
        <rdf:type rdf:resource="&glview;InstrumentType"/>
    </owl:NamedIndividual>
    


    <!-- http://schema.geolink.org/dev/voc/nvs/L05#375 -->

    <owl:NamedIndividual rdf:about="&glvoc_l05;375">
        <rdf:type rdf:resource="&glview;InstrumentType"/>
    </owl:NamedIndividual>
    


    <!-- http://schema.geolink.org/dev/voc/nvs/L05#376 -->

    <owl:NamedIndividual rdf:about="&glvoc_l05;376">
        <rdf:type rdf:resource="&glview;InstrumentType"/>
    </owl:NamedIndividual>
    


    <!-- http://schema.geolink.org/dev/voc/nvs/L05#377 -->

    <owl:NamedIndividual rdf:about="&glvoc_l05;377">
        <rdf:type rdf:resource="&glview;InstrumentType"/>
    </owl:NamedIndividual>
    


    <!-- http://schema.geolink.org/dev/voc/nvs/L05#378 -->

    <owl:NamedIndividual rdf:about="&glvoc_l05;378">
        <rdf:type rdf:resource="&glview;InstrumentType"/>
    </owl:NamedIndividual>
    


    <!-- http://schema.geolink.org/dev/voc/nvs/L05#379 -->

    <owl:NamedIndividual rdf:about="&glvoc_l05;379">
        <rdf:type rdf:resource="&glview;InstrumentType"/>
    </owl:NamedIndividual>
    


    <!-- http://schema.geolink.org/dev/voc/nvs/L05#380 -->

    <owl:NamedIndividual rdf:about="&glvoc_l05;380">
        <rdf:type rdf:resource="&glview;InstrumentType"/>
    </owl:NamedIndividual>
    


    <!-- http://schema.geolink.org/dev/voc/nvs/L05#381 -->

    <owl:NamedIndividual rdf:about="&glvoc_l05;381">
        <rdf:type rdf:resource="&glview;InstrumentType"/>
    </owl:NamedIndividual>
    


    <!-- http://schema.geolink.org/dev/voc/nvs/L05#382 -->

    <owl:NamedIndividual rdf:about="&glvoc_l05;382">
        <rdf:type rdf:resource="&glview;InstrumentType"/>
    </owl:NamedIndividual>
    


    <!-- http://schema.geolink.org/dev/voc/nvs/L05#383 -->

    <owl:NamedIndividual rdf:about="&glvoc_l05;383">
        <rdf:type rdf:resource="&glview;InstrumentType"/>
    </owl:NamedIndividual>
    


    <!-- http://schema.geolink.org/dev/voc/nvs/L05#384 -->

    <owl:NamedIndividual rdf:about="&glvoc_l05;384">
        <rdf:type rdf:resource="&glview;InstrumentType"/>
    </owl:NamedIndividual>
    


    <!-- http://schema.geolink.org/dev/voc/nvs/L05#385 -->

    <owl:NamedIndividual rdf:about="&glvoc_l05;385">
        <rdf:type rdf:resource="&glview;InstrumentType"/>
    </owl:NamedIndividual>
    


    <!-- http://schema.geolink.org/dev/voc/nvs/L05#386 -->

    <owl:NamedIndividual rdf:about="&glvoc_l05;386">
        <rdf:type rdf:resource="&glview;InstrumentType"/>
    </owl:NamedIndividual>
    


    <!-- http://schema.geolink.org/dev/voc/nvs/L05#387 -->

    <owl:NamedIndividual rdf:about="&glvoc_l05;387">
        <rdf:type rdf:resource="&glview;InstrumentType"/>
    </owl:NamedIndividual>
    


    <!-- http://schema.geolink.org/dev/voc/nvs/L05#388 -->

    <owl:NamedIndividual rdf:about="&glvoc_l05;388">
        <rdf:type rdf:resource="&glview;InstrumentType"/>
    </owl:NamedIndividual>
    


    <!-- http://schema.geolink.org/dev/voc/nvs/L05#50 -->

    <owl:NamedIndividual rdf:about="&glvoc_l05;50">
        <rdf:type rdf:resource="&glview;InstrumentType"/>
    </owl:NamedIndividual>
    


    <!-- http://schema.geolink.org/dev/voc/nvs/L05#51 -->

    <owl:NamedIndividual rdf:about="&glvoc_l05;51">
        <rdf:type rdf:resource="&glview;InstrumentType"/>
    </owl:NamedIndividual>
    


    <!-- http://schema.geolink.org/dev/voc/nvs/L05#52 -->

    <owl:NamedIndividual rdf:about="&glvoc_l05;52">
        <rdf:type rdf:resource="&glview;InstrumentType"/>
    </owl:NamedIndividual>
    


    <!-- http://schema.geolink.org/dev/voc/nvs/L05#53 -->

    <owl:NamedIndividual rdf:about="&glvoc_l05;53">
        <rdf:type rdf:resource="&glview;InstrumentType"/>
    </owl:NamedIndividual>
    


    <!-- http://schema.geolink.org/dev/voc/nvs/L05#54 -->

    <owl:NamedIndividual rdf:about="&glvoc_l05;54">
        <rdf:type rdf:resource="&glview;InstrumentType"/>
    </owl:NamedIndividual>
    


    <!-- http://schema.geolink.org/dev/voc/nvs/L05#55 -->

    <owl:NamedIndividual rdf:about="&glvoc_l05;55">
        <rdf:type rdf:resource="&glview;InstrumentType"/>
    </owl:NamedIndividual>
    


    <!-- http://schema.geolink.org/dev/voc/nvs/L05#56 -->

    <owl:NamedIndividual rdf:about="&glvoc_l05;56">
        <rdf:type rdf:resource="&glview;InstrumentType"/>
    </owl:NamedIndividual>
    


    <!-- http://schema.geolink.org/dev/voc/nvs/L05#57 -->

    <owl:NamedIndividual rdf:about="&glvoc_l05;57">
        <rdf:type rdf:resource="&glview;InstrumentType"/>
    </owl:NamedIndividual>
    


    <!-- http://schema.geolink.org/dev/voc/nvs/L05#58 -->

    <owl:NamedIndividual rdf:about="&glvoc_l05;58">
        <rdf:type rdf:resource="&glview;InstrumentType"/>
    </owl:NamedIndividual>
    


    <!-- http://schema.geolink.org/dev/voc/nvs/L05#59 -->

    <owl:NamedIndividual rdf:about="&glvoc_l05;59">
        <rdf:type rdf:resource="&glview;InstrumentType"/>
    </owl:NamedIndividual>
    


    <!-- http://schema.geolink.org/dev/voc/nvs/L05#60 -->

    <owl:NamedIndividual rdf:about="&glvoc_l05;60">
        <rdf:type rdf:resource="&glview;InstrumentType"/>
    </owl:NamedIndividual>
    


    <!-- http://schema.geolink.org/dev/voc/nvs/L05#61 -->

    <owl:NamedIndividual rdf:about="&glvoc_l05;61">
        <rdf:type rdf:resource="&glview;InstrumentType"/>
    </owl:NamedIndividual>
    


    <!-- http://schema.geolink.org/dev/voc/nvs/L05#62 -->

    <owl:NamedIndividual rdf:about="&glvoc_l05;62">
        <rdf:type rdf:resource="&glview;InstrumentType"/>
    </owl:NamedIndividual>
    


    <!-- http://schema.geolink.org/dev/voc/nvs/L05#63 -->

    <owl:NamedIndividual rdf:about="&glvoc_l05;63">
        <rdf:type rdf:resource="&glview;InstrumentType"/>
    </owl:NamedIndividual>
    


    <!-- http://schema.geolink.org/dev/voc/nvs/L05#64 -->

    <owl:NamedIndividual rdf:about="&glvoc_l05;64">
        <rdf:type rdf:resource="&glview;InstrumentType"/>
    </owl:NamedIndividual>
    


    <!-- http://schema.geolink.org/dev/voc/nvs/L05#65 -->

    <owl:NamedIndividual rdf:about="&glvoc_l05;65">
        <rdf:type rdf:resource="&glview;InstrumentType"/>
    </owl:NamedIndividual>
    


    <!-- http://schema.geolink.org/dev/voc/nvs/L05#66 -->

    <owl:NamedIndividual rdf:about="&glvoc_l05;66">
        <rdf:type rdf:resource="&glview;InstrumentType"/>
    </owl:NamedIndividual>
    


    <!-- http://schema.geolink.org/dev/voc/nvs/L05#67 -->

    <owl:NamedIndividual rdf:about="&glvoc_l05;67">
        <rdf:type rdf:resource="&glview;InstrumentType"/>
    </owl:NamedIndividual>
    


    <!-- http://schema.geolink.org/dev/voc/nvs/L05#68 -->

    <owl:NamedIndividual rdf:about="&glvoc_l05;68">
        <rdf:type rdf:resource="&glview;InstrumentType"/>
    </owl:NamedIndividual>
    


    <!-- http://schema.geolink.org/dev/voc/nvs/L05#69 -->

    <owl:NamedIndividual rdf:about="&glvoc_l05;69">
        <rdf:type rdf:resource="&glview;InstrumentType"/>
    </owl:NamedIndividual>
    


    <!-- http://schema.geolink.org/dev/voc/nvs/L05#81 -->

    <owl:NamedIndividual rdf:about="&glvoc_l05;81">
        <rdf:type rdf:resource="&glview;InstrumentType"/>
    </owl:NamedIndividual>
    


    <!-- http://schema.geolink.org/dev/voc/nvs/L05#82 -->

    <owl:NamedIndividual rdf:about="&glvoc_l05;82">
        <rdf:type rdf:resource="&glview;InstrumentType"/>
    </owl:NamedIndividual>
    


    <!-- http://schema.geolink.org/dev/voc/nvs/L05#83 -->

    <owl:NamedIndividual rdf:about="&glvoc_l05;83">
        <rdf:type rdf:resource="&glview;InstrumentType"/>
    </owl:NamedIndividual>
    


    <!-- http://schema.geolink.org/dev/voc/nvs/L05#84 -->

    <owl:NamedIndividual rdf:about="&glvoc_l05;84">
        <rdf:type rdf:resource="&glview;InstrumentType"/>
    </owl:NamedIndividual>
    


    <!-- http://schema.geolink.org/dev/voc/nvs/L05#85 -->

    <owl:NamedIndividual rdf:about="&glvoc_l05;85">
        <rdf:type rdf:resource="&glview;InstrumentType"/>
    </owl:NamedIndividual>
    


    <!-- http://schema.geolink.org/dev/voc/nvs/L05#90 -->

    <owl:NamedIndividual rdf:about="&glvoc_l05;90">
        <rdf:type rdf:resource="&glview;InstrumentType"/>
    </owl:NamedIndividual>
    


    <!-- http://schema.geolink.org/dev/voc/nvs/L05#91 -->

    <owl:NamedIndividual rdf:about="&glvoc_l05;91">
        <rdf:type rdf:resource="&glview;InstrumentType"/>
    </owl:NamedIndividual>
    


    <!-- http://schema.geolink.org/dev/voc/nvs/L05#999 -->

    <owl:NamedIndividual rdf:about="&glvoc_l05;999">
        <rdf:type rdf:resource="&glview;InstrumentType"/>
    </owl:NamedIndividual>
    


    <!-- 
    ///////////////////////////////////////////////////////////////////////////////////////
    //
    // Annotations
    //
    ///////////////////////////////////////////////////////////////////////////////////////
     -->

    <rdf:Description rdf:about="&glvoc_l05;311">
        <rdfs:label xml:lang="en">cameras</rdfs:label>
        <rdfs:comment xml:lang="en">All types of photographic equipment that may be deployed in aircraft or satellites including stills, video, film and digital systems.</rdfs:comment>
        <rdfs:seeAlso rdf:resource="http://vocab.nerc.ac.uk/collection/L05/current/311/"/>
    </rdf:Description>
    <rdf:Description rdf:about="&glvoc_l05;SBAG">
        <rdfs:label xml:lang="en">single-bubble airgun</rdfs:label>
        <rdfs:comment xml:lang="en">Array of air gun tuned in order to obtain the necessary energy wile reducing the size of the air guns.</rdfs:comment>
        <rdfs:seeAlso rdf:resource="http://vocab.nerc.ac.uk/collection/L05/current/SBAG/"/>
    </rdf:Description>
    <rdf:Description rdf:about="&glvoc_l05;310">
        <rdfs:label xml:lang="en">laser altimeters</rdfs:label>
        <rdfs:comment xml:lang="en">Instruments that determine the distance between the platform and the Earth&apos;s surface by timing reflected pulses of laser light.</rdfs:comment>
        <rdfs:seeAlso rdf:resource="http://vocab.nerc.ac.uk/collection/L05/current/310/"/>
    </rdf:Description>
    <rdf:Description rdf:about="&glvoc_l05;313">
        <rdfs:label xml:lang="en">bird detection radars</rdfs:label>
        <rdfs:comment xml:lang="en">X-band and S-band radar systems developed for the detection, tracking and counting of birds in flight.</rdfs:comment>
        <rdfs:seeAlso rdf:resource="http://vocab.nerc.ac.uk/collection/L05/current/313/"/>
    </rdf:Description>
    <rdf:Description rdf:about="&glvoc_l05;312">
        <rdfs:label xml:lang="en">bathymetric LiDARs</rdfs:label>
        <rdfs:comment xml:lang="en">Instruments that measure the depth of a water body by determining the distances from the platform to the surface and the bed by timing reflected pulses of laser light.</rdfs:comment>
        <rdfs:seeAlso rdf:resource="http://vocab.nerc.ac.uk/collection/L05/current/312/"/>
    </rdf:Description>
    <rdf:Description rdf:about="&glvoc_l05;TFSAMP">
        <rdfs:label xml:lang="en">thin film metal samplers</rdfs:label>
        <rdfs:comment xml:lang="en">Metal samplers comprising a filter, a diffusive gel layer and a resin layer that scavenge trace metals by diffusion from water bodies or in-situ sediment pore waters. A constant concentration gradient is set up in the gel from which the metal concentration in the sampled medium may be determined.</rdfs:comment>
        <rdfs:seeAlso rdf:resource="http://vocab.nerc.ac.uk/collection/L05/current/TFSAMP/"/>
    </rdf:Description>
    <rdf:Description rdf:about="&glvoc_l05;WPS">
        <rdfs:label xml:lang="en">water pressure sensors</rdfs:label>
        <rdfs:comment xml:lang="en">Sensors measuring hydrostatic pressure that are capable of withstanding the physical demands made by in-situ measurements in water bodies. Depending upon the mode of deployment they may measure sea level, waves, mooring performance or the depth of a profiling instrument.</rdfs:comment>
        <rdfs:seeAlso rdf:resource="http://vocab.nerc.ac.uk/collection/L05/current/WPS/"/>
    </rdf:Description>
    <rdf:Description rdf:about="&glvoc_l05;BOMR">
        <rdfs:label xml:lang="en">Boomer</rdfs:label>
        <rdfs:comment xml:lang="en">A marine seismic energy source in which capacitors are charged to high voltage and then discharged through a transducer in the water. The transducer consists of a flat coil with a spring-loaded aluminium plate. Eddy currents force the plates to separate sharply, producing a low pressure region between the plates into which the water rushes generating a pressure wave by implosion.</rdfs:comment>
        <rdfs:seeAlso rdf:resource="http://vocab.nerc.ac.uk/collection/L05/current/BOMR/"/>
    </rdf:Description>
    <rdf:Description rdf:about="&glvoc_l05;55">
        <rdfs:label xml:lang="en">sediment settling tubes</rdfs:label>
        <rdfs:comment xml:lang="en">A specialised water bottle that both collects water samples and provides a settling velocity experiment apparatus.</rdfs:comment>
        <rdfs:seeAlso rdf:resource="http://vocab.nerc.ac.uk/collection/L05/current/55/"/>
    </rdf:Description>
    <rdf:Description rdf:about="&glvoc_l05;56">
        <rdfs:label xml:lang="en">snow and ice samplers</rdfs:label>
        <rdfs:comment xml:lang="en">A device that collects a sample of frozen seawater or accumulated frozen precipitation.</rdfs:comment>
        <rdfs:seeAlso rdf:resource="http://vocab.nerc.ac.uk/collection/L05/current/56/"/>
    </rdf:Description>
    <rdf:Description rdf:about="&glvoc_l05;53">
        <rdfs:label xml:lang="en">rock corers</rdfs:label>
        <rdfs:comment xml:lang="en">A device that drills into rock extracting a cylindrical sample.</rdfs:comment>
        <rdfs:seeAlso rdf:resource="http://vocab.nerc.ac.uk/collection/L05/current/53/"/>
    </rdf:Description>
    <rdf:Description rdf:about="&glvoc_l05;302">
        <rdfs:label xml:lang="en">water body temperature sensor</rdfs:label>
        <rdfs:comment xml:lang="en">Sensors that measure the intensity and nature of electromagnetic radiation emitted from the Earth in a manner optimised for the determination of water body surface temperature.</rdfs:comment>
        <rdfs:seeAlso rdf:resource="http://vocab.nerc.ac.uk/collection/L05/current/302/"/>
    </rdf:Description>
    <rdf:Description rdf:about="&glvoc_l05;301">
        <rdfs:label xml:lang="en">satellite positioning systems</rdfs:label>
        <rdfs:comment xml:lang="en">A network of statellites that generate signals that allow a receiver to determine its position such as GPS.</rdfs:comment>
        <rdfs:seeAlso rdf:resource="http://vocab.nerc.ac.uk/collection/L05/current/301/"/>
    </rdf:Description>
    <rdf:Description rdf:about="&glvoc_l05;54">
        <rdfs:label xml:lang="en">rock dredges</rdfs:label>
        <rdfs:comment xml:lang="en">A device dragged across the seabed designed to collect loose rock samples.</rdfs:comment>
        <rdfs:seeAlso rdf:resource="http://vocab.nerc.ac.uk/collection/L05/current/54/"/>
    </rdf:Description>
    <rdf:Description rdf:about="&glvoc_l05;51">
        <rdfs:label xml:lang="en">unconsolidated sediment corers</rdfs:label>
        <rdfs:comment xml:lang="en">Devices designed to collect samples of unconsolidated sediment from between the surface and depths from centimetres to 10s of metres with minimal disturbance of the sediment structure.</rdfs:comment>
        <rdfs:seeAlso rdf:resource="http://vocab.nerc.ac.uk/collection/L05/current/51/"/>
    </rdf:Description>
    <rdf:Description rdf:about="&glvoc_l05;52">
        <rdfs:label xml:lang="en">sediment porewater samplers</rdfs:label>
        <rdfs:comment xml:lang="en">A device that collects samples of pore water from various horizons below the seabed.</rdfs:comment>
        <rdfs:seeAlso rdf:resource="http://vocab.nerc.ac.uk/collection/L05/current/52/"/>
    </rdf:Description>
    <rdf:Description rdf:about="&glvoc_l05;50">
        <rdfs:label xml:lang="en">sediment grabs</rdfs:label>
        <rdfs:comment xml:lang="en">A device that collects a sample of surface sediment including manually deployed equipment like a shovel or bucket.</rdfs:comment>
        <rdfs:seeAlso rdf:resource="http://vocab.nerc.ac.uk/collection/L05/current/50/"/>
    </rdf:Description>
    <rdf:Description rdf:about="&glvoc_l05;308">
        <rdfs:label xml:lang="en">atmospheric radiometers</rdfs:label>
        <rdfs:comment xml:lang="en">Sensors that measure the intensity an nature of electromagnetic radiation in a manner optimised for the quantification of atmospheric phenomena.</rdfs:comment>
        <rdfs:seeAlso rdf:resource="http://vocab.nerc.ac.uk/collection/L05/current/308/"/>
    </rdf:Description>
    <rdf:Description rdf:about="&glvoc_l05;307">
        <rdfs:label xml:lang="en">accelerometers</rdfs:label>
        <rdfs:comment xml:lang="en">Instruments that measure non-gravitational accelerations acting upon a spacecraft.</rdfs:comment>
        <rdfs:seeAlso rdf:resource="http://vocab.nerc.ac.uk/collection/L05/current/307/"/>
    </rdf:Description>
    <rdf:Description rdf:about="&glvoc_l05;309">
        <rdfs:label xml:lang="en">terrestrial radiometers</rdfs:label>
        <rdfs:comment xml:lang="en">Sensors that measure the intensity and nature of electromagnetic radiation in a manner optimised for the quantification of terrestrial phenomena.</rdfs:comment>
        <rdfs:seeAlso rdf:resource="http://vocab.nerc.ac.uk/collection/L05/current/309/"/>
    </rdf:Description>
    <rdf:Description rdf:about="&glvoc_l05;304">
        <rdfs:label xml:lang="en">ocean colour radiometers</rdfs:label>
        <rdfs:comment xml:lang="en">Sensors that measure the intensity and nature of electromagnetic radiation in a manner optimised for the determination of ocean chlorophyll concentration.</rdfs:comment>
        <rdfs:seeAlso rdf:resource="http://vocab.nerc.ac.uk/collection/L05/current/304/"/>
    </rdf:Description>
    <rdf:Description rdf:about="&glvoc_l05;303">
        <rdfs:label xml:lang="en">surface current radars</rdfs:label>
        <rdfs:comment xml:lang="en">Instruments that measure the speed and direction of sea surface travel by timing reflected radio waves.</rdfs:comment>
        <rdfs:seeAlso rdf:resource="http://vocab.nerc.ac.uk/collection/L05/current/303/"/>
    </rdf:Description>
    <rdf:Description rdf:about="&glvoc_l05;306">
        <rdfs:label xml:lang="en">synthetic aperture radars</rdfs:label>
        <rdfs:comment xml:lang="en">Instruments that generate maps of radar reflectivity through the synthesis of multiple pulses from a moving platform.</rdfs:comment>
        <rdfs:seeAlso rdf:resource="http://vocab.nerc.ac.uk/collection/L05/current/306/"/>
    </rdf:Description>
    <rdf:Description rdf:about="&glvoc_l05;305">
        <rdfs:label xml:lang="en">scatterometers</rdfs:label>
        <rdfs:comment xml:lang="en">Sensors that measure the reflection or scattering effect produced while scanning the surface of the earth. Primarily used to measure near surface winds over the oceans.</rdfs:comment>
        <rdfs:seeAlso rdf:resource="http://vocab.nerc.ac.uk/collection/L05/current/305/"/>
    </rdf:Description>
    <rdf:Description rdf:about="&glvoc_l05;LAB43">
        <rdfs:label xml:lang="en">plate readers</rdfs:label>
        <rdfs:comment xml:lang="en">Laboratory instruments detect biological, chemical or physical events in samples held in multiple (typically 6, 24, 96, 384 or 1536) wells arranged in a matrix in a flat plate. Samples in the plate wells are simultaneously assayed optically using techniques such as spectrophotometry or spectrofluorometry.</rdfs:comment>
        <rdfs:seeAlso rdf:resource="http://vocab.nerc.ac.uk/collection/L05/current/LAB43/"/>
    </rdf:Description>
    <rdf:Description rdf:about="&glvoc_l05;LAB44">
        <rdfs:label xml:lang="en">refractometers</rdfs:label>
        <rdfs:comment xml:lang="en">Instruments that measure the refractive index of a sample.</rdfs:comment>
        <rdfs:seeAlso rdf:resource="http://vocab.nerc.ac.uk/collection/L05/current/LAB44/"/>
    </rdf:Description>
    <rdf:Description rdf:about="&glvoc_l05;LAB41">
        <rdfs:label xml:lang="en">laboratory cameras</rdfs:label>
        <rdfs:comment xml:lang="en">All types of photographic equipment that are hand-held or part of laboratory apparatus including stills, video, film and digital systems.</rdfs:comment>
        <rdfs:seeAlso rdf:resource="http://vocab.nerc.ac.uk/collection/L05/current/LAB41/"/>
    </rdf:Description>
    <rdf:Description rdf:about="&glvoc_l05;LAB42">
        <rdfs:label xml:lang="en">laboratory optical rangefinders</rdfs:label>
        <rdfs:comment xml:lang="en">Devices used to detect the distance between sensor and sample or presence/absence of an object based a light (often infrared and possibly laser) transmitter and a photoelectric receiver.</rdfs:comment>
        <rdfs:seeAlso rdf:resource="http://vocab.nerc.ac.uk/collection/L05/current/LAB42/"/>
    </rdf:Description>
    <rdf:Description rdf:about="&glvoc_l05;MMIS">
        <rdfs:label xml:lang="en">multi-frame imaging sonar</rdfs:label>
        <rdfs:comment xml:lang="en">High-frequency (&gt;1 MHz), possibly multiple frequency, active sonar systems that provide images approaching the same quality as optical video cameras. They may be deployed in many ways including hand-held by divers, attached to profiling instruments, AUVs and ROVs, towed fish or moorings.  They have many scientific, commercial and military applications including observation and identification of fish, seabed characterisation, underwater vessel inspections and mine detection. Examples of this type of system are DIDSON (Dual-frequency IDentification SONar) and LIMIS (Limpet Mine Imaging Sonar).  Any instrument that may be considered the underwater acoustic equivalent of an optical video camera belongs in this category.</rdfs:comment>
        <rdfs:seeAlso rdf:resource="http://vocab.nerc.ac.uk/collection/L05/current/MMIS/"/>
    </rdf:Description>
    <rdf:Description rdf:about="&glvoc_l05;LAB40">
        <rdfs:label xml:lang="en">Volume measures</rdfs:label>
        <rdfs:comment xml:lang="en">Pieces of apparatus that determine the volume of a liquid sample or dispense measured volumes of liquid. Includes devices covering a wide range of sophistication from measuring cylinders, syringes and manual pipettes through to programmable electronic instruments.</rdfs:comment>
        <rdfs:seeAlso rdf:resource="http://vocab.nerc.ac.uk/collection/L05/current/LAB40/"/>
    </rdf:Description>
    <rdf:Description rdf:about="&glvoc_l05;BLUMS">
        <rdfs:label xml:lang="en">bioluminescence sensors</rdfs:label>
        <rdfs:comment xml:lang="en">Submersible instruments which measure visible emissions from bioluminescent organisms by stimulating intracellular chemiluminescence through mechanical-stressors, such as turbulent water-flow, and sensing by photodetectors, such as photodiodes or photomultiplier tubes. Excludes bioluminescence biosensors which detect the presence of target chemicals or compounds using engineered-bioluminescent bacteria.</rdfs:comment>
        <rdfs:seeAlso rdf:resource="http://vocab.nerc.ac.uk/collection/L05/current/BLUMS/"/>
    </rdf:Description>
    <rdf:Description rdf:about="&glvoc_l05;POS18">
        <rdfs:label xml:lang="en">Navy Navigation Satellite System receivers</rdfs:label>
        <rdfs:comment xml:lang="en">{
  &quot;mode&quot;: &quot;Doppler-derived localisation&quot;,
  &quot;accuracy&quot;: &quot;better than 10km or 2km if combined with relative water velocity em-log&quot;,
  &quot;#text&quot;: &quot;.&quot;
}</rdfs:comment>
        <rdfs:seeAlso rdf:resource="http://vocab.nerc.ac.uk/collection/L05/current/POS18/"/>
    </rdf:Description>
    <rdf:Description rdf:about="&glvoc_l05;66">
        <rdfs:label xml:lang="en">flushing drills</rdfs:label>
        <rdfs:comment xml:lang="en">Devices primarily designed to drill wells through sediment or rock that flush the drill spoil back to the surface where it is examined to provide lithological data through the process known as mud logging.</rdfs:comment>
        <rdfs:seeAlso rdf:resource="http://vocab.nerc.ac.uk/collection/L05/current/66/"/>
    </rdf:Description>
    <rdf:Description rdf:about="&glvoc_l05;POS17">
        <rdfs:label xml:lang="en">Argos doppler-localised transmitters</rdfs:label>
        <rdfs:comment xml:lang="en">{
  &quot;mode&quot;: &quot;Doppler-derived Argos localisation&quot;,
  &quot;accuracy&quot;: &quot;better than 250m (class 3) to worse than 1500m (class 0)&quot;,
  &quot;#text&quot;: &quot;.&quot;
}</rdfs:comment>
        <rdfs:seeAlso rdf:resource="http://vocab.nerc.ac.uk/collection/L05/current/POS17/"/>
    </rdf:Description>
    <rdf:Description rdf:about="&glvoc_l05;67">
        <rdfs:label xml:lang="en">high-speed plankton samplers</rdfs:label>
        <rdfs:comment xml:lang="en">A fine-meshed net or filter towed behind a moving vessel that collects a single sample for a tow. Samples microzooplankton, mesozooplankton and nekton.</rdfs:comment>
        <rdfs:seeAlso rdf:resource="http://vocab.nerc.ac.uk/collection/L05/current/67/"/>
    </rdf:Description>
    <rdf:Description rdf:about="&glvoc_l05;64">
        <rdfs:label xml:lang="en">active fishing gear</rdfs:label>
        <rdfs:comment xml:lang="en">Apparatus where capture is based on chasing the target species (e.g. a trawl).</rdfs:comment>
        <rdfs:seeAlso rdf:resource="http://vocab.nerc.ac.uk/collection/L05/current/64/"/>
    </rdf:Description>
    <rdf:Description rdf:about="&glvoc_l05;65">
        <rdfs:label xml:lang="en">gill nets</rdfs:label>
        <rdfs:comment xml:lang="en">Nets drifting in the sea or standing on the sea floor in which fish become entangled, usually through their gill covers.</rdfs:comment>
        <rdfs:seeAlso rdf:resource="http://vocab.nerc.ac.uk/collection/L05/current/65/"/>
    </rdf:Description>
    <rdf:Description rdf:about="&glvoc_l05;VSHC">
        <rdfs:label xml:lang="en">Vaporchoc</rdfs:label>
        <rdfs:comment xml:lang="en">A marine seismic energy source in which a quantity of superheated steam under high pressure is iniected into water. Subsequent condensation of the steam attenuates bubble oscillation.</rdfs:comment>
        <rdfs:seeAlso rdf:resource="http://vocab.nerc.ac.uk/collection/L05/current/VSHC/"/>
    </rdf:Description>
    <rdf:Description rdf:about="&glvoc_l05;POS19">
        <rdfs:label xml:lang="en">inertial navigation systems</rdfs:label>
        <rdfs:comment xml:lang="en">{
  &quot;notes&quot;: &quot;Systems that determine spatial position using high-accuracy inertial measurements plus input from other sensors such as doppler current sensors to determine platform 3-D location by interpolation between satellite network fixes.&quot;,
  &quot;#text&quot;: &quot;.&quot;
}</rdfs:comment>
        <rdfs:seeAlso rdf:resource="http://vocab.nerc.ac.uk/collection/L05/current/POS19/"/>
    </rdf:Description>
    <rdf:Description rdf:about="&glvoc_l05;62">
        <rdfs:label xml:lang="en">beam trawls</rdfs:label>
        <rdfs:comment xml:lang="en">Nets towed over the sea floor having the horizontal net opening provided by a wooden or metal beam that disrupts the surface of the bed.</rdfs:comment>
        <rdfs:seeAlso rdf:resource="http://vocab.nerc.ac.uk/collection/L05/current/62/"/>
    </rdf:Description>
    <rdf:Description rdf:about="&glvoc_l05;63">
        <rdfs:label xml:lang="en">passive fishing gear</rdfs:label>
        <rdfs:comment xml:lang="en">Apparatus where capture is based on the movement of the target species towards the gear (e.g. creels and fish traps).</rdfs:comment>
        <rdfs:seeAlso rdf:resource="http://vocab.nerc.ac.uk/collection/L05/current/63/"/>
    </rdf:Description>
    <rdf:Description rdf:about="&glvoc_l05;60">
        <rdfs:label xml:lang="en">sediment dredges</rdfs:label>
        <rdfs:comment xml:lang="en">Bucket-like containers hauled over the sea bed collecting integrated samples of surface sediment along a segment of ship track.</rdfs:comment>
        <rdfs:seeAlso rdf:resource="http://vocab.nerc.ac.uk/collection/L05/current/60/"/>
    </rdf:Description>
    <rdf:Description rdf:about="&glvoc_l05;61">
        <rdfs:label xml:lang="en">demersal trawl nets</rdfs:label>
        <rdfs:comment xml:lang="en">Nets towed over the sea floor designed to sample species living on or near the bottom.</rdfs:comment>
        <rdfs:seeAlso rdf:resource="http://vocab.nerc.ac.uk/collection/L05/current/61/"/>
    </rdf:Description>
    <rdf:Description rdf:about="&glvoc_l05;POS10">
        <rdfs:label xml:lang="en">Automatic Ranging Grid Overlay DM 54 receivers</rdfs:label>
        <rdfs:comment xml:lang="en">{
  &quot;frequency&quot;: &quot;1.6-2MHz&quot;,
  &quot;mode&quot;: &quot;hyperbolic&quot;,
  &quot;range&quot;: &quot;450km&quot;,
  &quot;accuracy&quot;: &quot;4-7m down to 20m at maximum range&quot;,
  &quot;operational&quot;: &quot;from 1977 (mid-80s in Europe)&quot;,
  &quot;notes&quot;: &quot;Survey positioning system.&quot;,
  &quot;#text&quot;: &quot;.&quot;
}</rdfs:comment>
        <rdfs:seeAlso rdf:resource="http://vocab.nerc.ac.uk/collection/L05/current/POS10/"/>
    </rdf:Description>
    <rdf:Description rdf:about="&glvoc_l05;POS12">
        <rdfs:label xml:lang="en">Systme leger de measure de distance receivers</rdfs:label>
        <rdfs:comment xml:lang="en">{
  &quot;frequency&quot;: &quot;420-450MHz&quot;,
  &quot;mode&quot;: &quot;hyperbolic or circular&quot;,
  &quot;range&quot;: &quot;400km hyperbolic; 75-100km circular&quot;,
  &quot;accuracy&quot;: &quot;better than 2m below horizon (10m above horizon)&quot;,
  &quot;operational&quot;: &quot;1980s to 1995&quot;,
  &quot;notes&quot;: &quot;Navigation and positioning system for the North Sea petroleum industry.&quot;,
  &quot;#text&quot;: &quot;.&quot;
}</rdfs:comment>
        <rdfs:seeAlso rdf:resource="http://vocab.nerc.ac.uk/collection/L05/current/POS12/"/>
    </rdf:Description>
    <rdf:Description rdf:about="&glvoc_l05;LAB38">
        <rdfs:label xml:lang="en">cavity enhanced absorption spectrometers</rdfs:label>
        <rdfs:comment xml:lang="en">Instruments that illuminate a sample inside an optical cavity, typically using laser light, and measure the concentration or amount of a species in gas phase by absorption spectroscopy. Techniques include cavity ring-down spectroscopy (CRDS) and integrated cavity output spectroscopy (ICOS).</rdfs:comment>
        <rdfs:seeAlso rdf:resource="http://vocab.nerc.ac.uk/collection/L05/current/LAB38/"/>
    </rdf:Description>
    <rdf:Description rdf:about="&glvoc_l05;POS11">
        <rdfs:label xml:lang="en">Trident receivers</rdfs:label>
        <rdfs:comment xml:lang="en">{
  &quot;frequency&quot;: &quot;420-450MHz&quot;,
  &quot;mode&quot;: &quot;circular&quot;,
  &quot;range&quot;: &quot;150km&quot;,
  &quot;accuracy&quot;: &quot;better than 3m&quot;,
  &quot;notes&quot;: &quot;Survey positioning system.&quot;,
  &quot;#text&quot;: &quot;.&quot;
}</rdfs:comment>
        <rdfs:seeAlso rdf:resource="http://vocab.nerc.ac.uk/collection/L05/current/POS11/"/>
    </rdf:Description>
    <rdf:Description rdf:about="&glvoc_l05;LAB39">
        <rdfs:label xml:lang="en">Geiger counters</rdfs:label>
        <rdfs:comment xml:lang="en">Instruments that measure the amount of alpha, beta or gamma radiation through quantification of the ionization of a low-pressure gas contained in a tube. Sometimes referred to as Geiger-Mller counters.</rdfs:comment>
        <rdfs:seeAlso rdf:resource="http://vocab.nerc.ac.uk/collection/L05/current/LAB39/"/>
    </rdf:Description>
    <rdf:Description rdf:about="&glvoc_l05;POS14">
        <rdfs:label xml:lang="en">Pulse8 receivers</rdfs:label>
        <rdfs:comment xml:lang="en">{
  &quot;frequency&quot;: &quot;100kHz&quot;,
  &quot;mode&quot;: &quot;hyperbolic&quot;,
  &quot;range&quot;: &quot;250km to 750km&quot;,
  &quot;accuracy&quot;: &quot;30m to 500m&quot;,
  &quot;operational&quot;: &quot;1970s to late 1990s&quot;,
  &quot;#text&quot;: &quot;.&quot;
}</rdfs:comment>
        <rdfs:seeAlso rdf:resource="http://vocab.nerc.ac.uk/collection/L05/current/POS14/"/>
    </rdf:Description>
    <rdf:Description rdf:about="&glvoc_l05;POS13">
        <rdfs:label xml:lang="en">Rana receivers</rdfs:label>
        <rdfs:comment xml:lang="en">{
  &quot;frequency&quot;: &quot;around 300-400kHz&quot;,
  &quot;mode&quot;: &quot;hyperbolic&quot;,
  &quot;#text&quot;: &quot;.&quot;
}</rdfs:comment>
        <rdfs:seeAlso rdf:resource="http://vocab.nerc.ac.uk/collection/L05/current/POS13/"/>
    </rdf:Description>
    <rdf:Description rdf:about="&glvoc_l05;POS16">
        <rdfs:label xml:lang="en">Argos GPS-localised transmitters</rdfs:label>
        <rdfs:comment xml:lang="en">{
  &quot;mode&quot;: &quot;GPS localisation&quot;,
  &quot;accuracy&quot;: &quot;better than 100m&quot;,
  &quot;#text&quot;: &quot;.&quot;
}</rdfs:comment>
        <rdfs:seeAlso rdf:resource="http://vocab.nerc.ac.uk/collection/L05/current/POS16/"/>
    </rdf:Description>
    <rdf:Description rdf:about="&glvoc_l05;POS15">
        <rdfs:label xml:lang="en">Omega receivers</rdfs:label>
        <rdfs:comment xml:lang="en">{
  &quot;frequency&quot;: &quot;10-14kHz&quot;,
  &quot;mode&quot;: &quot;hyperbolic&quot;,
  &quot;range&quot;: &quot;up to 15000km&quot;,
  &quot;accuracy&quot;: &quot;better than 7.4km&quot;,
  &quot;operational&quot;: &quot;1968-1997&quot;,
  &quot;notes&quot;: &quot;Global long-range but low accuracy navigation system&quot;,
  &quot;#text&quot;: &quot;.&quot;
}</rdfs:comment>
        <rdfs:seeAlso rdf:resource="http://vocab.nerc.ac.uk/collection/L05/current/POS15/"/>
    </rdf:Description>
    <rdf:Description rdf:about="&glvoc_l05;LAB32">
        <rdfs:label xml:lang="en">acoustic velocity systems</rdfs:label>
        <rdfs:comment xml:lang="en">Instruments that measure the speed or velocity of sound, including P-waves, in samples of solids, liquids or gases.</rdfs:comment>
        <rdfs:seeAlso rdf:resource="http://vocab.nerc.ac.uk/collection/L05/current/LAB32/"/>
    </rdf:Description>
    <rdf:Description rdf:about="&glvoc_l05;LAB33">
        <rdfs:label xml:lang="en">laboratory autosamplers</rdfs:label>
        <rdfs:comment xml:lang="en">Laboratory apparatus  that automatically introduces one or more samples with a predetermined volume or mass into an analytical instrument.</rdfs:comment>
        <rdfs:seeAlso rdf:resource="http://vocab.nerc.ac.uk/collection/L05/current/LAB33/"/>
    </rdf:Description>
    <rdf:Description rdf:about="&glvoc_l05;LAB30">
        <rdfs:label xml:lang="en">salinometers</rdfs:label>
        <rdfs:comment xml:lang="en">Instruments that measure the salinity of a collected water sample based on its electrical conductivity or optical properties.</rdfs:comment>
        <rdfs:seeAlso rdf:resource="http://vocab.nerc.ac.uk/collection/L05/current/LAB30/"/>
    </rdf:Description>
    <rdf:Description rdf:about="&glvoc_l05;LAB31">
        <rdfs:label xml:lang="en">magnetic susceptibility systems</rdfs:label>
        <rdfs:comment xml:lang="en">Sensors, probes and meters that measure the degree to which a sample or part thereof is influenced by a magnetic field.</rdfs:comment>
        <rdfs:seeAlso rdf:resource="http://vocab.nerc.ac.uk/collection/L05/current/LAB31/"/>
    </rdf:Description>
    <rdf:Description rdf:about="&glvoc_l05;LAB36">
        <rdfs:label xml:lang="en">flow injection analysers</rdfs:label>
        <rdfs:comment xml:lang="en">Instruments that inject a sample into a flowing carrier solution, adding reagents whilst controlling the environment to produce a chemical reaction before passing the sample to a detector.</rdfs:comment>
        <rdfs:seeAlso rdf:resource="http://vocab.nerc.ac.uk/collection/L05/current/LAB36/"/>
    </rdf:Description>
    <rdf:Description rdf:about="&glvoc_l05;LAB37">
        <rdfs:label xml:lang="en">flow cytometers</rdfs:label>
        <rdfs:comment xml:lang="en">Instruments that suspend cells in a stream of fluid past detection sensors whilst illuminating them with laser light. Used for cell counting, sorting, biomarker detection and protein engineering.</rdfs:comment>
        <rdfs:seeAlso rdf:resource="http://vocab.nerc.ac.uk/collection/L05/current/LAB37/"/>
    </rdf:Description>
    <rdf:Description rdf:about="&glvoc_l05;LAB34">
        <rdfs:label xml:lang="en">chemiluminescence analysers</rdfs:label>
        <rdfs:comment xml:lang="en">Laboratory apparatus that detemines the concentration of a chemical species by quantification of the electromagnetic radiation (usually visible light) produced by a chemical reaction.</rdfs:comment>
        <rdfs:seeAlso rdf:resource="http://vocab.nerc.ac.uk/collection/L05/current/LAB34/"/>
    </rdf:Description>
    <rdf:Description rdf:about="&glvoc_l05;LBTG">
        <rdfs:label xml:lang="en">labelling tags</rdfs:label>
        <rdfs:comment xml:lang="en">Passive devices attached to captured organisms to specifically identify them when recaptured after release.</rdfs:comment>
        <rdfs:seeAlso rdf:resource="http://vocab.nerc.ac.uk/collection/L05/current/LBTG/"/>
    </rdf:Description>
    <rdf:Description rdf:about="&glvoc_l05;LAB35">
        <rdfs:label xml:lang="en">voltammetry analysers</rdfs:label>
        <rdfs:comment xml:lang="en">Instruments that obtain information about an analyte by applying a potential and measuring the current produced in the analyte.</rdfs:comment>
        <rdfs:seeAlso rdf:resource="http://vocab.nerc.ac.uk/collection/L05/current/LAB35/"/>
    </rdf:Description>
    <rdf:Description rdf:about="&glvoc_l05;SNWG">
        <rdfs:label xml:lang="en">watergun</rdfs:label>
        <rdfs:comment xml:lang="en">A marine seismic energy source divided into two chambers, the firing chamber, which contains compressed air, and the other chamber, which is filled with water. When the gun is fired, the compressed air forces the shuttle downward and this expels the water from the lower chamber. The shot of water leaving the gun creates a void behind it and the collapse of water into this void creates an acoustic wave.</rdfs:comment>
        <rdfs:seeAlso rdf:resource="http://vocab.nerc.ac.uk/collection/L05/current/SNWG/"/>
    </rdf:Description>
    <rdf:Description rdf:about="&glvoc_l05;59">
        <rdfs:label xml:lang="en">sampling extent markers</rdfs:label>
        <rdfs:comment xml:lang="en">Devices that label the region within which sampling is to be confined such as permanent quadrats and location markers.</rdfs:comment>
        <rdfs:seeAlso rdf:resource="http://vocab.nerc.ac.uk/collection/L05/current/59/"/>
    </rdf:Description>
    <rdf:Description rdf:about="&glvoc_l05;57">
        <rdfs:label xml:lang="en">manual rock samplers</rdfs:label>
        <rdfs:comment xml:lang="en">A simple tool like a hammer, saw or even just a hand for the collection of rock samples.</rdfs:comment>
        <rdfs:seeAlso rdf:resource="http://vocab.nerc.ac.uk/collection/L05/current/57/"/>
    </rdf:Description>
    <rdf:Description rdf:about="&glvoc_l05;58">
        <rdfs:label xml:lang="en">continuous air samplers</rdfs:label>
        <rdfs:comment xml:lang="en">A device that continuously supplies a flow of air either to an analytical instrument, over a sensor or from which discrete samples may be drawn.</rdfs:comment>
        <rdfs:seeAlso rdf:resource="http://vocab.nerc.ac.uk/collection/L05/current/58/"/>
    </rdf:Description>
    <rdf:Description rdf:about="&glvoc_l05;POS07">
        <rdfs:label xml:lang="en">Sextants</rdfs:label>
        <rdfs:comment xml:lang="en">{
  &quot;notes&quot;: &quot;Optical instruments that accurately measure the angle between pairs of visible celestial bodies such as the sun, moon or stars. &quot;,
  &quot;#text&quot;: &quot;.&quot;
}</rdfs:comment>
        <rdfs:seeAlso rdf:resource="http://vocab.nerc.ac.uk/collection/L05/current/POS07/"/>
    </rdf:Description>
    <rdf:Description rdf:about="&glvoc_l05;POS06">
        <rdfs:label xml:lang="en">Marine chronometers</rdfs:label>
        <rdfs:comment xml:lang="en">{
  &quot;notes&quot;: &quot;Timepieces of sufficient precision to allow their use of portable time standards.&quot;,
  &quot;#text&quot;: &quot;.&quot;
}</rdfs:comment>
        <rdfs:seeAlso rdf:resource="http://vocab.nerc.ac.uk/collection/L05/current/POS06/"/>
    </rdf:Description>
    <rdf:Description rdf:about="&glvoc_l05;POS09">
        <rdfs:label xml:lang="en">Toran receivers</rdfs:label>
        <rdfs:comment xml:lang="en">{
  &quot;frequency&quot;: &quot;around 2MHz&quot;,
  &quot;mode&quot;: &quot;hyperbolic&quot;,
  &quot;range&quot;: &quot;150-200km&quot;,
  &quot;accuracy&quot;: &quot;better than 20m&quot;,
  &quot;notes&quot;: &quot;Mostly used for aircraft.&quot;,
  &quot;#text&quot;: &quot;.&quot;
}</rdfs:comment>
        <rdfs:seeAlso rdf:resource="http://vocab.nerc.ac.uk/collection/L05/current/POS09/"/>
    </rdf:Description>
    <rdf:Description rdf:about="&glvoc_l05;POS08">
        <rdfs:label xml:lang="en">Decca Navigator System HiFix receivers</rdfs:label>
        <rdfs:comment xml:lang="en">{
  &quot;frequency&quot;: &quot;1.6MHz&quot;,
  &quot;mode&quot;: &quot;hyperbolic&quot;,
  &quot;range&quot;: &quot;under 100km&quot;,
  &quot;accuracy&quot;: &quot;better than 10m: maximum accuracy at 50km range is 1.5m&quot;,
  &quot;operating&quot;: &quot;1962 to 2000&quot;,
  &quot;notes&quot;: &quot;Not for general navigation.  Chains usually set up for specific surveys.&quot;,
  &quot;#text&quot;: &quot;.&quot;
}</rdfs:comment>
        <rdfs:seeAlso rdf:resource="http://vocab.nerc.ac.uk/collection/L05/current/POS08/"/>
    </rdf:Description>
    <rdf:Description rdf:about="&glvoc_l05;GIAG">
        <rdfs:label xml:lang="en">GI-gun</rdfs:label>
        <rdfs:comment xml:lang="en">A marine seismic source where a pair of conventional airguns (one, the generator, fires in the conventional manner; the second, known as the injector) fires some milliseconds later to prevent bubble from collapsing. Could be used in true GI mode (volume of injector twice of volume of generator), harmonic mode (same volume of generator and injector) or true airgun (no delay between generator and injector).</rdfs:comment>
        <rdfs:seeAlso rdf:resource="http://vocab.nerc.ac.uk/collection/L05/current/GIAG/"/>
    </rdf:Description>
    <rdf:Description rdf:about="&glvoc_l05;LAB29">
        <rdfs:label xml:lang="en">rulers</rdfs:label>
        <rdfs:comment xml:lang="en">Devices that allow one or more physical dimensions of a sample or specimen to be determined by visible comparison against marked graduations in units of measurement of dimension length.</rdfs:comment>
        <rdfs:seeAlso rdf:resource="http://vocab.nerc.ac.uk/collection/L05/current/LAB29/"/>
    </rdf:Description>
    <rdf:Description rdf:about="&glvoc_l05;POS01">
        <rdfs:label xml:lang="en">Decca Navigator System main chain receivers</rdfs:label>
        <rdfs:comment xml:lang="en">{
  &quot;frequency&quot;: &quot;70 and 130kHz&quot;,
  &quot;mode&quot;: &quot;hyperbolic&quot;,
  &quot;range&quot;: &quot;450km (day) to 750km (night)&quot;,
  &quot;accuracy&quot;: &quot;50m(day) to 200m (night) in good conditions down to 2km near range limit&quot;,
  &quot;operating&quot;: &quot;WWII to 2001-03 (2000-03-31 in UK)&quot;,
  &quot;notes&quot;: &quot; Transmitter groups, each with a master and three slaves&quot;,
  &quot;#text&quot;: &quot;.&quot;
}</rdfs:comment>
        <rdfs:seeAlso rdf:resource="http://vocab.nerc.ac.uk/collection/L05/current/POS01/"/>
    </rdf:Description>
    <rdf:Description rdf:about="&glvoc_l05;LAB27">
        <rdfs:label xml:lang="en">particle sizers</rdfs:label>
        <rdfs:comment xml:lang="en">Instruments that measure the size spectrum of particulate material suspended in a water sample.</rdfs:comment>
        <rdfs:seeAlso rdf:resource="http://vocab.nerc.ac.uk/collection/L05/current/LAB27/"/>
    </rdf:Description>
    <rdf:Description rdf:about="&glvoc_l05;LAB28">
        <rdfs:label xml:lang="en">thermal conductivimeters</rdfs:label>
        <rdfs:comment xml:lang="en">Laboratory instruments that determine the thermal conductivity of rock or sediment samples (including unopened cores).</rdfs:comment>
        <rdfs:seeAlso rdf:resource="http://vocab.nerc.ac.uk/collection/L05/current/LAB28/"/>
    </rdf:Description>
    <rdf:Description rdf:about="&glvoc_l05;POS03">
        <rdfs:label xml:lang="en">NAVSTAR Global Positioning System receivers</rdfs:label>
        <rdfs:comment xml:lang="en">{
  &quot;accuracy&quot;: &quot;better than 100m&quot;,
  &quot;notes&quot;: &quot;Global navigation based on a network of satellites deployed and maintained by the USA.&quot;,
  &quot;#text&quot;: &quot;.&quot;
}</rdfs:comment>
        <rdfs:seeAlso rdf:resource="http://vocab.nerc.ac.uk/collection/L05/current/POS03/"/>
    </rdf:Description>
    <rdf:Description rdf:about="&glvoc_l05;POS02">
        <rdfs:label xml:lang="en">Global Navigation Satellite System receivers</rdfs:label>
        <rdfs:comment xml:lang="en">{
  &quot;notes&quot;: &quot;Based on a network of satellites deployed by the former Soviet Union.  The network was initiated in 1976 but fell into disrepair before full global coverage was reached during the political upheaval of the early 90s&quot;,
  &quot;#text&quot;: &quot;.&quot;
}</rdfs:comment>
        <rdfs:seeAlso rdf:resource="http://vocab.nerc.ac.uk/collection/L05/current/POS02/"/>
    </rdf:Description>
    <rdf:Description rdf:about="&glvoc_l05;POS05">
        <rdfs:label xml:lang="en">Long Range Navigation version C receivers</rdfs:label>
        <rdfs:comment xml:lang="en">{
  &quot;frequency&quot;: &quot;70-130kHz&quot;,
  &quot;mode&quot;: &quot;hyperbolic&quot;,
  &quot;range&quot;: &quot;950kmto 1700km (day): 650km to 1250km (day)&quot;,
  &quot;operational&quot;: &quot;1947 to 2010. Maintained as GPS backup in the EU.&quot;,
  &quot;notes&quot;: &quot;Global navigation based on transmitters in several European countries, Japan, Canada (until 2002-10) and USA (until 2010-02-08).&quot;,
  &quot;#text&quot;: &quot;.&quot;
}</rdfs:comment>
        <rdfs:seeAlso rdf:resource="http://vocab.nerc.ac.uk/collection/L05/current/POS05/"/>
    </rdf:Description>
    <rdf:Description rdf:about="&glvoc_l05;POS04">
        <rdfs:label xml:lang="en">Differential Global Positioning System receivers</rdfs:label>
        <rdfs:comment xml:lang="en">{
  &quot;accuracy&quot;: &quot;better than 100m to better than 10m&quot;,
  &quot;notes&quot;: &quot;GPS augmented by a network of fixed ground stations that continuously broadcast the difference between their true locations and the location determined from the satellites.&quot;,
  &quot;#text&quot;: &quot;.&quot;
}</rdfs:comment>
        <rdfs:seeAlso rdf:resource="http://vocab.nerc.ac.uk/collection/L05/current/POS04/"/>
    </rdf:Description>
    <rdf:Description rdf:about="&glvoc_l05;LAB21">
        <rdfs:label xml:lang="en">liquid scintillation counters</rdfs:label>
        <rdfs:comment xml:lang="en">Instruments assaying beta radiation by quantitative detection of visible light produced by the passage of rays or particles through a suitable scintillant incorporated into the sample.</rdfs:comment>
        <rdfs:seeAlso rdf:resource="http://vocab.nerc.ac.uk/collection/L05/current/LAB21/"/>
    </rdf:Description>
    <rdf:Description rdf:about="&glvoc_l05;LAB22">
        <rdfs:label xml:lang="en">gamma-ray spectrometers</rdfs:label>
        <rdfs:comment xml:lang="en">Instruments measuring the relative levels of electromagnetic radiation of different wavelengths in the gamma-ray waveband.</rdfs:comment>
        <rdfs:seeAlso rdf:resource="http://vocab.nerc.ac.uk/collection/L05/current/LAB22/"/>
    </rdf:Description>
    <rdf:Description rdf:about="&glvoc_l05;LAB20">
        <rdfs:label xml:lang="en">spectrophotometers</rdfs:label>
        <rdfs:comment xml:lang="en">Instruments measuring the relative absorption of electromagnetic radiation of different wavelengths in the near infra-red, visible and ultraviolet wavebands by samples.</rdfs:comment>
        <rdfs:seeAlso rdf:resource="http://vocab.nerc.ac.uk/collection/L05/current/LAB20/"/>
    </rdf:Description>
    <rdf:Description rdf:about="&glvoc_l05;LAB25">
        <rdfs:label xml:lang="en">X-ray fluorescence analysers</rdfs:label>
        <rdfs:comment xml:lang="en">Instruments that identify and quantify the elemental constituents of a sample from the spectrum of electromagnetic radiation emitted by the atoms in the sample when excited by X-ray radiation.</rdfs:comment>
        <rdfs:seeAlso rdf:resource="http://vocab.nerc.ac.uk/collection/L05/current/LAB25/"/>
    </rdf:Description>
    <rdf:Description rdf:about="&glvoc_l05;LAB26">
        <rdfs:label xml:lang="en">X-ray diffractometers</rdfs:label>
        <rdfs:comment xml:lang="en">Instruments that identify crystalline solids by measuring the characteristic spaces between layers of atoms or molecules in a crystal.</rdfs:comment>
        <rdfs:seeAlso rdf:resource="http://vocab.nerc.ac.uk/collection/L05/current/LAB26/"/>
    </rdf:Description>
    <rdf:Description rdf:about="&glvoc_l05;LAB23">
        <rdfs:label xml:lang="en">bench fluorometers</rdfs:label>
        <rdfs:comment xml:lang="en">Instruments that determinesthe amount of chlorophyll in in-vitro samples by measuring the quantity of red light (around 685nm) emitted following excitation by pulses of blue light (around 460-470nm).</rdfs:comment>
        <rdfs:seeAlso rdf:resource="http://vocab.nerc.ac.uk/collection/L05/current/LAB23/"/>
    </rdf:Description>
    <rdf:Description rdf:about="&glvoc_l05;LAB24">
        <rdfs:label xml:lang="en">gel permeation chromatographs</rdfs:label>
        <rdfs:comment xml:lang="en">Instruments that separate components in aqueous or organic solution based on molecular size generally for molecular weight determination.</rdfs:comment>
        <rdfs:seeAlso rdf:resource="http://vocab.nerc.ac.uk/collection/L05/current/LAB24/"/>
    </rdf:Description>
    <rdf:Description rdf:about="&glvoc_l05;68">
        <rdfs:label xml:lang="en">multinet</rdfs:label>
        <rdfs:comment xml:lang="en">A system comprising several nets that can be opened and closed sequentially to collect a series of samples during a tow or haul. Samples microzooplankton, mesozooplankton and nekton.</rdfs:comment>
        <rdfs:seeAlso rdf:resource="http://vocab.nerc.ac.uk/collection/L05/current/68/"/>
    </rdf:Description>
    <rdf:Description rdf:about="&glvoc_l05;69">
        <rdfs:label xml:lang="en">neuston net</rdfs:label>
        <rdfs:comment xml:lang="en">A fine-meshed net designed to collect samples living within a few centimetres of the sea surface. Samples microzooplankton, mesozooplankton and nekton.</rdfs:comment>
        <rdfs:seeAlso rdf:resource="http://vocab.nerc.ac.uk/collection/L05/current/69/"/>
    </rdf:Description>
    <rdf:Description rdf:about="&glvoc_l05;AQPL">
        <rdfs:label xml:lang="en">Aquapulse</rdfs:label>
        <rdfs:comment xml:lang="en">A marine seismic source where a propane-oxygen mixture is exploded inside a steel cylinder.</rdfs:comment>
        <rdfs:seeAlso rdf:resource="http://vocab.nerc.ac.uk/collection/L05/current/AQPL/"/>
    </rdf:Description>
    <rdf:Description rdf:about="&glvoc_l05;84">
        <rdfs:label xml:lang="en">sieves and filters</rdfs:label>
        <rdfs:comment xml:lang="en">Devices that separate solid particles larger than a particular size from a sample collected by another device that is a suspension of solid particles in a liquid or gas.</rdfs:comment>
        <rdfs:seeAlso rdf:resource="http://vocab.nerc.ac.uk/collection/L05/current/84/"/>
    </rdf:Description>
    <rdf:Description rdf:about="&glvoc_l05;85">
        <rdfs:label xml:lang="en">biorectors and chemostats</rdfs:label>
        <rdfs:comment xml:lang="en">Devices in which controlled conditions are maintained for a chemical process to be carried out by organisms or biochemically active substances derived from such organisms.</rdfs:comment>
        <rdfs:seeAlso rdf:resource="http://vocab.nerc.ac.uk/collection/L05/current/85/"/>
    </rdf:Description>
    <rdf:Description rdf:about="&glvoc_l05;82">
        <rdfs:label xml:lang="en">in-situ incubators</rdfs:label>
        <rdfs:comment xml:lang="en">A rig that allows water samples to be retained from where they were collected whilst physically separated from their surroundings.  Includes small-scale incubation rigs and mesocosms.</rdfs:comment>
        <rdfs:seeAlso rdf:resource="http://vocab.nerc.ac.uk/collection/L05/current/82/"/>
    </rdf:Description>
    <rdf:Description rdf:about="&glvoc_l05;83">
        <rdfs:label xml:lang="en">centrifuges</rdfs:label>
        <rdfs:comment xml:lang="en">Devices that separate the liquid and solid phases of a sample through forces exerted by rapid rotation.</rdfs:comment>
        <rdfs:seeAlso rdf:resource="http://vocab.nerc.ac.uk/collection/L05/current/83/"/>
    </rdf:Description>
    <rdf:Description rdf:about="&glvoc_l05;LAB18">
        <rdfs:label xml:lang="en">nuclear magnetic resonance spectrometers</rdfs:label>
        <rdfs:comment xml:lang="en">Instruments that identify and quantify magnetically active chemical entities by subjecting a sample to orthogonal magnetic and electrical fields.</rdfs:comment>
        <rdfs:seeAlso rdf:resource="http://vocab.nerc.ac.uk/collection/L05/current/LAB18/"/>
    </rdf:Description>
    <rdf:Description rdf:about="&glvoc_l05;81">
        <rdfs:label xml:lang="en">shipboard incubators</rdfs:label>
        <rdfs:comment xml:lang="en">A device mounted on a ship that holds water samples under conditions of controlled temperature or controlled temperature and illumination.</rdfs:comment>
        <rdfs:seeAlso rdf:resource="http://vocab.nerc.ac.uk/collection/L05/current/81/"/>
    </rdf:Description>
    <rdf:Description rdf:about="&glvoc_l05;LAB19">
        <rdfs:label xml:lang="en">gas chromatograph mass spectrometers</rdfs:label>
        <rdfs:comment xml:lang="en">Instruments separating gases, volatile substances or substances dissolved in a volatile solvent by transporting an inert gas through a column packed with a sorbent to a detector for assay by a mass spectrometer.</rdfs:comment>
        <rdfs:seeAlso rdf:resource="http://vocab.nerc.ac.uk/collection/L05/current/LAB19/"/>
    </rdf:Description>
    <rdf:Description rdf:about="&glvoc_l05;LAB16">
        <rdfs:label xml:lang="en">mass spectrometers</rdfs:label>
        <rdfs:comment xml:lang="en">Instruments used to measure the mass-to-charge ratio of ions most generally used to find the composition of a sample by generating a mass spectrum representing the masses of sample components.</rdfs:comment>
        <rdfs:seeAlso rdf:resource="http://vocab.nerc.ac.uk/collection/L05/current/LAB16/"/>
    </rdf:Description>
    <rdf:Description rdf:about="&glvoc_l05;LAB17">
        <rdfs:label xml:lang="en">accelerator mass spectrometers</rdfs:label>
        <rdfs:comment xml:lang="en">Instruments measuring the mass-to-charge ratio of the products of sample molecule disassociation, atom ionisation and ion acceleration in a particle accelerator.</rdfs:comment>
        <rdfs:seeAlso rdf:resource="http://vocab.nerc.ac.uk/collection/L05/current/LAB17/"/>
    </rdf:Description>
    <rdf:Description rdf:about="&glvoc_l05;999">
        <rdfs:label xml:lang="en">unknown</rdfs:label>
        <rdfs:comment xml:lang="en">The correct value is not known to and not computable by the creator of this information. However a correct value probably exists.</rdfs:comment>
        <rdfs:seeAlso rdf:resource="http://vocab.nerc.ac.uk/collection/L05/current/999/"/>
    </rdf:Description>
    <rdf:Description rdf:about="&glvoc_l05;LAB10">
        <rdfs:label xml:lang="en">atomic absorption spectrometers</rdfs:label>
        <rdfs:comment xml:lang="en">Instruments that volatilise the sample, illuminate the resultant vapour with light wavelengths matched to the analyte of interest and quantify the radiation absorbed, which is proportional to concentration.</rdfs:comment>
        <rdfs:seeAlso rdf:resource="http://vocab.nerc.ac.uk/collection/L05/current/LAB10/"/>
    </rdf:Description>
    <rdf:Description rdf:about="&glvoc_l05;LAB11">
        <rdfs:label xml:lang="en">high performance liquid chromatographs</rdfs:label>
        <rdfs:comment xml:lang="en">Instruments that separate and analyse mixtures of substances by high pressure pumping the sample through a column packed with microspheres coated with the stationary phase.</rdfs:comment>
        <rdfs:seeAlso rdf:resource="http://vocab.nerc.ac.uk/collection/L05/current/LAB11/"/>
    </rdf:Description>
    <rdf:Description rdf:about="&glvoc_l05;FLXS">
        <rdfs:label xml:lang="en">Flexichoc</rdfs:label>
        <rdfs:comment xml:lang="en">An implosive energy source for marine shooting. Two plates are separated by compressed air until they lock into position. The air between them is then pumped out creating a vacuum. On the signal the plates are unlocked and the water pressure forces them together creating a shock wave in the water.</rdfs:comment>
        <rdfs:seeAlso rdf:resource="http://vocab.nerc.ac.uk/collection/L05/current/FLXS/"/>
    </rdf:Description>
    <rdf:Description rdf:about="&glvoc_l05;LAB14">
        <rdfs:label xml:lang="en">inductively-coupled plasma atomic emission spectroscopes</rdfs:label>
        <rdfs:comment xml:lang="en">Instruments that pass nebulised samples into an inductively-coupled gas plasma (8-10000 K) where they are atomised and excited. The de-excitation optical emissions at characteristic wavelengths are spectroscopically analysed.</rdfs:comment>
        <rdfs:seeAlso rdf:resource="http://vocab.nerc.ac.uk/collection/L05/current/LAB14/"/>
    </rdf:Description>
    <rdf:Description rdf:about="&glvoc_l05;LAB15">
        <rdfs:label xml:lang="en">inductively-coupled plasma mass spectrometers</rdfs:label>
        <rdfs:comment xml:lang="en">Instruments that pass nebulised samples into an inductively-coupled gas plasma (8-10000 K) where they are atomised and ionised. Ions of specific mass-to-charge ratios are quantified in a quadrupole mass spectrometer.</rdfs:comment>
        <rdfs:seeAlso rdf:resource="http://vocab.nerc.ac.uk/collection/L05/current/LAB15/"/>
    </rdf:Description>
    <rdf:Description rdf:about="&glvoc_l05;LAB12">
        <rdfs:label xml:lang="en">titrators</rdfs:label>
        <rdfs:comment xml:lang="en">Instruments that incrementally add quantified aliquites of a reagent to a sample until the end-point of a chemical reaction is reached.</rdfs:comment>
        <rdfs:seeAlso rdf:resource="http://vocab.nerc.ac.uk/collection/L05/current/LAB12/"/>
    </rdf:Description>
    <rdf:Description rdf:about="&glvoc_l05;LAB13">
        <rdfs:label xml:lang="en">balances and scales</rdfs:label>
        <rdfs:comment xml:lang="en">Devices that determine the mass or weight of a sample.</rdfs:comment>
        <rdfs:seeAlso rdf:resource="http://vocab.nerc.ac.uk/collection/L05/current/LAB13/"/>
    </rdf:Description>
    <rdf:Description rdf:about="&glvoc_l05;COLCMP">
        <rdfs:label xml:lang="en">Colour comparators</rdfs:label>
        <rdfs:comment xml:lang="en">Sets of standard materials that provide reference colour charts for the quantification of the colour of an object by visual comparison.</rdfs:comment>
        <rdfs:seeAlso rdf:resource="http://vocab.nerc.ac.uk/collection/L05/current/COLCMP/"/>
    </rdf:Description>
    <rdf:Description rdf:about="&glvoc_l05;186">
        <rdfs:label xml:lang="en">radar altimeters</rdfs:label>
        <rdfs:comment xml:lang="en">Instruments that determine the distance between the platform and the Earth&apos;s surface by timing reflected electromagnetic radiation, usually microwaves.</rdfs:comment>
        <rdfs:seeAlso rdf:resource="http://vocab.nerc.ac.uk/collection/L05/current/186/"/>
    </rdf:Description>
    <rdf:Description rdf:about="&glvoc_l05;185">
        <rdfs:label xml:lang="en">sound velocity sensors</rdfs:label>
        <rdfs:comment xml:lang="en">Instrument that measures the velocity of sound in seawater.</rdfs:comment>
        <rdfs:seeAlso rdf:resource="http://vocab.nerc.ac.uk/collection/L05/current/185/"/>
    </rdf:Description>
    <rdf:Description rdf:about="&glvoc_l05;LAB07">
        <rdfs:label xml:lang="en">electron microscopes</rdfs:label>
        <rdfs:comment xml:lang="en">Instruments that generate enlarged images of samples using the phenomena of reflection and absorption of electrons behaving as waves.</rdfs:comment>
        <rdfs:seeAlso rdf:resource="http://vocab.nerc.ac.uk/collection/L05/current/LAB07/"/>
    </rdf:Description>
    <rdf:Description rdf:about="&glvoc_l05;POS21">
        <rdfs:label xml:lang="en">Hyperfix receivers</rdfs:label>
        <rdfs:comment xml:lang="en">{
  &quot;frequency&quot;: &quot;1.6-3.4MHz&quot;,
  &quot;mode&quot;: &quot;hyperbolic (usual), circular or combined&quot;,
  &quot;range&quot;: &quot;250km (night) to 700km (day)&quot;,
  &quot;accuracy&quot;: &quot;up to 0.5-1m&quot;,
  &quot;operating&quot;: &quot;until 2000&quot;,
  &quot;notes&quot;: &quot;Racal positioning system similar to Decca HiFix based on temporary or permanent transmitter chains comprising a master plus at least two slaves.&quot;,
  &quot;#text&quot;: &quot;.&quot;
}</rdfs:comment>
        <rdfs:seeAlso rdf:resource="http://vocab.nerc.ac.uk/collection/L05/current/POS21/"/>
    </rdf:Description>
    <rdf:Description rdf:about="&glvoc_l05;91">
        <rdfs:label xml:lang="en">observers</rdfs:label>
        <rdfs:comment xml:lang="en">Humans who estimate a parameter through observation of a phenomenon such as bird counts, bird song mappings and visual wave observations.</rdfs:comment>
        <rdfs:seeAlso rdf:resource="http://vocab.nerc.ac.uk/collection/L05/current/91/"/>
    </rdf:Description>
    <rdf:Description rdf:about="&glvoc_l05;CCOV">
        <rdfs:label xml:lang="en">cloud cover quantifiers</rdfs:label>
        <rdfs:comment xml:lang="en">Instruments that measure the proportion of the sky covered by cloud (cloud amount) and/or the height of the cloud above the ground (cloud base).</rdfs:comment>
        <rdfs:seeAlso rdf:resource="http://vocab.nerc.ac.uk/collection/L05/current/CCOV/"/>
    </rdf:Description>
    <rdf:Description rdf:about="&glvoc_l05;LAB08">
        <rdfs:label xml:lang="en">electron microprobes</rdfs:label>
        <rdfs:comment xml:lang="en">Instruments that chemically analyse a small area of a sample by bombarding it with electrons and spectroscopically assaying the resulting X-Ray emissions.</rdfs:comment>
        <rdfs:seeAlso rdf:resource="http://vocab.nerc.ac.uk/collection/L05/current/LAB08/"/>
    </rdf:Description>
    <rdf:Description rdf:about="&glvoc_l05;POS20">
        <rdfs:label xml:lang="en">Motorola Mini-Ranger receivers</rdfs:label>
        <rdfs:comment xml:lang="en">{
  &quot;frequency&quot;: &quot;5410-5890MHz&quot;,
  &quot;range&quot;: &quot;up to 75km&quot;,
  &quot;accuracy&quot;: &quot;up to 2m&quot;,
  &quot;notes&quot;: &quot;A family of short-wave receivers that determine position by determining the line-of-sight distance from 3 or more transmitters set up for the survey.&quot;,
  &quot;#text&quot;: &quot;.&quot;
}</rdfs:comment>
        <rdfs:seeAlso rdf:resource="http://vocab.nerc.ac.uk/collection/L05/current/POS20/"/>
    </rdf:Description>
    <rdf:Description rdf:about="&glvoc_l05;POS23">
        <rdfs:label xml:lang="en">radio tracking systems</rdfs:label>
        <rdfs:comment xml:lang="en">{
  &quot;notes&quot;: &quot;Directional radio receivers that determine the location of a mobile radio transmitter (such as a bird or animal tag) by triangulation.&quot;,
  &quot;#text&quot;: &quot;.&quot;
}</rdfs:comment>
        <rdfs:seeAlso rdf:resource="http://vocab.nerc.ac.uk/collection/L05/current/POS23/"/>
    </rdf:Description>
    <rdf:Description rdf:about="&glvoc_l05;LAB05">
        <rdfs:label xml:lang="en">optical microscopes</rdfs:label>
        <rdfs:comment xml:lang="en">Instruments that generate enlarged images of samples using the phenomena of reflection and absorption of visible light. Includes conventional and inverted instruments.</rdfs:comment>
        <rdfs:seeAlso rdf:resource="http://vocab.nerc.ac.uk/collection/L05/current/LAB05/"/>
    </rdf:Description>
    <rdf:Description rdf:about="&glvoc_l05;90">
        <rdfs:label xml:lang="en">manual biota samplers</rdfs:label>
        <rdfs:comment xml:lang="en">A simple tool like a hammer, saw or even just a hand for the collection of biota samples.</rdfs:comment>
        <rdfs:seeAlso rdf:resource="http://vocab.nerc.ac.uk/collection/L05/current/90/"/>
    </rdf:Description>
    <rdf:Description rdf:about="&glvoc_l05;LAB06">
        <rdfs:label xml:lang="en">fluorescence microscopes</rdfs:label>
        <rdfs:comment xml:lang="en">Instruments that generate enlarged images of samples using the phenomena of fluorescence and phosphorescence instead of, or in addition to, reflection and absorption of visible light. Includes conventional and inverted instruments.</rdfs:comment>
        <rdfs:seeAlso rdf:resource="http://vocab.nerc.ac.uk/collection/L05/current/LAB06/"/>
    </rdf:Description>
    <rdf:Description rdf:about="&glvoc_l05;POS22">
        <rdfs:label xml:lang="en">Trisponder navigation systems</rdfs:label>
        <rdfs:comment xml:lang="en">{
  &quot;range&quot;: &quot;80km&quot;,
  &quot;accuracy&quot;: &quot;1m (resolution 0.1m)&quot;,
  &quot;notes&quot;: &quot;Family of microwave short-range positioning systems with vessel equipment and three shore transponders (master and two slaves) set up specifically for surveys.&quot;,
  &quot;#text&quot;: &quot;.&quot;
}</rdfs:comment>
        <rdfs:seeAlso rdf:resource="http://vocab.nerc.ac.uk/collection/L05/current/POS22/"/>
    </rdf:Description>
    <rdf:Description rdf:about="&glvoc_l05;POS25">
        <rdfs:label xml:lang="en">Kinematic Global Positioning System receivers</rdfs:label>
        <rdfs:comment xml:lang="en">{
  &quot;accuracy&quot;: &quot;Horizontal Accuracy: Fixed RTK mode: 1-5cm, Float RTK mode: 20cm-1m. Vertical accuracy : twice the horizontal accuracy&quot;,
  &quot;operating&quot;: &quot;Since the mid-1990s&quot;,
  &quot;notes&quot;: &quot;Real Time Kinematic (RTK) satellite navigation technique based on the use of carrier phase measurements of the GPS signals where a single reference station or a network of reference stations provides the real-time corrections.&quot;,
  &quot;#text&quot;: &quot;.&quot;
}</rdfs:comment>
        <rdfs:seeAlso rdf:resource="http://vocab.nerc.ac.uk/collection/L05/current/POS25/"/>
    </rdf:Description>
    <rdf:Description rdf:about="&glvoc_l05;POS24">
        <rdfs:label xml:lang="en">dead reckoning</rdfs:label>
        <rdfs:comment xml:lang="en">{
  &quot;notes&quot;: &quot;The process of estimating current position based upon a previously determined position, or fix, and advancing that position based upon known or estimated speeds over elapsed time, and course.&quot;,
  &quot;#text&quot;: &quot;.&quot;
}</rdfs:comment>
        <rdfs:seeAlso rdf:resource="http://vocab.nerc.ac.uk/collection/L05/current/POS24/"/>
    </rdf:Description>
    <rdf:Description rdf:about="&glvoc_l05;FLXT">
        <rdfs:label xml:lang="en">Flexotir</rdfs:label>
        <rdfs:comment xml:lang="en">A seismic method for marine shooting whereby small charges are propelled through a rubber hose by water under pressure into a steel cage where they are detonated. Holes in the cage allow the water repelled by the explosion to flow out and in thus dissipating some of the energy in the bubble effect.</rdfs:comment>
        <rdfs:seeAlso rdf:resource="http://vocab.nerc.ac.uk/collection/L05/current/FLXT/"/>
    </rdf:Description>
    <rdf:Description rdf:about="&glvoc_l05;LAB09">
        <rdfs:label xml:lang="en">ion microprobes</rdfs:label>
        <rdfs:comment xml:lang="en">Instruments that isotopically analyse a small area of sample by bombarding it with ions to form a plasma that is analysed in a mass spectrometer.</rdfs:comment>
        <rdfs:seeAlso rdf:resource="http://vocab.nerc.ac.uk/collection/L05/current/LAB09/"/>
    </rdf:Description>
    <rdf:Description rdf:about="&glvoc_l05;POS26">
        <rdfs:label xml:lang="en">Ultra Short Baseline Positioning Systems</rdfs:label>
        <rdfs:comment xml:lang="en">Systems dedicated to the positioning of subsea vehicles such as ROV and AUV. They are based on acoustic transmitted signals between one or several transponders and one acoustic antenna installed on a surface vessel. The transponders are mounted on the underwater vehicle or are fixed on the seafloor. These underwater acoustic positioning systems are coupled with inertial navigation systems.</rdfs:comment>
        <rdfs:seeAlso rdf:resource="http://vocab.nerc.ac.uk/collection/L05/current/POS26/"/>
    </rdf:Description>
    <rdf:Description rdf:about="&glvoc_l05;LAB03">
        <rdfs:label xml:lang="en">colorimeters</rdfs:label>
        <rdfs:comment xml:lang="en">Instruments measuring the amount of light of a given wavelength absorbed by a sample of solution to determine the concentration of a specific coloured solute.</rdfs:comment>
        <rdfs:seeAlso rdf:resource="http://vocab.nerc.ac.uk/collection/L05/current/LAB03/"/>
    </rdf:Description>
    <rdf:Description rdf:about="&glvoc_l05;LAB04">
        <rdfs:label xml:lang="en">autoanalysers</rdfs:label>
        <rdfs:comment xml:lang="en">Instruments that continuously draw samples through plumbing adding reagents whilst controlling the environment to produce a chemical reaction before passing the sample to a detector, e.g. the automated colorimetric determination of nutrients.</rdfs:comment>
        <rdfs:seeAlso rdf:resource="http://vocab.nerc.ac.uk/collection/L05/current/LAB04/"/>
    </rdf:Description>
    <rdf:Description rdf:about="&glvoc_l05;EQUIL">
        <rdfs:label xml:lang="en">equilibrators</rdfs:label>
        <rdfs:comment xml:lang="en">Devices in which samples and carriers are brought into chemical equilibrium prior to analysis. For example, a shower head or tower full of marbles used to equilibrate water samples with air that is subsequently analysed for carbon dioxide to give pCO2 in the water sample.</rdfs:comment>
        <rdfs:seeAlso rdf:resource="http://vocab.nerc.ac.uk/collection/L05/current/EQUIL/"/>
    </rdf:Description>
    <rdf:Description rdf:about="&glvoc_l05;LAB01">
        <rdfs:label xml:lang="en">elemental analysers</rdfs:label>
        <rdfs:comment xml:lang="en">Instruments that quantify carbon, nitrogen and sometimes other elements by combusting the sample at very high temperature and assaying the resulting gaseous oxides. Usually used for samples including organic material.</rdfs:comment>
        <rdfs:seeAlso rdf:resource="http://vocab.nerc.ac.uk/collection/L05/current/LAB01/"/>
    </rdf:Description>
    <rdf:Description rdf:about="&glvoc_l05;LAB02">
        <rdfs:label xml:lang="en">gas chromatographs</rdfs:label>
        <rdfs:comment xml:lang="en">Instruments separating gases, volatile substances or substances dissolved in a volatile solvent by transporting an inert gas through a column packed with a sorbent to a detector for assay.</rdfs:comment>
        <rdfs:seeAlso rdf:resource="http://vocab.nerc.ac.uk/collection/L05/current/LAB02/"/>
    </rdf:Description>
    <rdf:Description rdf:about="&glvoc_l05;182">
        <rdfs:label xml:lang="en">inapplicable</rdfs:label>
        <rdfs:comment xml:lang="en">There is no appropriate value. To be used in cases where metadata elements cannot be set null due to schema constraints.</rdfs:comment>
        <rdfs:seeAlso rdf:resource="http://vocab.nerc.ac.uk/collection/L05/current/182/"/>
    </rdf:Description>
    <rdf:Description rdf:about="&glvoc_l05;181">
        <rdfs:label xml:lang="en">nutrient analysers</rdfs:label>
        <rdfs:comment xml:lang="en">Instrument that makes in-situ measurements of one or more of nitrate, nitrite, ammonium, urea, phosphate or silicate dissolved in the water column.</rdfs:comment>
        <rdfs:seeAlso rdf:resource="http://vocab.nerc.ac.uk/collection/L05/current/181/"/>
    </rdf:Description>
    <rdf:Description rdf:about="&glvoc_l05;184">
        <rdfs:label xml:lang="en">microstructure sensors</rdfs:label>
        <rdfs:comment xml:lang="en">Fast response sensors sampled at high frequency to determine the distribution of water body properties on a millimetric scale.</rdfs:comment>
        <rdfs:seeAlso rdf:resource="http://vocab.nerc.ac.uk/collection/L05/current/184/"/>
    </rdf:Description>
    <rdf:Description rdf:about="&glvoc_l05;183">
        <rdfs:label xml:lang="en">acoustic backscatter sensors</rdfs:label>
        <rdfs:comment xml:lang="en">Instrument that measures the amount of sound energy transmitted into the water column returned to the instrument.</rdfs:comment>
        <rdfs:seeAlso rdf:resource="http://vocab.nerc.ac.uk/collection/L05/current/183/"/>
    </rdf:Description>
    <rdf:Description rdf:about="&glvoc_l05;180">
        <rdfs:label xml:lang="en">underwater cameras</rdfs:label>
        <rdfs:comment xml:lang="en">All types of photographic equipment that may be deployed underwater including stills, video, film and digital systems.</rdfs:comment>
        <rdfs:seeAlso rdf:resource="http://vocab.nerc.ac.uk/collection/L05/current/180/"/>
    </rdf:Description>
    <rdf:Description rdf:about="&glvoc_l05;ERTQ">
        <rdfs:label xml:lang="en">earthquake</rdfs:label>
        <rdfs:comment xml:lang="en">A sudden release of stress in the Earth&apos;s crust that creates energy in the form of seimic waves.</rdfs:comment>
        <rdfs:seeAlso rdf:resource="http://vocab.nerc.ac.uk/collection/L05/current/ERTQ/"/>
    </rdf:Description>
    <rdf:Description rdf:about="&glvoc_l05;ARAG">
        <rdfs:label xml:lang="en">airgun array</rdfs:label>
        <rdfs:comment xml:lang="en">A marine seismic source where multiple airguns of different sizes are tuned so that  a broader frequency spectrum will be generated.</rdfs:comment>
        <rdfs:seeAlso rdf:resource="http://vocab.nerc.ac.uk/collection/L05/current/ARAG/"/>
    </rdf:Description>
    <rdf:Description rdf:about="&glvoc_l05;157">
        <rdfs:label xml:lang="en">multi-beam echosounders</rdfs:label>
        <rdfs:comment xml:lang="en">Instruments that measure water depth along several tracks parallel to the platform track by timing pulses of sound reflected on the seafloor.</rdfs:comment>
        <rdfs:seeAlso rdf:resource="http://vocab.nerc.ac.uk/collection/L05/current/157/"/>
    </rdf:Description>
    <rdf:Description rdf:about="&glvoc_l05;156">
        <rdfs:label xml:lang="en">single-beam echosounders</rdfs:label>
        <rdfs:comment xml:lang="en">Instruments that measure water depth at a single point below the platform by timing pulses of sound reflected on the seafloor.</rdfs:comment>
        <rdfs:seeAlso rdf:resource="http://vocab.nerc.ac.uk/collection/L05/current/156/"/>
    </rdf:Description>
    <rdf:Description rdf:about="&glvoc_l05;159">
        <rdfs:label xml:lang="en">magnetometers</rdfs:label>
        <rdfs:comment xml:lang="en">Instrument that makes measurements of the Earth&apos;s magnetic field.</rdfs:comment>
        <rdfs:seeAlso rdf:resource="http://vocab.nerc.ac.uk/collection/L05/current/159/"/>
    </rdf:Description>
    <rdf:Description rdf:about="&glvoc_l05;158">
        <rdfs:label xml:lang="en">gravimeters</rdfs:label>
        <rdfs:comment xml:lang="en">Instrument that makes measurements of the Earth&apos;s gravity field.</rdfs:comment>
        <rdfs:seeAlso rdf:resource="http://vocab.nerc.ac.uk/collection/L05/current/158/"/>
    </rdf:Description>
    <rdf:Description rdf:about="&glvoc_l05;153">
        <rdfs:label xml:lang="en">single-channel seismic reflection systems</rdfs:label>
        <rdfs:comment xml:lang="en">An energy source of unspecified frequency plus a single string of towed hydrophones (streamer) that determine geologic structure by detecting waves reflected by subsurface layers.</rdfs:comment>
        <rdfs:seeAlso rdf:resource="http://vocab.nerc.ac.uk/collection/L05/current/153/"/>
    </rdf:Description>
    <rdf:Description rdf:about="&glvoc_l05;152">
        <rdfs:label xml:lang="en">sidescan sonars</rdfs:label>
        <rdfs:comment xml:lang="en">Instruments with directional acoustic transmitters and receivers fitted to an underwater platform that emit fan-shaped pulses down toward the seafloor across a wide angle perpendicular to the path of the platform through the water.</rdfs:comment>
        <rdfs:seeAlso rdf:resource="http://vocab.nerc.ac.uk/collection/L05/current/152/"/>
    </rdf:Description>
    <rdf:Description rdf:about="&glvoc_l05;MVBR">
        <rdfs:label xml:lang="en">marine vibroseis</rdfs:label>
        <rdfs:comment xml:lang="en">A marine seismic source generating sweeps of controlled varying frequency (from a few Hz to hundreds of Hz) and duration.</rdfs:comment>
        <rdfs:seeAlso rdf:resource="http://vocab.nerc.ac.uk/collection/L05/current/MVBR/"/>
    </rdf:Description>
    <rdf:Description rdf:about="&glvoc_l05;155">
        <rdfs:label xml:lang="en">seismic refraction systems</rdfs:label>
        <rdfs:comment xml:lang="en">A network of seismometers or geophones plus an energy source that determine geologic structure by detecting waves refracted by subsurface layers.</rdfs:comment>
        <rdfs:seeAlso rdf:resource="http://vocab.nerc.ac.uk/collection/L05/current/155/"/>
    </rdf:Description>
    <rdf:Description rdf:about="&glvoc_l05;154">
        <rdfs:label xml:lang="en">multi-channel seismic reflection systems</rdfs:label>
        <rdfs:comment xml:lang="en">An energy source of unspecified frequency plus a multiple strings of towed hydrophones (streamers) that determine geologic structure by detecting waves reflected by subsurface layers.</rdfs:comment>
        <rdfs:seeAlso rdf:resource="http://vocab.nerc.ac.uk/collection/L05/current/154/"/>
    </rdf:Description>
    <rdf:Description rdf:about="&glvoc_l05;SNAG">
        <rdfs:label xml:lang="en">airgun</rdfs:label>
        <rdfs:comment xml:lang="en">A marine seismic source which injects a bubble of highly compressed air into the water. Oscillations of the bubble as it alternatively expands and contracts generate a sonic wave whose frequency depends on the amount of air in the bubble, its pressure, and the water depth.</rdfs:comment>
        <rdfs:seeAlso rdf:resource="http://vocab.nerc.ac.uk/collection/L05/current/SNAG/"/>
    </rdf:Description>
    <rdf:Description rdf:about="&glvoc_l05;151">
        <rdfs:label xml:lang="en">benthic incubation chambers</rdfs:label>
        <rdfs:comment xml:lang="en">A device that isolates a portion of seabed plus overlying water from its surroundings. Either returns the entire system to the surface or incorporates sampling devices and/or in-situ sensors.</rdfs:comment>
        <rdfs:seeAlso rdf:resource="http://vocab.nerc.ac.uk/collection/L05/current/151/"/>
    </rdf:Description>
    <rdf:Description rdf:about="&glvoc_l05;150">
        <rdfs:label xml:lang="en">particle sizers</rdfs:label>
        <rdfs:comment xml:lang="en">An instrument that measures the size spectrum of particles suspended in the water column.</rdfs:comment>
        <rdfs:seeAlso rdf:resource="http://vocab.nerc.ac.uk/collection/L05/current/150/"/>
    </rdf:Description>
    <rdf:Description rdf:about="&glvoc_l05;388">
        <rdfs:label xml:lang="en">flow meters</rdfs:label>
        <rdfs:comment xml:lang="en">Sensors that quantify the rate at which fluids (e.g. water or air) pass through sensor packages, instruments or sampling devices.</rdfs:comment>
        <rdfs:seeAlso rdf:resource="http://vocab.nerc.ac.uk/collection/L05/current/388/"/>
    </rdf:Description>
    <rdf:Description rdf:about="&glvoc_l05;387">
        <rdfs:label xml:lang="en">Aethalometers</rdfs:label>
        <rdfs:comment xml:lang="en">Instruments that quantify atmospheric particulate carbon (&apos;black carbon&apos;) concentrations.</rdfs:comment>
        <rdfs:seeAlso rdf:resource="http://vocab.nerc.ac.uk/collection/L05/current/387/"/>
    </rdf:Description>
    <rdf:Description rdf:about="&glvoc_l05;384">
        <rdfs:label xml:lang="en">ADVs and turbulence probes</rdfs:label>
        <rdfs:comment xml:lang="en">ADV is the acronym for acoustic doppler velocimeter. The group includes all in-situ instruments that make high frequency measurements of three-dimensional current velocity in order to determine the extent of turbulence within a water body.</rdfs:comment>
        <rdfs:seeAlso rdf:resource="http://vocab.nerc.ac.uk/collection/L05/current/384/"/>
    </rdf:Description>
    <rdf:Description rdf:about="&glvoc_l05;383">
        <rdfs:label xml:lang="en">metal analysers</rdfs:label>
        <rdfs:comment xml:lang="en">In-situ instruments that can determine the total, dissolved or particulate concentration of one or more metallic elements (including trace metalloids like arsenic) in a water body.</rdfs:comment>
        <rdfs:seeAlso rdf:resource="http://vocab.nerc.ac.uk/collection/L05/current/383/"/>
    </rdf:Description>
    <rdf:Description rdf:about="&glvoc_l05;386">
        <rdfs:label xml:lang="en">Aerosol physical characterisers</rdfs:label>
        <rdfs:comment xml:lang="en">Instruments that determine physical attributes such as size and abundance of atmospheric aerosols.</rdfs:comment>
        <rdfs:seeAlso rdf:resource="http://vocab.nerc.ac.uk/collection/L05/current/386/"/>
    </rdf:Description>
    <rdf:Description rdf:about="&glvoc_l05;385">
        <rdfs:label xml:lang="en">platform attitude sensors</rdfs:label>
        <rdfs:comment xml:lang="en">Instruments that measure platform orientation or rates of platform motion or acceleration in any direction or along any axis. Excludes inertial navigation systems that are designed to determine platform location with respect to an external co-ordinate reference system.</rdfs:comment>
        <rdfs:seeAlso rdf:resource="http://vocab.nerc.ac.uk/collection/L05/current/385/"/>
    </rdf:Description>
    <rdf:Description rdf:about="&glvoc_l05;380">
        <rdfs:label xml:lang="en">submarine cables</rdfs:label>
        <rdfs:comment xml:lang="en">Electrical conductors routed beneath the sea and connecting land stations.  Oceanographic interest focuses on changes in electrical resistance that may be related to the magnitude of Lagrangian currents.</rdfs:comment>
        <rdfs:seeAlso rdf:resource="http://vocab.nerc.ac.uk/collection/L05/current/380/"/>
    </rdf:Description>
    <rdf:Description rdf:about="&glvoc_l05;382">
        <rdfs:label xml:lang="en">atmospheric gas analysers</rdfs:label>
        <rdfs:comment xml:lang="en">In-situ instruments that can determine the proportion of one or more gaseous components of the atmosphere.</rdfs:comment>
        <rdfs:seeAlso rdf:resource="http://vocab.nerc.ac.uk/collection/L05/current/382/"/>
    </rdf:Description>
    <rdf:Description rdf:about="&glvoc_l05;381">
        <rdfs:label xml:lang="en">precipitation gauges</rdfs:label>
        <rdfs:comment xml:lang="en">Instruments that measure either the rate of fall or integrated amount of rain, snow, sleet, hail or graupel.</rdfs:comment>
        <rdfs:seeAlso rdf:resource="http://vocab.nerc.ac.uk/collection/L05/current/381/"/>
    </rdf:Description>
    <rdf:Description rdf:about="&glvoc_l05;EXLH">
        <rdfs:label xml:lang="en">high penetration low resolution explosives</rdfs:label>
        <rdfs:comment xml:lang="en">Groups all explosives that allows high penetration but low resolution surveys.</rdfs:comment>
        <rdfs:seeAlso rdf:resource="http://vocab.nerc.ac.uk/collection/L05/current/EXLH/"/>
    </rdf:Description>
    <rdf:Description rdf:about="&glvoc_l05;FFES">
        <rdfs:label xml:lang="en">Fish-finder echosounders</rdfs:label>
        <rdfs:comment xml:lang="en">Instruments primarily designed to detect shoals of fish through transmission and reception of acoustic signals.  They are often optimised for this purpose through the use of multiple frequencies.</rdfs:comment>
        <rdfs:seeAlso rdf:resource="http://vocab.nerc.ac.uk/collection/L05/current/FFES/"/>
    </rdf:Description>
    <rdf:Description rdf:about="&glvoc_l05;NATS">
        <rdfs:label xml:lang="en">natural source</rdfs:label>
        <rdfs:comment xml:lang="en">Any kind of natural source of acoustic waves, that can be used in passive seismics.</rdfs:comment>
        <rdfs:seeAlso rdf:resource="http://vocab.nerc.ac.uk/collection/L05/current/NATS/"/>
    </rdf:Description>
    <rdf:Description rdf:about="&glvoc_l05;CHRP">
        <rdfs:label xml:lang="en">Chirp</rdfs:label>
        <rdfs:comment xml:lang="en">Chirp systems emit a &apos;swept-frequency signal&apos;, meaning that the transmitted signal is emitted over a period of time and over a set range of frequencies. This repeatable (transmitted) waveform can be varied in terms of pulse length, frequency bandwidth, and phase/amplitude. A matched filter, or correlation process, collapses the swept frequency modulated (FM) received signal into a pulse of short duration, maximizing the signal-to-noise-ratio. The reflected signal is received by a tuned transducer array that generates the outgoing acoustic energy. Chirps operate within a range of 400Hz - 24 kHz and are used for the first 20-30 metres of unconsolidated sediments.</rdfs:comment>
        <rdfs:seeAlso rdf:resource="http://vocab.nerc.ac.uk/collection/L05/current/CHRP/"/>
    </rdf:Description>
    <rdf:Description rdf:about="&glvoc_l05;ATRANS">
        <rdfs:label xml:lang="en">atmospheric transparency quantifiers</rdfs:label>
        <rdfs:comment xml:lang="en">Instruments that quantify the degree of scattering and absorption of light passing through the atmosphere, including instruments that quantify aerosol and particulate concentrations (e.g. black carbon) and instruments measure meteorological visibility.</rdfs:comment>
        <rdfs:seeAlso rdf:resource="http://vocab.nerc.ac.uk/collection/L05/current/ATRANS/"/>
    </rdf:Description>
    <rdf:Description rdf:about="&glvoc_l05;TRTG">
        <rdfs:label xml:lang="en">tracking tags</rdfs:label>
        <rdfs:comment xml:lang="en">Passive devices activated by radio-frequency energy or active devices with power supplies attached to living organisms with the purpose of determining the location of those organisms at any given time after tagging and release.</rdfs:comment>
        <rdfs:seeAlso rdf:resource="http://vocab.nerc.ac.uk/collection/L05/current/TRTG/"/>
    </rdf:Description>
    <rdf:Description rdf:about="&glvoc_l05;355">
        <rdfs:label xml:lang="en">pH sensors</rdfs:label>
        <rdfs:comment xml:lang="en">Instruments that measure the hydrogen ion concentration in the water column.</rdfs:comment>
        <rdfs:seeAlso rdf:resource="http://vocab.nerc.ac.uk/collection/L05/current/355/"/>
    </rdf:Description>
    <rdf:Description rdf:about="&glvoc_l05;113">
        <rdfs:label xml:lang="en">fluorometers</rdfs:label>
        <rdfs:comment xml:lang="en">Instrument that measures the amount of stimulated electromagnetic radiation produced by pulses of electromagnetic radiation emitted into the water column.</rdfs:comment>
        <rdfs:seeAlso rdf:resource="http://vocab.nerc.ac.uk/collection/L05/current/113/"/>
    </rdf:Description>
    <rdf:Description rdf:about="&glvoc_l05;112">
        <rdfs:label xml:lang="en">inverted echosounders</rdfs:label>
        <rdfs:comment xml:lang="en">Instruments that locate acoustic reflectors such as fronts in the water column by transmitting pulses of sound from the seabed and determing reflection return times.</rdfs:comment>
        <rdfs:seeAlso rdf:resource="http://vocab.nerc.ac.uk/collection/L05/current/112/"/>
    </rdf:Description>
    <rdf:Description rdf:about="&glvoc_l05;354">
        <rdfs:label xml:lang="en">expendable CTDs</rdfs:label>
        <rdfs:comment xml:lang="en">Instruments that measure vertical profiles of sea temperature and salinity with a free falling disposable temperature and conductivity sensor package.</rdfs:comment>
        <rdfs:seeAlso rdf:resource="http://vocab.nerc.ac.uk/collection/L05/current/354/"/>
    </rdf:Description>
    <rdf:Description rdf:about="&glvoc_l05;357">
        <rdfs:label xml:lang="en">acoustic tracking systems</rdfs:label>
        <rdfs:comment xml:lang="en">A network of acoustic sensors that determine the location of a sound source by triangulation such as acoustically active float tracking systems.</rdfs:comment>
        <rdfs:seeAlso rdf:resource="http://vocab.nerc.ac.uk/collection/L05/current/357/"/>
    </rdf:Description>
    <rdf:Description rdf:about="&glvoc_l05;115">
        <rdfs:label xml:lang="en">current profilers</rdfs:label>
        <rdfs:comment xml:lang="en">Instrument that measures current speed and direction at multiple predetermined depths simultaneously.</rdfs:comment>
        <rdfs:seeAlso rdf:resource="http://vocab.nerc.ac.uk/collection/L05/current/115/"/>
    </rdf:Description>
    <rdf:Description rdf:about="&glvoc_l05;114">
        <rdfs:label xml:lang="en">current meters</rdfs:label>
        <rdfs:comment xml:lang="en">Instrument that measures current speed and direction at a single depth.</rdfs:comment>
        <rdfs:seeAlso rdf:resource="http://vocab.nerc.ac.uk/collection/L05/current/114/"/>
    </rdf:Description>
    <rdf:Description rdf:about="&glvoc_l05;356">
        <rdfs:label xml:lang="en">redox potential sensors</rdfs:label>
        <rdfs:comment xml:lang="en">Instruments that measure the tendency of the water column to either gain or lose electrons when it is subject to change by introduction of a new species.</rdfs:comment>
        <rdfs:seeAlso rdf:resource="http://vocab.nerc.ac.uk/collection/L05/current/356/"/>
    </rdf:Description>
    <rdf:Description rdf:about="&glvoc_l05;351">
        <rdfs:label xml:lang="en">dissolved gas sensors</rdfs:label>
        <rdfs:comment xml:lang="en">Instrument that measures the concentration of gases, generally oxygen, dissolved in the water column.</rdfs:comment>
        <rdfs:seeAlso rdf:resource="http://vocab.nerc.ac.uk/collection/L05/current/351/"/>
    </rdf:Description>
    <rdf:Description rdf:about="&glvoc_l05;350">
        <rdfs:label xml:lang="en">salinity sensor</rdfs:label>
        <rdfs:comment xml:lang="en">Instrument that simultaneously measures electrical conductivity and temperature in the water column to provide temperature and salinity data.</rdfs:comment>
        <rdfs:seeAlso rdf:resource="http://vocab.nerc.ac.uk/collection/L05/current/350/"/>
    </rdf:Description>
    <rdf:Description rdf:about="&glvoc_l05;353">
        <rdfs:label xml:lang="en">active fluorometers</rdfs:label>
        <rdfs:comment xml:lang="en">Fluorometers that measure photosynthetic parameters by taking measurements whilst manipulating the phytoplankton with controlled high-intensity illumination such as pump and probe and FRRF.</rdfs:comment>
        <rdfs:seeAlso rdf:resource="http://vocab.nerc.ac.uk/collection/L05/current/353/"/>
    </rdf:Description>
    <rdf:Description rdf:about="&glvoc_l05;111">
        <rdfs:label xml:lang="en">sea level recorders</rdfs:label>
        <rdfs:comment xml:lang="en">Instrument that make smoothed measuremeants of the elevation of the sea surface relative to a fixed vertical datum.</rdfs:comment>
        <rdfs:seeAlso rdf:resource="http://vocab.nerc.ac.uk/collection/L05/current/111/"/>
    </rdf:Description>
    <rdf:Description rdf:about="&glvoc_l05;MOD08">
        <rdfs:label xml:lang="en">Biological and biogeochemical models</rdfs:label>
        <rdfs:comment xml:lang="en">Numerical models that make predictions of biological parameters, including ecosystem models.</rdfs:comment>
        <rdfs:seeAlso rdf:resource="http://vocab.nerc.ac.uk/collection/L05/current/MOD08/"/>
    </rdf:Description>
    <rdf:Description rdf:about="&glvoc_l05;352">
        <rdfs:label xml:lang="en">plankton counters</rdfs:label>
        <rdfs:comment xml:lang="en">Instruments that categorise and count plankton in the water column.</rdfs:comment>
        <rdfs:seeAlso rdf:resource="http://vocab.nerc.ac.uk/collection/L05/current/352/"/>
    </rdf:Description>
    <rdf:Description rdf:about="&glvoc_l05;110">
        <rdfs:label xml:lang="en">wave recorders</rdfs:label>
        <rdfs:comment xml:lang="en">Instrument that measures water column surface wave parameters including height, period, direction and energy spectra.</rdfs:comment>
        <rdfs:seeAlso rdf:resource="http://vocab.nerc.ac.uk/collection/L05/current/110/"/>
    </rdf:Description>
    <rdf:Description rdf:about="&glvoc_l05;MOD06">
        <rdfs:label xml:lang="en">Meteorological models</rdfs:label>
        <rdfs:comment xml:lang="en">Numerical models that make predictions of weather parameters such as air temperature, pressure, humidity and winds.</rdfs:comment>
        <rdfs:seeAlso rdf:resource="http://vocab.nerc.ac.uk/collection/L05/current/MOD06/"/>
    </rdf:Description>
    <rdf:Description rdf:about="&glvoc_l05;MOD07">
        <rdfs:label xml:lang="en">Physical oceanographic models</rdfs:label>
        <rdfs:comment xml:lang="en">Numerical models that make predictions of physical oceanographic parameters such as water body temperature, salinity, currents and waves.</rdfs:comment>
        <rdfs:seeAlso rdf:resource="http://vocab.nerc.ac.uk/collection/L05/current/MOD07/"/>
    </rdf:Description>
    <rdf:Description rdf:about="&glvoc_l05;MOD04">
        <rdfs:label xml:lang="en">Ocean models</rdfs:label>
        <rdfs:comment xml:lang="en">Numerical models the make predictions in the hydrosphere assuming that it is a closed system that doesn&apos;t interact with the atmosphere.</rdfs:comment>
        <rdfs:seeAlso rdf:resource="http://vocab.nerc.ac.uk/collection/L05/current/MOD04/"/>
    </rdf:Description>
    <rdf:Description rdf:about="&glvoc_l05;MOD05">
        <rdfs:label xml:lang="en">Coupled models</rdfs:label>
        <rdfs:comment xml:lang="en">Numerical models that make predictions in both the atmosphere and the hydrosphere by considering both spheres as a single system.</rdfs:comment>
        <rdfs:seeAlso rdf:resource="http://vocab.nerc.ac.uk/collection/L05/current/MOD05/"/>
    </rdf:Description>
    <rdf:Description rdf:about="&glvoc_l05;MOD02">
        <rdfs:label xml:lang="en">Regional models</rdfs:label>
        <rdfs:comment xml:lang="en">Numerical models that make predictions within a limited geographic area.</rdfs:comment>
        <rdfs:seeAlso rdf:resource="http://vocab.nerc.ac.uk/collection/L05/current/MOD02/"/>
    </rdf:Description>
    <rdf:Description rdf:about="&glvoc_l05;359">
        <rdfs:label xml:lang="en">plummets</rdfs:label>
        <rdfs:comment xml:lang="en">Devices comprising a weight attached to the end of a graduated rope used to measure point water depths.</rdfs:comment>
        <rdfs:seeAlso rdf:resource="http://vocab.nerc.ac.uk/collection/L05/current/359/"/>
    </rdf:Description>
    <rdf:Description rdf:about="&glvoc_l05;116">
        <rdfs:label xml:lang="en">lowered current profilers</rdfs:label>
        <rdfs:comment xml:lang="en">An acoustic doppler current meter lowered and raised vertically from a surface platform, typically a ship.</rdfs:comment>
        <rdfs:seeAlso rdf:resource="http://vocab.nerc.ac.uk/collection/L05/current/116/"/>
    </rdf:Description>
    <rdf:Description rdf:about="&glvoc_l05;358">
        <rdfs:label xml:lang="en">bubble detectors</rdfs:label>
        <rdfs:comment xml:lang="en">Instruments that measure the concentration and size of air bubbles in the water column.</rdfs:comment>
        <rdfs:seeAlso rdf:resource="http://vocab.nerc.ac.uk/collection/L05/current/358/"/>
    </rdf:Description>
    <rdf:Description rdf:about="&glvoc_l05;MOD03">
        <rdfs:label xml:lang="en">Atmosphere models</rdfs:label>
        <rdfs:comment xml:lang="en">Numerical models the make predictions in the atmosphere assuming that it is a closed system that doesn&apos;t interact with the hydrosphere.</rdfs:comment>
        <rdfs:seeAlso rdf:resource="http://vocab.nerc.ac.uk/collection/L05/current/MOD03/"/>
    </rdf:Description>
    <rdf:Description rdf:about="&glvoc_l05;MOD01">
        <rdfs:label xml:lang="en">Global models</rdfs:label>
        <rdfs:comment xml:lang="en">Numerical models that make predictions over the whole globe.</rdfs:comment>
        <rdfs:seeAlso rdf:resource="http://vocab.nerc.ac.uk/collection/L05/current/MOD01/"/>
    </rdf:Description>
    <rdf:Description rdf:about="&glvoc_l05;102">
        <rdfs:label xml:lang="en">meteorological packages</rdfs:label>
        <rdfs:comment xml:lang="en">Instrument that makes routine meteorological measurements on the atmosphere, typically air pressure, temperature and humidity.</rdfs:comment>
        <rdfs:seeAlso rdf:resource="http://vocab.nerc.ac.uk/collection/L05/current/102/"/>
    </rdf:Description>
    <rdf:Description rdf:about="&glvoc_l05;11">
        <rdfs:label xml:lang="en">discrete air samplers</rdfs:label>
        <rdfs:comment xml:lang="en">A device that collects a sample of air from the atmosphere and stores it, usually under pressure, for subsequent analysis.</rdfs:comment>
        <rdfs:seeAlso rdf:resource="http://vocab.nerc.ac.uk/collection/L05/current/11/"/>
    </rdf:Description>
    <rdf:Description rdf:about="&glvoc_l05;101">
        <rdfs:label xml:lang="en">anemometers</rdfs:label>
        <rdfs:comment xml:lang="en">Instrument that measures wind speed and direction at a single elevation.</rdfs:comment>
        <rdfs:seeAlso rdf:resource="http://vocab.nerc.ac.uk/collection/L05/current/101/"/>
    </rdf:Description>
    <rdf:Description rdf:about="&glvoc_l05;12">
        <rdfs:label xml:lang="en">fog samplers</rdfs:label>
        <rdfs:comment xml:lang="en">A device that condenses a sample of fog from the atmosphere.</rdfs:comment>
        <rdfs:seeAlso rdf:resource="http://vocab.nerc.ac.uk/collection/L05/current/12/"/>
    </rdf:Description>
    <rdf:Description rdf:about="&glvoc_l05;103">
        <rdfs:label xml:lang="en">radiosondes</rdfs:label>
        <rdfs:comment xml:lang="en">A balloon-borne package equipped with a radio transmitter and meteorological sensors typically measuring temperature, pressure, and humidity.</rdfs:comment>
        <rdfs:seeAlso rdf:resource="http://vocab.nerc.ac.uk/collection/L05/current/103/"/>
    </rdf:Description>
    <rdf:Description rdf:about="&glvoc_l05;SPRK">
        <rdfs:label xml:lang="en">Sparker</rdfs:label>
        <rdfs:comment xml:lang="en">A seismic source in which an electrical discharge in water is the energy source.</rdfs:comment>
        <rdfs:seeAlso rdf:resource="http://vocab.nerc.ac.uk/collection/L05/current/SPRK/"/>
    </rdf:Description>
    <rdf:Description rdf:about="&glvoc_l05;ICEP">
        <rdfs:label xml:lang="en">ice thickness profilers</rdfs:label>
        <rdfs:comment xml:lang="en">Instruments that measure the freeboard, draught or thickness of ice sheets or sea ice. These are not to be confused with tethered ice profilers that are platforms that sample the water column beneath sea ice.</rdfs:comment>
        <rdfs:seeAlso rdf:resource="http://vocab.nerc.ac.uk/collection/L05/current/ICEP/"/>
    </rdf:Description>
    <rdf:Description rdf:about="&glvoc_l05;377">
        <rdfs:label xml:lang="en">water level markers</rdfs:label>
        <rdfs:comment xml:lang="en">Fixed physical markers that allow changes in the position of the boundary between a water body and the atmosphere by visible comparison against marked graduations in units of measurement of dimension length.</rdfs:comment>
        <rdfs:seeAlso rdf:resource="http://vocab.nerc.ac.uk/collection/L05/current/377/"/>
    </rdf:Description>
    <rdf:Description rdf:about="&glvoc_l05;22">
        <rdfs:label xml:lang="en">plankton nets</rdfs:label>
        <rdfs:comment xml:lang="en">A fine-meshed net designed for sampling microzooplankton, mesozooplankton or nekton.</rdfs:comment>
        <rdfs:seeAlso rdf:resource="http://vocab.nerc.ac.uk/collection/L05/current/22/"/>
    </rdf:Description>
    <rdf:Description rdf:about="&glvoc_l05;135">
        <rdfs:label xml:lang="en">thermistor chains</rdfs:label>
        <rdfs:comment xml:lang="en">A group of rigidly-mounted temperature sensors sampled by a common data logger held at various depths in the water column.</rdfs:comment>
        <rdfs:seeAlso rdf:resource="http://vocab.nerc.ac.uk/collection/L05/current/135/"/>
    </rdf:Description>
    <rdf:Description rdf:about="&glvoc_l05;134">
        <rdfs:label xml:lang="en">water temperature sensor</rdfs:label>
        <rdfs:comment xml:lang="en">An instrument that measures the temperature of the water with which it is in contact.</rdfs:comment>
        <rdfs:seeAlso rdf:resource="http://vocab.nerc.ac.uk/collection/L05/current/134/"/>
    </rdf:Description>
    <rdf:Description rdf:about="&glvoc_l05;376">
        <rdfs:label xml:lang="en">sediment surface markers</rdfs:label>
        <rdfs:comment xml:lang="en">Physical markers that allow changes in the position of the boundary between sediment and air or water by visible comparison against marked graduations in units of measurement of dimension length.</rdfs:comment>
        <rdfs:seeAlso rdf:resource="http://vocab.nerc.ac.uk/collection/L05/current/376/"/>
    </rdf:Description>
    <rdf:Description rdf:about="&glvoc_l05;23">
        <rdfs:label xml:lang="en">pelagic trawl nets</rdfs:label>
        <rdfs:comment xml:lang="en">A net towed through the water column designed to sample free-swimming nekton or fish.</rdfs:comment>
        <rdfs:seeAlso rdf:resource="http://vocab.nerc.ac.uk/collection/L05/current/23/"/>
    </rdf:Description>
    <rdf:Description rdf:about="&glvoc_l05;379">
        <rdfs:label xml:lang="en">altimeters</rdfs:label>
        <rdfs:comment xml:lang="en">Instruments that measure their distance above a specified elevation such as the sea surface or the seabed. Classification includes acoustic and pressure-based instruments that are designed to provide platform z co-ordinate spatial coverage in the atmosphere or a water body. It excludes remote sensing instruments such as LIDAR and satellite radar altimeters designed to map surface elevation.</rdfs:comment>
        <rdfs:seeAlso rdf:resource="http://vocab.nerc.ac.uk/collection/L05/current/379/"/>
    </rdf:Description>
    <rdf:Description rdf:about="&glvoc_l05;378">
        <rdfs:label xml:lang="en">sediment profile imagers</rdfs:label>
        <rdfs:comment xml:lang="en">Devices that provide in-situ still or video images of a section including bottom water, the undisturbed sediment-water interface and the upper sediment layers.</rdfs:comment>
        <rdfs:seeAlso rdf:resource="http://vocab.nerc.ac.uk/collection/L05/current/378/"/>
    </rdf:Description>
    <rdf:Description rdf:about="&glvoc_l05;21">
        <rdfs:label xml:lang="en">plankton recorders</rdfs:label>
        <rdfs:comment xml:lang="en">A device that continuously samples a flow of water, separating and fixing plankton for subsequent identification and counting.</rdfs:comment>
        <rdfs:seeAlso rdf:resource="http://vocab.nerc.ac.uk/collection/L05/current/21/"/>
    </rdf:Description>
    <rdf:Description rdf:about="&glvoc_l05;131">
        <rdfs:label xml:lang="en">CTD undulators</rdfs:label>
        <rdfs:comment xml:lang="en">A package towed at varying depths by a ship, always carrying pressure, temperature and conductivity sensors. Addional optional sensors include fluorometers, transmissometers and radiometers.</rdfs:comment>
        <rdfs:seeAlso rdf:resource="http://vocab.nerc.ac.uk/collection/L05/current/131/"/>
    </rdf:Description>
    <rdf:Description rdf:about="&glvoc_l05;373">
        <rdfs:label xml:lang="en">&gt;2000 Hz top-bandwidth single-channel seismic reflection systems</rdfs:label>
        <rdfs:comment xml:lang="en">An energy source with a frequency up to &gt;2000 Hz (sampling interval lower than 0.25 msec) plus a single string of towed hydrophones (streamer) that determine geologic structure by detecting waves reflected by subsurface layers.</rdfs:comment>
        <rdfs:seeAlso rdf:resource="http://vocab.nerc.ac.uk/collection/L05/current/373/"/>
    </rdf:Description>
    <rdf:Description rdf:about="&glvoc_l05;372">
        <rdfs:label xml:lang="en">2000 Hz top-bandwidth single-channel seismic reflection systems</rdfs:label>
        <rdfs:comment xml:lang="en">An energy source with a frequency up to 2000 Hz (sampling interval ranging from 0.5-0.25 msec) plus a single string of towed hydrophones (streamer) that determine geologic structure by detecting waves reflected by subsurface layers.</rdfs:comment>
        <rdfs:seeAlso rdf:resource="http://vocab.nerc.ac.uk/collection/L05/current/372/"/>
    </rdf:Description>
    <rdf:Description rdf:about="&glvoc_l05;130">
        <rdfs:label xml:lang="en">CTD</rdfs:label>
        <rdfs:comment xml:lang="en">A package lowered and raised vertically from a surface platform, usually a ship, always carrying pressure, temperature and conductivity sensors. Addional optional sensors include fluorometers, transmissometers and radiometers.  The package may also carry water bottles.</rdfs:comment>
        <rdfs:seeAlso rdf:resource="http://vocab.nerc.ac.uk/collection/L05/current/130/"/>
    </rdf:Description>
    <rdf:Description rdf:about="&glvoc_l05;133">
        <rdfs:label xml:lang="en">thermosalinographs</rdfs:label>
        <rdfs:comment xml:lang="en">Temperature and conductivity sensors mounted on a sea-surface platform continuously measuring a surface water supply.</rdfs:comment>
        <rdfs:seeAlso rdf:resource="http://vocab.nerc.ac.uk/collection/L05/current/133/"/>
    </rdf:Description>
    <rdf:Description rdf:about="&glvoc_l05;375">
        <rdfs:label xml:lang="en">250 Hz top-bandwidth multi-channel seismic reflection systems</rdfs:label>
        <rdfs:comment xml:lang="en">An energy source with a frequency up to 250 Hz (sampling interval ranging from 2-8 msec) plus a multiple strings of towed hydrophones (streamers) that determine geologic structure by detecting waves reflected by subsurface layers.</rdfs:comment>
        <rdfs:seeAlso rdf:resource="http://vocab.nerc.ac.uk/collection/L05/current/375/"/>
    </rdf:Description>
    <rdf:Description rdf:about="&glvoc_l05;374">
        <rdfs:label xml:lang="en">60 Hz top-bandwidth multi-channel seismic reflection systems</rdfs:label>
        <rdfs:comment xml:lang="en">An energy source with a frequency up to 60 Hz (sampling interval higher than 8 msec) plus a multiple strings of towed hydrophones (streamers) that determine geologic structure by detecting waves reflected by subsurface layers.</rdfs:comment>
        <rdfs:seeAlso rdf:resource="http://vocab.nerc.ac.uk/collection/L05/current/374/"/>
    </rdf:Description>
    <rdf:Description rdf:about="&glvoc_l05;132">
        <rdfs:label xml:lang="en">bathythermographs</rdfs:label>
        <rdfs:comment xml:lang="en">Instruments that measure vertical profiles of sea temperature by either lowering a pressure plus temperature senor package (MBT) or dropping a free falling disposable sensor (XBT).</rdfs:comment>
        <rdfs:seeAlso rdf:resource="http://vocab.nerc.ac.uk/collection/L05/current/132/"/>
    </rdf:Description>
    <rdf:Description rdf:about="&glvoc_l05;PERMON">
        <rdfs:label xml:lang="en">Performance monitors</rdfs:label>
        <rdfs:comment xml:lang="en">Sensors or instruments that monitor whether a platform or environmental sensors on the platform are functioning.</rdfs:comment>
        <rdfs:seeAlso rdf:resource="http://vocab.nerc.ac.uk/collection/L05/current/PERMON/"/>
    </rdf:Description>
    <rdf:Description rdf:about="&glvoc_l05;EXHL">
        <rdfs:label xml:lang="en">high resolution low penetration explosives</rdfs:label>
        <rdfs:comment xml:lang="en">Groups all explosives that allows high resolution but low penetration surveys.</rdfs:comment>
        <rdfs:seeAlso rdf:resource="http://vocab.nerc.ac.uk/collection/L05/current/EXHL/"/>
    </rdf:Description>
    <rdf:Description rdf:about="&glvoc_l05;371">
        <rdfs:label xml:lang="en">60 Hz top-bandwidth single-channel seismic reflection systems</rdfs:label>
        <rdfs:comment xml:lang="en">An energy source with a frequency up to 60 Hz (sampling interval higher than 8 msec) plus a single string of towed hydrophones (streamer) that determine geologic structure by detecting waves reflected by subsurface layers.</rdfs:comment>
        <rdfs:seeAlso rdf:resource="http://vocab.nerc.ac.uk/collection/L05/current/371/"/>
    </rdf:Description>
    <rdf:Description rdf:about="&glvoc_l05;370">
        <rdfs:label xml:lang="en">geothermometers</rdfs:label>
        <rdfs:comment xml:lang="en">Instruments carrying a sensor that determines the temperature (degree of hotness) within geological units.</rdfs:comment>
        <rdfs:seeAlso rdf:resource="http://vocab.nerc.ac.uk/collection/L05/current/370/"/>
    </rdf:Description>
    <rdf:Description rdf:about="&glvoc_l05;13">
        <rdfs:label xml:lang="en">aerosol samplers</rdfs:label>
        <rdfs:comment xml:lang="en">A device that collects a sample of aerosol (dry particles or liquid droplets) from the atmosphere.</rdfs:comment>
        <rdfs:seeAlso rdf:resource="http://vocab.nerc.ac.uk/collection/L05/current/13/"/>
    </rdf:Description>
    <rdf:Description rdf:about="&glvoc_l05;14">
        <rdfs:label xml:lang="en">precipitation samplers</rdfs:label>
        <rdfs:comment xml:lang="en">A device that collects a sample of precipitation (rain, hail or snow) as it falls.</rdfs:comment>
        <rdfs:seeAlso rdf:resource="http://vocab.nerc.ac.uk/collection/L05/current/14/"/>
    </rdf:Description>
    <rdf:Description rdf:about="&glvoc_l05;366">
        <rdfs:label xml:lang="en">&gt;2000 Hz top-bandwidth multi-channel seismic reflection systems</rdfs:label>
        <rdfs:comment xml:lang="en">An energy source with a frequency up to &gt;2000 Hz (sampling interval lower than 0.25 msec) plus a multiple strings of towed hydrophones (streamers) that determine geologic structure by detecting waves reflected by subsurface layers.</rdfs:comment>
        <rdfs:seeAlso rdf:resource="http://vocab.nerc.ac.uk/collection/L05/current/366/"/>
    </rdf:Description>
    <rdf:Description rdf:about="&glvoc_l05;124">
        <rdfs:label xml:lang="en">transmissometers</rdfs:label>
        <rdfs:comment xml:lang="en">Systems that measure the attenuation of electromagnetic radiation by the water column. Includes human observer plus Secchi Disk.</rdfs:comment>
        <rdfs:seeAlso rdf:resource="http://vocab.nerc.ac.uk/collection/L05/current/124/"/>
    </rdf:Description>
    <rdf:Description rdf:about="&glvoc_l05;33">
        <rdfs:label xml:lang="en">sediment traps</rdfs:label>
        <rdfs:comment xml:lang="en">A collector of particulates as they sink through the water column.</rdfs:comment>
        <rdfs:seeAlso rdf:resource="http://vocab.nerc.ac.uk/collection/L05/current/33/"/>
    </rdf:Description>
    <rdf:Description rdf:about="&glvoc_l05;365">
        <rdfs:label xml:lang="en">2000 Hz top-bandwidth multi-channel seismic reflection systems</rdfs:label>
        <rdfs:comment xml:lang="en">An energy source with a frequency up to 2000 Hz (sampling interval ranging from 0.5-0.25 msec) plus a multiple strings of towed hydrophones (streamers) that determine geologic structure by detecting waves reflected by subsurface layers.</rdfs:comment>
        <rdfs:seeAlso rdf:resource="http://vocab.nerc.ac.uk/collection/L05/current/365/"/>
    </rdf:Description>
    <rdf:Description rdf:about="&glvoc_l05;123">
        <rdfs:label xml:lang="en">optical backscatter sensors</rdfs:label>
        <rdfs:comment xml:lang="en">Instrument that measures the amount of electromagnetic radiation emitted into the water column returned to the instrument.</rdfs:comment>
        <rdfs:seeAlso rdf:resource="http://vocab.nerc.ac.uk/collection/L05/current/123/"/>
    </rdf:Description>
    <rdf:Description rdf:about="&glvoc_l05;31">
        <rdfs:label xml:lang="en">continuous water samplers</rdfs:label>
        <rdfs:comment xml:lang="en">A device that continuously supplies a flow of water either to an analytical instrument, over a sensor or from which samples may be drawn.</rdfs:comment>
        <rdfs:seeAlso rdf:resource="http://vocab.nerc.ac.uk/collection/L05/current/31/"/>
    </rdf:Description>
    <rdf:Description rdf:about="&glvoc_l05;368">
        <rdfs:label xml:lang="en">seismometers</rdfs:label>
        <rdfs:comment xml:lang="en">Devices placed on the ground or seabed to measure physical movement of that substrate.</rdfs:comment>
        <rdfs:seeAlso rdf:resource="http://vocab.nerc.ac.uk/collection/L05/current/368/"/>
    </rdf:Description>
    <rdf:Description rdf:about="&glvoc_l05;32">
        <rdfs:label xml:lang="en">particulates samplers</rdfs:label>
        <rdfs:comment xml:lang="en">A system that collects samples of water column particulates such as in-situ high volume filtration systems liks SAPs.</rdfs:comment>
        <rdfs:seeAlso rdf:resource="http://vocab.nerc.ac.uk/collection/L05/current/32/"/>
    </rdf:Description>
    <rdf:Description rdf:about="&glvoc_l05;367">
        <rdfs:label xml:lang="en">&gt;2000 Hz top-bandwidth sub-bottom penetrator and mud profiler systems</rdfs:label>
        <rdfs:comment xml:lang="en">Devices that provide information on unconsolidated sediment structure through transmission and reception of an energy source with a frequency corresponding to a sampling interval lower than 0.25 msec.</rdfs:comment>
        <rdfs:seeAlso rdf:resource="http://vocab.nerc.ac.uk/collection/L05/current/367/"/>
    </rdf:Description>
    <rdf:Description rdf:about="&glvoc_l05;362">
        <rdfs:label xml:lang="en">250 Hz top-bandwidth single-channel seismic reflection systems</rdfs:label>
        <rdfs:comment xml:lang="en">An energy source with a frequency up to 250 Hz (sampling interval ranging from 2-8 msec) plus a single string of towed hydrophones (streamer) that determine geologic structure by detecting waves reflected by subsurface layers.</rdfs:comment>
        <rdfs:seeAlso rdf:resource="http://vocab.nerc.ac.uk/collection/L05/current/362/"/>
    </rdf:Description>
    <rdf:Description rdf:about="&glvoc_l05;361">
        <rdfs:label xml:lang="en">penetrometers</rdfs:label>
        <rdfs:comment xml:lang="en">Dynamic or passive devices that determine the consistency or hardness of soil or sediment by measuring the depth or rate of penetration of a needle or cone rig into it when a known force is applied.</rdfs:comment>
        <rdfs:seeAlso rdf:resource="http://vocab.nerc.ac.uk/collection/L05/current/361/"/>
    </rdf:Description>
    <rdf:Description rdf:about="&glvoc_l05;30">
        <rdfs:label xml:lang="en">discrete water samplers</rdfs:label>
        <rdfs:comment xml:lang="en">A device that collects an in-situ discrete water sample from any depth and returns it to the surface without contamination by the waters through which it passes, such as a water bottle.</rdfs:comment>
        <rdfs:seeAlso rdf:resource="http://vocab.nerc.ac.uk/collection/L05/current/30/"/>
    </rdf:Description>
    <rdf:Description rdf:about="&glvoc_l05;364">
        <rdfs:label xml:lang="en">1000 Hz top-bandwidth multi-channel seismic reflection systems</rdfs:label>
        <rdfs:comment xml:lang="en">An energy source with a frequency up to 1000 Hz (sampling interval ranging from 2-0.5 msec) plus a multiple strings of towed hydrophones (streamers) that determine geologic structure by detecting waves reflected by subsurface layers.</rdfs:comment>
        <rdfs:seeAlso rdf:resource="http://vocab.nerc.ac.uk/collection/L05/current/364/"/>
    </rdf:Description>
    <rdf:Description rdf:about="&glvoc_l05;122">
        <rdfs:label xml:lang="en">radiometers</rdfs:label>
        <rdfs:comment xml:lang="en">Instrument that measures the intensity of electromagnetic radiation in either the atmosphere or the water column.</rdfs:comment>
        <rdfs:seeAlso rdf:resource="http://vocab.nerc.ac.uk/collection/L05/current/122/"/>
    </rdf:Description>
    <rdf:Description rdf:about="&glvoc_l05;121">
        <rdfs:label xml:lang="en">satellite tracking system</rdfs:label>
        <rdfs:comment xml:lang="en">A network of statellites that determines the position of a transponder by triangulation such as Argos.  Generally used to track surface buoys for the determination of Lagrangian currents.</rdfs:comment>
        <rdfs:seeAlso rdf:resource="http://vocab.nerc.ac.uk/collection/L05/current/121/"/>
    </rdf:Description>
    <rdf:Description rdf:about="&glvoc_l05;363">
        <rdfs:label xml:lang="en">1000 Hz top-bandwidth single-channel seismic reflection systems</rdfs:label>
        <rdfs:comment xml:lang="en">An energy source with a frequency up to 1000 Hz (sampling interval ranging from 2-0.5 msec) plus a single string of towed hydrophones (streamer) that determine geologic structure by detecting waves reflected by subsurface layers.</rdfs:comment>
        <rdfs:seeAlso rdf:resource="http://vocab.nerc.ac.uk/collection/L05/current/363/"/>
    </rdf:Description>
    <rdf:Description rdf:about="&glvoc_l05;EMSR">
        <rdfs:label xml:lang="en">elecromagnetic sensors</rdfs:label>
        <rdfs:comment xml:lang="en">In-situ sensors that simultaneuously measure electrical and magnetic fields.  They are usually moored on the seabed for long periods of time for determination of deep structure through monitoring magnetotelluric currents.  However, some may also be configured to be receivers for active electromagnetic surveys such as CSEM.</rdfs:comment>
        <rdfs:seeAlso rdf:resource="http://vocab.nerc.ac.uk/collection/L05/current/EMSR/"/>
    </rdf:Description>
    <rdf:Description rdf:about="&glvoc_l05;369">
        <rdfs:label xml:lang="en">hydrophones</rdfs:label>
        <rdfs:comment xml:lang="en">Devices containing transducers that convert underwater sound waves into electrical signals.</rdfs:comment>
        <rdfs:seeAlso rdf:resource="http://vocab.nerc.ac.uk/collection/L05/current/369/"/>
    </rdf:Description>
    <rdf:Description rdf:about="&glvoc_l05;360">
        <rdfs:label xml:lang="en">piezometers</rdfs:label>
        <rdfs:comment xml:lang="en">Devices that measure fluid  (air, gas, water, or oil) pressure within soil, sediment, rock or concrete providing information such as water table level in an aquifer system.</rdfs:comment>
        <rdfs:seeAlso rdf:resource="http://vocab.nerc.ac.uk/collection/L05/current/360/"/>
    </rdf:Description>
    <rdf:Description rdf:about="&glvoc_l05;CSEM">
        <rdfs:label xml:lang="en">controlled-source elecromagnetic systems</rdfs:label>
        <rdfs:comment xml:lang="en">Systems that measure sub-surface resistivity structure through the measurement of the electromegnetic fields resulting from stimulation by a towed source.  Includes systems incorporating both transmitter and receiver and systems where the transmitter and receiver are separate.</rdfs:comment>
        <rdfs:seeAlso rdf:resource="http://vocab.nerc.ac.uk/collection/L05/current/CSEM/"/>
    </rdf:Description>
    <rdf:Description rdf:about="&glvoc_l05;24">
        <rdfs:label xml:lang="en">benthos samplers</rdfs:label>
        <rdfs:comment xml:lang="en">A net or sledge dragged across the seabed designed to sample benthic fauna.</rdfs:comment>
        <rdfs:seeAlso rdf:resource="http://vocab.nerc.ac.uk/collection/L05/current/24/"/>
    </rdf:Description>
</rdf:RDF>



<!-- Generated by the OWL API (version 3.5.1) http://owlapi.sourceforge.net -->

