@prefix : <http://schema.geolink.org/1.0/voc/nvs/L06#> .
@prefix dc: <http://purl.org/dc/elements/1.1/> .
@prefix dcterms: <http://purl.org/dc/terms/> .
@prefix glbase: <http://schema.geolink.org/1.0/base/main#> .
@prefix idscheme: <http://schema.geolink.org/1.0/voc/identifierscheme#> .
@prefix owl: <http://www.w3.org/2002/07/owl#> .
@prefix rdf: <http://www.w3.org/1999/02/22-rdf-syntax-ns#> .
@prefix rdfs: <http://www.w3.org/2000/01/rdf-schema#> .
@prefix skos: <http://www.w3.org/2004/02/skos/core#> .
@prefix xml: <http://www.w3.org/XML/1998/namespace> .
@prefix xsd: <http://www.w3.org/2001/XMLSchema#> .
glbase:hasIdentifier a owl:ObjectProperty .
glbase:hasIdentifierScheme a owl:ObjectProperty .
glbase:hasIdentifierValue a owl:DatatypeProperty .
<http://schema.geolink.org/1.0/voc/nvs/L06> a owl:Ontology ;
    rdfs:label "SeaVoX Platform Categories" ;
    dcterms:creator "EarthCube GeoLink project"@en ;
    dcterms:date "2016-01-07 02:00:02.0" ;
    dcterms:title "SeaVoX Platform Categories" ;
    rdfs:comment "This ontology captures SeaVoX platform categories (e.g., vessel, mooring, etc.) as hosted in the NERC vocabulary server"@en ;
    rdfs:seeAlso <http://vocab.nerc.ac.uk/collection/L06/current/> .
<http://vocab.nerc.ac.uk/collection/L06/current/0/> a glbase:PlatformType,
        owl:Class,
        owl:NamedIndividual ;
    rdfs:label "unknown"@en ;
    dcterms:creator "SeaDataNet and MarineXML Vocabulary Content Governance Group" ;
    dcterms:date "2006-07-07 10:38:37.0" ;
    glbase:hasIdentifier [ glbase:hasIdentifierScheme idscheme:sdnl06 ;
            glbase:hasIdentifierValue "SDN:L06::0" ] ;
    rdfs:comment "The correct value is not known to, and not computable by, the creator of this information. However, a correct value probably exists."@en ;
    rdfs:subClassOf glbase:Platform .
<http://vocab.nerc.ac.uk/collection/L06/current/11/> a glbase:PlatformType,
        owl:Class,
        owl:NamedIndividual ;
    rdfs:label "fixed benthic node"@en ;
    dcterms:creator "SeaDataNet and MarineXML Vocabulary Content Governance Group" ;
    dcterms:date "2013-08-20 13:53:41.0" ;
    glbase:hasIdentifier [ glbase:hasIdentifierScheme idscheme:sdnl06 ;
            glbase:hasIdentifierValue "SDN:L06::11" ] ;
    rdfs:comment "A collection of oceanographic instruments mounted at a fixed position on the seabed (e.g. POL Monitoring Platform, seabed ADCP)."@en ;
    rdfs:subClassOf <http://vocab.nerc.ac.uk/collection/L06/current/10/>,
        <http://vocab.nerc.ac.uk/collection/L06/current/48/> .
<http://vocab.nerc.ac.uk/collection/L06/current/12/> a glbase:PlatformType,
        owl:Class,
        owl:NamedIndividual ;
    rdfs:label "sea bed vehicle"@en ;
    dcterms:creator "SeaDataNet and MarineXML Vocabulary Content Governance Group" ;
    dcterms:date "2006-07-07 10:38:37.0" ;
    glbase:hasIdentifier [ glbase:hasIdentifierScheme idscheme:sdnl06 ;
            glbase:hasIdentifierValue "SDN:L06::12" ] ;
    rdfs:comment "An instrumented platform that is propelled on wheels or tracks on the seabed (e.g benthic crawler)."@en ;
    rdfs:subClassOf <http://vocab.nerc.ac.uk/collection/L06/current/10/> .
<http://vocab.nerc.ac.uk/collection/L06/current/13/> a glbase:PlatformType,
        owl:Class,
        owl:NamedIndividual ;
    rdfs:label "beach/intertidal zone structure"@en ;
    dcterms:creator "SeaDataNet and MarineXML Vocabulary Content Governance Group" ;
    dcterms:date "2006-07-07 10:38:37.0" ;
    glbase:hasIdentifier [ glbase:hasIdentifierScheme idscheme:sdnl06 ;
            glbase:hasIdentifierValue "SDN:L06::13" ] ;
    rdfs:comment "A structure to which instrumentation may be attached that is either in air or under water depending on the state of the tide and weather conditions."@en ;
    rdfs:subClassOf <http://vocab.nerc.ac.uk/collection/L06/current/10/> .
<http://vocab.nerc.ac.uk/collection/L06/current/14/> a glbase:PlatformType,
        owl:Class,
        owl:NamedIndividual ;
    rdfs:label "land/onshore structure"@en ;
    dcterms:creator "SeaDataNet and MarineXML Vocabulary Content Governance Group" ;
    dcterms:date "2013-08-20 13:53:41.0" ;
    glbase:hasIdentifier [ glbase:hasIdentifierScheme idscheme:sdnl06 ;
            glbase:hasIdentifierValue "SDN:L06::14" ] ;
    rdfs:comment "A fixed man-made structure on land to which instrumentation may be attached (e.g. meteorological tower)."@en ;
    rdfs:subClassOf <http://vocab.nerc.ac.uk/collection/L06/current/10/> .
<http://vocab.nerc.ac.uk/collection/L06/current/15/> a glbase:PlatformType,
        owl:Class,
        owl:NamedIndividual ;
    rdfs:label "land/onshore vehicle"@en ;
    dcterms:creator "SeaDataNet and MarineXML Vocabulary Content Governance Group" ;
    dcterms:date "2012-07-19 09:21:27.0" ;
    glbase:hasIdentifier [ glbase:hasIdentifierScheme idscheme:sdnl06 ;
            glbase:hasIdentifierValue "SDN:L06::15" ] ;
    rdfs:comment "An instrumented vehicle or sample collector that operates on the solid surface of the Earth (e.g. mobile meteorological station, land crawler, snowmobile)."@en ;
    rdfs:subClassOf <http://vocab.nerc.ac.uk/collection/L06/current/10/> .
<http://vocab.nerc.ac.uk/collection/L06/current/16/> a glbase:PlatformType,
        owl:Class,
        owl:NamedIndividual ;
    rdfs:label "offshore structure"@en ;
    dcterms:creator "SeaDataNet and MarineXML Vocabulary Content Governance Group" ;
    dcterms:date "2013-08-20 13:53:41.0" ;
    glbase:hasIdentifier [ glbase:hasIdentifierScheme idscheme:sdnl06 ;
            glbase:hasIdentifierValue "SDN:L06::16" ] ;
    rdfs:comment "A fixed (for the duration of the measurements) man-made structure away from the coast to which instrumentation may be attached (e.g. oil rig, gas rig or jack-up barge)."@en ;
    rdfs:subClassOf <http://vocab.nerc.ac.uk/collection/L06/current/10/> .
<http://vocab.nerc.ac.uk/collection/L06/current/17/> a glbase:PlatformType,
        owl:Class,
        owl:NamedIndividual ;
    rdfs:label "coastal structure"@en ;
    dcterms:creator "SeaDataNet and MarineXML Vocabulary Content Governance Group" ;
    dcterms:date "2013-08-20 13:53:41.0" ;
    glbase:hasIdentifier [ glbase:hasIdentifierScheme idscheme:sdnl06 ;
            glbase:hasIdentifierValue "SDN:L06::17" ] ;
    rdfs:comment "A fixed man-made structure permanently linked to land with access to water at all states of the tide to which instrumentation may be attached (e.g. pier)."@en ;
    rdfs:subClassOf <http://vocab.nerc.ac.uk/collection/L06/current/10/> .
<http://vocab.nerc.ac.uk/collection/L06/current/18/> a glbase:PlatformType,
        owl:Class,
        owl:NamedIndividual ;
    rdfs:label "river station"@en ;
    dcterms:creator "SeaDataNet and MarineXML Vocabulary Content Governance Group" ;
    dcterms:date "2006-08-23 16:03:17.0" ;
    glbase:hasIdentifier [ glbase:hasIdentifierScheme idscheme:sdnl06 ;
            glbase:hasIdentifierValue "SDN:L06::18" ] ;
    rdfs:comment "An instrumented structure in a river upstream of its tidal limit."@en ;
    rdfs:subClassOf <http://vocab.nerc.ac.uk/collection/L06/current/10/> .
<http://vocab.nerc.ac.uk/collection/L06/current/19/> a glbase:PlatformType,
        owl:Class,
        owl:NamedIndividual ;
    rdfs:label "mesocosm bag"@en ;
    dcterms:creator "SeaDataNet and MarineXML Vocabulary Content Governance Group" ;
    dcterms:date "2006-07-07 10:38:37.0" ;
    glbase:hasIdentifier [ glbase:hasIdentifierScheme idscheme:sdnl06 ;
            glbase:hasIdentifierValue "SDN:L06::19" ] ;
    rdfs:comment "A large polythene bag containing a water sample suspended in the natural environment so that it shares ambient physical conditions such as temperature and light levels, but is chemically isolated to allow experiments such as fertilisation."@en ;
    rdfs:subClassOf <http://vocab.nerc.ac.uk/collection/L06/current/10/> .
<http://vocab.nerc.ac.uk/collection/L06/current/21/> a glbase:PlatformType,
        owl:Class,
        owl:NamedIndividual ;
    rdfs:label "propelled manned submersible"@en ;
    dcterms:creator "SeaDataNet and MarineXML Vocabulary Content Governance Group" ;
    dcterms:date "2013-08-20 13:53:41.0" ;
    glbase:hasIdentifier [ glbase:hasIdentifierScheme idscheme:sdnl06 ;
            glbase:hasIdentifierValue "SDN:L06::21" ] ;
    rdfs:comment "A platform operating in the water column that has both self-contained propulsion and at least one human operator on board (e.g. submarine)."@en ;
    rdfs:subClassOf <http://vocab.nerc.ac.uk/collection/L06/current/20/> .
<http://vocab.nerc.ac.uk/collection/L06/current/22/> a glbase:PlatformType,
        owl:Class,
        owl:NamedIndividual ;
    rdfs:label "propelled unmanned submersible"@en ;
    dcterms:creator "SeaDataNet and MarineXML Vocabulary Content Governance Group" ;
    dcterms:date "2006-07-07 10:38:37.0" ;
    glbase:hasIdentifier [ glbase:hasIdentifierScheme idscheme:sdnl06 ;
            glbase:hasIdentifierValue "SDN:L06::22" ] ;
    rdfs:comment "A platform operating in the water column attached to a mothership by an umbilical with limited propulsion and no human operator on board (e.g. ROV)."@en ;
    rdfs:subClassOf <http://vocab.nerc.ac.uk/collection/L06/current/20/> .
<http://vocab.nerc.ac.uk/collection/L06/current/23/> a glbase:PlatformType,
        owl:Class,
        owl:NamedIndividual ;
    rdfs:label "towed unmanned submersible"@en ;
    dcterms:creator "SeaDataNet and MarineXML Vocabulary Content Governance Group" ;
    dcterms:date "2013-08-20 13:53:41.0" ;
    glbase:hasIdentifier [ glbase:hasIdentifierScheme idscheme:sdnl06 ;
            glbase:hasIdentifierValue "SDN:L06::23" ] ;
    rdfs:comment "A vehicle towed by rigid cable through the water column at fixed or varying depth with no propulsion and no human operator (e.g. Towfish, Scanfish, UOR, SeaSoar)."@en ;
    rdfs:subClassOf <http://vocab.nerc.ac.uk/collection/L06/current/20/> .
<http://vocab.nerc.ac.uk/collection/L06/current/24/> a glbase:PlatformType,
        owl:Class,
        owl:NamedIndividual ;
    rdfs:label "drifting manned submersible"@en ;
    dcterms:creator "SeaDataNet and MarineXML Vocabulary Content Governance Group" ;
    dcterms:date "2006-07-07 10:38:37.0" ;
    glbase:hasIdentifier [ glbase:hasIdentifierScheme idscheme:sdnl06 ;
            glbase:hasIdentifierValue "SDN:L06::24" ] ;
    rdfs:comment "A platform operating in the water column attached to a mothership by an umbilical but with no means of propulsion that has at least one human operator on board (e.g. bathysphere)."@en ;
    rdfs:subClassOf <http://vocab.nerc.ac.uk/collection/L06/current/20/> .
<http://vocab.nerc.ac.uk/collection/L06/current/26/> a glbase:PlatformType,
        owl:Class,
        owl:NamedIndividual ;
    rdfs:label "lowered unmanned submersible"@en ;
    dcterms:creator "SeaDataNet and MarineXML Vocabulary Content Governance Group" ;
    dcterms:date "2008-12-04 09:08:25.0" ;
    glbase:hasIdentifier [ glbase:hasIdentifierScheme idscheme:sdnl06 ;
            glbase:hasIdentifierValue "SDN:L06::26" ] ;
    rdfs:comment "An unmanned platform lowered and raised vertically by a cable from the mothership.  Includes any type of profiling sensor mounting such as CTD frames, profiling radiometers and instrumented nets."@en ;
    rdfs:subClassOf <http://vocab.nerc.ac.uk/collection/L06/current/20/> .
<http://vocab.nerc.ac.uk/collection/L06/current/27/> a glbase:PlatformType,
        owl:Class,
        owl:NamedIndividual ;
    rdfs:label "sub-surface gliders"@en ;
    dcterms:creator "SeaDataNet and MarineXML Vocabulary Content Governance Group" ;
    dcterms:date "2013-08-20 13:56:39.0" ;
    glbase:hasIdentifier [ glbase:hasIdentifierScheme idscheme:sdnl06 ;
            glbase:hasIdentifierValue "SDN:L06::27" ] ;
    rdfs:comment "Platforms with buoyancy-based propulsion that are capable of operations at variable depths which are not constrained to be near the sea surface."@en ;
    rdfs:subClassOf <http://vocab.nerc.ac.uk/collection/L06/current/25/> .
<http://vocab.nerc.ac.uk/collection/L06/current/30/> a glbase:PlatformType,
        owl:Class,
        owl:NamedIndividual ;
    rdfs:label "ship"@en ;
    dcterms:creator "SeaDataNet and MarineXML Vocabulary Content Governance Group" ;
    dcterms:date "2006-07-07 10:38:37.0" ;
    glbase:hasIdentifier [ glbase:hasIdentifierScheme idscheme:sdnl06 ;
            glbase:hasIdentifierValue "SDN:L06::30" ] ;
    rdfs:comment "A large platform operating on the surface of the water column. Objective definitions for guidelines: >50m length (EU), >100 foot length (USA), >300 GRT weight (SOLAS). Subjective definition: a ship is a vessel big enough to carry a boat."@en ;
    rdfs:subClassOf <http://vocab.nerc.ac.uk/collection/L06/current/3Z/> .
<http://vocab.nerc.ac.uk/collection/L06/current/31/> a glbase:PlatformType,
        owl:Class,
        owl:NamedIndividual ;
    rdfs:label "research vessel"@en ;
    dcterms:creator "SeaDataNet and MarineXML Vocabulary Content Governance Group" ;
    dcterms:date "2007-11-20 14:59:20.0" ;
    glbase:hasIdentifier [ glbase:hasIdentifierScheme idscheme:sdnl06 ;
            glbase:hasIdentifierValue "SDN:L06::31" ] ;
    rdfs:comment "A platform of any size operating on the surface of the water column in unpredictable locations that is specifically equipped, manned and operated for scientific, usually oceanographic, research."@en ;
    rdfs:subClassOf <http://vocab.nerc.ac.uk/collection/L06/current/3Z/> .
<http://vocab.nerc.ac.uk/collection/L06/current/32/> a glbase:PlatformType,
        owl:Class,
        owl:NamedIndividual ;
    rdfs:label "vessel of opportunity"@en ;
    dcterms:creator "SeaDataNet and MarineXML Vocabulary Content Governance Group" ;
    dcterms:date "2006-07-07 10:38:37.0" ;
    glbase:hasIdentifier [ glbase:hasIdentifierScheme idscheme:sdnl06 ;
            glbase:hasIdentifierValue "SDN:L06::32" ] ;
    rdfs:comment "A platform for purpose of commerce of any size operating on the surface of the water column in unpredictable locations that regularly collects scientific (oceanographic and meteorological) data (e.g. an instrumented cargo vessel)."@en ;
    rdfs:subClassOf <http://vocab.nerc.ac.uk/collection/L06/current/3Z/> .
<http://vocab.nerc.ac.uk/collection/L06/current/33/> a glbase:PlatformType,
        owl:Class,
        owl:NamedIndividual ;
    rdfs:label "self-propelled small boat"@en ;
    dcterms:creator "SeaDataNet and MarineXML Vocabulary Content Governance Group" ;
    dcterms:date "2006-07-07 10:38:37.0" ;
    glbase:hasIdentifier [ glbase:hasIdentifierScheme idscheme:sdnl06 ;
            glbase:hasIdentifierValue "SDN:L06::33" ] ;
    rdfs:comment "A small self-propelled platform operating on the surface of the water column that may be easily removed from the water (e.g. shore-based RIBs, ships' boats)."@en ;
    rdfs:subClassOf <http://vocab.nerc.ac.uk/collection/L06/current/3Z/> .
<http://vocab.nerc.ac.uk/collection/L06/current/34/> a glbase:PlatformType,
        owl:Class,
        owl:NamedIndividual ;
    rdfs:label "vessel at fixed position"@en ;
    dcterms:creator "SeaDataNet and MarineXML Vocabulary Content Governance Group" ;
    dcterms:date "2006-07-07 10:38:37.0" ;
    glbase:hasIdentifier [ glbase:hasIdentifierScheme idscheme:sdnl06 ;
            glbase:hasIdentifierValue "SDN:L06::34" ] ;
    rdfs:comment "A platform of any size occupying a fixed location on the surface of the water column for prolonged periods collecting scientific (oceanographic and meteorological) data as a primary or secondary mission.  Includes light vessels and weather ships."@en ;
    rdfs:subClassOf <http://vocab.nerc.ac.uk/collection/L06/current/3Z/> .
<http://vocab.nerc.ac.uk/collection/L06/current/35/> a glbase:PlatformType,
        owl:Class,
        owl:NamedIndividual ;
    rdfs:label "vessel of opportunity on fixed route"@en ;
    dcterms:creator "SeaDataNet and MarineXML Vocabulary Content Governance Group" ;
    dcterms:date "2006-07-07 10:38:37.0" ;
    glbase:hasIdentifier [ glbase:hasIdentifierScheme idscheme:sdnl06 ;
            glbase:hasIdentifierValue "SDN:L06::35" ] ;
    rdfs:comment "A platform repeatedly following a predictable fixed track on the surface of the water column that collects scientific (oceanographic and meteorological) data (e.g. an instrumented ferry)."@en ;
    rdfs:subClassOf <http://vocab.nerc.ac.uk/collection/L06/current/3Z/> .
<http://vocab.nerc.ac.uk/collection/L06/current/36/> a glbase:PlatformType,
        owl:Class,
        owl:NamedIndividual ;
    rdfs:label "fishing vessel"@en ;
    dcterms:creator "SeaDataNet and MarineXML Vocabulary Content Governance Group" ;
    dcterms:date "2016-01-06 11:37:28.0" ;
    glbase:hasIdentifier [ glbase:hasIdentifierScheme idscheme:sdnl06 ;
            glbase:hasIdentifierValue "SDN:L06::36" ] ;
    rdfs:comment "A platform operating on the surface of the water column whose primary purpose is the commercial harvesting of fish or shellfish but may be engaged in scientific activities such as fish stock surveys or mooring deployments and recoveries."@en ;
    rdfs:subClassOf <http://vocab.nerc.ac.uk/collection/L06/current/3Z/> .
<http://vocab.nerc.ac.uk/collection/L06/current/37/> a glbase:PlatformType,
        owl:Class,
        owl:NamedIndividual ;
    rdfs:label "self-propelled boat"@en ;
    dcterms:creator "SeaDataNet and MarineXML Vocabulary Content Governance Group" ;
    dcterms:date "2006-07-07 10:38:37.0" ;
    glbase:hasIdentifier [ glbase:hasIdentifierScheme idscheme:sdnl06 ;
            glbase:hasIdentifierValue "SDN:L06::37" ] ;
    rdfs:comment "A small self-propelled platform operating on the surface of the water column in unpredictable locations that is smaller than a ship, but too large to easily remove from the water."@en ;
    rdfs:subClassOf <http://vocab.nerc.ac.uk/collection/L06/current/3Z/> .
<http://vocab.nerc.ac.uk/collection/L06/current/38/> a glbase:PlatformType,
        owl:Class,
        owl:NamedIndividual ;
    rdfs:label "man-powered boat"@en ;
    dcterms:creator "SeaDataNet and MarineXML Vocabulary Content Governance Group" ;
    dcterms:date "2006-07-07 10:38:37.0" ;
    glbase:hasIdentifier [ glbase:hasIdentifierScheme idscheme:sdnl06 ;
            glbase:hasIdentifierValue "SDN:L06::38" ] ;
    rdfs:comment "A platform operating on the surface of the water column that is manually propelled and may not be easily removed from the water (e.g. trireme)."@en ;
    rdfs:subClassOf <http://vocab.nerc.ac.uk/collection/L06/current/3Z/> .
<http://vocab.nerc.ac.uk/collection/L06/current/39/> a glbase:PlatformType,
        owl:Class,
        owl:NamedIndividual ;
    rdfs:label "naval vessel"@en ;
    dcterms:creator "SeaDataNet and MarineXML Vocabulary Content Governance Group" ;
    dcterms:date "2007-11-20 14:58:29.0" ;
    glbase:hasIdentifier [ glbase:hasIdentifierScheme idscheme:sdnl06 ;
            glbase:hasIdentifierValue "SDN:L06::39" ] ;
    rdfs:comment "A platform operating on the surface of the water column in unpredictable locations that is primarily equipped, manned and operated for military purposes.  Includes surface warships of all sizes and logistic support vessels."@en ;
    rdfs:subClassOf <http://vocab.nerc.ac.uk/collection/L06/current/3Z/> .
<http://vocab.nerc.ac.uk/collection/L06/current/3A/> a glbase:PlatformType,
        owl:Class,
        owl:NamedIndividual ;
    rdfs:label "man-powered small boat"@en ;
    dcterms:creator "SeaDataNet and MarineXML Vocabulary Content Governance Group" ;
    dcterms:date "2006-07-07 10:38:37.0" ;
    glbase:hasIdentifier [ glbase:hasIdentifierScheme idscheme:sdnl06 ;
            glbase:hasIdentifierValue "SDN:L06::3A" ] ;
    rdfs:comment "A platform operating on the surface of the water column that is manually propelled and may be easily removed from the water (e.g. rowing boat, canoe)."@en ;
    rdfs:subClassOf <http://vocab.nerc.ac.uk/collection/L06/current/3Z/> .
<http://vocab.nerc.ac.uk/collection/L06/current/3C/> a glbase:PlatformType,
        owl:Class,
        owl:NamedIndividual ;
    rdfs:label "surface gliders"@en ;
    dcterms:creator "SeaDataNet and MarineXML Vocabulary Content Governance Group" ;
    dcterms:date "2013-08-20 13:53:41.0" ;
    glbase:hasIdentifier [ glbase:hasIdentifierScheme idscheme:sdnl06 ;
            glbase:hasIdentifierValue "SDN:L06::3C" ] ;
    rdfs:comment "Platforms with buoyancy-based propulsion that operate at a single depth near the sea surface."@en ;
    rdfs:subClassOf <http://vocab.nerc.ac.uk/collection/L06/current/3B/> .
<http://vocab.nerc.ac.uk/collection/L06/current/3D/> a glbase:PlatformType,
        owl:Class,
        owl:NamedIndividual ;
    rdfs:label "drillship"@en ;
    dcterms:creator "SeaDataNet and MarineXML Vocabulary Content Governance Group" ;
    dcterms:date "2015-11-05 08:43:51.0" ;
    glbase:hasIdentifier [ glbase:hasIdentifierScheme idscheme:sdnl06 ;
            glbase:hasIdentifierValue "SDN:L06::3D" ] ;
    rdfs:comment "A drillship is a merchant vessel designed for use in exploratory offshore drilling of new oil and gas wells or for scientific drilling purposes."@en ;
    rdfs:subClassOf <http://vocab.nerc.ac.uk/collection/L06/current/3Z/> .
<http://vocab.nerc.ac.uk/collection/L06/current/41/> a glbase:PlatformType,
        owl:Class,
        owl:NamedIndividual ;
    rdfs:label "moored surface buoy"@en ;
    dcterms:creator "SeaDataNet and MarineXML Vocabulary Content Governance Group" ;
    dcterms:date "2013-08-20 13:53:41.0" ;
    glbase:hasIdentifier [ glbase:hasIdentifierScheme idscheme:sdnl06 ;
            glbase:hasIdentifierValue "SDN:L06::41" ] ;
    rdfs:comment "An unmanned instrumented platform operating on the surface of the water column loosely tethered to the seafloor to maintain a fixed position (e.g. ODAS buoy)."@en ;
    rdfs:subClassOf <http://vocab.nerc.ac.uk/collection/L06/current/48/> .
<http://vocab.nerc.ac.uk/collection/L06/current/43/> a glbase:PlatformType,
        owl:Class,
        owl:NamedIndividual ;
    rdfs:label "subsurface mooring"@en ;
    dcterms:creator "SeaDataNet and MarineXML Vocabulary Content Governance Group" ;
    dcterms:date "2006-07-07 10:38:37.0" ;
    glbase:hasIdentifier [ glbase:hasIdentifierScheme idscheme:sdnl06 ;
            glbase:hasIdentifierValue "SDN:L06::43" ] ;
    rdfs:comment "A collection of oceanographic instruments attached to wires suspended between anchors on the seabed and buoyant spheres in the water column."@en ;
    rdfs:subClassOf <http://vocab.nerc.ac.uk/collection/L06/current/48/> .
<http://vocab.nerc.ac.uk/collection/L06/current/44/> a glbase:PlatformType,
        owl:Class,
        owl:NamedIndividual ;
    rdfs:label "drifting subsurface float"@en ;
    dcterms:creator "SeaDataNet and MarineXML Vocabulary Content Governance Group" ;
    dcterms:date "2013-08-20 13:53:41.0" ;
    glbase:hasIdentifier [ glbase:hasIdentifierScheme idscheme:sdnl06 ;
            glbase:hasIdentifierValue "SDN:L06::44" ] ;
    rdfs:comment "An unmanned instrumented platform drifting freely in the water column at a depth governed by its density (e.g. Swallow float)."@en ;
    rdfs:subClassOf <http://vocab.nerc.ac.uk/collection/L06/current/47/> .
<http://vocab.nerc.ac.uk/collection/L06/current/45/> a glbase:PlatformType,
        owl:Class,
        owl:NamedIndividual ;
    rdfs:label "fixed subsurface vertical profiler"@en ;
    dcterms:creator "SeaDataNet and MarineXML Vocabulary Content Governance Group" ;
    dcterms:date "2013-08-20 13:53:41.0" ;
    glbase:hasIdentifier [ glbase:hasIdentifierScheme idscheme:sdnl06 ;
            glbase:hasIdentifierValue "SDN:L06::45" ] ;
    rdfs:comment "A platform that periodically makes an automated vertical traverse of the water column at a predetermined fixed location. (e.g. YSI vertical profiler, HOMER CTD)."@en ;
    rdfs:subClassOf <http://vocab.nerc.ac.uk/collection/L06/current/48/> .
<http://vocab.nerc.ac.uk/collection/L06/current/46/> a glbase:PlatformType,
        owl:Class,
        owl:NamedIndividual ;
    rdfs:label "drifting subsurface profiling float"@en ;
    dcterms:creator "SeaDataNet and MarineXML Vocabulary Content Governance Group" ;
    dcterms:date "2013-08-20 13:53:41.0" ;
    glbase:hasIdentifier [ glbase:hasIdentifierScheme idscheme:sdnl06 ;
            glbase:hasIdentifierValue "SDN:L06::46" ] ;
    rdfs:comment "An unmanned instrumented platform drifting freely in the water column that periodically makes vertical traverses through the water column (e.g. Argo float)."@en ;
    rdfs:subClassOf <http://vocab.nerc.ac.uk/collection/L06/current/47/> .
<http://vocab.nerc.ac.uk/collection/L06/current/49/> a glbase:PlatformType,
        owl:Class,
        owl:NamedIndividual ;
    rdfs:label "surface ice buoy"@en ;
    dcterms:creator "SeaDataNet and MarineXML Vocabulary Content Governance Group" ;
    dcterms:date "2013-08-20 14:00:20.0" ;
    glbase:hasIdentifier [ glbase:hasIdentifierScheme idscheme:sdnl06 ;
            glbase:hasIdentifierValue "SDN:L06::49" ] ;
    rdfs:comment "An undrogued (i.e. no sub-surface parachute) surface float that is deployed in regions where sea ice forms that moves with either ice or water depending upon the time of year."@en ;
    rdfs:subClassOf <http://vocab.nerc.ac.uk/collection/L06/current/42/> .
<http://vocab.nerc.ac.uk/collection/L06/current/51/> a glbase:PlatformType,
        owl:Class,
        owl:NamedIndividual ;
    rdfs:label "free-rising balloon"@en ;
    dcterms:creator "SeaDataNet and MarineXML Vocabulary Content Governance Group" ;
    dcterms:date "2006-07-07 10:48:26.0" ;
    glbase:hasIdentifier [ glbase:hasIdentifierScheme idscheme:sdnl06 ;
            glbase:hasIdentifierValue "SDN:L06::51" ] ;
    rdfs:comment "A container filled with a gas that is lighter than air, which is constrained to rise vertically at a fixed location."@en ;
    rdfs:subClassOf <http://vocab.nerc.ac.uk/collection/L06/current/50/> .
<http://vocab.nerc.ac.uk/collection/L06/current/52/> a glbase:PlatformType,
        owl:Class,
        owl:NamedIndividual ;
    rdfs:label "free-floating balloon"@en ;
    dcterms:creator "SeaDataNet and MarineXML Vocabulary Content Governance Group" ;
    dcterms:date "2006-07-07 10:48:37.0" ;
    glbase:hasIdentifier [ glbase:hasIdentifierScheme idscheme:sdnl06 ;
            glbase:hasIdentifierValue "SDN:L06::52" ] ;
    rdfs:comment "A container filled with a gas that is lighter than air, which is free to drift in the atmosphere."@en ;
    rdfs:subClassOf <http://vocab.nerc.ac.uk/collection/L06/current/50/> .
<http://vocab.nerc.ac.uk/collection/L06/current/53/> a glbase:PlatformType,
        owl:Class,
        owl:NamedIndividual ;
    rdfs:label "tethered balloon"@en ;
    dcterms:creator "SeaDataNet and MarineXML Vocabulary Content Governance Group" ;
    dcterms:date "2006-07-07 10:49:03.0" ;
    glbase:hasIdentifier [ glbase:hasIdentifierScheme idscheme:sdnl06 ;
            glbase:hasIdentifierValue "SDN:L06::53" ] ;
    rdfs:comment "A container filled with a gas that is lighter than air, which is tethered at a fixed height and location."@en ;
    rdfs:subClassOf <http://vocab.nerc.ac.uk/collection/L06/current/50/> .
<http://vocab.nerc.ac.uk/collection/L06/current/54/> a glbase:PlatformType,
        owl:Class,
        owl:NamedIndividual ;
    rdfs:label "airship"@en ;
    dcterms:creator "SeaDataNet and MarineXML Vocabulary Content Governance Group" ;
    dcterms:date "2006-07-07 10:38:37.0" ;
    glbase:hasIdentifier [ glbase:hasIdentifierScheme idscheme:sdnl06 ;
            glbase:hasIdentifierValue "SDN:L06::54" ] ;
    rdfs:comment "A self-propelled container filled with a gas that is lighter than air."@en ;
    rdfs:subClassOf <http://vocab.nerc.ac.uk/collection/L06/current/50/> .
<http://vocab.nerc.ac.uk/collection/L06/current/61/> a glbase:PlatformType,
        owl:Class,
        owl:NamedIndividual ;
    rdfs:label "research aeroplane"@en ;
    dcterms:creator "SeaDataNet and MarineXML Vocabulary Content Governance Group" ;
    dcterms:date "2006-07-07 10:38:37.0" ;
    glbase:hasIdentifier [ glbase:hasIdentifierScheme idscheme:sdnl06 ;
            glbase:hasIdentifierValue "SDN:L06::61" ] ;
    rdfs:comment "A fixed-wing self-propelled aircraft that is equipped, manned and operated for atmospheric, meteorological or oceanographic research."@en ;
    rdfs:subClassOf <http://vocab.nerc.ac.uk/collection/L06/current/60/> .
<http://vocab.nerc.ac.uk/collection/L06/current/62/> a glbase:PlatformType,
        owl:Class,
        owl:NamedIndividual ;
    rdfs:label "aeroplane"@en ;
    dcterms:creator "SeaDataNet and MarineXML Vocabulary Content Governance Group" ;
    dcterms:date "2006-07-07 10:38:37.0" ;
    glbase:hasIdentifier [ glbase:hasIdentifierScheme idscheme:sdnl06 ;
            glbase:hasIdentifierValue "SDN:L06::62" ] ;
    rdfs:comment "A fixed-wing self-propelled aircraft."@en ;
    rdfs:subClassOf <http://vocab.nerc.ac.uk/collection/L06/current/60/> .
<http://vocab.nerc.ac.uk/collection/L06/current/63/> a glbase:PlatformType,
        owl:Class,
        owl:NamedIndividual ;
    rdfs:label "rocket"@en ;
    dcterms:creator "SeaDataNet and MarineXML Vocabulary Content Governance Group" ;
    dcterms:date "2006-07-07 10:38:37.0" ;
    glbase:hasIdentifier [ glbase:hasIdentifierScheme idscheme:sdnl06 ;
            glbase:hasIdentifierValue "SDN:L06::63" ] ;
    rdfs:comment "A rocket is a vehicle, missile or aircraft which obtains thrust by the reaction to the ejection of fast moving exhaust gas from within a rocket engine."@en ;
    rdfs:subClassOf <http://vocab.nerc.ac.uk/collection/L06/current/60/> .
<http://vocab.nerc.ac.uk/collection/L06/current/64/> a glbase:PlatformType,
        owl:Class,
        owl:NamedIndividual ;
    rdfs:label "geostationary orbiting satellite"@en ;
    dcterms:creator "SeaDataNet and MarineXML Vocabulary Content Governance Group" ;
    dcterms:date "2006-07-07 10:38:37.0" ;
    glbase:hasIdentifier [ glbase:hasIdentifierScheme idscheme:sdnl06 ;
            glbase:hasIdentifierValue "SDN:L06::64" ] ;
    rdfs:comment "A vehicle operating beyond the Earth's atmosphere without human occupants that orbits the Earth at the same rate as the Earth's rotation keeping it over a fixed location on the Earth's surface.."@en ;
    rdfs:subClassOf <http://vocab.nerc.ac.uk/collection/L06/current/6Z/> .
<http://vocab.nerc.ac.uk/collection/L06/current/65/> a glbase:PlatformType,
        owl:Class,
        owl:NamedIndividual ;
    rdfs:label "orbiting satellite"@en ;
    dcterms:creator "SeaDataNet and MarineXML Vocabulary Content Governance Group" ;
    dcterms:date "2006-07-07 10:38:37.0" ;
    glbase:hasIdentifier [ glbase:hasIdentifierScheme idscheme:sdnl06 ;
            glbase:hasIdentifierValue "SDN:L06::65" ] ;
    rdfs:comment "A vehicle operating beyond the Earth's atmosphere without human occupants that orbits the Earth at a different rate to the Earth's rotation so it moves over the Earth's surface.."@en ;
    rdfs:subClassOf <http://vocab.nerc.ac.uk/collection/L06/current/6Z/> .
<http://vocab.nerc.ac.uk/collection/L06/current/66/> a glbase:PlatformType,
        owl:Class,
        owl:NamedIndividual ;
    rdfs:label "manned spacecraft"@en ;
    dcterms:creator "SeaDataNet and MarineXML Vocabulary Content Governance Group" ;
    dcterms:date "2006-07-07 10:38:37.0" ;
    glbase:hasIdentifier [ glbase:hasIdentifierScheme idscheme:sdnl06 ;
            glbase:hasIdentifierValue "SDN:L06::66" ] ;
    rdfs:comment "A vehicle operating beyond the Earth's atmosphere with human occupants."@en ;
    rdfs:subClassOf <http://vocab.nerc.ac.uk/collection/L06/current/6Z/> .
<http://vocab.nerc.ac.uk/collection/L06/current/67/> a glbase:PlatformType,
        owl:Class,
        owl:NamedIndividual ;
    rdfs:label "helicopter"@en ;
    dcterms:creator "SeaDataNet and MarineXML Vocabulary Content Governance Group" ;
    dcterms:date "2006-07-07 10:38:37.0" ;
    glbase:hasIdentifier [ glbase:hasIdentifierScheme idscheme:sdnl06 ;
            glbase:hasIdentifierValue "SDN:L06::67" ] ;
    rdfs:comment "An aircraft without wings that obtains its lift from the rotation of overhead blades."@en ;
    rdfs:subClassOf <http://vocab.nerc.ac.uk/collection/L06/current/60/> .
<http://vocab.nerc.ac.uk/collection/L06/current/68/> a glbase:PlatformType,
        owl:Class,
        owl:NamedIndividual ;
    rdfs:label "satellite"@en ;
    dcterms:creator "SeaDataNet and MarineXML Vocabulary Content Governance Group" ;
    dcterms:date "2006-07-07 10:38:37.0" ;
    glbase:hasIdentifier [ glbase:hasIdentifierScheme idscheme:sdnl06 ;
            glbase:hasIdentifierValue "SDN:L06::68" ] ;
    rdfs:comment "A vehicle operating beyond the Earth's atmosphere without human occupants that orbits the Earth."@en ;
    rdfs:subClassOf <http://vocab.nerc.ac.uk/collection/L06/current/6Z/> .
<http://vocab.nerc.ac.uk/collection/L06/current/69/> a glbase:PlatformType,
        owl:Class,
        owl:NamedIndividual ;
    rdfs:label "autogyro"@en ;
    dcterms:creator "SeaDataNet and MarineXML Vocabulary Content Governance Group" ;
    dcterms:date "2006-07-07 10:38:37.0" ;
    glbase:hasIdentifier [ glbase:hasIdentifierScheme idscheme:sdnl06 ;
            glbase:hasIdentifierValue "SDN:L06::69" ] ;
    rdfs:comment "An aircraft without wings that obtains its lift from the rotation of overhead blades, but obtains forward populsion from a fixed propellor."@en ;
    rdfs:subClassOf <http://vocab.nerc.ac.uk/collection/L06/current/60/> .
<http://vocab.nerc.ac.uk/collection/L06/current/6A/> a glbase:PlatformType,
        owl:Class,
        owl:NamedIndividual ;
    rdfs:label "glider"@en ;
    dcterms:creator "SeaDataNet and MarineXML Vocabulary Content Governance Group" ;
    dcterms:date "2006-07-07 10:38:37.0" ;
    glbase:hasIdentifier [ glbase:hasIdentifierScheme idscheme:sdnl06 ;
            glbase:hasIdentifierValue "SDN:L06::6A" ] ;
    rdfs:comment "A fixed-wing aircraft with no propulsion."@en ;
    rdfs:subClassOf <http://vocab.nerc.ac.uk/collection/L06/current/60/> .
<http://vocab.nerc.ac.uk/collection/L06/current/6B/> a glbase:PlatformType,
        owl:Class,
        owl:NamedIndividual ;
    rdfs:label "kite"@en ;
    dcterms:creator "SeaDataNet and MarineXML Vocabulary Content Governance Group" ;
    dcterms:date "2006-07-07 10:38:37.0" ;
    glbase:hasIdentifier [ glbase:hasIdentifierScheme idscheme:sdnl06 ;
            glbase:hasIdentifierValue "SDN:L06::6B" ] ;
    rdfs:comment "An aerofoil tethered to the ground held aloft by the wind."@en ;
    rdfs:subClassOf <http://vocab.nerc.ac.uk/collection/L06/current/60/> .
<http://vocab.nerc.ac.uk/collection/L06/current/6C/> a glbase:PlatformType,
        owl:Class,
        owl:NamedIndividual ;
    rdfs:label "parachute"@en ;
    dcterms:creator "SeaDataNet and MarineXML Vocabulary Content Governance Group" ;
    dcterms:date "2006-07-07 10:38:37.0" ;
    glbase:hasIdentifier [ glbase:hasIdentifierScheme idscheme:sdnl06 ;
            glbase:hasIdentifierValue "SDN:L06::6C" ] ;
    rdfs:comment "A fabric sheet designed to slow the descent of an object through the atmosphere."@en ;
    rdfs:subClassOf <http://vocab.nerc.ac.uk/collection/L06/current/60/> .
<http://vocab.nerc.ac.uk/collection/L06/current/6D/> a glbase:PlatformType,
        owl:Class,
        owl:NamedIndividual ;
    rdfs:label "unmanned aerial vehicle"@en ;
    dcterms:creator "SeaDataNet and MarineXML Vocabulary Content Governance Group" ;
    dcterms:date "2015-03-26 11:19:23.0" ;
    glbase:hasIdentifier [ glbase:hasIdentifierScheme idscheme:sdnl06 ;
            glbase:hasIdentifierValue "SDN:L06::6D" ] ;
    rdfs:comment "Any untethered heavier-than-air aircraft that is not occupied by people: may be a remotely piloted aircraft or an autonomous aircraft. Also referred to as a drone."@en ;
    rdfs:subClassOf <http://vocab.nerc.ac.uk/collection/L06/current/60/> .
<http://vocab.nerc.ac.uk/collection/L06/current/71/> a glbase:PlatformType,
        owl:Class,
        owl:NamedIndividual ;
    rdfs:label "human"@en ;
    dcterms:creator "SeaDataNet and MarineXML Vocabulary Content Governance Group" ;
    dcterms:date "2006-07-07 10:38:37.0" ;
    glbase:hasIdentifier [ glbase:hasIdentifierScheme idscheme:sdnl06 ;
            glbase:hasIdentifierValue "SDN:L06::71" ] ;
    rdfs:comment "A human being without specialised equipment operating on land or the surface of the water column."@en ;
    rdfs:subClassOf <http://vocab.nerc.ac.uk/collection/L06/current/70/> .
<http://vocab.nerc.ac.uk/collection/L06/current/72/> a glbase:PlatformType,
        owl:Class,
        owl:NamedIndividual ;
    rdfs:label "diver"@en ;
    dcterms:creator "SeaDataNet and MarineXML Vocabulary Content Governance Group" ;
    dcterms:date "2006-07-07 10:38:37.0" ;
    glbase:hasIdentifier [ glbase:hasIdentifierScheme idscheme:sdnl06 ;
            glbase:hasIdentifierValue "SDN:L06::72" ] ;
    rdfs:comment "A human being with self-contained equipment or surface-connected suit enabling operation within the water column."@en ;
    rdfs:subClassOf <http://vocab.nerc.ac.uk/collection/L06/current/70/> .
<http://vocab.nerc.ac.uk/collection/L06/current/73/> a glbase:PlatformType,
        owl:Class,
        owl:NamedIndividual ;
    rdfs:label "flightless bird"@en ;
    dcterms:creator "SeaDataNet and MarineXML Vocabulary Content Governance Group" ;
    dcterms:date "2006-07-07 10:38:37.0" ;
    glbase:hasIdentifier [ glbase:hasIdentifierScheme idscheme:sdnl06 ;
            glbase:hasIdentifierValue "SDN:L06::73" ] ;
    rdfs:comment "A bird that is unable to fly with the ability to exist within the water column (e.g. penguin)."@en ;
    rdfs:subClassOf <http://vocab.nerc.ac.uk/collection/L06/current/70/> .
<http://vocab.nerc.ac.uk/collection/L06/current/74/> a glbase:PlatformType,
        owl:Class,
        owl:NamedIndividual ;
    rdfs:label "seabird and duck"@en ;
    dcterms:creator "SeaDataNet and MarineXML Vocabulary Content Governance Group" ;
    dcterms:date "2006-07-07 10:38:37.0" ;
    glbase:hasIdentifier [ glbase:hasIdentifierScheme idscheme:sdnl06 ;
            glbase:hasIdentifierValue "SDN:L06::74" ] ;
    rdfs:comment "A flighted bird that is able to exist on the water column surface and dive into the water column (e.g. cormorants, auks, ducks and gulls)."@en ;
    rdfs:subClassOf <http://vocab.nerc.ac.uk/collection/L06/current/70/> .
<http://vocab.nerc.ac.uk/collection/L06/current/75/> a glbase:PlatformType,
        owl:Class,
        owl:NamedIndividual ;
    rdfs:label "cetacean"@en ;
    dcterms:creator "SeaDataNet and MarineXML Vocabulary Content Governance Group" ;
    dcterms:date "2006-07-07 10:38:37.0" ;
    glbase:hasIdentifier [ glbase:hasIdentifierScheme idscheme:sdnl06 ;
            glbase:hasIdentifierValue "SDN:L06::75" ] ;
    rdfs:comment "A mammal that exists within the water column but needing to regularly surface to breathe (i.e. dolphins and whales)."@en ;
    rdfs:subClassOf <http://vocab.nerc.ac.uk/collection/L06/current/70/> .
<http://vocab.nerc.ac.uk/collection/L06/current/76/> a glbase:PlatformType,
        owl:Class,
        owl:NamedIndividual ;
    rdfs:label "fish"@en ;
    dcterms:creator "SeaDataNet and MarineXML Vocabulary Content Governance Group" ;
    dcterms:date "2006-07-07 10:38:37.0" ;
    glbase:hasIdentifier [ glbase:hasIdentifierScheme idscheme:sdnl06 ;
            glbase:hasIdentifierValue "SDN:L06::76" ] ;
    rdfs:comment "A free-swimming creature that exists totally within the water column."@en ;
    rdfs:subClassOf <http://vocab.nerc.ac.uk/collection/L06/current/70/> .
<http://vocab.nerc.ac.uk/collection/L06/current/77/> a glbase:PlatformType,
        owl:Class,
        owl:NamedIndividual ;
    rdfs:label "land-sea mammals"@en ;
    dcterms:creator "SeaDataNet and MarineXML Vocabulary Content Governance Group" ;
    dcterms:date "2006-07-07 10:38:37.0" ;
    glbase:hasIdentifier [ glbase:hasIdentifierScheme idscheme:sdnl06 ;
            glbase:hasIdentifierValue "SDN:L06::77" ] ;
    rdfs:comment "A mammal that exists both on land and within the water column. Includes seals, sealions, sea-otters and walruses."@en ;
    rdfs:subClassOf <http://vocab.nerc.ac.uk/collection/L06/current/70/> .
<http://vocab.nerc.ac.uk/collection/L06/current/91/> a glbase:PlatformType,
        owl:Class,
        owl:NamedIndividual ;
    rdfs:label "ice island"@en ;
    dcterms:creator "SeaDataNet and MarineXML Vocabulary Content Governance Group" ;
    dcterms:date "2006-07-07 10:38:37.0" ;
    glbase:hasIdentifier [ glbase:hasIdentifierScheme idscheme:sdnl06 ;
            glbase:hasIdentifierValue "SDN:L06::91" ] ;
    rdfs:comment "A floating ice sheet detached from the coast."@en ;
    rdfs:subClassOf <http://vocab.nerc.ac.uk/collection/L06/current/90/> .
<http://vocab.nerc.ac.uk/collection/L06/current/92/> a glbase:PlatformType,
        owl:Class,
        owl:NamedIndividual ;
    rdfs:label "ice shelf"@en ;
    dcterms:creator "SeaDataNet and MarineXML Vocabulary Content Governance Group" ;
    dcterms:date "2006-07-07 10:38:37.0" ;
    glbase:hasIdentifier [ glbase:hasIdentifierScheme idscheme:sdnl06 ;
            glbase:hasIdentifierValue "SDN:L06::92" ] ;
    rdfs:comment "A floating ice sheet attached to the coast."@en ;
    rdfs:subClassOf <http://vocab.nerc.ac.uk/collection/L06/current/90/> .
<http://vocab.nerc.ac.uk/collection/L06/current/93/> a glbase:PlatformType,
        owl:Class,
        owl:NamedIndividual ;
    rdfs:label "pack ice"@en ;
    dcterms:creator "SeaDataNet and MarineXML Vocabulary Content Governance Group" ;
    dcterms:date "2013-08-20 14:05:34.0" ;
    glbase:hasIdentifier [ glbase:hasIdentifierScheme idscheme:sdnl06 ;
            glbase:hasIdentifierValue "SDN:L06::93" ] ;
    rdfs:comment "Sea ice not connected to land with an ice concetration of over 70 per cent."@en ;
    rdfs:subClassOf <http://vocab.nerc.ac.uk/collection/L06/current/90/> .
<http://vocab.nerc.ac.uk/collection/L06/current/94/> a glbase:PlatformType,
        owl:Class,
        owl:NamedIndividual ;
    rdfs:label "drift ice"@en ;
    dcterms:creator "SeaDataNet and MarineXML Vocabulary Content Governance Group" ;
    dcterms:date "2013-08-20 14:05:55.0" ;
    glbase:hasIdentifier [ glbase:hasIdentifierScheme idscheme:sdnl06 ;
            glbase:hasIdentifierValue "SDN:L06::94" ] ;
    rdfs:comment "Sea ice not connected to land with an ice concetration of under 70 per cent."@en ;
    rdfs:subClassOf <http://vocab.nerc.ac.uk/collection/L06/current/90/> .
<http://vocab.nerc.ac.uk/collection/L06/current/96/> a glbase:PlatformType,
        owl:Class,
        owl:NamedIndividual ;
    rdfs:label "amphibious crawler"@en ;
    dcterms:creator "SeaDataNet and MarineXML Vocabulary Content Governance Group" ;
    dcterms:date "2013-08-20 13:53:41.0" ;
    glbase:hasIdentifier [ glbase:hasIdentifierScheme idscheme:sdnl06 ;
            glbase:hasIdentifierValue "SDN:L06::96" ] ;
    rdfs:comment "A self-propelled vehicle capable of operation on land or the seabed (e.g. beach crawler)."@en ;
    rdfs:subClassOf <http://vocab.nerc.ac.uk/collection/L06/current/10/> .
<http://vocab.nerc.ac.uk/collection/L06/current/9A/> a glbase:PlatformType,
        owl:Class,
        owl:NamedIndividual ;
    rdfs:label "DUKW"@en ;
    dcterms:creator "SeaDataNet and MarineXML Vocabulary Content Governance Group" ;
    dcterms:date "2008-02-21 10:51:53.0" ;
    glbase:hasIdentifier [ glbase:hasIdentifierScheme idscheme:sdnl06 ;
            glbase:hasIdentifierValue "SDN:L06::9A" ] ;
    rdfs:comment "A six-wheel drive amphibious truck developed during the second World War."@en ;
    rdfs:subClassOf <http://vocab.nerc.ac.uk/collection/L06/current/95/> .
<http://vocab.nerc.ac.uk/collection/L06/current/9B/> a glbase:PlatformType,
        owl:Class,
        owl:NamedIndividual ;
    rdfs:label "hovercraft"@en ;
    dcterms:creator "SeaDataNet and MarineXML Vocabulary Content Governance Group" ;
    dcterms:date "2008-02-21 10:51:53.0" ;
    glbase:hasIdentifier [ glbase:hasIdentifierScheme idscheme:sdnl06 ;
            glbase:hasIdentifierValue "SDN:L06::9B" ] ;
    rdfs:comment "A craft capable of moving over water or land on a downwardly-propelled cushion of air."@en ;
    rdfs:subClassOf <http://vocab.nerc.ac.uk/collection/L06/current/95/> .
<http://vocab.nerc.ac.uk/collection/L06/current/25/> a glbase:PlatformType,
        owl:Class,
        owl:NamedIndividual ;
    rdfs:label "autonomous underwater vehicle"@en ;
    dcterms:creator "SeaDataNet and MarineXML Vocabulary Content Governance Group" ;
    dcterms:date "2006-07-07 10:38:37.0" ;
    glbase:hasIdentifier [ glbase:hasIdentifierScheme idscheme:sdnl06 ;
            glbase:hasIdentifierValue "SDN:L06::25" ] ;
    rdfs:comment "A free-roving platform operating in the water column with propulsion but no human operator on board (e.g. Autosub, Glider)."@en ;
    rdfs:subClassOf <http://vocab.nerc.ac.uk/collection/L06/current/20/> .
<http://vocab.nerc.ac.uk/collection/L06/current/3B/> a glbase:PlatformType,
        owl:Class,
        owl:NamedIndividual ;
    rdfs:label "autonomous surface water vehicle"@en ;
    dcterms:creator "SeaDataNet and MarineXML Vocabulary Content Governance Group" ;
    dcterms:date "2006-11-15 16:22:32.0" ;
    glbase:hasIdentifier [ glbase:hasIdentifierScheme idscheme:sdnl06 ;
            glbase:hasIdentifierValue "SDN:L06::3B" ] ;
    rdfs:comment "A self-propelled vehicle operating on the sea surface with no human occupants."@en ;
    rdfs:subClassOf <http://vocab.nerc.ac.uk/collection/L06/current/3Z/> .
<http://vocab.nerc.ac.uk/collection/L06/current/42/> a glbase:PlatformType,
        owl:Class,
        owl:NamedIndividual ;
    rdfs:label "drifting surface float"@en ;
    dcterms:creator "SeaDataNet and MarineXML Vocabulary Content Governance Group" ;
    dcterms:date "2006-07-07 10:38:37.0" ;
    glbase:hasIdentifier [ glbase:hasIdentifierScheme idscheme:sdnl06 ;
            glbase:hasIdentifierValue "SDN:L06::42" ] ;
    rdfs:comment "An unmanned instrumented platform operating on the surface of the water column often attached to a drogue to track currents rather than winds (e.g. Argos buoy)."@en ;
    rdfs:subClassOf <http://vocab.nerc.ac.uk/collection/L06/current/47/> .
<http://vocab.nerc.ac.uk/collection/L06/current/95/> a glbase:PlatformType,
        owl:Class,
        owl:NamedIndividual ;
    rdfs:label "amphibious vehicle"@en ;
    dcterms:creator "SeaDataNet and MarineXML Vocabulary Content Governance Group" ;
    dcterms:date "2008-02-21 10:45:42.0" ;
    glbase:hasIdentifier [ glbase:hasIdentifierScheme idscheme:sdnl06 ;
            glbase:hasIdentifierValue "SDN:L06::95" ] ;
    rdfs:comment "A self-propelled platform capable of operating on land and within or on the surface of a water body."@en ;
    rdfs:subClassOf glbase:Platform .
<http://vocab.nerc.ac.uk/collection/L06/current/47/> a glbase:PlatformType,
        owl:Class,
        owl:NamedIndividual ;
    rdfs:label "float"@en ;
    dcterms:creator "SeaDataNet and MarineXML Vocabulary Content Governance Group" ;
    dcterms:date "2008-02-21 09:50:08.0" ;
    glbase:hasIdentifier [ glbase:hasIdentifierScheme idscheme:sdnl06 ;
            glbase:hasIdentifierValue "SDN:L06::47" ] ;
    rdfs:comment "A free-floating platform either on the surface of the water column or at a predetermined depth within the water column."@en ;
    rdfs:subClassOf glbase:Platform .
<http://vocab.nerc.ac.uk/collection/L06/current/48/> a glbase:PlatformType,
        owl:Class,
        owl:NamedIndividual ;
    rdfs:label "mooring"@en ;
    dcterms:creator "SeaDataNet and MarineXML Vocabulary Content Governance Group" ;
    dcterms:date "2008-02-21 09:55:15.0" ;
    glbase:hasIdentifier [ glbase:hasIdentifierScheme idscheme:sdnl06 ;
            glbase:hasIdentifierValue "SDN:L06::48" ] ;
    rdfs:comment "A tethered collection of oceanographic instruments at a fixed location that may include seafloor, mid-water and surface components."@en ;
    rdfs:subClassOf glbase:Platform .
<http://vocab.nerc.ac.uk/collection/L06/current/50/> a glbase:PlatformType,
        owl:Class,
        owl:NamedIndividual ;
    rdfs:label "buoyant aircraft"@en ;
    dcterms:creator "SeaDataNet and MarineXML Vocabulary Content Governance Group" ;
    dcterms:date "2008-02-21 10:13:31.0" ;
    glbase:hasIdentifier [ glbase:hasIdentifierScheme idscheme:sdnl06 ;
            glbase:hasIdentifierValue "SDN:L06::50" ] ;
    rdfs:comment "A platform capable of flight in the atmosphere because it is lighter than air."@en ;
    rdfs:subClassOf glbase:Platform .
<http://vocab.nerc.ac.uk/collection/L06/current/6Z/> a glbase:PlatformType,
        owl:Class,
        owl:NamedIndividual ;
    rdfs:label "spacecraft"@en ;
    dcterms:creator "SeaDataNet and MarineXML Vocabulary Content Governance Group" ;
    dcterms:date "2013-08-20 13:53:41.0" ;
    glbase:hasIdentifier [ glbase:hasIdentifierScheme idscheme:sdnl06 ;
            glbase:hasIdentifierValue "SDN:L06::6Z" ] ;
    rdfs:comment "A platform operating beyond the Earth's atmosphere."@en ;
    rdfs:subClassOf glbase:Platform .
<http://vocab.nerc.ac.uk/collection/L06/current/90/> a glbase:PlatformType,
        owl:Class,
        owl:NamedIndividual ;
    rdfs:label "cryosphere"@en ;
    dcterms:creator "SeaDataNet and MarineXML Vocabulary Content Governance Group" ;
    dcterms:date "2008-02-21 10:31:40.0" ;
    glbase:hasIdentifier [ glbase:hasIdentifierScheme idscheme:sdnl06 ;
            glbase:hasIdentifierValue "SDN:L06::90" ] ;
    rdfs:comment "A frozen body of water on land, freshwater or sea."@en ;
    rdfs:subClassOf glbase:Platform .
<http://vocab.nerc.ac.uk/collection/L06/current/20/> a glbase:PlatformType,
        owl:Class,
        owl:NamedIndividual ;
    rdfs:label "submersible"@en ;
    dcterms:creator "SeaDataNet and MarineXML Vocabulary Content Governance Group" ;
    dcterms:date "2008-02-21 09:29:03.0" ;
    glbase:hasIdentifier [ glbase:hasIdentifierScheme idscheme:sdnl06 ;
            glbase:hasIdentifierValue "SDN:L06::20" ] ;
    rdfs:comment "A platform operating within a water body."@en ;
    rdfs:subClassOf glbase:Platform .
<http://vocab.nerc.ac.uk/collection/L06/current/70/> a glbase:PlatformType,
        owl:Class,
        owl:NamedIndividual ;
    rdfs:label "organism"@en ;
    dcterms:creator "SeaDataNet and MarineXML Vocabulary Content Governance Group" ;
    dcterms:date "2013-08-20 13:53:41.0" ;
    glbase:hasIdentifier [ glbase:hasIdentifierScheme idscheme:sdnl06 ;
            glbase:hasIdentifierValue "SDN:L06::70" ] ;
    rdfs:comment "A living creature carrying instruments or collecting samples."@en ;
    rdfs:subClassOf glbase:Platform .
<http://vocab.nerc.ac.uk/collection/L06/current/60/> a glbase:PlatformType,
        owl:Class,
        owl:NamedIndividual ;
    rdfs:label "non-buoyant aircraft"@en ;
    dcterms:creator "SeaDataNet and MarineXML Vocabulary Content Governance Group" ;
    dcterms:date "2008-02-21 10:46:32.0" ;
    glbase:hasIdentifier [ glbase:hasIdentifierScheme idscheme:sdnl06 ;
            glbase:hasIdentifierValue "SDN:L06::60" ] ;
    rdfs:comment "A platform capable of flight in the atmosphere despite its being heavier than air."@en ;
    rdfs:subClassOf glbase:Platform .
glbase:Platform a owl:Class .
<http://vocab.nerc.ac.uk/collection/L06/current/10/> a glbase:PlatformType,
        owl:Class,
        owl:NamedIndividual ;
    rdfs:label "land or seafloor"@en ;
    dcterms:creator "SeaDataNet and MarineXML Vocabulary Content Governance Group" ;
    dcterms:date "2008-02-21 09:22:38.0" ;
    glbase:hasIdentifier [ glbase:hasIdentifierScheme idscheme:sdnl06 ;
            glbase:hasIdentifierValue "SDN:L06::10" ] ;
    rdfs:comment "A platform located on the solid surface of the Earth either above or below sea level."@en ;
    rdfs:subClassOf glbase:Platform .
<http://vocab.nerc.ac.uk/collection/L06/current/3Z/> a glbase:PlatformType,
        owl:Class,
        owl:NamedIndividual ;
    rdfs:label "surface vessel"@en ;
    dcterms:creator "SeaDataNet and MarineXML Vocabulary Content Governance Group" ;
    dcterms:date "2008-02-21 09:44:01.0" ;
    glbase:hasIdentifier [ glbase:hasIdentifierScheme idscheme:sdnl06 ;
            glbase:hasIdentifierValue "SDN:L06::3Z" ] ;
    rdfs:comment "A mobile platform with propulsion operating on and restricted to the surface of a water body."@en ;
    rdfs:subClassOf glbase:Platform .
glbase:PlatformType a owl:Class .
glbase:hasPlatformType a owl:ObjectProperty .
[] a owl:Restriction ;
    rdfs:subClassOf <http://vocab.nerc.ac.uk/collection/L06/current/63/> ;
    owl:onProperty glbase:hasPlatformType ;
    owl:someValuesFrom [ a owl:Class ;
            owl:oneOf ( <http://vocab.nerc.ac.uk/collection/L06/current/63/> ) ] .
[] a owl:Restriction ;
    rdfs:subClassOf <http://vocab.nerc.ac.uk/collection/L06/current/6A/> ;
    owl:onProperty glbase:hasPlatformType ;
    owl:someValuesFrom [ a owl:Class ;
            owl:oneOf ( <http://vocab.nerc.ac.uk/collection/L06/current/6A/> ) ] .
[] a owl:Restriction ;
    rdfs:subClassOf <http://vocab.nerc.ac.uk/collection/L06/current/3A/> ;
    owl:onProperty glbase:hasPlatformType ;
    owl:someValuesFrom [ a owl:Class ;
            owl:oneOf ( <http://vocab.nerc.ac.uk/collection/L06/current/3A/> ) ] .
[] a owl:Restriction ;
    rdfs:subClassOf <http://vocab.nerc.ac.uk/collection/L06/current/31/> ;
    owl:onProperty glbase:hasPlatformType ;
    owl:someValuesFrom [ a owl:Class ;
            owl:oneOf ( <http://vocab.nerc.ac.uk/collection/L06/current/31/> ) ] .
[] a owl:Restriction ;
    rdfs:subClassOf <http://vocab.nerc.ac.uk/collection/L06/current/13/> ;
    owl:onProperty glbase:hasPlatformType ;
    owl:someValuesFrom [ a owl:Class ;
            owl:oneOf ( <http://vocab.nerc.ac.uk/collection/L06/current/13/> ) ] .
[] a owl:Restriction ;
    rdfs:subClassOf <http://vocab.nerc.ac.uk/collection/L06/current/18/> ;
    owl:onProperty glbase:hasPlatformType ;
    owl:someValuesFrom [ a owl:Class ;
            owl:oneOf ( <http://vocab.nerc.ac.uk/collection/L06/current/18/> ) ] .
[] a owl:Restriction ;
    rdfs:subClassOf <http://vocab.nerc.ac.uk/collection/L06/current/62/> ;
    owl:onProperty glbase:hasPlatformType ;
    owl:someValuesFrom [ a owl:Class ;
            owl:oneOf ( <http://vocab.nerc.ac.uk/collection/L06/current/62/> ) ] .
[] a owl:Restriction ;
    rdfs:subClassOf <http://vocab.nerc.ac.uk/collection/L06/current/95/> ;
    owl:onProperty glbase:hasPlatformType ;
    owl:someValuesFrom [ a owl:Class ;
            owl:oneOf ( <http://vocab.nerc.ac.uk/collection/L06/current/95/> ) ] .
[] a owl:Restriction ;
    rdfs:subClassOf <http://vocab.nerc.ac.uk/collection/L06/current/37/> ;
    owl:onProperty glbase:hasPlatformType ;
    owl:someValuesFrom [ a owl:Class ;
            owl:oneOf ( <http://vocab.nerc.ac.uk/collection/L06/current/37/> ) ] .
[] a owl:Restriction ;
    rdfs:subClassOf <http://vocab.nerc.ac.uk/collection/L06/current/30/> ;
    owl:onProperty glbase:hasPlatformType ;
    owl:someValuesFrom [ a owl:Class ;
            owl:oneOf ( <http://vocab.nerc.ac.uk/collection/L06/current/30/> ) ] .
[] a owl:Restriction ;
    rdfs:subClassOf <http://vocab.nerc.ac.uk/collection/L06/current/91/> ;
    owl:onProperty glbase:hasPlatformType ;
    owl:someValuesFrom [ a owl:Class ;
            owl:oneOf ( <http://vocab.nerc.ac.uk/collection/L06/current/91/> ) ] .
[] a owl:Restriction ;
    rdfs:subClassOf <http://vocab.nerc.ac.uk/collection/L06/current/6C/> ;
    owl:onProperty glbase:hasPlatformType ;
    owl:someValuesFrom [ a owl:Class ;
            owl:oneOf ( <http://vocab.nerc.ac.uk/collection/L06/current/6C/> ) ] .
[] a owl:Restriction ;
    rdfs:subClassOf <http://vocab.nerc.ac.uk/collection/L06/current/3B/> ;
    owl:onProperty glbase:hasPlatformType ;
    owl:someValuesFrom [ a owl:Class ;
            owl:oneOf ( <http://vocab.nerc.ac.uk/collection/L06/current/3B/> ) ] .
[] a owl:Restriction ;
    rdfs:subClassOf <http://vocab.nerc.ac.uk/collection/L06/current/3D/> ;
    owl:onProperty glbase:hasPlatformType ;
    owl:someValuesFrom [ a owl:Class ;
            owl:oneOf ( <http://vocab.nerc.ac.uk/collection/L06/current/3D/> ) ] .
[] a owl:Restriction ;
    rdfs:subClassOf <http://vocab.nerc.ac.uk/collection/L06/current/68/> ;
    owl:onProperty glbase:hasPlatformType ;
    owl:someValuesFrom [ a owl:Class ;
            owl:oneOf ( <http://vocab.nerc.ac.uk/collection/L06/current/68/> ) ] .
[] a owl:Restriction ;
    rdfs:subClassOf <http://vocab.nerc.ac.uk/collection/L06/current/11/> ;
    owl:onProperty glbase:hasPlatformType ;
    owl:someValuesFrom [ a owl:Class ;
            owl:oneOf ( <http://vocab.nerc.ac.uk/collection/L06/current/11/> ) ] .
[] a owl:Restriction ;
    rdfs:subClassOf <http://vocab.nerc.ac.uk/collection/L06/current/21/> ;
    owl:onProperty glbase:hasPlatformType ;
    owl:someValuesFrom [ a owl:Class ;
            owl:oneOf ( <http://vocab.nerc.ac.uk/collection/L06/current/21/> ) ] .
[] a owl:Restriction ;
    rdfs:subClassOf <http://vocab.nerc.ac.uk/collection/L06/current/14/> ;
    owl:onProperty glbase:hasPlatformType ;
    owl:someValuesFrom [ a owl:Class ;
            owl:oneOf ( <http://vocab.nerc.ac.uk/collection/L06/current/14/> ) ] .
[] a owl:Restriction ;
    rdfs:subClassOf <http://vocab.nerc.ac.uk/collection/L06/current/3Z/> ;
    owl:onProperty glbase:hasPlatformType ;
    owl:someValuesFrom [ a owl:Class ;
            owl:oneOf ( <http://vocab.nerc.ac.uk/collection/L06/current/3Z/> ) ] .
[] a owl:Restriction ;
    rdfs:subClassOf <http://vocab.nerc.ac.uk/collection/L06/current/10/> ;
    owl:onProperty glbase:hasPlatformType ;
    owl:someValuesFrom [ a owl:Class ;
            owl:oneOf ( <http://vocab.nerc.ac.uk/collection/L06/current/10/> ) ] .
[] a owl:Restriction ;
    rdfs:subClassOf <http://vocab.nerc.ac.uk/collection/L06/current/23/> ;
    owl:onProperty glbase:hasPlatformType ;
    owl:someValuesFrom [ a owl:Class ;
            owl:oneOf ( <http://vocab.nerc.ac.uk/collection/L06/current/23/> ) ] .
[] a owl:Restriction ;
    rdfs:subClassOf <http://vocab.nerc.ac.uk/collection/L06/current/15/> ;
    owl:onProperty glbase:hasPlatformType ;
    owl:someValuesFrom [ a owl:Class ;
            owl:oneOf ( <http://vocab.nerc.ac.uk/collection/L06/current/15/> ) ] .
[] a owl:Restriction ;
    rdfs:subClassOf <http://vocab.nerc.ac.uk/collection/L06/current/76/> ;
    owl:onProperty glbase:hasPlatformType ;
    owl:someValuesFrom [ a owl:Class ;
            owl:oneOf ( <http://vocab.nerc.ac.uk/collection/L06/current/76/> ) ] .
[] a owl:Restriction ;
    rdfs:subClassOf <http://vocab.nerc.ac.uk/collection/L06/current/43/> ;
    owl:onProperty glbase:hasPlatformType ;
    owl:someValuesFrom [ a owl:Class ;
            owl:oneOf ( <http://vocab.nerc.ac.uk/collection/L06/current/43/> ) ] .
[] a owl:Restriction ;
    rdfs:subClassOf <http://vocab.nerc.ac.uk/collection/L06/current/34/> ;
    owl:onProperty glbase:hasPlatformType ;
    owl:someValuesFrom [ a owl:Class ;
            owl:oneOf ( <http://vocab.nerc.ac.uk/collection/L06/current/34/> ) ] .
[] a owl:Restriction ;
    rdfs:subClassOf <http://vocab.nerc.ac.uk/collection/L06/current/75/> ;
    owl:onProperty glbase:hasPlatformType ;
    owl:someValuesFrom [ a owl:Class ;
            owl:oneOf ( <http://vocab.nerc.ac.uk/collection/L06/current/75/> ) ] .
[] a owl:Restriction ;
    rdfs:subClassOf <http://vocab.nerc.ac.uk/collection/L06/current/93/> ;
    owl:onProperty glbase:hasPlatformType ;
    owl:someValuesFrom [ a owl:Class ;
            owl:oneOf ( <http://vocab.nerc.ac.uk/collection/L06/current/93/> ) ] .
[] a owl:Restriction ;
    rdfs:subClassOf <http://vocab.nerc.ac.uk/collection/L06/current/6D/> ;
    owl:onProperty glbase:hasPlatformType ;
    owl:someValuesFrom [ a owl:Class ;
            owl:oneOf ( <http://vocab.nerc.ac.uk/collection/L06/current/6D/> ) ] .
[] a owl:Restriction ;
    rdfs:subClassOf <http://vocab.nerc.ac.uk/collection/L06/current/64/> ;
    owl:onProperty glbase:hasPlatformType ;
    owl:someValuesFrom [ a owl:Class ;
            owl:oneOf ( <http://vocab.nerc.ac.uk/collection/L06/current/64/> ) ] .
[] a owl:Restriction ;
    rdfs:subClassOf <http://vocab.nerc.ac.uk/collection/L06/current/42/> ;
    owl:onProperty glbase:hasPlatformType ;
    owl:someValuesFrom [ a owl:Class ;
            owl:oneOf ( <http://vocab.nerc.ac.uk/collection/L06/current/42/> ) ] .
[] a owl:Restriction ;
    rdfs:subClassOf <http://vocab.nerc.ac.uk/collection/L06/current/32/> ;
    owl:onProperty glbase:hasPlatformType ;
    owl:someValuesFrom [ a owl:Class ;
            owl:oneOf ( <http://vocab.nerc.ac.uk/collection/L06/current/32/> ) ] .
[] a owl:Restriction ;
    rdfs:subClassOf <http://vocab.nerc.ac.uk/collection/L06/current/6Z/> ;
    owl:onProperty glbase:hasPlatformType ;
    owl:someValuesFrom [ a owl:Class ;
            owl:oneOf ( <http://vocab.nerc.ac.uk/collection/L06/current/6Z/> ) ] .
[] a owl:Restriction ;
    rdfs:subClassOf <http://vocab.nerc.ac.uk/collection/L06/current/74/> ;
    owl:onProperty glbase:hasPlatformType ;
    owl:someValuesFrom [ a owl:Class ;
            owl:oneOf ( <http://vocab.nerc.ac.uk/collection/L06/current/74/> ) ] .
[] a owl:Restriction ;
    rdfs:subClassOf <http://vocab.nerc.ac.uk/collection/L06/current/16/> ;
    owl:onProperty glbase:hasPlatformType ;
    owl:someValuesFrom [ a owl:Class ;
            owl:oneOf ( <http://vocab.nerc.ac.uk/collection/L06/current/16/> ) ] .
[] a owl:Restriction ;
    rdfs:subClassOf <http://vocab.nerc.ac.uk/collection/L06/current/70/> ;
    owl:onProperty glbase:hasPlatformType ;
    owl:someValuesFrom [ a owl:Class ;
            owl:oneOf ( <http://vocab.nerc.ac.uk/collection/L06/current/70/> ) ] .
[] a owl:Restriction ;
    rdfs:subClassOf <http://vocab.nerc.ac.uk/collection/L06/current/12/> ;
    owl:onProperty glbase:hasPlatformType ;
    owl:someValuesFrom [ a owl:Class ;
            owl:oneOf ( <http://vocab.nerc.ac.uk/collection/L06/current/12/> ) ] .
[] a owl:Restriction ;
    rdfs:subClassOf <http://vocab.nerc.ac.uk/collection/L06/current/22/> ;
    owl:onProperty glbase:hasPlatformType ;
    owl:someValuesFrom [ a owl:Class ;
            owl:oneOf ( <http://vocab.nerc.ac.uk/collection/L06/current/22/> ) ] .
[] a owl:Restriction ;
    rdfs:subClassOf <http://vocab.nerc.ac.uk/collection/L06/current/6B/> ;
    owl:onProperty glbase:hasPlatformType ;
    owl:someValuesFrom [ a owl:Class ;
            owl:oneOf ( <http://vocab.nerc.ac.uk/collection/L06/current/6B/> ) ] .
[] a owl:Restriction ;
    rdfs:subClassOf <http://vocab.nerc.ac.uk/collection/L06/current/94/> ;
    owl:onProperty glbase:hasPlatformType ;
    owl:someValuesFrom [ a owl:Class ;
            owl:oneOf ( <http://vocab.nerc.ac.uk/collection/L06/current/94/> ) ] .
[] a owl:Restriction ;
    rdfs:subClassOf <http://vocab.nerc.ac.uk/collection/L06/current/69/> ;
    owl:onProperty glbase:hasPlatformType ;
    owl:someValuesFrom [ a owl:Class ;
            owl:oneOf ( <http://vocab.nerc.ac.uk/collection/L06/current/69/> ) ] .
[] a owl:Restriction ;
    rdfs:subClassOf <http://vocab.nerc.ac.uk/collection/L06/current/38/> ;
    owl:onProperty glbase:hasPlatformType ;
    owl:someValuesFrom [ a owl:Class ;
            owl:oneOf ( <http://vocab.nerc.ac.uk/collection/L06/current/38/> ) ] .
[] a owl:Restriction ;
    rdfs:subClassOf <http://vocab.nerc.ac.uk/collection/L06/current/47/> ;
    owl:onProperty glbase:hasPlatformType ;
    owl:someValuesFrom [ a owl:Class ;
            owl:oneOf ( <http://vocab.nerc.ac.uk/collection/L06/current/47/> ) ] .
[] a owl:Restriction ;
    rdfs:subClassOf <http://vocab.nerc.ac.uk/collection/L06/current/44/> ;
    owl:onProperty glbase:hasPlatformType ;
    owl:someValuesFrom [ a owl:Class ;
            owl:oneOf ( <http://vocab.nerc.ac.uk/collection/L06/current/44/> ) ] .
[] a owl:Restriction ;
    rdfs:subClassOf <http://vocab.nerc.ac.uk/collection/L06/current/39/> ;
    owl:onProperty glbase:hasPlatformType ;
    owl:someValuesFrom [ a owl:Class ;
            owl:oneOf ( <http://vocab.nerc.ac.uk/collection/L06/current/39/> ) ] .
[] a owl:Restriction ;
    rdfs:subClassOf <http://vocab.nerc.ac.uk/collection/L06/current/90/> ;
    owl:onProperty glbase:hasPlatformType ;
    owl:someValuesFrom [ a owl:Class ;
            owl:oneOf ( <http://vocab.nerc.ac.uk/collection/L06/current/90/> ) ] .
[] a owl:Restriction ;
    rdfs:subClassOf <http://vocab.nerc.ac.uk/collection/L06/current/50/> ;
    owl:onProperty glbase:hasPlatformType ;
    owl:someValuesFrom [ a owl:Class ;
            owl:oneOf ( <http://vocab.nerc.ac.uk/collection/L06/current/50/> ) ] .
[] a owl:Restriction ;
    rdfs:subClassOf <http://vocab.nerc.ac.uk/collection/L06/current/45/> ;
    owl:onProperty glbase:hasPlatformType ;
    owl:someValuesFrom [ a owl:Class ;
            owl:oneOf ( <http://vocab.nerc.ac.uk/collection/L06/current/45/> ) ] .
[] a owl:Restriction ;
    rdfs:subClassOf <http://vocab.nerc.ac.uk/collection/L06/current/3C/> ;
    owl:onProperty glbase:hasPlatformType ;
    owl:someValuesFrom [ a owl:Class ;
            owl:oneOf ( <http://vocab.nerc.ac.uk/collection/L06/current/3C/> ) ] .
[] a owl:Restriction ;
    rdfs:subClassOf <http://vocab.nerc.ac.uk/collection/L06/current/54/> ;
    owl:onProperty glbase:hasPlatformType ;
    owl:someValuesFrom [ a owl:Class ;
            owl:oneOf ( <http://vocab.nerc.ac.uk/collection/L06/current/54/> ) ] .
[] a owl:Restriction ;
    rdfs:subClassOf <http://vocab.nerc.ac.uk/collection/L06/current/19/> ;
    owl:onProperty glbase:hasPlatformType ;
    owl:someValuesFrom [ a owl:Class ;
            owl:oneOf ( <http://vocab.nerc.ac.uk/collection/L06/current/19/> ) ] .
[] a owl:Restriction ;
    rdfs:subClassOf <http://vocab.nerc.ac.uk/collection/L06/current/73/> ;
    owl:onProperty glbase:hasPlatformType ;
    owl:someValuesFrom [ a owl:Class ;
            owl:oneOf ( <http://vocab.nerc.ac.uk/collection/L06/current/73/> ) ] .
[] a owl:Restriction ;
    rdfs:subClassOf <http://vocab.nerc.ac.uk/collection/L06/current/48/> ;
    owl:onProperty glbase:hasPlatformType ;
    owl:someValuesFrom [ a owl:Class ;
            owl:oneOf ( <http://vocab.nerc.ac.uk/collection/L06/current/48/> ) ] .
[] a owl:Restriction ;
    rdfs:subClassOf <http://vocab.nerc.ac.uk/collection/L06/current/20/> ;
    owl:onProperty glbase:hasPlatformType ;
    owl:someValuesFrom [ a owl:Class ;
            owl:oneOf ( <http://vocab.nerc.ac.uk/collection/L06/current/20/> ) ] .
[] a owl:Restriction ;
    rdfs:subClassOf <http://vocab.nerc.ac.uk/collection/L06/current/72/> ;
    owl:onProperty glbase:hasPlatformType ;
    owl:someValuesFrom [ a owl:Class ;
            owl:oneOf ( <http://vocab.nerc.ac.uk/collection/L06/current/72/> ) ] .
[] a owl:Restriction ;
    rdfs:subClassOf <http://vocab.nerc.ac.uk/collection/L06/current/0/> ;
    owl:onProperty glbase:hasPlatformType ;
    owl:someValuesFrom [ a owl:Class ;
            owl:oneOf ( <http://vocab.nerc.ac.uk/collection/L06/current/0/> ) ] .
[] a owl:Restriction ;
    rdfs:subClassOf <http://vocab.nerc.ac.uk/collection/L06/current/51/> ;
    owl:onProperty glbase:hasPlatformType ;
    owl:someValuesFrom [ a owl:Class ;
            owl:oneOf ( <http://vocab.nerc.ac.uk/collection/L06/current/51/> ) ] .
[] a owl:Restriction ;
    rdfs:subClassOf <http://vocab.nerc.ac.uk/collection/L06/current/49/> ;
    owl:onProperty glbase:hasPlatformType ;
    owl:someValuesFrom [ a owl:Class ;
            owl:oneOf ( <http://vocab.nerc.ac.uk/collection/L06/current/49/> ) ] .
[] a owl:Restriction ;
    rdfs:subClassOf <http://vocab.nerc.ac.uk/collection/L06/current/9B/> ;
    owl:onProperty glbase:hasPlatformType ;
    owl:someValuesFrom [ a owl:Class ;
            owl:oneOf ( <http://vocab.nerc.ac.uk/collection/L06/current/9B/> ) ] .
[] a owl:Restriction ;
    rdfs:subClassOf <http://vocab.nerc.ac.uk/collection/L06/current/46/> ;
    owl:onProperty glbase:hasPlatformType ;
    owl:someValuesFrom [ a owl:Class ;
            owl:oneOf ( <http://vocab.nerc.ac.uk/collection/L06/current/46/> ) ] .
[] a owl:Restriction ;
    rdfs:subClassOf <http://vocab.nerc.ac.uk/collection/L06/current/9A/> ;
    owl:onProperty glbase:hasPlatformType ;
    owl:someValuesFrom [ a owl:Class ;
            owl:oneOf ( <http://vocab.nerc.ac.uk/collection/L06/current/9A/> ) ] .
[] a owl:Restriction ;
    rdfs:subClassOf <http://vocab.nerc.ac.uk/collection/L06/current/67/> ;
    owl:onProperty glbase:hasPlatformType ;
    owl:someValuesFrom [ a owl:Class ;
            owl:oneOf ( <http://vocab.nerc.ac.uk/collection/L06/current/67/> ) ] .
[] a owl:Restriction ;
    rdfs:subClassOf <http://vocab.nerc.ac.uk/collection/L06/current/26/> ;
    owl:onProperty glbase:hasPlatformType ;
    owl:someValuesFrom [ a owl:Class ;
            owl:oneOf ( <http://vocab.nerc.ac.uk/collection/L06/current/26/> ) ] .
[] a owl:Restriction ;
    rdfs:subClassOf <http://vocab.nerc.ac.uk/collection/L06/current/60/> ;
    owl:onProperty glbase:hasPlatformType ;
    owl:someValuesFrom [ a owl:Class ;
            owl:oneOf ( <http://vocab.nerc.ac.uk/collection/L06/current/60/> ) ] .
[] a owl:Restriction ;
    rdfs:subClassOf <http://vocab.nerc.ac.uk/collection/L06/current/35/> ;
    owl:onProperty glbase:hasPlatformType ;
    owl:someValuesFrom [ a owl:Class ;
            owl:oneOf ( <http://vocab.nerc.ac.uk/collection/L06/current/35/> ) ] .
[] a owl:Restriction ;
    rdfs:subClassOf <http://vocab.nerc.ac.uk/collection/L06/current/36/> ;
    owl:onProperty glbase:hasPlatformType ;
    owl:someValuesFrom [ a owl:Class ;
            owl:oneOf ( <http://vocab.nerc.ac.uk/collection/L06/current/36/> ) ] .
[] a owl:Restriction ;
    rdfs:subClassOf <http://vocab.nerc.ac.uk/collection/L06/current/27/> ;
    owl:onProperty glbase:hasPlatformType ;
    owl:someValuesFrom [ a owl:Class ;
            owl:oneOf ( <http://vocab.nerc.ac.uk/collection/L06/current/27/> ) ] .
[] a owl:Restriction ;
    rdfs:subClassOf <http://vocab.nerc.ac.uk/collection/L06/current/25/> ;
    owl:onProperty glbase:hasPlatformType ;
    owl:someValuesFrom [ a owl:Class ;
            owl:oneOf ( <http://vocab.nerc.ac.uk/collection/L06/current/25/> ) ] .
[] a owl:Restriction ;
    rdfs:subClassOf <http://vocab.nerc.ac.uk/collection/L06/current/71/> ;
    owl:onProperty glbase:hasPlatformType ;
    owl:someValuesFrom [ a owl:Class ;
            owl:oneOf ( <http://vocab.nerc.ac.uk/collection/L06/current/71/> ) ] .
[] a owl:Restriction ;
    rdfs:subClassOf <http://vocab.nerc.ac.uk/collection/L06/current/33/> ;
    owl:onProperty glbase:hasPlatformType ;
    owl:someValuesFrom [ a owl:Class ;
            owl:oneOf ( <http://vocab.nerc.ac.uk/collection/L06/current/33/> ) ] .
[] a owl:Restriction ;
    rdfs:subClassOf <http://vocab.nerc.ac.uk/collection/L06/current/52/> ;
    owl:onProperty glbase:hasPlatformType ;
    owl:someValuesFrom [ a owl:Class ;
            owl:oneOf ( <http://vocab.nerc.ac.uk/collection/L06/current/52/> ) ] .
[] a owl:Restriction ;
    rdfs:subClassOf <http://vocab.nerc.ac.uk/collection/L06/current/96/> ;
    owl:onProperty glbase:hasPlatformType ;
    owl:someValuesFrom [ a owl:Class ;
            owl:oneOf ( <http://vocab.nerc.ac.uk/collection/L06/current/96/> ) ] .
[] a owl:Restriction ;
    rdfs:subClassOf <http://vocab.nerc.ac.uk/collection/L06/current/66/> ;
    owl:onProperty glbase:hasPlatformType ;
    owl:someValuesFrom [ a owl:Class ;
            owl:oneOf ( <http://vocab.nerc.ac.uk/collection/L06/current/66/> ) ] .
[] a owl:Restriction ;
    rdfs:subClassOf <http://vocab.nerc.ac.uk/collection/L06/current/92/> ;
    owl:onProperty glbase:hasPlatformType ;
    owl:someValuesFrom [ a owl:Class ;
            owl:oneOf ( <http://vocab.nerc.ac.uk/collection/L06/current/92/> ) ] .
[] a owl:Restriction ;
    rdfs:subClassOf <http://vocab.nerc.ac.uk/collection/L06/current/77/> ;
    owl:onProperty glbase:hasPlatformType ;
    owl:someValuesFrom [ a owl:Class ;
            owl:oneOf ( <http://vocab.nerc.ac.uk/collection/L06/current/77/> ) ] .
[] a owl:Restriction ;
    rdfs:subClassOf <http://vocab.nerc.ac.uk/collection/L06/current/24/> ;
    owl:onProperty glbase:hasPlatformType ;
    owl:someValuesFrom [ a owl:Class ;
            owl:oneOf ( <http://vocab.nerc.ac.uk/collection/L06/current/24/> ) ] .
[] a owl:Restriction ;
    rdfs:subClassOf <http://vocab.nerc.ac.uk/collection/L06/current/61/> ;
    owl:onProperty glbase:hasPlatformType ;
    owl:someValuesFrom [ a owl:Class ;
            owl:oneOf ( <http://vocab.nerc.ac.uk/collection/L06/current/61/> ) ] .
[] a owl:Restriction ;
    rdfs:subClassOf <http://vocab.nerc.ac.uk/collection/L06/current/53/> ;
    owl:onProperty glbase:hasPlatformType ;
    owl:someValuesFrom [ a owl:Class ;
            owl:oneOf ( <http://vocab.nerc.ac.uk/collection/L06/current/53/> ) ] .
[] a owl:Restriction ;
    rdfs:subClassOf <http://vocab.nerc.ac.uk/collection/L06/current/41/> ;
    owl:onProperty glbase:hasPlatformType ;
    owl:someValuesFrom [ a owl:Class ;
            owl:oneOf ( <http://vocab.nerc.ac.uk/collection/L06/current/41/> ) ] .
[] a owl:Restriction ;
    rdfs:subClassOf <http://vocab.nerc.ac.uk/collection/L06/current/17/> ;
    owl:onProperty glbase:hasPlatformType ;
    owl:someValuesFrom [ a owl:Class ;
            owl:oneOf ( <http://vocab.nerc.ac.uk/collection/L06/current/17/> ) ] .
[] a owl:Restriction ;
    rdfs:subClassOf <http://vocab.nerc.ac.uk/collection/L06/current/65/> ;
    owl:onProperty glbase:hasPlatformType ;
    owl:someValuesFrom [ a owl:Class ;
            owl:oneOf ( <http://vocab.nerc.ac.uk/collection/L06/current/65/> ) ] .
