<rdf:RDF
    xmlns:rdf="http://www.w3.org/1999/02/22-rdf-syntax-ns#"
    xmlns:skos="http://www.w3.org/2004/02/skos/core#"
    xmlns:glview="http://schema.geolink.org/dev/view#"
    xmlns:owl="http://www.w3.org/2002/07/owl#"
    xmlns:dcterms="http://purl.org/dc/terms/"
    xmlns:xsd="http://www.w3.org/2001/XMLSchema#"
    xmlns:glvoc_P02="http://schema.geolink.org/dev/voc/nvs/P02#"
    xmlns:glvoc_P03="http://schema.geolink.org/dev/voc/nvs/P03#"
    xmlns:rdfs="http://www.w3.org/2000/01/rdf-schema#">
  <owl:Ontology rdf:about="http://schema.geolink.org/dev/voc/nvs/P02">
    <owl:imports rdf:resource="http://schema.geolink.org/dev/voc/nvs/P03"/>
    <rdfs:seeAlso rdf:resource="http://vocab.nerc.ac.uk/collection/P03/current/"/>
    <rdfs:seeAlso rdf:resource="http://vocab.nerc.ac.uk/collection/P02/current/"/>
    <rdfs:comment xml:lang="en">This ontology captures SeaDataNet Parameter Discovery Vocabulary from NERC vocabulary server with mapping to SeaDataNet Agreed Parameter Groups</rdfs:comment>
    <owl:versionInfo>87</owl:versionInfo>
    <dcterms:date>2015-02-04 02:00:02.0</dcterms:date>
    <rdfs:label>SeaDataNet Parameter Discovery Vocabulary</rdfs:label>
  </owl:Ontology>
  <owl:Class rdf:about="http://schema.geolink.org/dev/view#MeasurementType"/>
  <owl:Class rdf:about="http://schema.geolink.org/dev/view#Measurement"/>
  <owl:Class rdf:about="http://schema.geolink.org/dev/voc/nvs/P02#PCAH">
    <rdfs:subClassOf rdf:resource="http://schema.geolink.org/dev/voc/nvs/P03#C025"/>
    <rdfs:seeAlso rdf:resource="http://vocab.nerc.ac.uk/collection/P02/current/PCAH/"/>
    <rdfs:subClassOf rdf:resource="http://schema.geolink.org/dev/voc/nvs/P03#H001"/>
    <rdfs:label xml:lang="en">Concentration of polycyclic aromatic hydrocarbons (PAHs) in suspended particulate material</rdfs:label>
    <rdfs:subClassOf rdf:resource="http://schema.geolink.org/dev/voc/nvs/P03#G015"/>
    <rdfs:comment xml:lang="en">PAH concentrations in suspended particulate material, regarded as anything sampled by a water bottle, SAP, sediment trap etc.  This group is for SPM composition measurements (concentration per unit weight) and NOT concentrations per unit volume of the water column in the particulate phase.</rdfs:comment>
    <rdfs:subClassOf rdf:resource="http://schema.geolink.org/dev/voc/nvs/P03#C055"/>
    <rdf:type rdf:resource="http://schema.geolink.org/dev/view#MeasurementType"/>
    <rdf:type rdf:resource="http://www.w3.org/2002/07/owl#NamedIndividual"/>
  </owl:Class>
  <owl:ObjectProperty rdf:about="http://schema.geolink.org/dev/view#hasMeasurementType"/>
  <owl:Restriction>
    <rdfs:subClassOf>
      <glview:MeasurementType rdf:about="http://schema.geolink.org/dev/voc/nvs/P02#MFWW">
        <rdfs:subClassOf rdf:resource="http://schema.geolink.org/dev/voc/nvs/P03#B070"/>
        <rdfs:subClassOf rdf:resource="http://schema.geolink.org/dev/voc/nvs/P03#G055"/>
        <rdfs:seeAlso rdf:resource="http://vocab.nerc.ac.uk/collection/P02/current/MFWW/"/>
        <rdfs:comment xml:lang="en">Any zoobenthos wet weight biomass per unit area of the seabed parameters that are not included in parameter group ZWTX.</rdfs:comment>
        <rdfs:label xml:lang="en">Zoobenthos non taxonomy-related wet weight biomass per unit area of the bed</rdfs:label>
        <rdf:type rdf:resource="http://www.w3.org/2002/07/owl#NamedIndividual"/>
        <rdf:type rdf:resource="http://www.w3.org/2002/07/owl#Class"/>
      </glview:MeasurementType>
    </rdfs:subClassOf>
    <owl:someValuesFrom>
      <owl:Class>
        <owl:oneOf rdf:parseType="Collection">
          <glview:MeasurementType rdf:about="http://schema.geolink.org/dev/voc/nvs/P02#MFWW"/>
        </owl:oneOf>
      </owl:Class>
    </owl:someValuesFrom>
    <owl:onProperty rdf:resource="http://schema.geolink.org/dev/view#hasMeasurementType"/>
  </owl:Restriction>
  <owl:Restriction>
    <rdfs:subClassOf>
      <glview:MeasurementType rdf:about="http://schema.geolink.org/dev/voc/nvs/P02#MMAN">
        <rdfs:subClassOf rdf:resource="http://schema.geolink.org/dev/voc/nvs/P03#G005"/>
        <rdfs:subClassOf rdf:resource="http://schema.geolink.org/dev/voc/nvs/P03#GPYS"/>
        <rdfs:seeAlso rdf:resource="http://vocab.nerc.ac.uk/collection/P02/current/MMAN/"/>
        <rdfs:comment xml:lang="en">Parameterisations of the intensity and inclination of Earth's magnetic field</rdfs:comment>
        <rdfs:label xml:lang="en">Magnetics</rdfs:label>
        <rdf:type rdf:resource="http://www.w3.org/2002/07/owl#NamedIndividual"/>
        <rdf:type rdf:resource="http://www.w3.org/2002/07/owl#Class"/>
      </glview:MeasurementType>
    </rdfs:subClassOf>
    <owl:someValuesFrom>
      <owl:Class>
        <owl:oneOf rdf:parseType="Collection">
          <glview:MeasurementType rdf:about="http://schema.geolink.org/dev/voc/nvs/P02#MMAN"/>
        </owl:oneOf>
      </owl:Class>
    </owl:someValuesFrom>
    <owl:onProperty rdf:resource="http://schema.geolink.org/dev/view#hasMeasurementType"/>
  </owl:Restriction>
  <owl:Restriction>
    <rdfs:subClassOf>
      <glview:MeasurementType rdf:about="http://schema.geolink.org/dev/voc/nvs/P02#GP018">
        <rdfs:subClassOf rdf:resource="http://schema.geolink.org/dev/voc/nvs/P03#B015"/>
        <rdfs:seeAlso rdf:resource="http://vocab.nerc.ac.uk/collection/P02/current/GP018/"/>
        <rdfs:comment xml:lang="en">Parameters related to the reproduction of cetaceans (Order Cetacea)</rdfs:comment>
        <rdfs:label xml:lang="en">Cetacean reproduction</rdfs:label>
        <rdf:type rdf:resource="http://www.w3.org/2002/07/owl#NamedIndividual"/>
        <rdf:type rdf:resource="http://www.w3.org/2002/07/owl#Class"/>
      </glview:MeasurementType>
    </rdfs:subClassOf>
    <owl:someValuesFrom>
      <owl:Class>
        <owl:oneOf rdf:parseType="Collection">
          <glview:MeasurementType rdf:about="http://schema.geolink.org/dev/voc/nvs/P02#GP018"/>
        </owl:oneOf>
      </owl:Class>
    </owl:someValuesFrom>
    <owl:onProperty rdf:resource="http://schema.geolink.org/dev/view#hasMeasurementType"/>
  </owl:Restriction>
  <owl:Restriction>
    <rdfs:subClassOf>
      <glview:MeasurementType rdf:about="http://schema.geolink.org/dev/voc/nvs/P02#PCOC">
        <rdfs:subClassOf rdf:resource="http://schema.geolink.org/dev/voc/nvs/P03#C055"/>
        <rdfs:subClassOf rdf:resource="http://schema.geolink.org/dev/voc/nvs/P03#G015"/>
        <rdfs:subClassOf rdf:resource="http://schema.geolink.org/dev/voc/nvs/P03#H001"/>
        <rdfs:seeAlso rdf:resource="http://vocab.nerc.ac.uk/collection/P02/current/PCOC/"/>
        <rdfs:comment xml:lang="en">'Other' organic contaminant (substances regarded as harmful other than PCBs and PAHs) concentrations in suspended particulate material, regarded as anything sampled by a water bottle, SAP, sediment trap etc.  This group is for SPM composition measurements (concentration per unit weight) and NOT concentrations per unit volume of the water column in the particulate phase.</rdfs:comment>
        <rdfs:label xml:lang="en">Concentration of other organic contaminants in suspended particulate material</rdfs:label>
        <rdf:type rdf:resource="http://www.w3.org/2002/07/owl#NamedIndividual"/>
        <rdf:type rdf:resource="http://www.w3.org/2002/07/owl#Class"/>
      </glview:MeasurementType>
    </rdfs:subClassOf>
    <owl:someValuesFrom>
      <owl:Class>
        <owl:oneOf rdf:parseType="Collection">
          <glview:MeasurementType rdf:about="http://schema.geolink.org/dev/voc/nvs/P02#PCOC"/>
        </owl:oneOf>
      </owl:Class>
    </owl:someValuesFrom>
    <owl:onProperty rdf:resource="http://schema.geolink.org/dev/view#hasMeasurementType"/>
  </owl:Restriction>
  <owl:Restriction>
    <rdfs:subClassOf>
      <glview:MeasurementType rdf:about="http://schema.geolink.org/dev/voc/nvs/P02#PEWB">
        <rdfs:subClassOf rdf:resource="http://schema.geolink.org/dev/voc/nvs/P03#C055"/>
        <rdfs:subClassOf rdf:resource="http://schema.geolink.org/dev/voc/nvs/P03#H001"/>
        <rdfs:seeAlso rdf:resource="http://vocab.nerc.ac.uk/collection/P02/current/PEWB/"/>
        <rdfs:comment xml:lang="en">Concentration parameters for substances synthesised by man to kill other life forms in either solution or suspension (i.e.includes measurements in both the dissolved and particulate phases) in any body of salt or fresh water.</rdfs:comment>
        <rdfs:label xml:lang="en">Pesticide concentrations in water bodies</rdfs:label>
        <rdf:type rdf:resource="http://www.w3.org/2002/07/owl#NamedIndividual"/>
        <rdf:type rdf:resource="http://www.w3.org/2002/07/owl#Class"/>
      </glview:MeasurementType>
    </rdfs:subClassOf>
    <owl:someValuesFrom>
      <owl:Class>
        <owl:oneOf rdf:parseType="Collection">
          <glview:MeasurementType rdf:about="http://schema.geolink.org/dev/voc/nvs/P02#PEWB"/>
        </owl:oneOf>
      </owl:Class>
    </owl:someValuesFrom>
    <owl:onProperty rdf:resource="http://schema.geolink.org/dev/view#hasMeasurementType"/>
  </owl:Restriction>
  <owl:Restriction>
    <rdfs:subClassOf>
      <glview:MeasurementType rdf:about="http://schema.geolink.org/dev/voc/nvs/P02#BCOC">
        <rdfs:subClassOf rdf:resource="http://schema.geolink.org/dev/voc/nvs/P03#C055"/>
        <rdfs:subClassOf rdf:resource="http://schema.geolink.org/dev/voc/nvs/P03#B007"/>
        <rdfs:subClassOf rdf:resource="http://schema.geolink.org/dev/voc/nvs/P03#H001"/>
        <rdfs:seeAlso rdf:resource="http://vocab.nerc.ac.uk/collection/P02/current/BCOC/"/>
        <rdfs:comment xml:lang="en">Concentration parameters for carbon compounds regarded as environmentally harmful in either whole organisms or their constituent parts that are not included in other categories</rdfs:comment>
        <rdfs:label xml:lang="en">Concentration of other organic contaminants in biota</rdfs:label>
        <rdf:type rdf:resource="http://www.w3.org/2002/07/owl#NamedIndividual"/>
        <rdf:type rdf:resource="http://www.w3.org/2002/07/owl#Class"/>
      </glview:MeasurementType>
    </rdfs:subClassOf>
    <owl:someValuesFrom>
      <owl:Class>
        <owl:oneOf rdf:parseType="Collection">
          <glview:MeasurementType rdf:about="http://schema.geolink.org/dev/voc/nvs/P02#BCOC"/>
        </owl:oneOf>
      </owl:Class>
    </owl:someValuesFrom>
    <owl:onProperty rdf:resource="http://schema.geolink.org/dev/view#hasMeasurementType"/>
  </owl:Restriction>
  <owl:Restriction>
    <rdfs:subClassOf>
      <glview:MeasurementType rdf:about="http://schema.geolink.org/dev/voc/nvs/P02#AORG">
        <rdfs:subClassOf rdf:resource="http://schema.geolink.org/dev/voc/nvs/P03#M005"/>
        <rdfs:seeAlso rdf:resource="http://vocab.nerc.ac.uk/collection/P02/current/AORG/"/>
        <rdfs:comment xml:lang="en">Parameters quantifying uncategorised organic substance concentrations in atmospheric, generally aerosol, samples such as organic matter and DOC.</rdfs:comment>
        <rdfs:label xml:lang="en">Concentration of organic matter in the atmosphere</rdfs:label>
        <rdf:type rdf:resource="http://www.w3.org/2002/07/owl#NamedIndividual"/>
        <rdf:type rdf:resource="http://www.w3.org/2002/07/owl#Class"/>
      </glview:MeasurementType>
    </rdfs:subClassOf>
    <owl:someValuesFrom>
      <owl:Class>
        <owl:oneOf rdf:parseType="Collection">
          <glview:MeasurementType rdf:about="http://schema.geolink.org/dev/voc/nvs/P02#AORG"/>
        </owl:oneOf>
      </owl:Class>
    </owl:someValuesFrom>
    <owl:onProperty rdf:resource="http://schema.geolink.org/dev/view#hasMeasurementType"/>
  </owl:Restriction>
  <owl:Restriction>
    <rdfs:subClassOf>
      <glview:MeasurementType rdf:about="http://schema.geolink.org/dev/voc/nvs/P02#SHTA">
        <rdfs:subClassOf rdf:resource="http://schema.geolink.org/dev/voc/nvs/P03#O010"/>
        <rdfs:subClassOf rdf:resource="http://schema.geolink.org/dev/voc/nvs/P03#G035"/>
        <rdfs:subClassOf rdf:resource="http://schema.geolink.org/dev/voc/nvs/P03#G055"/>
        <rdfs:seeAlso rdf:resource="http://vocab.nerc.ac.uk/collection/P02/current/SHTA/"/>
        <rdfs:comment></rdfs:comment>
        <rdfs:label xml:lang="en">Hydrolytic activity in sediment</rdfs:label>
        <rdf:type rdf:resource="http://www.w3.org/2002/07/owl#NamedIndividual"/>
        <rdf:type rdf:resource="http://www.w3.org/2002/07/owl#Class"/>
      </glview:MeasurementType>
    </rdfs:subClassOf>
    <owl:someValuesFrom>
      <owl:Class>
        <owl:oneOf rdf:parseType="Collection">
          <glview:MeasurementType rdf:about="http://schema.geolink.org/dev/voc/nvs/P02#SHTA"/>
        </owl:oneOf>
      </owl:Class>
    </owl:someValuesFrom>
    <owl:onProperty rdf:resource="http://schema.geolink.org/dev/view#hasMeasurementType"/>
  </owl:Restriction>
  <owl:Restriction>
    <rdfs:subClassOf>
      <glview:MeasurementType rdf:about="http://schema.geolink.org/dev/voc/nvs/P02#HEAD">
        <rdfs:subClassOf rdf:resource="http://schema.geolink.org/dev/voc/nvs/P03#Z005"/>
        <rdfs:seeAlso rdf:resource="http://vocab.nerc.ac.uk/collection/P02/current/HEAD/"/>
        <rdfs:comment xml:lang="en">Parameters that describe the displacement of platforms or instruments in space relative to various origins</rdfs:comment>
        <rdfs:label xml:lang="en">Platform or instrument orientation</rdfs:label>
        <rdf:type rdf:resource="http://www.w3.org/2002/07/owl#NamedIndividual"/>
        <rdf:type rdf:resource="http://www.w3.org/2002/07/owl#Class"/>
      </glview:MeasurementType>
    </rdfs:subClassOf>
    <owl:someValuesFrom>
      <owl:Class>
        <owl:oneOf rdf:parseType="Collection">
          <glview:MeasurementType rdf:about="http://schema.geolink.org/dev/voc/nvs/P02#HEAD"/>
        </owl:oneOf>
      </owl:Class>
    </owl:someValuesFrom>
    <owl:onProperty rdf:resource="http://schema.geolink.org/dev/view#hasMeasurementType"/>
  </owl:Restriction>
  <owl:Restriction>
    <rdfs:subClassOf>
      <glview:MeasurementType rdf:about="http://schema.geolink.org/dev/voc/nvs/P02#BEPP">
        <rdfs:subClassOf rdf:resource="http://schema.geolink.org/dev/voc/nvs/P03#B030"/>
        <rdfs:subClassOf rdf:resource="http://schema.geolink.org/dev/voc/nvs/P03#O010"/>
        <rdfs:subClassOf rdf:resource="http://schema.geolink.org/dev/voc/nvs/P03#B055"/>
        <rdfs:seeAlso rdf:resource="http://vocab.nerc.ac.uk/collection/P02/current/BEPP/"/>
        <rdfs:comment xml:lang="en">Parameters associated with the quantification of primary production by plants living on (e.g. corals, seaweed and seagrass) or in (e.g. benthic diatoms) the seabed.  Primary production is defined as the fixation of carbon dioxide into either organic or inorganic carbon by living entities and so includes photosynthesis and calcification.</rdfs:comment>
        <rdfs:label xml:lang="en">Benthic primary production</rdfs:label>
        <rdf:type rdf:resource="http://www.w3.org/2002/07/owl#NamedIndividual"/>
        <rdf:type rdf:resource="http://www.w3.org/2002/07/owl#Class"/>
      </glview:MeasurementType>
    </rdfs:subClassOf>
    <owl:someValuesFrom>
      <owl:Class>
        <owl:oneOf rdf:parseType="Collection">
          <glview:MeasurementType rdf:about="http://schema.geolink.org/dev/voc/nvs/P02#BEPP"/>
        </owl:oneOf>
      </owl:Class>
    </owl:someValuesFrom>
    <owl:onProperty rdf:resource="http://schema.geolink.org/dev/view#hasMeasurementType"/>
  </owl:Restriction>
  <owl:Restriction>
    <rdfs:subClassOf>
      <glview:MeasurementType rdf:about="http://schema.geolink.org/dev/voc/nvs/P02#OPCN">
        <rdfs:subClassOf rdf:resource="http://schema.geolink.org/dev/voc/nvs/P03#C045"/>
        <rdfs:subClassOf rdf:resource="http://schema.geolink.org/dev/voc/nvs/P03#G015"/>
        <rdfs:seeAlso rdf:resource="http://vocab.nerc.ac.uk/collection/P02/current/OPCN/"/>
        <rdfs:comment xml:lang="en">Concentration parameters for silicon species (including opal) in SPM (material gathered by filtration or sediment trapping). Only includes parameters expressed per unit mass of SPM and not per unit volume of the water column</rdfs:comment>
        <rdfs:label xml:lang="en">Concentration of silicon species in suspended particulate material</rdfs:label>
        <rdf:type rdf:resource="http://www.w3.org/2002/07/owl#NamedIndividual"/>
        <rdf:type rdf:resource="http://www.w3.org/2002/07/owl#Class"/>
      </glview:MeasurementType>
    </rdfs:subClassOf>
    <owl:someValuesFrom>
      <owl:Class>
        <owl:oneOf rdf:parseType="Collection">
          <glview:MeasurementType rdf:about="http://schema.geolink.org/dev/voc/nvs/P02#OPCN"/>
        </owl:oneOf>
      </owl:Class>
    </owl:someValuesFrom>
    <owl:onProperty rdf:resource="http://schema.geolink.org/dev/view#hasMeasurementType"/>
  </owl:Restriction>
  <owl:Restriction>
    <rdfs:subClassOf>
      <glview:MeasurementType rdf:about="http://schema.geolink.org/dev/voc/nvs/P02#SALK">
        <rdfs:subClassOf rdf:resource="http://schema.geolink.org/dev/voc/nvs/P03#C025"/>
        <rdfs:subClassOf rdf:resource="http://schema.geolink.org/dev/voc/nvs/P03#G035"/>
        <rdfs:seeAlso rdf:resource="http://vocab.nerc.ac.uk/collection/P02/current/SALK/"/>
        <rdfs:comment xml:lang="en">Aliphatic hydrocarbon (alkane, alkene, alkyne, polycyclic aliphatics like hopane, terpenes etc.)  concentrations in sediment, which is considered to be anything from the bed sampled by a grab or corer, including 'fluff'</rdfs:comment>
        <rdfs:label xml:lang="en">Concentration of aliphatic hydrocarbons in sediment samples</rdfs:label>
        <rdf:type rdf:resource="http://www.w3.org/2002/07/owl#NamedIndividual"/>
        <rdf:type rdf:resource="http://www.w3.org/2002/07/owl#Class"/>
      </glview:MeasurementType>
    </rdfs:subClassOf>
    <owl:someValuesFrom>
      <owl:Class>
        <owl:oneOf rdf:parseType="Collection">
          <glview:MeasurementType rdf:about="http://schema.geolink.org/dev/voc/nvs/P02#SALK"/>
        </owl:oneOf>
      </owl:Class>
    </owl:someValuesFrom>
    <owl:onProperty rdf:resource="http://schema.geolink.org/dev/view#hasMeasurementType"/>
  </owl:Restriction>
  <owl:Restriction>
    <rdfs:subClassOf>
      <glview:MeasurementType rdf:about="http://schema.geolink.org/dev/voc/nvs/P02#WVSP">
        <rdfs:subClassOf rdf:resource="http://schema.geolink.org/dev/voc/nvs/P03#D034"/>
        <rdfs:seeAlso rdf:resource="http://vocab.nerc.ac.uk/collection/P02/current/WVSP/"/>
        <rdfs:comment xml:lang="en">Parameters for directional and non-directional spectral wave data, excluding wave directions derived from spectral data.</rdfs:comment>
        <rdfs:label xml:lang="en">Spectral wave data parameters</rdfs:label>
        <rdf:type rdf:resource="http://www.w3.org/2002/07/owl#NamedIndividual"/>
        <rdf:type rdf:resource="http://www.w3.org/2002/07/owl#Class"/>
      </glview:MeasurementType>
    </rdfs:subClassOf>
    <owl:someValuesFrom>
      <owl:Class>
        <owl:oneOf rdf:parseType="Collection">
          <glview:MeasurementType rdf:about="http://schema.geolink.org/dev/voc/nvs/P02#WVSP"/>
        </owl:oneOf>
      </owl:Class>
    </owl:someValuesFrom>
    <owl:onProperty rdf:resource="http://schema.geolink.org/dev/view#hasMeasurementType"/>
  </owl:Restriction>
  <owl:Restriction>
    <rdfs:subClassOf rdf:resource="http://schema.geolink.org/dev/voc/nvs/P02#OPCN"/>
    <owl:someValuesFrom>
      <owl:Class>
        <owl:oneOf rdf:parseType="Collection">
          <glview:MeasurementType rdf:about="http://schema.geolink.org/dev/voc/nvs/P02#OPCN"/>
        </owl:oneOf>
      </owl:Class>
    </owl:someValuesFrom>
    <owl:onProperty rdf:resource="http://schema.geolink.org/dev/view#hasMeasurementType"/>
  </owl:Restriction>
  <owl:Restriction>
    <rdfs:subClassOf>
      <glview:MeasurementType rdf:about="http://schema.geolink.org/dev/voc/nvs/P02#FPFX">
        <rdfs:subClassOf rdf:resource="http://schema.geolink.org/dev/voc/nvs/P03#B027"/>
        <rdfs:subClassOf rdf:resource="http://schema.geolink.org/dev/voc/nvs/P03#O005"/>
        <rdfs:seeAlso rdf:resource="http://vocab.nerc.ac.uk/collection/P02/current/FPFX/"/>
        <rdfs:comment xml:lang="en">Flux of biological detritus (material derived from the water column such as exuvia and faecal pellets) in the water column</rdfs:comment>
        <rdfs:label xml:lang="en">Sedimentation flux of biological detritus in the water column</rdfs:label>
        <rdf:type rdf:resource="http://www.w3.org/2002/07/owl#NamedIndividual"/>
        <rdf:type rdf:resource="http://www.w3.org/2002/07/owl#Class"/>
      </glview:MeasurementType>
    </rdfs:subClassOf>
    <owl:someValuesFrom>
      <owl:Class>
        <owl:oneOf rdf:parseType="Collection">
          <glview:MeasurementType rdf:about="http://schema.geolink.org/dev/voc/nvs/P02#FPFX"/>
        </owl:oneOf>
      </owl:Class>
    </owl:someValuesFrom>
    <owl:onProperty rdf:resource="http://schema.geolink.org/dev/view#hasMeasurementType"/>
  </owl:Restriction>
  <owl:Restriction>
    <rdfs:subClassOf>
      <owl:NamedIndividual rdf:about="http://schema.geolink.org/dev/voc/nvs/P02#OMPW">
        <rdfs:label xml:lang="en">Organometallic species concentration parameters in sediments</rdfs:label>
        <rdfs:subClassOf rdf:resource="http://schema.geolink.org/dev/voc/nvs/P03#H001"/>
        <rdfs:subClassOf rdf:resource="http://schema.geolink.org/dev/voc/nvs/P03#G050"/>
        <rdfs:subClassOf rdf:resource="http://schema.geolink.org/dev/voc/nvs/P03#C055"/>
        <rdfs:subClassOf rdf:resource="http://schema.geolink.org/dev/voc/nvs/P03#C035"/>
        <rdfs:comment xml:lang="en">All organometallic compound concentration parameters (including saturations for gaseous species) in all phases of sediments (including pore waters)</rdfs:comment>
        <rdfs:subClassOf rdf:resource="http://schema.geolink.org/dev/voc/nvs/P03#C050"/>
        <rdf:type rdf:resource="http://schema.geolink.org/dev/view#MeasurementType"/>
        <rdfs:subClassOf rdf:resource="http://schema.geolink.org/dev/voc/nvs/P03#G035"/>
        <rdfs:seeAlso rdf:resource="http://vocab.nerc.ac.uk/collection/P02/current/OMPW/"/>
        <rdf:type rdf:resource="http://www.w3.org/2002/07/owl#Class"/>
      </owl:NamedIndividual>
    </rdfs:subClassOf>
    <owl:someValuesFrom>
      <owl:Class>
        <owl:oneOf rdf:parseType="Collection">
          <owl:NamedIndividual rdf:about="http://schema.geolink.org/dev/voc/nvs/P02#OMPW"/>
        </owl:oneOf>
      </owl:Class>
    </owl:someValuesFrom>
    <owl:onProperty rdf:resource="http://schema.geolink.org/dev/view#hasMeasurementType"/>
  </owl:Restriction>
  <owl:Restriction>
    <rdfs:subClassOf>
      <glview:MeasurementType rdf:about="http://schema.geolink.org/dev/voc/nvs/P02#MFAB">
        <rdfs:subClassOf rdf:resource="http://schema.geolink.org/dev/voc/nvs/P03#B070"/>
        <rdfs:subClassOf rdf:resource="http://schema.geolink.org/dev/voc/nvs/P03#G055"/>
        <rdfs:seeAlso rdf:resource="http://vocab.nerc.ac.uk/collection/P02/current/MFAB/"/>
        <rdfs:comment xml:lang="en">Any enumeration (e.g. count, number per square metre) of animals living on or near the seabed designated by terms other than taxonomic names (e.g. total).</rdfs:comment>
        <rdfs:label xml:lang="en">Zoobenthos generic abundance</rdfs:label>
        <rdf:type rdf:resource="http://www.w3.org/2002/07/owl#NamedIndividual"/>
        <rdf:type rdf:resource="http://www.w3.org/2002/07/owl#Class"/>
      </glview:MeasurementType>
    </rdfs:subClassOf>
    <owl:someValuesFrom>
      <owl:Class>
        <owl:oneOf rdf:parseType="Collection">
          <glview:MeasurementType rdf:about="http://schema.geolink.org/dev/voc/nvs/P02#MFAB"/>
        </owl:oneOf>
      </owl:Class>
    </owl:someValuesFrom>
    <owl:onProperty rdf:resource="http://schema.geolink.org/dev/view#hasMeasurementType"/>
  </owl:Restriction>
  <owl:Restriction>
    <rdfs:subClassOf rdf:resource="http://schema.geolink.org/dev/voc/nvs/P02#PCOC"/>
    <owl:someValuesFrom>
      <owl:Class>
        <owl:oneOf rdf:parseType="Collection">
          <glview:MeasurementType rdf:about="http://schema.geolink.org/dev/voc/nvs/P02#PCOC"/>
        </owl:oneOf>
      </owl:Class>
    </owl:someValuesFrom>
    <owl:onProperty rdf:resource="http://schema.geolink.org/dev/view#hasMeasurementType"/>
  </owl:Restriction>
  <owl:Restriction>
    <rdfs:subClassOf>
      <glview:MeasurementType rdf:about="http://schema.geolink.org/dev/voc/nvs/P02#PNTX">
        <rdfs:subClassOf rdf:resource="http://schema.geolink.org/dev/voc/nvs/P03#B030"/>
        <rdfs:subClassOf rdf:resource="http://schema.geolink.org/dev/voc/nvs/P03#B070"/>
        <rdfs:seeAlso rdf:resource="http://vocab.nerc.ac.uk/collection/P02/current/PNTX/"/>
        <rdfs:comment xml:lang="en">Any enumeration (e.g. count, abundance) of free-floating autotrophic biological entities designated by terms other than taxonomic names (e.g. microphytoplankton, ciliate, flagellate) in any body of fresh or salt water.</rdfs:comment>
        <rdfs:label xml:lang="en">Phytoplankton generic abundance in water bodies</rdfs:label>
        <rdf:type rdf:resource="http://www.w3.org/2002/07/owl#NamedIndividual"/>
        <rdf:type rdf:resource="http://www.w3.org/2002/07/owl#Class"/>
      </glview:MeasurementType>
    </rdfs:subClassOf>
    <owl:someValuesFrom>
      <owl:Class>
        <owl:oneOf rdf:parseType="Collection">
          <glview:MeasurementType rdf:about="http://schema.geolink.org/dev/voc/nvs/P02#PNTX"/>
        </owl:oneOf>
      </owl:Class>
    </owl:someValuesFrom>
    <owl:onProperty rdf:resource="http://schema.geolink.org/dev/view#hasMeasurementType"/>
  </owl:Restriction>
  <owl:Restriction>
    <rdfs:subClassOf>
      <glview:MeasurementType rdf:about="http://schema.geolink.org/dev/voc/nvs/P02#GP088">
        <rdfs:subClassOf rdf:resource="http://schema.geolink.org/dev/voc/nvs/P03#B015"/>
        <rdfs:seeAlso rdf:resource="http://vocab.nerc.ac.uk/collection/P02/current/GP088/"/>
        <rdfs:comment xml:lang="en">Parameters describing the actions or reactions of birds (Class Aves), usually in response to the environment. Includes both parameters mapped to taxa and those mapped to non-taxonomic groupings.</rdfs:comment>
        <rdfs:label xml:lang="en">Bird behaviour</rdfs:label>
        <rdf:type rdf:resource="http://www.w3.org/2002/07/owl#NamedIndividual"/>
        <rdf:type rdf:resource="http://www.w3.org/2002/07/owl#Class"/>
      </glview:MeasurementType>
    </rdfs:subClassOf>
    <owl:someValuesFrom>
      <owl:Class>
        <owl:oneOf rdf:parseType="Collection">
          <glview:MeasurementType rdf:about="http://schema.geolink.org/dev/voc/nvs/P02#GP088"/>
        </owl:oneOf>
      </owl:Class>
    </owl:someValuesFrom>
    <owl:onProperty rdf:resource="http://schema.geolink.org/dev/view#hasMeasurementType"/>
  </owl:Restriction>
  <owl:Restriction>
    <rdfs:subClassOf>
      <glview:MeasurementType rdf:about="http://schema.geolink.org/dev/voc/nvs/P02#OPWC">
        <rdfs:subClassOf rdf:resource="http://schema.geolink.org/dev/voc/nvs/P03#B035"/>
        <rdfs:seeAlso rdf:resource="http://vocab.nerc.ac.uk/collection/P02/current/OPWC/"/>
        <rdfs:comment xml:lang="en">Includes all pigments that cannot be explicitly classified as chlorophylls, phaeopigments or carotenoids.  Generally, these are parameters where different pigments have been grouped together. Concentrations are expressed in terms of per unit volume or unit area of the water column.  Does not include data expressed per unit mass of SPM.</rdfs:comment>
        <rdfs:label xml:lang="en">Unclassified pigment concentrations in the water column</rdfs:label>
        <rdf:type rdf:resource="http://www.w3.org/2002/07/owl#NamedIndividual"/>
        <rdf:type rdf:resource="http://www.w3.org/2002/07/owl#Class"/>
      </glview:MeasurementType>
    </rdfs:subClassOf>
    <owl:someValuesFrom>
      <owl:Class>
        <owl:oneOf rdf:parseType="Collection">
          <glview:MeasurementType rdf:about="http://schema.geolink.org/dev/voc/nvs/P02#OPWC"/>
        </owl:oneOf>
      </owl:Class>
    </owl:someValuesFrom>
    <owl:onProperty rdf:resource="http://schema.geolink.org/dev/view#hasMeasurementType"/>
  </owl:Restriction>
  <owl:Restriction>
    <rdfs:subClassOf>
      <glview:MeasurementType rdf:about="http://schema.geolink.org/dev/voc/nvs/P02#ALAT">
        <rdfs:subClassOf rdf:resource="http://schema.geolink.org/dev/voc/nvs/P03#Z005"/>
        <rdfs:seeAlso rdf:resource="http://vocab.nerc.ac.uk/collection/P02/current/ALAT/"/>
        <rdfs:comment xml:lang="en">All forms of horizontal spatial coordinates such as lat/lon and grid references</rdfs:comment>
        <rdfs:label xml:lang="en">Horizontal spatial co-ordinates</rdfs:label>
        <rdf:type rdf:resource="http://www.w3.org/2002/07/owl#NamedIndividual"/>
        <rdf:type rdf:resource="http://www.w3.org/2002/07/owl#Class"/>
      </glview:MeasurementType>
    </rdfs:subClassOf>
    <owl:someValuesFrom>
      <owl:Class>
        <owl:oneOf rdf:parseType="Collection">
          <glview:MeasurementType rdf:about="http://schema.geolink.org/dev/voc/nvs/P02#ALAT"/>
        </owl:oneOf>
      </owl:Class>
    </owl:someValuesFrom>
    <owl:onProperty rdf:resource="http://schema.geolink.org/dev/view#hasMeasurementType"/>
  </owl:Restriction>
  <owl:Restriction>
    <rdfs:subClassOf>
      <glview:MeasurementType rdf:about="http://schema.geolink.org/dev/voc/nvs/P02#CLXX">
        <rdfs:subClassOf rdf:resource="http://schema.geolink.org/dev/voc/nvs/P03#C045"/>
        <rdfs:seeAlso rdf:resource="http://vocab.nerc.ac.uk/collection/P02/current/CLXX/"/>
        <rdfs:comment xml:lang="en">Concentrations of halogens as elements or their inorganic compounds in all phases of sediment pore water</rdfs:comment>
        <rdfs:label xml:lang="en">Concentration of inorganic halogens in sediment pore waters</rdfs:label>
        <rdf:type rdf:resource="http://www.w3.org/2002/07/owl#NamedIndividual"/>
        <rdf:type rdf:resource="http://www.w3.org/2002/07/owl#Class"/>
      </glview:MeasurementType>
    </rdfs:subClassOf>
    <owl:someValuesFrom>
      <owl:Class>
        <owl:oneOf rdf:parseType="Collection">
          <glview:MeasurementType rdf:about="http://schema.geolink.org/dev/voc/nvs/P02#CLXX"/>
        </owl:oneOf>
      </owl:Class>
    </owl:someValuesFrom>
    <owl:onProperty rdf:resource="http://schema.geolink.org/dev/view#hasMeasurementType"/>
  </owl:Restriction>
  <owl:Restriction>
    <rdfs:subClassOf>
      <glview:MeasurementType rdf:about="http://schema.geolink.org/dev/voc/nvs/P02#AMUP">
        <rdfs:subClassOf rdf:resource="http://schema.geolink.org/dev/voc/nvs/P03#O010"/>
        <rdfs:subClassOf rdf:resource="http://schema.geolink.org/dev/voc/nvs/P03#C040"/>
        <rdfs:seeAlso rdf:resource="http://vocab.nerc.ac.uk/collection/P02/current/AMUP/"/>
        <rdfs:comment xml:lang="en">Parameters quantifying the uptake rate of nitrogen from excretion products (ammonium and urea) by flora and fauna living in any body of salt or fresh water</rdfs:comment>
        <rdfs:label xml:lang="en">Regenerated production in water bodies</rdfs:label>
        <rdf:type rdf:resource="http://www.w3.org/2002/07/owl#NamedIndividual"/>
        <rdf:type rdf:resource="http://www.w3.org/2002/07/owl#Class"/>
      </glview:MeasurementType>
    </rdfs:subClassOf>
    <owl:someValuesFrom>
      <owl:Class>
        <owl:oneOf rdf:parseType="Collection">
          <glview:MeasurementType rdf:about="http://schema.geolink.org/dev/voc/nvs/P02#AMUP"/>
        </owl:oneOf>
      </owl:Class>
    </owl:someValuesFrom>
    <owl:onProperty rdf:resource="http://schema.geolink.org/dev/view#hasMeasurementType"/>
  </owl:Restriction>
  <owl:Restriction>
    <rdfs:subClassOf>
      <glview:MeasurementType rdf:about="http://schema.geolink.org/dev/voc/nvs/P02#MTSP">
        <rdfs:subClassOf rdf:resource="http://schema.geolink.org/dev/view#Measurement"/>
        <rdfs:seeAlso rdf:resource="http://vocab.nerc.ac.uk/collection/P02/current/MTSP/"/>
        <rdfs:comment xml:lang="en">Concentrations of metal elements in suspended particulate material collected by water column filtration, centrifugation or sediment trapping. Deprecated as semantic overlap with MTWP.</rdfs:comment>
        <rdfs:label xml:lang="en">Metal concentrations in suspended particulate material</rdfs:label>
        <rdf:type rdf:resource="http://www.w3.org/2002/07/owl#NamedIndividual"/>
        <rdf:type rdf:resource="http://www.w3.org/2002/07/owl#Class"/>
      </glview:MeasurementType>
    </rdfs:subClassOf>
    <owl:someValuesFrom>
      <owl:Class>
        <owl:oneOf rdf:parseType="Collection">
          <glview:MeasurementType rdf:about="http://schema.geolink.org/dev/voc/nvs/P02#MTSP"/>
        </owl:oneOf>
      </owl:Class>
    </owl:someValuesFrom>
    <owl:onProperty rdf:resource="http://schema.geolink.org/dev/view#hasMeasurementType"/>
  </owl:Restriction>
  <owl:Restriction>
    <rdfs:subClassOf rdf:resource="http://schema.geolink.org/dev/voc/nvs/P02#MMAN"/>
    <owl:someValuesFrom>
      <owl:Class>
        <owl:oneOf rdf:parseType="Collection">
          <glview:MeasurementType rdf:about="http://schema.geolink.org/dev/voc/nvs/P02#MMAN"/>
        </owl:oneOf>
      </owl:Class>
    </owl:someValuesFrom>
    <owl:onProperty rdf:resource="http://schema.geolink.org/dev/view#hasMeasurementType"/>
  </owl:Restriction>
  <owl:Restriction>
    <rdfs:subClassOf>
      <glview:MeasurementType rdf:about="http://schema.geolink.org/dev/voc/nvs/P02#ZATX">
        <rdfs:subClassOf rdf:resource="http://schema.geolink.org/dev/voc/nvs/P03#B045"/>
        <rdfs:subClassOf rdf:resource="http://schema.geolink.org/dev/voc/nvs/P03#B070"/>
        <rdfs:seeAlso rdf:resource="http://vocab.nerc.ac.uk/collection/P02/current/ZATX/"/>
        <rdfs:comment xml:lang="en">Zooplankton (mesozooplankton plus larger pelagic animals excluding fish, reptiles and mammals) abundance parameters presented at the level of taxa that may be mapped to entities in the ITIS taxonomy.  These may be at any taxonomic level from sub-species upwards.</rdfs:comment>
        <rdfs:label xml:lang="en">Zooplankton taxonomy-related abundance per unit volume of the water column</rdfs:label>
        <rdf:type rdf:resource="http://www.w3.org/2002/07/owl#NamedIndividual"/>
        <rdf:type rdf:resource="http://www.w3.org/2002/07/owl#Class"/>
      </glview:MeasurementType>
    </rdfs:subClassOf>
    <owl:someValuesFrom>
      <owl:Class>
        <owl:oneOf rdf:parseType="Collection">
          <glview:MeasurementType rdf:about="http://schema.geolink.org/dev/voc/nvs/P02#ZATX"/>
        </owl:oneOf>
      </owl:Class>
    </owl:someValuesFrom>
    <owl:onProperty rdf:resource="http://schema.geolink.org/dev/view#hasMeasurementType"/>
  </owl:Restriction>
  <owl:Restriction>
    <rdfs:subClassOf>
      <glview:MeasurementType rdf:about="http://schema.geolink.org/dev/voc/nvs/P02#HAAC">
        <rdfs:subClassOf rdf:resource="http://schema.geolink.org/dev/voc/nvs/P03#G035"/>
        <rdfs:subClassOf rdf:resource="http://schema.geolink.org/dev/voc/nvs/P03#C003"/>
        <rdfs:seeAlso rdf:resource="http://vocab.nerc.ac.uk/collection/P02/current/HAAC/"/>
        <rdfs:comment xml:lang="en">Parameters quantifying the amount of organic compounds containing both a carboxyl group and an amino group in unlithified seabed material.</rdfs:comment>
        <rdfs:label xml:lang="en">Amino acids in sediment</rdfs:label>
        <rdf:type rdf:resource="http://www.w3.org/2002/07/owl#NamedIndividual"/>
        <rdf:type rdf:resource="http://www.w3.org/2002/07/owl#Class"/>
      </glview:MeasurementType>
    </rdfs:subClassOf>
    <owl:someValuesFrom>
      <owl:Class>
        <owl:oneOf rdf:parseType="Collection">
          <glview:MeasurementType rdf:about="http://schema.geolink.org/dev/voc/nvs/P02#HAAC"/>
        </owl:oneOf>
      </owl:Class>
    </owl:someValuesFrom>
    <owl:onProperty rdf:resource="http://schema.geolink.org/dev/view#hasMeasurementType"/>
  </owl:Restriction>
  <owl:Restriction>
    <rdfs:subClassOf>
      <glview:MeasurementType rdf:about="http://schema.geolink.org/dev/voc/nvs/P02#BNTX">
        <rdfs:subClassOf rdf:resource="http://schema.geolink.org/dev/voc/nvs/P03#B070"/>
        <rdfs:subClassOf rdf:resource="http://schema.geolink.org/dev/voc/nvs/P03#B005"/>
        <rdfs:seeAlso rdf:resource="http://vocab.nerc.ac.uk/collection/P02/current/BNTX/"/>
        <rdfs:comment xml:lang="en">Any enumeration of bacteria (Kingdom Monera so includes cyanobacteria) designated by terms other than taxonomic names (e.g. total) in any body of fresh or salt water.</rdfs:comment>
        <rdfs:label xml:lang="en">Bacteria generic abundance in water bodies</rdfs:label>
        <rdf:type rdf:resource="http://www.w3.org/2002/07/owl#NamedIndividual"/>
        <rdf:type rdf:resource="http://www.w3.org/2002/07/owl#Class"/>
      </glview:MeasurementType>
    </rdfs:subClassOf>
    <owl:someValuesFrom>
      <owl:Class>
        <owl:oneOf rdf:parseType="Collection">
          <glview:MeasurementType rdf:about="http://schema.geolink.org/dev/voc/nvs/P02#BNTX"/>
        </owl:oneOf>
      </owl:Class>
    </owl:someValuesFrom>
    <owl:onProperty rdf:resource="http://schema.geolink.org/dev/view#hasMeasurementType"/>
  </owl:Restriction>
  <owl:Restriction>
    <rdfs:subClassOf>
      <glview:MeasurementType rdf:about="http://schema.geolink.org/dev/voc/nvs/P02#PPAB">
        <rdfs:subClassOf rdf:resource="http://schema.geolink.org/dev/voc/nvs/P03#D015"/>
        <rdfs:seeAlso rdf:resource="http://vocab.nerc.ac.uk/collection/P02/current/PPAB/"/>
        <rdfs:comment xml:lang="en">Water column spectral absorption parameters</rdfs:comment>
        <rdfs:label xml:lang="en">Light absorption in the water column</rdfs:label>
        <rdf:type rdf:resource="http://www.w3.org/2002/07/owl#NamedIndividual"/>
        <rdf:type rdf:resource="http://www.w3.org/2002/07/owl#Class"/>
      </glview:MeasurementType>
    </rdfs:subClassOf>
    <owl:someValuesFrom>
      <owl:Class>
        <owl:oneOf rdf:parseType="Collection">
          <glview:MeasurementType rdf:about="http://schema.geolink.org/dev/voc/nvs/P02#PPAB"/>
        </owl:oneOf>
      </owl:Class>
    </owl:someValuesFrom>
    <owl:onProperty rdf:resource="http://schema.geolink.org/dev/view#hasMeasurementType"/>
  </owl:Restriction>
  <owl:Restriction>
    <rdfs:subClassOf>
      <glview:MeasurementType rdf:about="http://schema.geolink.org/dev/voc/nvs/P02#FBAB">
        <rdfs:subClassOf rdf:resource="http://schema.geolink.org/dev/voc/nvs/P03#B070"/>
        <rdfs:subClassOf rdf:resource="http://schema.geolink.org/dev/voc/nvs/P03#B020"/>
        <rdfs:subClassOf rdf:resource="http://schema.geolink.org/dev/voc/nvs/P03#G055"/>
        <rdfs:seeAlso rdf:resource="http://vocab.nerc.ac.uk/collection/P02/current/FBAB/"/>
        <rdfs:comment xml:lang="en">Fish (Osteichthyes, Agnatha and Chondrichthyes) abundance per unit area of bed (sea, river, lake etc.) parameters presented at the level of taxa that may be mapped to entities in the ITIS taxonomy.  Includes animals normally considered as planktonic if they have been returned from sediment samples.</rdfs:comment>
        <rdfs:label xml:lang="en">Fish taxonomy-related abundance per unit area of the bed</rdfs:label>
        <rdf:type rdf:resource="http://www.w3.org/2002/07/owl#NamedIndividual"/>
        <rdf:type rdf:resource="http://www.w3.org/2002/07/owl#Class"/>
      </glview:MeasurementType>
    </rdfs:subClassOf>
    <owl:someValuesFrom>
      <owl:Class>
        <owl:oneOf rdf:parseType="Collection">
          <glview:MeasurementType rdf:about="http://schema.geolink.org/dev/voc/nvs/P02#FBAB"/>
        </owl:oneOf>
      </owl:Class>
    </owl:someValuesFrom>
    <owl:onProperty rdf:resource="http://schema.geolink.org/dev/view#hasMeasurementType"/>
  </owl:Restriction>
  <owl:Restriction>
    <rdfs:subClassOf>
      <glview:MeasurementType rdf:about="http://schema.geolink.org/dev/voc/nvs/P02#SDAC">
        <rdfs:subClassOf rdf:resource="http://schema.geolink.org/dev/voc/nvs/P03#GPYS"/>
        <rdfs:subClassOf rdf:resource="http://schema.geolink.org/dev/voc/nvs/P03#G012"/>
        <rdfs:seeAlso rdf:resource="http://vocab.nerc.ac.uk/collection/P02/current/SDAC/"/>
        <rdfs:comment xml:lang="en">Parameters relating to the elucidation of sediment structure by quantifying the proportion of waves from a low energy source reflected by sub-surface layers.</rdfs:comment>
        <rdfs:label xml:lang="en">Sediment acoustics</rdfs:label>
        <rdf:type rdf:resource="http://www.w3.org/2002/07/owl#NamedIndividual"/>
        <rdf:type rdf:resource="http://www.w3.org/2002/07/owl#Class"/>
      </glview:MeasurementType>
    </rdfs:subClassOf>
    <owl:someValuesFrom>
      <owl:Class>
        <owl:oneOf rdf:parseType="Collection">
          <glview:MeasurementType rdf:about="http://schema.geolink.org/dev/voc/nvs/P02#SDAC"/>
        </owl:oneOf>
      </owl:Class>
    </owl:someValuesFrom>
    <owl:onProperty rdf:resource="http://schema.geolink.org/dev/view#hasMeasurementType"/>
  </owl:Restriction>
  <owl:Restriction>
    <rdfs:subClassOf>
      <glview:MeasurementType rdf:about="http://schema.geolink.org/dev/voc/nvs/P02#BNUC">
        <rdfs:subClassOf rdf:resource="http://schema.geolink.org/dev/voc/nvs/P03#B070"/>
        <rdfs:subClassOf rdf:resource="http://schema.geolink.org/dev/voc/nvs/P03#B005"/>
        <rdfs:seeAlso rdf:resource="http://vocab.nerc.ac.uk/collection/P02/current/BNUC/"/>
        <rdfs:comment xml:lang="en">Any enumeration of bacteria (Kingdom Monera so includes cyanobacteria) designated by terms other than taxonomic names (e.g. total) in any soil or sediment.</rdfs:comment>
        <rdfs:label xml:lang="en">Bacteria generic abundance in sediment</rdfs:label>
        <rdf:type rdf:resource="http://www.w3.org/2002/07/owl#NamedIndividual"/>
        <rdf:type rdf:resource="http://www.w3.org/2002/07/owl#Class"/>
      </glview:MeasurementType>
    </rdfs:subClassOf>
    <owl:someValuesFrom>
      <owl:Class>
        <owl:oneOf rdf:parseType="Collection">
          <glview:MeasurementType rdf:about="http://schema.geolink.org/dev/voc/nvs/P02#BNUC"/>
        </owl:oneOf>
      </owl:Class>
    </owl:someValuesFrom>
    <owl:onProperty rdf:resource="http://schema.geolink.org/dev/view#hasMeasurementType"/>
  </owl:Restriction>
  <owl:Restriction>
    <rdfs:subClassOf>
      <glview:MeasurementType rdf:about="http://schema.geolink.org/dev/voc/nvs/P02#IATC">
        <rdfs:subClassOf rdf:resource="http://schema.geolink.org/dev/voc/nvs/P03#B045"/>
        <rdfs:subClassOf rdf:resource="http://schema.geolink.org/dev/voc/nvs/P03#B070"/>
        <rdfs:seeAlso rdf:resource="http://vocab.nerc.ac.uk/collection/P02/current/IATC/"/>
        <rdfs:comment xml:lang="en">Insecta carbon biomass parameters presented at the level of taxa that may be mapped to entities in the ITIS taxonomy.  These may be at any taxonomic level from sub-species upwards.</rdfs:comment>
        <rdfs:label xml:lang="en">Insecta taxonomy-related biomass expressed as carbon per unit volume of the water column</rdfs:label>
        <rdf:type rdf:resource="http://www.w3.org/2002/07/owl#NamedIndividual"/>
        <rdf:type rdf:resource="http://www.w3.org/2002/07/owl#Class"/>
      </glview:MeasurementType>
    </rdfs:subClassOf>
    <owl:someValuesFrom>
      <owl:Class>
        <owl:oneOf rdf:parseType="Collection">
          <glview:MeasurementType rdf:about="http://schema.geolink.org/dev/voc/nvs/P02#IATC"/>
        </owl:oneOf>
      </owl:Class>
    </owl:someValuesFrom>
    <owl:onProperty rdf:resource="http://schema.geolink.org/dev/view#hasMeasurementType"/>
  </owl:Restriction>
  <owl:Restriction>
    <rdfs:subClassOf rdf:resource="http://schema.geolink.org/dev/voc/nvs/P02#FPFX"/>
    <owl:someValuesFrom>
      <owl:Class>
        <owl:oneOf rdf:parseType="Collection">
          <glview:MeasurementType rdf:about="http://schema.geolink.org/dev/voc/nvs/P02#FPFX"/>
        </owl:oneOf>
      </owl:Class>
    </owl:someValuesFrom>
    <owl:onProperty rdf:resource="http://schema.geolink.org/dev/view#hasMeasurementType"/>
  </owl:Restriction>
  <owl:Restriction>
    <rdfs:subClassOf>
      <glview:MeasurementType rdf:about="http://schema.geolink.org/dev/voc/nvs/P02#CNDC">
        <rdfs:subClassOf rdf:resource="http://schema.geolink.org/dev/voc/nvs/P03#D025"/>
        <rdfs:seeAlso rdf:resource="http://vocab.nerc.ac.uk/collection/P02/current/CNDC/"/>
        <rdfs:comment xml:lang="en">Parameters quantifying the flow of electrical current through or the electrical resistance of a body of water at any point between the bed and the atmosphere</rdfs:comment>
        <rdfs:label xml:lang="en">Electrical conductivity of the water column</rdfs:label>
        <rdf:type rdf:resource="http://www.w3.org/2002/07/owl#NamedIndividual"/>
        <rdf:type rdf:resource="http://www.w3.org/2002/07/owl#Class"/>
      </glview:MeasurementType>
    </rdfs:subClassOf>
    <owl:someValuesFrom>
      <owl:Class>
        <owl:oneOf rdf:parseType="Collection">
          <glview:MeasurementType rdf:about="http://schema.geolink.org/dev/voc/nvs/P02#CNDC"/>
        </owl:oneOf>
      </owl:Class>
    </owl:someValuesFrom>
    <owl:onProperty rdf:resource="http://schema.geolink.org/dev/view#hasMeasurementType"/>
  </owl:Restriction>
  <owl:Restriction>
    <rdfs:subClassOf rdf:resource="http://schema.geolink.org/dev/voc/nvs/P02#PEWB"/>
    <owl:someValuesFrom>
      <owl:Class>
        <owl:oneOf rdf:parseType="Collection">
          <glview:MeasurementType rdf:about="http://schema.geolink.org/dev/voc/nvs/P02#PEWB"/>
        </owl:oneOf>
      </owl:Class>
    </owl:someValuesFrom>
    <owl:onProperty rdf:resource="http://schema.geolink.org/dev/view#hasMeasurementType"/>
  </owl:Restriction>
  <owl:Restriction>
    <rdfs:subClassOf>
      <glview:MeasurementType rdf:about="http://schema.geolink.org/dev/voc/nvs/P02#PU02">
        <rdfs:subClassOf rdf:resource="http://schema.geolink.org/dev/voc/nvs/P03#B070"/>
        <rdfs:subClassOf rdf:resource="http://schema.geolink.org/dev/voc/nvs/P03#B055"/>
        <rdfs:seeAlso rdf:resource="http://vocab.nerc.ac.uk/collection/P02/current/PU02/"/>
        <rdfs:comment xml:lang="en">Any enumeration (e.g. count, number per litre) of macroalgae (seaweeds) designated by terms other than taxonomic names (e.g. total) in any fresh or salt water body.</rdfs:comment>
        <rdfs:label xml:lang="en">Macroalgae generic abundance in water bodies</rdfs:label>
        <rdf:type rdf:resource="http://www.w3.org/2002/07/owl#NamedIndividual"/>
        <rdf:type rdf:resource="http://www.w3.org/2002/07/owl#Class"/>
      </glview:MeasurementType>
    </rdfs:subClassOf>
    <owl:someValuesFrom>
      <owl:Class>
        <owl:oneOf rdf:parseType="Collection">
          <glview:MeasurementType rdf:about="http://schema.geolink.org/dev/voc/nvs/P02#PU02"/>
        </owl:oneOf>
      </owl:Class>
    </owl:someValuesFrom>
    <owl:onProperty rdf:resource="http://schema.geolink.org/dev/view#hasMeasurementType"/>
  </owl:Restriction>
  <owl:Restriction>
    <rdfs:subClassOf>
      <glview:MeasurementType rdf:about="http://schema.geolink.org/dev/voc/nvs/P02#NTOT">
        <rdfs:subClassOf rdf:resource="http://schema.geolink.org/dev/voc/nvs/P03#C005"/>
        <rdfs:seeAlso rdf:resource="http://vocab.nerc.ac.uk/collection/P02/current/NTOT/"/>
        <rdfs:comment xml:lang="en">Concentrations of total and organic nitrogen in the particulate phase of the water column, which is a function of both the SPM concentration in the water column and the concentration of nitrogen per unit weight of SPM. Note that it is commonly assumed that all particulate nitrogen is organic.</rdfs:comment>
        <rdfs:label xml:lang="en">Particulate total and organic nitrogen concentrations in the water column</rdfs:label>
        <rdf:type rdf:resource="http://www.w3.org/2002/07/owl#NamedIndividual"/>
        <rdf:type rdf:resource="http://www.w3.org/2002/07/owl#Class"/>
      </glview:MeasurementType>
    </rdfs:subClassOf>
    <owl:someValuesFrom>
      <owl:Class>
        <owl:oneOf rdf:parseType="Collection">
          <glview:MeasurementType rdf:about="http://schema.geolink.org/dev/voc/nvs/P02#NTOT"/>
        </owl:oneOf>
      </owl:Class>
    </owl:someValuesFrom>
    <owl:onProperty rdf:resource="http://schema.geolink.org/dev/view#hasMeasurementType"/>
  </owl:Restriction>
  <owl:Restriction>
    <rdfs:subClassOf>
      <glview:MeasurementType rdf:about="http://schema.geolink.org/dev/voc/nvs/P02#FBAF">
        <rdfs:subClassOf rdf:resource="http://schema.geolink.org/dev/voc/nvs/P03#B070"/>
        <rdfs:subClassOf rdf:resource="http://schema.geolink.org/dev/voc/nvs/P03#B020"/>
        <rdfs:subClassOf rdf:resource="http://schema.geolink.org/dev/voc/nvs/P03#G055"/>
        <rdfs:seeAlso rdf:resource="http://vocab.nerc.ac.uk/collection/P02/current/FBAF/"/>
        <rdfs:comment xml:lang="en">Fish (Osteichthyes, Agnatha and Chondrichthyes) ash-free dry weight biomass per unit area of bed (sea, river, lake etc.) parameters presented at the level of taxa that may be mapped to entities in the ITIS taxonomy.  Includes animals normally considered as planktonic if they have been returned from sediment samples.</rdfs:comment>
        <rdfs:label xml:lang="en">Fish taxonomy-related ash-free dry weight biomass per unit area of the bed</rdfs:label>
        <rdf:type rdf:resource="http://www.w3.org/2002/07/owl#NamedIndividual"/>
        <rdf:type rdf:resource="http://www.w3.org/2002/07/owl#Class"/>
      </glview:MeasurementType>
    </rdfs:subClassOf>
    <owl:someValuesFrom>
      <owl:Class>
        <owl:oneOf rdf:parseType="Collection">
          <glview:MeasurementType rdf:about="http://schema.geolink.org/dev/voc/nvs/P02#FBAF"/>
        </owl:oneOf>
      </owl:Class>
    </owl:someValuesFrom>
    <owl:onProperty rdf:resource="http://schema.geolink.org/dev/view#hasMeasurementType"/>
  </owl:Restriction>
  <owl:Restriction>
    <rdfs:subClassOf>
      <glview:MeasurementType rdf:about="http://schema.geolink.org/dev/voc/nvs/P02#IS4R">
        <rdfs:subClassOf rdf:resource="http://schema.geolink.org/dev/voc/nvs/P03#O010"/>
        <rdfs:seeAlso rdf:resource="http://vocab.nerc.ac.uk/collection/P02/current/IS4R/"/>
        <rdfs:comment xml:lang="en">Reduction rates of any species in sediment cores</rdfs:comment>
        <rdfs:label xml:lang="en">Reduction rates in bed sediments</rdfs:label>
        <rdf:type rdf:resource="http://www.w3.org/2002/07/owl#NamedIndividual"/>
        <rdf:type rdf:resource="http://www.w3.org/2002/07/owl#Class"/>
      </glview:MeasurementType>
    </rdfs:subClassOf>
    <owl:someValuesFrom>
      <owl:Class>
        <owl:oneOf rdf:parseType="Collection">
          <glview:MeasurementType rdf:about="http://schema.geolink.org/dev/voc/nvs/P02#IS4R"/>
        </owl:oneOf>
      </owl:Class>
    </owl:someValuesFrom>
    <owl:onProperty rdf:resource="http://schema.geolink.org/dev/view#hasMeasurementType"/>
  </owl:Restriction>
  <owl:Restriction>
    <rdfs:subClassOf>
      <glview:MeasurementType rdf:about="http://schema.geolink.org/dev/voc/nvs/P02#CING">
        <rdfs:subClassOf rdf:resource="http://schema.geolink.org/dev/voc/nvs/P03#C005"/>
        <rdfs:seeAlso rdf:resource="http://vocab.nerc.ac.uk/collection/P02/current/CING/"/>
        <rdfs:comment xml:lang="en">Concentrations of inorganic carbon in the particulate phase of the water column as extracted by a fitration technique.  This is the particle-bound concentration per unit volume of the water column. Consequently, it is both a function of the SPM concentration in the water column and the concentration of inorganic carbon per unit weight of the SPM.</rdfs:comment>
        <rdfs:label xml:lang="en">Particulate inorganic carbon concentrations in the water column</rdfs:label>
        <rdf:type rdf:resource="http://www.w3.org/2002/07/owl#NamedIndividual"/>
        <rdf:type rdf:resource="http://www.w3.org/2002/07/owl#Class"/>
      </glview:MeasurementType>
    </rdfs:subClassOf>
    <owl:someValuesFrom>
      <owl:Class>
        <owl:oneOf rdf:parseType="Collection">
          <glview:MeasurementType rdf:about="http://schema.geolink.org/dev/voc/nvs/P02#CING"/>
        </owl:oneOf>
      </owl:Class>
    </owl:someValuesFrom>
    <owl:onProperty rdf:resource="http://schema.geolink.org/dev/view#hasMeasurementType"/>
  </owl:Restriction>
  <owl:Restriction>
    <rdfs:subClassOf>
      <glview:MeasurementType rdf:about="http://schema.geolink.org/dev/voc/nvs/P02#WCWT">
        <rdfs:subClassOf rdf:resource="http://schema.geolink.org/dev/voc/nvs/P03#G040"/>
        <rdfs:seeAlso rdf:resource="http://vocab.nerc.ac.uk/collection/P02/current/WCWT/"/>
        <rdfs:comment xml:lang="en">Sediment porosity (water content by volume) and water content by weight parameters</rdfs:comment>
        <rdfs:label xml:lang="en">Sediment water content, porosity and surface area</rdfs:label>
        <rdf:type rdf:resource="http://www.w3.org/2002/07/owl#NamedIndividual"/>
        <rdf:type rdf:resource="http://www.w3.org/2002/07/owl#Class"/>
      </glview:MeasurementType>
    </rdfs:subClassOf>
    <owl:someValuesFrom>
      <owl:Class>
        <owl:oneOf rdf:parseType="Collection">
          <glview:MeasurementType rdf:about="http://schema.geolink.org/dev/voc/nvs/P02#WCWT"/>
        </owl:oneOf>
      </owl:Class>
    </owl:someValuesFrom>
    <owl:onProperty rdf:resource="http://schema.geolink.org/dev/view#hasMeasurementType"/>
  </owl:Restriction>
  <owl:Restriction>
    <rdfs:subClassOf>
      <glview:MeasurementType rdf:about="http://schema.geolink.org/dev/voc/nvs/P02#PYTT">
        <rdfs:subClassOf rdf:resource="http://schema.geolink.org/dev/voc/nvs/P03#B070"/>
        <rdfs:seeAlso rdf:resource="http://vocab.nerc.ac.uk/collection/P02/current/PYTT/"/>
        <rdfs:comment xml:lang="en">Used for plankton abundance parameters where no differentiation between phytoplankton, microzooplankton or zooplankton is possible</rdfs:comment>
        <rdfs:label xml:lang="en">Plankton abundance per unit volume of the water column</rdfs:label>
        <rdf:type rdf:resource="http://www.w3.org/2002/07/owl#NamedIndividual"/>
        <rdf:type rdf:resource="http://www.w3.org/2002/07/owl#Class"/>
      </glview:MeasurementType>
    </rdfs:subClassOf>
    <owl:someValuesFrom>
      <owl:Class>
        <owl:oneOf rdf:parseType="Collection">
          <glview:MeasurementType rdf:about="http://schema.geolink.org/dev/voc/nvs/P02#PYTT"/>
        </owl:oneOf>
      </owl:Class>
    </owl:someValuesFrom>
    <owl:onProperty rdf:resource="http://schema.geolink.org/dev/view#hasMeasurementType"/>
  </owl:Restriction>
  <owl:Restriction>
    <rdfs:subClassOf>
      <glview:MeasurementType rdf:about="http://schema.geolink.org/dev/voc/nvs/P02#FCRT">
        <rdfs:subClassOf rdf:resource="http://schema.geolink.org/dev/voc/nvs/P03#B045"/>
        <rdfs:subClassOf rdf:resource="http://schema.geolink.org/dev/voc/nvs/P03#O010"/>
        <rdfs:seeAlso rdf:resource="http://vocab.nerc.ac.uk/collection/P02/current/FCRT/"/>
        <rdfs:comment xml:lang="en">Parameters quantifying the ingestion of food by zooplankton (mesozooplankton and larger but excluding fish) in terms of identified biota or chemical species and the effects of nutrition on life processes such as physiology and reproduction.</rdfs:comment>
        <rdfs:label xml:lang="en">Zooplankton feeding</rdfs:label>
        <rdf:type rdf:resource="http://www.w3.org/2002/07/owl#NamedIndividual"/>
        <rdf:type rdf:resource="http://www.w3.org/2002/07/owl#Class"/>
      </glview:MeasurementType>
    </rdfs:subClassOf>
    <owl:someValuesFrom>
      <owl:Class>
        <owl:oneOf rdf:parseType="Collection">
          <glview:MeasurementType rdf:about="http://schema.geolink.org/dev/voc/nvs/P02#FCRT"/>
        </owl:oneOf>
      </owl:Class>
    </owl:someValuesFrom>
    <owl:onProperty rdf:resource="http://schema.geolink.org/dev/view#hasMeasurementType"/>
  </owl:Restriction>
  <owl:Restriction>
    <rdfs:subClassOf>
      <glview:MeasurementType rdf:about="http://schema.geolink.org/dev/voc/nvs/P02#PASR">
        <rdfs:subClassOf rdf:resource="http://schema.geolink.org/dev/voc/nvs/P03#GPYS"/>
        <rdfs:subClassOf rdf:resource="http://schema.geolink.org/dev/voc/nvs/P03#G012"/>
        <rdfs:seeAlso rdf:resource="http://vocab.nerc.ac.uk/collection/P02/current/PASR/"/>
        <rdfs:comment xml:lang="en">Parameters quantifying the magnitude of naturally occurring low frequency earth movements such as used for earthquake seismology and natural noise studies.</rdfs:comment>
        <rdfs:label xml:lang="en">Passive seismic refraction</rdfs:label>
        <rdf:type rdf:resource="http://www.w3.org/2002/07/owl#NamedIndividual"/>
        <rdf:type rdf:resource="http://www.w3.org/2002/07/owl#Class"/>
      </glview:MeasurementType>
    </rdfs:subClassOf>
    <owl:someValuesFrom>
      <owl:Class>
        <owl:oneOf rdf:parseType="Collection">
          <glview:MeasurementType rdf:about="http://schema.geolink.org/dev/voc/nvs/P02#PASR"/>
        </owl:oneOf>
      </owl:Class>
    </owl:someValuesFrom>
    <owl:onProperty rdf:resource="http://schema.geolink.org/dev/view#hasMeasurementType"/>
  </owl:Restriction>
  <owl:Restriction>
    <rdfs:subClassOf>
      <glview:MeasurementType rdf:about="http://schema.geolink.org/dev/voc/nvs/P02#SPAG">
        <rdfs:subClassOf rdf:resource="http://schema.geolink.org/dev/voc/nvs/P03#G030"/>
        <rdfs:seeAlso rdf:resource="http://vocab.nerc.ac.uk/collection/P02/current/SPAG/"/>
        <rdfs:comment xml:lang="en">Measured or stratigraphically estimated ages of secondary mineral deposits in caves. This includes stalactites, stalagmites, flowstone, and crystal growths.</rdfs:comment>
        <rdfs:label xml:lang="en">Speleothem age</rdfs:label>
        <rdf:type rdf:resource="http://www.w3.org/2002/07/owl#NamedIndividual"/>
        <rdf:type rdf:resource="http://www.w3.org/2002/07/owl#Class"/>
      </glview:MeasurementType>
    </rdfs:subClassOf>
    <owl:someValuesFrom>
      <owl:Class>
        <owl:oneOf rdf:parseType="Collection">
          <glview:MeasurementType rdf:about="http://schema.geolink.org/dev/voc/nvs/P02#SPAG"/>
        </owl:oneOf>
      </owl:Class>
    </owl:someValuesFrom>
    <owl:onProperty rdf:resource="http://schema.geolink.org/dev/view#hasMeasurementType"/>
  </owl:Restriction>
  <owl:Restriction>
    <rdfs:subClassOf>
      <glview:MeasurementType rdf:about="http://schema.geolink.org/dev/voc/nvs/P02#DSCO">
        <rdfs:subClassOf rdf:resource="http://schema.geolink.org/dev/voc/nvs/P03#C045"/>
        <rdfs:seeAlso rdf:resource="http://vocab.nerc.ac.uk/collection/P02/current/DSCO/"/>
        <rdfs:comment xml:lang="en">Distribution coefficients of species between the dissolved and particulate phases of the water column</rdfs:comment>
        <rdfs:label xml:lang="en">Distribution coefficients in the water column</rdfs:label>
        <rdf:type rdf:resource="http://www.w3.org/2002/07/owl#NamedIndividual"/>
        <rdf:type rdf:resource="http://www.w3.org/2002/07/owl#Class"/>
      </glview:MeasurementType>
    </rdfs:subClassOf>
    <owl:someValuesFrom>
      <owl:Class>
        <owl:oneOf rdf:parseType="Collection">
          <glview:MeasurementType rdf:about="http://schema.geolink.org/dev/voc/nvs/P02#DSCO"/>
        </owl:oneOf>
      </owl:Class>
    </owl:someValuesFrom>
    <owl:onProperty rdf:resource="http://schema.geolink.org/dev/view#hasMeasurementType"/>
  </owl:Restriction>
  <owl:Restriction>
    <rdfs:subClassOf>
      <glview:MeasurementType rdf:about="http://schema.geolink.org/dev/voc/nvs/P02#MEPH">
        <rdfs:subClassOf rdf:resource="http://schema.geolink.org/dev/voc/nvs/P03#B045"/>
        <rdfs:seeAlso rdf:resource="http://vocab.nerc.ac.uk/collection/P02/current/MEPH/"/>
        <rdfs:comment></rdfs:comment>
        <rdfs:label xml:lang="en">Zooplankton egg hatch proportion</rdfs:label>
        <rdf:type rdf:resource="http://www.w3.org/2002/07/owl#NamedIndividual"/>
        <rdf:type rdf:resource="http://www.w3.org/2002/07/owl#Class"/>
      </glview:MeasurementType>
    </rdfs:subClassOf>
    <owl:someValuesFrom>
      <owl:Class>
        <owl:oneOf rdf:parseType="Collection">
          <glview:MeasurementType rdf:about="http://schema.geolink.org/dev/voc/nvs/P02#MEPH"/>
        </owl:oneOf>
      </owl:Class>
    </owl:someValuesFrom>
    <owl:onProperty rdf:resource="http://schema.geolink.org/dev/view#hasMeasurementType"/>
  </owl:Restriction>
  <owl:Restriction>
    <rdfs:subClassOf>
      <glview:MeasurementType rdf:about="http://schema.geolink.org/dev/voc/nvs/P02#PATX">
        <rdfs:subClassOf rdf:resource="http://schema.geolink.org/dev/voc/nvs/P03#B030"/>
        <rdfs:subClassOf rdf:resource="http://schema.geolink.org/dev/voc/nvs/P03#B070"/>
        <rdfs:seeAlso rdf:resource="http://vocab.nerc.ac.uk/collection/P02/current/PATX/"/>
        <rdfs:comment xml:lang="en">Any enumeration (e.g. count, abundance) of free-floating autotrophic biological entities designated by taxonomic names (e.g. species, genus, family) in any body of fresh or salt water.</rdfs:comment>
        <rdfs:label xml:lang="en">Phytoplankton taxonomic abundance in water bodies</rdfs:label>
        <rdf:type rdf:resource="http://www.w3.org/2002/07/owl#NamedIndividual"/>
        <rdf:type rdf:resource="http://www.w3.org/2002/07/owl#Class"/>
      </glview:MeasurementType>
    </rdfs:subClassOf>
    <owl:someValuesFrom>
      <owl:Class>
        <owl:oneOf rdf:parseType="Collection">
          <glview:MeasurementType rdf:about="http://schema.geolink.org/dev/voc/nvs/P02#PATX"/>
        </owl:oneOf>
      </owl:Class>
    </owl:someValuesFrom>
    <owl:onProperty rdf:resource="http://schema.geolink.org/dev/view#hasMeasurementType"/>
  </owl:Restriction>
  <owl:Restriction>
    <rdfs:subClassOf rdf:resource="http://schema.geolink.org/dev/voc/nvs/P02#PASR"/>
    <owl:someValuesFrom>
      <owl:Class>
        <owl:oneOf rdf:parseType="Collection">
          <glview:MeasurementType rdf:about="http://schema.geolink.org/dev/voc/nvs/P02#PASR"/>
        </owl:oneOf>
      </owl:Class>
    </owl:someValuesFrom>
    <owl:onProperty rdf:resource="http://schema.geolink.org/dev/view#hasMeasurementType"/>
  </owl:Restriction>
  <owl:Restriction>
    <rdfs:subClassOf>
      <glview:MeasurementType rdf:about="http://schema.geolink.org/dev/voc/nvs/P02#EPSI">
        <rdfs:subClassOf rdf:resource="http://schema.geolink.org/dev/voc/nvs/P03#D030"/>
        <rdfs:seeAlso rdf:resource="http://vocab.nerc.ac.uk/collection/P02/current/EPSI/"/>
        <rdfs:comment xml:lang="en">Measured parameters expressing turbulence in the water column plus parameters derived from these measurements</rdfs:comment>
        <rdfs:label xml:lang="en">Turbulence in the water column</rdfs:label>
        <rdf:type rdf:resource="http://www.w3.org/2002/07/owl#NamedIndividual"/>
        <rdf:type rdf:resource="http://www.w3.org/2002/07/owl#Class"/>
      </glview:MeasurementType>
    </rdfs:subClassOf>
    <owl:someValuesFrom>
      <owl:Class>
        <owl:oneOf rdf:parseType="Collection">
          <glview:MeasurementType rdf:about="http://schema.geolink.org/dev/voc/nvs/P02#EPSI"/>
        </owl:oneOf>
      </owl:Class>
    </owl:someValuesFrom>
    <owl:onProperty rdf:resource="http://schema.geolink.org/dev/view#hasMeasurementType"/>
  </owl:Restriction>
  <owl:Restriction>
    <rdfs:subClassOf>
      <glview:MeasurementType rdf:about="http://schema.geolink.org/dev/voc/nvs/P02#ZNTP">
        <rdfs:subClassOf rdf:resource="http://schema.geolink.org/dev/voc/nvs/P03#B045"/>
        <rdfs:subClassOf rdf:resource="http://schema.geolink.org/dev/voc/nvs/P03#B070"/>
        <rdfs:seeAlso rdf:resource="http://vocab.nerc.ac.uk/collection/P02/current/ZNTP/"/>
        <rdfs:comment xml:lang="en">Zooplankton (mesozooplankton plus larger pelagic animals excluding fish, reptiles and mammals) protein biomass per unit volume for entities that have not been identified by taxonomic name</rdfs:comment>
        <rdfs:label xml:lang="en">Zooplankton non taxonomy-related biomass expressed as protein per unit volume of the water column</rdfs:label>
        <rdf:type rdf:resource="http://www.w3.org/2002/07/owl#NamedIndividual"/>
        <rdf:type rdf:resource="http://www.w3.org/2002/07/owl#Class"/>
      </glview:MeasurementType>
    </rdfs:subClassOf>
    <owl:someValuesFrom>
      <owl:Class>
        <owl:oneOf rdf:parseType="Collection">
          <glview:MeasurementType rdf:about="http://schema.geolink.org/dev/voc/nvs/P02#ZNTP"/>
        </owl:oneOf>
      </owl:Class>
    </owl:someValuesFrom>
    <owl:onProperty rdf:resource="http://schema.geolink.org/dev/view#hasMeasurementType"/>
  </owl:Restriction>
  <owl:Restriction>
    <rdfs:subClassOf>
      <glview:MeasurementType rdf:about="http://schema.geolink.org/dev/voc/nvs/P02#ZNTC">
        <rdfs:subClassOf rdf:resource="http://schema.geolink.org/dev/voc/nvs/P03#B045"/>
        <rdfs:subClassOf rdf:resource="http://schema.geolink.org/dev/voc/nvs/P03#B070"/>
        <rdfs:seeAlso rdf:resource="http://vocab.nerc.ac.uk/collection/P02/current/ZNTC/"/>
        <rdfs:comment xml:lang="en">Zooplankton (mesozooplankton plus larger pelagic animals excluding fish, reptiles and mammals) carbon biomass per unit volume parameters not included in group ZCTC.  Usually used for generic names such as 'mesozooplankton'.</rdfs:comment>
        <rdfs:label xml:lang="en">Zooplankton non taxonomy-related biomass expressed as carbon per unit volume of the water column</rdfs:label>
        <rdf:type rdf:resource="http://www.w3.org/2002/07/owl#NamedIndividual"/>
        <rdf:type rdf:resource="http://www.w3.org/2002/07/owl#Class"/>
      </glview:MeasurementType>
    </rdfs:subClassOf>
    <owl:someValuesFrom>
      <owl:Class>
        <owl:oneOf rdf:parseType="Collection">
          <glview:MeasurementType rdf:about="http://schema.geolink.org/dev/voc/nvs/P02#ZNTC"/>
        </owl:oneOf>
      </owl:Class>
    </owl:someValuesFrom>
    <owl:onProperty rdf:resource="http://schema.geolink.org/dev/view#hasMeasurementType"/>
  </owl:Restriction>
  <owl:Restriction>
    <rdfs:subClassOf>
      <glview:MeasurementType rdf:about="http://schema.geolink.org/dev/voc/nvs/P02#ATPX">
        <rdfs:subClassOf rdf:resource="http://schema.geolink.org/dev/voc/nvs/P03#C050"/>
        <rdfs:seeAlso rdf:resource="http://vocab.nerc.ac.uk/collection/P02/current/ATPX/"/>
        <rdfs:comment xml:lang="en">Concentrations of adenylates (ADP, ATP etc) in all phases of the water column</rdfs:comment>
        <rdfs:label xml:lang="en">Concentration of adenlylates in the water column</rdfs:label>
        <rdf:type rdf:resource="http://www.w3.org/2002/07/owl#NamedIndividual"/>
        <rdf:type rdf:resource="http://www.w3.org/2002/07/owl#Class"/>
      </glview:MeasurementType>
    </rdfs:subClassOf>
    <owl:someValuesFrom>
      <owl:Class>
        <owl:oneOf rdf:parseType="Collection">
          <glview:MeasurementType rdf:about="http://schema.geolink.org/dev/voc/nvs/P02#ATPX"/>
        </owl:oneOf>
      </owl:Class>
    </owl:someValuesFrom>
    <owl:onProperty rdf:resource="http://schema.geolink.org/dev/view#hasMeasurementType"/>
  </owl:Restriction>
  <owl:Restriction>
    <rdfs:subClassOf>
      <owl:NamedIndividual rdf:about="http://schema.geolink.org/dev/voc/nvs/P02#ADUN">
        <rdfs:label xml:lang="en">Administrative units</rdfs:label>
        <rdfs:subClassOf rdf:resource="http://schema.geolink.org/dev/voc/nvs/P03#H002"/>
        <rdfs:subClassOf rdf:resource="http://schema.geolink.org/dev/voc/nvs/P03#B055"/>
        <rdfs:seeAlso rdf:resource="http://vocab.nerc.ac.uk/collection/P02/current/ADUN/"/>
        <rdfs:subClassOf rdf:resource="http://schema.geolink.org/dev/voc/nvs/P03#G055"/>
        <rdfs:subClassOf rdf:resource="http://schema.geolink.org/dev/voc/nvs/P03#H004"/>
        <rdfs:comment xml:lang="en">Parameters (including geometries, labels and categorizations) relating to areas where authorities have and-or excercise specific rights or obligations.</rdfs:comment>
        <rdfs:subClassOf rdf:resource="http://schema.geolink.org/dev/voc/nvs/P03#B050"/>
        <rdfs:subClassOf rdf:resource="http://schema.geolink.org/dev/voc/nvs/P03#B015"/>
        <rdf:type rdf:resource="http://schema.geolink.org/dev/view#MeasurementType"/>
        <rdfs:subClassOf rdf:resource="http://schema.geolink.org/dev/voc/nvs/P03#H005"/>
        <rdfs:subClassOf rdf:resource="http://schema.geolink.org/dev/voc/nvs/P03#B020"/>
        <rdf:type rdf:resource="http://www.w3.org/2002/07/owl#Class"/>
      </owl:NamedIndividual>
    </rdfs:subClassOf>
    <owl:someValuesFrom>
      <owl:Class>
        <owl:oneOf rdf:parseType="Collection">
          <owl:NamedIndividual rdf:about="http://schema.geolink.org/dev/voc/nvs/P02#ADUN"/>
        </owl:oneOf>
      </owl:Class>
    </owl:someValuesFrom>
    <owl:onProperty rdf:resource="http://schema.geolink.org/dev/view#hasMeasurementType"/>
  </owl:Restriction>
  <owl:Restriction>
    <rdfs:subClassOf rdf:resource="http://schema.geolink.org/dev/voc/nvs/P02#FBAF"/>
    <owl:someValuesFrom>
      <owl:Class>
        <owl:oneOf rdf:parseType="Collection">
          <glview:MeasurementType rdf:about="http://schema.geolink.org/dev/voc/nvs/P02#FBAF"/>
        </owl:oneOf>
      </owl:Class>
    </owl:someValuesFrom>
    <owl:onProperty rdf:resource="http://schema.geolink.org/dev/view#hasMeasurementType"/>
  </owl:Restriction>
  <owl:Restriction>
    <rdfs:subClassOf>
      <glview:MeasurementType rdf:about="http://schema.geolink.org/dev/voc/nvs/P02#IWAB">
        <rdfs:subClassOf rdf:resource="http://schema.geolink.org/dev/voc/nvs/P03#B070"/>
        <rdfs:subClassOf rdf:resource="http://schema.geolink.org/dev/voc/nvs/P03#G055"/>
        <rdfs:seeAlso rdf:resource="http://vocab.nerc.ac.uk/collection/P02/current/IWAB/"/>
        <rdfs:comment xml:lang="en">Insect (Class Insecta) and earthworm (Subclass Oligochaeta) abundance per unit area of bed (sea, river, lake etc.) parameters presented at the level of taxa that may be mapped to entities in the ITIS taxonomy.  Includes animals normally considered as planktonic if they have been returned from sediment samples. This parameter group has been implemented to separate predominantly freshwater taxa from predominantly marine taxa.</rdfs:comment>
        <rdfs:label xml:lang="en">Insect and earthworm taxonomy-related abundance per unit area of the bed</rdfs:label>
        <rdf:type rdf:resource="http://www.w3.org/2002/07/owl#NamedIndividual"/>
        <rdf:type rdf:resource="http://www.w3.org/2002/07/owl#Class"/>
      </glview:MeasurementType>
    </rdfs:subClassOf>
    <owl:someValuesFrom>
      <owl:Class>
        <owl:oneOf rdf:parseType="Collection">
          <glview:MeasurementType rdf:about="http://schema.geolink.org/dev/voc/nvs/P02#IWAB"/>
        </owl:oneOf>
      </owl:Class>
    </owl:someValuesFrom>
    <owl:onProperty rdf:resource="http://schema.geolink.org/dev/view#hasMeasurementType"/>
  </owl:Restriction>
  <owl:Restriction>
    <rdfs:subClassOf rdf:resource="http://schema.geolink.org/dev/voc/nvs/P02#SDAC"/>
    <owl:someValuesFrom>
      <owl:Class>
        <owl:oneOf rdf:parseType="Collection">
          <glview:MeasurementType rdf:about="http://schema.geolink.org/dev/voc/nvs/P02#SDAC"/>
        </owl:oneOf>
      </owl:Class>
    </owl:someValuesFrom>
    <owl:onProperty rdf:resource="http://schema.geolink.org/dev/view#hasMeasurementType"/>
  </owl:Restriction>
  <owl:Restriction>
    <rdfs:subClassOf>
      <glview:MeasurementType rdf:about="http://schema.geolink.org/dev/voc/nvs/P02#OMBI">
        <rdfs:subClassOf rdf:resource="http://schema.geolink.org/dev/voc/nvs/P03#C050"/>
        <rdfs:label xml:lang="en">Organometallic species concentration parameters in biota</rdfs:label>
        <rdfs:seeAlso rdf:resource="http://vocab.nerc.ac.uk/collection/P02/current/OMBI/"/>
        <rdfs:subClassOf rdf:resource="http://schema.geolink.org/dev/voc/nvs/P03#H001"/>
        <rdfs:subClassOf rdf:resource="http://schema.geolink.org/dev/voc/nvs/P03#B007"/>
        <rdfs:subClassOf rdf:resource="http://schema.geolink.org/dev/voc/nvs/P03#C055"/>
        <rdf:type rdf:resource="http://www.w3.org/2002/07/owl#Class"/>
        <rdfs:comment xml:lang="en">All measurements of the quantity or mass of any organometallic compound in any living organisms or their component parts</rdfs:comment>
        <rdfs:subClassOf rdf:resource="http://schema.geolink.org/dev/voc/nvs/P03#C035"/>
        <rdf:type rdf:resource="http://www.w3.org/2002/07/owl#NamedIndividual"/>
      </glview:MeasurementType>
    </rdfs:subClassOf>
    <owl:someValuesFrom>
      <owl:Class>
        <owl:oneOf rdf:parseType="Collection">
          <glview:MeasurementType rdf:about="http://schema.geolink.org/dev/voc/nvs/P02#OMBI"/>
        </owl:oneOf>
      </owl:Class>
    </owl:someValuesFrom>
    <owl:onProperty rdf:resource="http://schema.geolink.org/dev/view#hasMeasurementType"/>
  </owl:Restriction>
  <owl:Restriction>
    <rdfs:subClassOf>
      <glview:MeasurementType rdf:about="http://schema.geolink.org/dev/voc/nvs/P02#GOXP">
        <rdfs:subClassOf rdf:resource="http://schema.geolink.org/dev/voc/nvs/P03#O010"/>
        <rdfs:seeAlso rdf:resource="http://vocab.nerc.ac.uk/collection/P02/current/GOXP/"/>
        <rdfs:comment xml:lang="en">Parameters related to the rates of oxygen production and consumption</rdfs:comment>
        <rdfs:label xml:lang="en">Oxygen production and respiration in the water column</rdfs:label>
        <rdf:type rdf:resource="http://www.w3.org/2002/07/owl#NamedIndividual"/>
        <rdf:type rdf:resource="http://www.w3.org/2002/07/owl#Class"/>
      </glview:MeasurementType>
    </rdfs:subClassOf>
    <owl:someValuesFrom>
      <owl:Class>
        <owl:oneOf rdf:parseType="Collection">
          <glview:MeasurementType rdf:about="http://schema.geolink.org/dev/voc/nvs/P02#GOXP"/>
        </owl:oneOf>
      </owl:Class>
    </owl:someValuesFrom>
    <owl:onProperty rdf:resource="http://schema.geolink.org/dev/view#hasMeasurementType"/>
  </owl:Restriction>
  <owl:Restriction>
    <rdfs:subClassOf>
      <glview:MeasurementType rdf:about="http://schema.geolink.org/dev/voc/nvs/P02#SEBH">
        <rdfs:subClassOf rdf:resource="http://schema.geolink.org/dev/voc/nvs/P03#B015"/>
        <rdfs:seeAlso rdf:resource="http://vocab.nerc.ac.uk/collection/P02/current/SEBH/"/>
        <rdfs:comment xml:lang="en">Parameters describing the actions or reactions of seals (Family Phocidae), usually in response to the environment. Includes both parameters mapped to taxa and those mapped to non-taxonomic groupings.</rdfs:comment>
        <rdfs:label xml:lang="en">Seal behaviour</rdfs:label>
        <rdf:type rdf:resource="http://www.w3.org/2002/07/owl#NamedIndividual"/>
        <rdf:type rdf:resource="http://www.w3.org/2002/07/owl#Class"/>
      </glview:MeasurementType>
    </rdfs:subClassOf>
    <owl:someValuesFrom>
      <owl:Class>
        <owl:oneOf rdf:parseType="Collection">
          <glview:MeasurementType rdf:about="http://schema.geolink.org/dev/voc/nvs/P02#SEBH"/>
        </owl:oneOf>
      </owl:Class>
    </owl:someValuesFrom>
    <owl:onProperty rdf:resource="http://schema.geolink.org/dev/view#hasMeasurementType"/>
  </owl:Restriction>
  <owl:Restriction>
    <rdfs:subClassOf>
      <glview:MeasurementType rdf:about="http://schema.geolink.org/dev/voc/nvs/P02#PCFX">
        <rdfs:subClassOf rdf:resource="http://schema.geolink.org/dev/voc/nvs/P03#B027"/>
        <rdfs:subClassOf rdf:resource="http://schema.geolink.org/dev/voc/nvs/P03#O005"/>
        <rdfs:seeAlso rdf:resource="http://vocab.nerc.ac.uk/collection/P02/current/PCFX/"/>
        <rdfs:comment xml:lang="en">Fluxes of any biota or remains thereof (excluding faecal pellets which are classed as SPM) downwards through the water column</rdfs:comment>
        <rdfs:label xml:lang="en">Sedimentation flux of identified biota expressed as carbon in the water column</rdfs:label>
        <rdf:type rdf:resource="http://www.w3.org/2002/07/owl#NamedIndividual"/>
        <rdf:type rdf:resource="http://www.w3.org/2002/07/owl#Class"/>
      </glview:MeasurementType>
    </rdfs:subClassOf>
    <owl:someValuesFrom>
      <owl:Class>
        <owl:oneOf rdf:parseType="Collection">
          <glview:MeasurementType rdf:about="http://schema.geolink.org/dev/voc/nvs/P02#PCFX"/>
        </owl:oneOf>
      </owl:Class>
    </owl:someValuesFrom>
    <owl:onProperty rdf:resource="http://schema.geolink.org/dev/view#hasMeasurementType"/>
  </owl:Restriction>
  <owl:Restriction>
    <rdfs:subClassOf>
      <glview:MeasurementType rdf:about="http://schema.geolink.org/dev/voc/nvs/P02#SPHT">
        <rdfs:subClassOf rdf:resource="http://schema.geolink.org/dev/voc/nvs/P03#C045"/>
        <rdfs:seeAlso rdf:resource="http://vocab.nerc.ac.uk/collection/P02/current/SPHT/"/>
        <rdfs:comment xml:lang="en">Concentration parameters (including saturation if gaseous) for inorganic sulphur species in all phases of sediment pore waters</rdfs:comment>
        <rdfs:label xml:lang="en">Concentration of inorganic sulphur species in sediment pore water</rdfs:label>
        <rdf:type rdf:resource="http://www.w3.org/2002/07/owl#NamedIndividual"/>
        <rdf:type rdf:resource="http://www.w3.org/2002/07/owl#Class"/>
      </glview:MeasurementType>
    </rdfs:subClassOf>
    <owl:someValuesFrom>
      <owl:Class>
        <owl:oneOf rdf:parseType="Collection">
          <glview:MeasurementType rdf:about="http://schema.geolink.org/dev/voc/nvs/P02#SPHT"/>
        </owl:oneOf>
      </owl:Class>
    </owl:someValuesFrom>
    <owl:onProperty rdf:resource="http://schema.geolink.org/dev/view#hasMeasurementType"/>
  </owl:Restriction>
  <owl:Restriction>
    <rdfs:subClassOf>
      <glview:MeasurementType rdf:about="http://schema.geolink.org/dev/voc/nvs/P02#MDPW">
        <rdfs:subClassOf rdf:resource="http://schema.geolink.org/dev/voc/nvs/P03#G050"/>
        <rdfs:subClassOf rdf:resource="http://schema.geolink.org/dev/voc/nvs/P03#C035"/>
        <rdfs:seeAlso rdf:resource="http://vocab.nerc.ac.uk/collection/P02/current/MDPW/"/>
        <rdfs:comment xml:lang="en">Concentration parameters for trace metalloid elements in water occupying the space between sediment grains. Trace metalloids are considered as B, Ge, As, Sb, Te and Po (but not Si which is classed separately because of its major role in environmental chemistry)</rdfs:comment>
        <rdfs:label xml:lang="en">Trace metalloid concentrations in sediment pore water</rdfs:label>
        <rdf:type rdf:resource="http://www.w3.org/2002/07/owl#NamedIndividual"/>
        <rdf:type rdf:resource="http://www.w3.org/2002/07/owl#Class"/>
      </glview:MeasurementType>
    </rdfs:subClassOf>
    <owl:someValuesFrom>
      <owl:Class>
        <owl:oneOf rdf:parseType="Collection">
          <glview:MeasurementType rdf:about="http://schema.geolink.org/dev/voc/nvs/P02#MDPW"/>
        </owl:oneOf>
      </owl:Class>
    </owl:someValuesFrom>
    <owl:onProperty rdf:resource="http://schema.geolink.org/dev/view#hasMeasurementType"/>
  </owl:Restriction>
  <owl:Restriction>
    <rdfs:subClassOf>
      <glview:MeasurementType rdf:about="http://schema.geolink.org/dev/voc/nvs/P02#FDMS">
        <rdfs:subClassOf rdf:resource="http://schema.geolink.org/dev/voc/nvs/P03#M005"/>
        <rdfs:subClassOf rdf:resource="http://schema.geolink.org/dev/voc/nvs/P03#O005"/>
        <rdfs:seeAlso rdf:resource="http://vocab.nerc.ac.uk/collection/P02/current/FDMS/"/>
        <rdfs:comment xml:lang="en">Fluxes of any gaseous species from water column to atmosphere</rdfs:comment>
        <rdfs:label xml:lang="en">Gas fluxes between the water column and the atmosphere</rdfs:label>
        <rdf:type rdf:resource="http://www.w3.org/2002/07/owl#NamedIndividual"/>
        <rdf:type rdf:resource="http://www.w3.org/2002/07/owl#Class"/>
      </glview:MeasurementType>
    </rdfs:subClassOf>
    <owl:someValuesFrom>
      <owl:Class>
        <owl:oneOf rdf:parseType="Collection">
          <glview:MeasurementType rdf:about="http://schema.geolink.org/dev/voc/nvs/P02#FDMS"/>
        </owl:oneOf>
      </owl:Class>
    </owl:someValuesFrom>
    <owl:onProperty rdf:resource="http://schema.geolink.org/dev/view#hasMeasurementType"/>
  </owl:Restriction>
  <owl:Restriction>
    <rdfs:subClassOf>
      <glview:MeasurementType rdf:about="http://schema.geolink.org/dev/voc/nvs/P02#BRAD">
        <rdfs:subClassOf rdf:resource="http://schema.geolink.org/dev/voc/nvs/P03#C030"/>
        <rdfs:subClassOf rdf:resource="http://schema.geolink.org/dev/voc/nvs/P03#B007"/>
        <rdfs:seeAlso rdf:resource="http://vocab.nerc.ac.uk/collection/P02/current/BRAD/"/>
        <rdfs:comment xml:lang="en">All parameters associated with radioactivity in either whole organisms or their constituent parts</rdfs:comment>
        <rdfs:label xml:lang="en">Radioactivity in biota</rdfs:label>
        <rdf:type rdf:resource="http://www.w3.org/2002/07/owl#NamedIndividual"/>
        <rdf:type rdf:resource="http://www.w3.org/2002/07/owl#Class"/>
      </glview:MeasurementType>
    </rdfs:subClassOf>
    <owl:someValuesFrom>
      <owl:Class>
        <owl:oneOf rdf:parseType="Collection">
          <glview:MeasurementType rdf:about="http://schema.geolink.org/dev/voc/nvs/P02#BRAD"/>
        </owl:oneOf>
      </owl:Class>
    </owl:someValuesFrom>
    <owl:onProperty rdf:resource="http://schema.geolink.org/dev/view#hasMeasurementType"/>
  </owl:Restriction>
  <owl:Restriction>
    <rdfs:subClassOf>
      <glview:MeasurementType rdf:about="http://schema.geolink.org/dev/voc/nvs/P02#ZNTN">
        <rdfs:subClassOf rdf:resource="http://schema.geolink.org/dev/voc/nvs/P03#B045"/>
        <rdfs:subClassOf rdf:resource="http://schema.geolink.org/dev/voc/nvs/P03#B070"/>
        <rdfs:seeAlso rdf:resource="http://vocab.nerc.ac.uk/collection/P02/current/ZNTN/"/>
        <rdfs:comment xml:lang="en">Zooplankton (mesozooplankton plus larger pelagic animals excluding fish, reptiles and mammals) nitrogen biomass per unit volume parameters not included in group ZCTC.  Usually used for generic names such as 'mesozooplankton'.</rdfs:comment>
        <rdfs:label xml:lang="en">Zooplankton non taxonomy-related biomass expressed as nitrogen per unit volume of the water column</rdfs:label>
        <rdf:type rdf:resource="http://www.w3.org/2002/07/owl#NamedIndividual"/>
        <rdf:type rdf:resource="http://www.w3.org/2002/07/owl#Class"/>
      </glview:MeasurementType>
    </rdfs:subClassOf>
    <owl:someValuesFrom>
      <owl:Class>
        <owl:oneOf rdf:parseType="Collection">
          <glview:MeasurementType rdf:about="http://schema.geolink.org/dev/voc/nvs/P02#ZNTN"/>
        </owl:oneOf>
      </owl:Class>
    </owl:someValuesFrom>
    <owl:onProperty rdf:resource="http://schema.geolink.org/dev/view#hasMeasurementType"/>
  </owl:Restriction>
  <owl:Restriction>
    <rdfs:subClassOf rdf:resource="http://schema.geolink.org/dev/voc/nvs/P02#OMBI"/>
    <owl:someValuesFrom>
      <owl:Class>
        <owl:oneOf rdf:parseType="Collection">
          <glview:MeasurementType rdf:about="http://schema.geolink.org/dev/voc/nvs/P02#OMBI"/>
        </owl:oneOf>
      </owl:Class>
    </owl:someValuesFrom>
    <owl:onProperty rdf:resource="http://schema.geolink.org/dev/view#hasMeasurementType"/>
  </owl:Restriction>
  <owl:Restriction>
    <rdfs:subClassOf rdf:resource="http://schema.geolink.org/dev/voc/nvs/P02#ADUN"/>
    <owl:someValuesFrom>
      <owl:Class>
        <owl:oneOf rdf:parseType="Collection">
          <owl:NamedIndividual rdf:about="http://schema.geolink.org/dev/voc/nvs/P02#ADUN"/>
        </owl:oneOf>
      </owl:Class>
    </owl:someValuesFrom>
    <owl:onProperty rdf:resource="http://schema.geolink.org/dev/view#hasMeasurementType"/>
  </owl:Restriction>
  <owl:Restriction>
    <rdfs:subClassOf rdf:resource="http://schema.geolink.org/dev/voc/nvs/P02#PCOC"/>
    <owl:someValuesFrom>
      <owl:Class>
        <owl:oneOf rdf:parseType="Collection">
          <glview:MeasurementType rdf:about="http://schema.geolink.org/dev/voc/nvs/P02#PCOC"/>
        </owl:oneOf>
      </owl:Class>
    </owl:someValuesFrom>
    <owl:onProperty rdf:resource="http://schema.geolink.org/dev/view#hasMeasurementType"/>
  </owl:Restriction>
  <owl:Restriction>
    <rdfs:subClassOf rdf:resource="http://schema.geolink.org/dev/voc/nvs/P02#FCRT"/>
    <owl:someValuesFrom>
      <owl:Class>
        <owl:oneOf rdf:parseType="Collection">
          <glview:MeasurementType rdf:about="http://schema.geolink.org/dev/voc/nvs/P02#FCRT"/>
        </owl:oneOf>
      </owl:Class>
    </owl:someValuesFrom>
    <owl:onProperty rdf:resource="http://schema.geolink.org/dev/view#hasMeasurementType"/>
  </owl:Restriction>
  <owl:Restriction>
    <rdfs:subClassOf rdf:resource="http://schema.geolink.org/dev/voc/nvs/P02#FBAF"/>
    <owl:someValuesFrom>
      <owl:Class>
        <owl:oneOf rdf:parseType="Collection">
          <glview:MeasurementType rdf:about="http://schema.geolink.org/dev/voc/nvs/P02#FBAF"/>
        </owl:oneOf>
      </owl:Class>
    </owl:someValuesFrom>
    <owl:onProperty rdf:resource="http://schema.geolink.org/dev/view#hasMeasurementType"/>
  </owl:Restriction>
  <owl:Restriction>
    <rdfs:subClassOf>
      <glview:MeasurementType rdf:about="http://schema.geolink.org/dev/voc/nvs/P02#BATX">
        <rdfs:subClassOf rdf:resource="http://schema.geolink.org/dev/voc/nvs/P03#B070"/>
        <rdfs:subClassOf rdf:resource="http://schema.geolink.org/dev/voc/nvs/P03#B005"/>
        <rdfs:seeAlso rdf:resource="http://vocab.nerc.ac.uk/collection/P02/current/BATX/"/>
        <rdfs:comment xml:lang="en">Any enumeration of bacteria (Kingdom Monera so includes cyanobacteria) designated by taxonomic names (e.g. species, genus, family) in any body of fresh or salt water.</rdfs:comment>
        <rdfs:label xml:lang="en">Bacteria taxonomic abundance in water bodies</rdfs:label>
        <rdf:type rdf:resource="http://www.w3.org/2002/07/owl#NamedIndividual"/>
        <rdf:type rdf:resource="http://www.w3.org/2002/07/owl#Class"/>
      </glview:MeasurementType>
    </rdfs:subClassOf>
    <owl:someValuesFrom>
      <owl:Class>
        <owl:oneOf rdf:parseType="Collection">
          <glview:MeasurementType rdf:about="http://schema.geolink.org/dev/voc/nvs/P02#BATX"/>
        </owl:oneOf>
      </owl:Class>
    </owl:someValuesFrom>
    <owl:onProperty rdf:resource="http://schema.geolink.org/dev/view#hasMeasurementType"/>
  </owl:Restriction>
  <owl:Restriction>
    <rdfs:subClassOf>
      <glview:MeasurementType rdf:about="http://schema.geolink.org/dev/voc/nvs/P02#GP004">
        <rdfs:subClassOf rdf:resource="http://schema.geolink.org/dev/voc/nvs/P03#B015"/>
        <rdfs:seeAlso rdf:resource="http://vocab.nerc.ac.uk/collection/P02/current/GP004/"/>
        <rdfs:comment xml:lang="en">Parameters related to the reproduction of birds (Class Aves)</rdfs:comment>
        <rdfs:label xml:lang="en">Bird reproduction</rdfs:label>
        <rdf:type rdf:resource="http://www.w3.org/2002/07/owl#NamedIndividual"/>
        <rdf:type rdf:resource="http://www.w3.org/2002/07/owl#Class"/>
      </glview:MeasurementType>
    </rdfs:subClassOf>
    <owl:someValuesFrom>
      <owl:Class>
        <owl:oneOf rdf:parseType="Collection">
          <glview:MeasurementType rdf:about="http://schema.geolink.org/dev/voc/nvs/P02#GP004"/>
        </owl:oneOf>
      </owl:Class>
    </owl:someValuesFrom>
    <owl:onProperty rdf:resource="http://schema.geolink.org/dev/view#hasMeasurementType"/>
  </owl:Restriction>
  <owl:Restriction>
    <rdfs:subClassOf rdf:resource="http://schema.geolink.org/dev/voc/nvs/P02#ADUN"/>
    <owl:someValuesFrom>
      <owl:Class>
        <owl:oneOf rdf:parseType="Collection">
          <owl:NamedIndividual rdf:about="http://schema.geolink.org/dev/voc/nvs/P02#ADUN"/>
        </owl:oneOf>
      </owl:Class>
    </owl:someValuesFrom>
    <owl:onProperty rdf:resource="http://schema.geolink.org/dev/view#hasMeasurementType"/>
  </owl:Restriction>
  <owl:Restriction>
    <rdfs:subClassOf>
      <glview:MeasurementType rdf:about="http://schema.geolink.org/dev/voc/nvs/P02#NTPW">
        <rdfs:subClassOf rdf:resource="http://schema.geolink.org/dev/voc/nvs/P03#G050"/>
        <rdfs:subClassOf rdf:resource="http://schema.geolink.org/dev/voc/nvs/P03#C040"/>
        <rdfs:seeAlso rdf:resource="http://vocab.nerc.ac.uk/collection/P02/current/NTPW/"/>
        <rdfs:comment xml:lang="en">Nutrient (nitrate, nitrite, ammonium, phosphate, silicate and urea) concentrations in sediment pore waters</rdfs:comment>
        <rdfs:label xml:lang="en">Nutrient concentrations in sediment pore waters</rdfs:label>
        <rdf:type rdf:resource="http://www.w3.org/2002/07/owl#NamedIndividual"/>
        <rdf:type rdf:resource="http://www.w3.org/2002/07/owl#Class"/>
      </glview:MeasurementType>
    </rdfs:subClassOf>
    <owl:someValuesFrom>
      <owl:Class>
        <owl:oneOf rdf:parseType="Collection">
          <glview:MeasurementType rdf:about="http://schema.geolink.org/dev/voc/nvs/P02#NTPW"/>
        </owl:oneOf>
      </owl:Class>
    </owl:someValuesFrom>
    <owl:onProperty rdf:resource="http://schema.geolink.org/dev/view#hasMeasurementType"/>
  </owl:Restriction>
  <owl:Restriction>
    <rdfs:subClassOf rdf:resource="http://schema.geolink.org/dev/voc/nvs/P02#OMBI"/>
    <owl:someValuesFrom>
      <owl:Class>
        <owl:oneOf rdf:parseType="Collection">
          <glview:MeasurementType rdf:about="http://schema.geolink.org/dev/voc/nvs/P02#OMBI"/>
        </owl:oneOf>
      </owl:Class>
    </owl:someValuesFrom>
    <owl:onProperty rdf:resource="http://schema.geolink.org/dev/view#hasMeasurementType"/>
  </owl:Restriction>
  <owl:Restriction>
    <rdfs:subClassOf rdf:resource="http://schema.geolink.org/dev/voc/nvs/P02#BRAD"/>
    <owl:someValuesFrom>
      <owl:Class>
        <owl:oneOf rdf:parseType="Collection">
          <glview:MeasurementType rdf:about="http://schema.geolink.org/dev/voc/nvs/P02#BRAD"/>
        </owl:oneOf>
      </owl:Class>
    </owl:someValuesFrom>
    <owl:onProperty rdf:resource="http://schema.geolink.org/dev/view#hasMeasurementType"/>
  </owl:Restriction>
  <owl:Restriction>
    <rdfs:subClassOf rdf:resource="http://schema.geolink.org/dev/voc/nvs/P02#MDPW"/>
    <owl:someValuesFrom>
      <owl:Class>
        <owl:oneOf rdf:parseType="Collection">
          <glview:MeasurementType rdf:about="http://schema.geolink.org/dev/voc/nvs/P02#MDPW"/>
        </owl:oneOf>
      </owl:Class>
    </owl:someValuesFrom>
    <owl:onProperty rdf:resource="http://schema.geolink.org/dev/view#hasMeasurementType"/>
  </owl:Restriction>
  <owl:Restriction>
    <rdfs:subClassOf>
      <glview:MeasurementType rdf:about="http://schema.geolink.org/dev/voc/nvs/P02#CFTM">
        <rdfs:subClassOf rdf:resource="http://schema.geolink.org/dev/voc/nvs/P03#H001"/>
        <rdfs:subClassOf rdf:resource="http://schema.geolink.org/dev/voc/nvs/P03#O005"/>
        <rdfs:seeAlso rdf:resource="http://vocab.nerc.ac.uk/collection/P02/current/CFTM/"/>
        <rdfs:comment xml:lang="en">Parameters quanitifying the transfer of substances considered harmful from land to sea, including river discharge rates of contaminant species (but not freshwater discharge rates).</rdfs:comment>
        <rdfs:label xml:lang="en">Contaminant fluxes between the terrestrial and marine environment</rdfs:label>
        <rdf:type rdf:resource="http://www.w3.org/2002/07/owl#NamedIndividual"/>
        <rdf:type rdf:resource="http://www.w3.org/2002/07/owl#Class"/>
      </glview:MeasurementType>
    </rdfs:subClassOf>
    <owl:someValuesFrom>
      <owl:Class>
        <owl:oneOf rdf:parseType="Collection">
          <glview:MeasurementType rdf:about="http://schema.geolink.org/dev/voc/nvs/P02#CFTM"/>
        </owl:oneOf>
      </owl:Class>
    </owl:someValuesFrom>
    <owl:onProperty rdf:resource="http://schema.geolink.org/dev/view#hasMeasurementType"/>
  </owl:Restriction>
  <owl:Restriction>
    <rdfs:subClassOf>
      <glview:MeasurementType rdf:about="http://schema.geolink.org/dev/voc/nvs/P02#LITH">
        <rdfs:subClassOf rdf:resource="http://schema.geolink.org/dev/voc/nvs/P03#G045"/>
        <rdfs:seeAlso rdf:resource="http://vocab.nerc.ac.uk/collection/P02/current/LITH/"/>
        <rdfs:comment xml:lang="en">Parameters describing rocks on the basis of physical characteristics such as colour, structure, mineralogy and grain size</rdfs:comment>
        <rdfs:label xml:lang="en">Lithology</rdfs:label>
        <rdf:type rdf:resource="http://www.w3.org/2002/07/owl#NamedIndividual"/>
        <rdf:type rdf:resource="http://www.w3.org/2002/07/owl#Class"/>
      </glview:MeasurementType>
    </rdfs:subClassOf>
    <owl:someValuesFrom>
      <owl:Class>
        <owl:oneOf rdf:parseType="Collection">
          <glview:MeasurementType rdf:about="http://schema.geolink.org/dev/voc/nvs/P02#LITH"/>
        </owl:oneOf>
      </owl:Class>
    </owl:someValuesFrom>
    <owl:onProperty rdf:resource="http://schema.geolink.org/dev/view#hasMeasurementType"/>
  </owl:Restriction>
  <owl:Restriction>
    <rdfs:subClassOf rdf:resource="http://schema.geolink.org/dev/voc/nvs/P02#ZNTN"/>
    <owl:someValuesFrom>
      <owl:Class>
        <owl:oneOf rdf:parseType="Collection">
          <glview:MeasurementType rdf:about="http://schema.geolink.org/dev/voc/nvs/P02#ZNTN"/>
        </owl:oneOf>
      </owl:Class>
    </owl:someValuesFrom>
    <owl:onProperty rdf:resource="http://schema.geolink.org/dev/view#hasMeasurementType"/>
  </owl:Restriction>
  <owl:Restriction>
    <rdfs:subClassOf>
      <glview:MeasurementType rdf:about="http://schema.geolink.org/dev/voc/nvs/P02#ATEM">
        <rdfs:subClassOf rdf:resource="http://schema.geolink.org/dev/voc/nvs/P03#H001"/>
        <rdfs:subClassOf rdf:resource="http://schema.geolink.org/dev/voc/nvs/P03#O005"/>
        <rdfs:seeAlso rdf:resource="http://vocab.nerc.ac.uk/collection/P02/current/ATEM/"/>
        <rdfs:comment xml:lang="en">Parameters quantifying and describing the release of substances into the atmosphere as a result of human activity</rdfs:comment>
        <rdfs:label xml:lang="en">Atmospheric emissions</rdfs:label>
        <rdf:type rdf:resource="http://www.w3.org/2002/07/owl#NamedIndividual"/>
        <rdf:type rdf:resource="http://www.w3.org/2002/07/owl#Class"/>
      </glview:MeasurementType>
    </rdfs:subClassOf>
    <owl:someValuesFrom>
      <owl:Class>
        <owl:oneOf rdf:parseType="Collection">
          <glview:MeasurementType rdf:about="http://schema.geolink.org/dev/voc/nvs/P02#ATEM"/>
        </owl:oneOf>
      </owl:Class>
    </owl:someValuesFrom>
    <owl:onProperty rdf:resource="http://schema.geolink.org/dev/view#hasMeasurementType"/>
  </owl:Restriction>
  <owl:Restriction>
    <rdfs:subClassOf>
      <glview:MeasurementType rdf:about="http://schema.geolink.org/dev/voc/nvs/P02#ZCTN">
        <rdfs:subClassOf rdf:resource="http://schema.geolink.org/dev/voc/nvs/P03#B045"/>
        <rdfs:subClassOf rdf:resource="http://schema.geolink.org/dev/voc/nvs/P03#B070"/>
        <rdfs:seeAlso rdf:resource="http://vocab.nerc.ac.uk/collection/P02/current/ZCTN/"/>
        <rdfs:comment xml:lang="en">Zooplankton (mesozooplankton plus larger pelagic animals excluding fish, reptiles and mammals) nitrogen biomass parameters presented at the level of taxa that may be mapped to entities in the ITIS taxonomy.  These may be at any taxonomic level from sub-species upwards.</rdfs:comment>
        <rdfs:label xml:lang="en">Zooplankton taxonomy-related biomass expressed as nitrogen per unit volume of the water column</rdfs:label>
        <rdf:type rdf:resource="http://www.w3.org/2002/07/owl#NamedIndividual"/>
        <rdf:type rdf:resource="http://www.w3.org/2002/07/owl#Class"/>
      </glview:MeasurementType>
    </rdfs:subClassOf>
    <owl:someValuesFrom>
      <owl:Class>
        <owl:oneOf rdf:parseType="Collection">
          <glview:MeasurementType rdf:about="http://schema.geolink.org/dev/voc/nvs/P02#ZCTN"/>
        </owl:oneOf>
      </owl:Class>
    </owl:someValuesFrom>
    <owl:onProperty rdf:resource="http://schema.geolink.org/dev/view#hasMeasurementType"/>
  </owl:Restriction>
  <owl:Restriction>
    <rdfs:subClassOf>
      <glview:MeasurementType rdf:about="http://schema.geolink.org/dev/voc/nvs/P02#WCTR">
        <rdfs:subClassOf rdf:resource="http://schema.geolink.org/dev/voc/nvs/P03#D020"/>
        <rdfs:seeAlso rdf:resource="http://vocab.nerc.ac.uk/collection/P02/current/WCTR/"/>
        <rdfs:comment xml:lang="en">Parameters describing the amount in a sample of a tracer (rhodamine, SF6, 3He, etc.) that has been purposely released into  a water body to track water mass movements or quantify exchanges with the atmosphere.</rdfs:comment>
        <rdfs:label xml:lang="en">Water body released tracers</rdfs:label>
        <rdf:type rdf:resource="http://www.w3.org/2002/07/owl#NamedIndividual"/>
        <rdf:type rdf:resource="http://www.w3.org/2002/07/owl#Class"/>
      </glview:MeasurementType>
    </rdfs:subClassOf>
    <owl:someValuesFrom>
      <owl:Class>
        <owl:oneOf rdf:parseType="Collection">
          <glview:MeasurementType rdf:about="http://schema.geolink.org/dev/voc/nvs/P02#WCTR"/>
        </owl:oneOf>
      </owl:Class>
    </owl:someValuesFrom>
    <owl:onProperty rdf:resource="http://schema.geolink.org/dev/view#hasMeasurementType"/>
  </owl:Restriction>
  <owl:Restriction>
    <rdfs:subClassOf>
      <glview:MeasurementType rdf:about="http://schema.geolink.org/dev/voc/nvs/P02#HEAV">
        <rdfs:subClassOf rdf:resource="http://schema.geolink.org/dev/voc/nvs/P03#D034"/>
        <rdfs:seeAlso rdf:resource="http://vocab.nerc.ac.uk/collection/P02/current/HEAV/"/>
        <rdfs:comment xml:lang="en">Measurements of wave height that are not based on the statistical analysis of wave records, such as heave, surface roughness and visual height estimates</rdfs:comment>
        <rdfs:label xml:lang="en">Wave height estimates</rdfs:label>
        <rdf:type rdf:resource="http://www.w3.org/2002/07/owl#NamedIndividual"/>
        <rdf:type rdf:resource="http://www.w3.org/2002/07/owl#Class"/>
      </glview:MeasurementType>
    </rdfs:subClassOf>
    <owl:someValuesFrom>
      <owl:Class>
        <owl:oneOf rdf:parseType="Collection">
          <glview:MeasurementType rdf:about="http://schema.geolink.org/dev/voc/nvs/P02#HEAV"/>
        </owl:oneOf>
      </owl:Class>
    </owl:someValuesFrom>
    <owl:onProperty rdf:resource="http://schema.geolink.org/dev/view#hasMeasurementType"/>
  </owl:Restriction>
  <owl:Restriction>
    <rdfs:subClassOf>
      <glview:MeasurementType rdf:about="http://schema.geolink.org/dev/voc/nvs/P02#MTAT">
        <rdfs:subClassOf rdf:resource="http://schema.geolink.org/dev/voc/nvs/P03#C035"/>
        <rdfs:subClassOf rdf:resource="http://schema.geolink.org/dev/voc/nvs/P03#M005"/>
        <rdfs:seeAlso rdf:resource="http://vocab.nerc.ac.uk/collection/P02/current/MTAT/"/>
        <rdfs:comment xml:lang="en">Concentration of metal elements in any phase of the atmosphere</rdfs:comment>
        <rdfs:label xml:lang="en">Metal concentrations in the atmosphere</rdfs:label>
        <rdf:type rdf:resource="http://www.w3.org/2002/07/owl#NamedIndividual"/>
        <rdf:type rdf:resource="http://www.w3.org/2002/07/owl#Class"/>
      </glview:MeasurementType>
    </rdfs:subClassOf>
    <owl:someValuesFrom>
      <owl:Class>
        <owl:oneOf rdf:parseType="Collection">
          <glview:MeasurementType rdf:about="http://schema.geolink.org/dev/voc/nvs/P02#MTAT"/>
        </owl:oneOf>
      </owl:Class>
    </owl:someValuesFrom>
    <owl:onProperty rdf:resource="http://schema.geolink.org/dev/view#hasMeasurementType"/>
  </owl:Restriction>
  <owl:Restriction>
    <rdfs:subClassOf>
      <glview:MeasurementType rdf:about="http://schema.geolink.org/dev/voc/nvs/P02#WDNA">
        <rdfs:subClassOf rdf:resource="http://schema.geolink.org/dev/voc/nvs/P03#C050"/>
        <rdfs:subClassOf rdf:resource="http://schema.geolink.org/dev/voc/nvs/P03#B027"/>
        <rdfs:subClassOf rdf:resource="http://schema.geolink.org/dev/voc/nvs/P03#B005"/>
        <rdfs:seeAlso rdf:resource="http://vocab.nerc.ac.uk/collection/P02/current/WDNA/"/>
        <rdfs:comment xml:lang="en">Parameters quantifying the amount of naturally-produced organic (molecules containing carbon) compounds that are built from multiple instances of structural units (monomers) that are covalently-bonded to produce larger structures in any body of salt or fresh water. Includes polynucleotides (RNA and DNA), polypeptides and polysaccharides (e.g. cellulose).</rdfs:comment>
        <rdfs:label xml:lang="en">Concentrations of biopolymers in water bodies</rdfs:label>
        <rdf:type rdf:resource="http://www.w3.org/2002/07/owl#NamedIndividual"/>
        <rdf:type rdf:resource="http://www.w3.org/2002/07/owl#Class"/>
      </glview:MeasurementType>
    </rdfs:subClassOf>
    <owl:someValuesFrom>
      <owl:Class>
        <owl:oneOf rdf:parseType="Collection">
          <glview:MeasurementType rdf:about="http://schema.geolink.org/dev/voc/nvs/P02#WDNA"/>
        </owl:oneOf>
      </owl:Class>
    </owl:someValuesFrom>
    <owl:onProperty rdf:resource="http://schema.geolink.org/dev/view#hasMeasurementType"/>
  </owl:Restriction>
  <owl:Restriction>
    <rdfs:subClassOf>
      <glview:MeasurementType rdf:about="http://schema.geolink.org/dev/voc/nvs/P02#RPER">
        <rdfs:subClassOf rdf:resource="http://schema.geolink.org/dev/voc/nvs/P03#G040"/>
        <rdfs:seeAlso rdf:resource="http://vocab.nerc.ac.uk/collection/P02/current/RPER/"/>
        <rdfs:comment xml:lang="en">Parmeters describing the space for fluids or gases within a geologic unit comprising lithified sediments, igneous rock or metamorphic rock.</rdfs:comment>
        <rdfs:label xml:lang="en">Rock porosity and permeability</rdfs:label>
        <rdf:type rdf:resource="http://www.w3.org/2002/07/owl#NamedIndividual"/>
        <rdf:type rdf:resource="http://www.w3.org/2002/07/owl#Class"/>
      </glview:MeasurementType>
    </rdfs:subClassOf>
    <owl:someValuesFrom>
      <owl:Class>
        <owl:oneOf rdf:parseType="Collection">
          <glview:MeasurementType rdf:about="http://schema.geolink.org/dev/voc/nvs/P02#RPER"/>
        </owl:oneOf>
      </owl:Class>
    </owl:someValuesFrom>
    <owl:onProperty rdf:resource="http://schema.geolink.org/dev/view#hasMeasurementType"/>
  </owl:Restriction>
  <owl:Restriction>
    <rdfs:subClassOf>
      <glview:MeasurementType rdf:about="http://schema.geolink.org/dev/voc/nvs/P02#BLUM">
        <rdfs:subClassOf rdf:resource="http://schema.geolink.org/dev/voc/nvs/P03#D015"/>
        <rdfs:subClassOf rdf:resource="http://schema.geolink.org/dev/voc/nvs/P03#B027"/>
        <rdfs:seeAlso rdf:resource="http://vocab.nerc.ac.uk/collection/P02/current/BLUM/"/>
        <rdfs:comment xml:lang="en">Parameters describing the nature and intensity of light generated by biological activity in the water column.</rdfs:comment>
        <rdfs:label xml:lang="en">Bioluminescence parameters</rdfs:label>
        <rdf:type rdf:resource="http://www.w3.org/2002/07/owl#NamedIndividual"/>
        <rdf:type rdf:resource="http://www.w3.org/2002/07/owl#Class"/>
      </glview:MeasurementType>
    </rdfs:subClassOf>
    <owl:someValuesFrom>
      <owl:Class>
        <owl:oneOf rdf:parseType="Collection">
          <glview:MeasurementType rdf:about="http://schema.geolink.org/dev/voc/nvs/P02#BLUM"/>
        </owl:oneOf>
      </owl:Class>
    </owl:someValuesFrom>
    <owl:onProperty rdf:resource="http://schema.geolink.org/dev/view#hasMeasurementType"/>
  </owl:Restriction>
  <owl:Restriction>
    <rdfs:subClassOf>
      <glview:MeasurementType rdf:about="http://schema.geolink.org/dev/voc/nvs/P02#OZON">
        <rdfs:subClassOf rdf:resource="http://schema.geolink.org/dev/voc/nvs/P03#M005"/>
        <rdfs:seeAlso rdf:resource="http://vocab.nerc.ac.uk/collection/P02/current/OZON/"/>
        <rdfs:comment xml:lang="en">Ozone and oxygen concentration parameters in any phase of the atmosphere (but usually the gaseous phase)</rdfs:comment>
        <rdfs:label xml:lang="en">Ozone and oxygen concentrations in the atmosphere</rdfs:label>
        <rdf:type rdf:resource="http://www.w3.org/2002/07/owl#NamedIndividual"/>
        <rdf:type rdf:resource="http://www.w3.org/2002/07/owl#Class"/>
      </glview:MeasurementType>
    </rdfs:subClassOf>
    <owl:someValuesFrom>
      <owl:Class>
        <owl:oneOf rdf:parseType="Collection">
          <glview:MeasurementType rdf:about="http://schema.geolink.org/dev/voc/nvs/P02#OZON"/>
        </owl:oneOf>
      </owl:Class>
    </owl:someValuesFrom>
    <owl:onProperty rdf:resource="http://schema.geolink.org/dev/view#hasMeasurementType"/>
  </owl:Restriction>
  <owl:Restriction>
    <rdfs:subClassOf>
      <glview:MeasurementType rdf:about="http://schema.geolink.org/dev/voc/nvs/P02#GP005">
        <rdfs:subClassOf rdf:resource="http://schema.geolink.org/dev/voc/nvs/P03#B060"/>
        <rdfs:subClassOf rdf:resource="http://schema.geolink.org/dev/voc/nvs/P03#B020"/>
        <rdfs:seeAlso rdf:resource="http://vocab.nerc.ac.uk/collection/P02/current/GP005/"/>
        <rdfs:comment xml:lang="en">Parameters related to the infection of Fish (Osteichthyes, Agnatha and Chrondrichthyes) by parasites and disease. Includes visual assesements and analytical data.</rdfs:comment>
        <rdfs:label xml:lang="en">Fish disease and parasites</rdfs:label>
        <rdf:type rdf:resource="http://www.w3.org/2002/07/owl#NamedIndividual"/>
        <rdf:type rdf:resource="http://www.w3.org/2002/07/owl#Class"/>
      </glview:MeasurementType>
    </rdfs:subClassOf>
    <owl:someValuesFrom>
      <owl:Class>
        <owl:oneOf rdf:parseType="Collection">
          <glview:MeasurementType rdf:about="http://schema.geolink.org/dev/voc/nvs/P02#GP005"/>
        </owl:oneOf>
      </owl:Class>
    </owl:someValuesFrom>
    <owl:onProperty rdf:resource="http://schema.geolink.org/dev/view#hasMeasurementType"/>
  </owl:Restriction>
  <owl:Restriction>
    <rdfs:subClassOf rdf:resource="http://schema.geolink.org/dev/voc/nvs/P02#BLUM"/>
    <owl:someValuesFrom>
      <owl:Class>
        <owl:oneOf rdf:parseType="Collection">
          <glview:MeasurementType rdf:about="http://schema.geolink.org/dev/voc/nvs/P02#BLUM"/>
        </owl:oneOf>
      </owl:Class>
    </owl:someValuesFrom>
    <owl:onProperty rdf:resource="http://schema.geolink.org/dev/view#hasMeasurementType"/>
  </owl:Restriction>
  <owl:Restriction>
    <rdfs:subClassOf rdf:resource="http://schema.geolink.org/dev/voc/nvs/P02#BEPP"/>
    <owl:someValuesFrom>
      <owl:Class>
        <owl:oneOf rdf:parseType="Collection">
          <glview:MeasurementType rdf:about="http://schema.geolink.org/dev/voc/nvs/P02#BEPP"/>
        </owl:oneOf>
      </owl:Class>
    </owl:someValuesFrom>
    <owl:onProperty rdf:resource="http://schema.geolink.org/dev/view#hasMeasurementType"/>
  </owl:Restriction>
  <owl:Restriction>
    <rdfs:subClassOf>
      <glview:MeasurementType rdf:about="http://schema.geolink.org/dev/voc/nvs/P02#IAGE">
        <rdfs:subClassOf rdf:resource="http://schema.geolink.org/dev/voc/nvs/P03#M015"/>
        <rdfs:seeAlso rdf:resource="http://vocab.nerc.ac.uk/collection/P02/current/IAGE/"/>
        <rdfs:comment xml:lang="en">Measured or stratigraphically estimated age of ice</rdfs:comment>
        <rdfs:label xml:lang="en">Ice age</rdfs:label>
        <rdf:type rdf:resource="http://www.w3.org/2002/07/owl#NamedIndividual"/>
        <rdf:type rdf:resource="http://www.w3.org/2002/07/owl#Class"/>
      </glview:MeasurementType>
    </rdfs:subClassOf>
    <owl:someValuesFrom>
      <owl:Class>
        <owl:oneOf rdf:parseType="Collection">
          <glview:MeasurementType rdf:about="http://schema.geolink.org/dev/voc/nvs/P02#IAGE"/>
        </owl:oneOf>
      </owl:Class>
    </owl:someValuesFrom>
    <owl:onProperty rdf:resource="http://schema.geolink.org/dev/view#hasMeasurementType"/>
  </owl:Restriction>
  <owl:Restriction>
    <rdfs:subClassOf>
      <glview:MeasurementType rdf:about="http://schema.geolink.org/dev/voc/nvs/P02#MZCT">
        <rdfs:subClassOf rdf:resource="http://schema.geolink.org/dev/voc/nvs/P03#B025"/>
        <rdfs:subClassOf rdf:resource="http://schema.geolink.org/dev/voc/nvs/P03#O010"/>
        <rdfs:seeAlso rdf:resource="http://vocab.nerc.ac.uk/collection/P02/current/MZCT/"/>
        <rdfs:comment xml:lang="en">Parameters that express the consumption of the phytoplankton population by the microzooplankton.  Generally the results of dilution experiments on water samples screened through a 200-micron mesh.</rdfs:comment>
        <rdfs:label xml:lang="en">Microzooplankton grazing</rdfs:label>
        <rdf:type rdf:resource="http://www.w3.org/2002/07/owl#NamedIndividual"/>
        <rdf:type rdf:resource="http://www.w3.org/2002/07/owl#Class"/>
      </glview:MeasurementType>
    </rdfs:subClassOf>
    <owl:someValuesFrom>
      <owl:Class>
        <owl:oneOf rdf:parseType="Collection">
          <glview:MeasurementType rdf:about="http://schema.geolink.org/dev/voc/nvs/P02#MZCT"/>
        </owl:oneOf>
      </owl:Class>
    </owl:someValuesFrom>
    <owl:onProperty rdf:resource="http://schema.geolink.org/dev/view#hasMeasurementType"/>
  </owl:Restriction>
  <owl:Restriction>
    <rdfs:subClassOf>
      <glview:MeasurementType rdf:about="http://schema.geolink.org/dev/voc/nvs/P02#AMOX">
        <rdfs:subClassOf rdf:resource="http://schema.geolink.org/dev/voc/nvs/P03#O010"/>
        <rdfs:subClassOf rdf:resource="http://schema.geolink.org/dev/voc/nvs/P03#C005"/>
        <rdfs:subClassOf rdf:resource="http://schema.geolink.org/dev/voc/nvs/P03#C040"/>
        <rdfs:seeAlso rdf:resource="http://vocab.nerc.ac.uk/collection/P02/current/AMOX/"/>
        <rdfs:comment xml:lang="en">Parameters relating to the rate of nitrification (oxidation of reduced nitrogen such as ammonium) in the water column</rdfs:comment>
        <rdfs:label xml:lang="en">Nitrification rate in the water column</rdfs:label>
        <rdf:type rdf:resource="http://www.w3.org/2002/07/owl#NamedIndividual"/>
        <rdf:type rdf:resource="http://www.w3.org/2002/07/owl#Class"/>
      </glview:MeasurementType>
    </rdfs:subClassOf>
    <owl:someValuesFrom>
      <owl:Class>
        <owl:oneOf rdf:parseType="Collection">
          <glview:MeasurementType rdf:about="http://schema.geolink.org/dev/voc/nvs/P02#AMOX"/>
        </owl:oneOf>
      </owl:Class>
    </owl:someValuesFrom>
    <owl:onProperty rdf:resource="http://schema.geolink.org/dev/view#hasMeasurementType"/>
  </owl:Restriction>
  <owl:Restriction>
    <rdfs:subClassOf rdf:resource="http://schema.geolink.org/dev/voc/nvs/P02#MTAT"/>
    <owl:someValuesFrom>
      <owl:Class>
        <owl:oneOf rdf:parseType="Collection">
          <glview:MeasurementType rdf:about="http://schema.geolink.org/dev/voc/nvs/P02#MTAT"/>
        </owl:oneOf>
      </owl:Class>
    </owl:someValuesFrom>
    <owl:onProperty rdf:resource="http://schema.geolink.org/dev/view#hasMeasurementType"/>
  </owl:Restriction>
  <owl:Restriction>
    <rdfs:subClassOf>
      <glview:MeasurementType rdf:about="http://schema.geolink.org/dev/voc/nvs/P02#EXUV">
        <rdfs:subClassOf rdf:resource="http://schema.geolink.org/dev/voc/nvs/P03#B027"/>
        <rdfs:subClassOf rdf:resource="http://schema.geolink.org/dev/voc/nvs/P03#G015"/>
        <rdfs:seeAlso rdf:resource="http://vocab.nerc.ac.uk/collection/P02/current/EXUV/"/>
        <rdfs:comment xml:lang="en">Parameters quantifying and categorising biological detritus (eg exuvia and faecal pellets) in the water column that have been derived from the water column</rdfs:comment>
        <rdfs:label xml:lang="en">Biological detritus in the water column suspended particulate material</rdfs:label>
        <rdf:type rdf:resource="http://www.w3.org/2002/07/owl#NamedIndividual"/>
        <rdf:type rdf:resource="http://www.w3.org/2002/07/owl#Class"/>
      </glview:MeasurementType>
    </rdfs:subClassOf>
    <owl:someValuesFrom>
      <owl:Class>
        <owl:oneOf rdf:parseType="Collection">
          <glview:MeasurementType rdf:about="http://schema.geolink.org/dev/voc/nvs/P02#EXUV"/>
        </owl:oneOf>
      </owl:Class>
    </owl:someValuesFrom>
    <owl:onProperty rdf:resource="http://schema.geolink.org/dev/view#hasMeasurementType"/>
  </owl:Restriction>
  <owl:Restriction>
    <rdfs:subClassOf>
      <glview:MeasurementType rdf:about="http://schema.geolink.org/dev/voc/nvs/P02#OPFX">
        <rdfs:subClassOf rdf:resource="http://schema.geolink.org/dev/voc/nvs/P03#O005"/>
        <rdfs:seeAlso rdf:resource="http://vocab.nerc.ac.uk/collection/P02/current/OPFX/"/>
        <rdfs:comment xml:lang="en">Quantity of any inorganic species such as silicon (opal) and phosphorus passing through unit area of the water column in unit time. Carbon and nitrogen are regarded as organic and explicitly excluded</rdfs:comment>
        <rdfs:label xml:lang="en">Sedimentation flux of non-metallic inorganic species in the water column</rdfs:label>
        <rdf:type rdf:resource="http://www.w3.org/2002/07/owl#NamedIndividual"/>
        <rdf:type rdf:resource="http://www.w3.org/2002/07/owl#Class"/>
      </glview:MeasurementType>
    </rdfs:subClassOf>
    <owl:someValuesFrom>
      <owl:Class>
        <owl:oneOf rdf:parseType="Collection">
          <glview:MeasurementType rdf:about="http://schema.geolink.org/dev/voc/nvs/P02#OPFX"/>
        </owl:oneOf>
      </owl:Class>
    </owl:someValuesFrom>
    <owl:onProperty rdf:resource="http://schema.geolink.org/dev/view#hasMeasurementType"/>
  </owl:Restriction>
  <owl:Restriction>
    <rdfs:subClassOf>
      <glview:MeasurementType rdf:about="http://schema.geolink.org/dev/voc/nvs/P02#ACSR">
        <rdfs:subClassOf rdf:resource="http://schema.geolink.org/dev/voc/nvs/P03#GPYS"/>
        <rdfs:subClassOf rdf:resource="http://schema.geolink.org/dev/voc/nvs/P03#G012"/>
        <rdfs:seeAlso rdf:resource="http://vocab.nerc.ac.uk/collection/P02/current/ACSR/"/>
        <rdfs:comment xml:lang="en">Parameters quantifying the magnitude of earth movements resulting from artificial sources (such as explosions) far away from the measurement site.</rdfs:comment>
        <rdfs:label xml:lang="en">Active seismic refraction</rdfs:label>
        <rdf:type rdf:resource="http://www.w3.org/2002/07/owl#NamedIndividual"/>
        <rdf:type rdf:resource="http://www.w3.org/2002/07/owl#Class"/>
      </glview:MeasurementType>
    </rdfs:subClassOf>
    <owl:someValuesFrom>
      <owl:Class>
        <owl:oneOf rdf:parseType="Collection">
          <glview:MeasurementType rdf:about="http://schema.geolink.org/dev/voc/nvs/P02#ACSR"/>
        </owl:oneOf>
      </owl:Class>
    </owl:someValuesFrom>
    <owl:onProperty rdf:resource="http://schema.geolink.org/dev/view#hasMeasurementType"/>
  </owl:Restriction>
  <owl:Restriction>
    <rdfs:subClassOf>
      <glview:MeasurementType rdf:about="http://schema.geolink.org/dev/voc/nvs/P02#CBSD">
        <rdfs:subClassOf rdf:resource="http://schema.geolink.org/dev/voc/nvs/P03#C005"/>
        <rdfs:subClassOf rdf:resource="http://schema.geolink.org/dev/voc/nvs/P03#G035"/>
        <rdfs:seeAlso rdf:resource="http://vocab.nerc.ac.uk/collection/P02/current/CBSD/"/>
        <rdfs:comment xml:lang="en">Concentrations of total, organic and inorganic carbon per unit weight of sediment.  Sediment is understood to be the solid phase of the bed, including the recently settled material sometimes known as fluff collected from the bed surface.</rdfs:comment>
        <rdfs:label xml:lang="en">Carbon concentrations in sediment</rdfs:label>
        <rdf:type rdf:resource="http://www.w3.org/2002/07/owl#NamedIndividual"/>
        <rdf:type rdf:resource="http://www.w3.org/2002/07/owl#Class"/>
      </glview:MeasurementType>
    </rdfs:subClassOf>
    <owl:someValuesFrom>
      <owl:Class>
        <owl:oneOf rdf:parseType="Collection">
          <glview:MeasurementType rdf:about="http://schema.geolink.org/dev/voc/nvs/P02#CBSD"/>
        </owl:oneOf>
      </owl:Class>
    </owl:someValuesFrom>
    <owl:onProperty rdf:resource="http://schema.geolink.org/dev/view#hasMeasurementType"/>
  </owl:Restriction>
  <owl:Restriction>
    <rdfs:subClassOf>
      <glview:MeasurementType rdf:about="http://schema.geolink.org/dev/voc/nvs/P02#MARC">
        <rdfs:subClassOf rdf:resource="http://schema.geolink.org/dev/voc/nvs/P03#H005"/>
        <rdfs:seeAlso rdf:resource="http://vocab.nerc.ac.uk/collection/P02/current/MARC/"/>
        <rdfs:comment xml:lang="en">Parameters related to the study of human interaction with the sea through the investigation of associated physical remains, be they vessels, shore side facilities, port-related structures, cargoes, human remains or submerged landscapes</rdfs:comment>
        <rdfs:label xml:lang="en">Marine archaeology</rdfs:label>
        <rdf:type rdf:resource="http://www.w3.org/2002/07/owl#NamedIndividual"/>
        <rdf:type rdf:resource="http://www.w3.org/2002/07/owl#Class"/>
      </glview:MeasurementType>
    </rdfs:subClassOf>
    <owl:someValuesFrom>
      <owl:Class>
        <owl:oneOf rdf:parseType="Collection">
          <glview:MeasurementType rdf:about="http://schema.geolink.org/dev/voc/nvs/P02#MARC"/>
        </owl:oneOf>
      </owl:Class>
    </owl:someValuesFrom>
    <owl:onProperty rdf:resource="http://schema.geolink.org/dev/view#hasMeasurementType"/>
  </owl:Restriction>
  <owl:Restriction>
    <rdfs:subClassOf>
      <glview:MeasurementType rdf:about="http://schema.geolink.org/dev/voc/nvs/P02#CCPW">
        <rdfs:subClassOf rdf:resource="http://schema.geolink.org/dev/voc/nvs/P03#G050"/>
        <rdfs:subClassOf rdf:resource="http://schema.geolink.org/dev/voc/nvs/P03#C010"/>
        <rdfs:seeAlso rdf:resource="http://vocab.nerc.ac.uk/collection/P02/current/CCPW/"/>
        <rdfs:comment xml:lang="en">Carbonate system parameters (DIC/TCO2, pH, alkalinity, pCO2) in sediment pore waters</rdfs:comment>
        <rdfs:label xml:lang="en">Dissolved inorganic carbon in sediment pore waters</rdfs:label>
        <rdf:type rdf:resource="http://www.w3.org/2002/07/owl#NamedIndividual"/>
        <rdf:type rdf:resource="http://www.w3.org/2002/07/owl#Class"/>
      </glview:MeasurementType>
    </rdfs:subClassOf>
    <owl:someValuesFrom>
      <owl:Class>
        <owl:oneOf rdf:parseType="Collection">
          <glview:MeasurementType rdf:about="http://schema.geolink.org/dev/voc/nvs/P02#CCPW"/>
        </owl:oneOf>
      </owl:Class>
    </owl:someValuesFrom>
    <owl:onProperty rdf:resource="http://schema.geolink.org/dev/view#hasMeasurementType"/>
  </owl:Restriction>
  <owl:Restriction>
    <rdfs:subClassOf>
      <glview:MeasurementType rdf:about="http://schema.geolink.org/dev/voc/nvs/P02#ZNLG">
        <rdfs:subClassOf rdf:resource="http://schema.geolink.org/dev/voc/nvs/P03#C045"/>
        <rdfs:subClassOf rdf:resource="http://schema.geolink.org/dev/voc/nvs/P03#C050"/>
        <rdfs:subClassOf rdf:resource="http://schema.geolink.org/dev/voc/nvs/P03#C035"/>
        <rdfs:seeAlso rdf:resource="http://vocab.nerc.ac.uk/collection/P02/current/ZNLG/"/>
        <rdfs:comment xml:lang="en">Parameters concerned with the complexation of metals as ligands in the water column</rdfs:comment>
        <rdfs:label xml:lang="en">Metal ligand parameters in the water column</rdfs:label>
        <rdf:type rdf:resource="http://www.w3.org/2002/07/owl#NamedIndividual"/>
        <rdf:type rdf:resource="http://www.w3.org/2002/07/owl#Class"/>
      </glview:MeasurementType>
    </rdfs:subClassOf>
    <owl:someValuesFrom>
      <owl:Class>
        <owl:oneOf rdf:parseType="Collection">
          <glview:MeasurementType rdf:about="http://schema.geolink.org/dev/voc/nvs/P02#ZNLG"/>
        </owl:oneOf>
      </owl:Class>
    </owl:someValuesFrom>
    <owl:onProperty rdf:resource="http://schema.geolink.org/dev/view#hasMeasurementType"/>
  </owl:Restriction>
  <owl:Restriction>
    <rdfs:subClassOf>
      <glview:MeasurementType rdf:about="http://schema.geolink.org/dev/voc/nvs/P02#BDWC">
        <rdfs:subClassOf rdf:resource="http://schema.geolink.org/dev/voc/nvs/P03#B070"/>
        <rdfs:subClassOf rdf:resource="http://schema.geolink.org/dev/voc/nvs/P03#B005"/>
        <rdfs:seeAlso rdf:resource="http://vocab.nerc.ac.uk/collection/P02/current/BDWC/"/>
        <rdfs:comment xml:lang="en">Bacteria ash-free dry weight biomass in sediment parameters presented at the level of taxa that may be mapped to entities in the ITIS taxonomy.  The taxa may be at any taxonomic level from sub-species upwards.  Bacteria are defined as all taxa that fall into Kingdom Monera in the ITIS taxonomy, which includes cyanobacteria.</rdfs:comment>
        <rdfs:label xml:lang="en">Bacteria taxonomy-related ash-free dry weight biomass in sediment</rdfs:label>
        <rdf:type rdf:resource="http://www.w3.org/2002/07/owl#NamedIndividual"/>
        <rdf:type rdf:resource="http://www.w3.org/2002/07/owl#Class"/>
      </glview:MeasurementType>
    </rdfs:subClassOf>
    <owl:someValuesFrom>
      <owl:Class>
        <owl:oneOf rdf:parseType="Collection">
          <glview:MeasurementType rdf:about="http://schema.geolink.org/dev/voc/nvs/P02#BDWC"/>
        </owl:oneOf>
      </owl:Class>
    </owl:someValuesFrom>
    <owl:onProperty rdf:resource="http://schema.geolink.org/dev/view#hasMeasurementType"/>
  </owl:Restriction>
  <owl:Restriction>
    <rdfs:subClassOf>
      <glview:MeasurementType rdf:about="http://schema.geolink.org/dev/voc/nvs/P02#EXCR">
        <rdfs:subClassOf rdf:resource="http://schema.geolink.org/dev/voc/nvs/P03#B027"/>
        <rdfs:subClassOf rdf:resource="http://schema.geolink.org/dev/voc/nvs/P03#O010"/>
        <rdfs:seeAlso rdf:resource="http://vocab.nerc.ac.uk/collection/P02/current/EXCR/"/>
        <rdfs:comment xml:lang="en">Includes all parameters relating to all mechanisms of waste release except respiration.</rdfs:comment>
        <rdfs:label xml:lang="en">Excretion rate parameters in the water column</rdfs:label>
        <rdf:type rdf:resource="http://www.w3.org/2002/07/owl#NamedIndividual"/>
        <rdf:type rdf:resource="http://www.w3.org/2002/07/owl#Class"/>
      </glview:MeasurementType>
    </rdfs:subClassOf>
    <owl:someValuesFrom>
      <owl:Class>
        <owl:oneOf rdf:parseType="Collection">
          <glview:MeasurementType rdf:about="http://schema.geolink.org/dev/voc/nvs/P02#EXCR"/>
        </owl:oneOf>
      </owl:Class>
    </owl:someValuesFrom>
    <owl:onProperty rdf:resource="http://schema.geolink.org/dev/view#hasMeasurementType"/>
  </owl:Restriction>
  <owl:Restriction>
    <rdfs:subClassOf>
      <glview:MeasurementType rdf:about="http://schema.geolink.org/dev/voc/nvs/P02#SPGS">
        <rdfs:subClassOf rdf:resource="http://schema.geolink.org/dev/voc/nvs/P03#G015"/>
        <rdfs:seeAlso rdf:resource="http://vocab.nerc.ac.uk/collection/P02/current/SPGS/"/>
        <rdfs:comment xml:lang="en">Includes all SPM grain size measurements and derived statistics</rdfs:comment>
        <rdfs:label xml:lang="en">Suspended particulate material grain size parameters</rdfs:label>
        <rdf:type rdf:resource="http://www.w3.org/2002/07/owl#NamedIndividual"/>
        <rdf:type rdf:resource="http://www.w3.org/2002/07/owl#Class"/>
      </glview:MeasurementType>
    </rdfs:subClassOf>
    <owl:someValuesFrom>
      <owl:Class>
        <owl:oneOf rdf:parseType="Collection">
          <glview:MeasurementType rdf:about="http://schema.geolink.org/dev/voc/nvs/P02#SPGS"/>
        </owl:oneOf>
      </owl:Class>
    </owl:someValuesFrom>
    <owl:onProperty rdf:resource="http://schema.geolink.org/dev/view#hasMeasurementType"/>
  </owl:Restriction>
  <owl:Restriction>
    <rdfs:subClassOf>
      <glview:MeasurementType rdf:about="http://schema.geolink.org/dev/voc/nvs/P02#LWRD">
        <rdfs:subClassOf rdf:resource="http://schema.geolink.org/dev/voc/nvs/P03#M010"/>
        <rdfs:seeAlso rdf:resource="http://vocab.nerc.ac.uk/collection/P02/current/LWRD/"/>
        <rdfs:comment></rdfs:comment>
        <rdfs:label xml:lang="en">Long-wave radiation</rdfs:label>
        <rdf:type rdf:resource="http://www.w3.org/2002/07/owl#NamedIndividual"/>
        <rdf:type rdf:resource="http://www.w3.org/2002/07/owl#Class"/>
      </glview:MeasurementType>
    </rdfs:subClassOf>
    <owl:someValuesFrom>
      <owl:Class>
        <owl:oneOf rdf:parseType="Collection">
          <glview:MeasurementType rdf:about="http://schema.geolink.org/dev/voc/nvs/P02#LWRD"/>
        </owl:oneOf>
      </owl:Class>
    </owl:someValuesFrom>
    <owl:onProperty rdf:resource="http://schema.geolink.org/dev/view#hasMeasurementType"/>
  </owl:Restriction>
  <owl:Restriction>
    <rdfs:subClassOf>
      <glview:MeasurementType rdf:about="http://schema.geolink.org/dev/voc/nvs/P02#IACT">
        <rdfs:subClassOf rdf:resource="http://schema.geolink.org/dev/voc/nvs/P03#H005"/>
        <rdfs:seeAlso rdf:resource="http://vocab.nerc.ac.uk/collection/P02/current/IACT/"/>
        <rdfs:comment xml:lang="en">Parameters that quantify the level of industrial activity or industrial output</rdfs:comment>
        <rdfs:label xml:lang="en">Industrial activity</rdfs:label>
        <rdf:type rdf:resource="http://www.w3.org/2002/07/owl#NamedIndividual"/>
        <rdf:type rdf:resource="http://www.w3.org/2002/07/owl#Class"/>
      </glview:MeasurementType>
    </rdfs:subClassOf>
    <owl:someValuesFrom>
      <owl:Class>
        <owl:oneOf rdf:parseType="Collection">
          <glview:MeasurementType rdf:about="http://schema.geolink.org/dev/voc/nvs/P02#IACT"/>
        </owl:oneOf>
      </owl:Class>
    </owl:someValuesFrom>
    <owl:onProperty rdf:resource="http://schema.geolink.org/dev/view#hasMeasurementType"/>
  </owl:Restriction>
  <owl:Restriction>
    <rdfs:subClassOf>
      <glview:MeasurementType rdf:about="http://schema.geolink.org/dev/voc/nvs/P02#TVLT">
        <rdfs:subClassOf rdf:resource="http://schema.geolink.org/dev/voc/nvs/P03#D015"/>
        <rdfs:subClassOf rdf:resource="http://schema.geolink.org/dev/voc/nvs/P03#G015"/>
        <rdfs:seeAlso rdf:resource="http://vocab.nerc.ac.uk/collection/P02/current/TVLT/"/>
        <rdfs:comment xml:lang="en">Raw parameters (voltages and counts) from in-situ suspended particulate material sensors including transmissometers, nephelometers,in-situ particle sizers and ABS (including ADCP echo intensity).</rdfs:comment>
        <rdfs:label xml:lang="en">Raw suspended particulate material concentration sensor output</rdfs:label>
        <rdf:type rdf:resource="http://www.w3.org/2002/07/owl#NamedIndividual"/>
        <rdf:type rdf:resource="http://www.w3.org/2002/07/owl#Class"/>
      </glview:MeasurementType>
    </rdfs:subClassOf>
    <owl:someValuesFrom>
      <owl:Class>
        <owl:oneOf rdf:parseType="Collection">
          <glview:MeasurementType rdf:about="http://schema.geolink.org/dev/voc/nvs/P02#TVLT"/>
        </owl:oneOf>
      </owl:Class>
    </owl:someValuesFrom>
    <owl:onProperty rdf:resource="http://schema.geolink.org/dev/view#hasMeasurementType"/>
  </owl:Restriction>
  <owl:Restriction>
    <rdfs:subClassOf>
      <glview:MeasurementType rdf:about="http://schema.geolink.org/dev/voc/nvs/P02#RGAS">
        <rdfs:subClassOf rdf:resource="http://schema.geolink.org/dev/voc/nvs/P03#C015"/>
        <rdfs:subClassOf rdf:resource="http://schema.geolink.org/dev/voc/nvs/P03#M005"/>
        <rdfs:seeAlso rdf:resource="http://vocab.nerc.ac.uk/collection/P02/current/RGAS/"/>
        <rdfs:comment xml:lang="en">Raw concentration parameters from a gas analyser such as a LiCor</rdfs:comment>
        <rdfs:label xml:lang="en">Raw gas analyser output</rdfs:label>
        <rdf:type rdf:resource="http://www.w3.org/2002/07/owl#NamedIndividual"/>
        <rdf:type rdf:resource="http://www.w3.org/2002/07/owl#Class"/>
      </glview:MeasurementType>
    </rdfs:subClassOf>
    <owl:someValuesFrom>
      <owl:Class>
        <owl:oneOf rdf:parseType="Collection">
          <glview:MeasurementType rdf:about="http://schema.geolink.org/dev/voc/nvs/P02#RGAS"/>
        </owl:oneOf>
      </owl:Class>
    </owl:someValuesFrom>
    <owl:onProperty rdf:resource="http://schema.geolink.org/dev/view#hasMeasurementType"/>
  </owl:Restriction>
  <owl:Restriction>
    <rdfs:subClassOf>
      <glview:MeasurementType rdf:about="http://schema.geolink.org/dev/voc/nvs/P02#F001">
        <rdfs:subClassOf rdf:resource="http://schema.geolink.org/dev/view#Measurement"/>
        <rdfs:seeAlso rdf:resource="http://vocab.nerc.ac.uk/collection/P02/current/F001/"/>
        <rdfs:comment xml:lang="en">Lipids are defined as small water-insoluble biomolecules including fats, fatty acids, esters, sterols, isoprenoid compounds, etc..  Water body includes any body of fresh or salt water. As lipids are insoluble in water the concencentrations are associated with the particulate phase.</rdfs:comment>
        <rdfs:label xml:lang="en">Water body lipid concentrations</rdfs:label>
        <rdf:type rdf:resource="http://www.w3.org/2002/07/owl#NamedIndividual"/>
        <rdf:type rdf:resource="http://www.w3.org/2002/07/owl#Class"/>
      </glview:MeasurementType>
    </rdfs:subClassOf>
    <owl:someValuesFrom>
      <owl:Class>
        <owl:oneOf rdf:parseType="Collection">
          <glview:MeasurementType rdf:about="http://schema.geolink.org/dev/voc/nvs/P02#F001"/>
        </owl:oneOf>
      </owl:Class>
    </owl:someValuesFrom>
    <owl:onProperty rdf:resource="http://schema.geolink.org/dev/view#hasMeasurementType"/>
  </owl:Restriction>
  <owl:Restriction>
    <rdfs:subClassOf rdf:resource="http://schema.geolink.org/dev/voc/nvs/P02#RGAS"/>
    <owl:someValuesFrom>
      <owl:Class>
        <owl:oneOf rdf:parseType="Collection">
          <glview:MeasurementType rdf:about="http://schema.geolink.org/dev/voc/nvs/P02#RGAS"/>
        </owl:oneOf>
      </owl:Class>
    </owl:someValuesFrom>
    <owl:onProperty rdf:resource="http://schema.geolink.org/dev/view#hasMeasurementType"/>
  </owl:Restriction>
  <owl:Restriction>
    <rdfs:subClassOf>
      <glview:MeasurementType rdf:about="http://schema.geolink.org/dev/voc/nvs/P02#SICO">
        <rdfs:subClassOf rdf:resource="http://schema.geolink.org/dev/voc/nvs/P03#O005"/>
        <rdfs:seeAlso rdf:resource="http://vocab.nerc.ac.uk/collection/P02/current/SICO/"/>
        <rdfs:comment xml:lang="en">Fluxes of species other than metals and nutrients between the bed (ie the sediment) and the water column sometimes termed benthic fluxes or sediment demand</rdfs:comment>
        <rdfs:label xml:lang="en">Other fluxes between the bed and the water column</rdfs:label>
        <rdf:type rdf:resource="http://www.w3.org/2002/07/owl#NamedIndividual"/>
        <rdf:type rdf:resource="http://www.w3.org/2002/07/owl#Class"/>
      </glview:MeasurementType>
    </rdfs:subClassOf>
    <owl:someValuesFrom>
      <owl:Class>
        <owl:oneOf rdf:parseType="Collection">
          <glview:MeasurementType rdf:about="http://schema.geolink.org/dev/voc/nvs/P02#SICO"/>
        </owl:oneOf>
      </owl:Class>
    </owl:someValuesFrom>
    <owl:onProperty rdf:resource="http://schema.geolink.org/dev/view#hasMeasurementType"/>
  </owl:Restriction>
  <owl:Restriction>
    <rdfs:subClassOf>
      <glview:MeasurementType rdf:about="http://schema.geolink.org/dev/voc/nvs/P02#PCLM">
        <rdfs:subClassOf rdf:resource="http://schema.geolink.org/dev/voc/nvs/P03#H003"/>
        <rdfs:seeAlso rdf:resource="http://vocab.nerc.ac.uk/collection/P02/current/PCLM/"/>
        <rdfs:comment xml:lang="en">Parameterisations that describe climatic conditions in the past.  Includes climate indices, climate indicators and indirect measurements of climate-related phenomena such as sea level and water table depth.</rdfs:comment>
        <rdfs:label xml:lang="en">Palaeoclimatic indicators and parameters</rdfs:label>
        <rdf:type rdf:resource="http://www.w3.org/2002/07/owl#NamedIndividual"/>
        <rdf:type rdf:resource="http://www.w3.org/2002/07/owl#Class"/>
      </glview:MeasurementType>
    </rdfs:subClassOf>
    <owl:someValuesFrom>
      <owl:Class>
        <owl:oneOf rdf:parseType="Collection">
          <glview:MeasurementType rdf:about="http://schema.geolink.org/dev/voc/nvs/P02#PCLM"/>
        </owl:oneOf>
      </owl:Class>
    </owl:someValuesFrom>
    <owl:onProperty rdf:resource="http://schema.geolink.org/dev/view#hasMeasurementType"/>
  </owl:Restriction>
  <owl:Restriction>
    <rdfs:subClassOf>
      <glview:MeasurementType rdf:about="http://schema.geolink.org/dev/voc/nvs/P02#DOCU">
        <rdfs:subClassOf rdf:resource="http://schema.geolink.org/dev/voc/nvs/P03#O010"/>
        <rdfs:seeAlso rdf:resource="http://vocab.nerc.ac.uk/collection/P02/current/DOCU/"/>
        <rdfs:comment xml:lang="en">Any parameter relating to the rate of DOC concentration change in the water column</rdfs:comment>
        <rdfs:label xml:lang="en">Dissolved organic carbon uptake and production in the water column</rdfs:label>
        <rdf:type rdf:resource="http://www.w3.org/2002/07/owl#NamedIndividual"/>
        <rdf:type rdf:resource="http://www.w3.org/2002/07/owl#Class"/>
      </glview:MeasurementType>
    </rdfs:subClassOf>
    <owl:someValuesFrom>
      <owl:Class>
        <owl:oneOf rdf:parseType="Collection">
          <glview:MeasurementType rdf:about="http://schema.geolink.org/dev/voc/nvs/P02#DOCU"/>
        </owl:oneOf>
      </owl:Class>
    </owl:someValuesFrom>
    <owl:onProperty rdf:resource="http://schema.geolink.org/dev/view#hasMeasurementType"/>
  </owl:Restriction>
  <owl:Restriction>
    <rdfs:subClassOf>
      <glview:MeasurementType rdf:about="http://schema.geolink.org/dev/voc/nvs/P02#MSEP">
        <rdfs:subClassOf rdf:resource="http://schema.geolink.org/dev/voc/nvs/P03#B045"/>
        <rdfs:subClassOf rdf:resource="http://schema.geolink.org/dev/voc/nvs/P03#O010"/>
        <rdfs:seeAlso rdf:resource="http://vocab.nerc.ac.uk/collection/P02/current/MSEP/"/>
        <rdfs:comment xml:lang="en">All parameters related to zooplankton reproduction rates</rdfs:comment>
        <rdfs:label xml:lang="en">Zooplankton reproduction rate parameters</rdfs:label>
        <rdf:type rdf:resource="http://www.w3.org/2002/07/owl#NamedIndividual"/>
        <rdf:type rdf:resource="http://www.w3.org/2002/07/owl#Class"/>
      </glview:MeasurementType>
    </rdfs:subClassOf>
    <owl:someValuesFrom>
      <owl:Class>
        <owl:oneOf rdf:parseType="Collection">
          <glview:MeasurementType rdf:about="http://schema.geolink.org/dev/voc/nvs/P02#MSEP"/>
        </owl:oneOf>
      </owl:Class>
    </owl:someValuesFrom>
    <owl:onProperty rdf:resource="http://schema.geolink.org/dev/view#hasMeasurementType"/>
  </owl:Restriction>
  <owl:Restriction>
    <rdfs:subClassOf>
      <glview:MeasurementType rdf:about="http://schema.geolink.org/dev/voc/nvs/P02#GP048">
        <rdfs:subClassOf rdf:resource="http://schema.geolink.org/dev/voc/nvs/P03#H001"/>
        <rdfs:subClassOf rdf:resource="http://schema.geolink.org/dev/voc/nvs/P03#M005"/>
        <rdfs:seeAlso rdf:resource="http://vocab.nerc.ac.uk/collection/P02/current/GP048/"/>
        <rdfs:comment xml:lang="en">Parameters quantifying polychlorobiphenyl (PCB) concentrations in all phases of the atmosphere</rdfs:comment>
        <rdfs:label xml:lang="en">Concentration of polychlorobiphenyls (PCBs) in the atmosphere</rdfs:label>
        <rdf:type rdf:resource="http://www.w3.org/2002/07/owl#NamedIndividual"/>
        <rdf:type rdf:resource="http://www.w3.org/2002/07/owl#Class"/>
      </glview:MeasurementType>
    </rdfs:subClassOf>
    <owl:someValuesFrom>
      <owl:Class>
        <owl:oneOf rdf:parseType="Collection">
          <glview:MeasurementType rdf:about="http://schema.geolink.org/dev/voc/nvs/P02#GP048"/>
        </owl:oneOf>
      </owl:Class>
    </owl:someValuesFrom>
    <owl:onProperty rdf:resource="http://schema.geolink.org/dev/view#hasMeasurementType"/>
  </owl:Restriction>
  <owl:Restriction>
    <rdfs:subClassOf>
      <glview:MeasurementType rdf:about="http://schema.geolink.org/dev/voc/nvs/P02#ASAM">
        <rdfs:subClassOf rdf:resource="http://schema.geolink.org/dev/voc/nvs/P03#D005"/>
        <rdfs:seeAlso rdf:resource="http://vocab.nerc.ac.uk/collection/P02/current/ASAM/"/>
        <rdfs:comment xml:lang="en">Includes all parameters covering the strength of acoustic signal return, including absolute measurements of returning signal strength as well as parameters expressed as backscatter (the proportion of transmitted signal returned)</rdfs:comment>
        <rdfs:label xml:lang="en">Acoustic backscatter in the water column</rdfs:label>
        <rdf:type rdf:resource="http://www.w3.org/2002/07/owl#NamedIndividual"/>
        <rdf:type rdf:resource="http://www.w3.org/2002/07/owl#Class"/>
      </glview:MeasurementType>
    </rdfs:subClassOf>
    <owl:someValuesFrom>
      <owl:Class>
        <owl:oneOf rdf:parseType="Collection">
          <glview:MeasurementType rdf:about="http://schema.geolink.org/dev/voc/nvs/P02#ASAM"/>
        </owl:oneOf>
      </owl:Class>
    </owl:someValuesFrom>
    <owl:onProperty rdf:resource="http://schema.geolink.org/dev/view#hasMeasurementType"/>
  </owl:Restriction>
  <owl:Restriction>
    <rdfs:subClassOf>
      <glview:MeasurementType rdf:about="http://schema.geolink.org/dev/voc/nvs/P02#TOCH">
        <rdfs:subClassOf rdf:resource="http://schema.geolink.org/dev/voc/nvs/P03#C050"/>
        <rdfs:seeAlso rdf:resource="http://vocab.nerc.ac.uk/collection/P02/current/TOCH/"/>
        <rdfs:comment xml:lang="en">Concentrations of carbohydrates, phenols, alkanols (alcohols), aldehydes and simple (non-alkenone) ketones in all phases of any body of fresh or salt water</rdfs:comment>
        <rdfs:label xml:lang="en">Concentration of carbohydrates, phenols, alkanols (alcohols), aldehydes and ketones in water bodies</rdfs:label>
        <rdf:type rdf:resource="http://www.w3.org/2002/07/owl#NamedIndividual"/>
        <rdf:type rdf:resource="http://www.w3.org/2002/07/owl#Class"/>
      </glview:MeasurementType>
    </rdfs:subClassOf>
    <owl:someValuesFrom>
      <owl:Class>
        <owl:oneOf rdf:parseType="Collection">
          <glview:MeasurementType rdf:about="http://schema.geolink.org/dev/voc/nvs/P02#TOCH"/>
        </owl:oneOf>
      </owl:Class>
    </owl:someValuesFrom>
    <owl:onProperty rdf:resource="http://schema.geolink.org/dev/view#hasMeasurementType"/>
  </owl:Restriction>
  <owl:Restriction>
    <rdfs:subClassOf>
      <glview:MeasurementType rdf:about="http://schema.geolink.org/dev/voc/nvs/P02#STMP">
        <rdfs:subClassOf rdf:resource="http://schema.geolink.org/dev/voc/nvs/P03#GTHM"/>
        <rdfs:subClassOf rdf:resource="http://schema.geolink.org/dev/voc/nvs/P03#GPYS"/>
        <rdfs:seeAlso rdf:resource="http://vocab.nerc.ac.uk/collection/P02/current/STMP/"/>
        <rdfs:comment xml:lang="en">Parameters that describe the distribution of the degree of hotness within a body of rock or unlithified sediment.</rdfs:comment>
        <rdfs:label xml:lang="en">Temperature of geological units</rdfs:label>
        <rdf:type rdf:resource="http://www.w3.org/2002/07/owl#NamedIndividual"/>
        <rdf:type rdf:resource="http://www.w3.org/2002/07/owl#Class"/>
      </glview:MeasurementType>
    </rdfs:subClassOf>
    <owl:someValuesFrom>
      <owl:Class>
        <owl:oneOf rdf:parseType="Collection">
          <glview:MeasurementType rdf:about="http://schema.geolink.org/dev/voc/nvs/P02#STMP"/>
        </owl:oneOf>
      </owl:Class>
    </owl:someValuesFrom>
    <owl:onProperty rdf:resource="http://schema.geolink.org/dev/view#hasMeasurementType"/>
  </owl:Restriction>
  <owl:Restriction>
    <rdfs:subClassOf>
      <glview:MeasurementType rdf:about="http://schema.geolink.org/dev/voc/nvs/P02#CDRU">
        <rdfs:subClassOf rdf:resource="http://schema.geolink.org/dev/voc/nvs/P03#O010"/>
        <rdfs:seeAlso rdf:resource="http://vocab.nerc.ac.uk/collection/P02/current/CDRU/"/>
        <rdfs:comment xml:lang="en">Parameters relating to the uptake rates of metals from the dissolved phase into the particulate phase</rdfs:comment>
        <rdfs:label xml:lang="en">Metal uptake rates in the water column</rdfs:label>
        <rdf:type rdf:resource="http://www.w3.org/2002/07/owl#NamedIndividual"/>
        <rdf:type rdf:resource="http://www.w3.org/2002/07/owl#Class"/>
      </glview:MeasurementType>
    </rdfs:subClassOf>
    <owl:someValuesFrom>
      <owl:Class>
        <owl:oneOf rdf:parseType="Collection">
          <glview:MeasurementType rdf:about="http://schema.geolink.org/dev/voc/nvs/P02#CDRU"/>
        </owl:oneOf>
      </owl:Class>
    </owl:someValuesFrom>
    <owl:onProperty rdf:resource="http://schema.geolink.org/dev/view#hasMeasurementType"/>
  </owl:Restriction>
  <owl:Restriction>
    <rdfs:subClassOf>
      <glview:MeasurementType rdf:about="http://schema.geolink.org/dev/voc/nvs/P02#PHOS">
        <rdfs:subClassOf rdf:resource="http://schema.geolink.org/dev/voc/nvs/P03#C005"/>
        <rdfs:subClassOf rdf:resource="http://schema.geolink.org/dev/voc/nvs/P03#C040"/>
        <rdfs:seeAlso rdf:resource="http://vocab.nerc.ac.uk/collection/P02/current/PHOS/"/>
        <rdfs:comment xml:lang="en">Phosphate  concentration parameters (including statistical parameters such as standard deviation) in the water column</rdfs:comment>
        <rdfs:label xml:lang="en">Phosphate concentration parameters in the water column</rdfs:label>
        <rdf:type rdf:resource="http://www.w3.org/2002/07/owl#NamedIndividual"/>
        <rdf:type rdf:resource="http://www.w3.org/2002/07/owl#Class"/>
      </glview:MeasurementType>
    </rdfs:subClassOf>
    <owl:someValuesFrom>
      <owl:Class>
        <owl:oneOf rdf:parseType="Collection">
          <glview:MeasurementType rdf:about="http://schema.geolink.org/dev/voc/nvs/P02#PHOS"/>
        </owl:oneOf>
      </owl:Class>
    </owl:someValuesFrom>
    <owl:onProperty rdf:resource="http://schema.geolink.org/dev/view#hasMeasurementType"/>
  </owl:Restriction>
  <owl:Restriction>
    <rdfs:subClassOf>
      <glview:MeasurementType rdf:about="http://schema.geolink.org/dev/voc/nvs/P02#BCMT">
        <rdfs:subClassOf rdf:resource="http://schema.geolink.org/dev/voc/nvs/P03#C035"/>
        <rdfs:subClassOf rdf:resource="http://schema.geolink.org/dev/voc/nvs/P03#B007"/>
        <rdfs:subClassOf rdf:resource="http://schema.geolink.org/dev/voc/nvs/P03#H001"/>
        <rdfs:seeAlso rdf:resource="http://vocab.nerc.ac.uk/collection/P02/current/BCMT/"/>
        <rdfs:comment xml:lang="en">Metal concentrations in either whole organisms or their constituent parts.</rdfs:comment>
        <rdfs:label xml:lang="en">Metal concentrations in biota</rdfs:label>
        <rdf:type rdf:resource="http://www.w3.org/2002/07/owl#NamedIndividual"/>
        <rdf:type rdf:resource="http://www.w3.org/2002/07/owl#Class"/>
      </glview:MeasurementType>
    </rdfs:subClassOf>
    <owl:someValuesFrom>
      <owl:Class>
        <owl:oneOf rdf:parseType="Collection">
          <glview:MeasurementType rdf:about="http://schema.geolink.org/dev/voc/nvs/P02#BCMT"/>
        </owl:oneOf>
      </owl:Class>
    </owl:someValuesFrom>
    <owl:onProperty rdf:resource="http://schema.geolink.org/dev/view#hasMeasurementType"/>
  </owl:Restriction>
  <owl:Restriction>
    <rdfs:subClassOf>
      <glview:MeasurementType rdf:about="http://schema.geolink.org/dev/voc/nvs/P02#VATX">
        <rdfs:subClassOf rdf:resource="http://schema.geolink.org/dev/voc/nvs/P03#B030"/>
        <rdfs:seeAlso rdf:resource="http://vocab.nerc.ac.uk/collection/P02/current/VATX/"/>
        <rdfs:comment xml:lang="en">Any parameterisation of cell volume of free-floating autotrophic biological entities designated by taxonomic names (e.g. species, genus, family) in any body of fresh or salt water.</rdfs:comment>
        <rdfs:label xml:lang="en">Phytoplankton taxonomic volume in water bodies</rdfs:label>
        <rdf:type rdf:resource="http://www.w3.org/2002/07/owl#NamedIndividual"/>
        <rdf:type rdf:resource="http://www.w3.org/2002/07/owl#Class"/>
      </glview:MeasurementType>
    </rdfs:subClassOf>
    <owl:someValuesFrom>
      <owl:Class>
        <owl:oneOf rdf:parseType="Collection">
          <glview:MeasurementType rdf:about="http://schema.geolink.org/dev/voc/nvs/P02#VATX"/>
        </owl:oneOf>
      </owl:Class>
    </owl:someValuesFrom>
    <owl:onProperty rdf:resource="http://schema.geolink.org/dev/view#hasMeasurementType"/>
  </owl:Restriction>
  <owl:Restriction>
    <rdfs:subClassOf rdf:resource="http://schema.geolink.org/dev/voc/nvs/P02#CCPW"/>
    <owl:someValuesFrom>
      <owl:Class>
        <owl:oneOf rdf:parseType="Collection">
          <glview:MeasurementType rdf:about="http://schema.geolink.org/dev/voc/nvs/P02#CCPW"/>
        </owl:oneOf>
      </owl:Class>
    </owl:someValuesFrom>
    <owl:onProperty rdf:resource="http://schema.geolink.org/dev/view#hasMeasurementType"/>
  </owl:Restriction>
  <owl:Restriction>
    <rdfs:subClassOf>
      <glview:MeasurementType rdf:about="http://schema.geolink.org/dev/voc/nvs/P02#ZZZZ">
        <rdfs:subClassOf rdf:resource="http://schema.geolink.org/dev/voc/nvs/P03#Z005"/>
        <rdfs:seeAlso rdf:resource="http://vocab.nerc.ac.uk/collection/P02/current/ZZZZ/"/>
        <rdfs:comment xml:lang="en">The identity of the parameter is not declared.  Covers cases such as internal working parameters and dummy channels.</rdfs:comment>
        <rdfs:label xml:lang="en">Unspecified</rdfs:label>
        <rdf:type rdf:resource="http://www.w3.org/2002/07/owl#NamedIndividual"/>
        <rdf:type rdf:resource="http://www.w3.org/2002/07/owl#Class"/>
      </glview:MeasurementType>
    </rdfs:subClassOf>
    <owl:someValuesFrom>
      <owl:Class>
        <owl:oneOf rdf:parseType="Collection">
          <glview:MeasurementType rdf:about="http://schema.geolink.org/dev/voc/nvs/P02#ZZZZ"/>
        </owl:oneOf>
      </owl:Class>
    </owl:someValuesFrom>
    <owl:onProperty rdf:resource="http://schema.geolink.org/dev/view#hasMeasurementType"/>
  </owl:Restriction>
  <owl:Restriction>
    <rdfs:subClassOf>
      <glview:MeasurementType rdf:about="http://schema.geolink.org/dev/voc/nvs/P02#TDNT">
        <rdfs:subClassOf rdf:resource="http://schema.geolink.org/dev/voc/nvs/P03#C005"/>
        <rdfs:seeAlso rdf:resource="http://vocab.nerc.ac.uk/collection/P02/current/TDNT/"/>
        <rdfs:comment xml:lang="en">Concentration of total (organic plus inorganic) or organic dissolved nitrogen per unit volume of the water column.  Grouped together as organic nitrogen frequently determined as total nitrogen.</rdfs:comment>
        <rdfs:label xml:lang="en">Dissolved total and organic nitrogen concentrations in the water column</rdfs:label>
        <rdf:type rdf:resource="http://www.w3.org/2002/07/owl#NamedIndividual"/>
        <rdf:type rdf:resource="http://www.w3.org/2002/07/owl#Class"/>
      </glview:MeasurementType>
    </rdfs:subClassOf>
    <owl:someValuesFrom>
      <owl:Class>
        <owl:oneOf rdf:parseType="Collection">
          <glview:MeasurementType rdf:about="http://schema.geolink.org/dev/voc/nvs/P02#TDNT"/>
        </owl:oneOf>
      </owl:Class>
    </owl:someValuesFrom>
    <owl:onProperty rdf:resource="http://schema.geolink.org/dev/view#hasMeasurementType"/>
  </owl:Restriction>
  <owl:Restriction>
    <rdfs:subClassOf>
      <glview:MeasurementType rdf:about="http://schema.geolink.org/dev/voc/nvs/P02#WRAD">
        <rdfs:subClassOf rdf:resource="http://schema.geolink.org/dev/voc/nvs/P03#C030"/>
        <rdfs:seeAlso rdf:resource="http://vocab.nerc.ac.uk/collection/P02/current/WRAD/"/>
        <rdfs:comment xml:lang="en">All parameters associated with radiocativity in the water column, including radiation counts, isotope activities and activity ratios. Activities per unit mass of SPM are included</rdfs:comment>
        <rdfs:label xml:lang="en">Radioactivity in the water column</rdfs:label>
        <rdf:type rdf:resource="http://www.w3.org/2002/07/owl#NamedIndividual"/>
        <rdf:type rdf:resource="http://www.w3.org/2002/07/owl#Class"/>
      </glview:MeasurementType>
    </rdfs:subClassOf>
    <owl:someValuesFrom>
      <owl:Class>
        <owl:oneOf rdf:parseType="Collection">
          <glview:MeasurementType rdf:about="http://schema.geolink.org/dev/voc/nvs/P02#WRAD"/>
        </owl:oneOf>
      </owl:Class>
    </owl:someValuesFrom>
    <owl:onProperty rdf:resource="http://schema.geolink.org/dev/view#hasMeasurementType"/>
  </owl:Restriction>
  <owl:Restriction>
    <rdfs:subClassOf>
      <glview:MeasurementType rdf:about="http://schema.geolink.org/dev/voc/nvs/P02#CD10">
        <rdfs:subClassOf rdf:resource="http://schema.geolink.org/dev/voc/nvs/P03#G035"/>
        <rdfs:seeAlso rdf:resource="http://vocab.nerc.ac.uk/collection/P02/current/CD10/"/>
        <rdfs:comment xml:lang="en">Lipids are defined as small water-insoluble biomolecules including fats, fatty acids, esters, sterols, isoprenoid compounds, etc..  Sediment is defined as material collected by a corer (including fluff).</rdfs:comment>
        <rdfs:label xml:lang="en">Sediment lipid concentrations</rdfs:label>
        <rdf:type rdf:resource="http://www.w3.org/2002/07/owl#NamedIndividual"/>
        <rdf:type rdf:resource="http://www.w3.org/2002/07/owl#Class"/>
      </glview:MeasurementType>
    </rdfs:subClassOf>
    <owl:someValuesFrom>
      <owl:Class>
        <owl:oneOf rdf:parseType="Collection">
          <glview:MeasurementType rdf:about="http://schema.geolink.org/dev/voc/nvs/P02#CD10"/>
        </owl:oneOf>
      </owl:Class>
    </owl:someValuesFrom>
    <owl:onProperty rdf:resource="http://schema.geolink.org/dev/view#hasMeasurementType"/>
  </owl:Restriction>
  <owl:Restriction>
    <rdfs:subClassOf>
      <glview:MeasurementType rdf:about="http://schema.geolink.org/dev/voc/nvs/P02#VSRW">
        <rdfs:subClassOf rdf:resource="http://schema.geolink.org/dev/voc/nvs/P03#D015"/>
        <rdfs:seeAlso rdf:resource="http://vocab.nerc.ac.uk/collection/P02/current/VSRW/"/>
        <rdfs:comment xml:lang="en">Includes measurements at discrete wavelengths and PAR integrated values, measurements as photon and energy fluxes.</rdfs:comment>
        <rdfs:label xml:lang="en">Visible waveband radiance and irradiance measurements in the water column</rdfs:label>
        <rdf:type rdf:resource="http://www.w3.org/2002/07/owl#NamedIndividual"/>
        <rdf:type rdf:resource="http://www.w3.org/2002/07/owl#Class"/>
      </glview:MeasurementType>
    </rdfs:subClassOf>
    <owl:someValuesFrom>
      <owl:Class>
        <owl:oneOf rdf:parseType="Collection">
          <glview:MeasurementType rdf:about="http://schema.geolink.org/dev/voc/nvs/P02#VSRW"/>
        </owl:oneOf>
      </owl:Class>
    </owl:someValuesFrom>
    <owl:onProperty rdf:resource="http://schema.geolink.org/dev/view#hasMeasurementType"/>
  </owl:Restriction>
  <owl:Restriction>
    <rdfs:subClassOf>
      <glview:MeasurementType rdf:about="http://schema.geolink.org/dev/voc/nvs/P02#MTWT">
        <rdfs:subClassOf rdf:resource="http://schema.geolink.org/dev/voc/nvs/P03#C035"/>
        <rdfs:seeAlso rdf:resource="http://vocab.nerc.ac.uk/collection/P02/current/MTWT/"/>
        <rdfs:comment xml:lang="en">Concentration parameters for metal elements in the combined dissolved and particulate phases of any body of fresh or salt water.</rdfs:comment>
        <rdfs:label xml:lang="en">Total metal concentrations in water bodies</rdfs:label>
        <rdf:type rdf:resource="http://www.w3.org/2002/07/owl#NamedIndividual"/>
        <rdf:type rdf:resource="http://www.w3.org/2002/07/owl#Class"/>
      </glview:MeasurementType>
    </rdfs:subClassOf>
    <owl:someValuesFrom>
      <owl:Class>
        <owl:oneOf rdf:parseType="Collection">
          <glview:MeasurementType rdf:about="http://schema.geolink.org/dev/voc/nvs/P02#MTWT"/>
        </owl:oneOf>
      </owl:Class>
    </owl:someValuesFrom>
    <owl:onProperty rdf:resource="http://schema.geolink.org/dev/view#hasMeasurementType"/>
  </owl:Restriction>
  <owl:Restriction>
    <rdfs:subClassOf>
      <glview:MeasurementType rdf:about="http://schema.geolink.org/dev/voc/nvs/P02#MATX">
        <rdfs:subClassOf rdf:resource="http://schema.geolink.org/dev/voc/nvs/P03#B025"/>
        <rdfs:subClassOf rdf:resource="http://schema.geolink.org/dev/voc/nvs/P03#B070"/>
        <rdfs:seeAlso rdf:resource="http://vocab.nerc.ac.uk/collection/P02/current/MATX/"/>
        <rdfs:comment xml:lang="en">Any enumeration (e.g. count, number per litre) of microzooplankton (free swimming heterotrophic organisms smaller than 200um) designated by taxonomic names (e.g. species, genus or family) in any fresh or salt water body.</rdfs:comment>
        <rdfs:label xml:lang="en">Microzooplankton taxonomic abundance in water bodies</rdfs:label>
        <rdf:type rdf:resource="http://www.w3.org/2002/07/owl#NamedIndividual"/>
        <rdf:type rdf:resource="http://www.w3.org/2002/07/owl#Class"/>
      </glview:MeasurementType>
    </rdfs:subClassOf>
    <owl:someValuesFrom>
      <owl:Class>
        <owl:oneOf rdf:parseType="Collection">
          <glview:MeasurementType rdf:about="http://schema.geolink.org/dev/voc/nvs/P02#MATX"/>
        </owl:oneOf>
      </owl:Class>
    </owl:someValuesFrom>
    <owl:onProperty rdf:resource="http://schema.geolink.org/dev/view#hasMeasurementType"/>
  </owl:Restriction>
  <owl:Restriction>
    <rdfs:subClassOf>
      <glview:MeasurementType rdf:about="http://schema.geolink.org/dev/voc/nvs/P02#TPHS">
        <rdfs:subClassOf rdf:resource="http://schema.geolink.org/dev/voc/nvs/P03#C005"/>
        <rdfs:seeAlso rdf:resource="http://vocab.nerc.ac.uk/collection/P02/current/TPHS/"/>
        <rdfs:comment xml:lang="en">Concentrations of total and organic phosphorus in the particulate phase of the water column, which is a function of both the SPM concentration in the water column and the concentration of phosphorus per unit weight of SPM.</rdfs:comment>
        <rdfs:label xml:lang="en">Particulate total and organic phosphorus concentrations in the water column</rdfs:label>
        <rdf:type rdf:resource="http://www.w3.org/2002/07/owl#NamedIndividual"/>
        <rdf:type rdf:resource="http://www.w3.org/2002/07/owl#Class"/>
      </glview:MeasurementType>
    </rdfs:subClassOf>
    <owl:someValuesFrom>
      <owl:Class>
        <owl:oneOf rdf:parseType="Collection">
          <glview:MeasurementType rdf:about="http://schema.geolink.org/dev/voc/nvs/P02#TPHS"/>
        </owl:oneOf>
      </owl:Class>
    </owl:someValuesFrom>
    <owl:onProperty rdf:resource="http://schema.geolink.org/dev/view#hasMeasurementType"/>
  </owl:Restriction>
  <owl:Restriction>
    <rdfs:subClassOf>
      <glview:MeasurementType rdf:about="http://schema.geolink.org/dev/voc/nvs/P02#HBEX">
        <rdfs:subClassOf rdf:resource="http://schema.geolink.org/dev/voc/nvs/P03#B050"/>
        <rdfs:seeAlso rdf:resource="http://vocab.nerc.ac.uk/collection/P02/current/HBEX/"/>
        <rdfs:comment xml:lang="en">Parameters specifying the vertical and horizontal spatial extent of the ecological character of a place where an organism is found</rdfs:comment>
        <rdfs:label xml:lang="en">Habitat extent</rdfs:label>
        <rdf:type rdf:resource="http://www.w3.org/2002/07/owl#NamedIndividual"/>
        <rdf:type rdf:resource="http://www.w3.org/2002/07/owl#Class"/>
      </glview:MeasurementType>
    </rdfs:subClassOf>
    <owl:someValuesFrom>
      <owl:Class>
        <owl:oneOf rdf:parseType="Collection">
          <glview:MeasurementType rdf:about="http://schema.geolink.org/dev/voc/nvs/P02#HBEX"/>
        </owl:oneOf>
      </owl:Class>
    </owl:someValuesFrom>
    <owl:onProperty rdf:resource="http://schema.geolink.org/dev/view#hasMeasurementType"/>
  </owl:Restriction>
  <owl:Restriction>
    <rdfs:subClassOf>
      <glview:MeasurementType rdf:about="http://schema.geolink.org/dev/voc/nvs/P02#SIGT">
        <rdfs:subClassOf rdf:resource="http://schema.geolink.org/dev/voc/nvs/P03#D020"/>
        <rdfs:seeAlso rdf:resource="http://vocab.nerc.ac.uk/collection/P02/current/SIGT/"/>
        <rdfs:comment xml:lang="en">Absolute determinations of water column density plus parameters (generally expressed as density anomaly) derived from temperature and salinity</rdfs:comment>
        <rdfs:label xml:lang="en">Density of the water column</rdfs:label>
        <rdf:type rdf:resource="http://www.w3.org/2002/07/owl#NamedIndividual"/>
        <rdf:type rdf:resource="http://www.w3.org/2002/07/owl#Class"/>
      </glview:MeasurementType>
    </rdfs:subClassOf>
    <owl:someValuesFrom>
      <owl:Class>
        <owl:oneOf rdf:parseType="Collection">
          <glview:MeasurementType rdf:about="http://schema.geolink.org/dev/voc/nvs/P02#SIGT"/>
        </owl:oneOf>
      </owl:Class>
    </owl:someValuesFrom>
    <owl:onProperty rdf:resource="http://schema.geolink.org/dev/view#hasMeasurementType"/>
  </owl:Restriction>
  <owl:Restriction>
    <rdfs:subClassOf>
      <glview:MeasurementType rdf:about="http://schema.geolink.org/dev/voc/nvs/P02#PCO2">
        <rdfs:subClassOf rdf:resource="http://schema.geolink.org/dev/voc/nvs/P03#C010"/>
        <rdfs:seeAlso rdf:resource="http://vocab.nerc.ac.uk/collection/P02/current/PCO2/"/>
        <rdfs:comment></rdfs:comment>
        <rdfs:label xml:lang="en">Partial pressure (pCO2) and fugacity (fCO2) of carbon dioxide in the water column</rdfs:label>
        <rdf:type rdf:resource="http://www.w3.org/2002/07/owl#NamedIndividual"/>
        <rdf:type rdf:resource="http://www.w3.org/2002/07/owl#Class"/>
      </glview:MeasurementType>
    </rdfs:subClassOf>
    <owl:someValuesFrom>
      <owl:Class>
        <owl:oneOf rdf:parseType="Collection">
          <glview:MeasurementType rdf:about="http://schema.geolink.org/dev/voc/nvs/P02#PCO2"/>
        </owl:oneOf>
      </owl:Class>
    </owl:someValuesFrom>
    <owl:onProperty rdf:resource="http://schema.geolink.org/dev/view#hasMeasurementType"/>
  </owl:Restriction>
  <owl:Restriction>
    <rdfs:subClassOf>
      <glview:MeasurementType rdf:about="http://schema.geolink.org/dev/voc/nvs/P02#SEMO">
        <rdfs:subClassOf rdf:resource="http://schema.geolink.org/dev/voc/nvs/P03#B015"/>
        <rdfs:seeAlso rdf:resource="http://vocab.nerc.ac.uk/collection/P02/current/SEMO/"/>
        <rdfs:comment xml:lang="en">Parameters describing the causes and rate of mortality of Seals (Family Phocidae). Includes both parameters mapped to taxa and those mapped to non-taxonomic groupings.</rdfs:comment>
        <rdfs:label xml:lang="en">Seal mortality</rdfs:label>
        <rdf:type rdf:resource="http://www.w3.org/2002/07/owl#NamedIndividual"/>
        <rdf:type rdf:resource="http://www.w3.org/2002/07/owl#Class"/>
      </glview:MeasurementType>
    </rdfs:subClassOf>
    <owl:someValuesFrom>
      <owl:Class>
        <owl:oneOf rdf:parseType="Collection">
          <glview:MeasurementType rdf:about="http://schema.geolink.org/dev/voc/nvs/P02#SEMO"/>
        </owl:oneOf>
      </owl:Class>
    </owl:someValuesFrom>
    <owl:onProperty rdf:resource="http://schema.geolink.org/dev/view#hasMeasurementType"/>
  </owl:Restriction>
  <owl:Restriction>
    <rdfs:subClassOf rdf:resource="http://schema.geolink.org/dev/voc/nvs/P02#GP048"/>
    <owl:someValuesFrom>
      <owl:Class>
        <owl:oneOf rdf:parseType="Collection">
          <glview:MeasurementType rdf:about="http://schema.geolink.org/dev/voc/nvs/P02#GP048"/>
        </owl:oneOf>
      </owl:Class>
    </owl:someValuesFrom>
    <owl:onProperty rdf:resource="http://schema.geolink.org/dev/view#hasMeasurementType"/>
  </owl:Restriction>
  <owl:Restriction>
    <rdfs:subClassOf>
      <glview:MeasurementType rdf:about="http://schema.geolink.org/dev/voc/nvs/P02#MFAZ">
        <rdfs:subClassOf rdf:resource="http://schema.geolink.org/dev/voc/nvs/P03#B070"/>
        <rdfs:subClassOf rdf:resource="http://schema.geolink.org/dev/voc/nvs/P03#G055"/>
        <rdfs:seeAlso rdf:resource="http://vocab.nerc.ac.uk/collection/P02/current/MFAZ/"/>
        <rdfs:comment xml:lang="en">Any zoobenthos ash-free dry weight biomass per unit area of the littoral zone (between spring tide high and low water) parameters that are not fish or terrestrial animals (insecta/oligochaeta)</rdfs:comment>
        <rdfs:label xml:lang="en">Zoobenthos taxonomy-related ash-free dry weight biomass per unit area of the littoral zone</rdfs:label>
        <rdf:type rdf:resource="http://www.w3.org/2002/07/owl#NamedIndividual"/>
        <rdf:type rdf:resource="http://www.w3.org/2002/07/owl#Class"/>
      </glview:MeasurementType>
    </rdfs:subClassOf>
    <owl:someValuesFrom>
      <owl:Class>
        <owl:oneOf rdf:parseType="Collection">
          <glview:MeasurementType rdf:about="http://schema.geolink.org/dev/voc/nvs/P02#MFAZ"/>
        </owl:oneOf>
      </owl:Class>
    </owl:someValuesFrom>
    <owl:onProperty rdf:resource="http://schema.geolink.org/dev/view#hasMeasurementType"/>
  </owl:Restriction>
  <owl:Restriction>
    <rdfs:subClassOf>
      <glview:MeasurementType rdf:about="http://schema.geolink.org/dev/voc/nvs/P02#NTRI">
        <rdfs:subClassOf rdf:resource="http://schema.geolink.org/dev/voc/nvs/P03#C005"/>
        <rdfs:subClassOf rdf:resource="http://schema.geolink.org/dev/voc/nvs/P03#C040"/>
        <rdfs:seeAlso rdf:resource="http://vocab.nerc.ac.uk/collection/P02/current/NTRI/"/>
        <rdfs:comment xml:lang="en">Nitrite concentration parameters (including statistical parameters such as standard deviation) in the water column</rdfs:comment>
        <rdfs:label xml:lang="en">Nitrite concentration parameters in the water column</rdfs:label>
        <rdf:type rdf:resource="http://www.w3.org/2002/07/owl#NamedIndividual"/>
        <rdf:type rdf:resource="http://www.w3.org/2002/07/owl#Class"/>
      </glview:MeasurementType>
    </rdfs:subClassOf>
    <owl:someValuesFrom>
      <owl:Class>
        <owl:oneOf rdf:parseType="Collection">
          <glview:MeasurementType rdf:about="http://schema.geolink.org/dev/voc/nvs/P02#NTRI"/>
        </owl:oneOf>
      </owl:Class>
    </owl:someValuesFrom>
    <owl:onProperty rdf:resource="http://schema.geolink.org/dev/view#hasMeasurementType"/>
  </owl:Restriction>
  <owl:Restriction>
    <rdfs:subClassOf>
      <glview:MeasurementType rdf:about="http://schema.geolink.org/dev/voc/nvs/P02#GWCH">
        <rdfs:subClassOf rdf:resource="http://schema.geolink.org/dev/voc/nvs/P03#T001"/>
        <rdfs:seeAlso rdf:resource="http://vocab.nerc.ac.uk/collection/P02/current/GWCH/"/>
        <rdfs:comment xml:lang="en">Parameters quantifying the chemistry of terrestrial groundwater bodies such as aquifers and waters percolating through rock formations.</rdfs:comment>
        <rdfs:label xml:lang="en">Groundwater chemistry</rdfs:label>
        <rdf:type rdf:resource="http://www.w3.org/2002/07/owl#NamedIndividual"/>
        <rdf:type rdf:resource="http://www.w3.org/2002/07/owl#Class"/>
      </glview:MeasurementType>
    </rdfs:subClassOf>
    <owl:someValuesFrom>
      <owl:Class>
        <owl:oneOf rdf:parseType="Collection">
          <glview:MeasurementType rdf:about="http://schema.geolink.org/dev/voc/nvs/P02#GWCH"/>
        </owl:oneOf>
      </owl:Class>
    </owl:someValuesFrom>
    <owl:onProperty rdf:resource="http://schema.geolink.org/dev/view#hasMeasurementType"/>
  </owl:Restriction>
  <owl:Restriction>
    <rdfs:subClassOf rdf:resource="http://schema.geolink.org/dev/voc/nvs/P02#CFTM"/>
    <owl:someValuesFrom>
      <owl:Class>
        <owl:oneOf rdf:parseType="Collection">
          <glview:MeasurementType rdf:about="http://schema.geolink.org/dev/voc/nvs/P02#CFTM"/>
        </owl:oneOf>
      </owl:Class>
    </owl:someValuesFrom>
    <owl:onProperty rdf:resource="http://schema.geolink.org/dev/view#hasMeasurementType"/>
  </owl:Restriction>
  <owl:Restriction>
    <rdfs:subClassOf>
      <glview:MeasurementType rdf:about="http://schema.geolink.org/dev/voc/nvs/P02#MSIC">
        <rdfs:subClassOf rdf:resource="http://schema.geolink.org/dev/voc/nvs/P03#B045"/>
        <rdfs:subClassOf rdf:resource="http://schema.geolink.org/dev/voc/nvs/P03#B070"/>
        <rdfs:seeAlso rdf:resource="http://vocab.nerc.ac.uk/collection/P02/current/MSIC/"/>
        <rdfs:comment xml:lang="en">Integrated zooplankton (mesozooplankton and larger, exclusing fish, mammals, reptiles and insects) carbon biomass parameters</rdfs:comment>
        <rdfs:label xml:lang="en">Zooplankton carbon biomass per unit area of the water column</rdfs:label>
        <rdf:type rdf:resource="http://www.w3.org/2002/07/owl#NamedIndividual"/>
        <rdf:type rdf:resource="http://www.w3.org/2002/07/owl#Class"/>
      </glview:MeasurementType>
    </rdfs:subClassOf>
    <owl:someValuesFrom>
      <owl:Class>
        <owl:oneOf rdf:parseType="Collection">
          <glview:MeasurementType rdf:about="http://schema.geolink.org/dev/voc/nvs/P02#MSIC"/>
        </owl:oneOf>
      </owl:Class>
    </owl:someValuesFrom>
    <owl:onProperty rdf:resource="http://schema.geolink.org/dev/view#hasMeasurementType"/>
  </owl:Restriction>
  <owl:Restriction>
    <rdfs:subClassOf>
      <glview:MeasurementType rdf:about="http://schema.geolink.org/dev/voc/nvs/P02#TCNT">
        <rdfs:subClassOf rdf:resource="http://schema.geolink.org/dev/voc/nvs/P03#D025"/>
        <rdfs:seeAlso rdf:resource="http://vocab.nerc.ac.uk/collection/P02/current/TCNT/"/>
        <rdfs:comment xml:lang="en">Direct output parameters from TS instruments such as thermosalinograph or CTD</rdfs:comment>
        <rdfs:label xml:lang="en">Raw temperature and/or salinity instrument output</rdfs:label>
        <rdf:type rdf:resource="http://www.w3.org/2002/07/owl#NamedIndividual"/>
        <rdf:type rdf:resource="http://www.w3.org/2002/07/owl#Class"/>
      </glview:MeasurementType>
    </rdfs:subClassOf>
    <owl:someValuesFrom>
      <owl:Class>
        <owl:oneOf rdf:parseType="Collection">
          <glview:MeasurementType rdf:about="http://schema.geolink.org/dev/voc/nvs/P02#TCNT"/>
        </owl:oneOf>
      </owl:Class>
    </owl:someValuesFrom>
    <owl:onProperty rdf:resource="http://schema.geolink.org/dev/view#hasMeasurementType"/>
  </owl:Restriction>
  <owl:Restriction>
    <rdfs:subClassOf rdf:resource="http://schema.geolink.org/dev/voc/nvs/P02#ZNTP"/>
    <owl:someValuesFrom>
      <owl:Class>
        <owl:oneOf rdf:parseType="Collection">
          <glview:MeasurementType rdf:about="http://schema.geolink.org/dev/voc/nvs/P02#ZNTP"/>
        </owl:oneOf>
      </owl:Class>
    </owl:someValuesFrom>
    <owl:onProperty rdf:resource="http://schema.geolink.org/dev/view#hasMeasurementType"/>
  </owl:Restriction>
  <owl:Restriction>
    <rdfs:subClassOf>
      <glview:MeasurementType rdf:about="http://schema.geolink.org/dev/voc/nvs/P02#SRAD">
        <rdfs:subClassOf rdf:resource="http://schema.geolink.org/dev/voc/nvs/P03#C030"/>
        <rdfs:subClassOf rdf:resource="http://schema.geolink.org/dev/voc/nvs/P03#G035"/>
        <rdfs:seeAlso rdf:resource="http://vocab.nerc.ac.uk/collection/P02/current/SRAD/"/>
        <rdfs:comment xml:lang="en">Any parameters quantifying ionising radiation emitted by cores or samples comprising rock, sediment (including surface sediment such as fluff)</rdfs:comment>
        <rdfs:label xml:lang="en">Geological sample radioactivity</rdfs:label>
        <rdf:type rdf:resource="http://www.w3.org/2002/07/owl#NamedIndividual"/>
        <rdf:type rdf:resource="http://www.w3.org/2002/07/owl#Class"/>
      </glview:MeasurementType>
    </rdfs:subClassOf>
    <owl:someValuesFrom>
      <owl:Class>
        <owl:oneOf rdf:parseType="Collection">
          <glview:MeasurementType rdf:about="http://schema.geolink.org/dev/voc/nvs/P02#SRAD"/>
        </owl:oneOf>
      </owl:Class>
    </owl:someValuesFrom>
    <owl:onProperty rdf:resource="http://schema.geolink.org/dev/view#hasMeasurementType"/>
  </owl:Restriction>
  <owl:Restriction>
    <rdfs:subClassOf>
      <glview:MeasurementType rdf:about="http://schema.geolink.org/dev/voc/nvs/P02#SIPW">
        <rdfs:subClassOf rdf:resource="http://schema.geolink.org/dev/voc/nvs/P03#C030"/>
        <rdfs:subClassOf rdf:resource="http://schema.geolink.org/dev/voc/nvs/P03#G050"/>
        <rdfs:seeAlso rdf:resource="http://vocab.nerc.ac.uk/collection/P02/current/SIPW/"/>
        <rdfs:comment xml:lang="en">Parameters quantifying the relative proportions of stable isotopes in either the solute or solvent phase of sediment pore waters</rdfs:comment>
        <rdfs:label xml:lang="en">Stable isotope enrichment in sediment pore waters</rdfs:label>
        <rdf:type rdf:resource="http://www.w3.org/2002/07/owl#NamedIndividual"/>
        <rdf:type rdf:resource="http://www.w3.org/2002/07/owl#Class"/>
      </glview:MeasurementType>
    </rdfs:subClassOf>
    <owl:someValuesFrom>
      <owl:Class>
        <owl:oneOf rdf:parseType="Collection">
          <glview:MeasurementType rdf:about="http://schema.geolink.org/dev/voc/nvs/P02#SIPW"/>
        </owl:oneOf>
      </owl:Class>
    </owl:someValuesFrom>
    <owl:onProperty rdf:resource="http://schema.geolink.org/dev/view#hasMeasurementType"/>
  </owl:Restriction>
  <owl:Restriction>
    <rdfs:subClassOf>
      <glview:MeasurementType rdf:about="http://schema.geolink.org/dev/voc/nvs/P02#HFLW">
        <rdfs:subClassOf rdf:resource="http://schema.geolink.org/dev/voc/nvs/P03#GTHM"/>
        <rdfs:seeAlso rdf:resource="http://vocab.nerc.ac.uk/collection/P02/current/HFLW/"/>
        <rdfs:comment xml:lang="en">Parameters quantifying the  flux of thermal energy within the solid Earth or between the solid Earth and water bodies or atmosphere.</rdfs:comment>
        <rdfs:label xml:lang="en">Geothermal heat flow</rdfs:label>
        <rdf:type rdf:resource="http://www.w3.org/2002/07/owl#NamedIndividual"/>
        <rdf:type rdf:resource="http://www.w3.org/2002/07/owl#Class"/>
      </glview:MeasurementType>
    </rdfs:subClassOf>
    <owl:someValuesFrom>
      <owl:Class>
        <owl:oneOf rdf:parseType="Collection">
          <glview:MeasurementType rdf:about="http://schema.geolink.org/dev/voc/nvs/P02#HFLW"/>
        </owl:oneOf>
      </owl:Class>
    </owl:someValuesFrom>
    <owl:onProperty rdf:resource="http://schema.geolink.org/dev/view#hasMeasurementType"/>
  </owl:Restriction>
  <owl:Restriction>
    <rdfs:subClassOf>
      <glview:MeasurementType rdf:about="http://schema.geolink.org/dev/voc/nvs/P02#MDWD">
        <rdfs:subClassOf rdf:resource="http://schema.geolink.org/dev/voc/nvs/P03#C035"/>
        <rdfs:seeAlso rdf:resource="http://vocab.nerc.ac.uk/collection/P02/current/MDWD/"/>
        <rdfs:comment xml:lang="en">Concentration parameters for trace metalloid elements in the dissolved phase of the water column.  This may include a contribution from the particulate phase if this has not been totally removed by filtration and the metal in question is reactive (ie detected as if it were dissolved) to the analytical technique used. Trace metalloids are considered as B, Ge, As, Sb, Te and Po (but not Si which is classed separately because of its major role in environmental chemistry)</rdfs:comment>
        <rdfs:label xml:lang="en">Dissolved trace metalloid concentrations in the water column</rdfs:label>
        <rdf:type rdf:resource="http://www.w3.org/2002/07/owl#NamedIndividual"/>
        <rdf:type rdf:resource="http://www.w3.org/2002/07/owl#Class"/>
      </glview:MeasurementType>
    </rdfs:subClassOf>
    <owl:someValuesFrom>
      <owl:Class>
        <owl:oneOf rdf:parseType="Collection">
          <glview:MeasurementType rdf:about="http://schema.geolink.org/dev/voc/nvs/P02#MDWD"/>
        </owl:oneOf>
      </owl:Class>
    </owl:someValuesFrom>
    <owl:onProperty rdf:resource="http://schema.geolink.org/dev/view#hasMeasurementType"/>
  </owl:Restriction>
  <owl:Restriction>
    <rdfs:subClassOf>
      <glview:MeasurementType rdf:about="http://schema.geolink.org/dev/voc/nvs/P02#SCDO">
        <rdfs:subClassOf rdf:resource="http://schema.geolink.org/dev/voc/nvs/P03#O005"/>
        <rdfs:seeAlso rdf:resource="http://vocab.nerc.ac.uk/collection/P02/current/SCDO/"/>
        <rdfs:comment xml:lang="en">Parameters quantifying the exchange of metalsbetween the bed (ie the sediment) and the water column sometimes termed benthic fluxes</rdfs:comment>
        <rdfs:label xml:lang="en">Metal fluxes between the bed and the water column</rdfs:label>
        <rdf:type rdf:resource="http://www.w3.org/2002/07/owl#NamedIndividual"/>
        <rdf:type rdf:resource="http://www.w3.org/2002/07/owl#Class"/>
      </glview:MeasurementType>
    </rdfs:subClassOf>
    <owl:someValuesFrom>
      <owl:Class>
        <owl:oneOf rdf:parseType="Collection">
          <glview:MeasurementType rdf:about="http://schema.geolink.org/dev/voc/nvs/P02#SCDO"/>
        </owl:oneOf>
      </owl:Class>
    </owl:someValuesFrom>
    <owl:onProperty rdf:resource="http://schema.geolink.org/dev/view#hasMeasurementType"/>
  </owl:Restriction>
  <owl:Restriction>
    <rdfs:subClassOf>
      <glview:MeasurementType rdf:about="http://schema.geolink.org/dev/voc/nvs/P02#TFAA">
        <rdfs:subClassOf rdf:resource="http://schema.geolink.org/dev/voc/nvs/P03#C003"/>
        <rdfs:seeAlso rdf:resource="http://vocab.nerc.ac.uk/collection/P02/current/TFAA/"/>
        <rdfs:comment xml:lang="en">Parameters quantifying the amount of organic compounds containing both a carboxyl group and an amino group dissolved in a body of water.</rdfs:comment>
        <rdfs:label xml:lang="en">Dissolved amino acid concentrations in the water column</rdfs:label>
        <rdf:type rdf:resource="http://www.w3.org/2002/07/owl#NamedIndividual"/>
        <rdf:type rdf:resource="http://www.w3.org/2002/07/owl#Class"/>
      </glview:MeasurementType>
    </rdfs:subClassOf>
    <owl:someValuesFrom>
      <owl:Class>
        <owl:oneOf rdf:parseType="Collection">
          <glview:MeasurementType rdf:about="http://schema.geolink.org/dev/voc/nvs/P02#TFAA"/>
        </owl:oneOf>
      </owl:Class>
    </owl:someValuesFrom>
    <owl:onProperty rdf:resource="http://schema.geolink.org/dev/view#hasMeasurementType"/>
  </owl:Restriction>
  <owl:Restriction>
    <rdfs:subClassOf>
      <glview:MeasurementType rdf:about="http://schema.geolink.org/dev/voc/nvs/P02#MTIC">
        <rdfs:subClassOf rdf:resource="http://schema.geolink.org/dev/voc/nvs/P03#M015"/>
        <rdfs:subClassOf rdf:resource="http://schema.geolink.org/dev/voc/nvs/P03#C035"/>
        <rdfs:seeAlso rdf:resource="http://vocab.nerc.ac.uk/collection/P02/current/MTIC/"/>
        <rdfs:comment xml:lang="en">Concentration parameters for metallic elements in ice and snow</rdfs:comment>
        <rdfs:label xml:lang="en">Metal concentrations in the cryosphere</rdfs:label>
        <rdf:type rdf:resource="http://www.w3.org/2002/07/owl#NamedIndividual"/>
        <rdf:type rdf:resource="http://www.w3.org/2002/07/owl#Class"/>
      </glview:MeasurementType>
    </rdfs:subClassOf>
    <owl:someValuesFrom>
      <owl:Class>
        <owl:oneOf rdf:parseType="Collection">
          <glview:MeasurementType rdf:about="http://schema.geolink.org/dev/voc/nvs/P02#MTIC"/>
        </owl:oneOf>
      </owl:Class>
    </owl:someValuesFrom>
    <owl:onProperty rdf:resource="http://schema.geolink.org/dev/view#hasMeasurementType"/>
  </owl:Restriction>
  <owl:Restriction>
    <rdfs:subClassOf rdf:resource="http://schema.geolink.org/dev/voc/nvs/P02#OMPW"/>
    <owl:someValuesFrom>
      <owl:Class>
        <owl:oneOf rdf:parseType="Collection">
          <owl:NamedIndividual rdf:about="http://schema.geolink.org/dev/voc/nvs/P02#OMPW"/>
        </owl:oneOf>
      </owl:Class>
    </owl:someValuesFrom>
    <owl:onProperty rdf:resource="http://schema.geolink.org/dev/view#hasMeasurementType"/>
  </owl:Restriction>
  <owl:Restriction>
    <rdfs:subClassOf rdf:resource="http://schema.geolink.org/dev/voc/nvs/P02#SALK"/>
    <owl:someValuesFrom>
      <owl:Class>
        <owl:oneOf rdf:parseType="Collection">
          <glview:MeasurementType rdf:about="http://schema.geolink.org/dev/voc/nvs/P02#SALK"/>
        </owl:oneOf>
      </owl:Class>
    </owl:someValuesFrom>
    <owl:onProperty rdf:resource="http://schema.geolink.org/dev/view#hasMeasurementType"/>
  </owl:Restriction>
  <owl:Restriction>
    <rdfs:subClassOf>
      <glview:MeasurementType rdf:about="http://schema.geolink.org/dev/voc/nvs/P02#HBCH">
        <rdfs:subClassOf rdf:resource="http://schema.geolink.org/dev/voc/nvs/P03#B050"/>
        <rdfs:seeAlso rdf:resource="http://vocab.nerc.ac.uk/collection/P02/current/HBCH/"/>
        <rdfs:comment xml:lang="en">Parameters specifying the physical or chemical environment of a place where an organism is found.</rdfs:comment>
        <rdfs:label xml:lang="en">Habitat characterisation</rdfs:label>
        <rdf:type rdf:resource="http://www.w3.org/2002/07/owl#NamedIndividual"/>
        <rdf:type rdf:resource="http://www.w3.org/2002/07/owl#Class"/>
      </glview:MeasurementType>
    </rdfs:subClassOf>
    <owl:someValuesFrom>
      <owl:Class>
        <owl:oneOf rdf:parseType="Collection">
          <glview:MeasurementType rdf:about="http://schema.geolink.org/dev/voc/nvs/P02#HBCH"/>
        </owl:oneOf>
      </owl:Class>
    </owl:someValuesFrom>
    <owl:onProperty rdf:resource="http://schema.geolink.org/dev/view#hasMeasurementType"/>
  </owl:Restriction>
  <owl:Restriction>
    <rdfs:subClassOf rdf:resource="http://schema.geolink.org/dev/voc/nvs/P02#STMP"/>
    <owl:someValuesFrom>
      <owl:Class>
        <owl:oneOf rdf:parseType="Collection">
          <glview:MeasurementType rdf:about="http://schema.geolink.org/dev/voc/nvs/P02#STMP"/>
        </owl:oneOf>
      </owl:Class>
    </owl:someValuesFrom>
    <owl:onProperty rdf:resource="http://schema.geolink.org/dev/view#hasMeasurementType"/>
  </owl:Restriction>
  <owl:Restriction>
    <rdfs:subClassOf>
      <glview:MeasurementType rdf:about="http://schema.geolink.org/dev/voc/nvs/P02#AEYN">
        <rdfs:subClassOf rdf:resource="http://schema.geolink.org/dev/voc/nvs/P03#C025"/>
        <rdfs:subClassOf rdf:resource="http://schema.geolink.org/dev/voc/nvs/P03#M005"/>
        <rdfs:seeAlso rdf:resource="http://vocab.nerc.ac.uk/collection/P02/current/AEYN/"/>
        <rdfs:comment xml:lang="en">Alkene and alkyne concentrations in all phases of the atmosphere</rdfs:comment>
        <rdfs:label xml:lang="en">Concentration of alkenes and alkynes in the atmosphere</rdfs:label>
        <rdf:type rdf:resource="http://www.w3.org/2002/07/owl#NamedIndividual"/>
        <rdf:type rdf:resource="http://www.w3.org/2002/07/owl#Class"/>
      </glview:MeasurementType>
    </rdfs:subClassOf>
    <owl:someValuesFrom>
      <owl:Class>
        <owl:oneOf rdf:parseType="Collection">
          <glview:MeasurementType rdf:about="http://schema.geolink.org/dev/voc/nvs/P02#AEYN"/>
        </owl:oneOf>
      </owl:Class>
    </owl:someValuesFrom>
    <owl:onProperty rdf:resource="http://schema.geolink.org/dev/view#hasMeasurementType"/>
  </owl:Restriction>
  <owl:Restriction>
    <rdfs:subClassOf rdf:resource="http://schema.geolink.org/dev/voc/nvs/P02#MATX"/>
    <owl:someValuesFrom>
      <owl:Class>
        <owl:oneOf rdf:parseType="Collection">
          <glview:MeasurementType rdf:about="http://schema.geolink.org/dev/voc/nvs/P02#MATX"/>
        </owl:oneOf>
      </owl:Class>
    </owl:someValuesFrom>
    <owl:onProperty rdf:resource="http://schema.geolink.org/dev/view#hasMeasurementType"/>
  </owl:Restriction>
  <owl:Restriction>
    <rdfs:subClassOf>
      <glview:MeasurementType rdf:about="http://schema.geolink.org/dev/voc/nvs/P02#CBSP">
        <rdfs:subClassOf rdf:resource="http://schema.geolink.org/dev/voc/nvs/P03#G015"/>
        <rdfs:subClassOf rdf:resource="http://schema.geolink.org/dev/voc/nvs/P03#C005"/>
        <rdfs:seeAlso rdf:resource="http://vocab.nerc.ac.uk/collection/P02/current/CBSP/"/>
        <rdfs:comment xml:lang="en">Concentrations of total, organic and inorganic carbon per unit weight of suspended particulate material collected by water column filtration, centrifugation or sediment trapping.</rdfs:comment>
        <rdfs:label xml:lang="en">Carbon concentrations in suspended particulate material</rdfs:label>
        <rdf:type rdf:resource="http://www.w3.org/2002/07/owl#NamedIndividual"/>
        <rdf:type rdf:resource="http://www.w3.org/2002/07/owl#Class"/>
      </glview:MeasurementType>
    </rdfs:subClassOf>
    <owl:someValuesFrom>
      <owl:Class>
        <owl:oneOf rdf:parseType="Collection">
          <glview:MeasurementType rdf:about="http://schema.geolink.org/dev/voc/nvs/P02#CBSP"/>
        </owl:oneOf>
      </owl:Class>
    </owl:someValuesFrom>
    <owl:onProperty rdf:resource="http://schema.geolink.org/dev/view#hasMeasurementType"/>
  </owl:Restriction>
  <owl:Restriction>
    <rdfs:subClassOf rdf:resource="http://schema.geolink.org/dev/voc/nvs/P02#MFAZ"/>
    <owl:someValuesFrom>
      <owl:Class>
        <owl:oneOf rdf:parseType="Collection">
          <glview:MeasurementType rdf:about="http://schema.geolink.org/dev/voc/nvs/P02#MFAZ"/>
        </owl:oneOf>
      </owl:Class>
    </owl:someValuesFrom>
    <owl:onProperty rdf:resource="http://schema.geolink.org/dev/view#hasMeasurementType"/>
  </owl:Restriction>
  <owl:Restriction>
    <rdfs:subClassOf>
      <glview:MeasurementType rdf:about="http://schema.geolink.org/dev/voc/nvs/P02#HLDE">
        <rdfs:subClassOf rdf:resource="http://schema.geolink.org/dev/voc/nvs/P03#C020"/>
        <rdfs:seeAlso rdf:resource="http://vocab.nerc.ac.uk/collection/P02/current/HLDE/"/>
        <rdfs:comment xml:lang="en">Parameters relating to the rates of creation and consumption of volatile halocarbons (compounds comprising carbon atoms covalently bonded to fluorine, chlorine, bromine or iodine atoms) other than tracers (i.e. freons/chlorofluorocarbons) and contaminants in any body of fresh or salt water.</rdfs:comment>
        <rdfs:label xml:lang="en">Other halocarbon dynamics in water bodies</rdfs:label>
        <rdf:type rdf:resource="http://www.w3.org/2002/07/owl#NamedIndividual"/>
        <rdf:type rdf:resource="http://www.w3.org/2002/07/owl#Class"/>
      </glview:MeasurementType>
    </rdfs:subClassOf>
    <owl:someValuesFrom>
      <owl:Class>
        <owl:oneOf rdf:parseType="Collection">
          <glview:MeasurementType rdf:about="http://schema.geolink.org/dev/voc/nvs/P02#HLDE"/>
        </owl:oneOf>
      </owl:Class>
    </owl:someValuesFrom>
    <owl:onProperty rdf:resource="http://schema.geolink.org/dev/view#hasMeasurementType"/>
  </owl:Restriction>
  <owl:Restriction>
    <rdfs:subClassOf rdf:resource="http://schema.geolink.org/dev/voc/nvs/P02#MSIC"/>
    <owl:someValuesFrom>
      <owl:Class>
        <owl:oneOf rdf:parseType="Collection">
          <glview:MeasurementType rdf:about="http://schema.geolink.org/dev/voc/nvs/P02#MSIC"/>
        </owl:oneOf>
      </owl:Class>
    </owl:someValuesFrom>
    <owl:onProperty rdf:resource="http://schema.geolink.org/dev/view#hasMeasurementType"/>
  </owl:Restriction>
  <owl:Restriction>
    <rdfs:subClassOf>
      <glview:MeasurementType rdf:about="http://schema.geolink.org/dev/voc/nvs/P02#SEMP">
        <rdfs:subClassOf rdf:resource="http://schema.geolink.org/dev/voc/nvs/P03#B015"/>
        <rdfs:seeAlso rdf:resource="http://vocab.nerc.ac.uk/collection/P02/current/SEMP/"/>
        <rdfs:comment xml:lang="en">Parameters describing the size, shape or physiological activity including disease and parasite infection status of seals (Family Phocidae). Includes both parameters mapped to taxa and those mapped to non-taxonomic groupings.</rdfs:comment>
        <rdfs:label xml:lang="en">Seal morphology and physiology</rdfs:label>
        <rdf:type rdf:resource="http://www.w3.org/2002/07/owl#NamedIndividual"/>
        <rdf:type rdf:resource="http://www.w3.org/2002/07/owl#Class"/>
      </glview:MeasurementType>
    </rdfs:subClassOf>
    <owl:someValuesFrom>
      <owl:Class>
        <owl:oneOf rdf:parseType="Collection">
          <glview:MeasurementType rdf:about="http://schema.geolink.org/dev/voc/nvs/P02#SEMP"/>
        </owl:oneOf>
      </owl:Class>
    </owl:someValuesFrom>
    <owl:onProperty rdf:resource="http://schema.geolink.org/dev/view#hasMeasurementType"/>
  </owl:Restriction>
  <owl:Restriction>
    <rdfs:subClassOf>
      <glview:MeasurementType rdf:about="http://schema.geolink.org/dev/voc/nvs/P02#WCPH">
        <rdfs:subClassOf rdf:resource="http://schema.geolink.org/dev/voc/nvs/P03#UWPH"/>
        <rdfs:seeAlso rdf:resource="http://vocab.nerc.ac.uk/collection/P02/current/WCPH/"/>
        <rdfs:comment xml:lang="en">Digital images of the water column obtained using either still or video cameras</rdfs:comment>
        <rdfs:label xml:lang="en">Water column photography</rdfs:label>
        <rdf:type rdf:resource="http://www.w3.org/2002/07/owl#NamedIndividual"/>
        <rdf:type rdf:resource="http://www.w3.org/2002/07/owl#Class"/>
      </glview:MeasurementType>
    </rdfs:subClassOf>
    <owl:someValuesFrom>
      <owl:Class>
        <owl:oneOf rdf:parseType="Collection">
          <glview:MeasurementType rdf:about="http://schema.geolink.org/dev/voc/nvs/P02#WCPH"/>
        </owl:oneOf>
      </owl:Class>
    </owl:someValuesFrom>
    <owl:onProperty rdf:resource="http://schema.geolink.org/dev/view#hasMeasurementType"/>
  </owl:Restriction>
  <owl:Restriction>
    <rdfs:subClassOf rdf:resource="http://schema.geolink.org/dev/voc/nvs/P02#AEYN"/>
    <owl:someValuesFrom>
      <owl:Class>
        <owl:oneOf rdf:parseType="Collection">
          <glview:MeasurementType rdf:about="http://schema.geolink.org/dev/voc/nvs/P02#AEYN"/>
        </owl:oneOf>
      </owl:Class>
    </owl:someValuesFrom>
    <owl:onProperty rdf:resource="http://schema.geolink.org/dev/view#hasMeasurementType"/>
  </owl:Restriction>
  <owl:Restriction>
    <rdfs:subClassOf>
      <glview:MeasurementType rdf:about="http://schema.geolink.org/dev/voc/nvs/P02#MTWD">
        <rdfs:subClassOf rdf:resource="http://schema.geolink.org/dev/voc/nvs/P03#C035"/>
        <rdfs:seeAlso rdf:resource="http://vocab.nerc.ac.uk/collection/P02/current/MTWD/"/>
        <rdfs:comment xml:lang="en">Concentrations of metal elements in the dissolved phase of the water column.  This may include a contribution from the particulate phase if this has not been totally removed by filtration and the metal in question is reactive (ie detected as if it were dissolved) to the analytical technique used.</rdfs:comment>
        <rdfs:label xml:lang="en">Dissolved metal concentrations in the water column</rdfs:label>
        <rdf:type rdf:resource="http://www.w3.org/2002/07/owl#NamedIndividual"/>
        <rdf:type rdf:resource="http://www.w3.org/2002/07/owl#Class"/>
      </glview:MeasurementType>
    </rdfs:subClassOf>
    <owl:someValuesFrom>
      <owl:Class>
        <owl:oneOf rdf:parseType="Collection">
          <glview:MeasurementType rdf:about="http://schema.geolink.org/dev/voc/nvs/P02#MTWD"/>
        </owl:oneOf>
      </owl:Class>
    </owl:someValuesFrom>
    <owl:onProperty rdf:resource="http://schema.geolink.org/dev/view#hasMeasurementType"/>
  </owl:Restriction>
  <owl:Restriction>
    <rdfs:subClassOf>
      <glview:MeasurementType rdf:about="http://schema.geolink.org/dev/voc/nvs/P02#APDA">
        <rdfs:subClassOf rdf:resource="http://schema.geolink.org/dev/voc/nvs/P03#Z005"/>
        <rdfs:seeAlso rdf:resource="http://vocab.nerc.ac.uk/collection/P02/current/APDA/"/>
        <rdfs:comment xml:lang="en">All parameters relating to horizontal platform travel, including distance run</rdfs:comment>
        <rdfs:label xml:lang="en">Horizontal platform movement</rdfs:label>
        <rdf:type rdf:resource="http://www.w3.org/2002/07/owl#NamedIndividual"/>
        <rdf:type rdf:resource="http://www.w3.org/2002/07/owl#Class"/>
      </glview:MeasurementType>
    </rdfs:subClassOf>
    <owl:someValuesFrom>
      <owl:Class>
        <owl:oneOf rdf:parseType="Collection">
          <glview:MeasurementType rdf:about="http://schema.geolink.org/dev/voc/nvs/P02#APDA"/>
        </owl:oneOf>
      </owl:Class>
    </owl:someValuesFrom>
    <owl:onProperty rdf:resource="http://schema.geolink.org/dev/view#hasMeasurementType"/>
  </owl:Restriction>
  <owl:Restriction>
    <rdfs:subClassOf rdf:resource="http://schema.geolink.org/dev/voc/nvs/P02#SIPW"/>
    <owl:someValuesFrom>
      <owl:Class>
        <owl:oneOf rdf:parseType="Collection">
          <glview:MeasurementType rdf:about="http://schema.geolink.org/dev/voc/nvs/P02#SIPW"/>
        </owl:oneOf>
      </owl:Class>
    </owl:someValuesFrom>
    <owl:onProperty rdf:resource="http://schema.geolink.org/dev/view#hasMeasurementType"/>
  </owl:Restriction>
  <owl:Restriction>
    <rdfs:subClassOf>
      <glview:MeasurementType rdf:about="http://schema.geolink.org/dev/voc/nvs/P02#OXYC">
        <rdfs:subClassOf rdf:resource="http://schema.geolink.org/dev/voc/nvs/P03#C015"/>
        <rdfs:seeAlso rdf:resource="http://vocab.nerc.ac.uk/collection/P02/current/OXYC/"/>
        <rdfs:comment xml:lang="en">Raw parameters (usually membrane current and temperature) from dissolved oxygen sensors</rdfs:comment>
        <rdfs:label xml:lang="en">Raw oxygen sensor output</rdfs:label>
        <rdf:type rdf:resource="http://www.w3.org/2002/07/owl#NamedIndividual"/>
        <rdf:type rdf:resource="http://www.w3.org/2002/07/owl#Class"/>
      </glview:MeasurementType>
    </rdfs:subClassOf>
    <owl:someValuesFrom>
      <owl:Class>
        <owl:oneOf rdf:parseType="Collection">
          <glview:MeasurementType rdf:about="http://schema.geolink.org/dev/voc/nvs/P02#OXYC"/>
        </owl:oneOf>
      </owl:Class>
    </owl:someValuesFrom>
    <owl:onProperty rdf:resource="http://schema.geolink.org/dev/view#hasMeasurementType"/>
  </owl:Restriction>
  <owl:Restriction>
    <rdfs:subClassOf>
      <glview:MeasurementType rdf:about="http://schema.geolink.org/dev/voc/nvs/P02#SECC">
        <rdfs:subClassOf rdf:resource="http://schema.geolink.org/dev/voc/nvs/P03#D015"/>
        <rdfs:seeAlso rdf:resource="http://vocab.nerc.ac.uk/collection/P02/current/SECC/"/>
        <rdfs:comment xml:lang="en">Measurements of optical visibility in the water column</rdfs:comment>
        <rdfs:label xml:lang="en">Secchi disk depth</rdfs:label>
        <rdf:type rdf:resource="http://www.w3.org/2002/07/owl#NamedIndividual"/>
        <rdf:type rdf:resource="http://www.w3.org/2002/07/owl#Class"/>
      </glview:MeasurementType>
    </rdfs:subClassOf>
    <owl:someValuesFrom>
      <owl:Class>
        <owl:oneOf rdf:parseType="Collection">
          <glview:MeasurementType rdf:about="http://schema.geolink.org/dev/voc/nvs/P02#SECC"/>
        </owl:oneOf>
      </owl:Class>
    </owl:someValuesFrom>
    <owl:onProperty rdf:resource="http://schema.geolink.org/dev/view#hasMeasurementType"/>
  </owl:Restriction>
  <owl:Restriction>
    <rdfs:subClassOf>
      <glview:MeasurementType rdf:about="http://schema.geolink.org/dev/voc/nvs/P02#R410">
        <rdfs:subClassOf rdf:resource="http://schema.geolink.org/dev/voc/nvs/P03#D015"/>
        <rdfs:seeAlso rdf:resource="http://vocab.nerc.ac.uk/collection/P02/current/R410/"/>
        <rdfs:comment xml:lang="en">Parameters associated with the measurement of ocean colour, including visible waveband satellite spectral radiometer measurements, their calibration measurements (spectral water-leaving radiance and reflectance) and chart colour estimates.</rdfs:comment>
        <rdfs:label xml:lang="en">Ocean colour and earth-leaving visible waveband spectral radiation</rdfs:label>
        <rdf:type rdf:resource="http://www.w3.org/2002/07/owl#NamedIndividual"/>
        <rdf:type rdf:resource="http://www.w3.org/2002/07/owl#Class"/>
      </glview:MeasurementType>
    </rdfs:subClassOf>
    <owl:someValuesFrom>
      <owl:Class>
        <owl:oneOf rdf:parseType="Collection">
          <glview:MeasurementType rdf:about="http://schema.geolink.org/dev/voc/nvs/P02#R410"/>
        </owl:oneOf>
      </owl:Class>
    </owl:someValuesFrom>
    <owl:onProperty rdf:resource="http://schema.geolink.org/dev/view#hasMeasurementType"/>
  </owl:Restriction>
  <owl:Restriction>
    <rdfs:subClassOf>
      <glview:MeasurementType rdf:about="http://schema.geolink.org/dev/voc/nvs/P02#BCPB">
        <rdfs:subClassOf rdf:resource="http://schema.geolink.org/dev/voc/nvs/P03#C055"/>
        <rdfs:subClassOf rdf:resource="http://schema.geolink.org/dev/voc/nvs/P03#B007"/>
        <rdfs:subClassOf rdf:resource="http://schema.geolink.org/dev/voc/nvs/P03#H001"/>
        <rdfs:seeAlso rdf:resource="http://vocab.nerc.ac.uk/collection/P02/current/BCPB/"/>
        <rdfs:comment xml:lang="en">PCB concentrations in either whole organisms or their constituent parts</rdfs:comment>
        <rdfs:label xml:lang="en">Concentration of polychlorobiphenyls (PCBs) in biota</rdfs:label>
        <rdf:type rdf:resource="http://www.w3.org/2002/07/owl#NamedIndividual"/>
        <rdf:type rdf:resource="http://www.w3.org/2002/07/owl#Class"/>
      </glview:MeasurementType>
    </rdfs:subClassOf>
    <owl:someValuesFrom>
      <owl:Class>
        <owl:oneOf rdf:parseType="Collection">
          <glview:MeasurementType rdf:about="http://schema.geolink.org/dev/voc/nvs/P02#BCPB"/>
        </owl:oneOf>
      </owl:Class>
    </owl:someValuesFrom>
    <owl:onProperty rdf:resource="http://schema.geolink.org/dev/view#hasMeasurementType"/>
  </owl:Restriction>
  <owl:Restriction>
    <rdfs:subClassOf>
      <glview:MeasurementType rdf:about="http://schema.geolink.org/dev/voc/nvs/P02#AAFX">
        <rdfs:subClassOf rdf:resource="http://schema.geolink.org/dev/voc/nvs/P03#O005"/>
        <rdfs:subClassOf rdf:resource="http://schema.geolink.org/dev/voc/nvs/P03#C003"/>
        <rdfs:seeAlso rdf:resource="http://vocab.nerc.ac.uk/collection/P02/current/AAFX/"/>
        <rdfs:comment xml:lang="en">Parameters quantifying the amount of organic compounds containing both a carboxyl group and an amino group (including compounds such as salts and esters) sinking vertically as particles through a unit area of a water body in units time.</rdfs:comment>
        <rdfs:label xml:lang="en">Sedimentation flux of amino acids and associated compounds in water bodies</rdfs:label>
        <rdf:type rdf:resource="http://www.w3.org/2002/07/owl#NamedIndividual"/>
        <rdf:type rdf:resource="http://www.w3.org/2002/07/owl#Class"/>
      </glview:MeasurementType>
    </rdfs:subClassOf>
    <owl:someValuesFrom>
      <owl:Class>
        <owl:oneOf rdf:parseType="Collection">
          <glview:MeasurementType rdf:about="http://schema.geolink.org/dev/voc/nvs/P02#AAFX"/>
        </owl:oneOf>
      </owl:Class>
    </owl:someValuesFrom>
    <owl:onProperty rdf:resource="http://schema.geolink.org/dev/view#hasMeasurementType"/>
  </owl:Restriction>
  <owl:Restriction>
    <rdfs:subClassOf>
      <glview:MeasurementType rdf:about="http://schema.geolink.org/dev/voc/nvs/P02#WPRO">
        <rdfs:subClassOf rdf:resource="http://schema.geolink.org/dev/voc/nvs/P03#C050"/>
        <rdfs:seeAlso rdf:resource="http://vocab.nerc.ac.uk/collection/P02/current/WPRO/"/>
        <rdfs:comment xml:lang="en">Concentrations of proteins in all phases of the water column</rdfs:comment>
        <rdfs:label xml:lang="en">Concentration of proteins in the water column</rdfs:label>
        <rdf:type rdf:resource="http://www.w3.org/2002/07/owl#NamedIndividual"/>
        <rdf:type rdf:resource="http://www.w3.org/2002/07/owl#Class"/>
      </glview:MeasurementType>
    </rdfs:subClassOf>
    <owl:someValuesFrom>
      <owl:Class>
        <owl:oneOf rdf:parseType="Collection">
          <glview:MeasurementType rdf:about="http://schema.geolink.org/dev/voc/nvs/P02#WPRO"/>
        </owl:oneOf>
      </owl:Class>
    </owl:someValuesFrom>
    <owl:onProperty rdf:resource="http://schema.geolink.org/dev/view#hasMeasurementType"/>
  </owl:Restriction>
  <owl:Restriction>
    <rdfs:subClassOf>
      <glview:MeasurementType rdf:about="http://schema.geolink.org/dev/voc/nvs/P02#PXSP">
        <rdfs:subClassOf rdf:resource="http://schema.geolink.org/dev/voc/nvs/P03#G015"/>
        <rdfs:subClassOf rdf:resource="http://schema.geolink.org/dev/voc/nvs/P03#C005"/>
        <rdfs:seeAlso rdf:resource="http://vocab.nerc.ac.uk/collection/P02/current/PXSP/"/>
        <rdfs:comment xml:lang="en">Concentrations of total, organic and inorganic phosphorus per unit weight of suspended particulate material collected by water column filtration, centrifugation or sediment trapping.</rdfs:comment>
        <rdfs:label xml:lang="en">Phosphorus concentrations in suspended particulate material</rdfs:label>
        <rdf:type rdf:resource="http://www.w3.org/2002/07/owl#NamedIndividual"/>
        <rdf:type rdf:resource="http://www.w3.org/2002/07/owl#Class"/>
      </glview:MeasurementType>
    </rdfs:subClassOf>
    <owl:someValuesFrom>
      <owl:Class>
        <owl:oneOf rdf:parseType="Collection">
          <glview:MeasurementType rdf:about="http://schema.geolink.org/dev/voc/nvs/P02#PXSP"/>
        </owl:oneOf>
      </owl:Class>
    </owl:someValuesFrom>
    <owl:onProperty rdf:resource="http://schema.geolink.org/dev/view#hasMeasurementType"/>
  </owl:Restriction>
  <owl:Restriction>
    <rdfs:subClassOf>
      <glview:MeasurementType rdf:about="http://schema.geolink.org/dev/voc/nvs/P02#LITT">
        <rdfs:subClassOf rdf:resource="http://schema.geolink.org/dev/voc/nvs/P03#H001"/>
        <rdfs:seeAlso rdf:resource="http://vocab.nerc.ac.uk/collection/P02/current/LITT/"/>
        <rdfs:comment xml:lang="en">Parameters describing the abundance and nature of material classed as refuse introduced to the environment by activities of man.</rdfs:comment>
        <rdfs:label xml:lang="en">Litter abundance and type</rdfs:label>
        <rdf:type rdf:resource="http://www.w3.org/2002/07/owl#NamedIndividual"/>
        <rdf:type rdf:resource="http://www.w3.org/2002/07/owl#Class"/>
      </glview:MeasurementType>
    </rdfs:subClassOf>
    <owl:someValuesFrom>
      <owl:Class>
        <owl:oneOf rdf:parseType="Collection">
          <glview:MeasurementType rdf:about="http://schema.geolink.org/dev/voc/nvs/P02#LITT"/>
        </owl:oneOf>
      </owl:Class>
    </owl:someValuesFrom>
    <owl:onProperty rdf:resource="http://schema.geolink.org/dev/view#hasMeasurementType"/>
  </owl:Restriction>
  <owl:Restriction>
    <rdfs:subClassOf>
      <glview:MeasurementType rdf:about="http://schema.geolink.org/dev/voc/nvs/P02#MTWP">
        <rdfs:subClassOf rdf:resource="http://schema.geolink.org/dev/voc/nvs/P03#C035"/>
        <rdfs:subClassOf rdf:resource="http://schema.geolink.org/dev/voc/nvs/P03#G015"/>
        <rdfs:seeAlso rdf:resource="http://vocab.nerc.ac.uk/collection/P02/current/MTWP/"/>
        <rdfs:comment xml:lang="en">Concentration parameters for metallic elements in the particulate phase of the water column collected by fitration, centrifugation or sediment trapping</rdfs:comment>
        <rdfs:label xml:lang="en">Particulate metal concentrations in the water column</rdfs:label>
        <rdf:type rdf:resource="http://www.w3.org/2002/07/owl#NamedIndividual"/>
        <rdf:type rdf:resource="http://www.w3.org/2002/07/owl#Class"/>
      </glview:MeasurementType>
    </rdfs:subClassOf>
    <owl:someValuesFrom>
      <owl:Class>
        <owl:oneOf rdf:parseType="Collection">
          <glview:MeasurementType rdf:about="http://schema.geolink.org/dev/voc/nvs/P02#MTWP"/>
        </owl:oneOf>
      </owl:Class>
    </owl:someValuesFrom>
    <owl:onProperty rdf:resource="http://schema.geolink.org/dev/view#hasMeasurementType"/>
  </owl:Restriction>
  <owl:Restriction>
    <rdfs:subClassOf>
      <glview:MeasurementType rdf:about="http://schema.geolink.org/dev/voc/nvs/P02#ATTN">
        <rdfs:subClassOf rdf:resource="http://schema.geolink.org/dev/voc/nvs/P03#D015"/>
        <rdfs:seeAlso rdf:resource="http://vocab.nerc.ac.uk/collection/P02/current/ATTN/"/>
        <rdfs:comment xml:lang="en">Parameters relating to the rate of electromagnetic radiation intensity decrease as it travels through the water column</rdfs:comment>
        <rdfs:label xml:lang="en">Transmittance and attenuance of the water column</rdfs:label>
        <rdf:type rdf:resource="http://www.w3.org/2002/07/owl#NamedIndividual"/>
        <rdf:type rdf:resource="http://www.w3.org/2002/07/owl#Class"/>
      </glview:MeasurementType>
    </rdfs:subClassOf>
    <owl:someValuesFrom>
      <owl:Class>
        <owl:oneOf rdf:parseType="Collection">
          <glview:MeasurementType rdf:about="http://schema.geolink.org/dev/voc/nvs/P02#ATTN"/>
        </owl:oneOf>
      </owl:Class>
    </owl:someValuesFrom>
    <owl:onProperty rdf:resource="http://schema.geolink.org/dev/view#hasMeasurementType"/>
  </owl:Restriction>
  <owl:Restriction>
    <rdfs:subClassOf>
      <owl:NamedIndividual rdf:about="http://schema.geolink.org/dev/voc/nvs/P02#BCAH">
        <rdfs:subClassOf rdf:resource="http://schema.geolink.org/dev/voc/nvs/P03#C025"/>
        <rdfs:subClassOf rdf:resource="http://schema.geolink.org/dev/voc/nvs/P03#B007"/>
        <rdfs:subClassOf rdf:resource="http://schema.geolink.org/dev/voc/nvs/P03#C055"/>
        <rdf:type rdf:resource="http://schema.geolink.org/dev/view#MeasurementType"/>
        <rdfs:label xml:lang="en">Concentration of polycyclic aromatic hydrocarbons (PAHs) in biota</rdfs:label>
        <rdf:type rdf:resource="http://www.w3.org/2002/07/owl#Class"/>
        <rdfs:seeAlso rdf:resource="http://vocab.nerc.ac.uk/collection/P02/current/BCAH/"/>
        <rdfs:subClassOf rdf:resource="http://schema.geolink.org/dev/voc/nvs/P03#H001"/>
        <rdfs:comment xml:lang="en">PAH concentrations in either whole organisms or their constituent parts</rdfs:comment>
      </owl:NamedIndividual>
    </rdfs:subClassOf>
    <owl:someValuesFrom>
      <owl:Class>
        <owl:oneOf rdf:parseType="Collection">
          <owl:NamedIndividual rdf:about="http://schema.geolink.org/dev/voc/nvs/P02#BCAH"/>
        </owl:oneOf>
      </owl:Class>
    </owl:someValuesFrom>
    <owl:onProperty rdf:resource="http://schema.geolink.org/dev/view#hasMeasurementType"/>
  </owl:Restriction>
  <owl:Restriction>
    <rdfs:subClassOf>
      <glview:MeasurementType rdf:about="http://schema.geolink.org/dev/voc/nvs/P02#MSBD">
        <rdfs:subClassOf rdf:resource="http://schema.geolink.org/dev/voc/nvs/P03#B045"/>
        <rdfs:subClassOf rdf:resource="http://schema.geolink.org/dev/voc/nvs/P03#B070"/>
        <rdfs:seeAlso rdf:resource="http://vocab.nerc.ac.uk/collection/P02/current/MSBD/"/>
        <rdfs:comment xml:lang="en">Zooplankton (mesozooplankton and larger, exclusing fish, mammals, reptiles and insects) biomass determined by drying to constant weight.</rdfs:comment>
        <rdfs:label xml:lang="en">Zooplankton dry weight biomass per unit volume of the water column</rdfs:label>
        <rdf:type rdf:resource="http://www.w3.org/2002/07/owl#NamedIndividual"/>
        <rdf:type rdf:resource="http://www.w3.org/2002/07/owl#Class"/>
      </glview:MeasurementType>
    </rdfs:subClassOf>
    <owl:someValuesFrom>
      <owl:Class>
        <owl:oneOf rdf:parseType="Collection">
          <glview:MeasurementType rdf:about="http://schema.geolink.org/dev/voc/nvs/P02#MSBD"/>
        </owl:oneOf>
      </owl:Class>
    </owl:someValuesFrom>
    <owl:onProperty rdf:resource="http://schema.geolink.org/dev/view#hasMeasurementType"/>
  </owl:Restriction>
  <owl:Restriction>
    <rdfs:subClassOf>
      <glview:MeasurementType rdf:about="http://schema.geolink.org/dev/voc/nvs/P02#MTWC">
        <rdfs:subClassOf rdf:resource="http://schema.geolink.org/dev/voc/nvs/P03#C035"/>
        <rdfs:seeAlso rdf:resource="http://vocab.nerc.ac.uk/collection/P02/current/MTWC/"/>
        <rdfs:comment xml:lang="en">Concentrations of metal elements in the colloidal phase of the water column. Usually the dissolved concentration difference between conventionally filtered water and ultra-filtered water.</rdfs:comment>
        <rdfs:label xml:lang="en">Colloidal metal concentrations in the water column</rdfs:label>
        <rdf:type rdf:resource="http://www.w3.org/2002/07/owl#NamedIndividual"/>
        <rdf:type rdf:resource="http://www.w3.org/2002/07/owl#Class"/>
      </glview:MeasurementType>
    </rdfs:subClassOf>
    <owl:someValuesFrom>
      <owl:Class>
        <owl:oneOf rdf:parseType="Collection">
          <glview:MeasurementType rdf:about="http://schema.geolink.org/dev/voc/nvs/P02#MTWC"/>
        </owl:oneOf>
      </owl:Class>
    </owl:someValuesFrom>
    <owl:onProperty rdf:resource="http://schema.geolink.org/dev/view#hasMeasurementType"/>
  </owl:Restriction>
  <owl:Restriction>
    <rdfs:subClassOf rdf:resource="http://schema.geolink.org/dev/voc/nvs/P02#ADUN"/>
    <owl:someValuesFrom>
      <owl:Class>
        <owl:oneOf rdf:parseType="Collection">
          <owl:NamedIndividual rdf:about="http://schema.geolink.org/dev/voc/nvs/P02#ADUN"/>
        </owl:oneOf>
      </owl:Class>
    </owl:someValuesFrom>
    <owl:onProperty rdf:resource="http://schema.geolink.org/dev/view#hasMeasurementType"/>
  </owl:Restriction>
  <owl:Restriction>
    <rdfs:subClassOf>
      <glview:MeasurementType rdf:about="http://schema.geolink.org/dev/voc/nvs/P02#GREF">
        <rdfs:subClassOf rdf:resource="http://schema.geolink.org/dev/voc/nvs/P03#O010"/>
        <rdfs:subClassOf rdf:resource="http://schema.geolink.org/dev/voc/nvs/P03#B005"/>
        <rdfs:seeAlso rdf:resource="http://vocab.nerc.ac.uk/collection/P02/current/GREF/"/>
        <rdfs:comment></rdfs:comment>
        <rdfs:label xml:lang="en">Bacterial growth</rdfs:label>
        <rdf:type rdf:resource="http://www.w3.org/2002/07/owl#NamedIndividual"/>
        <rdf:type rdf:resource="http://www.w3.org/2002/07/owl#Class"/>
      </glview:MeasurementType>
    </rdfs:subClassOf>
    <owl:someValuesFrom>
      <owl:Class>
        <owl:oneOf rdf:parseType="Collection">
          <glview:MeasurementType rdf:about="http://schema.geolink.org/dev/voc/nvs/P02#GREF"/>
        </owl:oneOf>
      </owl:Class>
    </owl:someValuesFrom>
    <owl:onProperty rdf:resource="http://schema.geolink.org/dev/view#hasMeasurementType"/>
  </owl:Restriction>
  <owl:Restriction>
    <rdfs:subClassOf>
      <glview:MeasurementType rdf:about="http://schema.geolink.org/dev/voc/nvs/P02#PHSD">
        <rdfs:subClassOf rdf:resource="http://schema.geolink.org/dev/voc/nvs/P03#B035"/>
        <rdfs:subClassOf rdf:resource="http://schema.geolink.org/dev/voc/nvs/P03#G035"/>
        <rdfs:seeAlso rdf:resource="http://vocab.nerc.ac.uk/collection/P02/current/PHSD/"/>
        <rdfs:comment xml:lang="en">Includes all variants of phaeopigment (chlorophyll degradation products). Sediment is defined as any solids collected by a corer, including fluff..</rdfs:comment>
        <rdfs:label xml:lang="en">Phaeopigment concentrations in sediment</rdfs:label>
        <rdf:type rdf:resource="http://www.w3.org/2002/07/owl#NamedIndividual"/>
        <rdf:type rdf:resource="http://www.w3.org/2002/07/owl#Class"/>
      </glview:MeasurementType>
    </rdfs:subClassOf>
    <owl:someValuesFrom>
      <owl:Class>
        <owl:oneOf rdf:parseType="Collection">
          <glview:MeasurementType rdf:about="http://schema.geolink.org/dev/voc/nvs/P02#PHSD"/>
        </owl:oneOf>
      </owl:Class>
    </owl:someValuesFrom>
    <owl:onProperty rdf:resource="http://schema.geolink.org/dev/view#hasMeasurementType"/>
  </owl:Restriction>
  <owl:Restriction>
    <rdfs:subClassOf>
      <glview:MeasurementType rdf:about="http://schema.geolink.org/dev/voc/nvs/P02#CRYS">
        <rdfs:subClassOf rdf:resource="http://schema.geolink.org/dev/voc/nvs/P03#M015"/>
        <rdfs:seeAlso rdf:resource="http://vocab.nerc.ac.uk/collection/P02/current/CRYS/"/>
        <rdfs:comment xml:lang="en">Measurements of quantity (mass), thickness and spatial extent of snow and ice</rdfs:comment>
        <rdfs:label xml:lang="en">Snow and ice mass, thickness and extent</rdfs:label>
        <rdf:type rdf:resource="http://www.w3.org/2002/07/owl#NamedIndividual"/>
        <rdf:type rdf:resource="http://www.w3.org/2002/07/owl#Class"/>
      </glview:MeasurementType>
    </rdfs:subClassOf>
    <owl:someValuesFrom>
      <owl:Class>
        <owl:oneOf rdf:parseType="Collection">
          <glview:MeasurementType rdf:about="http://schema.geolink.org/dev/voc/nvs/P02#CRYS"/>
        </owl:oneOf>
      </owl:Class>
    </owl:someValuesFrom>
    <owl:onProperty rdf:resource="http://schema.geolink.org/dev/view#hasMeasurementType"/>
  </owl:Restriction>
  <owl:Restriction>
    <rdfs:subClassOf>
      <glview:MeasurementType rdf:about="http://schema.geolink.org/dev/voc/nvs/P02#PXSD">
        <rdfs:subClassOf>
          <glview:MeasurementType rdf:about="http://schema.geolink.org/dev/voc/nvs/P02#RMIN">
            <rdfs:subClassOf rdf:resource="http://schema.geolink.org/dev/voc/nvs/P03#C045"/>
            <rdfs:subClassOf rdf:resource="http://schema.geolink.org/dev/voc/nvs/P03#G035"/>
            <rdfs:seeAlso rdf:resource="http://vocab.nerc.ac.uk/collection/P02/current/RMIN/"/>
            <rdfs:comment xml:lang="en">Parameters specifying the proportions of inorganic components (major/minor/trace elements, trace metals etc.) in sediment or rock samples.  Major elements includes the H2O+ and H2O- parameters reported by convention in oxide weight per cent geochemical major element analyses.</rdfs:comment>
            <rdfs:label xml:lang="en">Inorganic chemical composition of sediment or rocks</rdfs:label>
            <rdf:type rdf:resource="http://www.w3.org/2002/07/owl#NamedIndividual"/>
            <rdf:type rdf:resource="http://www.w3.org/2002/07/owl#Class"/>
          </glview:MeasurementType>
        </rdfs:subClassOf>
        <rdfs:seeAlso rdf:resource="http://vocab.nerc.ac.uk/collection/P02/current/PXSD/"/>
        <rdfs:comment xml:lang="en">Concentrations of total, organic and inorganic phosphorus per unit weight of sediment.  Sediment is understood to be the solid phase of the bed, including the recently settled material sometimes known as fluff collected from the bed surface.</rdfs:comment>
        <rdfs:label xml:lang="en">Phosphorus concentrations in sediment</rdfs:label>
        <rdf:type rdf:resource="http://www.w3.org/2002/07/owl#NamedIndividual"/>
        <rdf:type rdf:resource="http://www.w3.org/2002/07/owl#Class"/>
      </glview:MeasurementType>
    </rdfs:subClassOf>
    <owl:someValuesFrom>
      <owl:Class>
        <owl:oneOf rdf:parseType="Collection">
          <glview:MeasurementType rdf:about="http://schema.geolink.org/dev/voc/nvs/P02#PXSD"/>
        </owl:oneOf>
      </owl:Class>
    </owl:someValuesFrom>
    <owl:onProperty rdf:resource="http://schema.geolink.org/dev/view#hasMeasurementType"/>
  </owl:Restriction>
  <owl:Restriction>
    <rdfs:subClassOf>
      <glview:MeasurementType rdf:about="http://schema.geolink.org/dev/voc/nvs/P02#A999">
        <rdfs:subClassOf rdf:resource="http://schema.geolink.org/dev/voc/nvs/P03#B025"/>
        <rdfs:seeAlso rdf:resource="http://vocab.nerc.ac.uk/collection/P02/current/A999/"/>
        <rdfs:comment xml:lang="en">Microzooplankton surface area per unit volume of the water column parameters presented at the level of taxa that may be mapped to entities in the ITIS taxonomy.  These may be at any taxonomic level from sub-species upwards.</rdfs:comment>
        <rdfs:label xml:lang="en">Microzooplankton taxonomy-related biosurface area per unit volume of the water column</rdfs:label>
        <rdf:type rdf:resource="http://www.w3.org/2002/07/owl#NamedIndividual"/>
        <rdf:type rdf:resource="http://www.w3.org/2002/07/owl#Class"/>
      </glview:MeasurementType>
    </rdfs:subClassOf>
    <owl:someValuesFrom>
      <owl:Class>
        <owl:oneOf rdf:parseType="Collection">
          <glview:MeasurementType rdf:about="http://schema.geolink.org/dev/voc/nvs/P02#A999"/>
        </owl:oneOf>
      </owl:Class>
    </owl:someValuesFrom>
    <owl:onProperty rdf:resource="http://schema.geolink.org/dev/view#hasMeasurementType"/>
  </owl:Restriction>
  <owl:Restriction>
    <rdfs:subClassOf>
      <glview:MeasurementType rdf:about="http://schema.geolink.org/dev/voc/nvs/P02#MTPW">
        <rdfs:subClassOf rdf:resource="http://schema.geolink.org/dev/voc/nvs/P03#G050"/>
        <rdfs:subClassOf rdf:resource="http://schema.geolink.org/dev/voc/nvs/P03#C035"/>
        <rdfs:seeAlso rdf:resource="http://vocab.nerc.ac.uk/collection/P02/current/MTPW/"/>
        <rdfs:comment xml:lang="en">Concentrations of metal elements in sediment pore waters</rdfs:comment>
        <rdfs:label xml:lang="en">Metal concentrations in sediment pore waters</rdfs:label>
        <rdf:type rdf:resource="http://www.w3.org/2002/07/owl#NamedIndividual"/>
        <rdf:type rdf:resource="http://www.w3.org/2002/07/owl#Class"/>
      </glview:MeasurementType>
    </rdfs:subClassOf>
    <owl:someValuesFrom>
      <owl:Class>
        <owl:oneOf rdf:parseType="Collection">
          <glview:MeasurementType rdf:about="http://schema.geolink.org/dev/voc/nvs/P02#MTPW"/>
        </owl:oneOf>
      </owl:Class>
    </owl:someValuesFrom>
    <owl:onProperty rdf:resource="http://schema.geolink.org/dev/view#hasMeasurementType"/>
  </owl:Restriction>
  <owl:Restriction>
    <rdfs:subClassOf>
      <glview:MeasurementType rdf:about="http://schema.geolink.org/dev/voc/nvs/P02#RAGE">
        <rdfs:subClassOf rdf:resource="http://schema.geolink.org/dev/voc/nvs/P03#G030"/>
        <rdfs:seeAlso rdf:resource="http://vocab.nerc.ac.uk/collection/P02/current/RAGE/"/>
        <rdfs:comment xml:lang="en">Measured or stratigraphically estimated ages of lithified sediments, igneous rock or metamorphic rock.</rdfs:comment>
        <rdfs:label xml:lang="en">Rock age</rdfs:label>
        <rdf:type rdf:resource="http://www.w3.org/2002/07/owl#NamedIndividual"/>
        <rdf:type rdf:resource="http://www.w3.org/2002/07/owl#Class"/>
      </glview:MeasurementType>
    </rdfs:subClassOf>
    <owl:someValuesFrom>
      <owl:Class>
        <owl:oneOf rdf:parseType="Collection">
          <glview:MeasurementType rdf:about="http://schema.geolink.org/dev/voc/nvs/P02#RAGE"/>
        </owl:oneOf>
      </owl:Class>
    </owl:someValuesFrom>
    <owl:onProperty rdf:resource="http://schema.geolink.org/dev/view#hasMeasurementType"/>
  </owl:Restriction>
  <owl:Restriction>
    <rdfs:subClassOf>
      <glview:MeasurementType rdf:about="http://schema.geolink.org/dev/voc/nvs/P02#RALT">
        <rdfs:subClassOf rdf:resource="http://schema.geolink.org/dev/voc/nvs/P03#G060"/>
        <rdfs:seeAlso rdf:resource="http://vocab.nerc.ac.uk/collection/P02/current/RALT/"/>
        <rdfs:comment xml:lang="en">Parameters decribing aspects of a geologic unit that are the result of bulk chemical, mineralogical or physical changes related to change in the physical or chemical environment.  Includes weathering, supergene alteration, hydrothermal alteration and metasomatic effects not considered metamorphic.</rdfs:comment>
        <rdfs:label xml:lang="en">Rock alteration</rdfs:label>
        <rdf:type rdf:resource="http://www.w3.org/2002/07/owl#NamedIndividual"/>
        <rdf:type rdf:resource="http://www.w3.org/2002/07/owl#Class"/>
      </glview:MeasurementType>
    </rdfs:subClassOf>
    <owl:someValuesFrom>
      <owl:Class>
        <owl:oneOf rdf:parseType="Collection">
          <glview:MeasurementType rdf:about="http://schema.geolink.org/dev/voc/nvs/P02#RALT"/>
        </owl:oneOf>
      </owl:Class>
    </owl:someValuesFrom>
    <owl:onProperty rdf:resource="http://schema.geolink.org/dev/view#hasMeasurementType"/>
  </owl:Restriction>
  <owl:Restriction>
    <rdfs:subClassOf rdf:resource="http://schema.geolink.org/dev/voc/nvs/P02#AAFX"/>
    <owl:someValuesFrom>
      <owl:Class>
        <owl:oneOf rdf:parseType="Collection">
          <glview:MeasurementType rdf:about="http://schema.geolink.org/dev/voc/nvs/P02#AAFX"/>
        </owl:oneOf>
      </owl:Class>
    </owl:someValuesFrom>
    <owl:onProperty rdf:resource="http://schema.geolink.org/dev/view#hasMeasurementType"/>
  </owl:Restriction>
  <owl:Restriction>
    <rdfs:subClassOf rdf:resource="http://schema.geolink.org/dev/voc/nvs/P02#PATX"/>
    <owl:someValuesFrom>
      <owl:Class>
        <owl:oneOf rdf:parseType="Collection">
          <glview:MeasurementType rdf:about="http://schema.geolink.org/dev/voc/nvs/P02#PATX"/>
        </owl:oneOf>
      </owl:Class>
    </owl:someValuesFrom>
    <owl:onProperty rdf:resource="http://schema.geolink.org/dev/view#hasMeasurementType"/>
  </owl:Restriction>
  <owl:Restriction>
    <rdfs:subClassOf>
      <glview:MeasurementType rdf:about="http://schema.geolink.org/dev/voc/nvs/P02#LGCR">
        <rdfs:subClassOf rdf:resource="http://schema.geolink.org/dev/view#Measurement"/>
        <rdfs:seeAlso rdf:resource="http://vocab.nerc.ac.uk/collection/P02/current/LGCR/"/>
        <rdfs:comment xml:lang="en">Parameters expressing the mean nett transport rates within the water column like Lagrangian currents. Note this is an unintentional duplicate of VDFC.</rdfs:comment>
        <rdfs:label xml:lang="en">Lagrangian currents and transport rates in the water column</rdfs:label>
        <rdf:type rdf:resource="http://www.w3.org/2002/07/owl#NamedIndividual"/>
        <rdf:type rdf:resource="http://www.w3.org/2002/07/owl#Class"/>
      </glview:MeasurementType>
    </rdfs:subClassOf>
    <owl:someValuesFrom>
      <owl:Class>
        <owl:oneOf rdf:parseType="Collection">
          <glview:MeasurementType rdf:about="http://schema.geolink.org/dev/voc/nvs/P02#LGCR"/>
        </owl:oneOf>
      </owl:Class>
    </owl:someValuesFrom>
    <owl:onProperty rdf:resource="http://schema.geolink.org/dev/view#hasMeasurementType"/>
  </owl:Restriction>
  <owl:Restriction>
    <rdfs:subClassOf>
      <glview:MeasurementType rdf:about="http://schema.geolink.org/dev/voc/nvs/P02#FNTX">
        <rdfs:subClassOf rdf:resource="http://schema.geolink.org/dev/voc/nvs/P03#B070"/>
        <rdfs:subClassOf rdf:resource="http://schema.geolink.org/dev/voc/nvs/P03#B020"/>
        <rdfs:seeAlso rdf:resource="http://vocab.nerc.ac.uk/collection/P02/current/FNTX/"/>
        <rdfs:comment xml:lang="en">Fish (Osteichthyes, Agnatha and Chrondrichthyes) abundance per unit volume parameters not included under FATX.  Most commonly used for the generic term 'fish' that maps to multiple taxa.</rdfs:comment>
        <rdfs:label xml:lang="en">Fish non taxonomy-related abundance per unit volume of the water column</rdfs:label>
        <rdf:type rdf:resource="http://www.w3.org/2002/07/owl#NamedIndividual"/>
        <rdf:type rdf:resource="http://www.w3.org/2002/07/owl#Class"/>
      </glview:MeasurementType>
    </rdfs:subClassOf>
    <owl:someValuesFrom>
      <owl:Class>
        <owl:oneOf rdf:parseType="Collection">
          <glview:MeasurementType rdf:about="http://schema.geolink.org/dev/voc/nvs/P02#FNTX"/>
        </owl:oneOf>
      </owl:Class>
    </owl:someValuesFrom>
    <owl:onProperty rdf:resource="http://schema.geolink.org/dev/view#hasMeasurementType"/>
  </owl:Restriction>
  <owl:Restriction>
    <rdfs:subClassOf>
      <glview:MeasurementType rdf:about="http://schema.geolink.org/dev/voc/nvs/P02#PHSE">
        <rdfs:subClassOf rdf:resource="http://schema.geolink.org/dev/voc/nvs/P03#C055"/>
        <rdfs:subClassOf rdf:resource="http://schema.geolink.org/dev/voc/nvs/P03#H001"/>
        <rdfs:subClassOf rdf:resource="http://schema.geolink.org/dev/voc/nvs/P03#G035"/>
        <rdfs:seeAlso rdf:resource="http://vocab.nerc.ac.uk/collection/P02/current/PHSE/"/>
        <rdfs:comment xml:lang="en">Concentration parameters for substances synthesised by man to modify bodily function or diagnose, cure, mitigate, treat, or prevent disease in sediment, which is considered to be anything from the bed sampled by a grab or corer, including 'fluff'.</rdfs:comment>
        <rdfs:label xml:lang="en">Pharmaceutical concentrations in sediments</rdfs:label>
        <rdf:type rdf:resource="http://www.w3.org/2002/07/owl#NamedIndividual"/>
        <rdf:type rdf:resource="http://www.w3.org/2002/07/owl#Class"/>
      </glview:MeasurementType>
    </rdfs:subClassOf>
    <owl:someValuesFrom>
      <owl:Class>
        <owl:oneOf rdf:parseType="Collection">
          <glview:MeasurementType rdf:about="http://schema.geolink.org/dev/voc/nvs/P02#PHSE"/>
        </owl:oneOf>
      </owl:Class>
    </owl:someValuesFrom>
    <owl:onProperty rdf:resource="http://schema.geolink.org/dev/view#hasMeasurementType"/>
  </owl:Restriction>
  <owl:Restriction>
    <rdfs:subClassOf>
      <glview:MeasurementType rdf:about="http://schema.geolink.org/dev/voc/nvs/P02#CDTA">
        <rdfs:subClassOf rdf:resource="http://schema.geolink.org/dev/voc/nvs/P03#M010"/>
        <rdfs:seeAlso rdf:resource="http://vocab.nerc.ac.uk/collection/P02/current/CDTA/"/>
        <rdfs:comment xml:lang="en">Parameters quantifying the degree of hotness of the atmosphere.  Specifically excludes indirect measurements of other parameters such as wet bulb temperatures.</rdfs:comment>
        <rdfs:label xml:lang="en">Air temperature</rdfs:label>
        <rdf:type rdf:resource="http://www.w3.org/2002/07/owl#NamedIndividual"/>
        <rdf:type rdf:resource="http://www.w3.org/2002/07/owl#Class"/>
      </glview:MeasurementType>
    </rdfs:subClassOf>
    <owl:someValuesFrom>
      <owl:Class>
        <owl:oneOf rdf:parseType="Collection">
          <glview:MeasurementType rdf:about="http://schema.geolink.org/dev/voc/nvs/P02#CDTA"/>
        </owl:oneOf>
      </owl:Class>
    </owl:someValuesFrom>
    <owl:onProperty rdf:resource="http://schema.geolink.org/dev/view#hasMeasurementType"/>
  </owl:Restriction>
  <owl:Restriction>
    <rdfs:subClassOf rdf:resource="http://schema.geolink.org/dev/voc/nvs/P02#IWAB"/>
    <owl:someValuesFrom>
      <owl:Class>
        <owl:oneOf rdf:parseType="Collection">
          <glview:MeasurementType rdf:about="http://schema.geolink.org/dev/voc/nvs/P02#IWAB"/>
        </owl:oneOf>
      </owl:Class>
    </owl:someValuesFrom>
    <owl:onProperty rdf:resource="http://schema.geolink.org/dev/view#hasMeasurementType"/>
  </owl:Restriction>
  <owl:Restriction>
    <rdfs:subClassOf>
      <glview:MeasurementType rdf:about="http://schema.geolink.org/dev/voc/nvs/P02#CPRP">
        <rdfs:subClassOf rdf:resource="http://schema.geolink.org/dev/voc/nvs/P03#M010"/>
        <rdfs:seeAlso rdf:resource="http://vocab.nerc.ac.uk/collection/P02/current/CPRP/"/>
        <rdfs:comment xml:lang="en">Parameters relating to all kinds of precipitation (rain, snow, etc.) and water loss from the surface of the Earth</rdfs:comment>
        <rdfs:label xml:lang="en">Precipitation and evaporation</rdfs:label>
        <rdf:type rdf:resource="http://www.w3.org/2002/07/owl#NamedIndividual"/>
        <rdf:type rdf:resource="http://www.w3.org/2002/07/owl#Class"/>
      </glview:MeasurementType>
    </rdfs:subClassOf>
    <owl:someValuesFrom>
      <owl:Class>
        <owl:oneOf rdf:parseType="Collection">
          <glview:MeasurementType rdf:about="http://schema.geolink.org/dev/voc/nvs/P02#CPRP"/>
        </owl:oneOf>
      </owl:Class>
    </owl:someValuesFrom>
    <owl:onProperty rdf:resource="http://schema.geolink.org/dev/view#hasMeasurementType"/>
  </owl:Restriction>
  <owl:Restriction>
    <rdfs:subClassOf rdf:resource="http://schema.geolink.org/dev/voc/nvs/P02#FDMS"/>
    <owl:someValuesFrom>
      <owl:Class>
        <owl:oneOf rdf:parseType="Collection">
          <glview:MeasurementType rdf:about="http://schema.geolink.org/dev/voc/nvs/P02#FDMS"/>
        </owl:oneOf>
      </owl:Class>
    </owl:someValuesFrom>
    <owl:onProperty rdf:resource="http://schema.geolink.org/dev/view#hasMeasurementType"/>
  </owl:Restriction>
  <owl:Restriction>
    <rdfs:subClassOf rdf:resource="http://schema.geolink.org/dev/voc/nvs/P02#MTPW"/>
    <owl:someValuesFrom>
      <owl:Class>
        <owl:oneOf rdf:parseType="Collection">
          <glview:MeasurementType rdf:about="http://schema.geolink.org/dev/voc/nvs/P02#MTPW"/>
        </owl:oneOf>
      </owl:Class>
    </owl:someValuesFrom>
    <owl:onProperty rdf:resource="http://schema.geolink.org/dev/view#hasMeasurementType"/>
  </owl:Restriction>
  <owl:Restriction>
    <rdfs:subClassOf>
      <glview:MeasurementType rdf:about="http://schema.geolink.org/dev/voc/nvs/P02#ATPC">
        <rdfs:subClassOf rdf:resource="http://schema.geolink.org/dev/voc/nvs/P03#M005"/>
        <rdfs:seeAlso rdf:resource="http://vocab.nerc.ac.uk/collection/P02/current/ATPC/"/>
        <rdfs:comment xml:lang="en">Parameters quantifying and categorising the particulate phases (solids and aerosols) of the atmosphere, excluding chemical composition</rdfs:comment>
        <rdfs:label xml:lang="en">Atmospheric particulates</rdfs:label>
        <rdf:type rdf:resource="http://www.w3.org/2002/07/owl#NamedIndividual"/>
        <rdf:type rdf:resource="http://www.w3.org/2002/07/owl#Class"/>
      </glview:MeasurementType>
    </rdfs:subClassOf>
    <owl:someValuesFrom>
      <owl:Class>
        <owl:oneOf rdf:parseType="Collection">
          <glview:MeasurementType rdf:about="http://schema.geolink.org/dev/voc/nvs/P02#ATPC"/>
        </owl:oneOf>
      </owl:Class>
    </owl:someValuesFrom>
    <owl:onProperty rdf:resource="http://schema.geolink.org/dev/view#hasMeasurementType"/>
  </owl:Restriction>
  <owl:Restriction>
    <rdfs:subClassOf>
      <glview:MeasurementType rdf:about="http://schema.geolink.org/dev/voc/nvs/P02#CBCC">
        <rdfs:subClassOf rdf:resource="http://schema.geolink.org/dev/voc/nvs/P03#B005"/>
        <rdfs:seeAlso rdf:resource="http://vocab.nerc.ac.uk/collection/P02/current/CBCC/"/>
        <rdfs:comment xml:lang="en">Parameters describing the size, shape or physiological activity of bacteria, defined as Kingdom Monera (includes cyanobacteria).  Includes parameters both parameters mapped to taxa and those mapped to non-taxonomic groupings.</rdfs:comment>
        <rdfs:label xml:lang="en">Bacteria morphology and physiology</rdfs:label>
        <rdf:type rdf:resource="http://www.w3.org/2002/07/owl#NamedIndividual"/>
        <rdf:type rdf:resource="http://www.w3.org/2002/07/owl#Class"/>
      </glview:MeasurementType>
    </rdfs:subClassOf>
    <owl:someValuesFrom>
      <owl:Class>
        <owl:oneOf rdf:parseType="Collection">
          <glview:MeasurementType rdf:about="http://schema.geolink.org/dev/voc/nvs/P02#CBCC"/>
        </owl:oneOf>
      </owl:Class>
    </owl:someValuesFrom>
    <owl:onProperty rdf:resource="http://schema.geolink.org/dev/view#hasMeasurementType"/>
  </owl:Restriction>
  <owl:Restriction>
    <rdfs:subClassOf>
      <glview:MeasurementType rdf:about="http://schema.geolink.org/dev/voc/nvs/P02#GPIG">
        <rdfs:subClassOf rdf:resource="http://schema.geolink.org/dev/voc/nvs/P03#B045"/>
        <rdfs:subClassOf rdf:resource="http://schema.geolink.org/dev/voc/nvs/P03#B035"/>
        <rdfs:seeAlso rdf:resource="http://vocab.nerc.ac.uk/collection/P02/current/GPIG/"/>
        <rdfs:comment xml:lang="en">Parameters identifying or quantifying zooplankton gut pigments</rdfs:comment>
        <rdfs:label xml:lang="en">Zooplankton gut pigments</rdfs:label>
        <rdf:type rdf:resource="http://www.w3.org/2002/07/owl#NamedIndividual"/>
        <rdf:type rdf:resource="http://www.w3.org/2002/07/owl#Class"/>
      </glview:MeasurementType>
    </rdfs:subClassOf>
    <owl:someValuesFrom>
      <owl:Class>
        <owl:oneOf rdf:parseType="Collection">
          <glview:MeasurementType rdf:about="http://schema.geolink.org/dev/voc/nvs/P02#GPIG"/>
        </owl:oneOf>
      </owl:Class>
    </owl:someValuesFrom>
    <owl:onProperty rdf:resource="http://schema.geolink.org/dev/view#hasMeasurementType"/>
  </owl:Restriction>
  <owl:Restriction>
    <rdfs:subClassOf>
      <glview:MeasurementType rdf:about="http://schema.geolink.org/dev/voc/nvs/P02#KRTS">
        <rdfs:subClassOf rdf:resource="http://schema.geolink.org/dev/voc/nvs/P03#D034"/>
        <rdfs:seeAlso rdf:resource="http://vocab.nerc.ac.uk/collection/P02/current/KRTS/"/>
        <rdfs:comment xml:lang="en">Statistical parameters derived from wave data expressing wave properties other than height, period and direction</rdfs:comment>
        <rdfs:label xml:lang="en">Other wave statistics</rdfs:label>
        <rdf:type rdf:resource="http://www.w3.org/2002/07/owl#NamedIndividual"/>
        <rdf:type rdf:resource="http://www.w3.org/2002/07/owl#Class"/>
      </glview:MeasurementType>
    </rdfs:subClassOf>
    <owl:someValuesFrom>
      <owl:Class>
        <owl:oneOf rdf:parseType="Collection">
          <glview:MeasurementType rdf:about="http://schema.geolink.org/dev/voc/nvs/P02#KRTS"/>
        </owl:oneOf>
      </owl:Class>
    </owl:someValuesFrom>
    <owl:onProperty rdf:resource="http://schema.geolink.org/dev/view#hasMeasurementType"/>
  </owl:Restriction>
  <owl:Restriction>
    <rdfs:subClassOf rdf:resource="http://schema.geolink.org/dev/voc/nvs/P02#CBSP"/>
    <owl:someValuesFrom>
      <owl:Class>
        <owl:oneOf rdf:parseType="Collection">
          <glview:MeasurementType rdf:about="http://schema.geolink.org/dev/voc/nvs/P02#CBSP"/>
        </owl:oneOf>
      </owl:Class>
    </owl:someValuesFrom>
    <owl:onProperty rdf:resource="http://schema.geolink.org/dev/view#hasMeasurementType"/>
  </owl:Restriction>
  <owl:Restriction>
    <rdfs:subClassOf>
      <glview:MeasurementType rdf:about="http://schema.geolink.org/dev/voc/nvs/P02#OHWC">
        <rdfs:subClassOf rdf:resource="http://schema.geolink.org/dev/voc/nvs/P03#C025"/>
        <rdfs:seeAlso rdf:resource="http://vocab.nerc.ac.uk/collection/P02/current/OHWC/"/>
        <rdfs:comment xml:lang="en">'Other' (not alkanes, alkenes, alkynes or PAHs) hydrocarbon concentration parameters (including saturation of gaseous species) in all phases of the water column.  Does not include parameters expressed per unit weight of SPM.</rdfs:comment>
        <rdfs:label xml:lang="en">Concentration of other hydrocarbons in the water column</rdfs:label>
        <rdf:type rdf:resource="http://www.w3.org/2002/07/owl#NamedIndividual"/>
        <rdf:type rdf:resource="http://www.w3.org/2002/07/owl#Class"/>
      </glview:MeasurementType>
    </rdfs:subClassOf>
    <owl:someValuesFrom>
      <owl:Class>
        <owl:oneOf rdf:parseType="Collection">
          <glview:MeasurementType rdf:about="http://schema.geolink.org/dev/voc/nvs/P02#OHWC"/>
        </owl:oneOf>
      </owl:Class>
    </owl:someValuesFrom>
    <owl:onProperty rdf:resource="http://schema.geolink.org/dev/view#hasMeasurementType"/>
  </owl:Restriction>
  <owl:Restriction>
    <rdfs:subClassOf>
      <glview:MeasurementType rdf:about="http://schema.geolink.org/dev/voc/nvs/P02#SABB">
        <rdfs:subClassOf rdf:resource="http://schema.geolink.org/dev/voc/nvs/P03#B070"/>
        <rdfs:subClassOf rdf:resource="http://schema.geolink.org/dev/voc/nvs/P03#H004"/>
        <rdfs:seeAlso rdf:resource="http://vocab.nerc.ac.uk/collection/P02/current/SABB/"/>
        <rdfs:comment xml:lang="en">Paramaters that quantify the numbers or amount of living material of shellfish (molluscs - including cephalopods - and crustaceans of interest to fisheries research and commercial fisheries) in any body of fresh or salt water.</rdfs:comment>
        <rdfs:label xml:lang="en">Shellfish abundance and biomass in water bodies</rdfs:label>
        <rdf:type rdf:resource="http://www.w3.org/2002/07/owl#NamedIndividual"/>
        <rdf:type rdf:resource="http://www.w3.org/2002/07/owl#Class"/>
      </glview:MeasurementType>
    </rdfs:subClassOf>
    <owl:someValuesFrom>
      <owl:Class>
        <owl:oneOf rdf:parseType="Collection">
          <glview:MeasurementType rdf:about="http://schema.geolink.org/dev/voc/nvs/P02#SABB"/>
        </owl:oneOf>
      </owl:Class>
    </owl:someValuesFrom>
    <owl:onProperty rdf:resource="http://schema.geolink.org/dev/view#hasMeasurementType"/>
  </owl:Restriction>
  <owl:Restriction>
    <rdfs:subClassOf>
      <glview:MeasurementType rdf:about="http://schema.geolink.org/dev/voc/nvs/P02#SR3D">
        <rdfs:subClassOf rdf:resource="http://schema.geolink.org/dev/voc/nvs/P03#GPYS"/>
        <rdfs:subClassOf rdf:resource="http://schema.geolink.org/dev/voc/nvs/P03#G012"/>
        <rdfs:subClassOf>
          <glview:MeasurementType rdf:about="http://schema.geolink.org/dev/voc/nvs/P02#SRFL">
            <rdfs:subClassOf rdf:resource="http://schema.geolink.org/dev/voc/nvs/P03#GPYS"/>
            <rdfs:subClassOf rdf:resource="http://schema.geolink.org/dev/voc/nvs/P03#G012"/>
            <rdfs:seeAlso rdf:resource="http://vocab.nerc.ac.uk/collection/P02/current/SRFL/"/>
            <rdfs:comment xml:lang="en">Parameters relating to the elucidation of geological structure by quantifying the proportion of waves from a high energy source reflected by sub-surface layers.</rdfs:comment>
            <rdfs:label xml:lang="en">Seismic reflection</rdfs:label>
            <rdf:type rdf:resource="http://www.w3.org/2002/07/owl#NamedIndividual"/>
            <rdf:type rdf:resource="http://www.w3.org/2002/07/owl#Class"/>
          </glview:MeasurementType>
        </rdfs:subClassOf>
        <rdfs:seeAlso rdf:resource="http://vocab.nerc.ac.uk/collection/P02/current/SR3D/"/>
        <rdfs:comment xml:lang="en">Parameters relating to structure beneath sea-bed determined by the reflection of seismic energy along multiple parallel tracks.</rdfs:comment>
        <rdfs:label xml:lang="en">Three-dimensional seismic reflection</rdfs:label>
        <rdf:type rdf:resource="http://www.w3.org/2002/07/owl#NamedIndividual"/>
        <rdf:type rdf:resource="http://www.w3.org/2002/07/owl#Class"/>
      </glview:MeasurementType>
    </rdfs:subClassOf>
    <owl:someValuesFrom>
      <owl:Class>
        <owl:oneOf rdf:parseType="Collection">
          <glview:MeasurementType rdf:about="http://schema.geolink.org/dev/voc/nvs/P02#SR3D"/>
        </owl:oneOf>
      </owl:Class>
    </owl:someValuesFrom>
    <owl:onProperty rdf:resource="http://schema.geolink.org/dev/view#hasMeasurementType"/>
  </owl:Restriction>
  <owl:Restriction>
    <rdfs:subClassOf>
      <glview:MeasurementType rdf:about="http://schema.geolink.org/dev/voc/nvs/P02#OHAT">
        <rdfs:subClassOf rdf:resource="http://schema.geolink.org/dev/voc/nvs/P03#C025"/>
        <rdfs:subClassOf rdf:resource="http://schema.geolink.org/dev/voc/nvs/P03#M005"/>
        <rdfs:seeAlso rdf:resource="http://vocab.nerc.ac.uk/collection/P02/current/OHAT/"/>
        <rdfs:comment xml:lang="en">'Other' (not alkanes, alkenes, alkynes or PAHs) hydrocarbon concentration parameters (including saturation of gaseous species) in all phases of the atmosphere.</rdfs:comment>
        <rdfs:label xml:lang="en">Concentration of other hydrocarbons in the atmosphere</rdfs:label>
        <rdf:type rdf:resource="http://www.w3.org/2002/07/owl#NamedIndividual"/>
        <rdf:type rdf:resource="http://www.w3.org/2002/07/owl#Class"/>
      </glview:MeasurementType>
    </rdfs:subClassOf>
    <owl:someValuesFrom>
      <owl:Class>
        <owl:oneOf rdf:parseType="Collection">
          <glview:MeasurementType rdf:about="http://schema.geolink.org/dev/voc/nvs/P02#OHAT"/>
        </owl:oneOf>
      </owl:Class>
    </owl:someValuesFrom>
    <owl:onProperty rdf:resource="http://schema.geolink.org/dev/view#hasMeasurementType"/>
  </owl:Restriction>
  <owl:Restriction>
    <rdfs:subClassOf rdf:resource="http://schema.geolink.org/dev/voc/nvs/P02#WDNA"/>
    <owl:someValuesFrom>
      <owl:Class>
        <owl:oneOf rdf:parseType="Collection">
          <glview:MeasurementType rdf:about="http://schema.geolink.org/dev/voc/nvs/P02#WDNA"/>
        </owl:oneOf>
      </owl:Class>
    </owl:someValuesFrom>
    <owl:onProperty rdf:resource="http://schema.geolink.org/dev/view#hasMeasurementType"/>
  </owl:Restriction>
  <owl:Restriction>
    <rdfs:subClassOf>
      <glview:MeasurementType rdf:about="http://schema.geolink.org/dev/voc/nvs/P02#DGPW">
        <rdfs:subClassOf rdf:resource="http://schema.geolink.org/dev/voc/nvs/P03#G050"/>
        <rdfs:subClassOf rdf:resource="http://schema.geolink.org/dev/voc/nvs/P03#C015"/>
        <rdfs:seeAlso rdf:resource="http://vocab.nerc.ac.uk/collection/P02/current/DGPW/"/>
        <rdfs:comment xml:lang="en">All concentration parameters (including saturation) for dissolved oxygen in sediment pore waters</rdfs:comment>
        <rdfs:label xml:lang="en">Dissolved oxygen concentration parameters in sediment pore waters</rdfs:label>
        <rdf:type rdf:resource="http://www.w3.org/2002/07/owl#NamedIndividual"/>
        <rdf:type rdf:resource="http://www.w3.org/2002/07/owl#Class"/>
      </glview:MeasurementType>
    </rdfs:subClassOf>
    <owl:someValuesFrom>
      <owl:Class>
        <owl:oneOf rdf:parseType="Collection">
          <glview:MeasurementType rdf:about="http://schema.geolink.org/dev/voc/nvs/P02#DGPW"/>
        </owl:oneOf>
      </owl:Class>
    </owl:someValuesFrom>
    <owl:onProperty rdf:resource="http://schema.geolink.org/dev/view#hasMeasurementType"/>
  </owl:Restriction>
  <owl:Restriction>
    <rdfs:subClassOf rdf:resource="http://schema.geolink.org/dev/voc/nvs/P02#AMOX"/>
    <owl:someValuesFrom>
      <owl:Class>
        <owl:oneOf rdf:parseType="Collection">
          <glview:MeasurementType rdf:about="http://schema.geolink.org/dev/voc/nvs/P02#AMOX"/>
        </owl:oneOf>
      </owl:Class>
    </owl:someValuesFrom>
    <owl:onProperty rdf:resource="http://schema.geolink.org/dev/view#hasMeasurementType"/>
  </owl:Restriction>
  <owl:Restriction>
    <rdfs:subClassOf>
      <glview:MeasurementType rdf:about="http://schema.geolink.org/dev/voc/nvs/P02#SCOC">
        <rdfs:subClassOf rdf:resource="http://schema.geolink.org/dev/voc/nvs/P03#C055"/>
        <rdfs:subClassOf rdf:resource="http://schema.geolink.org/dev/voc/nvs/P03#H001"/>
        <rdfs:subClassOf rdf:resource="http://schema.geolink.org/dev/voc/nvs/P03#G035"/>
        <rdfs:seeAlso rdf:resource="http://vocab.nerc.ac.uk/collection/P02/current/SCOC/"/>
        <rdfs:comment xml:lang="en">Concentration parameters for carbon compounds regarded as environmentally harmful in sediment, which is considered to be anything from the bed sampled by a grab or corer, including 'fluff' that are not included in other specific categories</rdfs:comment>
        <rdfs:label xml:lang="en">Concentration of other organic contaminants in sediment samples</rdfs:label>
        <rdf:type rdf:resource="http://www.w3.org/2002/07/owl#NamedIndividual"/>
        <rdf:type rdf:resource="http://www.w3.org/2002/07/owl#Class"/>
      </glview:MeasurementType>
    </rdfs:subClassOf>
    <owl:someValuesFrom>
      <owl:Class>
        <owl:oneOf rdf:parseType="Collection">
          <glview:MeasurementType rdf:about="http://schema.geolink.org/dev/voc/nvs/P02#SCOC"/>
        </owl:oneOf>
      </owl:Class>
    </owl:someValuesFrom>
    <owl:onProperty rdf:resource="http://schema.geolink.org/dev/view#hasMeasurementType"/>
  </owl:Restriction>
  <owl:Restriction>
    <rdfs:subClassOf>
      <glview:MeasurementType rdf:about="http://schema.geolink.org/dev/voc/nvs/P02#GTCH">
        <rdfs:subClassOf rdf:resource="http://schema.geolink.org/dev/voc/nvs/P03#G040"/>
        <rdfs:subClassOf rdf:resource="http://schema.geolink.org/dev/voc/nvs/P03#H002"/>
        <rdfs:seeAlso rdf:resource="http://vocab.nerc.ac.uk/collection/P02/current/GTCH/"/>
        <rdfs:comment xml:lang="en">Parameters quantifying the properties of rocks and sediments that are relevance to engineering such as physical strength and load-bearing capacity.  Includes the disciplines of rock mechanics and soil mechanics.</rdfs:comment>
        <rdfs:label xml:lang="en">Geotechnics</rdfs:label>
        <rdf:type rdf:resource="http://www.w3.org/2002/07/owl#NamedIndividual"/>
        <rdf:type rdf:resource="http://www.w3.org/2002/07/owl#Class"/>
      </glview:MeasurementType>
    </rdfs:subClassOf>
    <owl:someValuesFrom>
      <owl:Class>
        <owl:oneOf rdf:parseType="Collection">
          <glview:MeasurementType rdf:about="http://schema.geolink.org/dev/voc/nvs/P02#GTCH"/>
        </owl:oneOf>
      </owl:Class>
    </owl:someValuesFrom>
    <owl:onProperty rdf:resource="http://schema.geolink.org/dev/view#hasMeasurementType"/>
  </owl:Restriction>
  <owl:Restriction>
    <rdfs:subClassOf>
      <glview:MeasurementType rdf:about="http://schema.geolink.org/dev/voc/nvs/P02#ROGS">
        <rdfs:subClassOf rdf:resource="http://schema.geolink.org/dev/voc/nvs/P03#G040"/>
        <rdfs:seeAlso rdf:resource="http://vocab.nerc.ac.uk/collection/P02/current/ROGS/"/>
        <rdfs:comment xml:lang="en">Parameters specifying the physical dimensions of the particles comprising lithified sedimentary rocks (including expressions of shape such as aspect ratio) and statistics derived from their variation in a sample (e.g. mean, mode, sorting, skewness).</rdfs:comment>
        <rdfs:label xml:lang="en">Rock grain size</rdfs:label>
        <rdf:type rdf:resource="http://www.w3.org/2002/07/owl#NamedIndividual"/>
        <rdf:type rdf:resource="http://www.w3.org/2002/07/owl#Class"/>
      </glview:MeasurementType>
    </rdfs:subClassOf>
    <owl:someValuesFrom>
      <owl:Class>
        <owl:oneOf rdf:parseType="Collection">
          <glview:MeasurementType rdf:about="http://schema.geolink.org/dev/voc/nvs/P02#ROGS"/>
        </owl:oneOf>
      </owl:Class>
    </owl:someValuesFrom>
    <owl:onProperty rdf:resource="http://schema.geolink.org/dev/view#hasMeasurementType"/>
  </owl:Restriction>
  <owl:Restriction>
    <rdfs:subClassOf>
      <owl:NamedIndividual rdf:about="http://schema.geolink.org/dev/voc/nvs/P02#RBSC">
        <rdfs:subClassOf rdf:resource="http://schema.geolink.org/dev/voc/nvs/P03#D034"/>
        <rdfs:subClassOf rdf:resource="http://schema.geolink.org/dev/voc/nvs/P03#D030"/>
        <rdfs:subClassOf rdf:resource="http://schema.geolink.org/dev/voc/nvs/P03#M015"/>
        <rdfs:seeAlso rdf:resource="http://vocab.nerc.ac.uk/collection/P02/current/RBSC/"/>
        <rdfs:subClassOf rdf:resource="http://schema.geolink.org/dev/voc/nvs/P03#D032"/>
        <rdfs:label xml:lang="en">Radar backscatter</rdfs:label>
        <rdfs:subClassOf rdf:resource="http://schema.geolink.org/dev/voc/nvs/P03#M010"/>
        <rdf:type rdf:resource="http://www.w3.org/2002/07/owl#Class"/>
        <rdfs:comment xml:lang="en">Includes all parameters covering the strength of emitted microwave radiation return, including absolute measurements of returning signal strength as well as parameters expressed as backscatter (the proportion of transmitted signal returned)</rdfs:comment>
        <rdf:type rdf:resource="http://schema.geolink.org/dev/view#MeasurementType"/>
      </owl:NamedIndividual>
    </rdfs:subClassOf>
    <owl:someValuesFrom>
      <owl:Class>
        <owl:oneOf rdf:parseType="Collection">
          <owl:NamedIndividual rdf:about="http://schema.geolink.org/dev/voc/nvs/P02#RBSC"/>
        </owl:oneOf>
      </owl:Class>
    </owl:someValuesFrom>
    <owl:onProperty rdf:resource="http://schema.geolink.org/dev/view#hasMeasurementType"/>
  </owl:Restriction>
  <owl:Restriction>
    <rdfs:subClassOf>
      <glview:MeasurementType rdf:about="http://schema.geolink.org/dev/voc/nvs/P02#ISAT">
        <rdfs:subClassOf rdf:resource="http://schema.geolink.org/dev/voc/nvs/P03#C030"/>
        <rdfs:subClassOf rdf:resource="http://schema.geolink.org/dev/voc/nvs/P03#M005"/>
        <rdfs:seeAlso rdf:resource="http://vocab.nerc.ac.uk/collection/P02/current/ISAT/"/>
        <rdfs:comment xml:lang="en">Stable isotope enrichment parameters in both the gaseous and aerosol phases of the atmosphere</rdfs:comment>
        <rdfs:label xml:lang="en">Stable isotope enrichment in the atmosphere</rdfs:label>
        <rdf:type rdf:resource="http://www.w3.org/2002/07/owl#NamedIndividual"/>
        <rdf:type rdf:resource="http://www.w3.org/2002/07/owl#Class"/>
      </glview:MeasurementType>
    </rdfs:subClassOf>
    <owl:someValuesFrom>
      <owl:Class>
        <owl:oneOf rdf:parseType="Collection">
          <glview:MeasurementType rdf:about="http://schema.geolink.org/dev/voc/nvs/P02#ISAT"/>
        </owl:oneOf>
      </owl:Class>
    </owl:someValuesFrom>
    <owl:onProperty rdf:resource="http://schema.geolink.org/dev/view#hasMeasurementType"/>
  </owl:Restriction>
  <owl:Restriction>
    <rdfs:subClassOf>
      <glview:MeasurementType rdf:about="http://schema.geolink.org/dev/voc/nvs/P02#DENS">
        <rdfs:subClassOf rdf:resource="http://schema.geolink.org/dev/voc/nvs/P03#G015"/>
        <rdfs:seeAlso rdf:resource="http://vocab.nerc.ac.uk/collection/P02/current/DENS/"/>
        <rdfs:comment xml:lang="en">Parameters that do not easily fit into any of the other SPM data categories.</rdfs:comment>
        <rdfs:label xml:lang="en">Other physical and chemical properties of suspended particulate material</rdfs:label>
        <rdf:type rdf:resource="http://www.w3.org/2002/07/owl#NamedIndividual"/>
        <rdf:type rdf:resource="http://www.w3.org/2002/07/owl#Class"/>
      </glview:MeasurementType>
    </rdfs:subClassOf>
    <owl:someValuesFrom>
      <owl:Class>
        <owl:oneOf rdf:parseType="Collection">
          <glview:MeasurementType rdf:about="http://schema.geolink.org/dev/voc/nvs/P02#DENS"/>
        </owl:oneOf>
      </owl:Class>
    </owl:someValuesFrom>
    <owl:onProperty rdf:resource="http://schema.geolink.org/dev/view#hasMeasurementType"/>
  </owl:Restriction>
  <owl:Restriction>
    <rdfs:subClassOf>
      <glview:MeasurementType rdf:about="http://schema.geolink.org/dev/voc/nvs/P02#PSAL">
        <rdfs:subClassOf rdf:resource="http://schema.geolink.org/dev/voc/nvs/P03#D025"/>
        <rdfs:seeAlso rdf:resource="http://vocab.nerc.ac.uk/collection/P02/current/PSAL/"/>
        <rdfs:comment xml:lang="en">Parameters quantifying the concentration of sodium chloride in any body of water at any point between the bed and the atmosphere</rdfs:comment>
        <rdfs:label xml:lang="en">Salinity of the water column</rdfs:label>
        <rdf:type rdf:resource="http://www.w3.org/2002/07/owl#NamedIndividual"/>
        <rdf:type rdf:resource="http://www.w3.org/2002/07/owl#Class"/>
      </glview:MeasurementType>
    </rdfs:subClassOf>
    <owl:someValuesFrom>
      <owl:Class>
        <owl:oneOf rdf:parseType="Collection">
          <glview:MeasurementType rdf:about="http://schema.geolink.org/dev/voc/nvs/P02#PSAL"/>
        </owl:oneOf>
      </owl:Class>
    </owl:someValuesFrom>
    <owl:onProperty rdf:resource="http://schema.geolink.org/dev/view#hasMeasurementType"/>
  </owl:Restriction>
  <owl:Restriction>
    <rdfs:subClassOf rdf:resource="http://schema.geolink.org/dev/voc/nvs/P02#OMPW"/>
    <owl:someValuesFrom>
      <owl:Class>
        <owl:oneOf rdf:parseType="Collection">
          <owl:NamedIndividual rdf:about="http://schema.geolink.org/dev/voc/nvs/P02#OMPW"/>
        </owl:oneOf>
      </owl:Class>
    </owl:someValuesFrom>
    <owl:onProperty rdf:resource="http://schema.geolink.org/dev/view#hasMeasurementType"/>
  </owl:Restriction>
  <owl:Restriction>
    <rdfs:subClassOf rdf:resource="http://schema.geolink.org/dev/voc/nvs/P02#MTIC"/>
    <owl:someValuesFrom>
      <owl:Class>
        <owl:oneOf rdf:parseType="Collection">
          <glview:MeasurementType rdf:about="http://schema.geolink.org/dev/voc/nvs/P02#MTIC"/>
        </owl:oneOf>
      </owl:Class>
    </owl:someValuesFrom>
    <owl:onProperty rdf:resource="http://schema.geolink.org/dev/view#hasMeasurementType"/>
  </owl:Restriction>
  <owl:Restriction>
    <rdfs:subClassOf>
      <glview:MeasurementType rdf:about="http://schema.geolink.org/dev/voc/nvs/P02#PREX">
        <rdfs:subClassOf rdf:resource="http://schema.geolink.org/dev/voc/nvs/P03#D032"/>
        <rdfs:seeAlso rdf:resource="http://vocab.nerc.ac.uk/collection/P02/current/PREX/"/>
        <rdfs:comment xml:lang="en">Measurements of the displacement of the water column surface from a fixed, stable reference expressed as either total pressure or sea pressure</rdfs:comment>
        <rdfs:label xml:lang="en">Sea level expressed as pressure</rdfs:label>
        <rdf:type rdf:resource="http://www.w3.org/2002/07/owl#NamedIndividual"/>
        <rdf:type rdf:resource="http://www.w3.org/2002/07/owl#Class"/>
      </glview:MeasurementType>
    </rdfs:subClassOf>
    <owl:someValuesFrom>
      <owl:Class>
        <owl:oneOf rdf:parseType="Collection">
          <glview:MeasurementType rdf:about="http://schema.geolink.org/dev/voc/nvs/P02#PREX"/>
        </owl:oneOf>
      </owl:Class>
    </owl:someValuesFrom>
    <owl:onProperty rdf:resource="http://schema.geolink.org/dev/view#hasMeasurementType"/>
  </owl:Restriction>
  <owl:Restriction>
    <rdfs:subClassOf>
      <glview:MeasurementType rdf:about="http://schema.geolink.org/dev/voc/nvs/P02#CPSD">
        <rdfs:subClassOf rdf:resource="http://schema.geolink.org/dev/voc/nvs/P03#B035"/>
        <rdfs:subClassOf rdf:resource="http://schema.geolink.org/dev/voc/nvs/P03#G035"/>
        <rdfs:seeAlso rdf:resource="http://vocab.nerc.ac.uk/collection/P02/current/CPSD/"/>
        <rdfs:comment xml:lang="en">Includes all variants of chlorophyll.  Sediment includes anything collected by a grab or corer, including the fluff layer from the top of the consolidated sediment</rdfs:comment>
        <rdfs:label xml:lang="en">Chlorophyll pigment concentrations in sediment</rdfs:label>
        <rdf:type rdf:resource="http://www.w3.org/2002/07/owl#NamedIndividual"/>
        <rdf:type rdf:resource="http://www.w3.org/2002/07/owl#Class"/>
      </glview:MeasurementType>
    </rdfs:subClassOf>
    <owl:someValuesFrom>
      <owl:Class>
        <owl:oneOf rdf:parseType="Collection">
          <glview:MeasurementType rdf:about="http://schema.geolink.org/dev/voc/nvs/P02#CPSD"/>
        </owl:oneOf>
      </owl:Class>
    </owl:someValuesFrom>
    <owl:onProperty rdf:resource="http://schema.geolink.org/dev/view#hasMeasurementType"/>
  </owl:Restriction>
  <owl:Restriction>
    <rdfs:subClassOf rdf:resource="http://schema.geolink.org/dev/voc/nvs/P02#ISAT"/>
    <owl:someValuesFrom>
      <owl:Class>
        <owl:oneOf rdf:parseType="Collection">
          <glview:MeasurementType rdf:about="http://schema.geolink.org/dev/voc/nvs/P02#ISAT"/>
        </owl:oneOf>
      </owl:Class>
    </owl:someValuesFrom>
    <owl:onProperty rdf:resource="http://schema.geolink.org/dev/view#hasMeasurementType"/>
  </owl:Restriction>
  <owl:Restriction>
    <rdfs:subClassOf>
      <glview:MeasurementType rdf:about="http://schema.geolink.org/dev/voc/nvs/P02#CASD">
        <rdfs:subClassOf rdf:resource="http://schema.geolink.org/dev/voc/nvs/P03#C050"/>
        <rdfs:subClassOf rdf:resource="http://schema.geolink.org/dev/voc/nvs/P03#G035"/>
        <rdfs:seeAlso rdf:resource="http://vocab.nerc.ac.uk/collection/P02/current/CASD/"/>
        <rdfs:comment xml:lang="en">Concentrations of carbohydrates, phenols, alkanols (alcohols), ethers,aldehydes and simple (non-alkenone) ketones in unlithified sediment (material collected by a corer including fluff).</rdfs:comment>
        <rdfs:label xml:lang="en">Concentration of carbohydrates, phenols, alkanols (alcohols), ethers, aldehydes and ketones in sediment</rdfs:label>
        <rdf:type rdf:resource="http://www.w3.org/2002/07/owl#NamedIndividual"/>
        <rdf:type rdf:resource="http://www.w3.org/2002/07/owl#Class"/>
      </glview:MeasurementType>
    </rdfs:subClassOf>
    <owl:someValuesFrom>
      <owl:Class>
        <owl:oneOf rdf:parseType="Collection">
          <glview:MeasurementType rdf:about="http://schema.geolink.org/dev/voc/nvs/P02#CASD"/>
        </owl:oneOf>
      </owl:Class>
    </owl:someValuesFrom>
    <owl:onProperty rdf:resource="http://schema.geolink.org/dev/view#hasMeasurementType"/>
  </owl:Restriction>
  <owl:Restriction>
    <rdfs:subClassOf>
      <glview:MeasurementType rdf:about="http://schema.geolink.org/dev/voc/nvs/P02#REFF">
        <rdfs:subClassOf rdf:resource="http://schema.geolink.org/dev/voc/nvs/P03#G050"/>
        <rdfs:seeAlso rdf:resource="http://vocab.nerc.ac.uk/collection/P02/current/REFF/"/>
        <rdfs:comment></rdfs:comment>
        <rdfs:label xml:lang="en">Sediment resistivity</rdfs:label>
        <rdf:type rdf:resource="http://www.w3.org/2002/07/owl#NamedIndividual"/>
        <rdf:type rdf:resource="http://www.w3.org/2002/07/owl#Class"/>
      </glview:MeasurementType>
    </rdfs:subClassOf>
    <owl:someValuesFrom>
      <owl:Class>
        <owl:oneOf rdf:parseType="Collection">
          <glview:MeasurementType rdf:about="http://schema.geolink.org/dev/voc/nvs/P02#REFF"/>
        </owl:oneOf>
      </owl:Class>
    </owl:someValuesFrom>
    <owl:onProperty rdf:resource="http://schema.geolink.org/dev/view#hasMeasurementType"/>
  </owl:Restriction>
  <owl:Restriction>
    <rdfs:subClassOf rdf:resource="http://schema.geolink.org/dev/voc/nvs/P02#WDNA"/>
    <owl:someValuesFrom>
      <owl:Class>
        <owl:oneOf rdf:parseType="Collection">
          <glview:MeasurementType rdf:about="http://schema.geolink.org/dev/voc/nvs/P02#WDNA"/>
        </owl:oneOf>
      </owl:Class>
    </owl:someValuesFrom>
    <owl:onProperty rdf:resource="http://schema.geolink.org/dev/view#hasMeasurementType"/>
  </owl:Restriction>
  <owl:Restriction>
    <rdfs:subClassOf rdf:resource="http://schema.geolink.org/dev/voc/nvs/P02#FNTX"/>
    <owl:someValuesFrom>
      <owl:Class>
        <owl:oneOf rdf:parseType="Collection">
          <glview:MeasurementType rdf:about="http://schema.geolink.org/dev/voc/nvs/P02#FNTX"/>
        </owl:oneOf>
      </owl:Class>
    </owl:someValuesFrom>
    <owl:onProperty rdf:resource="http://schema.geolink.org/dev/view#hasMeasurementType"/>
  </owl:Restriction>
  <owl:Restriction>
    <rdfs:subClassOf>
      <glview:MeasurementType rdf:about="http://schema.geolink.org/dev/voc/nvs/P02#APZA">
        <rdfs:subClassOf rdf:resource="http://schema.geolink.org/dev/voc/nvs/P03#Z005"/>
        <rdfs:seeAlso rdf:resource="http://vocab.nerc.ac.uk/collection/P02/current/APZA/"/>
        <rdfs:comment xml:lang="en">Parameters quantifying the upward and downward motion of objects mounting sensors or collecting samples.</rdfs:comment>
        <rdfs:label xml:lang="en">Vertical platform movement</rdfs:label>
        <rdf:type rdf:resource="http://www.w3.org/2002/07/owl#NamedIndividual"/>
        <rdf:type rdf:resource="http://www.w3.org/2002/07/owl#Class"/>
      </glview:MeasurementType>
    </rdfs:subClassOf>
    <owl:someValuesFrom>
      <owl:Class>
        <owl:oneOf rdf:parseType="Collection">
          <glview:MeasurementType rdf:about="http://schema.geolink.org/dev/voc/nvs/P02#APZA"/>
        </owl:oneOf>
      </owl:Class>
    </owl:someValuesFrom>
    <owl:onProperty rdf:resource="http://schema.geolink.org/dev/view#hasMeasurementType"/>
  </owl:Restriction>
  <owl:Restriction>
    <rdfs:subClassOf rdf:resource="http://schema.geolink.org/dev/voc/nvs/P02#SR3D"/>
    <owl:someValuesFrom>
      <owl:Class>
        <owl:oneOf rdf:parseType="Collection">
          <glview:MeasurementType rdf:about="http://schema.geolink.org/dev/voc/nvs/P02#SR3D"/>
        </owl:oneOf>
      </owl:Class>
    </owl:someValuesFrom>
    <owl:onProperty rdf:resource="http://schema.geolink.org/dev/view#hasMeasurementType"/>
  </owl:Restriction>
  <owl:Restriction>
    <rdfs:subClassOf>
      <glview:MeasurementType rdf:about="http://schema.geolink.org/dev/voc/nvs/P02#OMET">
        <rdfs:subClassOf rdf:resource="http://schema.geolink.org/dev/voc/nvs/P03#M010"/>
        <rdfs:seeAlso rdf:resource="http://vocab.nerc.ac.uk/collection/P02/current/OMET/"/>
        <rdfs:comment xml:lang="en">Bucket group for parameters that cannot be classified elsewhere</rdfs:comment>
        <rdfs:label xml:lang="en">Other meteorological measurements</rdfs:label>
        <rdf:type rdf:resource="http://www.w3.org/2002/07/owl#NamedIndividual"/>
        <rdf:type rdf:resource="http://www.w3.org/2002/07/owl#Class"/>
      </glview:MeasurementType>
    </rdfs:subClassOf>
    <owl:someValuesFrom>
      <owl:Class>
        <owl:oneOf rdf:parseType="Collection">
          <glview:MeasurementType rdf:about="http://schema.geolink.org/dev/voc/nvs/P02#OMET"/>
        </owl:oneOf>
      </owl:Class>
    </owl:someValuesFrom>
    <owl:onProperty rdf:resource="http://schema.geolink.org/dev/view#hasMeasurementType"/>
  </owl:Restriction>
  <owl:Restriction>
    <rdfs:subClassOf>
      <glview:MeasurementType rdf:about="http://schema.geolink.org/dev/voc/nvs/P02#FNTM">
        <rdfs:subClassOf rdf:resource="http://schema.geolink.org/dev/voc/nvs/P03#B020"/>
        <rdfs:seeAlso rdf:resource="http://vocab.nerc.ac.uk/collection/P02/current/FNTM/"/>
        <rdfs:comment xml:lang="en">Fish (Osteichthyes, Agnatha and Chrondrichthyes) size and shape parameters not included under FATM.  Most commonly used for the generic term 'fish' that maps to multiple taxa.</rdfs:comment>
        <rdfs:label xml:lang="en">Fish non taxonomy-related morphology</rdfs:label>
        <rdf:type rdf:resource="http://www.w3.org/2002/07/owl#NamedIndividual"/>
        <rdf:type rdf:resource="http://www.w3.org/2002/07/owl#Class"/>
      </glview:MeasurementType>
    </rdfs:subClassOf>
    <owl:someValuesFrom>
      <owl:Class>
        <owl:oneOf rdf:parseType="Collection">
          <glview:MeasurementType rdf:about="http://schema.geolink.org/dev/voc/nvs/P02#FNTM"/>
        </owl:oneOf>
      </owl:Class>
    </owl:someValuesFrom>
    <owl:onProperty rdf:resource="http://schema.geolink.org/dev/view#hasMeasurementType"/>
  </owl:Restriction>
  <owl:Restriction>
    <rdfs:subClassOf>
      <glview:MeasurementType rdf:about="http://schema.geolink.org/dev/voc/nvs/P02#RFVL">
        <rdfs:subClassOf rdf:resource="http://schema.geolink.org/dev/voc/nvs/P03#D030"/>
        <rdfs:seeAlso rdf:resource="http://vocab.nerc.ac.uk/collection/P02/current/RFVL/"/>
        <rdfs:comment xml:lang="en">Parameters expressing the velocity (including scalar speeds and directions) of water column horizontal movement, commonly termed Eulerian currents</rdfs:comment>
        <rdfs:label xml:lang="en">Horizontal velocity of the water column (currents)</rdfs:label>
        <rdf:type rdf:resource="http://www.w3.org/2002/07/owl#NamedIndividual"/>
        <rdf:type rdf:resource="http://www.w3.org/2002/07/owl#Class"/>
      </glview:MeasurementType>
    </rdfs:subClassOf>
    <owl:someValuesFrom>
      <owl:Class>
        <owl:oneOf rdf:parseType="Collection">
          <glview:MeasurementType rdf:about="http://schema.geolink.org/dev/voc/nvs/P02#RFVL"/>
        </owl:oneOf>
      </owl:Class>
    </owl:someValuesFrom>
    <owl:onProperty rdf:resource="http://schema.geolink.org/dev/view#hasMeasurementType"/>
  </owl:Restriction>
  <owl:Restriction>
    <rdfs:subClassOf>
      <glview:MeasurementType rdf:about="http://schema.geolink.org/dev/voc/nvs/P02#CHEX">
        <rdfs:subClassOf rdf:resource="http://schema.geolink.org/dev/voc/nvs/P03#M010"/>
        <rdfs:seeAlso rdf:resource="http://vocab.nerc.ac.uk/collection/P02/current/CHEX/"/>
        <rdfs:comment xml:lang="en">Parameters describing the horizontal and vertical extent of cloud cover</rdfs:comment>
        <rdfs:label xml:lang="en">Cloud cover height and extent</rdfs:label>
        <rdf:type rdf:resource="http://www.w3.org/2002/07/owl#NamedIndividual"/>
        <rdf:type rdf:resource="http://www.w3.org/2002/07/owl#Class"/>
      </glview:MeasurementType>
    </rdfs:subClassOf>
    <owl:someValuesFrom>
      <owl:Class>
        <owl:oneOf rdf:parseType="Collection">
          <glview:MeasurementType rdf:about="http://schema.geolink.org/dev/voc/nvs/P02#CHEX"/>
        </owl:oneOf>
      </owl:Class>
    </owl:someValuesFrom>
    <owl:onProperty rdf:resource="http://schema.geolink.org/dev/view#hasMeasurementType"/>
  </owl:Restriction>
  <owl:Restriction>
    <rdfs:subClassOf rdf:resource="http://schema.geolink.org/dev/voc/nvs/P02#OMPW"/>
    <owl:someValuesFrom>
      <owl:Class>
        <owl:oneOf rdf:parseType="Collection">
          <owl:NamedIndividual rdf:about="http://schema.geolink.org/dev/voc/nvs/P02#OMPW"/>
        </owl:oneOf>
      </owl:Class>
    </owl:someValuesFrom>
    <owl:onProperty rdf:resource="http://schema.geolink.org/dev/view#hasMeasurementType"/>
  </owl:Restriction>
  <owl:Restriction>
    <rdfs:subClassOf rdf:resource="http://schema.geolink.org/dev/voc/nvs/P02#BNTX"/>
    <owl:someValuesFrom>
      <owl:Class>
        <owl:oneOf rdf:parseType="Collection">
          <glview:MeasurementType rdf:about="http://schema.geolink.org/dev/voc/nvs/P02#BNTX"/>
        </owl:oneOf>
      </owl:Class>
    </owl:someValuesFrom>
    <owl:onProperty rdf:resource="http://schema.geolink.org/dev/view#hasMeasurementType"/>
  </owl:Restriction>
  <owl:Restriction>
    <rdfs:subClassOf>
      <glview:MeasurementType rdf:about="http://schema.geolink.org/dev/voc/nvs/P02#RACC">
        <rdfs:subClassOf rdf:resource="http://schema.geolink.org/dev/voc/nvs/P03#G060"/>
        <rdfs:seeAlso rdf:resource="http://vocab.nerc.ac.uk/collection/P02/current/RACC/"/>
        <rdfs:comment xml:lang="en">Parameters quantifying the volume, mass or thickness of particulate material that gathers on the seabed per unit time.</rdfs:comment>
        <rdfs:label xml:lang="en">Sediment accumulation rate</rdfs:label>
        <rdf:type rdf:resource="http://www.w3.org/2002/07/owl#NamedIndividual"/>
        <rdf:type rdf:resource="http://www.w3.org/2002/07/owl#Class"/>
      </glview:MeasurementType>
    </rdfs:subClassOf>
    <owl:someValuesFrom>
      <owl:Class>
        <owl:oneOf rdf:parseType="Collection">
          <glview:MeasurementType rdf:about="http://schema.geolink.org/dev/voc/nvs/P02#RACC"/>
        </owl:oneOf>
      </owl:Class>
    </owl:someValuesFrom>
    <owl:onProperty rdf:resource="http://schema.geolink.org/dev/view#hasMeasurementType"/>
  </owl:Restriction>
  <owl:Restriction>
    <rdfs:subClassOf rdf:resource="http://schema.geolink.org/dev/voc/nvs/P02#ADUN"/>
    <owl:someValuesFrom>
      <owl:Class>
        <owl:oneOf rdf:parseType="Collection">
          <owl:NamedIndividual rdf:about="http://schema.geolink.org/dev/voc/nvs/P02#ADUN"/>
        </owl:oneOf>
      </owl:Class>
    </owl:someValuesFrom>
    <owl:onProperty rdf:resource="http://schema.geolink.org/dev/view#hasMeasurementType"/>
  </owl:Restriction>
  <owl:Restriction>
    <rdfs:subClassOf>
      <glview:MeasurementType rdf:about="http://schema.geolink.org/dev/voc/nvs/P02#MSBO">
        <rdfs:subClassOf rdf:resource="http://schema.geolink.org/dev/voc/nvs/P03#B045"/>
        <rdfs:subClassOf rdf:resource="http://schema.geolink.org/dev/voc/nvs/P03#B070"/>
        <rdfs:seeAlso rdf:resource="http://vocab.nerc.ac.uk/collection/P02/current/MSBO/"/>
        <rdfs:comment xml:lang="en">Zooplankton (mesozooplankton and larger, exclusing fish, mammals, reptiles and insects) biomass determined by gravimetric measurement of loss on ignition</rdfs:comment>
        <rdfs:label xml:lang="en">Zooplankton ash-free dry weight biomass per unit volume of the water column</rdfs:label>
        <rdf:type rdf:resource="http://www.w3.org/2002/07/owl#NamedIndividual"/>
        <rdf:type rdf:resource="http://www.w3.org/2002/07/owl#Class"/>
      </glview:MeasurementType>
    </rdfs:subClassOf>
    <owl:someValuesFrom>
      <owl:Class>
        <owl:oneOf rdf:parseType="Collection">
          <glview:MeasurementType rdf:about="http://schema.geolink.org/dev/voc/nvs/P02#MSBO"/>
        </owl:oneOf>
      </owl:Class>
    </owl:someValuesFrom>
    <owl:onProperty rdf:resource="http://schema.geolink.org/dev/view#hasMeasurementType"/>
  </owl:Restriction>
  <owl:Restriction>
    <rdfs:subClassOf rdf:resource="http://schema.geolink.org/dev/voc/nvs/P02#MFAB"/>
    <owl:someValuesFrom>
      <owl:Class>
        <owl:oneOf rdf:parseType="Collection">
          <glview:MeasurementType rdf:about="http://schema.geolink.org/dev/voc/nvs/P02#MFAB"/>
        </owl:oneOf>
      </owl:Class>
    </owl:someValuesFrom>
    <owl:onProperty rdf:resource="http://schema.geolink.org/dev/view#hasMeasurementType"/>
  </owl:Restriction>
  <owl:Restriction>
    <rdfs:subClassOf rdf:resource="http://schema.geolink.org/dev/voc/nvs/P02#SABB"/>
    <owl:someValuesFrom>
      <owl:Class>
        <owl:oneOf rdf:parseType="Collection">
          <glview:MeasurementType rdf:about="http://schema.geolink.org/dev/voc/nvs/P02#SABB"/>
        </owl:oneOf>
      </owl:Class>
    </owl:someValuesFrom>
    <owl:onProperty rdf:resource="http://schema.geolink.org/dev/view#hasMeasurementType"/>
  </owl:Restriction>
  <owl:Restriction>
    <rdfs:subClassOf rdf:resource="http://schema.geolink.org/dev/voc/nvs/P02#BCMT"/>
    <owl:someValuesFrom>
      <owl:Class>
        <owl:oneOf rdf:parseType="Collection">
          <glview:MeasurementType rdf:about="http://schema.geolink.org/dev/voc/nvs/P02#BCMT"/>
        </owl:oneOf>
      </owl:Class>
    </owl:someValuesFrom>
    <owl:onProperty rdf:resource="http://schema.geolink.org/dev/view#hasMeasurementType"/>
  </owl:Restriction>
  <owl:Restriction>
    <rdfs:subClassOf>
      <glview:MeasurementType rdf:about="http://schema.geolink.org/dev/voc/nvs/P02#CSDE">
        <rdfs:subClassOf rdf:resource="http://schema.geolink.org/dev/voc/nvs/P03#O010"/>
        <rdfs:seeAlso rdf:resource="http://vocab.nerc.ac.uk/collection/P02/current/CSDE/"/>
        <rdfs:comment xml:lang="en">Parameters relating to the rates of creation and consumption of organic sulphur compounds (such as DMS and carbonyl sulphide) in the water column</rdfs:comment>
        <rdfs:label xml:lang="en">Organic sulphur compound dynamics in the water column</rdfs:label>
        <rdf:type rdf:resource="http://www.w3.org/2002/07/owl#NamedIndividual"/>
        <rdf:type rdf:resource="http://www.w3.org/2002/07/owl#Class"/>
      </glview:MeasurementType>
    </rdfs:subClassOf>
    <owl:someValuesFrom>
      <owl:Class>
        <owl:oneOf rdf:parseType="Collection">
          <glview:MeasurementType rdf:about="http://schema.geolink.org/dev/voc/nvs/P02#CSDE"/>
        </owl:oneOf>
      </owl:Class>
    </owl:someValuesFrom>
    <owl:onProperty rdf:resource="http://schema.geolink.org/dev/view#hasMeasurementType"/>
  </owl:Restriction>
  <owl:Restriction>
    <rdfs:subClassOf rdf:resource="http://schema.geolink.org/dev/voc/nvs/P02#GREF"/>
    <owl:someValuesFrom>
      <owl:Class>
        <owl:oneOf rdf:parseType="Collection">
          <glview:MeasurementType rdf:about="http://schema.geolink.org/dev/voc/nvs/P02#GREF"/>
        </owl:oneOf>
      </owl:Class>
    </owl:someValuesFrom>
    <owl:onProperty rdf:resource="http://schema.geolink.org/dev/view#hasMeasurementType"/>
  </owl:Restriction>
  <owl:Restriction>
    <rdfs:subClassOf rdf:resource="http://schema.geolink.org/dev/voc/nvs/P02#AMOX"/>
    <owl:someValuesFrom>
      <owl:Class>
        <owl:oneOf rdf:parseType="Collection">
          <glview:MeasurementType rdf:about="http://schema.geolink.org/dev/voc/nvs/P02#AMOX"/>
        </owl:oneOf>
      </owl:Class>
    </owl:someValuesFrom>
    <owl:onProperty rdf:resource="http://schema.geolink.org/dev/view#hasMeasurementType"/>
  </owl:Restriction>
  <owl:Restriction>
    <rdfs:subClassOf>
      <glview:MeasurementType rdf:about="http://schema.geolink.org/dev/voc/nvs/P02#DBDX">
        <rdfs:subClassOf rdf:resource="http://schema.geolink.org/dev/voc/nvs/P03#G040"/>
        <rdfs:seeAlso rdf:resource="http://vocab.nerc.ac.uk/collection/P02/current/DBDX/"/>
        <rdfs:comment xml:lang="en">Parameters that describe the the mass per unit volume of any samples of rock or unlithified sediment.</rdfs:comment>
        <rdfs:label xml:lang="en">Geological sample density</rdfs:label>
        <rdf:type rdf:resource="http://www.w3.org/2002/07/owl#NamedIndividual"/>
        <rdf:type rdf:resource="http://www.w3.org/2002/07/owl#Class"/>
      </glview:MeasurementType>
    </rdfs:subClassOf>
    <owl:someValuesFrom>
      <owl:Class>
        <owl:oneOf rdf:parseType="Collection">
          <glview:MeasurementType rdf:about="http://schema.geolink.org/dev/voc/nvs/P02#DBDX"/>
        </owl:oneOf>
      </owl:Class>
    </owl:someValuesFrom>
    <owl:onProperty rdf:resource="http://schema.geolink.org/dev/view#hasMeasurementType"/>
  </owl:Restriction>
  <owl:Restriction>
    <rdfs:subClassOf>
      <glview:MeasurementType rdf:about="http://schema.geolink.org/dev/voc/nvs/P02#UREA">
        <rdfs:subClassOf rdf:resource="http://schema.geolink.org/dev/voc/nvs/P03#C005"/>
        <rdfs:subClassOf rdf:resource="http://schema.geolink.org/dev/voc/nvs/P03#C040"/>
        <rdfs:seeAlso rdf:resource="http://vocab.nerc.ac.uk/collection/P02/current/UREA/"/>
        <rdfs:comment xml:lang="en">Urea concentration parameters (including statistical parameters such as standard deviation) in the water column</rdfs:comment>
        <rdfs:label xml:lang="en">Urea concentration parameters in the water column</rdfs:label>
        <rdf:type rdf:resource="http://www.w3.org/2002/07/owl#NamedIndividual"/>
        <rdf:type rdf:resource="http://www.w3.org/2002/07/owl#Class"/>
      </glview:MeasurementType>
    </rdfs:subClassOf>
    <owl:someValuesFrom>
      <owl:Class>
        <owl:oneOf rdf:parseType="Collection">
          <glview:MeasurementType rdf:about="http://schema.geolink.org/dev/voc/nvs/P02#UREA"/>
        </owl:oneOf>
      </owl:Class>
    </owl:someValuesFrom>
    <owl:onProperty rdf:resource="http://schema.geolink.org/dev/view#hasMeasurementType"/>
  </owl:Restriction>
  <owl:Restriction>
    <rdfs:subClassOf>
      <glview:MeasurementType rdf:about="http://schema.geolink.org/dev/voc/nvs/P02#IRSP">
        <rdfs:subClassOf rdf:resource="http://schema.geolink.org/dev/voc/nvs/P03#G035"/>
        <rdfs:seeAlso rdf:resource="http://vocab.nerc.ac.uk/collection/P02/current/IRSP/"/>
        <rdfs:comment xml:lang="en">Stable isotope enrichment parameters in secondary mineral deposits in caves. This includes stalactites, stalagmites, flowstone, and crystal growths.</rdfs:comment>
        <rdfs:label xml:lang="en">Stable isotope enrichment in speleothems</rdfs:label>
        <rdf:type rdf:resource="http://www.w3.org/2002/07/owl#NamedIndividual"/>
        <rdf:type rdf:resource="http://www.w3.org/2002/07/owl#Class"/>
      </glview:MeasurementType>
    </rdfs:subClassOf>
    <owl:someValuesFrom>
      <owl:Class>
        <owl:oneOf rdf:parseType="Collection">
          <glview:MeasurementType rdf:about="http://schema.geolink.org/dev/voc/nvs/P02#IRSP"/>
        </owl:oneOf>
      </owl:Class>
    </owl:someValuesFrom>
    <owl:onProperty rdf:resource="http://schema.geolink.org/dev/view#hasMeasurementType"/>
  </owl:Restriction>
  <owl:Restriction>
    <rdfs:subClassOf>
      <glview:MeasurementType rdf:about="http://schema.geolink.org/dev/voc/nvs/P02#XMGS">
        <rdfs:subClassOf rdf:resource="http://schema.geolink.org/dev/voc/nvs/P03#G040"/>
        <rdfs:subClassOf rdf:resource="http://schema.geolink.org/dev/voc/nvs/P03#G005"/>
        <rdfs:subClassOf rdf:resource="http://schema.geolink.org/dev/voc/nvs/P03#G012"/>
        <rdfs:seeAlso rdf:resource="http://vocab.nerc.ac.uk/collection/P02/current/XMGS/"/>
        <rdfs:comment xml:lang="en">Any parameters quantifying the magnetic (e.g. magnetic susceptibility), electrical (e.g. resistivity) or acoustic (e.g. P-wave propogation speed) of sediment or rock cores and samples</rdfs:comment>
        <rdfs:label xml:lang="en">Geological sample magnetic, electrical and acoustic properties</rdfs:label>
        <rdf:type rdf:resource="http://www.w3.org/2002/07/owl#NamedIndividual"/>
        <rdf:type rdf:resource="http://www.w3.org/2002/07/owl#Class"/>
      </glview:MeasurementType>
    </rdfs:subClassOf>
    <owl:someValuesFrom>
      <owl:Class>
        <owl:oneOf rdf:parseType="Collection">
          <glview:MeasurementType rdf:about="http://schema.geolink.org/dev/voc/nvs/P02#XMGS"/>
        </owl:oneOf>
      </owl:Class>
    </owl:someValuesFrom>
    <owl:onProperty rdf:resource="http://schema.geolink.org/dev/view#hasMeasurementType"/>
  </owl:Restriction>
  <owl:Restriction>
    <rdfs:subClassOf rdf:resource="http://schema.geolink.org/dev/voc/nvs/P02#ADUN"/>
    <owl:someValuesFrom>
      <owl:Class>
        <owl:oneOf rdf:parseType="Collection">
          <owl:NamedIndividual rdf:about="http://schema.geolink.org/dev/voc/nvs/P02#ADUN"/>
        </owl:oneOf>
      </owl:Class>
    </owl:someValuesFrom>
    <owl:onProperty rdf:resource="http://schema.geolink.org/dev/view#hasMeasurementType"/>
  </owl:Restriction>
  <owl:Restriction>
    <rdfs:subClassOf>
      <glview:MeasurementType rdf:about="http://schema.geolink.org/dev/voc/nvs/P02#OPBS">
        <rdfs:subClassOf rdf:resource="http://schema.geolink.org/dev/voc/nvs/P03#D015"/>
        <rdfs:seeAlso rdf:resource="http://vocab.nerc.ac.uk/collection/P02/current/OPBS/"/>
        <rdfs:comment xml:lang="en">Includes all parameters covering the strength of electromagnetic radiation signal return, including absolute measurements of returning signal strength as well as parameters expressed as backscatter (the proportion of transmitted signal returned)</rdfs:comment>
        <rdfs:label xml:lang="en">Optical backscatter</rdfs:label>
        <rdf:type rdf:resource="http://www.w3.org/2002/07/owl#NamedIndividual"/>
        <rdf:type rdf:resource="http://www.w3.org/2002/07/owl#Class"/>
      </glview:MeasurementType>
    </rdfs:subClassOf>
    <owl:someValuesFrom>
      <owl:Class>
        <owl:oneOf rdf:parseType="Collection">
          <glview:MeasurementType rdf:about="http://schema.geolink.org/dev/voc/nvs/P02#OPBS"/>
        </owl:oneOf>
      </owl:Class>
    </owl:someValuesFrom>
    <owl:onProperty rdf:resource="http://schema.geolink.org/dev/view#hasMeasurementType"/>
  </owl:Restriction>
  <owl:Restriction>
    <rdfs:subClassOf rdf:resource="http://schema.geolink.org/dev/voc/nvs/P02#BCMT"/>
    <owl:someValuesFrom>
      <owl:Class>
        <owl:oneOf rdf:parseType="Collection">
          <glview:MeasurementType rdf:about="http://schema.geolink.org/dev/voc/nvs/P02#BCMT"/>
        </owl:oneOf>
      </owl:Class>
    </owl:someValuesFrom>
    <owl:onProperty rdf:resource="http://schema.geolink.org/dev/view#hasMeasurementType"/>
  </owl:Restriction>
  <owl:Restriction>
    <rdfs:subClassOf rdf:resource="http://schema.geolink.org/dev/voc/nvs/P02#UREA"/>
    <owl:someValuesFrom>
      <owl:Class>
        <owl:oneOf rdf:parseType="Collection">
          <glview:MeasurementType rdf:about="http://schema.geolink.org/dev/voc/nvs/P02#UREA"/>
        </owl:oneOf>
      </owl:Class>
    </owl:someValuesFrom>
    <owl:onProperty rdf:resource="http://schema.geolink.org/dev/view#hasMeasurementType"/>
  </owl:Restriction>
  <owl:Restriction>
    <rdfs:subClassOf>
      <glview:MeasurementType rdf:about="http://schema.geolink.org/dev/voc/nvs/P02#CYEU">
        <rdfs:subClassOf rdf:resource="http://schema.geolink.org/dev/voc/nvs/P03#B070"/>
        <rdfs:seeAlso rdf:resource="http://vocab.nerc.ac.uk/collection/P02/current/CYEU/"/>
        <rdfs:comment xml:lang="en">Used for plankton carbon biomass parameters where no differentiation between phytoplankton, microzooplankton or zooplankton is possible</rdfs:comment>
        <rdfs:label xml:lang="en">Plankton biomass expressed as carbon per unit volume of the water column</rdfs:label>
        <rdf:type rdf:resource="http://www.w3.org/2002/07/owl#NamedIndividual"/>
        <rdf:type rdf:resource="http://www.w3.org/2002/07/owl#Class"/>
      </glview:MeasurementType>
    </rdfs:subClassOf>
    <owl:someValuesFrom>
      <owl:Class>
        <owl:oneOf rdf:parseType="Collection">
          <glview:MeasurementType rdf:about="http://schema.geolink.org/dev/voc/nvs/P02#CYEU"/>
        </owl:oneOf>
      </owl:Class>
    </owl:someValuesFrom>
    <owl:onProperty rdf:resource="http://schema.geolink.org/dev/view#hasMeasurementType"/>
  </owl:Restriction>
  <owl:Restriction>
    <rdfs:subClassOf>
      <glview:MeasurementType rdf:about="http://schema.geolink.org/dev/voc/nvs/P02#GP085">
        <rdfs:subClassOf rdf:resource="http://schema.geolink.org/dev/voc/nvs/P03#B020"/>
        <rdfs:seeAlso rdf:resource="http://vocab.nerc.ac.uk/collection/P02/current/GP085/"/>
        <rdfs:comment xml:lang="en">Parameters describing the actions or reactions of fish (Osteichthyes, Agnatha and Chondrichthyes), usually in response to the environment. Includes both parameters mapped to taxa and those mapped to non-taxonomic groupings.</rdfs:comment>
        <rdfs:label xml:lang="en">Fish behaviour</rdfs:label>
        <rdf:type rdf:resource="http://www.w3.org/2002/07/owl#NamedIndividual"/>
        <rdf:type rdf:resource="http://www.w3.org/2002/07/owl#Class"/>
      </glview:MeasurementType>
    </rdfs:subClassOf>
    <owl:someValuesFrom>
      <owl:Class>
        <owl:oneOf rdf:parseType="Collection">
          <glview:MeasurementType rdf:about="http://schema.geolink.org/dev/voc/nvs/P02#GP085"/>
        </owl:oneOf>
      </owl:Class>
    </owl:someValuesFrom>
    <owl:onProperty rdf:resource="http://schema.geolink.org/dev/view#hasMeasurementType"/>
  </owl:Restriction>
  <owl:Restriction>
    <rdfs:subClassOf>
      <glview:MeasurementType rdf:about="http://schema.geolink.org/dev/voc/nvs/P02#DAAW">
        <rdfs:subClassOf rdf:resource="http://schema.geolink.org/dev/voc/nvs/P03#C003"/>
        <rdfs:seeAlso rdf:resource="http://vocab.nerc.ac.uk/collection/P02/current/DAAW/"/>
        <rdfs:comment xml:lang="en">Parameters quantifying the amount of organic compounds containing both a carboxyl group and an amino group in solids suspended in a body of water.</rdfs:comment>
        <rdfs:label xml:lang="en">Particulate amino acid concentrations in the water column</rdfs:label>
        <rdf:type rdf:resource="http://www.w3.org/2002/07/owl#NamedIndividual"/>
        <rdf:type rdf:resource="http://www.w3.org/2002/07/owl#Class"/>
      </glview:MeasurementType>
    </rdfs:subClassOf>
    <owl:someValuesFrom>
      <owl:Class>
        <owl:oneOf rdf:parseType="Collection">
          <glview:MeasurementType rdf:about="http://schema.geolink.org/dev/voc/nvs/P02#DAAW"/>
        </owl:oneOf>
      </owl:Class>
    </owl:someValuesFrom>
    <owl:onProperty rdf:resource="http://schema.geolink.org/dev/view#hasMeasurementType"/>
  </owl:Restriction>
  <owl:Restriction>
    <rdfs:subClassOf>
      <glview:MeasurementType rdf:about="http://schema.geolink.org/dev/voc/nvs/P02#ISIC">
        <rdfs:subClassOf>
          <glview:MeasurementType rdf:about="http://schema.geolink.org/dev/voc/nvs/P02#ICHM">
            <rdfs:subClassOf rdf:resource="http://schema.geolink.org/dev/voc/nvs/P03#M015"/>
            <rdfs:seeAlso rdf:resource="http://vocab.nerc.ac.uk/collection/P02/current/ICHM/"/>
            <rdfs:comment xml:lang="en">Parameters related to the chemical composition of any kind of water sample that was frozen solid at the time of sampling or measurement</rdfs:comment>
            <rdfs:label xml:lang="en">Snow and ice chemistry</rdfs:label>
            <rdf:type rdf:resource="http://www.w3.org/2002/07/owl#NamedIndividual"/>
            <rdf:type rdf:resource="http://www.w3.org/2002/07/owl#Class"/>
          </glview:MeasurementType>
        </rdfs:subClassOf>
        <rdfs:seeAlso rdf:resource="http://vocab.nerc.ac.uk/collection/P02/current/ISIC/"/>
        <rdfs:comment xml:lang="en">Concentration parameters for inorganic sulphur species in ice</rdfs:comment>
        <rdfs:label xml:lang="en">Concentration of inorganic sulphur species in ice</rdfs:label>
        <rdf:type rdf:resource="http://www.w3.org/2002/07/owl#NamedIndividual"/>
        <rdf:type rdf:resource="http://www.w3.org/2002/07/owl#Class"/>
      </glview:MeasurementType>
    </rdfs:subClassOf>
    <owl:someValuesFrom>
      <owl:Class>
        <owl:oneOf rdf:parseType="Collection">
          <glview:MeasurementType rdf:about="http://schema.geolink.org/dev/voc/nvs/P02#ISIC"/>
        </owl:oneOf>
      </owl:Class>
    </owl:someValuesFrom>
    <owl:onProperty rdf:resource="http://schema.geolink.org/dev/view#hasMeasurementType"/>
  </owl:Restriction>
  <owl:Restriction>
    <rdfs:subClassOf>
      <glview:MeasurementType rdf:about="http://schema.geolink.org/dev/voc/nvs/P02#MTSD">
        <rdfs:subClassOf rdf:resource="http://schema.geolink.org/dev/voc/nvs/P02#RMIN"/>
        <rdfs:seeAlso rdf:resource="http://vocab.nerc.ac.uk/collection/P02/current/MTSD/"/>
        <rdfs:comment xml:lang="en">Concentrations of metal elements per unit weight of sediment.  Sediment is understood to be the solid phase of the bed, including the recently settled material sometimes known as fluff collected from the bed surface.</rdfs:comment>
        <rdfs:label xml:lang="en">Metal concentrations in sediment</rdfs:label>
        <rdf:type rdf:resource="http://www.w3.org/2002/07/owl#NamedIndividual"/>
        <rdf:type rdf:resource="http://www.w3.org/2002/07/owl#Class"/>
      </glview:MeasurementType>
    </rdfs:subClassOf>
    <owl:someValuesFrom>
      <owl:Class>
        <owl:oneOf rdf:parseType="Collection">
          <glview:MeasurementType rdf:about="http://schema.geolink.org/dev/voc/nvs/P02#MTSD"/>
        </owl:oneOf>
      </owl:Class>
    </owl:someValuesFrom>
    <owl:onProperty rdf:resource="http://schema.geolink.org/dev/view#hasMeasurementType"/>
  </owl:Restriction>
  <owl:Restriction>
    <rdfs:subClassOf rdf:resource="http://schema.geolink.org/dev/voc/nvs/P02#OMPW"/>
    <owl:someValuesFrom>
      <owl:Class>
        <owl:oneOf rdf:parseType="Collection">
          <owl:NamedIndividual rdf:about="http://schema.geolink.org/dev/voc/nvs/P02#OMPW"/>
        </owl:oneOf>
      </owl:Class>
    </owl:someValuesFrom>
    <owl:onProperty rdf:resource="http://schema.geolink.org/dev/view#hasMeasurementType"/>
  </owl:Restriction>
  <owl:Restriction>
    <rdfs:subClassOf rdf:resource="http://schema.geolink.org/dev/voc/nvs/P02#MTWP"/>
    <owl:someValuesFrom>
      <owl:Class>
        <owl:oneOf rdf:parseType="Collection">
          <glview:MeasurementType rdf:about="http://schema.geolink.org/dev/voc/nvs/P02#MTWP"/>
        </owl:oneOf>
      </owl:Class>
    </owl:someValuesFrom>
    <owl:onProperty rdf:resource="http://schema.geolink.org/dev/view#hasMeasurementType"/>
  </owl:Restriction>
  <owl:Restriction>
    <rdfs:subClassOf rdf:resource="http://schema.geolink.org/dev/voc/nvs/P02#MSBD"/>
    <owl:someValuesFrom>
      <owl:Class>
        <owl:oneOf rdf:parseType="Collection">
          <glview:MeasurementType rdf:about="http://schema.geolink.org/dev/voc/nvs/P02#MSBD"/>
        </owl:oneOf>
      </owl:Class>
    </owl:someValuesFrom>
    <owl:onProperty rdf:resource="http://schema.geolink.org/dev/view#hasMeasurementType"/>
  </owl:Restriction>
  <owl:Restriction>
    <rdfs:subClassOf>
      <glview:MeasurementType rdf:about="http://schema.geolink.org/dev/voc/nvs/P02#HFLX">
        <rdfs:subClassOf rdf:resource="http://schema.geolink.org/dev/voc/nvs/P03#D020"/>
        <rdfs:subClassOf rdf:resource="http://schema.geolink.org/dev/voc/nvs/P03#O005"/>
        <rdfs:seeAlso rdf:resource="http://vocab.nerc.ac.uk/collection/P02/current/HFLX/"/>
        <rdfs:comment xml:lang="en">Parameters quantifying heat exchange between any body of water and the atmosphere</rdfs:comment>
        <rdfs:label xml:lang="en">Heat fluxes between the water column and the atmosphere</rdfs:label>
        <rdf:type rdf:resource="http://www.w3.org/2002/07/owl#NamedIndividual"/>
        <rdf:type rdf:resource="http://www.w3.org/2002/07/owl#Class"/>
      </glview:MeasurementType>
    </rdfs:subClassOf>
    <owl:someValuesFrom>
      <owl:Class>
        <owl:oneOf rdf:parseType="Collection">
          <glview:MeasurementType rdf:about="http://schema.geolink.org/dev/voc/nvs/P02#HFLX"/>
        </owl:oneOf>
      </owl:Class>
    </owl:someValuesFrom>
    <owl:onProperty rdf:resource="http://schema.geolink.org/dev/view#hasMeasurementType"/>
  </owl:Restriction>
  <owl:Restriction>
    <rdfs:subClassOf rdf:resource="http://schema.geolink.org/dev/voc/nvs/P02#ADUN"/>
    <owl:someValuesFrom>
      <owl:Class>
        <owl:oneOf rdf:parseType="Collection">
          <owl:NamedIndividual rdf:about="http://schema.geolink.org/dev/voc/nvs/P02#ADUN"/>
        </owl:oneOf>
      </owl:Class>
    </owl:someValuesFrom>
    <owl:onProperty rdf:resource="http://schema.geolink.org/dev/view#hasMeasurementType"/>
  </owl:Restriction>
  <owl:Restriction>
    <rdfs:subClassOf>
      <glview:MeasurementType rdf:about="http://schema.geolink.org/dev/voc/nvs/P02#FREP">
        <rdfs:subClassOf rdf:resource="http://schema.geolink.org/dev/voc/nvs/P03#B027"/>
        <rdfs:subClassOf rdf:resource="http://schema.geolink.org/dev/voc/nvs/P03#B020"/>
        <rdfs:subClassOf rdf:resource="http://schema.geolink.org/dev/voc/nvs/P03#H004"/>
        <rdfs:seeAlso rdf:resource="http://vocab.nerc.ac.uk/collection/P02/current/FREP/"/>
        <rdfs:comment xml:lang="en">Paramaters that quantify the fecundity, reproductive rates or nature of reproduction in fish (Osteichthyes, Agnatha and Chrondrichthyes).</rdfs:comment>
        <rdfs:label xml:lang="en">Fish reproduction</rdfs:label>
        <rdf:type rdf:resource="http://www.w3.org/2002/07/owl#NamedIndividual"/>
        <rdf:type rdf:resource="http://www.w3.org/2002/07/owl#Class"/>
      </glview:MeasurementType>
    </rdfs:subClassOf>
    <owl:someValuesFrom>
      <owl:Class>
        <owl:oneOf rdf:parseType="Collection">
          <glview:MeasurementType rdf:about="http://schema.geolink.org/dev/voc/nvs/P02#FREP"/>
        </owl:oneOf>
      </owl:Class>
    </owl:someValuesFrom>
    <owl:onProperty rdf:resource="http://schema.geolink.org/dev/view#hasMeasurementType"/>
  </owl:Restriction>
  <owl:Restriction>
    <rdfs:subClassOf>
      <glview:MeasurementType rdf:about="http://schema.geolink.org/dev/voc/nvs/P02#FPRT">
        <rdfs:subClassOf rdf:resource="http://schema.geolink.org/dev/voc/nvs/P03#B045"/>
        <rdfs:subClassOf rdf:resource="http://schema.geolink.org/dev/voc/nvs/P03#O010"/>
        <rdfs:seeAlso rdf:resource="http://vocab.nerc.ac.uk/collection/P02/current/FPRT/"/>
        <rdfs:comment xml:lang="en">Faecal pellet production and gut evacuation rates</rdfs:comment>
        <rdfs:label xml:lang="en">Zooplankton defecation rates in the water column</rdfs:label>
        <rdf:type rdf:resource="http://www.w3.org/2002/07/owl#NamedIndividual"/>
        <rdf:type rdf:resource="http://www.w3.org/2002/07/owl#Class"/>
      </glview:MeasurementType>
    </rdfs:subClassOf>
    <owl:someValuesFrom>
      <owl:Class>
        <owl:oneOf rdf:parseType="Collection">
          <glview:MeasurementType rdf:about="http://schema.geolink.org/dev/voc/nvs/P02#FPRT"/>
        </owl:oneOf>
      </owl:Class>
    </owl:someValuesFrom>
    <owl:onProperty rdf:resource="http://schema.geolink.org/dev/view#hasMeasurementType"/>
  </owl:Restriction>
  <owl:Restriction>
    <rdfs:subClassOf>
      <glview:MeasurementType rdf:about="http://schema.geolink.org/dev/voc/nvs/P02#OCAA">
        <rdfs:subClassOf rdf:resource="http://schema.geolink.org/dev/voc/nvs/P03#H001"/>
        <rdfs:subClassOf rdf:resource="http://schema.geolink.org/dev/voc/nvs/P03#M005"/>
        <rdfs:seeAlso rdf:resource="http://vocab.nerc.ac.uk/collection/P02/current/OCAA/"/>
        <rdfs:comment xml:lang="en">Parameters quantifying concentrations of organic contaminants (substances regarded as harmful) other than PCBs and PAHs in all phases of the atmosphere</rdfs:comment>
        <rdfs:label xml:lang="en">Concentration of other organic contaminants in the atmosphere</rdfs:label>
        <rdf:type rdf:resource="http://www.w3.org/2002/07/owl#NamedIndividual"/>
        <rdf:type rdf:resource="http://www.w3.org/2002/07/owl#Class"/>
      </glview:MeasurementType>
    </rdfs:subClassOf>
    <owl:someValuesFrom>
      <owl:Class>
        <owl:oneOf rdf:parseType="Collection">
          <glview:MeasurementType rdf:about="http://schema.geolink.org/dev/voc/nvs/P02#OCAA"/>
        </owl:oneOf>
      </owl:Class>
    </owl:someValuesFrom>
    <owl:onProperty rdf:resource="http://schema.geolink.org/dev/view#hasMeasurementType"/>
  </owl:Restriction>
  <owl:Restriction>
    <rdfs:subClassOf>
      <glview:MeasurementType rdf:about="http://schema.geolink.org/dev/voc/nvs/P02#PESD">
        <rdfs:subClassOf rdf:resource="http://schema.geolink.org/dev/voc/nvs/P03#C055"/>
        <rdfs:subClassOf rdf:resource="http://schema.geolink.org/dev/voc/nvs/P03#H001"/>
        <rdfs:subClassOf rdf:resource="http://schema.geolink.org/dev/voc/nvs/P03#G035"/>
        <rdfs:seeAlso rdf:resource="http://vocab.nerc.ac.uk/collection/P02/current/PESD/"/>
        <rdfs:comment xml:lang="en">Concentration parameters for substances synthesised by man to kill other life forms in sediment, which is considered to be anything from the bed sampled by a grab or corer, including 'fluff'.</rdfs:comment>
        <rdfs:label xml:lang="en">Pesticide concentrations in sediment</rdfs:label>
        <rdf:type rdf:resource="http://www.w3.org/2002/07/owl#NamedIndividual"/>
        <rdf:type rdf:resource="http://www.w3.org/2002/07/owl#Class"/>
      </glview:MeasurementType>
    </rdfs:subClassOf>
    <owl:someValuesFrom>
      <owl:Class>
        <owl:oneOf rdf:parseType="Collection">
          <glview:MeasurementType rdf:about="http://schema.geolink.org/dev/voc/nvs/P02#PESD"/>
        </owl:oneOf>
      </owl:Class>
    </owl:someValuesFrom>
    <owl:onProperty rdf:resource="http://schema.geolink.org/dev/view#hasMeasurementType"/>
  </owl:Restriction>
  <owl:Restriction>
    <rdfs:subClassOf>
      <glview:MeasurementType rdf:about="http://schema.geolink.org/dev/voc/nvs/P02#AMON">
        <rdfs:subClassOf rdf:resource="http://schema.geolink.org/dev/voc/nvs/P03#C005"/>
        <rdfs:subClassOf rdf:resource="http://schema.geolink.org/dev/voc/nvs/P03#C040"/>
        <rdfs:seeAlso rdf:resource="http://vocab.nerc.ac.uk/collection/P02/current/AMON/"/>
        <rdfs:comment xml:lang="en">Ammonium concentration parameters (including statistical parameters such as standard deviation) in the water column</rdfs:comment>
        <rdfs:label xml:lang="en">Ammonium concentration parameters in the water column</rdfs:label>
        <rdf:type rdf:resource="http://www.w3.org/2002/07/owl#NamedIndividual"/>
        <rdf:type rdf:resource="http://www.w3.org/2002/07/owl#Class"/>
      </glview:MeasurementType>
    </rdfs:subClassOf>
    <owl:someValuesFrom>
      <owl:Class>
        <owl:oneOf rdf:parseType="Collection">
          <glview:MeasurementType rdf:about="http://schema.geolink.org/dev/voc/nvs/P02#AMON"/>
        </owl:oneOf>
      </owl:Class>
    </owl:someValuesFrom>
    <owl:onProperty rdf:resource="http://schema.geolink.org/dev/view#hasMeasurementType"/>
  </owl:Restriction>
  <owl:Restriction>
    <rdfs:subClassOf>
      <glview:MeasurementType rdf:about="http://schema.geolink.org/dev/voc/nvs/P02#MZBN">
        <rdfs:subClassOf rdf:resource="http://schema.geolink.org/dev/voc/nvs/P03#B025"/>
        <rdfs:subClassOf rdf:resource="http://schema.geolink.org/dev/voc/nvs/P03#B070"/>
        <rdfs:seeAlso rdf:resource="http://vocab.nerc.ac.uk/collection/P02/current/MZBN/"/>
        <rdfs:comment xml:lang="en">Any enumeration (e.g. count, number per litre) of microzooplankton (free swimming heterotrophic organisms smaller than 200um) designated by terms other than taxonomic names (e.g. total) in any fresh or salt water body.</rdfs:comment>
        <rdfs:label xml:lang="en">Microzooplankton generic abundance in water bodies</rdfs:label>
        <rdf:type rdf:resource="http://www.w3.org/2002/07/owl#NamedIndividual"/>
        <rdf:type rdf:resource="http://www.w3.org/2002/07/owl#Class"/>
      </glview:MeasurementType>
    </rdfs:subClassOf>
    <owl:someValuesFrom>
      <owl:Class>
        <owl:oneOf rdf:parseType="Collection">
          <glview:MeasurementType rdf:about="http://schema.geolink.org/dev/voc/nvs/P02#MZBN"/>
        </owl:oneOf>
      </owl:Class>
    </owl:someValuesFrom>
    <owl:onProperty rdf:resource="http://schema.geolink.org/dev/view#hasMeasurementType"/>
  </owl:Restriction>
  <owl:Restriction>
    <rdfs:subClassOf>
      <glview:MeasurementType rdf:about="http://schema.geolink.org/dev/voc/nvs/P02#LIFX">
        <rdfs:subClassOf rdf:resource="http://schema.geolink.org/dev/voc/nvs/P03#O005"/>
        <rdfs:seeAlso rdf:resource="http://vocab.nerc.ac.uk/collection/P02/current/LIFX/"/>
        <rdfs:comment xml:lang="en">Fluxes of terrestrial biological or lithological material</rdfs:comment>
        <rdfs:label xml:lang="en">Sedimentation flux of terrestrially derived material in the water column</rdfs:label>
        <rdf:type rdf:resource="http://www.w3.org/2002/07/owl#NamedIndividual"/>
        <rdf:type rdf:resource="http://www.w3.org/2002/07/owl#Class"/>
      </glview:MeasurementType>
    </rdfs:subClassOf>
    <owl:someValuesFrom>
      <owl:Class>
        <owl:oneOf rdf:parseType="Collection">
          <glview:MeasurementType rdf:about="http://schema.geolink.org/dev/voc/nvs/P02#LIFX"/>
        </owl:oneOf>
      </owl:Class>
    </owl:someValuesFrom>
    <owl:onProperty rdf:resource="http://schema.geolink.org/dev/view#hasMeasurementType"/>
  </owl:Restriction>
  <owl:Restriction>
    <rdfs:subClassOf rdf:resource="http://schema.geolink.org/dev/voc/nvs/P02#XMGS"/>
    <owl:someValuesFrom>
      <owl:Class>
        <owl:oneOf rdf:parseType="Collection">
          <glview:MeasurementType rdf:about="http://schema.geolink.org/dev/voc/nvs/P02#XMGS"/>
        </owl:oneOf>
      </owl:Class>
    </owl:someValuesFrom>
    <owl:onProperty rdf:resource="http://schema.geolink.org/dev/view#hasMeasurementType"/>
  </owl:Restriction>
  <owl:Restriction>
    <rdfs:subClassOf>
      <glview:MeasurementType rdf:about="http://schema.geolink.org/dev/voc/nvs/P02#MDWP">
        <rdfs:subClassOf rdf:resource="http://schema.geolink.org/dev/voc/nvs/P03#C035"/>
        <rdfs:subClassOf rdf:resource="http://schema.geolink.org/dev/voc/nvs/P03#G015"/>
        <rdfs:seeAlso rdf:resource="http://vocab.nerc.ac.uk/collection/P02/current/MDWP/"/>
        <rdfs:comment xml:lang="en">Concentration parameters for trace metalloid elements in the particulate phase of the water column collected by fitration, centrifugation or sediment trapping. Trace metalloids are considered as B, Ge, As, Sb, Te and Po (but not Si which is classed separately because of its major role in environmental chemistry)</rdfs:comment>
        <rdfs:label xml:lang="en">Particulate trace metalloid concentrations in the water column</rdfs:label>
        <rdf:type rdf:resource="http://www.w3.org/2002/07/owl#NamedIndividual"/>
        <rdf:type rdf:resource="http://www.w3.org/2002/07/owl#Class"/>
      </glview:MeasurementType>
    </rdfs:subClassOf>
    <owl:someValuesFrom>
      <owl:Class>
        <owl:oneOf rdf:parseType="Collection">
          <glview:MeasurementType rdf:about="http://schema.geolink.org/dev/voc/nvs/P02#MDWP"/>
        </owl:oneOf>
      </owl:Class>
    </owl:someValuesFrom>
    <owl:onProperty rdf:resource="http://schema.geolink.org/dev/view#hasMeasurementType"/>
  </owl:Restriction>
  <owl:Restriction>
    <rdfs:subClassOf>
      <glview:MeasurementType rdf:about="http://schema.geolink.org/dev/voc/nvs/P02#ASLV">
        <rdfs:subClassOf rdf:resource="http://schema.geolink.org/dev/voc/nvs/P03#D032"/>
        <rdfs:seeAlso rdf:resource="http://vocab.nerc.ac.uk/collection/P02/current/ASLV/"/>
        <rdfs:comment xml:lang="en">Measurements and predictions of the displacement of the water column surface from a fixed, stable reference</rdfs:comment>
        <rdfs:label xml:lang="en">Sea level</rdfs:label>
        <rdf:type rdf:resource="http://www.w3.org/2002/07/owl#NamedIndividual"/>
        <rdf:type rdf:resource="http://www.w3.org/2002/07/owl#Class"/>
      </glview:MeasurementType>
    </rdfs:subClassOf>
    <owl:someValuesFrom>
      <owl:Class>
        <owl:oneOf rdf:parseType="Collection">
          <glview:MeasurementType rdf:about="http://schema.geolink.org/dev/voc/nvs/P02#ASLV"/>
        </owl:oneOf>
      </owl:Class>
    </owl:someValuesFrom>
    <owl:onProperty rdf:resource="http://schema.geolink.org/dev/view#hasMeasurementType"/>
  </owl:Restriction>
  <owl:Restriction>
    <rdfs:subClassOf>
      <glview:MeasurementType rdf:about="http://schema.geolink.org/dev/voc/nvs/P02#NTIC">
        <rdfs:subClassOf rdf:resource="http://schema.geolink.org/dev/voc/nvs/P02#ICHM"/>
        <rdfs:seeAlso rdf:resource="http://vocab.nerc.ac.uk/collection/P02/current/NTIC/"/>
        <rdfs:comment xml:lang="en">Nitrate concentration parameters in ice. Includes nitrate+nitrite, which is often loosely referred to as nitrate.</rdfs:comment>
        <rdfs:label xml:lang="en">Concentration of nitrates in ice</rdfs:label>
        <rdf:type rdf:resource="http://www.w3.org/2002/07/owl#NamedIndividual"/>
        <rdf:type rdf:resource="http://www.w3.org/2002/07/owl#Class"/>
      </glview:MeasurementType>
    </rdfs:subClassOf>
    <owl:someValuesFrom>
      <owl:Class>
        <owl:oneOf rdf:parseType="Collection">
          <glview:MeasurementType rdf:about="http://schema.geolink.org/dev/voc/nvs/P02#NTIC"/>
        </owl:oneOf>
      </owl:Class>
    </owl:someValuesFrom>
    <owl:onProperty rdf:resource="http://schema.geolink.org/dev/view#hasMeasurementType"/>
  </owl:Restriction>
  <owl:Restriction>
    <rdfs:subClassOf>
      <glview:MeasurementType rdf:about="http://schema.geolink.org/dev/voc/nvs/P02#GP068">
        <rdfs:subClassOf rdf:resource="http://schema.geolink.org/dev/voc/nvs/P03#B070"/>
        <rdfs:subClassOf rdf:resource="http://schema.geolink.org/dev/voc/nvs/P03#B015"/>
        <rdfs:seeAlso rdf:resource="http://vocab.nerc.ac.uk/collection/P02/current/GP068/"/>
        <rdfs:comment xml:lang="en">Parameters related to the abundance of reptiles (Class Reptilia)</rdfs:comment>
        <rdfs:label xml:lang="en">Reptile abundance</rdfs:label>
        <rdf:type rdf:resource="http://www.w3.org/2002/07/owl#NamedIndividual"/>
        <rdf:type rdf:resource="http://www.w3.org/2002/07/owl#Class"/>
      </glview:MeasurementType>
    </rdfs:subClassOf>
    <owl:someValuesFrom>
      <owl:Class>
        <owl:oneOf rdf:parseType="Collection">
          <glview:MeasurementType rdf:about="http://schema.geolink.org/dev/voc/nvs/P02#GP068"/>
        </owl:oneOf>
      </owl:Class>
    </owl:someValuesFrom>
    <owl:onProperty rdf:resource="http://schema.geolink.org/dev/view#hasMeasurementType"/>
  </owl:Restriction>
  <owl:Restriction>
    <rdfs:subClassOf rdf:resource="http://schema.geolink.org/dev/voc/nvs/P02#PESD"/>
    <owl:someValuesFrom>
      <owl:Class>
        <owl:oneOf rdf:parseType="Collection">
          <glview:MeasurementType rdf:about="http://schema.geolink.org/dev/voc/nvs/P02#PESD"/>
        </owl:oneOf>
      </owl:Class>
    </owl:someValuesFrom>
    <owl:onProperty rdf:resource="http://schema.geolink.org/dev/view#hasMeasurementType"/>
  </owl:Restriction>
  <owl:Restriction>
    <rdfs:subClassOf rdf:resource="http://schema.geolink.org/dev/voc/nvs/P02#AMUP"/>
    <owl:someValuesFrom>
      <owl:Class>
        <owl:oneOf rdf:parseType="Collection">
          <glview:MeasurementType rdf:about="http://schema.geolink.org/dev/voc/nvs/P02#AMUP"/>
        </owl:oneOf>
      </owl:Class>
    </owl:someValuesFrom>
    <owl:onProperty rdf:resource="http://schema.geolink.org/dev/view#hasMeasurementType"/>
  </owl:Restriction>
  <owl:Restriction>
    <rdfs:subClassOf>
      <glview:MeasurementType rdf:about="http://schema.geolink.org/dev/voc/nvs/P02#TRIS">
        <rdfs:subClassOf rdf:resource="http://schema.geolink.org/dev/voc/nvs/P03#C045"/>
        <rdfs:subClassOf rdf:resource="http://schema.geolink.org/dev/voc/nvs/P03#G035"/>
        <rdfs:seeAlso rdf:resource="http://vocab.nerc.ac.uk/collection/P02/current/TRIS/"/>
        <rdfs:comment xml:lang="en">Concentration parameters for inorganic sulphur species in sediment (anything collected by a corer including fluff)</rdfs:comment>
        <rdfs:label xml:lang="en">Concentration of inorganic sulphur species in sediment</rdfs:label>
        <rdf:type rdf:resource="http://www.w3.org/2002/07/owl#NamedIndividual"/>
        <rdf:type rdf:resource="http://www.w3.org/2002/07/owl#Class"/>
      </glview:MeasurementType>
    </rdfs:subClassOf>
    <owl:someValuesFrom>
      <owl:Class>
        <owl:oneOf rdf:parseType="Collection">
          <glview:MeasurementType rdf:about="http://schema.geolink.org/dev/voc/nvs/P02#TRIS"/>
        </owl:oneOf>
      </owl:Class>
    </owl:someValuesFrom>
    <owl:onProperty rdf:resource="http://schema.geolink.org/dev/view#hasMeasurementType"/>
  </owl:Restriction>
  <owl:Restriction>
    <rdfs:subClassOf>
      <glview:MeasurementType rdf:about="http://schema.geolink.org/dev/voc/nvs/P02#LSST">
        <rdfs:subClassOf rdf:resource="http://schema.geolink.org/dev/voc/nvs/P03#T001"/>
        <rdfs:seeAlso rdf:resource="http://vocab.nerc.ac.uk/collection/P02/current/LSST/"/>
        <rdfs:comment xml:lang="en">Parameters relating to land surface temperature including fire and other hot spot location</rdfs:comment>
        <rdfs:label xml:lang="en">Land surface temperature</rdfs:label>
        <rdf:type rdf:resource="http://www.w3.org/2002/07/owl#NamedIndividual"/>
        <rdf:type rdf:resource="http://www.w3.org/2002/07/owl#Class"/>
      </glview:MeasurementType>
    </rdfs:subClassOf>
    <owl:someValuesFrom>
      <owl:Class>
        <owl:oneOf rdf:parseType="Collection">
          <glview:MeasurementType rdf:about="http://schema.geolink.org/dev/voc/nvs/P02#LSST"/>
        </owl:oneOf>
      </owl:Class>
    </owl:someValuesFrom>
    <owl:onProperty rdf:resource="http://schema.geolink.org/dev/view#hasMeasurementType"/>
  </owl:Restriction>
  <owl:Restriction>
    <rdfs:subClassOf>
      <glview:MeasurementType rdf:about="http://schema.geolink.org/dev/voc/nvs/P02#RVDS">
        <rdfs:subClassOf rdf:resource="http://schema.geolink.org/dev/voc/nvs/P03#D030"/>
        <rdfs:subClassOf rdf:resource="http://schema.geolink.org/dev/voc/nvs/P03#H001"/>
        <rdfs:subClassOf rdf:resource="http://schema.geolink.org/dev/voc/nvs/P03#O005"/>
        <rdfs:seeAlso rdf:resource="http://vocab.nerc.ac.uk/collection/P02/current/RVDS/"/>
        <rdfs:comment xml:lang="en">Parameters related to the volume of water passing through a point in a river system per unit time, including the rates of freshwater, dissolved material and particulate load discharge from a river into the sea.</rdfs:comment>
        <rdfs:label xml:lang="en">River flow and discharge</rdfs:label>
        <rdf:type rdf:resource="http://www.w3.org/2002/07/owl#NamedIndividual"/>
        <rdf:type rdf:resource="http://www.w3.org/2002/07/owl#Class"/>
      </glview:MeasurementType>
    </rdfs:subClassOf>
    <owl:someValuesFrom>
      <owl:Class>
        <owl:oneOf rdf:parseType="Collection">
          <glview:MeasurementType rdf:about="http://schema.geolink.org/dev/voc/nvs/P02#RVDS"/>
        </owl:oneOf>
      </owl:Class>
    </owl:someValuesFrom>
    <owl:onProperty rdf:resource="http://schema.geolink.org/dev/view#hasMeasurementType"/>
  </owl:Restriction>
  <owl:Restriction>
    <rdfs:subClassOf rdf:resource="http://schema.geolink.org/dev/voc/nvs/P02#HFLX"/>
    <owl:someValuesFrom>
      <owl:Class>
        <owl:oneOf rdf:parseType="Collection">
          <glview:MeasurementType rdf:about="http://schema.geolink.org/dev/voc/nvs/P02#HFLX"/>
        </owl:oneOf>
      </owl:Class>
    </owl:someValuesFrom>
    <owl:onProperty rdf:resource="http://schema.geolink.org/dev/view#hasMeasurementType"/>
  </owl:Restriction>
  <owl:Restriction>
    <rdfs:subClassOf rdf:resource="http://schema.geolink.org/dev/voc/nvs/P02#OMBI"/>
    <owl:someValuesFrom>
      <owl:Class>
        <owl:oneOf rdf:parseType="Collection">
          <glview:MeasurementType rdf:about="http://schema.geolink.org/dev/voc/nvs/P02#OMBI"/>
        </owl:oneOf>
      </owl:Class>
    </owl:someValuesFrom>
    <owl:onProperty rdf:resource="http://schema.geolink.org/dev/view#hasMeasurementType"/>
  </owl:Restriction>
  <owl:Restriction>
    <rdfs:subClassOf>
      <glview:MeasurementType rdf:about="http://schema.geolink.org/dev/voc/nvs/P02#RTCO">
        <rdfs:subClassOf rdf:resource="http://schema.geolink.org/dev/voc/nvs/P03#GTHM"/>
        <rdfs:subClassOf rdf:resource="http://schema.geolink.org/dev/voc/nvs/P03#G040"/>
        <rdfs:seeAlso rdf:resource="http://vocab.nerc.ac.uk/collection/P02/current/RTCO/"/>
        <rdfs:comment xml:lang="en">Parameters that describe the degree to which sedimentary, igneous or metamorphic rocks are able to conduct heat</rdfs:comment>
        <rdfs:label xml:lang="en">Rock thermal conductivity</rdfs:label>
        <rdf:type rdf:resource="http://www.w3.org/2002/07/owl#NamedIndividual"/>
        <rdf:type rdf:resource="http://www.w3.org/2002/07/owl#Class"/>
      </glview:MeasurementType>
    </rdfs:subClassOf>
    <owl:someValuesFrom>
      <owl:Class>
        <owl:oneOf rdf:parseType="Collection">
          <glview:MeasurementType rdf:about="http://schema.geolink.org/dev/voc/nvs/P02#RTCO"/>
        </owl:oneOf>
      </owl:Class>
    </owl:someValuesFrom>
    <owl:onProperty rdf:resource="http://schema.geolink.org/dev/view#hasMeasurementType"/>
  </owl:Restriction>
  <owl:Restriction>
    <rdfs:subClassOf rdf:resource="http://schema.geolink.org/dev/voc/nvs/P02#CASD"/>
    <owl:someValuesFrom>
      <owl:Class>
        <owl:oneOf rdf:parseType="Collection">
          <glview:MeasurementType rdf:about="http://schema.geolink.org/dev/voc/nvs/P02#CASD"/>
        </owl:oneOf>
      </owl:Class>
    </owl:someValuesFrom>
    <owl:onProperty rdf:resource="http://schema.geolink.org/dev/view#hasMeasurementType"/>
  </owl:Restriction>
  <owl:Restriction>
    <rdfs:subClassOf rdf:resource="http://schema.geolink.org/dev/voc/nvs/P02#RMIN"/>
    <owl:someValuesFrom>
      <owl:Class>
        <owl:oneOf rdf:parseType="Collection">
          <glview:MeasurementType rdf:about="http://schema.geolink.org/dev/voc/nvs/P02#RMIN"/>
        </owl:oneOf>
      </owl:Class>
    </owl:someValuesFrom>
    <owl:onProperty rdf:resource="http://schema.geolink.org/dev/view#hasMeasurementType"/>
  </owl:Restriction>
  <owl:Restriction>
    <rdfs:subClassOf>
      <glview:MeasurementType rdf:about="http://schema.geolink.org/dev/voc/nvs/P02#OCPW">
        <rdfs:subClassOf rdf:resource="http://schema.geolink.org/dev/voc/nvs/P03#G050"/>
        <rdfs:subClassOf rdf:resource="http://schema.geolink.org/dev/voc/nvs/P03#C005"/>
        <rdfs:seeAlso rdf:resource="http://vocab.nerc.ac.uk/collection/P02/current/OCPW/"/>
        <rdfs:comment xml:lang="en">Concentrations of dissolved organic carbon in sediment pore waters</rdfs:comment>
        <rdfs:label xml:lang="en">Dissolved organic carbon concentrations in sediment pore waters</rdfs:label>
        <rdf:type rdf:resource="http://www.w3.org/2002/07/owl#NamedIndividual"/>
        <rdf:type rdf:resource="http://www.w3.org/2002/07/owl#Class"/>
      </glview:MeasurementType>
    </rdfs:subClassOf>
    <owl:someValuesFrom>
      <owl:Class>
        <owl:oneOf rdf:parseType="Collection">
          <glview:MeasurementType rdf:about="http://schema.geolink.org/dev/voc/nvs/P02#OCPW"/>
        </owl:oneOf>
      </owl:Class>
    </owl:someValuesFrom>
    <owl:onProperty rdf:resource="http://schema.geolink.org/dev/view#hasMeasurementType"/>
  </owl:Restriction>
  <owl:Restriction>
    <rdfs:subClassOf>
      <glview:MeasurementType rdf:about="http://schema.geolink.org/dev/voc/nvs/P02#PTDZ">
        <rdfs:subClassOf rdf:resource="http://schema.geolink.org/dev/voc/nvs/P03#D025"/>
        <rdfs:seeAlso rdf:resource="http://vocab.nerc.ac.uk/collection/P02/current/PTDZ/"/>
        <rdfs:comment xml:lang="en">Parameters expressing the variation of temperature in the water column either as a function of space or of time</rdfs:comment>
        <rdfs:label xml:lang="en">Temperature variation in the water column</rdfs:label>
        <rdf:type rdf:resource="http://www.w3.org/2002/07/owl#NamedIndividual"/>
        <rdf:type rdf:resource="http://www.w3.org/2002/07/owl#Class"/>
      </glview:MeasurementType>
    </rdfs:subClassOf>
    <owl:someValuesFrom>
      <owl:Class>
        <owl:oneOf rdf:parseType="Collection">
          <glview:MeasurementType rdf:about="http://schema.geolink.org/dev/voc/nvs/P02#PTDZ"/>
        </owl:oneOf>
      </owl:Class>
    </owl:someValuesFrom>
    <owl:onProperty rdf:resource="http://schema.geolink.org/dev/view#hasMeasurementType"/>
  </owl:Restriction>
  <owl:Restriction>
    <rdfs:subClassOf>
      <glview:MeasurementType rdf:about="http://schema.geolink.org/dev/voc/nvs/P02#EXCO">
        <rdfs:subClassOf rdf:resource="http://schema.geolink.org/dev/voc/nvs/P03#D015"/>
        <rdfs:seeAlso rdf:resource="http://vocab.nerc.ac.uk/collection/P02/current/EXCO/"/>
        <rdfs:comment xml:lang="en">Parameters relating to the extent of light penetration into the water column</rdfs:comment>
        <rdfs:label xml:lang="en">Light extinction and diffusion coefficients</rdfs:label>
        <rdf:type rdf:resource="http://www.w3.org/2002/07/owl#NamedIndividual"/>
        <rdf:type rdf:resource="http://www.w3.org/2002/07/owl#Class"/>
      </glview:MeasurementType>
    </rdfs:subClassOf>
    <owl:someValuesFrom>
      <owl:Class>
        <owl:oneOf rdf:parseType="Collection">
          <glview:MeasurementType rdf:about="http://schema.geolink.org/dev/voc/nvs/P02#EXCO"/>
        </owl:oneOf>
      </owl:Class>
    </owl:someValuesFrom>
    <owl:onProperty rdf:resource="http://schema.geolink.org/dev/view#hasMeasurementType"/>
  </owl:Restriction>
  <owl:Restriction>
    <rdfs:subClassOf>
      <glview:MeasurementType rdf:about="http://schema.geolink.org/dev/voc/nvs/P02#PHYG">
        <rdfs:subClassOf rdf:resource="http://schema.geolink.org/dev/voc/nvs/P03#O010"/>
        <rdfs:seeAlso rdf:resource="http://vocab.nerc.ac.uk/collection/P02/current/PHYG/"/>
        <rdfs:comment></rdfs:comment>
        <rdfs:label xml:lang="en">Phytoplankton growth</rdfs:label>
        <rdf:type rdf:resource="http://www.w3.org/2002/07/owl#NamedIndividual"/>
        <rdf:type rdf:resource="http://www.w3.org/2002/07/owl#Class"/>
      </glview:MeasurementType>
    </rdfs:subClassOf>
    <owl:someValuesFrom>
      <owl:Class>
        <owl:oneOf rdf:parseType="Collection">
          <glview:MeasurementType rdf:about="http://schema.geolink.org/dev/voc/nvs/P02#PHYG"/>
        </owl:oneOf>
      </owl:Class>
    </owl:someValuesFrom>
    <owl:onProperty rdf:resource="http://schema.geolink.org/dev/view#hasMeasurementType"/>
  </owl:Restriction>
  <owl:Restriction>
    <rdfs:subClassOf>
      <glview:MeasurementType rdf:about="http://schema.geolink.org/dev/voc/nvs/P02#LIBI">
        <rdfs:subClassOf rdf:resource="http://schema.geolink.org/dev/voc/nvs/P03#B007"/>
        <rdfs:seeAlso rdf:resource="http://vocab.nerc.ac.uk/collection/P02/current/LIBI/"/>
        <rdfs:comment xml:lang="en">Lipids are defined as small water-insoluble biomolecules including fats, fatty acids, esters, sterols, isoprenoid compounds, etc..  Biota includes any type of sample originating from a living organism.</rdfs:comment>
        <rdfs:label xml:lang="en">Biota lipid concentrations</rdfs:label>
        <rdf:type rdf:resource="http://www.w3.org/2002/07/owl#NamedIndividual"/>
        <rdf:type rdf:resource="http://www.w3.org/2002/07/owl#Class"/>
      </glview:MeasurementType>
    </rdfs:subClassOf>
    <owl:someValuesFrom>
      <owl:Class>
        <owl:oneOf rdf:parseType="Collection">
          <glview:MeasurementType rdf:about="http://schema.geolink.org/dev/voc/nvs/P02#LIBI"/>
        </owl:oneOf>
      </owl:Class>
    </owl:someValuesFrom>
    <owl:onProperty rdf:resource="http://schema.geolink.org/dev/view#hasMeasurementType"/>
  </owl:Restriction>
  <owl:Restriction>
    <rdfs:subClassOf>
      <glview:MeasurementType rdf:about="http://schema.geolink.org/dev/voc/nvs/P02#LERR">
        <rdfs:subClassOf rdf:resource="http://schema.geolink.org/dev/voc/nvs/P03#D030"/>
        <rdfs:seeAlso rdf:resource="http://vocab.nerc.ac.uk/collection/P02/current/LERR/"/>
        <rdfs:comment xml:lang="en">Parameters as logged by measuring devices, including raw counts/voltages and ADCP relative velocities</rdfs:comment>
        <rdfs:label xml:lang="en">Raw current meter output parameters</rdfs:label>
        <rdf:type rdf:resource="http://www.w3.org/2002/07/owl#NamedIndividual"/>
        <rdf:type rdf:resource="http://www.w3.org/2002/07/owl#Class"/>
      </glview:MeasurementType>
    </rdfs:subClassOf>
    <owl:someValuesFrom>
      <owl:Class>
        <owl:oneOf rdf:parseType="Collection">
          <glview:MeasurementType rdf:about="http://schema.geolink.org/dev/voc/nvs/P02#LERR"/>
        </owl:oneOf>
      </owl:Class>
    </owl:someValuesFrom>
    <owl:onProperty rdf:resource="http://schema.geolink.org/dev/view#hasMeasurementType"/>
  </owl:Restriction>
  <owl:Restriction>
    <rdfs:subClassOf>
      <glview:MeasurementType rdf:about="http://schema.geolink.org/dev/voc/nvs/P02#CARS">
        <rdfs:subClassOf rdf:resource="http://schema.geolink.org/dev/voc/nvs/P03#B035"/>
        <rdfs:subClassOf rdf:resource="http://schema.geolink.org/dev/voc/nvs/P03#G035"/>
        <rdfs:seeAlso rdf:resource="http://vocab.nerc.ac.uk/collection/P02/current/CARS/"/>
        <rdfs:comment xml:lang="en">Sediment includes anything collected by a grab or corer, including the fluff layer from the top of the consolidated sediment</rdfs:comment>
        <rdfs:label xml:lang="en">Carotenoid pigment concentrations in sediment</rdfs:label>
        <rdf:type rdf:resource="http://www.w3.org/2002/07/owl#NamedIndividual"/>
        <rdf:type rdf:resource="http://www.w3.org/2002/07/owl#Class"/>
      </glview:MeasurementType>
    </rdfs:subClassOf>
    <owl:someValuesFrom>
      <owl:Class>
        <owl:oneOf rdf:parseType="Collection">
          <glview:MeasurementType rdf:about="http://schema.geolink.org/dev/voc/nvs/P02#CARS"/>
        </owl:oneOf>
      </owl:Class>
    </owl:someValuesFrom>
    <owl:onProperty rdf:resource="http://schema.geolink.org/dev/view#hasMeasurementType"/>
  </owl:Restriction>
  <owl:Restriction>
    <rdfs:subClassOf rdf:resource="http://schema.geolink.org/dev/voc/nvs/P02#PESD"/>
    <owl:someValuesFrom>
      <owl:Class>
        <owl:oneOf rdf:parseType="Collection">
          <glview:MeasurementType rdf:about="http://schema.geolink.org/dev/voc/nvs/P02#PESD"/>
        </owl:oneOf>
      </owl:Class>
    </owl:someValuesFrom>
    <owl:onProperty rdf:resource="http://schema.geolink.org/dev/view#hasMeasurementType"/>
  </owl:Restriction>
  <owl:Restriction>
    <rdfs:subClassOf>
      <glview:MeasurementType rdf:about="http://schema.geolink.org/dev/voc/nvs/P02#SPOL">
        <rdfs:subClassOf rdf:resource="http://schema.geolink.org/dev/voc/nvs/P03#G055"/>
        <rdfs:seeAlso rdf:resource="http://vocab.nerc.ac.uk/collection/P02/current/SPOL/"/>
        <rdfs:comment></rdfs:comment>
        <rdfs:label xml:lang="en">Sediment pollen content</rdfs:label>
        <rdf:type rdf:resource="http://www.w3.org/2002/07/owl#NamedIndividual"/>
        <rdf:type rdf:resource="http://www.w3.org/2002/07/owl#Class"/>
      </glview:MeasurementType>
    </rdfs:subClassOf>
    <owl:someValuesFrom>
      <owl:Class>
        <owl:oneOf rdf:parseType="Collection">
          <glview:MeasurementType rdf:about="http://schema.geolink.org/dev/voc/nvs/P02#SPOL"/>
        </owl:oneOf>
      </owl:Class>
    </owl:someValuesFrom>
    <owl:onProperty rdf:resource="http://schema.geolink.org/dev/view#hasMeasurementType"/>
  </owl:Restriction>
  <owl:Restriction>
    <rdfs:subClassOf rdf:resource="http://schema.geolink.org/dev/voc/nvs/P02#RTCO"/>
    <owl:someValuesFrom>
      <owl:Class>
        <owl:oneOf rdf:parseType="Collection">
          <glview:MeasurementType rdf:about="http://schema.geolink.org/dev/voc/nvs/P02#RTCO"/>
        </owl:oneOf>
      </owl:Class>
    </owl:someValuesFrom>
    <owl:onProperty rdf:resource="http://schema.geolink.org/dev/view#hasMeasurementType"/>
  </owl:Restriction>
  <owl:Restriction>
    <rdfs:subClassOf>
      <glview:MeasurementType rdf:about="http://schema.geolink.org/dev/voc/nvs/P02#DVLP">
        <rdfs:subClassOf rdf:resource="http://schema.geolink.org/dev/voc/nvs/P03#B045"/>
        <rdfs:subClassOf rdf:resource="http://schema.geolink.org/dev/voc/nvs/P03#B027"/>
        <rdfs:seeAlso rdf:resource="http://vocab.nerc.ac.uk/collection/P02/current/DVLP/"/>
        <rdfs:comment xml:lang="en">Development stage parameters (such as proportion but excluding abundance or biomass) of zooplankton and zoobenthos. Benthic and planktonic animals have not been seggregated because there is a degree of overlap (eg shrimps).</rdfs:comment>
        <rdfs:label xml:lang="en">Zooplankton and zoobenthos development stage parameters</rdfs:label>
        <rdf:type rdf:resource="http://www.w3.org/2002/07/owl#NamedIndividual"/>
        <rdf:type rdf:resource="http://www.w3.org/2002/07/owl#Class"/>
      </glview:MeasurementType>
    </rdfs:subClassOf>
    <owl:someValuesFrom>
      <owl:Class>
        <owl:oneOf rdf:parseType="Collection">
          <glview:MeasurementType rdf:about="http://schema.geolink.org/dev/voc/nvs/P02#DVLP"/>
        </owl:oneOf>
      </owl:Class>
    </owl:someValuesFrom>
    <owl:onProperty rdf:resource="http://schema.geolink.org/dev/view#hasMeasurementType"/>
  </owl:Restriction>
  <owl:Restriction>
    <rdfs:subClassOf rdf:resource="http://schema.geolink.org/dev/voc/nvs/P02#MDWP"/>
    <owl:someValuesFrom>
      <owl:Class>
        <owl:oneOf rdf:parseType="Collection">
          <glview:MeasurementType rdf:about="http://schema.geolink.org/dev/voc/nvs/P02#MDWP"/>
        </owl:oneOf>
      </owl:Class>
    </owl:someValuesFrom>
    <owl:onProperty rdf:resource="http://schema.geolink.org/dev/view#hasMeasurementType"/>
  </owl:Restriction>
  <owl:Restriction>
    <rdfs:subClassOf rdf:resource="http://schema.geolink.org/dev/voc/nvs/P02#RVDS"/>
    <owl:someValuesFrom>
      <owl:Class>
        <owl:oneOf rdf:parseType="Collection">
          <glview:MeasurementType rdf:about="http://schema.geolink.org/dev/voc/nvs/P02#RVDS"/>
        </owl:oneOf>
      </owl:Class>
    </owl:someValuesFrom>
    <owl:onProperty rdf:resource="http://schema.geolink.org/dev/view#hasMeasurementType"/>
  </owl:Restriction>
  <owl:Restriction>
    <rdfs:subClassOf>
      <glview:MeasurementType rdf:about="http://schema.geolink.org/dev/voc/nvs/P02#FVLT">
        <rdfs:subClassOf rdf:resource="http://schema.geolink.org/dev/voc/nvs/P03#B035"/>
        <rdfs:seeAlso rdf:resource="http://vocab.nerc.ac.uk/collection/P02/current/FVLT/"/>
        <rdfs:comment xml:lang="en">Output as logged from any type fluorometer.</rdfs:comment>
        <rdfs:label xml:lang="en">Raw fluorometer output</rdfs:label>
        <rdf:type rdf:resource="http://www.w3.org/2002/07/owl#NamedIndividual"/>
        <rdf:type rdf:resource="http://www.w3.org/2002/07/owl#Class"/>
      </glview:MeasurementType>
    </rdfs:subClassOf>
    <owl:someValuesFrom>
      <owl:Class>
        <owl:oneOf rdf:parseType="Collection">
          <glview:MeasurementType rdf:about="http://schema.geolink.org/dev/voc/nvs/P02#FVLT"/>
        </owl:oneOf>
      </owl:Class>
    </owl:someValuesFrom>
    <owl:onProperty rdf:resource="http://schema.geolink.org/dev/view#hasMeasurementType"/>
  </owl:Restriction>
  <owl:Restriction>
    <rdfs:subClassOf rdf:resource="http://schema.geolink.org/dev/voc/nvs/P02#AMON"/>
    <owl:someValuesFrom>
      <owl:Class>
        <owl:oneOf rdf:parseType="Collection">
          <glview:MeasurementType rdf:about="http://schema.geolink.org/dev/voc/nvs/P02#AMON"/>
        </owl:oneOf>
      </owl:Class>
    </owl:someValuesFrom>
    <owl:onProperty rdf:resource="http://schema.geolink.org/dev/view#hasMeasurementType"/>
  </owl:Restriction>
  <owl:Restriction>
    <rdfs:subClassOf>
      <glview:MeasurementType rdf:about="http://schema.geolink.org/dev/voc/nvs/P02#ACNT">
        <rdfs:subClassOf rdf:resource="http://schema.geolink.org/dev/voc/nvs/P03#B055"/>
        <rdfs:seeAlso rdf:resource="http://vocab.nerc.ac.uk/collection/P02/current/ACNT/"/>
        <rdfs:comment xml:lang="en">Macroalgae (Rhodophycota, Chromphycota, Chlorophycota) and seagrass (Charophyta, Anthophyta) count parameters presented at the level of taxa at any level from sub-species upwards. Count includes presence/absence indicators.</rdfs:comment>
        <rdfs:label xml:lang="en">Macroalgae and seagrass taxonomy-related counts</rdfs:label>
        <rdf:type rdf:resource="http://www.w3.org/2002/07/owl#NamedIndividual"/>
        <rdf:type rdf:resource="http://www.w3.org/2002/07/owl#Class"/>
      </glview:MeasurementType>
    </rdfs:subClassOf>
    <owl:someValuesFrom>
      <owl:Class>
        <owl:oneOf rdf:parseType="Collection">
          <glview:MeasurementType rdf:about="http://schema.geolink.org/dev/voc/nvs/P02#ACNT"/>
        </owl:oneOf>
      </owl:Class>
    </owl:someValuesFrom>
    <owl:onProperty rdf:resource="http://schema.geolink.org/dev/view#hasMeasurementType"/>
  </owl:Restriction>
  <owl:Restriction>
    <rdfs:subClassOf>
      <glview:MeasurementType rdf:about="http://schema.geolink.org/dev/voc/nvs/P02#SATM">
        <rdfs:subClassOf rdf:resource="http://schema.geolink.org/dev/voc/nvs/P03#B027"/>
        <rdfs:subClassOf rdf:resource="http://schema.geolink.org/dev/voc/nvs/P03#H004"/>
        <rdfs:seeAlso rdf:resource="http://vocab.nerc.ac.uk/collection/P02/current/SATM/"/>
        <rdfs:comment xml:lang="en">Paramaters that quantify the size, shape, age and life processes (including mortality) of shellfish (molluscs - including cephalopods - and crustaceans of interest to fisheries research and commercial fisheries).</rdfs:comment>
        <rdfs:label xml:lang="en">Shellfish morphology, age and physiology</rdfs:label>
        <rdf:type rdf:resource="http://www.w3.org/2002/07/owl#NamedIndividual"/>
        <rdf:type rdf:resource="http://www.w3.org/2002/07/owl#Class"/>
      </glview:MeasurementType>
    </rdfs:subClassOf>
    <owl:someValuesFrom>
      <owl:Class>
        <owl:oneOf rdf:parseType="Collection">
          <glview:MeasurementType rdf:about="http://schema.geolink.org/dev/voc/nvs/P02#SATM"/>
        </owl:oneOf>
      </owl:Class>
    </owl:someValuesFrom>
    <owl:onProperty rdf:resource="http://schema.geolink.org/dev/view#hasMeasurementType"/>
  </owl:Restriction>
  <owl:Restriction>
    <rdfs:subClassOf>
      <glview:MeasurementType rdf:about="http://schema.geolink.org/dev/voc/nvs/P02#FOCA">
        <rdfs:subClassOf rdf:resource="http://schema.geolink.org/dev/voc/nvs/P03#B015"/>
        <rdfs:seeAlso rdf:resource="http://vocab.nerc.ac.uk/collection/P02/current/FOCA/"/>
        <rdfs:comment xml:lang="en">Parameters that specify the number of specified members of Family Phocidae present at a particular time and location, including presence/absence indicators.</rdfs:comment>
        <rdfs:label xml:lang="en">Seal abundance</rdfs:label>
        <rdf:type rdf:resource="http://www.w3.org/2002/07/owl#NamedIndividual"/>
        <rdf:type rdf:resource="http://www.w3.org/2002/07/owl#Class"/>
      </glview:MeasurementType>
    </rdfs:subClassOf>
    <owl:someValuesFrom>
      <owl:Class>
        <owl:oneOf rdf:parseType="Collection">
          <glview:MeasurementType rdf:about="http://schema.geolink.org/dev/voc/nvs/P02#FOCA"/>
        </owl:oneOf>
      </owl:Class>
    </owl:someValuesFrom>
    <owl:onProperty rdf:resource="http://schema.geolink.org/dev/view#hasMeasurementType"/>
  </owl:Restriction>
  <owl:Restriction>
    <rdfs:subClassOf rdf:resource="http://schema.geolink.org/dev/voc/nvs/P02#BCOC"/>
    <owl:someValuesFrom>
      <owl:Class>
        <owl:oneOf rdf:parseType="Collection">
          <glview:MeasurementType rdf:about="http://schema.geolink.org/dev/voc/nvs/P02#BCOC"/>
        </owl:oneOf>
      </owl:Class>
    </owl:someValuesFrom>
    <owl:onProperty rdf:resource="http://schema.geolink.org/dev/view#hasMeasurementType"/>
  </owl:Restriction>
  <owl:Restriction>
    <rdfs:subClassOf>
      <glview:MeasurementType rdf:about="http://schema.geolink.org/dev/voc/nvs/P02#CATX">
        <rdfs:subClassOf rdf:resource="http://schema.geolink.org/dev/voc/nvs/P03#B030"/>
        <rdfs:subClassOf rdf:resource="http://schema.geolink.org/dev/voc/nvs/P03#B070"/>
        <rdfs:seeAlso rdf:resource="http://vocab.nerc.ac.uk/collection/P02/current/CATX/"/>
        <rdfs:comment xml:lang="en">Any parameterisation of biomass (e.g. wet weight, dry weight, carbon, nitrogen etc.) of free-floating autotrophic biological entities identified by their taxonomic names (e.g. family, genus, species) in any body of fresh or salt water.</rdfs:comment>
        <rdfs:label xml:lang="en">Phytoplankton taxonomic biomass in water bodies</rdfs:label>
        <rdf:type rdf:resource="http://www.w3.org/2002/07/owl#NamedIndividual"/>
        <rdf:type rdf:resource="http://www.w3.org/2002/07/owl#Class"/>
      </glview:MeasurementType>
    </rdfs:subClassOf>
    <owl:someValuesFrom>
      <owl:Class>
        <owl:oneOf rdf:parseType="Collection">
          <glview:MeasurementType rdf:about="http://schema.geolink.org/dev/voc/nvs/P02#CATX"/>
        </owl:oneOf>
      </owl:Class>
    </owl:someValuesFrom>
    <owl:onProperty rdf:resource="http://schema.geolink.org/dev/view#hasMeasurementType"/>
  </owl:Restriction>
  <owl:Restriction>
    <rdfs:subClassOf>
      <glview:MeasurementType rdf:about="http://schema.geolink.org/dev/voc/nvs/P02#TNRP">
        <rdfs:subClassOf rdf:resource="http://schema.geolink.org/dev/voc/nvs/P03#O010"/>
        <rdfs:seeAlso rdf:resource="http://vocab.nerc.ac.uk/collection/P02/current/TNRP/"/>
        <rdfs:comment xml:lang="en">Parameters related to the rates of TCO2 production and consumption based on light/dark bottle incubations</rdfs:comment>
        <rdfs:label xml:lang="en">Dissolved inorganic carbon production and respiration in the water column</rdfs:label>
        <rdf:type rdf:resource="http://www.w3.org/2002/07/owl#NamedIndividual"/>
        <rdf:type rdf:resource="http://www.w3.org/2002/07/owl#Class"/>
      </glview:MeasurementType>
    </rdfs:subClassOf>
    <owl:someValuesFrom>
      <owl:Class>
        <owl:oneOf rdf:parseType="Collection">
          <glview:MeasurementType rdf:about="http://schema.geolink.org/dev/voc/nvs/P02#TNRP"/>
        </owl:oneOf>
      </owl:Class>
    </owl:someValuesFrom>
    <owl:onProperty rdf:resource="http://schema.geolink.org/dev/view#hasMeasurementType"/>
  </owl:Restriction>
  <owl:Restriction>
    <rdfs:subClassOf>
      <glview:MeasurementType rdf:about="http://schema.geolink.org/dev/voc/nvs/P02#SR2D">
        <rdfs:subClassOf rdf:resource="http://schema.geolink.org/dev/voc/nvs/P03#GPYS"/>
        <rdfs:subClassOf rdf:resource="http://schema.geolink.org/dev/voc/nvs/P03#G012"/>
        <rdfs:subClassOf rdf:resource="http://schema.geolink.org/dev/voc/nvs/P02#SRFL"/>
        <rdfs:seeAlso rdf:resource="http://vocab.nerc.ac.uk/collection/P02/current/SR2D/"/>
        <rdfs:comment xml:lang="en">Parameters relating to structure beneath sea-bed determined by the reflection of seismic energy along a single track.</rdfs:comment>
        <rdfs:label xml:lang="en">Two-dimensional seismic reflection</rdfs:label>
        <rdf:type rdf:resource="http://www.w3.org/2002/07/owl#NamedIndividual"/>
        <rdf:type rdf:resource="http://www.w3.org/2002/07/owl#Class"/>
      </glview:MeasurementType>
    </rdfs:subClassOf>
    <owl:someValuesFrom>
      <owl:Class>
        <owl:oneOf rdf:parseType="Collection">
          <glview:MeasurementType rdf:about="http://schema.geolink.org/dev/voc/nvs/P02#SR2D"/>
        </owl:oneOf>
      </owl:Class>
    </owl:someValuesFrom>
    <owl:onProperty rdf:resource="http://schema.geolink.org/dev/view#hasMeasurementType"/>
  </owl:Restriction>
  <owl:Restriction>
    <rdfs:subClassOf>
      <glview:MeasurementType rdf:about="http://schema.geolink.org/dev/voc/nvs/P02#SSTB">
        <rdfs:subClassOf rdf:resource="http://schema.geolink.org/dev/voc/nvs/P03#C030"/>
        <rdfs:subClassOf rdf:resource="http://schema.geolink.org/dev/voc/nvs/P03#G035"/>
        <rdfs:seeAlso rdf:resource="http://vocab.nerc.ac.uk/collection/P02/current/SSTB/"/>
        <rdfs:comment xml:lang="en">Stable isotope enrichment parameters in sediment, including biota-associated parameters such as isotope enrichment in foraminifera tests</rdfs:comment>
        <rdfs:label xml:lang="en">Stable isotope enrichment in sediment</rdfs:label>
        <rdf:type rdf:resource="http://www.w3.org/2002/07/owl#NamedIndividual"/>
        <rdf:type rdf:resource="http://www.w3.org/2002/07/owl#Class"/>
      </glview:MeasurementType>
    </rdfs:subClassOf>
    <owl:someValuesFrom>
      <owl:Class>
        <owl:oneOf rdf:parseType="Collection">
          <glview:MeasurementType rdf:about="http://schema.geolink.org/dev/voc/nvs/P02#SSTB"/>
        </owl:oneOf>
      </owl:Class>
    </owl:someValuesFrom>
    <owl:onProperty rdf:resource="http://schema.geolink.org/dev/view#hasMeasurementType"/>
  </owl:Restriction>
  <owl:Restriction>
    <rdfs:subClassOf>
      <glview:MeasurementType rdf:about="http://schema.geolink.org/dev/voc/nvs/P02#WCOC">
        <rdfs:subClassOf rdf:resource="http://schema.geolink.org/dev/voc/nvs/P03#C055"/>
        <rdfs:subClassOf rdf:resource="http://schema.geolink.org/dev/voc/nvs/P03#H001"/>
        <rdfs:seeAlso rdf:resource="http://vocab.nerc.ac.uk/collection/P02/current/WCOC/"/>
        <rdfs:comment xml:lang="en">Concentration parameters for carbon compounds regarded as environmentally harmful in solution or suspension (i.e.includes measurements in both the dissolved and particulate phases) in any body of salt or fresh water that are not included in other specific categories</rdfs:comment>
        <rdfs:label xml:lang="en">Concentration of other organic contaminants in the water column</rdfs:label>
        <rdf:type rdf:resource="http://www.w3.org/2002/07/owl#NamedIndividual"/>
        <rdf:type rdf:resource="http://www.w3.org/2002/07/owl#Class"/>
      </glview:MeasurementType>
    </rdfs:subClassOf>
    <owl:someValuesFrom>
      <owl:Class>
        <owl:oneOf rdf:parseType="Collection">
          <glview:MeasurementType rdf:about="http://schema.geolink.org/dev/voc/nvs/P02#WCOC"/>
        </owl:oneOf>
      </owl:Class>
    </owl:someValuesFrom>
    <owl:onProperty rdf:resource="http://schema.geolink.org/dev/view#hasMeasurementType"/>
  </owl:Restriction>
  <owl:Restriction>
    <rdfs:subClassOf rdf:resource="http://schema.geolink.org/dev/voc/nvs/P02#ICHM"/>
    <owl:someValuesFrom>
      <owl:Class>
        <owl:oneOf rdf:parseType="Collection">
          <glview:MeasurementType rdf:about="http://schema.geolink.org/dev/voc/nvs/P02#ICHM"/>
        </owl:oneOf>
      </owl:Class>
    </owl:someValuesFrom>
    <owl:onProperty rdf:resource="http://schema.geolink.org/dev/view#hasMeasurementType"/>
  </owl:Restriction>
  <owl:Restriction>
    <rdfs:subClassOf>
      <glview:MeasurementType rdf:about="http://schema.geolink.org/dev/voc/nvs/P02#CAPH">
        <rdfs:subClassOf rdf:resource="http://schema.geolink.org/dev/voc/nvs/P03#M010"/>
        <rdfs:seeAlso rdf:resource="http://vocab.nerc.ac.uk/collection/P02/current/CAPH/"/>
        <rdfs:comment xml:lang="en">Measurements of air pressure as the dependent variable (ie excluding air pressure measured to specify the z co-ordinate of a balloon or sonde), including derived parameters such as tendency (rate of change) and related parameters such as air density.</rdfs:comment>
        <rdfs:label xml:lang="en">Air pressure</rdfs:label>
        <rdf:type rdf:resource="http://www.w3.org/2002/07/owl#NamedIndividual"/>
        <rdf:type rdf:resource="http://www.w3.org/2002/07/owl#Class"/>
      </glview:MeasurementType>
    </rdfs:subClassOf>
    <owl:someValuesFrom>
      <owl:Class>
        <owl:oneOf rdf:parseType="Collection">
          <glview:MeasurementType rdf:about="http://schema.geolink.org/dev/voc/nvs/P02#CAPH"/>
        </owl:oneOf>
      </owl:Class>
    </owl:someValuesFrom>
    <owl:onProperty rdf:resource="http://schema.geolink.org/dev/view#hasMeasurementType"/>
  </owl:Restriction>
  <owl:Restriction>
    <rdfs:subClassOf rdf:resource="http://schema.geolink.org/dev/voc/nvs/P02#MSEP"/>
    <owl:someValuesFrom>
      <owl:Class>
        <owl:oneOf rdf:parseType="Collection">
          <glview:MeasurementType rdf:about="http://schema.geolink.org/dev/voc/nvs/P02#MSEP"/>
        </owl:oneOf>
      </owl:Class>
    </owl:someValuesFrom>
    <owl:onProperty rdf:resource="http://schema.geolink.org/dev/view#hasMeasurementType"/>
  </owl:Restriction>
  <owl:Restriction>
    <rdfs:subClassOf>
      <glview:MeasurementType rdf:about="http://schema.geolink.org/dev/voc/nvs/P02#ACYC">
        <rdfs:subClassOf rdf:resource="http://schema.geolink.org/dev/voc/nvs/P03#Z005"/>
        <rdfs:seeAlso rdf:resource="http://vocab.nerc.ac.uk/collection/P02/current/ACYC/"/>
        <rdfs:comment xml:lang="en">Data record, event, sample or measurement reference numbers</rdfs:comment>
        <rdfs:label xml:lang="en">Reference numbers</rdfs:label>
        <rdf:type rdf:resource="http://www.w3.org/2002/07/owl#NamedIndividual"/>
        <rdf:type rdf:resource="http://www.w3.org/2002/07/owl#Class"/>
      </glview:MeasurementType>
    </rdfs:subClassOf>
    <owl:someValuesFrom>
      <owl:Class>
        <owl:oneOf rdf:parseType="Collection">
          <glview:MeasurementType rdf:about="http://schema.geolink.org/dev/voc/nvs/P02#ACYC"/>
        </owl:oneOf>
      </owl:Class>
    </owl:someValuesFrom>
    <owl:onProperty rdf:resource="http://schema.geolink.org/dev/view#hasMeasurementType"/>
  </owl:Restriction>
  <owl:Restriction>
    <rdfs:subClassOf rdf:resource="http://schema.geolink.org/dev/voc/nvs/P02#EXCR"/>
    <owl:someValuesFrom>
      <owl:Class>
        <owl:oneOf rdf:parseType="Collection">
          <glview:MeasurementType rdf:about="http://schema.geolink.org/dev/voc/nvs/P02#EXCR"/>
        </owl:oneOf>
      </owl:Class>
    </owl:someValuesFrom>
    <owl:onProperty rdf:resource="http://schema.geolink.org/dev/view#hasMeasurementType"/>
  </owl:Restriction>
  <owl:Restriction>
    <rdfs:subClassOf rdf:resource="http://schema.geolink.org/dev/voc/nvs/P02#WCOC"/>
    <owl:someValuesFrom>
      <owl:Class>
        <owl:oneOf rdf:parseType="Collection">
          <glview:MeasurementType rdf:about="http://schema.geolink.org/dev/voc/nvs/P02#WCOC"/>
        </owl:oneOf>
      </owl:Class>
    </owl:someValuesFrom>
    <owl:onProperty rdf:resource="http://schema.geolink.org/dev/view#hasMeasurementType"/>
  </owl:Restriction>
  <owl:Restriction>
    <rdfs:subClassOf rdf:resource="http://schema.geolink.org/dev/voc/nvs/P02#OMPW"/>
    <owl:someValuesFrom>
      <owl:Class>
        <owl:oneOf rdf:parseType="Collection">
          <owl:NamedIndividual rdf:about="http://schema.geolink.org/dev/voc/nvs/P02#OMPW"/>
        </owl:oneOf>
      </owl:Class>
    </owl:someValuesFrom>
    <owl:onProperty rdf:resource="http://schema.geolink.org/dev/view#hasMeasurementType"/>
  </owl:Restriction>
  <owl:Restriction>
    <rdfs:subClassOf>
      <glview:MeasurementType rdf:about="http://schema.geolink.org/dev/voc/nvs/P02#BLEN">
        <rdfs:subClassOf rdf:resource="http://schema.geolink.org/dev/voc/nvs/P03#B045"/>
        <rdfs:subClassOf rdf:resource="http://schema.geolink.org/dev/voc/nvs/P03#B027"/>
        <rdfs:seeAlso rdf:resource="http://vocab.nerc.ac.uk/collection/P02/current/BLEN/"/>
        <rdfs:comment xml:lang="en">Morphological parameters of zooplankton and zoobenthos (essentially any animal except for insects, earthworms or fish), such as size, shape and weight.  Benthic and planktonic animals have not been seggregated because there is a degree of overlap (eg shrimps).</rdfs:comment>
        <rdfs:label xml:lang="en">Zooplankton and zoobenthos morphological parameters</rdfs:label>
        <rdf:type rdf:resource="http://www.w3.org/2002/07/owl#NamedIndividual"/>
        <rdf:type rdf:resource="http://www.w3.org/2002/07/owl#Class"/>
      </glview:MeasurementType>
    </rdfs:subClassOf>
    <owl:someValuesFrom>
      <owl:Class>
        <owl:oneOf rdf:parseType="Collection">
          <glview:MeasurementType rdf:about="http://schema.geolink.org/dev/voc/nvs/P02#BLEN"/>
        </owl:oneOf>
      </owl:Class>
    </owl:someValuesFrom>
    <owl:onProperty rdf:resource="http://schema.geolink.org/dev/view#hasMeasurementType"/>
  </owl:Restriction>
  <owl:Restriction>
    <rdfs:subClassOf>
      <glview:MeasurementType rdf:about="http://schema.geolink.org/dev/voc/nvs/P02#ENGP">
        <rdfs:subClassOf rdf:resource="http://schema.geolink.org/dev/voc/nvs/P03#Z005"/>
        <rdfs:seeAlso rdf:resource="http://vocab.nerc.ac.uk/collection/P02/current/ENGP/"/>
        <rdfs:comment xml:lang="en">Technical parameters that provide information on how well an instrument or data acquisition system is working</rdfs:comment>
        <rdfs:label xml:lang="en">Engineering parameters</rdfs:label>
        <rdf:type rdf:resource="http://www.w3.org/2002/07/owl#NamedIndividual"/>
        <rdf:type rdf:resource="http://www.w3.org/2002/07/owl#Class"/>
      </glview:MeasurementType>
    </rdfs:subClassOf>
    <owl:someValuesFrom>
      <owl:Class>
        <owl:oneOf rdf:parseType="Collection">
          <glview:MeasurementType rdf:about="http://schema.geolink.org/dev/voc/nvs/P02#ENGP"/>
        </owl:oneOf>
      </owl:Class>
    </owl:someValuesFrom>
    <owl:onProperty rdf:resource="http://schema.geolink.org/dev/view#hasMeasurementType"/>
  </owl:Restriction>
  <owl:Restriction>
    <rdfs:subClassOf>
      <glview:MeasurementType rdf:about="http://schema.geolink.org/dev/voc/nvs/P02#BPBP">
        <rdfs:subClassOf rdf:resource="http://schema.geolink.org/dev/voc/nvs/P03#B070"/>
        <rdfs:subClassOf rdf:resource="http://schema.geolink.org/dev/voc/nvs/P03#B005"/>
        <rdfs:seeAlso rdf:resource="http://vocab.nerc.ac.uk/collection/P02/current/BPBP/"/>
        <rdfs:comment></rdfs:comment>
        <rdfs:label xml:lang="en">Bacteria non taxonomy-related biomass expressed as protein per unit volume of the water column</rdfs:label>
        <rdf:type rdf:resource="http://www.w3.org/2002/07/owl#NamedIndividual"/>
        <rdf:type rdf:resource="http://www.w3.org/2002/07/owl#Class"/>
      </glview:MeasurementType>
    </rdfs:subClassOf>
    <owl:someValuesFrom>
      <owl:Class>
        <owl:oneOf rdf:parseType="Collection">
          <glview:MeasurementType rdf:about="http://schema.geolink.org/dev/voc/nvs/P02#BPBP"/>
        </owl:oneOf>
      </owl:Class>
    </owl:someValuesFrom>
    <owl:onProperty rdf:resource="http://schema.geolink.org/dev/view#hasMeasurementType"/>
  </owl:Restriction>
  <owl:Restriction>
    <rdfs:subClassOf>
      <glview:MeasurementType rdf:about="http://schema.geolink.org/dev/voc/nvs/P02#MLFX">
        <rdfs:subClassOf rdf:resource="http://schema.geolink.org/dev/voc/nvs/P03#O005"/>
        <rdfs:seeAlso rdf:resource="http://vocab.nerc.ac.uk/collection/P02/current/MLFX/"/>
        <rdfs:comment xml:lang="en">Parameters quantifying metal and metalloid fluxes as element concentration or isotope activities per unit area per unit time</rdfs:comment>
        <rdfs:label xml:lang="en">Sedimentation flux of metallic and metalloid elements and isotopes in water bodies</rdfs:label>
        <rdf:type rdf:resource="http://www.w3.org/2002/07/owl#NamedIndividual"/>
        <rdf:type rdf:resource="http://www.w3.org/2002/07/owl#Class"/>
      </glview:MeasurementType>
    </rdfs:subClassOf>
    <owl:someValuesFrom>
      <owl:Class>
        <owl:oneOf rdf:parseType="Collection">
          <glview:MeasurementType rdf:about="http://schema.geolink.org/dev/voc/nvs/P02#MLFX"/>
        </owl:oneOf>
      </owl:Class>
    </owl:someValuesFrom>
    <owl:onProperty rdf:resource="http://schema.geolink.org/dev/view#hasMeasurementType"/>
  </owl:Restriction>
  <owl:Restriction>
    <rdfs:subClassOf rdf:resource="http://schema.geolink.org/dev/voc/nvs/P02#SSTB"/>
    <owl:someValuesFrom>
      <owl:Class>
        <owl:oneOf rdf:parseType="Collection">
          <glview:MeasurementType rdf:about="http://schema.geolink.org/dev/voc/nvs/P02#SSTB"/>
        </owl:oneOf>
      </owl:Class>
    </owl:someValuesFrom>
    <owl:onProperty rdf:resource="http://schema.geolink.org/dev/view#hasMeasurementType"/>
  </owl:Restriction>
  <owl:Restriction>
    <rdfs:subClassOf rdf:resource="http://schema.geolink.org/dev/voc/nvs/P02#CATX"/>
    <owl:someValuesFrom>
      <owl:Class>
        <owl:oneOf rdf:parseType="Collection">
          <glview:MeasurementType rdf:about="http://schema.geolink.org/dev/voc/nvs/P02#CATX"/>
        </owl:oneOf>
      </owl:Class>
    </owl:someValuesFrom>
    <owl:onProperty rdf:resource="http://schema.geolink.org/dev/view#hasMeasurementType"/>
  </owl:Restriction>
  <owl:Restriction>
    <rdfs:subClassOf>
      <glview:MeasurementType rdf:about="http://schema.geolink.org/dev/voc/nvs/P02#PPWC">
        <rdfs:subClassOf rdf:resource="http://schema.geolink.org/dev/voc/nvs/P03#C055"/>
        <rdfs:subClassOf rdf:resource="http://schema.geolink.org/dev/voc/nvs/P03#H001"/>
        <rdfs:seeAlso rdf:resource="http://vocab.nerc.ac.uk/collection/P02/current/PPWC/"/>
        <rdfs:comment xml:lang="en">PCB concentrations in all phases of the water column. This group excludes SPM composition measurements (concentration per unit weight).</rdfs:comment>
        <rdfs:label xml:lang="en">Concentration of polychlorobiphenyls (PCBs) in the water column</rdfs:label>
        <rdf:type rdf:resource="http://www.w3.org/2002/07/owl#NamedIndividual"/>
        <rdf:type rdf:resource="http://www.w3.org/2002/07/owl#Class"/>
      </glview:MeasurementType>
    </rdfs:subClassOf>
    <owl:someValuesFrom>
      <owl:Class>
        <owl:oneOf rdf:parseType="Collection">
          <glview:MeasurementType rdf:about="http://schema.geolink.org/dev/voc/nvs/P02#PPWC"/>
        </owl:oneOf>
      </owl:Class>
    </owl:someValuesFrom>
    <owl:onProperty rdf:resource="http://schema.geolink.org/dev/view#hasMeasurementType"/>
  </owl:Restriction>
  <owl:Restriction>
    <rdfs:subClassOf>
      <glview:MeasurementType rdf:about="http://schema.geolink.org/dev/voc/nvs/P02#MPMN">
        <rdfs:subClassOf rdf:resource="http://schema.geolink.org/dev/voc/nvs/P03#Z005"/>
        <rdfs:seeAlso rdf:resource="http://vocab.nerc.ac.uk/collection/P02/current/MPMN/"/>
        <rdfs:comment xml:lang="en">Parameters expressing depth (possibly as pressure) of an instrument on a suspended underwater mooring.  These are primarily collected to monitor mooring performance by quantifying knock-down and should not be regarded as instrument z co-ordinates (accurate calibration is rare) or as sea level measurements.</rdfs:comment>
        <rdfs:label xml:lang="en">Moored instrument depth</rdfs:label>
        <rdf:type rdf:resource="http://www.w3.org/2002/07/owl#NamedIndividual"/>
        <rdf:type rdf:resource="http://www.w3.org/2002/07/owl#Class"/>
      </glview:MeasurementType>
    </rdfs:subClassOf>
    <owl:someValuesFrom>
      <owl:Class>
        <owl:oneOf rdf:parseType="Collection">
          <glview:MeasurementType rdf:about="http://schema.geolink.org/dev/voc/nvs/P02#MPMN"/>
        </owl:oneOf>
      </owl:Class>
    </owl:someValuesFrom>
    <owl:onProperty rdf:resource="http://schema.geolink.org/dev/view#hasMeasurementType"/>
  </owl:Restriction>
  <owl:Restriction>
    <rdfs:subClassOf rdf:resource="http://schema.geolink.org/dev/voc/nvs/P02#BEPP"/>
    <owl:someValuesFrom>
      <owl:Class>
        <owl:oneOf rdf:parseType="Collection">
          <glview:MeasurementType rdf:about="http://schema.geolink.org/dev/voc/nvs/P02#BEPP"/>
        </owl:oneOf>
      </owl:Class>
    </owl:someValuesFrom>
    <owl:onProperty rdf:resource="http://schema.geolink.org/dev/view#hasMeasurementType"/>
  </owl:Restriction>
  <owl:Restriction>
    <rdfs:subClassOf>
      <glview:MeasurementType rdf:about="http://schema.geolink.org/dev/voc/nvs/P02#SXCN">
        <rdfs:subClassOf rdf:resource="http://schema.geolink.org/dev/voc/nvs/P03#C045"/>
        <rdfs:subClassOf rdf:resource="http://schema.geolink.org/dev/voc/nvs/P03#G015"/>
        <rdfs:seeAlso rdf:resource="http://vocab.nerc.ac.uk/collection/P02/current/SXCN/"/>
        <rdfs:comment xml:lang="en">Concentration parameters for inorganic sulphur species in suspended particulate material (anything collected by filtration or sediment trapping).  Group does not include parameters expressing data per unit volume of the water column</rdfs:comment>
        <rdfs:label xml:lang="en">Concentration of inorganic sulphur species in suspended particulate material</rdfs:label>
        <rdf:type rdf:resource="http://www.w3.org/2002/07/owl#NamedIndividual"/>
        <rdf:type rdf:resource="http://www.w3.org/2002/07/owl#Class"/>
      </glview:MeasurementType>
    </rdfs:subClassOf>
    <owl:someValuesFrom>
      <owl:Class>
        <owl:oneOf rdf:parseType="Collection">
          <glview:MeasurementType rdf:about="http://schema.geolink.org/dev/voc/nvs/P02#SXCN"/>
        </owl:oneOf>
      </owl:Class>
    </owl:someValuesFrom>
    <owl:onProperty rdf:resource="http://schema.geolink.org/dev/view#hasMeasurementType"/>
  </owl:Restriction>
  <owl:Restriction>
    <rdfs:subClassOf>
      <glview:MeasurementType rdf:about="http://schema.geolink.org/dev/voc/nvs/P02#WQBI">
        <rdfs:subClassOf rdf:resource="http://schema.geolink.org/dev/view#Measurement"/>
        <rdfs:seeAlso rdf:resource="http://vocab.nerc.ac.uk/collection/P02/current/WQBI/"/>
        <rdfs:comment xml:lang="en">Parameters quantifying fauna and flora that indicate physical or chemical conditions in the water column such as colonisation depths and abundance of indicator species.</rdfs:comment>
        <rdfs:label xml:lang="en">Water quality bioindicators</rdfs:label>
        <rdf:type rdf:resource="http://www.w3.org/2002/07/owl#NamedIndividual"/>
        <rdf:type rdf:resource="http://www.w3.org/2002/07/owl#Class"/>
      </glview:MeasurementType>
    </rdfs:subClassOf>
    <owl:someValuesFrom>
      <owl:Class>
        <owl:oneOf rdf:parseType="Collection">
          <glview:MeasurementType rdf:about="http://schema.geolink.org/dev/voc/nvs/P02#WQBI"/>
        </owl:oneOf>
      </owl:Class>
    </owl:someValuesFrom>
    <owl:onProperty rdf:resource="http://schema.geolink.org/dev/view#hasMeasurementType"/>
  </owl:Restriction>
  <owl:Restriction>
    <rdfs:subClassOf>
      <glview:MeasurementType rdf:about="http://schema.geolink.org/dev/voc/nvs/P02#OSIC">
        <rdfs:subClassOf rdf:resource="http://schema.geolink.org/dev/voc/nvs/P02#ICHM"/>
        <rdfs:seeAlso rdf:resource="http://vocab.nerc.ac.uk/collection/P02/current/OSIC/"/>
        <rdfs:comment xml:lang="en">Concentration parameters for organic sulphur species in ice</rdfs:comment>
        <rdfs:label xml:lang="en">Concentration of organic sulphur species in ice</rdfs:label>
        <rdf:type rdf:resource="http://www.w3.org/2002/07/owl#NamedIndividual"/>
        <rdf:type rdf:resource="http://www.w3.org/2002/07/owl#Class"/>
      </glview:MeasurementType>
    </rdfs:subClassOf>
    <owl:someValuesFrom>
      <owl:Class>
        <owl:oneOf rdf:parseType="Collection">
          <glview:MeasurementType rdf:about="http://schema.geolink.org/dev/voc/nvs/P02#OSIC"/>
        </owl:oneOf>
      </owl:Class>
    </owl:someValuesFrom>
    <owl:onProperty rdf:resource="http://schema.geolink.org/dev/view#hasMeasurementType"/>
  </owl:Restriction>
  <owl:Restriction>
    <rdfs:subClassOf rdf:resource="http://schema.geolink.org/dev/voc/nvs/P02#TRIS"/>
    <owl:someValuesFrom>
      <owl:Class>
        <owl:oneOf rdf:parseType="Collection">
          <glview:MeasurementType rdf:about="http://schema.geolink.org/dev/voc/nvs/P02#TRIS"/>
        </owl:oneOf>
      </owl:Class>
    </owl:someValuesFrom>
    <owl:onProperty rdf:resource="http://schema.geolink.org/dev/view#hasMeasurementType"/>
  </owl:Restriction>
  <owl:Restriction>
    <rdfs:subClassOf rdf:resource="http://schema.geolink.org/dev/voc/nvs/P02#FPRT"/>
    <owl:someValuesFrom>
      <owl:Class>
        <owl:oneOf rdf:parseType="Collection">
          <glview:MeasurementType rdf:about="http://schema.geolink.org/dev/voc/nvs/P02#FPRT"/>
        </owl:oneOf>
      </owl:Class>
    </owl:someValuesFrom>
    <owl:onProperty rdf:resource="http://schema.geolink.org/dev/view#hasMeasurementType"/>
  </owl:Restriction>
  <owl:Restriction>
    <rdfs:subClassOf>
      <glview:MeasurementType rdf:about="http://schema.geolink.org/dev/voc/nvs/P02#DOXY">
        <rdfs:subClassOf rdf:resource="http://schema.geolink.org/dev/voc/nvs/P03#C015"/>
        <rdfs:seeAlso rdf:resource="http://vocab.nerc.ac.uk/collection/P02/current/DOXY/"/>
        <rdfs:comment xml:lang="en">All dissolved oxygen parameters (including saturation and utilisation) for the water column</rdfs:comment>
        <rdfs:label xml:lang="en">Dissolved oxygen parameters in the water column</rdfs:label>
        <rdf:type rdf:resource="http://www.w3.org/2002/07/owl#NamedIndividual"/>
        <rdf:type rdf:resource="http://www.w3.org/2002/07/owl#Class"/>
      </glview:MeasurementType>
    </rdfs:subClassOf>
    <owl:someValuesFrom>
      <owl:Class>
        <owl:oneOf rdf:parseType="Collection">
          <glview:MeasurementType rdf:about="http://schema.geolink.org/dev/voc/nvs/P02#DOXY"/>
        </owl:oneOf>
      </owl:Class>
    </owl:someValuesFrom>
    <owl:onProperty rdf:resource="http://schema.geolink.org/dev/view#hasMeasurementType"/>
  </owl:Restriction>
  <owl:Restriction>
    <rdfs:subClassOf>
      <glview:MeasurementType rdf:about="http://schema.geolink.org/dev/voc/nvs/P02#ACO2">
        <rdfs:subClassOf rdf:resource="http://schema.geolink.org/dev/voc/nvs/P03#M005"/>
        <rdfs:seeAlso rdf:resource="http://vocab.nerc.ac.uk/collection/P02/current/ACO2/"/>
        <rdfs:comment xml:lang="en">CO and CO2 concentration parameters in any phase of the atmosphere (but usuall the gaseous phase). Includes pCO2.</rdfs:comment>
        <rdfs:label xml:lang="en">Carbon monoxide and dioxide concentrations in the atmosphere</rdfs:label>
        <rdf:type rdf:resource="http://www.w3.org/2002/07/owl#NamedIndividual"/>
        <rdf:type rdf:resource="http://www.w3.org/2002/07/owl#Class"/>
      </glview:MeasurementType>
    </rdfs:subClassOf>
    <owl:someValuesFrom>
      <owl:Class>
        <owl:oneOf rdf:parseType="Collection">
          <glview:MeasurementType rdf:about="http://schema.geolink.org/dev/voc/nvs/P02#ACO2"/>
        </owl:oneOf>
      </owl:Class>
    </owl:someValuesFrom>
    <owl:onProperty rdf:resource="http://schema.geolink.org/dev/view#hasMeasurementType"/>
  </owl:Restriction>
  <owl:Restriction>
    <rdfs:subClassOf>
      <glview:MeasurementType rdf:about="http://schema.geolink.org/dev/voc/nvs/P02#FCST">
        <rdfs:subClassOf rdf:resource="http://schema.geolink.org/dev/voc/nvs/P03#H004"/>
        <rdfs:seeAlso rdf:resource="http://vocab.nerc.ac.uk/collection/P02/current/FCST/"/>
        <rdfs:comment xml:lang="en">Parameters quantifying and describing biota take by fishing activities</rdfs:comment>
        <rdfs:label xml:lang="en">Fish and shellfish catch statistics</rdfs:label>
        <rdf:type rdf:resource="http://www.w3.org/2002/07/owl#NamedIndividual"/>
        <rdf:type rdf:resource="http://www.w3.org/2002/07/owl#Class"/>
      </glview:MeasurementType>
    </rdfs:subClassOf>
    <owl:someValuesFrom>
      <owl:Class>
        <owl:oneOf rdf:parseType="Collection">
          <glview:MeasurementType rdf:about="http://schema.geolink.org/dev/voc/nvs/P02#FCST"/>
        </owl:oneOf>
      </owl:Class>
    </owl:someValuesFrom>
    <owl:onProperty rdf:resource="http://schema.geolink.org/dev/view#hasMeasurementType"/>
  </owl:Restriction>
  <owl:Restriction>
    <rdfs:subClassOf rdf:resource="http://schema.geolink.org/dev/voc/nvs/P02#SR2D"/>
    <owl:someValuesFrom>
      <owl:Class>
        <owl:oneOf rdf:parseType="Collection">
          <glview:MeasurementType rdf:about="http://schema.geolink.org/dev/voc/nvs/P02#SR2D"/>
        </owl:oneOf>
      </owl:Class>
    </owl:someValuesFrom>
    <owl:onProperty rdf:resource="http://schema.geolink.org/dev/view#hasMeasurementType"/>
  </owl:Restriction>
  <owl:Restriction>
    <rdfs:subClassOf rdf:resource="http://schema.geolink.org/dev/voc/nvs/P02#DGPW"/>
    <owl:someValuesFrom>
      <owl:Class>
        <owl:oneOf rdf:parseType="Collection">
          <glview:MeasurementType rdf:about="http://schema.geolink.org/dev/voc/nvs/P02#DGPW"/>
        </owl:oneOf>
      </owl:Class>
    </owl:someValuesFrom>
    <owl:onProperty rdf:resource="http://schema.geolink.org/dev/view#hasMeasurementType"/>
  </owl:Restriction>
  <owl:Restriction>
    <rdfs:subClassOf rdf:resource="http://schema.geolink.org/dev/voc/nvs/P02#BCOC"/>
    <owl:someValuesFrom>
      <owl:Class>
        <owl:oneOf rdf:parseType="Collection">
          <glview:MeasurementType rdf:about="http://schema.geolink.org/dev/voc/nvs/P02#BCOC"/>
        </owl:oneOf>
      </owl:Class>
    </owl:someValuesFrom>
    <owl:onProperty rdf:resource="http://schema.geolink.org/dev/view#hasMeasurementType"/>
  </owl:Restriction>
  <owl:Restriction>
    <rdfs:subClassOf rdf:resource="http://schema.geolink.org/dev/voc/nvs/P02#PPWC"/>
    <owl:someValuesFrom>
      <owl:Class>
        <owl:oneOf rdf:parseType="Collection">
          <glview:MeasurementType rdf:about="http://schema.geolink.org/dev/voc/nvs/P02#PPWC"/>
        </owl:oneOf>
      </owl:Class>
    </owl:someValuesFrom>
    <owl:onProperty rdf:resource="http://schema.geolink.org/dev/view#hasMeasurementType"/>
  </owl:Restriction>
  <owl:Restriction>
    <rdfs:subClassOf>
      <glview:MeasurementType rdf:about="http://schema.geolink.org/dev/voc/nvs/P02#IPRX">
        <rdfs:subClassOf rdf:resource="http://schema.geolink.org/dev/voc/nvs/P03#C045"/>
        <rdfs:seeAlso rdf:resource="http://vocab.nerc.ac.uk/collection/P02/current/IPRX/"/>
        <rdfs:comment xml:lang="en">Parameters related to compounds containing two oxygen atoms joined by a single bond but no carbon atoms in any body of fresh or salt water.</rdfs:comment>
        <rdfs:label xml:lang="en">Inorganic peroxides in water bodies</rdfs:label>
        <rdf:type rdf:resource="http://www.w3.org/2002/07/owl#NamedIndividual"/>
        <rdf:type rdf:resource="http://www.w3.org/2002/07/owl#Class"/>
      </glview:MeasurementType>
    </rdfs:subClassOf>
    <owl:someValuesFrom>
      <owl:Class>
        <owl:oneOf rdf:parseType="Collection">
          <glview:MeasurementType rdf:about="http://schema.geolink.org/dev/voc/nvs/P02#IPRX"/>
        </owl:oneOf>
      </owl:Class>
    </owl:someValuesFrom>
    <owl:onProperty rdf:resource="http://schema.geolink.org/dev/view#hasMeasurementType"/>
  </owl:Restriction>
  <owl:Restriction>
    <rdfs:subClassOf>
      <glview:MeasurementType rdf:about="http://schema.geolink.org/dev/voc/nvs/P02#V999">
        <rdfs:subClassOf rdf:resource="http://schema.geolink.org/dev/voc/nvs/P03#B025"/>
        <rdfs:seeAlso rdf:resource="http://vocab.nerc.ac.uk/collection/P02/current/V999/"/>
        <rdfs:comment xml:lang="en">Microzooplankton biovolume parameters presented at the level of taxa that may be mapped to entities in the ITIS taxonomy. These may be at any taxonomic level from sub-species upwards.</rdfs:comment>
        <rdfs:label xml:lang="en">Microzooplankton taxonomy-related biovolume per unit volume of the water column</rdfs:label>
        <rdf:type rdf:resource="http://www.w3.org/2002/07/owl#NamedIndividual"/>
        <rdf:type rdf:resource="http://www.w3.org/2002/07/owl#Class"/>
      </glview:MeasurementType>
    </rdfs:subClassOf>
    <owl:someValuesFrom>
      <owl:Class>
        <owl:oneOf rdf:parseType="Collection">
          <glview:MeasurementType rdf:about="http://schema.geolink.org/dev/voc/nvs/P02#V999"/>
        </owl:oneOf>
      </owl:Class>
    </owl:someValuesFrom>
    <owl:onProperty rdf:resource="http://schema.geolink.org/dev/view#hasMeasurementType"/>
  </owl:Restriction>
  <owl:Restriction>
    <rdfs:subClassOf rdf:resource="http://schema.geolink.org/dev/voc/nvs/P02#BPBP"/>
    <owl:someValuesFrom>
      <owl:Class>
        <owl:oneOf rdf:parseType="Collection">
          <glview:MeasurementType rdf:about="http://schema.geolink.org/dev/voc/nvs/P02#BPBP"/>
        </owl:oneOf>
      </owl:Class>
    </owl:someValuesFrom>
    <owl:onProperty rdf:resource="http://schema.geolink.org/dev/view#hasMeasurementType"/>
  </owl:Restriction>
  <owl:Restriction>
    <rdfs:subClassOf>
      <glview:MeasurementType rdf:about="http://schema.geolink.org/dev/voc/nvs/P02#TCFX">
        <rdfs:subClassOf rdf:resource="http://schema.geolink.org/dev/voc/nvs/P03#O005"/>
        <rdfs:seeAlso rdf:resource="http://vocab.nerc.ac.uk/collection/P02/current/TCFX/"/>
        <rdfs:comment xml:lang="en">Fluxes of particulate total, organic and inorganic carbon (including as CaCO3) and nitrogen (often measured as 'total' but assumed to be 'organic'). Organic matter is defined as matter lost on ignition.</rdfs:comment>
        <rdfs:label xml:lang="en">Sedimentation flux of carbon, nitrogen or organic matter in the water column</rdfs:label>
        <rdf:type rdf:resource="http://www.w3.org/2002/07/owl#NamedIndividual"/>
        <rdf:type rdf:resource="http://www.w3.org/2002/07/owl#Class"/>
      </glview:MeasurementType>
    </rdfs:subClassOf>
    <owl:someValuesFrom>
      <owl:Class>
        <owl:oneOf rdf:parseType="Collection">
          <glview:MeasurementType rdf:about="http://schema.geolink.org/dev/voc/nvs/P02#TCFX"/>
        </owl:oneOf>
      </owl:Class>
    </owl:someValuesFrom>
    <owl:onProperty rdf:resource="http://schema.geolink.org/dev/view#hasMeasurementType"/>
  </owl:Restriction>
  <owl:Restriction>
    <rdfs:subClassOf rdf:resource="http://schema.geolink.org/dev/voc/nvs/P02#GP068"/>
    <owl:someValuesFrom>
      <owl:Class>
        <owl:oneOf rdf:parseType="Collection">
          <glview:MeasurementType rdf:about="http://schema.geolink.org/dev/voc/nvs/P02#GP068"/>
        </owl:oneOf>
      </owl:Class>
    </owl:someValuesFrom>
    <owl:onProperty rdf:resource="http://schema.geolink.org/dev/view#hasMeasurementType"/>
  </owl:Restriction>
  <owl:Restriction>
    <rdfs:subClassOf rdf:resource="http://schema.geolink.org/dev/voc/nvs/P02#GTCH"/>
    <owl:someValuesFrom>
      <owl:Class>
        <owl:oneOf rdf:parseType="Collection">
          <glview:MeasurementType rdf:about="http://schema.geolink.org/dev/voc/nvs/P02#GTCH"/>
        </owl:oneOf>
      </owl:Class>
    </owl:someValuesFrom>
    <owl:onProperty rdf:resource="http://schema.geolink.org/dev/view#hasMeasurementType"/>
  </owl:Restriction>
  <owl:Restriction>
    <rdfs:subClassOf rdf:resource="http://schema.geolink.org/dev/voc/nvs/P02#RBSC"/>
    <owl:someValuesFrom>
      <owl:Class>
        <owl:oneOf rdf:parseType="Collection">
          <owl:NamedIndividual rdf:about="http://schema.geolink.org/dev/voc/nvs/P02#RBSC"/>
        </owl:oneOf>
      </owl:Class>
    </owl:someValuesFrom>
    <owl:onProperty rdf:resource="http://schema.geolink.org/dev/view#hasMeasurementType"/>
  </owl:Restriction>
  <owl:Restriction>
    <rdfs:subClassOf>
      <glview:MeasurementType rdf:about="http://schema.geolink.org/dev/voc/nvs/P02#MNGS">
        <rdfs:subClassOf rdf:resource="http://schema.geolink.org/dev/voc/nvs/P03#G040"/>
        <rdfs:seeAlso rdf:resource="http://vocab.nerc.ac.uk/collection/P02/current/MNGS/"/>
        <rdfs:comment xml:lang="en">Parameters specifying the physical dimensions of the particles comprising unlithified sediment (including expressions of shape such as aspect ratio) and statistics derived from their variation in a sample (e.g. mean, mode, sorting, skewness).</rdfs:comment>
        <rdfs:label xml:lang="en">Sediment grain size parameters</rdfs:label>
        <rdf:type rdf:resource="http://www.w3.org/2002/07/owl#NamedIndividual"/>
        <rdf:type rdf:resource="http://www.w3.org/2002/07/owl#Class"/>
      </glview:MeasurementType>
    </rdfs:subClassOf>
    <owl:someValuesFrom>
      <owl:Class>
        <owl:oneOf rdf:parseType="Collection">
          <glview:MeasurementType rdf:about="http://schema.geolink.org/dev/voc/nvs/P02#MNGS"/>
        </owl:oneOf>
      </owl:Class>
    </owl:someValuesFrom>
    <owl:onProperty rdf:resource="http://schema.geolink.org/dev/view#hasMeasurementType"/>
  </owl:Restriction>
  <owl:Restriction>
    <rdfs:subClassOf>
      <glview:MeasurementType rdf:about="http://schema.geolink.org/dev/voc/nvs/P02#ICEM">
        <rdfs:subClassOf rdf:resource="http://schema.geolink.org/dev/voc/nvs/P03#M015"/>
        <rdfs:seeAlso rdf:resource="http://vocab.nerc.ac.uk/collection/P02/current/ICEM/"/>
        <rdfs:comment xml:lang="en">Parameters specifying the speed and direction of sea or land ice and the stresses associated with this motion.</rdfs:comment>
        <rdfs:label xml:lang="en">Ice motion and related parameters</rdfs:label>
        <rdf:type rdf:resource="http://www.w3.org/2002/07/owl#NamedIndividual"/>
        <rdf:type rdf:resource="http://www.w3.org/2002/07/owl#Class"/>
      </glview:MeasurementType>
    </rdfs:subClassOf>
    <owl:someValuesFrom>
      <owl:Class>
        <owl:oneOf rdf:parseType="Collection">
          <glview:MeasurementType rdf:about="http://schema.geolink.org/dev/voc/nvs/P02#ICEM"/>
        </owl:oneOf>
      </owl:Class>
    </owl:someValuesFrom>
    <owl:onProperty rdf:resource="http://schema.geolink.org/dev/view#hasMeasurementType"/>
  </owl:Restriction>
  <owl:Restriction>
    <rdfs:subClassOf>
      <glview:MeasurementType rdf:about="http://schema.geolink.org/dev/voc/nvs/P02#RSIS">
        <rdfs:subClassOf rdf:resource="http://schema.geolink.org/dev/voc/nvs/P03#GPYS"/>
        <rdfs:seeAlso rdf:resource="http://vocab.nerc.ac.uk/collection/P02/current/RSIS/"/>
        <rdfs:comment xml:lang="en">Parameters quantifying the electrical properties of geological units in the field. Includes parameters used to determine resistivity structure for shallow sediment properties, porosities and presence of hydrocarbon (CSEM), deeper crust and mantle studies (Magnetotellurics) and ore body location (polarisation).</rdfs:comment>
        <rdfs:label xml:lang="en">Field resistivity,  electromagnetics  and polarisation</rdfs:label>
        <rdf:type rdf:resource="http://www.w3.org/2002/07/owl#NamedIndividual"/>
        <rdf:type rdf:resource="http://www.w3.org/2002/07/owl#Class"/>
      </glview:MeasurementType>
    </rdfs:subClassOf>
    <owl:someValuesFrom>
      <owl:Class>
        <owl:oneOf rdf:parseType="Collection">
          <glview:MeasurementType rdf:about="http://schema.geolink.org/dev/voc/nvs/P02#RSIS"/>
        </owl:oneOf>
      </owl:Class>
    </owl:someValuesFrom>
    <owl:onProperty rdf:resource="http://schema.geolink.org/dev/view#hasMeasurementType"/>
  </owl:Restriction>
  <owl:Restriction>
    <rdfs:subClassOf>
      <glview:MeasurementType rdf:about="http://schema.geolink.org/dev/voc/nvs/P02#TDPX">
        <rdfs:subClassOf rdf:resource="http://schema.geolink.org/dev/voc/nvs/P03#C005"/>
        <rdfs:seeAlso rdf:resource="http://vocab.nerc.ac.uk/collection/P02/current/TDPX/"/>
        <rdfs:comment xml:lang="en">Concentration of total (organic plus inorganic) or organic dissolved phosphorus per unit volume of the water column. Grouped together as organic phosphorus frequently determined as total phosphorus.</rdfs:comment>
        <rdfs:label xml:lang="en">Dissolved total or organic phosphorus concentration in the water column</rdfs:label>
        <rdf:type rdf:resource="http://www.w3.org/2002/07/owl#NamedIndividual"/>
        <rdf:type rdf:resource="http://www.w3.org/2002/07/owl#Class"/>
      </glview:MeasurementType>
    </rdfs:subClassOf>
    <owl:someValuesFrom>
      <owl:Class>
        <owl:oneOf rdf:parseType="Collection">
          <glview:MeasurementType rdf:about="http://schema.geolink.org/dev/voc/nvs/P02#TDPX"/>
        </owl:oneOf>
      </owl:Class>
    </owl:someValuesFrom>
    <owl:onProperty rdf:resource="http://schema.geolink.org/dev/view#hasMeasurementType"/>
  </owl:Restriction>
  <owl:Restriction>
    <rdfs:subClassOf>
      <glview:MeasurementType rdf:about="http://schema.geolink.org/dev/voc/nvs/P02#SICN">
        <rdfs:subClassOf rdf:resource="http://schema.geolink.org/dev/voc/nvs/P02#RMIN"/>
        <rdfs:seeAlso rdf:resource="http://vocab.nerc.ac.uk/collection/P02/current/SICN/"/>
        <rdfs:comment xml:lang="en">Concentration parameters for silicon species (including opal) in sediment (anything collected by a corer including fluff)</rdfs:comment>
        <rdfs:label xml:lang="en">Concentration of silicon species in sediment</rdfs:label>
        <rdf:type rdf:resource="http://www.w3.org/2002/07/owl#NamedIndividual"/>
        <rdf:type rdf:resource="http://www.w3.org/2002/07/owl#Class"/>
      </glview:MeasurementType>
    </rdfs:subClassOf>
    <owl:someValuesFrom>
      <owl:Class>
        <owl:oneOf rdf:parseType="Collection">
          <glview:MeasurementType rdf:about="http://schema.geolink.org/dev/voc/nvs/P02#SICN"/>
        </owl:oneOf>
      </owl:Class>
    </owl:someValuesFrom>
    <owl:onProperty rdf:resource="http://schema.geolink.org/dev/view#hasMeasurementType"/>
  </owl:Restriction>
  <owl:Restriction>
    <rdfs:subClassOf>
      <glview:MeasurementType rdf:about="http://schema.geolink.org/dev/voc/nvs/P02#NTUP">
        <rdfs:subClassOf rdf:resource="http://schema.geolink.org/dev/voc/nvs/P03#O010"/>
        <rdfs:subClassOf rdf:resource="http://schema.geolink.org/dev/voc/nvs/P03#C040"/>
        <rdfs:seeAlso rdf:resource="http://vocab.nerc.ac.uk/collection/P02/current/NTUP/"/>
        <rdfs:comment xml:lang="en">Parameters quantifying the uptake rate of nitrate or gaseous nitrogen by flora and fauna living in any body of salt or fresh water</rdfs:comment>
        <rdfs:label xml:lang="en">New production in water bodies</rdfs:label>
        <rdf:type rdf:resource="http://www.w3.org/2002/07/owl#NamedIndividual"/>
        <rdf:type rdf:resource="http://www.w3.org/2002/07/owl#Class"/>
      </glview:MeasurementType>
    </rdfs:subClassOf>
    <owl:someValuesFrom>
      <owl:Class>
        <owl:oneOf rdf:parseType="Collection">
          <glview:MeasurementType rdf:about="http://schema.geolink.org/dev/voc/nvs/P02#NTUP"/>
        </owl:oneOf>
      </owl:Class>
    </owl:someValuesFrom>
    <owl:onProperty rdf:resource="http://schema.geolink.org/dev/view#hasMeasurementType"/>
  </owl:Restriction>
  <owl:Restriction>
    <rdfs:subClassOf>
      <glview:MeasurementType rdf:about="http://schema.geolink.org/dev/voc/nvs/P02#ZCTC">
        <rdfs:subClassOf rdf:resource="http://schema.geolink.org/dev/voc/nvs/P03#B045"/>
        <rdfs:subClassOf rdf:resource="http://schema.geolink.org/dev/voc/nvs/P03#B070"/>
        <rdfs:seeAlso rdf:resource="http://vocab.nerc.ac.uk/collection/P02/current/ZCTC/"/>
        <rdfs:comment xml:lang="en">Zooplankton (mesozooplankton plus larger pelagic animals excluding fish, reptiles and mammals) carbon biomass parameters presented at the level of taxa that may be mapped to entities in the ITIS taxonomy.  These may be at any taxonomic level from sub-species upwards.</rdfs:comment>
        <rdfs:label xml:lang="en">Zooplankton taxonomy-related biomass expressed as carbon per unit volume of the water column</rdfs:label>
        <rdf:type rdf:resource="http://www.w3.org/2002/07/owl#NamedIndividual"/>
        <rdf:type rdf:resource="http://www.w3.org/2002/07/owl#Class"/>
      </glview:MeasurementType>
    </rdfs:subClassOf>
    <owl:someValuesFrom>
      <owl:Class>
        <owl:oneOf rdf:parseType="Collection">
          <glview:MeasurementType rdf:about="http://schema.geolink.org/dev/voc/nvs/P02#ZCTC"/>
        </owl:oneOf>
      </owl:Class>
    </owl:someValuesFrom>
    <owl:onProperty rdf:resource="http://schema.geolink.org/dev/view#hasMeasurementType"/>
  </owl:Restriction>
  <owl:Restriction>
    <rdfs:subClassOf>
      <glview:MeasurementType rdf:about="http://schema.geolink.org/dev/voc/nvs/P02#IATX">
        <rdfs:subClassOf rdf:resource="http://schema.geolink.org/dev/voc/nvs/P03#B045"/>
        <rdfs:subClassOf rdf:resource="http://schema.geolink.org/dev/voc/nvs/P03#B070"/>
        <rdfs:seeAlso rdf:resource="http://vocab.nerc.ac.uk/collection/P02/current/IATX/"/>
        <rdfs:comment xml:lang="en">Insecta abundance parameters presented at the level of taxa that may be mapped to entities in the ITIS taxonomy.  These may be at any taxonomic level from sub-species upwards.</rdfs:comment>
        <rdfs:label xml:lang="en">Insecta taxonomy-related abundance per unit volume of the water column</rdfs:label>
        <rdf:type rdf:resource="http://www.w3.org/2002/07/owl#NamedIndividual"/>
        <rdf:type rdf:resource="http://www.w3.org/2002/07/owl#Class"/>
      </glview:MeasurementType>
    </rdfs:subClassOf>
    <owl:someValuesFrom>
      <owl:Class>
        <owl:oneOf rdf:parseType="Collection">
          <glview:MeasurementType rdf:about="http://schema.geolink.org/dev/voc/nvs/P02#IATX"/>
        </owl:oneOf>
      </owl:Class>
    </owl:someValuesFrom>
    <owl:onProperty rdf:resource="http://schema.geolink.org/dev/view#hasMeasurementType"/>
  </owl:Restriction>
  <owl:Restriction>
    <rdfs:subClassOf>
      <glview:MeasurementType rdf:about="http://schema.geolink.org/dev/voc/nvs/P02#PHWB">
        <rdfs:subClassOf rdf:resource="http://schema.geolink.org/dev/voc/nvs/P03#C055"/>
        <rdfs:subClassOf rdf:resource="http://schema.geolink.org/dev/voc/nvs/P03#H001"/>
        <rdfs:seeAlso rdf:resource="http://vocab.nerc.ac.uk/collection/P02/current/PHWB/"/>
        <rdfs:comment xml:lang="en">Concentration parameters for substances synthesised by man to modify bodily function or diagnose, cure, mitigate, treat, or prevent disease in either solution or suspension (i.e.includes measurements in both the dissolved and particulate phases) in any body of salt or fresh water.</rdfs:comment>
        <rdfs:label xml:lang="en">Pharmaceutical concentrations in water bodies</rdfs:label>
        <rdf:type rdf:resource="http://www.w3.org/2002/07/owl#NamedIndividual"/>
        <rdf:type rdf:resource="http://www.w3.org/2002/07/owl#Class"/>
      </glview:MeasurementType>
    </rdfs:subClassOf>
    <owl:someValuesFrom>
      <owl:Class>
        <owl:oneOf rdf:parseType="Collection">
          <glview:MeasurementType rdf:about="http://schema.geolink.org/dev/voc/nvs/P02#PHWB"/>
        </owl:oneOf>
      </owl:Class>
    </owl:someValuesFrom>
    <owl:onProperty rdf:resource="http://schema.geolink.org/dev/view#hasMeasurementType"/>
  </owl:Restriction>
  <owl:Restriction>
    <rdfs:subClassOf rdf:resource="http://schema.geolink.org/dev/voc/nvs/P02#BCPB"/>
    <owl:someValuesFrom>
      <owl:Class>
        <owl:oneOf rdf:parseType="Collection">
          <glview:MeasurementType rdf:about="http://schema.geolink.org/dev/voc/nvs/P02#BCPB"/>
        </owl:oneOf>
      </owl:Class>
    </owl:someValuesFrom>
    <owl:onProperty rdf:resource="http://schema.geolink.org/dev/view#hasMeasurementType"/>
  </owl:Restriction>
  <owl:Restriction>
    <rdfs:subClassOf rdf:resource="http://schema.geolink.org/dev/voc/nvs/P02#NTUP"/>
    <owl:someValuesFrom>
      <owl:Class>
        <owl:oneOf rdf:parseType="Collection">
          <glview:MeasurementType rdf:about="http://schema.geolink.org/dev/voc/nvs/P02#NTUP"/>
        </owl:oneOf>
      </owl:Class>
    </owl:someValuesFrom>
    <owl:onProperty rdf:resource="http://schema.geolink.org/dev/view#hasMeasurementType"/>
  </owl:Restriction>
  <owl:Restriction>
    <rdfs:subClassOf rdf:resource="http://schema.geolink.org/dev/voc/nvs/P02#HAAC"/>
    <owl:someValuesFrom>
      <owl:Class>
        <owl:oneOf rdf:parseType="Collection">
          <glview:MeasurementType rdf:about="http://schema.geolink.org/dev/voc/nvs/P02#HAAC"/>
        </owl:oneOf>
      </owl:Class>
    </owl:someValuesFrom>
    <owl:onProperty rdf:resource="http://schema.geolink.org/dev/view#hasMeasurementType"/>
  </owl:Restriction>
  <owl:Restriction>
    <rdfs:subClassOf>
      <glview:MeasurementType rdf:about="http://schema.geolink.org/dev/voc/nvs/P02#GRZO">
        <rdfs:subClassOf rdf:resource="http://schema.geolink.org/dev/voc/nvs/P03#B045"/>
        <rdfs:subClassOf rdf:resource="http://schema.geolink.org/dev/voc/nvs/P03#O010"/>
        <rdfs:seeAlso rdf:resource="http://vocab.nerc.ac.uk/collection/P02/current/GRZO/"/>
        <rdfs:comment xml:lang="en">Parameters pertaining to zooplankton growth rates including biochemical proxies such as AARS activity</rdfs:comment>
        <rdfs:label xml:lang="en">Zooplankton growth rates</rdfs:label>
        <rdf:type rdf:resource="http://www.w3.org/2002/07/owl#NamedIndividual"/>
        <rdf:type rdf:resource="http://www.w3.org/2002/07/owl#Class"/>
      </glview:MeasurementType>
    </rdfs:subClassOf>
    <owl:someValuesFrom>
      <owl:Class>
        <owl:oneOf rdf:parseType="Collection">
          <glview:MeasurementType rdf:about="http://schema.geolink.org/dev/voc/nvs/P02#GRZO"/>
        </owl:oneOf>
      </owl:Class>
    </owl:someValuesFrom>
    <owl:onProperty rdf:resource="http://schema.geolink.org/dev/view#hasMeasurementType"/>
  </owl:Restriction>
  <owl:Restriction>
    <rdfs:subClassOf>
      <glview:MeasurementType rdf:about="http://schema.geolink.org/dev/voc/nvs/P02#CBFX">
        <rdfs:subClassOf rdf:resource="http://schema.geolink.org/dev/voc/nvs/P03#O005"/>
        <rdfs:seeAlso rdf:resource="http://vocab.nerc.ac.uk/collection/P02/current/CBFX/"/>
        <rdfs:comment></rdfs:comment>
        <rdfs:label xml:lang="en">Sedimentation flux of carbohydates in the water column</rdfs:label>
        <rdf:type rdf:resource="http://www.w3.org/2002/07/owl#NamedIndividual"/>
        <rdf:type rdf:resource="http://www.w3.org/2002/07/owl#Class"/>
      </glview:MeasurementType>
    </rdfs:subClassOf>
    <owl:someValuesFrom>
      <owl:Class>
        <owl:oneOf rdf:parseType="Collection">
          <glview:MeasurementType rdf:about="http://schema.geolink.org/dev/voc/nvs/P02#CBFX"/>
        </owl:oneOf>
      </owl:Class>
    </owl:someValuesFrom>
    <owl:onProperty rdf:resource="http://schema.geolink.org/dev/view#hasMeasurementType"/>
  </owl:Restriction>
  <owl:Restriction>
    <rdfs:subClassOf>
      <glview:MeasurementType rdf:about="http://schema.geolink.org/dev/voc/nvs/P02#SCOX">
        <rdfs:subClassOf rdf:resource="http://schema.geolink.org/dev/voc/nvs/P03#C015"/>
        <rdfs:seeAlso rdf:resource="http://vocab.nerc.ac.uk/collection/P02/current/SCOX/"/>
        <rdfs:comment xml:lang="en">All concentration parameters for inorganic dissolved gases other than oxygen and the noble gases in the water column</rdfs:comment>
        <rdfs:label xml:lang="en">Dissolved concentration parameters for other gases in the water column</rdfs:label>
        <rdf:type rdf:resource="http://www.w3.org/2002/07/owl#NamedIndividual"/>
        <rdf:type rdf:resource="http://www.w3.org/2002/07/owl#Class"/>
      </glview:MeasurementType>
    </rdfs:subClassOf>
    <owl:someValuesFrom>
      <owl:Class>
        <owl:oneOf rdf:parseType="Collection">
          <glview:MeasurementType rdf:about="http://schema.geolink.org/dev/voc/nvs/P02#SCOX"/>
        </owl:oneOf>
      </owl:Class>
    </owl:someValuesFrom>
    <owl:onProperty rdf:resource="http://schema.geolink.org/dev/view#hasMeasurementType"/>
  </owl:Restriction>
  <owl:Restriction>
    <rdfs:subClassOf>
      <glview:MeasurementType rdf:about="http://schema.geolink.org/dev/voc/nvs/P02#GP079">
        <rdfs:subClassOf rdf:resource="http://schema.geolink.org/dev/voc/nvs/P03#B045"/>
        <rdfs:subClassOf rdf:resource="http://schema.geolink.org/dev/voc/nvs/P03#B070"/>
        <rdfs:seeAlso rdf:resource="http://vocab.nerc.ac.uk/collection/P02/current/GP079/"/>
        <rdfs:comment xml:lang="en">Zooplankton (mesozooplankton and larger, exclusing fish, mammals, reptiles and insects) biomass determined by weighing unprocessed catch samples.</rdfs:comment>
        <rdfs:label xml:lang="en">Zooplankton wet weight biomass</rdfs:label>
        <rdf:type rdf:resource="http://www.w3.org/2002/07/owl#NamedIndividual"/>
        <rdf:type rdf:resource="http://www.w3.org/2002/07/owl#Class"/>
      </glview:MeasurementType>
    </rdfs:subClassOf>
    <owl:someValuesFrom>
      <owl:Class>
        <owl:oneOf rdf:parseType="Collection">
          <glview:MeasurementType rdf:about="http://schema.geolink.org/dev/voc/nvs/P02#GP079"/>
        </owl:oneOf>
      </owl:Class>
    </owl:someValuesFrom>
    <owl:onProperty rdf:resource="http://schema.geolink.org/dev/view#hasMeasurementType"/>
  </owl:Restriction>
  <owl:Restriction>
    <rdfs:subClassOf>
      <owl:NamedIndividual rdf:about="http://schema.geolink.org/dev/voc/nvs/P02#OMWC">
        <rdfs:label xml:lang="en">Organometallic species concentration parameters in water bodies</rdfs:label>
        <rdf:type rdf:resource="http://www.w3.org/2002/07/owl#Class"/>
        <rdfs:comment xml:lang="en">All organometallic compound concentration parameters (including saturations for gaseous species) in all phases of any body of fresh or salt water</rdfs:comment>
        <rdfs:subClassOf rdf:resource="http://schema.geolink.org/dev/voc/nvs/P03#H001"/>
        <rdfs:subClassOf rdf:resource="http://schema.geolink.org/dev/voc/nvs/P03#C035"/>
        <rdfs:subClassOf rdf:resource="http://schema.geolink.org/dev/voc/nvs/P03#C050"/>
        <rdfs:seeAlso rdf:resource="http://vocab.nerc.ac.uk/collection/P02/current/OMWC/"/>
        <rdfs:subClassOf rdf:resource="http://schema.geolink.org/dev/voc/nvs/P03#C055"/>
        <rdf:type rdf:resource="http://schema.geolink.org/dev/view#MeasurementType"/>
      </owl:NamedIndividual>
    </rdfs:subClassOf>
    <owl:someValuesFrom>
      <owl:Class>
        <owl:oneOf rdf:parseType="Collection">
          <owl:NamedIndividual rdf:about="http://schema.geolink.org/dev/voc/nvs/P02#OMWC"/>
        </owl:oneOf>
      </owl:Class>
    </owl:someValuesFrom>
    <owl:onProperty rdf:resource="http://schema.geolink.org/dev/view#hasMeasurementType"/>
  </owl:Restriction>
  <owl:Restriction>
    <rdfs:subClassOf rdf:resource="http://schema.geolink.org/dev/voc/nvs/P02#RBSC"/>
    <owl:someValuesFrom>
      <owl:Class>
        <owl:oneOf rdf:parseType="Collection">
          <owl:NamedIndividual rdf:about="http://schema.geolink.org/dev/voc/nvs/P02#RBSC"/>
        </owl:oneOf>
      </owl:Class>
    </owl:someValuesFrom>
    <owl:onProperty rdf:resource="http://schema.geolink.org/dev/view#hasMeasurementType"/>
  </owl:Restriction>
  <owl:Restriction>
    <rdfs:subClassOf rdf:resource="http://schema.geolink.org/dev/voc/nvs/P02#PNTX"/>
    <owl:someValuesFrom>
      <owl:Class>
        <owl:oneOf rdf:parseType="Collection">
          <glview:MeasurementType rdf:about="http://schema.geolink.org/dev/voc/nvs/P02#PNTX"/>
        </owl:oneOf>
      </owl:Class>
    </owl:someValuesFrom>
    <owl:onProperty rdf:resource="http://schema.geolink.org/dev/view#hasMeasurementType"/>
  </owl:Restriction>
  <owl:Restriction>
    <rdfs:subClassOf rdf:resource="http://schema.geolink.org/dev/voc/nvs/P02#OCPW"/>
    <owl:someValuesFrom>
      <owl:Class>
        <owl:oneOf rdf:parseType="Collection">
          <glview:MeasurementType rdf:about="http://schema.geolink.org/dev/voc/nvs/P02#OCPW"/>
        </owl:oneOf>
      </owl:Class>
    </owl:someValuesFrom>
    <owl:onProperty rdf:resource="http://schema.geolink.org/dev/view#hasMeasurementType"/>
  </owl:Restriction>
  <owl:Restriction>
    <rdfs:subClassOf rdf:resource="http://schema.geolink.org/dev/voc/nvs/P02#GRZO"/>
    <owl:someValuesFrom>
      <owl:Class>
        <owl:oneOf rdf:parseType="Collection">
          <glview:MeasurementType rdf:about="http://schema.geolink.org/dev/voc/nvs/P02#GRZO"/>
        </owl:oneOf>
      </owl:Class>
    </owl:someValuesFrom>
    <owl:onProperty rdf:resource="http://schema.geolink.org/dev/view#hasMeasurementType"/>
  </owl:Restriction>
  <owl:Restriction>
    <rdfs:subClassOf>
      <glview:MeasurementType rdf:about="http://schema.geolink.org/dev/voc/nvs/P02#LRZA">
        <rdfs:subClassOf rdf:resource="http://schema.geolink.org/dev/voc/nvs/P03#D030"/>
        <rdfs:seeAlso rdf:resource="http://vocab.nerc.ac.uk/collection/P02/current/LRZA/"/>
        <rdfs:comment xml:lang="en">Vertical water movement parameters including non-directional speeds</rdfs:comment>
        <rdfs:label xml:lang="en">Vertical velocity of the water column (currents)</rdfs:label>
        <rdf:type rdf:resource="http://www.w3.org/2002/07/owl#NamedIndividual"/>
        <rdf:type rdf:resource="http://www.w3.org/2002/07/owl#Class"/>
      </glview:MeasurementType>
    </rdfs:subClassOf>
    <owl:someValuesFrom>
      <owl:Class>
        <owl:oneOf rdf:parseType="Collection">
          <glview:MeasurementType rdf:about="http://schema.geolink.org/dev/voc/nvs/P02#LRZA"/>
        </owl:oneOf>
      </owl:Class>
    </owl:someValuesFrom>
    <owl:onProperty rdf:resource="http://schema.geolink.org/dev/view#hasMeasurementType"/>
  </owl:Restriction>
  <owl:Restriction>
    <rdfs:subClassOf>
      <glview:MeasurementType rdf:about="http://schema.geolink.org/dev/voc/nvs/P02#LVEG">
        <rdfs:subClassOf rdf:resource="http://schema.geolink.org/dev/voc/nvs/P03#T001"/>
        <rdfs:seeAlso rdf:resource="http://vocab.nerc.ac.uk/collection/P02/current/LVEG/"/>
        <rdfs:comment xml:lang="en">Parameters relating to land (including marshes and the intertidal zone) vegetation</rdfs:comment>
        <rdfs:label xml:lang="en">Land vegetation</rdfs:label>
        <rdf:type rdf:resource="http://www.w3.org/2002/07/owl#NamedIndividual"/>
        <rdf:type rdf:resource="http://www.w3.org/2002/07/owl#Class"/>
      </glview:MeasurementType>
    </rdfs:subClassOf>
    <owl:someValuesFrom>
      <owl:Class>
        <owl:oneOf rdf:parseType="Collection">
          <glview:MeasurementType rdf:about="http://schema.geolink.org/dev/voc/nvs/P02#LVEG"/>
        </owl:oneOf>
      </owl:Class>
    </owl:someValuesFrom>
    <owl:onProperty rdf:resource="http://schema.geolink.org/dev/view#hasMeasurementType"/>
  </owl:Restriction>
  <owl:Restriction>
    <rdfs:subClassOf>
      <glview:MeasurementType rdf:about="http://schema.geolink.org/dev/voc/nvs/P02#INLZ">
        <rdfs:subClassOf rdf:resource="http://schema.geolink.org/dev/voc/nvs/P03#B070"/>
        <rdfs:subClassOf rdf:resource="http://schema.geolink.org/dev/voc/nvs/P03#G055"/>
        <rdfs:seeAlso rdf:resource="http://vocab.nerc.ac.uk/collection/P02/current/INLZ/"/>
        <rdfs:comment xml:lang="en">Insect (Class Insecta) and earthworm (Subclass Oligochaeta) abundance per unit area of the littoral zone (between spring tide high and low water) parameters.</rdfs:comment>
        <rdfs:label xml:lang="en">Insect and earthworm taxonomy-related abundance per unit area of the littoral zone</rdfs:label>
        <rdf:type rdf:resource="http://www.w3.org/2002/07/owl#NamedIndividual"/>
        <rdf:type rdf:resource="http://www.w3.org/2002/07/owl#Class"/>
      </glview:MeasurementType>
    </rdfs:subClassOf>
    <owl:someValuesFrom>
      <owl:Class>
        <owl:oneOf rdf:parseType="Collection">
          <glview:MeasurementType rdf:about="http://schema.geolink.org/dev/voc/nvs/P02#INLZ"/>
        </owl:oneOf>
      </owl:Class>
    </owl:someValuesFrom>
    <owl:onProperty rdf:resource="http://schema.geolink.org/dev/view#hasMeasurementType"/>
  </owl:Restriction>
  <owl:Restriction>
    <rdfs:subClassOf>
      <glview:MeasurementType rdf:about="http://schema.geolink.org/dev/voc/nvs/P02#FATX">
        <rdfs:subClassOf rdf:resource="http://schema.geolink.org/dev/voc/nvs/P03#B070"/>
        <rdfs:subClassOf rdf:resource="http://schema.geolink.org/dev/voc/nvs/P03#B020"/>
        <rdfs:seeAlso rdf:resource="http://vocab.nerc.ac.uk/collection/P02/current/FATX/"/>
        <rdfs:comment xml:lang="en">Paramaters that quantify the numbers of fish (Osteichthyes, Agnatha and Chrondrichthyes) at a given location in any body of salt or fresh water.</rdfs:comment>
        <rdfs:label xml:lang="en">Fish abundance in water bodies</rdfs:label>
        <rdf:type rdf:resource="http://www.w3.org/2002/07/owl#NamedIndividual"/>
        <rdf:type rdf:resource="http://www.w3.org/2002/07/owl#Class"/>
      </glview:MeasurementType>
    </rdfs:subClassOf>
    <owl:someValuesFrom>
      <owl:Class>
        <owl:oneOf rdf:parseType="Collection">
          <glview:MeasurementType rdf:about="http://schema.geolink.org/dev/voc/nvs/P02#FATX"/>
        </owl:oneOf>
      </owl:Class>
    </owl:someValuesFrom>
    <owl:onProperty rdf:resource="http://schema.geolink.org/dev/view#hasMeasurementType"/>
  </owl:Restriction>
  <owl:Restriction>
    <rdfs:subClassOf>
      <glview:MeasurementType rdf:about="http://schema.geolink.org/dev/voc/nvs/P02#AASD">
        <rdfs:subClassOf rdf:resource="http://schema.geolink.org/dev/voc/nvs/P03#C050"/>
        <rdfs:subClassOf rdf:resource="http://schema.geolink.org/dev/voc/nvs/P03#G035"/>
        <rdfs:seeAlso rdf:resource="http://vocab.nerc.ac.uk/collection/P02/current/AASD/"/>
        <rdfs:comment xml:lang="en">Parameters quantifying the amount of alkenones (unsaturated aliphatic ketones) and alkenoates (carboxylic acid esters) in any unconsolidated sediment including fluff.</rdfs:comment>
        <rdfs:label xml:lang="en">Concentration of alkenones and alkenoates in sediment</rdfs:label>
        <rdf:type rdf:resource="http://www.w3.org/2002/07/owl#NamedIndividual"/>
        <rdf:type rdf:resource="http://www.w3.org/2002/07/owl#Class"/>
      </glview:MeasurementType>
    </rdfs:subClassOf>
    <owl:someValuesFrom>
      <owl:Class>
        <owl:oneOf rdf:parseType="Collection">
          <glview:MeasurementType rdf:about="http://schema.geolink.org/dev/voc/nvs/P02#AASD"/>
        </owl:oneOf>
      </owl:Class>
    </owl:someValuesFrom>
    <owl:onProperty rdf:resource="http://schema.geolink.org/dev/view#hasMeasurementType"/>
  </owl:Restriction>
  <owl:Restriction>
    <rdfs:subClassOf>
      <glview:MeasurementType rdf:about="http://schema.geolink.org/dev/voc/nvs/P02#RPOT">
        <rdfs:subClassOf rdf:resource="http://schema.geolink.org/dev/voc/nvs/P03#C045"/>
        <rdfs:subClassOf rdf:resource="http://schema.geolink.org/dev/voc/nvs/P03#G035"/>
        <rdfs:seeAlso rdf:resource="http://vocab.nerc.ac.uk/collection/P02/current/RPOT/"/>
        <rdfs:comment></rdfs:comment>
        <rdfs:label xml:lang="en">Redox potential in sediment</rdfs:label>
        <rdf:type rdf:resource="http://www.w3.org/2002/07/owl#NamedIndividual"/>
        <rdf:type rdf:resource="http://www.w3.org/2002/07/owl#Class"/>
      </glview:MeasurementType>
    </rdfs:subClassOf>
    <owl:someValuesFrom>
      <owl:Class>
        <owl:oneOf rdf:parseType="Collection">
          <glview:MeasurementType rdf:about="http://schema.geolink.org/dev/voc/nvs/P02#RPOT"/>
        </owl:oneOf>
      </owl:Class>
    </owl:someValuesFrom>
    <owl:onProperty rdf:resource="http://schema.geolink.org/dev/view#hasMeasurementType"/>
  </owl:Restriction>
  <owl:Restriction>
    <rdfs:subClassOf rdf:resource="http://schema.geolink.org/dev/voc/nvs/P02#SHTA"/>
    <owl:someValuesFrom>
      <owl:Class>
        <owl:oneOf rdf:parseType="Collection">
          <glview:MeasurementType rdf:about="http://schema.geolink.org/dev/voc/nvs/P02#SHTA"/>
        </owl:oneOf>
      </owl:Class>
    </owl:someValuesFrom>
    <owl:onProperty rdf:resource="http://schema.geolink.org/dev/view#hasMeasurementType"/>
  </owl:Restriction>
  <owl:Restriction>
    <rdfs:subClassOf>
      <glview:MeasurementType rdf:about="http://schema.geolink.org/dev/voc/nvs/P02#BNTC">
        <rdfs:subClassOf rdf:resource="http://schema.geolink.org/dev/voc/nvs/P03#B070"/>
        <rdfs:subClassOf rdf:resource="http://schema.geolink.org/dev/voc/nvs/P03#B005"/>
        <rdfs:seeAlso rdf:resource="http://vocab.nerc.ac.uk/collection/P02/current/BNTC/"/>
        <rdfs:comment xml:lang="en">Basically any bacteria carbon biomass parameters that aren't included in parameter group BATC because they cannot be mapped to specific taxa in the ITIS taxonomy.  Bacteria are defined as Kingdom Monera, which includes cyanobacteria.</rdfs:comment>
        <rdfs:label xml:lang="en">Bacteria non taxonomy-related biomass expressed as carbon per unit volume of the water column</rdfs:label>
        <rdf:type rdf:resource="http://www.w3.org/2002/07/owl#NamedIndividual"/>
        <rdf:type rdf:resource="http://www.w3.org/2002/07/owl#Class"/>
      </glview:MeasurementType>
    </rdfs:subClassOf>
    <owl:someValuesFrom>
      <owl:Class>
        <owl:oneOf rdf:parseType="Collection">
          <glview:MeasurementType rdf:about="http://schema.geolink.org/dev/voc/nvs/P02#BNTC"/>
        </owl:oneOf>
      </owl:Class>
    </owl:someValuesFrom>
    <owl:onProperty rdf:resource="http://schema.geolink.org/dev/view#hasMeasurementType"/>
  </owl:Restriction>
  <owl:Restriction>
    <rdfs:subClassOf>
      <glview:MeasurementType rdf:about="http://schema.geolink.org/dev/voc/nvs/P02#FIBM">
        <rdfs:subClassOf rdf:resource="http://schema.geolink.org/dev/voc/nvs/P03#B070"/>
        <rdfs:subClassOf rdf:resource="http://schema.geolink.org/dev/voc/nvs/P03#B020"/>
        <rdfs:subClassOf rdf:resource="http://schema.geolink.org/dev/voc/nvs/P03#H004"/>
        <rdfs:seeAlso rdf:resource="http://vocab.nerc.ac.uk/collection/P02/current/FIBM/"/>
        <rdfs:comment xml:lang="en">Parameters quantifying the mass of fish (Osteichthyes, Agnatha and Chrondrichthyes)in total or by species per unit area or per unit volume in any body of fresh or salt water expressed in any form (e.g. wet weight, dry weight, carbon, nitrogen, etc.).</rdfs:comment>
        <rdfs:label xml:lang="en">Fish biomass in water bodies</rdfs:label>
        <rdf:type rdf:resource="http://www.w3.org/2002/07/owl#NamedIndividual"/>
        <rdf:type rdf:resource="http://www.w3.org/2002/07/owl#Class"/>
      </glview:MeasurementType>
    </rdfs:subClassOf>
    <owl:someValuesFrom>
      <owl:Class>
        <owl:oneOf rdf:parseType="Collection">
          <glview:MeasurementType rdf:about="http://schema.geolink.org/dev/voc/nvs/P02#FIBM"/>
        </owl:oneOf>
      </owl:Class>
    </owl:someValuesFrom>
    <owl:onProperty rdf:resource="http://schema.geolink.org/dev/view#hasMeasurementType"/>
  </owl:Restriction>
  <owl:Restriction>
    <rdfs:subClassOf>
      <glview:MeasurementType rdf:about="http://schema.geolink.org/dev/voc/nvs/P02#IALZ">
        <rdfs:subClassOf rdf:resource="http://schema.geolink.org/dev/voc/nvs/P03#B070"/>
        <rdfs:subClassOf rdf:resource="http://schema.geolink.org/dev/voc/nvs/P03#G055"/>
        <rdfs:seeAlso rdf:resource="http://vocab.nerc.ac.uk/collection/P02/current/IALZ/"/>
        <rdfs:comment xml:lang="en">Insect (Class Insecta) and earthworm (Subclass Oligochaeta) ash-free dry weight biomass per unit area of the littoral zone (between spring tide high and low water) parameters.</rdfs:comment>
        <rdfs:label xml:lang="en">Insect and earthworm taxonomy-related ash-free dry weight biomass per unit area of the littoral zone</rdfs:label>
        <rdf:type rdf:resource="http://www.w3.org/2002/07/owl#NamedIndividual"/>
        <rdf:type rdf:resource="http://www.w3.org/2002/07/owl#Class"/>
      </glview:MeasurementType>
    </rdfs:subClassOf>
    <owl:someValuesFrom>
      <owl:Class>
        <owl:oneOf rdf:parseType="Collection">
          <glview:MeasurementType rdf:about="http://schema.geolink.org/dev/voc/nvs/P02#IALZ"/>
        </owl:oneOf>
      </owl:Class>
    </owl:someValuesFrom>
    <owl:onProperty rdf:resource="http://schema.geolink.org/dev/view#hasMeasurementType"/>
  </owl:Restriction>
  <owl:Restriction>
    <rdfs:subClassOf rdf:resource="http://schema.geolink.org/dev/voc/nvs/P02#OMWC"/>
    <owl:someValuesFrom>
      <owl:Class>
        <owl:oneOf rdf:parseType="Collection">
          <owl:NamedIndividual rdf:about="http://schema.geolink.org/dev/voc/nvs/P02#OMWC"/>
        </owl:oneOf>
      </owl:Class>
    </owl:someValuesFrom>
    <owl:onProperty rdf:resource="http://schema.geolink.org/dev/view#hasMeasurementType"/>
  </owl:Restriction>
  <owl:Restriction>
    <rdfs:subClassOf rdf:resource="http://schema.geolink.org/dev/voc/nvs/P02#SHTA"/>
    <owl:someValuesFrom>
      <owl:Class>
        <owl:oneOf rdf:parseType="Collection">
          <glview:MeasurementType rdf:about="http://schema.geolink.org/dev/voc/nvs/P02#SHTA"/>
        </owl:oneOf>
      </owl:Class>
    </owl:someValuesFrom>
    <owl:onProperty rdf:resource="http://schema.geolink.org/dev/view#hasMeasurementType"/>
  </owl:Restriction>
  <owl:Restriction>
    <rdfs:subClassOf>
      <glview:MeasurementType rdf:about="http://schema.geolink.org/dev/voc/nvs/P02#AAMN">
        <rdfs:subClassOf rdf:resource="http://schema.geolink.org/dev/voc/nvs/P03#M005"/>
        <rdfs:seeAlso rdf:resource="http://vocab.nerc.ac.uk/collection/P02/current/AAMN/"/>
        <rdfs:comment xml:lang="en">Concentrations of both organic (eg amines) and inorganic (eg ammonia and oxides of nitrogen) nitrogen species in all phases of the atmosphere</rdfs:comment>
        <rdfs:label xml:lang="en">Concentration of nitrogen species in the atmosphere</rdfs:label>
        <rdf:type rdf:resource="http://www.w3.org/2002/07/owl#NamedIndividual"/>
        <rdf:type rdf:resource="http://www.w3.org/2002/07/owl#Class"/>
      </glview:MeasurementType>
    </rdfs:subClassOf>
    <owl:someValuesFrom>
      <owl:Class>
        <owl:oneOf rdf:parseType="Collection">
          <glview:MeasurementType rdf:about="http://schema.geolink.org/dev/voc/nvs/P02#AAMN"/>
        </owl:oneOf>
      </owl:Class>
    </owl:someValuesFrom>
    <owl:onProperty rdf:resource="http://schema.geolink.org/dev/view#hasMeasurementType"/>
  </owl:Restriction>
  <owl:Restriction>
    <rdfs:subClassOf>
      <glview:MeasurementType rdf:about="http://schema.geolink.org/dev/voc/nvs/P02#HMSB">
        <rdfs:subClassOf rdf:resource="http://schema.geolink.org/dev/voc/nvs/P03#C050"/>
        <rdfs:seeAlso rdf:resource="http://vocab.nerc.ac.uk/collection/P02/current/HMSB/"/>
        <rdfs:comment xml:lang="en">Concentration (not 380nm light absorption) parameters for dissolved organic matter (includes humics, yellow matter, Gelbstoff) in the water column</rdfs:comment>
        <rdfs:label xml:lang="en">Concentration of dissolved organic matter in the water column</rdfs:label>
        <rdf:type rdf:resource="http://www.w3.org/2002/07/owl#NamedIndividual"/>
        <rdf:type rdf:resource="http://www.w3.org/2002/07/owl#Class"/>
      </glview:MeasurementType>
    </rdfs:subClassOf>
    <owl:someValuesFrom>
      <owl:Class>
        <owl:oneOf rdf:parseType="Collection">
          <glview:MeasurementType rdf:about="http://schema.geolink.org/dev/voc/nvs/P02#HMSB"/>
        </owl:oneOf>
      </owl:Class>
    </owl:someValuesFrom>
    <owl:onProperty rdf:resource="http://schema.geolink.org/dev/view#hasMeasurementType"/>
  </owl:Restriction>
  <owl:Restriction>
    <rdfs:subClassOf>
      <glview:MeasurementType rdf:about="http://schema.geolink.org/dev/voc/nvs/P02#TD00">
        <rdfs:subClassOf rdf:resource="http://schema.geolink.org/dev/voc/nvs/P03#G015"/>
        <rdfs:seeAlso rdf:resource="http://vocab.nerc.ac.uk/collection/P02/current/TD00/"/>
        <rdfs:comment xml:lang="en">Parameters quantifying and categorising terrestrially-derived detritus (eg dust and pollen) in the water column</rdfs:comment>
        <rdfs:label xml:lang="en">Terrestrial detritus in the water column suspended particulate material</rdfs:label>
        <rdf:type rdf:resource="http://www.w3.org/2002/07/owl#NamedIndividual"/>
        <rdf:type rdf:resource="http://www.w3.org/2002/07/owl#Class"/>
      </glview:MeasurementType>
    </rdfs:subClassOf>
    <owl:someValuesFrom>
      <owl:Class>
        <owl:oneOf rdf:parseType="Collection">
          <glview:MeasurementType rdf:about="http://schema.geolink.org/dev/voc/nvs/P02#TD00"/>
        </owl:oneOf>
      </owl:Class>
    </owl:someValuesFrom>
    <owl:onProperty rdf:resource="http://schema.geolink.org/dev/view#hasMeasurementType"/>
  </owl:Restriction>
  <owl:Restriction>
    <rdfs:subClassOf>
      <glview:MeasurementType rdf:about="http://schema.geolink.org/dev/voc/nvs/P02#FATM">
        <rdfs:subClassOf rdf:resource="http://schema.geolink.org/dev/voc/nvs/P03#B020"/>
        <rdfs:seeAlso rdf:resource="http://vocab.nerc.ac.uk/collection/P02/current/FATM/"/>
        <rdfs:comment xml:lang="en">Paramaters that quantify the size, shape, age and life processes (including mortality) of fish (Osteichthyes, Agnatha and Chrondrichthyes).</rdfs:comment>
        <rdfs:label xml:lang="en">Fish morphology, age and physiology</rdfs:label>
        <rdf:type rdf:resource="http://www.w3.org/2002/07/owl#NamedIndividual"/>
        <rdf:type rdf:resource="http://www.w3.org/2002/07/owl#Class"/>
      </glview:MeasurementType>
    </rdfs:subClassOf>
    <owl:someValuesFrom>
      <owl:Class>
        <owl:oneOf rdf:parseType="Collection">
          <glview:MeasurementType rdf:about="http://schema.geolink.org/dev/voc/nvs/P02#FATM"/>
        </owl:oneOf>
      </owl:Class>
    </owl:someValuesFrom>
    <owl:onProperty rdf:resource="http://schema.geolink.org/dev/view#hasMeasurementType"/>
  </owl:Restriction>
  <owl:Restriction>
    <rdfs:subClassOf rdf:resource="http://schema.geolink.org/dev/voc/nvs/P02#OHAT"/>
    <owl:someValuesFrom>
      <owl:Class>
        <owl:oneOf rdf:parseType="Collection">
          <glview:MeasurementType rdf:about="http://schema.geolink.org/dev/voc/nvs/P02#OHAT"/>
        </owl:oneOf>
      </owl:Class>
    </owl:someValuesFrom>
    <owl:onProperty rdf:resource="http://schema.geolink.org/dev/view#hasMeasurementType"/>
  </owl:Restriction>
  <owl:Restriction>
    <rdfs:subClassOf>
      <glview:MeasurementType rdf:about="http://schema.geolink.org/dev/voc/nvs/P02#MSFX">
        <rdfs:subClassOf rdf:resource="http://schema.geolink.org/dev/voc/nvs/P03#O005"/>
        <rdfs:seeAlso rdf:resource="http://vocab.nerc.ac.uk/collection/P02/current/MSFX/"/>
        <rdfs:comment xml:lang="en">Parameters expressing the total sedimentation flux in terms of particle mass, volume or counts</rdfs:comment>
        <rdfs:label xml:lang="en">Sedimentation flux quantification in the water column</rdfs:label>
        <rdf:type rdf:resource="http://www.w3.org/2002/07/owl#NamedIndividual"/>
        <rdf:type rdf:resource="http://www.w3.org/2002/07/owl#Class"/>
      </glview:MeasurementType>
    </rdfs:subClassOf>
    <owl:someValuesFrom>
      <owl:Class>
        <owl:oneOf rdf:parseType="Collection">
          <glview:MeasurementType rdf:about="http://schema.geolink.org/dev/voc/nvs/P02#MSFX"/>
        </owl:oneOf>
      </owl:Class>
    </owl:someValuesFrom>
    <owl:onProperty rdf:resource="http://schema.geolink.org/dev/view#hasMeasurementType"/>
  </owl:Restriction>
  <owl:Restriction>
    <rdfs:subClassOf rdf:resource="http://schema.geolink.org/dev/voc/nvs/P02#RPOT"/>
    <owl:someValuesFrom>
      <owl:Class>
        <owl:oneOf rdf:parseType="Collection">
          <glview:MeasurementType rdf:about="http://schema.geolink.org/dev/voc/nvs/P02#RPOT"/>
        </owl:oneOf>
      </owl:Class>
    </owl:someValuesFrom>
    <owl:onProperty rdf:resource="http://schema.geolink.org/dev/view#hasMeasurementType"/>
  </owl:Restriction>
  <owl:Restriction>
    <rdfs:subClassOf rdf:resource="http://schema.geolink.org/dev/voc/nvs/P02#AASD"/>
    <owl:someValuesFrom>
      <owl:Class>
        <owl:oneOf rdf:parseType="Collection">
          <glview:MeasurementType rdf:about="http://schema.geolink.org/dev/voc/nvs/P02#AASD"/>
        </owl:oneOf>
      </owl:Class>
    </owl:someValuesFrom>
    <owl:onProperty rdf:resource="http://schema.geolink.org/dev/view#hasMeasurementType"/>
  </owl:Restriction>
  <owl:Restriction>
    <rdfs:subClassOf>
      <glview:MeasurementType rdf:about="http://schema.geolink.org/dev/voc/nvs/P02#TRAN">
        <rdfs:subClassOf rdf:resource="http://schema.geolink.org/dev/voc/nvs/P03#H005"/>
        <rdfs:seeAlso rdf:resource="http://vocab.nerc.ac.uk/collection/P02/current/TRAN/"/>
        <rdfs:comment xml:lang="en">Parameters quantifying the level of activity moving people or cargo from one place to another.</rdfs:comment>
        <rdfs:label xml:lang="en">Transport activity</rdfs:label>
        <rdf:type rdf:resource="http://www.w3.org/2002/07/owl#NamedIndividual"/>
        <rdf:type rdf:resource="http://www.w3.org/2002/07/owl#Class"/>
      </glview:MeasurementType>
    </rdfs:subClassOf>
    <owl:someValuesFrom>
      <owl:Class>
        <owl:oneOf rdf:parseType="Collection">
          <glview:MeasurementType rdf:about="http://schema.geolink.org/dev/voc/nvs/P02#TRAN"/>
        </owl:oneOf>
      </owl:Class>
    </owl:someValuesFrom>
    <owl:onProperty rdf:resource="http://schema.geolink.org/dev/view#hasMeasurementType"/>
  </owl:Restriction>
  <owl:Restriction>
    <rdfs:subClassOf rdf:resource="http://schema.geolink.org/dev/voc/nvs/P02#IALZ"/>
    <owl:someValuesFrom>
      <owl:Class>
        <owl:oneOf rdf:parseType="Collection">
          <glview:MeasurementType rdf:about="http://schema.geolink.org/dev/voc/nvs/P02#IALZ"/>
        </owl:oneOf>
      </owl:Class>
    </owl:someValuesFrom>
    <owl:onProperty rdf:resource="http://schema.geolink.org/dev/view#hasMeasurementType"/>
  </owl:Restriction>
  <owl:Restriction>
    <rdfs:subClassOf rdf:resource="http://schema.geolink.org/dev/voc/nvs/P02#BNTC"/>
    <owl:someValuesFrom>
      <owl:Class>
        <owl:oneOf rdf:parseType="Collection">
          <glview:MeasurementType rdf:about="http://schema.geolink.org/dev/voc/nvs/P02#BNTC"/>
        </owl:oneOf>
      </owl:Class>
    </owl:someValuesFrom>
    <owl:onProperty rdf:resource="http://schema.geolink.org/dev/view#hasMeasurementType"/>
  </owl:Restriction>
  <owl:Restriction>
    <rdfs:subClassOf rdf:resource="http://schema.geolink.org/dev/voc/nvs/P02#OCAA"/>
    <owl:someValuesFrom>
      <owl:Class>
        <owl:oneOf rdf:parseType="Collection">
          <glview:MeasurementType rdf:about="http://schema.geolink.org/dev/voc/nvs/P02#OCAA"/>
        </owl:oneOf>
      </owl:Class>
    </owl:someValuesFrom>
    <owl:onProperty rdf:resource="http://schema.geolink.org/dev/view#hasMeasurementType"/>
  </owl:Restriction>
  <owl:Restriction>
    <rdfs:subClassOf>
      <glview:MeasurementType rdf:about="http://schema.geolink.org/dev/voc/nvs/P02#PHYC">
        <rdfs:subClassOf rdf:resource="http://schema.geolink.org/dev/voc/nvs/P03#B035"/>
        <rdfs:seeAlso rdf:resource="http://vocab.nerc.ac.uk/collection/P02/current/PHYC/"/>
        <rdfs:comment xml:lang="en">Concentration of phycobolin group pigments such as phycocyanin and phycoerythrin in the water column</rdfs:comment>
        <rdfs:label xml:lang="en">Phycobolin pigment concentrations in the water column</rdfs:label>
        <rdf:type rdf:resource="http://www.w3.org/2002/07/owl#NamedIndividual"/>
        <rdf:type rdf:resource="http://www.w3.org/2002/07/owl#Class"/>
      </glview:MeasurementType>
    </rdfs:subClassOf>
    <owl:someValuesFrom>
      <owl:Class>
        <owl:oneOf rdf:parseType="Collection">
          <glview:MeasurementType rdf:about="http://schema.geolink.org/dev/voc/nvs/P02#PHYC"/>
        </owl:oneOf>
      </owl:Class>
    </owl:someValuesFrom>
    <owl:onProperty rdf:resource="http://schema.geolink.org/dev/view#hasMeasurementType"/>
  </owl:Restriction>
  <owl:Restriction>
    <rdfs:subClassOf>
      <glview:MeasurementType rdf:about="http://schema.geolink.org/dev/voc/nvs/P02#FABD">
        <rdfs:subClassOf rdf:resource="http://schema.geolink.org/dev/voc/nvs/P03#B070"/>
        <rdfs:subClassOf rdf:resource="http://schema.geolink.org/dev/voc/nvs/P03#G055"/>
        <rdfs:seeAlso rdf:resource="http://vocab.nerc.ac.uk/collection/P02/current/FABD/"/>
        <rdfs:comment xml:lang="en">Any fauna (class Animalia) abundance per unit are of sea, river or lake bed.  Broad group overlapping a number of more specific groups that should be used preferentially, but this group is provided as an alternative to one-to-many mappings.</rdfs:comment>
        <rdfs:label xml:lang="en">Fauna abundance per unit area of the bed</rdfs:label>
        <rdf:type rdf:resource="http://www.w3.org/2002/07/owl#NamedIndividual"/>
        <rdf:type rdf:resource="http://www.w3.org/2002/07/owl#Class"/>
      </glview:MeasurementType>
    </rdfs:subClassOf>
    <owl:someValuesFrom>
      <owl:Class>
        <owl:oneOf rdf:parseType="Collection">
          <glview:MeasurementType rdf:about="http://schema.geolink.org/dev/voc/nvs/P02#FABD"/>
        </owl:oneOf>
      </owl:Class>
    </owl:someValuesFrom>
    <owl:onProperty rdf:resource="http://schema.geolink.org/dev/view#hasMeasurementType"/>
  </owl:Restriction>
  <owl:Restriction>
    <rdfs:subClassOf>
      <glview:MeasurementType rdf:about="http://schema.geolink.org/dev/voc/nvs/P02#MMST">
        <rdfs:subClassOf rdf:resource="http://schema.geolink.org/dev/voc/nvs/P03#H002"/>
        <rdfs:seeAlso rdf:resource="http://vocab.nerc.ac.uk/collection/P02/current/MMST/"/>
        <rdfs:comment xml:lang="en">Parameters relating to human built structures on the coast or offshore and their impact on the environment.</rdfs:comment>
        <rdfs:label xml:lang="en">Man-made structures</rdfs:label>
        <rdf:type rdf:resource="http://www.w3.org/2002/07/owl#NamedIndividual"/>
        <rdf:type rdf:resource="http://www.w3.org/2002/07/owl#Class"/>
      </glview:MeasurementType>
    </rdfs:subClassOf>
    <owl:someValuesFrom>
      <owl:Class>
        <owl:oneOf rdf:parseType="Collection">
          <glview:MeasurementType rdf:about="http://schema.geolink.org/dev/voc/nvs/P02#MMST"/>
        </owl:oneOf>
      </owl:Class>
    </owl:someValuesFrom>
    <owl:onProperty rdf:resource="http://schema.geolink.org/dev/view#hasMeasurementType"/>
  </owl:Restriction>
  <owl:Restriction>
    <rdfs:subClassOf rdf:resource="http://schema.geolink.org/dev/voc/nvs/P02#MSBO"/>
    <owl:someValuesFrom>
      <owl:Class>
        <owl:oneOf rdf:parseType="Collection">
          <glview:MeasurementType rdf:about="http://schema.geolink.org/dev/voc/nvs/P02#MSBO"/>
        </owl:oneOf>
      </owl:Class>
    </owl:someValuesFrom>
    <owl:onProperty rdf:resource="http://schema.geolink.org/dev/view#hasMeasurementType"/>
  </owl:Restriction>
  <owl:Restriction>
    <rdfs:subClassOf rdf:resource="http://schema.geolink.org/dev/voc/nvs/P02#OMWC"/>
    <owl:someValuesFrom>
      <owl:Class>
        <owl:oneOf rdf:parseType="Collection">
          <owl:NamedIndividual rdf:about="http://schema.geolink.org/dev/voc/nvs/P02#OMWC"/>
        </owl:oneOf>
      </owl:Class>
    </owl:someValuesFrom>
    <owl:onProperty rdf:resource="http://schema.geolink.org/dev/view#hasMeasurementType"/>
  </owl:Restriction>
  <owl:Restriction>
    <rdfs:subClassOf>
      <glview:MeasurementType rdf:about="http://schema.geolink.org/dev/voc/nvs/P02#AQYN">
        <rdfs:subClassOf rdf:resource="http://schema.geolink.org/dev/voc/nvs/P03#C025"/>
        <rdfs:seeAlso rdf:resource="http://vocab.nerc.ac.uk/collection/P02/current/AQYN/"/>
        <rdfs:comment xml:lang="en">Alkene and alkyne concentrations in all phases of the water column</rdfs:comment>
        <rdfs:label xml:lang="en">Concentration of alkenes and alkynes in the water column</rdfs:label>
        <rdf:type rdf:resource="http://www.w3.org/2002/07/owl#NamedIndividual"/>
        <rdf:type rdf:resource="http://www.w3.org/2002/07/owl#Class"/>
      </glview:MeasurementType>
    </rdfs:subClassOf>
    <owl:someValuesFrom>
      <owl:Class>
        <owl:oneOf rdf:parseType="Collection">
          <glview:MeasurementType rdf:about="http://schema.geolink.org/dev/voc/nvs/P02#AQYN"/>
        </owl:oneOf>
      </owl:Class>
    </owl:someValuesFrom>
    <owl:onProperty rdf:resource="http://schema.geolink.org/dev/view#hasMeasurementType"/>
  </owl:Restriction>
  <owl:Restriction>
    <rdfs:subClassOf>
      <glview:MeasurementType rdf:about="http://schema.geolink.org/dev/voc/nvs/P02#DCMX">
        <rdfs:subClassOf rdf:resource="http://schema.geolink.org/dev/voc/nvs/P03#C020"/>
        <rdfs:seeAlso rdf:resource="http://vocab.nerc.ac.uk/collection/P02/current/DCMX/"/>
        <rdfs:comment xml:lang="en">Concentrations of volatile halocarbons (compounds comprising carbon atoms covalently bonded to fluorine, chlorine, bromine or iodine atoms) other than tracers (i.e. freons/chlorofluorocarbons) and contaminants in any body of fresh or salt water.</rdfs:comment>
        <rdfs:label xml:lang="en">Other halocarbon concentrations in water bodies</rdfs:label>
        <rdf:type rdf:resource="http://www.w3.org/2002/07/owl#NamedIndividual"/>
        <rdf:type rdf:resource="http://www.w3.org/2002/07/owl#Class"/>
      </glview:MeasurementType>
    </rdfs:subClassOf>
    <owl:someValuesFrom>
      <owl:Class>
        <owl:oneOf rdf:parseType="Collection">
          <glview:MeasurementType rdf:about="http://schema.geolink.org/dev/voc/nvs/P02#DCMX"/>
        </owl:oneOf>
      </owl:Class>
    </owl:someValuesFrom>
    <owl:onProperty rdf:resource="http://schema.geolink.org/dev/view#hasMeasurementType"/>
  </owl:Restriction>
  <owl:Restriction>
    <rdfs:subClassOf>
      <glview:MeasurementType rdf:about="http://schema.geolink.org/dev/voc/nvs/P02#ACFL">
        <rdfs:subClassOf rdf:resource="http://schema.geolink.org/dev/voc/nvs/P03#Z005"/>
        <rdfs:seeAlso rdf:resource="http://vocab.nerc.ac.uk/collection/P02/current/ACFL/"/>
        <rdfs:comment></rdfs:comment>
        <rdfs:label xml:lang="en">Quality control flags</rdfs:label>
        <rdf:type rdf:resource="http://www.w3.org/2002/07/owl#NamedIndividual"/>
        <rdf:type rdf:resource="http://www.w3.org/2002/07/owl#Class"/>
      </glview:MeasurementType>
    </rdfs:subClassOf>
    <owl:someValuesFrom>
      <owl:Class>
        <owl:oneOf rdf:parseType="Collection">
          <glview:MeasurementType rdf:about="http://schema.geolink.org/dev/voc/nvs/P02#ACFL"/>
        </owl:oneOf>
      </owl:Class>
    </owl:someValuesFrom>
    <owl:onProperty rdf:resource="http://schema.geolink.org/dev/view#hasMeasurementType"/>
  </owl:Restriction>
  <owl:Restriction>
    <rdfs:subClassOf>
      <glview:MeasurementType rdf:about="http://schema.geolink.org/dev/voc/nvs/P02#SIAT">
        <rdfs:subClassOf rdf:resource="http://schema.geolink.org/dev/voc/nvs/P03#C045"/>
        <rdfs:subClassOf rdf:resource="http://schema.geolink.org/dev/voc/nvs/P03#M005"/>
        <rdfs:seeAlso rdf:resource="http://vocab.nerc.ac.uk/collection/P02/current/SIAT/"/>
        <rdfs:comment xml:lang="en">Concentration of inorganic silicon species (element or compounds) in any phase of the atmosphere</rdfs:comment>
        <rdfs:label xml:lang="en">Inorganic silicon species concentrations in the atmosphere</rdfs:label>
        <rdf:type rdf:resource="http://www.w3.org/2002/07/owl#NamedIndividual"/>
        <rdf:type rdf:resource="http://www.w3.org/2002/07/owl#Class"/>
      </glview:MeasurementType>
    </rdfs:subClassOf>
    <owl:someValuesFrom>
      <owl:Class>
        <owl:oneOf rdf:parseType="Collection">
          <glview:MeasurementType rdf:about="http://schema.geolink.org/dev/voc/nvs/P02#SIAT"/>
        </owl:oneOf>
      </owl:Class>
    </owl:someValuesFrom>
    <owl:onProperty rdf:resource="http://schema.geolink.org/dev/view#hasMeasurementType"/>
  </owl:Restriction>
  <owl:Restriction>
    <rdfs:subClassOf>
      <glview:MeasurementType rdf:about="http://schema.geolink.org/dev/voc/nvs/P02#UPTH">
        <rdfs:subClassOf rdf:resource="http://schema.geolink.org/dev/voc/nvs/P03#O010"/>
        <rdfs:subClassOf rdf:resource="http://schema.geolink.org/dev/voc/nvs/P03#B005"/>
        <rdfs:seeAlso rdf:resource="http://vocab.nerc.ac.uk/collection/P02/current/UPTH/"/>
        <rdfs:comment xml:lang="en">Parameters related to bacterial production determination by measurement of dissolved organic molecule (e.g. leucine, thymidine) uptake rates</rdfs:comment>
        <rdfs:label xml:lang="en">Bacterial production in the water column</rdfs:label>
        <rdf:type rdf:resource="http://www.w3.org/2002/07/owl#NamedIndividual"/>
        <rdf:type rdf:resource="http://www.w3.org/2002/07/owl#Class"/>
      </glview:MeasurementType>
    </rdfs:subClassOf>
    <owl:someValuesFrom>
      <owl:Class>
        <owl:oneOf rdf:parseType="Collection">
          <glview:MeasurementType rdf:about="http://schema.geolink.org/dev/voc/nvs/P02#UPTH"/>
        </owl:oneOf>
      </owl:Class>
    </owl:someValuesFrom>
    <owl:onProperty rdf:resource="http://schema.geolink.org/dev/view#hasMeasurementType"/>
  </owl:Restriction>
  <owl:Restriction>
    <rdfs:subClassOf rdf:resource="http://schema.geolink.org/dev/voc/nvs/P02#XMGS"/>
    <owl:someValuesFrom>
      <owl:Class>
        <owl:oneOf rdf:parseType="Collection">
          <glview:MeasurementType rdf:about="http://schema.geolink.org/dev/voc/nvs/P02#XMGS"/>
        </owl:oneOf>
      </owl:Class>
    </owl:someValuesFrom>
    <owl:onProperty rdf:resource="http://schema.geolink.org/dev/view#hasMeasurementType"/>
  </owl:Restriction>
  <owl:Restriction>
    <rdfs:subClassOf>
      <glview:MeasurementType rdf:about="http://schema.geolink.org/dev/voc/nvs/P02#TBGZ">
        <rdfs:subClassOf rdf:resource="http://schema.geolink.org/dev/voc/nvs/P03#O010"/>
        <rdfs:subClassOf rdf:resource="http://schema.geolink.org/dev/voc/nvs/P03#B005"/>
        <rdfs:seeAlso rdf:resource="http://vocab.nerc.ac.uk/collection/P02/current/TBGZ/"/>
        <rdfs:comment></rdfs:comment>
        <rdfs:label xml:lang="en">Bacterial consumption in the water column</rdfs:label>
        <rdf:type rdf:resource="http://www.w3.org/2002/07/owl#NamedIndividual"/>
        <rdf:type rdf:resource="http://www.w3.org/2002/07/owl#Class"/>
      </glview:MeasurementType>
    </rdfs:subClassOf>
    <owl:someValuesFrom>
      <owl:Class>
        <owl:oneOf rdf:parseType="Collection">
          <glview:MeasurementType rdf:about="http://schema.geolink.org/dev/voc/nvs/P02#TBGZ"/>
        </owl:oneOf>
      </owl:Class>
    </owl:someValuesFrom>
    <owl:onProperty rdf:resource="http://schema.geolink.org/dev/view#hasMeasurementType"/>
  </owl:Restriction>
  <owl:Restriction>
    <rdfs:subClassOf>
      <glview:MeasurementType rdf:about="http://schema.geolink.org/dev/voc/nvs/P02#COCC">
        <rdfs:subClassOf rdf:resource="http://schema.geolink.org/dev/voc/nvs/P03#C005"/>
        <rdfs:seeAlso rdf:resource="http://vocab.nerc.ac.uk/collection/P02/current/COCC/"/>
        <rdfs:comment xml:lang="en">Colloidal organic carbon per unit volume of the water column.</rdfs:comment>
        <rdfs:label xml:lang="en">Colloidal organic carbon concentration in the water column</rdfs:label>
        <rdf:type rdf:resource="http://www.w3.org/2002/07/owl#NamedIndividual"/>
        <rdf:type rdf:resource="http://www.w3.org/2002/07/owl#Class"/>
      </glview:MeasurementType>
    </rdfs:subClassOf>
    <owl:someValuesFrom>
      <owl:Class>
        <owl:oneOf rdf:parseType="Collection">
          <glview:MeasurementType rdf:about="http://schema.geolink.org/dev/voc/nvs/P02#COCC"/>
        </owl:oneOf>
      </owl:Class>
    </owl:someValuesFrom>
    <owl:onProperty rdf:resource="http://schema.geolink.org/dev/view#hasMeasurementType"/>
  </owl:Restriction>
  <owl:Restriction>
    <rdfs:subClassOf>
      <glview:MeasurementType rdf:about="http://schema.geolink.org/dev/voc/nvs/P02#PCHW">
        <rdfs:subClassOf rdf:resource="http://schema.geolink.org/dev/voc/nvs/P03#C055"/>
        <rdfs:subClassOf rdf:resource="http://schema.geolink.org/dev/voc/nvs/P03#C025"/>
        <rdfs:subClassOf rdf:resource="http://schema.geolink.org/dev/voc/nvs/P03#H001"/>
        <rdfs:seeAlso rdf:resource="http://vocab.nerc.ac.uk/collection/P02/current/PCHW/"/>
        <rdfs:comment xml:lang="en">PAH concentrations in all phases of the water column. This group includes concentrations per unit volume of the water column in the particulate phase, but not concentrations per unit wieght of SPM.</rdfs:comment>
        <rdfs:label xml:lang="en">Concentration of polycyclic aromatic hydrocarbons (PAHs) in the water column</rdfs:label>
        <rdf:type rdf:resource="http://www.w3.org/2002/07/owl#NamedIndividual"/>
        <rdf:type rdf:resource="http://www.w3.org/2002/07/owl#Class"/>
      </glview:MeasurementType>
    </rdfs:subClassOf>
    <owl:someValuesFrom>
      <owl:Class>
        <owl:oneOf rdf:parseType="Collection">
          <glview:MeasurementType rdf:about="http://schema.geolink.org/dev/voc/nvs/P02#PCHW"/>
        </owl:oneOf>
      </owl:Class>
    </owl:someValuesFrom>
    <owl:onProperty rdf:resource="http://schema.geolink.org/dev/view#hasMeasurementType"/>
  </owl:Restriction>
  <owl:Restriction>
    <rdfs:subClassOf>
      <glview:MeasurementType rdf:about="http://schema.geolink.org/dev/voc/nvs/P02#ZOOB">
        <rdfs:subClassOf rdf:resource="http://schema.geolink.org/dev/voc/nvs/P03#G055"/>
        <rdfs:seeAlso rdf:resource="http://vocab.nerc.ac.uk/collection/P02/current/ZOOB/"/>
        <rdfs:comment xml:lang="en">Zoobenthos count parameters presented at the level of taxa that may be mapped to entities in the ITIS taxonomy.  These may be at any taxonomic level from sub-species upwards. Count includes presence/absence indicators.</rdfs:comment>
        <rdfs:label xml:lang="en">Zoobenthos taxonomy-related counts</rdfs:label>
        <rdf:type rdf:resource="http://www.w3.org/2002/07/owl#NamedIndividual"/>
        <rdf:type rdf:resource="http://www.w3.org/2002/07/owl#Class"/>
      </glview:MeasurementType>
    </rdfs:subClassOf>
    <owl:someValuesFrom>
      <owl:Class>
        <owl:oneOf rdf:parseType="Collection">
          <glview:MeasurementType rdf:about="http://schema.geolink.org/dev/voc/nvs/P02#ZOOB"/>
        </owl:oneOf>
      </owl:Class>
    </owl:someValuesFrom>
    <owl:onProperty rdf:resource="http://schema.geolink.org/dev/view#hasMeasurementType"/>
  </owl:Restriction>
  <owl:Restriction>
    <rdfs:subClassOf>
      <glview:MeasurementType rdf:about="http://schema.geolink.org/dev/voc/nvs/P02#TDIN">
        <rdfs:subClassOf rdf:resource="http://schema.geolink.org/dev/voc/nvs/P03#C005"/>
        <rdfs:subClassOf rdf:resource="http://schema.geolink.org/dev/voc/nvs/P03#C040"/>
        <rdfs:seeAlso rdf:resource="http://vocab.nerc.ac.uk/collection/P02/current/TDIN/"/>
        <rdfs:comment xml:lang="en">Total concentration of all dissolved inorganic nitrogen species in the water column, usually derived by summation of individual nutrient concentrations (NO3+NO2+NH4). Some workers may also include urea.</rdfs:comment>
        <rdfs:label xml:lang="en">Dissolved inorganic nitrogen concentration in the water column</rdfs:label>
        <rdf:type rdf:resource="http://www.w3.org/2002/07/owl#NamedIndividual"/>
        <rdf:type rdf:resource="http://www.w3.org/2002/07/owl#Class"/>
      </glview:MeasurementType>
    </rdfs:subClassOf>
    <owl:someValuesFrom>
      <owl:Class>
        <owl:oneOf rdf:parseType="Collection">
          <glview:MeasurementType rdf:about="http://schema.geolink.org/dev/voc/nvs/P02#TDIN"/>
        </owl:oneOf>
      </owl:Class>
    </owl:someValuesFrom>
    <owl:onProperty rdf:resource="http://schema.geolink.org/dev/view#hasMeasurementType"/>
  </owl:Restriction>
  <owl:Restriction>
    <rdfs:subClassOf rdf:resource="http://schema.geolink.org/dev/voc/nvs/P02#GP079"/>
    <owl:someValuesFrom>
      <owl:Class>
        <owl:oneOf rdf:parseType="Collection">
          <glview:MeasurementType rdf:about="http://schema.geolink.org/dev/voc/nvs/P02#GP079"/>
        </owl:oneOf>
      </owl:Class>
    </owl:someValuesFrom>
    <owl:onProperty rdf:resource="http://schema.geolink.org/dev/view#hasMeasurementType"/>
  </owl:Restriction>
  <owl:Restriction>
    <rdfs:subClassOf>
      <glview:MeasurementType rdf:about="http://schema.geolink.org/dev/voc/nvs/P02#PNFX">
        <rdfs:subClassOf rdf:resource="http://schema.geolink.org/dev/voc/nvs/P03#B027"/>
        <rdfs:subClassOf rdf:resource="http://schema.geolink.org/dev/voc/nvs/P03#O005"/>
        <rdfs:seeAlso rdf:resource="http://vocab.nerc.ac.uk/collection/P02/current/PNFX/"/>
        <rdfs:comment xml:lang="en">Fluxes expressed as number per unit area per unit time of any biota or remains thereof (excluding faecal pellets which are classed as SPM) downwards through the water column</rdfs:comment>
        <rdfs:label xml:lang="en">Sedimentation flux of identified biota in the water column</rdfs:label>
        <rdf:type rdf:resource="http://www.w3.org/2002/07/owl#NamedIndividual"/>
        <rdf:type rdf:resource="http://www.w3.org/2002/07/owl#Class"/>
      </glview:MeasurementType>
    </rdfs:subClassOf>
    <owl:someValuesFrom>
      <owl:Class>
        <owl:oneOf rdf:parseType="Collection">
          <glview:MeasurementType rdf:about="http://schema.geolink.org/dev/voc/nvs/P02#PNFX"/>
        </owl:oneOf>
      </owl:Class>
    </owl:someValuesFrom>
    <owl:onProperty rdf:resource="http://schema.geolink.org/dev/view#hasMeasurementType"/>
  </owl:Restriction>
  <owl:Restriction>
    <rdfs:subClassOf>
      <glview:MeasurementType rdf:about="http://schema.geolink.org/dev/voc/nvs/P02#RMAJ">
        <rdfs:subClassOf rdf:resource="http://schema.geolink.org/dev/voc/nvs/P02#RMIN"/>
        <rdfs:seeAlso rdf:resource="http://vocab.nerc.ac.uk/collection/P02/current/RMAJ/"/>
        <rdfs:comment xml:lang="en">Concentrations of the elements classically regarded as major (&gt;1% by weight as oxide: namely: Si, Ti, Al, Fe3+, Fe2+, Mg, Mn, Ca, Na, and K) plus affiliated parameters such as H2O- (adsorbed water) and H2O+ (or loss on ignition) in rocks or sediments.</rdfs:comment>
        <rdfs:label xml:lang="en">Geological sample major element chemistry</rdfs:label>
        <rdf:type rdf:resource="http://www.w3.org/2002/07/owl#NamedIndividual"/>
        <rdf:type rdf:resource="http://www.w3.org/2002/07/owl#Class"/>
      </glview:MeasurementType>
    </rdfs:subClassOf>
    <owl:someValuesFrom>
      <owl:Class>
        <owl:oneOf rdf:parseType="Collection">
          <glview:MeasurementType rdf:about="http://schema.geolink.org/dev/voc/nvs/P02#RMAJ"/>
        </owl:oneOf>
      </owl:Class>
    </owl:someValuesFrom>
    <owl:onProperty rdf:resource="http://schema.geolink.org/dev/view#hasMeasurementType"/>
  </owl:Restriction>
  <owl:Restriction>
    <rdfs:subClassOf>
      <glview:MeasurementType rdf:about="http://schema.geolink.org/dev/voc/nvs/P02#CNTX">
        <rdfs:subClassOf rdf:resource="http://schema.geolink.org/dev/voc/nvs/P03#B030"/>
        <rdfs:subClassOf rdf:resource="http://schema.geolink.org/dev/voc/nvs/P03#B070"/>
        <rdfs:seeAlso rdf:resource="http://vocab.nerc.ac.uk/collection/P02/current/CNTX/"/>
        <rdfs:comment xml:lang="en">Any parameterisation of biomass (e.g. wet weight, dry weight, carbon, nitrogen etc.) of free-floating autotrophic biological entities designated by terms other than taxonomic names (e.g. microphytoplankton, ciliate, flagellate) in any body of fresh or salt water.</rdfs:comment>
        <rdfs:label xml:lang="en">Phytoplankton generic biomass in water bodies</rdfs:label>
        <rdf:type rdf:resource="http://www.w3.org/2002/07/owl#NamedIndividual"/>
        <rdf:type rdf:resource="http://www.w3.org/2002/07/owl#Class"/>
      </glview:MeasurementType>
    </rdfs:subClassOf>
    <owl:someValuesFrom>
      <owl:Class>
        <owl:oneOf rdf:parseType="Collection">
          <glview:MeasurementType rdf:about="http://schema.geolink.org/dev/voc/nvs/P02#CNTX"/>
        </owl:oneOf>
      </owl:Class>
    </owl:someValuesFrom>
    <owl:onProperty rdf:resource="http://schema.geolink.org/dev/view#hasMeasurementType"/>
  </owl:Restriction>
  <owl:Restriction>
    <rdfs:subClassOf rdf:resource="http://schema.geolink.org/dev/voc/nvs/P02#CBSD"/>
    <owl:someValuesFrom>
      <owl:Class>
        <owl:oneOf rdf:parseType="Collection">
          <glview:MeasurementType rdf:about="http://schema.geolink.org/dev/voc/nvs/P02#CBSD"/>
        </owl:oneOf>
      </owl:Class>
    </owl:someValuesFrom>
    <owl:onProperty rdf:resource="http://schema.geolink.org/dev/view#hasMeasurementType"/>
  </owl:Restriction>
  <owl:Restriction>
    <rdfs:subClassOf>
      <glview:MeasurementType rdf:about="http://schema.geolink.org/dev/voc/nvs/P02#IWDX">
        <rdfs:subClassOf rdf:resource="http://schema.geolink.org/dev/voc/nvs/P03#B070"/>
        <rdfs:subClassOf rdf:resource="http://schema.geolink.org/dev/voc/nvs/P03#G055"/>
        <rdfs:seeAlso rdf:resource="http://vocab.nerc.ac.uk/collection/P02/current/IWDX/"/>
        <rdfs:comment xml:lang="en">Insect (Class Insecta) and earthworm (Subclass Oligochaeta) ash-free dry weight biomass per unit area of bed (sea, river, lake etc.) parameters presented at the level of taxa that may be mapped to entities in the ITIS taxonomy.  Includes animals normally considered as planktonic if they have been returned from sediment samples. This parameter group has been implemented to separate predominantly freshwater taxa from predominantly marine taxa.</rdfs:comment>
        <rdfs:label xml:lang="en">Insect and earthworm taxonomy-related ash-free dry weight biomass per unit area of the bed</rdfs:label>
        <rdf:type rdf:resource="http://www.w3.org/2002/07/owl#NamedIndividual"/>
        <rdf:type rdf:resource="http://www.w3.org/2002/07/owl#Class"/>
      </glview:MeasurementType>
    </rdfs:subClassOf>
    <owl:someValuesFrom>
      <owl:Class>
        <owl:oneOf rdf:parseType="Collection">
          <glview:MeasurementType rdf:about="http://schema.geolink.org/dev/voc/nvs/P02#IWDX"/>
        </owl:oneOf>
      </owl:Class>
    </owl:someValuesFrom>
    <owl:onProperty rdf:resource="http://schema.geolink.org/dev/view#hasMeasurementType"/>
  </owl:Restriction>
  <owl:Restriction>
    <rdfs:subClassOf>
      <glview:MeasurementType rdf:about="http://schema.geolink.org/dev/voc/nvs/P02#MBAN">
        <rdfs:subClassOf rdf:resource="http://schema.geolink.org/dev/view#Measurement"/>
        <rdfs:seeAlso rdf:resource="http://vocab.nerc.ac.uk/collection/P02/current/MBAN/"/>
        <rdfs:comment xml:lang="en">Depth of the water column or elevation of land surface relative to sea surface, geoid or other datum</rdfs:comment>
        <rdfs:label xml:lang="en">Bathymetry and Elevation</rdfs:label>
        <rdf:type rdf:resource="http://www.w3.org/2002/07/owl#NamedIndividual"/>
        <rdf:type rdf:resource="http://www.w3.org/2002/07/owl#Class"/>
      </glview:MeasurementType>
    </rdfs:subClassOf>
    <owl:someValuesFrom>
      <owl:Class>
        <owl:oneOf rdf:parseType="Collection">
          <glview:MeasurementType rdf:about="http://schema.geolink.org/dev/voc/nvs/P02#MBAN"/>
        </owl:oneOf>
      </owl:Class>
    </owl:someValuesFrom>
    <owl:onProperty rdf:resource="http://schema.geolink.org/dev/view#hasMeasurementType"/>
  </owl:Restriction>
  <owl:Restriction>
    <rdfs:subClassOf>
      <glview:MeasurementType rdf:about="http://schema.geolink.org/dev/voc/nvs/P02#ATDP">
        <rdfs:subClassOf rdf:resource="http://schema.geolink.org/dev/voc/nvs/P03#M005"/>
        <rdfs:subClassOf rdf:resource="http://schema.geolink.org/dev/voc/nvs/P03#O005"/>
        <rdfs:seeAlso rdf:resource="http://vocab.nerc.ac.uk/collection/P02/current/ATDP/"/>
        <rdfs:comment xml:lang="en">Fluxes of chemical species from the atmosphere to sea or land surface including precipitation and aerosol deposition but excluding fluxes due to exchange of gases</rdfs:comment>
        <rdfs:label xml:lang="en">Atmospheric deposition rates</rdfs:label>
        <rdf:type rdf:resource="http://www.w3.org/2002/07/owl#NamedIndividual"/>
        <rdf:type rdf:resource="http://www.w3.org/2002/07/owl#Class"/>
      </glview:MeasurementType>
    </rdfs:subClassOf>
    <owl:someValuesFrom>
      <owl:Class>
        <owl:oneOf rdf:parseType="Collection">
          <glview:MeasurementType rdf:about="http://schema.geolink.org/dev/voc/nvs/P02#ATDP"/>
        </owl:oneOf>
      </owl:Class>
    </owl:someValuesFrom>
    <owl:onProperty rdf:resource="http://schema.geolink.org/dev/view#hasMeasurementType"/>
  </owl:Restriction>
  <owl:Restriction>
    <rdfs:subClassOf>
      <glview:MeasurementType rdf:about="http://schema.geolink.org/dev/voc/nvs/P02#WVST">
        <rdfs:subClassOf rdf:resource="http://schema.geolink.org/dev/voc/nvs/P03#D034"/>
        <rdfs:seeAlso rdf:resource="http://vocab.nerc.ac.uk/collection/P02/current/WVST/"/>
        <rdfs:comment xml:lang="en">Statistical parameters derived from wave records to express wave height and period.</rdfs:comment>
        <rdfs:label xml:lang="en">Wave height and period statistics</rdfs:label>
        <rdf:type rdf:resource="http://www.w3.org/2002/07/owl#NamedIndividual"/>
        <rdf:type rdf:resource="http://www.w3.org/2002/07/owl#Class"/>
      </glview:MeasurementType>
    </rdfs:subClassOf>
    <owl:someValuesFrom>
      <owl:Class>
        <owl:oneOf rdf:parseType="Collection">
          <glview:MeasurementType rdf:about="http://schema.geolink.org/dev/voc/nvs/P02#WVST"/>
        </owl:oneOf>
      </owl:Class>
    </owl:someValuesFrom>
    <owl:onProperty rdf:resource="http://schema.geolink.org/dev/view#hasMeasurementType"/>
  </owl:Restriction>
  <owl:Restriction>
    <rdfs:subClassOf rdf:resource="http://schema.geolink.org/dev/voc/nvs/P02#UPTH"/>
    <owl:someValuesFrom>
      <owl:Class>
        <owl:oneOf rdf:parseType="Collection">
          <glview:MeasurementType rdf:about="http://schema.geolink.org/dev/voc/nvs/P02#UPTH"/>
        </owl:oneOf>
      </owl:Class>
    </owl:someValuesFrom>
    <owl:onProperty rdf:resource="http://schema.geolink.org/dev/view#hasMeasurementType"/>
  </owl:Restriction>
  <owl:Restriction>
    <rdfs:subClassOf rdf:resource="http://schema.geolink.org/dev/voc/nvs/P02#PCHW"/>
    <owl:someValuesFrom>
      <owl:Class>
        <owl:oneOf rdf:parseType="Collection">
          <glview:MeasurementType rdf:about="http://schema.geolink.org/dev/voc/nvs/P02#PCHW"/>
        </owl:oneOf>
      </owl:Class>
    </owl:someValuesFrom>
    <owl:onProperty rdf:resource="http://schema.geolink.org/dev/view#hasMeasurementType"/>
  </owl:Restriction>
  <owl:Restriction>
    <rdfs:subClassOf>
      <glview:MeasurementType rdf:about="http://schema.geolink.org/dev/voc/nvs/P02#NUTV">
        <rdfs:subClassOf rdf:resource="http://schema.geolink.org/dev/voc/nvs/P03#C040"/>
        <rdfs:seeAlso rdf:resource="http://vocab.nerc.ac.uk/collection/P02/current/NUTV/"/>
        <rdfs:comment xml:lang="en">Direct output parameters from spectophotometric or chemical in-situ nutrient analysers</rdfs:comment>
        <rdfs:label xml:lang="en">Raw in-situ nutrient analyser output</rdfs:label>
        <rdf:type rdf:resource="http://www.w3.org/2002/07/owl#NamedIndividual"/>
        <rdf:type rdf:resource="http://www.w3.org/2002/07/owl#Class"/>
      </glview:MeasurementType>
    </rdfs:subClassOf>
    <owl:someValuesFrom>
      <owl:Class>
        <owl:oneOf rdf:parseType="Collection">
          <glview:MeasurementType rdf:about="http://schema.geolink.org/dev/voc/nvs/P02#NUTV"/>
        </owl:oneOf>
      </owl:Class>
    </owl:someValuesFrom>
    <owl:onProperty rdf:resource="http://schema.geolink.org/dev/view#hasMeasurementType"/>
  </owl:Restriction>
  <owl:Restriction>
    <rdfs:subClassOf>
      <glview:MeasurementType rdf:about="http://schema.geolink.org/dev/voc/nvs/P02#XRFC">
        <rdfs:subClassOf rdf:resource="http://schema.geolink.org/dev/voc/nvs/P02#RMIN"/>
        <rdfs:seeAlso rdf:resource="http://vocab.nerc.ac.uk/collection/P02/current/XRFC/"/>
        <rdfs:comment></rdfs:comment>
        <rdfs:label xml:lang="en">Raw X-Ray fluorometer (XRF) output from sediment samples</rdfs:label>
        <rdf:type rdf:resource="http://www.w3.org/2002/07/owl#NamedIndividual"/>
        <rdf:type rdf:resource="http://www.w3.org/2002/07/owl#Class"/>
      </glview:MeasurementType>
    </rdfs:subClassOf>
    <owl:someValuesFrom>
      <owl:Class>
        <owl:oneOf rdf:parseType="Collection">
          <glview:MeasurementType rdf:about="http://schema.geolink.org/dev/voc/nvs/P02#XRFC"/>
        </owl:oneOf>
      </owl:Class>
    </owl:someValuesFrom>
    <owl:onProperty rdf:resource="http://schema.geolink.org/dev/view#hasMeasurementType"/>
  </owl:Restriction>
  <owl:Restriction>
    <rdfs:subClassOf rdf:resource="http://schema.geolink.org/dev/voc/nvs/P02#ACSR"/>
    <owl:someValuesFrom>
      <owl:Class>
        <owl:oneOf rdf:parseType="Collection">
          <glview:MeasurementType rdf:about="http://schema.geolink.org/dev/voc/nvs/P02#ACSR"/>
        </owl:oneOf>
      </owl:Class>
    </owl:someValuesFrom>
    <owl:onProperty rdf:resource="http://schema.geolink.org/dev/view#hasMeasurementType"/>
  </owl:Restriction>
  <owl:Restriction>
    <rdfs:subClassOf rdf:resource="http://schema.geolink.org/dev/voc/nvs/P02#PCHW"/>
    <owl:someValuesFrom>
      <owl:Class>
        <owl:oneOf rdf:parseType="Collection">
          <glview:MeasurementType rdf:about="http://schema.geolink.org/dev/voc/nvs/P02#PCHW"/>
        </owl:oneOf>
      </owl:Class>
    </owl:someValuesFrom>
    <owl:onProperty rdf:resource="http://schema.geolink.org/dev/view#hasMeasurementType"/>
  </owl:Restriction>
  <owl:Restriction>
    <rdfs:subClassOf>
      <glview:MeasurementType rdf:about="http://schema.geolink.org/dev/voc/nvs/P02#TEMP">
        <rdfs:subClassOf rdf:resource="http://schema.geolink.org/dev/voc/nvs/P03#D025"/>
        <rdfs:seeAlso rdf:resource="http://vocab.nerc.ac.uk/collection/P02/current/TEMP/"/>
        <rdfs:comment xml:lang="en">Temperature parameters in any body of water at any point between the bed and the atmosphere excluding the top few microns sampled by radiometers known as the skin</rdfs:comment>
        <rdfs:label xml:lang="en">Temperature of the water column</rdfs:label>
        <rdf:type rdf:resource="http://www.w3.org/2002/07/owl#NamedIndividual"/>
        <rdf:type rdf:resource="http://www.w3.org/2002/07/owl#Class"/>
      </glview:MeasurementType>
    </rdfs:subClassOf>
    <owl:someValuesFrom>
      <owl:Class>
        <owl:oneOf rdf:parseType="Collection">
          <glview:MeasurementType rdf:about="http://schema.geolink.org/dev/voc/nvs/P02#TEMP"/>
        </owl:oneOf>
      </owl:Class>
    </owl:someValuesFrom>
    <owl:onProperty rdf:resource="http://schema.geolink.org/dev/view#hasMeasurementType"/>
  </owl:Restriction>
  <owl:Restriction>
    <rdfs:subClassOf>
      <glview:MeasurementType rdf:about="http://schema.geolink.org/dev/voc/nvs/P02#IDIS">
        <rdfs:subClassOf rdf:resource="http://schema.geolink.org/dev/voc/nvs/P03#H001"/>
        <rdfs:seeAlso rdf:resource="http://vocab.nerc.ac.uk/collection/P02/current/IDIS/"/>
        <rdfs:comment xml:lang="en">Parameters that quantify and specify material output into the environment as a result of industrial activity</rdfs:comment>
        <rdfs:label xml:lang="en">Industrial discharges</rdfs:label>
        <rdf:type rdf:resource="http://www.w3.org/2002/07/owl#NamedIndividual"/>
        <rdf:type rdf:resource="http://www.w3.org/2002/07/owl#Class"/>
      </glview:MeasurementType>
    </rdfs:subClassOf>
    <owl:someValuesFrom>
      <owl:Class>
        <owl:oneOf rdf:parseType="Collection">
          <glview:MeasurementType rdf:about="http://schema.geolink.org/dev/voc/nvs/P02#IDIS"/>
        </owl:oneOf>
      </owl:Class>
    </owl:someValuesFrom>
    <owl:onProperty rdf:resource="http://schema.geolink.org/dev/view#hasMeasurementType"/>
  </owl:Restriction>
  <owl:Restriction>
    <rdfs:subClassOf rdf:resource="http://schema.geolink.org/dev/voc/nvs/P02#ATDP"/>
    <owl:someValuesFrom>
      <owl:Class>
        <owl:oneOf rdf:parseType="Collection">
          <glview:MeasurementType rdf:about="http://schema.geolink.org/dev/voc/nvs/P02#ATDP"/>
        </owl:oneOf>
      </owl:Class>
    </owl:someValuesFrom>
    <owl:onProperty rdf:resource="http://schema.geolink.org/dev/view#hasMeasurementType"/>
  </owl:Restriction>
  <owl:Restriction>
    <rdfs:subClassOf rdf:resource="http://schema.geolink.org/dev/voc/nvs/P02#PNFX"/>
    <owl:someValuesFrom>
      <owl:Class>
        <owl:oneOf rdf:parseType="Collection">
          <glview:MeasurementType rdf:about="http://schema.geolink.org/dev/voc/nvs/P02#PNFX"/>
        </owl:oneOf>
      </owl:Class>
    </owl:someValuesFrom>
    <owl:onProperty rdf:resource="http://schema.geolink.org/dev/view#hasMeasurementType"/>
  </owl:Restriction>
  <owl:Restriction>
    <rdfs:subClassOf rdf:resource="http://schema.geolink.org/dev/voc/nvs/P02#RBSC"/>
    <owl:someValuesFrom>
      <owl:Class>
        <owl:oneOf rdf:parseType="Collection">
          <owl:NamedIndividual rdf:about="http://schema.geolink.org/dev/voc/nvs/P02#RBSC"/>
        </owl:oneOf>
      </owl:Class>
    </owl:someValuesFrom>
    <owl:onProperty rdf:resource="http://schema.geolink.org/dev/view#hasMeasurementType"/>
  </owl:Restriction>
  <owl:Restriction>
    <rdfs:subClassOf rdf:resource="http://schema.geolink.org/dev/voc/nvs/P02#CPSD"/>
    <owl:someValuesFrom>
      <owl:Class>
        <owl:oneOf rdf:parseType="Collection">
          <glview:MeasurementType rdf:about="http://schema.geolink.org/dev/voc/nvs/P02#CPSD"/>
        </owl:oneOf>
      </owl:Class>
    </owl:someValuesFrom>
    <owl:onProperty rdf:resource="http://schema.geolink.org/dev/view#hasMeasurementType"/>
  </owl:Restriction>
  <owl:Restriction>
    <rdfs:subClassOf>
      <glview:MeasurementType rdf:about="http://schema.geolink.org/dev/voc/nvs/P02#SCAH">
        <rdfs:comment xml:lang="en">PAH concentrations in sediment, which is considered to be anything from the bed sampled by a grab or corer, including 'fluff'</rdfs:comment>
        <rdfs:subClassOf rdf:resource="http://schema.geolink.org/dev/voc/nvs/P03#C025"/>
        <rdfs:subClassOf rdf:resource="http://schema.geolink.org/dev/voc/nvs/P03#G035"/>
        <rdfs:subClassOf rdf:resource="http://schema.geolink.org/dev/voc/nvs/P03#C055"/>
        <rdf:type rdf:resource="http://www.w3.org/2002/07/owl#Class"/>
        <rdfs:subClassOf rdf:resource="http://schema.geolink.org/dev/voc/nvs/P03#H001"/>
        <rdfs:seeAlso rdf:resource="http://vocab.nerc.ac.uk/collection/P02/current/SCAH/"/>
        <rdf:type rdf:resource="http://www.w3.org/2002/07/owl#NamedIndividual"/>
        <rdfs:label xml:lang="en">Concentration of polycyclic aromatic hydrocarbons (PAHs) in sediment samples</rdfs:label>
      </glview:MeasurementType>
    </rdfs:subClassOf>
    <owl:someValuesFrom>
      <owl:Class>
        <owl:oneOf rdf:parseType="Collection">
          <glview:MeasurementType rdf:about="http://schema.geolink.org/dev/voc/nvs/P02#SCAH"/>
        </owl:oneOf>
      </owl:Class>
    </owl:someValuesFrom>
    <owl:onProperty rdf:resource="http://schema.geolink.org/dev/view#hasMeasurementType"/>
  </owl:Restriction>
  <owl:Restriction>
    <rdfs:subClassOf>
      <glview:MeasurementType rdf:about="http://schema.geolink.org/dev/voc/nvs/P02#WSTB">
        <rdfs:subClassOf rdf:resource="http://schema.geolink.org/dev/voc/nvs/P03#C030"/>
        <rdfs:seeAlso rdf:resource="http://vocab.nerc.ac.uk/collection/P02/current/WSTB/"/>
        <rdfs:comment xml:lang="en">Stable isotope enrichment parameters in both the dissolved and particulate phases of the water column</rdfs:comment>
        <rdfs:label xml:lang="en">Stable isotope enrichment in the water column</rdfs:label>
        <rdf:type rdf:resource="http://www.w3.org/2002/07/owl#NamedIndividual"/>
        <rdf:type rdf:resource="http://www.w3.org/2002/07/owl#Class"/>
      </glview:MeasurementType>
    </rdfs:subClassOf>
    <owl:someValuesFrom>
      <owl:Class>
        <owl:oneOf rdf:parseType="Collection">
          <glview:MeasurementType rdf:about="http://schema.geolink.org/dev/voc/nvs/P02#WSTB"/>
        </owl:oneOf>
      </owl:Class>
    </owl:someValuesFrom>
    <owl:onProperty rdf:resource="http://schema.geolink.org/dev/view#hasMeasurementType"/>
  </owl:Restriction>
  <owl:Restriction>
    <rdfs:subClassOf>
      <glview:MeasurementType rdf:about="http://schema.geolink.org/dev/voc/nvs/P02#CEMP">
        <rdfs:subClassOf rdf:resource="http://schema.geolink.org/dev/voc/nvs/P03#B015"/>
        <rdfs:seeAlso rdf:resource="http://vocab.nerc.ac.uk/collection/P02/current/CEMP/"/>
        <rdfs:comment xml:lang="en">Parameters describing the size, shape or physiological activity including disease and parasite infection status of cetaceans (Order Cetacea). Includes both parameters mapped to taxa and those mapped to non-taxonomic groupings.</rdfs:comment>
        <rdfs:label xml:lang="en">Cetacean morphology and physiology</rdfs:label>
        <rdf:type rdf:resource="http://www.w3.org/2002/07/owl#NamedIndividual"/>
        <rdf:type rdf:resource="http://www.w3.org/2002/07/owl#Class"/>
      </glview:MeasurementType>
    </rdfs:subClassOf>
    <owl:someValuesFrom>
      <owl:Class>
        <owl:oneOf rdf:parseType="Collection">
          <glview:MeasurementType rdf:about="http://schema.geolink.org/dev/voc/nvs/P02#CEMP"/>
        </owl:oneOf>
      </owl:Class>
    </owl:someValuesFrom>
    <owl:onProperty rdf:resource="http://schema.geolink.org/dev/view#hasMeasurementType"/>
  </owl:Restriction>
  <owl:Restriction>
    <rdfs:subClassOf rdf:resource="http://schema.geolink.org/dev/voc/nvs/P02#TBGZ"/>
    <owl:someValuesFrom>
      <owl:Class>
        <owl:oneOf rdf:parseType="Collection">
          <glview:MeasurementType rdf:about="http://schema.geolink.org/dev/voc/nvs/P02#TBGZ"/>
        </owl:oneOf>
      </owl:Class>
    </owl:someValuesFrom>
    <owl:onProperty rdf:resource="http://schema.geolink.org/dev/view#hasMeasurementType"/>
  </owl:Restriction>
  <owl:Restriction>
    <rdfs:subClassOf rdf:resource="http://schema.geolink.org/dev/voc/nvs/P02#PHOS"/>
    <owl:someValuesFrom>
      <owl:Class>
        <owl:oneOf rdf:parseType="Collection">
          <glview:MeasurementType rdf:about="http://schema.geolink.org/dev/voc/nvs/P02#PHOS"/>
        </owl:oneOf>
      </owl:Class>
    </owl:someValuesFrom>
    <owl:onProperty rdf:resource="http://schema.geolink.org/dev/view#hasMeasurementType"/>
  </owl:Restriction>
  <owl:Restriction>
    <rdfs:subClassOf>
      <glview:MeasurementType rdf:about="http://schema.geolink.org/dev/voc/nvs/P02#SPCB">
        <rdfs:subClassOf rdf:resource="http://schema.geolink.org/dev/voc/nvs/P03#C055"/>
        <rdfs:subClassOf rdf:resource="http://schema.geolink.org/dev/voc/nvs/P03#H001"/>
        <rdfs:subClassOf rdf:resource="http://schema.geolink.org/dev/voc/nvs/P03#G035"/>
        <rdfs:seeAlso rdf:resource="http://vocab.nerc.ac.uk/collection/P02/current/SPCB/"/>
        <rdfs:comment xml:lang="en">PCB concentrations in sediment, which is considered to be anything from the bed sampled by a grab or corer, including 'fluff'</rdfs:comment>
        <rdfs:label xml:lang="en">Concentration of polychlorobiphenyls (PCBs) in sediment samples</rdfs:label>
        <rdf:type rdf:resource="http://www.w3.org/2002/07/owl#NamedIndividual"/>
        <rdf:type rdf:resource="http://www.w3.org/2002/07/owl#Class"/>
      </glview:MeasurementType>
    </rdfs:subClassOf>
    <owl:someValuesFrom>
      <owl:Class>
        <owl:oneOf rdf:parseType="Collection">
          <glview:MeasurementType rdf:about="http://schema.geolink.org/dev/voc/nvs/P02#SPCB"/>
        </owl:oneOf>
      </owl:Class>
    </owl:someValuesFrom>
    <owl:onProperty rdf:resource="http://schema.geolink.org/dev/view#hasMeasurementType"/>
  </owl:Restriction>
  <owl:Restriction>
    <rdfs:subClassOf rdf:resource="http://schema.geolink.org/dev/voc/nvs/P02#IWDX"/>
    <owl:someValuesFrom>
      <owl:Class>
        <owl:oneOf rdf:parseType="Collection">
          <glview:MeasurementType rdf:about="http://schema.geolink.org/dev/voc/nvs/P02#IWDX"/>
        </owl:oneOf>
      </owl:Class>
    </owl:someValuesFrom>
    <owl:onProperty rdf:resource="http://schema.geolink.org/dev/view#hasMeasurementType"/>
  </owl:Restriction>
  <owl:Restriction>
    <rdfs:subClassOf>
      <glview:MeasurementType rdf:about="http://schema.geolink.org/dev/voc/nvs/P02#PPRD">
        <rdfs:subClassOf rdf:resource="http://schema.geolink.org/dev/voc/nvs/P03#O010"/>
        <rdfs:seeAlso rdf:resource="http://vocab.nerc.ac.uk/collection/P02/current/PPRD/"/>
        <rdfs:comment xml:lang="en">Parameters associated with the quantification of primary production.  This is defined as the fixation of carbon dioxide into either organic or inorganic carbon by living entities and so includes photosynthesis and calcification.</rdfs:comment>
        <rdfs:label xml:lang="en">Primary production in the water column</rdfs:label>
        <rdf:type rdf:resource="http://www.w3.org/2002/07/owl#NamedIndividual"/>
        <rdf:type rdf:resource="http://www.w3.org/2002/07/owl#Class"/>
      </glview:MeasurementType>
    </rdfs:subClassOf>
    <owl:someValuesFrom>
      <owl:Class>
        <owl:oneOf rdf:parseType="Collection">
          <glview:MeasurementType rdf:about="http://schema.geolink.org/dev/voc/nvs/P02#PPRD"/>
        </owl:oneOf>
      </owl:Class>
    </owl:someValuesFrom>
    <owl:onProperty rdf:resource="http://schema.geolink.org/dev/view#hasMeasurementType"/>
  </owl:Restriction>
  <owl:Restriction>
    <rdfs:subClassOf>
      <glview:MeasurementType rdf:about="http://schema.geolink.org/dev/voc/nvs/P02#SUAT">
        <rdfs:subClassOf rdf:resource="http://schema.geolink.org/dev/voc/nvs/P03#C045"/>
        <rdfs:subClassOf rdf:resource="http://schema.geolink.org/dev/voc/nvs/P03#M005"/>
        <rdfs:seeAlso rdf:resource="http://vocab.nerc.ac.uk/collection/P02/current/SUAT/"/>
        <rdfs:comment xml:lang="en">Concentration of sulphur species (element or compounds) in any phase of the atmosphere. Includes sulphur dioxide.</rdfs:comment>
        <rdfs:label xml:lang="en">Sulphur species concentrations in the atmosphere</rdfs:label>
        <rdf:type rdf:resource="http://www.w3.org/2002/07/owl#NamedIndividual"/>
        <rdf:type rdf:resource="http://www.w3.org/2002/07/owl#Class"/>
      </glview:MeasurementType>
    </rdfs:subClassOf>
    <owl:someValuesFrom>
      <owl:Class>
        <owl:oneOf rdf:parseType="Collection">
          <glview:MeasurementType rdf:about="http://schema.geolink.org/dev/voc/nvs/P02#SUAT"/>
        </owl:oneOf>
      </owl:Class>
    </owl:someValuesFrom>
    <owl:onProperty rdf:resource="http://schema.geolink.org/dev/view#hasMeasurementType"/>
  </owl:Restriction>
  <owl:Restriction>
    <rdfs:subClassOf rdf:resource="http://schema.geolink.org/dev/voc/nvs/P02#PHSD"/>
    <owl:someValuesFrom>
      <owl:Class>
        <owl:oneOf rdf:parseType="Collection">
          <glview:MeasurementType rdf:about="http://schema.geolink.org/dev/voc/nvs/P02#PHSD"/>
        </owl:oneOf>
      </owl:Class>
    </owl:someValuesFrom>
    <owl:onProperty rdf:resource="http://schema.geolink.org/dev/view#hasMeasurementType"/>
  </owl:Restriction>
  <owl:Restriction>
    <rdfs:subClassOf rdf:resource="http://schema.geolink.org/dev/voc/nvs/P02#SRFL"/>
    <owl:someValuesFrom>
      <owl:Class>
        <owl:oneOf rdf:parseType="Collection">
          <glview:MeasurementType rdf:about="http://schema.geolink.org/dev/voc/nvs/P02#SRFL"/>
        </owl:oneOf>
      </owl:Class>
    </owl:someValuesFrom>
    <owl:onProperty rdf:resource="http://schema.geolink.org/dev/view#hasMeasurementType"/>
  </owl:Restriction>
  <owl:Restriction>
    <rdfs:subClassOf>
      <glview:MeasurementType rdf:about="http://schema.geolink.org/dev/voc/nvs/P02#PTOX">
        <rdfs:subClassOf rdf:resource="http://schema.geolink.org/dev/voc/nvs/P03#B007"/>
        <rdfs:seeAlso rdf:resource="http://vocab.nerc.ac.uk/collection/P02/current/PTOX/"/>
        <rdfs:comment xml:lang="en">Parameters associated with the concentration of algae-generated toxins in either whole organisms or their constituent parts</rdfs:comment>
        <rdfs:label xml:lang="en">Concentration of phycotoxins in biota</rdfs:label>
        <rdf:type rdf:resource="http://www.w3.org/2002/07/owl#NamedIndividual"/>
        <rdf:type rdf:resource="http://www.w3.org/2002/07/owl#Class"/>
      </glview:MeasurementType>
    </rdfs:subClassOf>
    <owl:someValuesFrom>
      <owl:Class>
        <owl:oneOf rdf:parseType="Collection">
          <glview:MeasurementType rdf:about="http://schema.geolink.org/dev/voc/nvs/P02#PTOX"/>
        </owl:oneOf>
      </owl:Class>
    </owl:someValuesFrom>
    <owl:onProperty rdf:resource="http://schema.geolink.org/dev/view#hasMeasurementType"/>
  </owl:Restriction>
  <owl:Restriction>
    <rdfs:subClassOf rdf:resource="http://schema.geolink.org/dev/voc/nvs/P02#BCAH"/>
    <owl:someValuesFrom>
      <owl:Class>
        <owl:oneOf rdf:parseType="Collection">
          <owl:NamedIndividual rdf:about="http://schema.geolink.org/dev/voc/nvs/P02#BCAH"/>
        </owl:oneOf>
      </owl:Class>
    </owl:someValuesFrom>
    <owl:onProperty rdf:resource="http://schema.geolink.org/dev/view#hasMeasurementType"/>
  </owl:Restriction>
  <owl:Restriction>
    <rdfs:subClassOf>
      <glview:MeasurementType rdf:about="http://schema.geolink.org/dev/voc/nvs/P02#MDBO">
        <rdfs:subClassOf rdf:resource="http://schema.geolink.org/dev/voc/nvs/P03#C035"/>
        <rdfs:subClassOf rdf:resource="http://schema.geolink.org/dev/voc/nvs/P03#B007"/>
        <rdfs:subClassOf rdf:resource="http://schema.geolink.org/dev/voc/nvs/P03#H001"/>
        <rdfs:seeAlso rdf:resource="http://vocab.nerc.ac.uk/collection/P02/current/MDBO/"/>
        <rdfs:comment xml:lang="en">Concentration parameters for trace metalloid elements in either whole organisms or their constituent parts. Trace metalloids are considered as B, Ge, As, Sb, Te and Po (but not Si which is classed separately because of its major role in environmental chemistry)</rdfs:comment>
        <rdfs:label xml:lang="en">Trace metalloid concentrations in biota</rdfs:label>
        <rdf:type rdf:resource="http://www.w3.org/2002/07/owl#NamedIndividual"/>
        <rdf:type rdf:resource="http://www.w3.org/2002/07/owl#Class"/>
      </glview:MeasurementType>
    </rdfs:subClassOf>
    <owl:someValuesFrom>
      <owl:Class>
        <owl:oneOf rdf:parseType="Collection">
          <glview:MeasurementType rdf:about="http://schema.geolink.org/dev/voc/nvs/P02#MDBO"/>
        </owl:oneOf>
      </owl:Class>
    </owl:someValuesFrom>
    <owl:onProperty rdf:resource="http://schema.geolink.org/dev/view#hasMeasurementType"/>
  </owl:Restriction>
  <owl:Restriction>
    <rdfs:subClassOf>
      <glview:MeasurementType rdf:about="http://schema.geolink.org/dev/voc/nvs/P02#CPCN">
        <rdfs:subClassOf rdf:resource="http://schema.geolink.org/dev/voc/nvs/P03#B035"/>
        <rdfs:subClassOf rdf:resource="http://schema.geolink.org/dev/voc/nvs/P03#G035"/>
        <rdfs:seeAlso rdf:resource="http://vocab.nerc.ac.uk/collection/P02/current/CPCN/"/>
        <rdfs:comment xml:lang="en">Includes all pigments that cannot be explicitly classified as chlorophylls, phaeopigments or carotenoids (usually groups of pigments). Sediment includes anything collected by a grab or corer, including the fluff layer from the top of the consolidated sediment.</rdfs:comment>
        <rdfs:label xml:lang="en">Unclassified pigment concentrations in sediment</rdfs:label>
        <rdf:type rdf:resource="http://www.w3.org/2002/07/owl#NamedIndividual"/>
        <rdf:type rdf:resource="http://www.w3.org/2002/07/owl#Class"/>
      </glview:MeasurementType>
    </rdfs:subClassOf>
    <owl:someValuesFrom>
      <owl:Class>
        <owl:oneOf rdf:parseType="Collection">
          <glview:MeasurementType rdf:about="http://schema.geolink.org/dev/voc/nvs/P02#CPCN"/>
        </owl:oneOf>
      </owl:Class>
    </owl:someValuesFrom>
    <owl:onProperty rdf:resource="http://schema.geolink.org/dev/view#hasMeasurementType"/>
  </owl:Restriction>
  <owl:Restriction>
    <rdfs:subClassOf>
      <glview:MeasurementType rdf:about="http://schema.geolink.org/dev/voc/nvs/P02#NTRA">
        <rdfs:subClassOf rdf:resource="http://schema.geolink.org/dev/voc/nvs/P03#C005"/>
        <rdfs:subClassOf rdf:resource="http://schema.geolink.org/dev/voc/nvs/P03#C040"/>
        <rdfs:seeAlso rdf:resource="http://vocab.nerc.ac.uk/collection/P02/current/NTRA/"/>
        <rdfs:comment xml:lang="en">Nitrate concentration parameters (including statistical parameters such as standard deviation) in the water column. Includes nitrate+nitrite, which is often loosely referred to as nitrate.</rdfs:comment>
        <rdfs:label xml:lang="en">Nitrate concentration parameters in the water column</rdfs:label>
        <rdf:type rdf:resource="http://www.w3.org/2002/07/owl#NamedIndividual"/>
        <rdf:type rdf:resource="http://www.w3.org/2002/07/owl#Class"/>
      </glview:MeasurementType>
    </rdfs:subClassOf>
    <owl:someValuesFrom>
      <owl:Class>
        <owl:oneOf rdf:parseType="Collection">
          <glview:MeasurementType rdf:about="http://schema.geolink.org/dev/voc/nvs/P02#NTRA"/>
        </owl:oneOf>
      </owl:Class>
    </owl:someValuesFrom>
    <owl:onProperty rdf:resource="http://schema.geolink.org/dev/view#hasMeasurementType"/>
  </owl:Restriction>
  <owl:Restriction>
    <rdfs:subClassOf>
      <glview:MeasurementType rdf:about="http://schema.geolink.org/dev/voc/nvs/P02#CEMO">
        <rdfs:subClassOf rdf:resource="http://schema.geolink.org/dev/voc/nvs/P03#B015"/>
        <rdfs:seeAlso rdf:resource="http://vocab.nerc.ac.uk/collection/P02/current/CEMO/"/>
        <rdfs:comment xml:lang="en">Parameters describing the causes and rate of mortality in cetaceans (Order Cetacea). Includes both parameters mapped to taxa and those mapped to non-taxonomic groupings.</rdfs:comment>
        <rdfs:label xml:lang="en">Cetacean mortality</rdfs:label>
        <rdf:type rdf:resource="http://www.w3.org/2002/07/owl#NamedIndividual"/>
        <rdf:type rdf:resource="http://www.w3.org/2002/07/owl#Class"/>
      </glview:MeasurementType>
    </rdfs:subClassOf>
    <owl:someValuesFrom>
      <owl:Class>
        <owl:oneOf rdf:parseType="Collection">
          <glview:MeasurementType rdf:about="http://schema.geolink.org/dev/voc/nvs/P02#CEMO"/>
        </owl:oneOf>
      </owl:Class>
    </owl:someValuesFrom>
    <owl:onProperty rdf:resource="http://schema.geolink.org/dev/view#hasMeasurementType"/>
  </owl:Restriction>
  <owl:Restriction>
    <rdfs:subClassOf>
      <glview:MeasurementType rdf:about="http://schema.geolink.org/dev/voc/nvs/P02#NTSD">
        <rdfs:subClassOf rdf:resource="http://schema.geolink.org/dev/voc/nvs/P03#C005"/>
        <rdfs:subClassOf rdf:resource="http://schema.geolink.org/dev/voc/nvs/P03#G035"/>
        <rdfs:seeAlso rdf:resource="http://vocab.nerc.ac.uk/collection/P02/current/NTSD/"/>
        <rdfs:comment xml:lang="en">Concentrations of total, organic and inorganic nitrogen per unit weight of sediment.  Sediment is understood to be the solid phase of the bed, including the recently settled material sometimes known as fluff collected from the bed surface.</rdfs:comment>
        <rdfs:label xml:lang="en">Nitrogen concentrations in sediment</rdfs:label>
        <rdf:type rdf:resource="http://www.w3.org/2002/07/owl#NamedIndividual"/>
        <rdf:type rdf:resource="http://www.w3.org/2002/07/owl#Class"/>
      </glview:MeasurementType>
    </rdfs:subClassOf>
    <owl:someValuesFrom>
      <owl:Class>
        <owl:oneOf rdf:parseType="Collection">
          <glview:MeasurementType rdf:about="http://schema.geolink.org/dev/voc/nvs/P02#NTSD"/>
        </owl:oneOf>
      </owl:Class>
    </owl:someValuesFrom>
    <owl:onProperty rdf:resource="http://schema.geolink.org/dev/view#hasMeasurementType"/>
  </owl:Restriction>
  <owl:Restriction>
    <rdfs:subClassOf>
      <glview:MeasurementType rdf:about="http://schema.geolink.org/dev/voc/nvs/P02#DMST">
        <rdfs:subClassOf rdf:resource="http://schema.geolink.org/dev/voc/nvs/P03#C050"/>
        <rdfs:seeAlso rdf:resource="http://vocab.nerc.ac.uk/collection/P02/current/DMST/"/>
        <rdfs:comment xml:lang="en">All organosulphur compound concentration parameters (including saturations for gaseous species) in all phases of the water column</rdfs:comment>
        <rdfs:label xml:lang="en">Organosulphur species concentration parameters in the water column</rdfs:label>
        <rdf:type rdf:resource="http://www.w3.org/2002/07/owl#NamedIndividual"/>
        <rdf:type rdf:resource="http://www.w3.org/2002/07/owl#Class"/>
      </glview:MeasurementType>
    </rdfs:subClassOf>
    <owl:someValuesFrom>
      <owl:Class>
        <owl:oneOf rdf:parseType="Collection">
          <glview:MeasurementType rdf:about="http://schema.geolink.org/dev/voc/nvs/P02#DMST"/>
        </owl:oneOf>
      </owl:Class>
    </owl:someValuesFrom>
    <owl:onProperty rdf:resource="http://schema.geolink.org/dev/view#hasMeasurementType"/>
  </owl:Restriction>
  <owl:Restriction>
    <rdfs:subClassOf rdf:resource="http://schema.geolink.org/dev/voc/nvs/P02#MDBO"/>
    <owl:someValuesFrom>
      <owl:Class>
        <owl:oneOf rdf:parseType="Collection">
          <glview:MeasurementType rdf:about="http://schema.geolink.org/dev/voc/nvs/P02#MDBO"/>
        </owl:oneOf>
      </owl:Class>
    </owl:someValuesFrom>
    <owl:onProperty rdf:resource="http://schema.geolink.org/dev/view#hasMeasurementType"/>
  </owl:Restriction>
  <owl:Restriction>
    <rdfs:subClassOf>
      <glview:MeasurementType rdf:about="http://schema.geolink.org/dev/voc/nvs/P02#SVEL">
        <rdfs:subClassOf rdf:resource="http://schema.geolink.org/dev/voc/nvs/P03#D005"/>
        <rdfs:seeAlso rdf:resource="http://vocab.nerc.ac.uk/collection/P02/current/SVEL/"/>
        <rdfs:comment></rdfs:comment>
        <rdfs:label xml:lang="en">Sound velocity and travel time in the water column</rdfs:label>
        <rdf:type rdf:resource="http://www.w3.org/2002/07/owl#NamedIndividual"/>
        <rdf:type rdf:resource="http://www.w3.org/2002/07/owl#Class"/>
      </glview:MeasurementType>
    </rdfs:subClassOf>
    <owl:someValuesFrom>
      <owl:Class>
        <owl:oneOf rdf:parseType="Collection">
          <glview:MeasurementType rdf:about="http://schema.geolink.org/dev/voc/nvs/P02#SVEL"/>
        </owl:oneOf>
      </owl:Class>
    </owl:someValuesFrom>
    <owl:onProperty rdf:resource="http://schema.geolink.org/dev/view#hasMeasurementType"/>
  </owl:Restriction>
  <owl:Restriction>
    <rdfs:subClassOf rdf:resource="http://schema.geolink.org/dev/voc/nvs/P02#SPCB"/>
    <owl:someValuesFrom>
      <owl:Class>
        <owl:oneOf rdf:parseType="Collection">
          <glview:MeasurementType rdf:about="http://schema.geolink.org/dev/voc/nvs/P02#SPCB"/>
        </owl:oneOf>
      </owl:Class>
    </owl:someValuesFrom>
    <owl:onProperty rdf:resource="http://schema.geolink.org/dev/view#hasMeasurementType"/>
  </owl:Restriction>
  <owl:Restriction>
    <rdfs:subClassOf rdf:resource="http://schema.geolink.org/dev/voc/nvs/P02#SXCN"/>
    <owl:someValuesFrom>
      <owl:Class>
        <owl:oneOf rdf:parseType="Collection">
          <glview:MeasurementType rdf:about="http://schema.geolink.org/dev/voc/nvs/P02#SXCN"/>
        </owl:oneOf>
      </owl:Class>
    </owl:someValuesFrom>
    <owl:onProperty rdf:resource="http://schema.geolink.org/dev/view#hasMeasurementType"/>
  </owl:Restriction>
  <owl:Restriction>
    <rdfs:subClassOf>
      <glview:MeasurementType rdf:about="http://schema.geolink.org/dev/voc/nvs/P02#VIRU">
        <rdfs:subClassOf rdf:resource="http://schema.geolink.org/dev/voc/nvs/P03#B070"/>
        <rdfs:subClassOf rdf:resource="http://schema.geolink.org/dev/voc/nvs/P03#B005"/>
        <rdfs:seeAlso rdf:resource="http://vocab.nerc.ac.uk/collection/P02/current/VIRU/"/>
        <rdfs:comment xml:lang="en">Any enumeration (e.g. count, number per square metre) of viruses in any body of fresh or salt water.</rdfs:comment>
        <rdfs:label xml:lang="en">Virus abundance in water bodies</rdfs:label>
        <rdf:type rdf:resource="http://www.w3.org/2002/07/owl#NamedIndividual"/>
        <rdf:type rdf:resource="http://www.w3.org/2002/07/owl#Class"/>
      </glview:MeasurementType>
    </rdfs:subClassOf>
    <owl:someValuesFrom>
      <owl:Class>
        <owl:oneOf rdf:parseType="Collection">
          <glview:MeasurementType rdf:about="http://schema.geolink.org/dev/voc/nvs/P02#VIRU"/>
        </owl:oneOf>
      </owl:Class>
    </owl:someValuesFrom>
    <owl:onProperty rdf:resource="http://schema.geolink.org/dev/view#hasMeasurementType"/>
  </owl:Restriction>
  <owl:Restriction>
    <rdfs:subClassOf>
      <glview:MeasurementType rdf:about="http://schema.geolink.org/dev/voc/nvs/P02#PHBI">
        <rdfs:subClassOf rdf:resource="http://schema.geolink.org/dev/voc/nvs/P03#C055"/>
        <rdfs:subClassOf rdf:resource="http://schema.geolink.org/dev/voc/nvs/P03#B007"/>
        <rdfs:subClassOf rdf:resource="http://schema.geolink.org/dev/voc/nvs/P03#H001"/>
        <rdfs:seeAlso rdf:resource="http://vocab.nerc.ac.uk/collection/P02/current/PHBI/"/>
        <rdfs:comment xml:lang="en">Concentration parameters for substances synthesised by man to modify bodily function or diagnose, cure, mitigate, treat, or prevent disease in either whole organisms or their constituent parts.</rdfs:comment>
        <rdfs:label xml:lang="en">Pharmaceutical concentrations in biota</rdfs:label>
        <rdf:type rdf:resource="http://www.w3.org/2002/07/owl#NamedIndividual"/>
        <rdf:type rdf:resource="http://www.w3.org/2002/07/owl#Class"/>
      </glview:MeasurementType>
    </rdfs:subClassOf>
    <owl:someValuesFrom>
      <owl:Class>
        <owl:oneOf rdf:parseType="Collection">
          <glview:MeasurementType rdf:about="http://schema.geolink.org/dev/voc/nvs/P02#PHBI"/>
        </owl:oneOf>
      </owl:Class>
    </owl:someValuesFrom>
    <owl:onProperty rdf:resource="http://schema.geolink.org/dev/view#hasMeasurementType"/>
  </owl:Restriction>
  <owl:Restriction>
    <rdfs:subClassOf rdf:resource="http://schema.geolink.org/dev/voc/nvs/P02#SRFL"/>
    <owl:someValuesFrom>
      <owl:Class>
        <owl:oneOf rdf:parseType="Collection">
          <glview:MeasurementType rdf:about="http://schema.geolink.org/dev/voc/nvs/P02#SRFL"/>
        </owl:oneOf>
      </owl:Class>
    </owl:someValuesFrom>
    <owl:onProperty rdf:resource="http://schema.geolink.org/dev/view#hasMeasurementType"/>
  </owl:Restriction>
  <owl:Restriction>
    <rdfs:subClassOf>
      <glview:MeasurementType rdf:about="http://schema.geolink.org/dev/voc/nvs/P02#VSRA">
        <rdfs:subClassOf rdf:resource="http://schema.geolink.org/dev/voc/nvs/P03#D015"/>
        <rdfs:subClassOf rdf:resource="http://schema.geolink.org/dev/voc/nvs/P03#M010"/>
        <rdfs:seeAlso rdf:resource="http://vocab.nerc.ac.uk/collection/P02/current/VSRA/"/>
        <rdfs:comment xml:lang="en">Includes visible waveband measurements at discrete wavelengths and PAR integrated values as photon and energy fluxes. Does not include satellite radiometer and associated calibration parameters (e.g. water-leaving radiance and reflectance)</rdfs:comment>
        <rdfs:label xml:lang="en">Visible waveband radiance and irradiance measurements in the atmosphere</rdfs:label>
        <rdf:type rdf:resource="http://www.w3.org/2002/07/owl#NamedIndividual"/>
        <rdf:type rdf:resource="http://www.w3.org/2002/07/owl#Class"/>
      </glview:MeasurementType>
    </rdfs:subClassOf>
    <owl:someValuesFrom>
      <owl:Class>
        <owl:oneOf rdf:parseType="Collection">
          <glview:MeasurementType rdf:about="http://schema.geolink.org/dev/voc/nvs/P02#VSRA"/>
        </owl:oneOf>
      </owl:Class>
    </owl:someValuesFrom>
    <owl:onProperty rdf:resource="http://schema.geolink.org/dev/view#hasMeasurementType"/>
  </owl:Restriction>
  <owl:Restriction>
    <rdfs:subClassOf rdf:resource="http://schema.geolink.org/dev/voc/nvs/P02#NTRA"/>
    <owl:someValuesFrom>
      <owl:Class>
        <owl:oneOf rdf:parseType="Collection">
          <glview:MeasurementType rdf:about="http://schema.geolink.org/dev/voc/nvs/P02#NTRA"/>
        </owl:oneOf>
      </owl:Class>
    </owl:someValuesFrom>
    <owl:onProperty rdf:resource="http://schema.geolink.org/dev/view#hasMeasurementType"/>
  </owl:Restriction>
  <owl:Restriction>
    <rdfs:subClassOf>
      <glview:MeasurementType rdf:about="http://schema.geolink.org/dev/voc/nvs/P02#BAUC">
        <rdfs:subClassOf rdf:resource="http://schema.geolink.org/dev/voc/nvs/P03#B070"/>
        <rdfs:subClassOf rdf:resource="http://schema.geolink.org/dev/voc/nvs/P03#B005"/>
        <rdfs:seeAlso rdf:resource="http://vocab.nerc.ac.uk/collection/P02/current/BAUC/"/>
        <rdfs:comment xml:lang="en">Any enumeration of bacteria (Kingdom Monera so includes cyanobacteria) designated by taxonomic names (e.g. species, genus, family) in any soil or sediment.</rdfs:comment>
        <rdfs:label xml:lang="en">Bacteria taxonomic abundance in sediment</rdfs:label>
        <rdf:type rdf:resource="http://www.w3.org/2002/07/owl#NamedIndividual"/>
        <rdf:type rdf:resource="http://www.w3.org/2002/07/owl#Class"/>
      </glview:MeasurementType>
    </rdfs:subClassOf>
    <owl:someValuesFrom>
      <owl:Class>
        <owl:oneOf rdf:parseType="Collection">
          <glview:MeasurementType rdf:about="http://schema.geolink.org/dev/voc/nvs/P02#BAUC"/>
        </owl:oneOf>
      </owl:Class>
    </owl:someValuesFrom>
    <owl:onProperty rdf:resource="http://schema.geolink.org/dev/view#hasMeasurementType"/>
  </owl:Restriction>
  <owl:Restriction>
    <rdfs:subClassOf rdf:resource="http://schema.geolink.org/dev/voc/nvs/P02#RMIN"/>
    <owl:someValuesFrom>
      <owl:Class>
        <owl:oneOf rdf:parseType="Collection">
          <glview:MeasurementType rdf:about="http://schema.geolink.org/dev/voc/nvs/P02#RMIN"/>
        </owl:oneOf>
      </owl:Class>
    </owl:someValuesFrom>
    <owl:onProperty rdf:resource="http://schema.geolink.org/dev/view#hasMeasurementType"/>
  </owl:Restriction>
  <owl:Restriction>
    <rdfs:subClassOf>
      <glview:MeasurementType rdf:about="http://schema.geolink.org/dev/voc/nvs/P02#ZADX">
        <rdfs:subClassOf rdf:resource="http://schema.geolink.org/dev/voc/nvs/P03#B070"/>
        <rdfs:subClassOf rdf:resource="http://schema.geolink.org/dev/voc/nvs/P03#G055"/>
        <rdfs:seeAlso rdf:resource="http://vocab.nerc.ac.uk/collection/P02/current/ZADX/"/>
        <rdfs:comment xml:lang="en">Any quantification of the dry mass of zoobenthos (animals living on, in or near the bed of any water body). Includes animals normally considered planktonic if collected in sediment and data expressed ash-free and in terms of carbon, nitrogen etc..</rdfs:comment>
        <rdfs:label xml:lang="en">Zoobenthos dry weight biomass</rdfs:label>
        <rdf:type rdf:resource="http://www.w3.org/2002/07/owl#NamedIndividual"/>
        <rdf:type rdf:resource="http://www.w3.org/2002/07/owl#Class"/>
      </glview:MeasurementType>
    </rdfs:subClassOf>
    <owl:someValuesFrom>
      <owl:Class>
        <owl:oneOf rdf:parseType="Collection">
          <glview:MeasurementType rdf:about="http://schema.geolink.org/dev/voc/nvs/P02#ZADX"/>
        </owl:oneOf>
      </owl:Class>
    </owl:someValuesFrom>
    <owl:onProperty rdf:resource="http://schema.geolink.org/dev/view#hasMeasurementType"/>
  </owl:Restriction>
  <owl:Restriction>
    <rdfs:subClassOf rdf:resource="http://schema.geolink.org/dev/voc/nvs/P02#SIAT"/>
    <owl:someValuesFrom>
      <owl:Class>
        <owl:oneOf rdf:parseType="Collection">
          <glview:MeasurementType rdf:about="http://schema.geolink.org/dev/voc/nvs/P02#SIAT"/>
        </owl:oneOf>
      </owl:Class>
    </owl:someValuesFrom>
    <owl:onProperty rdf:resource="http://schema.geolink.org/dev/view#hasMeasurementType"/>
  </owl:Restriction>
  <owl:Restriction>
    <rdfs:subClassOf>
      <glview:MeasurementType rdf:about="http://schema.geolink.org/dev/voc/nvs/P02#WSTR">
        <rdfs:subClassOf rdf:resource="http://schema.geolink.org/dev/voc/nvs/P03#M010"/>
        <rdfs:seeAlso rdf:resource="http://vocab.nerc.ac.uk/collection/P02/current/WSTR/"/>
        <rdfs:comment xml:lang="en">Parameters related to forces due to interactions between atmosphere and the surface of the earth or between atmospheric air masses</rdfs:comment>
        <rdfs:label xml:lang="en">Wind stress and shear</rdfs:label>
        <rdf:type rdf:resource="http://www.w3.org/2002/07/owl#NamedIndividual"/>
        <rdf:type rdf:resource="http://www.w3.org/2002/07/owl#Class"/>
      </glview:MeasurementType>
    </rdfs:subClassOf>
    <owl:someValuesFrom>
      <owl:Class>
        <owl:oneOf rdf:parseType="Collection">
          <glview:MeasurementType rdf:about="http://schema.geolink.org/dev/voc/nvs/P02#WSTR"/>
        </owl:oneOf>
      </owl:Class>
    </owl:someValuesFrom>
    <owl:onProperty rdf:resource="http://schema.geolink.org/dev/view#hasMeasurementType"/>
  </owl:Restriction>
  <owl:Restriction>
    <rdfs:subClassOf rdf:resource="http://schema.geolink.org/dev/voc/nvs/P02#NTSD"/>
    <owl:someValuesFrom>
      <owl:Class>
        <owl:oneOf rdf:parseType="Collection">
          <glview:MeasurementType rdf:about="http://schema.geolink.org/dev/voc/nvs/P02#NTSD"/>
        </owl:oneOf>
      </owl:Class>
    </owl:someValuesFrom>
    <owl:onProperty rdf:resource="http://schema.geolink.org/dev/view#hasMeasurementType"/>
  </owl:Restriction>
  <owl:Restriction>
    <rdfs:subClassOf>
      <glview:MeasurementType rdf:about="http://schema.geolink.org/dev/voc/nvs/P02#BDRV">
        <rdfs:subClassOf rdf:resource="http://schema.geolink.org/dev/voc/nvs/P03#B070"/>
        <rdfs:seeAlso rdf:resource="http://vocab.nerc.ac.uk/collection/P02/current/BDRV/"/>
        <rdfs:comment xml:lang="en">Parameters describing the variety of entity types encountered in a population of living organisms</rdfs:comment>
        <rdfs:label xml:lang="en">Biodiversity indices</rdfs:label>
        <rdf:type rdf:resource="http://www.w3.org/2002/07/owl#NamedIndividual"/>
        <rdf:type rdf:resource="http://www.w3.org/2002/07/owl#Class"/>
      </glview:MeasurementType>
    </rdfs:subClassOf>
    <owl:someValuesFrom>
      <owl:Class>
        <owl:oneOf rdf:parseType="Collection">
          <glview:MeasurementType rdf:about="http://schema.geolink.org/dev/voc/nvs/P02#BDRV"/>
        </owl:oneOf>
      </owl:Class>
    </owl:someValuesFrom>
    <owl:onProperty rdf:resource="http://schema.geolink.org/dev/view#hasMeasurementType"/>
  </owl:Restriction>
  <owl:Restriction>
    <rdfs:subClassOf rdf:resource="http://schema.geolink.org/dev/voc/nvs/P02#PHBI"/>
    <owl:someValuesFrom>
      <owl:Class>
        <owl:oneOf rdf:parseType="Collection">
          <glview:MeasurementType rdf:about="http://schema.geolink.org/dev/voc/nvs/P02#PHBI"/>
        </owl:oneOf>
      </owl:Class>
    </owl:someValuesFrom>
    <owl:onProperty rdf:resource="http://schema.geolink.org/dev/view#hasMeasurementType"/>
  </owl:Restriction>
  <owl:Restriction>
    <rdfs:subClassOf rdf:resource="http://schema.geolink.org/dev/voc/nvs/P02#OMWC"/>
    <owl:someValuesFrom>
      <owl:Class>
        <owl:oneOf rdf:parseType="Collection">
          <owl:NamedIndividual rdf:about="http://schema.geolink.org/dev/voc/nvs/P02#OMWC"/>
        </owl:oneOf>
      </owl:Class>
    </owl:someValuesFrom>
    <owl:onProperty rdf:resource="http://schema.geolink.org/dev/view#hasMeasurementType"/>
  </owl:Restriction>
  <owl:Restriction>
    <rdfs:subClassOf>
      <glview:MeasurementType rdf:about="http://schema.geolink.org/dev/voc/nvs/P02#ATVS">
        <rdfs:subClassOf rdf:resource="http://schema.geolink.org/dev/voc/nvs/P03#M010"/>
        <rdfs:seeAlso rdf:resource="http://vocab.nerc.ac.uk/collection/P02/current/ATVS/"/>
        <rdfs:comment xml:lang="en">Parameters relating to atmospheric clarity, such as optical transmittance/attenuance, and resultant visibility</rdfs:comment>
        <rdfs:label xml:lang="en">Atmospheric visibility and transparency</rdfs:label>
        <rdf:type rdf:resource="http://www.w3.org/2002/07/owl#NamedIndividual"/>
        <rdf:type rdf:resource="http://www.w3.org/2002/07/owl#Class"/>
      </glview:MeasurementType>
    </rdfs:subClassOf>
    <owl:someValuesFrom>
      <owl:Class>
        <owl:oneOf rdf:parseType="Collection">
          <glview:MeasurementType rdf:about="http://schema.geolink.org/dev/voc/nvs/P02#ATVS"/>
        </owl:oneOf>
      </owl:Class>
    </owl:someValuesFrom>
    <owl:onProperty rdf:resource="http://schema.geolink.org/dev/view#hasMeasurementType"/>
  </owl:Restriction>
  <owl:Restriction>
    <rdfs:subClassOf>
      <glview:MeasurementType rdf:about="http://schema.geolink.org/dev/voc/nvs/P02#GP012">
        <rdfs:subClassOf rdf:resource="http://schema.geolink.org/dev/voc/nvs/P03#B060"/>
        <rdfs:subClassOf rdf:resource="http://schema.geolink.org/dev/voc/nvs/P03#B055"/>
        <rdfs:seeAlso rdf:resource="http://vocab.nerc.ac.uk/collection/P02/current/GP012/"/>
        <rdfs:comment xml:lang="en">Parameters relating to diseases and parasites of macroalgae (Rhodophycota, Chromphycota, Chlorophycota)  and seagrass (Charophyta, Anthophyta) and damage to seagrass beds</rdfs:comment>
        <rdfs:label xml:lang="en">Macroalgae and seagrass infection and damage</rdfs:label>
        <rdf:type rdf:resource="http://www.w3.org/2002/07/owl#NamedIndividual"/>
        <rdf:type rdf:resource="http://www.w3.org/2002/07/owl#Class"/>
      </glview:MeasurementType>
    </rdfs:subClassOf>
    <owl:someValuesFrom>
      <owl:Class>
        <owl:oneOf rdf:parseType="Collection">
          <glview:MeasurementType rdf:about="http://schema.geolink.org/dev/voc/nvs/P02#GP012"/>
        </owl:oneOf>
      </owl:Class>
    </owl:someValuesFrom>
    <owl:onProperty rdf:resource="http://schema.geolink.org/dev/view#hasMeasurementType"/>
  </owl:Restriction>
  <owl:Restriction>
    <rdfs:subClassOf rdf:resource="http://schema.geolink.org/dev/voc/nvs/P02#VIRU"/>
    <owl:someValuesFrom>
      <owl:Class>
        <owl:oneOf rdf:parseType="Collection">
          <glview:MeasurementType rdf:about="http://schema.geolink.org/dev/voc/nvs/P02#VIRU"/>
        </owl:oneOf>
      </owl:Class>
    </owl:someValuesFrom>
    <owl:onProperty rdf:resource="http://schema.geolink.org/dev/view#hasMeasurementType"/>
  </owl:Restriction>
  <owl:Restriction>
    <rdfs:subClassOf rdf:resource="http://schema.geolink.org/dev/voc/nvs/P02#RVDS"/>
    <owl:someValuesFrom>
      <owl:Class>
        <owl:oneOf rdf:parseType="Collection">
          <glview:MeasurementType rdf:about="http://schema.geolink.org/dev/voc/nvs/P02#RVDS"/>
        </owl:oneOf>
      </owl:Class>
    </owl:someValuesFrom>
    <owl:onProperty rdf:resource="http://schema.geolink.org/dev/view#hasMeasurementType"/>
  </owl:Restriction>
  <owl:Restriction>
    <rdfs:subClassOf>
      <glview:MeasurementType rdf:about="http://schema.geolink.org/dev/voc/nvs/P02#ABAG">
        <rdfs:subClassOf rdf:resource="http://schema.geolink.org/dev/voc/nvs/P03#G015"/>
        <rdfs:seeAlso rdf:resource="http://vocab.nerc.ac.uk/collection/P02/current/ABAG/"/>
        <rdfs:comment xml:lang="en">Parameters relating to the abundance, size and morphology of particle aggregates in the SPM</rdfs:comment>
        <rdfs:label xml:lang="en">Suspended particulate material aggregates</rdfs:label>
        <rdf:type rdf:resource="http://www.w3.org/2002/07/owl#NamedIndividual"/>
        <rdf:type rdf:resource="http://www.w3.org/2002/07/owl#Class"/>
      </glview:MeasurementType>
    </rdfs:subClassOf>
    <owl:someValuesFrom>
      <owl:Class>
        <owl:oneOf rdf:parseType="Collection">
          <glview:MeasurementType rdf:about="http://schema.geolink.org/dev/voc/nvs/P02#ABAG"/>
        </owl:oneOf>
      </owl:Class>
    </owl:someValuesFrom>
    <owl:onProperty rdf:resource="http://schema.geolink.org/dev/view#hasMeasurementType"/>
  </owl:Restriction>
  <owl:Restriction>
    <rdfs:subClassOf>
      <glview:MeasurementType rdf:about="http://schema.geolink.org/dev/voc/nvs/P02#GP025">
        <rdfs:subClassOf rdf:resource="http://schema.geolink.org/dev/voc/nvs/P03#B015"/>
        <rdfs:seeAlso rdf:resource="http://vocab.nerc.ac.uk/collection/P02/current/GP025/"/>
        <rdfs:comment xml:lang="en">Parameters related to the reproduction of seals (Family Phocidae)</rdfs:comment>
        <rdfs:label xml:lang="en">Seal reproduction</rdfs:label>
        <rdf:type rdf:resource="http://www.w3.org/2002/07/owl#NamedIndividual"/>
        <rdf:type rdf:resource="http://www.w3.org/2002/07/owl#Class"/>
      </glview:MeasurementType>
    </rdfs:subClassOf>
    <owl:someValuesFrom>
      <owl:Class>
        <owl:oneOf rdf:parseType="Collection">
          <glview:MeasurementType rdf:about="http://schema.geolink.org/dev/voc/nvs/P02#GP025"/>
        </owl:oneOf>
      </owl:Class>
    </owl:someValuesFrom>
    <owl:onProperty rdf:resource="http://schema.geolink.org/dev/view#hasMeasurementType"/>
  </owl:Restriction>
  <owl:Restriction>
    <rdfs:subClassOf>
      <glview:MeasurementType rdf:about="http://schema.geolink.org/dev/voc/nvs/P02#ZBTX">
        <rdfs:subClassOf rdf:resource="http://schema.geolink.org/dev/voc/nvs/P03#B070"/>
        <rdfs:subClassOf rdf:resource="http://schema.geolink.org/dev/voc/nvs/P03#G055"/>
        <rdfs:seeAlso rdf:resource="http://vocab.nerc.ac.uk/collection/P02/current/ZBTX/"/>
        <rdfs:comment xml:lang="en">Any enumeration (e.g. count, number per square metre) of animals living on or near the seabed designated by taxonomic names (e.g. species, genus).</rdfs:comment>
        <rdfs:label xml:lang="en">Zoobenthos taxonomic abundance</rdfs:label>
        <rdf:type rdf:resource="http://www.w3.org/2002/07/owl#NamedIndividual"/>
        <rdf:type rdf:resource="http://www.w3.org/2002/07/owl#Class"/>
      </glview:MeasurementType>
    </rdfs:subClassOf>
    <owl:someValuesFrom>
      <owl:Class>
        <owl:oneOf rdf:parseType="Collection">
          <glview:MeasurementType rdf:about="http://schema.geolink.org/dev/voc/nvs/P02#ZBTX"/>
        </owl:oneOf>
      </owl:Class>
    </owl:someValuesFrom>
    <owl:onProperty rdf:resource="http://schema.geolink.org/dev/view#hasMeasurementType"/>
  </owl:Restriction>
  <owl:Restriction>
    <rdfs:subClassOf>
      <glview:MeasurementType rdf:about="http://schema.geolink.org/dev/voc/nvs/P02#MLES">
        <rdfs:subClassOf rdf:resource="http://schema.geolink.org/dev/voc/nvs/P03#H005"/>
        <rdfs:seeAlso rdf:resource="http://vocab.nerc.ac.uk/collection/P02/current/MLES/"/>
        <rdfs:comment xml:lang="en">Parameters quantifying the extent and nature of recreational activities in coastal waters, estuaries and their margins such as beaches.</rdfs:comment>
        <rdfs:label xml:lang="en">Marine environment leisure usage</rdfs:label>
        <rdf:type rdf:resource="http://www.w3.org/2002/07/owl#NamedIndividual"/>
        <rdf:type rdf:resource="http://www.w3.org/2002/07/owl#Class"/>
      </glview:MeasurementType>
    </rdfs:subClassOf>
    <owl:someValuesFrom>
      <owl:Class>
        <owl:oneOf rdf:parseType="Collection">
          <glview:MeasurementType rdf:about="http://schema.geolink.org/dev/voc/nvs/P02#MLES"/>
        </owl:oneOf>
      </owl:Class>
    </owl:someValuesFrom>
    <owl:onProperty rdf:resource="http://schema.geolink.org/dev/view#hasMeasurementType"/>
  </owl:Restriction>
  <owl:Restriction>
    <rdfs:subClassOf rdf:resource="http://schema.geolink.org/dev/voc/nvs/P02#PHBI"/>
    <owl:someValuesFrom>
      <owl:Class>
        <owl:oneOf rdf:parseType="Collection">
          <glview:MeasurementType rdf:about="http://schema.geolink.org/dev/voc/nvs/P02#PHBI"/>
        </owl:oneOf>
      </owl:Class>
    </owl:someValuesFrom>
    <owl:onProperty rdf:resource="http://schema.geolink.org/dev/view#hasMeasurementType"/>
  </owl:Restriction>
  <owl:Restriction>
    <rdfs:subClassOf>
      <glview:MeasurementType rdf:about="http://schema.geolink.org/dev/voc/nvs/P02#BABI">
        <rdfs:subClassOf rdf:resource="http://schema.geolink.org/dev/voc/nvs/P03#B007"/>
        <rdfs:subClassOf rdf:resource="http://schema.geolink.org/dev/voc/nvs/P03#B005"/>
        <rdfs:subClassOf rdf:resource="http://schema.geolink.org/dev/voc/nvs/P03#H001"/>
        <rdfs:seeAlso rdf:resource="http://vocab.nerc.ac.uk/collection/P02/current/BABI/"/>
        <rdfs:comment xml:lang="en">Parameters relating to the abundance and nature of bacteria (Kingdom Monera) infecting other biota.</rdfs:comment>
        <rdfs:label xml:lang="en">Bacteria in biota</rdfs:label>
        <rdf:type rdf:resource="http://www.w3.org/2002/07/owl#NamedIndividual"/>
        <rdf:type rdf:resource="http://www.w3.org/2002/07/owl#Class"/>
      </glview:MeasurementType>
    </rdfs:subClassOf>
    <owl:someValuesFrom>
      <owl:Class>
        <owl:oneOf rdf:parseType="Collection">
          <glview:MeasurementType rdf:about="http://schema.geolink.org/dev/voc/nvs/P02#BABI"/>
        </owl:oneOf>
      </owl:Class>
    </owl:someValuesFrom>
    <owl:onProperty rdf:resource="http://schema.geolink.org/dev/view#hasMeasurementType"/>
  </owl:Restriction>
  <owl:Restriction>
    <rdfs:subClassOf>
      <glview:MeasurementType rdf:about="http://schema.geolink.org/dev/voc/nvs/P02#ZNTX">
        <rdfs:subClassOf rdf:resource="http://schema.geolink.org/dev/voc/nvs/P03#B045"/>
        <rdfs:subClassOf rdf:resource="http://schema.geolink.org/dev/voc/nvs/P03#B070"/>
        <rdfs:seeAlso rdf:resource="http://vocab.nerc.ac.uk/collection/P02/current/ZNTX/"/>
        <rdfs:comment xml:lang="en">Zooplankton (mesozooplankton plus larger pelagic animals excluding fish, reptiles and mammals) abundance per unit volume parameters not included in group ZATX.  Usually used for generic names such as 'mesozooplankton'.</rdfs:comment>
        <rdfs:label xml:lang="en">Zooplankton non taxonomy-related abundance per unit volume of the water column</rdfs:label>
        <rdf:type rdf:resource="http://www.w3.org/2002/07/owl#NamedIndividual"/>
        <rdf:type rdf:resource="http://www.w3.org/2002/07/owl#Class"/>
      </glview:MeasurementType>
    </rdfs:subClassOf>
    <owl:someValuesFrom>
      <owl:Class>
        <owl:oneOf rdf:parseType="Collection">
          <glview:MeasurementType rdf:about="http://schema.geolink.org/dev/voc/nvs/P02#ZNTX"/>
        </owl:oneOf>
      </owl:Class>
    </owl:someValuesFrom>
    <owl:onProperty rdf:resource="http://schema.geolink.org/dev/view#hasMeasurementType"/>
  </owl:Restriction>
  <owl:Restriction>
    <rdfs:subClassOf>
      <glview:MeasurementType rdf:about="http://schema.geolink.org/dev/voc/nvs/P02#PHUP">
        <rdfs:subClassOf rdf:resource="http://schema.geolink.org/dev/voc/nvs/P03#O010"/>
        <rdfs:subClassOf rdf:resource="http://schema.geolink.org/dev/voc/nvs/P03#C040"/>
        <rdfs:seeAlso rdf:resource="http://vocab.nerc.ac.uk/collection/P02/current/PHUP/"/>
        <rdfs:comment xml:lang="en">Uptake of nutrients other than nitrogen species (ie phosphate and silicate) by the water column</rdfs:comment>
        <rdfs:label xml:lang="en">Uptake of other nutrients in the water column</rdfs:label>
        <rdf:type rdf:resource="http://www.w3.org/2002/07/owl#NamedIndividual"/>
        <rdf:type rdf:resource="http://www.w3.org/2002/07/owl#Class"/>
      </glview:MeasurementType>
    </rdfs:subClassOf>
    <owl:someValuesFrom>
      <owl:Class>
        <owl:oneOf rdf:parseType="Collection">
          <glview:MeasurementType rdf:about="http://schema.geolink.org/dev/voc/nvs/P02#PHUP"/>
        </owl:oneOf>
      </owl:Class>
    </owl:someValuesFrom>
    <owl:onProperty rdf:resource="http://schema.geolink.org/dev/view#hasMeasurementType"/>
  </owl:Restriction>
  <owl:Restriction>
    <rdfs:subClassOf>
      <glview:MeasurementType rdf:about="http://schema.geolink.org/dev/voc/nvs/P02#OGPW">
        <rdfs:subClassOf rdf:resource="http://schema.geolink.org/dev/voc/nvs/P03#C015"/>
        <rdfs:seeAlso rdf:resource="http://vocab.nerc.ac.uk/collection/P02/current/OGPW/"/>
        <rdfs:comment xml:lang="en">All concentration parameters for inorganic dissolved gases other than oxygen and the noble gases in sediment pore water samples</rdfs:comment>
        <rdfs:label xml:lang="en">Dissolved concentration parameters for other gases in sediment pore waters</rdfs:label>
        <rdf:type rdf:resource="http://www.w3.org/2002/07/owl#NamedIndividual"/>
        <rdf:type rdf:resource="http://www.w3.org/2002/07/owl#Class"/>
      </glview:MeasurementType>
    </rdfs:subClassOf>
    <owl:someValuesFrom>
      <owl:Class>
        <owl:oneOf rdf:parseType="Collection">
          <glview:MeasurementType rdf:about="http://schema.geolink.org/dev/voc/nvs/P02#OGPW"/>
        </owl:oneOf>
      </owl:Class>
    </owl:someValuesFrom>
    <owl:onProperty rdf:resource="http://schema.geolink.org/dev/view#hasMeasurementType"/>
  </owl:Restriction>
  <owl:Restriction>
    <rdfs:subClassOf rdf:resource="http://schema.geolink.org/dev/voc/nvs/P02#MZBN"/>
    <owl:someValuesFrom>
      <owl:Class>
        <owl:oneOf rdf:parseType="Collection">
          <glview:MeasurementType rdf:about="http://schema.geolink.org/dev/voc/nvs/P02#MZBN"/>
        </owl:oneOf>
      </owl:Class>
    </owl:someValuesFrom>
    <owl:onProperty rdf:resource="http://schema.geolink.org/dev/view#hasMeasurementType"/>
  </owl:Restriction>
  <owl:Restriction>
    <rdfs:subClassOf>
      <glview:MeasurementType rdf:about="http://schema.geolink.org/dev/voc/nvs/P02#IRBO">
        <rdfs:subClassOf rdf:resource="http://schema.geolink.org/dev/voc/nvs/P03#C030"/>
        <rdfs:subClassOf rdf:resource="http://schema.geolink.org/dev/voc/nvs/P03#B007"/>
        <rdfs:seeAlso rdf:resource="http://vocab.nerc.ac.uk/collection/P02/current/IRBO/"/>
        <rdfs:comment xml:lang="en">Stable isotope enrichment parameters from measurements on living (at the time of sampling) organisms or parts thereof</rdfs:comment>
        <rdfs:label xml:lang="en">Stable isotope enrichment in biota</rdfs:label>
        <rdf:type rdf:resource="http://www.w3.org/2002/07/owl#NamedIndividual"/>
        <rdf:type rdf:resource="http://www.w3.org/2002/07/owl#Class"/>
      </glview:MeasurementType>
    </rdfs:subClassOf>
    <owl:someValuesFrom>
      <owl:Class>
        <owl:oneOf rdf:parseType="Collection">
          <glview:MeasurementType rdf:about="http://schema.geolink.org/dev/voc/nvs/P02#IRBO"/>
        </owl:oneOf>
      </owl:Class>
    </owl:someValuesFrom>
    <owl:onProperty rdf:resource="http://schema.geolink.org/dev/view#hasMeasurementType"/>
  </owl:Restriction>
  <owl:Restriction>
    <rdfs:subClassOf rdf:resource="http://schema.geolink.org/dev/voc/nvs/P02#BABI"/>
    <owl:someValuesFrom>
      <owl:Class>
        <owl:oneOf rdf:parseType="Collection">
          <glview:MeasurementType rdf:about="http://schema.geolink.org/dev/voc/nvs/P02#BABI"/>
        </owl:oneOf>
      </owl:Class>
    </owl:someValuesFrom>
    <owl:onProperty rdf:resource="http://schema.geolink.org/dev/view#hasMeasurementType"/>
  </owl:Restriction>
  <owl:Restriction>
    <rdfs:subClassOf>
      <glview:MeasurementType rdf:about="http://schema.geolink.org/dev/voc/nvs/P02#SSTR">
        <rdfs:subClassOf rdf:resource="http://schema.geolink.org/dev/voc/nvs/P03#GSED"/>
        <rdfs:seeAlso rdf:resource="http://vocab.nerc.ac.uk/collection/P02/current/SSTR/"/>
        <rdfs:comment xml:lang="en">Parameters characterising structure in sedimentary rocks and unlithified sediment such as bedding, lamination and bioturbation.</rdfs:comment>
        <rdfs:label xml:lang="en">Sedimentary structure</rdfs:label>
        <rdf:type rdf:resource="http://www.w3.org/2002/07/owl#NamedIndividual"/>
        <rdf:type rdf:resource="http://www.w3.org/2002/07/owl#Class"/>
      </glview:MeasurementType>
    </rdfs:subClassOf>
    <owl:someValuesFrom>
      <owl:Class>
        <owl:oneOf rdf:parseType="Collection">
          <glview:MeasurementType rdf:about="http://schema.geolink.org/dev/voc/nvs/P02#SSTR"/>
        </owl:oneOf>
      </owl:Class>
    </owl:someValuesFrom>
    <owl:onProperty rdf:resource="http://schema.geolink.org/dev/view#hasMeasurementType"/>
  </owl:Restriction>
  <owl:Restriction>
    <rdfs:subClassOf rdf:resource="http://schema.geolink.org/dev/voc/nvs/P02#FATX"/>
    <owl:someValuesFrom>
      <owl:Class>
        <owl:oneOf rdf:parseType="Collection">
          <glview:MeasurementType rdf:about="http://schema.geolink.org/dev/voc/nvs/P02#FATX"/>
        </owl:oneOf>
      </owl:Class>
    </owl:someValuesFrom>
    <owl:onProperty rdf:resource="http://schema.geolink.org/dev/view#hasMeasurementType"/>
  </owl:Restriction>
  <owl:Restriction>
    <rdfs:subClassOf>
      <glview:MeasurementType rdf:about="http://schema.geolink.org/dev/voc/nvs/P02#BEST">
        <rdfs:subClassOf rdf:resource="http://schema.geolink.org/dev/voc/nvs/P03#G060"/>
        <rdfs:seeAlso rdf:resource="http://vocab.nerc.ac.uk/collection/P02/current/BEST/"/>
        <rdfs:comment xml:lang="en">Parameters quantifying the critera for and extent of sediment resuspension</rdfs:comment>
        <rdfs:label xml:lang="en">Sediment resuspension</rdfs:label>
        <rdf:type rdf:resource="http://www.w3.org/2002/07/owl#NamedIndividual"/>
        <rdf:type rdf:resource="http://www.w3.org/2002/07/owl#Class"/>
      </glview:MeasurementType>
    </rdfs:subClassOf>
    <owl:someValuesFrom>
      <owl:Class>
        <owl:oneOf rdf:parseType="Collection">
          <glview:MeasurementType rdf:about="http://schema.geolink.org/dev/voc/nvs/P02#BEST"/>
        </owl:oneOf>
      </owl:Class>
    </owl:someValuesFrom>
    <owl:onProperty rdf:resource="http://schema.geolink.org/dev/view#hasMeasurementType"/>
  </owl:Restriction>
  <owl:Restriction>
    <rdfs:subClassOf rdf:resource="http://schema.geolink.org/dev/voc/nvs/P02#MFWW"/>
    <owl:someValuesFrom>
      <owl:Class>
        <owl:oneOf rdf:parseType="Collection">
          <glview:MeasurementType rdf:about="http://schema.geolink.org/dev/voc/nvs/P02#MFWW"/>
        </owl:oneOf>
      </owl:Class>
    </owl:someValuesFrom>
    <owl:onProperty rdf:resource="http://schema.geolink.org/dev/view#hasMeasurementType"/>
  </owl:Restriction>
  <owl:Restriction>
    <rdfs:subClassOf>
      <glview:MeasurementType rdf:about="http://schema.geolink.org/dev/voc/nvs/P02#STCO">
        <rdfs:subClassOf rdf:resource="http://schema.geolink.org/dev/voc/nvs/P03#GTHM"/>
        <rdfs:subClassOf rdf:resource="http://schema.geolink.org/dev/voc/nvs/P03#G040"/>
        <rdfs:seeAlso rdf:resource="http://vocab.nerc.ac.uk/collection/P02/current/STCO/"/>
        <rdfs:comment xml:lang="en">Parameters that describe the degree to which unlithified sediment is able to conduct heat</rdfs:comment>
        <rdfs:label xml:lang="en">Sediment thermal conductivity</rdfs:label>
        <rdf:type rdf:resource="http://www.w3.org/2002/07/owl#NamedIndividual"/>
        <rdf:type rdf:resource="http://www.w3.org/2002/07/owl#Class"/>
      </glview:MeasurementType>
    </rdfs:subClassOf>
    <owl:someValuesFrom>
      <owl:Class>
        <owl:oneOf rdf:parseType="Collection">
          <glview:MeasurementType rdf:about="http://schema.geolink.org/dev/voc/nvs/P02#STCO"/>
        </owl:oneOf>
      </owl:Class>
    </owl:someValuesFrom>
    <owl:onProperty rdf:resource="http://schema.geolink.org/dev/view#hasMeasurementType"/>
  </owl:Restriction>
  <owl:Restriction>
    <rdfs:subClassOf>
      <glview:MeasurementType rdf:about="http://schema.geolink.org/dev/voc/nvs/P02#CAKN">
        <rdfs:subClassOf rdf:resource="http://schema.geolink.org/dev/voc/nvs/P03#C050"/>
        <rdfs:seeAlso rdf:resource="http://vocab.nerc.ac.uk/collection/P02/current/CAKN/"/>
        <rdfs:comment xml:lang="en">Concentrations of alkenones (unsaturated aliphatic ketones) and alkenoates (carboxylic acid esters) in all phases of the water column.</rdfs:comment>
        <rdfs:label xml:lang="en">Concentration of alkenones and alkenoates in the water column</rdfs:label>
        <rdf:type rdf:resource="http://www.w3.org/2002/07/owl#NamedIndividual"/>
        <rdf:type rdf:resource="http://www.w3.org/2002/07/owl#Class"/>
      </glview:MeasurementType>
    </rdfs:subClassOf>
    <owl:someValuesFrom>
      <owl:Class>
        <owl:oneOf rdf:parseType="Collection">
          <glview:MeasurementType rdf:about="http://schema.geolink.org/dev/voc/nvs/P02#CAKN"/>
        </owl:oneOf>
      </owl:Class>
    </owl:someValuesFrom>
    <owl:onProperty rdf:resource="http://schema.geolink.org/dev/view#hasMeasurementType"/>
  </owl:Restriction>
  <owl:Restriction>
    <rdfs:subClassOf>
      <glview:MeasurementType rdf:about="http://schema.geolink.org/dev/voc/nvs/P02#CSLR">
        <rdfs:subClassOf rdf:resource="http://schema.geolink.org/dev/voc/nvs/P03#M010"/>
        <rdfs:seeAlso rdf:resource="http://vocab.nerc.ac.uk/collection/P02/current/CSLR/"/>
        <rdfs:comment xml:lang="en">Parameters quantifying the irradiance of the sun impinging on the Earth's surface in the visible and infra-red waveband, generally accepted as wavelengths between 300 and 3000 nm</rdfs:comment>
        <rdfs:label xml:lang="en">Solar Radiation</rdfs:label>
        <rdf:type rdf:resource="http://www.w3.org/2002/07/owl#NamedIndividual"/>
        <rdf:type rdf:resource="http://www.w3.org/2002/07/owl#Class"/>
      </glview:MeasurementType>
    </rdfs:subClassOf>
    <owl:someValuesFrom>
      <owl:Class>
        <owl:oneOf rdf:parseType="Collection">
          <glview:MeasurementType rdf:about="http://schema.geolink.org/dev/voc/nvs/P02#CSLR"/>
        </owl:oneOf>
      </owl:Class>
    </owl:someValuesFrom>
    <owl:onProperty rdf:resource="http://schema.geolink.org/dev/view#hasMeasurementType"/>
  </owl:Restriction>
  <owl:Restriction>
    <rdfs:subClassOf>
      <glview:MeasurementType rdf:about="http://schema.geolink.org/dev/voc/nvs/P02#PSST">
        <rdfs:subClassOf rdf:resource="http://schema.geolink.org/dev/voc/nvs/P03#D025"/>
        <rdfs:seeAlso rdf:resource="http://vocab.nerc.ac.uk/collection/P02/current/PSST/"/>
        <rdfs:comment xml:lang="en">Temperature of the water column surface as measured by a radiometer.  It does NOT include temperature measurements in the upper few metres of the water column such as thermosalinograph data</rdfs:comment>
        <rdfs:label xml:lang="en">Skin temperature of the water column</rdfs:label>
        <rdf:type rdf:resource="http://www.w3.org/2002/07/owl#NamedIndividual"/>
        <rdf:type rdf:resource="http://www.w3.org/2002/07/owl#Class"/>
      </glview:MeasurementType>
    </rdfs:subClassOf>
    <owl:someValuesFrom>
      <owl:Class>
        <owl:oneOf rdf:parseType="Collection">
          <glview:MeasurementType rdf:about="http://schema.geolink.org/dev/voc/nvs/P02#PSST"/>
        </owl:oneOf>
      </owl:Class>
    </owl:someValuesFrom>
    <owl:onProperty rdf:resource="http://schema.geolink.org/dev/view#hasMeasurementType"/>
  </owl:Restriction>
  <owl:Restriction>
    <rdfs:subClassOf rdf:resource="http://schema.geolink.org/dev/voc/nvs/P02#BNUC"/>
    <owl:someValuesFrom>
      <owl:Class>
        <owl:oneOf rdf:parseType="Collection">
          <glview:MeasurementType rdf:about="http://schema.geolink.org/dev/voc/nvs/P02#BNUC"/>
        </owl:oneOf>
      </owl:Class>
    </owl:someValuesFrom>
    <owl:onProperty rdf:resource="http://schema.geolink.org/dev/view#hasMeasurementType"/>
  </owl:Restriction>
  <owl:Restriction>
    <rdfs:subClassOf rdf:resource="http://schema.geolink.org/dev/voc/nvs/P02#SCAH"/>
    <owl:someValuesFrom>
      <owl:Class>
        <owl:oneOf rdf:parseType="Collection">
          <glview:MeasurementType rdf:about="http://schema.geolink.org/dev/voc/nvs/P02#SCAH"/>
        </owl:oneOf>
      </owl:Class>
    </owl:someValuesFrom>
    <owl:onProperty rdf:resource="http://schema.geolink.org/dev/view#hasMeasurementType"/>
  </owl:Restriction>
  <owl:Restriction>
    <rdfs:subClassOf>
      <glview:MeasurementType rdf:about="http://schema.geolink.org/dev/voc/nvs/P02#A01X">
        <rdfs:subClassOf rdf:resource="http://schema.geolink.org/dev/voc/nvs/P03#O005"/>
        <rdfs:seeAlso rdf:resource="http://vocab.nerc.ac.uk/collection/P02/current/A01X/"/>
        <rdfs:comment xml:lang="en">Parameters quantifying the rate of alkenones (unsaturated aliphatic ketones) and alkenoates (carboxylic acid esters) sinking as particles through any body of water.</rdfs:comment>
        <rdfs:label xml:lang="en">Sedimentation flux of alkenones and alkenoates in the water column</rdfs:label>
        <rdf:type rdf:resource="http://www.w3.org/2002/07/owl#NamedIndividual"/>
        <rdf:type rdf:resource="http://www.w3.org/2002/07/owl#Class"/>
      </glview:MeasurementType>
    </rdfs:subClassOf>
    <owl:someValuesFrom>
      <owl:Class>
        <owl:oneOf rdf:parseType="Collection">
          <glview:MeasurementType rdf:about="http://schema.geolink.org/dev/voc/nvs/P02#A01X"/>
        </owl:oneOf>
      </owl:Class>
    </owl:someValuesFrom>
    <owl:onProperty rdf:resource="http://schema.geolink.org/dev/view#hasMeasurementType"/>
  </owl:Restriction>
  <owl:Restriction>
    <rdfs:subClassOf rdf:resource="http://schema.geolink.org/dev/voc/nvs/P02#BCPB"/>
    <owl:someValuesFrom>
      <owl:Class>
        <owl:oneOf rdf:parseType="Collection">
          <glview:MeasurementType rdf:about="http://schema.geolink.org/dev/voc/nvs/P02#BCPB"/>
        </owl:oneOf>
      </owl:Class>
    </owl:someValuesFrom>
    <owl:onProperty rdf:resource="http://schema.geolink.org/dev/view#hasMeasurementType"/>
  </owl:Restriction>
  <owl:Restriction>
    <rdfs:subClassOf>
      <glview:MeasurementType rdf:about="http://schema.geolink.org/dev/voc/nvs/P02#SSCN">
        <rdfs:subClassOf rdf:resource="http://schema.geolink.org/dev/voc/nvs/P03#G012"/>
        <rdfs:seeAlso rdf:resource="http://vocab.nerc.ac.uk/collection/P02/current/SSCN/"/>
        <rdfs:comment xml:lang="en">A technique for mapping the morphology of the seafloor using a sonar swath projected sideways from a towed underwater vehicle.</rdfs:comment>
        <rdfs:label xml:lang="en">Side-scan sonar</rdfs:label>
        <rdf:type rdf:resource="http://www.w3.org/2002/07/owl#NamedIndividual"/>
        <rdf:type rdf:resource="http://www.w3.org/2002/07/owl#Class"/>
      </glview:MeasurementType>
    </rdfs:subClassOf>
    <owl:someValuesFrom>
      <owl:Class>
        <owl:oneOf rdf:parseType="Collection">
          <glview:MeasurementType rdf:about="http://schema.geolink.org/dev/voc/nvs/P02#SSCN"/>
        </owl:oneOf>
      </owl:Class>
    </owl:someValuesFrom>
    <owl:onProperty rdf:resource="http://schema.geolink.org/dev/view#hasMeasurementType"/>
  </owl:Restriction>
  <owl:Restriction>
    <rdfs:subClassOf>
      <glview:MeasurementType rdf:about="http://schema.geolink.org/dev/voc/nvs/P02#CA11">
        <rdfs:subClassOf rdf:resource="http://schema.geolink.org/dev/voc/nvs/P02#CASD"/>
        <rdfs:seeAlso rdf:resource="http://vocab.nerc.ac.uk/collection/P02/current/CA11/"/>
        <rdfs:comment xml:lang="en">Concentration of alkanols, phenols and ethers per unit mass or unit volume of sediment (material collected by a corer including fluff)</rdfs:comment>
        <rdfs:label xml:lang="en">Concentration of alkanols (alcohols), phenols and ethers in sediment</rdfs:label>
        <rdf:type rdf:resource="http://www.w3.org/2002/07/owl#NamedIndividual"/>
        <rdf:type rdf:resource="http://www.w3.org/2002/07/owl#Class"/>
      </glview:MeasurementType>
    </rdfs:subClassOf>
    <owl:someValuesFrom>
      <owl:Class>
        <owl:oneOf rdf:parseType="Collection">
          <glview:MeasurementType rdf:about="http://schema.geolink.org/dev/voc/nvs/P02#CA11"/>
        </owl:oneOf>
      </owl:Class>
    </owl:someValuesFrom>
    <owl:onProperty rdf:resource="http://schema.geolink.org/dev/view#hasMeasurementType"/>
  </owl:Restriction>
  <owl:Restriction>
    <rdfs:subClassOf>
      <glview:MeasurementType rdf:about="http://schema.geolink.org/dev/voc/nvs/P02#IRIC">
        <rdfs:subClassOf rdf:resource="http://schema.geolink.org/dev/voc/nvs/P02#ICHM"/>
        <rdfs:seeAlso rdf:resource="http://vocab.nerc.ac.uk/collection/P02/current/IRIC/"/>
        <rdfs:comment xml:lang="en">Stable isotope enrichment parameters in frozen precipitation (snow, hail, ice and slush), its accumulations (e.g. glaciers), sea ice and frozen fresh water.</rdfs:comment>
        <rdfs:label xml:lang="en">Stable isotope enrichment in ice and snow</rdfs:label>
        <rdf:type rdf:resource="http://www.w3.org/2002/07/owl#NamedIndividual"/>
        <rdf:type rdf:resource="http://www.w3.org/2002/07/owl#Class"/>
      </glview:MeasurementType>
    </rdfs:subClassOf>
    <owl:someValuesFrom>
      <owl:Class>
        <owl:oneOf rdf:parseType="Collection">
          <glview:MeasurementType rdf:about="http://schema.geolink.org/dev/voc/nvs/P02#IRIC"/>
        </owl:oneOf>
      </owl:Class>
    </owl:someValuesFrom>
    <owl:onProperty rdf:resource="http://schema.geolink.org/dev/view#hasMeasurementType"/>
  </owl:Restriction>
  <owl:Restriction>
    <rdfs:subClassOf>
      <glview:MeasurementType rdf:about="http://schema.geolink.org/dev/voc/nvs/P02#ZCMP">
        <rdfs:subClassOf rdf:resource="http://schema.geolink.org/dev/voc/nvs/P03#B045"/>
        <rdfs:seeAlso rdf:resource="http://vocab.nerc.ac.uk/collection/P02/current/ZCMP/"/>
        <rdfs:comment xml:lang="en">Chemical composition of zooplankton expressed in terms of mass (or molar quantity) per specimen or per unit tissue mass</rdfs:comment>
        <rdfs:label xml:lang="en">Zooplankton chemical composition</rdfs:label>
        <rdf:type rdf:resource="http://www.w3.org/2002/07/owl#NamedIndividual"/>
        <rdf:type rdf:resource="http://www.w3.org/2002/07/owl#Class"/>
      </glview:MeasurementType>
    </rdfs:subClassOf>
    <owl:someValuesFrom>
      <owl:Class>
        <owl:oneOf rdf:parseType="Collection">
          <glview:MeasurementType rdf:about="http://schema.geolink.org/dev/voc/nvs/P02#ZCMP"/>
        </owl:oneOf>
      </owl:Class>
    </owl:someValuesFrom>
    <owl:onProperty rdf:resource="http://schema.geolink.org/dev/view#hasMeasurementType"/>
  </owl:Restriction>
  <owl:Restriction>
    <rdfs:subClassOf rdf:resource="http://schema.geolink.org/dev/voc/nvs/P02#ZBTX"/>
    <owl:someValuesFrom>
      <owl:Class>
        <owl:oneOf rdf:parseType="Collection">
          <glview:MeasurementType rdf:about="http://schema.geolink.org/dev/voc/nvs/P02#ZBTX"/>
        </owl:oneOf>
      </owl:Class>
    </owl:someValuesFrom>
    <owl:onProperty rdf:resource="http://schema.geolink.org/dev/view#hasMeasurementType"/>
  </owl:Restriction>
  <owl:Restriction>
    <rdfs:subClassOf rdf:resource="http://schema.geolink.org/dev/voc/nvs/P02#PHUP"/>
    <owl:someValuesFrom>
      <owl:Class>
        <owl:oneOf rdf:parseType="Collection">
          <glview:MeasurementType rdf:about="http://schema.geolink.org/dev/voc/nvs/P02#PHUP"/>
        </owl:oneOf>
      </owl:Class>
    </owl:someValuesFrom>
    <owl:onProperty rdf:resource="http://schema.geolink.org/dev/view#hasMeasurementType"/>
  </owl:Restriction>
  <owl:Restriction>
    <rdfs:subClassOf>
      <glview:MeasurementType rdf:about="http://schema.geolink.org/dev/voc/nvs/P02#D000">
        <rdfs:subClassOf rdf:resource="http://schema.geolink.org/dev/voc/nvs/P03#B030"/>
        <rdfs:subClassOf rdf:resource="http://schema.geolink.org/dev/voc/nvs/P03#B070"/>
        <rdfs:seeAlso rdf:resource="http://vocab.nerc.ac.uk/collection/P02/current/D000/"/>
        <rdfs:comment xml:lang="en">Determinations of the abundance of diatom remains in sediment linked to taxonomic identifications that may be mapped to entities in the ITIS taxonomy.  These may be at any taxonomic level from sub-species upwards</rdfs:comment>
        <rdfs:label xml:lang="en">Diatom taxonomy-related abundance per unit mass of sediment</rdfs:label>
        <rdf:type rdf:resource="http://www.w3.org/2002/07/owl#NamedIndividual"/>
        <rdf:type rdf:resource="http://www.w3.org/2002/07/owl#Class"/>
      </glview:MeasurementType>
    </rdfs:subClassOf>
    <owl:someValuesFrom>
      <owl:Class>
        <owl:oneOf rdf:parseType="Collection">
          <glview:MeasurementType rdf:about="http://schema.geolink.org/dev/voc/nvs/P02#D000"/>
        </owl:oneOf>
      </owl:Class>
    </owl:someValuesFrom>
    <owl:onProperty rdf:resource="http://schema.geolink.org/dev/view#hasMeasurementType"/>
  </owl:Restriction>
  <owl:Restriction>
    <rdfs:subClassOf rdf:resource="http://schema.geolink.org/dev/voc/nvs/P02#SCAH"/>
    <owl:someValuesFrom>
      <owl:Class>
        <owl:oneOf rdf:parseType="Collection">
          <glview:MeasurementType rdf:about="http://schema.geolink.org/dev/voc/nvs/P02#SCAH"/>
        </owl:oneOf>
      </owl:Class>
    </owl:someValuesFrom>
    <owl:onProperty rdf:resource="http://schema.geolink.org/dev/view#hasMeasurementType"/>
  </owl:Restriction>
  <owl:Restriction>
    <rdfs:subClassOf>
      <glview:MeasurementType rdf:about="http://schema.geolink.org/dev/voc/nvs/P02#LWET">
        <rdfs:subClassOf rdf:resource="http://schema.geolink.org/dev/voc/nvs/P03#T001"/>
        <rdfs:seeAlso rdf:resource="http://vocab.nerc.ac.uk/collection/P02/current/LWET/"/>
        <rdfs:comment xml:lang="en">Parameters relating to the water held by land masses such as soil and vegetation moisture content</rdfs:comment>
        <rdfs:label xml:lang="en">Terrestrial water content</rdfs:label>
        <rdf:type rdf:resource="http://www.w3.org/2002/07/owl#NamedIndividual"/>
        <rdf:type rdf:resource="http://www.w3.org/2002/07/owl#Class"/>
      </glview:MeasurementType>
    </rdfs:subClassOf>
    <owl:someValuesFrom>
      <owl:Class>
        <owl:oneOf rdf:parseType="Collection">
          <glview:MeasurementType rdf:about="http://schema.geolink.org/dev/voc/nvs/P02#LWET"/>
        </owl:oneOf>
      </owl:Class>
    </owl:someValuesFrom>
    <owl:onProperty rdf:resource="http://schema.geolink.org/dev/view#hasMeasurementType"/>
  </owl:Restriction>
  <owl:Restriction>
    <rdfs:subClassOf rdf:resource="http://schema.geolink.org/dev/voc/nvs/P02#IRBO"/>
    <owl:someValuesFrom>
      <owl:Class>
        <owl:oneOf rdf:parseType="Collection">
          <glview:MeasurementType rdf:about="http://schema.geolink.org/dev/voc/nvs/P02#IRBO"/>
        </owl:oneOf>
      </owl:Class>
    </owl:someValuesFrom>
    <owl:onProperty rdf:resource="http://schema.geolink.org/dev/view#hasMeasurementType"/>
  </owl:Restriction>
  <owl:Restriction>
    <rdfs:subClassOf rdf:resource="http://schema.geolink.org/dev/voc/nvs/P02#SUAT"/>
    <owl:someValuesFrom>
      <owl:Class>
        <owl:oneOf rdf:parseType="Collection">
          <glview:MeasurementType rdf:about="http://schema.geolink.org/dev/voc/nvs/P02#SUAT"/>
        </owl:oneOf>
      </owl:Class>
    </owl:someValuesFrom>
    <owl:onProperty rdf:resource="http://schema.geolink.org/dev/view#hasMeasurementType"/>
  </owl:Restriction>
  <owl:Restriction>
    <rdfs:subClassOf rdf:resource="http://schema.geolink.org/dev/voc/nvs/P02#SATM"/>
    <owl:someValuesFrom>
      <owl:Class>
        <owl:oneOf rdf:parseType="Collection">
          <glview:MeasurementType rdf:about="http://schema.geolink.org/dev/voc/nvs/P02#SATM"/>
        </owl:oneOf>
      </owl:Class>
    </owl:someValuesFrom>
    <owl:onProperty rdf:resource="http://schema.geolink.org/dev/view#hasMeasurementType"/>
  </owl:Restriction>
  <owl:Restriction>
    <rdfs:subClassOf>
      <glview:MeasurementType rdf:about="http://schema.geolink.org/dev/voc/nvs/P02#PEBI">
        <rdfs:subClassOf rdf:resource="http://schema.geolink.org/dev/voc/nvs/P03#C055"/>
        <rdfs:subClassOf rdf:resource="http://schema.geolink.org/dev/voc/nvs/P03#B007"/>
        <rdfs:subClassOf rdf:resource="http://schema.geolink.org/dev/voc/nvs/P03#H001"/>
        <rdfs:seeAlso rdf:resource="http://vocab.nerc.ac.uk/collection/P02/current/PEBI/"/>
        <rdfs:comment xml:lang="en">Concentration parameters for substances synthesised by man to kill other life forms in either whole organisms or their constituent parts.</rdfs:comment>
        <rdfs:label xml:lang="en">Pesticide concentrations in biota</rdfs:label>
        <rdf:type rdf:resource="http://www.w3.org/2002/07/owl#NamedIndividual"/>
        <rdf:type rdf:resource="http://www.w3.org/2002/07/owl#Class"/>
      </glview:MeasurementType>
    </rdfs:subClassOf>
    <owl:someValuesFrom>
      <owl:Class>
        <owl:oneOf rdf:parseType="Collection">
          <glview:MeasurementType rdf:about="http://schema.geolink.org/dev/voc/nvs/P02#PEBI"/>
        </owl:oneOf>
      </owl:Class>
    </owl:someValuesFrom>
    <owl:onProperty rdf:resource="http://schema.geolink.org/dev/view#hasMeasurementType"/>
  </owl:Restriction>
  <owl:Restriction>
    <rdfs:subClassOf>
      <glview:MeasurementType rdf:about="http://schema.geolink.org/dev/voc/nvs/P02#HLAT">
        <rdfs:subClassOf rdf:resource="http://schema.geolink.org/dev/voc/nvs/P03#C045"/>
        <rdfs:subClassOf rdf:resource="http://schema.geolink.org/dev/voc/nvs/P03#M005"/>
        <rdfs:seeAlso rdf:resource="http://vocab.nerc.ac.uk/collection/P02/current/HLAT/"/>
        <rdfs:comment xml:lang="en">Concentrations of halogens as elements or their inorganic compounds in all phases of the atmosphere.</rdfs:comment>
        <rdfs:label xml:lang="en">Concentration of inorganic halogens in the atmosphere</rdfs:label>
        <rdf:type rdf:resource="http://www.w3.org/2002/07/owl#NamedIndividual"/>
        <rdf:type rdf:resource="http://www.w3.org/2002/07/owl#Class"/>
      </glview:MeasurementType>
    </rdfs:subClassOf>
    <owl:someValuesFrom>
      <owl:Class>
        <owl:oneOf rdf:parseType="Collection">
          <glview:MeasurementType rdf:about="http://schema.geolink.org/dev/voc/nvs/P02#HLAT"/>
        </owl:oneOf>
      </owl:Class>
    </owl:someValuesFrom>
    <owl:onProperty rdf:resource="http://schema.geolink.org/dev/view#hasMeasurementType"/>
  </owl:Restriction>
  <owl:Restriction>
    <rdfs:subClassOf rdf:resource="http://schema.geolink.org/dev/voc/nvs/P02#GPIG"/>
    <owl:someValuesFrom>
      <owl:Class>
        <owl:oneOf rdf:parseType="Collection">
          <glview:MeasurementType rdf:about="http://schema.geolink.org/dev/voc/nvs/P02#GPIG"/>
        </owl:oneOf>
      </owl:Class>
    </owl:someValuesFrom>
    <owl:onProperty rdf:resource="http://schema.geolink.org/dev/view#hasMeasurementType"/>
  </owl:Restriction>
  <owl:Restriction>
    <rdfs:subClassOf rdf:resource="http://schema.geolink.org/dev/voc/nvs/P02#SPCB"/>
    <owl:someValuesFrom>
      <owl:Class>
        <owl:oneOf rdf:parseType="Collection">
          <glview:MeasurementType rdf:about="http://schema.geolink.org/dev/voc/nvs/P02#SPCB"/>
        </owl:oneOf>
      </owl:Class>
    </owl:someValuesFrom>
    <owl:onProperty rdf:resource="http://schema.geolink.org/dev/view#hasMeasurementType"/>
  </owl:Restriction>
  <owl:Restriction>
    <rdfs:subClassOf>
      <glview:MeasurementType rdf:about="http://schema.geolink.org/dev/voc/nvs/P02#SPWC">
        <rdfs:subClassOf rdf:resource="http://schema.geolink.org/dev/voc/nvs/P03#C045"/>
        <rdfs:seeAlso rdf:resource="http://vocab.nerc.ac.uk/collection/P02/current/SPWC/"/>
        <rdfs:comment xml:lang="en">Concentration parameters (including saturation if gaseous) for inorganic sulphur species in all phases of the water column</rdfs:comment>
        <rdfs:label xml:lang="en">Concentration of inorganic sulphur species in the water column</rdfs:label>
        <rdf:type rdf:resource="http://www.w3.org/2002/07/owl#NamedIndividual"/>
        <rdf:type rdf:resource="http://www.w3.org/2002/07/owl#Class"/>
      </glview:MeasurementType>
    </rdfs:subClassOf>
    <owl:someValuesFrom>
      <owl:Class>
        <owl:oneOf rdf:parseType="Collection">
          <glview:MeasurementType rdf:about="http://schema.geolink.org/dev/voc/nvs/P02#SPWC"/>
        </owl:oneOf>
      </owl:Class>
    </owl:someValuesFrom>
    <owl:onProperty rdf:resource="http://schema.geolink.org/dev/view#hasMeasurementType"/>
  </owl:Restriction>
  <owl:Restriction>
    <rdfs:subClassOf rdf:resource="http://schema.geolink.org/dev/voc/nvs/P02#IATC"/>
    <owl:someValuesFrom>
      <owl:Class>
        <owl:oneOf rdf:parseType="Collection">
          <glview:MeasurementType rdf:about="http://schema.geolink.org/dev/voc/nvs/P02#IATC"/>
        </owl:oneOf>
      </owl:Class>
    </owl:someValuesFrom>
    <owl:onProperty rdf:resource="http://schema.geolink.org/dev/view#hasMeasurementType"/>
  </owl:Restriction>
  <owl:Restriction>
    <rdfs:subClassOf rdf:resource="http://schema.geolink.org/dev/voc/nvs/P02#FREP"/>
    <owl:someValuesFrom>
      <owl:Class>
        <owl:oneOf rdf:parseType="Collection">
          <glview:MeasurementType rdf:about="http://schema.geolink.org/dev/voc/nvs/P02#FREP"/>
        </owl:oneOf>
      </owl:Class>
    </owl:someValuesFrom>
    <owl:onProperty rdf:resource="http://schema.geolink.org/dev/view#hasMeasurementType"/>
  </owl:Restriction>
  <owl:Restriction>
    <rdfs:subClassOf>
      <glview:MeasurementType rdf:about="http://schema.geolink.org/dev/voc/nvs/P02#GP067">
        <rdfs:subClassOf rdf:resource="http://schema.geolink.org/dev/voc/nvs/P03#B060"/>
        <rdfs:subClassOf rdf:resource="http://schema.geolink.org/dev/voc/nvs/P03#B015"/>
        <rdfs:seeAlso rdf:resource="http://vocab.nerc.ac.uk/collection/P02/current/GP067/"/>
        <rdfs:comment xml:lang="en">Parameters relating to diseases and parasites of reptiles (Class Reptilia)</rdfs:comment>
        <rdfs:label xml:lang="en">Reptile disease and parasites</rdfs:label>
        <rdf:type rdf:resource="http://www.w3.org/2002/07/owl#NamedIndividual"/>
        <rdf:type rdf:resource="http://www.w3.org/2002/07/owl#Class"/>
      </glview:MeasurementType>
    </rdfs:subClassOf>
    <owl:someValuesFrom>
      <owl:Class>
        <owl:oneOf rdf:parseType="Collection">
          <glview:MeasurementType rdf:about="http://schema.geolink.org/dev/voc/nvs/P02#GP067"/>
        </owl:oneOf>
      </owl:Class>
    </owl:someValuesFrom>
    <owl:onProperty rdf:resource="http://schema.geolink.org/dev/view#hasMeasurementType"/>
  </owl:Restriction>
  <owl:Restriction>
    <rdfs:subClassOf>
      <glview:MeasurementType rdf:about="http://schema.geolink.org/dev/voc/nvs/P02#SAMO">
        <rdfs:subClassOf rdf:resource="http://schema.geolink.org/dev/voc/nvs/P03#O005"/>
        <rdfs:subClassOf rdf:resource="http://schema.geolink.org/dev/voc/nvs/P03#C040"/>
        <rdfs:seeAlso rdf:resource="http://vocab.nerc.ac.uk/collection/P02/current/SAMO/"/>
        <rdfs:comment xml:lang="en">Parameters quantifying the exchange of nutrients between the bed (ie the sediment) and the water column sometimes termed benthic fluxes</rdfs:comment>
        <rdfs:label xml:lang="en">Nutrient fluxes between the bed and the water column</rdfs:label>
        <rdf:type rdf:resource="http://www.w3.org/2002/07/owl#NamedIndividual"/>
        <rdf:type rdf:resource="http://www.w3.org/2002/07/owl#Class"/>
      </glview:MeasurementType>
    </rdfs:subClassOf>
    <owl:someValuesFrom>
      <owl:Class>
        <owl:oneOf rdf:parseType="Collection">
          <glview:MeasurementType rdf:about="http://schema.geolink.org/dev/voc/nvs/P02#SAMO"/>
        </owl:oneOf>
      </owl:Class>
    </owl:someValuesFrom>
    <owl:onProperty rdf:resource="http://schema.geolink.org/dev/view#hasMeasurementType"/>
  </owl:Restriction>
  <owl:Restriction>
    <rdfs:subClassOf rdf:resource="http://schema.geolink.org/dev/voc/nvs/P02#BLEN"/>
    <owl:someValuesFrom>
      <owl:Class>
        <owl:oneOf rdf:parseType="Collection">
          <glview:MeasurementType rdf:about="http://schema.geolink.org/dev/voc/nvs/P02#BLEN"/>
        </owl:oneOf>
      </owl:Class>
    </owl:someValuesFrom>
    <owl:onProperty rdf:resource="http://schema.geolink.org/dev/view#hasMeasurementType"/>
  </owl:Restriction>
  <owl:Restriction>
    <rdfs:subClassOf rdf:resource="http://schema.geolink.org/dev/voc/nvs/P02#ATEM"/>
    <owl:someValuesFrom>
      <owl:Class>
        <owl:oneOf rdf:parseType="Collection">
          <glview:MeasurementType rdf:about="http://schema.geolink.org/dev/voc/nvs/P02#ATEM"/>
        </owl:oneOf>
      </owl:Class>
    </owl:someValuesFrom>
    <owl:onProperty rdf:resource="http://schema.geolink.org/dev/view#hasMeasurementType"/>
  </owl:Restriction>
  <owl:Restriction>
    <rdfs:subClassOf>
      <glview:MeasurementType rdf:about="http://schema.geolink.org/dev/voc/nvs/P02#GHDX">
        <rdfs:subClassOf rdf:resource="http://schema.geolink.org/dev/voc/nvs/P03#G055"/>
        <rdfs:seeAlso rdf:resource="http://vocab.nerc.ac.uk/collection/P02/current/GHDX/"/>
        <rdfs:comment xml:lang="en">Parameters relating to the size, shape and form of microfossils in sediment samples</rdfs:comment>
        <rdfs:label xml:lang="en">Sediment microfossil morphology parameters</rdfs:label>
        <rdf:type rdf:resource="http://www.w3.org/2002/07/owl#NamedIndividual"/>
        <rdf:type rdf:resource="http://www.w3.org/2002/07/owl#Class"/>
      </glview:MeasurementType>
    </rdfs:subClassOf>
    <owl:someValuesFrom>
      <owl:Class>
        <owl:oneOf rdf:parseType="Collection">
          <glview:MeasurementType rdf:about="http://schema.geolink.org/dev/voc/nvs/P02#GHDX"/>
        </owl:oneOf>
      </owl:Class>
    </owl:someValuesFrom>
    <owl:onProperty rdf:resource="http://schema.geolink.org/dev/view#hasMeasurementType"/>
  </owl:Restriction>
  <owl:Restriction>
    <rdfs:subClassOf>
      <glview:MeasurementType rdf:about="http://schema.geolink.org/dev/voc/nvs/P02#SACT">
        <rdfs:subClassOf rdf:resource="http://schema.geolink.org/dev/voc/nvs/P03#C050"/>
        <rdfs:seeAlso rdf:resource="http://vocab.nerc.ac.uk/collection/P02/current/SACT/"/>
        <rdfs:comment xml:lang="en">Parameters quantifying the amount of compounds that lower the surface tension of a liquid, the interfacial tension between two liquids, or that between a liquid and a solid in any body of salt or fresh water. The term surfactants includes detergents, wetting agents, emulsifiers, foaming agents and dispersants.</rdfs:comment>
        <rdfs:label xml:lang="en">Surfactant concentrations in water bodies</rdfs:label>
        <rdf:type rdf:resource="http://www.w3.org/2002/07/owl#NamedIndividual"/>
        <rdf:type rdf:resource="http://www.w3.org/2002/07/owl#Class"/>
      </glview:MeasurementType>
    </rdfs:subClassOf>
    <owl:someValuesFrom>
      <owl:Class>
        <owl:oneOf rdf:parseType="Collection">
          <glview:MeasurementType rdf:about="http://schema.geolink.org/dev/voc/nvs/P02#SACT"/>
        </owl:oneOf>
      </owl:Class>
    </owl:someValuesFrom>
    <owl:onProperty rdf:resource="http://schema.geolink.org/dev/view#hasMeasurementType"/>
  </owl:Restriction>
  <owl:Restriction>
    <rdfs:subClassOf>
      <glview:MeasurementType rdf:about="http://schema.geolink.org/dev/voc/nvs/P02#UVRD">
        <rdfs:subClassOf rdf:resource="http://schema.geolink.org/dev/voc/nvs/P03#M010"/>
        <rdfs:seeAlso rdf:resource="http://vocab.nerc.ac.uk/collection/P02/current/UVRD/"/>
        <rdfs:comment xml:lang="en">Parameters relating to the intensity of ultra-violet radiation in either the atmosphere or the water column</rdfs:comment>
        <rdfs:label xml:lang="en">Ultra-violet (UV) radiation</rdfs:label>
        <rdf:type rdf:resource="http://www.w3.org/2002/07/owl#NamedIndividual"/>
        <rdf:type rdf:resource="http://www.w3.org/2002/07/owl#Class"/>
      </glview:MeasurementType>
    </rdfs:subClassOf>
    <owl:someValuesFrom>
      <owl:Class>
        <owl:oneOf rdf:parseType="Collection">
          <glview:MeasurementType rdf:about="http://schema.geolink.org/dev/voc/nvs/P02#UVRD"/>
        </owl:oneOf>
      </owl:Class>
    </owl:someValuesFrom>
    <owl:onProperty rdf:resource="http://schema.geolink.org/dev/view#hasMeasurementType"/>
  </owl:Restriction>
  <owl:Restriction>
    <rdfs:subClassOf>
      <glview:MeasurementType rdf:about="http://schema.geolink.org/dev/voc/nvs/P02#GP001">
        <rdfs:subClassOf rdf:resource="http://schema.geolink.org/dev/voc/nvs/P03#H001"/>
        <rdfs:seeAlso rdf:resource="http://vocab.nerc.ac.uk/collection/P02/current/GP001/"/>
        <rdfs:comment xml:lang="en">Parameters quantifying the accidental spillage of liquid or dry pollutants from vessels or marine industries. Parameters may include quantities of pollutant, areas affected and event duration.</rdfs:comment>
        <rdfs:label xml:lang="en">Pollution events</rdfs:label>
        <rdf:type rdf:resource="http://www.w3.org/2002/07/owl#NamedIndividual"/>
        <rdf:type rdf:resource="http://www.w3.org/2002/07/owl#Class"/>
      </glview:MeasurementType>
    </rdfs:subClassOf>
    <owl:someValuesFrom>
      <owl:Class>
        <owl:oneOf rdf:parseType="Collection">
          <glview:MeasurementType rdf:about="http://schema.geolink.org/dev/voc/nvs/P02#GP001"/>
        </owl:oneOf>
      </owl:Class>
    </owl:someValuesFrom>
    <owl:onProperty rdf:resource="http://schema.geolink.org/dev/view#hasMeasurementType"/>
  </owl:Restriction>
  <owl:Restriction>
    <rdfs:subClassOf rdf:resource="http://schema.geolink.org/dev/voc/nvs/P02#HLAT"/>
    <owl:someValuesFrom>
      <owl:Class>
        <owl:oneOf rdf:parseType="Collection">
          <glview:MeasurementType rdf:about="http://schema.geolink.org/dev/voc/nvs/P02#HLAT"/>
        </owl:oneOf>
      </owl:Class>
    </owl:someValuesFrom>
    <owl:onProperty rdf:resource="http://schema.geolink.org/dev/view#hasMeasurementType"/>
  </owl:Restriction>
  <owl:Restriction>
    <rdfs:subClassOf rdf:resource="http://schema.geolink.org/dev/voc/nvs/P02#STCO"/>
    <owl:someValuesFrom>
      <owl:Class>
        <owl:oneOf rdf:parseType="Collection">
          <glview:MeasurementType rdf:about="http://schema.geolink.org/dev/voc/nvs/P02#STCO"/>
        </owl:oneOf>
      </owl:Class>
    </owl:someValuesFrom>
    <owl:onProperty rdf:resource="http://schema.geolink.org/dev/view#hasMeasurementType"/>
  </owl:Restriction>
  <owl:Restriction>
    <rdfs:subClassOf>
      <glview:MeasurementType rdf:about="http://schema.geolink.org/dev/voc/nvs/P02#MATC">
        <rdfs:subClassOf rdf:resource="http://schema.geolink.org/dev/voc/nvs/P03#B025"/>
        <rdfs:subClassOf rdf:resource="http://schema.geolink.org/dev/voc/nvs/P03#B070"/>
        <rdfs:seeAlso rdf:resource="http://vocab.nerc.ac.uk/collection/P02/current/MATC/"/>
        <rdfs:comment xml:lang="en">Microzooplankton carbon biomass parameters presented at the level of taxa that may be mapped to entities in the ITIS taxonomy.  These may be at any taxonomic level from sub-species upwards., but exclude morphological classifications such as 'heterotrophic flagellate'.</rdfs:comment>
        <rdfs:label xml:lang="en">Microzooplankton taxonomy-related biomass expressed as carbon per unit volume of the water column</rdfs:label>
        <rdf:type rdf:resource="http://www.w3.org/2002/07/owl#NamedIndividual"/>
        <rdf:type rdf:resource="http://www.w3.org/2002/07/owl#Class"/>
      </glview:MeasurementType>
    </rdfs:subClassOf>
    <owl:someValuesFrom>
      <owl:Class>
        <owl:oneOf rdf:parseType="Collection">
          <glview:MeasurementType rdf:about="http://schema.geolink.org/dev/voc/nvs/P02#MATC"/>
        </owl:oneOf>
      </owl:Class>
    </owl:someValuesFrom>
    <owl:onProperty rdf:resource="http://schema.geolink.org/dev/view#hasMeasurementType"/>
  </owl:Restriction>
  <owl:Restriction>
    <rdfs:subClassOf>
      <glview:MeasurementType rdf:about="http://schema.geolink.org/dev/voc/nvs/P02#CORG">
        <rdfs:subClassOf rdf:resource="http://schema.geolink.org/dev/voc/nvs/P03#C005"/>
        <rdfs:seeAlso rdf:resource="http://vocab.nerc.ac.uk/collection/P02/current/CORG/"/>
        <rdfs:comment xml:lang="en">Concentrations of total and organic carbon in the particulate phase of the water column as extracted by a filtration technique. This is the particle-bound concentration per unit volume of the water column and is both a function of the SPM concentration in the water column and the concentration of carbon per unit weight of SPM.  Total and organic carbon are classed together to circumvent confusion caused by total carbon data sets labelled 'POC' on the assumption that the inorganic carbon fraction is negligible</rdfs:comment>
        <rdfs:label xml:lang="en">Particulate total and organic carbon concentrations in the water column</rdfs:label>
        <rdf:type rdf:resource="http://www.w3.org/2002/07/owl#NamedIndividual"/>
        <rdf:type rdf:resource="http://www.w3.org/2002/07/owl#Class"/>
      </glview:MeasurementType>
    </rdfs:subClassOf>
    <owl:someValuesFrom>
      <owl:Class>
        <owl:oneOf rdf:parseType="Collection">
          <glview:MeasurementType rdf:about="http://schema.geolink.org/dev/voc/nvs/P02#CORG"/>
        </owl:oneOf>
      </owl:Class>
    </owl:someValuesFrom>
    <owl:onProperty rdf:resource="http://schema.geolink.org/dev/view#hasMeasurementType"/>
  </owl:Restriction>
  <owl:Restriction>
    <rdfs:subClassOf rdf:resource="http://schema.geolink.org/dev/voc/nvs/P02#ZNTC"/>
    <owl:someValuesFrom>
      <owl:Class>
        <owl:oneOf rdf:parseType="Collection">
          <glview:MeasurementType rdf:about="http://schema.geolink.org/dev/voc/nvs/P02#ZNTC"/>
        </owl:oneOf>
      </owl:Class>
    </owl:someValuesFrom>
    <owl:onProperty rdf:resource="http://schema.geolink.org/dev/view#hasMeasurementType"/>
  </owl:Restriction>
  <owl:Restriction>
    <rdfs:subClassOf rdf:resource="http://schema.geolink.org/dev/voc/nvs/P02#MZCT"/>
    <owl:someValuesFrom>
      <owl:Class>
        <owl:oneOf rdf:parseType="Collection">
          <glview:MeasurementType rdf:about="http://schema.geolink.org/dev/voc/nvs/P02#MZCT"/>
        </owl:oneOf>
      </owl:Class>
    </owl:someValuesFrom>
    <owl:onProperty rdf:resource="http://schema.geolink.org/dev/view#hasMeasurementType"/>
  </owl:Restriction>
  <owl:Restriction>
    <rdfs:subClassOf>
      <glview:MeasurementType rdf:about="http://schema.geolink.org/dev/voc/nvs/P02#ZWTX">
        <rdfs:subClassOf rdf:resource="http://schema.geolink.org/dev/voc/nvs/P03#B070"/>
        <rdfs:subClassOf rdf:resource="http://schema.geolink.org/dev/voc/nvs/P03#G055"/>
        <rdfs:seeAlso rdf:resource="http://vocab.nerc.ac.uk/collection/P02/current/ZWTX/"/>
        <rdfs:comment xml:lang="en">Zoobenthos wet weight biomass per unit area parameters presented at the level of taxa that may be mapped to entities in the ITIS taxonomy.  Includes animals considered as planktonic if they have been returned from sediment samples.</rdfs:comment>
        <rdfs:label xml:lang="en">Zoobenthos taxonomy-related wet weight biomass per unit area of the bed</rdfs:label>
        <rdf:type rdf:resource="http://www.w3.org/2002/07/owl#NamedIndividual"/>
        <rdf:type rdf:resource="http://www.w3.org/2002/07/owl#Class"/>
      </glview:MeasurementType>
    </rdfs:subClassOf>
    <owl:someValuesFrom>
      <owl:Class>
        <owl:oneOf rdf:parseType="Collection">
          <glview:MeasurementType rdf:about="http://schema.geolink.org/dev/voc/nvs/P02#ZWTX"/>
        </owl:oneOf>
      </owl:Class>
    </owl:someValuesFrom>
    <owl:onProperty rdf:resource="http://schema.geolink.org/dev/view#hasMeasurementType"/>
  </owl:Restriction>
  <owl:Restriction>
    <rdfs:subClassOf>
      <glview:MeasurementType rdf:about="http://schema.geolink.org/dev/voc/nvs/P02#NTSP">
        <rdfs:subClassOf rdf:resource="http://schema.geolink.org/dev/voc/nvs/P03#G015"/>
        <rdfs:subClassOf rdf:resource="http://schema.geolink.org/dev/voc/nvs/P03#C005"/>
        <rdfs:seeAlso rdf:resource="http://vocab.nerc.ac.uk/collection/P02/current/NTSP/"/>
        <rdfs:comment xml:lang="en">Concentrations of total, organic and inorganic nitrogen per unit weight of suspended particulate material collected by water column filtration, centrifugation or sediment trapping.  Note that it is common practice to assume all nitrogen in SPM is organic.</rdfs:comment>
        <rdfs:label xml:lang="en">Nitrogen concentrations in suspended particulate material</rdfs:label>
        <rdf:type rdf:resource="http://www.w3.org/2002/07/owl#NamedIndividual"/>
        <rdf:type rdf:resource="http://www.w3.org/2002/07/owl#Class"/>
      </glview:MeasurementType>
    </rdfs:subClassOf>
    <owl:someValuesFrom>
      <owl:Class>
        <owl:oneOf rdf:parseType="Collection">
          <glview:MeasurementType rdf:about="http://schema.geolink.org/dev/voc/nvs/P02#NTSP"/>
        </owl:oneOf>
      </owl:Class>
    </owl:someValuesFrom>
    <owl:onProperty rdf:resource="http://schema.geolink.org/dev/view#hasMeasurementType"/>
  </owl:Restriction>
  <owl:Restriction>
    <rdfs:subClassOf>
      <glview:MeasurementType rdf:about="http://schema.geolink.org/dev/voc/nvs/P02#SRFR">
        <rdfs:subClassOf rdf:resource="http://schema.geolink.org/dev/voc/nvs/P03#G012"/>
        <rdfs:seeAlso rdf:resource="http://vocab.nerc.ac.uk/collection/P02/current/SRFR/"/>
        <rdfs:comment xml:lang="en">Parameters relating to the elucidation of geological structure by quantifying the refration of waves from a high energy source by sub-surface layers.</rdfs:comment>
        <rdfs:label xml:lang="en">Seismic refraction</rdfs:label>
        <rdf:type rdf:resource="http://www.w3.org/2002/07/owl#NamedIndividual"/>
        <rdf:type rdf:resource="http://www.w3.org/2002/07/owl#Class"/>
      </glview:MeasurementType>
    </rdfs:subClassOf>
    <owl:someValuesFrom>
      <owl:Class>
        <owl:oneOf rdf:parseType="Collection">
          <glview:MeasurementType rdf:about="http://schema.geolink.org/dev/voc/nvs/P02#SRFR"/>
        </owl:oneOf>
      </owl:Class>
    </owl:someValuesFrom>
    <owl:onProperty rdf:resource="http://schema.geolink.org/dev/view#hasMeasurementType"/>
  </owl:Restriction>
  <owl:Restriction>
    <rdfs:subClassOf rdf:resource="http://schema.geolink.org/dev/voc/nvs/P02#OMBI"/>
    <owl:someValuesFrom>
      <owl:Class>
        <owl:oneOf rdf:parseType="Collection">
          <glview:MeasurementType rdf:about="http://schema.geolink.org/dev/voc/nvs/P02#OMBI"/>
        </owl:oneOf>
      </owl:Class>
    </owl:someValuesFrom>
    <owl:onProperty rdf:resource="http://schema.geolink.org/dev/view#hasMeasurementType"/>
  </owl:Restriction>
  <owl:Restriction>
    <rdfs:subClassOf>
      <glview:MeasurementType rdf:about="http://schema.geolink.org/dev/voc/nvs/P02#HZNV">
        <rdfs:subClassOf rdf:resource="http://schema.geolink.org/dev/voc/nvs/P03#H002"/>
        <rdfs:seeAlso rdf:resource="http://vocab.nerc.ac.uk/collection/P02/current/HZNV/"/>
        <rdfs:comment xml:lang="en">Parameters describing the location, nature and extent of objects that pose a threat to travel on the water column such as wrecks and obstructions</rdfs:comment>
        <rdfs:label xml:lang="en">Hazards to navigation</rdfs:label>
        <rdf:type rdf:resource="http://www.w3.org/2002/07/owl#NamedIndividual"/>
        <rdf:type rdf:resource="http://www.w3.org/2002/07/owl#Class"/>
      </glview:MeasurementType>
    </rdfs:subClassOf>
    <owl:someValuesFrom>
      <owl:Class>
        <owl:oneOf rdf:parseType="Collection">
          <glview:MeasurementType rdf:about="http://schema.geolink.org/dev/voc/nvs/P02#HZNV"/>
        </owl:oneOf>
      </owl:Class>
    </owl:someValuesFrom>
    <owl:onProperty rdf:resource="http://schema.geolink.org/dev/view#hasMeasurementType"/>
  </owl:Restriction>
  <owl:Restriction>
    <rdfs:subClassOf>
      <glview:MeasurementType rdf:about="http://schema.geolink.org/dev/voc/nvs/P02#CLTY">
        <rdfs:subClassOf rdf:resource="http://schema.geolink.org/dev/voc/nvs/P03#M010"/>
        <rdfs:seeAlso rdf:resource="http://vocab.nerc.ac.uk/collection/P02/current/CLTY/"/>
        <rdfs:comment xml:lang="en">Parameters that classify cloud cover into types such as cumulus and cirrus.</rdfs:comment>
        <rdfs:label xml:lang="en">Cloud type</rdfs:label>
        <rdf:type rdf:resource="http://www.w3.org/2002/07/owl#NamedIndividual"/>
        <rdf:type rdf:resource="http://www.w3.org/2002/07/owl#Class"/>
      </glview:MeasurementType>
    </rdfs:subClassOf>
    <owl:someValuesFrom>
      <owl:Class>
        <owl:oneOf rdf:parseType="Collection">
          <glview:MeasurementType rdf:about="http://schema.geolink.org/dev/voc/nvs/P02#CLTY"/>
        </owl:oneOf>
      </owl:Class>
    </owl:someValuesFrom>
    <owl:onProperty rdf:resource="http://schema.geolink.org/dev/view#hasMeasurementType"/>
  </owl:Restriction>
  <owl:Restriction>
    <rdfs:subClassOf>
      <glview:MeasurementType rdf:about="http://schema.geolink.org/dev/voc/nvs/P02#PPCB">
        <rdfs:subClassOf rdf:resource="http://schema.geolink.org/dev/voc/nvs/P03#C055"/>
        <rdfs:subClassOf rdf:resource="http://schema.geolink.org/dev/voc/nvs/P03#G015"/>
        <rdfs:subClassOf rdf:resource="http://schema.geolink.org/dev/voc/nvs/P03#H001"/>
        <rdfs:seeAlso rdf:resource="http://vocab.nerc.ac.uk/collection/P02/current/PPCB/"/>
        <rdfs:comment xml:lang="en">PCB concentrations in suspended particulate material, regarded as anything sampled by a water bottle, SAP, sediment trap etc.  This group is for SPM composition measurements (concentration per unit weight) and NOT concentrations per unit volume of the water column in the particulate phase.</rdfs:comment>
        <rdfs:label xml:lang="en">Concentration of polychlorobiphenyls (PCBs) in suspended particulate material</rdfs:label>
        <rdf:type rdf:resource="http://www.w3.org/2002/07/owl#NamedIndividual"/>
        <rdf:type rdf:resource="http://www.w3.org/2002/07/owl#Class"/>
      </glview:MeasurementType>
    </rdfs:subClassOf>
    <owl:someValuesFrom>
      <owl:Class>
        <owl:oneOf rdf:parseType="Collection">
          <glview:MeasurementType rdf:about="http://schema.geolink.org/dev/voc/nvs/P02#PPCB"/>
        </owl:oneOf>
      </owl:Class>
    </owl:someValuesFrom>
    <owl:onProperty rdf:resource="http://schema.geolink.org/dev/view#hasMeasurementType"/>
  </owl:Restriction>
  <owl:Restriction>
    <rdfs:subClassOf rdf:resource="http://schema.geolink.org/dev/voc/nvs/P02#MDBO"/>
    <owl:someValuesFrom>
      <owl:Class>
        <owl:oneOf rdf:parseType="Collection">
          <glview:MeasurementType rdf:about="http://schema.geolink.org/dev/voc/nvs/P02#MDBO"/>
        </owl:oneOf>
      </owl:Class>
    </owl:someValuesFrom>
    <owl:onProperty rdf:resource="http://schema.geolink.org/dev/view#hasMeasurementType"/>
  </owl:Restriction>
  <owl:Restriction>
    <rdfs:subClassOf>
      <glview:MeasurementType rdf:about="http://schema.geolink.org/dev/voc/nvs/P02#SAGE">
        <rdfs:subClassOf rdf:resource="http://schema.geolink.org/dev/voc/nvs/P03#G030"/>
        <rdfs:seeAlso rdf:resource="http://vocab.nerc.ac.uk/collection/P02/current/SAGE/"/>
        <rdfs:comment xml:lang="en">Measured or stratigraphically estimated ages of marine sediments</rdfs:comment>
        <rdfs:label xml:lang="en">Sediment age</rdfs:label>
        <rdf:type rdf:resource="http://www.w3.org/2002/07/owl#NamedIndividual"/>
        <rdf:type rdf:resource="http://www.w3.org/2002/07/owl#Class"/>
      </glview:MeasurementType>
    </rdfs:subClassOf>
    <owl:someValuesFrom>
      <owl:Class>
        <owl:oneOf rdf:parseType="Collection">
          <glview:MeasurementType rdf:about="http://schema.geolink.org/dev/voc/nvs/P02#SAGE"/>
        </owl:oneOf>
      </owl:Class>
    </owl:someValuesFrom>
    <owl:onProperty rdf:resource="http://schema.geolink.org/dev/view#hasMeasurementType"/>
  </owl:Restriction>
  <owl:Restriction>
    <rdfs:subClassOf rdf:resource="http://schema.geolink.org/dev/voc/nvs/P02#ADUN"/>
    <owl:someValuesFrom>
      <owl:Class>
        <owl:oneOf rdf:parseType="Collection">
          <owl:NamedIndividual rdf:about="http://schema.geolink.org/dev/voc/nvs/P02#ADUN"/>
        </owl:oneOf>
      </owl:Class>
    </owl:someValuesFrom>
    <owl:onProperty rdf:resource="http://schema.geolink.org/dev/view#hasMeasurementType"/>
  </owl:Restriction>
  <owl:Restriction>
    <rdfs:subClassOf>
      <glview:MeasurementType rdf:about="http://schema.geolink.org/dev/voc/nvs/P02#CLCN">
        <rdfs:subClassOf rdf:resource="http://schema.geolink.org/dev/voc/nvs/P02#RMIN"/>
        <rdfs:seeAlso rdf:resource="http://vocab.nerc.ac.uk/collection/P02/current/CLCN/"/>
        <rdfs:comment xml:lang="en">Concentrations of halogens as elements or simple inorganic compounds (eg iodate) in sediments (anything collected by a corer including fluff</rdfs:comment>
        <rdfs:label xml:lang="en">Concentration of inorganic halogens in sediment</rdfs:label>
        <rdf:type rdf:resource="http://www.w3.org/2002/07/owl#NamedIndividual"/>
        <rdf:type rdf:resource="http://www.w3.org/2002/07/owl#Class"/>
      </glview:MeasurementType>
    </rdfs:subClassOf>
    <owl:someValuesFrom>
      <owl:Class>
        <owl:oneOf rdf:parseType="Collection">
          <glview:MeasurementType rdf:about="http://schema.geolink.org/dev/voc/nvs/P02#CLCN"/>
        </owl:oneOf>
      </owl:Class>
    </owl:someValuesFrom>
    <owl:onProperty rdf:resource="http://schema.geolink.org/dev/view#hasMeasurementType"/>
  </owl:Restriction>
  <owl:Restriction>
    <rdfs:subClassOf>
      <glview:MeasurementType rdf:about="http://schema.geolink.org/dev/voc/nvs/P02#GWDR">
        <rdfs:subClassOf rdf:resource="http://schema.geolink.org/dev/voc/nvs/P03#D034"/>
        <rdfs:seeAlso rdf:resource="http://vocab.nerc.ac.uk/collection/P02/current/GWDR/"/>
        <rdfs:comment xml:lang="en">Direct measurements (including visual estimates) plus statistically derived parameters</rdfs:comment>
        <rdfs:label xml:lang="en">Wave direction</rdfs:label>
        <rdf:type rdf:resource="http://www.w3.org/2002/07/owl#NamedIndividual"/>
        <rdf:type rdf:resource="http://www.w3.org/2002/07/owl#Class"/>
      </glview:MeasurementType>
    </rdfs:subClassOf>
    <owl:someValuesFrom>
      <owl:Class>
        <owl:oneOf rdf:parseType="Collection">
          <glview:MeasurementType rdf:about="http://schema.geolink.org/dev/voc/nvs/P02#GWDR"/>
        </owl:oneOf>
      </owl:Class>
    </owl:someValuesFrom>
    <owl:onProperty rdf:resource="http://schema.geolink.org/dev/view#hasMeasurementType"/>
  </owl:Restriction>
  <owl:Restriction>
    <rdfs:subClassOf>
      <glview:MeasurementType rdf:about="http://schema.geolink.org/dev/voc/nvs/P02#CEBH">
        <rdfs:subClassOf rdf:resource="http://schema.geolink.org/dev/voc/nvs/P03#B015"/>
        <rdfs:seeAlso rdf:resource="http://vocab.nerc.ac.uk/collection/P02/current/CEBH/"/>
        <rdfs:comment xml:lang="en">Parameters describing the actions or reactions of cetaceans (Order Cetacea), usually in response to the environment. Includes both parameters mapped to taxa and those mapped to non-taxonomic groupings.</rdfs:comment>
        <rdfs:label xml:lang="en">Cetacean behaviour</rdfs:label>
        <rdf:type rdf:resource="http://www.w3.org/2002/07/owl#NamedIndividual"/>
        <rdf:type rdf:resource="http://www.w3.org/2002/07/owl#Class"/>
      </glview:MeasurementType>
    </rdfs:subClassOf>
    <owl:someValuesFrom>
      <owl:Class>
        <owl:oneOf rdf:parseType="Collection">
          <glview:MeasurementType rdf:about="http://schema.geolink.org/dev/voc/nvs/P02#CEBH"/>
        </owl:oneOf>
      </owl:Class>
    </owl:someValuesFrom>
    <owl:onProperty rdf:resource="http://schema.geolink.org/dev/view#hasMeasurementType"/>
  </owl:Restriction>
  <owl:Restriction>
    <rdfs:subClassOf>
      <glview:MeasurementType rdf:about="http://schema.geolink.org/dev/voc/nvs/P02#BRDD">
        <rdfs:subClassOf rdf:resource="http://schema.geolink.org/dev/voc/nvs/P03#B070"/>
        <rdfs:subClassOf rdf:resource="http://schema.geolink.org/dev/voc/nvs/P03#B015"/>
        <rdfs:seeAlso rdf:resource="http://vocab.nerc.ac.uk/collection/P02/current/BRDD/"/>
        <rdfs:comment xml:lang="en">Bird (Class Aves) abundance per unit area (of land or sea) presented at the level of taxa that may be mapped to entities in the ITIS taxonomy.These may be at any taxonomic level from sub-species upwards.</rdfs:comment>
        <rdfs:label xml:lang="en">Bird taxonomy-related abundance per unit area of surface</rdfs:label>
        <rdf:type rdf:resource="http://www.w3.org/2002/07/owl#NamedIndividual"/>
        <rdf:type rdf:resource="http://www.w3.org/2002/07/owl#Class"/>
      </glview:MeasurementType>
    </rdfs:subClassOf>
    <owl:someValuesFrom>
      <owl:Class>
        <owl:oneOf rdf:parseType="Collection">
          <glview:MeasurementType rdf:about="http://schema.geolink.org/dev/voc/nvs/P02#BRDD"/>
        </owl:oneOf>
      </owl:Class>
    </owl:someValuesFrom>
    <owl:onProperty rdf:resource="http://schema.geolink.org/dev/view#hasMeasurementType"/>
  </owl:Restriction>
  <owl:Restriction>
    <rdfs:subClassOf>
      <glview:MeasurementType rdf:about="http://schema.geolink.org/dev/voc/nvs/P02#RWCH">
        <rdfs:subClassOf rdf:resource="http://schema.geolink.org/dev/voc/nvs/P03#M005"/>
        <rdfs:seeAlso rdf:resource="http://vocab.nerc.ac.uk/collection/P02/current/RWCH/"/>
        <rdfs:comment xml:lang="en">Concentration of any chemical species in water collected from the atmosphere.  Includes rain, snow, hail and fog but excludes cloud samples or snow accumulations on the ground.</rdfs:comment>
        <rdfs:label xml:lang="en">Precipitation chemistry</rdfs:label>
        <rdf:type rdf:resource="http://www.w3.org/2002/07/owl#NamedIndividual"/>
        <rdf:type rdf:resource="http://www.w3.org/2002/07/owl#Class"/>
      </glview:MeasurementType>
    </rdfs:subClassOf>
    <owl:someValuesFrom>
      <owl:Class>
        <owl:oneOf rdf:parseType="Collection">
          <glview:MeasurementType rdf:about="http://schema.geolink.org/dev/voc/nvs/P02#RWCH"/>
        </owl:oneOf>
      </owl:Class>
    </owl:someValuesFrom>
    <owl:onProperty rdf:resource="http://schema.geolink.org/dev/view#hasMeasurementType"/>
  </owl:Restriction>
  <owl:Restriction>
    <rdfs:subClassOf rdf:resource="http://schema.geolink.org/dev/voc/nvs/P02#MATC"/>
    <owl:someValuesFrom>
      <owl:Class>
        <owl:oneOf rdf:parseType="Collection">
          <glview:MeasurementType rdf:about="http://schema.geolink.org/dev/voc/nvs/P02#MATC"/>
        </owl:oneOf>
      </owl:Class>
    </owl:someValuesFrom>
    <owl:onProperty rdf:resource="http://schema.geolink.org/dev/view#hasMeasurementType"/>
  </owl:Restriction>
  <owl:Restriction>
    <rdfs:subClassOf rdf:resource="http://schema.geolink.org/dev/voc/nvs/P02#SRAD"/>
    <owl:someValuesFrom>
      <owl:Class>
        <owl:oneOf rdf:parseType="Collection">
          <glview:MeasurementType rdf:about="http://schema.geolink.org/dev/voc/nvs/P02#SRAD"/>
        </owl:oneOf>
      </owl:Class>
    </owl:someValuesFrom>
    <owl:onProperty rdf:resource="http://schema.geolink.org/dev/view#hasMeasurementType"/>
  </owl:Restriction>
  <owl:Restriction>
    <rdfs:subClassOf>
      <glview:MeasurementType rdf:about="http://schema.geolink.org/dev/voc/nvs/P02#AHGT">
        <rdfs:subClassOf rdf:resource="http://schema.geolink.org/dev/voc/nvs/P03#Z005"/>
        <rdfs:seeAlso rdf:resource="http://vocab.nerc.ac.uk/collection/P02/current/AHGT/"/>
        <rdfs:comment xml:lang="en">All vertical spatial parameters including depth, height and pressure when used as an independent variable.</rdfs:comment>
        <rdfs:label xml:lang="en">Vertical spatial coordinates</rdfs:label>
        <rdf:type rdf:resource="http://www.w3.org/2002/07/owl#NamedIndividual"/>
        <rdf:type rdf:resource="http://www.w3.org/2002/07/owl#Class"/>
      </glview:MeasurementType>
    </rdfs:subClassOf>
    <owl:someValuesFrom>
      <owl:Class>
        <owl:oneOf rdf:parseType="Collection">
          <glview:MeasurementType rdf:about="http://schema.geolink.org/dev/voc/nvs/P02#AHGT"/>
        </owl:oneOf>
      </owl:Class>
    </owl:someValuesFrom>
    <owl:onProperty rdf:resource="http://schema.geolink.org/dev/view#hasMeasurementType"/>
  </owl:Restriction>
  <owl:Restriction>
    <rdfs:subClassOf rdf:resource="http://schema.geolink.org/dev/voc/nvs/P02#PPCB"/>
    <owl:someValuesFrom>
      <owl:Class>
        <owl:oneOf rdf:parseType="Collection">
          <glview:MeasurementType rdf:about="http://schema.geolink.org/dev/voc/nvs/P02#PPCB"/>
        </owl:oneOf>
      </owl:Class>
    </owl:someValuesFrom>
    <owl:onProperty rdf:resource="http://schema.geolink.org/dev/view#hasMeasurementType"/>
  </owl:Restriction>
  <owl:Restriction>
    <rdfs:subClassOf>
      <glview:MeasurementType rdf:about="http://schema.geolink.org/dev/voc/nvs/P02#HLWC">
        <rdfs:subClassOf rdf:resource="http://schema.geolink.org/dev/voc/nvs/P03#C045"/>
        <rdfs:seeAlso rdf:resource="http://vocab.nerc.ac.uk/collection/P02/current/HLWC/"/>
        <rdfs:comment xml:lang="en">Concentrations of halogens as elements or their inorganic compounds in all phases of any body of fresh or salt water</rdfs:comment>
        <rdfs:label xml:lang="en">Concentration of inorganic halogens in water bodies</rdfs:label>
        <rdf:type rdf:resource="http://www.w3.org/2002/07/owl#NamedIndividual"/>
        <rdf:type rdf:resource="http://www.w3.org/2002/07/owl#Class"/>
      </glview:MeasurementType>
    </rdfs:subClassOf>
    <owl:someValuesFrom>
      <owl:Class>
        <owl:oneOf rdf:parseType="Collection">
          <glview:MeasurementType rdf:about="http://schema.geolink.org/dev/voc/nvs/P02#HLWC"/>
        </owl:oneOf>
      </owl:Class>
    </owl:someValuesFrom>
    <owl:onProperty rdf:resource="http://schema.geolink.org/dev/view#hasMeasurementType"/>
  </owl:Restriction>
  <owl:Restriction>
    <rdfs:subClassOf>
      <glview:MeasurementType rdf:about="http://schema.geolink.org/dev/voc/nvs/P02#MDSD">
        <rdfs:subClassOf rdf:resource="http://schema.geolink.org/dev/voc/nvs/P02#RMIN"/>
        <rdfs:seeAlso rdf:resource="http://vocab.nerc.ac.uk/collection/P02/current/MDSD/"/>
        <rdfs:comment xml:lang="en">Concentration parameters for metalloid elements in sediment.  Sediment is understood to be the solid phase of the bed, including the recently settled material sometimes known as fluff collected from the bed surface. Metalloids are considered as B, Ge, As, Sb, Te and Po (but not Si which is classed separately because of its major role in environmental chemistry)</rdfs:comment>
        <rdfs:label xml:lang="en">Trace metalloid concentrations in sediment</rdfs:label>
        <rdf:type rdf:resource="http://www.w3.org/2002/07/owl#NamedIndividual"/>
        <rdf:type rdf:resource="http://www.w3.org/2002/07/owl#Class"/>
      </glview:MeasurementType>
    </rdfs:subClassOf>
    <owl:someValuesFrom>
      <owl:Class>
        <owl:oneOf rdf:parseType="Collection">
          <glview:MeasurementType rdf:about="http://schema.geolink.org/dev/voc/nvs/P02#MDSD"/>
        </owl:oneOf>
      </owl:Class>
    </owl:someValuesFrom>
    <owl:onProperty rdf:resource="http://schema.geolink.org/dev/view#hasMeasurementType"/>
  </owl:Restriction>
  <owl:Restriction>
    <rdfs:subClassOf>
      <glview:MeasurementType rdf:about="http://schema.geolink.org/dev/voc/nvs/P02#BCOS">
        <rdfs:subClassOf rdf:resource="http://schema.geolink.org/dev/voc/nvs/P03#B007"/>
        <rdfs:seeAlso rdf:resource="http://vocab.nerc.ac.uk/collection/P02/current/BCOS/"/>
        <rdfs:comment xml:lang="en">'Other'  (than metals or organic contaminants) substance concentrations in either whole organisms or their constituent parts.  This is a 'bucket' grouping that may be reclassified as the dictionary developes.</rdfs:comment>
        <rdfs:label xml:lang="en">Concentration of other substances in biota</rdfs:label>
        <rdf:type rdf:resource="http://www.w3.org/2002/07/owl#NamedIndividual"/>
        <rdf:type rdf:resource="http://www.w3.org/2002/07/owl#Class"/>
      </glview:MeasurementType>
    </rdfs:subClassOf>
    <owl:someValuesFrom>
      <owl:Class>
        <owl:oneOf rdf:parseType="Collection">
          <glview:MeasurementType rdf:about="http://schema.geolink.org/dev/voc/nvs/P02#BCOS"/>
        </owl:oneOf>
      </owl:Class>
    </owl:someValuesFrom>
    <owl:onProperty rdf:resource="http://schema.geolink.org/dev/view#hasMeasurementType"/>
  </owl:Restriction>
  <owl:Restriction>
    <rdfs:subClassOf rdf:resource="http://schema.geolink.org/dev/voc/nvs/P02#ZNTX"/>
    <owl:someValuesFrom>
      <owl:Class>
        <owl:oneOf rdf:parseType="Collection">
          <glview:MeasurementType rdf:about="http://schema.geolink.org/dev/voc/nvs/P02#ZNTX"/>
        </owl:oneOf>
      </owl:Class>
    </owl:someValuesFrom>
    <owl:onProperty rdf:resource="http://schema.geolink.org/dev/view#hasMeasurementType"/>
  </owl:Restriction>
  <owl:Restriction>
    <rdfs:subClassOf>
      <glview:MeasurementType rdf:about="http://schema.geolink.org/dev/voc/nvs/P02#GP069">
        <rdfs:subClassOf rdf:resource="http://schema.geolink.org/dev/voc/nvs/P03#B015"/>
        <rdfs:seeAlso rdf:resource="http://vocab.nerc.ac.uk/collection/P02/current/GP069/"/>
        <rdfs:comment xml:lang="en">Parameters related to the reproduction of reptiles (Class Reptilia)</rdfs:comment>
        <rdfs:label xml:lang="en">Reptile reproduction</rdfs:label>
        <rdf:type rdf:resource="http://www.w3.org/2002/07/owl#NamedIndividual"/>
        <rdf:type rdf:resource="http://www.w3.org/2002/07/owl#Class"/>
      </glview:MeasurementType>
    </rdfs:subClassOf>
    <owl:someValuesFrom>
      <owl:Class>
        <owl:oneOf rdf:parseType="Collection">
          <glview:MeasurementType rdf:about="http://schema.geolink.org/dev/voc/nvs/P02#GP069"/>
        </owl:oneOf>
      </owl:Class>
    </owl:someValuesFrom>
    <owl:onProperty rdf:resource="http://schema.geolink.org/dev/view#hasMeasurementType"/>
  </owl:Restriction>
  <owl:Restriction>
    <rdfs:subClassOf rdf:resource="http://schema.geolink.org/dev/voc/nvs/P02#ZATX"/>
    <owl:someValuesFrom>
      <owl:Class>
        <owl:oneOf rdf:parseType="Collection">
          <glview:MeasurementType rdf:about="http://schema.geolink.org/dev/voc/nvs/P02#ZATX"/>
        </owl:oneOf>
      </owl:Class>
    </owl:someValuesFrom>
    <owl:onProperty rdf:resource="http://schema.geolink.org/dev/view#hasMeasurementType"/>
  </owl:Restriction>
  <owl:Restriction>
    <rdfs:subClassOf rdf:resource="http://schema.geolink.org/dev/voc/nvs/P02#NTSP"/>
    <owl:someValuesFrom>
      <owl:Class>
        <owl:oneOf rdf:parseType="Collection">
          <glview:MeasurementType rdf:about="http://schema.geolink.org/dev/voc/nvs/P02#NTSP"/>
        </owl:oneOf>
      </owl:Class>
    </owl:someValuesFrom>
    <owl:onProperty rdf:resource="http://schema.geolink.org/dev/view#hasMeasurementType"/>
  </owl:Restriction>
  <owl:Restriction>
    <rdfs:subClassOf>
      <glview:MeasurementType rdf:about="http://schema.geolink.org/dev/voc/nvs/P02#GRAV">
        <rdfs:subClassOf rdf:resource="http://schema.geolink.org/dev/voc/nvs/P03#G005"/>
        <rdfs:subClassOf rdf:resource="http://schema.geolink.org/dev/voc/nvs/P03#GPYS"/>
        <rdfs:seeAlso rdf:resource="http://vocab.nerc.ac.uk/collection/P02/current/GRAV/"/>
        <rdfs:comment xml:lang="en">Parameters relating to the measurement of the Earth's gravity field</rdfs:comment>
        <rdfs:label xml:lang="en">Gravity</rdfs:label>
        <rdf:type rdf:resource="http://www.w3.org/2002/07/owl#NamedIndividual"/>
        <rdf:type rdf:resource="http://www.w3.org/2002/07/owl#Class"/>
      </glview:MeasurementType>
    </rdfs:subClassOf>
    <owl:someValuesFrom>
      <owl:Class>
        <owl:oneOf rdf:parseType="Collection">
          <glview:MeasurementType rdf:about="http://schema.geolink.org/dev/voc/nvs/P02#GRAV"/>
        </owl:oneOf>
      </owl:Class>
    </owl:someValuesFrom>
    <owl:onProperty rdf:resource="http://schema.geolink.org/dev/view#hasMeasurementType"/>
  </owl:Restriction>
  <owl:Restriction>
    <rdfs:subClassOf>
      <glview:MeasurementType rdf:about="http://schema.geolink.org/dev/voc/nvs/P02#RTMP">
        <rdfs:subClassOf rdf:resource="http://schema.geolink.org/dev/voc/nvs/P02#STMP"/>
        <rdfs:seeAlso rdf:resource="http://vocab.nerc.ac.uk/collection/P02/current/RTMP/"/>
        <rdfs:comment xml:lang="en">Parameters that describe the distribution of the degree of hotness within geologic units of lithified sedimentary, igneous of metamorphic rock.</rdfs:comment>
        <rdfs:label xml:lang="en">Rock temperature</rdfs:label>
        <rdf:type rdf:resource="http://www.w3.org/2002/07/owl#NamedIndividual"/>
        <rdf:type rdf:resource="http://www.w3.org/2002/07/owl#Class"/>
      </glview:MeasurementType>
    </rdfs:subClassOf>
    <owl:someValuesFrom>
      <owl:Class>
        <owl:oneOf rdf:parseType="Collection">
          <glview:MeasurementType rdf:about="http://schema.geolink.org/dev/voc/nvs/P02#RTMP"/>
        </owl:oneOf>
      </owl:Class>
    </owl:someValuesFrom>
    <owl:onProperty rdf:resource="http://schema.geolink.org/dev/view#hasMeasurementType"/>
  </owl:Restriction>
  <owl:Restriction>
    <rdfs:subClassOf rdf:resource="http://schema.geolink.org/dev/voc/nvs/P02#FIBM"/>
    <owl:someValuesFrom>
      <owl:Class>
        <owl:oneOf rdf:parseType="Collection">
          <glview:MeasurementType rdf:about="http://schema.geolink.org/dev/voc/nvs/P02#FIBM"/>
        </owl:oneOf>
      </owl:Class>
    </owl:someValuesFrom>
    <owl:onProperty rdf:resource="http://schema.geolink.org/dev/view#hasMeasurementType"/>
  </owl:Restriction>
  <owl:Restriction>
    <rdfs:subClassOf rdf:resource="http://schema.geolink.org/dev/voc/nvs/P02#PCFX"/>
    <owl:someValuesFrom>
      <owl:Class>
        <owl:oneOf rdf:parseType="Collection">
          <glview:MeasurementType rdf:about="http://schema.geolink.org/dev/voc/nvs/P02#PCFX"/>
        </owl:oneOf>
      </owl:Class>
    </owl:someValuesFrom>
    <owl:onProperty rdf:resource="http://schema.geolink.org/dev/view#hasMeasurementType"/>
  </owl:Restriction>
  <owl:Restriction>
    <rdfs:subClassOf rdf:resource="http://schema.geolink.org/dev/voc/nvs/P02#PU02"/>
    <owl:someValuesFrom>
      <owl:Class>
        <owl:oneOf rdf:parseType="Collection">
          <glview:MeasurementType rdf:about="http://schema.geolink.org/dev/voc/nvs/P02#PU02"/>
        </owl:oneOf>
      </owl:Class>
    </owl:someValuesFrom>
    <owl:onProperty rdf:resource="http://schema.geolink.org/dev/view#hasMeasurementType"/>
  </owl:Restriction>
  <owl:Restriction>
    <rdfs:subClassOf>
      <glview:MeasurementType rdf:about="http://schema.geolink.org/dev/voc/nvs/P02#AYMD">
        <rdfs:subClassOf rdf:resource="http://schema.geolink.org/dev/voc/nvs/P03#Z005"/>
        <rdfs:seeAlso rdf:resource="http://vocab.nerc.ac.uk/collection/P02/current/AYMD/"/>
        <rdfs:comment xml:lang="en">All date and time parameters</rdfs:comment>
        <rdfs:label xml:lang="en">Date and time</rdfs:label>
        <rdf:type rdf:resource="http://www.w3.org/2002/07/owl#NamedIndividual"/>
        <rdf:type rdf:resource="http://www.w3.org/2002/07/owl#Class"/>
      </glview:MeasurementType>
    </rdfs:subClassOf>
    <owl:someValuesFrom>
      <owl:Class>
        <owl:oneOf rdf:parseType="Collection">
          <glview:MeasurementType rdf:about="http://schema.geolink.org/dev/voc/nvs/P02#AYMD"/>
        </owl:oneOf>
      </owl:Class>
    </owl:someValuesFrom>
    <owl:onProperty rdf:resource="http://schema.geolink.org/dev/view#hasMeasurementType"/>
  </owl:Restriction>
  <owl:Restriction>
    <rdfs:subClassOf>
      <glview:MeasurementType rdf:about="http://schema.geolink.org/dev/voc/nvs/P02#EWSB">
        <rdfs:subClassOf rdf:resource="http://schema.geolink.org/dev/voc/nvs/P03#M010"/>
        <rdfs:seeAlso rdf:resource="http://vocab.nerc.ac.uk/collection/P02/current/EWSB/"/>
        <rdfs:comment xml:lang="en">Parameters quantifying the extent or direction of atmospheric movement. Obvious examples are wind velocity, windspeed and wind direction, but can also include derived parameters such as force, energy, power and power density.</rdfs:comment>
        <rdfs:label xml:lang="en">Wind strength and direction</rdfs:label>
        <rdf:type rdf:resource="http://www.w3.org/2002/07/owl#NamedIndividual"/>
        <rdf:type rdf:resource="http://www.w3.org/2002/07/owl#Class"/>
      </glview:MeasurementType>
    </rdfs:subClassOf>
    <owl:someValuesFrom>
      <owl:Class>
        <owl:oneOf rdf:parseType="Collection">
          <glview:MeasurementType rdf:about="http://schema.geolink.org/dev/voc/nvs/P02#EWSB"/>
        </owl:oneOf>
      </owl:Class>
    </owl:someValuesFrom>
    <owl:onProperty rdf:resource="http://schema.geolink.org/dev/view#hasMeasurementType"/>
  </owl:Restriction>
  <owl:Restriction>
    <rdfs:subClassOf rdf:resource="http://schema.geolink.org/dev/voc/nvs/P02#GP012"/>
    <owl:someValuesFrom>
      <owl:Class>
        <owl:oneOf rdf:parseType="Collection">
          <glview:MeasurementType rdf:about="http://schema.geolink.org/dev/voc/nvs/P02#GP012"/>
        </owl:oneOf>
      </owl:Class>
    </owl:someValuesFrom>
    <owl:onProperty rdf:resource="http://schema.geolink.org/dev/view#hasMeasurementType"/>
  </owl:Restriction>
  <owl:Restriction>
    <rdfs:subClassOf rdf:resource="http://schema.geolink.org/dev/voc/nvs/P02#BAUC"/>
    <owl:someValuesFrom>
      <owl:Class>
        <owl:oneOf rdf:parseType="Collection">
          <glview:MeasurementType rdf:about="http://schema.geolink.org/dev/voc/nvs/P02#BAUC"/>
        </owl:oneOf>
      </owl:Class>
    </owl:someValuesFrom>
    <owl:onProperty rdf:resource="http://schema.geolink.org/dev/view#hasMeasurementType"/>
  </owl:Restriction>
  <owl:Restriction>
    <rdfs:subClassOf rdf:resource="http://schema.geolink.org/dev/voc/nvs/P02#ZCTC"/>
    <owl:someValuesFrom>
      <owl:Class>
        <owl:oneOf rdf:parseType="Collection">
          <glview:MeasurementType rdf:about="http://schema.geolink.org/dev/voc/nvs/P02#ZCTC"/>
        </owl:oneOf>
      </owl:Class>
    </owl:someValuesFrom>
    <owl:onProperty rdf:resource="http://schema.geolink.org/dev/view#hasMeasurementType"/>
  </owl:Restriction>
  <owl:Restriction>
    <rdfs:subClassOf>
      <glview:MeasurementType rdf:about="http://schema.geolink.org/dev/voc/nvs/P02#SBPH">
        <rdfs:subClassOf rdf:resource="http://schema.geolink.org/dev/voc/nvs/P03#UWPH"/>
        <rdfs:seeAlso rdf:resource="http://vocab.nerc.ac.uk/collection/P02/current/SBPH/"/>
        <rdfs:comment xml:lang="en">Digital images of the seabed obtained using either still or video cameras</rdfs:comment>
        <rdfs:label xml:lang="en">Seabed photography</rdfs:label>
        <rdf:type rdf:resource="http://www.w3.org/2002/07/owl#NamedIndividual"/>
        <rdf:type rdf:resource="http://www.w3.org/2002/07/owl#Class"/>
      </glview:MeasurementType>
    </rdfs:subClassOf>
    <owl:someValuesFrom>
      <owl:Class>
        <owl:oneOf rdf:parseType="Collection">
          <glview:MeasurementType rdf:about="http://schema.geolink.org/dev/voc/nvs/P02#SBPH"/>
        </owl:oneOf>
      </owl:Class>
    </owl:someValuesFrom>
    <owl:onProperty rdf:resource="http://schema.geolink.org/dev/view#hasMeasurementType"/>
  </owl:Restriction>
  <owl:Restriction>
    <rdfs:subClassOf>
      <glview:MeasurementType rdf:about="http://schema.geolink.org/dev/voc/nvs/P02#TADN">
        <rdfs:subClassOf rdf:resource="http://schema.geolink.org/dev/voc/nvs/P03#C050"/>
        <rdfs:subClassOf rdf:resource="http://schema.geolink.org/dev/voc/nvs/P03#G035"/>
        <rdfs:seeAlso rdf:resource="http://vocab.nerc.ac.uk/collection/P02/current/TADN/"/>
        <rdfs:comment xml:lang="en">Concentrations of adenylates (ADP, ATP etc) per unit mass or unit volume of sediment (material collected by a corer including fluff)</rdfs:comment>
        <rdfs:label xml:lang="en">Concentration of adenylates in sediment</rdfs:label>
        <rdf:type rdf:resource="http://www.w3.org/2002/07/owl#NamedIndividual"/>
        <rdf:type rdf:resource="http://www.w3.org/2002/07/owl#Class"/>
      </glview:MeasurementType>
    </rdfs:subClassOf>
    <owl:someValuesFrom>
      <owl:Class>
        <owl:oneOf rdf:parseType="Collection">
          <glview:MeasurementType rdf:about="http://schema.geolink.org/dev/voc/nvs/P02#TADN"/>
        </owl:oneOf>
      </owl:Class>
    </owl:someValuesFrom>
    <owl:onProperty rdf:resource="http://schema.geolink.org/dev/view#hasMeasurementType"/>
  </owl:Restriction>
  <owl:Restriction>
    <rdfs:subClassOf>
      <glview:MeasurementType rdf:about="http://schema.geolink.org/dev/voc/nvs/P02#ALKY">
        <rdfs:subClassOf rdf:resource="http://schema.geolink.org/dev/voc/nvs/P03#C010"/>
        <rdfs:seeAlso rdf:resource="http://vocab.nerc.ac.uk/collection/P02/current/ALKY/"/>
        <rdfs:comment xml:lang="en">Parameters quantifying the hydrogen ion concentration in water bodies</rdfs:comment>
        <rdfs:label xml:lang="en">Alkalinity, acidity and pH of the water column</rdfs:label>
        <rdf:type rdf:resource="http://www.w3.org/2002/07/owl#NamedIndividual"/>
        <rdf:type rdf:resource="http://www.w3.org/2002/07/owl#Class"/>
      </glview:MeasurementType>
    </rdfs:subClassOf>
    <owl:someValuesFrom>
      <owl:Class>
        <owl:oneOf rdf:parseType="Collection">
          <glview:MeasurementType rdf:about="http://schema.geolink.org/dev/voc/nvs/P02#ALKY"/>
        </owl:oneOf>
      </owl:Class>
    </owl:someValuesFrom>
    <owl:onProperty rdf:resource="http://schema.geolink.org/dev/view#hasMeasurementType"/>
  </owl:Restriction>
  <owl:Restriction>
    <rdfs:subClassOf rdf:resource="http://schema.geolink.org/dev/voc/nvs/P02#BRDD"/>
    <owl:someValuesFrom>
      <owl:Class>
        <owl:oneOf rdf:parseType="Collection">
          <glview:MeasurementType rdf:about="http://schema.geolink.org/dev/voc/nvs/P02#BRDD"/>
        </owl:oneOf>
      </owl:Class>
    </owl:someValuesFrom>
    <owl:onProperty rdf:resource="http://schema.geolink.org/dev/view#hasMeasurementType"/>
  </owl:Restriction>
  <owl:Restriction>
    <rdfs:subClassOf>
      <glview:MeasurementType rdf:about="http://schema.geolink.org/dev/voc/nvs/P02#DALK">
        <rdfs:subClassOf rdf:resource="http://schema.geolink.org/dev/voc/nvs/P03#C025"/>
        <rdfs:seeAlso rdf:resource="http://vocab.nerc.ac.uk/collection/P02/current/DALK/"/>
        <rdfs:comment xml:lang="en">Alkane concentration parameters (including saturation of gaseous species) in all phases of the water column.  Does not include parameters expressed per unit weight of SPM.</rdfs:comment>
        <rdfs:label xml:lang="en">Concentration of alkanes in the water column</rdfs:label>
        <rdf:type rdf:resource="http://www.w3.org/2002/07/owl#NamedIndividual"/>
        <rdf:type rdf:resource="http://www.w3.org/2002/07/owl#Class"/>
      </glview:MeasurementType>
    </rdfs:subClassOf>
    <owl:someValuesFrom>
      <owl:Class>
        <owl:oneOf rdf:parseType="Collection">
          <glview:MeasurementType rdf:about="http://schema.geolink.org/dev/voc/nvs/P02#DALK"/>
        </owl:oneOf>
      </owl:Class>
    </owl:someValuesFrom>
    <owl:onProperty rdf:resource="http://schema.geolink.org/dev/view#hasMeasurementType"/>
  </owl:Restriction>
  <owl:Restriction>
    <rdfs:subClassOf>
      <glview:MeasurementType rdf:about="http://schema.geolink.org/dev/voc/nvs/P02#CLAY">
        <rdfs:subClassOf rdf:resource="http://schema.geolink.org/dev/voc/nvs/P03#G045"/>
        <rdfs:seeAlso rdf:resource="http://vocab.nerc.ac.uk/collection/P02/current/CLAY/"/>
        <rdfs:comment xml:lang="en">Parameters describing or quantifying the mineralogical composition of rocks and unlithified sediments.</rdfs:comment>
        <rdfs:label xml:lang="en">Mineralogical composition</rdfs:label>
        <rdf:type rdf:resource="http://www.w3.org/2002/07/owl#NamedIndividual"/>
        <rdf:type rdf:resource="http://www.w3.org/2002/07/owl#Class"/>
      </glview:MeasurementType>
    </rdfs:subClassOf>
    <owl:someValuesFrom>
      <owl:Class>
        <owl:oneOf rdf:parseType="Collection">
          <glview:MeasurementType rdf:about="http://schema.geolink.org/dev/voc/nvs/P02#CLAY"/>
        </owl:oneOf>
      </owl:Class>
    </owl:someValuesFrom>
    <owl:onProperty rdf:resource="http://schema.geolink.org/dev/view#hasMeasurementType"/>
  </owl:Restriction>
  <owl:Restriction>
    <rdfs:subClassOf rdf:resource="http://schema.geolink.org/dev/voc/nvs/P02#CARS"/>
    <owl:someValuesFrom>
      <owl:Class>
        <owl:oneOf rdf:parseType="Collection">
          <glview:MeasurementType rdf:about="http://schema.geolink.org/dev/voc/nvs/P02#CARS"/>
        </owl:oneOf>
      </owl:Class>
    </owl:someValuesFrom>
    <owl:onProperty rdf:resource="http://schema.geolink.org/dev/view#hasMeasurementType"/>
  </owl:Restriction>
  <owl:Restriction>
    <rdfs:subClassOf>
      <glview:MeasurementType rdf:about="http://schema.geolink.org/dev/voc/nvs/P02#TSED">
        <rdfs:subClassOf rdf:resource="http://schema.geolink.org/dev/voc/nvs/P03#G015"/>
        <rdfs:seeAlso rdf:resource="http://vocab.nerc.ac.uk/collection/P02/current/TSED/"/>
        <rdfs:comment xml:lang="en">Parameters quantifying SPM concentration in the water column by weight, by volume or in terms of turbidity</rdfs:comment>
        <rdfs:label xml:lang="en">Concentration of suspended particulate material in the water column</rdfs:label>
        <rdf:type rdf:resource="http://www.w3.org/2002/07/owl#NamedIndividual"/>
        <rdf:type rdf:resource="http://www.w3.org/2002/07/owl#Class"/>
      </glview:MeasurementType>
    </rdfs:subClassOf>
    <owl:someValuesFrom>
      <owl:Class>
        <owl:oneOf rdf:parseType="Collection">
          <glview:MeasurementType rdf:about="http://schema.geolink.org/dev/voc/nvs/P02#TSED"/>
        </owl:oneOf>
      </owl:Class>
    </owl:someValuesFrom>
    <owl:onProperty rdf:resource="http://schema.geolink.org/dev/view#hasMeasurementType"/>
  </owl:Restriction>
  <owl:Restriction>
    <rdfs:subClassOf rdf:resource="http://schema.geolink.org/dev/voc/nvs/P02#GRAV"/>
    <owl:someValuesFrom>
      <owl:Class>
        <owl:oneOf rdf:parseType="Collection">
          <glview:MeasurementType rdf:about="http://schema.geolink.org/dev/voc/nvs/P02#GRAV"/>
        </owl:oneOf>
      </owl:Class>
    </owl:someValuesFrom>
    <owl:onProperty rdf:resource="http://schema.geolink.org/dev/view#hasMeasurementType"/>
  </owl:Restriction>
  <owl:Restriction>
    <rdfs:subClassOf>
      <glview:MeasurementType rdf:about="http://schema.geolink.org/dev/voc/nvs/P02#STOM">
        <rdfs:subClassOf rdf:resource="http://schema.geolink.org/dev/voc/nvs/P03#G035"/>
        <rdfs:seeAlso rdf:resource="http://vocab.nerc.ac.uk/collection/P02/current/STOM/"/>
        <rdfs:comment xml:lang="en">Parameters quantifying the proportion of organic material in a soil or sediment sample</rdfs:comment>
        <rdfs:label xml:lang="en">Concentration of organic matter in sediments</rdfs:label>
        <rdf:type rdf:resource="http://www.w3.org/2002/07/owl#NamedIndividual"/>
        <rdf:type rdf:resource="http://www.w3.org/2002/07/owl#Class"/>
      </glview:MeasurementType>
    </rdfs:subClassOf>
    <owl:someValuesFrom>
      <owl:Class>
        <owl:oneOf rdf:parseType="Collection">
          <glview:MeasurementType rdf:about="http://schema.geolink.org/dev/voc/nvs/P02#STOM"/>
        </owl:oneOf>
      </owl:Class>
    </owl:someValuesFrom>
    <owl:onProperty rdf:resource="http://schema.geolink.org/dev/view#hasMeasurementType"/>
  </owl:Restriction>
  <owl:Restriction>
    <rdfs:subClassOf>
      <glview:MeasurementType rdf:about="http://schema.geolink.org/dev/voc/nvs/P02#BATC">
        <rdfs:subClassOf rdf:resource="http://schema.geolink.org/dev/voc/nvs/P03#B070"/>
        <rdfs:subClassOf rdf:resource="http://schema.geolink.org/dev/voc/nvs/P03#B005"/>
        <rdfs:seeAlso rdf:resource="http://vocab.nerc.ac.uk/collection/P02/current/BATC/"/>
        <rdfs:comment xml:lang="en">Bacteria carbon biomass parameters presented at the level of taxa that may be mapped to entities in the ITIS taxonomy.  These may be at any taxonomic level from sub-species upwards.  Bacteria are defined as all taxa that fall into Kingdom Monera in the ITIS taxonomy, which includes cyanobacteria.</rdfs:comment>
        <rdfs:label xml:lang="en">Bacteria taxonomy-related biomass expressed as carbon per unit volume of the water column</rdfs:label>
        <rdf:type rdf:resource="http://www.w3.org/2002/07/owl#NamedIndividual"/>
        <rdf:type rdf:resource="http://www.w3.org/2002/07/owl#Class"/>
      </glview:MeasurementType>
    </rdfs:subClassOf>
    <owl:someValuesFrom>
      <owl:Class>
        <owl:oneOf rdf:parseType="Collection">
          <glview:MeasurementType rdf:about="http://schema.geolink.org/dev/voc/nvs/P02#BATC"/>
        </owl:oneOf>
      </owl:Class>
    </owl:someValuesFrom>
    <owl:onProperty rdf:resource="http://schema.geolink.org/dev/view#hasMeasurementType"/>
  </owl:Restriction>
  <owl:Restriction>
    <rdfs:subClassOf rdf:resource="http://schema.geolink.org/dev/voc/nvs/P02#NTPW"/>
    <owl:someValuesFrom>
      <owl:Class>
        <owl:oneOf rdf:parseType="Collection">
          <glview:MeasurementType rdf:about="http://schema.geolink.org/dev/voc/nvs/P02#NTPW"/>
        </owl:oneOf>
      </owl:Class>
    </owl:someValuesFrom>
    <owl:onProperty rdf:resource="http://schema.geolink.org/dev/view#hasMeasurementType"/>
  </owl:Restriction>
  <owl:Restriction>
    <rdfs:subClassOf rdf:resource="http://schema.geolink.org/dev/voc/nvs/P02#SCAH"/>
    <owl:someValuesFrom>
      <owl:Class>
        <owl:oneOf rdf:parseType="Collection">
          <glview:MeasurementType rdf:about="http://schema.geolink.org/dev/voc/nvs/P02#SCAH"/>
        </owl:oneOf>
      </owl:Class>
    </owl:someValuesFrom>
    <owl:onProperty rdf:resource="http://schema.geolink.org/dev/view#hasMeasurementType"/>
  </owl:Restriction>
  <owl:Restriction>
    <rdfs:subClassOf rdf:resource="http://schema.geolink.org/dev/voc/nvs/P02#PPCB"/>
    <owl:someValuesFrom>
      <owl:Class>
        <owl:oneOf rdf:parseType="Collection">
          <glview:MeasurementType rdf:about="http://schema.geolink.org/dev/voc/nvs/P02#PPCB"/>
        </owl:oneOf>
      </owl:Class>
    </owl:someValuesFrom>
    <owl:onProperty rdf:resource="http://schema.geolink.org/dev/view#hasMeasurementType"/>
  </owl:Restriction>
  <owl:Restriction>
    <rdfs:subClassOf>
      <glview:MeasurementType rdf:about="http://schema.geolink.org/dev/voc/nvs/P02#NTRZ">
        <rdfs:subClassOf rdf:resource="http://schema.geolink.org/dev/voc/nvs/P02#NTRA"/>
        <rdfs:seeAlso rdf:resource="http://vocab.nerc.ac.uk/collection/P02/current/NTRZ/"/>
        <rdfs:comment xml:lang="en">Deprecated term from a misguided attempt to distinguish between NO3 and NO3+NO2 for discovery. Use parameter group NTRA instead</rdfs:comment>
        <rdfs:label xml:lang="en">Nitrate+nitrite concentration parameters in the water column</rdfs:label>
        <rdf:type rdf:resource="http://www.w3.org/2002/07/owl#NamedIndividual"/>
        <rdf:type rdf:resource="http://www.w3.org/2002/07/owl#Class"/>
      </glview:MeasurementType>
    </rdfs:subClassOf>
    <owl:someValuesFrom>
      <owl:Class>
        <owl:oneOf rdf:parseType="Collection">
          <glview:MeasurementType rdf:about="http://schema.geolink.org/dev/voc/nvs/P02#NTRZ"/>
        </owl:oneOf>
      </owl:Class>
    </owl:someValuesFrom>
    <owl:onProperty rdf:resource="http://schema.geolink.org/dev/view#hasMeasurementType"/>
  </owl:Restriction>
  <owl:Restriction>
    <rdfs:subClassOf rdf:resource="http://schema.geolink.org/dev/voc/nvs/P02#PXSP"/>
    <owl:someValuesFrom>
      <owl:Class>
        <owl:oneOf rdf:parseType="Collection">
          <glview:MeasurementType rdf:about="http://schema.geolink.org/dev/voc/nvs/P02#PXSP"/>
        </owl:oneOf>
      </owl:Class>
    </owl:someValuesFrom>
    <owl:onProperty rdf:resource="http://schema.geolink.org/dev/view#hasMeasurementType"/>
  </owl:Restriction>
  <owl:Restriction>
    <rdfs:subClassOf rdf:resource="http://schema.geolink.org/dev/voc/nvs/P02#ZWTX"/>
    <owl:someValuesFrom>
      <owl:Class>
        <owl:oneOf rdf:parseType="Collection">
          <glview:MeasurementType rdf:about="http://schema.geolink.org/dev/voc/nvs/P02#ZWTX"/>
        </owl:oneOf>
      </owl:Class>
    </owl:someValuesFrom>
    <owl:onProperty rdf:resource="http://schema.geolink.org/dev/view#hasMeasurementType"/>
  </owl:Restriction>
  <owl:Restriction>
    <rdfs:subClassOf rdf:resource="http://schema.geolink.org/dev/voc/nvs/P02#FIBM"/>
    <owl:someValuesFrom>
      <owl:Class>
        <owl:oneOf rdf:parseType="Collection">
          <glview:MeasurementType rdf:about="http://schema.geolink.org/dev/voc/nvs/P02#FIBM"/>
        </owl:oneOf>
      </owl:Class>
    </owl:someValuesFrom>
    <owl:onProperty rdf:resource="http://schema.geolink.org/dev/view#hasMeasurementType"/>
  </owl:Restriction>
  <owl:Restriction>
    <rdfs:subClassOf>
      <glview:MeasurementType rdf:about="http://schema.geolink.org/dev/voc/nvs/P02#PHAT">
        <rdfs:subClassOf rdf:resource="http://schema.geolink.org/dev/voc/nvs/P03#M005"/>
        <rdfs:subClassOf rdf:resource="http://schema.geolink.org/dev/voc/nvs/P03#C005"/>
        <rdfs:seeAlso rdf:resource="http://vocab.nerc.ac.uk/collection/P02/current/PHAT/"/>
        <rdfs:comment xml:lang="en">Concentration of inorganic phosphorus species (element or compounds) in any phase of the atmosphere</rdfs:comment>
        <rdfs:label xml:lang="en">Inorganic phosphorus species concentrations in the atmosphere</rdfs:label>
        <rdf:type rdf:resource="http://www.w3.org/2002/07/owl#NamedIndividual"/>
        <rdf:type rdf:resource="http://www.w3.org/2002/07/owl#Class"/>
      </glview:MeasurementType>
    </rdfs:subClassOf>
    <owl:someValuesFrom>
      <owl:Class>
        <owl:oneOf rdf:parseType="Collection">
          <glview:MeasurementType rdf:about="http://schema.geolink.org/dev/voc/nvs/P02#PHAT"/>
        </owl:oneOf>
      </owl:Class>
    </owl:someValuesFrom>
    <owl:onProperty rdf:resource="http://schema.geolink.org/dev/view#hasMeasurementType"/>
  </owl:Restriction>
  <owl:Restriction>
    <rdfs:subClassOf>
      <glview:MeasurementType rdf:about="http://schema.geolink.org/dev/voc/nvs/P02#ZFIT">
        <rdfs:subClassOf rdf:resource="http://schema.geolink.org/dev/voc/nvs/P03#G055"/>
        <rdfs:seeAlso rdf:resource="http://vocab.nerc.ac.uk/collection/P02/current/ZFIT/"/>
        <rdfs:comment xml:lang="en">Parameters indicating the health of zooplankton and zoobenthos taxa, such as fecundity, egg condition, presence of parasites/diseases etc.</rdfs:comment>
        <rdfs:label xml:lang="en">Zooplankton and zoobenthos physiological condition parameters</rdfs:label>
        <rdf:type rdf:resource="http://www.w3.org/2002/07/owl#NamedIndividual"/>
        <rdf:type rdf:resource="http://www.w3.org/2002/07/owl#Class"/>
      </glview:MeasurementType>
    </rdfs:subClassOf>
    <owl:someValuesFrom>
      <owl:Class>
        <owl:oneOf rdf:parseType="Collection">
          <glview:MeasurementType rdf:about="http://schema.geolink.org/dev/voc/nvs/P02#ZFIT"/>
        </owl:oneOf>
      </owl:Class>
    </owl:someValuesFrom>
    <owl:onProperty rdf:resource="http://schema.geolink.org/dev/view#hasMeasurementType"/>
  </owl:Restriction>
  <owl:Restriction>
    <rdfs:subClassOf rdf:resource="http://schema.geolink.org/dev/voc/nvs/P02#GP067"/>
    <owl:someValuesFrom>
      <owl:Class>
        <owl:oneOf rdf:parseType="Collection">
          <glview:MeasurementType rdf:about="http://schema.geolink.org/dev/voc/nvs/P02#GP067"/>
        </owl:oneOf>
      </owl:Class>
    </owl:someValuesFrom>
    <owl:onProperty rdf:resource="http://schema.geolink.org/dev/view#hasMeasurementType"/>
  </owl:Restriction>
  <owl:Restriction>
    <rdfs:subClassOf>
      <glview:MeasurementType rdf:about="http://schema.geolink.org/dev/voc/nvs/P02#CARO">
        <rdfs:subClassOf rdf:resource="http://schema.geolink.org/dev/voc/nvs/P03#B035"/>
        <rdfs:seeAlso rdf:resource="http://vocab.nerc.ac.uk/collection/P02/current/CARO/"/>
        <rdfs:comment></rdfs:comment>
        <rdfs:label xml:lang="en">Carotenoid pigment concentrations in the water column</rdfs:label>
        <rdf:type rdf:resource="http://www.w3.org/2002/07/owl#NamedIndividual"/>
        <rdf:type rdf:resource="http://www.w3.org/2002/07/owl#Class"/>
      </glview:MeasurementType>
    </rdfs:subClassOf>
    <owl:someValuesFrom>
      <owl:Class>
        <owl:oneOf rdf:parseType="Collection">
          <glview:MeasurementType rdf:about="http://schema.geolink.org/dev/voc/nvs/P02#CARO"/>
        </owl:oneOf>
      </owl:Class>
    </owl:someValuesFrom>
    <owl:onProperty rdf:resource="http://schema.geolink.org/dev/view#hasMeasurementType"/>
  </owl:Restriction>
  <owl:Restriction>
    <rdfs:subClassOf rdf:resource="http://schema.geolink.org/dev/voc/nvs/P02#FREP"/>
    <owl:someValuesFrom>
      <owl:Class>
        <owl:oneOf rdf:parseType="Collection">
          <glview:MeasurementType rdf:about="http://schema.geolink.org/dev/voc/nvs/P02#FREP"/>
        </owl:oneOf>
      </owl:Class>
    </owl:someValuesFrom>
    <owl:onProperty rdf:resource="http://schema.geolink.org/dev/view#hasMeasurementType"/>
  </owl:Restriction>
  <owl:Restriction>
    <rdfs:subClassOf>
      <glview:MeasurementType rdf:about="http://schema.geolink.org/dev/voc/nvs/P02#GWAM">
        <rdfs:subClassOf rdf:resource="http://schema.geolink.org/dev/voc/nvs/P03#T001"/>
        <rdfs:seeAlso rdf:resource="http://vocab.nerc.ac.uk/collection/P02/current/GWAM/"/>
        <rdfs:comment xml:lang="en">Parameters quantifying the amount of groundwater in a given system such as aquifer water level and rate of flow of water through rock formations.</rdfs:comment>
        <rdfs:label xml:lang="en">Groundwater amount</rdfs:label>
        <rdf:type rdf:resource="http://www.w3.org/2002/07/owl#NamedIndividual"/>
        <rdf:type rdf:resource="http://www.w3.org/2002/07/owl#Class"/>
      </glview:MeasurementType>
    </rdfs:subClassOf>
    <owl:someValuesFrom>
      <owl:Class>
        <owl:oneOf rdf:parseType="Collection">
          <glview:MeasurementType rdf:about="http://schema.geolink.org/dev/voc/nvs/P02#GWAM"/>
        </owl:oneOf>
      </owl:Class>
    </owl:someValuesFrom>
    <owl:onProperty rdf:resource="http://schema.geolink.org/dev/view#hasMeasurementType"/>
  </owl:Restriction>
  <owl:Restriction>
    <rdfs:subClassOf rdf:resource="http://schema.geolink.org/dev/voc/nvs/P02#PEBI"/>
    <owl:someValuesFrom>
      <owl:Class>
        <owl:oneOf rdf:parseType="Collection">
          <glview:MeasurementType rdf:about="http://schema.geolink.org/dev/voc/nvs/P02#PEBI"/>
        </owl:oneOf>
      </owl:Class>
    </owl:someValuesFrom>
    <owl:onProperty rdf:resource="http://schema.geolink.org/dev/view#hasMeasurementType"/>
  </owl:Restriction>
  <owl:Restriction>
    <rdfs:subClassOf>
      <glview:MeasurementType rdf:about="http://schema.geolink.org/dev/voc/nvs/P02#FEFF">
        <rdfs:subClassOf rdf:resource="http://schema.geolink.org/dev/voc/nvs/P03#H004"/>
        <rdfs:seeAlso rdf:resource="http://vocab.nerc.ac.uk/collection/P02/current/FEFF/"/>
        <rdfs:comment xml:lang="en">Parameters that quantify or classify the physical or financial resources used in fishing activities</rdfs:comment>
        <rdfs:label xml:lang="en">Fishing effort</rdfs:label>
        <rdf:type rdf:resource="http://www.w3.org/2002/07/owl#NamedIndividual"/>
        <rdf:type rdf:resource="http://www.w3.org/2002/07/owl#Class"/>
      </glview:MeasurementType>
    </rdfs:subClassOf>
    <owl:someValuesFrom>
      <owl:Class>
        <owl:oneOf rdf:parseType="Collection">
          <glview:MeasurementType rdf:about="http://schema.geolink.org/dev/voc/nvs/P02#FEFF"/>
        </owl:oneOf>
      </owl:Class>
    </owl:someValuesFrom>
    <owl:onProperty rdf:resource="http://schema.geolink.org/dev/view#hasMeasurementType"/>
  </owl:Restriction>
  <owl:Restriction>
    <rdfs:subClassOf rdf:resource="http://schema.geolink.org/dev/voc/nvs/P02#TVLT"/>
    <owl:someValuesFrom>
      <owl:Class>
        <owl:oneOf rdf:parseType="Collection">
          <glview:MeasurementType rdf:about="http://schema.geolink.org/dev/voc/nvs/P02#TVLT"/>
        </owl:oneOf>
      </owl:Class>
    </owl:someValuesFrom>
    <owl:onProperty rdf:resource="http://schema.geolink.org/dev/view#hasMeasurementType"/>
  </owl:Restriction>
  <owl:Restriction>
    <rdfs:subClassOf>
      <glview:MeasurementType rdf:about="http://schema.geolink.org/dev/voc/nvs/P02#CHUM">
        <rdfs:subClassOf rdf:resource="http://schema.geolink.org/dev/voc/nvs/P03#M010"/>
        <rdfs:seeAlso rdf:resource="http://vocab.nerc.ac.uk/collection/P02/current/CHUM/"/>
        <rdfs:comment xml:lang="en">Parameters that either quantify the water content of moist air or are specifically used in its determination (eg wet bulb air temperature)</rdfs:comment>
        <rdfs:label xml:lang="en">Atmospheric humidity</rdfs:label>
        <rdf:type rdf:resource="http://www.w3.org/2002/07/owl#NamedIndividual"/>
        <rdf:type rdf:resource="http://www.w3.org/2002/07/owl#Class"/>
      </glview:MeasurementType>
    </rdfs:subClassOf>
    <owl:someValuesFrom>
      <owl:Class>
        <owl:oneOf rdf:parseType="Collection">
          <glview:MeasurementType rdf:about="http://schema.geolink.org/dev/voc/nvs/P02#CHUM"/>
        </owl:oneOf>
      </owl:Class>
    </owl:someValuesFrom>
    <owl:onProperty rdf:resource="http://schema.geolink.org/dev/view#hasMeasurementType"/>
  </owl:Restriction>
  <owl:Restriction>
    <rdfs:subClassOf rdf:resource="http://schema.geolink.org/dev/voc/nvs/P02#PEBI"/>
    <owl:someValuesFrom>
      <owl:Class>
        <owl:oneOf rdf:parseType="Collection">
          <glview:MeasurementType rdf:about="http://schema.geolink.org/dev/voc/nvs/P02#PEBI"/>
        </owl:oneOf>
      </owl:Class>
    </owl:someValuesFrom>
    <owl:onProperty rdf:resource="http://schema.geolink.org/dev/view#hasMeasurementType"/>
  </owl:Restriction>
  <owl:Restriction>
    <rdfs:subClassOf>
      <glview:MeasurementType rdf:about="http://schema.geolink.org/dev/voc/nvs/P02#BPRP">
        <rdfs:subClassOf rdf:resource="http://schema.geolink.org/dev/voc/nvs/P03#B027"/>
        <rdfs:seeAlso rdf:resource="http://vocab.nerc.ac.uk/collection/P02/current/BPRP/"/>
        <rdfs:comment xml:lang="en">Parameters that quantify any attribute of an unspecified biological entity and therefore do not map to the biologically classified P02 categories. This concept was created deprecated as a fix.</rdfs:comment>
        <rdfs:label xml:lang="en">Biota properties</rdfs:label>
        <rdf:type rdf:resource="http://www.w3.org/2002/07/owl#NamedIndividual"/>
        <rdf:type rdf:resource="http://www.w3.org/2002/07/owl#Class"/>
      </glview:MeasurementType>
    </rdfs:subClassOf>
    <owl:someValuesFrom>
      <owl:Class>
        <owl:oneOf rdf:parseType="Collection">
          <glview:MeasurementType rdf:about="http://schema.geolink.org/dev/voc/nvs/P02#BPRP"/>
        </owl:oneOf>
      </owl:Class>
    </owl:someValuesFrom>
    <owl:onProperty rdf:resource="http://schema.geolink.org/dev/view#hasMeasurementType"/>
  </owl:Restriction>
  <owl:Restriction>
    <rdfs:subClassOf rdf:resource="http://schema.geolink.org/dev/voc/nvs/P02#ZADX"/>
    <owl:someValuesFrom>
      <owl:Class>
        <owl:oneOf rdf:parseType="Collection">
          <glview:MeasurementType rdf:about="http://schema.geolink.org/dev/voc/nvs/P02#ZADX"/>
        </owl:oneOf>
      </owl:Class>
    </owl:someValuesFrom>
    <owl:onProperty rdf:resource="http://schema.geolink.org/dev/view#hasMeasurementType"/>
  </owl:Restriction>
  <owl:Restriction>
    <rdfs:subClassOf rdf:resource="http://schema.geolink.org/dev/voc/nvs/P02#BABI"/>
    <owl:someValuesFrom>
      <owl:Class>
        <owl:oneOf rdf:parseType="Collection">
          <glview:MeasurementType rdf:about="http://schema.geolink.org/dev/voc/nvs/P02#BABI"/>
        </owl:oneOf>
      </owl:Class>
    </owl:someValuesFrom>
    <owl:onProperty rdf:resource="http://schema.geolink.org/dev/view#hasMeasurementType"/>
  </owl:Restriction>
  <owl:Restriction>
    <rdfs:subClassOf rdf:resource="http://schema.geolink.org/dev/voc/nvs/P02#PCAH"/>
    <owl:someValuesFrom>
      <owl:Class>
        <owl:oneOf rdf:parseType="Collection">
          <owl:Class rdf:about="http://schema.geolink.org/dev/voc/nvs/P02#PCAH"/>
        </owl:oneOf>
      </owl:Class>
    </owl:someValuesFrom>
    <owl:onProperty rdf:resource="http://schema.geolink.org/dev/view#hasMeasurementType"/>
  </owl:Restriction>
  <owl:Restriction>
    <rdfs:subClassOf rdf:resource="http://schema.geolink.org/dev/voc/nvs/P02#TADN"/>
    <owl:someValuesFrom>
      <owl:Class>
        <owl:oneOf rdf:parseType="Collection">
          <glview:MeasurementType rdf:about="http://schema.geolink.org/dev/voc/nvs/P02#TADN"/>
        </owl:oneOf>
      </owl:Class>
    </owl:someValuesFrom>
    <owl:onProperty rdf:resource="http://schema.geolink.org/dev/view#hasMeasurementType"/>
  </owl:Restriction>
  <owl:Restriction>
    <rdfs:subClassOf>
      <glview:MeasurementType rdf:about="http://schema.geolink.org/dev/voc/nvs/P02#ZATP">
        <rdfs:subClassOf rdf:resource="http://schema.geolink.org/dev/voc/nvs/P03#B045"/>
        <rdfs:subClassOf rdf:resource="http://schema.geolink.org/dev/voc/nvs/P03#B070"/>
        <rdfs:seeAlso rdf:resource="http://vocab.nerc.ac.uk/collection/P02/current/ZATP/"/>
        <rdfs:comment xml:lang="en">Zooplankton (mesozooplankton plus larger pelagic animals excluding fish, reptiles and mammals) protein biomass per unit volume for entities that have been identified by taxonomic name</rdfs:comment>
        <rdfs:label xml:lang="en">Zooplankton taxonomy-related biomass expressed as protein per unit volume of the water column</rdfs:label>
        <rdf:type rdf:resource="http://www.w3.org/2002/07/owl#NamedIndividual"/>
        <rdf:type rdf:resource="http://www.w3.org/2002/07/owl#Class"/>
      </glview:MeasurementType>
    </rdfs:subClassOf>
    <owl:someValuesFrom>
      <owl:Class>
        <owl:oneOf rdf:parseType="Collection">
          <glview:MeasurementType rdf:about="http://schema.geolink.org/dev/voc/nvs/P02#ZATP"/>
        </owl:oneOf>
      </owl:Class>
    </owl:someValuesFrom>
    <owl:onProperty rdf:resource="http://schema.geolink.org/dev/view#hasMeasurementType"/>
  </owl:Restriction>
  <owl:Restriction>
    <rdfs:subClassOf>
      <glview:MeasurementType rdf:about="http://schema.geolink.org/dev/voc/nvs/P02#SPRO">
        <rdfs:subClassOf rdf:resource="http://schema.geolink.org/dev/voc/nvs/P03#C050"/>
        <rdfs:subClassOf rdf:resource="http://schema.geolink.org/dev/voc/nvs/P03#G035"/>
        <rdfs:seeAlso rdf:resource="http://vocab.nerc.ac.uk/collection/P02/current/SPRO/"/>
        <rdfs:comment xml:lang="en">Concentrations of proteins per unit mass or unit volume of sediment (material collected by a corer including fluff)</rdfs:comment>
        <rdfs:label xml:lang="en">Concentration of proteins in sediment</rdfs:label>
        <rdf:type rdf:resource="http://www.w3.org/2002/07/owl#NamedIndividual"/>
        <rdf:type rdf:resource="http://www.w3.org/2002/07/owl#Class"/>
      </glview:MeasurementType>
    </rdfs:subClassOf>
    <owl:someValuesFrom>
      <owl:Class>
        <owl:oneOf rdf:parseType="Collection">
          <glview:MeasurementType rdf:about="http://schema.geolink.org/dev/voc/nvs/P02#SPRO"/>
        </owl:oneOf>
      </owl:Class>
    </owl:someValuesFrom>
    <owl:onProperty rdf:resource="http://schema.geolink.org/dev/view#hasMeasurementType"/>
  </owl:Restriction>
  <owl:Restriction>
    <rdfs:subClassOf>
      <glview:MeasurementType rdf:about="http://schema.geolink.org/dev/voc/nvs/P02#QDMD">
        <rdfs:subClassOf rdf:resource="http://schema.geolink.org/dev/voc/nvs/P03#H001"/>
        <rdfs:seeAlso rdf:resource="http://vocab.nerc.ac.uk/collection/P02/current/QDMD/"/>
        <rdfs:comment xml:lang="en">Parameters quantifying the amount of liquids (e.g. ship's ballast) or solids (e.g. dredge spoil) deposited into the water column as a result of man's activities</rdfs:comment>
        <rdfs:label xml:lang="en">Quantity of material dumped</rdfs:label>
        <rdf:type rdf:resource="http://www.w3.org/2002/07/owl#NamedIndividual"/>
        <rdf:type rdf:resource="http://www.w3.org/2002/07/owl#Class"/>
      </glview:MeasurementType>
    </rdfs:subClassOf>
    <owl:someValuesFrom>
      <owl:Class>
        <owl:oneOf rdf:parseType="Collection">
          <glview:MeasurementType rdf:about="http://schema.geolink.org/dev/voc/nvs/P02#QDMD"/>
        </owl:oneOf>
      </owl:Class>
    </owl:someValuesFrom>
    <owl:onProperty rdf:resource="http://schema.geolink.org/dev/view#hasMeasurementType"/>
  </owl:Restriction>
  <owl:Restriction>
    <rdfs:subClassOf>
      <glview:MeasurementType rdf:about="http://schema.geolink.org/dev/voc/nvs/P02#CPWC">
        <rdfs:subClassOf rdf:resource="http://schema.geolink.org/dev/voc/nvs/P03#B035"/>
        <rdfs:seeAlso rdf:resource="http://vocab.nerc.ac.uk/collection/P02/current/CPWC/"/>
        <rdfs:comment xml:lang="en">Includes all variants of chlorophyll expressed in terms of per unit volume or unit area of the water column.  Does not include data expressed per unit mass of SPM.</rdfs:comment>
        <rdfs:label xml:lang="en">Chlorophyll pigment concentrations in the water column</rdfs:label>
        <rdf:type rdf:resource="http://www.w3.org/2002/07/owl#NamedIndividual"/>
        <rdf:type rdf:resource="http://www.w3.org/2002/07/owl#Class"/>
      </glview:MeasurementType>
    </rdfs:subClassOf>
    <owl:someValuesFrom>
      <owl:Class>
        <owl:oneOf rdf:parseType="Collection">
          <glview:MeasurementType rdf:about="http://schema.geolink.org/dev/voc/nvs/P02#CPWC"/>
        </owl:oneOf>
      </owl:Class>
    </owl:someValuesFrom>
    <owl:onProperty rdf:resource="http://schema.geolink.org/dev/view#hasMeasurementType"/>
  </owl:Restriction>
  <owl:Restriction>
    <rdfs:subClassOf>
      <glview:MeasurementType rdf:about="http://schema.geolink.org/dev/voc/nvs/P02#MZBC">
        <rdfs:subClassOf rdf:resource="http://schema.geolink.org/dev/voc/nvs/P03#B025"/>
        <rdfs:subClassOf rdf:resource="http://schema.geolink.org/dev/voc/nvs/P03#B070"/>
        <rdfs:seeAlso rdf:resource="http://vocab.nerc.ac.uk/collection/P02/current/MZBC/"/>
        <rdfs:comment xml:lang="en">Basically, any microzooplankton carbon biomass measurement that isn't included in parameter group MATC.  May include data integrations such as 'total microzooplankton'.</rdfs:comment>
        <rdfs:label xml:lang="en">Microzooplankton non taxonomy-related biomass expressed as carbon per unit volume of the water column</rdfs:label>
        <rdf:type rdf:resource="http://www.w3.org/2002/07/owl#NamedIndividual"/>
        <rdf:type rdf:resource="http://www.w3.org/2002/07/owl#Class"/>
      </glview:MeasurementType>
    </rdfs:subClassOf>
    <owl:someValuesFrom>
      <owl:Class>
        <owl:oneOf rdf:parseType="Collection">
          <glview:MeasurementType rdf:about="http://schema.geolink.org/dev/voc/nvs/P02#MZBC"/>
        </owl:oneOf>
      </owl:Class>
    </owl:someValuesFrom>
    <owl:onProperty rdf:resource="http://schema.geolink.org/dev/view#hasMeasurementType"/>
  </owl:Restriction>
  <owl:Restriction>
    <rdfs:subClassOf>
      <glview:MeasurementType rdf:about="http://schema.geolink.org/dev/voc/nvs/P02#MINC">
        <rdfs:subClassOf rdf:resource="http://schema.geolink.org/dev/voc/nvs/P03#G045"/>
        <rdfs:subClassOf rdf:resource="http://schema.geolink.org/dev/voc/nvs/P03#G035"/>
        <rdfs:seeAlso rdf:resource="http://vocab.nerc.ac.uk/collection/P02/current/MINC/"/>
        <rdfs:comment xml:lang="en">Chemical analyses of minerals extracted from rocks or sediment or analysed in-situ using techniques like the electron microprobe.</rdfs:comment>
        <rdfs:label xml:lang="en">Mineral chemistry</rdfs:label>
        <rdf:type rdf:resource="http://www.w3.org/2002/07/owl#NamedIndividual"/>
        <rdf:type rdf:resource="http://www.w3.org/2002/07/owl#Class"/>
      </glview:MeasurementType>
    </rdfs:subClassOf>
    <owl:someValuesFrom>
      <owl:Class>
        <owl:oneOf rdf:parseType="Collection">
          <glview:MeasurementType rdf:about="http://schema.geolink.org/dev/voc/nvs/P02#MINC"/>
        </owl:oneOf>
      </owl:Class>
    </owl:someValuesFrom>
    <owl:onProperty rdf:resource="http://schema.geolink.org/dev/view#hasMeasurementType"/>
  </owl:Restriction>
  <owl:Restriction>
    <rdfs:subClassOf>
      <glview:MeasurementType rdf:about="http://schema.geolink.org/dev/voc/nvs/P02#MFLZ">
        <rdfs:subClassOf rdf:resource="http://schema.geolink.org/dev/voc/nvs/P03#B070"/>
        <rdfs:subClassOf rdf:resource="http://schema.geolink.org/dev/voc/nvs/P03#G055"/>
        <rdfs:seeAlso rdf:resource="http://vocab.nerc.ac.uk/collection/P02/current/MFLZ/"/>
        <rdfs:comment xml:lang="en">Any zoobenthos abundance per unit area of the littoral zone (between spring tide high and low water) parameters that are not fish or terrestrial animals (insecta/oligochaeta)</rdfs:comment>
        <rdfs:label xml:lang="en">Zoobenthos taxonomy-related abundance per unit area of the littoral zone</rdfs:label>
        <rdf:type rdf:resource="http://www.w3.org/2002/07/owl#NamedIndividual"/>
        <rdf:type rdf:resource="http://www.w3.org/2002/07/owl#Class"/>
      </glview:MeasurementType>
    </rdfs:subClassOf>
    <owl:someValuesFrom>
      <owl:Class>
        <owl:oneOf rdf:parseType="Collection">
          <glview:MeasurementType rdf:about="http://schema.geolink.org/dev/voc/nvs/P02#MFLZ"/>
        </owl:oneOf>
      </owl:Class>
    </owl:someValuesFrom>
    <owl:onProperty rdf:resource="http://schema.geolink.org/dev/view#hasMeasurementType"/>
  </owl:Restriction>
  <owl:Restriction>
    <rdfs:subClassOf>
      <glview:MeasurementType rdf:about="http://schema.geolink.org/dev/voc/nvs/P02#GP050">
        <rdfs:subClassOf rdf:resource="http://schema.geolink.org/dev/voc/nvs/P03#H001"/>
        <rdfs:subClassOf rdf:resource="http://schema.geolink.org/dev/voc/nvs/P03#M005"/>
        <rdfs:seeAlso rdf:resource="http://vocab.nerc.ac.uk/collection/P02/current/GP050/"/>
        <rdfs:comment xml:lang="en">Parameters quantifying polycyclic aromatic hydrocarbon (PAH) concentrations in all phases of the atmosphere</rdfs:comment>
        <rdfs:label xml:lang="en">Concentration of polycyclic aromatic hydrocarbons (PAHs) in the atmosphere</rdfs:label>
        <rdf:type rdf:resource="http://www.w3.org/2002/07/owl#NamedIndividual"/>
        <rdf:type rdf:resource="http://www.w3.org/2002/07/owl#Class"/>
      </glview:MeasurementType>
    </rdfs:subClassOf>
    <owl:someValuesFrom>
      <owl:Class>
        <owl:oneOf rdf:parseType="Collection">
          <glview:MeasurementType rdf:about="http://schema.geolink.org/dev/voc/nvs/P02#GP050"/>
        </owl:oneOf>
      </owl:Class>
    </owl:someValuesFrom>
    <owl:onProperty rdf:resource="http://schema.geolink.org/dev/view#hasMeasurementType"/>
  </owl:Restriction>
  <owl:Restriction>
    <rdfs:subClassOf rdf:resource="http://schema.geolink.org/dev/voc/nvs/P02#DVLP"/>
    <owl:someValuesFrom>
      <owl:Class>
        <owl:oneOf rdf:parseType="Collection">
          <glview:MeasurementType rdf:about="http://schema.geolink.org/dev/voc/nvs/P02#DVLP"/>
        </owl:oneOf>
      </owl:Class>
    </owl:someValuesFrom>
    <owl:onProperty rdf:resource="http://schema.geolink.org/dev/view#hasMeasurementType"/>
  </owl:Restriction>
  <owl:Restriction>
    <rdfs:subClassOf>
      <glview:MeasurementType rdf:about="http://schema.geolink.org/dev/voc/nvs/P02#GP010">
        <rdfs:subClassOf rdf:resource="http://schema.geolink.org/dev/voc/nvs/P03#B060"/>
        <rdfs:seeAlso rdf:resource="http://vocab.nerc.ac.uk/collection/P02/current/GP010/"/>
        <rdfs:comment xml:lang="en">Parameters describing the effects of substances on living organisms.</rdfs:comment>
        <rdfs:label xml:lang="en">Bioassay and contaminant biological impact</rdfs:label>
        <rdf:type rdf:resource="http://www.w3.org/2002/07/owl#NamedIndividual"/>
        <rdf:type rdf:resource="http://www.w3.org/2002/07/owl#Class"/>
      </glview:MeasurementType>
    </rdfs:subClassOf>
    <owl:someValuesFrom>
      <owl:Class>
        <owl:oneOf rdf:parseType="Collection">
          <glview:MeasurementType rdf:about="http://schema.geolink.org/dev/voc/nvs/P02#GP010"/>
        </owl:oneOf>
      </owl:Class>
    </owl:someValuesFrom>
    <owl:onProperty rdf:resource="http://schema.geolink.org/dev/view#hasMeasurementType"/>
  </owl:Restriction>
  <owl:Restriction>
    <rdfs:subClassOf>
      <glview:MeasurementType rdf:about="http://schema.geolink.org/dev/voc/nvs/P02#NOYS">
        <rdfs:subClassOf rdf:resource="http://schema.geolink.org/dev/voc/nvs/P03#D005"/>
        <rdfs:seeAlso rdf:resource="http://vocab.nerc.ac.uk/collection/P02/current/NOYS/"/>
        <rdfs:comment></rdfs:comment>
        <rdfs:label xml:lang="en">Acoustic noise in the water column</rdfs:label>
        <rdf:type rdf:resource="http://www.w3.org/2002/07/owl#NamedIndividual"/>
        <rdf:type rdf:resource="http://www.w3.org/2002/07/owl#Class"/>
      </glview:MeasurementType>
    </rdfs:subClassOf>
    <owl:someValuesFrom>
      <owl:Class>
        <owl:oneOf rdf:parseType="Collection">
          <glview:MeasurementType rdf:about="http://schema.geolink.org/dev/voc/nvs/P02#NOYS"/>
        </owl:oneOf>
      </owl:Class>
    </owl:someValuesFrom>
    <owl:onProperty rdf:resource="http://schema.geolink.org/dev/view#hasMeasurementType"/>
  </owl:Restriction>
  <owl:Restriction>
    <rdfs:subClassOf rdf:resource="http://schema.geolink.org/dev/voc/nvs/P02#FBAB"/>
    <owl:someValuesFrom>
      <owl:Class>
        <owl:oneOf rdf:parseType="Collection">
          <glview:MeasurementType rdf:about="http://schema.geolink.org/dev/voc/nvs/P02#FBAB"/>
        </owl:oneOf>
      </owl:Class>
    </owl:someValuesFrom>
    <owl:onProperty rdf:resource="http://schema.geolink.org/dev/view#hasMeasurementType"/>
  </owl:Restriction>
  <owl:Restriction>
    <rdfs:subClassOf>
      <glview:MeasurementType rdf:about="http://schema.geolink.org/dev/voc/nvs/P02#SDNA">
        <rdfs:subClassOf rdf:resource="http://schema.geolink.org/dev/voc/nvs/P03#C050"/>
        <rdfs:subClassOf rdf:resource="http://schema.geolink.org/dev/voc/nvs/P03#G035"/>
        <rdfs:seeAlso rdf:resource="http://vocab.nerc.ac.uk/collection/P02/current/SDNA/"/>
        <rdfs:comment xml:lang="en">Parameters quantifying the amount of naturally-produced organic (molecules containing carbon) compounds that are built from multiple instances of structural units (monomers) that are covalently-bonded to produce larger structures in any sediment (material collected by a corer including fluff). Includes polynucleotides (RNA and DNA), polypeptides and polysaccharides (e.g. cellulose).</rdfs:comment>
        <rdfs:label xml:lang="en">Concentrations of biopolymers in sediment</rdfs:label>
        <rdf:type rdf:resource="http://www.w3.org/2002/07/owl#NamedIndividual"/>
        <rdf:type rdf:resource="http://www.w3.org/2002/07/owl#Class"/>
      </glview:MeasurementType>
    </rdfs:subClassOf>
    <owl:someValuesFrom>
      <owl:Class>
        <owl:oneOf rdf:parseType="Collection">
          <glview:MeasurementType rdf:about="http://schema.geolink.org/dev/voc/nvs/P02#SDNA"/>
        </owl:oneOf>
      </owl:Class>
    </owl:someValuesFrom>
    <owl:onProperty rdf:resource="http://schema.geolink.org/dev/view#hasMeasurementType"/>
  </owl:Restriction>
  <owl:Restriction>
    <rdfs:subClassOf rdf:resource="http://schema.geolink.org/dev/voc/nvs/P02#CNTX"/>
    <owl:someValuesFrom>
      <owl:Class>
        <owl:oneOf rdf:parseType="Collection">
          <glview:MeasurementType rdf:about="http://schema.geolink.org/dev/voc/nvs/P02#CNTX"/>
        </owl:oneOf>
      </owl:Class>
    </owl:someValuesFrom>
    <owl:onProperty rdf:resource="http://schema.geolink.org/dev/view#hasMeasurementType"/>
  </owl:Restriction>
  <owl:Restriction>
    <rdfs:subClassOf rdf:resource="http://schema.geolink.org/dev/voc/nvs/P02#MZBC"/>
    <owl:someValuesFrom>
      <owl:Class>
        <owl:oneOf rdf:parseType="Collection">
          <glview:MeasurementType rdf:about="http://schema.geolink.org/dev/voc/nvs/P02#MZBC"/>
        </owl:oneOf>
      </owl:Class>
    </owl:someValuesFrom>
    <owl:onProperty rdf:resource="http://schema.geolink.org/dev/view#hasMeasurementType"/>
  </owl:Restriction>
  <owl:Restriction>
    <rdfs:subClassOf>
      <glview:MeasurementType rdf:about="http://schema.geolink.org/dev/voc/nvs/P02#RBHY">
        <rdfs:subClassOf rdf:resource="http://schema.geolink.org/dev/voc/nvs/P03#B027"/>
        <rdfs:seeAlso rdf:resource="http://vocab.nerc.ac.uk/collection/P02/current/RBHY/"/>
        <rdfs:comment xml:lang="en">Any parameters relating to molecular biology or genetics</rdfs:comment>
        <rdfs:label xml:lang="en">Molecular biology parameters</rdfs:label>
        <rdf:type rdf:resource="http://www.w3.org/2002/07/owl#NamedIndividual"/>
        <rdf:type rdf:resource="http://www.w3.org/2002/07/owl#Class"/>
      </glview:MeasurementType>
    </rdfs:subClassOf>
    <owl:someValuesFrom>
      <owl:Class>
        <owl:oneOf rdf:parseType="Collection">
          <glview:MeasurementType rdf:about="http://schema.geolink.org/dev/voc/nvs/P02#RBHY"/>
        </owl:oneOf>
      </owl:Class>
    </owl:someValuesFrom>
    <owl:onProperty rdf:resource="http://schema.geolink.org/dev/view#hasMeasurementType"/>
  </owl:Restriction>
  <owl:Restriction>
    <rdfs:subClassOf rdf:resource="http://schema.geolink.org/dev/voc/nvs/P02#ZATP"/>
    <owl:someValuesFrom>
      <owl:Class>
        <owl:oneOf rdf:parseType="Collection">
          <glview:MeasurementType rdf:about="http://schema.geolink.org/dev/voc/nvs/P02#ZATP"/>
        </owl:oneOf>
      </owl:Class>
    </owl:someValuesFrom>
    <owl:onProperty rdf:resource="http://schema.geolink.org/dev/view#hasMeasurementType"/>
  </owl:Restriction>
  <owl:Restriction>
    <rdfs:subClassOf rdf:resource="http://schema.geolink.org/dev/voc/nvs/P02#SPRO"/>
    <owl:someValuesFrom>
      <owl:Class>
        <owl:oneOf rdf:parseType="Collection">
          <glview:MeasurementType rdf:about="http://schema.geolink.org/dev/voc/nvs/P02#SPRO"/>
        </owl:oneOf>
      </owl:Class>
    </owl:someValuesFrom>
    <owl:onProperty rdf:resource="http://schema.geolink.org/dev/view#hasMeasurementType"/>
  </owl:Restriction>
  <owl:Restriction>
    <rdfs:subClassOf>
      <glview:MeasurementType rdf:about="http://schema.geolink.org/dev/voc/nvs/P02#GERA">
        <rdfs:subClassOf rdf:resource="http://schema.geolink.org/dev/voc/nvs/P03#GPYS"/>
        <rdfs:seeAlso rdf:resource="http://vocab.nerc.ac.uk/collection/P02/current/GERA/"/>
        <rdfs:comment xml:lang="en">Parameters quantifying the level of radioactive emissions from in-situ geologic units</rdfs:comment>
        <rdfs:label xml:lang="en">Radiation geophysics</rdfs:label>
        <rdf:type rdf:resource="http://www.w3.org/2002/07/owl#NamedIndividual"/>
        <rdf:type rdf:resource="http://www.w3.org/2002/07/owl#Class"/>
      </glview:MeasurementType>
    </rdfs:subClassOf>
    <owl:someValuesFrom>
      <owl:Class>
        <owl:oneOf rdf:parseType="Collection">
          <glview:MeasurementType rdf:about="http://schema.geolink.org/dev/voc/nvs/P02#GERA"/>
        </owl:oneOf>
      </owl:Class>
    </owl:someValuesFrom>
    <owl:onProperty rdf:resource="http://schema.geolink.org/dev/view#hasMeasurementType"/>
  </owl:Restriction>
  <owl:Restriction>
    <rdfs:subClassOf rdf:resource="http://schema.geolink.org/dev/voc/nvs/P02#MINC"/>
    <owl:someValuesFrom>
      <owl:Class>
        <owl:oneOf rdf:parseType="Collection">
          <glview:MeasurementType rdf:about="http://schema.geolink.org/dev/voc/nvs/P02#MINC"/>
        </owl:oneOf>
      </owl:Class>
    </owl:someValuesFrom>
    <owl:onProperty rdf:resource="http://schema.geolink.org/dev/view#hasMeasurementType"/>
  </owl:Restriction>
  <owl:Restriction>
    <rdfs:subClassOf rdf:resource="http://schema.geolink.org/dev/voc/nvs/P02#TDIN"/>
    <owl:someValuesFrom>
      <owl:Class>
        <owl:oneOf rdf:parseType="Collection">
          <glview:MeasurementType rdf:about="http://schema.geolink.org/dev/voc/nvs/P02#TDIN"/>
        </owl:oneOf>
      </owl:Class>
    </owl:someValuesFrom>
    <owl:onProperty rdf:resource="http://schema.geolink.org/dev/view#hasMeasurementType"/>
  </owl:Restriction>
  <owl:Restriction>
    <rdfs:subClassOf rdf:resource="http://schema.geolink.org/dev/voc/nvs/P02#INLZ"/>
    <owl:someValuesFrom>
      <owl:Class>
        <owl:oneOf rdf:parseType="Collection">
          <glview:MeasurementType rdf:about="http://schema.geolink.org/dev/voc/nvs/P02#INLZ"/>
        </owl:oneOf>
      </owl:Class>
    </owl:someValuesFrom>
    <owl:onProperty rdf:resource="http://schema.geolink.org/dev/view#hasMeasurementType"/>
  </owl:Restriction>
  <owl:Restriction>
    <rdfs:subClassOf>
      <glview:MeasurementType rdf:about="http://schema.geolink.org/dev/voc/nvs/P02#MXLM">
        <rdfs:subClassOf rdf:resource="http://schema.geolink.org/dev/voc/nvs/P03#D020"/>
        <rdfs:seeAlso rdf:resource="http://vocab.nerc.ac.uk/collection/P02/current/MXLM/"/>
        <rdfs:comment xml:lang="en">Parameters describing or predicting water column structure plus parameters quantifying the dynamic stability of that structure</rdfs:comment>
        <rdfs:label xml:lang="en">Structure and stability of the water column</rdfs:label>
        <rdf:type rdf:resource="http://www.w3.org/2002/07/owl#NamedIndividual"/>
        <rdf:type rdf:resource="http://www.w3.org/2002/07/owl#Class"/>
      </glview:MeasurementType>
    </rdfs:subClassOf>
    <owl:someValuesFrom>
      <owl:Class>
        <owl:oneOf rdf:parseType="Collection">
          <glview:MeasurementType rdf:about="http://schema.geolink.org/dev/voc/nvs/P02#MXLM"/>
        </owl:oneOf>
      </owl:Class>
    </owl:someValuesFrom>
    <owl:onProperty rdf:resource="http://schema.geolink.org/dev/view#hasMeasurementType"/>
  </owl:Restriction>
  <owl:Restriction>
    <rdfs:subClassOf>
      <glview:MeasurementType rdf:about="http://schema.geolink.org/dev/voc/nvs/P02#AALK">
        <rdfs:subClassOf rdf:resource="http://schema.geolink.org/dev/voc/nvs/P03#C025"/>
        <rdfs:subClassOf rdf:resource="http://schema.geolink.org/dev/voc/nvs/P03#M005"/>
        <rdfs:seeAlso rdf:resource="http://vocab.nerc.ac.uk/collection/P02/current/AALK/"/>
        <rdfs:comment xml:lang="en">Alkane concentrations in all phases of the atmosphere</rdfs:comment>
        <rdfs:label xml:lang="en">Concentration of alkanes in the atmosphere</rdfs:label>
        <rdf:type rdf:resource="http://www.w3.org/2002/07/owl#NamedIndividual"/>
        <rdf:type rdf:resource="http://www.w3.org/2002/07/owl#Class"/>
      </glview:MeasurementType>
    </rdfs:subClassOf>
    <owl:someValuesFrom>
      <owl:Class>
        <owl:oneOf rdf:parseType="Collection">
          <glview:MeasurementType rdf:about="http://schema.geolink.org/dev/voc/nvs/P02#AALK"/>
        </owl:oneOf>
      </owl:Class>
    </owl:someValuesFrom>
    <owl:onProperty rdf:resource="http://schema.geolink.org/dev/view#hasMeasurementType"/>
  </owl:Restriction>
  <owl:Restriction>
    <rdfs:subClassOf>
      <glview:MeasurementType rdf:about="http://schema.geolink.org/dev/voc/nvs/P02#FR11">
        <rdfs:subClassOf rdf:resource="http://schema.geolink.org/dev/voc/nvs/P03#C020"/>
        <rdfs:seeAlso rdf:resource="http://vocab.nerc.ac.uk/collection/P02/current/FR11/"/>
        <rdfs:comment xml:lang="en">Concentrations of chlorofluorocarbons (also known as freons or CFCs) in sny body of water</rdfs:comment>
        <rdfs:label xml:lang="en">Chlorofluorocarbon concentrations in the water column</rdfs:label>
        <rdf:type rdf:resource="http://www.w3.org/2002/07/owl#NamedIndividual"/>
        <rdf:type rdf:resource="http://www.w3.org/2002/07/owl#Class"/>
      </glview:MeasurementType>
    </rdfs:subClassOf>
    <owl:someValuesFrom>
      <owl:Class>
        <owl:oneOf rdf:parseType="Collection">
          <glview:MeasurementType rdf:about="http://schema.geolink.org/dev/voc/nvs/P02#FR11"/>
        </owl:oneOf>
      </owl:Class>
    </owl:someValuesFrom>
    <owl:onProperty rdf:resource="http://schema.geolink.org/dev/view#hasMeasurementType"/>
  </owl:Restriction>
  <owl:Restriction>
    <rdfs:subClassOf>
      <glview:MeasurementType rdf:about="http://schema.geolink.org/dev/voc/nvs/P02#AXFX">
        <rdfs:subClassOf rdf:resource="http://schema.geolink.org/dev/voc/nvs/P03#B035"/>
        <rdfs:subClassOf rdf:resource="http://schema.geolink.org/dev/voc/nvs/P03#O005"/>
        <rdfs:seeAlso rdf:resource="http://vocab.nerc.ac.uk/collection/P02/current/AXFX/"/>
        <rdfs:comment></rdfs:comment>
        <rdfs:label xml:lang="en">Sedimentation flux of pigments in the water column</rdfs:label>
        <rdf:type rdf:resource="http://www.w3.org/2002/07/owl#NamedIndividual"/>
        <rdf:type rdf:resource="http://www.w3.org/2002/07/owl#Class"/>
      </glview:MeasurementType>
    </rdfs:subClassOf>
    <owl:someValuesFrom>
      <owl:Class>
        <owl:oneOf rdf:parseType="Collection">
          <glview:MeasurementType rdf:about="http://schema.geolink.org/dev/voc/nvs/P02#AXFX"/>
        </owl:oneOf>
      </owl:Class>
    </owl:someValuesFrom>
    <owl:onProperty rdf:resource="http://schema.geolink.org/dev/view#hasMeasurementType"/>
  </owl:Restriction>
  <owl:Restriction>
    <rdfs:subClassOf rdf:resource="http://schema.geolink.org/dev/voc/nvs/P02#BATX"/>
    <owl:someValuesFrom>
      <owl:Class>
        <owl:oneOf rdf:parseType="Collection">
          <glview:MeasurementType rdf:about="http://schema.geolink.org/dev/voc/nvs/P02#BATX"/>
        </owl:oneOf>
      </owl:Class>
    </owl:someValuesFrom>
    <owl:onProperty rdf:resource="http://schema.geolink.org/dev/view#hasMeasurementType"/>
  </owl:Restriction>
  <owl:Restriction>
    <rdfs:subClassOf>
      <glview:MeasurementType rdf:about="http://schema.geolink.org/dev/voc/nvs/P02#IPHY">
        <rdfs:subClassOf rdf:resource="http://schema.geolink.org/dev/voc/nvs/P03#M015"/>
        <rdfs:seeAlso rdf:resource="http://vocab.nerc.ac.uk/collection/P02/current/IPHY/"/>
        <rdfs:comment xml:lang="en">Parameters related to physical properties (e.g. colour, density, in-situ temperature) or characteristics (e.g. sea ice type) of any kind of water sample that was in its solid state at the time of sampling or measurement</rdfs:comment>
        <rdfs:label xml:lang="en">Snow and ice physical properties and characteristics</rdfs:label>
        <rdf:type rdf:resource="http://www.w3.org/2002/07/owl#NamedIndividual"/>
        <rdf:type rdf:resource="http://www.w3.org/2002/07/owl#Class"/>
      </glview:MeasurementType>
    </rdfs:subClassOf>
    <owl:someValuesFrom>
      <owl:Class>
        <owl:oneOf rdf:parseType="Collection">
          <glview:MeasurementType rdf:about="http://schema.geolink.org/dev/voc/nvs/P02#IPHY"/>
        </owl:oneOf>
      </owl:Class>
    </owl:someValuesFrom>
    <owl:onProperty rdf:resource="http://schema.geolink.org/dev/view#hasMeasurementType"/>
  </owl:Restriction>
  <owl:Restriction>
    <rdfs:subClassOf rdf:resource="http://schema.geolink.org/dev/voc/nvs/P02#MFLZ"/>
    <owl:someValuesFrom>
      <owl:Class>
        <owl:oneOf rdf:parseType="Collection">
          <glview:MeasurementType rdf:about="http://schema.geolink.org/dev/voc/nvs/P02#MFLZ"/>
        </owl:oneOf>
      </owl:Class>
    </owl:someValuesFrom>
    <owl:onProperty rdf:resource="http://schema.geolink.org/dev/view#hasMeasurementType"/>
  </owl:Restriction>
  <owl:Restriction>
    <rdfs:subClassOf rdf:resource="http://schema.geolink.org/dev/voc/nvs/P02#D000"/>
    <owl:someValuesFrom>
      <owl:Class>
        <owl:oneOf rdf:parseType="Collection">
          <glview:MeasurementType rdf:about="http://schema.geolink.org/dev/voc/nvs/P02#D000"/>
        </owl:oneOf>
      </owl:Class>
    </owl:someValuesFrom>
    <owl:onProperty rdf:resource="http://schema.geolink.org/dev/view#hasMeasurementType"/>
  </owl:Restriction>
  <owl:Restriction>
    <rdfs:subClassOf rdf:resource="http://schema.geolink.org/dev/voc/nvs/P02#SAMO"/>
    <owl:someValuesFrom>
      <owl:Class>
        <owl:oneOf rdf:parseType="Collection">
          <glview:MeasurementType rdf:about="http://schema.geolink.org/dev/voc/nvs/P02#SAMO"/>
        </owl:oneOf>
      </owl:Class>
    </owl:someValuesFrom>
    <owl:onProperty rdf:resource="http://schema.geolink.org/dev/view#hasMeasurementType"/>
  </owl:Restriction>
  <owl:Restriction>
    <rdfs:subClassOf rdf:resource="http://schema.geolink.org/dev/voc/nvs/P02#FBAB"/>
    <owl:someValuesFrom>
      <owl:Class>
        <owl:oneOf rdf:parseType="Collection">
          <glview:MeasurementType rdf:about="http://schema.geolink.org/dev/voc/nvs/P02#FBAB"/>
        </owl:oneOf>
      </owl:Class>
    </owl:someValuesFrom>
    <owl:onProperty rdf:resource="http://schema.geolink.org/dev/view#hasMeasurementType"/>
  </owl:Restriction>
  <owl:Restriction>
    <rdfs:subClassOf rdf:resource="http://schema.geolink.org/dev/voc/nvs/P02#PHSE"/>
    <owl:someValuesFrom>
      <owl:Class>
        <owl:oneOf rdf:parseType="Collection">
          <glview:MeasurementType rdf:about="http://schema.geolink.org/dev/voc/nvs/P02#PHSE"/>
        </owl:oneOf>
      </owl:Class>
    </owl:someValuesFrom>
    <owl:onProperty rdf:resource="http://schema.geolink.org/dev/view#hasMeasurementType"/>
  </owl:Restriction>
  <owl:Restriction>
    <rdfs:subClassOf rdf:resource="http://schema.geolink.org/dev/voc/nvs/P02#FABD"/>
    <owl:someValuesFrom>
      <owl:Class>
        <owl:oneOf rdf:parseType="Collection">
          <glview:MeasurementType rdf:about="http://schema.geolink.org/dev/voc/nvs/P02#FABD"/>
        </owl:oneOf>
      </owl:Class>
    </owl:someValuesFrom>
    <owl:onProperty rdf:resource="http://schema.geolink.org/dev/view#hasMeasurementType"/>
  </owl:Restriction>
  <owl:Restriction>
    <rdfs:subClassOf rdf:resource="http://schema.geolink.org/dev/voc/nvs/P02#SCOC"/>
    <owl:someValuesFrom>
      <owl:Class>
        <owl:oneOf rdf:parseType="Collection">
          <glview:MeasurementType rdf:about="http://schema.geolink.org/dev/voc/nvs/P02#SCOC"/>
        </owl:oneOf>
      </owl:Class>
    </owl:someValuesFrom>
    <owl:onProperty rdf:resource="http://schema.geolink.org/dev/view#hasMeasurementType"/>
  </owl:Restriction>
  <owl:Restriction>
    <rdfs:subClassOf>
      <glview:MeasurementType rdf:about="http://schema.geolink.org/dev/voc/nvs/P02#SIXX">
        <rdfs:subClassOf rdf:resource="http://schema.geolink.org/dev/voc/nvs/P03#C045"/>
        <rdfs:seeAlso rdf:resource="http://vocab.nerc.ac.uk/collection/P02/current/SIXX/"/>
        <rdfs:comment xml:lang="en">Concentration parameters for silicon species (including opal) in all phases of the water column</rdfs:comment>
        <rdfs:label xml:lang="en">Concentration of silicon species in the water column</rdfs:label>
        <rdf:type rdf:resource="http://www.w3.org/2002/07/owl#NamedIndividual"/>
        <rdf:type rdf:resource="http://www.w3.org/2002/07/owl#Class"/>
      </glview:MeasurementType>
    </rdfs:subClassOf>
    <owl:someValuesFrom>
      <owl:Class>
        <owl:oneOf rdf:parseType="Collection">
          <glview:MeasurementType rdf:about="http://schema.geolink.org/dev/voc/nvs/P02#SIXX"/>
        </owl:oneOf>
      </owl:Class>
    </owl:someValuesFrom>
    <owl:onProperty rdf:resource="http://schema.geolink.org/dev/view#hasMeasurementType"/>
  </owl:Restriction>
  <owl:Restriction>
    <rdfs:subClassOf rdf:resource="http://schema.geolink.org/dev/voc/nvs/P02#EXUV"/>
    <owl:someValuesFrom>
      <owl:Class>
        <owl:oneOf rdf:parseType="Collection">
          <glview:MeasurementType rdf:about="http://schema.geolink.org/dev/voc/nvs/P02#EXUV"/>
        </owl:oneOf>
      </owl:Class>
    </owl:someValuesFrom>
    <owl:onProperty rdf:resource="http://schema.geolink.org/dev/view#hasMeasurementType"/>
  </owl:Restriction>
  <owl:Restriction>
    <rdfs:subClassOf>
      <glview:MeasurementType rdf:about="http://schema.geolink.org/dev/voc/nvs/P02#TMES">
        <rdfs:subClassOf rdf:resource="http://schema.geolink.org/dev/voc/nvs/P03#Z005"/>
        <rdfs:seeAlso rdf:resource="http://vocab.nerc.ac.uk/collection/P02/current/TMES/"/>
        <rdfs:comment xml:lang="en">Data parameters that carry information relating to a measured parameter such as measurement temperatures, integration depths, quantities sampled and incubation durations</rdfs:comment>
        <rdfs:label xml:lang="en">Metadata parameters</rdfs:label>
        <rdf:type rdf:resource="http://www.w3.org/2002/07/owl#NamedIndividual"/>
        <rdf:type rdf:resource="http://www.w3.org/2002/07/owl#Class"/>
      </glview:MeasurementType>
    </rdfs:subClassOf>
    <owl:someValuesFrom>
      <owl:Class>
        <owl:oneOf rdf:parseType="Collection">
          <glview:MeasurementType rdf:about="http://schema.geolink.org/dev/voc/nvs/P02#TMES"/>
        </owl:oneOf>
      </owl:Class>
    </owl:someValuesFrom>
    <owl:onProperty rdf:resource="http://schema.geolink.org/dev/view#hasMeasurementType"/>
  </owl:Restriction>
  <owl:Restriction>
    <rdfs:subClassOf>
      <glview:MeasurementType rdf:about="http://schema.geolink.org/dev/voc/nvs/P02#SLCA">
        <rdfs:subClassOf rdf:resource="http://schema.geolink.org/dev/voc/nvs/P03#C040"/>
        <rdfs:seeAlso rdf:resource="http://vocab.nerc.ac.uk/collection/P02/current/SLCA/"/>
        <rdfs:comment xml:lang="en">Silicate concentration parameters (including statistical parameters such as standard deviation) in the water column</rdfs:comment>
        <rdfs:label xml:lang="en">Silicate concentration parameters in the water column</rdfs:label>
        <rdf:type rdf:resource="http://www.w3.org/2002/07/owl#NamedIndividual"/>
        <rdf:type rdf:resource="http://www.w3.org/2002/07/owl#Class"/>
      </glview:MeasurementType>
    </rdfs:subClassOf>
    <owl:someValuesFrom>
      <owl:Class>
        <owl:oneOf rdf:parseType="Collection">
          <glview:MeasurementType rdf:about="http://schema.geolink.org/dev/voc/nvs/P02#SLCA"/>
        </owl:oneOf>
      </owl:Class>
    </owl:someValuesFrom>
    <owl:onProperty rdf:resource="http://schema.geolink.org/dev/view#hasMeasurementType"/>
  </owl:Restriction>
  <owl:Restriction>
    <rdfs:subClassOf>
      <glview:MeasurementType rdf:about="http://schema.geolink.org/dev/voc/nvs/P02#PHWC">
        <rdfs:subClassOf rdf:resource="http://schema.geolink.org/dev/voc/nvs/P03#B035"/>
        <rdfs:seeAlso rdf:resource="http://vocab.nerc.ac.uk/collection/P02/current/PHWC/"/>
        <rdfs:comment xml:lang="en">Includes all variants of phaeopigment (chlorophyll degradation products) expressed in terms of per unit volume or unit area of the water column.  Does not include data expressed per unit mass of SPM.</rdfs:comment>
        <rdfs:label xml:lang="en">Phaeopigment concentrations in the water column</rdfs:label>
        <rdf:type rdf:resource="http://www.w3.org/2002/07/owl#NamedIndividual"/>
        <rdf:type rdf:resource="http://www.w3.org/2002/07/owl#Class"/>
      </glview:MeasurementType>
    </rdfs:subClassOf>
    <owl:someValuesFrom>
      <owl:Class>
        <owl:oneOf rdf:parseType="Collection">
          <glview:MeasurementType rdf:about="http://schema.geolink.org/dev/voc/nvs/P02#PHWC"/>
        </owl:oneOf>
      </owl:Class>
    </owl:someValuesFrom>
    <owl:onProperty rdf:resource="http://schema.geolink.org/dev/view#hasMeasurementType"/>
  </owl:Restriction>
  <owl:Restriction>
    <rdfs:subClassOf>
      <glview:MeasurementType rdf:about="http://schema.geolink.org/dev/voc/nvs/P02#CETA">
        <rdfs:subClassOf rdf:resource="http://schema.geolink.org/dev/voc/nvs/P03#B015"/>
        <rdfs:seeAlso rdf:resource="http://vocab.nerc.ac.uk/collection/P02/current/CETA/"/>
        <rdfs:comment xml:lang="en">Parameters that specify the number of specified members of Order Cetacea present at a particular time and location, including presence/absence indicators.</rdfs:comment>
        <rdfs:label xml:lang="en">Cetacean abundance</rdfs:label>
        <rdf:type rdf:resource="http://www.w3.org/2002/07/owl#NamedIndividual"/>
        <rdf:type rdf:resource="http://www.w3.org/2002/07/owl#Class"/>
      </glview:MeasurementType>
    </rdfs:subClassOf>
    <owl:someValuesFrom>
      <owl:Class>
        <owl:oneOf rdf:parseType="Collection">
          <glview:MeasurementType rdf:about="http://schema.geolink.org/dev/voc/nvs/P02#CETA"/>
        </owl:oneOf>
      </owl:Class>
    </owl:someValuesFrom>
    <owl:onProperty rdf:resource="http://schema.geolink.org/dev/view#hasMeasurementType"/>
  </owl:Restriction>
  <owl:Restriction>
    <rdfs:subClassOf>
      <glview:MeasurementType rdf:about="http://schema.geolink.org/dev/voc/nvs/P02#GP087">
        <rdfs:subClassOf rdf:resource="http://schema.geolink.org/dev/voc/nvs/P03#H004"/>
        <rdfs:seeAlso rdf:resource="http://vocab.nerc.ac.uk/collection/P02/current/GP087/"/>
        <rdfs:comment xml:lang="en">Parameters describing the extent, intensity, timing and method of fisheries</rdfs:comment>
        <rdfs:label xml:lang="en">Fishery characterisation</rdfs:label>
        <rdf:type rdf:resource="http://www.w3.org/2002/07/owl#NamedIndividual"/>
        <rdf:type rdf:resource="http://www.w3.org/2002/07/owl#Class"/>
      </glview:MeasurementType>
    </rdfs:subClassOf>
    <owl:someValuesFrom>
      <owl:Class>
        <owl:oneOf rdf:parseType="Collection">
          <glview:MeasurementType rdf:about="http://schema.geolink.org/dev/voc/nvs/P02#GP087"/>
        </owl:oneOf>
      </owl:Class>
    </owl:someValuesFrom>
    <owl:onProperty rdf:resource="http://schema.geolink.org/dev/view#hasMeasurementType"/>
  </owl:Restriction>
  <owl:Restriction>
    <rdfs:subClassOf>
      <glview:MeasurementType rdf:about="http://schema.geolink.org/dev/voc/nvs/P02#ZV00">
        <rdfs:subClassOf rdf:resource="http://schema.geolink.org/dev/voc/nvs/P03#B045"/>
        <rdfs:seeAlso rdf:resource="http://vocab.nerc.ac.uk/collection/P02/current/ZV00/"/>
        <rdfs:comment></rdfs:comment>
        <rdfs:label xml:lang="en">Zooplankton biovolume</rdfs:label>
        <rdf:type rdf:resource="http://www.w3.org/2002/07/owl#NamedIndividual"/>
        <rdf:type rdf:resource="http://www.w3.org/2002/07/owl#Class"/>
      </glview:MeasurementType>
    </rdfs:subClassOf>
    <owl:someValuesFrom>
      <owl:Class>
        <owl:oneOf rdf:parseType="Collection">
          <glview:MeasurementType rdf:about="http://schema.geolink.org/dev/voc/nvs/P02#ZV00"/>
        </owl:oneOf>
      </owl:Class>
    </owl:someValuesFrom>
    <owl:onProperty rdf:resource="http://schema.geolink.org/dev/view#hasMeasurementType"/>
  </owl:Restriction>
  <owl:Restriction>
    <rdfs:subClassOf>
      <glview:MeasurementType rdf:about="http://schema.geolink.org/dev/voc/nvs/P02#FCNT">
        <rdfs:subClassOf rdf:resource="http://schema.geolink.org/dev/voc/nvs/P03#B020"/>
        <rdfs:seeAlso rdf:resource="http://vocab.nerc.ac.uk/collection/P02/current/FCNT/"/>
        <rdfs:comment xml:lang="en">Fish (Osteichthyes, Agnatha and Chrondrichthyes) count parameters presented at the level of taxa that may be mapped to entities in the ITIS taxonomy.  These may be at any taxonomic level from sub-species upwards. Count includes presence/absence indicators.</rdfs:comment>
        <rdfs:label xml:lang="en">Fish taxonomy-related counts</rdfs:label>
        <rdf:type rdf:resource="http://www.w3.org/2002/07/owl#NamedIndividual"/>
        <rdf:type rdf:resource="http://www.w3.org/2002/07/owl#Class"/>
      </glview:MeasurementType>
    </rdfs:subClassOf>
    <owl:someValuesFrom>
      <owl:Class>
        <owl:oneOf rdf:parseType="Collection">
          <glview:MeasurementType rdf:about="http://schema.geolink.org/dev/voc/nvs/P02#FCNT"/>
        </owl:oneOf>
      </owl:Class>
    </owl:someValuesFrom>
    <owl:onProperty rdf:resource="http://schema.geolink.org/dev/view#hasMeasurementType"/>
  </owl:Restriction>
  <owl:Restriction>
    <rdfs:subClassOf>
      <glview:MeasurementType rdf:about="http://schema.geolink.org/dev/voc/nvs/P02#BATT">
        <rdfs:subClassOf rdf:resource="http://schema.geolink.org/dev/voc/nvs/P03#B005"/>
        <rdfs:seeAlso rdf:resource="http://vocab.nerc.ac.uk/collection/P02/current/BATT/"/>
        <rdfs:comment></rdfs:comment>
        <rdfs:label xml:lang="en">Bacteria environmental parameters</rdfs:label>
        <rdf:type rdf:resource="http://www.w3.org/2002/07/owl#NamedIndividual"/>
        <rdf:type rdf:resource="http://www.w3.org/2002/07/owl#Class"/>
      </glview:MeasurementType>
    </rdfs:subClassOf>
    <owl:someValuesFrom>
      <owl:Class>
        <owl:oneOf rdf:parseType="Collection">
          <glview:MeasurementType rdf:about="http://schema.geolink.org/dev/voc/nvs/P02#BATT"/>
        </owl:oneOf>
      </owl:Class>
    </owl:someValuesFrom>
    <owl:onProperty rdf:resource="http://schema.geolink.org/dev/view#hasMeasurementType"/>
  </owl:Restriction>
  <owl:Restriction>
    <rdfs:subClassOf>
      <glview:MeasurementType rdf:about="http://schema.geolink.org/dev/voc/nvs/P02#HEXC">
        <rdfs:subClassOf rdf:resource="http://schema.geolink.org/dev/voc/nvs/P03#C015"/>
        <rdfs:seeAlso rdf:resource="http://vocab.nerc.ac.uk/collection/P02/current/HEXC/"/>
        <rdfs:comment xml:lang="en">All concentration parameters including saturations and statistics such as standard deviations</rdfs:comment>
        <rdfs:label xml:lang="en">Dissolved noble gas concentration parameters in the water column</rdfs:label>
        <rdf:type rdf:resource="http://www.w3.org/2002/07/owl#NamedIndividual"/>
        <rdf:type rdf:resource="http://www.w3.org/2002/07/owl#Class"/>
      </glview:MeasurementType>
    </rdfs:subClassOf>
    <owl:someValuesFrom>
      <owl:Class>
        <owl:oneOf rdf:parseType="Collection">
          <glview:MeasurementType rdf:about="http://schema.geolink.org/dev/voc/nvs/P02#HEXC"/>
        </owl:oneOf>
      </owl:Class>
    </owl:someValuesFrom>
    <owl:onProperty rdf:resource="http://schema.geolink.org/dev/view#hasMeasurementType"/>
  </owl:Restriction>
  <owl:Restriction>
    <rdfs:subClassOf rdf:resource="http://schema.geolink.org/dev/voc/nvs/P02#PHWB"/>
    <owl:someValuesFrom>
      <owl:Class>
        <owl:oneOf rdf:parseType="Collection">
          <glview:MeasurementType rdf:about="http://schema.geolink.org/dev/voc/nvs/P02#PHWB"/>
        </owl:oneOf>
      </owl:Class>
    </owl:someValuesFrom>
    <owl:onProperty rdf:resource="http://schema.geolink.org/dev/view#hasMeasurementType"/>
  </owl:Restriction>
  <owl:Restriction>
    <rdfs:subClassOf rdf:resource="http://schema.geolink.org/dev/voc/nvs/P02#CPCN"/>
    <owl:someValuesFrom>
      <owl:Class>
        <owl:oneOf rdf:parseType="Collection">
          <glview:MeasurementType rdf:about="http://schema.geolink.org/dev/voc/nvs/P02#CPCN"/>
        </owl:oneOf>
      </owl:Class>
    </owl:someValuesFrom>
    <owl:onProperty rdf:resource="http://schema.geolink.org/dev/view#hasMeasurementType"/>
  </owl:Restriction>
  <owl:Restriction>
    <rdfs:subClassOf rdf:resource="http://schema.geolink.org/dev/voc/nvs/P02#SDNA"/>
    <owl:someValuesFrom>
      <owl:Class>
        <owl:oneOf rdf:parseType="Collection">
          <glview:MeasurementType rdf:about="http://schema.geolink.org/dev/voc/nvs/P02#SDNA"/>
        </owl:oneOf>
      </owl:Class>
    </owl:someValuesFrom>
    <owl:onProperty rdf:resource="http://schema.geolink.org/dev/view#hasMeasurementType"/>
  </owl:Restriction>
  <owl:Restriction>
    <rdfs:subClassOf rdf:resource="http://schema.geolink.org/dev/voc/nvs/P02#SCOC"/>
    <owl:someValuesFrom>
      <owl:Class>
        <owl:oneOf rdf:parseType="Collection">
          <glview:MeasurementType rdf:about="http://schema.geolink.org/dev/voc/nvs/P02#SCOC"/>
        </owl:oneOf>
      </owl:Class>
    </owl:someValuesFrom>
    <owl:onProperty rdf:resource="http://schema.geolink.org/dev/view#hasMeasurementType"/>
  </owl:Restriction>
  <owl:Restriction>
    <rdfs:subClassOf rdf:resource="http://schema.geolink.org/dev/voc/nvs/P02#AXFX"/>
    <owl:someValuesFrom>
      <owl:Class>
        <owl:oneOf rdf:parseType="Collection">
          <glview:MeasurementType rdf:about="http://schema.geolink.org/dev/voc/nvs/P02#AXFX"/>
        </owl:oneOf>
      </owl:Class>
    </owl:someValuesFrom>
    <owl:onProperty rdf:resource="http://schema.geolink.org/dev/view#hasMeasurementType"/>
  </owl:Restriction>
  <owl:Restriction>
    <rdfs:subClassOf rdf:resource="http://schema.geolink.org/dev/voc/nvs/P02#AALK"/>
    <owl:someValuesFrom>
      <owl:Class>
        <owl:oneOf rdf:parseType="Collection">
          <glview:MeasurementType rdf:about="http://schema.geolink.org/dev/voc/nvs/P02#AALK"/>
        </owl:oneOf>
      </owl:Class>
    </owl:someValuesFrom>
    <owl:onProperty rdf:resource="http://schema.geolink.org/dev/view#hasMeasurementType"/>
  </owl:Restriction>
  <owl:Restriction>
    <rdfs:subClassOf>
      <glview:MeasurementType rdf:about="http://schema.geolink.org/dev/voc/nvs/P02#GP080">
        <rdfs:subClassOf rdf:resource="http://schema.geolink.org/dev/voc/nvs/P03#H004"/>
        <rdfs:seeAlso rdf:resource="http://vocab.nerc.ac.uk/collection/P02/current/GP080/"/>
        <rdfs:comment xml:lang="en">Parameters quantifying the capture of non-target species during commercial and non-commercial fishing trips</rdfs:comment>
        <rdfs:label xml:lang="en">Fishing by-catch</rdfs:label>
        <rdf:type rdf:resource="http://www.w3.org/2002/07/owl#NamedIndividual"/>
        <rdf:type rdf:resource="http://www.w3.org/2002/07/owl#Class"/>
      </glview:MeasurementType>
    </rdfs:subClassOf>
    <owl:someValuesFrom>
      <owl:Class>
        <owl:oneOf rdf:parseType="Collection">
          <glview:MeasurementType rdf:about="http://schema.geolink.org/dev/voc/nvs/P02#GP080"/>
        </owl:oneOf>
      </owl:Class>
    </owl:someValuesFrom>
    <owl:onProperty rdf:resource="http://schema.geolink.org/dev/view#hasMeasurementType"/>
  </owl:Restriction>
  <owl:Restriction>
    <rdfs:subClassOf>
      <glview:MeasurementType rdf:about="http://schema.geolink.org/dev/voc/nvs/P02#LVLT">
        <rdfs:subClassOf rdf:resource="http://schema.geolink.org/dev/voc/nvs/P03#D015"/>
        <rdfs:seeAlso rdf:resource="http://vocab.nerc.ac.uk/collection/P02/current/LVLT/"/>
        <rdfs:comment></rdfs:comment>
        <rdfs:label xml:lang="en">Raw light meter output</rdfs:label>
        <rdf:type rdf:resource="http://www.w3.org/2002/07/owl#NamedIndividual"/>
        <rdf:type rdf:resource="http://www.w3.org/2002/07/owl#Class"/>
      </glview:MeasurementType>
    </rdfs:subClassOf>
    <owl:someValuesFrom>
      <owl:Class>
        <owl:oneOf rdf:parseType="Collection">
          <glview:MeasurementType rdf:about="http://schema.geolink.org/dev/voc/nvs/P02#LVLT"/>
        </owl:oneOf>
      </owl:Class>
    </owl:someValuesFrom>
    <owl:onProperty rdf:resource="http://schema.geolink.org/dev/view#hasMeasurementType"/>
  </owl:Restriction>
  <owl:Restriction>
    <rdfs:subClassOf rdf:resource="http://schema.geolink.org/dev/voc/nvs/P02#PCAH"/>
    <owl:someValuesFrom>
      <owl:Class>
        <owl:oneOf rdf:parseType="Collection">
          <owl:Class rdf:about="http://schema.geolink.org/dev/voc/nvs/P02#PCAH"/>
        </owl:oneOf>
      </owl:Class>
    </owl:someValuesFrom>
    <owl:onProperty rdf:resource="http://schema.geolink.org/dev/view#hasMeasurementType"/>
  </owl:Restriction>
  <owl:Restriction>
    <rdfs:subClassOf>
      <glview:MeasurementType rdf:about="http://schema.geolink.org/dev/voc/nvs/P02#DPEV">
        <rdfs:subClassOf rdf:resource="http://schema.geolink.org/dev/voc/nvs/P03#GSED"/>
        <rdfs:seeAlso rdf:resource="http://vocab.nerc.ac.uk/collection/P02/current/DPEV/"/>
        <rdfs:comment xml:lang="en">Parameters characterising the environment in which sediments were deposited either by observation or interpretation of sedimentary rocks and unlithified sediments.</rdfs:comment>
        <rdfs:label xml:lang="en">Depositional environment</rdfs:label>
        <rdf:type rdf:resource="http://www.w3.org/2002/07/owl#NamedIndividual"/>
        <rdf:type rdf:resource="http://www.w3.org/2002/07/owl#Class"/>
      </glview:MeasurementType>
    </rdfs:subClassOf>
    <owl:someValuesFrom>
      <owl:Class>
        <owl:oneOf rdf:parseType="Collection">
          <glview:MeasurementType rdf:about="http://schema.geolink.org/dev/voc/nvs/P02#DPEV"/>
        </owl:oneOf>
      </owl:Class>
    </owl:someValuesFrom>
    <owl:onProperty rdf:resource="http://schema.geolink.org/dev/view#hasMeasurementType"/>
  </owl:Restriction>
  <owl:Restriction>
    <rdfs:subClassOf>
      <glview:MeasurementType rdf:about="http://schema.geolink.org/dev/voc/nvs/P02#VDFC">
        <rdfs:subClassOf rdf:resource="http://schema.geolink.org/dev/view#Measurement"/>
        <rdfs:seeAlso rdf:resource="http://vocab.nerc.ac.uk/collection/P02/current/VDFC/"/>
        <rdfs:comment xml:lang="en">Parameters describing the transport of material, heat or energy in the water column</rdfs:comment>
        <rdfs:label xml:lang="en">Transport in the water column</rdfs:label>
        <rdf:type rdf:resource="http://www.w3.org/2002/07/owl#NamedIndividual"/>
        <rdf:type rdf:resource="http://www.w3.org/2002/07/owl#Class"/>
      </glview:MeasurementType>
    </rdfs:subClassOf>
    <owl:someValuesFrom>
      <owl:Class>
        <owl:oneOf rdf:parseType="Collection">
          <glview:MeasurementType rdf:about="http://schema.geolink.org/dev/voc/nvs/P02#VDFC"/>
        </owl:oneOf>
      </owl:Class>
    </owl:someValuesFrom>
    <owl:onProperty rdf:resource="http://schema.geolink.org/dev/view#hasMeasurementType"/>
  </owl:Restriction>
  <owl:Restriction>
    <rdfs:subClassOf>
      <glview:MeasurementType rdf:about="http://schema.geolink.org/dev/voc/nvs/P02#AATX">
        <rdfs:subClassOf rdf:resource="http://schema.geolink.org/dev/voc/nvs/P03#B030"/>
        <rdfs:seeAlso rdf:resource="http://vocab.nerc.ac.uk/collection/P02/current/AATX/"/>
        <rdfs:comment xml:lang="en">Any parameterisation of cell surface area of free-floating autotrophic biological entities designated by taxonomic names (e.g. species, genus, family) in any body of fresh or salt water.</rdfs:comment>
        <rdfs:label xml:lang="en">Phytoplankton taxonomic surface area in water bodies</rdfs:label>
        <rdf:type rdf:resource="http://www.w3.org/2002/07/owl#NamedIndividual"/>
        <rdf:type rdf:resource="http://www.w3.org/2002/07/owl#Class"/>
      </glview:MeasurementType>
    </rdfs:subClassOf>
    <owl:someValuesFrom>
      <owl:Class>
        <owl:oneOf rdf:parseType="Collection">
          <glview:MeasurementType rdf:about="http://schema.geolink.org/dev/voc/nvs/P02#AATX"/>
        </owl:oneOf>
      </owl:Class>
    </owl:someValuesFrom>
    <owl:onProperty rdf:resource="http://schema.geolink.org/dev/view#hasMeasurementType"/>
  </owl:Restriction>
  <owl:Restriction>
    <rdfs:subClassOf>
      <glview:MeasurementType rdf:about="http://schema.geolink.org/dev/voc/nvs/P02#CMFL">
        <rdfs:subClassOf rdf:resource="http://schema.geolink.org/dev/voc/nvs/P03#O010"/>
        <rdfs:seeAlso rdf:resource="http://vocab.nerc.ac.uk/collection/P02/current/CMFL/"/>
        <rdfs:comment xml:lang="en">Parameters measured by variable fluorescence instruments such as pump and probe and fast repetition rate fluorometers</rdfs:comment>
        <rdfs:label xml:lang="en">Variable fluorescence parameters</rdfs:label>
        <rdf:type rdf:resource="http://www.w3.org/2002/07/owl#NamedIndividual"/>
        <rdf:type rdf:resource="http://www.w3.org/2002/07/owl#Class"/>
      </glview:MeasurementType>
    </rdfs:subClassOf>
    <owl:someValuesFrom>
      <owl:Class>
        <owl:oneOf rdf:parseType="Collection">
          <glview:MeasurementType rdf:about="http://schema.geolink.org/dev/voc/nvs/P02#CMFL"/>
        </owl:oneOf>
      </owl:Class>
    </owl:someValuesFrom>
    <owl:onProperty rdf:resource="http://schema.geolink.org/dev/view#hasMeasurementType"/>
  </owl:Restriction>
  <owl:Restriction>
    <rdfs:subClassOf rdf:resource="http://schema.geolink.org/dev/voc/nvs/P02#NTRI"/>
    <owl:someValuesFrom>
      <owl:Class>
        <owl:oneOf rdf:parseType="Collection">
          <glview:MeasurementType rdf:about="http://schema.geolink.org/dev/voc/nvs/P02#NTRI"/>
        </owl:oneOf>
      </owl:Class>
    </owl:someValuesFrom>
    <owl:onProperty rdf:resource="http://schema.geolink.org/dev/view#hasMeasurementType"/>
  </owl:Restriction>
  <owl:Restriction>
    <rdfs:subClassOf>
      <glview:MeasurementType rdf:about="http://schema.geolink.org/dev/voc/nvs/P02#SREP">
        <rdfs:subClassOf rdf:resource="http://schema.geolink.org/dev/voc/nvs/P03#B027"/>
        <rdfs:subClassOf rdf:resource="http://schema.geolink.org/dev/voc/nvs/P03#H004"/>
        <rdfs:seeAlso rdf:resource="http://vocab.nerc.ac.uk/collection/P02/current/SREP/"/>
        <rdfs:comment xml:lang="en">Paramaters that quantify the fecundity, reproductive rates or nature of reproduction in shellfish (molluscs - including cephalopods - and crustaceans of interest to fisheries research and commercial fisheries).</rdfs:comment>
        <rdfs:label xml:lang="en">Shellfish reproduction</rdfs:label>
        <rdf:type rdf:resource="http://www.w3.org/2002/07/owl#NamedIndividual"/>
        <rdf:type rdf:resource="http://www.w3.org/2002/07/owl#Class"/>
      </glview:MeasurementType>
    </rdfs:subClassOf>
    <owl:someValuesFrom>
      <owl:Class>
        <owl:oneOf rdf:parseType="Collection">
          <glview:MeasurementType rdf:about="http://schema.geolink.org/dev/voc/nvs/P02#SREP"/>
        </owl:oneOf>
      </owl:Class>
    </owl:someValuesFrom>
    <owl:onProperty rdf:resource="http://schema.geolink.org/dev/view#hasMeasurementType"/>
  </owl:Restriction>
  <owl:Restriction>
    <rdfs:subClassOf>
      <glview:MeasurementType rdf:about="http://schema.geolink.org/dev/voc/nvs/P02#EXSV">
        <rdfs:subClassOf rdf:resource="http://schema.geolink.org/dev/voc/nvs/P03#Z005"/>
        <rdfs:seeAlso rdf:resource="http://vocab.nerc.ac.uk/collection/P02/current/EXSV/"/>
        <rdfs:comment xml:lang="en">Measurements made at a given time of any state variable in a sample that is the subject of an experiment that will change the composition over time, such as the water sample in an incubation experiment.</rdfs:comment>
        <rdfs:label xml:lang="en">Experiment state variables</rdfs:label>
        <rdf:type rdf:resource="http://www.w3.org/2002/07/owl#NamedIndividual"/>
        <rdf:type rdf:resource="http://www.w3.org/2002/07/owl#Class"/>
      </glview:MeasurementType>
    </rdfs:subClassOf>
    <owl:someValuesFrom>
      <owl:Class>
        <owl:oneOf rdf:parseType="Collection">
          <glview:MeasurementType rdf:about="http://schema.geolink.org/dev/voc/nvs/P02#EXSV"/>
        </owl:oneOf>
      </owl:Class>
    </owl:someValuesFrom>
    <owl:onProperty rdf:resource="http://schema.geolink.org/dev/view#hasMeasurementType"/>
  </owl:Restriction>
  <owl:Restriction>
    <rdfs:subClassOf rdf:resource="http://schema.geolink.org/dev/voc/nvs/P02#BCAH"/>
    <owl:someValuesFrom>
      <owl:Class>
        <owl:oneOf rdf:parseType="Collection">
          <owl:NamedIndividual rdf:about="http://schema.geolink.org/dev/voc/nvs/P02#BCAH"/>
        </owl:oneOf>
      </owl:Class>
    </owl:someValuesFrom>
    <owl:onProperty rdf:resource="http://schema.geolink.org/dev/view#hasMeasurementType"/>
  </owl:Restriction>
  <owl:Restriction>
    <rdfs:subClassOf rdf:resource="http://schema.geolink.org/dev/voc/nvs/P02#GP005"/>
    <owl:someValuesFrom>
      <owl:Class>
        <owl:oneOf rdf:parseType="Collection">
          <glview:MeasurementType rdf:about="http://schema.geolink.org/dev/voc/nvs/P02#GP005"/>
        </owl:oneOf>
      </owl:Class>
    </owl:someValuesFrom>
    <owl:onProperty rdf:resource="http://schema.geolink.org/dev/view#hasMeasurementType"/>
  </owl:Restriction>
  <owl:Restriction>
    <rdfs:subClassOf rdf:resource="http://schema.geolink.org/dev/voc/nvs/P02#PHSE"/>
    <owl:someValuesFrom>
      <owl:Class>
        <owl:oneOf rdf:parseType="Collection">
          <glview:MeasurementType rdf:about="http://schema.geolink.org/dev/voc/nvs/P02#PHSE"/>
        </owl:oneOf>
      </owl:Class>
    </owl:someValuesFrom>
    <owl:onProperty rdf:resource="http://schema.geolink.org/dev/view#hasMeasurementType"/>
  </owl:Restriction>
  <owl:Restriction>
    <rdfs:subClassOf>
      <glview:MeasurementType rdf:about="http://schema.geolink.org/dev/voc/nvs/P02#BRDA">
        <rdfs:subClassOf rdf:resource="http://schema.geolink.org/dev/voc/nvs/P03#B015"/>
        <rdfs:seeAlso rdf:resource="http://vocab.nerc.ac.uk/collection/P02/current/BRDA/"/>
        <rdfs:comment xml:lang="en">Parameters quantifying the number of birds (Class Aves) in a survey but not expressed per unit area. Includes presence/absence indicators.</rdfs:comment>
        <rdfs:label xml:lang="en">Bird counts</rdfs:label>
        <rdf:type rdf:resource="http://www.w3.org/2002/07/owl#NamedIndividual"/>
        <rdf:type rdf:resource="http://www.w3.org/2002/07/owl#Class"/>
      </glview:MeasurementType>
    </rdfs:subClassOf>
    <owl:someValuesFrom>
      <owl:Class>
        <owl:oneOf rdf:parseType="Collection">
          <glview:MeasurementType rdf:about="http://schema.geolink.org/dev/voc/nvs/P02#BRDA"/>
        </owl:oneOf>
      </owl:Class>
    </owl:someValuesFrom>
    <owl:onProperty rdf:resource="http://schema.geolink.org/dev/view#hasMeasurementType"/>
  </owl:Restriction>
  <owl:Restriction>
    <rdfs:subClassOf>
      <glview:MeasurementType rdf:about="http://schema.geolink.org/dev/voc/nvs/P02#XKEY">
        <rdfs:subClassOf rdf:resource="http://schema.geolink.org/dev/voc/nvs/P03#Z005"/>
        <rdfs:seeAlso rdf:resource="http://vocab.nerc.ac.uk/collection/P02/current/XKEY/"/>
        <rdfs:comment xml:lang="en">Parameters used to encode information specifying access rights to data, usually in terms of authorised roles</rdfs:comment>
        <rdfs:label xml:lang="en">Security tags and keys</rdfs:label>
        <rdf:type rdf:resource="http://www.w3.org/2002/07/owl#NamedIndividual"/>
        <rdf:type rdf:resource="http://www.w3.org/2002/07/owl#Class"/>
      </glview:MeasurementType>
    </rdfs:subClassOf>
    <owl:someValuesFrom>
      <owl:Class>
        <owl:oneOf rdf:parseType="Collection">
          <glview:MeasurementType rdf:about="http://schema.geolink.org/dev/voc/nvs/P02#XKEY"/>
        </owl:oneOf>
      </owl:Class>
    </owl:someValuesFrom>
    <owl:onProperty rdf:resource="http://schema.geolink.org/dev/view#hasMeasurementType"/>
  </owl:Restriction>
  <owl:Restriction>
    <rdfs:subClassOf rdf:resource="http://schema.geolink.org/dev/voc/nvs/P02#BDWC"/>
    <owl:someValuesFrom>
      <owl:Class>
        <owl:oneOf rdf:parseType="Collection">
          <glview:MeasurementType rdf:about="http://schema.geolink.org/dev/voc/nvs/P02#BDWC"/>
        </owl:oneOf>
      </owl:Class>
    </owl:someValuesFrom>
    <owl:onProperty rdf:resource="http://schema.geolink.org/dev/view#hasMeasurementType"/>
  </owl:Restriction>
  <owl:Restriction>
    <rdfs:subClassOf>
      <glview:MeasurementType rdf:about="http://schema.geolink.org/dev/voc/nvs/P02#COGE">
        <rdfs:subClassOf rdf:resource="http://schema.geolink.org/dev/voc/nvs/P03#T001"/>
        <rdfs:seeAlso rdf:resource="http://vocab.nerc.ac.uk/collection/P02/current/COGE/"/>
        <rdfs:comment xml:lang="en">All parameters associated with coastal landforms such as beaches and dunes including morphology, evolution and associated transport phenomena</rdfs:comment>
        <rdfs:label xml:lang="en">Coastal geomorphology</rdfs:label>
        <rdf:type rdf:resource="http://www.w3.org/2002/07/owl#NamedIndividual"/>
        <rdf:type rdf:resource="http://www.w3.org/2002/07/owl#Class"/>
      </glview:MeasurementType>
    </rdfs:subClassOf>
    <owl:someValuesFrom>
      <owl:Class>
        <owl:oneOf rdf:parseType="Collection">
          <glview:MeasurementType rdf:about="http://schema.geolink.org/dev/voc/nvs/P02#COGE"/>
        </owl:oneOf>
      </owl:Class>
    </owl:someValuesFrom>
    <owl:onProperty rdf:resource="http://schema.geolink.org/dev/view#hasMeasurementType"/>
  </owl:Restriction>
  <owl:Restriction>
    <rdfs:subClassOf rdf:resource="http://schema.geolink.org/dev/voc/nvs/P02#BCAH"/>
    <owl:someValuesFrom>
      <owl:Class>
        <owl:oneOf rdf:parseType="Collection">
          <owl:NamedIndividual rdf:about="http://schema.geolink.org/dev/voc/nvs/P02#BCAH"/>
        </owl:oneOf>
      </owl:Class>
    </owl:someValuesFrom>
    <owl:onProperty rdf:resource="http://schema.geolink.org/dev/view#hasMeasurementType"/>
  </owl:Restriction>
  <owl:Restriction>
    <rdfs:subClassOf rdf:resource="http://schema.geolink.org/dev/voc/nvs/P02#GP050"/>
    <owl:someValuesFrom>
      <owl:Class>
        <owl:oneOf rdf:parseType="Collection">
          <glview:MeasurementType rdf:about="http://schema.geolink.org/dev/voc/nvs/P02#GP050"/>
        </owl:oneOf>
      </owl:Class>
    </owl:someValuesFrom>
    <owl:onProperty rdf:resource="http://schema.geolink.org/dev/view#hasMeasurementType"/>
  </owl:Restriction>
  <owl:Restriction>
    <rdfs:subClassOf rdf:resource="http://schema.geolink.org/dev/voc/nvs/P02#SREP"/>
    <owl:someValuesFrom>
      <owl:Class>
        <owl:oneOf rdf:parseType="Collection">
          <glview:MeasurementType rdf:about="http://schema.geolink.org/dev/voc/nvs/P02#SREP"/>
        </owl:oneOf>
      </owl:Class>
    </owl:someValuesFrom>
    <owl:onProperty rdf:resource="http://schema.geolink.org/dev/view#hasMeasurementType"/>
  </owl:Restriction>
  <owl:Restriction>
    <rdfs:subClassOf>
      <glview:MeasurementType rdf:about="http://schema.geolink.org/dev/voc/nvs/P02#AAWC">
        <rdfs:subClassOf rdf:resource="http://schema.geolink.org/dev/voc/nvs/P03#C050"/>
        <rdfs:seeAlso rdf:resource="http://vocab.nerc.ac.uk/collection/P02/current/AAWC/"/>
        <rdfs:comment xml:lang="en">Alkanamine concentrations in all phases of the water column</rdfs:comment>
        <rdfs:label xml:lang="en">Concentration of alkanamines (amines) in the water column</rdfs:label>
        <rdf:type rdf:resource="http://www.w3.org/2002/07/owl#NamedIndividual"/>
        <rdf:type rdf:resource="http://www.w3.org/2002/07/owl#Class"/>
      </glview:MeasurementType>
    </rdfs:subClassOf>
    <owl:someValuesFrom>
      <owl:Class>
        <owl:oneOf rdf:parseType="Collection">
          <glview:MeasurementType rdf:about="http://schema.geolink.org/dev/voc/nvs/P02#AAWC"/>
        </owl:oneOf>
      </owl:Class>
    </owl:someValuesFrom>
    <owl:onProperty rdf:resource="http://schema.geolink.org/dev/view#hasMeasurementType"/>
  </owl:Restriction>
  <owl:Restriction>
    <rdfs:subClassOf rdf:resource="http://schema.geolink.org/dev/voc/nvs/P02#ZCTN"/>
    <owl:someValuesFrom>
      <owl:Class>
        <owl:oneOf rdf:parseType="Collection">
          <glview:MeasurementType rdf:about="http://schema.geolink.org/dev/voc/nvs/P02#ZCTN"/>
        </owl:oneOf>
      </owl:Class>
    </owl:someValuesFrom>
    <owl:onProperty rdf:resource="http://schema.geolink.org/dev/view#hasMeasurementType"/>
  </owl:Restriction>
  <owl:Restriction>
    <rdfs:subClassOf rdf:resource="http://schema.geolink.org/dev/voc/nvs/P02#IATX"/>
    <owl:someValuesFrom>
      <owl:Class>
        <owl:oneOf rdf:parseType="Collection">
          <glview:MeasurementType rdf:about="http://schema.geolink.org/dev/voc/nvs/P02#IATX"/>
        </owl:oneOf>
      </owl:Class>
    </owl:someValuesFrom>
    <owl:onProperty rdf:resource="http://schema.geolink.org/dev/view#hasMeasurementType"/>
  </owl:Restriction>
  <owl:Restriction>
    <rdfs:subClassOf rdf:resource="http://schema.geolink.org/dev/voc/nvs/P02#ZNLG"/>
    <owl:someValuesFrom>
      <owl:Class>
        <owl:oneOf rdf:parseType="Collection">
          <glview:MeasurementType rdf:about="http://schema.geolink.org/dev/voc/nvs/P02#ZNLG"/>
        </owl:oneOf>
      </owl:Class>
    </owl:someValuesFrom>
    <owl:onProperty rdf:resource="http://schema.geolink.org/dev/view#hasMeasurementType"/>
  </owl:Restriction>
  <owl:Restriction>
    <rdfs:subClassOf rdf:resource="http://schema.geolink.org/dev/voc/nvs/P02#PCAH"/>
    <owl:someValuesFrom>
      <owl:Class>
        <owl:oneOf rdf:parseType="Collection">
          <owl:Class rdf:about="http://schema.geolink.org/dev/voc/nvs/P02#PCAH"/>
        </owl:oneOf>
      </owl:Class>
    </owl:someValuesFrom>
    <owl:onProperty rdf:resource="http://schema.geolink.org/dev/view#hasMeasurementType"/>
  </owl:Restriction>
  <owl:Restriction>
    <rdfs:subClassOf rdf:resource="http://schema.geolink.org/dev/voc/nvs/P02#RBSC"/>
    <owl:someValuesFrom>
      <owl:Class>
        <owl:oneOf rdf:parseType="Collection">
          <owl:NamedIndividual rdf:about="http://schema.geolink.org/dev/voc/nvs/P02#RBSC"/>
        </owl:oneOf>
      </owl:Class>
    </owl:someValuesFrom>
    <owl:onProperty rdf:resource="http://schema.geolink.org/dev/view#hasMeasurementType"/>
  </owl:Restriction>
  <owl:Restriction>
    <rdfs:subClassOf>
      <glview:MeasurementType rdf:about="http://schema.geolink.org/dev/voc/nvs/P02#DOCC">
        <rdfs:subClassOf rdf:resource="http://schema.geolink.org/dev/voc/nvs/P03#C005"/>
        <rdfs:seeAlso rdf:resource="http://vocab.nerc.ac.uk/collection/P02/current/DOCC/"/>
        <rdfs:comment xml:lang="en">DOC per unit volume of the water column.  Note that this includes some parameters that are strictly defined as total carbon, because the water was unfiltered on the assumption that POC was negligible.</rdfs:comment>
        <rdfs:label xml:lang="en">Dissolved organic carbon concentration in the water column</rdfs:label>
        <rdf:type rdf:resource="http://www.w3.org/2002/07/owl#NamedIndividual"/>
        <rdf:type rdf:resource="http://www.w3.org/2002/07/owl#Class"/>
      </glview:MeasurementType>
    </rdfs:subClassOf>
    <owl:someValuesFrom>
      <owl:Class>
        <owl:oneOf rdf:parseType="Collection">
          <glview:MeasurementType rdf:about="http://schema.geolink.org/dev/voc/nvs/P02#DOCC"/>
        </owl:oneOf>
      </owl:Class>
    </owl:someValuesFrom>
    <owl:onProperty rdf:resource="http://schema.geolink.org/dev/view#hasMeasurementType"/>
  </owl:Restriction>
  <owl:Restriction>
    <rdfs:subClassOf>
      <glview:MeasurementType rdf:about="http://schema.geolink.org/dev/voc/nvs/P02#TCO2">
        <rdfs:subClassOf rdf:resource="http://schema.geolink.org/dev/voc/nvs/P03#C005"/>
        <rdfs:subClassOf rdf:resource="http://schema.geolink.org/dev/voc/nvs/P03#C010"/>
        <rdfs:seeAlso rdf:resource="http://vocab.nerc.ac.uk/collection/P02/current/TCO2/"/>
        <rdfs:comment></rdfs:comment>
        <rdfs:label xml:lang="en">Total dissolved inorganic carbon (TCO2) concentration in the water column</rdfs:label>
        <rdf:type rdf:resource="http://www.w3.org/2002/07/owl#NamedIndividual"/>
        <rdf:type rdf:resource="http://www.w3.org/2002/07/owl#Class"/>
      </glview:MeasurementType>
    </rdfs:subClassOf>
    <owl:someValuesFrom>
      <owl:Class>
        <owl:oneOf rdf:parseType="Collection">
          <glview:MeasurementType rdf:about="http://schema.geolink.org/dev/voc/nvs/P02#TCO2"/>
        </owl:oneOf>
      </owl:Class>
    </owl:someValuesFrom>
    <owl:onProperty rdf:resource="http://schema.geolink.org/dev/view#hasMeasurementType"/>
  </owl:Restriction>
  <owl:Restriction>
    <rdfs:subClassOf>
      <glview:MeasurementType rdf:about="http://schema.geolink.org/dev/voc/nvs/P02#HLIC">
        <rdfs:subClassOf rdf:resource="http://schema.geolink.org/dev/voc/nvs/P02#ICHM"/>
        <rdfs:seeAlso rdf:resource="http://vocab.nerc.ac.uk/collection/P02/current/HLIC/"/>
        <rdfs:comment xml:lang="en">Concentrations of halogens as elements or their inorganic compounds in ice</rdfs:comment>
        <rdfs:label xml:lang="en">Concentration of inorganic halogens in ice</rdfs:label>
        <rdf:type rdf:resource="http://www.w3.org/2002/07/owl#NamedIndividual"/>
        <rdf:type rdf:resource="http://www.w3.org/2002/07/owl#Class"/>
      </glview:MeasurementType>
    </rdfs:subClassOf>
    <owl:someValuesFrom>
      <owl:Class>
        <owl:oneOf rdf:parseType="Collection">
          <glview:MeasurementType rdf:about="http://schema.geolink.org/dev/voc/nvs/P02#HLIC"/>
        </owl:oneOf>
      </owl:Class>
    </owl:someValuesFrom>
    <owl:onProperty rdf:resource="http://schema.geolink.org/dev/view#hasMeasurementType"/>
  </owl:Restriction>
  <owl:Restriction>
    <rdfs:subClassOf>
      <glview:MeasurementType rdf:about="http://schema.geolink.org/dev/voc/nvs/P02#MDSV">
        <rdfs:subClassOf rdf:resource="http://schema.geolink.org/dev/voc/nvs/P03#G015"/>
        <rdfs:seeAlso rdf:resource="http://vocab.nerc.ac.uk/collection/P02/current/MDSV/"/>
        <rdfs:comment></rdfs:comment>
        <rdfs:label xml:lang="en">Suspended particulate material setting velocity parameters</rdfs:label>
        <rdf:type rdf:resource="http://www.w3.org/2002/07/owl#NamedIndividual"/>
        <rdf:type rdf:resource="http://www.w3.org/2002/07/owl#Class"/>
      </glview:MeasurementType>
    </rdfs:subClassOf>
    <owl:someValuesFrom>
      <owl:Class>
        <owl:oneOf rdf:parseType="Collection">
          <glview:MeasurementType rdf:about="http://schema.geolink.org/dev/voc/nvs/P02#MDSV"/>
        </owl:oneOf>
      </owl:Class>
    </owl:someValuesFrom>
    <owl:onProperty rdf:resource="http://schema.geolink.org/dev/view#hasMeasurementType"/>
  </owl:Restriction>
  <owl:Restriction>
    <rdfs:subClassOf rdf:resource="http://schema.geolink.org/dev/voc/nvs/P02#PHAT"/>
    <owl:someValuesFrom>
      <owl:Class>
        <owl:oneOf rdf:parseType="Collection">
          <glview:MeasurementType rdf:about="http://schema.geolink.org/dev/voc/nvs/P02#PHAT"/>
        </owl:oneOf>
      </owl:Class>
    </owl:someValuesFrom>
    <owl:onProperty rdf:resource="http://schema.geolink.org/dev/view#hasMeasurementType"/>
  </owl:Restriction>
  <owl:Restriction>
    <rdfs:subClassOf>
      <glview:MeasurementType rdf:about="http://schema.geolink.org/dev/voc/nvs/P02#COAS">
        <rdfs:subClassOf rdf:resource="http://schema.geolink.org/dev/voc/nvs/P03#T001"/>
        <rdfs:seeAlso rdf:resource="http://vocab.nerc.ac.uk/collection/P02/current/COAS/"/>
        <rdfs:comment xml:lang="en">Parameters relating to the mapping of terrestrial features, including coastlines</rdfs:comment>
        <rdfs:label xml:lang="en">Terrestrial mapping</rdfs:label>
        <rdf:type rdf:resource="http://www.w3.org/2002/07/owl#NamedIndividual"/>
        <rdf:type rdf:resource="http://www.w3.org/2002/07/owl#Class"/>
      </glview:MeasurementType>
    </rdfs:subClassOf>
    <owl:someValuesFrom>
      <owl:Class>
        <owl:oneOf rdf:parseType="Collection">
          <glview:MeasurementType rdf:about="http://schema.geolink.org/dev/voc/nvs/P02#COAS"/>
        </owl:oneOf>
      </owl:Class>
    </owl:someValuesFrom>
    <owl:onProperty rdf:resource="http://schema.geolink.org/dev/view#hasMeasurementType"/>
  </owl:Restriction>
  <owl:Restriction>
    <rdfs:subClassOf>
      <glview:MeasurementType rdf:about="http://schema.geolink.org/dev/voc/nvs/P02#WBRX">
        <rdfs:subClassOf rdf:resource="http://schema.geolink.org/dev/voc/nvs/P03#C045"/>
        <rdfs:seeAlso rdf:resource="http://vocab.nerc.ac.uk/collection/P02/current/WBRX/"/>
        <rdfs:comment xml:lang="en">A measure of the tendency of any body of fresh or salt water to either gain or lose electrons when it is subject to change by introduction of a new species.</rdfs:comment>
        <rdfs:label xml:lang="en">Water body redox potential</rdfs:label>
        <rdf:type rdf:resource="http://www.w3.org/2002/07/owl#NamedIndividual"/>
        <rdf:type rdf:resource="http://www.w3.org/2002/07/owl#Class"/>
      </glview:MeasurementType>
    </rdfs:subClassOf>
    <owl:someValuesFrom>
      <owl:Class>
        <owl:oneOf rdf:parseType="Collection">
          <glview:MeasurementType rdf:about="http://schema.geolink.org/dev/voc/nvs/P02#WBRX"/>
        </owl:oneOf>
      </owl:Class>
    </owl:someValuesFrom>
    <owl:onProperty rdf:resource="http://schema.geolink.org/dev/view#hasMeasurementType"/>
  </owl:Restriction>
  <owl:Restriction>
    <rdfs:subClassOf rdf:resource="http://schema.geolink.org/dev/voc/nvs/P02#BATC"/>
    <owl:someValuesFrom>
      <owl:Class>
        <owl:oneOf rdf:parseType="Collection">
          <glview:MeasurementType rdf:about="http://schema.geolink.org/dev/voc/nvs/P02#BATC"/>
        </owl:oneOf>
      </owl:Class>
    </owl:someValuesFrom>
    <owl:onProperty rdf:resource="http://schema.geolink.org/dev/view#hasMeasurementType"/>
  </owl:Restriction>
  <owl:Restriction>
    <rdfs:subClassOf rdf:resource="http://schema.geolink.org/dev/voc/nvs/P02#TCO2"/>
    <owl:someValuesFrom>
      <owl:Class>
        <owl:oneOf rdf:parseType="Collection">
          <glview:MeasurementType rdf:about="http://schema.geolink.org/dev/voc/nvs/P02#TCO2"/>
        </owl:oneOf>
      </owl:Class>
    </owl:someValuesFrom>
    <owl:onProperty rdf:resource="http://schema.geolink.org/dev/view#hasMeasurementType"/>
  </owl:Restriction>
  <owl:Restriction>
    <rdfs:subClassOf>
      <glview:MeasurementType rdf:about="http://schema.geolink.org/dev/voc/nvs/P02#CXAA">
        <rdfs:subClassOf rdf:resource="http://schema.geolink.org/dev/voc/nvs/P03#M005"/>
        <rdfs:seeAlso rdf:resource="http://vocab.nerc.ac.uk/collection/P02/current/CXAA/"/>
        <rdfs:comment xml:lang="en">Parameters quantifying the concentration of acids containing a carboxyl (-C(=O)OH) group, their anions or their salts in any phase of the atmosphere</rdfs:comment>
        <rdfs:label xml:lang="en">Concentrations of carboxylic acids and carboxylates in the atmosphere</rdfs:label>
        <rdf:type rdf:resource="http://www.w3.org/2002/07/owl#NamedIndividual"/>
        <rdf:type rdf:resource="http://www.w3.org/2002/07/owl#Class"/>
      </glview:MeasurementType>
    </rdfs:subClassOf>
    <owl:someValuesFrom>
      <owl:Class>
        <owl:oneOf rdf:parseType="Collection">
          <glview:MeasurementType rdf:about="http://schema.geolink.org/dev/voc/nvs/P02#CXAA"/>
        </owl:oneOf>
      </owl:Class>
    </owl:someValuesFrom>
    <owl:onProperty rdf:resource="http://schema.geolink.org/dev/view#hasMeasurementType"/>
  </owl:Restriction>
  <owl:Restriction>
    <rdfs:subClassOf rdf:resource="http://schema.geolink.org/dev/voc/nvs/P02#VSRA"/>
    <owl:someValuesFrom>
      <owl:Class>
        <owl:oneOf rdf:parseType="Collection">
          <glview:MeasurementType rdf:about="http://schema.geolink.org/dev/voc/nvs/P02#VSRA"/>
        </owl:oneOf>
      </owl:Class>
    </owl:someValuesFrom>
    <owl:onProperty rdf:resource="http://schema.geolink.org/dev/view#hasMeasurementType"/>
  </owl:Restriction>
  <owl:Restriction>
    <rdfs:subClassOf rdf:resource="http://schema.geolink.org/dev/voc/nvs/P02#ZNLG"/>
    <owl:someValuesFrom>
      <owl:Class>
        <owl:oneOf rdf:parseType="Collection">
          <glview:MeasurementType rdf:about="http://schema.geolink.org/dev/voc/nvs/P02#ZNLG"/>
        </owl:oneOf>
      </owl:Class>
    </owl:someValuesFrom>
    <owl:onProperty rdf:resource="http://schema.geolink.org/dev/view#hasMeasurementType"/>
  </owl:Restriction>
  <owl:Restriction>
    <rdfs:subClassOf rdf:resource="http://schema.geolink.org/dev/voc/nvs/P02#PCAH"/>
    <owl:someValuesFrom>
      <owl:Class>
        <owl:oneOf rdf:parseType="Collection">
          <owl:Class rdf:about="http://schema.geolink.org/dev/voc/nvs/P02#PCAH"/>
        </owl:oneOf>
      </owl:Class>
    </owl:someValuesFrom>
    <owl:onProperty rdf:resource="http://schema.geolink.org/dev/view#hasMeasurementType"/>
  </owl:Restriction>
</rdf:RDF>
