@prefix : <http://schema.geolink.org/1.0/voc/nvs/P02#> .
@prefix dc: <http://purl.org/dc/elements/1.1/> .
@prefix dcterms: <http://purl.org/dc/terms/> .
@prefix glbase: <http://schema.geolink.org/1.0/base/main#> .
@prefix idscheme: <http://schema.geolink.org/1.0/voc/identifierscheme#> .
@prefix owl: <http://www.w3.org/2002/07/owl#> .
@prefix rdf: <http://www.w3.org/1999/02/22-rdf-syntax-ns#> .
@prefix rdfs: <http://www.w3.org/2000/01/rdf-schema#> .
@prefix skos: <http://www.w3.org/2004/02/skos/core#> .
@prefix xml: <http://www.w3.org/XML/1998/namespace> .
@prefix xsd: <http://www.w3.org/2001/XMLSchema#> .
glbase:hasIdentifier a owl:ObjectProperty .
glbase:hasIdentifierScheme a owl:ObjectProperty .
glbase:hasIdentifierValue a owl:DatatypeProperty .
<http://schema.geolink.org/1.0/voc/nvs/P02> a owl:Ontology ;
    rdfs:label "SeaDataNet Parameter Discovery Vocabulary" ;
    dcterms:creator "EarthCube GeoLink project"@en ;
    dcterms:date "2015-11-17 02:00:02.0" ;
    dcterms:title "SeaDataNet Parameter Discovery Vocabulary" ;
    rdfs:comment "This ontology captures SeaDataNet device catalog from the NERC vocabulary server with mapping to SeaDataNet device categories"@en ;
    rdfs:seeAlso <http://vocab.nerc.ac.uk/collection/P02/current/> ;
    owl:imports <http://schema.geolink.org/1.0/voc/nvs/P03> .
<http://vocab.nerc.ac.uk/collection/P03/current/H003/> a owl:Class .
<http://vocab.nerc.ac.uk/collection/P02/current/A01X/> a glbase:MeasurementType,
        owl:Class,
        owl:NamedIndividual ;
    rdfs:label "Sedimentation flux of alkenones and alkenoates in the water column"@en ;
    dcterms:creator "SeaDataNet" ;
    dcterms:date "2012-03-01 16:14:45.0" ;
    glbase:hasIdentifier [ glbase:hasIdentifierScheme idscheme:sdn ;
            glbase:hasIdentifierValue "SDN:P02::A01X" ] ;
    rdfs:comment "Parameters quantifying the rate of alkenones (unsaturated aliphatic ketones) and alkenoates (carboxylic acid esters) sinking as particles through any body of water."@en ;
    rdfs:subClassOf <http://vocab.nerc.ac.uk/collection/P03/current/O005/> ;
    owl:deprecated "false" .
<http://vocab.nerc.ac.uk/collection/P02/current/A999/> a glbase:MeasurementType,
        owl:Class,
        owl:NamedIndividual ;
    rdfs:label "Microzooplankton taxonomy-related biosurface area per unit volume of the water column"@en ;
    dcterms:creator "SeaDataNet" ;
    dcterms:date "2003-06-10 13:53:19.0" ;
    glbase:hasIdentifier [ glbase:hasIdentifierScheme idscheme:sdn ;
            glbase:hasIdentifierValue "SDN:P02::A999" ] ;
    rdfs:comment "Microzooplankton surface area per unit volume of the water column parameters presented at the level of taxa that may be mapped to entities in the ITIS taxonomy.  These may be at any taxonomic level from sub-species upwards."@en ;
    rdfs:subClassOf <http://vocab.nerc.ac.uk/collection/P03/current/B025/> ;
    owl:deprecated "false" .
<http://vocab.nerc.ac.uk/collection/P02/current/AAFX/> a glbase:MeasurementType,
        owl:Class,
        owl:NamedIndividual ;
    rdfs:label "Sedimentation flux of amino acids and associated compounds in water bodies"@en ;
    dcterms:creator "SeaDataNet" ;
    dcterms:date "2011-09-08 10:07:59.0" ;
    glbase:hasIdentifier [ glbase:hasIdentifierScheme idscheme:sdn ;
            glbase:hasIdentifierValue "SDN:P02::AAFX" ] ;
    rdfs:comment "Parameters quantifying the amount of organic compounds containing both a carboxyl group and an amino group (including compounds such as salts and esters) sinking vertically as particles through a unit area of a water body in units time."@en ;
    rdfs:subClassOf <http://vocab.nerc.ac.uk/collection/P03/current/C003/>,
        <http://vocab.nerc.ac.uk/collection/P03/current/O005/> ;
    owl:deprecated "false" .
<http://vocab.nerc.ac.uk/collection/P02/current/AALK/> a glbase:MeasurementType,
        owl:Class,
        owl:NamedIndividual ;
    rdfs:label "Concentration of alkanes in the atmosphere"@en ;
    dcterms:creator "SeaDataNet" ;
    dcterms:date "2004-06-24 17:10:00.0" ;
    glbase:hasIdentifier [ glbase:hasIdentifierScheme idscheme:sdn ;
            glbase:hasIdentifierValue "SDN:P02::AALK" ] ;
    rdfs:comment "Alkane concentrations in all phases of the atmosphere"@en ;
    rdfs:subClassOf <http://vocab.nerc.ac.uk/collection/P03/current/C025/>,
        <http://vocab.nerc.ac.uk/collection/P03/current/M005/> ;
    owl:deprecated "false" .
<http://vocab.nerc.ac.uk/collection/P02/current/AAMN/> a glbase:MeasurementType,
        owl:Class,
        owl:NamedIndividual ;
    rdfs:label "Concentration of nitrogen species in the atmosphere"@en ;
    dcterms:creator "SeaDataNet" ;
    dcterms:date "2004-08-18 09:12:08.0" ;
    glbase:hasIdentifier [ glbase:hasIdentifierScheme idscheme:sdn ;
            glbase:hasIdentifierValue "SDN:P02::AAMN" ] ;
    rdfs:comment "Concentrations of both organic (eg amines) and inorganic (eg ammonia and oxides of nitrogen) nitrogen species in all phases of the atmosphere"@en ;
    rdfs:subClassOf <http://vocab.nerc.ac.uk/collection/P03/current/M005/> ;
    owl:deprecated "false" .
<http://vocab.nerc.ac.uk/collection/P02/current/AASD/> a glbase:MeasurementType,
        owl:Class,
        owl:NamedIndividual ;
    rdfs:label "Concentration of alkenones and alkenoates in sediment"@en ;
    dcterms:creator "SeaDataNet" ;
    dcterms:date "2012-03-02 16:22:50.0" ;
    glbase:hasIdentifier [ glbase:hasIdentifierScheme idscheme:sdn ;
            glbase:hasIdentifierValue "SDN:P02::AASD" ] ;
    rdfs:comment "Parameters quantifying the amount of alkenones (unsaturated aliphatic ketones) and alkenoates (carboxylic acid esters) in any unconsolidated sediment including fluff."@en ;
    rdfs:subClassOf <http://vocab.nerc.ac.uk/collection/P03/current/C050/>,
        <http://vocab.nerc.ac.uk/collection/P03/current/G035/> ;
    owl:deprecated "false" .
<http://vocab.nerc.ac.uk/collection/P02/current/AATX/> a glbase:MeasurementType,
        owl:Class,
        owl:NamedIndividual ;
    rdfs:label "Phytoplankton taxonomic surface area in water bodies"@en ;
    dcterms:creator "SeaDataNet" ;
    dcterms:date "2010-10-21 13:52:21.0" ;
    glbase:hasIdentifier [ glbase:hasIdentifierScheme idscheme:sdn ;
            glbase:hasIdentifierValue "SDN:P02::AATX" ] ;
    rdfs:comment "Any parameterisation of cell surface area of free-floating autotrophic biological entities designated by taxonomic names (e.g. species, genus, family) in any body of fresh or salt water."@en ;
    rdfs:subClassOf <http://vocab.nerc.ac.uk/collection/P03/current/B030/> ;
    owl:deprecated "false" .
<http://vocab.nerc.ac.uk/collection/P02/current/AAWC/> a glbase:MeasurementType,
        owl:Class,
        owl:NamedIndividual ;
    rdfs:label "Concentration of alkanamines (amines) in the water column"@en ;
    dcterms:creator "SeaDataNet" ;
    dcterms:date "2004-08-13 09:38:00.0" ;
    glbase:hasIdentifier [ glbase:hasIdentifierScheme idscheme:sdn ;
            glbase:hasIdentifierValue "SDN:P02::AAWC" ] ;
    rdfs:comment "Alkanamine concentrations in all phases of the water column"@en ;
    rdfs:subClassOf <http://vocab.nerc.ac.uk/collection/P03/current/C050/> ;
    owl:deprecated "false" .
<http://vocab.nerc.ac.uk/collection/P02/current/ABAG/> a glbase:MeasurementType,
        owl:Class,
        owl:NamedIndividual ;
    rdfs:label "Suspended particulate material aggregates"@en ;
    dcterms:creator "SeaDataNet" ;
    dcterms:date "2004-08-17 14:50:43.0" ;
    glbase:hasIdentifier [ glbase:hasIdentifierScheme idscheme:sdn ;
            glbase:hasIdentifierValue "SDN:P02::ABAG" ] ;
    rdfs:comment "Parameters relating to the abundance, size and morphology of particle aggregates in the SPM"@en ;
    rdfs:subClassOf <http://vocab.nerc.ac.uk/collection/P03/current/G015/> ;
    owl:deprecated "false" .
<http://vocab.nerc.ac.uk/collection/P02/current/ACFL/> a glbase:MeasurementType,
        owl:Class,
        owl:NamedIndividual ;
    rdfs:label "Quality control flags"@en ;
    dcterms:creator "SeaDataNet" ;
    dcterms:date "2004-08-20 10:36:40.0" ;
    glbase:hasIdentifier [ glbase:hasIdentifierScheme idscheme:sdn ;
            glbase:hasIdentifierValue "SDN:P02::ACFL" ] ;
    rdfs:comment "" ;
    rdfs:subClassOf <http://vocab.nerc.ac.uk/collection/P03/current/Z005/> ;
    owl:deprecated "false" .
<http://vocab.nerc.ac.uk/collection/P02/current/ACNT/> a glbase:MeasurementType,
        owl:Class,
        owl:NamedIndividual ;
    rdfs:label "Macroalgae and seagrass taxonomy-related counts"@en ;
    dcterms:creator "SeaDataNet" ;
    dcterms:date "2007-01-08 16:45:03.0" ;
    glbase:hasIdentifier [ glbase:hasIdentifierScheme idscheme:sdn ;
            glbase:hasIdentifierValue "SDN:P02::ACNT" ] ;
    rdfs:comment "Macroalgae (Rhodophycota, Chromphycota, Chlorophycota) and seagrass (Charophyta, Anthophyta) count parameters presented at the level of taxa at any level from sub-species upwards. Count includes presence/absence indicators."@en ;
    rdfs:subClassOf <http://vocab.nerc.ac.uk/collection/P03/current/B055/> ;
    owl:deprecated "false" .
<http://vocab.nerc.ac.uk/collection/P02/current/ACO2/> a glbase:MeasurementType,
        owl:Class,
        owl:NamedIndividual ;
    rdfs:label "Carbon monoxide and dioxide concentrations in the atmosphere"@en ;
    dcterms:creator "SeaDataNet" ;
    dcterms:date "2006-06-05 12:17:29.0" ;
    glbase:hasIdentifier [ glbase:hasIdentifierScheme idscheme:sdn ;
            glbase:hasIdentifierValue "SDN:P02::ACO2" ] ;
    rdfs:comment "CO and CO2 concentration parameters in any phase of the atmosphere (but usuall the gaseous phase). Includes pCO2."@en ;
    rdfs:subClassOf <http://vocab.nerc.ac.uk/collection/P03/current/M005/> ;
    owl:deprecated "false" .
<http://vocab.nerc.ac.uk/collection/P02/current/ACSR/> a glbase:MeasurementType,
        owl:Class,
        owl:NamedIndividual ;
    rdfs:label "Active seismic refraction"@en ;
    dcterms:creator "SeaDataNet" ;
    dcterms:date "2010-02-21 17:24:30.0" ;
    glbase:hasIdentifier [ glbase:hasIdentifierScheme idscheme:sdn ;
            glbase:hasIdentifierValue "SDN:P02::ACSR" ] ;
    rdfs:comment "Parameters quantifying the magnitude of earth movements resulting from artificial sources (such as explosions) far away from the measurement site."@en ;
    rdfs:subClassOf <http://vocab.nerc.ac.uk/collection/P03/current/G012/>,
        <http://vocab.nerc.ac.uk/collection/P03/current/GPYS/> ;
    owl:deprecated "false" .
<http://vocab.nerc.ac.uk/collection/P02/current/ACYC/> a glbase:MeasurementType,
        owl:Class,
        owl:NamedIndividual ;
    rdfs:label "Reference numbers"@en ;
    dcterms:creator "SeaDataNet" ;
    dcterms:date "2004-08-20 11:00:40.0" ;
    glbase:hasIdentifier [ glbase:hasIdentifierScheme idscheme:sdn ;
            glbase:hasIdentifierValue "SDN:P02::ACYC" ] ;
    rdfs:comment "Data record, event, sample or measurement reference numbers"@en ;
    rdfs:subClassOf <http://vocab.nerc.ac.uk/collection/P03/current/Z005/> ;
    owl:deprecated "false" .
<http://vocab.nerc.ac.uk/collection/P02/current/ADUN/> a glbase:MeasurementType,
        owl:Class,
        owl:NamedIndividual ;
    rdfs:label "Administrative units"@en ;
    dcterms:creator "SeaDataNet" ;
    dcterms:date "2012-07-17 07:51:20.0" ;
    glbase:hasIdentifier [ glbase:hasIdentifierScheme idscheme:sdn ;
            glbase:hasIdentifierValue "SDN:P02::ADUN" ] ;
    rdfs:comment "Parameters (including geometries, labels and categorizations) relating to areas where authorities have and-or excercise specific rights or obligations."@en ;
    rdfs:subClassOf <http://vocab.nerc.ac.uk/collection/P03/current/B015/>,
        <http://vocab.nerc.ac.uk/collection/P03/current/B020/>,
        <http://vocab.nerc.ac.uk/collection/P03/current/B050/>,
        <http://vocab.nerc.ac.uk/collection/P03/current/B055/>,
        <http://vocab.nerc.ac.uk/collection/P03/current/G055/>,
        <http://vocab.nerc.ac.uk/collection/P03/current/H002/>,
        <http://vocab.nerc.ac.uk/collection/P03/current/H004/>,
        <http://vocab.nerc.ac.uk/collection/P03/current/H005/> ;
    owl:deprecated "false" .
<http://vocab.nerc.ac.uk/collection/P02/current/AEYN/> a glbase:MeasurementType,
        owl:Class,
        owl:NamedIndividual ;
    rdfs:label "Concentration of alkenes and alkynes in the atmosphere"@en ;
    dcterms:creator "SeaDataNet" ;
    dcterms:date "2004-07-30 14:35:00.0" ;
    glbase:hasIdentifier [ glbase:hasIdentifierScheme idscheme:sdn ;
            glbase:hasIdentifierValue "SDN:P02::AEYN" ] ;
    rdfs:comment "Alkene and alkyne concentrations in all phases of the atmosphere"@en ;
    rdfs:subClassOf <http://vocab.nerc.ac.uk/collection/P03/current/C025/>,
        <http://vocab.nerc.ac.uk/collection/P03/current/M005/> ;
    owl:deprecated "false" .
<http://vocab.nerc.ac.uk/collection/P02/current/AHGT/> a glbase:MeasurementType,
        owl:Class,
        owl:NamedIndividual ;
    rdfs:label "Vertical spatial coordinates"@en ;
    dcterms:creator "SeaDataNet" ;
    dcterms:date "2004-03-25 16:36:18.0" ;
    glbase:hasIdentifier [ glbase:hasIdentifierScheme idscheme:sdn ;
            glbase:hasIdentifierValue "SDN:P02::AHGT" ] ;
    rdfs:comment "All vertical spatial parameters including depth, height and pressure when used as an independent variable."@en ;
    rdfs:subClassOf <http://vocab.nerc.ac.uk/collection/P03/current/Z005/> ;
    owl:deprecated "false" .
<http://vocab.nerc.ac.uk/collection/P02/current/ALAT/> a glbase:MeasurementType,
        owl:Class,
        owl:NamedIndividual ;
    rdfs:label "Horizontal spatial co-ordinates"@en ;
    dcterms:creator "SeaDataNet" ;
    dcterms:date "2004-03-25 16:18:08.0" ;
    glbase:hasIdentifier [ glbase:hasIdentifierScheme idscheme:sdn ;
            glbase:hasIdentifierValue "SDN:P02::ALAT" ] ;
    rdfs:comment "All forms of horizontal spatial coordinates such as lat/lon and grid references"@en ;
    rdfs:subClassOf <http://vocab.nerc.ac.uk/collection/P03/current/Z005/> ;
    owl:deprecated "false" .
<http://vocab.nerc.ac.uk/collection/P02/current/ALKY/> a glbase:MeasurementType,
        owl:Class,
        owl:NamedIndividual ;
    rdfs:label "Alkalinity, acidity and pH of the water column"@en ;
    dcterms:creator "SeaDataNet" ;
    dcterms:date "2008-08-15 10:11:46.0" ;
    glbase:hasIdentifier [ glbase:hasIdentifierScheme idscheme:sdn ;
            glbase:hasIdentifierValue "SDN:P02::ALKY" ] ;
    rdfs:comment "Parameters quantifying the hydrogen ion concentration in water bodies"@en ;
    rdfs:subClassOf <http://vocab.nerc.ac.uk/collection/P03/current/C010/> ;
    owl:deprecated "false" .
<http://vocab.nerc.ac.uk/collection/P02/current/AMON/> a glbase:MeasurementType,
        owl:Class,
        owl:NamedIndividual ;
    rdfs:label "Ammonium and ammonia concentration parameters in water bodies"@en ;
    dcterms:creator "SeaDataNet" ;
    dcterms:date "2015-11-16 12:09:46.0" ;
    glbase:hasIdentifier [ glbase:hasIdentifierScheme idscheme:sdn ;
            glbase:hasIdentifierValue "SDN:P02::AMON" ] ;
    rdfs:comment """Ammonium and ammonia concentration parameters 
(including statistical parameters such as standard deviation) in any body of fresh or salt water."""@en ;
    rdfs:subClassOf <http://vocab.nerc.ac.uk/collection/P03/current/C005/>,
        <http://vocab.nerc.ac.uk/collection/P03/current/C040/> ;
    owl:deprecated "false" .
<http://vocab.nerc.ac.uk/collection/P02/current/AMOX/> a glbase:MeasurementType,
        owl:Class,
        owl:NamedIndividual ;
    rdfs:label "Nitrification rate in the water column"@en ;
    dcterms:creator "SeaDataNet" ;
    dcterms:date "2004-07-29 10:24:29.0" ;
    glbase:hasIdentifier [ glbase:hasIdentifierScheme idscheme:sdn ;
            glbase:hasIdentifierValue "SDN:P02::AMOX" ] ;
    rdfs:comment "Parameters relating to the rate of nitrification (oxidation of reduced nitrogen such as ammonium) in the water column"@en ;
    rdfs:subClassOf <http://vocab.nerc.ac.uk/collection/P03/current/C005/>,
        <http://vocab.nerc.ac.uk/collection/P03/current/C040/>,
        <http://vocab.nerc.ac.uk/collection/P03/current/O010/> ;
    owl:deprecated "false" .
<http://vocab.nerc.ac.uk/collection/P02/current/AMUP/> a glbase:MeasurementType,
        owl:Class,
        owl:NamedIndividual ;
    rdfs:label "Regenerated production in water bodies"@en ;
    dcterms:creator "SeaDataNet" ;
    dcterms:date "2009-11-15 16:13:39.0" ;
    glbase:hasIdentifier [ glbase:hasIdentifierScheme idscheme:sdn ;
            glbase:hasIdentifierValue "SDN:P02::AMUP" ] ;
    rdfs:comment "Parameters quantifying the uptake rate of nitrogen from excretion products (ammonium and urea) by flora and fauna living in any body of salt or fresh water"@en ;
    rdfs:subClassOf <http://vocab.nerc.ac.uk/collection/P03/current/C040/>,
        <http://vocab.nerc.ac.uk/collection/P03/current/O010/> ;
    owl:deprecated "false" .
<http://vocab.nerc.ac.uk/collection/P02/current/AORG/> a glbase:MeasurementType,
        owl:Class,
        owl:NamedIndividual ;
    rdfs:label "Concentration of organic matter in the atmosphere"@en ;
    dcterms:creator "SeaDataNet" ;
    dcterms:date "2008-03-05 08:35:42.0" ;
    glbase:hasIdentifier [ glbase:hasIdentifierScheme idscheme:sdn ;
            glbase:hasIdentifierValue "SDN:P02::AORG" ] ;
    rdfs:comment "Parameters quantifying uncategorised organic substance concentrations in atmospheric, generally aerosol, samples such as organic matter and DOC."@en ;
    rdfs:subClassOf <http://vocab.nerc.ac.uk/collection/P03/current/M005/> ;
    owl:deprecated "false" .
<http://vocab.nerc.ac.uk/collection/P02/current/APDA/> a glbase:MeasurementType,
        owl:Class,
        owl:NamedIndividual ;
    rdfs:label "Horizontal platform movement"@en ;
    dcterms:creator "SeaDataNet" ;
    dcterms:date "2004-08-20 11:05:57.0" ;
    glbase:hasIdentifier [ glbase:hasIdentifierScheme idscheme:sdn ;
            glbase:hasIdentifierValue "SDN:P02::APDA" ] ;
    rdfs:comment "All parameters relating to horizontal platform travel, including distance run"@en ;
    rdfs:subClassOf <http://vocab.nerc.ac.uk/collection/P03/current/Z005/> ;
    owl:deprecated "false" .
<http://vocab.nerc.ac.uk/collection/P02/current/APZA/> a glbase:MeasurementType,
        owl:Class,
        owl:NamedIndividual ;
    rdfs:label "Vertical platform movement"@en ;
    dcterms:creator "SeaDataNet" ;
    dcterms:date "2008-12-09 11:15:07.0" ;
    glbase:hasIdentifier [ glbase:hasIdentifierScheme idscheme:sdn ;
            glbase:hasIdentifierValue "SDN:P02::APZA" ] ;
    rdfs:comment "Parameters quantifying the upward and downward motion of objects mounting sensors or collecting samples."@en ;
    rdfs:subClassOf <http://vocab.nerc.ac.uk/collection/P03/current/Z005/> ;
    owl:deprecated "false" .
<http://vocab.nerc.ac.uk/collection/P02/current/AQYN/> a glbase:MeasurementType,
        owl:Class,
        owl:NamedIndividual ;
    rdfs:label "Concentration of alkenes and alkynes in the water column"@en ;
    dcterms:creator "SeaDataNet" ;
    dcterms:date "2004-07-30 14:35:00.0" ;
    glbase:hasIdentifier [ glbase:hasIdentifierScheme idscheme:sdn ;
            glbase:hasIdentifierValue "SDN:P02::AQYN" ] ;
    rdfs:comment "Alkene and alkyne concentrations in all phases of the water column"@en ;
    rdfs:subClassOf <http://vocab.nerc.ac.uk/collection/P03/current/C025/> ;
    owl:deprecated "false" .
<http://vocab.nerc.ac.uk/collection/P02/current/ASAM/> a glbase:MeasurementType,
        owl:Class,
        owl:NamedIndividual ;
    rdfs:label "Acoustic backscatter in the water column"@en ;
    dcterms:creator "SeaDataNet" ;
    dcterms:date "2004-06-28 16:32:47.0" ;
    glbase:hasIdentifier [ glbase:hasIdentifierScheme idscheme:sdn ;
            glbase:hasIdentifierValue "SDN:P02::ASAM" ] ;
    rdfs:comment "Includes all parameters covering the strength of acoustic signal return, including absolute measurements of returning signal strength as well as parameters expressed as backscatter (the proportion of transmitted signal returned)"@en ;
    rdfs:subClassOf <http://vocab.nerc.ac.uk/collection/P03/current/D005/> ;
    owl:deprecated "false" .
<http://vocab.nerc.ac.uk/collection/P02/current/ASLV/> a glbase:MeasurementType,
        owl:Class,
        owl:NamedIndividual ;
    rdfs:label "Sea level"@en ;
    dcterms:creator "SeaDataNet" ;
    dcterms:date "2007-06-19 11:32:16.0" ;
    glbase:hasIdentifier [ glbase:hasIdentifierScheme idscheme:sdn ;
            glbase:hasIdentifierValue "SDN:P02::ASLV" ] ;
    rdfs:comment "Measurements and predictions of the displacement of the water column surface from a fixed, stable reference"@en ;
    rdfs:subClassOf <http://vocab.nerc.ac.uk/collection/P03/current/D032/> ;
    owl:deprecated "false" .
<http://vocab.nerc.ac.uk/collection/P02/current/ATDP/> a glbase:MeasurementType,
        owl:Class,
        owl:NamedIndividual ;
    rdfs:label "Atmospheric deposition rates"@en ;
    dcterms:creator "SeaDataNet" ;
    dcterms:date "2006-07-07 12:36:43.0" ;
    glbase:hasIdentifier [ glbase:hasIdentifierScheme idscheme:sdn ;
            glbase:hasIdentifierValue "SDN:P02::ATDP" ] ;
    rdfs:comment "Fluxes of chemical species from the atmosphere to sea or land surface including precipitation and aerosol deposition but excluding fluxes due to exchange of gases"@en ;
    rdfs:subClassOf <http://vocab.nerc.ac.uk/collection/P03/current/M005/>,
        <http://vocab.nerc.ac.uk/collection/P03/current/O005/> ;
    owl:deprecated "false" .
<http://vocab.nerc.ac.uk/collection/P02/current/ATEM/> a glbase:MeasurementType,
        owl:Class,
        owl:NamedIndividual ;
    rdfs:label "Atmospheric emissions"@en ;
    dcterms:creator "SeaDataNet" ;
    dcterms:date "2008-12-09 10:17:11.0" ;
    glbase:hasIdentifier [ glbase:hasIdentifierScheme idscheme:sdn ;
            glbase:hasIdentifierValue "SDN:P02::ATEM" ] ;
    rdfs:comment "Parameters quantifying and describing the release of substances into the atmosphere as a result of human activity"@en ;
    rdfs:subClassOf <http://vocab.nerc.ac.uk/collection/P03/current/H001/>,
        <http://vocab.nerc.ac.uk/collection/P03/current/O005/> ;
    owl:deprecated "false" .
<http://vocab.nerc.ac.uk/collection/P02/current/ATPC/> a glbase:MeasurementType,
        owl:Class,
        owl:NamedIndividual ;
    rdfs:label "Atmospheric particulates"@en ;
    dcterms:creator "SeaDataNet" ;
    dcterms:date "2006-05-26 13:26:07.0" ;
    glbase:hasIdentifier [ glbase:hasIdentifierScheme idscheme:sdn ;
            glbase:hasIdentifierValue "SDN:P02::ATPC" ] ;
    rdfs:comment "Parameters quantifying and categorising the particulate phases (solids and aerosols) of the atmosphere, excluding chemical composition"@en ;
    rdfs:subClassOf <http://vocab.nerc.ac.uk/collection/P03/current/M005/> ;
    owl:deprecated "false" .
<http://vocab.nerc.ac.uk/collection/P02/current/ATPX/> a glbase:MeasurementType,
        owl:Class,
        owl:NamedIndividual ;
    rdfs:label "Concentration of adenlylates in the water column"@en ;
    dcterms:creator "SeaDataNet" ;
    dcterms:date "2004-08-13 11:11:26.0" ;
    glbase:hasIdentifier [ glbase:hasIdentifierScheme idscheme:sdn ;
            glbase:hasIdentifierValue "SDN:P02::ATPX" ] ;
    rdfs:comment "Concentrations of adenylates (ADP, ATP etc) in all phases of the water column"@en ;
    rdfs:subClassOf <http://vocab.nerc.ac.uk/collection/P03/current/C050/> ;
    owl:deprecated "false" .
<http://vocab.nerc.ac.uk/collection/P02/current/ATTN/> a glbase:MeasurementType,
        owl:Class,
        owl:NamedIndividual ;
    rdfs:label "Transmittance and attenuance of the water column"@en ;
    dcterms:creator "SeaDataNet" ;
    dcterms:date "2007-11-21 16:25:20.0" ;
    glbase:hasIdentifier [ glbase:hasIdentifierScheme idscheme:sdn ;
            glbase:hasIdentifierValue "SDN:P02::ATTN" ] ;
    rdfs:comment "Parameters relating to the rate of electromagnetic radiation intensity decrease as it travels through the water column"@en ;
    rdfs:subClassOf <http://vocab.nerc.ac.uk/collection/P03/current/D015/> ;
    owl:deprecated "false" .
<http://vocab.nerc.ac.uk/collection/P02/current/ATVS/> a glbase:MeasurementType,
        owl:Class,
        owl:NamedIndividual ;
    rdfs:label "Atmospheric visibility and transparency"@en ;
    dcterms:creator "SeaDataNet" ;
    dcterms:date "2006-05-26 09:57:58.0" ;
    glbase:hasIdentifier [ glbase:hasIdentifierScheme idscheme:sdn ;
            glbase:hasIdentifierValue "SDN:P02::ATVS" ] ;
    rdfs:comment "Parameters relating to atmospheric clarity, such as optical transmittance/attenuance, and resultant visibility"@en ;
    rdfs:subClassOf <http://vocab.nerc.ac.uk/collection/P03/current/M010/> ;
    owl:deprecated "false" .
<http://vocab.nerc.ac.uk/collection/P02/current/AXFX/> a glbase:MeasurementType,
        owl:Class,
        owl:NamedIndividual ;
    rdfs:label "Sedimentation flux of pigments in the water column"@en ;
    dcterms:creator "SeaDataNet" ;
    dcterms:date "2004-07-29 16:41:40.0" ;
    glbase:hasIdentifier [ glbase:hasIdentifierScheme idscheme:sdn ;
            glbase:hasIdentifierValue "SDN:P02::AXFX" ] ;
    rdfs:comment "" ;
    rdfs:subClassOf <http://vocab.nerc.ac.uk/collection/P03/current/B035/>,
        <http://vocab.nerc.ac.uk/collection/P03/current/O005/> ;
    owl:deprecated "false" .
<http://vocab.nerc.ac.uk/collection/P02/current/AYMD/> a glbase:MeasurementType,
        owl:Class,
        owl:NamedIndividual ;
    rdfs:label "Date and time"@en ;
    dcterms:creator "SeaDataNet" ;
    dcterms:date "2004-03-25 16:28:17.0" ;
    glbase:hasIdentifier [ glbase:hasIdentifierScheme idscheme:sdn ;
            glbase:hasIdentifierValue "SDN:P02::AYMD" ] ;
    rdfs:comment "All date and time parameters"@en ;
    rdfs:subClassOf <http://vocab.nerc.ac.uk/collection/P03/current/Z005/> ;
    owl:deprecated "false" .
<http://vocab.nerc.ac.uk/collection/P02/current/BABI/> a glbase:MeasurementType,
        owl:Class,
        owl:NamedIndividual ;
    rdfs:label "Bacteria in biota"@en ;
    dcterms:creator "SeaDataNet" ;
    dcterms:date "2008-01-30 07:53:20.0" ;
    glbase:hasIdentifier [ glbase:hasIdentifierScheme idscheme:sdn ;
            glbase:hasIdentifierValue "SDN:P02::BABI" ] ;
    rdfs:comment "Parameters relating to the abundance and nature of bacteria (Kingdom Monera) infecting other biota."@en ;
    rdfs:subClassOf <http://vocab.nerc.ac.uk/collection/P03/current/B005/>,
        <http://vocab.nerc.ac.uk/collection/P03/current/B007/>,
        <http://vocab.nerc.ac.uk/collection/P03/current/H001/> ;
    owl:deprecated "false" .
<http://vocab.nerc.ac.uk/collection/P02/current/BATC/> a glbase:MeasurementType,
        owl:Class,
        owl:NamedIndividual ;
    rdfs:label "Bacteria taxonomy-related biomass expressed as carbon per unit volume of the water column"@en ;
    dcterms:creator "SeaDataNet" ;
    dcterms:date "2004-04-14 11:15:00.0" ;
    glbase:hasIdentifier [ glbase:hasIdentifierScheme idscheme:sdn ;
            glbase:hasIdentifierValue "SDN:P02::BATC" ] ;
    rdfs:comment "Bacteria carbon biomass parameters presented at the level of taxa that may be mapped to entities in the ITIS taxonomy.  These may be at any taxonomic level from sub-species upwards.  Bacteria are defined as all taxa that fall into Kingdom Monera in the ITIS taxonomy, which includes cyanobacteria."@en ;
    rdfs:subClassOf <http://vocab.nerc.ac.uk/collection/P03/current/B005/>,
        <http://vocab.nerc.ac.uk/collection/P03/current/B070/> ;
    owl:deprecated "false" .
<http://vocab.nerc.ac.uk/collection/P02/current/BATT/> a glbase:MeasurementType,
        owl:Class,
        owl:NamedIndividual ;
    rdfs:label "Bacteria environmental parameters"@en ;
    dcterms:creator "SeaDataNet" ;
    dcterms:date "2003-06-10 13:53:19.0" ;
    glbase:hasIdentifier [ glbase:hasIdentifierScheme idscheme:sdn ;
            glbase:hasIdentifierValue "SDN:P02::BATT" ] ;
    rdfs:comment "" ;
    rdfs:subClassOf <http://vocab.nerc.ac.uk/collection/P03/current/B005/> ;
    owl:deprecated "false" .
<http://vocab.nerc.ac.uk/collection/P02/current/BATX/> a glbase:MeasurementType,
        owl:Class,
        owl:NamedIndividual ;
    rdfs:label "Bacteria taxonomic abundance in water bodies"@en ;
    dcterms:creator "SeaDataNet" ;
    dcterms:date "2010-10-22 10:06:41.0" ;
    glbase:hasIdentifier [ glbase:hasIdentifierScheme idscheme:sdn ;
            glbase:hasIdentifierValue "SDN:P02::BATX" ] ;
    rdfs:comment "Any enumeration of bacteria (Kingdom Monera so includes cyanobacteria) designated by taxonomic names (e.g. species, genus, family) in any body of fresh or salt water."@en ;
    rdfs:subClassOf <http://vocab.nerc.ac.uk/collection/P03/current/B005/>,
        <http://vocab.nerc.ac.uk/collection/P03/current/B070/> ;
    owl:deprecated "false" .
<http://vocab.nerc.ac.uk/collection/P02/current/BAUC/> a glbase:MeasurementType,
        owl:Class,
        owl:NamedIndividual ;
    rdfs:label "Bacteria taxonomic abundance in sediment"@en ;
    dcterms:creator "SeaDataNet" ;
    dcterms:date "2010-10-22 10:06:41.0" ;
    glbase:hasIdentifier [ glbase:hasIdentifierScheme idscheme:sdn ;
            glbase:hasIdentifierValue "SDN:P02::BAUC" ] ;
    rdfs:comment "Any enumeration of bacteria (Kingdom Monera so includes cyanobacteria) designated by taxonomic names (e.g. species, genus, family) in any soil or sediment."@en ;
    rdfs:subClassOf <http://vocab.nerc.ac.uk/collection/P03/current/B005/>,
        <http://vocab.nerc.ac.uk/collection/P03/current/B070/> ;
    owl:deprecated "false" .
<http://vocab.nerc.ac.uk/collection/P02/current/BCAH/> a glbase:MeasurementType,
        owl:Class,
        owl:NamedIndividual ;
    rdfs:label "Concentration of polycyclic aromatic hydrocarbons (PAHs) in biota"@en ;
    dcterms:creator "SeaDataNet" ;
    dcterms:date "2004-04-30 09:21:00.0" ;
    glbase:hasIdentifier [ glbase:hasIdentifierScheme idscheme:sdn ;
            glbase:hasIdentifierValue "SDN:P02::BCAH" ] ;
    rdfs:comment "PAH concentrations in either whole organisms or their constituent parts"@en ;
    rdfs:subClassOf <http://vocab.nerc.ac.uk/collection/P03/current/B007/>,
        <http://vocab.nerc.ac.uk/collection/P03/current/C025/>,
        <http://vocab.nerc.ac.uk/collection/P03/current/C055/>,
        <http://vocab.nerc.ac.uk/collection/P03/current/H001/> ;
    owl:deprecated "false" .
<http://vocab.nerc.ac.uk/collection/P02/current/BCMT/> a glbase:MeasurementType,
        owl:Class,
        owl:NamedIndividual ;
    rdfs:label "Metal concentrations in biota"@en ;
    dcterms:creator "SeaDataNet" ;
    dcterms:date "2008-09-12 09:34:02.0" ;
    glbase:hasIdentifier [ glbase:hasIdentifierScheme idscheme:sdn ;
            glbase:hasIdentifierValue "SDN:P02::BCMT" ] ;
    rdfs:comment "Metal concentrations in either whole organisms or their constituent parts."@en ;
    rdfs:subClassOf <http://vocab.nerc.ac.uk/collection/P03/current/B007/>,
        <http://vocab.nerc.ac.uk/collection/P03/current/C035/>,
        <http://vocab.nerc.ac.uk/collection/P03/current/H001/> ;
    owl:deprecated "false" .
<http://vocab.nerc.ac.uk/collection/P02/current/BCOC/> a glbase:MeasurementType,
        owl:Class,
        owl:NamedIndividual ;
    rdfs:label "Concentration of other organic contaminants in biota"@en ;
    dcterms:creator "SeaDataNet" ;
    dcterms:date "2010-01-27 11:43:34.0" ;
    glbase:hasIdentifier [ glbase:hasIdentifierScheme idscheme:sdn ;
            glbase:hasIdentifierValue "SDN:P02::BCOC" ] ;
    rdfs:comment "Concentration parameters for carbon compounds regarded as environmentally harmful in either whole organisms or their constituent parts that are not included in other categories"@en ;
    rdfs:subClassOf <http://vocab.nerc.ac.uk/collection/P03/current/B007/>,
        <http://vocab.nerc.ac.uk/collection/P03/current/C055/>,
        <http://vocab.nerc.ac.uk/collection/P03/current/H001/> ;
    owl:deprecated "false" .
<http://vocab.nerc.ac.uk/collection/P02/current/BCOS/> a glbase:MeasurementType,
        owl:Class,
        owl:NamedIndividual ;
    rdfs:label "Concentration of other substances in biota"@en ;
    dcterms:creator "SeaDataNet" ;
    dcterms:date "2004-04-30 09:20:00.0" ;
    glbase:hasIdentifier [ glbase:hasIdentifierScheme idscheme:sdn ;
            glbase:hasIdentifierValue "SDN:P02::BCOS" ] ;
    rdfs:comment "'Other'  (than metals or organic contaminants) substance concentrations in either whole organisms or their constituent parts.  This is a 'bucket' grouping that may be reclassified as the dictionary developes."@en ;
    rdfs:subClassOf <http://vocab.nerc.ac.uk/collection/P03/current/B007/> ;
    owl:deprecated "false" .
<http://vocab.nerc.ac.uk/collection/P02/current/BCPB/> a glbase:MeasurementType,
        owl:Class,
        owl:NamedIndividual ;
    rdfs:label "Concentration of polychlorobiphenyls (PCBs) in biota"@en ;
    dcterms:creator "SeaDataNet" ;
    dcterms:date "2004-04-30 09:20:00.0" ;
    glbase:hasIdentifier [ glbase:hasIdentifierScheme idscheme:sdn ;
            glbase:hasIdentifierValue "SDN:P02::BCPB" ] ;
    rdfs:comment "PCB concentrations in either whole organisms or their constituent parts"@en ;
    rdfs:subClassOf <http://vocab.nerc.ac.uk/collection/P03/current/B007/>,
        <http://vocab.nerc.ac.uk/collection/P03/current/C055/>,
        <http://vocab.nerc.ac.uk/collection/P03/current/H001/> ;
    owl:deprecated "false" .
<http://vocab.nerc.ac.uk/collection/P02/current/BDRV/> a glbase:MeasurementType,
        owl:Class,
        owl:NamedIndividual ;
    rdfs:label "Biodiversity indices"@en ;
    dcterms:creator "SeaDataNet" ;
    dcterms:date "2011-07-26 08:59:48.0" ;
    glbase:hasIdentifier [ glbase:hasIdentifierScheme idscheme:sdn ;
            glbase:hasIdentifierValue "SDN:P02::BDRV" ] ;
    rdfs:comment "Parameters describing the variety of entity types encountered in a population of living organisms"@en ;
    rdfs:subClassOf <http://vocab.nerc.ac.uk/collection/P03/current/B070/> ;
    owl:deprecated "false" .
<http://vocab.nerc.ac.uk/collection/P02/current/BDWC/> a glbase:MeasurementType,
        owl:Class,
        owl:NamedIndividual ;
    rdfs:label "Bacteria taxonomy-related ash-free dry weight biomass in sediment"@en ;
    dcterms:creator "SeaDataNet" ;
    dcterms:date "2004-10-22 12:04:00.0" ;
    glbase:hasIdentifier [ glbase:hasIdentifierScheme idscheme:sdn ;
            glbase:hasIdentifierValue "SDN:P02::BDWC" ] ;
    rdfs:comment "Bacteria ash-free dry weight biomass in sediment parameters presented at the level of taxa that may be mapped to entities in the ITIS taxonomy.  The taxa may be at any taxonomic level from sub-species upwards.  Bacteria are defined as all taxa that fall into Kingdom Monera in the ITIS taxonomy, which includes cyanobacteria."@en ;
    rdfs:subClassOf <http://vocab.nerc.ac.uk/collection/P03/current/B005/>,
        <http://vocab.nerc.ac.uk/collection/P03/current/B070/> ;
    owl:deprecated "false" .
<http://vocab.nerc.ac.uk/collection/P02/current/BEPP/> a glbase:MeasurementType,
        owl:Class,
        owl:NamedIndividual ;
    rdfs:label "Benthic primary production"@en ;
    dcterms:creator "SeaDataNet" ;
    dcterms:date "2015-02-03 10:19:46.0" ;
    glbase:hasIdentifier [ glbase:hasIdentifierScheme idscheme:sdn ;
            glbase:hasIdentifierValue "SDN:P02::BEPP" ] ;
    rdfs:comment "Parameters associated with the quantification of primary production by plants living on (e.g. corals, seaweed and seagrass) or in (e.g. benthic diatoms) the seabed.  Primary production is defined as the fixation of carbon dioxide into either organic or inorganic carbon by living entities and so includes photosynthesis and calcification."@en ;
    rdfs:subClassOf <http://vocab.nerc.ac.uk/collection/P03/current/B030/>,
        <http://vocab.nerc.ac.uk/collection/P03/current/B055/>,
        <http://vocab.nerc.ac.uk/collection/P03/current/O010/> ;
    owl:deprecated "false" .
<http://vocab.nerc.ac.uk/collection/P02/current/BEST/> a glbase:MeasurementType,
        owl:Class,
        owl:NamedIndividual ;
    rdfs:label "Sediment resuspension"@en ;
    dcterms:creator "SeaDataNet" ;
    dcterms:date "2004-08-17 13:57:45.0" ;
    glbase:hasIdentifier [ glbase:hasIdentifierScheme idscheme:sdn ;
            glbase:hasIdentifierValue "SDN:P02::BEST" ] ;
    rdfs:comment "Parameters quantifying the critera for and extent of sediment resuspension"@en ;
    rdfs:subClassOf <http://vocab.nerc.ac.uk/collection/P03/current/G060/> ;
    owl:deprecated "false" .
<http://vocab.nerc.ac.uk/collection/P02/current/BLEN/> a glbase:MeasurementType,
        owl:Class,
        owl:NamedIndividual ;
    rdfs:label "Zooplankton and zoobenthos morphological parameters"@en ;
    dcterms:creator "SeaDataNet" ;
    dcterms:date "2006-09-29 17:06:50.0" ;
    glbase:hasIdentifier [ glbase:hasIdentifierScheme idscheme:sdn ;
            glbase:hasIdentifierValue "SDN:P02::BLEN" ] ;
    rdfs:comment "Morphological parameters of zooplankton and zoobenthos (essentially any animal except for insects, earthworms or fish), such as size, shape and weight.  Benthic and planktonic animals have not been seggregated because there is a degree of overlap (eg shrimps)."@en ;
    rdfs:subClassOf <http://vocab.nerc.ac.uk/collection/P03/current/B027/>,
        <http://vocab.nerc.ac.uk/collection/P03/current/B045/> ;
    owl:deprecated "false" .
<http://vocab.nerc.ac.uk/collection/P02/current/BLUM/> a glbase:MeasurementType,
        owl:Class,
        owl:NamedIndividual ;
    rdfs:label "Bioluminescence parameters"@en ;
    dcterms:creator "SeaDataNet" ;
    dcterms:date "2007-09-24 16:17:57.0" ;
    glbase:hasIdentifier [ glbase:hasIdentifierScheme idscheme:sdn ;
            glbase:hasIdentifierValue "SDN:P02::BLUM" ] ;
    rdfs:comment "Parameters describing the nature and intensity of light generated by biological activity in the water column."@en ;
    rdfs:subClassOf <http://vocab.nerc.ac.uk/collection/P03/current/B027/>,
        <http://vocab.nerc.ac.uk/collection/P03/current/D015/> ;
    owl:deprecated "false" .
<http://vocab.nerc.ac.uk/collection/P02/current/BNTC/> a glbase:MeasurementType,
        owl:Class,
        owl:NamedIndividual ;
    rdfs:label "Bacteria non taxonomy-related biomass expressed as carbon per unit volume of the water column"@en ;
    dcterms:creator "SeaDataNet" ;
    dcterms:date "2004-04-14 11:15:00.0" ;
    glbase:hasIdentifier [ glbase:hasIdentifierScheme idscheme:sdn ;
            glbase:hasIdentifierValue "SDN:P02::BNTC" ] ;
    rdfs:comment "Basically any bacteria carbon biomass parameters that aren't included in parameter group BATC because they cannot be mapped to specific taxa in the ITIS taxonomy.  Bacteria are defined as Kingdom Monera, which includes cyanobacteria."@en ;
    rdfs:subClassOf <http://vocab.nerc.ac.uk/collection/P03/current/B005/>,
        <http://vocab.nerc.ac.uk/collection/P03/current/B070/> ;
    owl:deprecated "false" .
<http://vocab.nerc.ac.uk/collection/P02/current/BNTX/> a glbase:MeasurementType,
        owl:Class,
        owl:NamedIndividual ;
    rdfs:label "Bacteria generic abundance in water bodies"@en ;
    dcterms:creator "SeaDataNet" ;
    dcterms:date "2010-10-22 10:06:41.0" ;
    glbase:hasIdentifier [ glbase:hasIdentifierScheme idscheme:sdn ;
            glbase:hasIdentifierValue "SDN:P02::BNTX" ] ;
    rdfs:comment "Any enumeration of bacteria (Kingdom Monera so includes cyanobacteria) designated by terms other than taxonomic names (e.g. total) in any body of fresh or salt water."@en ;
    rdfs:subClassOf <http://vocab.nerc.ac.uk/collection/P03/current/B005/>,
        <http://vocab.nerc.ac.uk/collection/P03/current/B070/> ;
    owl:deprecated "false" .
<http://vocab.nerc.ac.uk/collection/P02/current/BNUC/> a glbase:MeasurementType,
        owl:Class,
        owl:NamedIndividual ;
    rdfs:label "Bacteria generic abundance in sediment"@en ;
    dcterms:creator "SeaDataNet" ;
    dcterms:date "2010-10-22 10:06:41.0" ;
    glbase:hasIdentifier [ glbase:hasIdentifierScheme idscheme:sdn ;
            glbase:hasIdentifierValue "SDN:P02::BNUC" ] ;
    rdfs:comment "Any enumeration of bacteria (Kingdom Monera so includes cyanobacteria) designated by terms other than taxonomic names (e.g. total) in any soil or sediment."@en ;
    rdfs:subClassOf <http://vocab.nerc.ac.uk/collection/P03/current/B005/>,
        <http://vocab.nerc.ac.uk/collection/P03/current/B070/> ;
    owl:deprecated "false" .
<http://vocab.nerc.ac.uk/collection/P02/current/BPBP/> a glbase:MeasurementType,
        owl:Class,
        owl:NamedIndividual ;
    rdfs:label "Bacteria non taxonomy-related biomass expressed as protein per unit volume of the water column"@en ;
    dcterms:creator "SeaDataNet" ;
    dcterms:date "2003-06-10 13:53:19.0" ;
    glbase:hasIdentifier [ glbase:hasIdentifierScheme idscheme:sdn ;
            glbase:hasIdentifierValue "SDN:P02::BPBP" ] ;
    rdfs:comment "" ;
    rdfs:subClassOf <http://vocab.nerc.ac.uk/collection/P03/current/B005/>,
        <http://vocab.nerc.ac.uk/collection/P03/current/B070/> ;
    owl:deprecated "false" .
<http://vocab.nerc.ac.uk/collection/P02/current/BPRP/> a glbase:MeasurementType,
        owl:Class,
        owl:NamedIndividual ;
    rdfs:label "Biota properties"@en ;
    dcterms:creator "SeaDataNet" ;
    dcterms:date "2013-11-20 09:50:48.0" ;
    glbase:hasIdentifier [ glbase:hasIdentifierScheme idscheme:sdn ;
            glbase:hasIdentifierValue "SDN:P02::BPRP" ] ;
    rdfs:comment "Parameters that quantify any attribute of an unspecified biological entity and therefore do not map to the biologically classified P02 categories. This concept was created deprecated as a fix."@en ;
    rdfs:subClassOf <http://vocab.nerc.ac.uk/collection/P03/current/B027/> ;
    owl:deprecated "false" .
<http://vocab.nerc.ac.uk/collection/P02/current/BRAD/> a glbase:MeasurementType,
        owl:Class,
        owl:NamedIndividual ;
    rdfs:label "Radioactivity in biota"@en ;
    dcterms:creator "SeaDataNet" ;
    dcterms:date "2007-02-26 08:05:24.0" ;
    glbase:hasIdentifier [ glbase:hasIdentifierScheme idscheme:sdn ;
            glbase:hasIdentifierValue "SDN:P02::BRAD" ] ;
    rdfs:comment "All parameters associated with radioactivity in either whole organisms or their constituent parts"@en ;
    rdfs:subClassOf <http://vocab.nerc.ac.uk/collection/P03/current/B007/>,
        <http://vocab.nerc.ac.uk/collection/P03/current/C030/> ;
    owl:deprecated "false" .
<http://vocab.nerc.ac.uk/collection/P02/current/BRDA/> a glbase:MeasurementType,
        owl:Class,
        owl:NamedIndividual ;
    rdfs:label "Bird counts"@en ;
    dcterms:creator "SeaDataNet" ;
    dcterms:date "2014-03-26 09:14:08.0" ;
    glbase:hasIdentifier [ glbase:hasIdentifierScheme idscheme:sdn ;
            glbase:hasIdentifierValue "SDN:P02::BRDA" ] ;
    rdfs:comment "Parameters quantifying the number of birds (Class Aves) in a survey but not expressed per unit area. Includes presence/absence indicators."@en ;
    rdfs:subClassOf <http://vocab.nerc.ac.uk/collection/P03/current/B015/> ;
    owl:deprecated "false" .
<http://vocab.nerc.ac.uk/collection/P02/current/BRDD/> a glbase:MeasurementType,
        owl:Class,
        owl:NamedIndividual ;
    rdfs:label "Bird taxonomy-related abundance per unit area of surface"@en ;
    dcterms:creator "SeaDataNet" ;
    dcterms:date "2005-09-23 10:41:38.0" ;
    glbase:hasIdentifier [ glbase:hasIdentifierScheme idscheme:sdn ;
            glbase:hasIdentifierValue "SDN:P02::BRDD" ] ;
    rdfs:comment "Bird (Class Aves) abundance per unit area (of land or sea) presented at the level of taxa that may be mapped to entities in the ITIS taxonomy.These may be at any taxonomic level from sub-species upwards."@en ;
    rdfs:subClassOf <http://vocab.nerc.ac.uk/collection/P03/current/B015/>,
        <http://vocab.nerc.ac.uk/collection/P03/current/B070/> ;
    owl:deprecated "false" .
<http://vocab.nerc.ac.uk/collection/P02/current/CA11/> a glbase:MeasurementType,
        owl:Class,
        owl:NamedIndividual ;
    rdfs:label "Concentration of alkanols (alcohols), phenols and ethers in sediment"@en ;
    dcterms:creator "SeaDataNet" ;
    dcterms:date "2011-02-24 16:52:36.0" ;
    glbase:hasIdentifier [ glbase:hasIdentifierScheme idscheme:sdn ;
            glbase:hasIdentifierValue "SDN:P02::CA11" ] ;
    rdfs:comment "Concentration of alkanols, phenols and ethers per unit mass or unit volume of sediment (material collected by a corer including fluff)"@en ;
    rdfs:subClassOf <http://vocab.nerc.ac.uk/collection/P02/current/CASD/> ;
    owl:deprecated "true" .
<http://vocab.nerc.ac.uk/collection/P02/current/CAKN/> a glbase:MeasurementType,
        owl:Class,
        owl:NamedIndividual ;
    rdfs:label "Concentration of alkenones and alkenoates in the water column"@en ;
    dcterms:creator "SeaDataNet" ;
    dcterms:date "2012-03-01 16:12:48.0" ;
    glbase:hasIdentifier [ glbase:hasIdentifierScheme idscheme:sdn ;
            glbase:hasIdentifierValue "SDN:P02::CAKN" ] ;
    rdfs:comment "Concentrations of alkenones (unsaturated aliphatic ketones) and alkenoates (carboxylic acid esters) in all phases of the water column."@en ;
    rdfs:subClassOf <http://vocab.nerc.ac.uk/collection/P03/current/C050/> ;
    owl:deprecated "false" .
<http://vocab.nerc.ac.uk/collection/P02/current/CAPH/> a glbase:MeasurementType,
        owl:Class,
        owl:NamedIndividual ;
    rdfs:label "Air pressure"@en ;
    dcterms:creator "SeaDataNet" ;
    dcterms:date "2007-02-23 15:09:47.0" ;
    glbase:hasIdentifier [ glbase:hasIdentifierScheme idscheme:sdn ;
            glbase:hasIdentifierValue "SDN:P02::CAPH" ] ;
    rdfs:comment "Measurements of air pressure as the dependent variable (ie excluding air pressure measured to specify the z co-ordinate of a balloon or sonde), including derived parameters such as tendency (rate of change) and related parameters such as air density."@en ;
    rdfs:subClassOf <http://vocab.nerc.ac.uk/collection/P03/current/M010/> ;
    owl:deprecated "false" .
<http://vocab.nerc.ac.uk/collection/P02/current/CARO/> a glbase:MeasurementType,
        owl:Class,
        owl:NamedIndividual ;
    rdfs:label "Carotenoid and flavenoid pigment concentrations in water bodies"@en ;
    dcterms:creator "SeaDataNet" ;
    dcterms:date "2015-09-08 09:02:34.0" ;
    glbase:hasIdentifier [ glbase:hasIdentifierScheme idscheme:sdn ;
            glbase:hasIdentifierValue "SDN:P02::CARO" ] ;
    rdfs:comment "" ;
    rdfs:subClassOf <http://vocab.nerc.ac.uk/collection/P03/current/B035/> ;
    owl:deprecated "false" .
<http://vocab.nerc.ac.uk/collection/P02/current/CARS/> a glbase:MeasurementType,
        owl:Class,
        owl:NamedIndividual ;
    rdfs:label "Carotenoid pigment concentrations in sediment"@en ;
    dcterms:creator "SeaDataNet" ;
    dcterms:date "2004-07-07 16:05:00.0" ;
    glbase:hasIdentifier [ glbase:hasIdentifierScheme idscheme:sdn ;
            glbase:hasIdentifierValue "SDN:P02::CARS" ] ;
    rdfs:comment "Sediment includes anything collected by a grab or corer, including the fluff layer from the top of the consolidated sediment"@en ;
    rdfs:subClassOf <http://vocab.nerc.ac.uk/collection/P03/current/B035/>,
        <http://vocab.nerc.ac.uk/collection/P03/current/G035/> ;
    owl:deprecated "false" .
<http://vocab.nerc.ac.uk/collection/P02/current/CATX/> a glbase:MeasurementType,
        owl:Class,
        owl:NamedIndividual ;
    rdfs:label "Phytoplankton taxonomic biomass in water bodies"@en ;
    dcterms:creator "SeaDataNet" ;
    dcterms:date "2010-10-21 13:41:28.0" ;
    glbase:hasIdentifier [ glbase:hasIdentifierScheme idscheme:sdn ;
            glbase:hasIdentifierValue "SDN:P02::CATX" ] ;
    rdfs:comment "Any parameterisation of biomass (e.g. wet weight, dry weight, carbon, nitrogen etc.) of free-floating autotrophic biological entities identified by their taxonomic names (e.g. family, genus, species) in any body of fresh or salt water."@en ;
    rdfs:subClassOf <http://vocab.nerc.ac.uk/collection/P03/current/B030/>,
        <http://vocab.nerc.ac.uk/collection/P03/current/B070/> ;
    owl:deprecated "false" .
<http://vocab.nerc.ac.uk/collection/P02/current/CBCC/> a glbase:MeasurementType,
        owl:Class,
        owl:NamedIndividual ;
    rdfs:label "Bacteria morphology and physiology"@en ;
    dcterms:creator "SeaDataNet" ;
    dcterms:date "2004-04-14 11:56:10.0" ;
    glbase:hasIdentifier [ glbase:hasIdentifierScheme idscheme:sdn ;
            glbase:hasIdentifierValue "SDN:P02::CBCC" ] ;
    rdfs:comment "Parameters describing the size, shape or physiological activity of bacteria, defined as Kingdom Monera (includes cyanobacteria).  Includes parameters both parameters mapped to taxa and those mapped to non-taxonomic groupings."@en ;
    rdfs:subClassOf <http://vocab.nerc.ac.uk/collection/P03/current/B005/> ;
    owl:deprecated "false" .
<http://vocab.nerc.ac.uk/collection/P02/current/CBFX/> a glbase:MeasurementType,
        owl:Class,
        owl:NamedIndividual ;
    rdfs:label "Sedimentation flux of carbohydates in the water column"@en ;
    dcterms:creator "SeaDataNet" ;
    dcterms:date "2004-10-22 12:10:00.0" ;
    glbase:hasIdentifier [ glbase:hasIdentifierScheme idscheme:sdn ;
            glbase:hasIdentifierValue "SDN:P02::CBFX" ] ;
    rdfs:comment "" ;
    rdfs:subClassOf <http://vocab.nerc.ac.uk/collection/P03/current/O005/> ;
    owl:deprecated "false" .
<http://vocab.nerc.ac.uk/collection/P02/current/CBSD/> a glbase:MeasurementType,
        owl:Class,
        owl:NamedIndividual ;
    rdfs:label "Carbon concentrations in sediment"@en ;
    dcterms:creator "SeaDataNet" ;
    dcterms:date "2006-06-13 09:21:23.0" ;
    glbase:hasIdentifier [ glbase:hasIdentifierScheme idscheme:sdn ;
            glbase:hasIdentifierValue "SDN:P02::CBSD" ] ;
    rdfs:comment "Concentrations of total, organic and inorganic carbon per unit weight of sediment.  Sediment is understood to be the solid phase of the bed, including the recently settled material sometimes known as fluff collected from the bed surface."@en ;
    rdfs:subClassOf <http://vocab.nerc.ac.uk/collection/P03/current/C005/>,
        <http://vocab.nerc.ac.uk/collection/P03/current/G035/> ;
    owl:deprecated "false" .
<http://vocab.nerc.ac.uk/collection/P02/current/CBSP/> a glbase:MeasurementType,
        owl:Class,
        owl:NamedIndividual ;
    rdfs:label "Carbon concentrations in suspended particulate material"@en ;
    dcterms:creator "SeaDataNet" ;
    dcterms:date "2006-05-26 14:55:39.0" ;
    glbase:hasIdentifier [ glbase:hasIdentifierScheme idscheme:sdn ;
            glbase:hasIdentifierValue "SDN:P02::CBSP" ] ;
    rdfs:comment "Concentrations of total, organic and inorganic carbon per unit weight of suspended particulate material collected by water column filtration, centrifugation or sediment trapping."@en ;
    rdfs:subClassOf <http://vocab.nerc.ac.uk/collection/P03/current/C005/>,
        <http://vocab.nerc.ac.uk/collection/P03/current/G015/> ;
    owl:deprecated "false" .
<http://vocab.nerc.ac.uk/collection/P02/current/CCPW/> a glbase:MeasurementType,
        owl:Class,
        owl:NamedIndividual ;
    rdfs:label "Dissolved inorganic carbon in sediment pore waters"@en ;
    dcterms:creator "SeaDataNet" ;
    dcterms:date "2013-11-19 12:24:46.0" ;
    glbase:hasIdentifier [ glbase:hasIdentifierScheme idscheme:sdn ;
            glbase:hasIdentifierValue "SDN:P02::CCPW" ] ;
    rdfs:comment "Carbonate system parameters (DIC/TCO2, pH, alkalinity, pCO2) in sediment pore waters"@en ;
    rdfs:subClassOf <http://vocab.nerc.ac.uk/collection/P03/current/C010/>,
        <http://vocab.nerc.ac.uk/collection/P03/current/G050/> ;
    owl:deprecated "false" .
<http://vocab.nerc.ac.uk/collection/P02/current/CD10/> a glbase:MeasurementType,
        owl:Class,
        owl:NamedIndividual ;
    rdfs:label "Sediment lipid concentrations"@en ;
    dcterms:creator "SeaDataNet" ;
    dcterms:date "2012-03-01 16:10:50.0" ;
    glbase:hasIdentifier [ glbase:hasIdentifierScheme idscheme:sdn ;
            glbase:hasIdentifierValue "SDN:P02::CD10" ] ;
    rdfs:comment "Lipids are defined as small water-insoluble biomolecules including fats, fatty acids, esters, sterols, isoprenoid compounds, etc..  Sediment is defined as material collected by a corer (including fluff)."@en ;
    rdfs:subClassOf <http://vocab.nerc.ac.uk/collection/P03/current/G035/> ;
    owl:deprecated "false" .
<http://vocab.nerc.ac.uk/collection/P02/current/CDRU/> a glbase:MeasurementType,
        owl:Class,
        owl:NamedIndividual ;
    rdfs:label "Metal uptake rates in the water column"@en ;
    dcterms:creator "SeaDataNet" ;
    dcterms:date "2004-07-29 10:47:18.0" ;
    glbase:hasIdentifier [ glbase:hasIdentifierScheme idscheme:sdn ;
            glbase:hasIdentifierValue "SDN:P02::CDRU" ] ;
    rdfs:comment "Parameters relating to the uptake rates of metals from the dissolved phase into the particulate phase"@en ;
    rdfs:subClassOf <http://vocab.nerc.ac.uk/collection/P03/current/O010/> ;
    owl:deprecated "false" .
<http://vocab.nerc.ac.uk/collection/P02/current/CDTA/> a glbase:MeasurementType,
        owl:Class,
        owl:NamedIndividual ;
    rdfs:label "Air temperature"@en ;
    dcterms:creator "SeaDataNet" ;
    dcterms:date "2008-11-04 13:00:56.0" ;
    glbase:hasIdentifier [ glbase:hasIdentifierScheme idscheme:sdn ;
            glbase:hasIdentifierValue "SDN:P02::CDTA" ] ;
    rdfs:comment "Parameters quantifying the degree of hotness of the atmosphere.  Specifically excludes indirect measurements of other parameters such as wet bulb temperatures."@en ;
    rdfs:subClassOf <http://vocab.nerc.ac.uk/collection/P03/current/M010/> ;
    owl:deprecated "false" .
<http://vocab.nerc.ac.uk/collection/P02/current/CEBH/> a glbase:MeasurementType,
        owl:Class,
        owl:NamedIndividual ;
    rdfs:label "Cetacean behaviour"@en ;
    dcterms:creator "SeaDataNet" ;
    dcterms:date "2008-01-30 07:53:20.0" ;
    glbase:hasIdentifier [ glbase:hasIdentifierScheme idscheme:sdn ;
            glbase:hasIdentifierValue "SDN:P02::CEBH" ] ;
    rdfs:comment "Parameters describing the actions or reactions of cetaceans (Order Cetacea), usually in response to the environment. Includes both parameters mapped to taxa and those mapped to non-taxonomic groupings."@en ;
    rdfs:subClassOf <http://vocab.nerc.ac.uk/collection/P03/current/B015/> ;
    owl:deprecated "false" .
<http://vocab.nerc.ac.uk/collection/P02/current/CEMO/> a glbase:MeasurementType,
        owl:Class,
        owl:NamedIndividual ;
    rdfs:label "Cetacean mortality"@en ;
    dcterms:creator "SeaDataNet" ;
    dcterms:date "2008-02-04 15:04:16.0" ;
    glbase:hasIdentifier [ glbase:hasIdentifierScheme idscheme:sdn ;
            glbase:hasIdentifierValue "SDN:P02::CEMO" ] ;
    rdfs:comment "Parameters describing the causes and rate of mortality in cetaceans (Order Cetacea). Includes both parameters mapped to taxa and those mapped to non-taxonomic groupings."@en ;
    rdfs:subClassOf <http://vocab.nerc.ac.uk/collection/P03/current/B015/> ;
    owl:deprecated "false" .
<http://vocab.nerc.ac.uk/collection/P02/current/CEMP/> a glbase:MeasurementType,
        owl:Class,
        owl:NamedIndividual ;
    rdfs:label "Cetacean morphology and physiology"@en ;
    dcterms:creator "SeaDataNet" ;
    dcterms:date "2008-01-30 07:53:20.0" ;
    glbase:hasIdentifier [ glbase:hasIdentifierScheme idscheme:sdn ;
            glbase:hasIdentifierValue "SDN:P02::CEMP" ] ;
    rdfs:comment "Parameters describing the size, shape or physiological activity including disease and parasite infection status of cetaceans (Order Cetacea). Includes both parameters mapped to taxa and those mapped to non-taxonomic groupings."@en ;
    rdfs:subClassOf <http://vocab.nerc.ac.uk/collection/P03/current/B015/> ;
    owl:deprecated "false" .
<http://vocab.nerc.ac.uk/collection/P02/current/CETA/> a glbase:MeasurementType,
        owl:Class,
        owl:NamedIndividual ;
    rdfs:label "Cetacean abundance"@en ;
    dcterms:creator "SeaDataNet" ;
    dcterms:date "2010-06-16 15:28:49.0" ;
    glbase:hasIdentifier [ glbase:hasIdentifierScheme idscheme:sdn ;
            glbase:hasIdentifierValue "SDN:P02::CETA" ] ;
    rdfs:comment "Parameters that specify the number of specified members of Order Cetacea present at a particular time and location, including presence/absence indicators."@en ;
    rdfs:subClassOf <http://vocab.nerc.ac.uk/collection/P03/current/B015/> ;
    owl:deprecated "false" .
<http://vocab.nerc.ac.uk/collection/P02/current/CFTM/> a glbase:MeasurementType,
        owl:Class,
        owl:NamedIndividual ;
    rdfs:label "Contaminant fluxes between the terrestrial and marine environment"@en ;
    dcterms:creator "SeaDataNet" ;
    dcterms:date "2008-12-09 10:17:11.0" ;
    glbase:hasIdentifier [ glbase:hasIdentifierScheme idscheme:sdn ;
            glbase:hasIdentifierValue "SDN:P02::CFTM" ] ;
    rdfs:comment "Parameters quanitifying the transfer of substances considered harmful from land to sea, including river discharge rates of contaminant species (but not freshwater discharge rates)."@en ;
    rdfs:subClassOf <http://vocab.nerc.ac.uk/collection/P03/current/H001/>,
        <http://vocab.nerc.ac.uk/collection/P03/current/O005/> ;
    owl:deprecated "false" .
<http://vocab.nerc.ac.uk/collection/P02/current/CHEX/> a glbase:MeasurementType,
        owl:Class,
        owl:NamedIndividual ;
    rdfs:label "Cloud cover height and extent"@en ;
    dcterms:creator "SeaDataNet" ;
    dcterms:date "2004-08-20 11:25:47.0" ;
    glbase:hasIdentifier [ glbase:hasIdentifierScheme idscheme:sdn ;
            glbase:hasIdentifierValue "SDN:P02::CHEX" ] ;
    rdfs:comment "Parameters describing the horizontal and vertical extent of cloud cover"@en ;
    rdfs:subClassOf <http://vocab.nerc.ac.uk/collection/P03/current/M010/> ;
    owl:deprecated "false" .
<http://vocab.nerc.ac.uk/collection/P02/current/CHUM/> a glbase:MeasurementType,
        owl:Class,
        owl:NamedIndividual ;
    rdfs:label "Atmospheric humidity"@en ;
    dcterms:creator "SeaDataNet" ;
    dcterms:date "2004-08-18 09:51:46.0" ;
    glbase:hasIdentifier [ glbase:hasIdentifierScheme idscheme:sdn ;
            glbase:hasIdentifierValue "SDN:P02::CHUM" ] ;
    rdfs:comment "Parameters that either quantify the water content of moist air or are specifically used in its determination (eg wet bulb air temperature)"@en ;
    rdfs:subClassOf <http://vocab.nerc.ac.uk/collection/P03/current/M010/> ;
    owl:deprecated "false" .
<http://vocab.nerc.ac.uk/collection/P02/current/CING/> a glbase:MeasurementType,
        owl:Class,
        owl:NamedIndividual ;
    rdfs:label "Particulate inorganic carbon concentrations in the water column"@en ;
    dcterms:creator "SeaDataNet" ;
    dcterms:date "2003-06-10 13:53:19.0" ;
    glbase:hasIdentifier [ glbase:hasIdentifierScheme idscheme:sdn ;
            glbase:hasIdentifierValue "SDN:P02::CING" ] ;
    rdfs:comment "Concentrations of inorganic carbon in the particulate phase of the water column as extracted by a fitration technique.  This is the particle-bound concentration per unit volume of the water column. Consequently, it is both a function of the SPM concentration in the water column and the concentration of inorganic carbon per unit weight of the SPM."@en ;
    rdfs:subClassOf <http://vocab.nerc.ac.uk/collection/P03/current/C005/> ;
    owl:deprecated "false" .
<http://vocab.nerc.ac.uk/collection/P02/current/CLAY/> a glbase:MeasurementType,
        owl:Class,
        owl:NamedIndividual ;
    rdfs:label "Mineralogical composition"@en ;
    dcterms:creator "SeaDataNet" ;
    dcterms:date "2010-10-01 09:16:22.0" ;
    glbase:hasIdentifier [ glbase:hasIdentifierScheme idscheme:sdn ;
            glbase:hasIdentifierValue "SDN:P02::CLAY" ] ;
    rdfs:comment "Parameters describing or quantifying the mineralogical composition of rocks and unlithified sediments."@en ;
    rdfs:subClassOf <http://vocab.nerc.ac.uk/collection/P03/current/G045/> ;
    owl:deprecated "false" .
<http://vocab.nerc.ac.uk/collection/P02/current/CLCN/> a glbase:MeasurementType,
        owl:Class,
        owl:NamedIndividual ;
    rdfs:label "Concentration of inorganic halogens in sediment"@en ;
    dcterms:creator "SeaDataNet" ;
    dcterms:date "2010-11-05 11:54:45.0" ;
    glbase:hasIdentifier [ glbase:hasIdentifierScheme idscheme:sdn ;
            glbase:hasIdentifierValue "SDN:P02::CLCN" ] ;
    rdfs:comment "Concentrations of halogens as elements or simple inorganic compounds (eg iodate) in sediments (anything collected by a corer including fluff"@en ;
    rdfs:subClassOf <http://vocab.nerc.ac.uk/collection/P02/current/RMIN/> ;
    owl:deprecated "true" .
<http://vocab.nerc.ac.uk/collection/P02/current/CLTY/> a glbase:MeasurementType,
        owl:Class,
        owl:NamedIndividual ;
    rdfs:label "Cloud type"@en ;
    dcterms:creator "SeaDataNet" ;
    dcterms:date "2009-10-12 15:31:31.0" ;
    glbase:hasIdentifier [ glbase:hasIdentifierScheme idscheme:sdn ;
            glbase:hasIdentifierValue "SDN:P02::CLTY" ] ;
    rdfs:comment "Parameters that classify cloud cover into types such as cumulus and cirrus."@en ;
    rdfs:subClassOf <http://vocab.nerc.ac.uk/collection/P03/current/M010/> ;
    owl:deprecated "false" .
<http://vocab.nerc.ac.uk/collection/P02/current/CLXX/> a glbase:MeasurementType,
        owl:Class,
        owl:NamedIndividual ;
    rdfs:label "Concentration of inorganic halogens in sediment pore waters"@en ;
    dcterms:creator "SeaDataNet" ;
    dcterms:date "2010-07-02 09:42:02.0" ;
    glbase:hasIdentifier [ glbase:hasIdentifierScheme idscheme:sdn ;
            glbase:hasIdentifierValue "SDN:P02::CLXX" ] ;
    rdfs:comment "Concentrations of halogens as elements or their inorganic compounds in all phases of sediment pore water"@en ;
    rdfs:subClassOf <http://vocab.nerc.ac.uk/collection/P03/current/C045/> ;
    owl:deprecated "false" .
<http://vocab.nerc.ac.uk/collection/P02/current/CMFL/> a glbase:MeasurementType,
        owl:Class,
        owl:NamedIndividual ;
    rdfs:label "Variable fluorescence parameters"@en ;
    dcterms:creator "SeaDataNet" ;
    dcterms:date "2005-02-03 11:20:50.0" ;
    glbase:hasIdentifier [ glbase:hasIdentifierScheme idscheme:sdn ;
            glbase:hasIdentifierValue "SDN:P02::CMFL" ] ;
    rdfs:comment "Parameters measured by variable fluorescence instruments such as pump and probe and fast repetition rate fluorometers"@en ;
    rdfs:subClassOf <http://vocab.nerc.ac.uk/collection/P03/current/O010/> ;
    owl:deprecated "false" .
<http://vocab.nerc.ac.uk/collection/P02/current/CNDC/> a glbase:MeasurementType,
        owl:Class,
        owl:NamedIndividual ;
    rdfs:label "Electrical conductivity of the water column"@en ;
    dcterms:creator "SeaDataNet" ;
    dcterms:date "2007-03-02 11:40:14.0" ;
    glbase:hasIdentifier [ glbase:hasIdentifierScheme idscheme:sdn ;
            glbase:hasIdentifierValue "SDN:P02::CNDC" ] ;
    rdfs:comment "Parameters quantifying the flow of electrical current through or the electrical resistance of a body of water at any point between the bed and the atmosphere"@en ;
    rdfs:subClassOf <http://vocab.nerc.ac.uk/collection/P03/current/D025/> ;
    owl:deprecated "false" .
<http://vocab.nerc.ac.uk/collection/P02/current/CNTX/> a glbase:MeasurementType,
        owl:Class,
        owl:NamedIndividual ;
    rdfs:label "Phytoplankton generic biomass in water bodies"@en ;
    dcterms:creator "SeaDataNet" ;
    dcterms:date "2010-10-21 13:43:45.0" ;
    glbase:hasIdentifier [ glbase:hasIdentifierScheme idscheme:sdn ;
            glbase:hasIdentifierValue "SDN:P02::CNTX" ] ;
    rdfs:comment "Any parameterisation of biomass (e.g. wet weight, dry weight, carbon, nitrogen etc.) of free-floating autotrophic biological entities designated by terms other than taxonomic names (e.g. microphytoplankton, ciliate, flagellate) in any body of fresh or salt water."@en ;
    rdfs:subClassOf <http://vocab.nerc.ac.uk/collection/P03/current/B030/>,
        <http://vocab.nerc.ac.uk/collection/P03/current/B070/> ;
    owl:deprecated "false" .
<http://vocab.nerc.ac.uk/collection/P02/current/COAS/> a glbase:MeasurementType,
        owl:Class,
        owl:NamedIndividual ;
    rdfs:label "Terrestrial mapping"@en ;
    dcterms:creator "SeaDataNet" ;
    dcterms:date "2006-05-26 14:47:05.0" ;
    glbase:hasIdentifier [ glbase:hasIdentifierScheme idscheme:sdn ;
            glbase:hasIdentifierValue "SDN:P02::COAS" ] ;
    rdfs:comment "Parameters relating to the mapping of terrestrial features, including coastlines"@en ;
    rdfs:subClassOf <http://vocab.nerc.ac.uk/collection/P03/current/T001/> ;
    owl:deprecated "false" .
<http://vocab.nerc.ac.uk/collection/P02/current/COCC/> a glbase:MeasurementType,
        owl:Class,
        owl:NamedIndividual ;
    rdfs:label "Colloidal organic carbon concentration in the water column"@en ;
    dcterms:creator "SeaDataNet" ;
    dcterms:date "2004-08-02 11:30:00.0" ;
    glbase:hasIdentifier [ glbase:hasIdentifierScheme idscheme:sdn ;
            glbase:hasIdentifierValue "SDN:P02::COCC" ] ;
    rdfs:comment "Colloidal organic carbon per unit volume of the water column."@en ;
    rdfs:subClassOf <http://vocab.nerc.ac.uk/collection/P03/current/C005/> ;
    owl:deprecated "false" .
<http://vocab.nerc.ac.uk/collection/P02/current/COGE/> a glbase:MeasurementType,
        owl:Class,
        owl:NamedIndividual ;
    rdfs:label "Coastal geomorphology"@en ;
    dcterms:creator "SeaDataNet" ;
    dcterms:date "2007-02-26 08:22:53.0" ;
    glbase:hasIdentifier [ glbase:hasIdentifierScheme idscheme:sdn ;
            glbase:hasIdentifierValue "SDN:P02::COGE" ] ;
    rdfs:comment "All parameters associated with coastal landforms such as beaches and dunes including morphology, evolution and associated transport phenomena"@en ;
    rdfs:subClassOf <http://vocab.nerc.ac.uk/collection/P03/current/T001/> ;
    owl:deprecated "false" .
<http://vocab.nerc.ac.uk/collection/P02/current/CORG/> a glbase:MeasurementType,
        owl:Class,
        owl:NamedIndividual ;
    rdfs:label "Particulate total and organic carbon concentrations in the water column"@en ;
    dcterms:creator "SeaDataNet" ;
    dcterms:date "2003-06-10 13:53:19.0" ;
    glbase:hasIdentifier [ glbase:hasIdentifierScheme idscheme:sdn ;
            glbase:hasIdentifierValue "SDN:P02::CORG" ] ;
    rdfs:comment "Concentrations of total and organic carbon in the particulate phase of the water column as extracted by a filtration technique. This is the particle-bound concentration per unit volume of the water column and is both a function of the SPM concentration in the water column and the concentration of carbon per unit weight of SPM.  Total and organic carbon are classed together to circumvent confusion caused by total carbon data sets labelled 'POC' on the assumption that the inorganic carbon fraction is negligible"@en ;
    rdfs:subClassOf <http://vocab.nerc.ac.uk/collection/P03/current/C005/> ;
    owl:deprecated "false" .
<http://vocab.nerc.ac.uk/collection/P02/current/CPCN/> a glbase:MeasurementType,
        owl:Class,
        owl:NamedIndividual ;
    rdfs:label "Unclassified pigment concentrations in sediment"@en ;
    dcterms:creator "SeaDataNet" ;
    dcterms:date "2004-10-22 11:43:33.0" ;
    glbase:hasIdentifier [ glbase:hasIdentifierScheme idscheme:sdn ;
            glbase:hasIdentifierValue "SDN:P02::CPCN" ] ;
    rdfs:comment "Includes all pigments that cannot be explicitly classified as chlorophylls, phaeopigments or carotenoids (usually groups of pigments). Sediment includes anything collected by a grab or corer, including the fluff layer from the top of the consolidated sediment."@en ;
    rdfs:subClassOf <http://vocab.nerc.ac.uk/collection/P03/current/B035/>,
        <http://vocab.nerc.ac.uk/collection/P03/current/G035/> ;
    owl:deprecated "false" .
<http://vocab.nerc.ac.uk/collection/P02/current/CPRP/> a glbase:MeasurementType,
        owl:Class,
        owl:NamedIndividual ;
    rdfs:label "Precipitation and evaporation"@en ;
    dcterms:creator "SeaDataNet" ;
    dcterms:date "2006-06-13 14:28:34.0" ;
    glbase:hasIdentifier [ glbase:hasIdentifierScheme idscheme:sdn ;
            glbase:hasIdentifierValue "SDN:P02::CPRP" ] ;
    rdfs:comment "Parameters relating to all kinds of precipitation (rain, snow, etc.) and water loss from the surface of the Earth"@en ;
    rdfs:subClassOf <http://vocab.nerc.ac.uk/collection/P03/current/M010/> ;
    owl:deprecated "false" .
<http://vocab.nerc.ac.uk/collection/P02/current/CPSD/> a glbase:MeasurementType,
        owl:Class,
        owl:NamedIndividual ;
    rdfs:label "Chlorophyll pigment concentrations in sediment"@en ;
    dcterms:creator "SeaDataNet" ;
    dcterms:date "2004-06-30 13:25:00.0" ;
    glbase:hasIdentifier [ glbase:hasIdentifierScheme idscheme:sdn ;
            glbase:hasIdentifierValue "SDN:P02::CPSD" ] ;
    rdfs:comment "Includes all variants of chlorophyll.  Sediment includes anything collected by a grab or corer, including the fluff layer from the top of the consolidated sediment"@en ;
    rdfs:subClassOf <http://vocab.nerc.ac.uk/collection/P03/current/B035/>,
        <http://vocab.nerc.ac.uk/collection/P03/current/G035/> ;
    owl:deprecated "false" .
<http://vocab.nerc.ac.uk/collection/P02/current/CPWC/> a glbase:MeasurementType,
        owl:Class,
        owl:NamedIndividual ;
    rdfs:label "Chlorophyll pigment concentrations in water bodies"@en ;
    dcterms:creator "SeaDataNet" ;
    dcterms:date "2015-11-16 11:57:22.0" ;
    glbase:hasIdentifier [ glbase:hasIdentifierScheme idscheme:sdn ;
            glbase:hasIdentifierValue "SDN:P02::CPWC" ] ;
    rdfs:comment """Includes all variants of chlorophyll expressed in terms of per unit volume, 
per unit area of any body of fresh or salt water, or as a relative colour index (e.g. PCI). 
Does not include data expressed per unit mass of SPM."""@en ;
    rdfs:subClassOf <http://vocab.nerc.ac.uk/collection/P03/current/B035/> ;
    owl:deprecated "false" .
<http://vocab.nerc.ac.uk/collection/P02/current/CRYS/> a glbase:MeasurementType,
        owl:Class,
        owl:NamedIndividual ;
    rdfs:label "Snow and ice mass, thickness and extent"@en ;
    dcterms:creator "SeaDataNet" ;
    dcterms:date "2011-02-18 11:01:12.0" ;
    glbase:hasIdentifier [ glbase:hasIdentifierScheme idscheme:sdn ;
            glbase:hasIdentifierValue "SDN:P02::CRYS" ] ;
    rdfs:comment "Measurements of quantity (mass), thickness and spatial extent of snow and ice"@en ;
    rdfs:subClassOf <http://vocab.nerc.ac.uk/collection/P03/current/M015/> ;
    owl:deprecated "false" .
<http://vocab.nerc.ac.uk/collection/P02/current/CSDE/> a glbase:MeasurementType,
        owl:Class,
        owl:NamedIndividual ;
    rdfs:label "Organic sulphur compound dynamics in the water column"@en ;
    dcterms:creator "SeaDataNet" ;
    dcterms:date "2004-07-29 10:58:32.0" ;
    glbase:hasIdentifier [ glbase:hasIdentifierScheme idscheme:sdn ;
            glbase:hasIdentifierValue "SDN:P02::CSDE" ] ;
    rdfs:comment "Parameters relating to the rates of creation and consumption of organic sulphur compounds (such as DMS and carbonyl sulphide) in the water column"@en ;
    rdfs:subClassOf <http://vocab.nerc.ac.uk/collection/P03/current/O010/> ;
    owl:deprecated "false" .
<http://vocab.nerc.ac.uk/collection/P02/current/CSLR/> a glbase:MeasurementType,
        owl:Class,
        owl:NamedIndividual ;
    rdfs:label "Solar Radiation"@en ;
    dcterms:creator "SeaDataNet" ;
    dcterms:date "2008-11-04 13:04:58.0" ;
    glbase:hasIdentifier [ glbase:hasIdentifierScheme idscheme:sdn ;
            glbase:hasIdentifierValue "SDN:P02::CSLR" ] ;
    rdfs:comment "Parameters quantifying the irradiance of the sun impinging on the Earth's surface in the visible and infra-red waveband, generally accepted as wavelengths between 300 and 3000 nm"@en ;
    rdfs:subClassOf <http://vocab.nerc.ac.uk/collection/P03/current/M010/> ;
    owl:deprecated "false" .
<http://vocab.nerc.ac.uk/collection/P02/current/CXAA/> a glbase:MeasurementType,
        owl:Class,
        owl:NamedIndividual ;
    rdfs:label "Concentrations of carboxylic acids and carboxylates in the atmosphere"@en ;
    dcterms:creator "SeaDataNet" ;
    dcterms:date "2008-12-09 10:17:11.0" ;
    glbase:hasIdentifier [ glbase:hasIdentifierScheme idscheme:sdn ;
            glbase:hasIdentifierValue "SDN:P02::CXAA" ] ;
    rdfs:comment "Parameters quantifying the concentration of acids containing a carboxyl (-C(=O)OH) group, their anions or their salts in any phase of the atmosphere"@en ;
    rdfs:subClassOf <http://vocab.nerc.ac.uk/collection/P03/current/M005/> ;
    owl:deprecated "false" .
<http://vocab.nerc.ac.uk/collection/P02/current/CYEU/> a glbase:MeasurementType,
        owl:Class,
        owl:NamedIndividual ;
    rdfs:label "Plankton biomass expressed as carbon per unit volume of the water column"@en ;
    dcterms:creator "SeaDataNet" ;
    dcterms:date "2003-08-04 15:26:48.0" ;
    glbase:hasIdentifier [ glbase:hasIdentifierScheme idscheme:sdn ;
            glbase:hasIdentifierValue "SDN:P02::CYEU" ] ;
    rdfs:comment "Used for plankton carbon biomass parameters where no differentiation between phytoplankton, microzooplankton or zooplankton is possible"@en ;
    rdfs:subClassOf <http://vocab.nerc.ac.uk/collection/P03/current/B070/> ;
    owl:deprecated "false" .
<http://vocab.nerc.ac.uk/collection/P02/current/D000/> a glbase:MeasurementType,
        owl:Class,
        owl:NamedIndividual ;
    rdfs:label "Diatom taxonomy-related abundance per unit mass of sediment"@en ;
    dcterms:creator "SeaDataNet" ;
    dcterms:date "2003-11-24 08:07:56.0" ;
    glbase:hasIdentifier [ glbase:hasIdentifierScheme idscheme:sdn ;
            glbase:hasIdentifierValue "SDN:P02::D000" ] ;
    rdfs:comment "Determinations of the abundance of diatom remains in sediment linked to taxonomic identifications that may be mapped to entities in the ITIS taxonomy.  These may be at any taxonomic level from sub-species upwards"@en ;
    rdfs:subClassOf <http://vocab.nerc.ac.uk/collection/P03/current/B030/>,
        <http://vocab.nerc.ac.uk/collection/P03/current/B070/> ;
    owl:deprecated "false" .
<http://vocab.nerc.ac.uk/collection/P02/current/DAAW/> a glbase:MeasurementType,
        owl:Class,
        owl:NamedIndividual ;
    rdfs:label "Particulate amino acid concentrations in the water column"@en ;
    dcterms:creator "SeaDataNet" ;
    dcterms:date "2008-12-09 11:09:48.0" ;
    glbase:hasIdentifier [ glbase:hasIdentifierScheme idscheme:sdn ;
            glbase:hasIdentifierValue "SDN:P02::DAAW" ] ;
    rdfs:comment "Parameters quantifying the amount of organic compounds containing both a carboxyl group and an amino group in solids suspended in a body of water."@en ;
    rdfs:subClassOf <http://vocab.nerc.ac.uk/collection/P03/current/C003/> ;
    owl:deprecated "false" .
<http://vocab.nerc.ac.uk/collection/P02/current/DALK/> a glbase:MeasurementType,
        owl:Class,
        owl:NamedIndividual ;
    rdfs:label "Concentration of alkanes in the water column"@en ;
    dcterms:creator "SeaDataNet" ;
    dcterms:date "2004-06-18 15:36:00.0" ;
    glbase:hasIdentifier [ glbase:hasIdentifierScheme idscheme:sdn ;
            glbase:hasIdentifierValue "SDN:P02::DALK" ] ;
    rdfs:comment "Alkane concentration parameters (including saturation of gaseous species) in all phases of the water column.  Does not include parameters expressed per unit weight of SPM."@en ;
    rdfs:subClassOf <http://vocab.nerc.ac.uk/collection/P03/current/C025/> ;
    owl:deprecated "false" .
<http://vocab.nerc.ac.uk/collection/P02/current/DBDX/> a glbase:MeasurementType,
        owl:Class,
        owl:NamedIndividual ;
    rdfs:label "Geological sample density"@en ;
    dcterms:creator "SeaDataNet" ;
    dcterms:date "2010-11-04 11:16:05.0" ;
    glbase:hasIdentifier [ glbase:hasIdentifierScheme idscheme:sdn ;
            glbase:hasIdentifierValue "SDN:P02::DBDX" ] ;
    rdfs:comment "Parameters that describe the the mass per unit volume of any samples of rock or unlithified sediment."@en ;
    rdfs:subClassOf <http://vocab.nerc.ac.uk/collection/P03/current/G040/> ;
    owl:deprecated "false" .
<http://vocab.nerc.ac.uk/collection/P02/current/DCMX/> a glbase:MeasurementType,
        owl:Class,
        owl:NamedIndividual ;
    rdfs:label "Other halocarbon concentrations in water bodies"@en ;
    dcterms:creator "SeaDataNet" ;
    dcterms:date "2010-11-08 15:08:09.0" ;
    glbase:hasIdentifier [ glbase:hasIdentifierScheme idscheme:sdn ;
            glbase:hasIdentifierValue "SDN:P02::DCMX" ] ;
    rdfs:comment "Concentrations of volatile halocarbons (compounds comprising carbon atoms covalently bonded to fluorine, chlorine, bromine or iodine atoms) other than tracers (i.e. freons/chlorofluorocarbons) and contaminants in any body of fresh or salt water."@en ;
    rdfs:subClassOf <http://vocab.nerc.ac.uk/collection/P03/current/C020/> ;
    owl:deprecated "false" .
<http://vocab.nerc.ac.uk/collection/P02/current/DENS/> a glbase:MeasurementType,
        owl:Class,
        owl:NamedIndividual ;
    rdfs:label "Other physical and chemical properties of suspended particulate material"@en ;
    dcterms:creator "SeaDataNet" ;
    dcterms:date "2004-10-26 14:42:51.0" ;
    glbase:hasIdentifier [ glbase:hasIdentifierScheme idscheme:sdn ;
            glbase:hasIdentifierValue "SDN:P02::DENS" ] ;
    rdfs:comment "Parameters that do not easily fit into any of the other SPM data categories."@en ;
    rdfs:subClassOf <http://vocab.nerc.ac.uk/collection/P03/current/G015/> ;
    owl:deprecated "false" .
<http://vocab.nerc.ac.uk/collection/P02/current/DGPW/> a glbase:MeasurementType,
        owl:Class,
        owl:NamedIndividual ;
    rdfs:label "Dissolved oxygen concentration parameters in sediment pore waters"@en ;
    dcterms:creator "SeaDataNet" ;
    dcterms:date "2004-08-11 15:34:43.0" ;
    glbase:hasIdentifier [ glbase:hasIdentifierScheme idscheme:sdn ;
            glbase:hasIdentifierValue "SDN:P02::DGPW" ] ;
    rdfs:comment "All concentration parameters (including saturation) for dissolved oxygen in sediment pore waters"@en ;
    rdfs:subClassOf <http://vocab.nerc.ac.uk/collection/P03/current/C015/>,
        <http://vocab.nerc.ac.uk/collection/P03/current/G050/> ;
    owl:deprecated "false" .
<http://vocab.nerc.ac.uk/collection/P02/current/DMST/> a glbase:MeasurementType,
        owl:Class,
        owl:NamedIndividual ;
    rdfs:label "Organosulphur and organoselenium species concentration parameters in water bodies"@en ;
    dcterms:creator "SeaDataNet" ;
    dcterms:date "2015-11-16 12:05:19.0" ;
    glbase:hasIdentifier [ glbase:hasIdentifierScheme idscheme:sdn ;
            glbase:hasIdentifierValue "SDN:P02::DMST" ] ;
    rdfs:comment """All organosulphur and organoselenium compound concentration parameters (including saturations for gaseous species) 
in all phases of any body of fresh or salt water."""@en ;
    rdfs:subClassOf <http://vocab.nerc.ac.uk/collection/P03/current/C050/> ;
    owl:deprecated "false" .
<http://vocab.nerc.ac.uk/collection/P02/current/DOCC/> a glbase:MeasurementType,
        owl:Class,
        owl:NamedIndividual ;
    rdfs:label "Dissolved organic carbon concentration in the water column"@en ;
    dcterms:creator "SeaDataNet" ;
    dcterms:date "2004-05-19 17:10:00.0" ;
    glbase:hasIdentifier [ glbase:hasIdentifierScheme idscheme:sdn ;
            glbase:hasIdentifierValue "SDN:P02::DOCC" ] ;
    rdfs:comment "DOC per unit volume of the water column.  Note that this includes some parameters that are strictly defined as total carbon, because the water was unfiltered on the assumption that POC was negligible."@en ;
    rdfs:subClassOf <http://vocab.nerc.ac.uk/collection/P03/current/C005/> ;
    owl:deprecated "false" .
<http://vocab.nerc.ac.uk/collection/P02/current/DOCU/> a glbase:MeasurementType,
        owl:Class,
        owl:NamedIndividual ;
    rdfs:label "Dissolved organic carbon uptake and production in the water column"@en ;
    dcterms:creator "SeaDataNet" ;
    dcterms:date "2004-08-19 10:46:22.0" ;
    glbase:hasIdentifier [ glbase:hasIdentifierScheme idscheme:sdn ;
            glbase:hasIdentifierValue "SDN:P02::DOCU" ] ;
    rdfs:comment "Any parameter relating to the rate of DOC concentration change in the water column"@en ;
    rdfs:subClassOf <http://vocab.nerc.ac.uk/collection/P03/current/O010/> ;
    owl:deprecated "false" .
<http://vocab.nerc.ac.uk/collection/P02/current/DPEV/> a glbase:MeasurementType,
        owl:Class,
        owl:NamedIndividual ;
    rdfs:label "Depositional environment"@en ;
    dcterms:creator "SeaDataNet" ;
    dcterms:date "2010-10-01 09:40:24.0" ;
    glbase:hasIdentifier [ glbase:hasIdentifierScheme idscheme:sdn ;
            glbase:hasIdentifierValue "SDN:P02::DPEV" ] ;
    rdfs:comment "Parameters characterising the environment in which sediments were deposited either by observation or interpretation of sedimentary rocks and unlithified sediments."@en ;
    rdfs:subClassOf <http://vocab.nerc.ac.uk/collection/P03/current/GSED/> ;
    owl:deprecated "false" .
<http://vocab.nerc.ac.uk/collection/P02/current/DSCO/> a glbase:MeasurementType,
        owl:Class,
        owl:NamedIndividual ;
    rdfs:label "Distribution coefficients in the water column"@en ;
    dcterms:creator "SeaDataNet" ;
    dcterms:date "2004-08-11 15:42:00.0" ;
    glbase:hasIdentifier [ glbase:hasIdentifierScheme idscheme:sdn ;
            glbase:hasIdentifierValue "SDN:P02::DSCO" ] ;
    rdfs:comment "Distribution coefficients of species between the dissolved and particulate phases of the water column"@en ;
    rdfs:subClassOf <http://vocab.nerc.ac.uk/collection/P03/current/C045/> ;
    owl:deprecated "false" .
<http://vocab.nerc.ac.uk/collection/P02/current/DVLP/> a glbase:MeasurementType,
        owl:Class,
        owl:NamedIndividual ;
    rdfs:label "Zooplankton and zoobenthos development stage parameters"@en ;
    dcterms:creator "SeaDataNet" ;
    dcterms:date "2009-07-28 12:23:25.0" ;
    glbase:hasIdentifier [ glbase:hasIdentifierScheme idscheme:sdn ;
            glbase:hasIdentifierValue "SDN:P02::DVLP" ] ;
    rdfs:comment "Development stage parameters (such as proportion but excluding abundance or biomass) of zooplankton and zoobenthos. Benthic and planktonic animals have not been seggregated because there is a degree of overlap (eg shrimps)."@en ;
    rdfs:subClassOf <http://vocab.nerc.ac.uk/collection/P03/current/B027/>,
        <http://vocab.nerc.ac.uk/collection/P03/current/B045/> ;
    owl:deprecated "false" .
<http://vocab.nerc.ac.uk/collection/P02/current/ENGP/> a glbase:MeasurementType,
        owl:Class,
        owl:NamedIndividual ;
    rdfs:label "Engineering parameters"@en ;
    dcterms:creator "SeaDataNet" ;
    dcterms:date "2005-08-31 09:41:37.0" ;
    glbase:hasIdentifier [ glbase:hasIdentifierScheme idscheme:sdn ;
            glbase:hasIdentifierValue "SDN:P02::ENGP" ] ;
    rdfs:comment "Technical parameters that provide information on how well an instrument or data acquisition system is working"@en ;
    rdfs:subClassOf <http://vocab.nerc.ac.uk/collection/P03/current/Z005/> ;
    owl:deprecated "false" .
<http://vocab.nerc.ac.uk/collection/P02/current/EPSI/> a glbase:MeasurementType,
        owl:Class,
        owl:NamedIndividual ;
    rdfs:label "Turbulence in the water column"@en ;
    dcterms:creator "SeaDataNet" ;
    dcterms:date "2004-08-16 11:46:33.0" ;
    glbase:hasIdentifier [ glbase:hasIdentifierScheme idscheme:sdn ;
            glbase:hasIdentifierValue "SDN:P02::EPSI" ] ;
    rdfs:comment "Measured parameters expressing turbulence in the water column plus parameters derived from these measurements"@en ;
    rdfs:subClassOf <http://vocab.nerc.ac.uk/collection/P03/current/D030/> ;
    owl:deprecated "false" .
<http://vocab.nerc.ac.uk/collection/P02/current/EWSB/> a glbase:MeasurementType,
        owl:Class,
        owl:NamedIndividual ;
    rdfs:label "Wind strength and direction"@en ;
    dcterms:creator "SeaDataNet" ;
    dcterms:date "2014-05-27 12:10:12.0" ;
    glbase:hasIdentifier [ glbase:hasIdentifierScheme idscheme:sdn ;
            glbase:hasIdentifierValue "SDN:P02::EWSB" ] ;
    rdfs:comment "Parameters quantifying the extent or direction of atmospheric movement. Obvious examples are wind velocity, windspeed and wind direction, but can also include derived parameters such as force, energy, power and power density."@en ;
    rdfs:subClassOf <http://vocab.nerc.ac.uk/collection/P03/current/M010/> ;
    owl:deprecated "false" .
<http://vocab.nerc.ac.uk/collection/P02/current/EXCO/> a glbase:MeasurementType,
        owl:Class,
        owl:NamedIndividual ;
    rdfs:label "Light extinction and diffusion coefficients"@en ;
    dcterms:creator "SeaDataNet" ;
    dcterms:date "2007-11-21 16:27:57.0" ;
    glbase:hasIdentifier [ glbase:hasIdentifierScheme idscheme:sdn ;
            glbase:hasIdentifierValue "SDN:P02::EXCO" ] ;
    rdfs:comment "Parameters relating to the extent of light penetration into the water column"@en ;
    rdfs:subClassOf <http://vocab.nerc.ac.uk/collection/P03/current/D015/> ;
    owl:deprecated "false" .
<http://vocab.nerc.ac.uk/collection/P02/current/EXCR/> a glbase:MeasurementType,
        owl:Class,
        owl:NamedIndividual ;
    rdfs:label "Excretion rate parameters in the water column"@en ;
    dcterms:creator "SeaDataNet" ;
    dcterms:date "2004-07-28 16:08:00.0" ;
    glbase:hasIdentifier [ glbase:hasIdentifierScheme idscheme:sdn ;
            glbase:hasIdentifierValue "SDN:P02::EXCR" ] ;
    rdfs:comment "Includes all parameters relating to all mechanisms of waste release except respiration."@en ;
    rdfs:subClassOf <http://vocab.nerc.ac.uk/collection/P03/current/B027/>,
        <http://vocab.nerc.ac.uk/collection/P03/current/O010/> ;
    owl:deprecated "false" .
<http://vocab.nerc.ac.uk/collection/P02/current/EXSV/> a glbase:MeasurementType,
        owl:Class,
        owl:NamedIndividual ;
    rdfs:label "Experiment state variables"@en ;
    dcterms:creator "SeaDataNet" ;
    dcterms:date "2014-10-08 09:56:52.0" ;
    glbase:hasIdentifier [ glbase:hasIdentifierScheme idscheme:sdn ;
            glbase:hasIdentifierValue "SDN:P02::EXSV" ] ;
    rdfs:comment "Measurements made at a given time of any state variable in a sample that is the subject of an experiment that will change the composition over time, such as the water sample in an incubation experiment."@en ;
    rdfs:subClassOf <http://vocab.nerc.ac.uk/collection/P03/current/Z005/> ;
    owl:deprecated "false" .
<http://vocab.nerc.ac.uk/collection/P02/current/EXUV/> a glbase:MeasurementType,
        owl:Class,
        owl:NamedIndividual ;
    rdfs:label "Biological detritus in the water column suspended particulate material"@en ;
    dcterms:creator "SeaDataNet" ;
    dcterms:date "2004-08-18 08:41:50.0" ;
    glbase:hasIdentifier [ glbase:hasIdentifierScheme idscheme:sdn ;
            glbase:hasIdentifierValue "SDN:P02::EXUV" ] ;
    rdfs:comment "Parameters quantifying and categorising biological detritus (eg exuvia and faecal pellets) in the water column that have been derived from the water column"@en ;
    rdfs:subClassOf <http://vocab.nerc.ac.uk/collection/P03/current/B027/>,
        <http://vocab.nerc.ac.uk/collection/P03/current/G015/> ;
    owl:deprecated "false" .
<http://vocab.nerc.ac.uk/collection/P02/current/F001/> a glbase:MeasurementType,
        owl:Class,
        owl:NamedIndividual ;
    rdfs:label "Water body lipid concentrations"@en ;
    dcterms:creator "SeaDataNet" ;
    dcterms:date "2012-03-01 16:10:50.0" ;
    glbase:hasIdentifier [ glbase:hasIdentifierScheme idscheme:sdn ;
            glbase:hasIdentifierValue "SDN:P02::F001" ] ;
    rdfs:comment "Lipids are defined as small water-insoluble biomolecules including fats, fatty acids, esters, sterols, isoprenoid compounds, etc..  Water body includes any body of fresh or salt water. As lipids are insoluble in water the concencentrations are associated with the particulate phase."@en ;
    rdfs:subClassOf <http://schema.geolink.org/1.0/voc/nvs/P03#SeaDataNetParameter> ;
    owl:deprecated "false" .
<http://vocab.nerc.ac.uk/collection/P02/current/FABD/> a glbase:MeasurementType,
        owl:Class,
        owl:NamedIndividual ;
    rdfs:label "Fauna abundance per unit area of the bed"@en ;
    dcterms:creator "SeaDataNet" ;
    dcterms:date "2005-09-23 10:46:34.0" ;
    glbase:hasIdentifier [ glbase:hasIdentifierScheme idscheme:sdn ;
            glbase:hasIdentifierValue "SDN:P02::FABD" ] ;
    rdfs:comment "Any fauna (class Animalia) abundance per unit are of sea, river or lake bed.  Broad group overlapping a number of more specific groups that should be used preferentially, but this group is provided as an alternative to one-to-many mappings."@en ;
    rdfs:subClassOf <http://vocab.nerc.ac.uk/collection/P03/current/B070/>,
        <http://vocab.nerc.ac.uk/collection/P03/current/G055/> ;
    owl:deprecated "false" .
<http://vocab.nerc.ac.uk/collection/P02/current/FATM/> a glbase:MeasurementType,
        owl:Class,
        owl:NamedIndividual ;
    rdfs:label "Fish morphology, age and physiology"@en ;
    dcterms:creator "SeaDataNet" ;
    dcterms:date "2010-07-30 11:57:26.0" ;
    glbase:hasIdentifier [ glbase:hasIdentifierScheme idscheme:sdn ;
            glbase:hasIdentifierValue "SDN:P02::FATM" ] ;
    rdfs:comment "Paramaters that quantify the size, shape, age and life processes (including mortality) of fish (Osteichthyes, Agnatha and Chrondrichthyes)."@en ;
    rdfs:subClassOf <http://vocab.nerc.ac.uk/collection/P03/current/B020/> ;
    owl:deprecated "false" .
<http://vocab.nerc.ac.uk/collection/P02/current/FATX/> a glbase:MeasurementType,
        owl:Class,
        owl:NamedIndividual ;
    rdfs:label "Fish abundance in water bodies"@en ;
    dcterms:creator "SeaDataNet" ;
    dcterms:date "2010-07-30 11:55:54.0" ;
    glbase:hasIdentifier [ glbase:hasIdentifierScheme idscheme:sdn ;
            glbase:hasIdentifierValue "SDN:P02::FATX" ] ;
    rdfs:comment "Paramaters that quantify the numbers of fish (Osteichthyes, Agnatha and Chrondrichthyes) at a given location in any body of salt or fresh water."@en ;
    rdfs:subClassOf <http://vocab.nerc.ac.uk/collection/P03/current/B020/>,
        <http://vocab.nerc.ac.uk/collection/P03/current/B070/> ;
    owl:deprecated "false" .
<http://vocab.nerc.ac.uk/collection/P02/current/FBAB/> a glbase:MeasurementType,
        owl:Class,
        owl:NamedIndividual ;
    rdfs:label "Fish taxonomy-related abundance per unit area of the bed"@en ;
    dcterms:creator "SeaDataNet" ;
    dcterms:date "2004-04-28 09:29:00.0" ;
    glbase:hasIdentifier [ glbase:hasIdentifierScheme idscheme:sdn ;
            glbase:hasIdentifierValue "SDN:P02::FBAB" ] ;
    rdfs:comment "Fish (Osteichthyes, Agnatha and Chondrichthyes) abundance per unit area of bed (sea, river, lake etc.) parameters presented at the level of taxa that may be mapped to entities in the ITIS taxonomy.  Includes animals normally considered as planktonic if they have been returned from sediment samples."@en ;
    rdfs:subClassOf <http://vocab.nerc.ac.uk/collection/P03/current/B020/>,
        <http://vocab.nerc.ac.uk/collection/P03/current/B070/>,
        <http://vocab.nerc.ac.uk/collection/P03/current/G055/> ;
    owl:deprecated "false" .
<http://vocab.nerc.ac.uk/collection/P02/current/FBAF/> a glbase:MeasurementType,
        owl:Class,
        owl:NamedIndividual ;
    rdfs:label "Fish taxonomy-related ash-free dry weight biomass per unit area of the bed"@en ;
    dcterms:creator "SeaDataNet" ;
    dcterms:date "2004-04-28 09:28:00.0" ;
    glbase:hasIdentifier [ glbase:hasIdentifierScheme idscheme:sdn ;
            glbase:hasIdentifierValue "SDN:P02::FBAF" ] ;
    rdfs:comment "Fish (Osteichthyes, Agnatha and Chondrichthyes) ash-free dry weight biomass per unit area of bed (sea, river, lake etc.) parameters presented at the level of taxa that may be mapped to entities in the ITIS taxonomy.  Includes animals normally considered as planktonic if they have been returned from sediment samples."@en ;
    rdfs:subClassOf <http://vocab.nerc.ac.uk/collection/P03/current/B020/>,
        <http://vocab.nerc.ac.uk/collection/P03/current/B070/>,
        <http://vocab.nerc.ac.uk/collection/P03/current/G055/> ;
    owl:deprecated "false" .
<http://vocab.nerc.ac.uk/collection/P02/current/FCNT/> a glbase:MeasurementType,
        owl:Class,
        owl:NamedIndividual ;
    rdfs:label "Fish taxonomy-related counts"@en ;
    dcterms:creator "SeaDataNet" ;
    dcterms:date "2008-11-19 15:32:58.0" ;
    glbase:hasIdentifier [ glbase:hasIdentifierScheme idscheme:sdn ;
            glbase:hasIdentifierValue "SDN:P02::FCNT" ] ;
    rdfs:comment "Fish (Osteichthyes, Agnatha and Chrondrichthyes) count parameters presented at the level of taxa that may be mapped to entities in the ITIS taxonomy.  These may be at any taxonomic level from sub-species upwards. Count includes presence/absence indicators."@en ;
    rdfs:subClassOf <http://vocab.nerc.ac.uk/collection/P03/current/B020/> ;
    owl:deprecated "false" .
<http://vocab.nerc.ac.uk/collection/P02/current/FCRT/> a glbase:MeasurementType,
        owl:Class,
        owl:NamedIndividual ;
    rdfs:label "Zooplankton feeding"@en ;
    dcterms:creator "SeaDataNet" ;
    dcterms:date "2007-03-02 11:26:48.0" ;
    glbase:hasIdentifier [ glbase:hasIdentifierScheme idscheme:sdn ;
            glbase:hasIdentifierValue "SDN:P02::FCRT" ] ;
    rdfs:comment "Parameters quantifying the ingestion of food by zooplankton (mesozooplankton and larger but excluding fish) in terms of identified biota or chemical species and the effects of nutrition on life processes such as physiology and reproduction."@en ;
    rdfs:subClassOf <http://vocab.nerc.ac.uk/collection/P03/current/B045/>,
        <http://vocab.nerc.ac.uk/collection/P03/current/O010/> ;
    owl:deprecated "false" .
<http://vocab.nerc.ac.uk/collection/P02/current/FCST/> a glbase:MeasurementType,
        owl:Class,
        owl:NamedIndividual ;
    rdfs:label "Fish and shellfish catch statistics"@en ;
    dcterms:creator "SeaDataNet" ;
    dcterms:date "2010-07-30 11:45:06.0" ;
    glbase:hasIdentifier [ glbase:hasIdentifierScheme idscheme:sdn ;
            glbase:hasIdentifierValue "SDN:P02::FCST" ] ;
    rdfs:comment "Parameters quantifying and describing biota take by fishing activities"@en ;
    rdfs:subClassOf <http://vocab.nerc.ac.uk/collection/P03/current/H004/> ;
    owl:deprecated "false" .
<http://vocab.nerc.ac.uk/collection/P02/current/FDMS/> a glbase:MeasurementType,
        owl:Class,
        owl:NamedIndividual ;
    rdfs:label "Gas fluxes between the water column and the atmosphere"@en ;
    dcterms:creator "SeaDataNet" ;
    dcterms:date "2004-08-19 09:25:41.0" ;
    glbase:hasIdentifier [ glbase:hasIdentifierScheme idscheme:sdn ;
            glbase:hasIdentifierValue "SDN:P02::FDMS" ] ;
    rdfs:comment "Fluxes of any gaseous species from water column to atmosphere"@en ;
    rdfs:subClassOf <http://vocab.nerc.ac.uk/collection/P03/current/M005/>,
        <http://vocab.nerc.ac.uk/collection/P03/current/O005/> ;
    owl:deprecated "false" .
<http://vocab.nerc.ac.uk/collection/P02/current/FEFF/> a glbase:MeasurementType,
        owl:Class,
        owl:NamedIndividual ;
    rdfs:label "Fishing effort"@en ;
    dcterms:creator "SeaDataNet" ;
    dcterms:date "2014-05-01 12:46:41.0" ;
    glbase:hasIdentifier [ glbase:hasIdentifierScheme idscheme:sdn ;
            glbase:hasIdentifierValue "SDN:P02::FEFF" ] ;
    rdfs:comment "Parameters that quantify or classify the physical or financial resources used in fishing activities"@en ;
    rdfs:subClassOf <http://vocab.nerc.ac.uk/collection/P03/current/H004/> ;
    owl:deprecated "false" .
<http://vocab.nerc.ac.uk/collection/P02/current/FIBM/> a glbase:MeasurementType,
        owl:Class,
        owl:NamedIndividual ;
    rdfs:label "Fish biomass in water bodies"@en ;
    dcterms:creator "SeaDataNet" ;
    dcterms:date "2010-05-04 08:19:31.0" ;
    glbase:hasIdentifier [ glbase:hasIdentifierScheme idscheme:sdn ;
            glbase:hasIdentifierValue "SDN:P02::FIBM" ] ;
    rdfs:comment "Parameters quantifying the mass of fish (Osteichthyes, Agnatha and Chrondrichthyes)in total or by species per unit area or per unit volume in any body of fresh or salt water expressed in any form (e.g. wet weight, dry weight, carbon, nitrogen, etc.)."@en ;
    rdfs:subClassOf <http://vocab.nerc.ac.uk/collection/P03/current/B020/>,
        <http://vocab.nerc.ac.uk/collection/P03/current/B070/>,
        <http://vocab.nerc.ac.uk/collection/P03/current/H004/> ;
    owl:deprecated "false" .
<http://vocab.nerc.ac.uk/collection/P02/current/FNTM/> a glbase:MeasurementType,
        owl:Class,
        owl:NamedIndividual ;
    rdfs:label "Fish non taxonomy-related morphology"@en ;
    dcterms:creator "SeaDataNet" ;
    dcterms:date "2008-11-19 15:32:58.0" ;
    glbase:hasIdentifier [ glbase:hasIdentifierScheme idscheme:sdn ;
            glbase:hasIdentifierValue "SDN:P02::FNTM" ] ;
    rdfs:comment "Fish (Osteichthyes, Agnatha and Chrondrichthyes) size and shape parameters not included under FATM.  Most commonly used for the generic term 'fish' that maps to multiple taxa."@en ;
    rdfs:subClassOf <http://vocab.nerc.ac.uk/collection/P03/current/B020/> ;
    owl:deprecated "false" .
<http://vocab.nerc.ac.uk/collection/P02/current/FNTX/> a glbase:MeasurementType,
        owl:Class,
        owl:NamedIndividual ;
    rdfs:label "Fish non taxonomy-related abundance per unit volume of the water column"@en ;
    dcterms:creator "SeaDataNet" ;
    dcterms:date "2008-11-19 15:32:58.0" ;
    glbase:hasIdentifier [ glbase:hasIdentifierScheme idscheme:sdn ;
            glbase:hasIdentifierValue "SDN:P02::FNTX" ] ;
    rdfs:comment "Fish (Osteichthyes, Agnatha and Chrondrichthyes) abundance per unit volume parameters not included under FATX.  Most commonly used for the generic term 'fish' that maps to multiple taxa."@en ;
    rdfs:subClassOf <http://vocab.nerc.ac.uk/collection/P03/current/B020/>,
        <http://vocab.nerc.ac.uk/collection/P03/current/B070/> ;
    owl:deprecated "false" .
<http://vocab.nerc.ac.uk/collection/P02/current/FOCA/> a glbase:MeasurementType,
        owl:Class,
        owl:NamedIndividual ;
    rdfs:label "Seal abundance"@en ;
    dcterms:creator "SeaDataNet" ;
    dcterms:date "2010-06-16 15:32:23.0" ;
    glbase:hasIdentifier [ glbase:hasIdentifierScheme idscheme:sdn ;
            glbase:hasIdentifierValue "SDN:P02::FOCA" ] ;
    rdfs:comment "Parameters that specify the number of specified members of Family Phocidae present at a particular time and location, including presence/absence indicators."@en ;
    rdfs:subClassOf <http://vocab.nerc.ac.uk/collection/P03/current/B015/> ;
    owl:deprecated "false" .
<http://vocab.nerc.ac.uk/collection/P02/current/FPFX/> a glbase:MeasurementType,
        owl:Class,
        owl:NamedIndividual ;
    rdfs:label "Sedimentation flux of biological detritus in the water column"@en ;
    dcterms:creator "SeaDataNet" ;
    dcterms:date "2004-08-18 12:22:09.0" ;
    glbase:hasIdentifier [ glbase:hasIdentifierScheme idscheme:sdn ;
            glbase:hasIdentifierValue "SDN:P02::FPFX" ] ;
    rdfs:comment "Flux of biological detritus (material derived from the water column such as exuvia and faecal pellets) in the water column"@en ;
    rdfs:subClassOf <http://vocab.nerc.ac.uk/collection/P03/current/B027/>,
        <http://vocab.nerc.ac.uk/collection/P03/current/O005/> ;
    owl:deprecated "false" .
<http://vocab.nerc.ac.uk/collection/P02/current/FPRT/> a glbase:MeasurementType,
        owl:Class,
        owl:NamedIndividual ;
    rdfs:label "Zooplankton defecation rates in the water column"@en ;
    dcterms:creator "SeaDataNet" ;
    dcterms:date "2007-03-30 08:16:12.0" ;
    glbase:hasIdentifier [ glbase:hasIdentifierScheme idscheme:sdn ;
            glbase:hasIdentifierValue "SDN:P02::FPRT" ] ;
    rdfs:comment "Faecal pellet production and gut evacuation rates"@en ;
    rdfs:subClassOf <http://vocab.nerc.ac.uk/collection/P03/current/B045/>,
        <http://vocab.nerc.ac.uk/collection/P03/current/O010/> ;
    owl:deprecated "false" .
<http://vocab.nerc.ac.uk/collection/P02/current/FR11/> a glbase:MeasurementType,
        owl:Class,
        owl:NamedIndividual ;
    rdfs:label "Chlorofluorocarbon concentrations in the water column"@en ;
    dcterms:creator "SeaDataNet" ;
    dcterms:date "2009-09-25 14:43:11.0" ;
    glbase:hasIdentifier [ glbase:hasIdentifierScheme idscheme:sdn ;
            glbase:hasIdentifierValue "SDN:P02::FR11" ] ;
    rdfs:comment "Concentrations of chlorofluorocarbons (also known as freons or CFCs) in sny body of water"@en ;
    rdfs:subClassOf <http://vocab.nerc.ac.uk/collection/P03/current/C020/> ;
    owl:deprecated "false" .
<http://vocab.nerc.ac.uk/collection/P02/current/FREP/> a glbase:MeasurementType,
        owl:Class,
        owl:NamedIndividual ;
    rdfs:label "Fish reproduction"@en ;
    dcterms:creator "SeaDataNet" ;
    dcterms:date "2010-07-30 12:03:03.0" ;
    glbase:hasIdentifier [ glbase:hasIdentifierScheme idscheme:sdn ;
            glbase:hasIdentifierValue "SDN:P02::FREP" ] ;
    rdfs:comment "Paramaters that quantify the fecundity, reproductive rates or nature of reproduction in fish (Osteichthyes, Agnatha and Chrondrichthyes)."@en ;
    rdfs:subClassOf <http://vocab.nerc.ac.uk/collection/P03/current/B020/>,
        <http://vocab.nerc.ac.uk/collection/P03/current/B027/>,
        <http://vocab.nerc.ac.uk/collection/P03/current/H004/> ;
    owl:deprecated "false" .
<http://vocab.nerc.ac.uk/collection/P02/current/FVLT/> a glbase:MeasurementType,
        owl:Class,
        owl:NamedIndividual ;
    rdfs:label "Raw fluorometer output"@en ;
    dcterms:creator "SeaDataNet" ;
    dcterms:date "2004-02-25 09:06:42.0" ;
    glbase:hasIdentifier [ glbase:hasIdentifierScheme idscheme:sdn ;
            glbase:hasIdentifierValue "SDN:P02::FVLT" ] ;
    rdfs:comment "Output as logged from any type fluorometer."@en ;
    rdfs:subClassOf <http://vocab.nerc.ac.uk/collection/P03/current/B035/> ;
    owl:deprecated "false" .
<http://vocab.nerc.ac.uk/collection/P02/current/GERA/> a glbase:MeasurementType,
        owl:Class,
        owl:NamedIndividual ;
    rdfs:label "Radiation geophysics"@en ;
    dcterms:creator "SeaDataNet" ;
    dcterms:date "2010-10-22 12:26:30.0" ;
    glbase:hasIdentifier [ glbase:hasIdentifierScheme idscheme:sdn ;
            glbase:hasIdentifierValue "SDN:P02::GERA" ] ;
    rdfs:comment "Parameters quantifying the level of radioactive emissions from in-situ geologic units"@en ;
    rdfs:subClassOf <http://vocab.nerc.ac.uk/collection/P03/current/GPYS/> ;
    owl:deprecated "false" .
<http://vocab.nerc.ac.uk/collection/P02/current/GHDX/> a glbase:MeasurementType,
        owl:Class,
        owl:NamedIndividual ;
    rdfs:label "Sediment microfossil morphology parameters"@en ;
    dcterms:creator "SeaDataNet" ;
    dcterms:date "2004-08-17 14:08:51.0" ;
    glbase:hasIdentifier [ glbase:hasIdentifierScheme idscheme:sdn ;
            glbase:hasIdentifierValue "SDN:P02::GHDX" ] ;
    rdfs:comment "Parameters relating to the size, shape and form of microfossils in sediment samples"@en ;
    rdfs:subClassOf <http://vocab.nerc.ac.uk/collection/P03/current/G055/> ;
    owl:deprecated "false" .
<http://vocab.nerc.ac.uk/collection/P02/current/GOXP/> a glbase:MeasurementType,
        owl:Class,
        owl:NamedIndividual ;
    rdfs:label "Oxygen production and respiration in the water column"@en ;
    dcterms:creator "SeaDataNet" ;
    dcterms:date "2004-07-29 11:28:06.0" ;
    glbase:hasIdentifier [ glbase:hasIdentifierScheme idscheme:sdn ;
            glbase:hasIdentifierValue "SDN:P02::GOXP" ] ;
    rdfs:comment "Parameters related to the rates of oxygen production and consumption"@en ;
    rdfs:subClassOf <http://vocab.nerc.ac.uk/collection/P02/current/DOXY/>,
        <http://vocab.nerc.ac.uk/collection/P03/current/O010/> ;
    owl:deprecated "false" .
<http://vocab.nerc.ac.uk/collection/P02/current/GP001/> a glbase:MeasurementType,
        owl:Class,
        owl:NamedIndividual ;
    rdfs:label "Pollution events"@en ;
    dcterms:creator "SeaDataNet" ;
    dcterms:date "2008-12-09 10:17:11.0" ;
    glbase:hasIdentifier [ glbase:hasIdentifierScheme idscheme:sdn ;
            glbase:hasIdentifierValue "SDN:P02::GP001" ] ;
    rdfs:comment "Parameters quantifying the accidental spillage of liquid or dry pollutants from vessels or marine industries. Parameters may include quantities of pollutant, areas affected and event duration."@en ;
    rdfs:subClassOf <http://vocab.nerc.ac.uk/collection/P03/current/H001/> ;
    owl:deprecated "false" .
<http://vocab.nerc.ac.uk/collection/P02/current/GP004/> a glbase:MeasurementType,
        owl:Class,
        owl:NamedIndividual ;
    rdfs:label "Bird reproduction"@en ;
    dcterms:creator "SeaDataNet" ;
    dcterms:date "2008-12-09 10:17:11.0" ;
    glbase:hasIdentifier [ glbase:hasIdentifierScheme idscheme:sdn ;
            glbase:hasIdentifierValue "SDN:P02::GP004" ] ;
    rdfs:comment "Parameters related to the reproduction of birds (Class Aves)"@en ;
    rdfs:subClassOf <http://vocab.nerc.ac.uk/collection/P03/current/B015/> ;
    owl:deprecated "false" .
<http://vocab.nerc.ac.uk/collection/P02/current/GP005/> a glbase:MeasurementType,
        owl:Class,
        owl:NamedIndividual ;
    rdfs:label "Fish disease and parasites"@en ;
    dcterms:creator "SeaDataNet" ;
    dcterms:date "2008-12-09 10:17:11.0" ;
    glbase:hasIdentifier [ glbase:hasIdentifierScheme idscheme:sdn ;
            glbase:hasIdentifierValue "SDN:P02::GP005" ] ;
    rdfs:comment "Parameters related to the infection of Fish (Osteichthyes, Agnatha and Chrondrichthyes) by parasites and disease. Includes visual assesements and analytical data."@en ;
    rdfs:subClassOf <http://vocab.nerc.ac.uk/collection/P03/current/B020/>,
        <http://vocab.nerc.ac.uk/collection/P03/current/B060/> ;
    owl:deprecated "false" .
<http://vocab.nerc.ac.uk/collection/P02/current/GP010/> a glbase:MeasurementType,
        owl:Class,
        owl:NamedIndividual ;
    rdfs:label "Bioassay and contaminant biological impact"@en ;
    dcterms:creator "SeaDataNet" ;
    dcterms:date "2008-12-09 10:17:11.0" ;
    glbase:hasIdentifier [ glbase:hasIdentifierScheme idscheme:sdn ;
            glbase:hasIdentifierValue "SDN:P02::GP010" ] ;
    rdfs:comment "Parameters describing the effects of substances on living organisms."@en ;
    rdfs:subClassOf <http://vocab.nerc.ac.uk/collection/P03/current/B060/> ;
    owl:deprecated "false" .
<http://vocab.nerc.ac.uk/collection/P02/current/GP012/> a glbase:MeasurementType,
        owl:Class,
        owl:NamedIndividual ;
    rdfs:label "Macroalgae and seagrass infection and damage"@en ;
    dcterms:creator "SeaDataNet" ;
    dcterms:date "2008-12-09 10:17:11.0" ;
    glbase:hasIdentifier [ glbase:hasIdentifierScheme idscheme:sdn ;
            glbase:hasIdentifierValue "SDN:P02::GP012" ] ;
    rdfs:comment "Parameters relating to diseases and parasites of macroalgae (Rhodophycota, Chromphycota, Chlorophycota)  and seagrass (Charophyta, Anthophyta) and damage to seagrass beds"@en ;
    rdfs:subClassOf <http://vocab.nerc.ac.uk/collection/P03/current/B055/>,
        <http://vocab.nerc.ac.uk/collection/P03/current/B060/> ;
    owl:deprecated "false" .
<http://vocab.nerc.ac.uk/collection/P02/current/GP018/> a glbase:MeasurementType,
        owl:Class,
        owl:NamedIndividual ;
    rdfs:label "Cetacean reproduction"@en ;
    dcterms:creator "SeaDataNet" ;
    dcterms:date "2008-12-09 10:17:11.0" ;
    glbase:hasIdentifier [ glbase:hasIdentifierScheme idscheme:sdn ;
            glbase:hasIdentifierValue "SDN:P02::GP018" ] ;
    rdfs:comment "Parameters related to the reproduction of cetaceans (Order Cetacea)"@en ;
    rdfs:subClassOf <http://vocab.nerc.ac.uk/collection/P03/current/B015/> ;
    owl:deprecated "false" .
<http://vocab.nerc.ac.uk/collection/P02/current/GP025/> a glbase:MeasurementType,
        owl:Class,
        owl:NamedIndividual ;
    rdfs:label "Seal reproduction"@en ;
    dcterms:creator "SeaDataNet" ;
    dcterms:date "2008-12-09 10:17:11.0" ;
    glbase:hasIdentifier [ glbase:hasIdentifierScheme idscheme:sdn ;
            glbase:hasIdentifierValue "SDN:P02::GP025" ] ;
    rdfs:comment "Parameters related to the reproduction of seals (Family Phocidae)"@en ;
    rdfs:subClassOf <http://vocab.nerc.ac.uk/collection/P03/current/B015/> ;
    owl:deprecated "false" .
<http://vocab.nerc.ac.uk/collection/P02/current/GP048/> a glbase:MeasurementType,
        owl:Class,
        owl:NamedIndividual ;
    rdfs:label "Concentration of polychlorobiphenyls (PCBs) in the atmosphere"@en ;
    dcterms:creator "SeaDataNet" ;
    dcterms:date "2008-12-09 10:17:11.0" ;
    glbase:hasIdentifier [ glbase:hasIdentifierScheme idscheme:sdn ;
            glbase:hasIdentifierValue "SDN:P02::GP048" ] ;
    rdfs:comment "Parameters quantifying polychlorobiphenyl (PCB) concentrations in all phases of the atmosphere"@en ;
    rdfs:subClassOf <http://vocab.nerc.ac.uk/collection/P03/current/H001/>,
        <http://vocab.nerc.ac.uk/collection/P03/current/M005/> ;
    owl:deprecated "false" .
<http://vocab.nerc.ac.uk/collection/P02/current/GP050/> a glbase:MeasurementType,
        owl:Class,
        owl:NamedIndividual ;
    rdfs:label "Concentration of polycyclic aromatic hydrocarbons (PAHs) in the atmosphere"@en ;
    dcterms:creator "SeaDataNet" ;
    dcterms:date "2008-12-09 10:17:11.0" ;
    glbase:hasIdentifier [ glbase:hasIdentifierScheme idscheme:sdn ;
            glbase:hasIdentifierValue "SDN:P02::GP050" ] ;
    rdfs:comment "Parameters quantifying polycyclic aromatic hydrocarbon (PAH) concentrations in all phases of the atmosphere"@en ;
    rdfs:subClassOf <http://vocab.nerc.ac.uk/collection/P03/current/H001/>,
        <http://vocab.nerc.ac.uk/collection/P03/current/M005/> ;
    owl:deprecated "false" .
<http://vocab.nerc.ac.uk/collection/P02/current/GP067/> a glbase:MeasurementType,
        owl:Class,
        owl:NamedIndividual ;
    rdfs:label "Reptile disease and parasites"@en ;
    dcterms:creator "SeaDataNet" ;
    dcterms:date "2008-12-09 10:17:11.0" ;
    glbase:hasIdentifier [ glbase:hasIdentifierScheme idscheme:sdn ;
            glbase:hasIdentifierValue "SDN:P02::GP067" ] ;
    rdfs:comment "Parameters relating to diseases and parasites of reptiles (Class Reptilia)"@en ;
    rdfs:subClassOf <http://vocab.nerc.ac.uk/collection/P03/current/B015/>,
        <http://vocab.nerc.ac.uk/collection/P03/current/B060/> ;
    owl:deprecated "false" .
<http://vocab.nerc.ac.uk/collection/P02/current/GP068/> a glbase:MeasurementType,
        owl:Class,
        owl:NamedIndividual ;
    rdfs:label "Reptile abundance"@en ;
    dcterms:creator "SeaDataNet" ;
    dcterms:date "2008-12-09 10:17:11.0" ;
    glbase:hasIdentifier [ glbase:hasIdentifierScheme idscheme:sdn ;
            glbase:hasIdentifierValue "SDN:P02::GP068" ] ;
    rdfs:comment "Parameters related to the abundance of reptiles (Class Reptilia)"@en ;
    rdfs:subClassOf <http://vocab.nerc.ac.uk/collection/P03/current/B015/>,
        <http://vocab.nerc.ac.uk/collection/P03/current/B070/> ;
    owl:deprecated "false" .
<http://vocab.nerc.ac.uk/collection/P02/current/GP069/> a glbase:MeasurementType,
        owl:Class,
        owl:NamedIndividual ;
    rdfs:label "Reptile reproduction"@en ;
    dcterms:creator "SeaDataNet" ;
    dcterms:date "2008-12-09 10:17:11.0" ;
    glbase:hasIdentifier [ glbase:hasIdentifierScheme idscheme:sdn ;
            glbase:hasIdentifierValue "SDN:P02::GP069" ] ;
    rdfs:comment "Parameters related to the reproduction of reptiles (Class Reptilia)"@en ;
    rdfs:subClassOf <http://vocab.nerc.ac.uk/collection/P03/current/B015/> ;
    owl:deprecated "false" .
<http://vocab.nerc.ac.uk/collection/P02/current/GP079/> a glbase:MeasurementType,
        owl:Class,
        owl:NamedIndividual ;
    rdfs:label "Zooplankton wet weight biomass"@en ;
    dcterms:creator "SeaDataNet" ;
    dcterms:date "2008-12-09 10:17:11.0" ;
    glbase:hasIdentifier [ glbase:hasIdentifierScheme idscheme:sdn ;
            glbase:hasIdentifierValue "SDN:P02::GP079" ] ;
    rdfs:comment "Zooplankton (mesozooplankton and larger, exclusing fish, mammals, reptiles and insects) biomass determined by weighing unprocessed catch samples."@en ;
    rdfs:subClassOf <http://vocab.nerc.ac.uk/collection/P03/current/B045/>,
        <http://vocab.nerc.ac.uk/collection/P03/current/B070/> ;
    owl:deprecated "false" .
<http://vocab.nerc.ac.uk/collection/P02/current/GP080/> a glbase:MeasurementType,
        owl:Class,
        owl:NamedIndividual ;
    rdfs:label "Fishing by-catch"@en ;
    dcterms:creator "SeaDataNet" ;
    dcterms:date "2008-12-09 10:17:11.0" ;
    glbase:hasIdentifier [ glbase:hasIdentifierScheme idscheme:sdn ;
            glbase:hasIdentifierValue "SDN:P02::GP080" ] ;
    rdfs:comment "Parameters quantifying the capture of non-target species during commercial and non-commercial fishing trips"@en ;
    rdfs:subClassOf <http://vocab.nerc.ac.uk/collection/P03/current/H004/> ;
    owl:deprecated "false" .
<http://vocab.nerc.ac.uk/collection/P02/current/GP085/> a glbase:MeasurementType,
        owl:Class,
        owl:NamedIndividual ;
    rdfs:label "Fish behaviour"@en ;
    dcterms:creator "SeaDataNet" ;
    dcterms:date "2008-12-09 10:17:11.0" ;
    glbase:hasIdentifier [ glbase:hasIdentifierScheme idscheme:sdn ;
            glbase:hasIdentifierValue "SDN:P02::GP085" ] ;
    rdfs:comment "Parameters describing the actions or reactions of fish (Osteichthyes, Agnatha and Chondrichthyes), usually in response to the environment. Includes both parameters mapped to taxa and those mapped to non-taxonomic groupings."@en ;
    rdfs:subClassOf <http://vocab.nerc.ac.uk/collection/P03/current/B020/> ;
    owl:deprecated "false" .
<http://vocab.nerc.ac.uk/collection/P02/current/GP087/> a glbase:MeasurementType,
        owl:Class,
        owl:NamedIndividual ;
    rdfs:label "Fishery characterisation"@en ;
    dcterms:creator "SeaDataNet" ;
    dcterms:date "2008-12-09 10:17:11.0" ;
    glbase:hasIdentifier [ glbase:hasIdentifierScheme idscheme:sdn ;
            glbase:hasIdentifierValue "SDN:P02::GP087" ] ;
    rdfs:comment "Parameters describing the extent, intensity, timing and method of fisheries"@en ;
    rdfs:subClassOf <http://vocab.nerc.ac.uk/collection/P03/current/H004/> ;
    owl:deprecated "false" .
<http://vocab.nerc.ac.uk/collection/P02/current/GP088/> a glbase:MeasurementType,
        owl:Class,
        owl:NamedIndividual ;
    rdfs:label "Bird behaviour"@en ;
    dcterms:creator "SeaDataNet" ;
    dcterms:date "2008-12-09 10:17:11.0" ;
    glbase:hasIdentifier [ glbase:hasIdentifierScheme idscheme:sdn ;
            glbase:hasIdentifierValue "SDN:P02::GP088" ] ;
    rdfs:comment "Parameters describing the actions or reactions of birds (Class Aves), usually in response to the environment. Includes both parameters mapped to taxa and those mapped to non-taxonomic groupings."@en ;
    rdfs:subClassOf <http://vocab.nerc.ac.uk/collection/P03/current/B015/> ;
    owl:deprecated "false" .
<http://vocab.nerc.ac.uk/collection/P02/current/GPIG/> a glbase:MeasurementType,
        owl:Class,
        owl:NamedIndividual ;
    rdfs:label "Zooplankton gut pigments"@en ;
    dcterms:creator "SeaDataNet" ;
    dcterms:date "2004-07-08 09:57:35.0" ;
    glbase:hasIdentifier [ glbase:hasIdentifierScheme idscheme:sdn ;
            glbase:hasIdentifierValue "SDN:P02::GPIG" ] ;
    rdfs:comment "Parameters identifying or quantifying zooplankton gut pigments"@en ;
    rdfs:subClassOf <http://vocab.nerc.ac.uk/collection/P03/current/B035/>,
        <http://vocab.nerc.ac.uk/collection/P03/current/B045/> ;
    owl:deprecated "false" .
<http://vocab.nerc.ac.uk/collection/P02/current/GRAV/> a glbase:MeasurementType,
        owl:Class,
        owl:NamedIndividual ;
    rdfs:label "Gravity"@en ;
    dcterms:creator "SeaDataNet" ;
    dcterms:date "2007-11-21 16:22:51.0" ;
    glbase:hasIdentifier [ glbase:hasIdentifierScheme idscheme:sdn ;
            glbase:hasIdentifierValue "SDN:P02::GRAV" ] ;
    rdfs:comment "Parameters relating to the measurement of the Earth's gravity field"@en ;
    rdfs:subClassOf <http://vocab.nerc.ac.uk/collection/P03/current/G005/>,
        <http://vocab.nerc.ac.uk/collection/P03/current/GPYS/> ;
    owl:deprecated "false" .
<http://vocab.nerc.ac.uk/collection/P02/current/GREF/> a glbase:MeasurementType,
        owl:Class,
        owl:NamedIndividual ;
    rdfs:label "Bacterial growth"@en ;
    dcterms:creator "SeaDataNet" ;
    dcterms:date "2004-08-19 10:33:17.0" ;
    glbase:hasIdentifier [ glbase:hasIdentifierScheme idscheme:sdn ;
            glbase:hasIdentifierValue "SDN:P02::GREF" ] ;
    rdfs:comment "" ;
    rdfs:subClassOf <http://vocab.nerc.ac.uk/collection/P03/current/B005/>,
        <http://vocab.nerc.ac.uk/collection/P03/current/O010/> ;
    owl:deprecated "false" .
<http://vocab.nerc.ac.uk/collection/P02/current/GRZO/> a glbase:MeasurementType,
        owl:Class,
        owl:NamedIndividual ;
    rdfs:label "Zooplankton growth rates"@en ;
    dcterms:creator "SeaDataNet" ;
    dcterms:date "2005-08-02 16:38:53.0" ;
    glbase:hasIdentifier [ glbase:hasIdentifierScheme idscheme:sdn ;
            glbase:hasIdentifierValue "SDN:P02::GRZO" ] ;
    rdfs:comment "Parameters pertaining to zooplankton growth rates including biochemical proxies such as AARS activity"@en ;
    rdfs:subClassOf <http://vocab.nerc.ac.uk/collection/P03/current/B045/>,
        <http://vocab.nerc.ac.uk/collection/P03/current/O010/> ;
    owl:deprecated "false" .
<http://vocab.nerc.ac.uk/collection/P02/current/GTCH/> a glbase:MeasurementType,
        owl:Class,
        owl:NamedIndividual ;
    rdfs:label "Geotechnics"@en ;
    dcterms:creator "SeaDataNet" ;
    dcterms:date "2010-07-02 10:24:05.0" ;
    glbase:hasIdentifier [ glbase:hasIdentifierScheme idscheme:sdn ;
            glbase:hasIdentifierValue "SDN:P02::GTCH" ] ;
    rdfs:comment "Parameters quantifying the properties of rocks and sediments that are relevance to engineering such as physical strength and load-bearing capacity.  Includes the disciplines of rock mechanics and soil mechanics."@en ;
    rdfs:subClassOf <http://vocab.nerc.ac.uk/collection/P03/current/G040/>,
        <http://vocab.nerc.ac.uk/collection/P03/current/H002/> ;
    owl:deprecated "false" .
<http://vocab.nerc.ac.uk/collection/P02/current/GWAM/> a glbase:MeasurementType,
        owl:Class,
        owl:NamedIndividual ;
    rdfs:label "Groundwater amount"@en ;
    dcterms:creator "SeaDataNet" ;
    dcterms:date "2009-06-01 11:34:47.0" ;
    glbase:hasIdentifier [ glbase:hasIdentifierScheme idscheme:sdn ;
            glbase:hasIdentifierValue "SDN:P02::GWAM" ] ;
    rdfs:comment "Parameters quantifying the amount of groundwater in a given system such as aquifer water level and rate of flow of water through rock formations."@en ;
    rdfs:subClassOf <http://vocab.nerc.ac.uk/collection/P03/current/T001/> ;
    owl:deprecated "false" .
<http://vocab.nerc.ac.uk/collection/P02/current/GWCH/> a glbase:MeasurementType,
        owl:Class,
        owl:NamedIndividual ;
    rdfs:label "Groundwater chemistry"@en ;
    dcterms:creator "SeaDataNet" ;
    dcterms:date "2009-06-01 11:34:00.0" ;
    glbase:hasIdentifier [ glbase:hasIdentifierScheme idscheme:sdn ;
            glbase:hasIdentifierValue "SDN:P02::GWCH" ] ;
    rdfs:comment "Parameters quantifying the chemistry of terrestrial groundwater bodies such as aquifers and waters percolating through rock formations."@en ;
    rdfs:subClassOf <http://vocab.nerc.ac.uk/collection/P03/current/T001/> ;
    owl:deprecated "false" .
<http://vocab.nerc.ac.uk/collection/P02/current/GWDR/> a glbase:MeasurementType,
        owl:Class,
        owl:NamedIndividual ;
    rdfs:label "Wave direction"@en ;
    dcterms:creator "SeaDataNet" ;
    dcterms:date "2004-08-16 13:05:46.0" ;
    glbase:hasIdentifier [ glbase:hasIdentifierScheme idscheme:sdn ;
            glbase:hasIdentifierValue "SDN:P02::GWDR" ] ;
    rdfs:comment "Direct measurements (including visual estimates) plus statistically derived parameters"@en ;
    rdfs:subClassOf <http://vocab.nerc.ac.uk/collection/P03/current/D034/> ;
    owl:deprecated "false" .
<http://vocab.nerc.ac.uk/collection/P02/current/HAAC/> a glbase:MeasurementType,
        owl:Class,
        owl:NamedIndividual ;
    rdfs:label "Amino acids in sediment"@en ;
    dcterms:creator "SeaDataNet" ;
    dcterms:date "2008-12-09 11:10:47.0" ;
    glbase:hasIdentifier [ glbase:hasIdentifierScheme idscheme:sdn ;
            glbase:hasIdentifierValue "SDN:P02::HAAC" ] ;
    rdfs:comment "Parameters quantifying the amount of organic compounds containing both a carboxyl group and an amino group in unlithified seabed material."@en ;
    rdfs:subClassOf <http://vocab.nerc.ac.uk/collection/P03/current/C003/>,
        <http://vocab.nerc.ac.uk/collection/P03/current/G035/> ;
    owl:deprecated "false" .
<http://vocab.nerc.ac.uk/collection/P02/current/HBCH/> a glbase:MeasurementType,
        owl:Class,
        owl:NamedIndividual ;
    rdfs:label "Habitat characterisation"@en ;
    dcterms:creator "SeaDataNet" ;
    dcterms:date "2008-02-20 08:35:42.0" ;
    glbase:hasIdentifier [ glbase:hasIdentifierScheme idscheme:sdn ;
            glbase:hasIdentifierValue "SDN:P02::HBCH" ] ;
    rdfs:comment "Parameters specifying the physical or chemical environment of a place where an organism is found."@en ;
    rdfs:subClassOf <http://vocab.nerc.ac.uk/collection/P03/current/B050/> ;
    owl:deprecated "false" .
<http://vocab.nerc.ac.uk/collection/P02/current/HBEX/> a glbase:MeasurementType,
        owl:Class,
        owl:NamedIndividual ;
    rdfs:label "Habitat extent"@en ;
    dcterms:creator "SeaDataNet" ;
    dcterms:date "2008-02-20 08:34:08.0" ;
    glbase:hasIdentifier [ glbase:hasIdentifierScheme idscheme:sdn ;
            glbase:hasIdentifierValue "SDN:P02::HBEX" ] ;
    rdfs:comment "Parameters specifying the vertical and horizontal spatial extent of the ecological character of a place where an organism is found"@en ;
    rdfs:subClassOf <http://vocab.nerc.ac.uk/collection/P03/current/B050/> ;
    owl:deprecated "false" .
<http://vocab.nerc.ac.uk/collection/P02/current/HEAD/> a glbase:MeasurementType,
        owl:Class,
        owl:NamedIndividual ;
    rdfs:label "Platform or instrument orientation"@en ;
    dcterms:creator "SeaDataNet" ;
    dcterms:date "2004-08-13 15:29:46.0" ;
    glbase:hasIdentifier [ glbase:hasIdentifierScheme idscheme:sdn ;
            glbase:hasIdentifierValue "SDN:P02::HEAD" ] ;
    rdfs:comment "Parameters that describe the displacement of platforms or instruments in space relative to various origins"@en ;
    rdfs:subClassOf <http://vocab.nerc.ac.uk/collection/P03/current/Z005/> ;
    owl:deprecated "false" .
<http://vocab.nerc.ac.uk/collection/P02/current/HEAV/> a glbase:MeasurementType,
        owl:Class,
        owl:NamedIndividual ;
    rdfs:label "Wave height estimates"@en ;
    dcterms:creator "SeaDataNet" ;
    dcterms:date "2006-06-13 15:25:06.0" ;
    glbase:hasIdentifier [ glbase:hasIdentifierScheme idscheme:sdn ;
            glbase:hasIdentifierValue "SDN:P02::HEAV" ] ;
    rdfs:comment "Measurements of wave height that are not based on the statistical analysis of wave records, such as heave, surface roughness and visual height estimates"@en ;
    rdfs:subClassOf <http://vocab.nerc.ac.uk/collection/P03/current/D034/> ;
    owl:deprecated "false" .
<http://vocab.nerc.ac.uk/collection/P02/current/HEXC/> a glbase:MeasurementType,
        owl:Class,
        owl:NamedIndividual ;
    rdfs:label "Dissolved noble gas concentration parameters in the water column"@en ;
    dcterms:creator "SeaDataNet" ;
    dcterms:date "2004-08-11 14:15:49.0" ;
    glbase:hasIdentifier [ glbase:hasIdentifierScheme idscheme:sdn ;
            glbase:hasIdentifierValue "SDN:P02::HEXC" ] ;
    rdfs:comment "All concentration parameters including saturations and statistics such as standard deviations"@en ;
    rdfs:subClassOf <http://vocab.nerc.ac.uk/collection/P03/current/C015/> ;
    owl:deprecated "false" .
<http://vocab.nerc.ac.uk/collection/P02/current/HFLW/> a glbase:MeasurementType,
        owl:Class,
        owl:NamedIndividual ;
    rdfs:label "Geothermal heat flow"@en ;
    dcterms:creator "SeaDataNet" ;
    dcterms:date "2010-10-22 12:29:12.0" ;
    glbase:hasIdentifier [ glbase:hasIdentifierScheme idscheme:sdn ;
            glbase:hasIdentifierValue "SDN:P02::HFLW" ] ;
    rdfs:comment "Parameters quantifying the  flux of thermal energy within the solid Earth or between the solid Earth and water bodies or atmosphere."@en ;
    rdfs:subClassOf <http://vocab.nerc.ac.uk/collection/P03/current/GTHM/> ;
    owl:deprecated "false" .
<http://vocab.nerc.ac.uk/collection/P02/current/HFLX/> a glbase:MeasurementType,
        owl:Class,
        owl:NamedIndividual ;
    rdfs:label "Heat fluxes between the water column and the atmosphere"@en ;
    dcterms:creator "SeaDataNet" ;
    dcterms:date "2007-02-23 14:49:48.0" ;
    glbase:hasIdentifier [ glbase:hasIdentifierScheme idscheme:sdn ;
            glbase:hasIdentifierValue "SDN:P02::HFLX" ] ;
    rdfs:comment "Parameters quantifying heat exchange between any body of water and the atmosphere"@en ;
    rdfs:subClassOf <http://vocab.nerc.ac.uk/collection/P03/current/D020/>,
        <http://vocab.nerc.ac.uk/collection/P03/current/O005/> ;
    owl:deprecated "false" .
<http://vocab.nerc.ac.uk/collection/P02/current/HLAT/> a glbase:MeasurementType,
        owl:Class,
        owl:NamedIndividual ;
    rdfs:label "Concentration of inorganic halogens in the atmosphere"@en ;
    dcterms:creator "SeaDataNet" ;
    dcterms:date "2010-07-02 09:42:02.0" ;
    glbase:hasIdentifier [ glbase:hasIdentifierScheme idscheme:sdn ;
            glbase:hasIdentifierValue "SDN:P02::HLAT" ] ;
    rdfs:comment "Concentrations of halogens as elements or their inorganic compounds in all phases of the atmosphere."@en ;
    rdfs:subClassOf <http://vocab.nerc.ac.uk/collection/P03/current/C045/>,
        <http://vocab.nerc.ac.uk/collection/P03/current/M005/> ;
    owl:deprecated "false" .
<http://vocab.nerc.ac.uk/collection/P02/current/HLDE/> a glbase:MeasurementType,
        owl:Class,
        owl:NamedIndividual ;
    rdfs:label "Other halocarbon dynamics in water bodies"@en ;
    dcterms:creator "SeaDataNet" ;
    dcterms:date "2010-11-08 15:08:09.0" ;
    glbase:hasIdentifier [ glbase:hasIdentifierScheme idscheme:sdn ;
            glbase:hasIdentifierValue "SDN:P02::HLDE" ] ;
    rdfs:comment "Parameters relating to the rates of creation and consumption of volatile halocarbons (compounds comprising carbon atoms covalently bonded to fluorine, chlorine, bromine or iodine atoms) other than tracers (i.e. freons/chlorofluorocarbons) and contaminants in any body of fresh or salt water."@en ;
    rdfs:subClassOf <http://vocab.nerc.ac.uk/collection/P03/current/C020/> ;
    owl:deprecated "false" .
<http://vocab.nerc.ac.uk/collection/P02/current/HLIC/> a glbase:MeasurementType,
        owl:Class,
        owl:NamedIndividual ;
    rdfs:label "Concentration of inorganic halogens in ice"@en ;
    dcterms:creator "SeaDataNet" ;
    dcterms:date "2011-02-18 12:17:16.0" ;
    glbase:hasIdentifier [ glbase:hasIdentifierScheme idscheme:sdn ;
            glbase:hasIdentifierValue "SDN:P02::HLIC" ] ;
    rdfs:comment "Concentrations of halogens as elements or their inorganic compounds in ice"@en ;
    rdfs:subClassOf <http://vocab.nerc.ac.uk/collection/P02/current/ICHM/> ;
    owl:deprecated "true" .
<http://vocab.nerc.ac.uk/collection/P02/current/HLWC/> a glbase:MeasurementType,
        owl:Class,
        owl:NamedIndividual ;
    rdfs:label "Concentration of inorganic halogens in water bodies"@en ;
    dcterms:creator "SeaDataNet" ;
    dcterms:date "2010-07-02 09:44:29.0" ;
    glbase:hasIdentifier [ glbase:hasIdentifierScheme idscheme:sdn ;
            glbase:hasIdentifierValue "SDN:P02::HLWC" ] ;
    rdfs:comment "Concentrations of halogens as elements or their inorganic compounds in all phases of any body of fresh or salt water"@en ;
    rdfs:subClassOf <http://vocab.nerc.ac.uk/collection/P03/current/C045/> ;
    owl:deprecated "false" .
<http://vocab.nerc.ac.uk/collection/P02/current/HMSB/> a glbase:MeasurementType,
        owl:Class,
        owl:NamedIndividual ;
    rdfs:label "Concentration of dissolved organic matter in the water column"@en ;
    dcterms:creator "SeaDataNet" ;
    dcterms:date "2006-06-05 13:33:38.0" ;
    glbase:hasIdentifier [ glbase:hasIdentifierScheme idscheme:sdn ;
            glbase:hasIdentifierValue "SDN:P02::HMSB" ] ;
    rdfs:comment "Concentration (not 380nm light absorption) parameters for dissolved organic matter (includes humics, yellow matter, Gelbstoff) in the water column"@en ;
    rdfs:subClassOf <http://vocab.nerc.ac.uk/collection/P03/current/C050/> ;
    owl:deprecated "false" .
<http://vocab.nerc.ac.uk/collection/P02/current/HZNV/> a glbase:MeasurementType,
        owl:Class,
        owl:NamedIndividual ;
    rdfs:label "Hazards to navigation"@en ;
    dcterms:creator "SeaDataNet" ;
    dcterms:date "2009-04-20 08:27:53.0" ;
    glbase:hasIdentifier [ glbase:hasIdentifierScheme idscheme:sdn ;
            glbase:hasIdentifierValue "SDN:P02::HZNV" ] ;
    rdfs:comment "Parameters describing the location, nature and extent of objects that pose a threat to travel on the water column such as wrecks and obstructions"@en ;
    rdfs:subClassOf <http://vocab.nerc.ac.uk/collection/P03/current/H002/> ;
    owl:deprecated "false" .
<http://vocab.nerc.ac.uk/collection/P02/current/IACT/> a glbase:MeasurementType,
        owl:Class,
        owl:NamedIndividual ;
    rdfs:label "Industrial activity"@en ;
    dcterms:creator "SeaDataNet" ;
    dcterms:date "2008-12-09 10:17:11.0" ;
    glbase:hasIdentifier [ glbase:hasIdentifierScheme idscheme:sdn ;
            glbase:hasIdentifierValue "SDN:P02::IACT" ] ;
    rdfs:comment "Parameters that quantify the level of industrial activity or industrial output"@en ;
    rdfs:subClassOf <http://vocab.nerc.ac.uk/collection/P03/current/H005/> ;
    owl:deprecated "false" .
<http://vocab.nerc.ac.uk/collection/P02/current/IAGE/> a glbase:MeasurementType,
        owl:Class,
        owl:NamedIndividual ;
    rdfs:label "Ice age"@en ;
    dcterms:creator "SeaDataNet" ;
    dcterms:date "2006-02-20 11:55:04.0" ;
    glbase:hasIdentifier [ glbase:hasIdentifierScheme idscheme:sdn ;
            glbase:hasIdentifierValue "SDN:P02::IAGE" ] ;
    rdfs:comment "Measured or stratigraphically estimated age of ice"@en ;
    rdfs:subClassOf <http://vocab.nerc.ac.uk/collection/P03/current/M015/> ;
    owl:deprecated "false" .
<http://vocab.nerc.ac.uk/collection/P02/current/IALZ/> a glbase:MeasurementType,
        owl:Class,
        owl:NamedIndividual ;
    rdfs:label "Insect and earthworm taxonomy-related ash-free dry weight biomass per unit area of the littoral zone"@en ;
    dcterms:creator "SeaDataNet" ;
    dcterms:date "2015-04-08 15:27:34.0" ;
    glbase:hasIdentifier [ glbase:hasIdentifierScheme idscheme:sdn ;
            glbase:hasIdentifierValue "SDN:P02::IALZ" ] ;
    rdfs:comment "Insect (Class Insecta) and earthworm (Subclass Oligochaeta) ash-free dry weight biomass per unit area of the littoral zone (between spring tide high and low water) parameters."@en ;
    rdfs:subClassOf <http://vocab.nerc.ac.uk/collection/P03/current/B070/>,
        <http://vocab.nerc.ac.uk/collection/P03/current/G055/> ;
    owl:deprecated "true" .
<http://vocab.nerc.ac.uk/collection/P02/current/IATC/> a glbase:MeasurementType,
        owl:Class,
        owl:NamedIndividual ;
    rdfs:label "Insecta taxonomy-related biomass expressed as carbon per unit volume of the water column"@en ;
    dcterms:creator "SeaDataNet" ;
    dcterms:date "2004-04-22 08:25:00.0" ;
    glbase:hasIdentifier [ glbase:hasIdentifierScheme idscheme:sdn ;
            glbase:hasIdentifierValue "SDN:P02::IATC" ] ;
    rdfs:comment "Insecta carbon biomass parameters presented at the level of taxa that may be mapped to entities in the ITIS taxonomy.  These may be at any taxonomic level from sub-species upwards."@en ;
    rdfs:subClassOf <http://vocab.nerc.ac.uk/collection/P03/current/B045/>,
        <http://vocab.nerc.ac.uk/collection/P03/current/B070/> ;
    owl:deprecated "false" .
<http://vocab.nerc.ac.uk/collection/P02/current/IATX/> a glbase:MeasurementType,
        owl:Class,
        owl:NamedIndividual ;
    rdfs:label "Insecta taxonomy-related abundance per unit volume of the water column"@en ;
    dcterms:creator "SeaDataNet" ;
    dcterms:date "2004-04-19 16:35:00.0" ;
    glbase:hasIdentifier [ glbase:hasIdentifierScheme idscheme:sdn ;
            glbase:hasIdentifierValue "SDN:P02::IATX" ] ;
    rdfs:comment "Insecta abundance parameters presented at the level of taxa that may be mapped to entities in the ITIS taxonomy.  These may be at any taxonomic level from sub-species upwards."@en ;
    rdfs:subClassOf <http://vocab.nerc.ac.uk/collection/P03/current/B045/>,
        <http://vocab.nerc.ac.uk/collection/P03/current/B070/> ;
    owl:deprecated "false" .
<http://vocab.nerc.ac.uk/collection/P02/current/ICEM/> a glbase:MeasurementType,
        owl:Class,
        owl:NamedIndividual ;
    rdfs:label "Ice motion and related parameters"@en ;
    dcterms:creator "SeaDataNet" ;
    dcterms:date "2007-09-24 16:19:08.0" ;
    glbase:hasIdentifier [ glbase:hasIdentifierScheme idscheme:sdn ;
            glbase:hasIdentifierValue "SDN:P02::ICEM" ] ;
    rdfs:comment "Parameters specifying the speed and direction of sea or land ice and the stresses associated with this motion."@en ;
    rdfs:subClassOf <http://vocab.nerc.ac.uk/collection/P03/current/M015/> ;
    owl:deprecated "false" .
<http://vocab.nerc.ac.uk/collection/P02/current/IDIS/> a glbase:MeasurementType,
        owl:Class,
        owl:NamedIndividual ;
    rdfs:label "Industrial discharges"@en ;
    dcterms:creator "SeaDataNet" ;
    dcterms:date "2008-12-09 10:17:11.0" ;
    glbase:hasIdentifier [ glbase:hasIdentifierScheme idscheme:sdn ;
            glbase:hasIdentifierValue "SDN:P02::IDIS" ] ;
    rdfs:comment "Parameters that quantify and specify material output into the environment as a result of industrial activity"@en ;
    rdfs:subClassOf <http://vocab.nerc.ac.uk/collection/P03/current/H001/> ;
    owl:deprecated "false" .
<http://vocab.nerc.ac.uk/collection/P02/current/INLZ/> a glbase:MeasurementType,
        owl:Class,
        owl:NamedIndividual ;
    rdfs:label "Insect and earthworm taxonomy-related abundance per unit area of the littoral zone"@en ;
    dcterms:creator "SeaDataNet" ;
    dcterms:date "2015-04-08 15:26:45.0" ;
    glbase:hasIdentifier [ glbase:hasIdentifierScheme idscheme:sdn ;
            glbase:hasIdentifierValue "SDN:P02::INLZ" ] ;
    rdfs:comment "Insect (Class Insecta) and earthworm (Subclass Oligochaeta) abundance per unit area of the littoral zone (between spring tide high and low water) parameters."@en ;
    rdfs:subClassOf <http://vocab.nerc.ac.uk/collection/P03/current/B070/>,
        <http://vocab.nerc.ac.uk/collection/P03/current/G055/> ;
    owl:deprecated "true" .
<http://vocab.nerc.ac.uk/collection/P02/current/IPHY/> a glbase:MeasurementType,
        owl:Class,
        owl:NamedIndividual ;
    rdfs:label "Snow and ice physical properties and characteristics"@en ;
    dcterms:creator "SeaDataNet" ;
    dcterms:date "2011-02-18 11:04:05.0" ;
    glbase:hasIdentifier [ glbase:hasIdentifierScheme idscheme:sdn ;
            glbase:hasIdentifierValue "SDN:P02::IPHY" ] ;
    rdfs:comment "Parameters related to physical properties (e.g. colour, density, in-situ temperature) or characteristics (e.g. sea ice type) of any kind of water sample that was in its solid state at the time of sampling or measurement"@en ;
    rdfs:subClassOf <http://vocab.nerc.ac.uk/collection/P03/current/M015/> ;
    owl:deprecated "false" .
<http://vocab.nerc.ac.uk/collection/P02/current/IPRX/> a glbase:MeasurementType,
        owl:Class,
        owl:NamedIndividual ;
    rdfs:label "Inorganic peroxides in water bodies"@en ;
    dcterms:creator "SeaDataNet" ;
    dcterms:date "2011-07-26 09:03:07.0" ;
    glbase:hasIdentifier [ glbase:hasIdentifierScheme idscheme:sdn ;
            glbase:hasIdentifierValue "SDN:P02::IPRX" ] ;
    rdfs:comment "Parameters related to compounds containing two oxygen atoms joined by a single bond but no carbon atoms in any body of fresh or salt water."@en ;
    rdfs:subClassOf <http://vocab.nerc.ac.uk/collection/P03/current/C045/> ;
    owl:deprecated "false" .
<http://vocab.nerc.ac.uk/collection/P02/current/IRBO/> a glbase:MeasurementType,
        owl:Class,
        owl:NamedIndividual ;
    rdfs:label "Stable isotope enrichment in biota"@en ;
    dcterms:creator "SeaDataNet" ;
    dcterms:date "2008-06-30 15:13:59.0" ;
    glbase:hasIdentifier [ glbase:hasIdentifierScheme idscheme:sdn ;
            glbase:hasIdentifierValue "SDN:P02::IRBO" ] ;
    rdfs:comment "Stable isotope enrichment parameters from measurements on living (at the time of sampling) organisms or parts thereof"@en ;
    rdfs:subClassOf <http://vocab.nerc.ac.uk/collection/P03/current/B007/>,
        <http://vocab.nerc.ac.uk/collection/P03/current/C030/> ;
    owl:deprecated "false" .
<http://vocab.nerc.ac.uk/collection/P02/current/IRIC/> a glbase:MeasurementType,
        owl:Class,
        owl:NamedIndividual ;
    rdfs:label "Stable isotope enrichment in ice and snow"@en ;
    dcterms:creator "SeaDataNet" ;
    dcterms:date "2011-02-18 14:11:41.0" ;
    glbase:hasIdentifier [ glbase:hasIdentifierScheme idscheme:sdn ;
            glbase:hasIdentifierValue "SDN:P02::IRIC" ] ;
    rdfs:comment "Stable isotope enrichment parameters in frozen precipitation (snow, hail, ice and slush), its accumulations (e.g. glaciers), sea ice and frozen fresh water."@en ;
    rdfs:subClassOf <http://vocab.nerc.ac.uk/collection/P02/current/ICHM/> ;
    owl:deprecated "true" .
<http://vocab.nerc.ac.uk/collection/P02/current/IRSP/> a glbase:MeasurementType,
        owl:Class,
        owl:NamedIndividual ;
    rdfs:label "Stable isotope enrichment in speleothems"@en ;
    dcterms:creator "SeaDataNet" ;
    dcterms:date "2006-06-21 09:23:05.0" ;
    glbase:hasIdentifier [ glbase:hasIdentifierScheme idscheme:sdn ;
            glbase:hasIdentifierValue "SDN:P02::IRSP" ] ;
    rdfs:comment "Stable isotope enrichment parameters in secondary mineral deposits in caves. This includes stalactites, stalagmites, flowstone, and crystal growths."@en ;
    rdfs:subClassOf <http://vocab.nerc.ac.uk/collection/P03/current/G035/> ;
    owl:deprecated "false" .
<http://vocab.nerc.ac.uk/collection/P02/current/IS4R/> a glbase:MeasurementType,
        owl:Class,
        owl:NamedIndividual ;
    rdfs:label "Reduction rates in bed sediments"@en ;
    dcterms:creator "SeaDataNet" ;
    dcterms:date "2004-08-19 11:44:47.0" ;
    glbase:hasIdentifier [ glbase:hasIdentifierScheme idscheme:sdn ;
            glbase:hasIdentifierValue "SDN:P02::IS4R" ] ;
    rdfs:comment "Reduction rates of any species in sediment cores"@en ;
    rdfs:subClassOf <http://vocab.nerc.ac.uk/collection/P03/current/O010/> ;
    owl:deprecated "false" .
<http://vocab.nerc.ac.uk/collection/P02/current/ISAT/> a glbase:MeasurementType,
        owl:Class,
        owl:NamedIndividual ;
    rdfs:label "Stable isotope enrichment in the atmosphere"@en ;
    dcterms:creator "SeaDataNet" ;
    dcterms:date "2010-02-21 17:29:42.0" ;
    glbase:hasIdentifier [ glbase:hasIdentifierScheme idscheme:sdn ;
            glbase:hasIdentifierValue "SDN:P02::ISAT" ] ;
    rdfs:comment "Stable isotope enrichment parameters in both the gaseous and aerosol phases of the atmosphere"@en ;
    rdfs:subClassOf <http://vocab.nerc.ac.uk/collection/P03/current/C030/>,
        <http://vocab.nerc.ac.uk/collection/P03/current/M005/> ;
    owl:deprecated "false" .
<http://vocab.nerc.ac.uk/collection/P02/current/ISIC/> a glbase:MeasurementType,
        owl:Class,
        owl:NamedIndividual ;
    rdfs:label "Concentration of inorganic sulphur species in ice"@en ;
    dcterms:creator "SeaDataNet" ;
    dcterms:date "2011-02-18 14:28:40.0" ;
    glbase:hasIdentifier [ glbase:hasIdentifierScheme idscheme:sdn ;
            glbase:hasIdentifierValue "SDN:P02::ISIC" ] ;
    rdfs:comment "Concentration parameters for inorganic sulphur species in ice"@en ;
    rdfs:subClassOf <http://vocab.nerc.ac.uk/collection/P02/current/ICHM/> ;
    owl:deprecated "true" .
<http://vocab.nerc.ac.uk/collection/P02/current/IWAB/> a glbase:MeasurementType,
        owl:Class,
        owl:NamedIndividual ;
    rdfs:label "Insect and earthworm taxonomy-related abundance per unit area of the bed"@en ;
    dcterms:creator "SeaDataNet" ;
    dcterms:date "2004-04-28 09:31:00.0" ;
    glbase:hasIdentifier [ glbase:hasIdentifierScheme idscheme:sdn ;
            glbase:hasIdentifierValue "SDN:P02::IWAB" ] ;
    rdfs:comment "Insect (Class Insecta) and earthworm (Subclass Oligochaeta) abundance per unit area of bed (sea, river, lake etc.) parameters presented at the level of taxa that may be mapped to entities in the ITIS taxonomy.  Includes animals normally considered as planktonic if they have been returned from sediment samples. This parameter group has been implemented to separate predominantly freshwater taxa from predominantly marine taxa."@en ;
    rdfs:subClassOf <http://vocab.nerc.ac.uk/collection/P03/current/B070/>,
        <http://vocab.nerc.ac.uk/collection/P03/current/G055/> ;
    owl:deprecated "false" .
<http://vocab.nerc.ac.uk/collection/P02/current/IWDX/> a glbase:MeasurementType,
        owl:Class,
        owl:NamedIndividual ;
    rdfs:label "Insect and earthworm taxonomy-related ash-free dry weight biomass per unit area of the bed"@en ;
    dcterms:creator "SeaDataNet" ;
    dcterms:date "2004-04-28 09:22:00.0" ;
    glbase:hasIdentifier [ glbase:hasIdentifierScheme idscheme:sdn ;
            glbase:hasIdentifierValue "SDN:P02::IWDX" ] ;
    rdfs:comment "Insect (Class Insecta) and earthworm (Subclass Oligochaeta) ash-free dry weight biomass per unit area of bed (sea, river, lake etc.) parameters presented at the level of taxa that may be mapped to entities in the ITIS taxonomy.  Includes animals normally considered as planktonic if they have been returned from sediment samples. This parameter group has been implemented to separate predominantly freshwater taxa from predominantly marine taxa."@en ;
    rdfs:subClassOf <http://vocab.nerc.ac.uk/collection/P03/current/B070/>,
        <http://vocab.nerc.ac.uk/collection/P03/current/G055/> ;
    owl:deprecated "false" .
<http://vocab.nerc.ac.uk/collection/P02/current/KRTS/> a glbase:MeasurementType,
        owl:Class,
        owl:NamedIndividual ;
    rdfs:label "Other wave statistics"@en ;
    dcterms:creator "SeaDataNet" ;
    dcterms:date "2010-11-08 15:08:09.0" ;
    glbase:hasIdentifier [ glbase:hasIdentifierScheme idscheme:sdn ;
            glbase:hasIdentifierValue "SDN:P02::KRTS" ] ;
    rdfs:comment "Statistical parameters derived from wave data expressing wave properties other than height, period and direction"@en ;
    rdfs:subClassOf <http://vocab.nerc.ac.uk/collection/P03/current/D034/> ;
    owl:deprecated "false" .
<http://vocab.nerc.ac.uk/collection/P02/current/LERR/> a glbase:MeasurementType,
        owl:Class,
        owl:NamedIndividual ;
    rdfs:label "Raw current meter output parameters"@en ;
    dcterms:creator "SeaDataNet" ;
    dcterms:date "2004-08-17 12:16:41.0" ;
    glbase:hasIdentifier [ glbase:hasIdentifierScheme idscheme:sdn ;
            glbase:hasIdentifierValue "SDN:P02::LERR" ] ;
    rdfs:comment "Parameters as logged by measuring devices, including raw counts/voltages and ADCP relative velocities"@en ;
    rdfs:subClassOf <http://vocab.nerc.ac.uk/collection/P03/current/D030/> ;
    owl:deprecated "false" .
<http://vocab.nerc.ac.uk/collection/P02/current/LGCR/> a glbase:MeasurementType,
        owl:Class,
        owl:NamedIndividual ;
    rdfs:label "Lagrangian currents and transport rates in the water column"@en ;
    dcterms:creator "SeaDataNet" ;
    dcterms:date "2007-01-18 16:36:09.0" ;
    glbase:hasIdentifier [ glbase:hasIdentifierScheme idscheme:sdn ;
            glbase:hasIdentifierValue "SDN:P02::LGCR" ] ;
    rdfs:comment "Parameters expressing the mean nett transport rates within the water column like Lagrangian currents. Note this is an unintentional duplicate of VDFC."@en ;
    rdfs:subClassOf <http://schema.geolink.org/1.0/voc/nvs/P03#SeaDataNetParameter> ;
    owl:deprecated "false" .
<http://vocab.nerc.ac.uk/collection/P02/current/LIBI/> a glbase:MeasurementType,
        owl:Class,
        owl:NamedIndividual ;
    rdfs:label "Biota lipid concentrations"@en ;
    dcterms:creator "SeaDataNet" ;
    dcterms:date "2012-03-01 16:10:50.0" ;
    glbase:hasIdentifier [ glbase:hasIdentifierScheme idscheme:sdn ;
            glbase:hasIdentifierValue "SDN:P02::LIBI" ] ;
    rdfs:comment "Lipids are defined as small water-insoluble biomolecules including fats, fatty acids, esters, sterols, isoprenoid compounds, etc..  Biota includes any type of sample originating from a living organism."@en ;
    rdfs:subClassOf <http://vocab.nerc.ac.uk/collection/P03/current/B007/> ;
    owl:deprecated "false" .
<http://vocab.nerc.ac.uk/collection/P02/current/LIFX/> a glbase:MeasurementType,
        owl:Class,
        owl:NamedIndividual ;
    rdfs:label "Sedimentation flux of terrestrially derived material in the water column"@en ;
    dcterms:creator "SeaDataNet" ;
    dcterms:date "2004-10-22 15:25:00.0" ;
    glbase:hasIdentifier [ glbase:hasIdentifierScheme idscheme:sdn ;
            glbase:hasIdentifierValue "SDN:P02::LIFX" ] ;
    rdfs:comment "Fluxes of terrestrial biological or lithological material"@en ;
    rdfs:subClassOf <http://vocab.nerc.ac.uk/collection/P03/current/O005/> ;
    owl:deprecated "false" .
<http://vocab.nerc.ac.uk/collection/P02/current/LITH/> a glbase:MeasurementType,
        owl:Class,
        owl:NamedIndividual ;
    rdfs:label "Lithology"@en ;
    dcterms:creator "SeaDataNet" ;
    dcterms:date "2008-01-30 07:53:20.0" ;
    glbase:hasIdentifier [ glbase:hasIdentifierScheme idscheme:sdn ;
            glbase:hasIdentifierValue "SDN:P02::LITH" ] ;
    rdfs:comment "Parameters describing rocks on the basis of physical characteristics such as colour, structure, mineralogy and grain size"@en ;
    rdfs:subClassOf <http://vocab.nerc.ac.uk/collection/P03/current/G045/> ;
    owl:deprecated "false" .
<http://vocab.nerc.ac.uk/collection/P02/current/LITT/> a glbase:MeasurementType,
        owl:Class,
        owl:NamedIndividual ;
    rdfs:label "Litter abundance and type"@en ;
    dcterms:creator "SeaDataNet" ;
    dcterms:date "2008-01-30 07:53:20.0" ;
    glbase:hasIdentifier [ glbase:hasIdentifierScheme idscheme:sdn ;
            glbase:hasIdentifierValue "SDN:P02::LITT" ] ;
    rdfs:comment "Parameters describing the abundance and nature of material classed as refuse introduced to the environment by activities of man."@en ;
    rdfs:subClassOf <http://vocab.nerc.ac.uk/collection/P03/current/H001/> ;
    owl:deprecated "false" .
<http://vocab.nerc.ac.uk/collection/P02/current/LRZA/> a glbase:MeasurementType,
        owl:Class,
        owl:NamedIndividual ;
    rdfs:label "Vertical velocity of the water column (currents)"@en ;
    dcterms:creator "SeaDataNet" ;
    dcterms:date "2004-08-23 17:01:00.0" ;
    glbase:hasIdentifier [ glbase:hasIdentifierScheme idscheme:sdn ;
            glbase:hasIdentifierValue "SDN:P02::LRZA" ] ;
    rdfs:comment "Vertical water movement parameters including non-directional speeds"@en ;
    rdfs:subClassOf <http://vocab.nerc.ac.uk/collection/P03/current/D030/> ;
    owl:deprecated "false" .
<http://vocab.nerc.ac.uk/collection/P02/current/LSST/> a glbase:MeasurementType,
        owl:Class,
        owl:NamedIndividual ;
    rdfs:label "Land surface temperature"@en ;
    dcterms:creator "SeaDataNet" ;
    dcterms:date "2006-05-26 10:16:40.0" ;
    glbase:hasIdentifier [ glbase:hasIdentifierScheme idscheme:sdn ;
            glbase:hasIdentifierValue "SDN:P02::LSST" ] ;
    rdfs:comment "Parameters relating to land surface temperature including fire and other hot spot location"@en ;
    rdfs:subClassOf <http://vocab.nerc.ac.uk/collection/P03/current/T001/> ;
    owl:deprecated "false" .
<http://vocab.nerc.ac.uk/collection/P02/current/LVEG/> a glbase:MeasurementType,
        owl:Class,
        owl:NamedIndividual ;
    rdfs:label "Land vegetation"@en ;
    dcterms:creator "SeaDataNet" ;
    dcterms:date "2006-05-26 10:18:46.0" ;
    glbase:hasIdentifier [ glbase:hasIdentifierScheme idscheme:sdn ;
            glbase:hasIdentifierValue "SDN:P02::LVEG" ] ;
    rdfs:comment "Parameters relating to land (including marshes and the intertidal zone) vegetation"@en ;
    rdfs:subClassOf <http://vocab.nerc.ac.uk/collection/P03/current/T001/> ;
    owl:deprecated "false" .
<http://vocab.nerc.ac.uk/collection/P02/current/LVLT/> a glbase:MeasurementType,
        owl:Class,
        owl:NamedIndividual ;
    rdfs:label "Raw light meter output"@en ;
    dcterms:creator "SeaDataNet" ;
    dcterms:date "2003-06-10 13:53:19.0" ;
    glbase:hasIdentifier [ glbase:hasIdentifierScheme idscheme:sdn ;
            glbase:hasIdentifierValue "SDN:P02::LVLT" ] ;
    rdfs:comment "" ;
    rdfs:subClassOf <http://vocab.nerc.ac.uk/collection/P03/current/D015/> ;
    owl:deprecated "false" .
<http://vocab.nerc.ac.uk/collection/P02/current/LWET/> a glbase:MeasurementType,
        owl:Class,
        owl:NamedIndividual ;
    rdfs:label "Terrestrial water content"@en ;
    dcterms:creator "SeaDataNet" ;
    dcterms:date "2006-05-26 13:36:40.0" ;
    glbase:hasIdentifier [ glbase:hasIdentifierScheme idscheme:sdn ;
            glbase:hasIdentifierValue "SDN:P02::LWET" ] ;
    rdfs:comment "Parameters relating to the water held by land masses such as soil and vegetation moisture content"@en ;
    rdfs:subClassOf <http://vocab.nerc.ac.uk/collection/P03/current/T001/> ;
    owl:deprecated "false" .
<http://vocab.nerc.ac.uk/collection/P02/current/LWRD/> a glbase:MeasurementType,
        owl:Class,
        owl:NamedIndividual ;
    rdfs:label "Long-wave radiation"@en ;
    dcterms:creator "SeaDataNet" ;
    dcterms:date "2003-06-10 13:53:19.0" ;
    glbase:hasIdentifier [ glbase:hasIdentifierScheme idscheme:sdn ;
            glbase:hasIdentifierValue "SDN:P02::LWRD" ] ;
    rdfs:comment "" ;
    rdfs:subClassOf <http://vocab.nerc.ac.uk/collection/P03/current/M010/> ;
    owl:deprecated "false" .
<http://vocab.nerc.ac.uk/collection/P02/current/MARC/> a glbase:MeasurementType,
        owl:Class,
        owl:NamedIndividual ;
    rdfs:label "Marine archaeology"@en ;
    dcterms:creator "SeaDataNet" ;
    dcterms:date "2011-03-24 08:27:01.0" ;
    glbase:hasIdentifier [ glbase:hasIdentifierScheme idscheme:sdn ;
            glbase:hasIdentifierValue "SDN:P02::MARC" ] ;
    rdfs:comment "Parameters related to the study of human interaction with the sea through the investigation of associated physical remains, be they vessels, shore side facilities, port-related structures, cargoes, human remains or submerged landscapes"@en ;
    rdfs:subClassOf <http://vocab.nerc.ac.uk/collection/P03/current/H005/> ;
    owl:deprecated "false" .
<http://vocab.nerc.ac.uk/collection/P02/current/MATC/> a glbase:MeasurementType,
        owl:Class,
        owl:NamedIndividual ;
    rdfs:label "Microzooplankton taxonomy-related biomass expressed as carbon per unit volume of the water column"@en ;
    dcterms:creator "SeaDataNet" ;
    dcterms:date "2004-04-19 14:15:00.0" ;
    glbase:hasIdentifier [ glbase:hasIdentifierScheme idscheme:sdn ;
            glbase:hasIdentifierValue "SDN:P02::MATC" ] ;
    rdfs:comment "Microzooplankton carbon biomass parameters presented at the level of taxa that may be mapped to entities in the ITIS taxonomy.  These may be at any taxonomic level from sub-species upwards., but exclude morphological classifications such as 'heterotrophic flagellate'."@en ;
    rdfs:subClassOf <http://vocab.nerc.ac.uk/collection/P03/current/B025/>,
        <http://vocab.nerc.ac.uk/collection/P03/current/B070/> ;
    owl:deprecated "false" .
<http://vocab.nerc.ac.uk/collection/P02/current/MATX/> a glbase:MeasurementType,
        owl:Class,
        owl:NamedIndividual ;
    rdfs:label "Microzooplankton taxonomic abundance in water bodies"@en ;
    dcterms:creator "SeaDataNet" ;
    dcterms:date "2010-10-22 10:06:41.0" ;
    glbase:hasIdentifier [ glbase:hasIdentifierScheme idscheme:sdn ;
            glbase:hasIdentifierValue "SDN:P02::MATX" ] ;
    rdfs:comment "Any enumeration (e.g. count, number per litre) of microzooplankton (free swimming heterotrophic organisms smaller than 200um) designated by taxonomic names (e.g. species, genus or family) in any fresh or salt water body."@en ;
    rdfs:subClassOf <http://vocab.nerc.ac.uk/collection/P03/current/B025/>,
        <http://vocab.nerc.ac.uk/collection/P03/current/B070/> ;
    owl:deprecated "false" .
<http://vocab.nerc.ac.uk/collection/P02/current/MBAN/> a glbase:MeasurementType,
        owl:Class,
        owl:NamedIndividual ;
    rdfs:label "Bathymetry and Elevation"@en ;
    dcterms:creator "SeaDataNet" ;
    dcterms:date "2006-09-29 16:58:04.0" ;
    glbase:hasIdentifier [ glbase:hasIdentifierScheme idscheme:sdn ;
            glbase:hasIdentifierValue "SDN:P02::MBAN" ] ;
    rdfs:comment "Depth of the water column or elevation of land surface relative to sea surface, geoid or other datum"@en ;
    rdfs:subClassOf <http://schema.geolink.org/1.0/voc/nvs/P03#SeaDataNetParameter> ;
    owl:deprecated "false" .
<http://vocab.nerc.ac.uk/collection/P02/current/MDBO/> a glbase:MeasurementType,
        owl:Class,
        owl:NamedIndividual ;
    rdfs:label "Trace metalloid concentrations in biota"@en ;
    dcterms:creator "SeaDataNet" ;
    dcterms:date "2010-01-27 14:18:10.0" ;
    glbase:hasIdentifier [ glbase:hasIdentifierScheme idscheme:sdn ;
            glbase:hasIdentifierValue "SDN:P02::MDBO" ] ;
    rdfs:comment "Concentration parameters for trace metalloid elements in either whole organisms or their constituent parts. Trace metalloids are considered as B, Ge, As, Sb, Te and Po (but not Si which is classed separately because of its major role in environmental chemistry)"@en ;
    rdfs:subClassOf <http://vocab.nerc.ac.uk/collection/P03/current/B007/>,
        <http://vocab.nerc.ac.uk/collection/P03/current/C035/>,
        <http://vocab.nerc.ac.uk/collection/P03/current/H001/> ;
    owl:deprecated "false" .
<http://vocab.nerc.ac.uk/collection/P02/current/MDPW/> a glbase:MeasurementType,
        owl:Class,
        owl:NamedIndividual ;
    rdfs:label "Trace metalloid concentrations in sediment pore water"@en ;
    dcterms:creator "SeaDataNet" ;
    dcterms:date "2010-01-27 14:18:10.0" ;
    glbase:hasIdentifier [ glbase:hasIdentifierScheme idscheme:sdn ;
            glbase:hasIdentifierValue "SDN:P02::MDPW" ] ;
    rdfs:comment "Concentration parameters for trace metalloid elements in water occupying the space between sediment grains. Trace metalloids are considered as B, Ge, As, Sb, Te and Po (but not Si which is classed separately because of its major role in environmental chemistry)"@en ;
    rdfs:subClassOf <http://vocab.nerc.ac.uk/collection/P03/current/C035/>,
        <http://vocab.nerc.ac.uk/collection/P03/current/G050/> ;
    owl:deprecated "false" .
<http://vocab.nerc.ac.uk/collection/P02/current/MDSD/> a glbase:MeasurementType,
        owl:Class,
        owl:NamedIndividual ;
    rdfs:label "Trace metalloid concentrations in sediment"@en ;
    dcterms:creator "SeaDataNet" ;
    dcterms:date "2010-11-05 12:10:54.0" ;
    glbase:hasIdentifier [ glbase:hasIdentifierScheme idscheme:sdn ;
            glbase:hasIdentifierValue "SDN:P02::MDSD" ] ;
    rdfs:comment "Concentration parameters for metalloid elements in sediment.  Sediment is understood to be the solid phase of the bed, including the recently settled material sometimes known as fluff collected from the bed surface. Metalloids are considered as B, Ge, As, Sb, Te and Po (but not Si which is classed separately because of its major role in environmental chemistry)"@en ;
    rdfs:subClassOf <http://vocab.nerc.ac.uk/collection/P02/current/RMIN/> ;
    owl:deprecated "true" .
<http://vocab.nerc.ac.uk/collection/P02/current/MDSV/> a glbase:MeasurementType,
        owl:Class,
        owl:NamedIndividual ;
    rdfs:label "Suspended particulate material setting velocity parameters"@en ;
    dcterms:creator "SeaDataNet" ;
    dcterms:date "2004-05-27 16:23:12.0" ;
    glbase:hasIdentifier [ glbase:hasIdentifierScheme idscheme:sdn ;
            glbase:hasIdentifierValue "SDN:P02::MDSV" ] ;
    rdfs:comment "" ;
    rdfs:subClassOf <http://vocab.nerc.ac.uk/collection/P03/current/G015/> ;
    owl:deprecated "false" .
<http://vocab.nerc.ac.uk/collection/P02/current/MDWD/> a glbase:MeasurementType,
        owl:Class,
        owl:NamedIndividual ;
    rdfs:label "Dissolved trace metalloid concentrations in the water column"@en ;
    dcterms:creator "SeaDataNet" ;
    dcterms:date "2010-01-27 14:18:10.0" ;
    glbase:hasIdentifier [ glbase:hasIdentifierScheme idscheme:sdn ;
            glbase:hasIdentifierValue "SDN:P02::MDWD" ] ;
    rdfs:comment "Concentration parameters for trace metalloid elements in the dissolved phase of the water column.  This may include a contribution from the particulate phase if this has not been totally removed by filtration and the metal in question is reactive (ie detected as if it were dissolved) to the analytical technique used. Trace metalloids are considered as B, Ge, As, Sb, Te and Po (but not Si which is classed separately because of its major role in environmental chemistry)"@en ;
    rdfs:subClassOf <http://vocab.nerc.ac.uk/collection/P03/current/C035/> ;
    owl:deprecated "false" .
<http://vocab.nerc.ac.uk/collection/P02/current/MDWP/> a glbase:MeasurementType,
        owl:Class,
        owl:NamedIndividual ;
    rdfs:label "Particulate trace metalloid concentrations in the water column"@en ;
    dcterms:creator "SeaDataNet" ;
    dcterms:date "2010-01-27 14:18:10.0" ;
    glbase:hasIdentifier [ glbase:hasIdentifierScheme idscheme:sdn ;
            glbase:hasIdentifierValue "SDN:P02::MDWP" ] ;
    rdfs:comment "Concentration parameters for trace metalloid elements in the particulate phase of the water column collected by fitration, centrifugation or sediment trapping. Trace metalloids are considered as B, Ge, As, Sb, Te and Po (but not Si which is classed separately because of its major role in environmental chemistry)"@en ;
    rdfs:subClassOf <http://vocab.nerc.ac.uk/collection/P03/current/C035/>,
        <http://vocab.nerc.ac.uk/collection/P03/current/G015/> ;
    owl:deprecated "false" .
<http://vocab.nerc.ac.uk/collection/P02/current/MEPH/> a glbase:MeasurementType,
        owl:Class,
        owl:NamedIndividual ;
    rdfs:label "Zooplankton egg hatch proportion"@en ;
    dcterms:creator "SeaDataNet" ;
    dcterms:date "2003-08-08 13:43:14.0" ;
    glbase:hasIdentifier [ glbase:hasIdentifierScheme idscheme:sdn ;
            glbase:hasIdentifierValue "SDN:P02::MEPH" ] ;
    rdfs:comment "" ;
    rdfs:subClassOf <http://vocab.nerc.ac.uk/collection/P03/current/B045/> ;
    owl:deprecated "false" .
<http://vocab.nerc.ac.uk/collection/P02/current/MFAB/> a glbase:MeasurementType,
        owl:Class,
        owl:NamedIndividual ;
    rdfs:label "Zoobenthos generic abundance"@en ;
    dcterms:creator "SeaDataNet" ;
    dcterms:date "2010-10-22 10:08:34.0" ;
    glbase:hasIdentifier [ glbase:hasIdentifierScheme idscheme:sdn ;
            glbase:hasIdentifierValue "SDN:P02::MFAB" ] ;
    rdfs:comment "Any enumeration (e.g. count, number per square metre) of animals living on or near the seabed designated by terms other than taxonomic names (e.g. total)."@en ;
    rdfs:subClassOf <http://vocab.nerc.ac.uk/collection/P03/current/B070/>,
        <http://vocab.nerc.ac.uk/collection/P03/current/G055/> ;
    owl:deprecated "false" .
<http://vocab.nerc.ac.uk/collection/P02/current/MFAZ/> a glbase:MeasurementType,
        owl:Class,
        owl:NamedIndividual ;
    rdfs:label "Zoobenthos taxonomy-related ash-free dry weight biomass per unit area of the littoral zone"@en ;
    dcterms:creator "SeaDataNet" ;
    dcterms:date "2015-04-08 15:23:44.0" ;
    glbase:hasIdentifier [ glbase:hasIdentifierScheme idscheme:sdn ;
            glbase:hasIdentifierValue "SDN:P02::MFAZ" ] ;
    rdfs:comment "Any zoobenthos ash-free dry weight biomass per unit area of the littoral zone (between spring tide high and low water) parameters that are not fish or terrestrial animals (insecta/oligochaeta)"@en ;
    rdfs:subClassOf <http://vocab.nerc.ac.uk/collection/P03/current/B070/>,
        <http://vocab.nerc.ac.uk/collection/P03/current/G055/> ;
    owl:deprecated "true" .
<http://vocab.nerc.ac.uk/collection/P02/current/MFLZ/> a glbase:MeasurementType,
        owl:Class,
        owl:NamedIndividual ;
    rdfs:label "Zoobenthos taxonomy-related abundance per unit area of the littoral zone"@en ;
    dcterms:creator "SeaDataNet" ;
    dcterms:date "2015-04-08 15:22:45.0" ;
    glbase:hasIdentifier [ glbase:hasIdentifierScheme idscheme:sdn ;
            glbase:hasIdentifierValue "SDN:P02::MFLZ" ] ;
    rdfs:comment "Any zoobenthos abundance per unit area of the littoral zone (between spring tide high and low water) parameters that are not fish or terrestrial animals (insecta/oligochaeta)"@en ;
    rdfs:subClassOf <http://vocab.nerc.ac.uk/collection/P03/current/B070/>,
        <http://vocab.nerc.ac.uk/collection/P03/current/G055/> ;
    owl:deprecated "true" .
<http://vocab.nerc.ac.uk/collection/P02/current/MFWW/> a glbase:MeasurementType,
        owl:Class,
        owl:NamedIndividual ;
    rdfs:label "Zoobenthos non taxonomy-related wet weight biomass per unit area of the bed"@en ;
    dcterms:creator "SeaDataNet" ;
    dcterms:date "2004-04-26 15:17:17.0" ;
    glbase:hasIdentifier [ glbase:hasIdentifierScheme idscheme:sdn ;
            glbase:hasIdentifierValue "SDN:P02::MFWW" ] ;
    rdfs:comment "Any zoobenthos wet weight biomass per unit area of the seabed parameters that are not included in parameter group ZWTX."@en ;
    rdfs:subClassOf <http://vocab.nerc.ac.uk/collection/P03/current/B070/>,
        <http://vocab.nerc.ac.uk/collection/P03/current/G055/> ;
    owl:deprecated "false" .
<http://vocab.nerc.ac.uk/collection/P02/current/MINC/> a glbase:MeasurementType,
        owl:Class,
        owl:NamedIndividual ;
    rdfs:label "Mineral chemistry"@en ;
    dcterms:creator "SeaDataNet" ;
    dcterms:date "2007-09-24 16:12:07.0" ;
    glbase:hasIdentifier [ glbase:hasIdentifierScheme idscheme:sdn ;
            glbase:hasIdentifierValue "SDN:P02::MINC" ] ;
    rdfs:comment "Chemical analyses of minerals extracted from rocks or sediment or analysed in-situ using techniques like the electron microprobe."@en ;
    rdfs:subClassOf <http://vocab.nerc.ac.uk/collection/P03/current/G035/>,
        <http://vocab.nerc.ac.uk/collection/P03/current/G045/> ;
    owl:deprecated "false" .
<http://vocab.nerc.ac.uk/collection/P02/current/MLES/> a glbase:MeasurementType,
        owl:Class,
        owl:NamedIndividual ;
    rdfs:label "Marine environment leisure usage"@en ;
    dcterms:creator "SeaDataNet" ;
    dcterms:date "2011-10-27 15:00:57.0" ;
    glbase:hasIdentifier [ glbase:hasIdentifierScheme idscheme:sdn ;
            glbase:hasIdentifierValue "SDN:P02::MLES" ] ;
    rdfs:comment "Parameters quantifying the extent and nature of recreational activities in coastal waters, estuaries and their margins such as beaches."@en ;
    rdfs:subClassOf <http://vocab.nerc.ac.uk/collection/P03/current/H005/> ;
    owl:deprecated "false" .
<http://vocab.nerc.ac.uk/collection/P02/current/MLFX/> a glbase:MeasurementType,
        owl:Class,
        owl:NamedIndividual ;
    rdfs:label "Sedimentation flux of metallic and metalloid elements and isotopes in water bodies"@en ;
    dcterms:creator "SeaDataNet" ;
    dcterms:date "2011-10-18 14:30:54.0" ;
    glbase:hasIdentifier [ glbase:hasIdentifierScheme idscheme:sdn ;
            glbase:hasIdentifierValue "SDN:P02::MLFX" ] ;
    rdfs:comment "Parameters quantifying metal and metalloid fluxes as element concentration or isotope activities per unit area per unit time"@en ;
    rdfs:subClassOf <http://vocab.nerc.ac.uk/collection/P03/current/O005/> ;
    owl:deprecated "false" .
<http://vocab.nerc.ac.uk/collection/P02/current/MMAN/> a glbase:MeasurementType,
        owl:Class,
        owl:NamedIndividual ;
    rdfs:label "Magnetics"@en ;
    dcterms:creator "SeaDataNet" ;
    dcterms:date "2010-10-22 13:34:10.0" ;
    glbase:hasIdentifier [ glbase:hasIdentifierScheme idscheme:sdn ;
            glbase:hasIdentifierValue "SDN:P02::MMAN" ] ;
    rdfs:comment "Parameterisations of the intensity and inclination of Earth's magnetic field"@en ;
    rdfs:subClassOf <http://vocab.nerc.ac.uk/collection/P03/current/G005/>,
        <http://vocab.nerc.ac.uk/collection/P03/current/GPYS/> ;
    owl:deprecated "false" .
<http://vocab.nerc.ac.uk/collection/P02/current/MMST/> a glbase:MeasurementType,
        owl:Class,
        owl:NamedIndividual ;
    rdfs:label "Man-made structures"@en ;
    dcterms:creator "SeaDataNet" ;
    dcterms:date "2008-01-30 07:53:20.0" ;
    glbase:hasIdentifier [ glbase:hasIdentifierScheme idscheme:sdn ;
            glbase:hasIdentifierValue "SDN:P02::MMST" ] ;
    rdfs:comment "Parameters relating to human built structures on the coast or offshore and their impact on the environment."@en ;
    rdfs:subClassOf <http://vocab.nerc.ac.uk/collection/P03/current/H002/> ;
    owl:deprecated "false" .
<http://vocab.nerc.ac.uk/collection/P02/current/MNGS/> a glbase:MeasurementType,
        owl:Class,
        owl:NamedIndividual ;
    rdfs:label "Sediment grain size parameters"@en ;
    dcterms:creator "SeaDataNet" ;
    dcterms:date "2010-02-19 12:03:05.0" ;
    glbase:hasIdentifier [ glbase:hasIdentifierScheme idscheme:sdn ;
            glbase:hasIdentifierValue "SDN:P02::MNGS" ] ;
    rdfs:comment "Parameters specifying the physical dimensions of the particles comprising unlithified sediment (including expressions of shape such as aspect ratio) and statistics derived from their variation in a sample (e.g. mean, mode, sorting, skewness)."@en ;
    rdfs:subClassOf <http://vocab.nerc.ac.uk/collection/P03/current/G040/> ;
    owl:deprecated "false" .
<http://vocab.nerc.ac.uk/collection/P02/current/MPMN/> a glbase:MeasurementType,
        owl:Class,
        owl:NamedIndividual ;
    rdfs:label "Moored instrument depth"@en ;
    dcterms:creator "SeaDataNet" ;
    dcterms:date "2004-08-17 09:22:00.0" ;
    glbase:hasIdentifier [ glbase:hasIdentifierScheme idscheme:sdn ;
            glbase:hasIdentifierValue "SDN:P02::MPMN" ] ;
    rdfs:comment "Parameters expressing depth (possibly as pressure) of an instrument on a suspended underwater mooring.  These are primarily collected to monitor mooring performance by quantifying knock-down and should not be regarded as instrument z co-ordinates (accurate calibration is rare) or as sea level measurements."@en ;
    rdfs:subClassOf <http://vocab.nerc.ac.uk/collection/P03/current/Z005/> ;
    owl:deprecated "false" .
<http://vocab.nerc.ac.uk/collection/P02/current/MSBD/> a glbase:MeasurementType,
        owl:Class,
        owl:NamedIndividual ;
    rdfs:label "Zooplankton dry weight biomass per unit volume of the water column"@en ;
    dcterms:creator "SeaDataNet" ;
    dcterms:date "2004-04-23 09:17:15.0" ;
    glbase:hasIdentifier [ glbase:hasIdentifierScheme idscheme:sdn ;
            glbase:hasIdentifierValue "SDN:P02::MSBD" ] ;
    rdfs:comment "Zooplankton (mesozooplankton and larger, exclusing fish, mammals, reptiles and insects) biomass determined by drying to constant weight."@en ;
    rdfs:subClassOf <http://vocab.nerc.ac.uk/collection/P03/current/B045/>,
        <http://vocab.nerc.ac.uk/collection/P03/current/B070/> ;
    owl:deprecated "false" .
<http://vocab.nerc.ac.uk/collection/P02/current/MSBO/> a glbase:MeasurementType,
        owl:Class,
        owl:NamedIndividual ;
    rdfs:label "Zooplankton ash-free dry weight biomass per unit volume of the water column"@en ;
    dcterms:creator "SeaDataNet" ;
    dcterms:date "2004-04-23 09:13:58.0" ;
    glbase:hasIdentifier [ glbase:hasIdentifierScheme idscheme:sdn ;
            glbase:hasIdentifierValue "SDN:P02::MSBO" ] ;
    rdfs:comment "Zooplankton (mesozooplankton and larger, exclusing fish, mammals, reptiles and insects) biomass determined by gravimetric measurement of loss on ignition"@en ;
    rdfs:subClassOf <http://vocab.nerc.ac.uk/collection/P03/current/B045/>,
        <http://vocab.nerc.ac.uk/collection/P03/current/B070/> ;
    owl:deprecated "false" .
<http://vocab.nerc.ac.uk/collection/P02/current/MSEP/> a glbase:MeasurementType,
        owl:Class,
        owl:NamedIndividual ;
    rdfs:label "Zooplankton reproduction rate parameters"@en ;
    dcterms:creator "SeaDataNet" ;
    dcterms:date "2003-06-10 13:53:19.0" ;
    glbase:hasIdentifier [ glbase:hasIdentifierScheme idscheme:sdn ;
            glbase:hasIdentifierValue "SDN:P02::MSEP" ] ;
    rdfs:comment "All parameters related to zooplankton reproduction rates"@en ;
    rdfs:subClassOf <http://vocab.nerc.ac.uk/collection/P03/current/B045/>,
        <http://vocab.nerc.ac.uk/collection/P03/current/O010/> ;
    owl:deprecated "false" .
<http://vocab.nerc.ac.uk/collection/P02/current/MSFX/> a glbase:MeasurementType,
        owl:Class,
        owl:NamedIndividual ;
    rdfs:label "Sedimentation flux quantification in the water column"@en ;
    dcterms:creator "SeaDataNet" ;
    dcterms:date "2004-08-19 09:28:07.0" ;
    glbase:hasIdentifier [ glbase:hasIdentifierScheme idscheme:sdn ;
            glbase:hasIdentifierValue "SDN:P02::MSFX" ] ;
    rdfs:comment "Parameters expressing the total sedimentation flux in terms of particle mass, volume or counts"@en ;
    rdfs:subClassOf <http://vocab.nerc.ac.uk/collection/P03/current/O005/> ;
    owl:deprecated "false" .
<http://vocab.nerc.ac.uk/collection/P02/current/MSIC/> a glbase:MeasurementType,
        owl:Class,
        owl:NamedIndividual ;
    rdfs:label "Zooplankton carbon biomass per unit area of the water column"@en ;
    dcterms:creator "SeaDataNet" ;
    dcterms:date "2003-06-10 13:53:19.0" ;
    glbase:hasIdentifier [ glbase:hasIdentifierScheme idscheme:sdn ;
            glbase:hasIdentifierValue "SDN:P02::MSIC" ] ;
    rdfs:comment "Integrated zooplankton (mesozooplankton and larger, exclusing fish, mammals, reptiles and insects) carbon biomass parameters"@en ;
    rdfs:subClassOf <http://vocab.nerc.ac.uk/collection/P03/current/B045/>,
        <http://vocab.nerc.ac.uk/collection/P03/current/B070/> ;
    owl:deprecated "false" .
<http://vocab.nerc.ac.uk/collection/P02/current/MTAT/> a glbase:MeasurementType,
        owl:Class,
        owl:NamedIndividual ;
    rdfs:label "Metal concentrations in the atmosphere"@en ;
    dcterms:creator "SeaDataNet" ;
    dcterms:date "2008-09-12 08:42:00.0" ;
    glbase:hasIdentifier [ glbase:hasIdentifierScheme idscheme:sdn ;
            glbase:hasIdentifierValue "SDN:P02::MTAT" ] ;
    rdfs:comment "Concentration of metal elements in any phase of the atmosphere"@en ;
    rdfs:subClassOf <http://vocab.nerc.ac.uk/collection/P03/current/C035/>,
        <http://vocab.nerc.ac.uk/collection/P03/current/M005/> ;
    owl:deprecated "false" .
<http://vocab.nerc.ac.uk/collection/P02/current/MTIC/> a glbase:MeasurementType,
        owl:Class,
        owl:NamedIndividual ;
    rdfs:label "Metal concentrations in the cryosphere"@en ;
    dcterms:creator "SeaDataNet" ;
    dcterms:date "2008-09-12 08:48:26.0" ;
    glbase:hasIdentifier [ glbase:hasIdentifierScheme idscheme:sdn ;
            glbase:hasIdentifierValue "SDN:P02::MTIC" ] ;
    rdfs:comment "Concentration parameters for metallic elements in ice and snow"@en ;
    rdfs:subClassOf <http://vocab.nerc.ac.uk/collection/P03/current/C035/>,
        <http://vocab.nerc.ac.uk/collection/P03/current/M015/> ;
    owl:deprecated "false" .
<http://vocab.nerc.ac.uk/collection/P02/current/MTPW/> a glbase:MeasurementType,
        owl:Class,
        owl:NamedIndividual ;
    rdfs:label "Metal concentrations in sediment pore waters"@en ;
    dcterms:creator "SeaDataNet" ;
    dcterms:date "2004-05-12 10:25:00.0" ;
    glbase:hasIdentifier [ glbase:hasIdentifierScheme idscheme:sdn ;
            glbase:hasIdentifierValue "SDN:P02::MTPW" ] ;
    rdfs:comment "Concentrations of metal elements in sediment pore waters"@en ;
    rdfs:subClassOf <http://vocab.nerc.ac.uk/collection/P03/current/C035/>,
        <http://vocab.nerc.ac.uk/collection/P03/current/G050/> ;
    owl:deprecated "false" .
<http://vocab.nerc.ac.uk/collection/P02/current/MTSD/> a glbase:MeasurementType,
        owl:Class,
        owl:NamedIndividual ;
    rdfs:label "Metal concentrations in sediment"@en ;
    dcterms:creator "SeaDataNet" ;
    dcterms:date "2010-11-05 10:42:04.0" ;
    glbase:hasIdentifier [ glbase:hasIdentifierScheme idscheme:sdn ;
            glbase:hasIdentifierValue "SDN:P02::MTSD" ] ;
    rdfs:comment "Concentrations of metal elements per unit weight of sediment.  Sediment is understood to be the solid phase of the bed, including the recently settled material sometimes known as fluff collected from the bed surface."@en ;
    rdfs:subClassOf <http://vocab.nerc.ac.uk/collection/P02/current/RMIN/> ;
    owl:deprecated "true" .
<http://vocab.nerc.ac.uk/collection/P02/current/MTWC/> a glbase:MeasurementType,
        owl:Class,
        owl:NamedIndividual ;
    rdfs:label "Colloidal metal concentrations in the water column"@en ;
    dcterms:creator "SeaDataNet" ;
    dcterms:date "2004-05-12 12:00:00.0" ;
    glbase:hasIdentifier [ glbase:hasIdentifierScheme idscheme:sdn ;
            glbase:hasIdentifierValue "SDN:P02::MTWC" ] ;
    rdfs:comment "Concentrations of metal elements in the colloidal phase of the water column. Usually the dissolved concentration difference between conventionally filtered water and ultra-filtered water."@en ;
    rdfs:subClassOf <http://vocab.nerc.ac.uk/collection/P03/current/C035/> ;
    owl:deprecated "false" .
<http://vocab.nerc.ac.uk/collection/P02/current/MTWD/> a glbase:MeasurementType,
        owl:Class,
        owl:NamedIndividual ;
    rdfs:label "Dissolved metal concentrations in the water column"@en ;
    dcterms:creator "SeaDataNet" ;
    dcterms:date "2004-05-12 11:35:00.0" ;
    glbase:hasIdentifier [ glbase:hasIdentifierScheme idscheme:sdn ;
            glbase:hasIdentifierValue "SDN:P02::MTWD" ] ;
    rdfs:comment "Concentrations of metal elements in the dissolved phase of the water column.  This may include a contribution from the particulate phase if this has not been totally removed by filtration and the metal in question is reactive (ie detected as if it were dissolved) to the analytical technique used."@en ;
    rdfs:subClassOf <http://vocab.nerc.ac.uk/collection/P03/current/C035/> ;
    owl:deprecated "false" .
<http://vocab.nerc.ac.uk/collection/P02/current/MTWT/> a glbase:MeasurementType,
        owl:Class,
        owl:NamedIndividual ;
    rdfs:label "Total metal concentrations in water bodies"@en ;
    dcterms:creator "SeaDataNet" ;
    dcterms:date "2010-01-27 14:25:50.0" ;
    glbase:hasIdentifier [ glbase:hasIdentifierScheme idscheme:sdn ;
            glbase:hasIdentifierValue "SDN:P02::MTWT" ] ;
    rdfs:comment "Concentration parameters for metal elements in the combined dissolved and particulate phases of any body of fresh or salt water."@en ;
    rdfs:subClassOf <http://vocab.nerc.ac.uk/collection/P03/current/C035/> ;
    owl:deprecated "false" .
<http://vocab.nerc.ac.uk/collection/P02/current/MXLM/> a glbase:MeasurementType,
        owl:Class,
        owl:NamedIndividual ;
    rdfs:label "Structure and stability of the water column"@en ;
    dcterms:creator "SeaDataNet" ;
    dcterms:date "2004-08-16 11:54:33.0" ;
    glbase:hasIdentifier [ glbase:hasIdentifierScheme idscheme:sdn ;
            glbase:hasIdentifierValue "SDN:P02::MXLM" ] ;
    rdfs:comment "Parameters describing or predicting water column structure plus parameters quantifying the dynamic stability of that structure"@en ;
    rdfs:subClassOf <http://vocab.nerc.ac.uk/collection/P03/current/D020/> ;
    owl:deprecated "false" .
<http://vocab.nerc.ac.uk/collection/P02/current/MZBC/> a glbase:MeasurementType,
        owl:Class,
        owl:NamedIndividual ;
    rdfs:label "Microzooplankton non taxonomy-related biomass expressed as carbon per unit volume of the water column"@en ;
    dcterms:creator "SeaDataNet" ;
    dcterms:date "2004-04-19 15:25:41.0" ;
    glbase:hasIdentifier [ glbase:hasIdentifierScheme idscheme:sdn ;
            glbase:hasIdentifierValue "SDN:P02::MZBC" ] ;
    rdfs:comment "Basically, any microzooplankton carbon biomass measurement that isn't included in parameter group MATC.  May include data integrations such as 'total microzooplankton'."@en ;
    rdfs:subClassOf <http://vocab.nerc.ac.uk/collection/P03/current/B025/>,
        <http://vocab.nerc.ac.uk/collection/P03/current/B070/> ;
    owl:deprecated "false" .
<http://vocab.nerc.ac.uk/collection/P02/current/MZBN/> a glbase:MeasurementType,
        owl:Class,
        owl:NamedIndividual ;
    rdfs:label "Microzooplankton generic abundance in water bodies"@en ;
    dcterms:creator "SeaDataNet" ;
    dcterms:date "2010-10-22 10:06:41.0" ;
    glbase:hasIdentifier [ glbase:hasIdentifierScheme idscheme:sdn ;
            glbase:hasIdentifierValue "SDN:P02::MZBN" ] ;
    rdfs:comment "Any enumeration (e.g. count, number per litre) of microzooplankton (free swimming heterotrophic organisms smaller than 200um) designated by terms other than taxonomic names (e.g. total) in any fresh or salt water body."@en ;
    rdfs:subClassOf <http://vocab.nerc.ac.uk/collection/P03/current/B025/>,
        <http://vocab.nerc.ac.uk/collection/P03/current/B070/> ;
    owl:deprecated "false" .
<http://vocab.nerc.ac.uk/collection/P02/current/MZCT/> a glbase:MeasurementType,
        owl:Class,
        owl:NamedIndividual ;
    rdfs:label "Microzooplankton grazing"@en ;
    dcterms:creator "SeaDataNet" ;
    dcterms:date "2004-04-19 15:35:55.0" ;
    glbase:hasIdentifier [ glbase:hasIdentifierScheme idscheme:sdn ;
            glbase:hasIdentifierValue "SDN:P02::MZCT" ] ;
    rdfs:comment "Parameters that express the consumption of the phytoplankton population by the microzooplankton.  Generally the results of dilution experiments on water samples screened through a 200-micron mesh."@en ;
    rdfs:subClassOf <http://vocab.nerc.ac.uk/collection/P03/current/B025/>,
        <http://vocab.nerc.ac.uk/collection/P03/current/O010/> ;
    owl:deprecated "false" .
<http://vocab.nerc.ac.uk/collection/P02/current/NOYS/> a glbase:MeasurementType,
        owl:Class,
        owl:NamedIndividual ;
    rdfs:label "Acoustic noise in the water column"@en ;
    dcterms:creator "SeaDataNet" ;
    dcterms:date "2003-06-10 13:53:19.0" ;
    glbase:hasIdentifier [ glbase:hasIdentifierScheme idscheme:sdn ;
            glbase:hasIdentifierValue "SDN:P02::NOYS" ] ;
    rdfs:comment "" ;
    rdfs:subClassOf <http://vocab.nerc.ac.uk/collection/P03/current/D005/> ;
    owl:deprecated "false" .
<http://vocab.nerc.ac.uk/collection/P02/current/NTIC/> a glbase:MeasurementType,
        owl:Class,
        owl:NamedIndividual ;
    rdfs:label "Concentration of nitrates in ice"@en ;
    dcterms:creator "SeaDataNet" ;
    dcterms:date "2011-02-18 14:34:22.0" ;
    glbase:hasIdentifier [ glbase:hasIdentifierScheme idscheme:sdn ;
            glbase:hasIdentifierValue "SDN:P02::NTIC" ] ;
    rdfs:comment "Nitrate concentration parameters in ice. Includes nitrate+nitrite, which is often loosely referred to as nitrate."@en ;
    rdfs:subClassOf <http://vocab.nerc.ac.uk/collection/P02/current/ICHM/> ;
    owl:deprecated "true" .
<http://vocab.nerc.ac.uk/collection/P02/current/NTOT/> a glbase:MeasurementType,
        owl:Class,
        owl:NamedIndividual ;
    rdfs:label "Particulate total and organic nitrogen concentrations in the water column"@en ;
    dcterms:creator "SeaDataNet" ;
    dcterms:date "2004-08-02 14:06:46.0" ;
    glbase:hasIdentifier [ glbase:hasIdentifierScheme idscheme:sdn ;
            glbase:hasIdentifierValue "SDN:P02::NTOT" ] ;
    rdfs:comment "Concentrations of total and organic nitrogen in the particulate phase of the water column, which is a function of both the SPM concentration in the water column and the concentration of nitrogen per unit weight of SPM. Note that it is commonly assumed that all particulate nitrogen is organic."@en ;
    rdfs:subClassOf <http://vocab.nerc.ac.uk/collection/P03/current/C005/> ;
    owl:deprecated "false" .
<http://vocab.nerc.ac.uk/collection/P02/current/NTPW/> a glbase:MeasurementType,
        owl:Class,
        owl:NamedIndividual ;
    rdfs:label "Nutrient concentrations in sediment pore waters"@en ;
    dcterms:creator "SeaDataNet" ;
    dcterms:date "2004-05-27 09:00:00.0" ;
    glbase:hasIdentifier [ glbase:hasIdentifierScheme idscheme:sdn ;
            glbase:hasIdentifierValue "SDN:P02::NTPW" ] ;
    rdfs:comment "Nutrient (nitrate, nitrite, ammonium, phosphate, silicate and urea) concentrations in sediment pore waters"@en ;
    rdfs:subClassOf <http://vocab.nerc.ac.uk/collection/P03/current/C040/>,
        <http://vocab.nerc.ac.uk/collection/P03/current/G050/> ;
    owl:deprecated "false" .
<http://vocab.nerc.ac.uk/collection/P02/current/NTRI/> a glbase:MeasurementType,
        owl:Class,
        owl:NamedIndividual ;
    rdfs:label "Nitrite concentration parameters in the water column"@en ;
    dcterms:creator "SeaDataNet" ;
    dcterms:date "2004-05-27 09:51:38.0" ;
    glbase:hasIdentifier [ glbase:hasIdentifierScheme idscheme:sdn ;
            glbase:hasIdentifierValue "SDN:P02::NTRI" ] ;
    rdfs:comment "Nitrite concentration parameters (including statistical parameters such as standard deviation) in the water column"@en ;
    rdfs:subClassOf <http://vocab.nerc.ac.uk/collection/P03/current/C005/>,
        <http://vocab.nerc.ac.uk/collection/P03/current/C040/> ;
    owl:deprecated "false" .
<http://vocab.nerc.ac.uk/collection/P02/current/NTRZ/> a glbase:MeasurementType,
        owl:Class,
        owl:NamedIndividual ;
    rdfs:label "Nitrate+nitrite concentration parameters in the water column"@en ;
    dcterms:creator "SeaDataNet" ;
    dcterms:date "2008-11-19 15:18:24.0" ;
    glbase:hasIdentifier [ glbase:hasIdentifierScheme idscheme:sdn ;
            glbase:hasIdentifierValue "SDN:P02::NTRZ" ] ;
    rdfs:comment "Deprecated term from a misguided attempt to distinguish between NO3 and NO3+NO2 for discovery. Use parameter group NTRA instead"@en ;
    rdfs:subClassOf <http://vocab.nerc.ac.uk/collection/P02/current/NTRA/> ;
    owl:deprecated "true" .
<http://vocab.nerc.ac.uk/collection/P02/current/NTSD/> a glbase:MeasurementType,
        owl:Class,
        owl:NamedIndividual ;
    rdfs:label "Nitrogen concentrations in sediment"@en ;
    dcterms:creator "SeaDataNet" ;
    dcterms:date "2004-08-02 12:43:00.0" ;
    glbase:hasIdentifier [ glbase:hasIdentifierScheme idscheme:sdn ;
            glbase:hasIdentifierValue "SDN:P02::NTSD" ] ;
    rdfs:comment "Concentrations of total, organic and inorganic nitrogen per unit weight of sediment.  Sediment is understood to be the solid phase of the bed, including the recently settled material sometimes known as fluff collected from the bed surface."@en ;
    rdfs:subClassOf <http://vocab.nerc.ac.uk/collection/P03/current/C005/>,
        <http://vocab.nerc.ac.uk/collection/P03/current/G035/> ;
    owl:deprecated "false" .
<http://vocab.nerc.ac.uk/collection/P02/current/NTSP/> a glbase:MeasurementType,
        owl:Class,
        owl:NamedIndividual ;
    rdfs:label "Nitrogen concentrations in suspended particulate material"@en ;
    dcterms:creator "SeaDataNet" ;
    dcterms:date "2004-08-02 12:35:00.0" ;
    glbase:hasIdentifier [ glbase:hasIdentifierScheme idscheme:sdn ;
            glbase:hasIdentifierValue "SDN:P02::NTSP" ] ;
    rdfs:comment "Concentrations of total, organic and inorganic nitrogen per unit weight of suspended particulate material collected by water column filtration, centrifugation or sediment trapping.  Note that it is common practice to assume all nitrogen in SPM is organic."@en ;
    rdfs:subClassOf <http://vocab.nerc.ac.uk/collection/P03/current/C005/>,
        <http://vocab.nerc.ac.uk/collection/P03/current/G015/> ;
    owl:deprecated "false" .
<http://vocab.nerc.ac.uk/collection/P02/current/NTUP/> a glbase:MeasurementType,
        owl:Class,
        owl:NamedIndividual ;
    rdfs:label "New production in water bodies"@en ;
    dcterms:creator "SeaDataNet" ;
    dcterms:date "2009-11-15 16:11:26.0" ;
    glbase:hasIdentifier [ glbase:hasIdentifierScheme idscheme:sdn ;
            glbase:hasIdentifierValue "SDN:P02::NTUP" ] ;
    rdfs:comment "Parameters quantifying the uptake rate of nitrate or gaseous nitrogen by flora and fauna living in any body of salt or fresh water"@en ;
    rdfs:subClassOf <http://vocab.nerc.ac.uk/collection/P03/current/C040/>,
        <http://vocab.nerc.ac.uk/collection/P03/current/O010/> ;
    owl:deprecated "false" .
<http://vocab.nerc.ac.uk/collection/P02/current/NUTV/> a glbase:MeasurementType,
        owl:Class,
        owl:NamedIndividual ;
    rdfs:label "Raw in-situ nutrient analyser output"@en ;
    dcterms:creator "SeaDataNet" ;
    dcterms:date "2005-07-08 16:15:08.0" ;
    glbase:hasIdentifier [ glbase:hasIdentifierScheme idscheme:sdn ;
            glbase:hasIdentifierValue "SDN:P02::NUTV" ] ;
    rdfs:comment "Direct output parameters from spectophotometric or chemical in-situ nutrient analysers"@en ;
    rdfs:subClassOf <http://vocab.nerc.ac.uk/collection/P03/current/C040/> ;
    owl:deprecated "false" .
<http://vocab.nerc.ac.uk/collection/P02/current/OCAA/> a glbase:MeasurementType,
        owl:Class,
        owl:NamedIndividual ;
    rdfs:label "Concentration of other organic contaminants in the atmosphere"@en ;
    dcterms:creator "SeaDataNet" ;
    dcterms:date "2008-12-09 10:17:11.0" ;
    glbase:hasIdentifier [ glbase:hasIdentifierScheme idscheme:sdn ;
            glbase:hasIdentifierValue "SDN:P02::OCAA" ] ;
    rdfs:comment "Parameters quantifying concentrations of organic contaminants (substances regarded as harmful) other than PCBs and PAHs in all phases of the atmosphere"@en ;
    rdfs:subClassOf <http://vocab.nerc.ac.uk/collection/P03/current/H001/>,
        <http://vocab.nerc.ac.uk/collection/P03/current/M005/> ;
    owl:deprecated "false" .
<http://vocab.nerc.ac.uk/collection/P02/current/OCPW/> a glbase:MeasurementType,
        owl:Class,
        owl:NamedIndividual ;
    rdfs:label "Dissolved organic carbon concentrations in sediment pore waters"@en ;
    dcterms:creator "SeaDataNet" ;
    dcterms:date "2004-05-27 09:00:00.0" ;
    glbase:hasIdentifier [ glbase:hasIdentifierScheme idscheme:sdn ;
            glbase:hasIdentifierValue "SDN:P02::OCPW" ] ;
    rdfs:comment "Concentrations of dissolved organic carbon in sediment pore waters"@en ;
    rdfs:subClassOf <http://vocab.nerc.ac.uk/collection/P03/current/C005/>,
        <http://vocab.nerc.ac.uk/collection/P03/current/G050/> ;
    owl:deprecated "false" .
<http://vocab.nerc.ac.uk/collection/P02/current/OGPW/> a glbase:MeasurementType,
        owl:Class,
        owl:NamedIndividual ;
    rdfs:label "Dissolved concentration parameters for other gases in sediment pore waters"@en ;
    dcterms:creator "SeaDataNet" ;
    dcterms:date "2010-11-08 15:08:09.0" ;
    glbase:hasIdentifier [ glbase:hasIdentifierScheme idscheme:sdn ;
            glbase:hasIdentifierValue "SDN:P02::OGPW" ] ;
    rdfs:comment "All concentration parameters for inorganic dissolved gases other than oxygen and the noble gases in sediment pore water samples"@en ;
    rdfs:subClassOf <http://vocab.nerc.ac.uk/collection/P03/current/C015/> ;
    owl:deprecated "false" .
<http://vocab.nerc.ac.uk/collection/P02/current/OHAT/> a glbase:MeasurementType,
        owl:Class,
        owl:NamedIndividual ;
    rdfs:label "Concentration of other hydrocarbons in the atmosphere"@en ;
    dcterms:creator "SeaDataNet" ;
    dcterms:date "2010-11-08 15:08:09.0" ;
    glbase:hasIdentifier [ glbase:hasIdentifierScheme idscheme:sdn ;
            glbase:hasIdentifierValue "SDN:P02::OHAT" ] ;
    rdfs:comment "'Other' (not alkanes, alkenes, alkynes or PAHs) hydrocarbon concentration parameters (including saturation of gaseous species) in all phases of the atmosphere."@en ;
    rdfs:subClassOf <http://vocab.nerc.ac.uk/collection/P03/current/C025/>,
        <http://vocab.nerc.ac.uk/collection/P03/current/M005/> ;
    owl:deprecated "false" .
<http://vocab.nerc.ac.uk/collection/P02/current/OHWC/> a glbase:MeasurementType,
        owl:Class,
        owl:NamedIndividual ;
    rdfs:label "Concentration of other hydrocarbons in the water column"@en ;
    dcterms:creator "SeaDataNet" ;
    dcterms:date "2010-11-08 15:08:09.0" ;
    glbase:hasIdentifier [ glbase:hasIdentifierScheme idscheme:sdn ;
            glbase:hasIdentifierValue "SDN:P02::OHWC" ] ;
    rdfs:comment "'Other' (not alkanes, alkenes, alkynes or PAHs) hydrocarbon concentration parameters (including saturation of gaseous species) in all phases of the water column.  Does not include parameters expressed per unit weight of SPM."@en ;
    rdfs:subClassOf <http://vocab.nerc.ac.uk/collection/P03/current/C025/> ;
    owl:deprecated "false" .
<http://vocab.nerc.ac.uk/collection/P02/current/OMBI/> a glbase:MeasurementType,
        owl:Class,
        owl:NamedIndividual ;
    rdfs:label "Organometallic species concentration parameters in biota"@en ;
    dcterms:creator "SeaDataNet" ;
    dcterms:date "2010-05-19 10:55:30.0" ;
    glbase:hasIdentifier [ glbase:hasIdentifierScheme idscheme:sdn ;
            glbase:hasIdentifierValue "SDN:P02::OMBI" ] ;
    rdfs:comment "All measurements of the quantity or mass of any organometallic compound in any living organisms or their component parts"@en ;
    rdfs:subClassOf <http://vocab.nerc.ac.uk/collection/P03/current/B007/>,
        <http://vocab.nerc.ac.uk/collection/P03/current/C035/>,
        <http://vocab.nerc.ac.uk/collection/P03/current/C050/>,
        <http://vocab.nerc.ac.uk/collection/P03/current/C055/>,
        <http://vocab.nerc.ac.uk/collection/P03/current/H001/> ;
    owl:deprecated "false" .
<http://vocab.nerc.ac.uk/collection/P02/current/OMET/> a glbase:MeasurementType,
        owl:Class,
        owl:NamedIndividual ;
    rdfs:label "Other meteorological measurements"@en ;
    dcterms:creator "SeaDataNet" ;
    dcterms:date "2010-11-08 15:08:09.0" ;
    glbase:hasIdentifier [ glbase:hasIdentifierScheme idscheme:sdn ;
            glbase:hasIdentifierValue "SDN:P02::OMET" ] ;
    rdfs:comment "Bucket group for parameters that cannot be classified elsewhere"@en ;
    rdfs:subClassOf <http://vocab.nerc.ac.uk/collection/P03/current/M010/> ;
    owl:deprecated "false" .
<http://vocab.nerc.ac.uk/collection/P02/current/OMPW/> a glbase:MeasurementType,
        owl:Class,
        owl:NamedIndividual ;
    rdfs:label "Organometallic and organometalloid species concentration parameters in sediments"@en ;
    dcterms:creator "SeaDataNet" ;
    dcterms:date "2015-11-16 12:32:32.0" ;
    glbase:hasIdentifier [ glbase:hasIdentifierScheme idscheme:sdn ;
            glbase:hasIdentifierValue "SDN:P02::OMPW" ] ;
    rdfs:comment """All organometallic and orgamometalloid compound concentration parameters (including saturations for gaseous species) 
in all phases of sediments (including pore waters)"""@en ;
    rdfs:subClassOf <http://vocab.nerc.ac.uk/collection/P03/current/C035/>,
        <http://vocab.nerc.ac.uk/collection/P03/current/C050/>,
        <http://vocab.nerc.ac.uk/collection/P03/current/C055/>,
        <http://vocab.nerc.ac.uk/collection/P03/current/G035/>,
        <http://vocab.nerc.ac.uk/collection/P03/current/G050/>,
        <http://vocab.nerc.ac.uk/collection/P03/current/H001/> ;
    owl:deprecated "false" .
<http://vocab.nerc.ac.uk/collection/P02/current/OMWC/> a glbase:MeasurementType,
        owl:Class,
        owl:NamedIndividual ;
    rdfs:label "Organometallic and organometalloid species concentration parameters in water bodies"@en ;
    dcterms:creator "SeaDataNet" ;
    dcterms:date "2015-11-16 12:07:36.0" ;
    glbase:hasIdentifier [ glbase:hasIdentifierScheme idscheme:sdn ;
            glbase:hasIdentifierValue "SDN:P02::OMWC" ] ;
    rdfs:comment """All organometallic and organometalloid compound concentration parameters 
(including saturations for gaseous species) in all phases of any body of fresh or salt water."""@en ;
    rdfs:subClassOf <http://vocab.nerc.ac.uk/collection/P03/current/C035/>,
        <http://vocab.nerc.ac.uk/collection/P03/current/C050/>,
        <http://vocab.nerc.ac.uk/collection/P03/current/C055/>,
        <http://vocab.nerc.ac.uk/collection/P03/current/H001/> ;
    owl:deprecated "false" .
<http://vocab.nerc.ac.uk/collection/P02/current/OPBS/> a glbase:MeasurementType,
        owl:Class,
        owl:NamedIndividual ;
    rdfs:label "Optical backscatter"@en ;
    dcterms:creator "SeaDataNet" ;
    dcterms:date "2008-11-04 12:58:25.0" ;
    glbase:hasIdentifier [ glbase:hasIdentifierScheme idscheme:sdn ;
            glbase:hasIdentifierValue "SDN:P02::OPBS" ] ;
    rdfs:comment "Includes all parameters covering the strength of electromagnetic radiation signal return, including absolute measurements of returning signal strength as well as parameters expressed as backscatter (the proportion of transmitted signal returned)"@en ;
    rdfs:subClassOf <http://vocab.nerc.ac.uk/collection/P03/current/D015/> ;
    owl:deprecated "false" .
<http://vocab.nerc.ac.uk/collection/P02/current/OPCN/> a glbase:MeasurementType,
        owl:Class,
        owl:NamedIndividual ;
    rdfs:label "Concentration of silicon species in suspended particulate material"@en ;
    dcterms:creator "SeaDataNet" ;
    dcterms:date "2004-08-13 14:37:15.0" ;
    glbase:hasIdentifier [ glbase:hasIdentifierScheme idscheme:sdn ;
            glbase:hasIdentifierValue "SDN:P02::OPCN" ] ;
    rdfs:comment "Concentration parameters for silicon species (including opal) in SPM (material gathered by filtration or sediment trapping). Only includes parameters expressed per unit mass of SPM and not per unit volume of the water column"@en ;
    rdfs:subClassOf <http://vocab.nerc.ac.uk/collection/P03/current/C045/>,
        <http://vocab.nerc.ac.uk/collection/P03/current/G015/> ;
    owl:deprecated "false" .
<http://vocab.nerc.ac.uk/collection/P02/current/OPFX/> a glbase:MeasurementType,
        owl:Class,
        owl:NamedIndividual ;
    rdfs:label "Sedimentation flux of non-metallic inorganic species in the water column"@en ;
    dcterms:creator "SeaDataNet" ;
    dcterms:date "2006-06-13 09:18:26.0" ;
    glbase:hasIdentifier [ glbase:hasIdentifierScheme idscheme:sdn ;
            glbase:hasIdentifierValue "SDN:P02::OPFX" ] ;
    rdfs:comment "Quantity of any inorganic species such as silicon (opal) and phosphorus passing through unit area of the water column in unit time. Carbon and nitrogen are regarded as organic and explicitly excluded"@en ;
    rdfs:subClassOf <http://vocab.nerc.ac.uk/collection/P03/current/O005/> ;
    owl:deprecated "false" .
<http://vocab.nerc.ac.uk/collection/P02/current/OPWC/> a glbase:MeasurementType,
        owl:Class,
        owl:NamedIndividual ;
    rdfs:label "Unclassified pigment concentrations in the water column"@en ;
    dcterms:creator "SeaDataNet" ;
    dcterms:date "2004-07-07 16:41:00.0" ;
    glbase:hasIdentifier [ glbase:hasIdentifierScheme idscheme:sdn ;
            glbase:hasIdentifierValue "SDN:P02::OPWC" ] ;
    rdfs:comment "Includes all pigments that cannot be explicitly classified as chlorophylls, phaeopigments or carotenoids.  Generally, these are parameters where different pigments have been grouped together. Concentrations are expressed in terms of per unit volume or unit area of the water column.  Does not include data expressed per unit mass of SPM."@en ;
    rdfs:subClassOf <http://vocab.nerc.ac.uk/collection/P03/current/B035/> ;
    owl:deprecated "false" .
<http://vocab.nerc.ac.uk/collection/P02/current/OSIC/> a glbase:MeasurementType,
        owl:Class,
        owl:NamedIndividual ;
    rdfs:label "Concentration of organic sulphur species in ice"@en ;
    dcterms:creator "SeaDataNet" ;
    dcterms:date "2011-02-18 14:38:14.0" ;
    glbase:hasIdentifier [ glbase:hasIdentifierScheme idscheme:sdn ;
            glbase:hasIdentifierValue "SDN:P02::OSIC" ] ;
    rdfs:comment "Concentration parameters for organic sulphur species in ice"@en ;
    rdfs:subClassOf <http://vocab.nerc.ac.uk/collection/P02/current/ICHM/> ;
    owl:deprecated "true" .
<http://vocab.nerc.ac.uk/collection/P02/current/OXYC/> a glbase:MeasurementType,
        owl:Class,
        owl:NamedIndividual ;
    rdfs:label "Raw oxygen sensor output"@en ;
    dcterms:creator "SeaDataNet" ;
    dcterms:date "2004-08-11 15:07:28.0" ;
    glbase:hasIdentifier [ glbase:hasIdentifierScheme idscheme:sdn ;
            glbase:hasIdentifierValue "SDN:P02::OXYC" ] ;
    rdfs:comment "Raw parameters (usually membrane current and temperature) from dissolved oxygen sensors"@en ;
    rdfs:subClassOf <http://vocab.nerc.ac.uk/collection/P03/current/C015/> ;
    owl:deprecated "false" .
<http://vocab.nerc.ac.uk/collection/P02/current/OZON/> a glbase:MeasurementType,
        owl:Class,
        owl:NamedIndividual ;
    rdfs:label "Ozone and oxygen concentrations in the atmosphere"@en ;
    dcterms:creator "SeaDataNet" ;
    dcterms:date "2006-06-05 12:27:47.0" ;
    glbase:hasIdentifier [ glbase:hasIdentifierScheme idscheme:sdn ;
            glbase:hasIdentifierValue "SDN:P02::OZON" ] ;
    rdfs:comment "Ozone and oxygen concentration parameters in any phase of the atmosphere (but usually the gaseous phase)"@en ;
    rdfs:subClassOf <http://vocab.nerc.ac.uk/collection/P03/current/M005/> ;
    owl:deprecated "false" .
<http://vocab.nerc.ac.uk/collection/P02/current/PASR/> a glbase:MeasurementType,
        owl:Class,
        owl:NamedIndividual ;
    rdfs:label "Passive seismic refraction"@en ;
    dcterms:creator "SeaDataNet" ;
    dcterms:date "2010-02-21 17:24:44.0" ;
    glbase:hasIdentifier [ glbase:hasIdentifierScheme idscheme:sdn ;
            glbase:hasIdentifierValue "SDN:P02::PASR" ] ;
    rdfs:comment "Parameters quantifying the magnitude of naturally occurring low frequency earth movements such as used for earthquake seismology and natural noise studies."@en ;
    rdfs:subClassOf <http://vocab.nerc.ac.uk/collection/P03/current/G012/>,
        <http://vocab.nerc.ac.uk/collection/P03/current/GPYS/> ;
    owl:deprecated "false" .
<http://vocab.nerc.ac.uk/collection/P02/current/PATX/> a glbase:MeasurementType,
        owl:Class,
        owl:NamedIndividual ;
    rdfs:label "Phytoplankton taxonomic abundance in water bodies"@en ;
    dcterms:creator "SeaDataNet" ;
    dcterms:date "2010-10-22 10:06:41.0" ;
    glbase:hasIdentifier [ glbase:hasIdentifierScheme idscheme:sdn ;
            glbase:hasIdentifierValue "SDN:P02::PATX" ] ;
    rdfs:comment "Any enumeration (e.g. count, abundance) of free-floating autotrophic biological entities designated by taxonomic names (e.g. species, genus, family) in any body of fresh or salt water."@en ;
    rdfs:subClassOf <http://vocab.nerc.ac.uk/collection/P03/current/B030/>,
        <http://vocab.nerc.ac.uk/collection/P03/current/B070/> ;
    owl:deprecated "false" .
<http://vocab.nerc.ac.uk/collection/P02/current/PCAH/> a glbase:MeasurementType,
        owl:Class,
        owl:NamedIndividual ;
    rdfs:label "Concentration of polycyclic aromatic hydrocarbons (PAHs) in suspended particulate material"@en ;
    dcterms:creator "SeaDataNet" ;
    dcterms:date "2008-11-25 15:43:03.0" ;
    glbase:hasIdentifier [ glbase:hasIdentifierScheme idscheme:sdn ;
            glbase:hasIdentifierValue "SDN:P02::PCAH" ] ;
    rdfs:comment "PAH concentrations in suspended particulate material, regarded as anything sampled by a water bottle, SAP, sediment trap etc.  This group is for SPM composition measurements (concentration per unit weight) and NOT concentrations per unit volume of the water column in the particulate phase."@en ;
    rdfs:subClassOf <http://vocab.nerc.ac.uk/collection/P03/current/C025/>,
        <http://vocab.nerc.ac.uk/collection/P03/current/C055/>,
        <http://vocab.nerc.ac.uk/collection/P03/current/G015/>,
        <http://vocab.nerc.ac.uk/collection/P03/current/H001/> ;
    owl:deprecated "false" .
<http://vocab.nerc.ac.uk/collection/P02/current/PCFX/> a glbase:MeasurementType,
        owl:Class,
        owl:NamedIndividual ;
    rdfs:label "Sedimentation flux of identified biota expressed as carbon in the water column"@en ;
    dcterms:creator "SeaDataNet" ;
    dcterms:date "2004-05-18 16:44:49.0" ;
    glbase:hasIdentifier [ glbase:hasIdentifierScheme idscheme:sdn ;
            glbase:hasIdentifierValue "SDN:P02::PCFX" ] ;
    rdfs:comment "Fluxes of any biota or remains thereof (excluding faecal pellets which are classed as SPM) downwards through the water column"@en ;
    rdfs:subClassOf <http://vocab.nerc.ac.uk/collection/P03/current/B027/>,
        <http://vocab.nerc.ac.uk/collection/P03/current/O005/> ;
    owl:deprecated "false" .
<http://vocab.nerc.ac.uk/collection/P02/current/PCHW/> a glbase:MeasurementType,
        owl:Class,
        owl:NamedIndividual ;
    rdfs:label "Concentration of polycyclic aromatic hydrocarbons (PAHs) in the water column"@en ;
    dcterms:creator "SeaDataNet" ;
    dcterms:date "2008-11-25 15:43:03.0" ;
    glbase:hasIdentifier [ glbase:hasIdentifierScheme idscheme:sdn ;
            glbase:hasIdentifierValue "SDN:P02::PCHW" ] ;
    rdfs:comment "PAH concentrations in all phases of the water column. This group includes concentrations per unit volume of the water column in the particulate phase, but not concentrations per unit wieght of SPM."@en ;
    rdfs:subClassOf <http://vocab.nerc.ac.uk/collection/P03/current/C025/>,
        <http://vocab.nerc.ac.uk/collection/P03/current/C055/>,
        <http://vocab.nerc.ac.uk/collection/P03/current/H001/> ;
    owl:deprecated "false" .
<http://vocab.nerc.ac.uk/collection/P02/current/PCLM/> a glbase:MeasurementType,
        owl:Class,
        owl:NamedIndividual ;
    rdfs:label "Palaeoclimatic indicators and parameters"@en ;
    dcterms:creator "SeaDataNet" ;
    dcterms:date "2008-07-01 08:38:51.0" ;
    glbase:hasIdentifier [ glbase:hasIdentifierScheme idscheme:sdn ;
            glbase:hasIdentifierValue "SDN:P02::PCLM" ] ;
    rdfs:comment "Parameterisations that describe climatic conditions in the past.  Includes climate indices, climate indicators and indirect measurements of climate-related phenomena such as sea level and water table depth."@en ;
    rdfs:subClassOf <http://vocab.nerc.ac.uk/collection/P03/current/H003/> ;
    owl:deprecated "false" .
<http://vocab.nerc.ac.uk/collection/P02/current/PCO2/> a glbase:MeasurementType,
        owl:Class,
        owl:NamedIndividual ;
    rdfs:label "Partial pressure (pCO2) and fugacity (fCO2) of carbon dioxide in the water column"@en ;
    dcterms:creator "SeaDataNet" ;
    dcterms:date "2004-08-11 09:08:12.0" ;
    glbase:hasIdentifier [ glbase:hasIdentifierScheme idscheme:sdn ;
            glbase:hasIdentifierValue "SDN:P02::PCO2" ] ;
    rdfs:comment "" ;
    rdfs:subClassOf <http://vocab.nerc.ac.uk/collection/P03/current/C010/> ;
    owl:deprecated "false" .
<http://vocab.nerc.ac.uk/collection/P02/current/PCOC/> a glbase:MeasurementType,
        owl:Class,
        owl:NamedIndividual ;
    rdfs:label "Concentration of other organic contaminants in suspended particulate material"@en ;
    dcterms:creator "SeaDataNet" ;
    dcterms:date "2004-05-28 08:15:00.0" ;
    glbase:hasIdentifier [ glbase:hasIdentifierScheme idscheme:sdn ;
            glbase:hasIdentifierValue "SDN:P02::PCOC" ] ;
    rdfs:comment "'Other' organic contaminant (substances regarded as harmful other than PCBs and PAHs) concentrations in suspended particulate material, regarded as anything sampled by a water bottle, SAP, sediment trap etc.  This group is for SPM composition measurements (concentration per unit weight) and NOT concentrations per unit volume of the water column in the particulate phase."@en ;
    rdfs:subClassOf <http://vocab.nerc.ac.uk/collection/P03/current/C055/>,
        <http://vocab.nerc.ac.uk/collection/P03/current/G015/>,
        <http://vocab.nerc.ac.uk/collection/P03/current/H001/> ;
    owl:deprecated "false" .
<http://vocab.nerc.ac.uk/collection/P02/current/PEBI/> a glbase:MeasurementType,
        owl:Class,
        owl:NamedIndividual ;
    rdfs:label "Pesticide concentrations in biota"@en ;
    dcterms:creator "SeaDataNet" ;
    dcterms:date "2010-01-27 14:18:10.0" ;
    glbase:hasIdentifier [ glbase:hasIdentifierScheme idscheme:sdn ;
            glbase:hasIdentifierValue "SDN:P02::PEBI" ] ;
    rdfs:comment "Concentration parameters for substances synthesised by man to kill other life forms in either whole organisms or their constituent parts."@en ;
    rdfs:subClassOf <http://vocab.nerc.ac.uk/collection/P03/current/B007/>,
        <http://vocab.nerc.ac.uk/collection/P03/current/C055/>,
        <http://vocab.nerc.ac.uk/collection/P03/current/H001/> ;
    owl:deprecated "false" .
<http://vocab.nerc.ac.uk/collection/P02/current/PESD/> a glbase:MeasurementType,
        owl:Class,
        owl:NamedIndividual ;
    rdfs:label "Pesticide concentrations in sediment"@en ;
    dcterms:creator "SeaDataNet" ;
    dcterms:date "2010-01-27 14:18:10.0" ;
    glbase:hasIdentifier [ glbase:hasIdentifierScheme idscheme:sdn ;
            glbase:hasIdentifierValue "SDN:P02::PESD" ] ;
    rdfs:comment "Concentration parameters for substances synthesised by man to kill other life forms in sediment, which is considered to be anything from the bed sampled by a grab or corer, including 'fluff'."@en ;
    rdfs:subClassOf <http://vocab.nerc.ac.uk/collection/P03/current/C055/>,
        <http://vocab.nerc.ac.uk/collection/P03/current/G035/>,
        <http://vocab.nerc.ac.uk/collection/P03/current/H001/> ;
    owl:deprecated "false" .
<http://vocab.nerc.ac.uk/collection/P02/current/PEWB/> a glbase:MeasurementType,
        owl:Class,
        owl:NamedIndividual ;
    rdfs:label "Pesticide concentrations in water bodies"@en ;
    dcterms:creator "SeaDataNet" ;
    dcterms:date "2010-01-27 14:18:10.0" ;
    glbase:hasIdentifier [ glbase:hasIdentifierScheme idscheme:sdn ;
            glbase:hasIdentifierValue "SDN:P02::PEWB" ] ;
    rdfs:comment "Concentration parameters for substances synthesised by man to kill other life forms in either solution or suspension (i.e.includes measurements in both the dissolved and particulate phases) in any body of salt or fresh water."@en ;
    rdfs:subClassOf <http://vocab.nerc.ac.uk/collection/P03/current/C055/>,
        <http://vocab.nerc.ac.uk/collection/P03/current/H001/> ;
    owl:deprecated "false" .
<http://vocab.nerc.ac.uk/collection/P02/current/PHAT/> a glbase:MeasurementType,
        owl:Class,
        owl:NamedIndividual ;
    rdfs:label "Inorganic phosphorus species concentrations in the atmosphere"@en ;
    dcterms:creator "SeaDataNet" ;
    dcterms:date "2005-09-23 10:41:38.0" ;
    glbase:hasIdentifier [ glbase:hasIdentifierScheme idscheme:sdn ;
            glbase:hasIdentifierValue "SDN:P02::PHAT" ] ;
    rdfs:comment "Concentration of inorganic phosphorus species (element or compounds) in any phase of the atmosphere"@en ;
    rdfs:subClassOf <http://vocab.nerc.ac.uk/collection/P03/current/C005/>,
        <http://vocab.nerc.ac.uk/collection/P03/current/M005/> ;
    owl:deprecated "false" .
<http://vocab.nerc.ac.uk/collection/P02/current/PHBI/> a glbase:MeasurementType,
        owl:Class,
        owl:NamedIndividual ;
    rdfs:label "Pharmaceutical concentrations in biota"@en ;
    dcterms:creator "SeaDataNet" ;
    dcterms:date "2010-01-27 14:18:10.0" ;
    glbase:hasIdentifier [ glbase:hasIdentifierScheme idscheme:sdn ;
            glbase:hasIdentifierValue "SDN:P02::PHBI" ] ;
    rdfs:comment "Concentration parameters for substances synthesised by man to modify bodily function or diagnose, cure, mitigate, treat, or prevent disease in either whole organisms or their constituent parts."@en ;
    rdfs:subClassOf <http://vocab.nerc.ac.uk/collection/P03/current/B007/>,
        <http://vocab.nerc.ac.uk/collection/P03/current/C055/>,
        <http://vocab.nerc.ac.uk/collection/P03/current/H001/> ;
    owl:deprecated "false" .
<http://vocab.nerc.ac.uk/collection/P02/current/PHLT/> a glbase:MeasurementType,
        owl:Class,
        owl:NamedIndividual ;
    rdfs:label "Raw pH sensor output"@en ;
    dcterms:creator "SeaDataNet" ;
    dcterms:date "2015-11-16 13:22:28.0" ;
    glbase:hasIdentifier [ glbase:hasIdentifierScheme idscheme:sdn ;
            glbase:hasIdentifierValue "SDN:P02::PHLT" ] ;
    rdfs:comment "Raw pH parameter output from any type of pH sensor."@en ;
    rdfs:subClassOf <http://vocab.nerc.ac.uk/collection/P03/current/C010/> ;
    owl:deprecated "false" .
<http://vocab.nerc.ac.uk/collection/P02/current/PHOS/> a glbase:MeasurementType,
        owl:Class,
        owl:NamedIndividual ;
    rdfs:label "Phosphate concentration parameters in the water column"@en ;
    dcterms:creator "SeaDataNet" ;
    dcterms:date "2004-05-27 10:03:09.0" ;
    glbase:hasIdentifier [ glbase:hasIdentifierScheme idscheme:sdn ;
            glbase:hasIdentifierValue "SDN:P02::PHOS" ] ;
    rdfs:comment "Phosphate  concentration parameters (including statistical parameters such as standard deviation) in the water column"@en ;
    rdfs:subClassOf <http://vocab.nerc.ac.uk/collection/P03/current/C005/>,
        <http://vocab.nerc.ac.uk/collection/P03/current/C040/> ;
    owl:deprecated "false" .
<http://vocab.nerc.ac.uk/collection/P02/current/PHSD/> a glbase:MeasurementType,
        owl:Class,
        owl:NamedIndividual ;
    rdfs:label "Phaeopigment concentrations in sediment"@en ;
    dcterms:creator "SeaDataNet" ;
    dcterms:date "2004-07-07 16:40:00.0" ;
    glbase:hasIdentifier [ glbase:hasIdentifierScheme idscheme:sdn ;
            glbase:hasIdentifierValue "SDN:P02::PHSD" ] ;
    rdfs:comment "Includes all variants of phaeopigment (chlorophyll degradation products). Sediment is defined as any solids collected by a corer, including fluff.."@en ;
    rdfs:subClassOf <http://vocab.nerc.ac.uk/collection/P03/current/B035/>,
        <http://vocab.nerc.ac.uk/collection/P03/current/G035/> ;
    owl:deprecated "false" .
<http://vocab.nerc.ac.uk/collection/P02/current/PHSE/> a glbase:MeasurementType,
        owl:Class,
        owl:NamedIndividual ;
    rdfs:label "Pharmaceutical concentrations in sediments"@en ;
    dcterms:creator "SeaDataNet" ;
    dcterms:date "2010-01-27 14:18:10.0" ;
    glbase:hasIdentifier [ glbase:hasIdentifierScheme idscheme:sdn ;
            glbase:hasIdentifierValue "SDN:P02::PHSE" ] ;
    rdfs:comment "Concentration parameters for substances synthesised by man to modify bodily function or diagnose, cure, mitigate, treat, or prevent disease in sediment, which is considered to be anything from the bed sampled by a grab or corer, including 'fluff'."@en ;
    rdfs:subClassOf <http://vocab.nerc.ac.uk/collection/P03/current/C055/>,
        <http://vocab.nerc.ac.uk/collection/P03/current/G035/>,
        <http://vocab.nerc.ac.uk/collection/P03/current/H001/> ;
    owl:deprecated "false" .
<http://vocab.nerc.ac.uk/collection/P02/current/PHUP/> a glbase:MeasurementType,
        owl:Class,
        owl:NamedIndividual ;
    rdfs:label "Uptake of other nutrients in the water column"@en ;
    dcterms:creator "SeaDataNet" ;
    dcterms:date "2010-11-08 15:08:09.0" ;
    glbase:hasIdentifier [ glbase:hasIdentifierScheme idscheme:sdn ;
            glbase:hasIdentifierValue "SDN:P02::PHUP" ] ;
    rdfs:comment "Uptake of nutrients other than nitrogen species (ie phosphate and silicate) by the water column"@en ;
    rdfs:subClassOf <http://vocab.nerc.ac.uk/collection/P03/current/C040/>,
        <http://vocab.nerc.ac.uk/collection/P03/current/O010/> ;
    owl:deprecated "false" .
<http://vocab.nerc.ac.uk/collection/P02/current/PHWB/> a glbase:MeasurementType,
        owl:Class,
        owl:NamedIndividual ;
    rdfs:label "Pharmaceutical concentrations in water bodies"@en ;
    dcterms:creator "SeaDataNet" ;
    dcterms:date "2010-01-27 14:18:10.0" ;
    glbase:hasIdentifier [ glbase:hasIdentifierScheme idscheme:sdn ;
            glbase:hasIdentifierValue "SDN:P02::PHWB" ] ;
    rdfs:comment "Concentration parameters for substances synthesised by man to modify bodily function or diagnose, cure, mitigate, treat, or prevent disease in either solution or suspension (i.e.includes measurements in both the dissolved and particulate phases) in any body of salt or fresh water."@en ;
    rdfs:subClassOf <http://vocab.nerc.ac.uk/collection/P03/current/C055/>,
        <http://vocab.nerc.ac.uk/collection/P03/current/H001/> ;
    owl:deprecated "false" .
<http://vocab.nerc.ac.uk/collection/P02/current/PHWC/> a glbase:MeasurementType,
        owl:Class,
        owl:NamedIndividual ;
    rdfs:label "Phaeopigment concentrations in the water column"@en ;
    dcterms:creator "SeaDataNet" ;
    dcterms:date "2004-07-07 16:40:00.0" ;
    glbase:hasIdentifier [ glbase:hasIdentifierScheme idscheme:sdn ;
            glbase:hasIdentifierValue "SDN:P02::PHWC" ] ;
    rdfs:comment "Includes all variants of phaeopigment (chlorophyll degradation products) expressed in terms of per unit volume or unit area of the water column.  Does not include data expressed per unit mass of SPM."@en ;
    rdfs:subClassOf <http://vocab.nerc.ac.uk/collection/P03/current/B035/> ;
    owl:deprecated "false" .
<http://vocab.nerc.ac.uk/collection/P02/current/PHYC/> a glbase:MeasurementType,
        owl:Class,
        owl:NamedIndividual ;
    rdfs:label "Phycobolin pigment concentrations in the water column"@en ;
    dcterms:creator "SeaDataNet" ;
    dcterms:date "2004-09-27 08:25:54.0" ;
    glbase:hasIdentifier [ glbase:hasIdentifierScheme idscheme:sdn ;
            glbase:hasIdentifierValue "SDN:P02::PHYC" ] ;
    rdfs:comment "Concentration of phycobolin group pigments such as phycocyanin and phycoerythrin in the water column"@en ;
    rdfs:subClassOf <http://vocab.nerc.ac.uk/collection/P03/current/B035/> ;
    owl:deprecated "false" .
<http://vocab.nerc.ac.uk/collection/P02/current/PHYG/> a glbase:MeasurementType,
        owl:Class,
        owl:NamedIndividual ;
    rdfs:label "Phytoplankton growth"@en ;
    dcterms:creator "SeaDataNet" ;
    dcterms:date "2004-08-19 10:34:58.0" ;
    glbase:hasIdentifier [ glbase:hasIdentifierScheme idscheme:sdn ;
            glbase:hasIdentifierValue "SDN:P02::PHYG" ] ;
    rdfs:comment "" ;
    rdfs:subClassOf <http://vocab.nerc.ac.uk/collection/P03/current/O010/> ;
    owl:deprecated "false" .
<http://vocab.nerc.ac.uk/collection/P02/current/PNFX/> a glbase:MeasurementType,
        owl:Class,
        owl:NamedIndividual ;
    rdfs:label "Sedimentation flux of identified biota in the water column"@en ;
    dcterms:creator "SeaDataNet" ;
    dcterms:date "2004-05-18 16:47:44.0" ;
    glbase:hasIdentifier [ glbase:hasIdentifierScheme idscheme:sdn ;
            glbase:hasIdentifierValue "SDN:P02::PNFX" ] ;
    rdfs:comment "Fluxes expressed as number per unit area per unit time of any biota or remains thereof (excluding faecal pellets which are classed as SPM) downwards through the water column"@en ;
    rdfs:subClassOf <http://vocab.nerc.ac.uk/collection/P03/current/B027/>,
        <http://vocab.nerc.ac.uk/collection/P03/current/O005/> ;
    owl:deprecated "false" .
<http://vocab.nerc.ac.uk/collection/P02/current/PNTX/> a glbase:MeasurementType,
        owl:Class,
        owl:NamedIndividual ;
    rdfs:label "Phytoplankton generic abundance in water bodies"@en ;
    dcterms:creator "SeaDataNet" ;
    dcterms:date "2010-10-22 10:06:41.0" ;
    glbase:hasIdentifier [ glbase:hasIdentifierScheme idscheme:sdn ;
            glbase:hasIdentifierValue "SDN:P02::PNTX" ] ;
    rdfs:comment "Any enumeration (e.g. count, abundance) of free-floating autotrophic biological entities designated by terms other than taxonomic names (e.g. microphytoplankton, ciliate, flagellate) in any body of fresh or salt water."@en ;
    rdfs:subClassOf <http://vocab.nerc.ac.uk/collection/P03/current/B030/>,
        <http://vocab.nerc.ac.uk/collection/P03/current/B070/> ;
    owl:deprecated "false" .
<http://vocab.nerc.ac.uk/collection/P02/current/PPAB/> a glbase:MeasurementType,
        owl:Class,
        owl:NamedIndividual ;
    rdfs:label "Light absorption in the water column"@en ;
    dcterms:creator "SeaDataNet" ;
    dcterms:date "2004-07-30 14:27:59.0" ;
    glbase:hasIdentifier [ glbase:hasIdentifierScheme idscheme:sdn ;
            glbase:hasIdentifierValue "SDN:P02::PPAB" ] ;
    rdfs:comment "Water column spectral absorption parameters"@en ;
    rdfs:subClassOf <http://vocab.nerc.ac.uk/collection/P03/current/D015/> ;
    owl:deprecated "false" .
<http://vocab.nerc.ac.uk/collection/P02/current/PPCB/> a glbase:MeasurementType,
        owl:Class,
        owl:NamedIndividual ;
    rdfs:label "Concentration of polychlorobiphenyls (PCBs) in suspended particulate material"@en ;
    dcterms:creator "SeaDataNet" ;
    dcterms:date "2008-11-25 15:43:03.0" ;
    glbase:hasIdentifier [ glbase:hasIdentifierScheme idscheme:sdn ;
            glbase:hasIdentifierValue "SDN:P02::PPCB" ] ;
    rdfs:comment "PCB concentrations in suspended particulate material, regarded as anything sampled by a water bottle, SAP, sediment trap etc.  This group is for SPM composition measurements (concentration per unit weight) and NOT concentrations per unit volume of the water column in the particulate phase."@en ;
    rdfs:subClassOf <http://vocab.nerc.ac.uk/collection/P03/current/C055/>,
        <http://vocab.nerc.ac.uk/collection/P03/current/G015/>,
        <http://vocab.nerc.ac.uk/collection/P03/current/H001/> ;
    owl:deprecated "false" .
<http://vocab.nerc.ac.uk/collection/P02/current/PPRD/> a glbase:MeasurementType,
        owl:Class,
        owl:NamedIndividual ;
    rdfs:label "Primary production in the water column"@en ;
    dcterms:creator "SeaDataNet" ;
    dcterms:date "2003-06-10 13:53:19.0" ;
    glbase:hasIdentifier [ glbase:hasIdentifierScheme idscheme:sdn ;
            glbase:hasIdentifierValue "SDN:P02::PPRD" ] ;
    rdfs:comment "Parameters associated with the quantification of primary production.  This is defined as the fixation of carbon dioxide into either organic or inorganic carbon by living entities and so includes photosynthesis and calcification."@en ;
    rdfs:subClassOf <http://vocab.nerc.ac.uk/collection/P03/current/O010/> ;
    owl:deprecated "false" .
<http://vocab.nerc.ac.uk/collection/P02/current/PPWC/> a glbase:MeasurementType,
        owl:Class,
        owl:NamedIndividual ;
    rdfs:label "Concentration of polychlorobiphenyls (PCBs) in the water column"@en ;
    dcterms:creator "SeaDataNet" ;
    dcterms:date "2008-11-25 15:43:03.0" ;
    glbase:hasIdentifier [ glbase:hasIdentifierScheme idscheme:sdn ;
            glbase:hasIdentifierValue "SDN:P02::PPWC" ] ;
    rdfs:comment "PCB concentrations in all phases of the water column. This group excludes SPM composition measurements (concentration per unit weight)."@en ;
    rdfs:subClassOf <http://vocab.nerc.ac.uk/collection/P03/current/C055/>,
        <http://vocab.nerc.ac.uk/collection/P03/current/H001/> ;
    owl:deprecated "false" .
<http://vocab.nerc.ac.uk/collection/P02/current/PREX/> a glbase:MeasurementType,
        owl:Class,
        owl:NamedIndividual ;
    rdfs:label "Sea level expressed as pressure"@en ;
    dcterms:creator "SeaDataNet" ;
    dcterms:date "2013-11-15 10:30:47.0" ;
    glbase:hasIdentifier [ glbase:hasIdentifierScheme idscheme:sdn ;
            glbase:hasIdentifierValue "SDN:P02::PREX" ] ;
    rdfs:comment "Measurements of the displacement of the water column surface from a fixed, stable reference expressed as either total pressure or sea pressure"@en ;
    rdfs:subClassOf <http://vocab.nerc.ac.uk/collection/P03/current/D032/> ;
    owl:deprecated "true" .
<http://vocab.nerc.ac.uk/collection/P02/current/PSAL/> a glbase:MeasurementType,
        owl:Class,
        owl:NamedIndividual ;
    rdfs:label "Salinity of the water column"@en ;
    dcterms:creator "SeaDataNet" ;
    dcterms:date "2007-03-02 11:36:26.0" ;
    glbase:hasIdentifier [ glbase:hasIdentifierScheme idscheme:sdn ;
            glbase:hasIdentifierValue "SDN:P02::PSAL" ] ;
    rdfs:comment "Parameters quantifying the concentration of sodium chloride in any body of water at any point between the bed and the atmosphere"@en ;
    rdfs:subClassOf <http://vocab.nerc.ac.uk/collection/P03/current/D025/> ;
    owl:deprecated "false" .
<http://vocab.nerc.ac.uk/collection/P02/current/PSST/> a glbase:MeasurementType,
        owl:Class,
        owl:NamedIndividual ;
    rdfs:label "Skin temperature of the water column"@en ;
    dcterms:creator "SeaDataNet" ;
    dcterms:date "2004-07-29 15:34:56.0" ;
    glbase:hasIdentifier [ glbase:hasIdentifierScheme idscheme:sdn ;
            glbase:hasIdentifierValue "SDN:P02::PSST" ] ;
    rdfs:comment "Temperature of the water column surface as measured by a radiometer.  It does NOT include temperature measurements in the upper few metres of the water column such as thermosalinograph data"@en ;
    rdfs:subClassOf <http://vocab.nerc.ac.uk/collection/P03/current/D025/> ;
    owl:deprecated "false" .
<http://vocab.nerc.ac.uk/collection/P02/current/PTDZ/> a glbase:MeasurementType,
        owl:Class,
        owl:NamedIndividual ;
    rdfs:label "Temperature variation in the water column"@en ;
    dcterms:creator "SeaDataNet" ;
    dcterms:date "2003-06-10 13:53:19.0" ;
    glbase:hasIdentifier [ glbase:hasIdentifierScheme idscheme:sdn ;
            glbase:hasIdentifierValue "SDN:P02::PTDZ" ] ;
    rdfs:comment "Parameters expressing the variation of temperature in the water column either as a function of space or of time"@en ;
    rdfs:subClassOf <http://vocab.nerc.ac.uk/collection/P03/current/D025/> ;
    owl:deprecated "false" .
<http://vocab.nerc.ac.uk/collection/P02/current/PTOX/> a glbase:MeasurementType,
        owl:Class,
        owl:NamedIndividual ;
    rdfs:label "Concentration of phycotoxins in biota"@en ;
    dcterms:creator "SeaDataNet" ;
    dcterms:date "2006-06-05 14:32:17.0" ;
    glbase:hasIdentifier [ glbase:hasIdentifierScheme idscheme:sdn ;
            glbase:hasIdentifierValue "SDN:P02::PTOX" ] ;
    rdfs:comment "Parameters associated with the concentration of algae-generated toxins in either whole organisms or their constituent parts"@en ;
    rdfs:subClassOf <http://vocab.nerc.ac.uk/collection/P03/current/B007/> ;
    owl:deprecated "false" .
<http://vocab.nerc.ac.uk/collection/P02/current/PU02/> a glbase:MeasurementType,
        owl:Class,
        owl:NamedIndividual ;
    rdfs:label "Macroalgae generic abundance in water bodies"@en ;
    dcterms:creator "SeaDataNet" ;
    dcterms:date "2010-10-22 10:06:41.0" ;
    glbase:hasIdentifier [ glbase:hasIdentifierScheme idscheme:sdn ;
            glbase:hasIdentifierValue "SDN:P02::PU02" ] ;
    rdfs:comment "Any enumeration (e.g. count, number per litre) of macroalgae (seaweeds) designated by terms other than taxonomic names (e.g. total) in any fresh or salt water body."@en ;
    rdfs:subClassOf <http://vocab.nerc.ac.uk/collection/P03/current/B055/>,
        <http://vocab.nerc.ac.uk/collection/P03/current/B070/> ;
    owl:deprecated "false" .
<http://vocab.nerc.ac.uk/collection/P02/current/PXSD/> a glbase:MeasurementType,
        owl:Class,
        owl:NamedIndividual ;
    rdfs:label "Phosphorus concentrations in sediment"@en ;
    dcterms:creator "SeaDataNet" ;
    dcterms:date "2010-11-05 12:19:16.0" ;
    glbase:hasIdentifier [ glbase:hasIdentifierScheme idscheme:sdn ;
            glbase:hasIdentifierValue "SDN:P02::PXSD" ] ;
    rdfs:comment "Concentrations of total, organic and inorganic phosphorus per unit weight of sediment.  Sediment is understood to be the solid phase of the bed, including the recently settled material sometimes known as fluff collected from the bed surface."@en ;
    rdfs:subClassOf <http://vocab.nerc.ac.uk/collection/P02/current/RMIN/> ;
    owl:deprecated "true" .
<http://vocab.nerc.ac.uk/collection/P02/current/PXSP/> a glbase:MeasurementType,
        owl:Class,
        owl:NamedIndividual ;
    rdfs:label "Phosphorus concentrations in suspended particulate material"@en ;
    dcterms:creator "SeaDataNet" ;
    dcterms:date "2004-08-02 14:10:30.0" ;
    glbase:hasIdentifier [ glbase:hasIdentifierScheme idscheme:sdn ;
            glbase:hasIdentifierValue "SDN:P02::PXSP" ] ;
    rdfs:comment "Concentrations of total, organic and inorganic phosphorus per unit weight of suspended particulate material collected by water column filtration, centrifugation or sediment trapping."@en ;
    rdfs:subClassOf <http://vocab.nerc.ac.uk/collection/P03/current/C005/>,
        <http://vocab.nerc.ac.uk/collection/P03/current/G015/> ;
    owl:deprecated "false" .
<http://vocab.nerc.ac.uk/collection/P02/current/PYTT/> a glbase:MeasurementType,
        owl:Class,
        owl:NamedIndividual ;
    rdfs:label "Plankton abundance per unit volume of the water column"@en ;
    dcterms:creator "SeaDataNet" ;
    dcterms:date "2003-06-10 13:53:19.0" ;
    glbase:hasIdentifier [ glbase:hasIdentifierScheme idscheme:sdn ;
            glbase:hasIdentifierValue "SDN:P02::PYTT" ] ;
    rdfs:comment "Used for plankton abundance parameters where no differentiation between phytoplankton, microzooplankton or zooplankton is possible"@en ;
    rdfs:subClassOf <http://vocab.nerc.ac.uk/collection/P03/current/B070/> ;
    owl:deprecated "false" .
<http://vocab.nerc.ac.uk/collection/P02/current/QDMD/> a glbase:MeasurementType,
        owl:Class,
        owl:NamedIndividual ;
    rdfs:label "Quantity of material dumped"@en ;
    dcterms:creator "SeaDataNet" ;
    dcterms:date "2008-08-15 10:07:03.0" ;
    glbase:hasIdentifier [ glbase:hasIdentifierScheme idscheme:sdn ;
            glbase:hasIdentifierValue "SDN:P02::QDMD" ] ;
    rdfs:comment "Parameters quantifying the amount of liquids (e.g. ship's ballast) or solids (e.g. dredge spoil) deposited into the water column as a result of man's activities"@en ;
    rdfs:subClassOf <http://vocab.nerc.ac.uk/collection/P03/current/H001/> ;
    owl:deprecated "false" .
<http://vocab.nerc.ac.uk/collection/P02/current/R410/> a glbase:MeasurementType,
        owl:Class,
        owl:NamedIndividual ;
    rdfs:label "Ocean colour and earth-leaving visible waveband spectral radiation"@en ;
    dcterms:creator "SeaDataNet" ;
    dcterms:date "2006-06-05 14:11:44.0" ;
    glbase:hasIdentifier [ glbase:hasIdentifierScheme idscheme:sdn ;
            glbase:hasIdentifierValue "SDN:P02::R410" ] ;
    rdfs:comment "Parameters associated with the measurement of ocean colour, including visible waveband satellite spectral radiometer measurements, their calibration measurements (spectral water-leaving radiance and reflectance) and chart colour estimates."@en ;
    rdfs:subClassOf <http://vocab.nerc.ac.uk/collection/P03/current/D015/> ;
    owl:deprecated "false" .
<http://vocab.nerc.ac.uk/collection/P02/current/RACC/> a glbase:MeasurementType,
        owl:Class,
        owl:NamedIndividual ;
    rdfs:label "Sediment accumulation rate"@en ;
    dcterms:creator "SeaDataNet" ;
    dcterms:date "2008-11-04 13:30:30.0" ;
    glbase:hasIdentifier [ glbase:hasIdentifierScheme idscheme:sdn ;
            glbase:hasIdentifierValue "SDN:P02::RACC" ] ;
    rdfs:comment "Parameters quantifying the volume, mass or thickness of particulate material that gathers on the seabed per unit time."@en ;
    rdfs:subClassOf <http://vocab.nerc.ac.uk/collection/P03/current/G060/> ;
    owl:deprecated "false" .
<http://vocab.nerc.ac.uk/collection/P02/current/RAGE/> a glbase:MeasurementType,
        owl:Class,
        owl:NamedIndividual ;
    rdfs:label "Rock age"@en ;
    dcterms:creator "SeaDataNet" ;
    dcterms:date "2010-02-21 17:23:51.0" ;
    glbase:hasIdentifier [ glbase:hasIdentifierScheme idscheme:sdn ;
            glbase:hasIdentifierValue "SDN:P02::RAGE" ] ;
    rdfs:comment "Measured or stratigraphically estimated ages of lithified sediments, igneous rock or metamorphic rock."@en ;
    rdfs:subClassOf <http://vocab.nerc.ac.uk/collection/P03/current/G030/> ;
    owl:deprecated "false" .
<http://vocab.nerc.ac.uk/collection/P02/current/RALT/> a glbase:MeasurementType,
        owl:Class,
        owl:NamedIndividual ;
    rdfs:label "Rock alteration"@en ;
    dcterms:creator "SeaDataNet" ;
    dcterms:date "2010-02-21 17:26:59.0" ;
    glbase:hasIdentifier [ glbase:hasIdentifierScheme idscheme:sdn ;
            glbase:hasIdentifierValue "SDN:P02::RALT" ] ;
    rdfs:comment "Parameters decribing aspects of a geologic unit that are the result of bulk chemical, mineralogical or physical changes related to change in the physical or chemical environment.  Includes weathering, supergene alteration, hydrothermal alteration and metasomatic effects not considered metamorphic."@en ;
    rdfs:subClassOf <http://vocab.nerc.ac.uk/collection/P03/current/G060/> ;
    owl:deprecated "false" .
<http://vocab.nerc.ac.uk/collection/P02/current/RBHY/> a glbase:MeasurementType,
        owl:Class,
        owl:NamedIndividual ;
    rdfs:label "Molecular biology parameters"@en ;
    dcterms:creator "SeaDataNet" ;
    dcterms:date "2004-04-30 15:19:08.0" ;
    glbase:hasIdentifier [ glbase:hasIdentifierScheme idscheme:sdn ;
            glbase:hasIdentifierValue "SDN:P02::RBHY" ] ;
    rdfs:comment "Any parameters relating to molecular biology or genetics"@en ;
    rdfs:subClassOf <http://vocab.nerc.ac.uk/collection/P03/current/B027/> ;
    owl:deprecated "false" .
<http://vocab.nerc.ac.uk/collection/P02/current/RBSC/> a glbase:MeasurementType,
        owl:Class,
        owl:NamedIndividual ;
    rdfs:label "Radar backscatter"@en ;
    dcterms:creator "SeaDataNet" ;
    dcterms:date "2009-05-20 15:08:16.0" ;
    glbase:hasIdentifier [ glbase:hasIdentifierScheme idscheme:sdn ;
            glbase:hasIdentifierValue "SDN:P02::RBSC" ] ;
    rdfs:comment "Includes all parameters covering the strength of emitted microwave radiation return, including absolute measurements of returning signal strength as well as parameters expressed as backscatter (the proportion of transmitted signal returned)"@en ;
    rdfs:subClassOf <http://vocab.nerc.ac.uk/collection/P03/current/D030/>,
        <http://vocab.nerc.ac.uk/collection/P03/current/D032/>,
        <http://vocab.nerc.ac.uk/collection/P03/current/D034/>,
        <http://vocab.nerc.ac.uk/collection/P03/current/M010/>,
        <http://vocab.nerc.ac.uk/collection/P03/current/M015/> ;
    owl:deprecated "false" .
<http://vocab.nerc.ac.uk/collection/P02/current/REFF/> a glbase:MeasurementType,
        owl:Class,
        owl:NamedIndividual ;
    rdfs:label "Sediment resistivity"@en ;
    dcterms:creator "SeaDataNet" ;
    dcterms:date "2004-08-17 14:12:44.0" ;
    glbase:hasIdentifier [ glbase:hasIdentifierScheme idscheme:sdn ;
            glbase:hasIdentifierValue "SDN:P02::REFF" ] ;
    rdfs:comment "" ;
    rdfs:subClassOf <http://vocab.nerc.ac.uk/collection/P03/current/G050/> ;
    owl:deprecated "false" .
<http://vocab.nerc.ac.uk/collection/P02/current/RFVL/> a glbase:MeasurementType,
        owl:Class,
        owl:NamedIndividual ;
    rdfs:label "Horizontal velocity of the water column (currents)"@en ;
    dcterms:creator "SeaDataNet" ;
    dcterms:date "2007-01-18 16:38:20.0" ;
    glbase:hasIdentifier [ glbase:hasIdentifierScheme idscheme:sdn ;
            glbase:hasIdentifierValue "SDN:P02::RFVL" ] ;
    rdfs:comment "Parameters expressing the velocity (including scalar speeds and directions) of water column horizontal movement, commonly termed Eulerian currents"@en ;
    rdfs:subClassOf <http://vocab.nerc.ac.uk/collection/P03/current/D030/> ;
    owl:deprecated "false" .
<http://vocab.nerc.ac.uk/collection/P02/current/RGAS/> a glbase:MeasurementType,
        owl:Class,
        owl:NamedIndividual ;
    rdfs:label "Raw gas analyser output"@en ;
    dcterms:creator "SeaDataNet" ;
    dcterms:date "2007-09-24 11:56:11.0" ;
    glbase:hasIdentifier [ glbase:hasIdentifierScheme idscheme:sdn ;
            glbase:hasIdentifierValue "SDN:P02::RGAS" ] ;
    rdfs:comment "Raw concentration parameters from a gas analyser such as a LiCor"@en ;
    rdfs:subClassOf <http://vocab.nerc.ac.uk/collection/P03/current/C015/>,
        <http://vocab.nerc.ac.uk/collection/P03/current/M005/> ;
    owl:deprecated "false" .
<http://vocab.nerc.ac.uk/collection/P02/current/RMAJ/> a glbase:MeasurementType,
        owl:Class,
        owl:NamedIndividual ;
    rdfs:label "Geological sample major element chemistry"@en ;
    dcterms:creator "SeaDataNet" ;
    dcterms:date "2010-11-05 12:53:24.0" ;
    glbase:hasIdentifier [ glbase:hasIdentifierScheme idscheme:sdn ;
            glbase:hasIdentifierValue "SDN:P02::RMAJ" ] ;
    rdfs:comment "Concentrations of the elements classically regarded as major (>1% by weight as oxide: namely: Si, Ti, Al, Fe3+, Fe2+, Mg, Mn, Ca, Na, and K) plus affiliated parameters such as H2O- (adsorbed water) and H2O+ (or loss on ignition) in rocks or sediments."@en ;
    rdfs:subClassOf <http://vocab.nerc.ac.uk/collection/P02/current/RMIN/> ;
    owl:deprecated "true" .
<http://vocab.nerc.ac.uk/collection/P02/current/ROGS/> a glbase:MeasurementType,
        owl:Class,
        owl:NamedIndividual ;
    rdfs:label "Rock grain size"@en ;
    dcterms:creator "SeaDataNet" ;
    dcterms:date "2010-02-21 17:28:35.0" ;
    glbase:hasIdentifier [ glbase:hasIdentifierScheme idscheme:sdn ;
            glbase:hasIdentifierValue "SDN:P02::ROGS" ] ;
    rdfs:comment "Parameters specifying the physical dimensions of the particles comprising lithified sedimentary rocks (including expressions of shape such as aspect ratio) and statistics derived from their variation in a sample (e.g. mean, mode, sorting, skewness)."@en ;
    rdfs:subClassOf <http://vocab.nerc.ac.uk/collection/P03/current/G040/> ;
    owl:deprecated "false" .
<http://vocab.nerc.ac.uk/collection/P02/current/RPER/> a glbase:MeasurementType,
        owl:Class,
        owl:NamedIndividual ;
    rdfs:label "Rock porosity and permeability"@en ;
    dcterms:creator "SeaDataNet" ;
    dcterms:date "2010-02-21 17:26:42.0" ;
    glbase:hasIdentifier [ glbase:hasIdentifierScheme idscheme:sdn ;
            glbase:hasIdentifierValue "SDN:P02::RPER" ] ;
    rdfs:comment "Parmeters describing the space for fluids or gases within a geologic unit comprising lithified sediments, igneous rock or metamorphic rock."@en ;
    rdfs:subClassOf <http://vocab.nerc.ac.uk/collection/P03/current/G040/> ;
    owl:deprecated "false" .
<http://vocab.nerc.ac.uk/collection/P02/current/RPOT/> a glbase:MeasurementType,
        owl:Class,
        owl:NamedIndividual ;
    rdfs:label "Redox potential in sediment"@en ;
    dcterms:creator "SeaDataNet" ;
    dcterms:date "2003-06-10 13:53:19.0" ;
    glbase:hasIdentifier [ glbase:hasIdentifierScheme idscheme:sdn ;
            glbase:hasIdentifierValue "SDN:P02::RPOT" ] ;
    rdfs:comment "" ;
    rdfs:subClassOf <http://vocab.nerc.ac.uk/collection/P03/current/C045/>,
        <http://vocab.nerc.ac.uk/collection/P03/current/G035/> ;
    owl:deprecated "false" .
<http://vocab.nerc.ac.uk/collection/P02/current/RSIS/> a glbase:MeasurementType,
        owl:Class,
        owl:NamedIndividual ;
    rdfs:label "Field resistivity,  electromagnetics  and polarisation"@en ;
    dcterms:creator "SeaDataNet" ;
    dcterms:date "2011-09-16 11:32:12.0" ;
    glbase:hasIdentifier [ glbase:hasIdentifierScheme idscheme:sdn ;
            glbase:hasIdentifierValue "SDN:P02::RSIS" ] ;
    rdfs:comment "Parameters quantifying the electrical properties of geological units in the field. Includes parameters used to determine resistivity structure for shallow sediment properties, porosities and presence of hydrocarbon (CSEM), deeper crust and mantle studies (Magnetotellurics) and ore body location (polarisation)."@en ;
    rdfs:subClassOf <http://vocab.nerc.ac.uk/collection/P03/current/GPYS/> ;
    owl:deprecated "false" .
<http://vocab.nerc.ac.uk/collection/P02/current/RTCO/> a glbase:MeasurementType,
        owl:Class,
        owl:NamedIndividual ;
    rdfs:label "Rock thermal conductivity"@en ;
    dcterms:creator "SeaDataNet" ;
    dcterms:date "2010-02-21 17:28:15.0" ;
    glbase:hasIdentifier [ glbase:hasIdentifierScheme idscheme:sdn ;
            glbase:hasIdentifierValue "SDN:P02::RTCO" ] ;
    rdfs:comment "Parameters that describe the degree to which sedimentary, igneous or metamorphic rocks are able to conduct heat"@en ;
    rdfs:subClassOf <http://vocab.nerc.ac.uk/collection/P03/current/G040/>,
        <http://vocab.nerc.ac.uk/collection/P03/current/GTHM/> ;
    owl:deprecated "false" .
<http://vocab.nerc.ac.uk/collection/P02/current/RTMP/> a glbase:MeasurementType,
        owl:Class,
        owl:NamedIndividual ;
    rdfs:label "Rock temperature"@en ;
    dcterms:creator "SeaDataNet" ;
    dcterms:date "2010-11-05 13:00:34.0" ;
    glbase:hasIdentifier [ glbase:hasIdentifierScheme idscheme:sdn ;
            glbase:hasIdentifierValue "SDN:P02::RTMP" ] ;
    rdfs:comment "Parameters that describe the distribution of the degree of hotness within geologic units of lithified sedimentary, igneous of metamorphic rock."@en ;
    rdfs:subClassOf <http://vocab.nerc.ac.uk/collection/P02/current/STMP/> ;
    owl:deprecated "true" .
<http://vocab.nerc.ac.uk/collection/P02/current/RVDS/> a glbase:MeasurementType,
        owl:Class,
        owl:NamedIndividual ;
    rdfs:label "River flow and discharge"@en ;
    dcterms:creator "SeaDataNet" ;
    dcterms:date "2010-11-08 08:56:52.0" ;
    glbase:hasIdentifier [ glbase:hasIdentifierScheme idscheme:sdn ;
            glbase:hasIdentifierValue "SDN:P02::RVDS" ] ;
    rdfs:comment "Parameters related to the volume of water passing through a point in a river system per unit time, including the rates of freshwater, dissolved material and particulate load discharge from a river into the sea."@en ;
    rdfs:subClassOf <http://vocab.nerc.ac.uk/collection/P03/current/D030/>,
        <http://vocab.nerc.ac.uk/collection/P03/current/H001/>,
        <http://vocab.nerc.ac.uk/collection/P03/current/O005/> ;
    owl:deprecated "false" .
<http://vocab.nerc.ac.uk/collection/P02/current/RWCH/> a glbase:MeasurementType,
        owl:Class,
        owl:NamedIndividual ;
    rdfs:label "Precipitation chemistry"@en ;
    dcterms:creator "SeaDataNet" ;
    dcterms:date "2008-12-09 10:34:11.0" ;
    glbase:hasIdentifier [ glbase:hasIdentifierScheme idscheme:sdn ;
            glbase:hasIdentifierValue "SDN:P02::RWCH" ] ;
    rdfs:comment "Concentration of any chemical species in water collected from the atmosphere.  Includes rain, snow, hail and fog but excludes cloud samples or snow accumulations on the ground."@en ;
    rdfs:subClassOf <http://vocab.nerc.ac.uk/collection/P03/current/M005/> ;
    owl:deprecated "false" .
<http://vocab.nerc.ac.uk/collection/P02/current/SABB/> a glbase:MeasurementType,
        owl:Class,
        owl:NamedIndividual ;
    rdfs:label "Shellfish abundance and biomass in water bodies"@en ;
    dcterms:creator "SeaDataNet" ;
    dcterms:date "2010-07-30 12:17:07.0" ;
    glbase:hasIdentifier [ glbase:hasIdentifierScheme idscheme:sdn ;
            glbase:hasIdentifierValue "SDN:P02::SABB" ] ;
    rdfs:comment "Paramaters that quantify the numbers or amount of living material of shellfish (molluscs - including cephalopods - and crustaceans of interest to fisheries research and commercial fisheries) in any body of fresh or salt water."@en ;
    rdfs:subClassOf <http://vocab.nerc.ac.uk/collection/P03/current/B070/>,
        <http://vocab.nerc.ac.uk/collection/P03/current/H004/> ;
    owl:deprecated "false" .
<http://vocab.nerc.ac.uk/collection/P02/current/SACT/> a glbase:MeasurementType,
        owl:Class,
        owl:NamedIndividual ;
    rdfs:label "Surfactant concentrations in water bodies"@en ;
    dcterms:creator "SeaDataNet" ;
    dcterms:date "2011-10-18 14:35:03.0" ;
    glbase:hasIdentifier [ glbase:hasIdentifierScheme idscheme:sdn ;
            glbase:hasIdentifierValue "SDN:P02::SACT" ] ;
    rdfs:comment "Parameters quantifying the amount of compounds that lower the surface tension of a liquid, the interfacial tension between two liquids, or that between a liquid and a solid in any body of salt or fresh water. The term surfactants includes detergents, wetting agents, emulsifiers, foaming agents and dispersants."@en ;
    rdfs:subClassOf <http://vocab.nerc.ac.uk/collection/P03/current/C050/> ;
    owl:deprecated "false" .
<http://vocab.nerc.ac.uk/collection/P02/current/SAGE/> a glbase:MeasurementType,
        owl:Class,
        owl:NamedIndividual ;
    rdfs:label "Sediment age"@en ;
    dcterms:creator "SeaDataNet" ;
    dcterms:date "2003-06-10 13:53:19.0" ;
    glbase:hasIdentifier [ glbase:hasIdentifierScheme idscheme:sdn ;
            glbase:hasIdentifierValue "SDN:P02::SAGE" ] ;
    rdfs:comment "Measured or stratigraphically estimated ages of marine sediments"@en ;
    rdfs:subClassOf <http://vocab.nerc.ac.uk/collection/P03/current/G030/> ;
    owl:deprecated "false" .
<http://vocab.nerc.ac.uk/collection/P02/current/SALK/> a glbase:MeasurementType,
        owl:Class,
        owl:NamedIndividual ;
    rdfs:label "Concentration of aliphatic hydrocarbons in sediment samples"@en ;
    dcterms:creator "SeaDataNet" ;
    dcterms:date "2012-03-01 16:27:53.0" ;
    glbase:hasIdentifier [ glbase:hasIdentifierScheme idscheme:sdn ;
            glbase:hasIdentifierValue "SDN:P02::SALK" ] ;
    rdfs:comment "Aliphatic hydrocarbon (alkane, alkene, alkyne, polycyclic aliphatics like hopane, terpenes etc.)  concentrations in sediment, which is considered to be anything from the bed sampled by a grab or corer, including 'fluff'"@en ;
    rdfs:subClassOf <http://vocab.nerc.ac.uk/collection/P03/current/C025/>,
        <http://vocab.nerc.ac.uk/collection/P03/current/G035/> ;
    owl:deprecated "false" .
<http://vocab.nerc.ac.uk/collection/P02/current/SAMO/> a glbase:MeasurementType,
        owl:Class,
        owl:NamedIndividual ;
    rdfs:label "Nutrient fluxes between the bed and the water column"@en ;
    dcterms:creator "SeaDataNet" ;
    dcterms:date "2004-08-18 15:41:50.0" ;
    glbase:hasIdentifier [ glbase:hasIdentifierScheme idscheme:sdn ;
            glbase:hasIdentifierValue "SDN:P02::SAMO" ] ;
    rdfs:comment "Parameters quantifying the exchange of nutrients between the bed (ie the sediment) and the water column sometimes termed benthic fluxes"@en ;
    rdfs:subClassOf <http://vocab.nerc.ac.uk/collection/P03/current/C040/>,
        <http://vocab.nerc.ac.uk/collection/P03/current/O005/> ;
    owl:deprecated "false" .
<http://vocab.nerc.ac.uk/collection/P02/current/SATM/> a glbase:MeasurementType,
        owl:Class,
        owl:NamedIndividual ;
    rdfs:label "Shellfish morphology, age and physiology"@en ;
    dcterms:creator "SeaDataNet" ;
    dcterms:date "2010-07-30 12:14:14.0" ;
    glbase:hasIdentifier [ glbase:hasIdentifierScheme idscheme:sdn ;
            glbase:hasIdentifierValue "SDN:P02::SATM" ] ;
    rdfs:comment "Paramaters that quantify the size, shape, age and life processes (including mortality) of shellfish (molluscs - including cephalopods - and crustaceans of interest to fisheries research and commercial fisheries)."@en ;
    rdfs:subClassOf <http://vocab.nerc.ac.uk/collection/P03/current/B027/>,
        <http://vocab.nerc.ac.uk/collection/P03/current/H004/> ;
    owl:deprecated "false" .
<http://vocab.nerc.ac.uk/collection/P02/current/SBPH/> a glbase:MeasurementType,
        owl:Class,
        owl:NamedIndividual ;
    rdfs:label "Seabed photography"@en ;
    dcterms:creator "SeaDataNet" ;
    dcterms:date "2009-04-20 08:33:04.0" ;
    glbase:hasIdentifier [ glbase:hasIdentifierScheme idscheme:sdn ;
            glbase:hasIdentifierValue "SDN:P02::SBPH" ] ;
    rdfs:comment "Digital images of the seabed obtained using either still or video cameras"@en ;
    rdfs:subClassOf <http://vocab.nerc.ac.uk/collection/P03/current/UWPH/> ;
    owl:deprecated "false" .
<http://vocab.nerc.ac.uk/collection/P02/current/SCAH/> a glbase:MeasurementType,
        owl:Class,
        owl:NamedIndividual ;
    rdfs:label "Concentration of polycyclic aromatic hydrocarbons (PAHs) in sediment samples"@en ;
    dcterms:creator "SeaDataNet" ;
    dcterms:date "2004-05-28 09:21:00.0" ;
    glbase:hasIdentifier [ glbase:hasIdentifierScheme idscheme:sdn ;
            glbase:hasIdentifierValue "SDN:P02::SCAH" ] ;
    rdfs:comment "PAH concentrations in sediment, which is considered to be anything from the bed sampled by a grab or corer, including 'fluff'"@en ;
    rdfs:subClassOf <http://vocab.nerc.ac.uk/collection/P03/current/C025/>,
        <http://vocab.nerc.ac.uk/collection/P03/current/C055/>,
        <http://vocab.nerc.ac.uk/collection/P03/current/G035/>,
        <http://vocab.nerc.ac.uk/collection/P03/current/H001/> ;
    owl:deprecated "false" .
<http://vocab.nerc.ac.uk/collection/P02/current/SCDO/> a glbase:MeasurementType,
        owl:Class,
        owl:NamedIndividual ;
    rdfs:label "Metal fluxes between the bed and the water column"@en ;
    dcterms:creator "SeaDataNet" ;
    dcterms:date "2004-08-18 15:49:27.0" ;
    glbase:hasIdentifier [ glbase:hasIdentifierScheme idscheme:sdn ;
            glbase:hasIdentifierValue "SDN:P02::SCDO" ] ;
    rdfs:comment "Parameters quantifying the exchange of metalsbetween the bed (ie the sediment) and the water column sometimes termed benthic fluxes"@en ;
    rdfs:subClassOf <http://vocab.nerc.ac.uk/collection/P03/current/O005/> ;
    owl:deprecated "false" .
<http://vocab.nerc.ac.uk/collection/P02/current/SCOC/> a glbase:MeasurementType,
        owl:Class,
        owl:NamedIndividual ;
    rdfs:label "Concentration of other organic contaminants in sediment samples"@en ;
    dcterms:creator "SeaDataNet" ;
    dcterms:date "2010-01-27 14:00:34.0" ;
    glbase:hasIdentifier [ glbase:hasIdentifierScheme idscheme:sdn ;
            glbase:hasIdentifierValue "SDN:P02::SCOC" ] ;
    rdfs:comment "Concentration parameters for carbon compounds regarded as environmentally harmful in sediment, which is considered to be anything from the bed sampled by a grab or corer, including 'fluff' that are not included in other specific categories"@en ;
    rdfs:subClassOf <http://vocab.nerc.ac.uk/collection/P03/current/C055/>,
        <http://vocab.nerc.ac.uk/collection/P03/current/G035/>,
        <http://vocab.nerc.ac.uk/collection/P03/current/H001/> ;
    owl:deprecated "false" .
<http://vocab.nerc.ac.uk/collection/P02/current/SCOX/> a glbase:MeasurementType,
        owl:Class,
        owl:NamedIndividual ;
    rdfs:label "Dissolved concentration parameters for other gases in the water column"@en ;
    dcterms:creator "SeaDataNet" ;
    dcterms:date "2010-11-08 15:08:09.0" ;
    glbase:hasIdentifier [ glbase:hasIdentifierScheme idscheme:sdn ;
            glbase:hasIdentifierValue "SDN:P02::SCOX" ] ;
    rdfs:comment "All concentration parameters for inorganic dissolved gases other than oxygen and the noble gases in the water column"@en ;
    rdfs:subClassOf <http://vocab.nerc.ac.uk/collection/P03/current/C015/> ;
    owl:deprecated "false" .
<http://vocab.nerc.ac.uk/collection/P02/current/SDAC/> a glbase:MeasurementType,
        owl:Class,
        owl:NamedIndividual ;
    rdfs:label "Sediment acoustics"@en ;
    dcterms:creator "SeaDataNet" ;
    dcterms:date "2007-11-22 11:35:40.0" ;
    glbase:hasIdentifier [ glbase:hasIdentifierScheme idscheme:sdn ;
            glbase:hasIdentifierValue "SDN:P02::SDAC" ] ;
    rdfs:comment "Parameters relating to the elucidation of sediment structure by quantifying the proportion of waves from a low energy source reflected by sub-surface layers."@en ;
    rdfs:subClassOf <http://vocab.nerc.ac.uk/collection/P03/current/G012/>,
        <http://vocab.nerc.ac.uk/collection/P03/current/GPYS/> ;
    owl:deprecated "false" .
<http://vocab.nerc.ac.uk/collection/P02/current/SDNA/> a glbase:MeasurementType,
        owl:Class,
        owl:NamedIndividual ;
    rdfs:label "Concentrations of biopolymers in sediment"@en ;
    dcterms:creator "SeaDataNet" ;
    dcterms:date "2014-02-20 09:20:24.0" ;
    glbase:hasIdentifier [ glbase:hasIdentifierScheme idscheme:sdn ;
            glbase:hasIdentifierValue "SDN:P02::SDNA" ] ;
    rdfs:comment "Parameters quantifying the amount of naturally-produced organic (molecules containing carbon) compounds that are built from multiple instances of structural units (monomers) that are covalently-bonded to produce larger structures in any sediment (material collected by a corer including fluff). Includes polynucleotides (RNA and DNA), polypeptides and polysaccharides (e.g. cellulose)."@en ;
    rdfs:subClassOf <http://vocab.nerc.ac.uk/collection/P03/current/C050/>,
        <http://vocab.nerc.ac.uk/collection/P03/current/G035/> ;
    owl:deprecated "false" .
<http://vocab.nerc.ac.uk/collection/P02/current/SEBH/> a glbase:MeasurementType,
        owl:Class,
        owl:NamedIndividual ;
    rdfs:label "Seal behaviour"@en ;
    dcterms:creator "SeaDataNet" ;
    dcterms:date "2008-01-30 07:53:20.0" ;
    glbase:hasIdentifier [ glbase:hasIdentifierScheme idscheme:sdn ;
            glbase:hasIdentifierValue "SDN:P02::SEBH" ] ;
    rdfs:comment "Parameters describing the actions or reactions of seals (Family Phocidae), usually in response to the environment. Includes both parameters mapped to taxa and those mapped to non-taxonomic groupings."@en ;
    rdfs:subClassOf <http://vocab.nerc.ac.uk/collection/P03/current/B015/> ;
    owl:deprecated "false" .
<http://vocab.nerc.ac.uk/collection/P02/current/SECC/> a glbase:MeasurementType,
        owl:Class,
        owl:NamedIndividual ;
    rdfs:label "Secchi disk depth"@en ;
    dcterms:creator "SeaDataNet" ;
    dcterms:date "2003-06-10 13:53:19.0" ;
    glbase:hasIdentifier [ glbase:hasIdentifierScheme idscheme:sdn ;
            glbase:hasIdentifierValue "SDN:P02::SECC" ] ;
    rdfs:comment "Measurements of optical visibility in the water column"@en ;
    rdfs:subClassOf <http://vocab.nerc.ac.uk/collection/P03/current/D015/> ;
    owl:deprecated "false" .
<http://vocab.nerc.ac.uk/collection/P02/current/SEMO/> a glbase:MeasurementType,
        owl:Class,
        owl:NamedIndividual ;
    rdfs:label "Seal mortality"@en ;
    dcterms:creator "SeaDataNet" ;
    dcterms:date "2008-02-04 15:04:29.0" ;
    glbase:hasIdentifier [ glbase:hasIdentifierScheme idscheme:sdn ;
            glbase:hasIdentifierValue "SDN:P02::SEMO" ] ;
    rdfs:comment "Parameters describing the causes and rate of mortality of Seals (Family Phocidae). Includes both parameters mapped to taxa and those mapped to non-taxonomic groupings."@en ;
    rdfs:subClassOf <http://vocab.nerc.ac.uk/collection/P03/current/B015/> ;
    owl:deprecated "false" .
<http://vocab.nerc.ac.uk/collection/P02/current/SEMP/> a glbase:MeasurementType,
        owl:Class,
        owl:NamedIndividual ;
    rdfs:label "Seal morphology and physiology"@en ;
    dcterms:creator "SeaDataNet" ;
    dcterms:date "2008-01-30 07:53:20.0" ;
    glbase:hasIdentifier [ glbase:hasIdentifierScheme idscheme:sdn ;
            glbase:hasIdentifierValue "SDN:P02::SEMP" ] ;
    rdfs:comment "Parameters describing the size, shape or physiological activity including disease and parasite infection status of seals (Family Phocidae). Includes both parameters mapped to taxa and those mapped to non-taxonomic groupings."@en ;
    rdfs:subClassOf <http://vocab.nerc.ac.uk/collection/P03/current/B015/> ;
    owl:deprecated "false" .
<http://vocab.nerc.ac.uk/collection/P02/current/SHTA/> a glbase:MeasurementType,
        owl:Class,
        owl:NamedIndividual ;
    rdfs:label "Hydrolytic activity in sediment"@en ;
    dcterms:creator "SeaDataNet" ;
    dcterms:date "2004-08-20 10:05:20.0" ;
    glbase:hasIdentifier [ glbase:hasIdentifierScheme idscheme:sdn ;
            glbase:hasIdentifierValue "SDN:P02::SHTA" ] ;
    rdfs:comment "" ;
    rdfs:subClassOf <http://vocab.nerc.ac.uk/collection/P03/current/G035/>,
        <http://vocab.nerc.ac.uk/collection/P03/current/G055/>,
        <http://vocab.nerc.ac.uk/collection/P03/current/O010/> ;
    owl:deprecated "false" .
<http://vocab.nerc.ac.uk/collection/P02/current/SIAT/> a glbase:MeasurementType,
        owl:Class,
        owl:NamedIndividual ;
    rdfs:label "Inorganic silicon species concentrations in the atmosphere"@en ;
    dcterms:creator "SeaDataNet" ;
    dcterms:date "2005-09-23 10:41:38.0" ;
    glbase:hasIdentifier [ glbase:hasIdentifierScheme idscheme:sdn ;
            glbase:hasIdentifierValue "SDN:P02::SIAT" ] ;
    rdfs:comment "Concentration of inorganic silicon species (element or compounds) in any phase of the atmosphere"@en ;
    rdfs:subClassOf <http://vocab.nerc.ac.uk/collection/P03/current/C045/>,
        <http://vocab.nerc.ac.uk/collection/P03/current/M005/> ;
    owl:deprecated "false" .
<http://vocab.nerc.ac.uk/collection/P02/current/SICN/> a glbase:MeasurementType,
        owl:Class,
        owl:NamedIndividual ;
    rdfs:label "Concentration of silicon species in sediment"@en ;
    dcterms:creator "SeaDataNet" ;
    dcterms:date "2010-11-05 12:41:29.0" ;
    glbase:hasIdentifier [ glbase:hasIdentifierScheme idscheme:sdn ;
            glbase:hasIdentifierValue "SDN:P02::SICN" ] ;
    rdfs:comment "Concentration parameters for silicon species (including opal) in sediment (anything collected by a corer including fluff)"@en ;
    rdfs:subClassOf <http://vocab.nerc.ac.uk/collection/P02/current/RMIN/> ;
    owl:deprecated "true" .
<http://vocab.nerc.ac.uk/collection/P02/current/SICO/> a glbase:MeasurementType,
        owl:Class,
        owl:NamedIndividual ;
    rdfs:label "Other fluxes between the bed and the water column"@en ;
    dcterms:creator "SeaDataNet" ;
    dcterms:date "2010-11-08 15:08:09.0" ;
    glbase:hasIdentifier [ glbase:hasIdentifierScheme idscheme:sdn ;
            glbase:hasIdentifierValue "SDN:P02::SICO" ] ;
    rdfs:comment "Fluxes of species other than metals and nutrients between the bed (ie the sediment) and the water column sometimes termed benthic fluxes or sediment demand"@en ;
    rdfs:subClassOf <http://vocab.nerc.ac.uk/collection/P03/current/O005/> ;
    owl:deprecated "false" .
<http://vocab.nerc.ac.uk/collection/P02/current/SIGT/> a glbase:MeasurementType,
        owl:Class,
        owl:NamedIndividual ;
    rdfs:label "Density of the water column"@en ;
    dcterms:creator "SeaDataNet" ;
    dcterms:date "2004-08-16 11:31:09.0" ;
    glbase:hasIdentifier [ glbase:hasIdentifierScheme idscheme:sdn ;
            glbase:hasIdentifierValue "SDN:P02::SIGT" ] ;
    rdfs:comment "Absolute determinations of water column density plus parameters (generally expressed as density anomaly) derived from temperature and salinity"@en ;
    rdfs:subClassOf <http://vocab.nerc.ac.uk/collection/P03/current/D020/> ;
    owl:deprecated "false" .
<http://vocab.nerc.ac.uk/collection/P02/current/SIPW/> a glbase:MeasurementType,
        owl:Class,
        owl:NamedIndividual ;
    rdfs:label "Stable isotope enrichment in sediment pore waters"@en ;
    dcterms:creator "SeaDataNet" ;
    dcterms:date "2008-07-01 08:37:30.0" ;
    glbase:hasIdentifier [ glbase:hasIdentifierScheme idscheme:sdn ;
            glbase:hasIdentifierValue "SDN:P02::SIPW" ] ;
    rdfs:comment "Parameters quantifying the relative proportions of stable isotopes in either the solute or solvent phase of sediment pore waters"@en ;
    rdfs:subClassOf <http://vocab.nerc.ac.uk/collection/P03/current/C030/>,
        <http://vocab.nerc.ac.uk/collection/P03/current/G050/> ;
    owl:deprecated "false" .
<http://vocab.nerc.ac.uk/collection/P02/current/SIXX/> a glbase:MeasurementType,
        owl:Class,
        owl:NamedIndividual ;
    rdfs:label "Concentration of silicon species in the water column"@en ;
    dcterms:creator "SeaDataNet" ;
    dcterms:date "2004-08-13 14:33:19.0" ;
    glbase:hasIdentifier [ glbase:hasIdentifierScheme idscheme:sdn ;
            glbase:hasIdentifierValue "SDN:P02::SIXX" ] ;
    rdfs:comment "Concentration parameters for silicon species (including opal) in all phases of the water column"@en ;
    rdfs:subClassOf <http://vocab.nerc.ac.uk/collection/P03/current/C045/> ;
    owl:deprecated "false" .
<http://vocab.nerc.ac.uk/collection/P02/current/SLCA/> a glbase:MeasurementType,
        owl:Class,
        owl:NamedIndividual ;
    rdfs:label "Silicate concentration parameters in the water column"@en ;
    dcterms:creator "SeaDataNet" ;
    dcterms:date "2004-05-27 10:07:25.0" ;
    glbase:hasIdentifier [ glbase:hasIdentifierScheme idscheme:sdn ;
            glbase:hasIdentifierValue "SDN:P02::SLCA" ] ;
    rdfs:comment "Silicate concentration parameters (including statistical parameters such as standard deviation) in the water column"@en ;
    rdfs:subClassOf <http://vocab.nerc.ac.uk/collection/P03/current/C040/> ;
    owl:deprecated "false" .
<http://vocab.nerc.ac.uk/collection/P02/current/SPAG/> a glbase:MeasurementType,
        owl:Class,
        owl:NamedIndividual ;
    rdfs:label "Speleothem age"@en ;
    dcterms:creator "SeaDataNet" ;
    dcterms:date "2006-06-21 09:23:05.0" ;
    glbase:hasIdentifier [ glbase:hasIdentifierScheme idscheme:sdn ;
            glbase:hasIdentifierValue "SDN:P02::SPAG" ] ;
    rdfs:comment "Measured or stratigraphically estimated ages of secondary mineral deposits in caves. This includes stalactites, stalagmites, flowstone, and crystal growths."@en ;
    rdfs:subClassOf <http://vocab.nerc.ac.uk/collection/P03/current/G030/> ;
    owl:deprecated "false" .
<http://vocab.nerc.ac.uk/collection/P02/current/SPCB/> a glbase:MeasurementType,
        owl:Class,
        owl:NamedIndividual ;
    rdfs:label "Concentration of polychlorobiphenyls (PCBs) in sediment samples"@en ;
    dcterms:creator "SeaDataNet" ;
    dcterms:date "2004-05-28 08:10:00.0" ;
    glbase:hasIdentifier [ glbase:hasIdentifierScheme idscheme:sdn ;
            glbase:hasIdentifierValue "SDN:P02::SPCB" ] ;
    rdfs:comment "PCB concentrations in sediment, which is considered to be anything from the bed sampled by a grab or corer, including 'fluff'"@en ;
    rdfs:subClassOf <http://vocab.nerc.ac.uk/collection/P03/current/C055/>,
        <http://vocab.nerc.ac.uk/collection/P03/current/G035/>,
        <http://vocab.nerc.ac.uk/collection/P03/current/H001/> ;
    owl:deprecated "false" .
<http://vocab.nerc.ac.uk/collection/P02/current/SPGS/> a glbase:MeasurementType,
        owl:Class,
        owl:NamedIndividual ;
    rdfs:label "Suspended particulate material grain size parameters"@en ;
    dcterms:creator "SeaDataNet" ;
    dcterms:date "2004-10-26 14:53:00.0" ;
    glbase:hasIdentifier [ glbase:hasIdentifierScheme idscheme:sdn ;
            glbase:hasIdentifierValue "SDN:P02::SPGS" ] ;
    rdfs:comment "Includes all SPM grain size measurements and derived statistics"@en ;
    rdfs:subClassOf <http://vocab.nerc.ac.uk/collection/P03/current/G015/> ;
    owl:deprecated "false" .
<http://vocab.nerc.ac.uk/collection/P02/current/SPHT/> a glbase:MeasurementType,
        owl:Class,
        owl:NamedIndividual ;
    rdfs:label "Concentration of inorganic sulphur species in sediment pore water"@en ;
    dcterms:creator "SeaDataNet" ;
    dcterms:date "2004-08-13 12:35:54.0" ;
    glbase:hasIdentifier [ glbase:hasIdentifierScheme idscheme:sdn ;
            glbase:hasIdentifierValue "SDN:P02::SPHT" ] ;
    rdfs:comment "Concentration parameters (including saturation if gaseous) for inorganic sulphur species in all phases of sediment pore waters"@en ;
    rdfs:subClassOf <http://vocab.nerc.ac.uk/collection/P03/current/C045/> ;
    owl:deprecated "false" .
<http://vocab.nerc.ac.uk/collection/P02/current/SPOL/> a glbase:MeasurementType,
        owl:Class,
        owl:NamedIndividual ;
    rdfs:label "Sediment pollen content"@en ;
    dcterms:creator "SeaDataNet" ;
    dcterms:date "2003-06-10 13:53:19.0" ;
    glbase:hasIdentifier [ glbase:hasIdentifierScheme idscheme:sdn ;
            glbase:hasIdentifierValue "SDN:P02::SPOL" ] ;
    rdfs:comment "" ;
    rdfs:subClassOf <http://vocab.nerc.ac.uk/collection/P03/current/G055/> ;
    owl:deprecated "false" .
<http://vocab.nerc.ac.uk/collection/P02/current/SPRO/> a glbase:MeasurementType,
        owl:Class,
        owl:NamedIndividual ;
    rdfs:label "Concentration of proteins in sediment"@en ;
    dcterms:creator "SeaDataNet" ;
    dcterms:date "2004-08-13 11:31:01.0" ;
    glbase:hasIdentifier [ glbase:hasIdentifierScheme idscheme:sdn ;
            glbase:hasIdentifierValue "SDN:P02::SPRO" ] ;
    rdfs:comment "Concentrations of proteins per unit mass or unit volume of sediment (material collected by a corer including fluff)"@en ;
    rdfs:subClassOf <http://vocab.nerc.ac.uk/collection/P03/current/C050/>,
        <http://vocab.nerc.ac.uk/collection/P03/current/G035/> ;
    owl:deprecated "false" .
<http://vocab.nerc.ac.uk/collection/P02/current/SPWC/> a glbase:MeasurementType,
        owl:Class,
        owl:NamedIndividual ;
    rdfs:label "Concentration of inorganic sulphur species in the water column"@en ;
    dcterms:creator "SeaDataNet" ;
    dcterms:date "2004-08-13 12:47:00.0" ;
    glbase:hasIdentifier [ glbase:hasIdentifierScheme idscheme:sdn ;
            glbase:hasIdentifierValue "SDN:P02::SPWC" ] ;
    rdfs:comment "Concentration parameters (including saturation if gaseous) for inorganic sulphur species in all phases of the water column"@en ;
    rdfs:subClassOf <http://vocab.nerc.ac.uk/collection/P03/current/C045/> ;
    owl:deprecated "false" .
<http://vocab.nerc.ac.uk/collection/P02/current/SR2D/> a glbase:MeasurementType,
        owl:Class,
        owl:NamedIndividual ;
    rdfs:label "Two-dimensional seismic reflection"@en ;
    dcterms:creator "SeaDataNet" ;
    dcterms:date "2010-02-21 17:25:39.0" ;
    glbase:hasIdentifier [ glbase:hasIdentifierScheme idscheme:sdn ;
            glbase:hasIdentifierValue "SDN:P02::SR2D" ] ;
    rdfs:comment "Parameters relating to structure beneath sea-bed determined by the reflection of seismic energy along a single track."@en ;
    rdfs:subClassOf <http://vocab.nerc.ac.uk/collection/P02/current/SRFL/>,
        <http://vocab.nerc.ac.uk/collection/P03/current/G012/>,
        <http://vocab.nerc.ac.uk/collection/P03/current/GPYS/> ;
    owl:deprecated "false" .
<http://vocab.nerc.ac.uk/collection/P02/current/SR3D/> a glbase:MeasurementType,
        owl:Class,
        owl:NamedIndividual ;
    rdfs:label "Three-dimensional seismic reflection"@en ;
    dcterms:creator "SeaDataNet" ;
    dcterms:date "2010-02-21 17:25:54.0" ;
    glbase:hasIdentifier [ glbase:hasIdentifierScheme idscheme:sdn ;
            glbase:hasIdentifierValue "SDN:P02::SR3D" ] ;
    rdfs:comment "Parameters relating to structure beneath sea-bed determined by the reflection of seismic energy along multiple parallel tracks."@en ;
    rdfs:subClassOf <http://vocab.nerc.ac.uk/collection/P02/current/SRFL/>,
        <http://vocab.nerc.ac.uk/collection/P03/current/G012/>,
        <http://vocab.nerc.ac.uk/collection/P03/current/GPYS/> ;
    owl:deprecated "false" .
<http://vocab.nerc.ac.uk/collection/P02/current/SRAD/> a glbase:MeasurementType,
        owl:Class,
        owl:NamedIndividual ;
    rdfs:label "Geological sample radioactivity"@en ;
    dcterms:creator "SeaDataNet" ;
    dcterms:date "2010-10-22 10:24:53.0" ;
    glbase:hasIdentifier [ glbase:hasIdentifierScheme idscheme:sdn ;
            glbase:hasIdentifierValue "SDN:P02::SRAD" ] ;
    rdfs:comment "Any parameters quantifying ionising radiation emitted by cores or samples comprising rock, sediment (including surface sediment such as fluff)"@en ;
    rdfs:subClassOf <http://vocab.nerc.ac.uk/collection/P03/current/C030/>,
        <http://vocab.nerc.ac.uk/collection/P03/current/G035/> ;
    owl:deprecated "false" .
<http://vocab.nerc.ac.uk/collection/P02/current/SREP/> a glbase:MeasurementType,
        owl:Class,
        owl:NamedIndividual ;
    rdfs:label "Shellfish reproduction"@en ;
    dcterms:creator "SeaDataNet" ;
    dcterms:date "2010-07-30 12:05:29.0" ;
    glbase:hasIdentifier [ glbase:hasIdentifierScheme idscheme:sdn ;
            glbase:hasIdentifierValue "SDN:P02::SREP" ] ;
    rdfs:comment "Paramaters that quantify the fecundity, reproductive rates or nature of reproduction in shellfish (molluscs - including cephalopods - and crustaceans of interest to fisheries research and commercial fisheries)."@en ;
    rdfs:subClassOf <http://vocab.nerc.ac.uk/collection/P03/current/B027/>,
        <http://vocab.nerc.ac.uk/collection/P03/current/H004/> ;
    owl:deprecated "false" .
<http://vocab.nerc.ac.uk/collection/P02/current/SRFR/> a glbase:MeasurementType,
        owl:Class,
        owl:NamedIndividual ;
    rdfs:label "Seismic refraction"@en ;
    dcterms:creator "SeaDataNet" ;
    dcterms:date "2007-11-22 11:35:40.0" ;
    glbase:hasIdentifier [ glbase:hasIdentifierScheme idscheme:sdn ;
            glbase:hasIdentifierValue "SDN:P02::SRFR" ] ;
    rdfs:comment "Parameters relating to the elucidation of geological structure by quantifying the refration of waves from a high energy source by sub-surface layers."@en ;
    rdfs:subClassOf <http://vocab.nerc.ac.uk/collection/P03/current/G012/> ;
    owl:deprecated "false" .
<http://vocab.nerc.ac.uk/collection/P02/current/SSCN/> a glbase:MeasurementType,
        owl:Class,
        owl:NamedIndividual ;
    rdfs:label "Side-scan sonar"@en ;
    dcterms:creator "SeaDataNet" ;
    dcterms:date "2006-06-28 17:37:15.0" ;
    glbase:hasIdentifier [ glbase:hasIdentifierScheme idscheme:sdn ;
            glbase:hasIdentifierValue "SDN:P02::SSCN" ] ;
    rdfs:comment "A technique for mapping the morphology of the seafloor using a sonar swath projected sideways from a towed underwater vehicle."@en ;
    rdfs:subClassOf <http://vocab.nerc.ac.uk/collection/P03/current/G012/> ;
    owl:deprecated "false" .
<http://vocab.nerc.ac.uk/collection/P02/current/SSTB/> a glbase:MeasurementType,
        owl:Class,
        owl:NamedIndividual ;
    rdfs:label "Stable isotope enrichment in sediment"@en ;
    dcterms:creator "SeaDataNet" ;
    dcterms:date "2008-07-01 08:38:07.0" ;
    glbase:hasIdentifier [ glbase:hasIdentifierScheme idscheme:sdn ;
            glbase:hasIdentifierValue "SDN:P02::SSTB" ] ;
    rdfs:comment "Stable isotope enrichment parameters in sediment, including biota-associated parameters such as isotope enrichment in foraminifera tests"@en ;
    rdfs:subClassOf <http://vocab.nerc.ac.uk/collection/P03/current/C030/>,
        <http://vocab.nerc.ac.uk/collection/P03/current/G035/> ;
    owl:deprecated "false" .
<http://vocab.nerc.ac.uk/collection/P02/current/SSTR/> a glbase:MeasurementType,
        owl:Class,
        owl:NamedIndividual ;
    rdfs:label "Sedimentary structure"@en ;
    dcterms:creator "SeaDataNet" ;
    dcterms:date "2010-10-01 09:30:27.0" ;
    glbase:hasIdentifier [ glbase:hasIdentifierScheme idscheme:sdn ;
            glbase:hasIdentifierValue "SDN:P02::SSTR" ] ;
    rdfs:comment "Parameters characterising structure in sedimentary rocks and unlithified sediment such as bedding, lamination and bioturbation."@en ;
    rdfs:subClassOf <http://vocab.nerc.ac.uk/collection/P03/current/GSED/> ;
    owl:deprecated "false" .
<http://vocab.nerc.ac.uk/collection/P02/current/STCO/> a glbase:MeasurementType,
        owl:Class,
        owl:NamedIndividual ;
    rdfs:label "Sediment thermal conductivity"@en ;
    dcterms:creator "SeaDataNet" ;
    dcterms:date "2010-02-21 17:28:04.0" ;
    glbase:hasIdentifier [ glbase:hasIdentifierScheme idscheme:sdn ;
            glbase:hasIdentifierValue "SDN:P02::STCO" ] ;
    rdfs:comment "Parameters that describe the degree to which unlithified sediment is able to conduct heat"@en ;
    rdfs:subClassOf <http://vocab.nerc.ac.uk/collection/P03/current/G040/>,
        <http://vocab.nerc.ac.uk/collection/P03/current/GTHM/> ;
    owl:deprecated "false" .
<http://vocab.nerc.ac.uk/collection/P02/current/STOM/> a glbase:MeasurementType,
        owl:Class,
        owl:NamedIndividual ;
    rdfs:label "Concentration of organic matter in sediments"@en ;
    dcterms:creator "SeaDataNet" ;
    dcterms:date "2008-06-30 10:31:40.0" ;
    glbase:hasIdentifier [ glbase:hasIdentifierScheme idscheme:sdn ;
            glbase:hasIdentifierValue "SDN:P02::STOM" ] ;
    rdfs:comment "Parameters quantifying the proportion of organic material in a soil or sediment sample"@en ;
    rdfs:subClassOf <http://vocab.nerc.ac.uk/collection/P03/current/G035/> ;
    owl:deprecated "false" .
<http://vocab.nerc.ac.uk/collection/P02/current/SUAT/> a glbase:MeasurementType,
        owl:Class,
        owl:NamedIndividual ;
    rdfs:label "Sulphur species concentrations in the atmosphere"@en ;
    dcterms:creator "SeaDataNet" ;
    dcterms:date "2006-06-05 11:38:28.0" ;
    glbase:hasIdentifier [ glbase:hasIdentifierScheme idscheme:sdn ;
            glbase:hasIdentifierValue "SDN:P02::SUAT" ] ;
    rdfs:comment "Concentration of sulphur species (element or compounds) in any phase of the atmosphere. Includes sulphur dioxide."@en ;
    rdfs:subClassOf <http://vocab.nerc.ac.uk/collection/P03/current/C045/>,
        <http://vocab.nerc.ac.uk/collection/P03/current/M005/> ;
    owl:deprecated "false" .
<http://vocab.nerc.ac.uk/collection/P02/current/SVEL/> a glbase:MeasurementType,
        owl:Class,
        owl:NamedIndividual ;
    rdfs:label "Sound velocity and travel time in the water column"@en ;
    dcterms:creator "SeaDataNet" ;
    dcterms:date "2004-08-19 08:17:17.0" ;
    glbase:hasIdentifier [ glbase:hasIdentifierScheme idscheme:sdn ;
            glbase:hasIdentifierValue "SDN:P02::SVEL" ] ;
    rdfs:comment "" ;
    rdfs:subClassOf <http://vocab.nerc.ac.uk/collection/P03/current/D005/> ;
    owl:deprecated "false" .
<http://vocab.nerc.ac.uk/collection/P02/current/SXCN/> a glbase:MeasurementType,
        owl:Class,
        owl:NamedIndividual ;
    rdfs:label "Concentration of inorganic sulphur species in suspended particulate material"@en ;
    dcterms:creator "SeaDataNet" ;
    dcterms:date "2004-08-13 14:10:16.0" ;
    glbase:hasIdentifier [ glbase:hasIdentifierScheme idscheme:sdn ;
            glbase:hasIdentifierValue "SDN:P02::SXCN" ] ;
    rdfs:comment "Concentration parameters for inorganic sulphur species in suspended particulate material (anything collected by filtration or sediment trapping).  Group does not include parameters expressing data per unit volume of the water column"@en ;
    rdfs:subClassOf <http://vocab.nerc.ac.uk/collection/P03/current/C045/>,
        <http://vocab.nerc.ac.uk/collection/P03/current/G015/> ;
    owl:deprecated "false" .
<http://vocab.nerc.ac.uk/collection/P02/current/TADN/> a glbase:MeasurementType,
        owl:Class,
        owl:NamedIndividual ;
    rdfs:label "Concentration of adenylates in sediment"@en ;
    dcterms:creator "SeaDataNet" ;
    dcterms:date "2004-08-13 11:17:06.0" ;
    glbase:hasIdentifier [ glbase:hasIdentifierScheme idscheme:sdn ;
            glbase:hasIdentifierValue "SDN:P02::TADN" ] ;
    rdfs:comment "Concentrations of adenylates (ADP, ATP etc) per unit mass or unit volume of sediment (material collected by a corer including fluff)"@en ;
    rdfs:subClassOf <http://vocab.nerc.ac.uk/collection/P03/current/C050/>,
        <http://vocab.nerc.ac.uk/collection/P03/current/G035/> ;
    owl:deprecated "false" .
<http://vocab.nerc.ac.uk/collection/P02/current/TBGZ/> a glbase:MeasurementType,
        owl:Class,
        owl:NamedIndividual ;
    rdfs:label "Bacterial consumption in the water column"@en ;
    dcterms:creator "SeaDataNet" ;
    dcterms:date "2004-08-19 10:30:38.0" ;
    glbase:hasIdentifier [ glbase:hasIdentifierScheme idscheme:sdn ;
            glbase:hasIdentifierValue "SDN:P02::TBGZ" ] ;
    rdfs:comment "" ;
    rdfs:subClassOf <http://vocab.nerc.ac.uk/collection/P03/current/B005/>,
        <http://vocab.nerc.ac.uk/collection/P03/current/O010/> ;
    owl:deprecated "false" .
<http://vocab.nerc.ac.uk/collection/P02/current/TCFX/> a glbase:MeasurementType,
        owl:Class,
        owl:NamedIndividual ;
    rdfs:label "Sedimentation flux of carbon, nitrogen or organic matter in the water column"@en ;
    dcterms:creator "SeaDataNet" ;
    dcterms:date "2008-11-25 15:43:03.0" ;
    glbase:hasIdentifier [ glbase:hasIdentifierScheme idscheme:sdn ;
            glbase:hasIdentifierValue "SDN:P02::TCFX" ] ;
    rdfs:comment "Fluxes of particulate total, organic and inorganic carbon (including as CaCO3) and nitrogen (often measured as 'total' but assumed to be 'organic'). Organic matter is defined as matter lost on ignition."@en ;
    rdfs:subClassOf <http://vocab.nerc.ac.uk/collection/P03/current/O005/> ;
    owl:deprecated "false" .
<http://vocab.nerc.ac.uk/collection/P02/current/TCNT/> a glbase:MeasurementType,
        owl:Class,
        owl:NamedIndividual ;
    rdfs:label "Raw temperature and/or salinity instrument output"@en ;
    dcterms:creator "SeaDataNet" ;
    dcterms:date "2003-11-06 00:00:00.0" ;
    glbase:hasIdentifier [ glbase:hasIdentifierScheme idscheme:sdn ;
            glbase:hasIdentifierValue "SDN:P02::TCNT" ] ;
    rdfs:comment "Direct output parameters from TS instruments such as thermosalinograph or CTD"@en ;
    rdfs:subClassOf <http://vocab.nerc.ac.uk/collection/P03/current/D025/> ;
    owl:deprecated "false" .
<http://vocab.nerc.ac.uk/collection/P02/current/TCO2/> a glbase:MeasurementType,
        owl:Class,
        owl:NamedIndividual ;
    rdfs:label "Total dissolved inorganic carbon (TCO2) concentration in the water column"@en ;
    dcterms:creator "SeaDataNet" ;
    dcterms:date "2003-06-10 13:53:19.0" ;
    glbase:hasIdentifier [ glbase:hasIdentifierScheme idscheme:sdn ;
            glbase:hasIdentifierValue "SDN:P02::TCO2" ] ;
    rdfs:comment "" ;
    rdfs:subClassOf <http://vocab.nerc.ac.uk/collection/P03/current/C005/>,
        <http://vocab.nerc.ac.uk/collection/P03/current/C010/> ;
    owl:deprecated "false" .
<http://vocab.nerc.ac.uk/collection/P02/current/TD00/> a glbase:MeasurementType,
        owl:Class,
        owl:NamedIndividual ;
    rdfs:label "Terrestrial detritus in the water column suspended particulate material"@en ;
    dcterms:creator "SeaDataNet" ;
    dcterms:date "2004-08-18 08:43:46.0" ;
    glbase:hasIdentifier [ glbase:hasIdentifierScheme idscheme:sdn ;
            glbase:hasIdentifierValue "SDN:P02::TD00" ] ;
    rdfs:comment "Parameters quantifying and categorising terrestrially-derived detritus (eg dust and pollen) in the water column"@en ;
    rdfs:subClassOf <http://vocab.nerc.ac.uk/collection/P03/current/G015/> ;
    owl:deprecated "false" .
<http://vocab.nerc.ac.uk/collection/P02/current/TDIN/> a glbase:MeasurementType,
        owl:Class,
        owl:NamedIndividual ;
    rdfs:label "Dissolved inorganic nitrogen concentration in the water column"@en ;
    dcterms:creator "SeaDataNet" ;
    dcterms:date "2003-06-10 13:53:19.0" ;
    glbase:hasIdentifier [ glbase:hasIdentifierScheme idscheme:sdn ;
            glbase:hasIdentifierValue "SDN:P02::TDIN" ] ;
    rdfs:comment "Total concentration of all dissolved inorganic nitrogen species in the water column, usually derived by summation of individual nutrient concentrations (NO3+NO2+NH4). Some workers may also include urea."@en ;
    rdfs:subClassOf <http://vocab.nerc.ac.uk/collection/P03/current/C005/>,
        <http://vocab.nerc.ac.uk/collection/P03/current/C040/> ;
    owl:deprecated "false" .
<http://vocab.nerc.ac.uk/collection/P02/current/TDNT/> a glbase:MeasurementType,
        owl:Class,
        owl:NamedIndividual ;
    rdfs:label "Dissolved total and organic nitrogen concentrations in the water column"@en ;
    dcterms:creator "SeaDataNet" ;
    dcterms:date "2004-10-22 13:57:38.0" ;
    glbase:hasIdentifier [ glbase:hasIdentifierScheme idscheme:sdn ;
            glbase:hasIdentifierValue "SDN:P02::TDNT" ] ;
    rdfs:comment "Concentration of total (organic plus inorganic) or organic dissolved nitrogen per unit volume of the water column.  Grouped together as organic nitrogen frequently determined as total nitrogen."@en ;
    rdfs:subClassOf <http://vocab.nerc.ac.uk/collection/P03/current/C005/> ;
    owl:deprecated "false" .
<http://vocab.nerc.ac.uk/collection/P02/current/TDPX/> a glbase:MeasurementType,
        owl:Class,
        owl:NamedIndividual ;
    rdfs:label "Dissolved total or organic phosphorus concentration in the water column"@en ;
    dcterms:creator "SeaDataNet" ;
    dcterms:date "2004-10-22 14:01:05.0" ;
    glbase:hasIdentifier [ glbase:hasIdentifierScheme idscheme:sdn ;
            glbase:hasIdentifierValue "SDN:P02::TDPX" ] ;
    rdfs:comment "Concentration of total (organic plus inorganic) or organic dissolved phosphorus per unit volume of the water column. Grouped together as organic phosphorus frequently determined as total phosphorus."@en ;
    rdfs:subClassOf <http://vocab.nerc.ac.uk/collection/P03/current/C005/> ;
    owl:deprecated "false" .
<http://vocab.nerc.ac.uk/collection/P02/current/TEMP/> a glbase:MeasurementType,
        owl:Class,
        owl:NamedIndividual ;
    rdfs:label "Temperature of the water column"@en ;
    dcterms:creator "SeaDataNet" ;
    dcterms:date "2007-03-02 11:33:02.0" ;
    glbase:hasIdentifier [ glbase:hasIdentifierScheme idscheme:sdn ;
            glbase:hasIdentifierValue "SDN:P02::TEMP" ] ;
    rdfs:comment "Temperature parameters in any body of water at any point between the bed and the atmosphere excluding the top few microns sampled by radiometers known as the skin"@en ;
    rdfs:subClassOf <http://vocab.nerc.ac.uk/collection/P03/current/D025/> ;
    owl:deprecated "false" .
<http://vocab.nerc.ac.uk/collection/P02/current/TFAA/> a glbase:MeasurementType,
        owl:Class,
        owl:NamedIndividual ;
    rdfs:label "Dissolved amino acid concentrations in the water column"@en ;
    dcterms:creator "SeaDataNet" ;
    dcterms:date "2008-12-09 11:24:54.0" ;
    glbase:hasIdentifier [ glbase:hasIdentifierScheme idscheme:sdn ;
            glbase:hasIdentifierValue "SDN:P02::TFAA" ] ;
    rdfs:comment "Parameters quantifying the amount of organic compounds containing both a carboxyl group and an amino group dissolved in a body of water."@en ;
    rdfs:subClassOf <http://vocab.nerc.ac.uk/collection/P03/current/C003/> ;
    owl:deprecated "false" .
<http://vocab.nerc.ac.uk/collection/P02/current/TMES/> a glbase:MeasurementType,
        owl:Class,
        owl:NamedIndividual ;
    rdfs:label "Metadata parameters"@en ;
    dcterms:creator "SeaDataNet" ;
    dcterms:date "2004-08-17 11:46:57.0" ;
    glbase:hasIdentifier [ glbase:hasIdentifierScheme idscheme:sdn ;
            glbase:hasIdentifierValue "SDN:P02::TMES" ] ;
    rdfs:comment "Data parameters that carry information relating to a measured parameter such as measurement temperatures, integration depths, quantities sampled and incubation durations"@en ;
    rdfs:subClassOf <http://vocab.nerc.ac.uk/collection/P03/current/Z005/> ;
    owl:deprecated "false" .
<http://vocab.nerc.ac.uk/collection/P02/current/TNRP/> a glbase:MeasurementType,
        owl:Class,
        owl:NamedIndividual ;
    rdfs:label "Dissolved inorganic carbon production and respiration in the water column"@en ;
    dcterms:creator "SeaDataNet" ;
    dcterms:date "2004-08-19 10:40:19.0" ;
    glbase:hasIdentifier [ glbase:hasIdentifierScheme idscheme:sdn ;
            glbase:hasIdentifierValue "SDN:P02::TNRP" ] ;
    rdfs:comment "Parameters related to the rates of TCO2 production and consumption based on light/dark bottle incubations"@en ;
    rdfs:subClassOf <http://vocab.nerc.ac.uk/collection/P03/current/O010/> ;
    owl:deprecated "false" .
<http://vocab.nerc.ac.uk/collection/P02/current/TOCH/> a glbase:MeasurementType,
        owl:Class,
        owl:NamedIndividual ;
    rdfs:label "Concentration of carbohydrates, phenols, alkanols (alcohols), aldehydes and ketones in water bodies"@en ;
    dcterms:creator "SeaDataNet" ;
    dcterms:date "2012-03-01 16:21:17.0" ;
    glbase:hasIdentifier [ glbase:hasIdentifierScheme idscheme:sdn ;
            glbase:hasIdentifierValue "SDN:P02::TOCH" ] ;
    rdfs:comment "Concentrations of carbohydrates, phenols, alkanols (alcohols), aldehydes and simple (non-alkenone) ketones in all phases of any body of fresh or salt water"@en ;
    rdfs:subClassOf <http://vocab.nerc.ac.uk/collection/P03/current/C050/> ;
    owl:deprecated "false" .
<http://vocab.nerc.ac.uk/collection/P02/current/TPHS/> a glbase:MeasurementType,
        owl:Class,
        owl:NamedIndividual ;
    rdfs:label "Particulate total and organic phosphorus concentrations in the water column"@en ;
    dcterms:creator "SeaDataNet" ;
    dcterms:date "2004-10-25 09:12:47.0" ;
    glbase:hasIdentifier [ glbase:hasIdentifierScheme idscheme:sdn ;
            glbase:hasIdentifierValue "SDN:P02::TPHS" ] ;
    rdfs:comment "Concentrations of total and organic phosphorus in the particulate phase of the water column, which is a function of both the SPM concentration in the water column and the concentration of phosphorus per unit weight of SPM."@en ;
    rdfs:subClassOf <http://vocab.nerc.ac.uk/collection/P03/current/C005/> ;
    owl:deprecated "false" .
<http://vocab.nerc.ac.uk/collection/P02/current/TRAN/> a glbase:MeasurementType,
        owl:Class,
        owl:NamedIndividual ;
    rdfs:label "Transport activity"@en ;
    dcterms:creator "SeaDataNet" ;
    dcterms:date "2008-12-09 10:17:11.0" ;
    glbase:hasIdentifier [ glbase:hasIdentifierScheme idscheme:sdn ;
            glbase:hasIdentifierValue "SDN:P02::TRAN" ] ;
    rdfs:comment "Parameters quantifying the level of activity moving people or cargo from one place to another."@en ;
    rdfs:subClassOf <http://vocab.nerc.ac.uk/collection/P03/current/H005/> ;
    owl:deprecated "false" .
<http://vocab.nerc.ac.uk/collection/P02/current/TRIS/> a glbase:MeasurementType,
        owl:Class,
        owl:NamedIndividual ;
    rdfs:label "Concentration of inorganic sulphur species in sediment"@en ;
    dcterms:creator "SeaDataNet" ;
    dcterms:date "2004-08-13 14:05:26.0" ;
    glbase:hasIdentifier [ glbase:hasIdentifierScheme idscheme:sdn ;
            glbase:hasIdentifierValue "SDN:P02::TRIS" ] ;
    rdfs:comment "Concentration parameters for inorganic sulphur species in sediment (anything collected by a corer including fluff)"@en ;
    rdfs:subClassOf <http://vocab.nerc.ac.uk/collection/P03/current/C045/>,
        <http://vocab.nerc.ac.uk/collection/P03/current/G035/> ;
    owl:deprecated "false" .
<http://vocab.nerc.ac.uk/collection/P02/current/TSED/> a glbase:MeasurementType,
        owl:Class,
        owl:NamedIndividual ;
    rdfs:label "Concentration of suspended particulate material in the water column"@en ;
    dcterms:creator "SeaDataNet" ;
    dcterms:date "2004-08-17 14:25:41.0" ;
    glbase:hasIdentifier [ glbase:hasIdentifierScheme idscheme:sdn ;
            glbase:hasIdentifierValue "SDN:P02::TSED" ] ;
    rdfs:comment "Parameters quantifying SPM concentration in the water column by weight, by volume or in terms of turbidity"@en ;
    rdfs:subClassOf <http://vocab.nerc.ac.uk/collection/P03/current/G015/> ;
    owl:deprecated "false" .
<http://vocab.nerc.ac.uk/collection/P02/current/TVLT/> a glbase:MeasurementType,
        owl:Class,
        owl:NamedIndividual ;
    rdfs:label "Raw suspended particulate material concentration sensor output"@en ;
    dcterms:creator "SeaDataNet" ;
    dcterms:date "2014-01-21 12:11:37.0" ;
    glbase:hasIdentifier [ glbase:hasIdentifierScheme idscheme:sdn ;
            glbase:hasIdentifierValue "SDN:P02::TVLT" ] ;
    rdfs:comment "Raw parameters (voltages and counts) from in-situ suspended particulate material sensors including transmissometers, nephelometers,in-situ particle sizers and ABS (including ADCP echo intensity)."@en ;
    rdfs:subClassOf <http://vocab.nerc.ac.uk/collection/P03/current/D015/>,
        <http://vocab.nerc.ac.uk/collection/P03/current/G015/> ;
    owl:deprecated "false" .
<http://vocab.nerc.ac.uk/collection/P02/current/UPTH/> a glbase:MeasurementType,
        owl:Class,
        owl:NamedIndividual ;
    rdfs:label "Bacterial production in the water column"@en ;
    dcterms:creator "SeaDataNet" ;
    dcterms:date "2005-04-27 12:10:16.0" ;
    glbase:hasIdentifier [ glbase:hasIdentifierScheme idscheme:sdn ;
            glbase:hasIdentifierValue "SDN:P02::UPTH" ] ;
    rdfs:comment "Parameters related to bacterial production determination by measurement of dissolved organic molecule (e.g. leucine, thymidine) uptake rates"@en ;
    rdfs:subClassOf <http://vocab.nerc.ac.uk/collection/P03/current/B005/>,
        <http://vocab.nerc.ac.uk/collection/P03/current/O010/> ;
    owl:deprecated "false" .
<http://vocab.nerc.ac.uk/collection/P02/current/UREA/> a glbase:MeasurementType,
        owl:Class,
        owl:NamedIndividual ;
    rdfs:label "Urea concentration parameters in the water column"@en ;
    dcterms:creator "SeaDataNet" ;
    dcterms:date "2004-05-27 10:06:04.0" ;
    glbase:hasIdentifier [ glbase:hasIdentifierScheme idscheme:sdn ;
            glbase:hasIdentifierValue "SDN:P02::UREA" ] ;
    rdfs:comment "Urea concentration parameters (including statistical parameters such as standard deviation) in the water column"@en ;
    rdfs:subClassOf <http://vocab.nerc.ac.uk/collection/P03/current/C005/>,
        <http://vocab.nerc.ac.uk/collection/P03/current/C040/> ;
    owl:deprecated "false" .
<http://vocab.nerc.ac.uk/collection/P02/current/UVRD/> a glbase:MeasurementType,
        owl:Class,
        owl:NamedIndividual ;
    rdfs:label "Ultra-violet (UV) radiation"@en ;
    dcterms:creator "SeaDataNet" ;
    dcterms:date "2007-11-21 16:30:18.0" ;
    glbase:hasIdentifier [ glbase:hasIdentifierScheme idscheme:sdn ;
            glbase:hasIdentifierValue "SDN:P02::UVRD" ] ;
    rdfs:comment "Parameters relating to the intensity of ultra-violet radiation in either the atmosphere or the water column"@en ;
    rdfs:subClassOf <http://vocab.nerc.ac.uk/collection/P03/current/M010/> ;
    owl:deprecated "false" .
<http://vocab.nerc.ac.uk/collection/P02/current/V999/> a glbase:MeasurementType,
        owl:Class,
        owl:NamedIndividual ;
    rdfs:label "Microzooplankton taxonomy-related biovolume per unit volume of the water column"@en ;
    dcterms:creator "SeaDataNet" ;
    dcterms:date "2003-06-10 13:53:19.0" ;
    glbase:hasIdentifier [ glbase:hasIdentifierScheme idscheme:sdn ;
            glbase:hasIdentifierValue "SDN:P02::V999" ] ;
    rdfs:comment "Microzooplankton biovolume parameters presented at the level of taxa that may be mapped to entities in the ITIS taxonomy. These may be at any taxonomic level from sub-species upwards."@en ;
    rdfs:subClassOf <http://vocab.nerc.ac.uk/collection/P03/current/B025/> ;
    owl:deprecated "false" .
<http://vocab.nerc.ac.uk/collection/P02/current/VATX/> a glbase:MeasurementType,
        owl:Class,
        owl:NamedIndividual ;
    rdfs:label "Phytoplankton taxonomic volume in water bodies"@en ;
    dcterms:creator "SeaDataNet" ;
    dcterms:date "2010-10-21 13:53:17.0" ;
    glbase:hasIdentifier [ glbase:hasIdentifierScheme idscheme:sdn ;
            glbase:hasIdentifierValue "SDN:P02::VATX" ] ;
    rdfs:comment "Any parameterisation of cell volume of free-floating autotrophic biological entities designated by taxonomic names (e.g. species, genus, family) in any body of fresh or salt water."@en ;
    rdfs:subClassOf <http://vocab.nerc.ac.uk/collection/P03/current/B030/> ;
    owl:deprecated "false" .
<http://vocab.nerc.ac.uk/collection/P02/current/VDFC/> a glbase:MeasurementType,
        owl:Class,
        owl:NamedIndividual ;
    rdfs:label "Transport in the water column"@en ;
    dcterms:creator "SeaDataNet" ;
    dcterms:date "2004-08-16 11:57:26.0" ;
    glbase:hasIdentifier [ glbase:hasIdentifierScheme idscheme:sdn ;
            glbase:hasIdentifierValue "SDN:P02::VDFC" ] ;
    rdfs:comment "Parameters describing the transport of material, heat or energy in the water column"@en ;
    rdfs:subClassOf <http://schema.geolink.org/1.0/voc/nvs/P03#SeaDataNetParameter> ;
    owl:deprecated "false" .
<http://vocab.nerc.ac.uk/collection/P02/current/VIRU/> a glbase:MeasurementType,
        owl:Class,
        owl:NamedIndividual ;
    rdfs:label "Virus abundance in water bodies"@en ;
    dcterms:creator "SeaDataNet" ;
    dcterms:date "2010-10-22 10:10:30.0" ;
    glbase:hasIdentifier [ glbase:hasIdentifierScheme idscheme:sdn ;
            glbase:hasIdentifierValue "SDN:P02::VIRU" ] ;
    rdfs:comment "Any enumeration (e.g. count, number per square metre) of viruses in any body of fresh or salt water."@en ;
    rdfs:subClassOf <http://vocab.nerc.ac.uk/collection/P03/current/B005/>,
        <http://vocab.nerc.ac.uk/collection/P03/current/B070/> ;
    owl:deprecated "false" .
<http://vocab.nerc.ac.uk/collection/P02/current/VSRA/> a glbase:MeasurementType,
        owl:Class,
        owl:NamedIndividual ;
    rdfs:label "Visible waveband radiance and irradiance measurements in the atmosphere"@en ;
    dcterms:creator "SeaDataNet" ;
    dcterms:date "2006-06-05 14:02:32.0" ;
    glbase:hasIdentifier [ glbase:hasIdentifierScheme idscheme:sdn ;
            glbase:hasIdentifierValue "SDN:P02::VSRA" ] ;
    rdfs:comment "Includes visible waveband measurements at discrete wavelengths and PAR integrated values as photon and energy fluxes. Does not include satellite radiometer and associated calibration parameters (e.g. water-leaving radiance and reflectance)"@en ;
    rdfs:subClassOf <http://vocab.nerc.ac.uk/collection/P03/current/D015/>,
        <http://vocab.nerc.ac.uk/collection/P03/current/M010/> ;
    owl:deprecated "false" .
<http://vocab.nerc.ac.uk/collection/P02/current/VSRW/> a glbase:MeasurementType,
        owl:Class,
        owl:NamedIndividual ;
    rdfs:label "Visible waveband radiance and irradiance measurements in the water column"@en ;
    dcterms:creator "SeaDataNet" ;
    dcterms:date "2004-07-30 08:37:00.0" ;
    glbase:hasIdentifier [ glbase:hasIdentifierScheme idscheme:sdn ;
            glbase:hasIdentifierValue "SDN:P02::VSRW" ] ;
    rdfs:comment "Includes measurements at discrete wavelengths and PAR integrated values, measurements as photon and energy fluxes."@en ;
    rdfs:subClassOf <http://vocab.nerc.ac.uk/collection/P03/current/D015/> ;
    owl:deprecated "false" .
<http://vocab.nerc.ac.uk/collection/P02/current/WBRX/> a glbase:MeasurementType,
        owl:Class,
        owl:NamedIndividual ;
    rdfs:label "Water body redox potential"@en ;
    dcterms:creator "SeaDataNet" ;
    dcterms:date "2012-02-16 09:27:29.0" ;
    glbase:hasIdentifier [ glbase:hasIdentifierScheme idscheme:sdn ;
            glbase:hasIdentifierValue "SDN:P02::WBRX" ] ;
    rdfs:comment "A measure of the tendency of any body of fresh or salt water to either gain or lose electrons when it is subject to change by introduction of a new species."@en ;
    rdfs:subClassOf <http://vocab.nerc.ac.uk/collection/P03/current/C045/> ;
    owl:deprecated "false" .
<http://vocab.nerc.ac.uk/collection/P02/current/WCOC/> a glbase:MeasurementType,
        owl:Class,
        owl:NamedIndividual ;
    rdfs:label "Concentration of other organic contaminants in the water column"@en ;
    dcterms:creator "SeaDataNet" ;
    dcterms:date "2010-01-27 12:37:34.0" ;
    glbase:hasIdentifier [ glbase:hasIdentifierScheme idscheme:sdn ;
            glbase:hasIdentifierValue "SDN:P02::WCOC" ] ;
    rdfs:comment "Concentration parameters for carbon compounds regarded as environmentally harmful in solution or suspension (i.e.includes measurements in both the dissolved and particulate phases) in any body of salt or fresh water that are not included in other specific categories"@en ;
    rdfs:subClassOf <http://vocab.nerc.ac.uk/collection/P03/current/C055/>,
        <http://vocab.nerc.ac.uk/collection/P03/current/H001/> ;
    owl:deprecated "false" .
<http://vocab.nerc.ac.uk/collection/P02/current/WCPH/> a glbase:MeasurementType,
        owl:Class,
        owl:NamedIndividual ;
    rdfs:label "Water column photography"@en ;
    dcterms:creator "SeaDataNet" ;
    dcterms:date "2009-04-20 08:34:10.0" ;
    glbase:hasIdentifier [ glbase:hasIdentifierScheme idscheme:sdn ;
            glbase:hasIdentifierValue "SDN:P02::WCPH" ] ;
    rdfs:comment "Digital images of the water column obtained using either still or video cameras"@en ;
    rdfs:subClassOf <http://vocab.nerc.ac.uk/collection/P03/current/UWPH/> ;
    owl:deprecated "false" .
<http://vocab.nerc.ac.uk/collection/P02/current/WCTR/> a glbase:MeasurementType,
        owl:Class,
        owl:NamedIndividual ;
    rdfs:label "Water body released tracers"@en ;
    dcterms:creator "SeaDataNet" ;
    dcterms:date "2010-10-01 09:50:05.0" ;
    glbase:hasIdentifier [ glbase:hasIdentifierScheme idscheme:sdn ;
            glbase:hasIdentifierValue "SDN:P02::WCTR" ] ;
    rdfs:comment "Parameters describing the amount in a sample of a tracer (rhodamine, SF6, 3He, etc.) that has been purposely released into  a water body to track water mass movements or quantify exchanges with the atmosphere."@en ;
    rdfs:subClassOf <http://vocab.nerc.ac.uk/collection/P03/current/D020/> ;
    owl:deprecated "false" .
<http://vocab.nerc.ac.uk/collection/P02/current/WCWT/> a glbase:MeasurementType,
        owl:Class,
        owl:NamedIndividual ;
    rdfs:label "Sediment water content, porosity and surface area"@en ;
    dcterms:creator "SeaDataNet" ;
    dcterms:date "2004-08-17 12:50:43.0" ;
    glbase:hasIdentifier [ glbase:hasIdentifierScheme idscheme:sdn ;
            glbase:hasIdentifierValue "SDN:P02::WCWT" ] ;
    rdfs:comment "Sediment porosity (water content by volume) and water content by weight parameters"@en ;
    rdfs:subClassOf <http://vocab.nerc.ac.uk/collection/P03/current/G040/> ;
    owl:deprecated "false" .
<http://vocab.nerc.ac.uk/collection/P02/current/WDNA/> a glbase:MeasurementType,
        owl:Class,
        owl:NamedIndividual ;
    rdfs:label "Concentrations of biopolymers in water bodies"@en ;
    dcterms:creator "SeaDataNet" ;
    dcterms:date "2014-02-20 09:18:00.0" ;
    glbase:hasIdentifier [ glbase:hasIdentifierScheme idscheme:sdn ;
            glbase:hasIdentifierValue "SDN:P02::WDNA" ] ;
    rdfs:comment "Parameters quantifying the amount of naturally-produced organic (molecules containing carbon) compounds that are built from multiple instances of structural units (monomers) that are covalently-bonded to produce larger structures in any body of salt or fresh water. Includes polynucleotides (RNA and DNA), polypeptides and polysaccharides (e.g. cellulose)."@en ;
    rdfs:subClassOf <http://vocab.nerc.ac.uk/collection/P03/current/B005/>,
        <http://vocab.nerc.ac.uk/collection/P03/current/B027/>,
        <http://vocab.nerc.ac.uk/collection/P03/current/C050/> ;
    owl:deprecated "false" .
<http://vocab.nerc.ac.uk/collection/P02/current/WPRO/> a glbase:MeasurementType,
        owl:Class,
        owl:NamedIndividual ;
    rdfs:label "Concentration of proteins in the water column"@en ;
    dcterms:creator "SeaDataNet" ;
    dcterms:date "2004-08-13 11:31:01.0" ;
    glbase:hasIdentifier [ glbase:hasIdentifierScheme idscheme:sdn ;
            glbase:hasIdentifierValue "SDN:P02::WPRO" ] ;
    rdfs:comment "Concentrations of proteins in all phases of the water column"@en ;
    rdfs:subClassOf <http://vocab.nerc.ac.uk/collection/P03/current/C050/> ;
    owl:deprecated "false" .
<http://vocab.nerc.ac.uk/collection/P02/current/WQBI/> a glbase:MeasurementType,
        owl:Class,
        owl:NamedIndividual ;
    rdfs:label "Water quality bioindicators"@en ;
    dcterms:creator "SeaDataNet" ;
    dcterms:date "2009-04-20 08:24:21.0" ;
    glbase:hasIdentifier [ glbase:hasIdentifierScheme idscheme:sdn ;
            glbase:hasIdentifierValue "SDN:P02::WQBI" ] ;
    rdfs:comment "Parameters quantifying fauna and flora that indicate physical or chemical conditions in the water column such as colonisation depths and abundance of indicator species."@en ;
    rdfs:subClassOf <http://schema.geolink.org/1.0/voc/nvs/P03#SeaDataNetParameter> ;
    owl:deprecated "false" .
<http://vocab.nerc.ac.uk/collection/P02/current/WRAD/> a glbase:MeasurementType,
        owl:Class,
        owl:NamedIndividual ;
    rdfs:label "Radioactivity in the water column"@en ;
    dcterms:creator "SeaDataNet" ;
    dcterms:date "2004-05-28 08:35:00.0" ;
    glbase:hasIdentifier [ glbase:hasIdentifierScheme idscheme:sdn ;
            glbase:hasIdentifierValue "SDN:P02::WRAD" ] ;
    rdfs:comment "All parameters associated with radiocativity in the water column, including radiation counts, isotope activities and activity ratios. Activities per unit mass of SPM are included"@en ;
    rdfs:subClassOf <http://vocab.nerc.ac.uk/collection/P03/current/C030/> ;
    owl:deprecated "false" .
<http://vocab.nerc.ac.uk/collection/P02/current/WSTB/> a glbase:MeasurementType,
        owl:Class,
        owl:NamedIndividual ;
    rdfs:label "Stable isotope enrichment in the water column"@en ;
    dcterms:creator "SeaDataNet" ;
    dcterms:date "2008-07-01 08:38:26.0" ;
    glbase:hasIdentifier [ glbase:hasIdentifierScheme idscheme:sdn ;
            glbase:hasIdentifierValue "SDN:P02::WSTB" ] ;
    rdfs:comment "Stable isotope enrichment parameters in both the dissolved and particulate phases of the water column"@en ;
    rdfs:subClassOf <http://vocab.nerc.ac.uk/collection/P03/current/C030/> ;
    owl:deprecated "false" .
<http://vocab.nerc.ac.uk/collection/P02/current/WSTR/> a glbase:MeasurementType,
        owl:Class,
        owl:NamedIndividual ;
    rdfs:label "Wind stress and shear"@en ;
    dcterms:creator "SeaDataNet" ;
    dcterms:date "2007-02-23 14:59:38.0" ;
    glbase:hasIdentifier [ glbase:hasIdentifierScheme idscheme:sdn ;
            glbase:hasIdentifierValue "SDN:P02::WSTR" ] ;
    rdfs:comment "Parameters related to forces due to interactions between atmosphere and the surface of the earth or between atmospheric air masses"@en ;
    rdfs:subClassOf <http://vocab.nerc.ac.uk/collection/P03/current/M010/> ;
    owl:deprecated "false" .
<http://vocab.nerc.ac.uk/collection/P02/current/WVSP/> a glbase:MeasurementType,
        owl:Class,
        owl:NamedIndividual ;
    rdfs:label "Spectral wave data parameters"@en ;
    dcterms:creator "SeaDataNet" ;
    dcterms:date "2004-07-30 15:09:00.0" ;
    glbase:hasIdentifier [ glbase:hasIdentifierScheme idscheme:sdn ;
            glbase:hasIdentifierValue "SDN:P02::WVSP" ] ;
    rdfs:comment "Parameters for directional and non-directional spectral wave data, excluding wave directions derived from spectral data."@en ;
    rdfs:subClassOf <http://vocab.nerc.ac.uk/collection/P03/current/D034/> ;
    owl:deprecated "false" .
<http://vocab.nerc.ac.uk/collection/P02/current/WVST/> a glbase:MeasurementType,
        owl:Class,
        owl:NamedIndividual ;
    rdfs:label "Wave height and period statistics"@en ;
    dcterms:creator "SeaDataNet" ;
    dcterms:date "2004-07-30 15:10:00.0" ;
    glbase:hasIdentifier [ glbase:hasIdentifierScheme idscheme:sdn ;
            glbase:hasIdentifierValue "SDN:P02::WVST" ] ;
    rdfs:comment "Statistical parameters derived from wave records to express wave height and period."@en ;
    rdfs:subClassOf <http://vocab.nerc.ac.uk/collection/P03/current/D034/> ;
    owl:deprecated "false" .
<http://vocab.nerc.ac.uk/collection/P02/current/XKEY/> a glbase:MeasurementType,
        owl:Class,
        owl:NamedIndividual ;
    rdfs:label "Security tags and keys"@en ;
    dcterms:creator "SeaDataNet" ;
    dcterms:date "2008-12-09 11:17:27.0" ;
    glbase:hasIdentifier [ glbase:hasIdentifierScheme idscheme:sdn ;
            glbase:hasIdentifierValue "SDN:P02::XKEY" ] ;
    rdfs:comment "Parameters used to encode information specifying access rights to data, usually in terms of authorised roles"@en ;
    rdfs:subClassOf <http://vocab.nerc.ac.uk/collection/P03/current/Z005/> ;
    owl:deprecated "false" .
<http://vocab.nerc.ac.uk/collection/P02/current/XMGS/> a glbase:MeasurementType,
        owl:Class,
        owl:NamedIndividual ;
    rdfs:label "Geological sample magnetic, electrical and acoustic properties"@en ;
    dcterms:creator "SeaDataNet" ;
    dcterms:date "2010-12-15 13:11:07.0" ;
    glbase:hasIdentifier [ glbase:hasIdentifierScheme idscheme:sdn ;
            glbase:hasIdentifierValue "SDN:P02::XMGS" ] ;
    rdfs:comment "Any parameters quantifying the magnetic (e.g. magnetic susceptibility), electrical (e.g. resistivity) or acoustic (e.g. P-wave propogation speed) of sediment or rock cores and samples"@en ;
    rdfs:subClassOf <http://vocab.nerc.ac.uk/collection/P03/current/G005/>,
        <http://vocab.nerc.ac.uk/collection/P03/current/G012/>,
        <http://vocab.nerc.ac.uk/collection/P03/current/G040/> ;
    owl:deprecated "false" .
<http://vocab.nerc.ac.uk/collection/P02/current/XRFC/> a glbase:MeasurementType,
        owl:Class,
        owl:NamedIndividual ;
    rdfs:label "Raw X-Ray fluorometer (XRF) output from sediment samples"@en ;
    dcterms:creator "SeaDataNet" ;
    dcterms:date "2010-11-05 12:26:31.0" ;
    glbase:hasIdentifier [ glbase:hasIdentifierScheme idscheme:sdn ;
            glbase:hasIdentifierValue "SDN:P02::XRFC" ] ;
    rdfs:comment "" ;
    rdfs:subClassOf <http://vocab.nerc.ac.uk/collection/P02/current/RMIN/> ;
    owl:deprecated "true" .
<http://vocab.nerc.ac.uk/collection/P02/current/ZADX/> a glbase:MeasurementType,
        owl:Class,
        owl:NamedIndividual ;
    rdfs:label "Zoobenthos dry weight biomass"@en ;
    dcterms:creator "SeaDataNet" ;
    dcterms:date "2013-08-01 09:07:37.0" ;
    glbase:hasIdentifier [ glbase:hasIdentifierScheme idscheme:sdn ;
            glbase:hasIdentifierValue "SDN:P02::ZADX" ] ;
    rdfs:comment "Any quantification of the dry mass of zoobenthos (animals living on, in or near the bed of any water body). Includes animals normally considered planktonic if collected in sediment and data expressed ash-free and in terms of carbon, nitrogen etc.."@en ;
    rdfs:subClassOf <http://vocab.nerc.ac.uk/collection/P03/current/B070/>,
        <http://vocab.nerc.ac.uk/collection/P03/current/G055/> ;
    owl:deprecated "false" .
<http://vocab.nerc.ac.uk/collection/P02/current/ZATP/> a glbase:MeasurementType,
        owl:Class,
        owl:NamedIndividual ;
    rdfs:label "Zooplankton taxonomy-related biomass expressed as protein per unit volume of the water column"@en ;
    dcterms:creator "SeaDataNet" ;
    dcterms:date "2005-08-18 09:55:05.0" ;
    glbase:hasIdentifier [ glbase:hasIdentifierScheme idscheme:sdn ;
            glbase:hasIdentifierValue "SDN:P02::ZATP" ] ;
    rdfs:comment "Zooplankton (mesozooplankton plus larger pelagic animals excluding fish, reptiles and mammals) protein biomass per unit volume for entities that have been identified by taxonomic name"@en ;
    rdfs:subClassOf <http://vocab.nerc.ac.uk/collection/P03/current/B045/>,
        <http://vocab.nerc.ac.uk/collection/P03/current/B070/> ;
    owl:deprecated "false" .
<http://vocab.nerc.ac.uk/collection/P02/current/ZATX/> a glbase:MeasurementType,
        owl:Class,
        owl:NamedIndividual ;
    rdfs:label "Zooplankton taxonomy-related abundance per unit volume of the water column"@en ;
    dcterms:creator "SeaDataNet" ;
    dcterms:date "2004-04-19 16:35:00.0" ;
    glbase:hasIdentifier [ glbase:hasIdentifierScheme idscheme:sdn ;
            glbase:hasIdentifierValue "SDN:P02::ZATX" ] ;
    rdfs:comment "Zooplankton (mesozooplankton plus larger pelagic animals excluding fish, reptiles and mammals) abundance parameters presented at the level of taxa that may be mapped to entities in the ITIS taxonomy.  These may be at any taxonomic level from sub-species upwards."@en ;
    rdfs:subClassOf <http://vocab.nerc.ac.uk/collection/P03/current/B045/>,
        <http://vocab.nerc.ac.uk/collection/P03/current/B070/> ;
    owl:deprecated "false" .
<http://vocab.nerc.ac.uk/collection/P02/current/ZBTX/> a glbase:MeasurementType,
        owl:Class,
        owl:NamedIndividual ;
    rdfs:label "Zoobenthos taxonomic abundance"@en ;
    dcterms:creator "SeaDataNet" ;
    dcterms:date "2010-10-22 10:03:50.0" ;
    glbase:hasIdentifier [ glbase:hasIdentifierScheme idscheme:sdn ;
            glbase:hasIdentifierValue "SDN:P02::ZBTX" ] ;
    rdfs:comment "Any enumeration (e.g. count, number per square metre) of animals living on or near the seabed designated by taxonomic names (e.g. species, genus)."@en ;
    rdfs:subClassOf <http://vocab.nerc.ac.uk/collection/P03/current/B070/>,
        <http://vocab.nerc.ac.uk/collection/P03/current/G055/> ;
    owl:deprecated "false" .
<http://vocab.nerc.ac.uk/collection/P02/current/ZCMP/> a glbase:MeasurementType,
        owl:Class,
        owl:NamedIndividual ;
    rdfs:label "Zooplankton chemical composition"@en ;
    dcterms:creator "SeaDataNet" ;
    dcterms:date "2005-08-01 15:41:59.0" ;
    glbase:hasIdentifier [ glbase:hasIdentifierScheme idscheme:sdn ;
            glbase:hasIdentifierValue "SDN:P02::ZCMP" ] ;
    rdfs:comment "Chemical composition of zooplankton expressed in terms of mass (or molar quantity) per specimen or per unit tissue mass"@en ;
    rdfs:subClassOf <http://vocab.nerc.ac.uk/collection/P03/current/B045/> ;
    owl:deprecated "false" .
<http://vocab.nerc.ac.uk/collection/P02/current/ZCTC/> a glbase:MeasurementType,
        owl:Class,
        owl:NamedIndividual ;
    rdfs:label "Zooplankton taxonomy-related biomass expressed as carbon per unit volume of the water column"@en ;
    dcterms:creator "SeaDataNet" ;
    dcterms:date "2004-04-20 08:50:00.0" ;
    glbase:hasIdentifier [ glbase:hasIdentifierScheme idscheme:sdn ;
            glbase:hasIdentifierValue "SDN:P02::ZCTC" ] ;
    rdfs:comment "Zooplankton (mesozooplankton plus larger pelagic animals excluding fish, reptiles and mammals) carbon biomass parameters presented at the level of taxa that may be mapped to entities in the ITIS taxonomy.  These may be at any taxonomic level from sub-species upwards."@en ;
    rdfs:subClassOf <http://vocab.nerc.ac.uk/collection/P03/current/B045/>,
        <http://vocab.nerc.ac.uk/collection/P03/current/B070/> ;
    owl:deprecated "false" .
<http://vocab.nerc.ac.uk/collection/P02/current/ZCTN/> a glbase:MeasurementType,
        owl:Class,
        owl:NamedIndividual ;
    rdfs:label "Zooplankton taxonomy-related biomass expressed as nitrogen per unit volume of the water column"@en ;
    dcterms:creator "SeaDataNet" ;
    dcterms:date "2009-01-23 08:41:26.0" ;
    glbase:hasIdentifier [ glbase:hasIdentifierScheme idscheme:sdn ;
            glbase:hasIdentifierValue "SDN:P02::ZCTN" ] ;
    rdfs:comment "Zooplankton (mesozooplankton plus larger pelagic animals excluding fish, reptiles and mammals) nitrogen biomass parameters presented at the level of taxa that may be mapped to entities in the ITIS taxonomy.  These may be at any taxonomic level from sub-species upwards."@en ;
    rdfs:subClassOf <http://vocab.nerc.ac.uk/collection/P03/current/B045/>,
        <http://vocab.nerc.ac.uk/collection/P03/current/B070/> ;
    owl:deprecated "false" .
<http://vocab.nerc.ac.uk/collection/P02/current/ZFIT/> a glbase:MeasurementType,
        owl:Class,
        owl:NamedIndividual ;
    rdfs:label "Zooplankton and zoobenthos physiological condition parameters"@en ;
    dcterms:creator "SeaDataNet" ;
    dcterms:date "2014-08-04 08:52:15.0" ;
    glbase:hasIdentifier [ glbase:hasIdentifierScheme idscheme:sdn ;
            glbase:hasIdentifierValue "SDN:P02::ZFIT" ] ;
    rdfs:comment "Parameters indicating the health of zooplankton and zoobenthos taxa, such as fecundity, egg condition, presence of parasites/diseases etc."@en ;
    rdfs:subClassOf <http://vocab.nerc.ac.uk/collection/P03/current/G055/> ;
    owl:deprecated "false" .
<http://vocab.nerc.ac.uk/collection/P02/current/ZNLG/> a glbase:MeasurementType,
        owl:Class,
        owl:NamedIndividual ;
    rdfs:label "Metal ligand parameters in the water column"@en ;
    dcterms:creator "SeaDataNet" ;
    dcterms:date "2004-08-11 16:06:28.0" ;
    glbase:hasIdentifier [ glbase:hasIdentifierScheme idscheme:sdn ;
            glbase:hasIdentifierValue "SDN:P02::ZNLG" ] ;
    rdfs:comment "Parameters concerned with the complexation of metals as ligands in the water column"@en ;
    rdfs:subClassOf <http://vocab.nerc.ac.uk/collection/P03/current/C035/>,
        <http://vocab.nerc.ac.uk/collection/P03/current/C045/>,
        <http://vocab.nerc.ac.uk/collection/P03/current/C050/> ;
    owl:deprecated "false" .
<http://vocab.nerc.ac.uk/collection/P02/current/ZNTC/> a glbase:MeasurementType,
        owl:Class,
        owl:NamedIndividual ;
    rdfs:label "Zooplankton non taxonomy-related biomass expressed as carbon per unit volume of the water column"@en ;
    dcterms:creator "SeaDataNet" ;
    dcterms:date "2004-04-20 08:52:00.0" ;
    glbase:hasIdentifier [ glbase:hasIdentifierScheme idscheme:sdn ;
            glbase:hasIdentifierValue "SDN:P02::ZNTC" ] ;
    rdfs:comment "Zooplankton (mesozooplankton plus larger pelagic animals excluding fish, reptiles and mammals) carbon biomass per unit volume parameters not included in group ZCTC.  Usually used for generic names such as 'mesozooplankton'."@en ;
    rdfs:subClassOf <http://vocab.nerc.ac.uk/collection/P03/current/B045/>,
        <http://vocab.nerc.ac.uk/collection/P03/current/B070/> ;
    owl:deprecated "false" .
<http://vocab.nerc.ac.uk/collection/P02/current/ZNTN/> a glbase:MeasurementType,
        owl:Class,
        owl:NamedIndividual ;
    rdfs:label "Zooplankton non taxonomy-related biomass expressed as nitrogen per unit volume of the water column"@en ;
    dcterms:creator "SeaDataNet" ;
    dcterms:date "2010-07-19 09:38:40.0" ;
    glbase:hasIdentifier [ glbase:hasIdentifierScheme idscheme:sdn ;
            glbase:hasIdentifierValue "SDN:P02::ZNTN" ] ;
    rdfs:comment "Zooplankton (mesozooplankton plus larger pelagic animals excluding fish, reptiles and mammals) nitrogen biomass per unit volume parameters not included in group ZCTC.  Usually used for generic names such as 'mesozooplankton'."@en ;
    rdfs:subClassOf <http://vocab.nerc.ac.uk/collection/P03/current/B045/>,
        <http://vocab.nerc.ac.uk/collection/P03/current/B070/> ;
    owl:deprecated "false" .
<http://vocab.nerc.ac.uk/collection/P02/current/ZNTP/> a glbase:MeasurementType,
        owl:Class,
        owl:NamedIndividual ;
    rdfs:label "Zooplankton non taxonomy-related biomass expressed as protein per unit volume of the water column"@en ;
    dcterms:creator "SeaDataNet" ;
    dcterms:date "2005-08-18 09:54:26.0" ;
    glbase:hasIdentifier [ glbase:hasIdentifierScheme idscheme:sdn ;
            glbase:hasIdentifierValue "SDN:P02::ZNTP" ] ;
    rdfs:comment "Zooplankton (mesozooplankton plus larger pelagic animals excluding fish, reptiles and mammals) protein biomass per unit volume for entities that have not been identified by taxonomic name"@en ;
    rdfs:subClassOf <http://vocab.nerc.ac.uk/collection/P03/current/B045/>,
        <http://vocab.nerc.ac.uk/collection/P03/current/B070/> ;
    owl:deprecated "false" .
<http://vocab.nerc.ac.uk/collection/P02/current/ZNTX/> a glbase:MeasurementType,
        owl:Class,
        owl:NamedIndividual ;
    rdfs:label "Zooplankton non taxonomy-related abundance per unit volume of the water column"@en ;
    dcterms:creator "SeaDataNet" ;
    dcterms:date "2004-04-19 16:35:00.0" ;
    glbase:hasIdentifier [ glbase:hasIdentifierScheme idscheme:sdn ;
            glbase:hasIdentifierValue "SDN:P02::ZNTX" ] ;
    rdfs:comment "Zooplankton (mesozooplankton plus larger pelagic animals excluding fish, reptiles and mammals) abundance per unit volume parameters not included in group ZATX.  Usually used for generic names such as 'mesozooplankton'."@en ;
    rdfs:subClassOf <http://vocab.nerc.ac.uk/collection/P03/current/B045/>,
        <http://vocab.nerc.ac.uk/collection/P03/current/B070/> ;
    owl:deprecated "false" .
<http://vocab.nerc.ac.uk/collection/P02/current/ZOOB/> a glbase:MeasurementType,
        owl:Class,
        owl:NamedIndividual ;
    rdfs:label "Zoobenthos taxonomy-related counts"@en ;
    dcterms:creator "SeaDataNet" ;
    dcterms:date "2007-01-08 16:44:29.0" ;
    glbase:hasIdentifier [ glbase:hasIdentifierScheme idscheme:sdn ;
            glbase:hasIdentifierValue "SDN:P02::ZOOB" ] ;
    rdfs:comment "Zoobenthos count parameters presented at the level of taxa that may be mapped to entities in the ITIS taxonomy.  These may be at any taxonomic level from sub-species upwards. Count includes presence/absence indicators."@en ;
    rdfs:subClassOf <http://vocab.nerc.ac.uk/collection/P03/current/G055/> ;
    owl:deprecated "false" .
<http://vocab.nerc.ac.uk/collection/P02/current/ZV00/> a glbase:MeasurementType,
        owl:Class,
        owl:NamedIndividual ;
    rdfs:label "Zooplankton biovolume"@en ;
    dcterms:creator "SeaDataNet" ;
    dcterms:date "2003-06-10 13:53:19.0" ;
    glbase:hasIdentifier [ glbase:hasIdentifierScheme idscheme:sdn ;
            glbase:hasIdentifierValue "SDN:P02::ZV00" ] ;
    rdfs:comment "" ;
    rdfs:subClassOf <http://vocab.nerc.ac.uk/collection/P03/current/B045/> ;
    owl:deprecated "false" .
<http://vocab.nerc.ac.uk/collection/P02/current/ZWTX/> a glbase:MeasurementType,
        owl:Class,
        owl:NamedIndividual ;
    rdfs:label "Zoobenthos taxonomy-related wet weight biomass per unit area of the bed"@en ;
    dcterms:creator "SeaDataNet" ;
    dcterms:date "2004-04-26 14:55:05.0" ;
    glbase:hasIdentifier [ glbase:hasIdentifierScheme idscheme:sdn ;
            glbase:hasIdentifierValue "SDN:P02::ZWTX" ] ;
    rdfs:comment "Zoobenthos wet weight biomass per unit area parameters presented at the level of taxa that may be mapped to entities in the ITIS taxonomy.  Includes animals considered as planktonic if they have been returned from sediment samples."@en ;
    rdfs:subClassOf <http://vocab.nerc.ac.uk/collection/P03/current/B070/>,
        <http://vocab.nerc.ac.uk/collection/P03/current/G055/> ;
    owl:deprecated "false" .
<http://vocab.nerc.ac.uk/collection/P02/current/ZZZZ/> a glbase:MeasurementType,
        owl:Class,
        owl:NamedIndividual ;
    rdfs:label "Unspecified"@en ;
    dcterms:creator "SeaDataNet" ;
    dcterms:date "2008-12-09 10:56:20.0" ;
    glbase:hasIdentifier [ glbase:hasIdentifierScheme idscheme:sdn ;
            glbase:hasIdentifierValue "SDN:P02::ZZZZ" ] ;
    rdfs:comment "The identity of the parameter is not declared.  Covers cases such as internal working parameters and dummy channels."@en ;
    rdfs:subClassOf <http://vocab.nerc.ac.uk/collection/P03/current/Z005/> ;
    owl:deprecated "false" .
<http://vocab.nerc.ac.uk/collection/P03/current/GSED/> a owl:Class .
<http://vocab.nerc.ac.uk/collection/P03/current/UWPH/> a owl:Class .
<http://vocab.nerc.ac.uk/collection/P02/current/CASD/> a glbase:MeasurementType,
        owl:Class,
        owl:NamedIndividual ;
    rdfs:label "Concentration of carbohydrates, phenols, alkanols (alcohols), ethers, aldehydes and ketones in sediment"@en ;
    dcterms:creator "SeaDataNet" ;
    dcterms:date "2012-03-01 16:21:17.0" ;
    glbase:hasIdentifier [ glbase:hasIdentifierScheme idscheme:sdn ;
            glbase:hasIdentifierValue "SDN:P02::CASD" ] ;
    rdfs:comment "Concentrations of carbohydrates, phenols, alkanols (alcohols), ethers,aldehydes and simple (non-alkenone) ketones in unlithified sediment (material collected by a corer including fluff)."@en ;
    rdfs:subClassOf <http://vocab.nerc.ac.uk/collection/P03/current/C050/>,
        <http://vocab.nerc.ac.uk/collection/P03/current/G035/> ;
    owl:deprecated "false" .
<http://vocab.nerc.ac.uk/collection/P02/current/DOXY/> a glbase:MeasurementType,
        owl:Class,
        owl:NamedIndividual ;
    rdfs:label "Dissolved oxygen parameters in the water column"@en ;
    dcterms:creator "SeaDataNet" ;
    dcterms:date "2004-10-22 13:07:05.0" ;
    glbase:hasIdentifier [ glbase:hasIdentifierScheme idscheme:sdn ;
            glbase:hasIdentifierValue "SDN:P02::DOXY" ] ;
    rdfs:comment "All dissolved oxygen parameters (including saturation and utilisation) for the water column"@en ;
    rdfs:subClassOf <http://vocab.nerc.ac.uk/collection/P03/current/C015/> ;
    owl:deprecated "false" .
<http://vocab.nerc.ac.uk/collection/P02/current/MTSP/> a glbase:MeasurementType,
        owl:Class,
        owl:NamedIndividual ;
    rdfs:label "Metal concentrations in suspended particulate material"@en ;
    dcterms:creator "SeaDataNet" ;
    dcterms:date "2008-09-12 09:06:32.0" ;
    glbase:hasIdentifier [ glbase:hasIdentifierScheme idscheme:sdn ;
            glbase:hasIdentifierValue "SDN:P02::MTSP" ] ;
    rdfs:comment "Concentrations of metal elements in suspended particulate material collected by water column filtration, centrifugation or sediment trapping. Deprecated as semantic overlap with MTWP."@en ;
    rdfs:subClassOf <http://schema.geolink.org/1.0/voc/nvs/P03#SeaDataNetParameter> ;
    owl:deprecated "true" ;
    owl:equivalentClass <http://vocab.nerc.ac.uk/collection/P02/current/MTWP/> .
<http://vocab.nerc.ac.uk/collection/P02/current/MTWP/> a glbase:MeasurementType,
        owl:Class,
        owl:NamedIndividual ;
    rdfs:label "Particulate metal concentrations in the water column"@en ;
    dcterms:creator "SeaDataNet" ;
    dcterms:date "2008-09-12 09:03:59.0" ;
    glbase:hasIdentifier [ glbase:hasIdentifierScheme idscheme:sdn ;
            glbase:hasIdentifierValue "SDN:P02::MTWP" ] ;
    rdfs:comment "Concentration parameters for metallic elements in the particulate phase of the water column collected by fitration, centrifugation or sediment trapping"@en ;
    rdfs:subClassOf <http://vocab.nerc.ac.uk/collection/P03/current/C035/>,
        <http://vocab.nerc.ac.uk/collection/P03/current/G015/> ;
    owl:deprecated "false" ;
    owl:equivalentClass <http://vocab.nerc.ac.uk/collection/P02/current/MTSP/> .
<http://vocab.nerc.ac.uk/collection/P02/current/NTRA/> a glbase:MeasurementType,
        owl:Class,
        owl:NamedIndividual ;
    rdfs:label "Nitrate concentration parameters in the water column"@en ;
    dcterms:creator "SeaDataNet" ;
    dcterms:date "2007-02-01 09:10:12.0" ;
    glbase:hasIdentifier [ glbase:hasIdentifierScheme idscheme:sdn ;
            glbase:hasIdentifierValue "SDN:P02::NTRA" ] ;
    rdfs:comment "Nitrate concentration parameters (including statistical parameters such as standard deviation) in the water column. Includes nitrate+nitrite, which is often loosely referred to as nitrate."@en ;
    rdfs:subClassOf <http://vocab.nerc.ac.uk/collection/P03/current/C005/>,
        <http://vocab.nerc.ac.uk/collection/P03/current/C040/> ;
    owl:deprecated "false" .
<http://vocab.nerc.ac.uk/collection/P02/current/STMP/> a glbase:MeasurementType,
        owl:Class,
        owl:NamedIndividual ;
    rdfs:label "Temperature of geological units"@en ;
    dcterms:creator "SeaDataNet" ;
    dcterms:date "2010-11-04 11:07:14.0" ;
    glbase:hasIdentifier [ glbase:hasIdentifierScheme idscheme:sdn ;
            glbase:hasIdentifierValue "SDN:P02::STMP" ] ;
    rdfs:comment "Parameters that describe the distribution of the degree of hotness within a body of rock or unlithified sediment."@en ;
    rdfs:subClassOf <http://vocab.nerc.ac.uk/collection/P03/current/GPYS/>,
        <http://vocab.nerc.ac.uk/collection/P03/current/GTHM/> ;
    owl:deprecated "false" .
<http://vocab.nerc.ac.uk/collection/P03/current/B050/> a owl:Class .
<http://vocab.nerc.ac.uk/collection/P03/current/C020/> a owl:Class .
<http://vocab.nerc.ac.uk/collection/P03/current/D005/> a owl:Class .
<http://vocab.nerc.ac.uk/collection/P03/current/D032/> a owl:Class .
<http://vocab.nerc.ac.uk/collection/P03/current/G005/> a owl:Class .
<http://vocab.nerc.ac.uk/collection/P03/current/G030/> a owl:Class .
<http://vocab.nerc.ac.uk/collection/P03/current/G045/> a owl:Class .
<http://vocab.nerc.ac.uk/collection/P03/current/G060/> a owl:Class .
<http://vocab.nerc.ac.uk/collection/P02/current/SRFL/> a glbase:MeasurementType,
        owl:Class,
        owl:NamedIndividual ;
    rdfs:label "Seismic reflection"@en ;
    dcterms:creator "SeaDataNet" ;
    dcterms:date "2007-11-22 11:35:40.0" ;
    glbase:hasIdentifier [ glbase:hasIdentifierScheme idscheme:sdn ;
            glbase:hasIdentifierValue "SDN:P02::SRFL" ] ;
    rdfs:comment "Parameters relating to the elucidation of geological structure by quantifying the proportion of waves from a high energy source reflected by sub-surface layers."@en ;
    rdfs:subClassOf <http://vocab.nerc.ac.uk/collection/P03/current/G012/>,
        <http://vocab.nerc.ac.uk/collection/P03/current/GPYS/> ;
    owl:deprecated "false" .
<http://vocab.nerc.ac.uk/collection/P03/current/B060/> a owl:Class .
<http://vocab.nerc.ac.uk/collection/P03/current/C003/> a owl:Class .
<http://vocab.nerc.ac.uk/collection/P03/current/D020/> a owl:Class .
<http://vocab.nerc.ac.uk/collection/P03/current/GTHM/> a owl:Class .
<http://vocab.nerc.ac.uk/collection/P03/current/H002/> a owl:Class .
<http://vocab.nerc.ac.uk/collection/P03/current/B055/> a owl:Class .
<http://vocab.nerc.ac.uk/collection/P03/current/C010/> a owl:Class .
<http://vocab.nerc.ac.uk/collection/P03/current/H005/> a owl:Class .
<http://schema.geolink.org/1.0/voc/nvs/P03#SeaDataNetParameter> a owl:Class .
<http://vocab.nerc.ac.uk/collection/P03/current/D025/> a owl:Class .
<http://vocab.nerc.ac.uk/collection/P03/current/D030/> a owl:Class .
<http://vocab.nerc.ac.uk/collection/P03/current/D034/> a owl:Class .
<http://vocab.nerc.ac.uk/collection/P02/current/ICHM/> a glbase:MeasurementType,
        owl:Class,
        owl:NamedIndividual ;
    rdfs:label "Snow and ice chemistry"@en ;
    dcterms:creator "SeaDataNet" ;
    dcterms:date "2011-02-18 11:02:39.0" ;
    glbase:hasIdentifier [ glbase:hasIdentifierScheme idscheme:sdn ;
            glbase:hasIdentifierValue "SDN:P02::ICHM" ] ;
    rdfs:comment "Parameters related to the chemical composition of any kind of water sample that was frozen solid at the time of sampling or measurement"@en ;
    rdfs:subClassOf <http://vocab.nerc.ac.uk/collection/P03/current/M015/> ;
    owl:deprecated "false" .
<http://vocab.nerc.ac.uk/collection/P03/current/B025/> a owl:Class .
<http://vocab.nerc.ac.uk/collection/P03/current/C015/> a owl:Class .
<http://vocab.nerc.ac.uk/collection/P03/current/M015/> a owl:Class .
<http://vocab.nerc.ac.uk/collection/P03/current/T001/> a owl:Class .
<http://vocab.nerc.ac.uk/collection/P03/current/B030/> a owl:Class .
<http://vocab.nerc.ac.uk/collection/P03/current/C030/> a owl:Class .
<http://vocab.nerc.ac.uk/collection/P02/current/RMIN/> a glbase:MeasurementType,
        owl:Class,
        owl:NamedIndividual ;
    rdfs:label "Inorganic chemical composition of sediment or rocks"@en ;
    dcterms:creator "SeaDataNet" ;
    dcterms:date "2010-11-05 10:04:18.0" ;
    glbase:hasIdentifier [ glbase:hasIdentifierScheme idscheme:sdn ;
            glbase:hasIdentifierValue "SDN:P02::RMIN" ] ;
    rdfs:comment "Parameters specifying the proportions of inorganic components (major/minor/trace elements, trace metals etc.) in sediment or rock samples.  Major elements includes the H2O+ and H2O- parameters reported by convention in oxide weight per cent geochemical major element analyses."@en ;
    rdfs:subClassOf <http://vocab.nerc.ac.uk/collection/P03/current/C045/>,
        <http://vocab.nerc.ac.uk/collection/P03/current/G035/> ;
    owl:deprecated "false" .
<http://vocab.nerc.ac.uk/collection/P03/current/G012/> a owl:Class .
<http://vocab.nerc.ac.uk/collection/P03/current/G040/> a owl:Class .
<http://vocab.nerc.ac.uk/collection/P03/current/G050/> a owl:Class .
<http://vocab.nerc.ac.uk/collection/P03/current/H004/> a owl:Class .
<http://vocab.nerc.ac.uk/collection/P03/current/C025/> a owl:Class .
<http://vocab.nerc.ac.uk/collection/P03/current/D015/> a owl:Class .
<http://vocab.nerc.ac.uk/collection/P03/current/GPYS/> a owl:Class .
<http://vocab.nerc.ac.uk/collection/P03/current/B020/> a owl:Class .
<http://vocab.nerc.ac.uk/collection/P03/current/B035/> a owl:Class .
<http://vocab.nerc.ac.uk/collection/P03/current/B007/> a owl:Class .
<http://vocab.nerc.ac.uk/collection/P03/current/B027/> a owl:Class .
<http://vocab.nerc.ac.uk/collection/P03/current/C040/> a owl:Class .
<http://vocab.nerc.ac.uk/collection/P03/current/Z005/> a owl:Class .
<http://vocab.nerc.ac.uk/collection/P03/current/M010/> a owl:Class .
<http://vocab.nerc.ac.uk/collection/P03/current/B005/> a owl:Class .
<http://vocab.nerc.ac.uk/collection/P03/current/C035/> a owl:Class .
<http://vocab.nerc.ac.uk/collection/P03/current/C045/> a owl:Class .
<http://vocab.nerc.ac.uk/collection/P03/current/B015/> a owl:Class .
<http://vocab.nerc.ac.uk/collection/P03/current/C050/> a owl:Class .
<http://vocab.nerc.ac.uk/collection/P03/current/G015/> a owl:Class .
<http://vocab.nerc.ac.uk/collection/P03/current/G055/> a owl:Class .
<http://vocab.nerc.ac.uk/collection/P03/current/C055/> a owl:Class .
<http://vocab.nerc.ac.uk/collection/P03/current/O005/> a owl:Class .
<http://vocab.nerc.ac.uk/collection/P03/current/M005/> a owl:Class .
<http://vocab.nerc.ac.uk/collection/P03/current/C005/> a owl:Class .
<http://vocab.nerc.ac.uk/collection/P03/current/B045/> a owl:Class .
<http://vocab.nerc.ac.uk/collection/P03/current/O010/> a owl:Class .
<http://vocab.nerc.ac.uk/collection/P03/current/G035/> a owl:Class .
<http://vocab.nerc.ac.uk/collection/P03/current/H001/> a owl:Class .
<http://vocab.nerc.ac.uk/collection/P03/current/B070/> a owl:Class .
glbase:MeasurementType a owl:Class .
glbase:hasMeasurementType a owl:ObjectProperty .
[] a owl:Restriction ;
    rdfs:subClassOf <http://vocab.nerc.ac.uk/collection/P02/current/GRZO/> ;
    owl:onProperty glbase:hasMeasurementType ;
    owl:someValuesFrom [ a owl:Class ;
            owl:oneOf ( <http://vocab.nerc.ac.uk/collection/P02/current/GRZO/> ) ] .
[] a owl:Restriction ;
    rdfs:subClassOf <http://vocab.nerc.ac.uk/collection/P02/current/CPRP/> ;
    owl:onProperty glbase:hasMeasurementType ;
    owl:someValuesFrom [ a owl:Class ;
            owl:oneOf ( <http://vocab.nerc.ac.uk/collection/P02/current/CPRP/> ) ] .
[] a owl:Restriction ;
    rdfs:subClassOf <http://vocab.nerc.ac.uk/collection/P02/current/FR11/> ;
    owl:onProperty glbase:hasMeasurementType ;
    owl:someValuesFrom [ a owl:Class ;
            owl:oneOf ( <http://vocab.nerc.ac.uk/collection/P02/current/FR11/> ) ] .
[] a owl:Restriction ;
    rdfs:subClassOf <http://vocab.nerc.ac.uk/collection/P02/current/BPRP/> ;
    owl:onProperty glbase:hasMeasurementType ;
    owl:someValuesFrom [ a owl:Class ;
            owl:oneOf ( <http://vocab.nerc.ac.uk/collection/P02/current/BPRP/> ) ] .
[] a owl:Restriction ;
    rdfs:subClassOf <http://vocab.nerc.ac.uk/collection/P02/current/GOXP/> ;
    owl:onProperty glbase:hasMeasurementType ;
    owl:someValuesFrom [ a owl:Class ;
            owl:oneOf ( <http://vocab.nerc.ac.uk/collection/P02/current/GOXP/> ) ] .
[] a owl:Restriction ;
    rdfs:subClassOf <http://vocab.nerc.ac.uk/collection/P02/current/PHWC/> ;
    owl:onProperty glbase:hasMeasurementType ;
    owl:someValuesFrom [ a owl:Class ;
            owl:oneOf ( <http://vocab.nerc.ac.uk/collection/P02/current/PHWC/> ) ] .
[] a owl:Restriction ;
    rdfs:subClassOf <http://vocab.nerc.ac.uk/collection/P02/current/HLWC/> ;
    owl:onProperty glbase:hasMeasurementType ;
    owl:someValuesFrom [ a owl:Class ;
            owl:oneOf ( <http://vocab.nerc.ac.uk/collection/P02/current/HLWC/> ) ] .
[] a owl:Restriction ;
    rdfs:subClassOf <http://vocab.nerc.ac.uk/collection/P02/current/HEAV/> ;
    owl:onProperty glbase:hasMeasurementType ;
    owl:someValuesFrom [ a owl:Class ;
            owl:oneOf ( <http://vocab.nerc.ac.uk/collection/P02/current/HEAV/> ) ] .
[] a owl:Restriction ;
    rdfs:subClassOf <http://vocab.nerc.ac.uk/collection/P02/current/MPMN/> ;
    owl:onProperty glbase:hasMeasurementType ;
    owl:someValuesFrom [ a owl:Class ;
            owl:oneOf ( <http://vocab.nerc.ac.uk/collection/P02/current/MPMN/> ) ] .
[] a owl:Restriction ;
    rdfs:subClassOf <http://vocab.nerc.ac.uk/collection/P02/current/FREP/> ;
    owl:onProperty glbase:hasMeasurementType ;
    owl:someValuesFrom [ a owl:Class ;
            owl:oneOf ( <http://vocab.nerc.ac.uk/collection/P02/current/FREP/> ) ] .
[] a owl:Restriction ;
    rdfs:subClassOf <http://vocab.nerc.ac.uk/collection/P02/current/HEAD/> ;
    owl:onProperty glbase:hasMeasurementType ;
    owl:someValuesFrom [ a owl:Class ;
            owl:oneOf ( <http://vocab.nerc.ac.uk/collection/P02/current/HEAD/> ) ] .
[] a owl:Restriction ;
    rdfs:subClassOf <http://vocab.nerc.ac.uk/collection/P02/current/PCAH/> ;
    owl:onProperty glbase:hasMeasurementType ;
    owl:someValuesFrom [ a owl:Class ;
            owl:oneOf ( <http://vocab.nerc.ac.uk/collection/P02/current/PCAH/> ) ] .
[] a owl:Restriction ;
    rdfs:subClassOf <http://vocab.nerc.ac.uk/collection/P02/current/OMBI/> ;
    owl:onProperty glbase:hasMeasurementType ;
    owl:someValuesFrom [ a owl:Class ;
            owl:oneOf ( <http://vocab.nerc.ac.uk/collection/P02/current/OMBI/> ) ] .
[] a owl:Restriction ;
    rdfs:subClassOf <http://vocab.nerc.ac.uk/collection/P02/current/WCTR/> ;
    owl:onProperty glbase:hasMeasurementType ;
    owl:someValuesFrom [ a owl:Class ;
            owl:oneOf ( <http://vocab.nerc.ac.uk/collection/P02/current/WCTR/> ) ] .
[] a owl:Restriction ;
    rdfs:subClassOf <http://vocab.nerc.ac.uk/collection/P02/current/MEPH/> ;
    owl:onProperty glbase:hasMeasurementType ;
    owl:someValuesFrom [ a owl:Class ;
            owl:oneOf ( <http://vocab.nerc.ac.uk/collection/P02/current/MEPH/> ) ] .
[] a owl:Restriction ;
    rdfs:subClassOf <http://vocab.nerc.ac.uk/collection/P02/current/NTRA/> ;
    owl:onProperty glbase:hasMeasurementType ;
    owl:someValuesFrom [ a owl:Class ;
            owl:oneOf ( <http://vocab.nerc.ac.uk/collection/P02/current/NTRA/> ) ] .
[] a owl:Restriction ;
    rdfs:subClassOf <http://vocab.nerc.ac.uk/collection/P02/current/LGCR/> ;
    owl:onProperty glbase:hasMeasurementType ;
    owl:someValuesFrom [ a owl:Class ;
            owl:oneOf ( <http://vocab.nerc.ac.uk/collection/P02/current/LGCR/> ) ] .
[] a owl:Restriction ;
    rdfs:subClassOf <http://vocab.nerc.ac.uk/collection/P02/current/LIBI/> ;
    owl:onProperty glbase:hasMeasurementType ;
    owl:someValuesFrom [ a owl:Class ;
            owl:oneOf ( <http://vocab.nerc.ac.uk/collection/P02/current/LIBI/> ) ] .
[] a owl:Restriction ;
    rdfs:subClassOf <http://vocab.nerc.ac.uk/collection/P02/current/NUTV/> ;
    owl:onProperty glbase:hasMeasurementType ;
    owl:someValuesFrom [ a owl:Class ;
            owl:oneOf ( <http://vocab.nerc.ac.uk/collection/P02/current/NUTV/> ) ] .
[] a owl:Restriction ;
    rdfs:subClassOf <http://vocab.nerc.ac.uk/collection/P02/current/D000/> ;
    owl:onProperty glbase:hasMeasurementType ;
    owl:someValuesFrom [ a owl:Class ;
            owl:oneOf ( <http://vocab.nerc.ac.uk/collection/P02/current/D000/> ) ] .
[] a owl:Restriction ;
    rdfs:subClassOf <http://vocab.nerc.ac.uk/collection/P02/current/PCO2/> ;
    owl:onProperty glbase:hasMeasurementType ;
    owl:someValuesFrom [ a owl:Class ;
            owl:oneOf ( <http://vocab.nerc.ac.uk/collection/P02/current/PCO2/> ) ] .
[] a owl:Restriction ;
    rdfs:subClassOf <http://vocab.nerc.ac.uk/collection/P02/current/PPRD/> ;
    owl:onProperty glbase:hasMeasurementType ;
    owl:someValuesFrom [ a owl:Class ;
            owl:oneOf ( <http://vocab.nerc.ac.uk/collection/P02/current/PPRD/> ) ] .
[] a owl:Restriction ;
    rdfs:subClassOf <http://vocab.nerc.ac.uk/collection/P02/current/SEMO/> ;
    owl:onProperty glbase:hasMeasurementType ;
    owl:someValuesFrom [ a owl:Class ;
            owl:oneOf ( <http://vocab.nerc.ac.uk/collection/P02/current/SEMO/> ) ] .
[] a owl:Restriction ;
    rdfs:subClassOf <http://vocab.nerc.ac.uk/collection/P02/current/MZCT/> ;
    owl:onProperty glbase:hasMeasurementType ;
    owl:someValuesFrom [ a owl:Class ;
            owl:oneOf ( <http://vocab.nerc.ac.uk/collection/P02/current/MZCT/> ) ] .
[] a owl:Restriction ;
    rdfs:subClassOf <http://vocab.nerc.ac.uk/collection/P02/current/OHAT/> ;
    owl:onProperty glbase:hasMeasurementType ;
    owl:someValuesFrom [ a owl:Class ;
            owl:oneOf ( <http://vocab.nerc.ac.uk/collection/P02/current/OHAT/> ) ] .
[] a owl:Restriction ;
    rdfs:subClassOf <http://vocab.nerc.ac.uk/collection/P02/current/PHWB/> ;
    owl:onProperty glbase:hasMeasurementType ;
    owl:someValuesFrom [ a owl:Class ;
            owl:oneOf ( <http://vocab.nerc.ac.uk/collection/P02/current/PHWB/> ) ] .
[] a owl:Restriction ;
    rdfs:subClassOf <http://vocab.nerc.ac.uk/collection/P02/current/WDNA/> ;
    owl:onProperty glbase:hasMeasurementType ;
    owl:someValuesFrom [ a owl:Class ;
            owl:oneOf ( <http://vocab.nerc.ac.uk/collection/P02/current/WDNA/> ) ] .
[] a owl:Restriction ;
    rdfs:subClassOf <http://vocab.nerc.ac.uk/collection/P02/current/MNGS/> ;
    owl:onProperty glbase:hasMeasurementType ;
    owl:someValuesFrom [ a owl:Class ;
            owl:oneOf ( <http://vocab.nerc.ac.uk/collection/P02/current/MNGS/> ) ] .
[] a owl:Restriction ;
    rdfs:subClassOf <http://vocab.nerc.ac.uk/collection/P02/current/GP069/> ;
    owl:onProperty glbase:hasMeasurementType ;
    owl:someValuesFrom [ a owl:Class ;
            owl:oneOf ( <http://vocab.nerc.ac.uk/collection/P02/current/GP069/> ) ] .
[] a owl:Restriction ;
    rdfs:subClassOf <http://vocab.nerc.ac.uk/collection/P02/current/ATTN/> ;
    owl:onProperty glbase:hasMeasurementType ;
    owl:someValuesFrom [ a owl:Class ;
            owl:oneOf ( <http://vocab.nerc.ac.uk/collection/P02/current/ATTN/> ) ] .
[] a owl:Restriction ;
    rdfs:subClassOf <http://vocab.nerc.ac.uk/collection/P02/current/LITT/> ;
    owl:onProperty glbase:hasMeasurementType ;
    owl:someValuesFrom [ a owl:Class ;
            owl:oneOf ( <http://vocab.nerc.ac.uk/collection/P02/current/LITT/> ) ] .
[] a owl:Restriction ;
    rdfs:subClassOf <http://vocab.nerc.ac.uk/collection/P02/current/RSIS/> ;
    owl:onProperty glbase:hasMeasurementType ;
    owl:someValuesFrom [ a owl:Class ;
            owl:oneOf ( <http://vocab.nerc.ac.uk/collection/P02/current/RSIS/> ) ] .
[] a owl:Restriction ;
    rdfs:subClassOf <http://vocab.nerc.ac.uk/collection/P02/current/BRAD/> ;
    owl:onProperty glbase:hasMeasurementType ;
    owl:someValuesFrom [ a owl:Class ;
            owl:oneOf ( <http://vocab.nerc.ac.uk/collection/P02/current/BRAD/> ) ] .
[] a owl:Restriction ;
    rdfs:subClassOf <http://vocab.nerc.ac.uk/collection/P02/current/IWDX/> ;
    owl:onProperty glbase:hasMeasurementType ;
    owl:someValuesFrom [ a owl:Class ;
            owl:oneOf ( <http://vocab.nerc.ac.uk/collection/P02/current/IWDX/> ) ] .
[] a owl:Restriction ;
    rdfs:subClassOf <http://vocab.nerc.ac.uk/collection/P02/current/GP085/> ;
    owl:onProperty glbase:hasMeasurementType ;
    owl:someValuesFrom [ a owl:Class ;
            owl:oneOf ( <http://vocab.nerc.ac.uk/collection/P02/current/GP085/> ) ] .
[] a owl:Restriction ;
    rdfs:subClassOf <http://vocab.nerc.ac.uk/collection/P02/current/BCAH/> ;
    owl:onProperty glbase:hasMeasurementType ;
    owl:someValuesFrom [ a owl:Class ;
            owl:oneOf ( <http://vocab.nerc.ac.uk/collection/P02/current/BCAH/> ) ] .
[] a owl:Restriction ;
    rdfs:subClassOf <http://vocab.nerc.ac.uk/collection/P02/current/CSLR/> ;
    owl:onProperty glbase:hasMeasurementType ;
    owl:someValuesFrom [ a owl:Class ;
            owl:oneOf ( <http://vocab.nerc.ac.uk/collection/P02/current/CSLR/> ) ] .
[] a owl:Restriction ;
    rdfs:subClassOf <http://vocab.nerc.ac.uk/collection/P02/current/AMON/> ;
    owl:onProperty glbase:hasMeasurementType ;
    owl:someValuesFrom [ a owl:Class ;
            owl:oneOf ( <http://vocab.nerc.ac.uk/collection/P02/current/AMON/> ) ] .
[] a owl:Restriction ;
    rdfs:subClassOf <http://vocab.nerc.ac.uk/collection/P02/current/SPWC/> ;
    owl:onProperty glbase:hasMeasurementType ;
    owl:someValuesFrom [ a owl:Class ;
            owl:oneOf ( <http://vocab.nerc.ac.uk/collection/P02/current/SPWC/> ) ] .
[] a owl:Restriction ;
    rdfs:subClassOf <http://vocab.nerc.ac.uk/collection/P02/current/SPHT/> ;
    owl:onProperty glbase:hasMeasurementType ;
    owl:someValuesFrom [ a owl:Class ;
            owl:oneOf ( <http://vocab.nerc.ac.uk/collection/P02/current/SPHT/> ) ] .
[] a owl:Restriction ;
    rdfs:subClassOf <http://vocab.nerc.ac.uk/collection/P02/current/GP080/> ;
    owl:onProperty glbase:hasMeasurementType ;
    owl:someValuesFrom [ a owl:Class ;
            owl:oneOf ( <http://vocab.nerc.ac.uk/collection/P02/current/GP080/> ) ] .
[] a owl:Restriction ;
    rdfs:subClassOf <http://vocab.nerc.ac.uk/collection/P02/current/SSTB/> ;
    owl:onProperty glbase:hasMeasurementType ;
    owl:someValuesFrom [ a owl:Class ;
            owl:oneOf ( <http://vocab.nerc.ac.uk/collection/P02/current/SSTB/> ) ] .
[] a owl:Restriction ;
    rdfs:subClassOf <http://vocab.nerc.ac.uk/collection/P02/current/CBCC/> ;
    owl:onProperty glbase:hasMeasurementType ;
    owl:someValuesFrom [ a owl:Class ;
            owl:oneOf ( <http://vocab.nerc.ac.uk/collection/P02/current/CBCC/> ) ] .
[] a owl:Restriction ;
    rdfs:subClassOf <http://vocab.nerc.ac.uk/collection/P02/current/IPHY/> ;
    owl:onProperty glbase:hasMeasurementType ;
    owl:someValuesFrom [ a owl:Class ;
            owl:oneOf ( <http://vocab.nerc.ac.uk/collection/P02/current/IPHY/> ) ] .
[] a owl:Restriction ;
    rdfs:subClassOf <http://vocab.nerc.ac.uk/collection/P02/current/CPCN/> ;
    owl:onProperty glbase:hasMeasurementType ;
    owl:someValuesFrom [ a owl:Class ;
            owl:oneOf ( <http://vocab.nerc.ac.uk/collection/P02/current/CPCN/> ) ] .
[] a owl:Restriction ;
    rdfs:subClassOf <http://vocab.nerc.ac.uk/collection/P02/current/BEPP/> ;
    owl:onProperty glbase:hasMeasurementType ;
    owl:someValuesFrom [ a owl:Class ;
            owl:oneOf ( <http://vocab.nerc.ac.uk/collection/P02/current/BEPP/> ) ] .
[] a owl:Restriction ;
    rdfs:subClassOf <http://vocab.nerc.ac.uk/collection/P02/current/MTSP/> ;
    owl:onProperty glbase:hasMeasurementType ;
    owl:someValuesFrom [ a owl:Class ;
            owl:oneOf ( <http://vocab.nerc.ac.uk/collection/P02/current/MTSP/> ) ] .
[] a owl:Restriction ;
    rdfs:subClassOf <http://vocab.nerc.ac.uk/collection/P02/current/CARO/> ;
    owl:onProperty glbase:hasMeasurementType ;
    owl:someValuesFrom [ a owl:Class ;
            owl:oneOf ( <http://vocab.nerc.ac.uk/collection/P02/current/CARO/> ) ] .
[] a owl:Restriction ;
    rdfs:subClassOf <http://vocab.nerc.ac.uk/collection/P02/current/R410/> ;
    owl:onProperty glbase:hasMeasurementType ;
    owl:someValuesFrom [ a owl:Class ;
            owl:oneOf ( <http://vocab.nerc.ac.uk/collection/P02/current/R410/> ) ] .
[] a owl:Restriction ;
    rdfs:subClassOf <http://vocab.nerc.ac.uk/collection/P02/current/GP010/> ;
    owl:onProperty glbase:hasMeasurementType ;
    owl:someValuesFrom [ a owl:Class ;
            owl:oneOf ( <http://vocab.nerc.ac.uk/collection/P02/current/GP010/> ) ] .
[] a owl:Restriction ;
    rdfs:subClassOf <http://vocab.nerc.ac.uk/collection/P02/current/AQYN/> ;
    owl:onProperty glbase:hasMeasurementType ;
    owl:someValuesFrom [ a owl:Class ;
            owl:oneOf ( <http://vocab.nerc.ac.uk/collection/P02/current/AQYN/> ) ] .
[] a owl:Restriction ;
    rdfs:subClassOf <http://vocab.nerc.ac.uk/collection/P02/current/TNRP/> ;
    owl:onProperty glbase:hasMeasurementType ;
    owl:someValuesFrom [ a owl:Class ;
            owl:oneOf ( <http://vocab.nerc.ac.uk/collection/P02/current/TNRP/> ) ] .
[] a owl:Restriction ;
    rdfs:subClassOf <http://vocab.nerc.ac.uk/collection/P02/current/MMAN/> ;
    owl:onProperty glbase:hasMeasurementType ;
    owl:someValuesFrom [ a owl:Class ;
            owl:oneOf ( <http://vocab.nerc.ac.uk/collection/P02/current/MMAN/> ) ] .
[] a owl:Restriction ;
    rdfs:subClassOf <http://vocab.nerc.ac.uk/collection/P02/current/SHTA/> ;
    owl:onProperty glbase:hasMeasurementType ;
    owl:someValuesFrom [ a owl:Class ;
            owl:oneOf ( <http://vocab.nerc.ac.uk/collection/P02/current/SHTA/> ) ] .
[] a owl:Restriction ;
    rdfs:subClassOf <http://vocab.nerc.ac.uk/collection/P02/current/AHGT/> ;
    owl:onProperty glbase:hasMeasurementType ;
    owl:someValuesFrom [ a owl:Class ;
            owl:oneOf ( <http://vocab.nerc.ac.uk/collection/P02/current/AHGT/> ) ] .
[] a owl:Restriction ;
    rdfs:subClassOf <http://vocab.nerc.ac.uk/collection/P02/current/OPWC/> ;
    owl:onProperty glbase:hasMeasurementType ;
    owl:someValuesFrom [ a owl:Class ;
            owl:oneOf ( <http://vocab.nerc.ac.uk/collection/P02/current/OPWC/> ) ] .
[] a owl:Restriction ;
    rdfs:subClassOf <http://vocab.nerc.ac.uk/collection/P02/current/SDAC/> ;
    owl:onProperty glbase:hasMeasurementType ;
    owl:someValuesFrom [ a owl:Class ;
            owl:oneOf ( <http://vocab.nerc.ac.uk/collection/P02/current/SDAC/> ) ] .
[] a owl:Restriction ;
    rdfs:subClassOf <http://vocab.nerc.ac.uk/collection/P02/current/PCFX/> ;
    owl:onProperty glbase:hasMeasurementType ;
    owl:someValuesFrom [ a owl:Class ;
            owl:oneOf ( <http://vocab.nerc.ac.uk/collection/P02/current/PCFX/> ) ] .
[] a owl:Restriction ;
    rdfs:subClassOf <http://vocab.nerc.ac.uk/collection/P02/current/ZCMP/> ;
    owl:onProperty glbase:hasMeasurementType ;
    owl:someValuesFrom [ a owl:Class ;
            owl:oneOf ( <http://vocab.nerc.ac.uk/collection/P02/current/ZCMP/> ) ] .
[] a owl:Restriction ;
    rdfs:subClassOf <http://vocab.nerc.ac.uk/collection/P02/current/DSCO/> ;
    owl:onProperty glbase:hasMeasurementType ;
    owl:someValuesFrom [ a owl:Class ;
            owl:oneOf ( <http://vocab.nerc.ac.uk/collection/P02/current/DSCO/> ) ] .
[] a owl:Restriction ;
    rdfs:subClassOf <http://vocab.nerc.ac.uk/collection/P02/current/FNTM/> ;
    owl:onProperty glbase:hasMeasurementType ;
    owl:someValuesFrom [ a owl:Class ;
            owl:oneOf ( <http://vocab.nerc.ac.uk/collection/P02/current/FNTM/> ) ] .
[] a owl:Restriction ;
    rdfs:subClassOf <http://vocab.nerc.ac.uk/collection/P02/current/BDWC/> ;
    owl:onProperty glbase:hasMeasurementType ;
    owl:someValuesFrom [ a owl:Class ;
            owl:oneOf ( <http://vocab.nerc.ac.uk/collection/P02/current/BDWC/> ) ] .
[] a owl:Restriction ;
    rdfs:subClassOf <http://vocab.nerc.ac.uk/collection/P02/current/SREP/> ;
    owl:onProperty glbase:hasMeasurementType ;
    owl:someValuesFrom [ a owl:Class ;
            owl:oneOf ( <http://vocab.nerc.ac.uk/collection/P02/current/SREP/> ) ] .
[] a owl:Restriction ;
    rdfs:subClassOf <http://vocab.nerc.ac.uk/collection/P02/current/AASD/> ;
    owl:onProperty glbase:hasMeasurementType ;
    owl:someValuesFrom [ a owl:Class ;
            owl:oneOf ( <http://vocab.nerc.ac.uk/collection/P02/current/AASD/> ) ] .
[] a owl:Restriction ;
    rdfs:subClassOf <http://vocab.nerc.ac.uk/collection/P02/current/ZNLG/> ;
    owl:onProperty glbase:hasMeasurementType ;
    owl:someValuesFrom [ a owl:Class ;
            owl:oneOf ( <http://vocab.nerc.ac.uk/collection/P02/current/ZNLG/> ) ] .
[] a owl:Restriction ;
    rdfs:subClassOf <http://vocab.nerc.ac.uk/collection/P02/current/BNTC/> ;
    owl:onProperty glbase:hasMeasurementType ;
    owl:someValuesFrom [ a owl:Class ;
            owl:oneOf ( <http://vocab.nerc.ac.uk/collection/P02/current/BNTC/> ) ] .
[] a owl:Restriction ;
    rdfs:subClassOf <http://vocab.nerc.ac.uk/collection/P02/current/IRBO/> ;
    owl:onProperty glbase:hasMeasurementType ;
    owl:someValuesFrom [ a owl:Class ;
            owl:oneOf ( <http://vocab.nerc.ac.uk/collection/P02/current/IRBO/> ) ] .
[] a owl:Restriction ;
    rdfs:subClassOf <http://vocab.nerc.ac.uk/collection/P02/current/BABI/> ;
    owl:onProperty glbase:hasMeasurementType ;
    owl:someValuesFrom [ a owl:Class ;
            owl:oneOf ( <http://vocab.nerc.ac.uk/collection/P02/current/BABI/> ) ] .
[] a owl:Restriction ;
    rdfs:subClassOf <http://vocab.nerc.ac.uk/collection/P02/current/SICN/> ;
    owl:onProperty glbase:hasMeasurementType ;
    owl:someValuesFrom [ a owl:Class ;
            owl:oneOf ( <http://vocab.nerc.ac.uk/collection/P02/current/SICN/> ) ] .
[] a owl:Restriction ;
    rdfs:subClassOf <http://vocab.nerc.ac.uk/collection/P02/current/CBSP/> ;
    owl:onProperty glbase:hasMeasurementType ;
    owl:someValuesFrom [ a owl:Class ;
            owl:oneOf ( <http://vocab.nerc.ac.uk/collection/P02/current/CBSP/> ) ] .
[] a owl:Restriction ;
    rdfs:subClassOf <http://vocab.nerc.ac.uk/collection/P02/current/SUAT/> ;
    owl:onProperty glbase:hasMeasurementType ;
    owl:someValuesFrom [ a owl:Class ;
            owl:oneOf ( <http://vocab.nerc.ac.uk/collection/P02/current/SUAT/> ) ] .
[] a owl:Restriction ;
    rdfs:subClassOf <http://vocab.nerc.ac.uk/collection/P02/current/LVLT/> ;
    owl:onProperty glbase:hasMeasurementType ;
    owl:someValuesFrom [ a owl:Class ;
            owl:oneOf ( <http://vocab.nerc.ac.uk/collection/P02/current/LVLT/> ) ] .
[] a owl:Restriction ;
    rdfs:subClassOf <http://vocab.nerc.ac.uk/collection/P02/current/AMOX/> ;
    owl:onProperty glbase:hasMeasurementType ;
    owl:someValuesFrom [ a owl:Class ;
            owl:oneOf ( <http://vocab.nerc.ac.uk/collection/P02/current/AMOX/> ) ] .
[] a owl:Restriction ;
    rdfs:subClassOf <http://vocab.nerc.ac.uk/collection/P02/current/CATX/> ;
    owl:onProperty glbase:hasMeasurementType ;
    owl:someValuesFrom [ a owl:Class ;
            owl:oneOf ( <http://vocab.nerc.ac.uk/collection/P02/current/CATX/> ) ] .
[] a owl:Restriction ;
    rdfs:subClassOf <http://vocab.nerc.ac.uk/collection/P02/current/HLDE/> ;
    owl:onProperty glbase:hasMeasurementType ;
    owl:someValuesFrom [ a owl:Class ;
            owl:oneOf ( <http://vocab.nerc.ac.uk/collection/P02/current/HLDE/> ) ] .
[] a owl:Restriction ;
    rdfs:subClassOf <http://vocab.nerc.ac.uk/collection/P02/current/VIRU/> ;
    owl:onProperty glbase:hasMeasurementType ;
    owl:someValuesFrom [ a owl:Class ;
            owl:oneOf ( <http://vocab.nerc.ac.uk/collection/P02/current/VIRU/> ) ] .
[] a owl:Restriction ;
    rdfs:subClassOf <http://vocab.nerc.ac.uk/collection/P02/current/NTOT/> ;
    owl:onProperty glbase:hasMeasurementType ;
    owl:someValuesFrom [ a owl:Class ;
            owl:oneOf ( <http://vocab.nerc.ac.uk/collection/P02/current/NTOT/> ) ] .
[] a owl:Restriction ;
    rdfs:subClassOf <http://vocab.nerc.ac.uk/collection/P02/current/MZBC/> ;
    owl:onProperty glbase:hasMeasurementType ;
    owl:someValuesFrom [ a owl:Class ;
            owl:oneOf ( <http://vocab.nerc.ac.uk/collection/P02/current/MZBC/> ) ] .
[] a owl:Restriction ;
    rdfs:subClassOf <http://vocab.nerc.ac.uk/collection/P02/current/SVEL/> ;
    owl:onProperty glbase:hasMeasurementType ;
    owl:someValuesFrom [ a owl:Class ;
            owl:oneOf ( <http://vocab.nerc.ac.uk/collection/P02/current/SVEL/> ) ] .
[] a owl:Restriction ;
    rdfs:subClassOf <http://vocab.nerc.ac.uk/collection/P02/current/PEBI/> ;
    owl:onProperty glbase:hasMeasurementType ;
    owl:someValuesFrom [ a owl:Class ;
            owl:oneOf ( <http://vocab.nerc.ac.uk/collection/P02/current/PEBI/> ) ] .
[] a owl:Restriction ;
    rdfs:subClassOf <http://vocab.nerc.ac.uk/collection/P02/current/LWRD/> ;
    owl:onProperty glbase:hasMeasurementType ;
    owl:someValuesFrom [ a owl:Class ;
            owl:oneOf ( <http://vocab.nerc.ac.uk/collection/P02/current/LWRD/> ) ] .
[] a owl:Restriction ;
    rdfs:subClassOf <http://vocab.nerc.ac.uk/collection/P02/current/MINC/> ;
    owl:onProperty glbase:hasMeasurementType ;
    owl:someValuesFrom [ a owl:Class ;
            owl:oneOf ( <http://vocab.nerc.ac.uk/collection/P02/current/MINC/> ) ] .
[] a owl:Restriction ;
    rdfs:subClassOf <http://vocab.nerc.ac.uk/collection/P02/current/PCLM/> ;
    owl:onProperty glbase:hasMeasurementType ;
    owl:someValuesFrom [ a owl:Class ;
            owl:oneOf ( <http://vocab.nerc.ac.uk/collection/P02/current/PCLM/> ) ] .
[] a owl:Restriction ;
    rdfs:subClassOf <http://vocab.nerc.ac.uk/collection/P02/current/PNTX/> ;
    owl:onProperty glbase:hasMeasurementType ;
    owl:someValuesFrom [ a owl:Class ;
            owl:oneOf ( <http://vocab.nerc.ac.uk/collection/P02/current/PNTX/> ) ] .
[] a owl:Restriction ;
    rdfs:subClassOf <http://vocab.nerc.ac.uk/collection/P02/current/MTWP/> ;
    owl:onProperty glbase:hasMeasurementType ;
    owl:someValuesFrom [ a owl:Class ;
            owl:oneOf ( <http://vocab.nerc.ac.uk/collection/P02/current/MTWP/> ) ] .
[] a owl:Restriction ;
    rdfs:subClassOf <http://vocab.nerc.ac.uk/collection/P02/current/TBGZ/> ;
    owl:onProperty glbase:hasMeasurementType ;
    owl:someValuesFrom [ a owl:Class ;
            owl:oneOf ( <http://vocab.nerc.ac.uk/collection/P02/current/TBGZ/> ) ] .
[] a owl:Restriction ;
    rdfs:subClassOf <http://vocab.nerc.ac.uk/collection/P02/current/PSST/> ;
    owl:onProperty glbase:hasMeasurementType ;
    owl:someValuesFrom [ a owl:Class ;
            owl:oneOf ( <http://vocab.nerc.ac.uk/collection/P02/current/PSST/> ) ] .
[] a owl:Restriction ;
    rdfs:subClassOf <http://vocab.nerc.ac.uk/collection/P02/current/SPAG/> ;
    owl:onProperty glbase:hasMeasurementType ;
    owl:someValuesFrom [ a owl:Class ;
            owl:oneOf ( <http://vocab.nerc.ac.uk/collection/P02/current/SPAG/> ) ] .
[] a owl:Restriction ;
    rdfs:subClassOf <http://vocab.nerc.ac.uk/collection/P02/current/OXYC/> ;
    owl:onProperty glbase:hasMeasurementType ;
    owl:someValuesFrom [ a owl:Class ;
            owl:oneOf ( <http://vocab.nerc.ac.uk/collection/P02/current/OXYC/> ) ] .
[] a owl:Restriction ;
    rdfs:subClassOf <http://vocab.nerc.ac.uk/collection/P02/current/MARC/> ;
    owl:onProperty glbase:hasMeasurementType ;
    owl:someValuesFrom [ a owl:Class ;
            owl:oneOf ( <http://vocab.nerc.ac.uk/collection/P02/current/MARC/> ) ] .
[] a owl:Restriction ;
    rdfs:subClassOf <http://vocab.nerc.ac.uk/collection/P02/current/F001/> ;
    owl:onProperty glbase:hasMeasurementType ;
    owl:someValuesFrom [ a owl:Class ;
            owl:oneOf ( <http://vocab.nerc.ac.uk/collection/P02/current/F001/> ) ] .
[] a owl:Restriction ;
    rdfs:subClassOf <http://vocab.nerc.ac.uk/collection/P02/current/DOCU/> ;
    owl:onProperty glbase:hasMeasurementType ;
    owl:someValuesFrom [ a owl:Class ;
            owl:oneOf ( <http://vocab.nerc.ac.uk/collection/P02/current/DOCU/> ) ] .
[] a owl:Restriction ;
    rdfs:subClassOf <http://vocab.nerc.ac.uk/collection/P02/current/FPRT/> ;
    owl:onProperty glbase:hasMeasurementType ;
    owl:someValuesFrom [ a owl:Class ;
            owl:oneOf ( <http://vocab.nerc.ac.uk/collection/P02/current/FPRT/> ) ] .
[] a owl:Restriction ;
    rdfs:subClassOf <http://vocab.nerc.ac.uk/collection/P02/current/OMPW/> ;
    owl:onProperty glbase:hasMeasurementType ;
    owl:someValuesFrom [ a owl:Class ;
            owl:oneOf ( <http://vocab.nerc.ac.uk/collection/P02/current/OMPW/> ) ] .
[] a owl:Restriction ;
    rdfs:subClassOf <http://vocab.nerc.ac.uk/collection/P02/current/ZNTC/> ;
    owl:onProperty glbase:hasMeasurementType ;
    owl:someValuesFrom [ a owl:Class ;
            owl:oneOf ( <http://vocab.nerc.ac.uk/collection/P02/current/ZNTC/> ) ] .
[] a owl:Restriction ;
    rdfs:subClassOf <http://vocab.nerc.ac.uk/collection/P02/current/LIFX/> ;
    owl:onProperty glbase:hasMeasurementType ;
    owl:someValuesFrom [ a owl:Class ;
            owl:oneOf ( <http://vocab.nerc.ac.uk/collection/P02/current/LIFX/> ) ] .
[] a owl:Restriction ;
    rdfs:subClassOf <http://vocab.nerc.ac.uk/collection/P02/current/GTCH/> ;
    owl:onProperty glbase:hasMeasurementType ;
    owl:someValuesFrom [ a owl:Class ;
            owl:oneOf ( <http://vocab.nerc.ac.uk/collection/P02/current/GTCH/> ) ] .
[] a owl:Restriction ;
    rdfs:subClassOf <http://vocab.nerc.ac.uk/collection/P02/current/PEWB/> ;
    owl:onProperty glbase:hasMeasurementType ;
    owl:someValuesFrom [ a owl:Class ;
            owl:oneOf ( <http://vocab.nerc.ac.uk/collection/P02/current/PEWB/> ) ] .
[] a owl:Restriction ;
    rdfs:subClassOf <http://vocab.nerc.ac.uk/collection/P02/current/STMP/> ;
    owl:onProperty glbase:hasMeasurementType ;
    owl:someValuesFrom [ a owl:Class ;
            owl:oneOf ( <http://vocab.nerc.ac.uk/collection/P02/current/STMP/> ) ] .
[] a owl:Restriction ;
    rdfs:subClassOf <http://vocab.nerc.ac.uk/collection/P02/current/FPFX/> ;
    owl:onProperty glbase:hasMeasurementType ;
    owl:someValuesFrom [ a owl:Class ;
            owl:oneOf ( <http://vocab.nerc.ac.uk/collection/P02/current/FPFX/> ) ] .
[] a owl:Restriction ;
    rdfs:subClassOf <http://vocab.nerc.ac.uk/collection/P02/current/DOCC/> ;
    owl:onProperty glbase:hasMeasurementType ;
    owl:someValuesFrom [ a owl:Class ;
            owl:oneOf ( <http://vocab.nerc.ac.uk/collection/P02/current/DOCC/> ) ] .
[] a owl:Restriction ;
    rdfs:subClassOf <http://vocab.nerc.ac.uk/collection/P02/current/SPOL/> ;
    owl:onProperty glbase:hasMeasurementType ;
    owl:someValuesFrom [ a owl:Class ;
            owl:oneOf ( <http://vocab.nerc.ac.uk/collection/P02/current/SPOL/> ) ] .
[] a owl:Restriction ;
    rdfs:subClassOf <http://vocab.nerc.ac.uk/collection/P02/current/CDRU/> ;
    owl:onProperty glbase:hasMeasurementType ;
    owl:someValuesFrom [ a owl:Class ;
            owl:oneOf ( <http://vocab.nerc.ac.uk/collection/P02/current/CDRU/> ) ] .
[] a owl:Restriction ;
    rdfs:subClassOf <http://vocab.nerc.ac.uk/collection/P02/current/PYTT/> ;
    owl:onProperty glbase:hasMeasurementType ;
    owl:someValuesFrom [ a owl:Class ;
            owl:oneOf ( <http://vocab.nerc.ac.uk/collection/P02/current/PYTT/> ) ] .
[] a owl:Restriction ;
    rdfs:subClassOf <http://vocab.nerc.ac.uk/collection/P02/current/STCO/> ;
    owl:onProperty glbase:hasMeasurementType ;
    owl:someValuesFrom [ a owl:Class ;
            owl:oneOf ( <http://vocab.nerc.ac.uk/collection/P02/current/STCO/> ) ] .
[] a owl:Restriction ;
    rdfs:subClassOf <http://vocab.nerc.ac.uk/collection/P02/current/BAUC/> ;
    owl:onProperty glbase:hasMeasurementType ;
    owl:someValuesFrom [ a owl:Class ;
            owl:oneOf ( <http://vocab.nerc.ac.uk/collection/P02/current/BAUC/> ) ] .
[] a owl:Restriction ;
    rdfs:subClassOf <http://vocab.nerc.ac.uk/collection/P02/current/MTIC/> ;
    owl:onProperty glbase:hasMeasurementType ;
    owl:someValuesFrom [ a owl:Class ;
            owl:oneOf ( <http://vocab.nerc.ac.uk/collection/P02/current/MTIC/> ) ] .
[] a owl:Restriction ;
    rdfs:subClassOf <http://vocab.nerc.ac.uk/collection/P02/current/ATVS/> ;
    owl:onProperty glbase:hasMeasurementType ;
    owl:someValuesFrom [ a owl:Class ;
            owl:oneOf ( <http://vocab.nerc.ac.uk/collection/P02/current/ATVS/> ) ] .
[] a owl:Restriction ;
    rdfs:subClassOf <http://vocab.nerc.ac.uk/collection/P02/current/IAGE/> ;
    owl:onProperty glbase:hasMeasurementType ;
    owl:someValuesFrom [ a owl:Class ;
            owl:oneOf ( <http://vocab.nerc.ac.uk/collection/P02/current/IAGE/> ) ] .
[] a owl:Restriction ;
    rdfs:subClassOf <http://vocab.nerc.ac.uk/collection/P02/current/MFLZ/> ;
    owl:onProperty glbase:hasMeasurementType ;
    owl:someValuesFrom [ a owl:Class ;
            owl:oneOf ( <http://vocab.nerc.ac.uk/collection/P02/current/MFLZ/> ) ] .
[] a owl:Restriction ;
    rdfs:subClassOf <http://vocab.nerc.ac.uk/collection/P02/current/GPIG/> ;
    owl:onProperty glbase:hasMeasurementType ;
    owl:someValuesFrom [ a owl:Class ;
            owl:oneOf ( <http://vocab.nerc.ac.uk/collection/P02/current/GPIG/> ) ] .
[] a owl:Restriction ;
    rdfs:subClassOf <http://vocab.nerc.ac.uk/collection/P02/current/CLXX/> ;
    owl:onProperty glbase:hasMeasurementType ;
    owl:someValuesFrom [ a owl:Class ;
            owl:oneOf ( <http://vocab.nerc.ac.uk/collection/P02/current/CLXX/> ) ] .
[] a owl:Restriction ;
    rdfs:subClassOf <http://vocab.nerc.ac.uk/collection/P02/current/SRFR/> ;
    owl:onProperty glbase:hasMeasurementType ;
    owl:someValuesFrom [ a owl:Class ;
            owl:oneOf ( <http://vocab.nerc.ac.uk/collection/P02/current/SRFR/> ) ] .
[] a owl:Restriction ;
    rdfs:subClassOf <http://vocab.nerc.ac.uk/collection/P02/current/BCOC/> ;
    owl:onProperty glbase:hasMeasurementType ;
    owl:someValuesFrom [ a owl:Class ;
            owl:oneOf ( <http://vocab.nerc.ac.uk/collection/P02/current/BCOC/> ) ] .
[] a owl:Restriction ;
    rdfs:subClassOf <http://vocab.nerc.ac.uk/collection/P02/current/NTUP/> ;
    owl:onProperty glbase:hasMeasurementType ;
    owl:someValuesFrom [ a owl:Class ;
            owl:oneOf ( <http://vocab.nerc.ac.uk/collection/P02/current/NTUP/> ) ] .
[] a owl:Restriction ;
    rdfs:subClassOf <http://vocab.nerc.ac.uk/collection/P02/current/CAKN/> ;
    owl:onProperty glbase:hasMeasurementType ;
    owl:someValuesFrom [ a owl:Class ;
            owl:oneOf ( <http://vocab.nerc.ac.uk/collection/P02/current/CAKN/> ) ] .
[] a owl:Restriction ;
    rdfs:subClassOf <http://vocab.nerc.ac.uk/collection/P02/current/SIXX/> ;
    owl:onProperty glbase:hasMeasurementType ;
    owl:someValuesFrom [ a owl:Class ;
            owl:oneOf ( <http://vocab.nerc.ac.uk/collection/P02/current/SIXX/> ) ] .
[] a owl:Restriction ;
    rdfs:subClassOf <http://vocab.nerc.ac.uk/collection/P02/current/APZA/> ;
    owl:onProperty glbase:hasMeasurementType ;
    owl:someValuesFrom [ a owl:Class ;
            owl:oneOf ( <http://vocab.nerc.ac.uk/collection/P02/current/APZA/> ) ] .
[] a owl:Restriction ;
    rdfs:subClassOf <http://vocab.nerc.ac.uk/collection/P02/current/SAGE/> ;
    owl:onProperty glbase:hasMeasurementType ;
    owl:someValuesFrom [ a owl:Class ;
            owl:oneOf ( <http://vocab.nerc.ac.uk/collection/P02/current/SAGE/> ) ] .
[] a owl:Restriction ;
    rdfs:subClassOf <http://vocab.nerc.ac.uk/collection/P02/current/ZADX/> ;
    owl:onProperty glbase:hasMeasurementType ;
    owl:someValuesFrom [ a owl:Class ;
            owl:oneOf ( <http://vocab.nerc.ac.uk/collection/P02/current/ZADX/> ) ] .
[] a owl:Restriction ;
    rdfs:subClassOf <http://vocab.nerc.ac.uk/collection/P02/current/PU02/> ;
    owl:onProperty glbase:hasMeasurementType ;
    owl:someValuesFrom [ a owl:Class ;
            owl:oneOf ( <http://vocab.nerc.ac.uk/collection/P02/current/PU02/> ) ] .
[] a owl:Restriction ;
    rdfs:subClassOf <http://vocab.nerc.ac.uk/collection/P02/current/BPBP/> ;
    owl:onProperty glbase:hasMeasurementType ;
    owl:someValuesFrom [ a owl:Class ;
            owl:oneOf ( <http://vocab.nerc.ac.uk/collection/P02/current/BPBP/> ) ] .
[] a owl:Restriction ;
    rdfs:subClassOf <http://vocab.nerc.ac.uk/collection/P02/current/ENGP/> ;
    owl:onProperty glbase:hasMeasurementType ;
    owl:someValuesFrom [ a owl:Class ;
            owl:oneOf ( <http://vocab.nerc.ac.uk/collection/P02/current/ENGP/> ) ] .
[] a owl:Restriction ;
    rdfs:subClassOf <http://vocab.nerc.ac.uk/collection/P02/current/RBHY/> ;
    owl:onProperty glbase:hasMeasurementType ;
    owl:someValuesFrom [ a owl:Class ;
            owl:oneOf ( <http://vocab.nerc.ac.uk/collection/P02/current/RBHY/> ) ] .
[] a owl:Restriction ;
    rdfs:subClassOf <http://vocab.nerc.ac.uk/collection/P02/current/ASLV/> ;
    owl:onProperty glbase:hasMeasurementType ;
    owl:someValuesFrom [ a owl:Class ;
            owl:oneOf ( <http://vocab.nerc.ac.uk/collection/P02/current/ASLV/> ) ] .
[] a owl:Restriction ;
    rdfs:subClassOf <http://vocab.nerc.ac.uk/collection/P02/current/BLUM/> ;
    owl:onProperty glbase:hasMeasurementType ;
    owl:someValuesFrom [ a owl:Class ;
            owl:oneOf ( <http://vocab.nerc.ac.uk/collection/P02/current/BLUM/> ) ] .
[] a owl:Restriction ;
    rdfs:subClassOf <http://vocab.nerc.ac.uk/collection/P02/current/GP068/> ;
    owl:onProperty glbase:hasMeasurementType ;
    owl:someValuesFrom [ a owl:Class ;
            owl:oneOf ( <http://vocab.nerc.ac.uk/collection/P02/current/GP068/> ) ] .
[] a owl:Restriction ;
    rdfs:subClassOf <http://vocab.nerc.ac.uk/collection/P02/current/HBEX/> ;
    owl:onProperty glbase:hasMeasurementType ;
    owl:someValuesFrom [ a owl:Class ;
            owl:oneOf ( <http://vocab.nerc.ac.uk/collection/P02/current/HBEX/> ) ] .
[] a owl:Restriction ;
    rdfs:subClassOf <http://vocab.nerc.ac.uk/collection/P02/current/BCMT/> ;
    owl:onProperty glbase:hasMeasurementType ;
    owl:someValuesFrom [ a owl:Class ;
            owl:oneOf ( <http://vocab.nerc.ac.uk/collection/P02/current/BCMT/> ) ] .
[] a owl:Restriction ;
    rdfs:subClassOf <http://vocab.nerc.ac.uk/collection/P02/current/OGPW/> ;
    owl:onProperty glbase:hasMeasurementType ;
    owl:someValuesFrom [ a owl:Class ;
            owl:oneOf ( <http://vocab.nerc.ac.uk/collection/P02/current/OGPW/> ) ] .
[] a owl:Restriction ;
    rdfs:subClassOf <http://vocab.nerc.ac.uk/collection/P02/current/REFF/> ;
    owl:onProperty glbase:hasMeasurementType ;
    owl:someValuesFrom [ a owl:Class ;
            owl:oneOf ( <http://vocab.nerc.ac.uk/collection/P02/current/REFF/> ) ] .
[] a owl:Restriction ;
    rdfs:subClassOf <http://vocab.nerc.ac.uk/collection/P02/current/RFVL/> ;
    owl:onProperty glbase:hasMeasurementType ;
    owl:someValuesFrom [ a owl:Class ;
            owl:oneOf ( <http://vocab.nerc.ac.uk/collection/P02/current/RFVL/> ) ] .
[] a owl:Restriction ;
    rdfs:subClassOf <http://vocab.nerc.ac.uk/collection/P02/current/IS4R/> ;
    owl:onProperty glbase:hasMeasurementType ;
    owl:someValuesFrom [ a owl:Class ;
            owl:oneOf ( <http://vocab.nerc.ac.uk/collection/P02/current/IS4R/> ) ] .
[] a owl:Restriction ;
    rdfs:subClassOf <http://vocab.nerc.ac.uk/collection/P02/current/HZNV/> ;
    owl:onProperty glbase:hasMeasurementType ;
    owl:someValuesFrom [ a owl:Class ;
            owl:oneOf ( <http://vocab.nerc.ac.uk/collection/P02/current/HZNV/> ) ] .
[] a owl:Restriction ;
    rdfs:subClassOf <http://vocab.nerc.ac.uk/collection/P02/current/PESD/> ;
    owl:onProperty glbase:hasMeasurementType ;
    owl:someValuesFrom [ a owl:Class ;
            owl:oneOf ( <http://vocab.nerc.ac.uk/collection/P02/current/PESD/> ) ] .
[] a owl:Restriction ;
    rdfs:subClassOf <http://vocab.nerc.ac.uk/collection/P02/current/VDFC/> ;
    owl:onProperty glbase:hasMeasurementType ;
    owl:someValuesFrom [ a owl:Class ;
            owl:oneOf ( <http://vocab.nerc.ac.uk/collection/P02/current/VDFC/> ) ] .
[] a owl:Restriction ;
    rdfs:subClassOf <http://vocab.nerc.ac.uk/collection/P02/current/SRAD/> ;
    owl:onProperty glbase:hasMeasurementType ;
    owl:someValuesFrom [ a owl:Class ;
            owl:oneOf ( <http://vocab.nerc.ac.uk/collection/P02/current/SRAD/> ) ] .
[] a owl:Restriction ;
    rdfs:subClassOf <http://vocab.nerc.ac.uk/collection/P02/current/ATEM/> ;
    owl:onProperty glbase:hasMeasurementType ;
    owl:someValuesFrom [ a owl:Class ;
            owl:oneOf ( <http://vocab.nerc.ac.uk/collection/P02/current/ATEM/> ) ] .
[] a owl:Restriction ;
    rdfs:subClassOf <http://vocab.nerc.ac.uk/collection/P02/current/RPOT/> ;
    owl:onProperty glbase:hasMeasurementType ;
    owl:someValuesFrom [ a owl:Class ;
            owl:oneOf ( <http://vocab.nerc.ac.uk/collection/P02/current/RPOT/> ) ] .
[] a owl:Restriction ;
    rdfs:subClassOf <http://vocab.nerc.ac.uk/collection/P02/current/MSBD/> ;
    owl:onProperty glbase:hasMeasurementType ;
    owl:someValuesFrom [ a owl:Class ;
            owl:oneOf ( <http://vocab.nerc.ac.uk/collection/P02/current/MSBD/> ) ] .
[] a owl:Restriction ;
    rdfs:subClassOf <http://vocab.nerc.ac.uk/collection/P02/current/DCMX/> ;
    owl:onProperty glbase:hasMeasurementType ;
    owl:someValuesFrom [ a owl:Class ;
            owl:oneOf ( <http://vocab.nerc.ac.uk/collection/P02/current/DCMX/> ) ] .
[] a owl:Restriction ;
    rdfs:subClassOf <http://vocab.nerc.ac.uk/collection/P02/current/AAMN/> ;
    owl:onProperty glbase:hasMeasurementType ;
    owl:someValuesFrom [ a owl:Class ;
            owl:oneOf ( <http://vocab.nerc.ac.uk/collection/P02/current/AAMN/> ) ] .
[] a owl:Restriction ;
    rdfs:subClassOf <http://vocab.nerc.ac.uk/collection/P02/current/GP067/> ;
    owl:onProperty glbase:hasMeasurementType ;
    owl:someValuesFrom [ a owl:Class ;
            owl:oneOf ( <http://vocab.nerc.ac.uk/collection/P02/current/GP067/> ) ] .
[] a owl:Restriction ;
    rdfs:subClassOf <http://vocab.nerc.ac.uk/collection/P02/current/CHUM/> ;
    owl:onProperty glbase:hasMeasurementType ;
    owl:someValuesFrom [ a owl:Class ;
            owl:oneOf ( <http://vocab.nerc.ac.uk/collection/P02/current/CHUM/> ) ] .
[] a owl:Restriction ;
    rdfs:subClassOf <http://vocab.nerc.ac.uk/collection/P02/current/ACYC/> ;
    owl:onProperty glbase:hasMeasurementType ;
    owl:someValuesFrom [ a owl:Class ;
            owl:oneOf ( <http://vocab.nerc.ac.uk/collection/P02/current/ACYC/> ) ] .
[] a owl:Restriction ;
    rdfs:subClassOf <http://vocab.nerc.ac.uk/collection/P02/current/DPEV/> ;
    owl:onProperty glbase:hasMeasurementType ;
    owl:someValuesFrom [ a owl:Class ;
            owl:oneOf ( <http://vocab.nerc.ac.uk/collection/P02/current/DPEV/> ) ] .
[] a owl:Restriction ;
    rdfs:subClassOf <http://vocab.nerc.ac.uk/collection/P02/current/CEBH/> ;
    owl:onProperty glbase:hasMeasurementType ;
    owl:someValuesFrom [ a owl:Class ;
            owl:oneOf ( <http://vocab.nerc.ac.uk/collection/P02/current/CEBH/> ) ] .
[] a owl:Restriction ;
    rdfs:subClassOf <http://vocab.nerc.ac.uk/collection/P02/current/MLES/> ;
    owl:onProperty glbase:hasMeasurementType ;
    owl:someValuesFrom [ a owl:Class ;
            owl:oneOf ( <http://vocab.nerc.ac.uk/collection/P02/current/MLES/> ) ] .
[] a owl:Restriction ;
    rdfs:subClassOf <http://vocab.nerc.ac.uk/collection/P02/current/FABD/> ;
    owl:onProperty glbase:hasMeasurementType ;
    owl:someValuesFrom [ a owl:Class ;
            owl:oneOf ( <http://vocab.nerc.ac.uk/collection/P02/current/FABD/> ) ] .
[] a owl:Restriction ;
    rdfs:subClassOf <http://vocab.nerc.ac.uk/collection/P02/current/TD00/> ;
    owl:onProperty glbase:hasMeasurementType ;
    owl:someValuesFrom [ a owl:Class ;
            owl:oneOf ( <http://vocab.nerc.ac.uk/collection/P02/current/TD00/> ) ] .
[] a owl:Restriction ;
    rdfs:subClassOf <http://vocab.nerc.ac.uk/collection/P02/current/GP001/> ;
    owl:onProperty glbase:hasMeasurementType ;
    owl:someValuesFrom [ a owl:Class ;
            owl:oneOf ( <http://vocab.nerc.ac.uk/collection/P02/current/GP001/> ) ] .
[] a owl:Restriction ;
    rdfs:subClassOf <http://vocab.nerc.ac.uk/collection/P02/current/RTMP/> ;
    owl:onProperty glbase:hasMeasurementType ;
    owl:someValuesFrom [ a owl:Class ;
            owl:oneOf ( <http://vocab.nerc.ac.uk/collection/P02/current/RTMP/> ) ] .
[] a owl:Restriction ;
    rdfs:subClassOf <http://vocab.nerc.ac.uk/collection/P02/current/APDA/> ;
    owl:onProperty glbase:hasMeasurementType ;
    owl:someValuesFrom [ a owl:Class ;
            owl:oneOf ( <http://vocab.nerc.ac.uk/collection/P02/current/APDA/> ) ] .
[] a owl:Restriction ;
    rdfs:subClassOf <http://vocab.nerc.ac.uk/collection/P02/current/CXAA/> ;
    owl:onProperty glbase:hasMeasurementType ;
    owl:someValuesFrom [ a owl:Class ;
            owl:oneOf ( <http://vocab.nerc.ac.uk/collection/P02/current/CXAA/> ) ] .
[] a owl:Restriction ;
    rdfs:subClassOf <http://vocab.nerc.ac.uk/collection/P02/current/CPWC/> ;
    owl:onProperty glbase:hasMeasurementType ;
    owl:someValuesFrom [ a owl:Class ;
            owl:oneOf ( <http://vocab.nerc.ac.uk/collection/P02/current/CPWC/> ) ] .
[] a owl:Restriction ;
    rdfs:subClassOf <http://vocab.nerc.ac.uk/collection/P02/current/FATM/> ;
    owl:onProperty glbase:hasMeasurementType ;
    owl:someValuesFrom [ a owl:Class ;
            owl:oneOf ( <http://vocab.nerc.ac.uk/collection/P02/current/FATM/> ) ] .
[] a owl:Restriction ;
    rdfs:subClassOf <http://vocab.nerc.ac.uk/collection/P02/current/DBDX/> ;
    owl:onProperty glbase:hasMeasurementType ;
    owl:someValuesFrom [ a owl:Class ;
            owl:oneOf ( <http://vocab.nerc.ac.uk/collection/P02/current/DBDX/> ) ] .
[] a owl:Restriction ;
    rdfs:subClassOf <http://vocab.nerc.ac.uk/collection/P02/current/RWCH/> ;
    owl:onProperty glbase:hasMeasurementType ;
    owl:someValuesFrom [ a owl:Class ;
            owl:oneOf ( <http://vocab.nerc.ac.uk/collection/P02/current/RWCH/> ) ] .
[] a owl:Restriction ;
    rdfs:subClassOf <http://vocab.nerc.ac.uk/collection/P02/current/ZATX/> ;
    owl:onProperty glbase:hasMeasurementType ;
    owl:someValuesFrom [ a owl:Class ;
            owl:oneOf ( <http://vocab.nerc.ac.uk/collection/P02/current/ZATX/> ) ] .
[] a owl:Restriction ;
    rdfs:subClassOf <http://vocab.nerc.ac.uk/collection/P02/current/VSRA/> ;
    owl:onProperty glbase:hasMeasurementType ;
    owl:someValuesFrom [ a owl:Class ;
            owl:oneOf ( <http://vocab.nerc.ac.uk/collection/P02/current/VSRA/> ) ] .
[] a owl:Restriction ;
    rdfs:subClassOf <http://vocab.nerc.ac.uk/collection/P02/current/WSTR/> ;
    owl:onProperty glbase:hasMeasurementType ;
    owl:someValuesFrom [ a owl:Class ;
            owl:oneOf ( <http://vocab.nerc.ac.uk/collection/P02/current/WSTR/> ) ] .
[] a owl:Restriction ;
    rdfs:subClassOf <http://vocab.nerc.ac.uk/collection/P02/current/TCFX/> ;
    owl:onProperty glbase:hasMeasurementType ;
    owl:someValuesFrom [ a owl:Class ;
            owl:oneOf ( <http://vocab.nerc.ac.uk/collection/P02/current/TCFX/> ) ] .
[] a owl:Restriction ;
    rdfs:subClassOf <http://vocab.nerc.ac.uk/collection/P02/current/SCAH/> ;
    owl:onProperty glbase:hasMeasurementType ;
    owl:someValuesFrom [ a owl:Class ;
            owl:oneOf ( <http://vocab.nerc.ac.uk/collection/P02/current/SCAH/> ) ] .
[] a owl:Restriction ;
    rdfs:subClassOf <http://vocab.nerc.ac.uk/collection/P02/current/BLEN/> ;
    owl:onProperty glbase:hasMeasurementType ;
    owl:someValuesFrom [ a owl:Class ;
            owl:oneOf ( <http://vocab.nerc.ac.uk/collection/P02/current/BLEN/> ) ] .
[] a owl:Restriction ;
    rdfs:subClassOf <http://vocab.nerc.ac.uk/collection/P02/current/MDWD/> ;
    owl:onProperty glbase:hasMeasurementType ;
    owl:someValuesFrom [ a owl:Class ;
            owl:oneOf ( <http://vocab.nerc.ac.uk/collection/P02/current/MDWD/> ) ] .
[] a owl:Restriction ;
    rdfs:subClassOf <http://vocab.nerc.ac.uk/collection/P02/current/MDWP/> ;
    owl:onProperty glbase:hasMeasurementType ;
    owl:someValuesFrom [ a owl:Class ;
            owl:oneOf ( <http://vocab.nerc.ac.uk/collection/P02/current/MDWP/> ) ] .
[] a owl:Restriction ;
    rdfs:subClassOf <http://vocab.nerc.ac.uk/collection/P02/current/CYEU/> ;
    owl:onProperty glbase:hasMeasurementType ;
    owl:someValuesFrom [ a owl:Class ;
            owl:oneOf ( <http://vocab.nerc.ac.uk/collection/P02/current/CYEU/> ) ] .
[] a owl:Restriction ;
    rdfs:subClassOf <http://vocab.nerc.ac.uk/collection/P02/current/IATX/> ;
    owl:onProperty glbase:hasMeasurementType ;
    owl:someValuesFrom [ a owl:Class ;
            owl:oneOf ( <http://vocab.nerc.ac.uk/collection/P02/current/IATX/> ) ] .
[] a owl:Restriction ;
    rdfs:subClassOf <http://vocab.nerc.ac.uk/collection/P02/current/SAMO/> ;
    owl:onProperty glbase:hasMeasurementType ;
    owl:someValuesFrom [ a owl:Class ;
            owl:oneOf ( <http://vocab.nerc.ac.uk/collection/P02/current/SAMO/> ) ] .
[] a owl:Restriction ;
    rdfs:subClassOf <http://vocab.nerc.ac.uk/collection/P02/current/XKEY/> ;
    owl:onProperty glbase:hasMeasurementType ;
    owl:someValuesFrom [ a owl:Class ;
            owl:oneOf ( <http://vocab.nerc.ac.uk/collection/P02/current/XKEY/> ) ] .
[] a owl:Restriction ;
    rdfs:subClassOf <http://vocab.nerc.ac.uk/collection/P02/current/SR2D/> ;
    owl:onProperty glbase:hasMeasurementType ;
    owl:someValuesFrom [ a owl:Class ;
            owl:oneOf ( <http://vocab.nerc.ac.uk/collection/P02/current/SR2D/> ) ] .
[] a owl:Restriction ;
    rdfs:subClassOf <http://vocab.nerc.ac.uk/collection/P02/current/WPRO/> ;
    owl:onProperty glbase:hasMeasurementType ;
    owl:someValuesFrom [ a owl:Class ;
            owl:oneOf ( <http://vocab.nerc.ac.uk/collection/P02/current/WPRO/> ) ] .
[] a owl:Restriction ;
    rdfs:subClassOf <http://vocab.nerc.ac.uk/collection/P02/current/WSTB/> ;
    owl:onProperty glbase:hasMeasurementType ;
    owl:someValuesFrom [ a owl:Class ;
            owl:oneOf ( <http://vocab.nerc.ac.uk/collection/P02/current/WSTB/> ) ] .
[] a owl:Restriction ;
    rdfs:subClassOf <http://vocab.nerc.ac.uk/collection/P02/current/EXSV/> ;
    owl:onProperty glbase:hasMeasurementType ;
    owl:someValuesFrom [ a owl:Class ;
            owl:oneOf ( <http://vocab.nerc.ac.uk/collection/P02/current/EXSV/> ) ] .
[] a owl:Restriction ;
    rdfs:subClassOf <http://vocab.nerc.ac.uk/collection/P02/current/TRAN/> ;
    owl:onProperty glbase:hasMeasurementType ;
    owl:someValuesFrom [ a owl:Class ;
            owl:oneOf ( <http://vocab.nerc.ac.uk/collection/P02/current/TRAN/> ) ] .
[] a owl:Restriction ;
    rdfs:subClassOf <http://vocab.nerc.ac.uk/collection/P02/current/OCPW/> ;
    owl:onProperty glbase:hasMeasurementType ;
    owl:someValuesFrom [ a owl:Class ;
            owl:oneOf ( <http://vocab.nerc.ac.uk/collection/P02/current/OCPW/> ) ] .
[] a owl:Restriction ;
    rdfs:subClassOf <http://vocab.nerc.ac.uk/collection/P02/current/PREX/> ;
    owl:onProperty glbase:hasMeasurementType ;
    owl:someValuesFrom [ a owl:Class ;
            owl:oneOf ( <http://vocab.nerc.ac.uk/collection/P02/current/PREX/> ) ] .
[] a owl:Restriction ;
    rdfs:subClassOf <http://vocab.nerc.ac.uk/collection/P02/current/CDTA/> ;
    owl:onProperty glbase:hasMeasurementType ;
    owl:someValuesFrom [ a owl:Class ;
            owl:oneOf ( <http://vocab.nerc.ac.uk/collection/P02/current/CDTA/> ) ] .
[] a owl:Restriction ;
    rdfs:subClassOf <http://vocab.nerc.ac.uk/collection/P02/current/NTRZ/> ;
    owl:onProperty glbase:hasMeasurementType ;
    owl:someValuesFrom [ a owl:Class ;
            owl:oneOf ( <http://vocab.nerc.ac.uk/collection/P02/current/NTRZ/> ) ] .
[] a owl:Restriction ;
    rdfs:subClassOf <http://vocab.nerc.ac.uk/collection/P02/current/SRFL/> ;
    owl:onProperty glbase:hasMeasurementType ;
    owl:someValuesFrom [ a owl:Class ;
            owl:oneOf ( <http://vocab.nerc.ac.uk/collection/P02/current/SRFL/> ) ] .
[] a owl:Restriction ;
    rdfs:subClassOf <http://vocab.nerc.ac.uk/collection/P02/current/UPTH/> ;
    owl:onProperty glbase:hasMeasurementType ;
    owl:someValuesFrom [ a owl:Class ;
            owl:oneOf ( <http://vocab.nerc.ac.uk/collection/P02/current/UPTH/> ) ] .
[] a owl:Restriction ;
    rdfs:subClassOf <http://vocab.nerc.ac.uk/collection/P02/current/RPER/> ;
    owl:onProperty glbase:hasMeasurementType ;
    owl:someValuesFrom [ a owl:Class ;
            owl:oneOf ( <http://vocab.nerc.ac.uk/collection/P02/current/RPER/> ) ] .
[] a owl:Restriction ;
    rdfs:subClassOf <http://vocab.nerc.ac.uk/collection/P02/current/TCNT/> ;
    owl:onProperty glbase:hasMeasurementType ;
    owl:someValuesFrom [ a owl:Class ;
            owl:oneOf ( <http://vocab.nerc.ac.uk/collection/P02/current/TCNT/> ) ] .
[] a owl:Restriction ;
    rdfs:subClassOf <http://vocab.nerc.ac.uk/collection/P02/current/TDIN/> ;
    owl:onProperty glbase:hasMeasurementType ;
    owl:someValuesFrom [ a owl:Class ;
            owl:oneOf ( <http://vocab.nerc.ac.uk/collection/P02/current/TDIN/> ) ] .
[] a owl:Restriction ;
    rdfs:subClassOf <http://vocab.nerc.ac.uk/collection/P02/current/DALK/> ;
    owl:onProperty glbase:hasMeasurementType ;
    owl:someValuesFrom [ a owl:Class ;
            owl:oneOf ( <http://vocab.nerc.ac.uk/collection/P02/current/DALK/> ) ] .
[] a owl:Restriction ;
    rdfs:subClassOf <http://vocab.nerc.ac.uk/collection/P02/current/HFLW/> ;
    owl:onProperty glbase:hasMeasurementType ;
    owl:someValuesFrom [ a owl:Class ;
            owl:oneOf ( <http://vocab.nerc.ac.uk/collection/P02/current/HFLW/> ) ] .
[] a owl:Restriction ;
    rdfs:subClassOf <http://vocab.nerc.ac.uk/collection/P02/current/ASAM/> ;
    owl:onProperty glbase:hasMeasurementType ;
    owl:someValuesFrom [ a owl:Class ;
            owl:oneOf ( <http://vocab.nerc.ac.uk/collection/P02/current/ASAM/> ) ] .
[] a owl:Restriction ;
    rdfs:subClassOf <http://vocab.nerc.ac.uk/collection/P02/current/TDNT/> ;
    owl:onProperty glbase:hasMeasurementType ;
    owl:someValuesFrom [ a owl:Class ;
            owl:oneOf ( <http://vocab.nerc.ac.uk/collection/P02/current/TDNT/> ) ] .
[] a owl:Restriction ;
    rdfs:subClassOf <http://vocab.nerc.ac.uk/collection/P02/current/BRDD/> ;
    owl:onProperty glbase:hasMeasurementType ;
    owl:someValuesFrom [ a owl:Class ;
            owl:oneOf ( <http://vocab.nerc.ac.uk/collection/P02/current/BRDD/> ) ] .
[] a owl:Restriction ;
    rdfs:subClassOf <http://vocab.nerc.ac.uk/collection/P02/current/CMFL/> ;
    owl:onProperty glbase:hasMeasurementType ;
    owl:someValuesFrom [ a owl:Class ;
            owl:oneOf ( <http://vocab.nerc.ac.uk/collection/P02/current/CMFL/> ) ] .
[] a owl:Restriction ;
    rdfs:subClassOf <http://vocab.nerc.ac.uk/collection/P02/current/GWAM/> ;
    owl:onProperty glbase:hasMeasurementType ;
    owl:someValuesFrom [ a owl:Class ;
            owl:oneOf ( <http://vocab.nerc.ac.uk/collection/P02/current/GWAM/> ) ] .
[] a owl:Restriction ;
    rdfs:subClassOf <http://vocab.nerc.ac.uk/collection/P02/current/IRIC/> ;
    owl:onProperty glbase:hasMeasurementType ;
    owl:someValuesFrom [ a owl:Class ;
            owl:oneOf ( <http://vocab.nerc.ac.uk/collection/P02/current/IRIC/> ) ] .
[] a owl:Restriction ;
    rdfs:subClassOf <http://vocab.nerc.ac.uk/collection/P02/current/XRFC/> ;
    owl:onProperty glbase:hasMeasurementType ;
    owl:someValuesFrom [ a owl:Class ;
            owl:oneOf ( <http://vocab.nerc.ac.uk/collection/P02/current/XRFC/> ) ] .
[] a owl:Restriction ;
    rdfs:subClassOf <http://vocab.nerc.ac.uk/collection/P02/current/FNTX/> ;
    owl:onProperty glbase:hasMeasurementType ;
    owl:someValuesFrom [ a owl:Class ;
            owl:oneOf ( <http://vocab.nerc.ac.uk/collection/P02/current/FNTX/> ) ] .
[] a owl:Restriction ;
    rdfs:subClassOf <http://vocab.nerc.ac.uk/collection/P02/current/SIPW/> ;
    owl:onProperty glbase:hasMeasurementType ;
    owl:someValuesFrom [ a owl:Class ;
            owl:oneOf ( <http://vocab.nerc.ac.uk/collection/P02/current/SIPW/> ) ] .
[] a owl:Restriction ;
    rdfs:subClassOf <http://vocab.nerc.ac.uk/collection/P02/current/ZNTP/> ;
    owl:onProperty glbase:hasMeasurementType ;
    owl:someValuesFrom [ a owl:Class ;
            owl:oneOf ( <http://vocab.nerc.ac.uk/collection/P02/current/ZNTP/> ) ] .
[] a owl:Restriction ;
    rdfs:subClassOf <http://vocab.nerc.ac.uk/collection/P02/current/AATX/> ;
    owl:onProperty glbase:hasMeasurementType ;
    owl:someValuesFrom [ a owl:Class ;
            owl:oneOf ( <http://vocab.nerc.ac.uk/collection/P02/current/AATX/> ) ] .
[] a owl:Restriction ;
    rdfs:subClassOf <http://vocab.nerc.ac.uk/collection/P02/current/SR3D/> ;
    owl:onProperty glbase:hasMeasurementType ;
    owl:someValuesFrom [ a owl:Class ;
            owl:oneOf ( <http://vocab.nerc.ac.uk/collection/P02/current/SR3D/> ) ] .
[] a owl:Restriction ;
    rdfs:subClassOf <http://vocab.nerc.ac.uk/collection/P02/current/AAFX/> ;
    owl:onProperty glbase:hasMeasurementType ;
    owl:someValuesFrom [ a owl:Class ;
            owl:oneOf ( <http://vocab.nerc.ac.uk/collection/P02/current/AAFX/> ) ] .
[] a owl:Restriction ;
    rdfs:subClassOf <http://vocab.nerc.ac.uk/collection/P02/current/WVST/> ;
    owl:onProperty glbase:hasMeasurementType ;
    owl:someValuesFrom [ a owl:Class ;
            owl:oneOf ( <http://vocab.nerc.ac.uk/collection/P02/current/WVST/> ) ] .
[] a owl:Restriction ;
    rdfs:subClassOf <http://vocab.nerc.ac.uk/collection/P02/current/VSRW/> ;
    owl:onProperty glbase:hasMeasurementType ;
    owl:someValuesFrom [ a owl:Class ;
            owl:oneOf ( <http://vocab.nerc.ac.uk/collection/P02/current/VSRW/> ) ] .
[] a owl:Restriction ;
    rdfs:subClassOf <http://vocab.nerc.ac.uk/collection/P02/current/ATPX/> ;
    owl:onProperty glbase:hasMeasurementType ;
    owl:someValuesFrom [ a owl:Class ;
            owl:oneOf ( <http://vocab.nerc.ac.uk/collection/P02/current/ATPX/> ) ] .
[] a owl:Restriction ;
    rdfs:subClassOf <http://vocab.nerc.ac.uk/collection/P02/current/HLAT/> ;
    owl:onProperty glbase:hasMeasurementType ;
    owl:someValuesFrom [ a owl:Class ;
            owl:oneOf ( <http://vocab.nerc.ac.uk/collection/P02/current/HLAT/> ) ] .
[] a owl:Restriction ;
    rdfs:subClassOf <http://vocab.nerc.ac.uk/collection/P02/current/UREA/> ;
    owl:onProperty glbase:hasMeasurementType ;
    owl:someValuesFrom [ a owl:Class ;
            owl:oneOf ( <http://vocab.nerc.ac.uk/collection/P02/current/UREA/> ) ] .
[] a owl:Restriction ;
    rdfs:subClassOf <http://vocab.nerc.ac.uk/collection/P02/current/ATPC/> ;
    owl:onProperty glbase:hasMeasurementType ;
    owl:someValuesFrom [ a owl:Class ;
            owl:oneOf ( <http://vocab.nerc.ac.uk/collection/P02/current/ATPC/> ) ] .
[] a owl:Restriction ;
    rdfs:subClassOf <http://vocab.nerc.ac.uk/collection/P02/current/SABB/> ;
    owl:onProperty glbase:hasMeasurementType ;
    owl:someValuesFrom [ a owl:Class ;
            owl:oneOf ( <http://vocab.nerc.ac.uk/collection/P02/current/SABB/> ) ] .
[] a owl:Restriction ;
    rdfs:subClassOf <http://vocab.nerc.ac.uk/collection/P02/current/COAS/> ;
    owl:onProperty glbase:hasMeasurementType ;
    owl:someValuesFrom [ a owl:Class ;
            owl:oneOf ( <http://vocab.nerc.ac.uk/collection/P02/current/COAS/> ) ] .
[] a owl:Restriction ;
    rdfs:subClassOf <http://vocab.nerc.ac.uk/collection/P02/current/SATM/> ;
    owl:onProperty glbase:hasMeasurementType ;
    owl:someValuesFrom [ a owl:Class ;
            owl:oneOf ( <http://vocab.nerc.ac.uk/collection/P02/current/SATM/> ) ] .
[] a owl:Restriction ;
    rdfs:subClassOf <http://vocab.nerc.ac.uk/collection/P02/current/MSEP/> ;
    owl:onProperty glbase:hasMeasurementType ;
    owl:someValuesFrom [ a owl:Class ;
            owl:oneOf ( <http://vocab.nerc.ac.uk/collection/P02/current/MSEP/> ) ] .
[] a owl:Restriction ;
    rdfs:subClassOf <http://vocab.nerc.ac.uk/collection/P02/current/BRDA/> ;
    owl:onProperty glbase:hasMeasurementType ;
    owl:someValuesFrom [ a owl:Class ;
            owl:oneOf ( <http://vocab.nerc.ac.uk/collection/P02/current/BRDA/> ) ] .
[] a owl:Restriction ;
    rdfs:subClassOf <http://vocab.nerc.ac.uk/collection/P02/current/TCO2/> ;
    owl:onProperty glbase:hasMeasurementType ;
    owl:someValuesFrom [ a owl:Class ;
            owl:oneOf ( <http://vocab.nerc.ac.uk/collection/P02/current/TCO2/> ) ] .
[] a owl:Restriction ;
    rdfs:subClassOf <http://vocab.nerc.ac.uk/collection/P02/current/MBAN/> ;
    owl:onProperty glbase:hasMeasurementType ;
    owl:someValuesFrom [ a owl:Class ;
            owl:oneOf ( <http://vocab.nerc.ac.uk/collection/P02/current/MBAN/> ) ] .
[] a owl:Restriction ;
    rdfs:subClassOf <http://vocab.nerc.ac.uk/collection/P02/current/PHSE/> ;
    owl:onProperty glbase:hasMeasurementType ;
    owl:someValuesFrom [ a owl:Class ;
            owl:oneOf ( <http://vocab.nerc.ac.uk/collection/P02/current/PHSE/> ) ] .
[] a owl:Restriction ;
    rdfs:subClassOf <http://vocab.nerc.ac.uk/collection/P02/current/VATX/> ;
    owl:onProperty glbase:hasMeasurementType ;
    owl:someValuesFrom [ a owl:Class ;
            owl:oneOf ( <http://vocab.nerc.ac.uk/collection/P02/current/VATX/> ) ] .
[] a owl:Restriction ;
    rdfs:subClassOf <http://vocab.nerc.ac.uk/collection/P02/current/GWDR/> ;
    owl:onProperty glbase:hasMeasurementType ;
    owl:someValuesFrom [ a owl:Class ;
            owl:oneOf ( <http://vocab.nerc.ac.uk/collection/P02/current/GWDR/> ) ] .
[] a owl:Restriction ;
    rdfs:subClassOf <http://vocab.nerc.ac.uk/collection/P02/current/ALAT/> ;
    owl:onProperty glbase:hasMeasurementType ;
    owl:someValuesFrom [ a owl:Class ;
            owl:oneOf ( <http://vocab.nerc.ac.uk/collection/P02/current/ALAT/> ) ] .
[] a owl:Restriction ;
    rdfs:subClassOf <http://vocab.nerc.ac.uk/collection/P02/current/MXLM/> ;
    owl:onProperty glbase:hasMeasurementType ;
    owl:someValuesFrom [ a owl:Class ;
            owl:oneOf ( <http://vocab.nerc.ac.uk/collection/P02/current/MXLM/> ) ] .
[] a owl:Restriction ;
    rdfs:subClassOf <http://vocab.nerc.ac.uk/collection/P02/current/PPAB/> ;
    owl:onProperty glbase:hasMeasurementType ;
    owl:someValuesFrom [ a owl:Class ;
            owl:oneOf ( <http://vocab.nerc.ac.uk/collection/P02/current/PPAB/> ) ] .
[] a owl:Restriction ;
    rdfs:subClassOf <http://vocab.nerc.ac.uk/collection/P02/current/HBCH/> ;
    owl:onProperty glbase:hasMeasurementType ;
    owl:someValuesFrom [ a owl:Class ;
            owl:oneOf ( <http://vocab.nerc.ac.uk/collection/P02/current/HBCH/> ) ] .
[] a owl:Restriction ;
    rdfs:subClassOf <http://vocab.nerc.ac.uk/collection/P02/current/NTSD/> ;
    owl:onProperty glbase:hasMeasurementType ;
    owl:someValuesFrom [ a owl:Class ;
            owl:oneOf ( <http://vocab.nerc.ac.uk/collection/P02/current/NTSD/> ) ] .
[] a owl:Restriction ;
    rdfs:subClassOf <http://vocab.nerc.ac.uk/collection/P02/current/PATX/> ;
    owl:onProperty glbase:hasMeasurementType ;
    owl:someValuesFrom [ a owl:Class ;
            owl:oneOf ( <http://vocab.nerc.ac.uk/collection/P02/current/PATX/> ) ] .
[] a owl:Restriction ;
    rdfs:subClassOf <http://vocab.nerc.ac.uk/collection/P02/current/NTIC/> ;
    owl:onProperty glbase:hasMeasurementType ;
    owl:someValuesFrom [ a owl:Class ;
            owl:oneOf ( <http://vocab.nerc.ac.uk/collection/P02/current/NTIC/> ) ] .
[] a owl:Restriction ;
    rdfs:subClassOf <http://vocab.nerc.ac.uk/collection/P02/current/LVEG/> ;
    owl:onProperty glbase:hasMeasurementType ;
    owl:someValuesFrom [ a owl:Class ;
            owl:oneOf ( <http://vocab.nerc.ac.uk/collection/P02/current/LVEG/> ) ] .
[] a owl:Restriction ;
    rdfs:subClassOf <http://vocab.nerc.ac.uk/collection/P02/current/BATC/> ;
    owl:onProperty glbase:hasMeasurementType ;
    owl:someValuesFrom [ a owl:Class ;
            owl:oneOf ( <http://vocab.nerc.ac.uk/collection/P02/current/BATC/> ) ] .
[] a owl:Restriction ;
    rdfs:subClassOf <http://vocab.nerc.ac.uk/collection/P02/current/GWCH/> ;
    owl:onProperty glbase:hasMeasurementType ;
    owl:someValuesFrom [ a owl:Class ;
            owl:oneOf ( <http://vocab.nerc.ac.uk/collection/P02/current/GWCH/> ) ] .
[] a owl:Restriction ;
    rdfs:subClassOf <http://vocab.nerc.ac.uk/collection/P02/current/FCST/> ;
    owl:onProperty glbase:hasMeasurementType ;
    owl:someValuesFrom [ a owl:Class ;
            owl:oneOf ( <http://vocab.nerc.ac.uk/collection/P02/current/FCST/> ) ] .
[] a owl:Restriction ;
    rdfs:subClassOf <http://vocab.nerc.ac.uk/collection/P02/current/WCPH/> ;
    owl:onProperty glbase:hasMeasurementType ;
    owl:someValuesFrom [ a owl:Class ;
            owl:oneOf ( <http://vocab.nerc.ac.uk/collection/P02/current/WCPH/> ) ] .
[] a owl:Restriction ;
    rdfs:subClassOf <http://vocab.nerc.ac.uk/collection/P02/current/PHUP/> ;
    owl:onProperty glbase:hasMeasurementType ;
    owl:someValuesFrom [ a owl:Class ;
            owl:oneOf ( <http://vocab.nerc.ac.uk/collection/P02/current/PHUP/> ) ] .
[] a owl:Restriction ;
    rdfs:subClassOf <http://vocab.nerc.ac.uk/collection/P02/current/AEYN/> ;
    owl:onProperty glbase:hasMeasurementType ;
    owl:someValuesFrom [ a owl:Class ;
            owl:oneOf ( <http://vocab.nerc.ac.uk/collection/P02/current/AEYN/> ) ] .
[] a owl:Restriction ;
    rdfs:subClassOf <http://vocab.nerc.ac.uk/collection/P02/current/SCOC/> ;
    owl:onProperty glbase:hasMeasurementType ;
    owl:someValuesFrom [ a owl:Class ;
            owl:oneOf ( <http://vocab.nerc.ac.uk/collection/P02/current/SCOC/> ) ] .
[] a owl:Restriction ;
    rdfs:subClassOf <http://vocab.nerc.ac.uk/collection/P02/current/SIGT/> ;
    owl:onProperty glbase:hasMeasurementType ;
    owl:someValuesFrom [ a owl:Class ;
            owl:oneOf ( <http://vocab.nerc.ac.uk/collection/P02/current/SIGT/> ) ] .
[] a owl:Restriction ;
    rdfs:subClassOf <http://vocab.nerc.ac.uk/collection/P02/current/LITH/> ;
    owl:onProperty glbase:hasMeasurementType ;
    owl:someValuesFrom [ a owl:Class ;
            owl:oneOf ( <http://vocab.nerc.ac.uk/collection/P02/current/LITH/> ) ] .
[] a owl:Restriction ;
    rdfs:subClassOf <http://vocab.nerc.ac.uk/collection/P02/current/RBSC/> ;
    owl:onProperty glbase:hasMeasurementType ;
    owl:someValuesFrom [ a owl:Class ;
            owl:oneOf ( <http://vocab.nerc.ac.uk/collection/P02/current/RBSC/> ) ] .
[] a owl:Restriction ;
    rdfs:subClassOf <http://vocab.nerc.ac.uk/collection/P02/current/ZZZZ/> ;
    owl:onProperty glbase:hasMeasurementType ;
    owl:someValuesFrom [ a owl:Class ;
            owl:oneOf ( <http://vocab.nerc.ac.uk/collection/P02/current/ZZZZ/> ) ] .
[] a owl:Restriction ;
    rdfs:subClassOf <http://vocab.nerc.ac.uk/collection/P02/current/ALKY/> ;
    owl:onProperty glbase:hasMeasurementType ;
    owl:someValuesFrom [ a owl:Class ;
            owl:oneOf ( <http://vocab.nerc.ac.uk/collection/P02/current/ALKY/> ) ] .
[] a owl:Restriction ;
    rdfs:subClassOf <http://vocab.nerc.ac.uk/collection/P02/current/TMES/> ;
    owl:onProperty glbase:hasMeasurementType ;
    owl:someValuesFrom [ a owl:Class ;
            owl:oneOf ( <http://vocab.nerc.ac.uk/collection/P02/current/TMES/> ) ] .
[] a owl:Restriction ;
    rdfs:subClassOf <http://vocab.nerc.ac.uk/collection/P02/current/RACC/> ;
    owl:onProperty glbase:hasMeasurementType ;
    owl:someValuesFrom [ a owl:Class ;
            owl:oneOf ( <http://vocab.nerc.ac.uk/collection/P02/current/RACC/> ) ] .
[] a owl:Restriction ;
    rdfs:subClassOf <http://vocab.nerc.ac.uk/collection/P02/current/CBSD/> ;
    owl:onProperty glbase:hasMeasurementType ;
    owl:someValuesFrom [ a owl:Class ;
            owl:oneOf ( <http://vocab.nerc.ac.uk/collection/P02/current/CBSD/> ) ] .
[] a owl:Restriction ;
    rdfs:subClassOf <http://vocab.nerc.ac.uk/collection/P02/current/SLCA/> ;
    owl:onProperty glbase:hasMeasurementType ;
    owl:someValuesFrom [ a owl:Class ;
            owl:oneOf ( <http://vocab.nerc.ac.uk/collection/P02/current/SLCA/> ) ] .
[] a owl:Restriction ;
    rdfs:subClassOf <http://vocab.nerc.ac.uk/collection/P02/current/MSFX/> ;
    owl:onProperty glbase:hasMeasurementType ;
    owl:someValuesFrom [ a owl:Class ;
            owl:oneOf ( <http://vocab.nerc.ac.uk/collection/P02/current/MSFX/> ) ] .
[] a owl:Restriction ;
    rdfs:subClassOf <http://vocab.nerc.ac.uk/collection/P02/current/PTDZ/> ;
    owl:onProperty glbase:hasMeasurementType ;
    owl:someValuesFrom [ a owl:Class ;
            owl:oneOf ( <http://vocab.nerc.ac.uk/collection/P02/current/PTDZ/> ) ] .
[] a owl:Restriction ;
    rdfs:subClassOf <http://vocab.nerc.ac.uk/collection/P02/current/TEMP/> ;
    owl:onProperty glbase:hasMeasurementType ;
    owl:someValuesFrom [ a owl:Class ;
            owl:oneOf ( <http://vocab.nerc.ac.uk/collection/P02/current/TEMP/> ) ] .
[] a owl:Restriction ;
    rdfs:subClassOf <http://vocab.nerc.ac.uk/collection/P02/current/IACT/> ;
    owl:onProperty glbase:hasMeasurementType ;
    owl:someValuesFrom [ a owl:Class ;
            owl:oneOf ( <http://vocab.nerc.ac.uk/collection/P02/current/IACT/> ) ] .
[] a owl:Restriction ;
    rdfs:subClassOf <http://vocab.nerc.ac.uk/collection/P02/current/ISAT/> ;
    owl:onProperty glbase:hasMeasurementType ;
    owl:someValuesFrom [ a owl:Class ;
            owl:oneOf ( <http://vocab.nerc.ac.uk/collection/P02/current/ISAT/> ) ] .
[] a owl:Restriction ;
    rdfs:subClassOf <http://vocab.nerc.ac.uk/collection/P02/current/LRZA/> ;
    owl:onProperty glbase:hasMeasurementType ;
    owl:someValuesFrom [ a owl:Class ;
            owl:oneOf ( <http://vocab.nerc.ac.uk/collection/P02/current/LRZA/> ) ] .
[] a owl:Restriction ;
    rdfs:subClassOf <http://vocab.nerc.ac.uk/collection/P02/current/PASR/> ;
    owl:onProperty glbase:hasMeasurementType ;
    owl:someValuesFrom [ a owl:Class ;
            owl:oneOf ( <http://vocab.nerc.ac.uk/collection/P02/current/PASR/> ) ] .
[] a owl:Restriction ;
    rdfs:subClassOf <http://vocab.nerc.ac.uk/collection/P02/current/CORG/> ;
    owl:onProperty glbase:hasMeasurementType ;
    owl:someValuesFrom [ a owl:Class ;
            owl:oneOf ( <http://vocab.nerc.ac.uk/collection/P02/current/CORG/> ) ] .
[] a owl:Restriction ;
    rdfs:subClassOf <http://vocab.nerc.ac.uk/collection/P02/current/MTSD/> ;
    owl:onProperty glbase:hasMeasurementType ;
    owl:someValuesFrom [ a owl:Class ;
            owl:oneOf ( <http://vocab.nerc.ac.uk/collection/P02/current/MTSD/> ) ] .
[] a owl:Restriction ;
    rdfs:subClassOf <http://vocab.nerc.ac.uk/collection/P02/current/KRTS/> ;
    owl:onProperty glbase:hasMeasurementType ;
    owl:someValuesFrom [ a owl:Class ;
            owl:oneOf ( <http://vocab.nerc.ac.uk/collection/P02/current/KRTS/> ) ] .
[] a owl:Restriction ;
    rdfs:subClassOf <http://vocab.nerc.ac.uk/collection/P02/current/TPHS/> ;
    owl:onProperty glbase:hasMeasurementType ;
    owl:someValuesFrom [ a owl:Class ;
            owl:oneOf ( <http://vocab.nerc.ac.uk/collection/P02/current/TPHS/> ) ] .
[] a owl:Restriction ;
    rdfs:subClassOf <http://vocab.nerc.ac.uk/collection/P02/current/CHEX/> ;
    owl:onProperty glbase:hasMeasurementType ;
    owl:someValuesFrom [ a owl:Class ;
            owl:oneOf ( <http://vocab.nerc.ac.uk/collection/P02/current/CHEX/> ) ] .
[] a owl:Restriction ;
    rdfs:subClassOf <http://vocab.nerc.ac.uk/collection/P02/current/ACNT/> ;
    owl:onProperty glbase:hasMeasurementType ;
    owl:someValuesFrom [ a owl:Class ;
            owl:oneOf ( <http://vocab.nerc.ac.uk/collection/P02/current/ACNT/> ) ] .
[] a owl:Restriction ;
    rdfs:subClassOf <http://vocab.nerc.ac.uk/collection/P02/current/MATC/> ;
    owl:onProperty glbase:hasMeasurementType ;
    owl:someValuesFrom [ a owl:Class ;
            owl:oneOf ( <http://vocab.nerc.ac.uk/collection/P02/current/MATC/> ) ] .
[] a owl:Restriction ;
    rdfs:subClassOf <http://vocab.nerc.ac.uk/collection/P02/current/DVLP/> ;
    owl:onProperty glbase:hasMeasurementType ;
    owl:someValuesFrom [ a owl:Class ;
            owl:oneOf ( <http://vocab.nerc.ac.uk/collection/P02/current/DVLP/> ) ] .
[] a owl:Restriction ;
    rdfs:subClassOf <http://vocab.nerc.ac.uk/collection/P02/current/EXCR/> ;
    owl:onProperty glbase:hasMeasurementType ;
    owl:someValuesFrom [ a owl:Class ;
            owl:oneOf ( <http://vocab.nerc.ac.uk/collection/P02/current/EXCR/> ) ] .
[] a owl:Restriction ;
    rdfs:subClassOf <http://vocab.nerc.ac.uk/collection/P02/current/ZATP/> ;
    owl:onProperty glbase:hasMeasurementType ;
    owl:someValuesFrom [ a owl:Class ;
            owl:oneOf ( <http://vocab.nerc.ac.uk/collection/P02/current/ZATP/> ) ] .
[] a owl:Restriction ;
    rdfs:subClassOf <http://vocab.nerc.ac.uk/collection/P02/current/PSAL/> ;
    owl:onProperty glbase:hasMeasurementType ;
    owl:someValuesFrom [ a owl:Class ;
            owl:oneOf ( <http://vocab.nerc.ac.uk/collection/P02/current/PSAL/> ) ] .
[] a owl:Restriction ;
    rdfs:subClassOf <http://vocab.nerc.ac.uk/collection/P02/current/SPCB/> ;
    owl:onProperty glbase:hasMeasurementType ;
    owl:someValuesFrom [ a owl:Class ;
            owl:oneOf ( <http://vocab.nerc.ac.uk/collection/P02/current/SPCB/> ) ] .
[] a owl:Restriction ;
    rdfs:subClassOf <http://vocab.nerc.ac.uk/collection/P02/current/BCPB/> ;
    owl:onProperty glbase:hasMeasurementType ;
    owl:someValuesFrom [ a owl:Class ;
            owl:oneOf ( <http://vocab.nerc.ac.uk/collection/P02/current/BCPB/> ) ] .
[] a owl:Restriction ;
    rdfs:subClassOf <http://vocab.nerc.ac.uk/collection/P02/current/TVLT/> ;
    owl:onProperty glbase:hasMeasurementType ;
    owl:someValuesFrom [ a owl:Class ;
            owl:oneOf ( <http://vocab.nerc.ac.uk/collection/P02/current/TVLT/> ) ] .
[] a owl:Restriction ;
    rdfs:subClassOf <http://vocab.nerc.ac.uk/collection/P02/current/AYMD/> ;
    owl:onProperty glbase:hasMeasurementType ;
    owl:someValuesFrom [ a owl:Class ;
            owl:oneOf ( <http://vocab.nerc.ac.uk/collection/P02/current/AYMD/> ) ] .
[] a owl:Restriction ;
    rdfs:subClassOf <http://vocab.nerc.ac.uk/collection/P02/current/OPBS/> ;
    owl:onProperty glbase:hasMeasurementType ;
    owl:someValuesFrom [ a owl:Class ;
            owl:oneOf ( <http://vocab.nerc.ac.uk/collection/P02/current/OPBS/> ) ] .
[] a owl:Restriction ;
    rdfs:subClassOf <http://vocab.nerc.ac.uk/collection/P02/current/GP012/> ;
    owl:onProperty glbase:hasMeasurementType ;
    owl:someValuesFrom [ a owl:Class ;
            owl:oneOf ( <http://vocab.nerc.ac.uk/collection/P02/current/GP012/> ) ] .
[] a owl:Restriction ;
    rdfs:subClassOf <http://vocab.nerc.ac.uk/collection/P02/current/RMIN/> ;
    owl:onProperty glbase:hasMeasurementType ;
    owl:someValuesFrom [ a owl:Class ;
            owl:oneOf ( <http://vocab.nerc.ac.uk/collection/P02/current/RMIN/> ) ] .
[] a owl:Restriction ;
    rdfs:subClassOf <http://vocab.nerc.ac.uk/collection/P02/current/ZNTN/> ;
    owl:onProperty glbase:hasMeasurementType ;
    owl:someValuesFrom [ a owl:Class ;
            owl:oneOf ( <http://vocab.nerc.ac.uk/collection/P02/current/ZNTN/> ) ] .
[] a owl:Restriction ;
    rdfs:subClassOf <http://vocab.nerc.ac.uk/collection/P02/current/ZOOB/> ;
    owl:onProperty glbase:hasMeasurementType ;
    owl:someValuesFrom [ a owl:Class ;
            owl:oneOf ( <http://vocab.nerc.ac.uk/collection/P02/current/ZOOB/> ) ] .
[] a owl:Restriction ;
    rdfs:subClassOf <http://vocab.nerc.ac.uk/collection/P02/current/OHWC/> ;
    owl:onProperty glbase:hasMeasurementType ;
    owl:someValuesFrom [ a owl:Class ;
            owl:oneOf ( <http://vocab.nerc.ac.uk/collection/P02/current/OHWC/> ) ] .
[] a owl:Restriction ;
    rdfs:subClassOf <http://vocab.nerc.ac.uk/collection/P02/current/CD10/> ;
    owl:onProperty glbase:hasMeasurementType ;
    owl:someValuesFrom [ a owl:Class ;
            owl:oneOf ( <http://vocab.nerc.ac.uk/collection/P02/current/CD10/> ) ] .
[] a owl:Restriction ;
    rdfs:subClassOf <http://vocab.nerc.ac.uk/collection/P02/current/HEXC/> ;
    owl:onProperty glbase:hasMeasurementType ;
    owl:someValuesFrom [ a owl:Class ;
            owl:oneOf ( <http://vocab.nerc.ac.uk/collection/P02/current/HEXC/> ) ] .
[] a owl:Restriction ;
    rdfs:subClassOf <http://vocab.nerc.ac.uk/collection/P02/current/ATDP/> ;
    owl:onProperty glbase:hasMeasurementType ;
    owl:someValuesFrom [ a owl:Class ;
            owl:oneOf ( <http://vocab.nerc.ac.uk/collection/P02/current/ATDP/> ) ] .
[] a owl:Restriction ;
    rdfs:subClassOf <http://vocab.nerc.ac.uk/collection/P02/current/NTPW/> ;
    owl:onProperty glbase:hasMeasurementType ;
    owl:someValuesFrom [ a owl:Class ;
            owl:oneOf ( <http://vocab.nerc.ac.uk/collection/P02/current/NTPW/> ) ] .
[] a owl:Restriction ;
    rdfs:subClassOf <http://vocab.nerc.ac.uk/collection/P02/current/ICEM/> ;
    owl:onProperty glbase:hasMeasurementType ;
    owl:someValuesFrom [ a owl:Class ;
            owl:oneOf ( <http://vocab.nerc.ac.uk/collection/P02/current/ICEM/> ) ] .
[] a owl:Restriction ;
    rdfs:subClassOf <http://vocab.nerc.ac.uk/collection/P02/current/NTSP/> ;
    owl:onProperty glbase:hasMeasurementType ;
    owl:someValuesFrom [ a owl:Class ;
            owl:oneOf ( <http://vocab.nerc.ac.uk/collection/P02/current/NTSP/> ) ] .
[] a owl:Restriction ;
    rdfs:subClassOf <http://vocab.nerc.ac.uk/collection/P02/current/OPFX/> ;
    owl:onProperty glbase:hasMeasurementType ;
    owl:someValuesFrom [ a owl:Class ;
            owl:oneOf ( <http://vocab.nerc.ac.uk/collection/P02/current/OPFX/> ) ] .
[] a owl:Restriction ;
    rdfs:subClassOf <http://vocab.nerc.ac.uk/collection/P02/current/AORG/> ;
    owl:onProperty glbase:hasMeasurementType ;
    owl:someValuesFrom [ a owl:Class ;
            owl:oneOf ( <http://vocab.nerc.ac.uk/collection/P02/current/AORG/> ) ] .
[] a owl:Restriction ;
    rdfs:subClassOf <http://vocab.nerc.ac.uk/collection/P02/current/MDSV/> ;
    owl:onProperty glbase:hasMeasurementType ;
    owl:someValuesFrom [ a owl:Class ;
            owl:oneOf ( <http://vocab.nerc.ac.uk/collection/P02/current/MDSV/> ) ] .
[] a owl:Restriction ;
    rdfs:subClassOf <http://vocab.nerc.ac.uk/collection/P02/current/CBFX/> ;
    owl:onProperty glbase:hasMeasurementType ;
    owl:someValuesFrom [ a owl:Class ;
            owl:oneOf ( <http://vocab.nerc.ac.uk/collection/P02/current/CBFX/> ) ] .
[] a owl:Restriction ;
    rdfs:subClassOf <http://vocab.nerc.ac.uk/collection/P02/current/MFWW/> ;
    owl:onProperty glbase:hasMeasurementType ;
    owl:someValuesFrom [ a owl:Class ;
            owl:oneOf ( <http://vocab.nerc.ac.uk/collection/P02/current/MFWW/> ) ] .
[] a owl:Restriction ;
    rdfs:subClassOf <http://vocab.nerc.ac.uk/collection/P02/current/MSIC/> ;
    owl:onProperty glbase:hasMeasurementType ;
    owl:someValuesFrom [ a owl:Class ;
            owl:oneOf ( <http://vocab.nerc.ac.uk/collection/P02/current/MSIC/> ) ] .
[] a owl:Restriction ;
    rdfs:subClassOf <http://vocab.nerc.ac.uk/collection/P02/current/CNTX/> ;
    owl:onProperty glbase:hasMeasurementType ;
    owl:someValuesFrom [ a owl:Class ;
            owl:oneOf ( <http://vocab.nerc.ac.uk/collection/P02/current/CNTX/> ) ] .
[] a owl:Restriction ;
    rdfs:subClassOf <http://vocab.nerc.ac.uk/collection/P02/current/COCC/> ;
    owl:onProperty glbase:hasMeasurementType ;
    owl:someValuesFrom [ a owl:Class ;
            owl:oneOf ( <http://vocab.nerc.ac.uk/collection/P02/current/COCC/> ) ] .
[] a owl:Restriction ;
    rdfs:subClassOf <http://vocab.nerc.ac.uk/collection/P02/current/OCAA/> ;
    owl:onProperty glbase:hasMeasurementType ;
    owl:someValuesFrom [ a owl:Class ;
            owl:oneOf ( <http://vocab.nerc.ac.uk/collection/P02/current/OCAA/> ) ] .
[] a owl:Restriction ;
    rdfs:subClassOf <http://vocab.nerc.ac.uk/collection/P02/current/MMST/> ;
    owl:onProperty glbase:hasMeasurementType ;
    owl:someValuesFrom [ a owl:Class ;
            owl:oneOf ( <http://vocab.nerc.ac.uk/collection/P02/current/MMST/> ) ] .
[] a owl:Restriction ;
    rdfs:subClassOf <http://vocab.nerc.ac.uk/collection/P02/current/PXSD/> ;
    owl:onProperty glbase:hasMeasurementType ;
    owl:someValuesFrom [ a owl:Class ;
            owl:oneOf ( <http://vocab.nerc.ac.uk/collection/P02/current/PXSD/> ) ] .
[] a owl:Restriction ;
    rdfs:subClassOf <http://vocab.nerc.ac.uk/collection/P02/current/V999/> ;
    owl:onProperty glbase:hasMeasurementType ;
    owl:someValuesFrom [ a owl:Class ;
            owl:oneOf ( <http://vocab.nerc.ac.uk/collection/P02/current/V999/> ) ] .
[] a owl:Restriction ;
    rdfs:subClassOf <http://vocab.nerc.ac.uk/collection/P02/current/SALK/> ;
    owl:onProperty glbase:hasMeasurementType ;
    owl:someValuesFrom [ a owl:Class ;
            owl:oneOf ( <http://vocab.nerc.ac.uk/collection/P02/current/SALK/> ) ] .
[] a owl:Restriction ;
    rdfs:subClassOf <http://vocab.nerc.ac.uk/collection/P02/current/A01X/> ;
    owl:onProperty glbase:hasMeasurementType ;
    owl:someValuesFrom [ a owl:Class ;
            owl:oneOf ( <http://vocab.nerc.ac.uk/collection/P02/current/A01X/> ) ] .
[] a owl:Restriction ;
    rdfs:subClassOf <http://vocab.nerc.ac.uk/collection/P02/current/CNDC/> ;
    owl:onProperty glbase:hasMeasurementType ;
    owl:someValuesFrom [ a owl:Class ;
            owl:oneOf ( <http://vocab.nerc.ac.uk/collection/P02/current/CNDC/> ) ] .
[] a owl:Restriction ;
    rdfs:subClassOf <http://vocab.nerc.ac.uk/collection/P02/current/CSDE/> ;
    owl:onProperty glbase:hasMeasurementType ;
    owl:someValuesFrom [ a owl:Class ;
            owl:oneOf ( <http://vocab.nerc.ac.uk/collection/P02/current/CSDE/> ) ] .
[] a owl:Restriction ;
    rdfs:subClassOf <http://vocab.nerc.ac.uk/collection/P02/current/CLCN/> ;
    owl:onProperty glbase:hasMeasurementType ;
    owl:someValuesFrom [ a owl:Class ;
            owl:oneOf ( <http://vocab.nerc.ac.uk/collection/P02/current/CLCN/> ) ] .
[] a owl:Restriction ;
    rdfs:subClassOf <http://vocab.nerc.ac.uk/collection/P02/current/BEST/> ;
    owl:onProperty glbase:hasMeasurementType ;
    owl:someValuesFrom [ a owl:Class ;
            owl:oneOf ( <http://vocab.nerc.ac.uk/collection/P02/current/BEST/> ) ] .
[] a owl:Restriction ;
    rdfs:subClassOf <http://vocab.nerc.ac.uk/collection/P02/current/CPSD/> ;
    owl:onProperty glbase:hasMeasurementType ;
    owl:someValuesFrom [ a owl:Class ;
            owl:oneOf ( <http://vocab.nerc.ac.uk/collection/P02/current/CPSD/> ) ] .
[] a owl:Restriction ;
    rdfs:subClassOf <http://vocab.nerc.ac.uk/collection/P02/current/FEFF/> ;
    owl:onProperty glbase:hasMeasurementType ;
    owl:someValuesFrom [ a owl:Class ;
            owl:oneOf ( <http://vocab.nerc.ac.uk/collection/P02/current/FEFF/> ) ] .
[] a owl:Restriction ;
    rdfs:subClassOf <http://vocab.nerc.ac.uk/collection/P02/current/CRYS/> ;
    owl:onProperty glbase:hasMeasurementType ;
    owl:someValuesFrom [ a owl:Class ;
            owl:oneOf ( <http://vocab.nerc.ac.uk/collection/P02/current/CRYS/> ) ] .
[] a owl:Restriction ;
    rdfs:subClassOf <http://vocab.nerc.ac.uk/collection/P02/current/MTWT/> ;
    owl:onProperty glbase:hasMeasurementType ;
    owl:someValuesFrom [ a owl:Class ;
            owl:oneOf ( <http://vocab.nerc.ac.uk/collection/P02/current/MTWT/> ) ] .
[] a owl:Restriction ;
    rdfs:subClassOf <http://vocab.nerc.ac.uk/collection/P02/current/FVLT/> ;
    owl:onProperty glbase:hasMeasurementType ;
    owl:someValuesFrom [ a owl:Class ;
            owl:oneOf ( <http://vocab.nerc.ac.uk/collection/P02/current/FVLT/> ) ] .
[] a owl:Restriction ;
    rdfs:subClassOf <http://vocab.nerc.ac.uk/collection/P02/current/MZBN/> ;
    owl:onProperty glbase:hasMeasurementType ;
    owl:someValuesFrom [ a owl:Class ;
            owl:oneOf ( <http://vocab.nerc.ac.uk/collection/P02/current/MZBN/> ) ] .
[] a owl:Restriction ;
    rdfs:subClassOf <http://vocab.nerc.ac.uk/collection/P02/current/SEBH/> ;
    owl:onProperty glbase:hasMeasurementType ;
    owl:someValuesFrom [ a owl:Class ;
            owl:oneOf ( <http://vocab.nerc.ac.uk/collection/P02/current/SEBH/> ) ] .
[] a owl:Restriction ;
    rdfs:subClassOf <http://vocab.nerc.ac.uk/collection/P02/current/ISIC/> ;
    owl:onProperty glbase:hasMeasurementType ;
    owl:someValuesFrom [ a owl:Class ;
            owl:oneOf ( <http://vocab.nerc.ac.uk/collection/P02/current/ISIC/> ) ] .
[] a owl:Restriction ;
    rdfs:subClassOf <http://vocab.nerc.ac.uk/collection/P02/current/ACFL/> ;
    owl:onProperty glbase:hasMeasurementType ;
    owl:someValuesFrom [ a owl:Class ;
            owl:oneOf ( <http://vocab.nerc.ac.uk/collection/P02/current/ACFL/> ) ] .
[] a owl:Restriction ;
    rdfs:subClassOf <http://vocab.nerc.ac.uk/collection/P02/current/NOYS/> ;
    owl:onProperty glbase:hasMeasurementType ;
    owl:someValuesFrom [ a owl:Class ;
            owl:oneOf ( <http://vocab.nerc.ac.uk/collection/P02/current/NOYS/> ) ] .
[] a owl:Restriction ;
    rdfs:subClassOf <http://vocab.nerc.ac.uk/collection/P02/current/SSTR/> ;
    owl:onProperty glbase:hasMeasurementType ;
    owl:someValuesFrom [ a owl:Class ;
            owl:oneOf ( <http://vocab.nerc.ac.uk/collection/P02/current/SSTR/> ) ] .
[] a owl:Restriction ;
    rdfs:subClassOf <http://vocab.nerc.ac.uk/collection/P02/current/PHYC/> ;
    owl:onProperty glbase:hasMeasurementType ;
    owl:someValuesFrom [ a owl:Class ;
            owl:oneOf ( <http://vocab.nerc.ac.uk/collection/P02/current/PHYC/> ) ] .
[] a owl:Restriction ;
    rdfs:subClassOf <http://vocab.nerc.ac.uk/collection/P02/current/GP050/> ;
    owl:onProperty glbase:hasMeasurementType ;
    owl:someValuesFrom [ a owl:Class ;
            owl:oneOf ( <http://vocab.nerc.ac.uk/collection/P02/current/GP050/> ) ] .
[] a owl:Restriction ;
    rdfs:subClassOf <http://vocab.nerc.ac.uk/collection/P02/current/TOCH/> ;
    owl:onProperty glbase:hasMeasurementType ;
    owl:someValuesFrom [ a owl:Class ;
            owl:oneOf ( <http://vocab.nerc.ac.uk/collection/P02/current/TOCH/> ) ] .
[] a owl:Restriction ;
    rdfs:subClassOf <http://vocab.nerc.ac.uk/collection/P02/current/PHOS/> ;
    owl:onProperty glbase:hasMeasurementType ;
    owl:someValuesFrom [ a owl:Class ;
            owl:oneOf ( <http://vocab.nerc.ac.uk/collection/P02/current/PHOS/> ) ] .
[] a owl:Restriction ;
    rdfs:subClassOf <http://vocab.nerc.ac.uk/collection/P02/current/WRAD/> ;
    owl:onProperty glbase:hasMeasurementType ;
    owl:someValuesFrom [ a owl:Class ;
            owl:oneOf ( <http://vocab.nerc.ac.uk/collection/P02/current/WRAD/> ) ] .
[] a owl:Restriction ;
    rdfs:subClassOf <http://vocab.nerc.ac.uk/collection/P02/current/GRAV/> ;
    owl:onProperty glbase:hasMeasurementType ;
    owl:someValuesFrom [ a owl:Class ;
            owl:oneOf ( <http://vocab.nerc.ac.uk/collection/P02/current/GRAV/> ) ] .
[] a owl:Restriction ;
    rdfs:subClassOf <http://vocab.nerc.ac.uk/collection/P02/current/BNTX/> ;
    owl:onProperty glbase:hasMeasurementType ;
    owl:someValuesFrom [ a owl:Class ;
            owl:oneOf ( <http://vocab.nerc.ac.uk/collection/P02/current/BNTX/> ) ] .
[] a owl:Restriction ;
    rdfs:subClassOf <http://vocab.nerc.ac.uk/collection/P02/current/CAPH/> ;
    owl:onProperty glbase:hasMeasurementType ;
    owl:someValuesFrom [ a owl:Class ;
            owl:oneOf ( <http://vocab.nerc.ac.uk/collection/P02/current/CAPH/> ) ] .
[] a owl:Restriction ;
    rdfs:subClassOf <http://vocab.nerc.ac.uk/collection/P02/current/GP087/> ;
    owl:onProperty glbase:hasMeasurementType ;
    owl:someValuesFrom [ a owl:Class ;
            owl:oneOf ( <http://vocab.nerc.ac.uk/collection/P02/current/GP087/> ) ] .
[] a owl:Restriction ;
    rdfs:subClassOf <http://vocab.nerc.ac.uk/collection/P02/current/EPSI/> ;
    owl:onProperty glbase:hasMeasurementType ;
    owl:someValuesFrom [ a owl:Class ;
            owl:oneOf ( <http://vocab.nerc.ac.uk/collection/P02/current/EPSI/> ) ] .
[] a owl:Restriction ;
    rdfs:subClassOf <http://vocab.nerc.ac.uk/collection/P02/current/FCRT/> ;
    owl:onProperty glbase:hasMeasurementType ;
    owl:someValuesFrom [ a owl:Class ;
            owl:oneOf ( <http://vocab.nerc.ac.uk/collection/P02/current/FCRT/> ) ] .
[] a owl:Restriction ;
    rdfs:subClassOf <http://vocab.nerc.ac.uk/collection/P02/current/OMWC/> ;
    owl:onProperty glbase:hasMeasurementType ;
    owl:someValuesFrom [ a owl:Class ;
            owl:oneOf ( <http://vocab.nerc.ac.uk/collection/P02/current/OMWC/> ) ] .
[] a owl:Restriction ;
    rdfs:subClassOf <http://vocab.nerc.ac.uk/collection/P02/current/MATX/> ;
    owl:onProperty glbase:hasMeasurementType ;
    owl:someValuesFrom [ a owl:Class ;
            owl:oneOf ( <http://vocab.nerc.ac.uk/collection/P02/current/MATX/> ) ] .
[] a owl:Restriction ;
    rdfs:subClassOf <http://vocab.nerc.ac.uk/collection/P02/current/GP018/> ;
    owl:onProperty glbase:hasMeasurementType ;
    owl:someValuesFrom [ a owl:Class ;
            owl:oneOf ( <http://vocab.nerc.ac.uk/collection/P02/current/GP018/> ) ] .
[] a owl:Restriction ;
    rdfs:subClassOf <http://vocab.nerc.ac.uk/collection/P02/current/BDRV/> ;
    owl:onProperty glbase:hasMeasurementType ;
    owl:someValuesFrom [ a owl:Class ;
            owl:oneOf ( <http://vocab.nerc.ac.uk/collection/P02/current/BDRV/> ) ] .
[] a owl:Restriction ;
    rdfs:subClassOf <http://vocab.nerc.ac.uk/collection/P02/current/PPWC/> ;
    owl:onProperty glbase:hasMeasurementType ;
    owl:someValuesFrom [ a owl:Class ;
            owl:oneOf ( <http://vocab.nerc.ac.uk/collection/P02/current/PPWC/> ) ] .
[] a owl:Restriction ;
    rdfs:subClassOf <http://vocab.nerc.ac.uk/collection/P02/current/TADN/> ;
    owl:onProperty glbase:hasMeasurementType ;
    owl:someValuesFrom [ a owl:Class ;
            owl:oneOf ( <http://vocab.nerc.ac.uk/collection/P02/current/TADN/> ) ] .
[] a owl:Restriction ;
    rdfs:subClassOf <http://vocab.nerc.ac.uk/collection/P02/current/MFAZ/> ;
    owl:onProperty glbase:hasMeasurementType ;
    owl:someValuesFrom [ a owl:Class ;
            owl:oneOf ( <http://vocab.nerc.ac.uk/collection/P02/current/MFAZ/> ) ] .
[] a owl:Restriction ;
    rdfs:subClassOf <http://vocab.nerc.ac.uk/collection/P02/current/ROGS/> ;
    owl:onProperty glbase:hasMeasurementType ;
    owl:someValuesFrom [ a owl:Class ;
            owl:oneOf ( <http://vocab.nerc.ac.uk/collection/P02/current/ROGS/> ) ] .
[] a owl:Restriction ;
    rdfs:subClassOf <http://vocab.nerc.ac.uk/collection/P02/current/HLIC/> ;
    owl:onProperty glbase:hasMeasurementType ;
    owl:someValuesFrom [ a owl:Class ;
            owl:oneOf ( <http://vocab.nerc.ac.uk/collection/P02/current/HLIC/> ) ] .
[] a owl:Restriction ;
    rdfs:subClassOf <http://vocab.nerc.ac.uk/collection/P02/current/SDNA/> ;
    owl:onProperty glbase:hasMeasurementType ;
    owl:someValuesFrom [ a owl:Class ;
            owl:oneOf ( <http://vocab.nerc.ac.uk/collection/P02/current/SDNA/> ) ] .
[] a owl:Restriction ;
    rdfs:subClassOf <http://vocab.nerc.ac.uk/collection/P02/current/TDPX/> ;
    owl:onProperty glbase:hasMeasurementType ;
    owl:someValuesFrom [ a owl:Class ;
            owl:oneOf ( <http://vocab.nerc.ac.uk/collection/P02/current/TDPX/> ) ] .
[] a owl:Restriction ;
    rdfs:subClassOf <http://vocab.nerc.ac.uk/collection/P02/current/ZCTN/> ;
    owl:onProperty glbase:hasMeasurementType ;
    owl:someValuesFrom [ a owl:Class ;
            owl:oneOf ( <http://vocab.nerc.ac.uk/collection/P02/current/ZCTN/> ) ] .
[] a owl:Restriction ;
    rdfs:subClassOf <http://vocab.nerc.ac.uk/collection/P02/current/ZBTX/> ;
    owl:onProperty glbase:hasMeasurementType ;
    owl:someValuesFrom [ a owl:Class ;
            owl:oneOf ( <http://vocab.nerc.ac.uk/collection/P02/current/ZBTX/> ) ] .
[] a owl:Restriction ;
    rdfs:subClassOf <http://vocab.nerc.ac.uk/collection/P02/current/OSIC/> ;
    owl:onProperty glbase:hasMeasurementType ;
    owl:someValuesFrom [ a owl:Class ;
            owl:oneOf ( <http://vocab.nerc.ac.uk/collection/P02/current/OSIC/> ) ] .
[] a owl:Restriction ;
    rdfs:subClassOf <http://vocab.nerc.ac.uk/collection/P02/current/HFLX/> ;
    owl:onProperty glbase:hasMeasurementType ;
    owl:someValuesFrom [ a owl:Class ;
            owl:oneOf ( <http://vocab.nerc.ac.uk/collection/P02/current/HFLX/> ) ] .
[] a owl:Restriction ;
    rdfs:subClassOf <http://vocab.nerc.ac.uk/collection/P02/current/PPCB/> ;
    owl:onProperty glbase:hasMeasurementType ;
    owl:someValuesFrom [ a owl:Class ;
            owl:oneOf ( <http://vocab.nerc.ac.uk/collection/P02/current/PPCB/> ) ] .
[] a owl:Restriction ;
    rdfs:subClassOf <http://vocab.nerc.ac.uk/collection/P02/current/ZFIT/> ;
    owl:onProperty glbase:hasMeasurementType ;
    owl:someValuesFrom [ a owl:Class ;
            owl:oneOf ( <http://vocab.nerc.ac.uk/collection/P02/current/ZFIT/> ) ] .
[] a owl:Restriction ;
    rdfs:subClassOf <http://vocab.nerc.ac.uk/collection/P02/current/AMUP/> ;
    owl:onProperty glbase:hasMeasurementType ;
    owl:someValuesFrom [ a owl:Class ;
            owl:oneOf ( <http://vocab.nerc.ac.uk/collection/P02/current/AMUP/> ) ] .
[] a owl:Restriction ;
    rdfs:subClassOf <http://vocab.nerc.ac.uk/collection/P02/current/GP088/> ;
    owl:onProperty glbase:hasMeasurementType ;
    owl:someValuesFrom [ a owl:Class ;
            owl:oneOf ( <http://vocab.nerc.ac.uk/collection/P02/current/GP088/> ) ] .
[] a owl:Restriction ;
    rdfs:subClassOf <http://vocab.nerc.ac.uk/collection/P02/current/PXSP/> ;
    owl:onProperty glbase:hasMeasurementType ;
    owl:someValuesFrom [ a owl:Class ;
            owl:oneOf ( <http://vocab.nerc.ac.uk/collection/P02/current/PXSP/> ) ] .
[] a owl:Restriction ;
    rdfs:subClassOf <http://vocab.nerc.ac.uk/collection/P02/current/ZCTC/> ;
    owl:onProperty glbase:hasMeasurementType ;
    owl:someValuesFrom [ a owl:Class ;
            owl:oneOf ( <http://vocab.nerc.ac.uk/collection/P02/current/ZCTC/> ) ] .
[] a owl:Restriction ;
    rdfs:subClassOf <http://vocab.nerc.ac.uk/collection/P02/current/ACO2/> ;
    owl:onProperty glbase:hasMeasurementType ;
    owl:someValuesFrom [ a owl:Class ;
            owl:oneOf ( <http://vocab.nerc.ac.uk/collection/P02/current/ACO2/> ) ] .
[] a owl:Restriction ;
    rdfs:subClassOf <http://vocab.nerc.ac.uk/collection/P02/current/NTRI/> ;
    owl:onProperty glbase:hasMeasurementType ;
    owl:someValuesFrom [ a owl:Class ;
            owl:oneOf ( <http://vocab.nerc.ac.uk/collection/P02/current/NTRI/> ) ] .
[] a owl:Restriction ;
    rdfs:subClassOf <http://vocab.nerc.ac.uk/collection/P02/current/PHSD/> ;
    owl:onProperty glbase:hasMeasurementType ;
    owl:someValuesFrom [ a owl:Class ;
            owl:oneOf ( <http://vocab.nerc.ac.uk/collection/P02/current/PHSD/> ) ] .
[] a owl:Restriction ;
    rdfs:subClassOf <http://vocab.nerc.ac.uk/collection/P02/current/CLTY/> ;
    owl:onProperty glbase:hasMeasurementType ;
    owl:someValuesFrom [ a owl:Class ;
            owl:oneOf ( <http://vocab.nerc.ac.uk/collection/P02/current/CLTY/> ) ] .
[] a owl:Restriction ;
    rdfs:subClassOf <http://vocab.nerc.ac.uk/collection/P02/current/GP048/> ;
    owl:onProperty glbase:hasMeasurementType ;
    owl:someValuesFrom [ a owl:Class ;
            owl:oneOf ( <http://vocab.nerc.ac.uk/collection/P02/current/GP048/> ) ] .
[] a owl:Restriction ;
    rdfs:subClassOf <http://vocab.nerc.ac.uk/collection/P02/current/ZV00/> ;
    owl:onProperty glbase:hasMeasurementType ;
    owl:someValuesFrom [ a owl:Class ;
            owl:oneOf ( <http://vocab.nerc.ac.uk/collection/P02/current/ZV00/> ) ] .
[] a owl:Restriction ;
    rdfs:subClassOf <http://vocab.nerc.ac.uk/collection/P02/current/MDBO/> ;
    owl:onProperty glbase:hasMeasurementType ;
    owl:someValuesFrom [ a owl:Class ;
            owl:oneOf ( <http://vocab.nerc.ac.uk/collection/P02/current/MDBO/> ) ] .
[] a owl:Restriction ;
    rdfs:subClassOf <http://vocab.nerc.ac.uk/collection/P02/current/SECC/> ;
    owl:onProperty glbase:hasMeasurementType ;
    owl:someValuesFrom [ a owl:Class ;
            owl:oneOf ( <http://vocab.nerc.ac.uk/collection/P02/current/SECC/> ) ] .
[] a owl:Restriction ;
    rdfs:subClassOf <http://vocab.nerc.ac.uk/collection/P02/current/TSED/> ;
    owl:onProperty glbase:hasMeasurementType ;
    owl:someValuesFrom [ a owl:Class ;
            owl:oneOf ( <http://vocab.nerc.ac.uk/collection/P02/current/TSED/> ) ] .
[] a owl:Restriction ;
    rdfs:subClassOf <http://vocab.nerc.ac.uk/collection/P02/current/GP079/> ;
    owl:onProperty glbase:hasMeasurementType ;
    owl:someValuesFrom [ a owl:Class ;
            owl:oneOf ( <http://vocab.nerc.ac.uk/collection/P02/current/GP079/> ) ] .
[] a owl:Restriction ;
    rdfs:subClassOf <http://vocab.nerc.ac.uk/collection/P02/current/GREF/> ;
    owl:onProperty glbase:hasMeasurementType ;
    owl:someValuesFrom [ a owl:Class ;
            owl:oneOf ( <http://vocab.nerc.ac.uk/collection/P02/current/GREF/> ) ] .
[] a owl:Restriction ;
    rdfs:subClassOf <http://vocab.nerc.ac.uk/collection/P02/current/CING/> ;
    owl:onProperty glbase:hasMeasurementType ;
    owl:someValuesFrom [ a owl:Class ;
            owl:oneOf ( <http://vocab.nerc.ac.uk/collection/P02/current/CING/> ) ] .
[] a owl:Restriction ;
    rdfs:subClassOf <http://vocab.nerc.ac.uk/collection/P02/current/CEMO/> ;
    owl:onProperty glbase:hasMeasurementType ;
    owl:someValuesFrom [ a owl:Class ;
            owl:oneOf ( <http://vocab.nerc.ac.uk/collection/P02/current/CEMO/> ) ] .
[] a owl:Restriction ;
    rdfs:subClassOf <http://vocab.nerc.ac.uk/collection/P02/current/MLFX/> ;
    owl:onProperty glbase:hasMeasurementType ;
    owl:someValuesFrom [ a owl:Class ;
            owl:oneOf ( <http://vocab.nerc.ac.uk/collection/P02/current/MLFX/> ) ] .
[] a owl:Restriction ;
    rdfs:subClassOf <http://vocab.nerc.ac.uk/collection/P02/current/PHBI/> ;
    owl:onProperty glbase:hasMeasurementType ;
    owl:someValuesFrom [ a owl:Class ;
            owl:oneOf ( <http://vocab.nerc.ac.uk/collection/P02/current/PHBI/> ) ] .
[] a owl:Restriction ;
    rdfs:subClassOf <http://vocab.nerc.ac.uk/collection/P02/current/LWET/> ;
    owl:onProperty glbase:hasMeasurementType ;
    owl:someValuesFrom [ a owl:Class ;
            owl:oneOf ( <http://vocab.nerc.ac.uk/collection/P02/current/LWET/> ) ] .
[] a owl:Restriction ;
    rdfs:subClassOf <http://vocab.nerc.ac.uk/collection/P02/current/SACT/> ;
    owl:onProperty glbase:hasMeasurementType ;
    owl:someValuesFrom [ a owl:Class ;
            owl:oneOf ( <http://vocab.nerc.ac.uk/collection/P02/current/SACT/> ) ] .
[] a owl:Restriction ;
    rdfs:subClassOf <http://vocab.nerc.ac.uk/collection/P02/current/FBAF/> ;
    owl:onProperty glbase:hasMeasurementType ;
    owl:someValuesFrom [ a owl:Class ;
            owl:oneOf ( <http://vocab.nerc.ac.uk/collection/P02/current/FBAF/> ) ] .
[] a owl:Restriction ;
    rdfs:subClassOf <http://vocab.nerc.ac.uk/collection/P02/current/QDMD/> ;
    owl:onProperty glbase:hasMeasurementType ;
    owl:someValuesFrom [ a owl:Class ;
            owl:oneOf ( <http://vocab.nerc.ac.uk/collection/P02/current/QDMD/> ) ] .
[] a owl:Restriction ;
    rdfs:subClassOf <http://vocab.nerc.ac.uk/collection/P02/current/WQBI/> ;
    owl:onProperty glbase:hasMeasurementType ;
    owl:someValuesFrom [ a owl:Class ;
            owl:oneOf ( <http://vocab.nerc.ac.uk/collection/P02/current/WQBI/> ) ] .
[] a owl:Restriction ;
    rdfs:subClassOf <http://vocab.nerc.ac.uk/collection/P02/current/GP005/> ;
    owl:onProperty glbase:hasMeasurementType ;
    owl:someValuesFrom [ a owl:Class ;
            owl:oneOf ( <http://vocab.nerc.ac.uk/collection/P02/current/GP005/> ) ] .
[] a owl:Restriction ;
    rdfs:subClassOf <http://vocab.nerc.ac.uk/collection/P02/current/CA11/> ;
    owl:onProperty glbase:hasMeasurementType ;
    owl:someValuesFrom [ a owl:Class ;
            owl:oneOf ( <http://vocab.nerc.ac.uk/collection/P02/current/CA11/> ) ] .
[] a owl:Restriction ;
    rdfs:subClassOf <http://vocab.nerc.ac.uk/collection/P02/current/ADUN/> ;
    owl:onProperty glbase:hasMeasurementType ;
    owl:someValuesFrom [ a owl:Class ;
            owl:oneOf ( <http://vocab.nerc.ac.uk/collection/P02/current/ADUN/> ) ] .
[] a owl:Restriction ;
    rdfs:subClassOf <http://vocab.nerc.ac.uk/collection/P02/current/WCOC/> ;
    owl:onProperty glbase:hasMeasurementType ;
    owl:someValuesFrom [ a owl:Class ;
            owl:oneOf ( <http://vocab.nerc.ac.uk/collection/P02/current/WCOC/> ) ] .
[] a owl:Restriction ;
    rdfs:subClassOf <http://vocab.nerc.ac.uk/collection/P02/current/CETA/> ;
    owl:onProperty glbase:hasMeasurementType ;
    owl:someValuesFrom [ a owl:Class ;
            owl:oneOf ( <http://vocab.nerc.ac.uk/collection/P02/current/CETA/> ) ] .
[] a owl:Restriction ;
    rdfs:subClassOf <http://vocab.nerc.ac.uk/collection/P02/current/OPCN/> ;
    owl:onProperty glbase:hasMeasurementType ;
    owl:someValuesFrom [ a owl:Class ;
            owl:oneOf ( <http://vocab.nerc.ac.uk/collection/P02/current/OPCN/> ) ] .
[] a owl:Restriction ;
    rdfs:subClassOf <http://vocab.nerc.ac.uk/collection/P02/current/MFAB/> ;
    owl:onProperty glbase:hasMeasurementType ;
    owl:someValuesFrom [ a owl:Class ;
            owl:oneOf ( <http://vocab.nerc.ac.uk/collection/P02/current/MFAB/> ) ] .
[] a owl:Restriction ;
    rdfs:subClassOf <http://vocab.nerc.ac.uk/collection/P02/current/ACSR/> ;
    owl:onProperty glbase:hasMeasurementType ;
    owl:someValuesFrom [ a owl:Class ;
            owl:oneOf ( <http://vocab.nerc.ac.uk/collection/P02/current/ACSR/> ) ] .
[] a owl:Restriction ;
    rdfs:subClassOf <http://vocab.nerc.ac.uk/collection/P02/current/HAAC/> ;
    owl:onProperty glbase:hasMeasurementType ;
    owl:someValuesFrom [ a owl:Class ;
            owl:oneOf ( <http://vocab.nerc.ac.uk/collection/P02/current/HAAC/> ) ] .
[] a owl:Restriction ;
    rdfs:subClassOf <http://vocab.nerc.ac.uk/collection/P02/current/EXUV/> ;
    owl:onProperty glbase:hasMeasurementType ;
    owl:someValuesFrom [ a owl:Class ;
            owl:oneOf ( <http://vocab.nerc.ac.uk/collection/P02/current/EXUV/> ) ] .
[] a owl:Restriction ;
    rdfs:subClassOf <http://vocab.nerc.ac.uk/collection/P02/current/SEMP/> ;
    owl:onProperty glbase:hasMeasurementType ;
    owl:someValuesFrom [ a owl:Class ;
            owl:oneOf ( <http://vocab.nerc.ac.uk/collection/P02/current/SEMP/> ) ] .
[] a owl:Restriction ;
    rdfs:subClassOf <http://vocab.nerc.ac.uk/collection/P02/current/ZNTX/> ;
    owl:onProperty glbase:hasMeasurementType ;
    owl:someValuesFrom [ a owl:Class ;
            owl:oneOf ( <http://vocab.nerc.ac.uk/collection/P02/current/ZNTX/> ) ] .
[] a owl:Restriction ;
    rdfs:subClassOf <http://vocab.nerc.ac.uk/collection/P02/current/IRSP/> ;
    owl:onProperty glbase:hasMeasurementType ;
    owl:someValuesFrom [ a owl:Class ;
            owl:oneOf ( <http://vocab.nerc.ac.uk/collection/P02/current/IRSP/> ) ] .
[] a owl:Restriction ;
    rdfs:subClassOf <http://vocab.nerc.ac.uk/collection/P02/current/FOCA/> ;
    owl:onProperty glbase:hasMeasurementType ;
    owl:someValuesFrom [ a owl:Class ;
            owl:oneOf ( <http://vocab.nerc.ac.uk/collection/P02/current/FOCA/> ) ] .
[] a owl:Restriction ;
    rdfs:subClassOf <http://vocab.nerc.ac.uk/collection/P02/current/IWAB/> ;
    owl:onProperty glbase:hasMeasurementType ;
    owl:someValuesFrom [ a owl:Class ;
            owl:oneOf ( <http://vocab.nerc.ac.uk/collection/P02/current/IWAB/> ) ] .
[] a owl:Restriction ;
    rdfs:subClassOf <http://vocab.nerc.ac.uk/collection/P02/current/FIBM/> ;
    owl:onProperty glbase:hasMeasurementType ;
    owl:someValuesFrom [ a owl:Class ;
            owl:oneOf ( <http://vocab.nerc.ac.uk/collection/P02/current/FIBM/> ) ] .
[] a owl:Restriction ;
    rdfs:subClassOf <http://vocab.nerc.ac.uk/collection/P02/current/IATC/> ;
    owl:onProperty glbase:hasMeasurementType ;
    owl:someValuesFrom [ a owl:Class ;
            owl:oneOf ( <http://vocab.nerc.ac.uk/collection/P02/current/IATC/> ) ] .
[] a owl:Restriction ;
    rdfs:subClassOf <http://vocab.nerc.ac.uk/collection/P02/current/DENS/> ;
    owl:onProperty glbase:hasMeasurementType ;
    owl:someValuesFrom [ a owl:Class ;
            owl:oneOf ( <http://vocab.nerc.ac.uk/collection/P02/current/DENS/> ) ] .
[] a owl:Restriction ;
    rdfs:subClassOf <http://vocab.nerc.ac.uk/collection/P02/current/TFAA/> ;
    owl:onProperty glbase:hasMeasurementType ;
    owl:someValuesFrom [ a owl:Class ;
            owl:oneOf ( <http://vocab.nerc.ac.uk/collection/P02/current/TFAA/> ) ] .
[] a owl:Restriction ;
    rdfs:subClassOf <http://vocab.nerc.ac.uk/collection/P02/current/DMST/> ;
    owl:onProperty glbase:hasMeasurementType ;
    owl:someValuesFrom [ a owl:Class ;
            owl:oneOf ( <http://vocab.nerc.ac.uk/collection/P02/current/DMST/> ) ] .
[] a owl:Restriction ;
    rdfs:subClassOf <http://vocab.nerc.ac.uk/collection/P02/current/SSCN/> ;
    owl:onProperty glbase:hasMeasurementType ;
    owl:someValuesFrom [ a owl:Class ;
            owl:oneOf ( <http://vocab.nerc.ac.uk/collection/P02/current/SSCN/> ) ] .
[] a owl:Restriction ;
    rdfs:subClassOf <http://vocab.nerc.ac.uk/collection/P02/current/CEMP/> ;
    owl:onProperty glbase:hasMeasurementType ;
    owl:someValuesFrom [ a owl:Class ;
            owl:oneOf ( <http://vocab.nerc.ac.uk/collection/P02/current/CEMP/> ) ] .
[] a owl:Restriction ;
    rdfs:subClassOf <http://vocab.nerc.ac.uk/collection/P02/current/MDPW/> ;
    owl:onProperty glbase:hasMeasurementType ;
    owl:someValuesFrom [ a owl:Class ;
            owl:oneOf ( <http://vocab.nerc.ac.uk/collection/P02/current/MDPW/> ) ] .
[] a owl:Restriction ;
    rdfs:subClassOf <http://vocab.nerc.ac.uk/collection/P02/current/OZON/> ;
    owl:onProperty glbase:hasMeasurementType ;
    owl:someValuesFrom [ a owl:Class ;
            owl:oneOf ( <http://vocab.nerc.ac.uk/collection/P02/current/OZON/> ) ] .
[] a owl:Restriction ;
    rdfs:subClassOf <http://vocab.nerc.ac.uk/collection/P02/current/RGAS/> ;
    owl:onProperty glbase:hasMeasurementType ;
    owl:someValuesFrom [ a owl:Class ;
            owl:oneOf ( <http://vocab.nerc.ac.uk/collection/P02/current/RGAS/> ) ] .
[] a owl:Restriction ;
    rdfs:subClassOf <http://vocab.nerc.ac.uk/collection/P02/current/CASD/> ;
    owl:onProperty glbase:hasMeasurementType ;
    owl:someValuesFrom [ a owl:Class ;
            owl:oneOf ( <http://vocab.nerc.ac.uk/collection/P02/current/CASD/> ) ] .
[] a owl:Restriction ;
    rdfs:subClassOf <http://vocab.nerc.ac.uk/collection/P02/current/SBPH/> ;
    owl:onProperty glbase:hasMeasurementType ;
    owl:someValuesFrom [ a owl:Class ;
            owl:oneOf ( <http://vocab.nerc.ac.uk/collection/P02/current/SBPH/> ) ] .
[] a owl:Restriction ;
    rdfs:subClassOf <http://vocab.nerc.ac.uk/collection/P02/current/LERR/> ;
    owl:onProperty glbase:hasMeasurementType ;
    owl:someValuesFrom [ a owl:Class ;
            owl:oneOf ( <http://vocab.nerc.ac.uk/collection/P02/current/LERR/> ) ] .
[] a owl:Restriction ;
    rdfs:subClassOf <http://vocab.nerc.ac.uk/collection/P02/current/DOXY/> ;
    owl:onProperty glbase:hasMeasurementType ;
    owl:someValuesFrom [ a owl:Class ;
            owl:oneOf ( <http://vocab.nerc.ac.uk/collection/P02/current/DOXY/> ) ] .
[] a owl:Restriction ;
    rdfs:subClassOf <http://vocab.nerc.ac.uk/collection/P02/current/FBAB/> ;
    owl:onProperty glbase:hasMeasurementType ;
    owl:someValuesFrom [ a owl:Class ;
            owl:oneOf ( <http://vocab.nerc.ac.uk/collection/P02/current/FBAB/> ) ] .
[] a owl:Restriction ;
    rdfs:subClassOf <http://vocab.nerc.ac.uk/collection/P02/current/MSBO/> ;
    owl:onProperty glbase:hasMeasurementType ;
    owl:someValuesFrom [ a owl:Class ;
            owl:oneOf ( <http://vocab.nerc.ac.uk/collection/P02/current/MSBO/> ) ] .
[] a owl:Restriction ;
    rdfs:subClassOf <http://vocab.nerc.ac.uk/collection/P02/current/RALT/> ;
    owl:onProperty glbase:hasMeasurementType ;
    owl:someValuesFrom [ a owl:Class ;
            owl:oneOf ( <http://vocab.nerc.ac.uk/collection/P02/current/RALT/> ) ] .
[] a owl:Restriction ;
    rdfs:subClassOf <http://vocab.nerc.ac.uk/collection/P02/current/DAAW/> ;
    owl:onProperty glbase:hasMeasurementType ;
    owl:someValuesFrom [ a owl:Class ;
            owl:oneOf ( <http://vocab.nerc.ac.uk/collection/P02/current/DAAW/> ) ] .
[] a owl:Restriction ;
    rdfs:subClassOf <http://vocab.nerc.ac.uk/collection/P02/current/UVRD/> ;
    owl:onProperty glbase:hasMeasurementType ;
    owl:someValuesFrom [ a owl:Class ;
            owl:oneOf ( <http://vocab.nerc.ac.uk/collection/P02/current/UVRD/> ) ] .
[] a owl:Restriction ;
    rdfs:subClassOf <http://vocab.nerc.ac.uk/collection/P02/current/HMSB/> ;
    owl:onProperty glbase:hasMeasurementType ;
    owl:someValuesFrom [ a owl:Class ;
            owl:oneOf ( <http://vocab.nerc.ac.uk/collection/P02/current/HMSB/> ) ] .
[] a owl:Restriction ;
    rdfs:subClassOf <http://vocab.nerc.ac.uk/collection/P02/current/FATX/> ;
    owl:onProperty glbase:hasMeasurementType ;
    owl:someValuesFrom [ a owl:Class ;
            owl:oneOf ( <http://vocab.nerc.ac.uk/collection/P02/current/FATX/> ) ] .
[] a owl:Restriction ;
    rdfs:subClassOf <http://vocab.nerc.ac.uk/collection/P02/current/XMGS/> ;
    owl:onProperty glbase:hasMeasurementType ;
    owl:someValuesFrom [ a owl:Class ;
            owl:oneOf ( <http://vocab.nerc.ac.uk/collection/P02/current/XMGS/> ) ] .
[] a owl:Restriction ;
    rdfs:subClassOf <http://vocab.nerc.ac.uk/collection/P02/current/PHLT/> ;
    owl:onProperty glbase:hasMeasurementType ;
    owl:someValuesFrom [ a owl:Class ;
            owl:oneOf ( <http://vocab.nerc.ac.uk/collection/P02/current/PHLT/> ) ] .
[] a owl:Restriction ;
    rdfs:subClassOf <http://vocab.nerc.ac.uk/collection/P02/current/OMET/> ;
    owl:onProperty glbase:hasMeasurementType ;
    owl:someValuesFrom [ a owl:Class ;
            owl:oneOf ( <http://vocab.nerc.ac.uk/collection/P02/current/OMET/> ) ] .
[] a owl:Restriction ;
    rdfs:subClassOf <http://vocab.nerc.ac.uk/collection/P02/current/FDMS/> ;
    owl:onProperty glbase:hasMeasurementType ;
    owl:someValuesFrom [ a owl:Class ;
            owl:oneOf ( <http://vocab.nerc.ac.uk/collection/P02/current/FDMS/> ) ] .
[] a owl:Restriction ;
    rdfs:subClassOf <http://vocab.nerc.ac.uk/collection/P02/current/PCHW/> ;
    owl:onProperty glbase:hasMeasurementType ;
    owl:someValuesFrom [ a owl:Class ;
            owl:oneOf ( <http://vocab.nerc.ac.uk/collection/P02/current/PCHW/> ) ] .
[] a owl:Restriction ;
    rdfs:subClassOf <http://vocab.nerc.ac.uk/collection/P02/current/WCWT/> ;
    owl:onProperty glbase:hasMeasurementType ;
    owl:someValuesFrom [ a owl:Class ;
            owl:oneOf ( <http://vocab.nerc.ac.uk/collection/P02/current/WCWT/> ) ] .
[] a owl:Restriction ;
    rdfs:subClassOf <http://vocab.nerc.ac.uk/collection/P02/current/PCOC/> ;
    owl:onProperty glbase:hasMeasurementType ;
    owl:someValuesFrom [ a owl:Class ;
            owl:oneOf ( <http://vocab.nerc.ac.uk/collection/P02/current/PCOC/> ) ] .
[] a owl:Restriction ;
    rdfs:subClassOf <http://vocab.nerc.ac.uk/collection/P02/current/SPRO/> ;
    owl:onProperty glbase:hasMeasurementType ;
    owl:someValuesFrom [ a owl:Class ;
            owl:oneOf ( <http://vocab.nerc.ac.uk/collection/P02/current/SPRO/> ) ] .
[] a owl:Restriction ;
    rdfs:subClassOf <http://vocab.nerc.ac.uk/collection/P02/current/WBRX/> ;
    owl:onProperty glbase:hasMeasurementType ;
    owl:someValuesFrom [ a owl:Class ;
            owl:oneOf ( <http://vocab.nerc.ac.uk/collection/P02/current/WBRX/> ) ] .
[] a owl:Restriction ;
    rdfs:subClassOf <http://vocab.nerc.ac.uk/collection/P02/current/SIAT/> ;
    owl:onProperty glbase:hasMeasurementType ;
    owl:someValuesFrom [ a owl:Class ;
            owl:oneOf ( <http://vocab.nerc.ac.uk/collection/P02/current/SIAT/> ) ] .
[] a owl:Restriction ;
    rdfs:subClassOf <http://vocab.nerc.ac.uk/collection/P02/current/INLZ/> ;
    owl:onProperty glbase:hasMeasurementType ;
    owl:someValuesFrom [ a owl:Class ;
            owl:oneOf ( <http://vocab.nerc.ac.uk/collection/P02/current/INLZ/> ) ] .
[] a owl:Restriction ;
    rdfs:subClassOf <http://vocab.nerc.ac.uk/collection/P02/current/GHDX/> ;
    owl:onProperty glbase:hasMeasurementType ;
    owl:someValuesFrom [ a owl:Class ;
            owl:oneOf ( <http://vocab.nerc.ac.uk/collection/P02/current/GHDX/> ) ] .
[] a owl:Restriction ;
    rdfs:subClassOf <http://vocab.nerc.ac.uk/collection/P02/current/CFTM/> ;
    owl:onProperty glbase:hasMeasurementType ;
    owl:someValuesFrom [ a owl:Class ;
            owl:oneOf ( <http://vocab.nerc.ac.uk/collection/P02/current/CFTM/> ) ] .
[] a owl:Restriction ;
    rdfs:subClassOf <http://vocab.nerc.ac.uk/collection/P02/current/RVDS/> ;
    owl:onProperty glbase:hasMeasurementType ;
    owl:someValuesFrom [ a owl:Class ;
            owl:oneOf ( <http://vocab.nerc.ac.uk/collection/P02/current/RVDS/> ) ] .
[] a owl:Restriction ;
    rdfs:subClassOf <http://vocab.nerc.ac.uk/collection/P02/current/MDSD/> ;
    owl:onProperty glbase:hasMeasurementType ;
    owl:someValuesFrom [ a owl:Class ;
            owl:oneOf ( <http://vocab.nerc.ac.uk/collection/P02/current/MDSD/> ) ] .
[] a owl:Restriction ;
    rdfs:subClassOf <http://vocab.nerc.ac.uk/collection/P02/current/IDIS/> ;
    owl:onProperty glbase:hasMeasurementType ;
    owl:someValuesFrom [ a owl:Class ;
            owl:oneOf ( <http://vocab.nerc.ac.uk/collection/P02/current/IDIS/> ) ] .
[] a owl:Restriction ;
    rdfs:subClassOf <http://vocab.nerc.ac.uk/collection/P02/current/SCOX/> ;
    owl:onProperty glbase:hasMeasurementType ;
    owl:someValuesFrom [ a owl:Class ;
            owl:oneOf ( <http://vocab.nerc.ac.uk/collection/P02/current/SCOX/> ) ] .
[] a owl:Restriction ;
    rdfs:subClassOf <http://vocab.nerc.ac.uk/collection/P02/current/GP025/> ;
    owl:onProperty glbase:hasMeasurementType ;
    owl:someValuesFrom [ a owl:Class ;
            owl:oneOf ( <http://vocab.nerc.ac.uk/collection/P02/current/GP025/> ) ] .
[] a owl:Restriction ;
    rdfs:subClassOf <http://vocab.nerc.ac.uk/collection/P02/current/STOM/> ;
    owl:onProperty glbase:hasMeasurementType ;
    owl:someValuesFrom [ a owl:Class ;
            owl:oneOf ( <http://vocab.nerc.ac.uk/collection/P02/current/STOM/> ) ] .
[] a owl:Restriction ;
    rdfs:subClassOf <http://vocab.nerc.ac.uk/collection/P02/current/SPGS/> ;
    owl:onProperty glbase:hasMeasurementType ;
    owl:someValuesFrom [ a owl:Class ;
            owl:oneOf ( <http://vocab.nerc.ac.uk/collection/P02/current/SPGS/> ) ] .
[] a owl:Restriction ;
    rdfs:subClassOf <http://vocab.nerc.ac.uk/collection/P02/current/EWSB/> ;
    owl:onProperty glbase:hasMeasurementType ;
    owl:someValuesFrom [ a owl:Class ;
            owl:oneOf ( <http://vocab.nerc.ac.uk/collection/P02/current/EWSB/> ) ] .
[] a owl:Restriction ;
    rdfs:subClassOf <http://vocab.nerc.ac.uk/collection/P02/current/ZWTX/> ;
    owl:onProperty glbase:hasMeasurementType ;
    owl:someValuesFrom [ a owl:Class ;
            owl:oneOf ( <http://vocab.nerc.ac.uk/collection/P02/current/ZWTX/> ) ] .
[] a owl:Restriction ;
    rdfs:subClassOf <http://vocab.nerc.ac.uk/collection/P02/current/FCNT/> ;
    owl:onProperty glbase:hasMeasurementType ;
    owl:someValuesFrom [ a owl:Class ;
            owl:oneOf ( <http://vocab.nerc.ac.uk/collection/P02/current/FCNT/> ) ] .
[] a owl:Restriction ;
    rdfs:subClassOf <http://vocab.nerc.ac.uk/collection/P02/current/GP004/> ;
    owl:onProperty glbase:hasMeasurementType ;
    owl:someValuesFrom [ a owl:Class ;
            owl:oneOf ( <http://vocab.nerc.ac.uk/collection/P02/current/GP004/> ) ] .
[] a owl:Restriction ;
    rdfs:subClassOf <http://vocab.nerc.ac.uk/collection/P02/current/ICHM/> ;
    owl:onProperty glbase:hasMeasurementType ;
    owl:someValuesFrom [ a owl:Class ;
            owl:oneOf ( <http://vocab.nerc.ac.uk/collection/P02/current/ICHM/> ) ] .
[] a owl:Restriction ;
    rdfs:subClassOf <http://vocab.nerc.ac.uk/collection/P02/current/BCOS/> ;
    owl:onProperty glbase:hasMeasurementType ;
    owl:someValuesFrom [ a owl:Class ;
            owl:oneOf ( <http://vocab.nerc.ac.uk/collection/P02/current/BCOS/> ) ] .
[] a owl:Restriction ;
    rdfs:subClassOf <http://vocab.nerc.ac.uk/collection/P02/current/CARS/> ;
    owl:onProperty glbase:hasMeasurementType ;
    owl:someValuesFrom [ a owl:Class ;
            owl:oneOf ( <http://vocab.nerc.ac.uk/collection/P02/current/CARS/> ) ] .
[] a owl:Restriction ;
    rdfs:subClassOf <http://vocab.nerc.ac.uk/collection/P02/current/BNUC/> ;
    owl:onProperty glbase:hasMeasurementType ;
    owl:someValuesFrom [ a owl:Class ;
            owl:oneOf ( <http://vocab.nerc.ac.uk/collection/P02/current/BNUC/> ) ] .
[] a owl:Restriction ;
    rdfs:subClassOf <http://vocab.nerc.ac.uk/collection/P02/current/COGE/> ;
    owl:onProperty glbase:hasMeasurementType ;
    owl:someValuesFrom [ a owl:Class ;
            owl:oneOf ( <http://vocab.nerc.ac.uk/collection/P02/current/COGE/> ) ] .
[] a owl:Restriction ;
    rdfs:subClassOf <http://vocab.nerc.ac.uk/collection/P02/current/AXFX/> ;
    owl:onProperty glbase:hasMeasurementType ;
    owl:someValuesFrom [ a owl:Class ;
            owl:oneOf ( <http://vocab.nerc.ac.uk/collection/P02/current/AXFX/> ) ] .
[] a owl:Restriction ;
    rdfs:subClassOf <http://vocab.nerc.ac.uk/collection/P02/current/MTPW/> ;
    owl:onProperty glbase:hasMeasurementType ;
    owl:someValuesFrom [ a owl:Class ;
            owl:oneOf ( <http://vocab.nerc.ac.uk/collection/P02/current/MTPW/> ) ] .
[] a owl:Restriction ;
    rdfs:subClassOf <http://vocab.nerc.ac.uk/collection/P02/current/MTWC/> ;
    owl:onProperty glbase:hasMeasurementType ;
    owl:someValuesFrom [ a owl:Class ;
            owl:oneOf ( <http://vocab.nerc.ac.uk/collection/P02/current/MTWC/> ) ] .
[] a owl:Restriction ;
    rdfs:subClassOf <http://vocab.nerc.ac.uk/collection/P02/current/SXCN/> ;
    owl:onProperty glbase:hasMeasurementType ;
    owl:someValuesFrom [ a owl:Class ;
            owl:oneOf ( <http://vocab.nerc.ac.uk/collection/P02/current/SXCN/> ) ] .
[] a owl:Restriction ;
    rdfs:subClassOf <http://vocab.nerc.ac.uk/collection/P02/current/SICO/> ;
    owl:onProperty glbase:hasMeasurementType ;
    owl:someValuesFrom [ a owl:Class ;
            owl:oneOf ( <http://vocab.nerc.ac.uk/collection/P02/current/SICO/> ) ] .
[] a owl:Restriction ;
    rdfs:subClassOf <http://vocab.nerc.ac.uk/collection/P02/current/IALZ/> ;
    owl:onProperty glbase:hasMeasurementType ;
    owl:someValuesFrom [ a owl:Class ;
            owl:oneOf ( <http://vocab.nerc.ac.uk/collection/P02/current/IALZ/> ) ] .
[] a owl:Restriction ;
    rdfs:subClassOf <http://vocab.nerc.ac.uk/collection/P02/current/PHAT/> ;
    owl:onProperty glbase:hasMeasurementType ;
    owl:someValuesFrom [ a owl:Class ;
            owl:oneOf ( <http://vocab.nerc.ac.uk/collection/P02/current/PHAT/> ) ] .
[] a owl:Restriction ;
    rdfs:subClassOf <http://vocab.nerc.ac.uk/collection/P02/current/DGPW/> ;
    owl:onProperty glbase:hasMeasurementType ;
    owl:someValuesFrom [ a owl:Class ;
            owl:oneOf ( <http://vocab.nerc.ac.uk/collection/P02/current/DGPW/> ) ] .
[] a owl:Restriction ;
    rdfs:subClassOf <http://vocab.nerc.ac.uk/collection/P02/current/A999/> ;
    owl:onProperty glbase:hasMeasurementType ;
    owl:someValuesFrom [ a owl:Class ;
            owl:oneOf ( <http://vocab.nerc.ac.uk/collection/P02/current/A999/> ) ] .
[] a owl:Restriction ;
    rdfs:subClassOf <http://vocab.nerc.ac.uk/collection/P02/current/MTAT/> ;
    owl:onProperty glbase:hasMeasurementType ;
    owl:someValuesFrom [ a owl:Class ;
            owl:oneOf ( <http://vocab.nerc.ac.uk/collection/P02/current/MTAT/> ) ] .
[] a owl:Restriction ;
    rdfs:subClassOf <http://vocab.nerc.ac.uk/collection/P02/current/CLAY/> ;
    owl:onProperty glbase:hasMeasurementType ;
    owl:someValuesFrom [ a owl:Class ;
            owl:oneOf ( <http://vocab.nerc.ac.uk/collection/P02/current/CLAY/> ) ] .
[] a owl:Restriction ;
    rdfs:subClassOf <http://vocab.nerc.ac.uk/collection/P02/current/IPRX/> ;
    owl:onProperty glbase:hasMeasurementType ;
    owl:someValuesFrom [ a owl:Class ;
            owl:oneOf ( <http://vocab.nerc.ac.uk/collection/P02/current/IPRX/> ) ] .
[] a owl:Restriction ;
    rdfs:subClassOf <http://vocab.nerc.ac.uk/collection/P02/current/LSST/> ;
    owl:onProperty glbase:hasMeasurementType ;
    owl:someValuesFrom [ a owl:Class ;
            owl:oneOf ( <http://vocab.nerc.ac.uk/collection/P02/current/LSST/> ) ] .
[] a owl:Restriction ;
    rdfs:subClassOf <http://vocab.nerc.ac.uk/collection/P02/current/WVSP/> ;
    owl:onProperty glbase:hasMeasurementType ;
    owl:someValuesFrom [ a owl:Class ;
            owl:oneOf ( <http://vocab.nerc.ac.uk/collection/P02/current/WVSP/> ) ] .
[] a owl:Restriction ;
    rdfs:subClassOf <http://vocab.nerc.ac.uk/collection/P02/current/AAWC/> ;
    owl:onProperty glbase:hasMeasurementType ;
    owl:someValuesFrom [ a owl:Class ;
            owl:oneOf ( <http://vocab.nerc.ac.uk/collection/P02/current/AAWC/> ) ] .
[] a owl:Restriction ;
    rdfs:subClassOf <http://vocab.nerc.ac.uk/collection/P02/current/EXCO/> ;
    owl:onProperty glbase:hasMeasurementType ;
    owl:someValuesFrom [ a owl:Class ;
            owl:oneOf ( <http://vocab.nerc.ac.uk/collection/P02/current/EXCO/> ) ] .
[] a owl:Restriction ;
    rdfs:subClassOf <http://vocab.nerc.ac.uk/collection/P02/current/RMAJ/> ;
    owl:onProperty glbase:hasMeasurementType ;
    owl:someValuesFrom [ a owl:Class ;
            owl:oneOf ( <http://vocab.nerc.ac.uk/collection/P02/current/RMAJ/> ) ] .
[] a owl:Restriction ;
    rdfs:subClassOf <http://vocab.nerc.ac.uk/collection/P02/current/GERA/> ;
    owl:onProperty glbase:hasMeasurementType ;
    owl:someValuesFrom [ a owl:Class ;
            owl:oneOf ( <http://vocab.nerc.ac.uk/collection/P02/current/GERA/> ) ] .
[] a owl:Restriction ;
    rdfs:subClassOf <http://vocab.nerc.ac.uk/collection/P02/current/SCDO/> ;
    owl:onProperty glbase:hasMeasurementType ;
    owl:someValuesFrom [ a owl:Class ;
            owl:oneOf ( <http://vocab.nerc.ac.uk/collection/P02/current/SCDO/> ) ] .
[] a owl:Restriction ;
    rdfs:subClassOf <http://vocab.nerc.ac.uk/collection/P02/current/TRIS/> ;
    owl:onProperty glbase:hasMeasurementType ;
    owl:someValuesFrom [ a owl:Class ;
            owl:oneOf ( <http://vocab.nerc.ac.uk/collection/P02/current/TRIS/> ) ] .
[] a owl:Restriction ;
    rdfs:subClassOf <http://vocab.nerc.ac.uk/collection/P02/current/BATT/> ;
    owl:onProperty glbase:hasMeasurementType ;
    owl:someValuesFrom [ a owl:Class ;
            owl:oneOf ( <http://vocab.nerc.ac.uk/collection/P02/current/BATT/> ) ] .
[] a owl:Restriction ;
    rdfs:subClassOf <http://vocab.nerc.ac.uk/collection/P02/current/PHYG/> ;
    owl:onProperty glbase:hasMeasurementType ;
    owl:someValuesFrom [ a owl:Class ;
            owl:oneOf ( <http://vocab.nerc.ac.uk/collection/P02/current/PHYG/> ) ] .
[] a owl:Restriction ;
    rdfs:subClassOf <http://vocab.nerc.ac.uk/collection/P02/current/AALK/> ;
    owl:onProperty glbase:hasMeasurementType ;
    owl:someValuesFrom [ a owl:Class ;
            owl:oneOf ( <http://vocab.nerc.ac.uk/collection/P02/current/AALK/> ) ] .
[] a owl:Restriction ;
    rdfs:subClassOf <http://vocab.nerc.ac.uk/collection/P02/current/PTOX/> ;
    owl:onProperty glbase:hasMeasurementType ;
    owl:someValuesFrom [ a owl:Class ;
            owl:oneOf ( <http://vocab.nerc.ac.uk/collection/P02/current/PTOX/> ) ] .
[] a owl:Restriction ;
    rdfs:subClassOf <http://vocab.nerc.ac.uk/collection/P02/current/MTWD/> ;
    owl:onProperty glbase:hasMeasurementType ;
    owl:someValuesFrom [ a owl:Class ;
            owl:oneOf ( <http://vocab.nerc.ac.uk/collection/P02/current/MTWD/> ) ] .
[] a owl:Restriction ;
    rdfs:subClassOf <http://vocab.nerc.ac.uk/collection/P02/current/BATX/> ;
    owl:onProperty glbase:hasMeasurementType ;
    owl:someValuesFrom [ a owl:Class ;
            owl:oneOf ( <http://vocab.nerc.ac.uk/collection/P02/current/BATX/> ) ] .
[] a owl:Restriction ;
    rdfs:subClassOf <http://vocab.nerc.ac.uk/collection/P02/current/CCPW/> ;
    owl:onProperty glbase:hasMeasurementType ;
    owl:someValuesFrom [ a owl:Class ;
            owl:oneOf ( <http://vocab.nerc.ac.uk/collection/P02/current/CCPW/> ) ] .
[] a owl:Restriction ;
    rdfs:subClassOf <http://vocab.nerc.ac.uk/collection/P02/current/RAGE/> ;
    owl:onProperty glbase:hasMeasurementType ;
    owl:someValuesFrom [ a owl:Class ;
            owl:oneOf ( <http://vocab.nerc.ac.uk/collection/P02/current/RAGE/> ) ] .
[] a owl:Restriction ;
    rdfs:subClassOf <http://vocab.nerc.ac.uk/collection/P02/current/RTCO/> ;
    owl:onProperty glbase:hasMeasurementType ;
    owl:someValuesFrom [ a owl:Class ;
            owl:oneOf ( <http://vocab.nerc.ac.uk/collection/P02/current/RTCO/> ) ] .
[] a owl:Restriction ;
    rdfs:subClassOf <http://vocab.nerc.ac.uk/collection/P02/current/PNFX/> ;
    owl:onProperty glbase:hasMeasurementType ;
    owl:someValuesFrom [ a owl:Class ;
            owl:oneOf ( <http://vocab.nerc.ac.uk/collection/P02/current/PNFX/> ) ] .
[] a owl:Restriction ;
    rdfs:subClassOf <http://vocab.nerc.ac.uk/collection/P02/current/ABAG/> ;
    owl:onProperty glbase:hasMeasurementType ;
    owl:someValuesFrom [ a owl:Class ;
            owl:oneOf ( <http://vocab.nerc.ac.uk/collection/P02/current/ABAG/> ) ] .
