<?xml version="1.0"?>
<rdf:RDF xmlns="http://schema.geolink.org/1.0/pattern/agentrole#"
     xml:base="http://schema.geolink.org/1.0/pattern/agentrole"
     xmlns:agentrole="http://schema.geolink.org/1.0/pattern/agentrole#"
     xmlns:rdf="http://www.w3.org/1999/02/22-rdf-syntax-ns#"
     xmlns:owl="http://www.w3.org/2002/07/owl#"
     xmlns:xml="http://www.w3.org/XML/1998/namespace"
     xmlns:xsd="http://www.w3.org/2001/XMLSchema#"
     xmlns:rdfs="http://www.w3.org/2000/01/rdf-schema#">
    <owl:Ontology rdf:about="http://schema.geolink.org/1.0/pattern/agentrole">
        <owl:imports rdf:resource="http://schema.geolink.org/1.0/pattern/agentrole-to-owltime"/>
        <owl:imports rdf:resource="http://schema.geolink.org/1.0/pattern/agent"/>
        <rdfs:label>GeoLink Agent Role Pattern</rdfs:label>
        <rdfs:comment>The Agent Role pattern describes a role that may be performed by an agent within a particular context, i.e., in an organization, a cruise, a project, etc.</rdfs:comment>
    </owl:Ontology>
    


    <!-- 
    ///////////////////////////////////////////////////////////////////////////////////////
    //
    // Object Properties
    //
    ///////////////////////////////////////////////////////////////////////////////////////
     -->

    


    <!-- http://schema.geolink.org/1.0/pattern/agentrole#endsAtTime -->

    <owl:ObjectProperty rdf:about="http://schema.geolink.org/1.0/pattern/agentrole#endsAtTime">
        <rdfs:comment>endsAtTime provides the ending time of a role.</rdfs:comment>
        <rdfs:label>endsAtTime</rdfs:label>
    </owl:ObjectProperty>
    


    <!-- http://schema.geolink.org/1.0/pattern/agentrole#hasAgentRoleType -->

    <owl:ObjectProperty rdf:about="http://schema.geolink.org/1.0/pattern/agentrole#hasAgentRoleType">
        <rdfs:label>hasAgentRoleType</rdfs:label>
    </owl:ObjectProperty>
    


    <!-- http://schema.geolink.org/1.0/pattern/agentrole#isAgentRoleIn -->

    <owl:ObjectProperty rdf:about="http://schema.geolink.org/1.0/pattern/agentrole#isAgentRoleIn">
        <owl:inverseOf rdf:resource="http://schema.geolink.org/1.0/pattern/agentrole#providesAgentRole"/>
        <rdfs:domain rdf:resource="http://schema.geolink.org/1.0/pattern/agentrole#AgentRole"/>
        <rdfs:comment>isAgentRoleIn connects a role to the thing thing in which the role is performed by the agent.</rdfs:comment>
        <rdfs:label>isAgentRoleIn</rdfs:label>
    </owl:ObjectProperty>
    


    <!-- http://schema.geolink.org/1.0/pattern/agentrole#isPerformedBy -->

    <owl:ObjectProperty rdf:about="http://schema.geolink.org/1.0/pattern/agentrole#isPerformedBy">
        <rdfs:comment>isPerformedBy connects  a role to the agent that performs it.</rdfs:comment>
        <rdfs:label>isPerformedBy</rdfs:label>
    </owl:ObjectProperty>
    


    <!-- http://schema.geolink.org/1.0/pattern/agentrole#providesAgentRole -->

    <owl:ObjectProperty rdf:about="http://schema.geolink.org/1.0/pattern/agentrole#providesAgentRole">
        <rdfs:range rdf:resource="http://schema.geolink.org/1.0/pattern/agentrole#AgentRole"/>
        <rdfs:comment>providesAgentRole is the inverse of isAgentRoleIn.</rdfs:comment>
        <rdfs:label>providesAgentRole</rdfs:label>
    </owl:ObjectProperty>
    


    <!-- http://schema.geolink.org/1.0/pattern/agentrole#startsAtTime -->

    <owl:ObjectProperty rdf:about="http://schema.geolink.org/1.0/pattern/agentrole#startsAtTime">
        <rdfs:comment>startsAtTime provides the starting time of a role.</rdfs:comment>
        <rdfs:label>startsAtTime</rdfs:label>
    </owl:ObjectProperty>
    


    <!-- 
    ///////////////////////////////////////////////////////////////////////////////////////
    //
    // Classes
    //
    ///////////////////////////////////////////////////////////////////////////////////////
     -->

    


    <!-- http://schema.geolink.org/1.0/pattern/agentrole#Agent -->

    <owl:Class rdf:about="http://schema.geolink.org/1.0/pattern/agentrole#Agent">
        <rdfs:comment>Hook of the Agent class in Agent Role pattern, which corresponds to the main class of the Agent pattern.</rdfs:comment>
        <rdfs:label>Agent</rdfs:label>
    </owl:Class>
    


    <!-- http://schema.geolink.org/1.0/pattern/agentrole#AgentRole -->

    <owl:Class rdf:about="http://schema.geolink.org/1.0/pattern/agentrole#AgentRole">
        <rdfs:subClassOf>
            <owl:Restriction>
                <owl:onProperty rdf:resource="http://schema.geolink.org/1.0/pattern/agentrole#endsAtTime"/>
                <owl:allValuesFrom rdf:resource="http://schema.geolink.org/1.0/pattern/agentrole#TimeInstant"/>
            </owl:Restriction>
        </rdfs:subClassOf>
        <rdfs:subClassOf>
            <owl:Restriction>
                <owl:onProperty rdf:resource="http://schema.geolink.org/1.0/pattern/agentrole#hasAgentRoleType"/>
                <owl:allValuesFrom rdf:resource="http://schema.geolink.org/1.0/pattern/agentrole#AgentRoleType"/>
            </owl:Restriction>
        </rdfs:subClassOf>
        <rdfs:subClassOf>
            <owl:Restriction>
                <owl:onProperty rdf:resource="http://schema.geolink.org/1.0/pattern/agentrole#isPerformedBy"/>
                <owl:allValuesFrom rdf:resource="http://schema.geolink.org/1.0/pattern/agentrole#Agent"/>
            </owl:Restriction>
        </rdfs:subClassOf>
        <rdfs:subClassOf>
            <owl:Restriction>
                <owl:onProperty rdf:resource="http://schema.geolink.org/1.0/pattern/agentrole#startsAtTime"/>
                <owl:allValuesFrom rdf:resource="http://schema.geolink.org/1.0/pattern/agentrole#TimeInstant"/>
            </owl:Restriction>
        </rdfs:subClassOf>
        <rdfs:subClassOf>
            <owl:Restriction>
                <owl:onProperty rdf:resource="http://schema.geolink.org/1.0/pattern/agentrole#endsAtTime"/>
                <owl:qualifiedCardinality rdf:datatype="http://www.w3.org/2001/XMLSchema#nonNegativeInteger">1</owl:qualifiedCardinality>
                <owl:onClass rdf:resource="http://schema.geolink.org/1.0/pattern/agentrole#TimeInstant"/>
            </owl:Restriction>
        </rdfs:subClassOf>
        <rdfs:subClassOf>
            <owl:Restriction>
                <owl:onProperty rdf:resource="http://schema.geolink.org/1.0/pattern/agentrole#isAgentRoleIn"/>
                <owl:cardinality rdf:datatype="http://www.w3.org/2001/XMLSchema#nonNegativeInteger">1</owl:cardinality>
            </owl:Restriction>
        </rdfs:subClassOf>
        <rdfs:subClassOf>
            <owl:Restriction>
                <owl:onProperty rdf:resource="http://schema.geolink.org/1.0/pattern/agentrole#isPerformedBy"/>
                <owl:qualifiedCardinality rdf:datatype="http://www.w3.org/2001/XMLSchema#nonNegativeInteger">1</owl:qualifiedCardinality>
                <owl:onClass rdf:resource="http://schema.geolink.org/1.0/pattern/agentrole#Agent"/>
            </owl:Restriction>
        </rdfs:subClassOf>
        <rdfs:subClassOf>
            <owl:Restriction>
                <owl:onProperty rdf:resource="http://schema.geolink.org/1.0/pattern/agentrole#startsAtTime"/>
                <owl:qualifiedCardinality rdf:datatype="http://www.w3.org/2001/XMLSchema#nonNegativeInteger">1</owl:qualifiedCardinality>
                <owl:onClass rdf:resource="http://schema.geolink.org/1.0/pattern/agentrole#TimeInstant"/>
            </owl:Restriction>
        </rdfs:subClassOf>
        <rdfs:comment>An instance of AgentRole represents a role performed by an agent, which is temporally restricted by a starting and ending time.  Every agent role is performed by exactly one agent. One can create a subclass of AgentRole to model a particular kind of roles.</rdfs:comment>
        <rdfs:label>AgentRole</rdfs:label>
    </owl:Class>
    


    <!-- http://schema.geolink.org/1.0/pattern/agentrole#AgentRoleType -->

    <owl:Class rdf:about="http://schema.geolink.org/1.0/pattern/agentrole#AgentRoleType">
        <rdfs:comment>Class that contains types of agent roles. Allows one to put types of agent roles (which can be seen as subclasses of AgentRole) as named individuals, and the axiomatization could infer anonymous subclasses of AgentRole from those individuals.</rdfs:comment>
        <rdfs:label>AgentRoleType</rdfs:label>
    </owl:Class>
    


    <!-- http://schema.geolink.org/1.0/pattern/agentrole#TimeInstant -->

    <owl:Class rdf:about="http://schema.geolink.org/1.0/pattern/agentrole#TimeInstant">
        <rdfs:comment>TimeInstant represents a time point, analogous to how time point is modeled in the OWL Time ontology.</rdfs:comment>
        <rdfs:label>TimeInstant</rdfs:label>
    </owl:Class>
    


    <!-- 
    ///////////////////////////////////////////////////////////////////////////////////////
    //
    // General axioms
    //
    ///////////////////////////////////////////////////////////////////////////////////////
     -->

    <owl:Restriction>
        <owl:onProperty rdf:resource="http://schema.geolink.org/1.0/pattern/agentrole#endsAtTime"/>
        <owl:someValuesFrom rdf:resource="http://schema.geolink.org/1.0/pattern/agentrole#TimeInstant"/>
        <rdfs:subClassOf rdf:resource="http://schema.geolink.org/1.0/pattern/agentrole#AgentRole"/>
    </owl:Restriction>
    <owl:Restriction>
        <owl:onProperty rdf:resource="http://schema.geolink.org/1.0/pattern/agentrole#hasAgentRoleType"/>
        <owl:someValuesFrom rdf:resource="http://schema.geolink.org/1.0/pattern/agentrole#AgentRoleType"/>
        <rdfs:subClassOf rdf:resource="http://schema.geolink.org/1.0/pattern/agentrole#AgentRole"/>
    </owl:Restriction>
    <owl:Restriction>
        <owl:onProperty rdf:resource="http://schema.geolink.org/1.0/pattern/agentrole#isAgentRoleIn"/>
        <owl:someValuesFrom rdf:resource="http://www.w3.org/2002/07/owl#Thing"/>
        <rdfs:subClassOf rdf:resource="http://schema.geolink.org/1.0/pattern/agentrole#AgentRole"/>
    </owl:Restriction>
    <owl:Restriction>
        <owl:onProperty rdf:resource="http://schema.geolink.org/1.0/pattern/agentrole#isPerformedBy"/>
        <owl:someValuesFrom rdf:resource="http://schema.geolink.org/1.0/pattern/agentrole#Agent"/>
        <rdfs:subClassOf rdf:resource="http://schema.geolink.org/1.0/pattern/agentrole#AgentRole"/>
    </owl:Restriction>
    <owl:Restriction>
        <owl:onProperty rdf:resource="http://schema.geolink.org/1.0/pattern/agentrole#startsAtTime"/>
        <owl:someValuesFrom rdf:resource="http://schema.geolink.org/1.0/pattern/agentrole#TimeInstant"/>
        <rdfs:subClassOf rdf:resource="http://schema.geolink.org/1.0/pattern/agentrole#AgentRole"/>
    </owl:Restriction>
    <rdf:Description>
        <rdf:type rdf:resource="http://www.w3.org/2002/07/owl#AllDisjointClasses"/>
        <owl:members rdf:parseType="Collection">
            <rdf:Description rdf:about="http://schema.geolink.org/1.0/pattern/agentrole#Agent"/>
            <rdf:Description rdf:about="http://schema.geolink.org/1.0/pattern/agentrole#AgentRole"/>
            <rdf:Description rdf:about="http://schema.geolink.org/1.0/pattern/agentrole#TimeInstant"/>
        </owl:members>
    </rdf:Description>
</rdf:RDF>



<!-- Generated by the OWL API (version 4.2.6.20160910-2108) https://github.com/owlcs/owlapi -->

