<?xml version="1.0"?>


<!DOCTYPE rdf:RDF [
    <!ENTITY owl "http://www.w3.org/2002/07/owl#" >
    <!ENTITY xsd "http://www.w3.org/2001/XMLSchema#" >
    <!ENTITY rdfs "http://www.w3.org/2000/01/rdf-schema#" >
    <!ENTITY rdf "http://www.w3.org/1999/02/22-rdf-syntax-ns#" >
]>


<rdf:RDF xmlns="http://schema.geolink.org/dev/pattern/agent#"
     xml:base="http://schema.geolink.org/dev/pattern/agent"
     xmlns:rdf="http://www.w3.org/1999/02/22-rdf-syntax-ns#"
     xmlns:owl="http://www.w3.org/2002/07/owl#"
     xmlns:xsd="http://www.w3.org/2001/XMLSchema#"
     xmlns:rdfs="http://www.w3.org/2000/01/rdf-schema#">
    <owl:Ontology rdf:about="http://schema.geolink.org/dev/pattern/agent">
        <rdfs:label>GeoLink Agent Pattern</rdfs:label>
        <rdfs:comment>The Agent pattern is a very simplistic pattern stub intended to model agents such as people or organization.  Alignments are specified with the Agent Role pattern</rdfs:comment>
        <owl:imports rdf:resource="http://schema.geolink.org/dev/pattern/agent-to-agentrole"/>
    </owl:Ontology>
    


    <!-- 
    ///////////////////////////////////////////////////////////////////////////////////////
    //
    // Object Properties
    //
    ///////////////////////////////////////////////////////////////////////////////////////
     -->

    


    <!-- http://schema.geolink.org/dev/pattern/agent#performsAgentRole -->

    <owl:ObjectProperty rdf:about="http://schema.geolink.org/dev/pattern/agent#performsAgentRole">
        <rdfs:label>performsAgentRole</rdfs:label>
    </owl:ObjectProperty>
    


    <!-- 
    ///////////////////////////////////////////////////////////////////////////////////////
    //
    // Classes
    //
    ///////////////////////////////////////////////////////////////////////////////////////
     -->

    


    <!-- http://schema.geolink.org/dev/pattern/agent#Agent -->

    <owl:Class rdf:about="http://schema.geolink.org/dev/pattern/agent#Agent">
        <rdfs:label>Agent</rdfs:label>
        <rdfs:subClassOf>
            <owl:Restriction>
                <owl:onProperty rdf:resource="http://schema.geolink.org/dev/pattern/agent#performsAgentRole"/>
                <owl:allValuesFrom rdf:resource="http://schema.geolink.org/dev/pattern/agent#AgentRole"/>
            </owl:Restriction>
        </rdfs:subClassOf>
        <owl:disjointWith rdf:resource="http://schema.geolink.org/dev/pattern/agent#AgentRole"/>
        <rdfs:comment>Agents may perform a role (an instance of AgentRole class), e.g., in the context of events, organizations, etc.</rdfs:comment>
    </owl:Class>
    


    <!-- http://schema.geolink.org/dev/pattern/agent#AgentRole -->

    <owl:Class rdf:about="http://schema.geolink.org/dev/pattern/agent#AgentRole">
        <rdfs:label>AgentRole</rdfs:label>
        <rdfs:comment>AgentRole represents roles that can be performed by an agent, e.g., in the context of events, organizations, etc.</rdfs:comment>
    </owl:Class>
    


    <!-- 
    ///////////////////////////////////////////////////////////////////////////////////////
    //
    // General axioms
    //
    ///////////////////////////////////////////////////////////////////////////////////////
     -->

    <owl:Restriction>
        <rdfs:subClassOf rdf:resource="http://schema.geolink.org/dev/pattern/agent#Agent"/>
        <owl:onProperty rdf:resource="http://schema.geolink.org/dev/pattern/agent#performsAgentRole"/>
        <owl:someValuesFrom rdf:resource="http://schema.geolink.org/dev/pattern/agent#AgentRole"/>
    </owl:Restriction>
</rdf:RDF>



<!-- Generated by the OWL API (version 3.5.1) http://owlapi.sourceforge.net -->

