<?xml version="1.0"?>
<rdf:RDF xmlns="http://schema.geolink.org/1.0/pattern/cruise#"
     xml:base="http://schema.geolink.org/1.0/pattern/cruise"
     xmlns:rdf="http://www.w3.org/1999/02/22-rdf-syntax-ns#"
     xmlns:terms="http://purl.org/dc/terms/"
     xmlns:owl="http://www.w3.org/2002/07/owl#"
     xmlns:xml="http://www.w3.org/XML/1998/namespace"
     xmlns:cruise="http://schema.geolink.org/1.0/pattern/cruise#"
     xmlns:xsd="http://www.w3.org/2001/XMLSchema#"
     xmlns:skos="http://www.w3.org/2004/02/skos/core#"
     xmlns:rdfs="http://www.w3.org/2000/01/rdf-schema#"
     xmlns:dc="http://purl.org/dc/elements/1.1/">
    <owl:Ontology rdf:about="http://schema.geolink.org/1.0/pattern/cruise">
        <owl:imports rdf:resource="http://schema.geolink.org/1.0/pattern/place"/>
        <owl:imports rdf:resource="http://schema.geolink.org/1.0/pattern/informationobject"/>
        <owl:imports rdf:resource="http://schema.geolink.org/1.0/pattern/agentrole"/>
        <owl:imports rdf:resource="http://schema.geolink.org/1.0/pattern/event"/>
        <owl:imports rdf:resource="http://schema.geolink.org/1.0/pattern/program"/>
        <owl:imports rdf:resource="http://schema.geolink.org/1.0/pattern/vessel"/>
        <owl:imports rdf:resource="http://schema.geolink.org/1.0/pattern/fundingaward"/>
        <owl:imports rdf:resource="http://schema.geolink.org/1.0/pattern/trajectory"/>
        <rdfs:comment>The Cruise pattern describes ocean science cruises. This pattern is obtained by combining and reusing existing patterns, while keeping the amount of abstract ontological commitments to a minimum.

The Cruise pattern can be dissected into three parts. First, a cruise is an abstraction of a path/route undertaken by a vessel, which is a physical object, through space within a certain time duration. This is captured by modeling a cruise to have exactly one trajectory, consisting of spatiotemporal segments traversed by a vessel. Second, a cruise can be understood as an event, which provides role performed by agents, pertaining activities conducted in/during a cruise. Our modeling of event through the Event pattern views events as something that not only provide roles to agents, but also occurs within some spatiotemporal boundary. Consequently, the first and second parts mentioned earlier can be together seen as a kind of complicated event. In fact, both the first and second parts motivate the alignment with the Agent pattern, Agent Role pattern, and obviously, the Event pattern. Alignment with the Event pattern is in particular rather complicated since the spatiotemporal information of a cruise is implicitly given by its associated trajectory.

Next, for the third part, we understand that a cruise may have other, non-spatiotemporal information relevant to it. For instance, information about funding awards that fund it, or programs associated with it. This is modeled by reusing the Information Object pattern. Note that every information object can be realized by a number of information realization, which includes digital objects (papers, reports, etc.) about the cruise. All the above modeling choices allows us to distinguish a cruise from both the information object that describes it and the physical object, i.e., vessel, by which it is undertaken.</rdfs:comment>
        <rdfs:label>GeoLink Cruise Pattern</rdfs:label>
    </owl:Ontology>
    


    <!-- 
    ///////////////////////////////////////////////////////////////////////////////////////
    //
    // Annotation properties
    //
    ///////////////////////////////////////////////////////////////////////////////////////
     -->

    


    <!-- http://schema.geolink.org/1.0/pattern/cruise#DASE_RULE -->

    <owl:AnnotationProperty rdf:about="http://schema.geolink.org/1.0/pattern/cruise#DASE_RULE"/>
    


    <!-- 
    ///////////////////////////////////////////////////////////////////////////////////////
    //
    // Object Properties
    //
    ///////////////////////////////////////////////////////////////////////////////////////
     -->

    


    <!-- http://schema.geolink.org/1.0/pattern/cruise#atPort -->

    <owl:ObjectProperty rdf:about="http://schema.geolink.org/1.0/pattern/cruise#atPort">
        <owl:propertyChainAxiom rdf:parseType="Collection">
            <rdf:Description rdf:about="http://schema.geolink.org/1.0/pattern/trajectory#hasPosition"/>
            <rdf:Description>
                <owl:inverseOf rdf:resource="http://schema.geolink.org/1.0/pattern/place#hasSpatialFootprint"/>
            </rdf:Description>
            <rdf:Description rdf:about="http://schema.geolink.org/1.0/pattern/cruise#r_Port"/>
        </owl:propertyChainAxiom>
        <rdfs:comment>atPort connects a fix to an instance of Port. It is used when the fix corresponds to a port stop in the beginning, middle, or end of a cruise.</rdfs:comment>
        <rdfs:label>atPort</rdfs:label>
    </owl:ObjectProperty>
    <owl:Axiom>
        <owl:annotatedSource rdf:resource="http://schema.geolink.org/1.0/pattern/cruise#atPort"/>
        <owl:annotatedProperty rdf:resource="http://www.w3.org/2002/07/owl#propertyChainAxiom"/>
        <owl:annotatedTarget rdf:parseType="Collection">
            <rdf:Description rdf:about="http://schema.geolink.org/1.0/pattern/trajectory#hasPosition"/>
            <rdf:Description>
                <owl:inverseOf rdf:resource="http://schema.geolink.org/1.0/pattern/place#hasSpatialFootprint"/>
            </rdf:Description>
            <rdf:Description rdf:about="http://schema.geolink.org/1.0/pattern/cruise#r_Port"/>
        </owl:annotatedTarget>
        <DASE_RULE rdf:datatype="http://www.w3.org/2001/XMLSchema#string">R2___trajectory:hasPosition(?x,?y) ^ place:hasSpatialFootprint(?z,?y) ^ :Port(?z) -&gt; :atPort(?x,?z)___If position of a fix corresponds to a (spatial footprint of a) port, then that fix is at that port.___http://schema.geolink.org/1.0/pattern/cruise#freshObjectProperty1</DASE_RULE>
    </owl:Axiom>
    


    <!-- http://schema.geolink.org/1.0/pattern/cruise#hasRelatedCruise -->

    <owl:ObjectProperty rdf:about="http://schema.geolink.org/1.0/pattern/cruise#hasRelatedCruise">
        <rdfs:label>hasRelatedCruise</rdfs:label>
    </owl:ObjectProperty>
    


    <!-- http://schema.geolink.org/1.0/pattern/cruise#hasTrajectory -->

    <owl:ObjectProperty rdf:about="http://schema.geolink.org/1.0/pattern/cruise#hasTrajectory">
        <rdfs:comment>The hasTrajectory connects a cruise to its trajectory.</rdfs:comment>
        <rdfs:label>hasTrajectory</rdfs:label>
    </owl:ObjectProperty>
    


    <!-- http://schema.geolink.org/1.0/pattern/cruise#r_Port -->

    <owl:ObjectProperty rdf:about="http://schema.geolink.org/1.0/pattern/cruise#r_Port">
        <rdfs:comment>The class Port typecasted as an object property. Logically, r_Port(x,x) &lt;-&gt; Port(x)</rdfs:comment>
        <rdfs:label>r_Port</rdfs:label>
    </owl:ObjectProperty>
    


    <!-- http://schema.geolink.org/1.0/pattern/cruise#traveledBy -->

    <owl:ObjectProperty rdf:about="http://schema.geolink.org/1.0/pattern/cruise#traveledBy">
        <owl:propertyChainAxiom rdf:parseType="Collection">
            <rdf:Description>
                <owl:inverseOf rdf:resource="http://schema.geolink.org/1.0/pattern/cruise#hasTrajectory"/>
            </rdf:Description>
            <rdf:Description rdf:about="http://schema.geolink.org/1.0/pattern/cruise#undertakenBy"/>
        </owl:propertyChainAxiom>
        <rdfs:comment>If a cruise is undertaken by a vessel, then its trajectory is traveled by the vessel.</rdfs:comment>
        <rdfs:label>traveledBy</rdfs:label>
    </owl:ObjectProperty>
    


    <!-- http://schema.geolink.org/1.0/pattern/cruise#undertakenBy -->

    <owl:ObjectProperty rdf:about="http://schema.geolink.org/1.0/pattern/cruise#undertakenBy">
        <rdfs:comment>This connects a cruise to the vessel on which the cruise is conducted.</rdfs:comment>
        <rdfs:label>undertakenBy</rdfs:label>
    </owl:ObjectProperty>
    


    <!-- http://schema.geolink.org/1.0/pattern/trajectory#traversedBy -->

    <rdf:Description rdf:about="http://schema.geolink.org/1.0/pattern/trajectory#traversedBy">
        <owl:propertyChainAxiom rdf:parseType="Collection">
            <rdf:Description>
                <owl:inverseOf rdf:resource="http://schema.geolink.org/1.0/pattern/trajectory#hasSegment"/>
            </rdf:Description>
            <rdf:Description rdf:about="http://schema.geolink.org/1.0/pattern/cruise#traveledBy"/>
        </owl:propertyChainAxiom>
    </rdf:Description>
    <owl:Axiom>
        <owl:annotatedSource rdf:resource="http://schema.geolink.org/1.0/pattern/trajectory#traversedBy"/>
        <owl:annotatedProperty rdf:resource="http://www.w3.org/2002/07/owl#propertyChainAxiom"/>
        <owl:annotatedTarget rdf:parseType="Collection">
            <rdf:Description>
                <owl:inverseOf rdf:resource="http://schema.geolink.org/1.0/pattern/trajectory#hasSegment"/>
            </rdf:Description>
            <rdf:Description rdf:about="http://schema.geolink.org/1.0/pattern/cruise#traveledBy"/>
        </owl:annotatedTarget>
        <rdfs:comment>This axiom is equivalent to the rule: 
:traveledBy(?x,?y) ^ trajectory:hasSegment(?x,?z) -&gt; trajectory:traversedBy(?z,?y)</rdfs:comment>
    </owl:Axiom>
    


    <!-- 
    ///////////////////////////////////////////////////////////////////////////////////////
    //
    // Classes
    //
    ///////////////////////////////////////////////////////////////////////////////////////
     -->

    


    <!-- http://schema.geolink.org/1.0/pattern/cruise#Cruise -->

    <owl:Class rdf:about="http://schema.geolink.org/1.0/pattern/cruise#Cruise">
        <rdfs:subClassOf rdf:resource="http://schema.geolink.org/1.0/pattern/event#Event"/>
        <rdfs:subClassOf>
            <owl:Restriction>
                <owl:onProperty rdf:resource="http://schema.geolink.org/1.0/pattern/agentrole#providesAgentRole"/>
                <owl:allValuesFrom rdf:resource="http://schema.geolink.org/1.0/pattern/agentrole#AgentRole"/>
            </owl:Restriction>
        </rdfs:subClassOf>
        <rdfs:subClassOf>
            <owl:Restriction>
                <owl:onProperty rdf:resource="http://schema.geolink.org/1.0/pattern/cruise#hasRelatedCruise"/>
                <owl:allValuesFrom rdf:resource="http://schema.geolink.org/1.0/pattern/cruise#Cruise"/>
            </owl:Restriction>
        </rdfs:subClassOf>
        <rdfs:subClassOf>
            <owl:Restriction>
                <owl:onProperty rdf:resource="http://schema.geolink.org/1.0/pattern/cruise#hasTrajectory"/>
                <owl:allValuesFrom rdf:resource="http://schema.geolink.org/1.0/pattern/cruise#CruiseTrajectory"/>
            </owl:Restriction>
        </rdfs:subClassOf>
        <rdfs:subClassOf>
            <owl:Restriction>
                <owl:onProperty rdf:resource="http://schema.geolink.org/1.0/pattern/cruise#undertakenBy"/>
                <owl:allValuesFrom rdf:resource="http://schema.geolink.org/1.0/pattern/vessel#Vessel"/>
            </owl:Restriction>
        </rdfs:subClassOf>
        <rdfs:subClassOf>
            <owl:Restriction>
                <owl:onProperty rdf:resource="http://schema.geolink.org/1.0/pattern/fundingaward#fundedBy"/>
                <owl:allValuesFrom rdf:resource="http://schema.geolink.org/1.0/pattern/fundingaward#FundingAward"/>
            </owl:Restriction>
        </rdfs:subClassOf>
        <rdfs:subClassOf>
            <owl:Restriction>
                <owl:onProperty rdf:resource="http://schema.geolink.org/1.0/pattern/informationobject#describedBy"/>
                <owl:allValuesFrom rdf:resource="http://schema.geolink.org/1.0/pattern/informationobject#InformationObject"/>
            </owl:Restriction>
        </rdfs:subClassOf>
        <rdfs:subClassOf>
            <owl:Restriction>
                <owl:onProperty rdf:resource="http://schema.geolink.org/1.0/pattern/program#associatedWithProgram"/>
                <owl:allValuesFrom rdf:resource="http://schema.geolink.org/1.0/pattern/program#Program"/>
            </owl:Restriction>
        </rdfs:subClassOf>
        <rdfs:subClassOf>
            <owl:Restriction>
                <owl:onProperty rdf:resource="http://schema.geolink.org/1.0/pattern/cruise#hasTrajectory"/>
                <owl:qualifiedCardinality rdf:datatype="http://www.w3.org/2001/XMLSchema#nonNegativeInteger">1</owl:qualifiedCardinality>
                <owl:onClass rdf:resource="http://schema.geolink.org/1.0/pattern/cruise#CruiseTrajectory"/>
            </owl:Restriction>
        </rdfs:subClassOf>
        <rdfs:subClassOf>
            <owl:Restriction>
                <owl:onProperty rdf:resource="http://schema.geolink.org/1.0/pattern/cruise#undertakenBy"/>
                <owl:qualifiedCardinality rdf:datatype="http://www.w3.org/2001/XMLSchema#nonNegativeInteger">1</owl:qualifiedCardinality>
                <owl:onClass rdf:resource="http://schema.geolink.org/1.0/pattern/vessel#Vessel"/>
            </owl:Restriction>
        </rdfs:subClassOf>
        <rdfs:subClassOf>
            <owl:Restriction>
                <owl:onProperty rdf:resource="http://schema.geolink.org/1.0/pattern/informationobject#describedBy"/>
                <owl:qualifiedCardinality rdf:datatype="http://www.w3.org/2001/XMLSchema#nonNegativeInteger">1</owl:qualifiedCardinality>
                <owl:onClass rdf:resource="http://schema.geolink.org/1.0/pattern/informationobject#InformationObject"/>
            </owl:Restriction>
        </rdfs:subClassOf>
        <rdfs:comment>A cruise is an event through the alignment with Event pattern. A cruise has exactly one trajectory, is undertaken by exactly one vessel, and is described by exactly one information object. Additionally, this information object describes exactly only the cruise. If a cruise is undertaken by a vessel, then the trajectory of the cruise has to be traveled by the vessel. Note that since isTraveledBy is implied by a property chain, OWL 2 specification forbids us to express a cardinality restriction using this peroperty. Consequently, we cannot axiomatize that the trajectory of a cruise can only be traveled by one vessel.

Involvements of agents in a cruise is modeled via the AgentRole, which is aligned to the Agent Role pattern. A cruise may be funded by some funding award, associated with some program, and related to some other cruise. These information are attached to the information object associated with a cruise.</rdfs:comment>
        <rdfs:label>Cruise</rdfs:label>
    </owl:Class>
    


    <!-- http://schema.geolink.org/1.0/pattern/cruise#CruiseTrajectory -->

    <owl:Class rdf:about="http://schema.geolink.org/1.0/pattern/cruise#CruiseTrajectory">
        <rdfs:subClassOf rdf:resource="http://schema.geolink.org/1.0/pattern/trajectory#Trajectory"/>
        <rdfs:subClassOf>
            <owl:Restriction>
                <owl:onProperty rdf:resource="http://schema.geolink.org/1.0/pattern/trajectory#hasFix"/>
                <owl:someValuesFrom>
                    <owl:Class>
                        <owl:intersectionOf rdf:parseType="Collection">
                            <rdf:Description rdf:about="http://schema.geolink.org/1.0/pattern/trajectory#StartingFix"/>
                            <owl:Restriction>
                                <owl:onProperty rdf:resource="http://schema.geolink.org/1.0/pattern/trajectory#hasNextFix"/>
                                <owl:someValuesFrom rdf:resource="http://schema.geolink.org/1.0/pattern/trajectory#Fix"/>
                            </owl:Restriction>
                        </owl:intersectionOf>
                    </owl:Class>
                </owl:someValuesFrom>
            </owl:Restriction>
        </rdfs:subClassOf>
        <rdfs:subClassOf>
            <owl:Restriction>
                <owl:onProperty rdf:resource="http://schema.geolink.org/1.0/pattern/cruise#traveledBy"/>
                <owl:allValuesFrom rdf:resource="http://schema.geolink.org/1.0/pattern/vessel#Vessel"/>
            </owl:Restriction>
        </rdfs:subClassOf>
        <rdfs:comment>A trajectory is given by a collection of fixes, representing time-stamped locations. Non-spatiotemporal information specific to a fix can be included by assigning it some attributes, for example, to indicate that the fix is the arrival to some port stop. The ordering of the fixes is based on their temporal information, although such an ordering is not axiomatized in this pattern. Between two consecutive fixes, we can define a segment, which is traversed by some moving object. There is no requirement forcing that all segments in the trajectory can only be traversed by the same moving object.

In the context of GeoLink project, the data typically already contains ordering of fixes, i.e., the nextFix relation is explicit in the data, and thus, segments are auto-instantiated from it. This is motivated by real scenarios whereby indeed only properties of fixes will often be known, in particular their locations, and temporal extension, whether they are at ports, whether they are arrival or departure fixes from ports, and in which sequence the fixes occurred. The traversing vessel will usually also be known. However, trajectory segments to which the trajectory pattern attaches information about the vessel are usually not explicitly represented in the data.</rdfs:comment>
        <rdfs:label>Trajectory</rdfs:label>
    </owl:Class>
    


    <!-- http://schema.geolink.org/1.0/pattern/cruise#Port -->

    <owl:Class rdf:about="http://schema.geolink.org/1.0/pattern/cruise#Port">
        <rdfs:subClassOf rdf:resource="http://schema.geolink.org/1.0/pattern/place#Place"/>
        <rdfs:subClassOf>
            <owl:Restriction>
                <owl:onProperty rdf:resource="http://schema.geolink.org/1.0/pattern/place#hasSpatialFootprint"/>
                <owl:allValuesFrom rdf:resource="http://schema.geolink.org/1.0/pattern/trajectory#Position"/>
            </owl:Restriction>
        </rdfs:subClassOf>
        <rdfs:subClassOf>
            <owl:Restriction>
                <owl:onProperty rdf:resource="http://schema.geolink.org/1.0/pattern/cruise#r_Port"/>
                <owl:hasSelf rdf:datatype="http://www.w3.org/2001/XMLSchema#boolean">true</owl:hasSelf>
            </owl:Restriction>
        </rdfs:subClassOf>
        <rdfs:comment>Represents ports that may be relevant for a cruise.</rdfs:comment>
        <rdfs:label>Port</rdfs:label>
    </owl:Class>
    <owl:Axiom>
        <owl:annotatedSource rdf:resource="http://schema.geolink.org/1.0/pattern/cruise#Port"/>
        <owl:annotatedProperty rdf:resource="http://www.w3.org/2000/01/rdf-schema#subClassOf"/>
        <owl:annotatedTarget>
            <owl:Restriction>
                <owl:onProperty rdf:resource="http://schema.geolink.org/1.0/pattern/cruise#r_Port"/>
                <owl:hasSelf rdf:datatype="http://www.w3.org/2001/XMLSchema#boolean">true</owl:hasSelf>
            </owl:Restriction>
        </owl:annotatedTarget>
        <DASE_RULE rdf:datatype="http://www.w3.org/2001/XMLSchema#string">R2___trajectory:hasPosition(?x,?y) ^ place:hasSpatialFootprint(?z,?y) ^ :Port(?z) -&gt; :atPort(?x,?z)___If position of a fix corresponds to a (spatial footprint of a) port, then that fix is at that port.___http://schema.geolink.org/1.0/pattern/cruise#freshObjectProperty1</DASE_RULE>
    </owl:Axiom>
    


    <!-- http://schema.geolink.org/1.0/pattern/vessel#Vessel -->

    <rdf:Description rdf:about="http://schema.geolink.org/1.0/pattern/vessel#Vessel">
        <rdfs:subClassOf rdf:resource="http://schema.geolink.org/1.0/pattern/trajectory#MovingObject"/>
    </rdf:Description>
    


    <!-- 
    ///////////////////////////////////////////////////////////////////////////////////////
    //
    // General axioms
    //
    ///////////////////////////////////////////////////////////////////////////////////////
     -->

    <owl:Class>
        <owl:intersectionOf rdf:parseType="Collection">
            <rdf:Description rdf:about="http://schema.geolink.org/1.0/pattern/trajectory#Fix"/>
            <owl:Restriction>
                <owl:onProperty rdf:resource="http://schema.geolink.org/1.0/pattern/cruise#atPort"/>
                <owl:someValuesFrom rdf:resource="http://schema.geolink.org/1.0/pattern/cruise#Port"/>
            </owl:Restriction>
        </owl:intersectionOf>
        <rdfs:subClassOf>
            <owl:Restriction>
                <owl:onProperty>
                    <rdf:Description>
                        <owl:inverseOf rdf:resource="http://schema.geolink.org/1.0/pattern/trajectory#hasFix"/>
                    </rdf:Description>
                </owl:onProperty>
                <owl:allValuesFrom rdf:resource="http://schema.geolink.org/1.0/pattern/cruise#CruiseTrajectory"/>
            </owl:Restriction>
        </rdfs:subClassOf>
    </owl:Class>
    <owl:Axiom>
        <owl:annotatedSource>
            <owl:Class>
                <owl:intersectionOf rdf:parseType="Collection">
                    <rdf:Description rdf:about="http://schema.geolink.org/1.0/pattern/trajectory#Fix"/>
                    <owl:Restriction>
                        <owl:onProperty>
                            <rdf:Description>
                                <owl:inverseOf rdf:resource="http://schema.geolink.org/1.0/pattern/trajectory#hasFix"/>
                            </rdf:Description>
                        </owl:onProperty>
                        <owl:someValuesFrom rdf:resource="http://schema.geolink.org/1.0/pattern/cruise#CruiseTrajectory"/>
                    </owl:Restriction>
                </owl:intersectionOf>
                <rdfs:subClassOf>
                    <owl:Restriction>
                        <owl:onProperty rdf:resource="http://schema.geolink.org/1.0/pattern/cruise#atPort"/>
                        <owl:allValuesFrom rdf:resource="http://schema.geolink.org/1.0/pattern/cruise#Port"/>
                    </owl:Restriction>
                </rdfs:subClassOf>
            </owl:Class>
        </owl:annotatedSource>
        <owl:annotatedProperty rdf:resource="http://www.w3.org/2000/01/rdf-schema#subClassOf"/>
        <owl:annotatedTarget>
            <owl:Restriction>
                <owl:onProperty rdf:resource="http://schema.geolink.org/1.0/pattern/cruise#atPort"/>
                <owl:allValuesFrom rdf:resource="http://schema.geolink.org/1.0/pattern/cruise#Port"/>
            </owl:Restriction>
        </owl:annotatedTarget>
        <rdfs:comment>Scoped range of atPort is Port where the scope is (inverse hasFix some CruiseTrajectory)</rdfs:comment>
    </owl:Axiom>
    <owl:Class>
        <owl:intersectionOf rdf:parseType="Collection">
            <rdf:Description rdf:about="http://schema.geolink.org/1.0/pattern/trajectory#Segment"/>
            <owl:Restriction>
                <owl:onProperty rdf:resource="http://schema.geolink.org/1.0/pattern/trajectory#traversedBy"/>
                <owl:someValuesFrom rdf:resource="http://schema.geolink.org/1.0/pattern/vessel#Vessel"/>
            </owl:Restriction>
        </owl:intersectionOf>
        <rdfs:subClassOf>
            <owl:Restriction>
                <owl:onProperty>
                    <rdf:Description>
                        <owl:inverseOf rdf:resource="http://schema.geolink.org/1.0/pattern/trajectory#hasSegment"/>
                    </rdf:Description>
                </owl:onProperty>
                <owl:allValuesFrom rdf:resource="http://schema.geolink.org/1.0/pattern/cruise#CruiseTrajectory"/>
            </owl:Restriction>
        </rdfs:subClassOf>
    </owl:Class>
    <owl:Axiom>
        <owl:annotatedSource>
            <owl:Class>
                <owl:intersectionOf rdf:parseType="Collection">
                    <rdf:Description rdf:about="http://schema.geolink.org/1.0/pattern/trajectory#Segment"/>
                    <owl:Restriction>
                        <owl:onProperty>
                            <rdf:Description>
                                <owl:inverseOf rdf:resource="http://schema.geolink.org/1.0/pattern/trajectory#hasSegment"/>
                            </rdf:Description>
                        </owl:onProperty>
                        <owl:someValuesFrom rdf:resource="http://schema.geolink.org/1.0/pattern/cruise#CruiseTrajectory"/>
                    </owl:Restriction>
                </owl:intersectionOf>
                <rdfs:subClassOf>
                    <owl:Restriction>
                        <owl:onProperty rdf:resource="http://schema.geolink.org/1.0/pattern/trajectory#traversedBy"/>
                        <owl:allValuesFrom rdf:resource="http://schema.geolink.org/1.0/pattern/vessel#Vessel"/>
                    </owl:Restriction>
                </rdfs:subClassOf>
            </owl:Class>
        </owl:annotatedSource>
        <owl:annotatedProperty rdf:resource="http://www.w3.org/2000/01/rdf-schema#subClassOf"/>
        <owl:annotatedTarget>
            <owl:Restriction>
                <owl:onProperty rdf:resource="http://schema.geolink.org/1.0/pattern/trajectory#traversedBy"/>
                <owl:allValuesFrom rdf:resource="http://schema.geolink.org/1.0/pattern/vessel#Vessel"/>
            </owl:Restriction>
        </owl:annotatedTarget>
        <rdfs:comment>Cruise trajectory&apos;s segments are traversed by a vessel</rdfs:comment>
    </owl:Axiom>
    <owl:Restriction>
        <owl:onProperty rdf:resource="http://schema.geolink.org/1.0/pattern/cruise#atPort"/>
        <owl:someValuesFrom rdf:resource="http://schema.geolink.org/1.0/pattern/cruise#Port"/>
        <rdfs:subClassOf rdf:resource="http://schema.geolink.org/1.0/pattern/trajectory#Fix"/>
    </owl:Restriction>
    <owl:Restriction>
        <owl:onProperty rdf:resource="http://schema.geolink.org/1.0/pattern/cruise#hasRelatedCruise"/>
        <owl:someValuesFrom rdf:resource="http://schema.geolink.org/1.0/pattern/cruise#Cruise"/>
        <rdfs:subClassOf rdf:resource="http://schema.geolink.org/1.0/pattern/cruise#Cruise"/>
    </owl:Restriction>
    <owl:Restriction>
        <owl:onProperty rdf:resource="http://schema.geolink.org/1.0/pattern/cruise#hasTrajectory"/>
        <owl:someValuesFrom rdf:resource="http://schema.geolink.org/1.0/pattern/cruise#CruiseTrajectory"/>
        <rdfs:subClassOf rdf:resource="http://schema.geolink.org/1.0/pattern/cruise#Cruise"/>
    </owl:Restriction>
    <owl:Restriction>
        <owl:onProperty rdf:resource="http://schema.geolink.org/1.0/pattern/cruise#traveledBy"/>
        <owl:someValuesFrom rdf:resource="http://schema.geolink.org/1.0/pattern/vessel#Vessel"/>
        <rdfs:subClassOf rdf:resource="http://schema.geolink.org/1.0/pattern/cruise#CruiseTrajectory"/>
    </owl:Restriction>
    <owl:Restriction>
        <owl:onProperty rdf:resource="http://schema.geolink.org/1.0/pattern/cruise#undertakenBy"/>
        <owl:someValuesFrom rdf:resource="http://schema.geolink.org/1.0/pattern/vessel#Vessel"/>
        <rdfs:subClassOf rdf:resource="http://schema.geolink.org/1.0/pattern/cruise#Cruise"/>
    </owl:Restriction>
    <rdf:Description>
        <rdf:type rdf:resource="http://www.w3.org/2002/07/owl#AllDisjointClasses"/>
        <owl:members rdf:parseType="Collection">
            <rdf:Description rdf:about="http://schema.geolink.org/1.0/pattern/agentrole#AgentRole"/>
            <rdf:Description rdf:about="http://schema.geolink.org/1.0/pattern/cruise#Cruise"/>
            <rdf:Description rdf:about="http://schema.geolink.org/1.0/pattern/cruise#CruiseTrajectory"/>
            <rdf:Description rdf:about="http://schema.geolink.org/1.0/pattern/cruise#Port"/>
            <rdf:Description rdf:about="http://schema.geolink.org/1.0/pattern/fundingaward#FundingAward"/>
            <rdf:Description rdf:about="http://schema.geolink.org/1.0/pattern/informationobject#InformationObject"/>
            <rdf:Description rdf:about="http://schema.geolink.org/1.0/pattern/program#Program"/>
            <rdf:Description rdf:about="http://schema.geolink.org/1.0/pattern/trajectory#Fix"/>
            <rdf:Description rdf:about="http://schema.geolink.org/1.0/pattern/trajectory#Position"/>
            <rdf:Description rdf:about="http://schema.geolink.org/1.0/pattern/trajectory#Segment"/>
            <rdf:Description rdf:about="http://schema.geolink.org/1.0/pattern/vessel#Vessel"/>
        </owl:members>
    </rdf:Description>
</rdf:RDF>



<!-- Generated by the OWL API (version 4.2.6.20160910-2108) https://github.com/owlcs/owlapi -->

