<?xml version="1.0" encoding="UTF-8"?><rdf:RDF xmlns:rdf="http://www.w3.org/1999/02/22-rdf-syntax-ns#" xmlns:skos="http://www.w3.org/2004/02/skos/core#" xmlns:dc="http://purl.org/dc/terms/" xmlns:rdfs="http://www.w3.org/2000/01/rdf-schema#" xmlns:grg="http://www.isotc211.org/schemas/grg/" xmlns:owl="http://www.w3.org/2002/07/owl#" xmlns:void="http://rdfs.org/ns/void#">
<skos:Collection rdf:about="http://vocab.nerc.ac.uk/collection/L22/current/">
<skos:prefLabel>SeaVoX Device Catalogue</skos:prefLabel>
<dc:title>SeaVoX Device Catalogue</dc:title>
<skos:altLabel>SeaVoX Device Catalogue</skos:altLabel>
<dc:alternative>SeaVoX Device Catalogue</dc:alternative>
<dc:description>Terms for distinct sampling or measuring devices that may be identified in the real world in terms of manufacturer and model number.</dc:description>
<dc:date>2014-02-15 02:00:02.0</dc:date>
<owl:versionInfo>152</owl:versionInfo>
<grg:RE_RegisterManager>British Oceanographic Data Centre</grg:RE_RegisterManager>
<dc:publisher>Natural Environment Research Council</dc:publisher>
<dc:creator>SeaDataNet and MarineXML Vocabulary Content Governance Group</dc:creator>
<grg:RE_RegisterOwner>SeaDataNet and MarineXML Vocabulary Content Governance Group</grg:RE_RegisterOwner>
<rdfs:comment>Group set up under the joint auspices of the SeaDataNet project and the Intergovernmental Oceanographic Commission MarineXML Steering Group for controlled vocabulary governance in the marine domain</rdfs:comment>
<skos:member>
<skos:Concept rdf:about="http://vocab.nerc.ac.uk/collection/L22/current/TOOL0292/">
<dc:identifier>SDN:L22::TOOL0292</dc:identifier>
<skos:notation>SDN:L22::TOOL0292</skos:notation>
<skos:prefLabel xml:lang="en">ASL Environmental Sciences IPS4 Ice Profiler Sonar</skos:prefLabel>
<skos:altLabel>ASL IPS4 ice profiler</skos:altLabel>
<skos:definition xml:lang="en">The ASL Environmental Sciences ISP4 is an upward looking sonar device for measuring ice keel drafts. Distance between the instrument and ice keel is measured by sonar at an operating frequency of 420 kHz with a beam width of 1.8 degrees and sampling rate of up to 2Hz. Water depth is measured by a pressure sensor and ice draft is calculated by difference. It has a depth range of 175 metres in ice or 225 metres in water and a precision of 0.05 metres.</skos:definition>
<owl:versionInfo>2</owl:versionInfo>
<dc:date>2010-11-18 12:39:41.0</dc:date>
<skos:note xml:lang="en">accepted</skos:note>
<owl:deprecated>false</owl:deprecated>
<skos:broader rdf:resource="http://vocab.nerc.ac.uk/collection/L05/current/ICEP/"/>
<void:inDataset rdf:resource="http://vocab.nerc.ac.uk/.well-known/void"/>
</skos:Concept>
</skos:member>
<skos:member>
<skos:Concept rdf:about="http://vocab.nerc.ac.uk/collection/L22/current/TOOL0590/">
<dc:identifier>SDN:L22::TOOL0590</dc:identifier>
<skos:notation>SDN:L22::TOOL0590</skos:notation>
<skos:prefLabel xml:lang="en">Aanderaa CTR7 thermistor conductivity chain</skos:prefLabel>
<skos:altLabel>AA CTR7 TC chain</skos:altLabel>
<skos:definition xml:lang="en">An instrument with up to 5 induction conductivity and thermistor temperature sensor pairs along a string held vertically in the water column and connected to a 12-channel Aanderaa DL7 data logger. The twelfth channel may be used for an optional pressure sensor housed in one of the senor pairs Overall accuracy (+/-) 0.1C for temperature and 0.3 mS/cm for conductivity.  Further information may be found in http://www.bodc.ac.uk/data/documents/nodb/78767/.</skos:definition>
<owl:versionInfo>1</owl:versionInfo>
<dc:date>2013-01-17 10:07:40.0</dc:date>
<skos:note xml:lang="en">accepted</skos:note>
<owl:deprecated>false</owl:deprecated>
<skos:broader rdf:resource="http://vocab.nerc.ac.uk/collection/L05/current/134/"/>
<skos:broader rdf:resource="http://vocab.nerc.ac.uk/collection/L05/current/135/"/>
<void:inDataset rdf:resource="http://vocab.nerc.ac.uk/.well-known/void"/>
</skos:Concept>
</skos:member>
<skos:member>
<skos:Concept rdf:about="http://vocab.nerc.ac.uk/collection/L22/current/TOOL0103/">
<dc:identifier>SDN:L22::TOOL0103</dc:identifier>
<skos:notation>SDN:L22::TOOL0103</skos:notation>
<skos:prefLabel xml:lang="en">Aanderaa Oxygen Optode 3835</skos:prefLabel>
<skos:altLabel>AA Optode 3835</skos:altLabel>
<skos:definition xml:lang="en">A dissolved oxygen sensor primarily designed to mount on RCM 9 or RDCP 600 or similat OEM applications. Measurement based on the ability of selected substances to act as dynamic fluorescence quenchers. The fluorescent indicator is a special platinum porphyrin complex embedded in a gas permeable foil that is exposed to the surrounding water. A black optical isolation coating protects the complex from sunlight and fluorescent particles in the water. This sensing foil is attached to a window providing optical access for the measuring system from inside a watertight titanium housing.The foil is excited by modulated blue light, and the phase of a returned red light is measured. By linearizing and temperature compensating, with an incorporated temperature sensor, the absolute O2 concentration can be determined.</skos:definition>
<owl:versionInfo>1</owl:versionInfo>
<dc:date>2010-05-18 16:10:58.0</dc:date>
<skos:note xml:lang="en">accepted</skos:note>
<owl:deprecated>false</owl:deprecated>
<skos:broader rdf:resource="http://vocab.nerc.ac.uk/collection/L05/current/351/"/>
<void:inDataset rdf:resource="http://vocab.nerc.ac.uk/.well-known/void"/>
</skos:Concept>
</skos:member>
<skos:member>
<skos:Concept rdf:about="http://vocab.nerc.ac.uk/collection/L22/current/TOOL0369/">
<dc:identifier>SDN:L22::TOOL0369</dc:identifier>
<skos:notation>SDN:L22::TOOL0369</skos:notation>
<skos:prefLabel xml:lang="en">Aanderaa Oxygen Optode 3975</skos:prefLabel>
<skos:altLabel>AA Optode 3975</skos:altLabel>
<skos:definition xml:lang="en">A dissolved oxygen sensor which provides analogue output to third party data loggers. Measurement is based on the ability of selected substances to act as dynamic fluorescence quenchers. The fluorescent indicator is a special platinum porphyrin complex embedded in a gas permeable foil that is exposed to the surrounding water. A black optical isolation coating protects the complex from sunlight and fluorescent particles in the water. This sensing foil is attached to a window providing optical access for the measuring system from inside a watertight titanium housing.The foil is excited by modulated blue light, and the phase of a returned red light is measured. By linearizing and temperature compensating, with an incorporated temperature sensor, the absolute O2 concentration can be determined.</skos:definition>
<owl:versionInfo>1</owl:versionInfo>
<dc:date>2011-02-09 11:25:51.0</dc:date>
<skos:note xml:lang="en">accepted</skos:note>
<owl:deprecated>false</owl:deprecated>
<skos:broader rdf:resource="http://vocab.nerc.ac.uk/collection/L05/current/351/"/>
<void:inDataset rdf:resource="http://vocab.nerc.ac.uk/.well-known/void"/>
</skos:Concept>
</skos:member>
<skos:member>
<skos:Concept rdf:about="http://vocab.nerc.ac.uk/collection/L22/current/TOOL0102/">
<dc:identifier>SDN:L22::TOOL0102</dc:identifier>
<skos:notation>SDN:L22::TOOL0102</skos:notation>
<skos:prefLabel xml:lang="en">Aanderaa Oxygen Optode 4130</skos:prefLabel>
<skos:altLabel>AA Optode 4130</skos:altLabel>
<skos:definition xml:lang="en">A dissolved oxygen sensor for use with Aanderaa data loggers. Measurement based on the ability of selected substances to act as dynamic fluorescence quenchers. The fluorescent indicator is a special platinum porphyrin complex embedded in a gas permeable foil that is exposed to the surrounding water. A black optical isolation coating protects the complex from sunlight and fluorescent particles in the water. This sensing foil is attached to a window providing optical access for the measuring system from inside a watertight titanium housing.The foil is excited by modulated blue light, and the phase of a returned red light is measured. By linearizing and temperature compensating, with an incorporated temperature sensor, the absolute O2 concentration can be determined.</skos:definition>
<owl:versionInfo>1</owl:versionInfo>
<dc:date>2010-05-18 16:10:58.0</dc:date>
<skos:note xml:lang="en">accepted</skos:note>
<owl:deprecated>false</owl:deprecated>
<skos:broader rdf:resource="http://vocab.nerc.ac.uk/collection/L05/current/351/"/>
<void:inDataset rdf:resource="http://vocab.nerc.ac.uk/.well-known/void"/>
</skos:Concept>
</skos:member>
<skos:member>
<skos:Concept rdf:about="http://vocab.nerc.ac.uk/collection/L22/current/TOOL0101/">
<dc:identifier>SDN:L22::TOOL0101</dc:identifier>
<skos:notation>SDN:L22::TOOL0101</skos:notation>
<skos:prefLabel xml:lang="en">Aanderaa Oxygen Optode 4175</skos:prefLabel>
<skos:altLabel>AA Optode 4175</skos:altLabel>
<skos:definition xml:lang="en">A dissolved oxygen sensor for OEM applications. Measurement based on the ability of selected substances to act as dynamic fluorescence quenchers. The fluorescent indicator is a special platinum porphyrin complex embedded in a gas permeable foil that is exposed to the surrounding water. A black optical isolation coating protects the complex from sunlight and fluorescent particles in the water. This sensing foil is attached to a window providing optical access for the measuring system from inside a watertight titanium housing.The foil is excited by modulated blue light, and the phase of a returned red light is measured. By linearizing and temperature compensating, with an incorporated temperature sensor, the absolute O2 concentration can be determined. Further information may be found on the BODC document server at URL: http://www.bodc.ac.uk/data/documents/nodb/119483/.</skos:definition>
<owl:versionInfo>2</owl:versionInfo>
<dc:date>2010-11-18 12:39:41.0</dc:date>
<skos:note xml:lang="en">accepted</skos:note>
<owl:deprecated>false</owl:deprecated>
<skos:broader rdf:resource="http://vocab.nerc.ac.uk/collection/L05/current/351/"/>
<void:inDataset rdf:resource="http://vocab.nerc.ac.uk/.well-known/void"/>
</skos:Concept>
</skos:member>
<skos:member>
<skos:Concept rdf:about="http://vocab.nerc.ac.uk/collection/L22/current/TOOL0026/">
<dc:identifier>SDN:L22::TOOL0026</dc:identifier>
<skos:notation>SDN:L22::TOOL0026</skos:notation>
<skos:prefLabel xml:lang="en">Aanderaa RCM 11 Recording Current Meter</skos:prefLabel>
<skos:altLabel>RCM 11</skos:altLabel>
<skos:definition xml:lang="en">The RCM 11 is a single-point doppler recording current meter pressure cased to operate at depths of up to 6000 metres. Further information may be found on the BODC document server at URL http://www.bodc.ac.uk/data/documents/nodb/106028/</skos:definition>
<owl:versionInfo>1</owl:versionInfo>
<dc:date>2010-09-07 11:22:02.0</dc:date>
<skos:note xml:lang="en">accepted</skos:note>
<owl:deprecated>false</owl:deprecated>
<skos:broader rdf:resource="http://vocab.nerc.ac.uk/collection/L05/current/114/"/>
<void:inDataset rdf:resource="http://vocab.nerc.ac.uk/.well-known/void"/>
</skos:Concept>
</skos:member>
<skos:member>
<skos:Concept rdf:about="http://vocab.nerc.ac.uk/collection/L22/current/TOOL0211/">
<dc:identifier>SDN:L22::TOOL0211</dc:identifier>
<skos:notation>SDN:L22::TOOL0211</skos:notation>
<skos:prefLabel xml:lang="en">Aanderaa RCM 4/5 Recording Current Meter</skos:prefLabel>
<skos:altLabel>RCM 4/5</skos:altLabel>
<skos:definition xml:lang="en">Family of self-recording current meters with Savonius Rotors recording averaged speed and a magnetic compass recording spot directions. The meter has a balanced weight vane which aligns it with the current flow and is mounted using shackles between segments of mooring line. Optional temperature, pressure and conductivity sensors may be fitted. The RCM5 has a strengthened casing allowing deployment to 6000m. For more details see http://www.bodc.ac.uk/data/documents/nodb/4872/</skos:definition>
<owl:versionInfo>2</owl:versionInfo>
<dc:date>2010-11-18 12:39:41.0</dc:date>
<skos:note xml:lang="en">accepted</skos:note>
<owl:deprecated>false</owl:deprecated>
<skos:broader rdf:resource="http://vocab.nerc.ac.uk/collection/L05/current/114/"/>
<void:inDataset rdf:resource="http://vocab.nerc.ac.uk/.well-known/void"/>
</skos:Concept>
</skos:member>
<skos:member>
<skos:Concept rdf:about="http://vocab.nerc.ac.uk/collection/L22/current/TOOL0212/">
<dc:identifier>SDN:L22::TOOL0212</dc:identifier>
<skos:notation>SDN:L22::TOOL0212</skos:notation>
<skos:prefLabel xml:lang="en">Aanderaa RCM 4/5 temperature and salinity recorders</skos:prefLabel>
<skos:altLabel>RCM 4/5 TS</skos:altLabel>
<skos:definition xml:lang="en">Withdrawn RCM4 or RCM5 current meters fitted with conductivity and temperature sensors given a new lease of life as temperature and salinity recorders.</skos:definition>
<owl:versionInfo>1</owl:versionInfo>
<dc:date>2010-05-18 16:10:58.0</dc:date>
<skos:note xml:lang="en">accepted</skos:note>
<owl:deprecated>false</owl:deprecated>
<skos:broader rdf:resource="http://vocab.nerc.ac.uk/collection/L05/current/350/"/>
<skos:broader rdf:resource="http://vocab.nerc.ac.uk/collection/L05/current/134/"/>
<void:inDataset rdf:resource="http://vocab.nerc.ac.uk/.well-known/void"/>
</skos:Concept>
</skos:member>
<skos:member>
<skos:Concept rdf:about="http://vocab.nerc.ac.uk/collection/L22/current/TOOL0121/">
<dc:identifier>SDN:L22::TOOL0121</dc:identifier>
<skos:notation>SDN:L22::TOOL0121</skos:notation>
<skos:prefLabel xml:lang="en">Aanderaa RCM 7/8 Recording Current Meter</skos:prefLabel>
<skos:altLabel>RCM 7/8</skos:altLabel>
<skos:definition xml:lang="en">Family of self-recording paddle wheel current meters with different pressure cases that record the vector averaged speed and direction over a sampling interval. The paddle wheel rotor is magnetically coupled to an electronic counter. The meter has a balanced weight vane which aligns it with the current flow. For more details see http://www.bodc.ac.uk/data/documents/nodb/65611/.</skos:definition>
<owl:versionInfo>1</owl:versionInfo>
<dc:date>2010-05-18 16:10:58.0</dc:date>
<skos:note xml:lang="en">accepted</skos:note>
<owl:deprecated>false</owl:deprecated>
<skos:related rdf:resource="http://vocab.nerc.ac.uk/collection/P01/current/LCSAEL01/"/>
<skos:related rdf:resource="http://vocab.nerc.ac.uk/collection/P01/current/PREXPS01/"/>
<skos:related rdf:resource="http://vocab.nerc.ac.uk/collection/P01/current/PSALPR01/"/>
<skos:related rdf:resource="http://vocab.nerc.ac.uk/collection/P01/current/CNDCPR01/"/>
<skos:related rdf:resource="http://vocab.nerc.ac.uk/collection/P01/current/TEMPPR01/"/>
<skos:related rdf:resource="http://vocab.nerc.ac.uk/collection/P01/current/LCDAEL01/"/>
<skos:related rdf:resource="http://vocab.nerc.ac.uk/collection/P01/current/PREXPR01/"/>
<skos:broader rdf:resource="http://vocab.nerc.ac.uk/collection/L05/current/114/"/>
<void:inDataset rdf:resource="http://vocab.nerc.ac.uk/.well-known/void"/>
</skos:Concept>
</skos:member>
<skos:member>
<skos:Concept rdf:about="http://vocab.nerc.ac.uk/collection/L22/current/TOOL0028/">
<dc:identifier>SDN:L22::TOOL0028</dc:identifier>
<skos:notation>SDN:L22::TOOL0028</skos:notation>
<skos:prefLabel xml:lang="en">Aanderaa RCM 9 IW Recording Current Meter</skos:prefLabel>
<skos:altLabel>RCM 9 IW</skos:altLabel>
<skos:definition xml:lang="en">The RCM 9 IW is a single-point doppler recording current meter with a medium weight case to operate at depths of up to 2000 metres. Further information may be found on the BODC document server at URL http://www.bodc.ac.uk/data/documents/nodb/106028/</skos:definition>
<owl:versionInfo>1</owl:versionInfo>
<dc:date>2010-09-07 11:26:56.0</dc:date>
<skos:note xml:lang="en">accepted</skos:note>
<owl:deprecated>false</owl:deprecated>
<skos:broader rdf:resource="http://vocab.nerc.ac.uk/collection/L05/current/114/"/>
<void:inDataset rdf:resource="http://vocab.nerc.ac.uk/.well-known/void"/>
</skos:Concept>
</skos:member>
<skos:member>
<skos:Concept rdf:about="http://vocab.nerc.ac.uk/collection/L22/current/TOOL0027/">
<dc:identifier>SDN:L22::TOOL0027</dc:identifier>
<skos:notation>SDN:L22::TOOL0027</skos:notation>
<skos:prefLabel xml:lang="en">Aanderaa RCM 9 LW Recording Current Meter</skos:prefLabel>
<skos:altLabel>RCM 9 LW</skos:altLabel>
<skos:definition xml:lang="en">The RCM 9 LW is a single-point doppler recording current meter with a lightweight case to operate at depths of up to 300 metres. Further information may be found on the BODC document server at URL http://www.bodc.ac.uk/data/documents/nodb/106028/</skos:definition>
<owl:versionInfo>1</owl:versionInfo>
<dc:date>2010-09-07 11:25:23.0</dc:date>
<skos:note xml:lang="en">accepted</skos:note>
<owl:deprecated>false</owl:deprecated>
<skos:broader rdf:resource="http://vocab.nerc.ac.uk/collection/L05/current/114/"/>
<void:inDataset rdf:resource="http://vocab.nerc.ac.uk/.well-known/void"/>
</skos:Concept>
</skos:member>
<skos:member>
<skos:Concept rdf:about="http://vocab.nerc.ac.uk/collection/L22/current/TOOL0029/">
<dc:identifier>SDN:L22::TOOL0029</dc:identifier>
<skos:notation>SDN:L22::TOOL0029</skos:notation>
<skos:prefLabel xml:lang="en">Aanderaa RCM 9/11 Recording Current Meter</skos:prefLabel>
<skos:altLabel>RCM 9/11</skos:altLabel>
<skos:definition xml:lang="en">The RCM 9/11 a family of single-point doppler recording current meter with a different casing options to allow working at depths of up to 300 (RCM 9 LW), 2000 (RCM 9 IW) or 6000 (RCM 11) metres. Further information may be found on the BODC document server at URL http://www.bodc.ac.uk/data/documents/nodb/106028/</skos:definition>
<owl:versionInfo>1</owl:versionInfo>
<dc:date>2009-11-30 11:56:35.0</dc:date>
<skos:note xml:lang="en">accepted</skos:note>
<owl:deprecated>false</owl:deprecated>
<skos:broader rdf:resource="http://vocab.nerc.ac.uk/collection/L05/current/114/"/>
<skos:broader rdf:resource="http://vocab.nerc.ac.uk/collection/L05/current/134/"/>
<void:inDataset rdf:resource="http://vocab.nerc.ac.uk/.well-known/void"/>
</skos:Concept>
</skos:member>
<skos:member>
<skos:Concept rdf:about="http://vocab.nerc.ac.uk/collection/L22/current/TOOL0166/">
<dc:identifier>SDN:L22::TOOL0166</dc:identifier>
<skos:notation>SDN:L22::TOOL0166</skos:notation>
<skos:prefLabel xml:lang="en">Aanderaa RDCP 600 Recording Doppler Current Profiler</skos:prefLabel>
<skos:altLabel>Aanderaa RDCP 600</skos:altLabel>
<skos:definition xml:lang="en">The RDCP 600 is a medium range, 600kHz self-recording Doppler Current Profiler. The standard RDCP 600 can be deployed to a depth of 300m, with a velocity range of 0-500 cm/s, vertical velocity accuracy of 1.0 cm/s and horizontal velocity accuracy of 0.5cm/s.</skos:definition>
<owl:versionInfo>1</owl:versionInfo>
<dc:date>2010-05-18 16:10:58.0</dc:date>
<skos:note xml:lang="en">accepted</skos:note>
<owl:deprecated>false</owl:deprecated>
<skos:broader rdf:resource="http://vocab.nerc.ac.uk/collection/L05/current/115/"/>
<void:inDataset rdf:resource="http://vocab.nerc.ac.uk/.well-known/void"/>
</skos:Concept>
</skos:member>
<skos:member>
<skos:Concept rdf:about="http://vocab.nerc.ac.uk/collection/L22/current/TOOL0306/">
<dc:identifier>SDN:L22::TOOL0306</dc:identifier>
<skos:notation>SDN:L22::TOOL0306</skos:notation>
<skos:prefLabel xml:lang="en">Aanderaa Seaguard Recording Current Meter</skos:prefLabel>
<skos:altLabel>Aanderaa Seaguard RCM</skos:altLabel>
<skos:definition xml:lang="en">A multi-frequency Doppler current sensor for measuring horizontal current speed and direction. The shallow water (SW), intermediate water (IW) and deep water (DW) models can be deployed to 300 m, 2000 m and 6000 m, respectively. The instrument has a maximum sampling rate of 0.5 Hz, a velocity range of 0 – 300 cm s-1, and incorporates an electronic compass and a tilt sensor. A number of additional oceanographic sensors may also be attached. Further details can be found at http://www.bodc.ac.uk/data/documents/nodb/pdf/Aanderaa_Seaguard_RCM.pdf</skos:definition>
<owl:versionInfo>1</owl:versionInfo>
<dc:date>2010-09-06 12:45:22.0</dc:date>
<skos:note xml:lang="en">accepted</skos:note>
<owl:deprecated>false</owl:deprecated>
<skos:broader rdf:resource="http://vocab.nerc.ac.uk/collection/L05/current/114/"/>
<void:inDataset rdf:resource="http://vocab.nerc.ac.uk/.well-known/void"/>
</skos:Concept>
</skos:member>
<skos:member>
<skos:Concept rdf:about="http://vocab.nerc.ac.uk/collection/L22/current/TOOL0629/">
<dc:identifier>SDN:L22::TOOL0629</dc:identifier>
<skos:notation>SDN:L22::TOOL0629</skos:notation>
<skos:prefLabel xml:lang="en">Aanderaa WLR 5 Water Level Recorder</skos:prefLabel>
<skos:altLabel>WLR 5</skos:altLabel>
<skos:definition xml:lang="en">A bottom pressure recorder for measuring sea level in shallow waters with optional Fenwall thermistor temperature sensor logging to an internal magnetic tape unit. More information is available in http://www.bodc.ac.uk/data/documents/nodb/67867/.</skos:definition>
<owl:versionInfo>1</owl:versionInfo>
<dc:date>2013-07-25 15:31:48.0</dc:date>
<skos:note xml:lang="en">accepted</skos:note>
<owl:deprecated>false</owl:deprecated>
<skos:broader rdf:resource="http://vocab.nerc.ac.uk/collection/L05/current/111/"/>
<skos:broader rdf:resource="http://vocab.nerc.ac.uk/collection/L05/current/134/"/>
<void:inDataset rdf:resource="http://vocab.nerc.ac.uk/.well-known/void"/>
</skos:Concept>
</skos:member>
<skos:member>
<skos:Concept rdf:about="http://vocab.nerc.ac.uk/collection/L22/current/TOOL0031/">
<dc:identifier>SDN:L22::TOOL0031</dc:identifier>
<skos:notation>SDN:L22::TOOL0031</skos:notation>
<skos:prefLabel xml:lang="en">Aanderaa WLR 7 Water Level Recorder</skos:prefLabel>
<skos:altLabel>WLR 7</skos:altLabel>
<skos:definition xml:lang="en">A bottom pressure recorder for measuring sea level in shallow waters with optional Fenwall thermistor temperature sensor logging to an internal solid-state data storage unit. More information is available in http://www.bodc.ac.uk/data/documents/nodb/225584/.</skos:definition>
<owl:versionInfo>2</owl:versionInfo>
<dc:date>2013-07-25 16:07:40.0</dc:date>
<skos:note xml:lang="en">accepted</skos:note>
<owl:deprecated>false</owl:deprecated>
<skos:broader rdf:resource="http://vocab.nerc.ac.uk/collection/L05/current/111/"/>
<skos:broader rdf:resource="http://vocab.nerc.ac.uk/collection/L05/current/134/"/>
<void:inDataset rdf:resource="http://vocab.nerc.ac.uk/.well-known/void"/>
</skos:Concept>
</skos:member>
<skos:member>
<skos:Concept rdf:about="http://vocab.nerc.ac.uk/collection/L22/current/TOOL0030/">
<dc:identifier>SDN:L22::TOOL0030</dc:identifier>
<skos:notation>SDN:L22::TOOL0030</skos:notation>
<skos:prefLabel xml:lang="en">Aanderaa WLR 8 Water Level Recorder</skos:prefLabel>
<skos:altLabel>WLR 8</skos:altLabel>
<skos:definition xml:lang="en">The WLR 8 is a bottom pressure recorder recording sea level with deployment depths of up to 6000 metres. Further information may be found on the BODC document server at URL http://www.bodc.ac.uk/data/documents/nodb/135903/</skos:definition>
<owl:versionInfo>1</owl:versionInfo>
<dc:date>2009-11-30 11:56:35.0</dc:date>
<skos:note xml:lang="en">accepted</skos:note>
<owl:deprecated>false</owl:deprecated>
<skos:broader rdf:resource="http://vocab.nerc.ac.uk/collection/L05/current/134/"/>
<skos:broader rdf:resource="http://vocab.nerc.ac.uk/collection/L05/current/111/"/>
<void:inDataset rdf:resource="http://vocab.nerc.ac.uk/.well-known/void"/>
</skos:Concept>
</skos:member>
<skos:member>
<skos:Concept rdf:about="http://vocab.nerc.ac.uk/collection/L22/current/TOOL0498/">
<dc:identifier>SDN:L22::TOOL0498</dc:identifier>
<skos:notation>SDN:L22::TOOL0498</skos:notation>
<skos:prefLabel xml:lang="en">Aanderaa conductivity sensor 3919A</skos:prefLabel>
<skos:altLabel>Aanderaa 3919A cond sensor</skos:altLabel>
<skos:definition xml:lang="en">An inductive conductivity sensor designed to operate over a range of 0-7.5 S/m with a resolution of 0.0002 S/m and an accuracy of +/- 0.005 S/m. The instrument includes a temperature sensor with a range of -5 to 40 degC, a resolution of 0.01 degC and an accuracy of +/-0.1 degC. The shallow water (SW) version of the instrument is rated to 300 m, the intermediate water (IW) version to 2000 m and the deep water (DW) version to 6000 m. The instrument has a titanium casing and can be interfaced with the Aanderaa RCM9/11 or RDCP, or used for standalone operations.</skos:definition>
<owl:versionInfo>1</owl:versionInfo>
<dc:date>2012-06-13 14:30:27.0</dc:date>
<skos:note xml:lang="en">accepted</skos:note>
<owl:deprecated>false</owl:deprecated>
<skos:broader rdf:resource="http://vocab.nerc.ac.uk/collection/L05/current/350/"/>
<void:inDataset rdf:resource="http://vocab.nerc.ac.uk/.well-known/void"/>
</skos:Concept>
</skos:member>
<skos:member>
<skos:Concept rdf:about="http://vocab.nerc.ac.uk/collection/L22/current/TOOL0499/">
<dc:identifier>SDN:L22::TOOL0499</dc:identifier>
<skos:notation>SDN:L22::TOOL0499</skos:notation>
<skos:prefLabel xml:lang="en">Aanderaa conductivity sensor 3919B</skos:prefLabel>
<skos:altLabel>Aanderaa 3919B cond sensor</skos:altLabel>
<skos:definition xml:lang="en">An inductive conductivity sensor designed to operate over a range of 0-7.5 S/m with a resolution of 0.0002 S/m and an accuracy of +/- 0.0018 S/m. The instrument includes a temperature sensor with a range of -5 to 40 degC, a resolution of 0.01 degC and an accuracy of +/-0.1 degC. The shallow water (SW) version of the instrument is rated to 300 m, the intermediate water (IW) version to 2000 m and the deep water (DW) version to 6000 m. The instrument has a titanium casing and can be interfaced with the Aanderaa RCM9/11 or RDCP, or used for standalone operations.</skos:definition>
<owl:versionInfo>1</owl:versionInfo>
<dc:date>2012-06-13 14:30:27.0</dc:date>
<skos:note xml:lang="en">accepted</skos:note>
<owl:deprecated>false</owl:deprecated>
<skos:broader rdf:resource="http://vocab.nerc.ac.uk/collection/L05/current/350/"/>
<void:inDataset rdf:resource="http://vocab.nerc.ac.uk/.well-known/void"/>
</skos:Concept>
</skos:member>
<skos:member>
<skos:Concept rdf:about="http://vocab.nerc.ac.uk/collection/L22/current/TOOL0626/">
<dc:identifier>SDN:L22::TOOL0626</dc:identifier>
<skos:notation>SDN:L22::TOOL0626</skos:notation>
<skos:prefLabel xml:lang="en">Aanderaa conductivity sensor 4319A</skos:prefLabel>
<skos:altLabel>Aanderaa 4319A</skos:altLabel>
<skos:definition xml:lang="en">An inductive conductivity sensor designed to operate over a range of 0-7.5 S/m with a resolution of 0.0002 S/m and an accuracy of +/- 0.005 S/m. The instrument includes a temperature sensor with a range of -5 to 40 degC, a resolution of 0.01 degC and an accuracy of +/-0.1 degC. The shallow water (SW) version of the instrument is rated to 300 m, the intermediate water (IW) version to 2000 m and the deep water (DW) version to 6000 m. The instrument has a titanium casing and can be interfaced with the Aanderaa RCM9/11 or RDCP, or used for standalone operations. Unlike the Aanderaa 3919A, the 4319A incorporates SmartGuard data logger connectivity, and updated AADI protocol.</skos:definition>
<owl:versionInfo>1</owl:versionInfo>
<dc:date>2013-06-12 15:42:34.0</dc:date>
<skos:note xml:lang="en">accepted</skos:note>
<owl:deprecated>false</owl:deprecated>
<skos:broader rdf:resource="http://vocab.nerc.ac.uk/collection/L05/current/350/"/>
<void:inDataset rdf:resource="http://vocab.nerc.ac.uk/.well-known/void"/>
</skos:Concept>
</skos:member>
<skos:member>
<skos:Concept rdf:about="http://vocab.nerc.ac.uk/collection/L22/current/TOOL0627/">
<dc:identifier>SDN:L22::TOOL0627</dc:identifier>
<skos:notation>SDN:L22::TOOL0627</skos:notation>
<skos:prefLabel xml:lang="en">Aanderaa conductivity sensor 4319B</skos:prefLabel>
<skos:altLabel>Aanderaa 4319B</skos:altLabel>
<skos:definition xml:lang="en">An inductive conductivity sensor designed to operate over a range of 0-7.5 S/m with a resolution of 0.0002 S/m and an accuracy of +/- 0.0018 S/m. The instrument includes a temperature sensor with a range of -5 to 40 degC, a resolution of 0.01 degC and an accuracy of +/-0.1 degC. The shallow water (SW) version of the instrument is rated to 300 m, the intermediate water (IW) version to 2000 m and the deep water (DW) version to 6000 m. The instrument has a titanium casing and can be interfaced with the Aanderaa RCM9/11 or RDCP, or used for standalone operations. Unlike the Aanderaa 3919A, the 4319A incorporates SmartGuard data logger connectivity, and updated AADI protocol.</skos:definition>
<owl:versionInfo>1</owl:versionInfo>
<dc:date>2013-06-12 15:43:27.0</dc:date>
<skos:note xml:lang="en">accepted</skos:note>
<owl:deprecated>false</owl:deprecated>
<skos:broader rdf:resource="http://vocab.nerc.ac.uk/collection/L05/current/350/"/>
<void:inDataset rdf:resource="http://vocab.nerc.ac.uk/.well-known/void"/>
</skos:Concept>
</skos:member>
<skos:member>
<skos:Concept rdf:about="http://vocab.nerc.ac.uk/collection/L22/current/TOOL0171/">
<dc:identifier>SDN:L22::TOOL0171</dc:identifier>
<skos:notation>SDN:L22::TOOL0171</skos:notation>
<skos:prefLabel xml:lang="en">Aanderaa doppler current sensor 4100</skos:prefLabel>
<skos:altLabel>AA current sensor 4100</skos:altLabel>
<skos:definition xml:lang="en">A 2 MHz vector averaging sensor for measuring current speed and direction. It can be deployed to a depth of 300 m, with a velocity range of 0-300 cm/s and a velocity accuracy of 0.15 cm/s. It has a directional accuracy of 5° for 0-15° tilt and 7.5° for 15-35° tilt. 4100R model also available with adjustable ping rate.</skos:definition>
<owl:versionInfo>1</owl:versionInfo>
<dc:date>2010-05-18 16:10:58.0</dc:date>
<skos:note xml:lang="en">accepted</skos:note>
<owl:deprecated>false</owl:deprecated>
<skos:broader rdf:resource="http://vocab.nerc.ac.uk/collection/L05/current/114/"/>
<void:inDataset rdf:resource="http://vocab.nerc.ac.uk/.well-known/void"/>
</skos:Concept>
</skos:member>
<skos:member>
<skos:Concept rdf:about="http://vocab.nerc.ac.uk/collection/L22/current/TOOL0589/">
<dc:identifier>SDN:L22::TOOL0589</dc:identifier>
<skos:notation>SDN:L22::TOOL0589</skos:notation>
<skos:prefLabel xml:lang="en">Aanderaa thermistor chain</skos:prefLabel>
<skos:altLabel>AA T chain</skos:altLabel>
<skos:definition xml:lang="en">An instrument with 11 Fenwal 2K iso-curve thermistors mounted along a string from 10 to 400m long held vertically in the water column and connected to a 12-channel Aanderaa TR or SeaData data logger rated to 2000m depth.  The twelfth channel was used for an internal reference number,  a Bourdon tube pressure sensor (Aanderaa) or an additional thermistor (SeaData) housed in the logger.  Overall accuracy (+/-) is between 0.1 and 0.2C.  Further information may be found in http://www.bodc.ac.uk/data/documents/nodb/67001/.</skos:definition>
<owl:versionInfo>1</owl:versionInfo>
<dc:date>2013-01-17 10:07:40.0</dc:date>
<skos:note xml:lang="en">accepted</skos:note>
<owl:deprecated>false</owl:deprecated>
<skos:broader rdf:resource="http://vocab.nerc.ac.uk/collection/L05/current/135/"/>
<skos:broader rdf:resource="http://vocab.nerc.ac.uk/collection/L05/current/134/"/>
<skos:broader rdf:resource="http://vocab.nerc.ac.uk/collection/L05/current/350/"/>
<void:inDataset rdf:resource="http://vocab.nerc.ac.uk/.well-known/void"/>
</skos:Concept>
</skos:member>
<skos:member>
<skos:Concept rdf:about="http://vocab.nerc.ac.uk/collection/L22/current/NETT0001/">
<dc:identifier>SDN:L22::NETT0001</dc:identifier>
<skos:notation>SDN:L22::NETT0001</skos:notation>
<skos:prefLabel xml:lang="en">Adriatic plankton sampler - Krsinic (1990)</skos:prefLabel>
<skos:altLabel>Adriatic plankton sampler</skos:altLabel>
<skos:definition xml:lang="en">Construction is a 50 cm diameter cylindrical sampler sent to depth with the cylinder net (0.25 mm mesh) closed and upside down (cod-end facing upward). A messenger releases the bottom margin of cylinder allowing it to drop open (115 cm length) and at the same time closing half circle doors. A second messenger releases the first support bridle and the sampler turns right side up. Sampler collects about 250 litres of water [Wiebe and Benfield 2003 Plate 11 A].</skos:definition>
<owl:versionInfo>2</owl:versionInfo>
<dc:date>2012-05-11 10:27:07.0</dc:date>
<skos:note xml:lang="en">accepted</skos:note>
<owl:deprecated>false</owl:deprecated>
<skos:broader rdf:resource="http://vocab.nerc.ac.uk/collection/L05/current/22/"/>
<void:inDataset rdf:resource="http://vocab.nerc.ac.uk/.well-known/void"/>
</skos:Concept>
</skos:member>
<skos:member>
<skos:Concept rdf:about="http://vocab.nerc.ac.uk/collection/L22/current/TOOL0297/">
<dc:identifier>SDN:L22::TOOL0297</dc:identifier>
<skos:notation>SDN:L22::TOOL0297</skos:notation>
<skos:prefLabel xml:lang="en">Aerodyne High Resolution Time-of-Flight Aerosol Mass Spectrometer</skos:prefLabel>
<skos:altLabel>Aerodyne HR Tof AMS</skos:altLabel>
<skos:definition xml:lang="en">An in-situ instrument that provides quantitative size and chemical mass loading information in real-time for non-refractory sub-micron atmospheric aerosol particles from high-resolution time-of-flight and mass-spectrometer measurements. The HR-ToF-AMS variant has a detection limit for nitrate of 0.003 (V-mode) or 0.05 (W-mode) ug/m3.</skos:definition>
<owl:versionInfo>1</owl:versionInfo>
<dc:date>2010-05-18 16:10:58.0</dc:date>
<skos:note xml:lang="en">accepted</skos:note>
<owl:deprecated>false</owl:deprecated>
<skos:broader rdf:resource="http://vocab.nerc.ac.uk/collection/L05/current/386/"/>
<void:inDataset rdf:resource="http://vocab.nerc.ac.uk/.well-known/void"/>
</skos:Concept>
</skos:member>
<skos:member>
<skos:Concept rdf:about="http://vocab.nerc.ac.uk/collection/L22/current/TOOL0569/">
<dc:identifier>SDN:L22::TOOL0569</dc:identifier>
<skos:notation>SDN:L22::TOOL0569</skos:notation>
<skos:prefLabel xml:lang="en">Agilent 6850 networked gas chromatograph</skos:prefLabel>
<skos:altLabel>Agilent 6850 GC</skos:altLabel>
<skos:definition xml:lang="en">A single channel, networked, gas chromatograph that separates and analyses compounds into separate components and can be used for chemical, petrochemical and petroleum analyses. The sample is introduced into the injector and then vaporised in the instrument. A chemically inert gas (e.g. helium and nitrogen) carries the vaporised solute into the column that is maintained in a temperature controlled oven. As the solute elutes from the column, it enters the heated detector. An electronic signal is generated upon interaction of the solute with the detector. The Agilent 6850 has a similar performance to the Agilent 6890N GC, but is half as wide. The local interface provides run control and status information and the instrument comes network-ready with a built-in LAN communications interface. There is a choice of detectors available, the Flame Ionization Detector (FID), Thermal Conductivity Detector (TCD) or Mass Selective Detector (MSD). There is an option of split/splitless or packed inlets, a variety of automated sample introduction systems and products available for headspace analysis. This model is no longer in production.</skos:definition>
<owl:versionInfo>1</owl:versionInfo>
<dc:date>2012-11-05 11:03:23.0</dc:date>
<skos:note xml:lang="en">accepted</skos:note>
<owl:deprecated>false</owl:deprecated>
<skos:broader rdf:resource="http://vocab.nerc.ac.uk/collection/L05/current/LAB02/"/>
<void:inDataset rdf:resource="http://vocab.nerc.ac.uk/.well-known/void"/>
</skos:Concept>
</skos:member>
<skos:member>
<skos:Concept rdf:about="http://vocab.nerc.ac.uk/collection/L22/current/TOOL0649/">
<dc:identifier>SDN:L22::TOOL0649</dc:identifier>
<skos:notation>SDN:L22::TOOL0649</skos:notation>
<skos:prefLabel xml:lang="en">Agilent 6890 networked gas chromatograph</skos:prefLabel>
<skos:altLabel>Agilent 6890N GC</skos:altLabel>
<skos:definition xml:lang="en">A networked gas chromatograph that separates and analyses gas mixtures in water or air. The instrument includes a dual channel design supporting two inlets and two detectors. An automatic liquid sampling system is integrated into the mainframe control. Atmospheric pressure and temperature compensation is standard. The instrument supports 6 column oven ramps with 7 plateaus. The 6890N is customisable depending on the application, with choices of inlets, columns, detectors and sampling systems. All detectors include electronic pneumatics control and electronic on/off for all detector gases. Carrier and makeup gas settings are selectable for He, H2, N2, and argon/methane. The instrument has a 7683 ALS interface and incorporates local area network technology as standard. The Agilent 6890N replaced the HP Agilent 5890, and is no longer in production having itself been replaced by the 7890.</skos:definition>
<owl:versionInfo>1</owl:versionInfo>
<dc:date>2013-10-14 14:10:43.0</dc:date>
<skos:note xml:lang="en">accepted</skos:note>
<owl:deprecated>false</owl:deprecated>
<skos:broader rdf:resource="http://vocab.nerc.ac.uk/collection/L05/current/LAB02/"/>
<void:inDataset rdf:resource="http://vocab.nerc.ac.uk/.well-known/void"/>
</skos:Concept>
</skos:member>
<skos:member>
<skos:Concept rdf:about="http://vocab.nerc.ac.uk/collection/L22/current/TOOL0464/">
<dc:identifier>SDN:L22::TOOL0464</dc:identifier>
<skos:notation>SDN:L22::TOOL0464</skos:notation>
<skos:prefLabel xml:lang="en">Agilent 7500ce inductively coupled plasma mass spectrometer</skos:prefLabel>
<skos:altLabel>Agilent 7500ce ICP-MS</skos:altLabel>
<skos:definition xml:lang="en">A laboratory benchtop inductively coupled plasma mass spectrometer (ICP-MS) for metal analysis. The instrument comprises a sample introduction system (micromist glass concentric nebuliser, quartz Scott-type spray chamber, peristaltic pump), an interface of nickel cones and dual on-axis extraction lenses, a vacuum system, mass flow controllers (plasma, auxiliary, makeup, and carrier gas and two Octopole Reaction System (ORS) reaction gas lines), a shieldtorch system (STS), an all-solid state digitally-driven 27 MHz RF generator and an off-axis Omega lens. The octopole cell of the ORS can be used with no gas, operated in collision mode using pure He cell gas or used in H2 reaction mode for ultra-trace Se analysis and semiconductor applications. All three of these modes come as standard in the 7500ce model. The instrument has been discontinued.</skos:definition>
<owl:versionInfo>1</owl:versionInfo>
<dc:date>2012-02-21 16:06:42.0</dc:date>
<skos:note xml:lang="en">accepted</skos:note>
<owl:deprecated>false</owl:deprecated>
<skos:broader rdf:resource="http://vocab.nerc.ac.uk/collection/L05/current/LAB15/"/>
<void:inDataset rdf:resource="http://vocab.nerc.ac.uk/.well-known/void"/>
</skos:Concept>
</skos:member>
<skos:member>
<skos:Concept rdf:about="http://vocab.nerc.ac.uk/collection/L22/current/TOOL0463/">
<dc:identifier>SDN:L22::TOOL0463</dc:identifier>
<skos:notation>SDN:L22::TOOL0463</skos:notation>
<skos:prefLabel xml:lang="en">Agilent 7500cx inductively coupled plasma mass spectrometer</skos:prefLabel>
<skos:altLabel>Agilent 7500cx ICP-MS</skos:altLabel>
<skos:definition xml:lang="en">A laboratory benchtop inductively coupled plasma mass spectrometer (ICP-MS) for metal analysis. The instrument comprises a sample introduction system (micromist glass concentric nebuliser, quartz Scott-type spray chamber, peristaltic pump), an interface of nickel cones and dual on-axis extraction lenses, a vacuum system, mass flow controllers (plasma, auxiliary, makeup, and carrier gas and two Octopole Reaction System (ORS) reaction gas lines), a shieldtorch system (SIS), an all-solid state digitally-driven 27 MHz RF generator and an off-axis Omega lens. The octopole cell of the ORS can be used with no gas or operated in collision mode using pure helium cell gas. As an optional extra for the 7500cx model, the cell can also be used in hydrogen reaction mode for ultra-trace Se analysis and semiconductor applications. The instrument has been discontinued.</skos:definition>
<owl:versionInfo>2</owl:versionInfo>
<dc:date>2012-02-21 10:03:56.0</dc:date>
<skos:note xml:lang="en">accepted</skos:note>
<owl:deprecated>false</owl:deprecated>
<skos:broader rdf:resource="http://vocab.nerc.ac.uk/collection/L05/current/LAB15/"/>
<void:inDataset rdf:resource="http://vocab.nerc.ac.uk/.well-known/void"/>
</skos:Concept>
</skos:member>
<skos:member>
<skos:Concept rdf:about="http://vocab.nerc.ac.uk/collection/L22/current/TOOL0478/">
<dc:identifier>SDN:L22::TOOL0478</dc:identifier>
<skos:notation>SDN:L22::TOOL0478</skos:notation>
<skos:prefLabel xml:lang="en">Agilent Integrated Autosampler I-AS</skos:prefLabel>
<skos:altLabel>Agilent I-AS autosampler</skos:altLabel>
<skos:definition xml:lang="en">A laboratory autosampler for low volume and ultra-trace analyses. The instrument features a peristaltic pump and continuously flowing rinse port so that the probe is always rinsed with fresh wash solution, eliminating the risk of cross contamination during a long sample sequence. It uses non-metal materials to minimise the risk of trace metal contamination. The autosampler was designed for use with the Agilent 7500 series ICP-MS but can also be used with the Agilent 4500 series ICP-MS.</skos:definition>
<owl:versionInfo>1</owl:versionInfo>
<dc:date>2012-03-06 15:57:11.0</dc:date>
<skos:note xml:lang="en">accepted</skos:note>
<owl:deprecated>false</owl:deprecated>
<skos:broader rdf:resource="http://vocab.nerc.ac.uk/collection/L05/current/LAB33/"/>
<void:inDataset rdf:resource="http://vocab.nerc.ac.uk/.well-known/void"/>
</skos:Concept>
</skos:member>
<skos:member>
<skos:Concept rdf:about="http://vocab.nerc.ac.uk/collection/L22/current/TOOL0414/">
<dc:identifier>SDN:L22::TOOL0414</dc:identifier>
<skos:notation>SDN:L22::TOOL0414</skos:notation>
<skos:prefLabel xml:lang="en">Alpkem RFA-300 colorimetric autoanalyser</skos:prefLabel>
<skos:altLabel>Alpkem RFA-300 AA</skos:altLabel>
<skos:definition xml:lang="en">A rapid flow analyser (RFA) that may be used to measure nutrient concentrations in seawater. It is an air-segmented, continuous flow instrument comprising a sampler, a peristaltic pump which simultaneously pumps samples, reagents and air bubbles through the system, analytical cartridge, heating bath, colorimeter, data station, and printer. The RFA-300 was a precursor to the smaller Alpkem RFA/2 (also RFA II or RFA-2).</skos:definition>
<owl:versionInfo>1</owl:versionInfo>
<dc:date>2011-08-05 09:08:32.0</dc:date>
<skos:note xml:lang="en">accepted</skos:note>
<owl:deprecated>false</owl:deprecated>
<skos:broader rdf:resource="http://vocab.nerc.ac.uk/collection/L05/current/LAB03/"/>
<skos:broader rdf:resource="http://vocab.nerc.ac.uk/collection/L05/current/LAB04/"/>
<void:inDataset rdf:resource="http://vocab.nerc.ac.uk/.well-known/void"/>
</skos:Concept>
</skos:member>
<skos:member>
<skos:Concept rdf:about="http://vocab.nerc.ac.uk/collection/L22/current/TOOL0244/">
<dc:identifier>SDN:L22::TOOL0244</dc:identifier>
<skos:notation>SDN:L22::TOOL0244</skos:notation>
<skos:prefLabel xml:lang="en">Alpkem RFA/2 colorimetric autoanalyser</skos:prefLabel>
<skos:altLabel>Alpkem RFA/2 AA</skos:altLabel>
<skos:definition xml:lang="en">A rapid flow analyser that may be used to measure nutrient concentrations in seawater. It is a continuous flow instrument consisting of a sampler, peristaltic pump, analytical cartridge, heating bath, colorimeter, data station, and printer.</skos:definition>
<owl:versionInfo>2</owl:versionInfo>
<dc:date>2010-11-18 12:39:41.0</dc:date>
<skos:note xml:lang="en">accepted</skos:note>
<owl:deprecated>false</owl:deprecated>
<skos:broader rdf:resource="http://vocab.nerc.ac.uk/collection/L05/current/LAB03/"/>
<skos:broader rdf:resource="http://vocab.nerc.ac.uk/collection/L05/current/LAB04/"/>
<void:inDataset rdf:resource="http://vocab.nerc.ac.uk/.well-known/void"/>
</skos:Concept>
</skos:member>
<skos:member>
<skos:Concept rdf:about="http://vocab.nerc.ac.uk/collection/L22/current/TOOL0335/">
<dc:identifier>SDN:L22::TOOL0335</dc:identifier>
<skos:notation>SDN:L22::TOOL0335</skos:notation>
<skos:prefLabel xml:lang="en">Analogue tide gauge</skos:prefLabel>
<skos:altLabel>Analogue TG</skos:altLabel>
<skos:definition xml:lang="en">Generic term for instruments that transform the damped level of the sea surface into a marking on a chart by a continous pen recorder or an analogue display that may be read and written into a ledger.</skos:definition>
<owl:versionInfo>1</owl:versionInfo>
<dc:date>2010-09-06 12:45:22.0</dc:date>
<skos:note xml:lang="en">accepted</skos:note>
<owl:deprecated>false</owl:deprecated>
<skos:broader rdf:resource="http://vocab.nerc.ac.uk/collection/L05/current/111/"/>
<void:inDataset rdf:resource="http://vocab.nerc.ac.uk/.well-known/void"/>
</skos:Concept>
</skos:member>
<skos:member>
<skos:Concept rdf:about="http://vocab.nerc.ac.uk/collection/L22/current/TOOL0224/">
<dc:identifier>SDN:L22::TOOL0224</dc:identifier>
<skos:notation>SDN:L22::TOOL0224</skos:notation>
<skos:prefLabel xml:lang="en">Apogee CS300 pyranometer</skos:prefLabel>
<skos:altLabel>CS300 pyranometer</skos:altLabel>
<skos:definition xml:lang="en">A silicon pyranometer with a spectral range of 300-1100nm. Accuracy for total daily radiation is +-5%. Marketed by Campbell Scientific.</skos:definition>
<owl:versionInfo>1</owl:versionInfo>
<dc:date>2010-05-18 16:10:58.0</dc:date>
<skos:note xml:lang="en">accepted</skos:note>
<owl:deprecated>false</owl:deprecated>
<skos:broader rdf:resource="http://vocab.nerc.ac.uk/collection/L05/current/122/"/>
<void:inDataset rdf:resource="http://vocab.nerc.ac.uk/.well-known/void"/>
</skos:Concept>
</skos:member>
<skos:member>
<skos:Concept rdf:about="http://vocab.nerc.ac.uk/collection/L22/current/TOOL0041/">
<dc:identifier>SDN:L22::TOOL0041</dc:identifier>
<skos:notation>SDN:L22::TOOL0041</skos:notation>
<skos:prefLabel xml:lang="en">Applied Microsystems CTD-12</skos:prefLabel>
<skos:altLabel>AML CTD-12</skos:altLabel>
<skos:definition xml:lang="en">A self-contained CTD with platinized 4-electrode glass conductivity cell, pressure-protected thermistor temperature sensor and a semiconductor strain gauge pressure sensor plus integral data logger.</skos:definition>
<owl:versionInfo>1</owl:versionInfo>
<dc:date>2009-11-30 11:56:35.0</dc:date>
<skos:note xml:lang="en">accepted</skos:note>
<owl:deprecated>false</owl:deprecated>
<skos:related rdf:resource="http://vocab.nerc.ac.uk/collection/P01/current/TEMPST01/"/>
<skos:related rdf:resource="http://vocab.nerc.ac.uk/collection/P01/current/CNDCST01/"/>
<skos:related rdf:resource="http://vocab.nerc.ac.uk/collection/P01/current/PRESPR01/"/>
<skos:related rdf:resource="http://vocab.nerc.ac.uk/collection/P01/current/SIGTPR01/"/>
<skos:related rdf:resource="http://vocab.nerc.ac.uk/collection/P01/current/POTMCV01/"/>
<skos:related rdf:resource="http://vocab.nerc.ac.uk/collection/P01/current/PSALST01/"/>
<skos:broader rdf:resource="http://vocab.nerc.ac.uk/collection/L05/current/134/"/>
<skos:broader rdf:resource="http://vocab.nerc.ac.uk/collection/L05/current/350/"/>
<void:inDataset rdf:resource="http://vocab.nerc.ac.uk/.well-known/void"/>
</skos:Concept>
</skos:member>
<skos:member>
<skos:Concept rdf:about="http://vocab.nerc.ac.uk/collection/L22/current/TOOL0433/">
<dc:identifier>SDN:L22::TOOL0433</dc:identifier>
<skos:notation>SDN:L22::TOOL0433</skos:notation>
<skos:prefLabel xml:lang="en">Applied Microsystems CTD-12 plus</skos:prefLabel>
<skos:altLabel>AML CTD-12+</skos:altLabel>
<skos:definition xml:lang="en">A self-contained CTD with platinized 4-electrode glass conductivity cell, pressure-protected, aged thermistor temperature sensor, a semiconductor strain gauge pressure sensor and an integral data logger. The CTD offers the options of logging data continuously, at user selected depth increments, at user selected time increments, or upon request. Data can be viewed in real time and downloaded on recovery of the CTD. The instrument can be used for profiling to 5000 m or for in-situ long term deployments and has a sampling frequency of 11 Hz. It can support four additional sensors, the options being temperature-compensated pressure, dissolved oxygen, pH, redox, turbidity, radiometer and fluorometer.</skos:definition>
<owl:versionInfo>1</owl:versionInfo>
<dc:date>2011-11-02 11:37:25.0</dc:date>
<skos:note xml:lang="en">accepted</skos:note>
<owl:deprecated>false</owl:deprecated>
<skos:broader rdf:resource="http://vocab.nerc.ac.uk/collection/L05/current/130/"/>
<skos:broader rdf:resource="http://vocab.nerc.ac.uk/collection/L05/current/134/"/>
<skos:broader rdf:resource="http://vocab.nerc.ac.uk/collection/L05/current/350/"/>
<void:inDataset rdf:resource="http://vocab.nerc.ac.uk/.well-known/void"/>
</skos:Concept>
</skos:member>
<skos:member>
<skos:Concept rdf:about="http://vocab.nerc.ac.uk/collection/L22/current/TOOL0434/">
<dc:identifier>SDN:L22::TOOL0434</dc:identifier>
<skos:notation>SDN:L22::TOOL0434</skos:notation>
<skos:prefLabel xml:lang="en">Applied Microsystems Micro CTD</skos:prefLabel>
<skos:altLabel>AML Micro CTD</skos:altLabel>
<skos:definition xml:lang="en">A small, high accuracy CTD including a 4-electrode conductivity cell, temperature sensor, strain gauge pressure sensor and Delrin housing. No pump is required. Sampling frequency is user-selectable up to 25Hz and the instrument has three sampling modes: continuous; defined increment of time or pressure; and on request. The unit is externally-powered and provides real time data as it has no internal data logging capabilities. It can support up to 2 optional additional analogue channels or one additional digital channel. The instrument has a maximum depth range of 6000m.</skos:definition>
<owl:versionInfo>1</owl:versionInfo>
<dc:date>2011-11-02 11:37:25.0</dc:date>
<skos:note xml:lang="en">accepted</skos:note>
<owl:deprecated>false</owl:deprecated>
<skos:broader rdf:resource="http://vocab.nerc.ac.uk/collection/L05/current/134/"/>
<skos:broader rdf:resource="http://vocab.nerc.ac.uk/collection/L05/current/130/"/>
<skos:broader rdf:resource="http://vocab.nerc.ac.uk/collection/L05/current/350/"/>
<void:inDataset rdf:resource="http://vocab.nerc.ac.uk/.well-known/void"/>
</skos:Concept>
</skos:member>
<skos:member>
<skos:Concept rdf:about="http://vocab.nerc.ac.uk/collection/L22/current/TOOL0447/">
<dc:identifier>SDN:L22::TOOL0447</dc:identifier>
<skos:notation>SDN:L22::TOOL0447</skos:notation>
<skos:prefLabel xml:lang="en">Applied Microsystems Sound Velocity Profiler model 16</skos:prefLabel>
<skos:altLabel>AML SVP16</skos:altLabel>
<skos:definition xml:lang="en">An autonomous, battery-powered sound velocity profiler that uses a "sing-around" sensor to measure sound velocity in the water column. It has a range of 1300-1500 m/s, an accuracy of +/-0.25 m/s and a resolution of 0.13 m/s. A built-in microprocessor enables samples to be logged at pre-determined depth increments or for changes in sound velocity greater than 1 m/s. The standard model has a depth rating of 1000 m but other options are available up to a maximum rating of 5000 m. The instrument is no longer in production.</skos:definition>
<owl:versionInfo>1</owl:versionInfo>
<dc:date>2012-01-05 09:34:05.0</dc:date>
<skos:note xml:lang="en">accepted</skos:note>
<owl:deprecated>false</owl:deprecated>
<skos:broader rdf:resource="http://vocab.nerc.ac.uk/collection/L05/current/185/"/>
<void:inDataset rdf:resource="http://vocab.nerc.ac.uk/.well-known/void"/>
</skos:Concept>
</skos:member>
<skos:member>
<skos:Concept rdf:about="http://vocab.nerc.ac.uk/collection/L22/current/TOOL0152/">
<dc:identifier>SDN:L22::TOOL0152</dc:identifier>
<skos:notation>SDN:L22::TOOL0152</skos:notation>
<skos:prefLabel xml:lang="en">Applied Microsystems conductivity and temperature array</skos:prefLabel>
<skos:altLabel>AML CT array</skos:altLabel>
<skos:definition xml:lang="en">A data logger based on the AML MC7 micro-CTD with 3 remote conductivity plus temperature sensors. The logger can sample on command, at a fixed rate or in burst mode and has a real-time feed.</skos:definition>
<owl:versionInfo>2</owl:versionInfo>
<dc:date>2010-11-18 12:39:41.0</dc:date>
<skos:note xml:lang="en">accepted</skos:note>
<owl:deprecated>false</owl:deprecated>
<skos:broader rdf:resource="http://vocab.nerc.ac.uk/collection/L05/current/350/"/>
<skos:broader rdf:resource="http://vocab.nerc.ac.uk/collection/L05/current/134/"/>
<void:inDataset rdf:resource="http://vocab.nerc.ac.uk/.well-known/void"/>
</skos:Concept>
</skos:member>
<skos:member>
<skos:Concept rdf:about="http://vocab.nerc.ac.uk/collection/L22/current/NETT0003/">
<dc:identifier>SDN:L22::NETT0003</dc:identifier>
<skos:notation>SDN:L22::NETT0003</skos:notation>
<skos:prefLabel xml:lang="en">Apstein net - Apstein (1896); Dakin (1908)</skos:prefLabel>
<skos:altLabel>Apstein net</skos:altLabel>
<skos:definition xml:lang="en">Construction is a 14 cm diameter mouth (20 cm long conical mouth piece) 40 cm diameter conical net mouth. 100 cm long net of No. 20 silk. Dakin (1908) also describes a "butterfly" closing mechanism for this net.</skos:definition>
<owl:versionInfo>1</owl:versionInfo>
<dc:date>2011-10-21 14:18:49.0</dc:date>
<skos:note xml:lang="en">accepted</skos:note>
<owl:deprecated>false</owl:deprecated>
<skos:broader rdf:resource="http://vocab.nerc.ac.uk/collection/L05/current/22/"/>
<void:inDataset rdf:resource="http://vocab.nerc.ac.uk/.well-known/void"/>
</skos:Concept>
</skos:member>
<skos:member>
<skos:Concept rdf:about="http://vocab.nerc.ac.uk/collection/L22/current/TOOL0390/">
<dc:identifier>SDN:L22::TOOL0390</dc:identifier>
<skos:notation>SDN:L22::TOOL0390</skos:notation>
<skos:prefLabel xml:lang="en">Ashtech ADU2 Global Positioning System receiver</skos:prefLabel>
<skos:altLabel>Ashtech ADU2 GPS</skos:altLabel>
<skos:definition xml:lang="en">A GPS receiver providing three-dimensional position, velocity and attitude information at a rate of up to 2 Hz. The ADU2 uses four antennae and a 48-channel receiver for Position Dilution of Precision (PDOP)-based satellite tracking. Real-time horizontal position accuracy is ≥ 5 m in autonomous mode and ≥ 1 m in differential mode.</skos:definition>
<owl:versionInfo>1</owl:versionInfo>
<dc:date>2011-04-14 09:29:16.0</dc:date>
<skos:note xml:lang="en">accepted</skos:note>
<owl:deprecated>false</owl:deprecated>
<skos:broader rdf:resource="http://vocab.nerc.ac.uk/collection/L05/current/POS03/"/>
<void:inDataset rdf:resource="http://vocab.nerc.ac.uk/.well-known/void"/>
</skos:Concept>
</skos:member>
<skos:member>
<skos:Concept rdf:about="http://vocab.nerc.ac.uk/collection/L22/current/TOOL0389/">
<dc:identifier>SDN:L22::TOOL0389</dc:identifier>
<skos:notation>SDN:L22::TOOL0389</skos:notation>
<skos:prefLabel xml:lang="en">Ashtech ADU5 Global Positioning System receiver</skos:prefLabel>
<skos:altLabel>Ashtech ADU5 GPS</skos:altLabel>
<skos:definition xml:lang="en">A GPS receiver providing three-dimensional position, velocity and attitude information at a rate of up to 5 Hz. The ADU5 uses four antennae and 56 channels for satellite tracking and reliable positioning. It incorporates signals from Satellite Based Augmentation Systems (SBAS) and includes a 2-channel 300-kHz beacon receiver for differential GPS (DGPS) operations. Real-time horizontal position accuracy is ≥ 3 m in autonomous mode and ≥ 40 cm in differential mode.</skos:definition>
<owl:versionInfo>1</owl:versionInfo>
<dc:date>2011-04-14 09:29:16.0</dc:date>
<skos:note xml:lang="en">accepted</skos:note>
<owl:deprecated>false</owl:deprecated>
<skos:broader rdf:resource="http://vocab.nerc.ac.uk/collection/L05/current/POS04/"/>
<void:inDataset rdf:resource="http://vocab.nerc.ac.uk/.well-known/void"/>
</skos:Concept>
</skos:member>
<skos:member>
<skos:Concept rdf:about="http://vocab.nerc.ac.uk/collection/L22/current/TOOL0524/">
<dc:identifier>SDN:L22::TOOL0524</dc:identifier>
<skos:notation>SDN:L22::TOOL0524</skos:notation>
<skos:prefLabel xml:lang="en">Ashtech G12 Global Positioning System receiver</skos:prefLabel>
<skos:altLabel>Ashtech G12 GPS</skos:altLabel>
<skos:definition xml:lang="en">A 12-channel, all-in-view Global Positioning System (GPS) receiver. It is Differential GPS (DGPS) ready, with a horizontal accuracy of 90 cm in GPS mode and 40 cm in DGPS mode. Update rate is selectable up to 10 Hz.</skos:definition>
<owl:versionInfo>2</owl:versionInfo>
<dc:date>2012-07-16 16:22:59.0</dc:date>
<skos:note xml:lang="en">accepted</skos:note>
<owl:deprecated>false</owl:deprecated>
<skos:broader rdf:resource="http://vocab.nerc.ac.uk/collection/L05/current/POS04/"/>
<skos:broader rdf:resource="http://vocab.nerc.ac.uk/collection/L05/current/POS03/"/>
<void:inDataset rdf:resource="http://vocab.nerc.ac.uk/.well-known/void"/>
</skos:Concept>
</skos:member>
<skos:member>
<skos:Concept rdf:about="http://vocab.nerc.ac.uk/collection/L22/current/TOOL0388/">
<dc:identifier>SDN:L22::TOOL0388</dc:identifier>
<skos:notation>SDN:L22::TOOL0388</skos:notation>
<skos:prefLabel xml:lang="en">Ashtech GG24 Global Positioning System and Global Navigation Satellite System receiver</skos:prefLabel>
<skos:altLabel>Ashtech GG24 GPS+GLONASS</skos:altLabel>
<skos:definition xml:lang="en">A receiver which utilises both GPS and GLONASS satellite constellations for all-in-view positioning at a rate of up to 2 Hz (standard), or 5 Hz (optional). The GG24 has 12 channels for GPS and 12 for GLONASS, providing real-time horizontal position accuracy of ≥ 3.2 m in autonomous mode and ≥ 40 cm in differential mode.</skos:definition>
<owl:versionInfo>1</owl:versionInfo>
<dc:date>2011-04-14 09:29:16.0</dc:date>
<skos:note xml:lang="en">accepted</skos:note>
<owl:deprecated>false</owl:deprecated>
<skos:broader rdf:resource="http://vocab.nerc.ac.uk/collection/L05/current/POS03/"/>
<skos:broader rdf:resource="http://vocab.nerc.ac.uk/collection/L05/current/POS02/"/>
<void:inDataset rdf:resource="http://vocab.nerc.ac.uk/.well-known/void"/>
</skos:Concept>
</skos:member>
<skos:member>
<skos:Concept rdf:about="http://vocab.nerc.ac.uk/collection/L22/current/TOOL0415/">
<dc:identifier>SDN:L22::TOOL0415</dc:identifier>
<skos:notation>SDN:L22::TOOL0415</skos:notation>
<skos:prefLabel xml:lang="en">Astoria Pacific micro-segmented flow analyser</skos:prefLabel>
<skos:altLabel>Astoria analyser</skos:altLabel>
<skos:definition xml:lang="en">A continuous flow analyser that can be used to measure nutrient concentrations in seawater. The six channel digital detector allows analysis of four to six parameters from a single sample. The system consists of a sampler, a peristaltic pump, reaction cartridge, colorimeter and data acquisition software. The pump pushes a sample into the reaction cartridge, where the sample and reagent are brought together. Air-segmentation bubbles are introduced to help facilitate the mixing of sample and reagents. The sample is then analysed colorimetrically. This instrument is an upgrade of the Alpkem RFA-300, which was bought from OI Analytical by Astoria Pacific Inc.</skos:definition>
<owl:versionInfo>1</owl:versionInfo>
<dc:date>2011-08-05 09:08:32.0</dc:date>
<skos:note xml:lang="en">accepted</skos:note>
<owl:deprecated>false</owl:deprecated>
<skos:broader rdf:resource="http://vocab.nerc.ac.uk/collection/L05/current/LAB04/"/>
<skos:broader rdf:resource="http://vocab.nerc.ac.uk/collection/L05/current/LAB03/"/>
<void:inDataset rdf:resource="http://vocab.nerc.ac.uk/.well-known/void"/>
</skos:Concept>
</skos:member>
<skos:member>
<skos:Concept rdf:about="http://vocab.nerc.ac.uk/collection/L22/current/TOOL0283/">
<dc:identifier>SDN:L22::TOOL0283</dc:identifier>
<skos:notation>SDN:L22::TOOL0283</skos:notation>
<skos:prefLabel xml:lang="en">Atmospheric thermometer</skos:prefLabel>
<skos:altLabel>Air thermometer</skos:altLabel>
<skos:definition xml:lang="en">A generic term for a device that measures atmospheric temperature. The term is for use where details of the make, model number and measurement principle are not known.</skos:definition>
<owl:versionInfo>1</owl:versionInfo>
<dc:date>2010-05-18 16:10:58.0</dc:date>
<skos:note xml:lang="en">accepted</skos:note>
<owl:deprecated>false</owl:deprecated>
<skos:broader rdf:resource="http://vocab.nerc.ac.uk/collection/L05/current/102/"/>
<void:inDataset rdf:resource="http://vocab.nerc.ac.uk/.well-known/void"/>
</skos:Concept>
</skos:member>
<skos:member>
<skos:Concept rdf:about="http://vocab.nerc.ac.uk/collection/L22/current/TOOL0240/">
<dc:identifier>SDN:L22::TOOL0240</dc:identifier>
<skos:notation>SDN:L22::TOOL0240</skos:notation>
<skos:prefLabel xml:lang="en">Autolab bench salinometer</skos:prefLabel>
<skos:altLabel>Autolab salinometer</skos:altLabel>
<skos:definition xml:lang="en">A laboratory instrument that determines salinity of a water sample by comparison of its electrical conductivity with a standard solution.</skos:definition>
<owl:versionInfo>1</owl:versionInfo>
<dc:date>2010-05-18 16:10:58.0</dc:date>
<skos:note xml:lang="en">accepted</skos:note>
<owl:deprecated>false</owl:deprecated>
<skos:broader rdf:resource="http://vocab.nerc.ac.uk/collection/L05/current/LAB30/"/>
<void:inDataset rdf:resource="http://vocab.nerc.ac.uk/.well-known/void"/>
</skos:Concept>
</skos:member>
<skos:member>
<skos:Concept rdf:about="http://vocab.nerc.ac.uk/collection/L22/current/TOOL0635/">
<dc:identifier>SDN:L22::TOOL0635</dc:identifier>
<skos:notation>SDN:L22::TOOL0635</skos:notation>
<skos:prefLabel xml:lang="en">Automated Coulometer (Robinson and Williams, 1992)</skos:prefLabel>
<skos:altLabel>Automated coulometer</skos:altLabel>
<skos:definition xml:lang="en">An automated coulometric titration system used for the continual measurement of dissolved inorganic carbon (TCO2), developed by Robinson and Williams (1992). The instrument consists of a sampling pipette, CO2 extractor-stripper, scrubbers and a coulometer interfaced with a PC. The equivalence point is detected photometrically with thymolphthalein as the indicator. It is based on the Johnson et al. (1987) 5011 coulometer manufactured by UIC, but with a number of improvements, including: improved analytical time of 6 minutes; solid state optical liquid-level switches; a three-way mixer valve to allow interchange between sample and standard input; and replacement of PTFE tubing with stainless steel. The Robinson and Williams (1992) coulometer achieves an analytical precision (1 SD) of +/-0.5-1.0 umol/kg (0.025-0.05 percent) and accuracy of 0.15 percent.</skos:definition>
<owl:versionInfo>1</owl:versionInfo>
<dc:date>2013-08-14 15:42:08.0</dc:date>
<skos:note xml:lang="en">accepted</skos:note>
<owl:deprecated>false</owl:deprecated>
<skos:broader rdf:resource="http://vocab.nerc.ac.uk/collection/L05/current/LAB12/"/>
<skos:broader rdf:resource="http://vocab.nerc.ac.uk/collection/L05/current/LAB04/"/>
<void:inDataset rdf:resource="http://vocab.nerc.ac.uk/.well-known/void"/>
</skos:Concept>
</skos:member>
<skos:member>
<skos:Concept rdf:about="http://vocab.nerc.ac.uk/collection/L22/current/NETT0005/">
<dc:identifier>SDN:L22::NETT0005</dc:identifier>
<skos:notation>SDN:L22::NETT0005</skos:notation>
<skos:prefLabel xml:lang="en">Automatic high-speed plankton sampler - Williamson (1962, 1963)</skos:prefLabel>
<skos:altLabel>Automatic high-speed plankton sampler</skos:altLabel>
<skos:definition xml:lang="en">A sampler that has a series of 21 nets attached to the bottom of rectangular "trap doors" which are sequentially closed by means of a cam/screw assembly driven by a ships log (propellor).  Each net is about 6.35 cm long and made of nylon cloth with 23.6 meshes per cm.  The body of the device is 29.2 cm tall x 14 cm wide x 114 cm long not including the side fins. The aperture is 1.9 cm x 1.9 cm  Effective sampling speeds 5 to 11 knots and sample length is 1 to 20 cm.</skos:definition>
<owl:versionInfo>1</owl:versionInfo>
<dc:date>2011-10-21 14:18:49.0</dc:date>
<skos:note xml:lang="en">accepted</skos:note>
<owl:deprecated>false</owl:deprecated>
<skos:broader rdf:resource="http://vocab.nerc.ac.uk/collection/L05/current/68/"/>
<skos:broader rdf:resource="http://vocab.nerc.ac.uk/collection/L05/current/67/"/>
<void:inDataset rdf:resource="http://vocab.nerc.ac.uk/.well-known/void"/>
</skos:Concept>
</skos:member>
<skos:member>
<skos:Concept rdf:about="http://vocab.nerc.ac.uk/collection/L22/current/NETT0004/">
<dc:identifier>SDN:L22::NETT0004</dc:identifier>
<skos:notation>SDN:L22::NETT0004</skos:notation>
<skos:prefLabel xml:lang="en">Autosampling and Recording Instrumental Environmental Sampler - Dunn et al. (1993)</skos:prefLabel>
<skos:altLabel>ARIES</skos:altLabel>
<skos:definition xml:lang="en">A stretched version of the Lowestoft modified Gulf III (similar to Williams et al., LHPR frame) mounting three sampling systems.  The nose cone had a 35.6 cm diameter opening expanding to 76 cm diameter.  Instead of an LHPR box, a 2000 cm long by 16 cm wide belt was outfitted with 110 6-cm diameter cod-ends with 0.2 mm mesh. A drive motor periodically incremented the belt moving the nets from a feed spool into a position to collect a sample at the back of the net and then onto a take-up spool.  Water samples were collected with 60 250 ml bottles mounted in a carousel similar to a conventional rosette sampler.  A data logger recorded temperature, conductivity, pressure, flow, and sampling events at rates between 1 second and 60 minutes.  User selected plankton and water sampling rates were 1 to 60 minutes.  An acoustical telemetry system transmitted depth for realtime monitoring of the system.  Towing speed is 4-5 kts [Wiebe and Benfield 2003 Plate 27 C]</skos:definition>
<owl:versionInfo>2</owl:versionInfo>
<dc:date>2012-06-21 14:43:33.0</dc:date>
<skos:note xml:lang="en">accepted</skos:note>
<owl:deprecated>false</owl:deprecated>
<skos:broader rdf:resource="http://vocab.nerc.ac.uk/collection/L05/current/30/"/>
<skos:broader rdf:resource="http://vocab.nerc.ac.uk/collection/L05/current/21/"/>
<skos:broader rdf:resource="http://vocab.nerc.ac.uk/collection/L05/current/388/"/>
<skos:broader rdf:resource="http://vocab.nerc.ac.uk/collection/L05/current/134/"/>
<skos:broader rdf:resource="http://vocab.nerc.ac.uk/collection/L05/current/350/"/>
<void:inDataset rdf:resource="http://vocab.nerc.ac.uk/.well-known/void"/>
</skos:Concept>
</skos:member>
<skos:member>
<skos:Concept rdf:about="http://vocab.nerc.ac.uk/collection/L22/current/TOOL0501/">
<dc:identifier>SDN:L22::TOOL0501</dc:identifier>
<skos:notation>SDN:L22::TOOL0501</skos:notation>
<skos:prefLabel xml:lang="en">Autosampling and Recording Instrumental Environmental Sampler rosette water bottle</skos:prefLabel>
<skos:altLabel>ARIES water sample bottle</skos:altLabel>
<skos:definition xml:lang="en">A custom made water sampling bottle designed to fit on the ARIES net rosette sampler. The bottle comprises a free-flooding tube with hinged sealing lids at each end. The lids of each tube are connected by an internal length of silicone elastic. Prior to sampling the lids are held open by pins slotted into pivoting levers. When sampling is complete for one bottle the levels at each end of the next tube in the carousel are simultaneously turned by a rotating arm, thus releasing the lids and closing the tube. Each tube is 40 cm long and has an external diameter of 42 mm and a capacity of 250 ml.</skos:definition>
<owl:versionInfo>1</owl:versionInfo>
<dc:date>2012-06-21 16:09:48.0</dc:date>
<skos:note xml:lang="en">accepted</skos:note>
<owl:deprecated>false</owl:deprecated>
<skos:broader rdf:resource="http://vocab.nerc.ac.uk/collection/L05/current/30/"/>
<void:inDataset rdf:resource="http://vocab.nerc.ac.uk/.well-known/void"/>
</skos:Concept>
</skos:member>
<skos:member>
<skos:Concept rdf:about="http://vocab.nerc.ac.uk/collection/L22/current/TOOL0519/">
<dc:identifier>SDN:L22::TOOL0519</dc:identifier>
<skos:notation>SDN:L22::TOOL0519</skos:notation>
<skos:prefLabel xml:lang="en">BD Biosciences FACSAria II Flow Cytometer</skos:prefLabel>
<skos:altLabel>BD FACSAria II Flow Cytometer</skos:altLabel>
<skos:definition xml:lang="en">A high-speed fixed-alignment benchtop cell sorter. The cytometer can be operated at varied pressures and can acquire up to 70,000 events per second. It is capable of multicolour analysis of up to 13 fluorescent markers and two scatter parameters at a time. The system consists of three major components: a fluidics cart, optics system and cytometer electronics. This model has been discontinued. BD Biosciences is a component of BD, previously known as Becton Dickinson.</skos:definition>
<owl:versionInfo>1</owl:versionInfo>
<dc:date>2012-07-04 10:02:10.0</dc:date>
<skos:note xml:lang="en">accepted</skos:note>
<owl:deprecated>false</owl:deprecated>
<skos:broader rdf:resource="http://vocab.nerc.ac.uk/collection/L05/current/LAB37/"/>
<void:inDataset rdf:resource="http://vocab.nerc.ac.uk/.well-known/void"/>
</skos:Concept>
</skos:member>
<skos:member>
<skos:Concept rdf:about="http://vocab.nerc.ac.uk/collection/L22/current/NETT0007/">
<dc:identifier>SDN:L22::NETT0007</dc:identifier>
<skos:notation>SDN:L22::NETT0007</skos:notation>
<skos:prefLabel xml:lang="en">BIOMAPER-II - Wiebe et al (1999, 2002)</skos:prefLabel>
<skos:altLabel>BIOMAPER-II</skos:altLabel>
<skos:definition xml:lang="en">An integrated instrument platform for coupled biological and physical measurements that has a 5 frequency split-beam acoustic system, a VPR system, an environmental sensing system and a bio-optical system. An electro-optical towing cable is used for two-way data communications and the system can be towed oscillating to depths of 300 m [Wiebe and Benfield 2003 Plate 41 A-E].</skos:definition>
<owl:versionInfo>1</owl:versionInfo>
<dc:date>2011-10-21 14:18:49.0</dc:date>
<skos:note xml:lang="en">accepted</skos:note>
<owl:deprecated>false</owl:deprecated>
<skos:broader rdf:resource="http://vocab.nerc.ac.uk/collection/L05/current/134/"/>
<skos:broader rdf:resource="http://vocab.nerc.ac.uk/collection/L05/current/350/"/>
<skos:broader rdf:resource="http://vocab.nerc.ac.uk/collection/L05/current/130/"/>
<skos:broader rdf:resource="http://vocab.nerc.ac.uk/collection/L05/current/180/"/>
<skos:broader rdf:resource="http://vocab.nerc.ac.uk/collection/L05/current/183/"/>
<skos:broader rdf:resource="http://vocab.nerc.ac.uk/collection/L05/current/122/"/>
<skos:broader rdf:resource="http://vocab.nerc.ac.uk/collection/L05/current/124/"/>
<skos:broader rdf:resource="http://vocab.nerc.ac.uk/collection/L05/current/113/"/>
<void:inDataset rdf:resource="http://vocab.nerc.ac.uk/.well-known/void"/>
</skos:Concept>
</skos:member>
<skos:member>
<skos:Concept rdf:about="http://vocab.nerc.ac.uk/collection/L22/current/NETT0008/">
<dc:identifier>SDN:L22::NETT0008</dc:identifier>
<skos:notation>SDN:L22::NETT0008</skos:notation>
<skos:prefLabel xml:lang="en">BIONESS 1m - Sameoto, Jaroszynski and Fraser (1979, 1980)</skos:prefLabel>
<skos:altLabel>BIONESS</skos:altLabel>
<skos:definition xml:lang="en">Construction is a 100 cm x 100 cm mouth opening with 10 nets.  The system is powered electrically on conducting wire and controlled from a surface deck unit. Data logging includes depth, roll, pitch, flowmeter revolutions,  temperature and conductivity.  There is also a 1/4 m system. This system has basic design similarities to that of Be MPS system [Wiebe and Benfield 2003 Plate 30 C, D].</skos:definition>
<owl:versionInfo>1</owl:versionInfo>
<dc:date>2011-10-21 14:18:49.0</dc:date>
<skos:note xml:lang="en">accepted</skos:note>
<owl:deprecated>false</owl:deprecated>
<skos:broader rdf:resource="http://vocab.nerc.ac.uk/collection/L05/current/23/"/>
<skos:broader rdf:resource="http://vocab.nerc.ac.uk/collection/L05/current/68/"/>
<skos:broader rdf:resource="http://vocab.nerc.ac.uk/collection/L05/current/388/"/>
<skos:broader rdf:resource="http://vocab.nerc.ac.uk/collection/L05/current/130/"/>
<skos:broader rdf:resource="http://vocab.nerc.ac.uk/collection/L05/current/134/"/>
<skos:broader rdf:resource="http://vocab.nerc.ac.uk/collection/L05/current/350/"/>
<skos:broader rdf:resource="http://vocab.nerc.ac.uk/collection/L05/current/385/"/>
<void:inDataset rdf:resource="http://vocab.nerc.ac.uk/.well-known/void"/>
</skos:Concept>
</skos:member>
<skos:member>
<skos:Concept rdf:about="http://vocab.nerc.ac.uk/collection/L22/current/TOOL0564/">
<dc:identifier>SDN:L22::TOOL0564</dc:identifier>
<skos:notation>SDN:L22::TOOL0564</skos:notation>
<skos:prefLabel xml:lang="en">BIOPROBE benthic lander</skos:prefLabel>
<skos:altLabel>BIOPROBE lander</skos:altLabel>
<skos:definition xml:lang="en">A seabed lander comprising a stainless steel tripod with instrument cage, water samplers, water pump, compass, camera system, transmissometer or optical backscatter sensor, 3 current meters, thermistor temperature sensor and an electronic control unit with data logging. The components are independently housed to allow for changes in experimental setup. Sensor operation, data recording and water sampling are synchronised. The water sampling system consists of four cylindrical 15 litre polyethylene bottles, with inlets located 10, 15, 25 and 40 cm off the seabed. The bottles are connected to a centrifugal pump and during the sampling procedure fresh water in the four bottles is replaced by the near-bottom water. The instrument cage is located at the top of the tripod, well above the boundary layer sampling section and the sensors are controlled by a master electronics unit.</skos:definition>
<owl:versionInfo>1</owl:versionInfo>
<dc:date>2012-10-15 14:57:16.0</dc:date>
<skos:note xml:lang="en">accepted</skos:note>
<owl:deprecated>false</owl:deprecated>
<skos:broader rdf:resource="http://vocab.nerc.ac.uk/collection/L05/current/114/"/>
<skos:broader rdf:resource="http://vocab.nerc.ac.uk/collection/L05/current/30/"/>
<skos:broader rdf:resource="http://vocab.nerc.ac.uk/collection/L05/current/123/"/>
<skos:broader rdf:resource="http://vocab.nerc.ac.uk/collection/L05/current/180/"/>
<skos:broader rdf:resource="http://vocab.nerc.ac.uk/collection/L05/current/134/"/>
<skos:broader rdf:resource="http://vocab.nerc.ac.uk/collection/L05/current/124/"/>
<void:inDataset rdf:resource="http://vocab.nerc.ac.uk/.well-known/void"/>
</skos:Concept>
</skos:member>
<skos:member>
<skos:Concept rdf:about="http://vocab.nerc.ac.uk/collection/L22/current/TOOL0597/">
<dc:identifier>SDN:L22::TOOL0597</dc:identifier>
<skos:notation>SDN:L22::TOOL0597</skos:notation>
<skos:prefLabel xml:lang="en">Bangor Ocean Colour Sensor</skos:prefLabel>
<skos:altLabel>Bangor OCS</skos:altLabel>
<skos:definition xml:lang="en">An ocean colour sensor set measuring upwelling irradiance at 440, 490, 570 and 670 nm that was designed and built by the School of Ocean Sciences, Bangor University.  Data were integrated over a 30-second period and logged every 10 or 30 minutes.</skos:definition>
<owl:versionInfo>1</owl:versionInfo>
<dc:date>2013-01-31 15:26:40.0</dc:date>
<skos:note xml:lang="en">accepted</skos:note>
<owl:deprecated>false</owl:deprecated>
<skos:broader rdf:resource="http://vocab.nerc.ac.uk/collection/L05/current/122/"/>
<void:inDataset rdf:resource="http://vocab.nerc.ac.uk/.well-known/void"/>
</skos:Concept>
</skos:member>
<skos:member>
<skos:Concept rdf:about="http://vocab.nerc.ac.uk/collection/L22/current/TOOL0281/">
<dc:identifier>SDN:L22::TOOL0281</dc:identifier>
<skos:notation>SDN:L22::TOOL0281</skos:notation>
<skos:prefLabel xml:lang="en">Barometer</skos:prefLabel>
<skos:altLabel>Barometer</skos:altLabel>
<skos:definition xml:lang="en">A generic term for a device that measures atmospheric pressure. The term is for use where details of the make, model number and measurement principle are not known.</skos:definition>
<owl:versionInfo>1</owl:versionInfo>
<dc:date>2010-05-18 16:10:58.0</dc:date>
<skos:note xml:lang="en">accepted</skos:note>
<owl:deprecated>false</owl:deprecated>
<skos:broader rdf:resource="http://vocab.nerc.ac.uk/collection/L05/current/102/"/>
<void:inDataset rdf:resource="http://vocab.nerc.ac.uk/.well-known/void"/>
</skos:Concept>
</skos:member>
<skos:member>
<skos:Concept rdf:about="http://vocab.nerc.ac.uk/collection/L22/current/TOOL0656/">
<dc:identifier>SDN:L22::TOOL0656</dc:identifier>
<skos:notation>SDN:L22::TOOL0656</skos:notation>
<skos:prefLabel xml:lang="en">Bartington Magnetic Susceptibility MS2E point sensor</skos:prefLabel>
<skos:altLabel>Bartington MS2E</skos:altLabel>
<skos:definition xml:lang="en">A portable, 2 kHz, MS2 magnetic susceptability point meter used to analyse the flat surface of split drill or soft sediment cores at high spatial resolution. The MS2E has a sensing area mounted on a ceramic tube which allows the sensor to be placed directly on the flat surface of a split core. The area of response from the probe is 3.8 mm x 10.5 mm (at 50% maximum response) allowing for high spatial resolution measurements along the core surface. The sensor operates by generating a low intensity (approx. 80 A/m RMS), non-saturating, alternating current magnetic field. The MS2 family of sensors have a volume specific maximum resolution of 2 x 10^-6 SI (2 x 10^-7 CGS).</skos:definition>
<owl:versionInfo>1</owl:versionInfo>
<dc:date>2013-12-02 12:24:49.0</dc:date>
<skos:note xml:lang="en">accepted</skos:note>
<owl:deprecated>false</owl:deprecated>
<skos:broader rdf:resource="http://vocab.nerc.ac.uk/collection/L05/current/LAB31/"/>
<void:inDataset rdf:resource="http://vocab.nerc.ac.uk/.well-known/void"/>
</skos:Concept>
</skos:member>
<skos:member>
<skos:Concept rdf:about="http://vocab.nerc.ac.uk/collection/L22/current/NETT0017/">
<dc:identifier>SDN:L22::NETT0017</dc:identifier>
<skos:notation>SDN:L22::NETT0017</skos:notation>
<skos:prefLabel xml:lang="en">Bary Catcher high-speed plankton sampler - Bary et al. (1958)</skos:prefLabel>
<skos:altLabel>Bary Catcher HSS</skos:altLabel>
<skos:definition xml:lang="en">Has a 22.9 cm diameter mouth opening behind a closing valve. The tube chamber is 19.5 cm diameter.  The overall length of the outer fiberglass shell is 213 cm. Two metal nets can be used, one with 15.70 meshes per cm and one with 3.9 meshes per cm. Has depth-flowmeter (like that of Currie and Foxton, 1957) in the tail. Towed up to 10 knots. More than one unit can be attached to the wire. Can be used for vertical or horizontal towing [Wiebe and Benfield 2003 Plate 18 B, C].</skos:definition>
<owl:versionInfo>1</owl:versionInfo>
<dc:date>2011-10-21 14:18:49.0</dc:date>
<skos:note xml:lang="en">accepted</skos:note>
<owl:deprecated>false</owl:deprecated>
<skos:broader rdf:resource="http://vocab.nerc.ac.uk/collection/L05/current/388/"/>
<skos:broader rdf:resource="http://vocab.nerc.ac.uk/collection/L05/current/67/"/>
<void:inDataset rdf:resource="http://vocab.nerc.ac.uk/.well-known/void"/>
</skos:Concept>
</skos:member>
<skos:member>
<skos:Concept rdf:about="http://vocab.nerc.ac.uk/collection/L22/current/TOOL0658/">
<dc:identifier>SDN:L22::TOOL0658</dc:identifier>
<skos:notation>SDN:L22::TOOL0658</skos:notation>
<skos:prefLabel xml:lang="en">Baumer OADM 20I4560/S14C laser distance sensor</skos:prefLabel>
<skos:altLabel>Baumer OADM 20I4560/S14C laser</skos:altLabel>
<skos:definition xml:lang="en">Laser line sensor for measuring distances to rough surfaces using traingulation from a pulsed red laser diode light source (laser class 2, 675 nm) and detection by a photoelectric array. The sensing range is 30 - 130 mm (resolution &lt; 0.06 mm, linearity error +/- 0.2 mm, response time &lt; 10 ms). The sensor has 5 pin connector and is analogue output (4 - 20 mA / 0 - 10 VDC).</skos:definition>
<owl:versionInfo>1</owl:versionInfo>
<dc:date>2013-12-09 12:30:16.0</dc:date>
<skos:note xml:lang="en">accepted</skos:note>
<owl:deprecated>false</owl:deprecated>
<skos:broader rdf:resource="http://vocab.nerc.ac.uk/collection/L05/current/LAB42/"/>
<void:inDataset rdf:resource="http://vocab.nerc.ac.uk/.well-known/void"/>
</skos:Concept>
</skos:member>
<skos:member>
<skos:Concept rdf:about="http://vocab.nerc.ac.uk/collection/L22/current/TOOL0632/">
<dc:identifier>SDN:L22::TOOL0632</dc:identifier>
<skos:notation>SDN:L22::TOOL0632</skos:notation>
<skos:prefLabel xml:lang="en">Beckman Coulter LS 6000 Series Scintillation System</skos:prefLabel>
<skos:altLabel>Beckman LS 6000 Scintillation system</skos:altLabel>
<skos:definition xml:lang="en">A benchtop liquid scintillation analyser for counting the level of radioactive decay in a sample. Typically the instrument features a Multichannel Analyzer and a quench monitor.  Sample capacity is either 336 standard vials, or 648 miniature vials. It has an operating ambient temperature range of 15-35 degC.</skos:definition>
<owl:versionInfo>1</owl:versionInfo>
<dc:date>2013-07-31 12:02:32.0</dc:date>
<skos:note xml:lang="en">accepted</skos:note>
<owl:deprecated>false</owl:deprecated>
<skos:broader rdf:resource="http://vocab.nerc.ac.uk/collection/L05/current/LAB21/"/>
<void:inDataset rdf:resource="http://vocab.nerc.ac.uk/.well-known/void"/>
</skos:Concept>
</skos:member>
<skos:member>
<skos:Concept rdf:about="http://vocab.nerc.ac.uk/collection/L22/current/TOOL0521/">
<dc:identifier>SDN:L22::TOOL0521</dc:identifier>
<skos:notation>SDN:L22::TOOL0521</skos:notation>
<skos:prefLabel xml:lang="en">Becton Dickinson FACSort Flow Cytometer</skos:prefLabel>
<skos:altLabel>BD FACSort Cytometer</skos:altLabel>
<skos:definition xml:lang="en">A fixed-alignment, 5 detector benchtop cell sorter. The cytometer can sort cells at a rate of 300 per second and can be used at three selectable flow rates. The cytometer uses an argon-ion laser and has a variable sample pressure. Seven data channels are available for data acquisition. The cytometer consists of an optics, electronics and fluidics system. Becton Dickinson is now BD Biosciences.</skos:definition>
<owl:versionInfo>1</owl:versionInfo>
<dc:date>2012-07-05 15:53:41.0</dc:date>
<skos:note xml:lang="en">accepted</skos:note>
<owl:deprecated>false</owl:deprecated>
<skos:broader rdf:resource="http://vocab.nerc.ac.uk/collection/L05/current/LAB37/"/>
<void:inDataset rdf:resource="http://vocab.nerc.ac.uk/.well-known/void"/>
</skos:Concept>
</skos:member>
<skos:member>
<skos:Concept rdf:about="http://vocab.nerc.ac.uk/collection/L22/current/TOOL0134/">
<dc:identifier>SDN:L22::TOOL0134</dc:identifier>
<skos:notation>SDN:L22::TOOL0134</skos:notation>
<skos:prefLabel xml:lang="en">Benthos PSA-916T Sonar Altimeter</skos:prefLabel>
<skos:altLabel>PSA-916T Altimeter</skos:altLabel>
<skos:definition xml:lang="en">A titanium sonar altimeter with 200 kHz operating frequency and 14 deg conical band width. It has a range of 100 m and is depth rated to 6000 m.</skos:definition>
<owl:versionInfo>1</owl:versionInfo>
<dc:date>2010-05-18 16:10:58.0</dc:date>
<skos:note xml:lang="en">accepted</skos:note>
<owl:deprecated>false</owl:deprecated>
<skos:broader rdf:resource="http://vocab.nerc.ac.uk/collection/L05/current/379/"/>
<void:inDataset rdf:resource="http://vocab.nerc.ac.uk/.well-known/void"/>
</skos:Concept>
</skos:member>
<skos:member>
<skos:Concept rdf:about="http://vocab.nerc.ac.uk/collection/L22/current/TOOL0440/">
<dc:identifier>SDN:L22::TOOL0440</dc:identifier>
<skos:notation>SDN:L22::TOOL0440</skos:notation>
<skos:prefLabel xml:lang="en">Biospherical Instruments MER-2040A Profiling Spectroradiometer</skos:prefLabel>
<skos:altLabel>MER-2040A profiling spectroradiometer</skos:altLabel>
<skos:definition xml:lang="en">An underwater radiometer designed for multiwavelength profiling and surface measurements of irradiance, radiance, temperature, and remote sensing reflectance in the SeaWiFS wavelength bands. The standard instrument comes with 8 (expandable to 13) channels each of downwelling irradiance and upwelling radiance (or optionally, irradiance), a spectral range of 340-780nm, a depth transducer (200m full scale, 500m optional) and a dual axis inclinometer. The optical sensors are based on high stability, solid-state photodetectors, each with its own narrow-band (10 nm) interference filters. Additional, externally-mounted blocking filters are used where needed. The irradiance sensor is composed of an array of detectors that view a common cosine-corrected optical collector. The radiance sensor is a constructed from an array of telescopes, which define the collection angle (10° field of view), and are coupled to individual detectors. Each detector is connected to an electrometer amplifier, forming an array of amplifiers that are scanned under microprocessor control at approximately one channel per millisecond. The instrument can be modified to measure ultraviolet radiance and irradiance, vector (cosine) upwelling irradiance, and scalar upwelling and downwelling irradiance. A variety of additional sensors can be added to the MER-2040A to form a CTD with auxiliary sensors. Options include PAR, fluorescence, water current, transmissance, temperature, conductivity, oxygen and high resolution pressure sensors.</skos:definition>
<owl:versionInfo>1</owl:versionInfo>
<dc:date>2011-11-16 08:14:57.0</dc:date>
<skos:note xml:lang="en">accepted</skos:note>
<owl:deprecated>false</owl:deprecated>
<skos:broader rdf:resource="http://vocab.nerc.ac.uk/collection/L05/current/122/"/>
<void:inDataset rdf:resource="http://vocab.nerc.ac.uk/.well-known/void"/>
</skos:Concept>
</skos:member>
<skos:member>
<skos:Concept rdf:about="http://vocab.nerc.ac.uk/collection/L22/current/TOOL0443/">
<dc:identifier>SDN:L22::TOOL0443</dc:identifier>
<skos:notation>SDN:L22::TOOL0443</skos:notation>
<skos:prefLabel xml:lang="en">Biospherical Instruments Profiling Reflectance Radiometer PRR-600</skos:prefLabel>
<skos:altLabel>PRR-600 profiling reflectance radiometer</skos:altLabel>
<skos:definition xml:lang="en">An underwater radiometer designed for multiwavelength profiling and surface measurements of irradiance, radiance, temperature, and remote sensing reflectance in the SeaWiFS wavelength bands. The standard instrument comes with 6 (expandable to 7) channels each of downwelling irradiance and upwelling radiance, and the user can select from 9 specialised detector channels at 412, 443, 490, 510, 555, 665, 683, 780 nm and Photosynthetically Active Radiation (PAR: 400 to 700 nm). The optical sensors are based on photodetectors, each with its own narrow-band (10 nm) interference filters. The PRR-600 irradiance collector is Teflon, backed with 100% acrylic, optimized for excellent cosine response in water. The instrument is designed to be hand-lowered, and includes a temperature sensor and pressure transducer with a 200m depth range. It is powered and controlled from a deck unit and data are transmitted to the deck via a conductive cable. There is the option to include additional upwelling and downwelling sensors, tilt and roll sensors, and two analog input channels. The instrument can also be configured for moorings, free-fall deployment, and low profile for towed applications.</skos:definition>
<owl:versionInfo>1</owl:versionInfo>
<dc:date>2011-11-16 08:14:57.0</dc:date>
<skos:note xml:lang="en">accepted</skos:note>
<owl:deprecated>false</owl:deprecated>
<skos:broader rdf:resource="http://vocab.nerc.ac.uk/collection/L05/current/134/"/>
<skos:broader rdf:resource="http://vocab.nerc.ac.uk/collection/L05/current/122/"/>
<void:inDataset rdf:resource="http://vocab.nerc.ac.uk/.well-known/void"/>
</skos:Concept>
</skos:member>
<skos:member>
<skos:Concept rdf:about="http://vocab.nerc.ac.uk/collection/L22/current/TOOL0286/">
<dc:identifier>SDN:L22::TOOL0286</dc:identifier>
<skos:notation>SDN:L22::TOOL0286</skos:notation>
<skos:prefLabel xml:lang="en">Biospherical QCD-905L underwater PAR sensor</skos:prefLabel>
<skos:altLabel>QCD-905L underwater PAR</skos:altLabel>
<skos:definition xml:lang="en">Aluminum quantum cosine PAR sensor with log output for depths to 10,000m and 12 bit ADC systems. Single channel analog output voltage is proportional to the log of incident PAR (Photosynthetically Available Radiation: 400-700 nm) irradiance.</skos:definition>
<owl:versionInfo>1</owl:versionInfo>
<dc:date>2010-05-18 16:10:58.0</dc:date>
<skos:note xml:lang="en">accepted</skos:note>
<owl:deprecated>false</owl:deprecated>
<skos:broader rdf:resource="http://vocab.nerc.ac.uk/collection/L05/current/122/"/>
<void:inDataset rdf:resource="http://vocab.nerc.ac.uk/.well-known/void"/>
</skos:Concept>
</skos:member>
<skos:member>
<skos:Concept rdf:about="http://vocab.nerc.ac.uk/collection/L22/current/TOOL0288/">
<dc:identifier>SDN:L22::TOOL0288</dc:identifier>
<skos:notation>SDN:L22::TOOL0288</skos:notation>
<skos:prefLabel xml:lang="en">Biospherical QCP-2300 underwater PAR sensor</skos:prefLabel>
<skos:altLabel>QCP-2300 underwater PAR</skos:altLabel>
<skos:definition xml:lang="en">Log output quantum cosine PAR profiling sensor. For use with 12 bit ADC systems. Single channel analog output voltage is proportional to the log of incident PAR (Photosynthetically Available Radiation: 400-700 nm) irradiance. Cosine corrected for use underwater to depths up to 1000 m.</skos:definition>
<owl:versionInfo>1</owl:versionInfo>
<dc:date>2010-05-18 16:10:58.0</dc:date>
<skos:note xml:lang="en">accepted</skos:note>
<owl:deprecated>false</owl:deprecated>
<skos:broader rdf:resource="http://vocab.nerc.ac.uk/collection/L05/current/122/"/>
<void:inDataset rdf:resource="http://vocab.nerc.ac.uk/.well-known/void"/>
</skos:Concept>
</skos:member>
<skos:member>
<skos:Concept rdf:about="http://vocab.nerc.ac.uk/collection/L22/current/TOOL0070/">
<dc:identifier>SDN:L22::TOOL0070</dc:identifier>
<skos:notation>SDN:L22::TOOL0070</skos:notation>
<skos:prefLabel xml:lang="en">Biospherical QSP-200L underwater PAR</skos:prefLabel>
<skos:altLabel>QSP-200L underwater PAR</skos:altLabel>
<skos:definition xml:lang="en">Underwater radiometer with a PAR spectral response (400-700nm). Standard configuration had a spherical collector measuring 4-pi scalar irradiance but a flat plate cosine collector was available as an identically-designated option</skos:definition>
<owl:versionInfo>2</owl:versionInfo>
<dc:date>2010-11-18 12:39:41.0</dc:date>
<skos:note xml:lang="en">accepted</skos:note>
<owl:deprecated>false</owl:deprecated>
<skos:broader rdf:resource="http://vocab.nerc.ac.uk/collection/L05/current/122/"/>
<void:inDataset rdf:resource="http://vocab.nerc.ac.uk/.well-known/void"/>
</skos:Concept>
</skos:member>
<skos:member>
<skos:Concept rdf:about="http://vocab.nerc.ac.uk/collection/L22/current/TOOL0071/">
<dc:identifier>SDN:L22::TOOL0071</dc:identifier>
<skos:notation>SDN:L22::TOOL0071</skos:notation>
<skos:prefLabel xml:lang="en">Biospherical QSR-240 surface PAR</skos:prefLabel>
<skos:altLabel>QSR-240 surface PAR</skos:altLabel>
<skos:definition xml:lang="en">Shipboard radiometer with a PAR spectral response (400-700nm) designed to monitor surface irradiance during underwater light profile measurement. Hemispherical collector measuring 2-pi scalar irradiance</skos:definition>
<owl:versionInfo>2</owl:versionInfo>
<dc:date>2010-11-18 12:39:41.0</dc:date>
<skos:note xml:lang="en">accepted</skos:note>
<owl:deprecated>false</owl:deprecated>
<skos:broader rdf:resource="http://vocab.nerc.ac.uk/collection/L05/current/122/"/>
<void:inDataset rdf:resource="http://vocab.nerc.ac.uk/.well-known/void"/>
</skos:Concept>
</skos:member>
<skos:member>
<skos:Concept rdf:about="http://vocab.nerc.ac.uk/collection/L22/current/TOOL0609/">
<dc:identifier>SDN:L22::TOOL0609</dc:identifier>
<skos:notation>SDN:L22::TOOL0609</skos:notation>
<skos:prefLabel xml:lang="en">Biral HSS VPF-730 Visibility and Present Weather Sensor</skos:prefLabel>
<skos:altLabel>Biral VPF-730 sensor</skos:altLabel>
<skos:definition xml:lang="en">An infrared forward scatter meter  which measures horizontal visibility and precipitation. The sensor measures the amount of light scattered by small suspended particulates (i.e. fog, haze and smoke aerosols) or larger particles (i.e. rain, snow, ice pellets, drizzle and mist) passing through the sample volume. The sensor calculates the atmosphere EXtinction COefficient (EXCO) from which the Meteorological Optical Range (MOR) is calculated. Using an infra-red light source and intelligent sensing technology the measurements are unaffected by other light-sources.</skos:definition>
<owl:versionInfo>1</owl:versionInfo>
<dc:date>2013-03-22 16:47:03.0</dc:date>
<skos:note xml:lang="en">accepted</skos:note>
<owl:deprecated>false</owl:deprecated>
<skos:broader rdf:resource="http://vocab.nerc.ac.uk/collection/L05/current/381/"/>
<skos:broader rdf:resource="http://vocab.nerc.ac.uk/collection/L05/current/ATRANS/"/>
<void:inDataset rdf:resource="http://vocab.nerc.ac.uk/.well-known/void"/>
</skos:Concept>
</skos:member>
<skos:member>
<skos:Concept rdf:about="http://vocab.nerc.ac.uk/collection/L22/current/TOOL0006/">
<dc:identifier>SDN:L22::TOOL0006</dc:identifier>
<skos:notation>SDN:L22::TOOL0006</skos:notation>
<skos:prefLabel xml:lang="en">Bissett-Bermann 9006 STD system</skos:prefLabel>
<skos:altLabel>B-B 9006 STD</skos:altLabel>
<skos:definition xml:lang="en">The Bissett-Bermann 9006 was an STD (salinity, temperature depth) profiler.  Output was analogue, producing plots of salinity and temperature versus depth that were subsequently manually digitised.</skos:definition>
<owl:versionInfo>2</owl:versionInfo>
<dc:date>2010-11-18 12:39:41.0</dc:date>
<skos:note xml:lang="en">accepted</skos:note>
<owl:deprecated>false</owl:deprecated>
<skos:broader rdf:resource="http://vocab.nerc.ac.uk/collection/L05/current/134/"/>
<skos:broader rdf:resource="http://vocab.nerc.ac.uk/collection/L05/current/350/"/>
<skos:broader rdf:resource="http://vocab.nerc.ac.uk/collection/L05/current/130/"/>
<void:inDataset rdf:resource="http://vocab.nerc.ac.uk/.well-known/void"/>
</skos:Concept>
</skos:member>
<skos:member>
<skos:Concept rdf:about="http://vocab.nerc.ac.uk/collection/L22/current/TOOL0005/">
<dc:identifier>SDN:L22::TOOL0005</dc:identifier>
<skos:notation>SDN:L22::TOOL0005</skos:notation>
<skos:prefLabel xml:lang="en">Bissett-Bermann 9040 CTD system</skos:prefLabel>
<skos:altLabel>B-B 9040 CTD</skos:altLabel>
<skos:definition xml:lang="en">This instrument, also known as the Plessey 9040, incorporates pressure, temperature and conductivity sensors whose output may be digitally logged in addition to the derived parameters depth, salinity and sound velocity. An optional dissolved oxygen sensor is available. Salinity accuracy is quoted at +/-0.02 ppt and temperature accuracy is quoted at +/-0.02 C in normal oceanographic conditions.</skos:definition>
<owl:versionInfo>2</owl:versionInfo>
<dc:date>2010-11-18 12:39:41.0</dc:date>
<skos:note xml:lang="en">accepted</skos:note>
<owl:deprecated>false</owl:deprecated>
<skos:related rdf:resource="http://vocab.nerc.ac.uk/collection/P01/current/PSALPR01/"/>
<skos:related rdf:resource="http://vocab.nerc.ac.uk/collection/P01/current/DEPHPR01/"/>
<skos:related rdf:resource="http://vocab.nerc.ac.uk/collection/P01/current/PRESPR01/"/>
<skos:related rdf:resource="http://vocab.nerc.ac.uk/collection/P01/current/TEMPST01/"/>
<skos:broader rdf:resource="http://vocab.nerc.ac.uk/collection/L05/current/134/"/>
<skos:broader rdf:resource="http://vocab.nerc.ac.uk/collection/L05/current/350/"/>
<skos:broader rdf:resource="http://vocab.nerc.ac.uk/collection/L05/current/130/"/>
<void:inDataset rdf:resource="http://vocab.nerc.ac.uk/.well-known/void"/>
</skos:Concept>
</skos:member>
<skos:member>
<skos:Concept rdf:about="http://vocab.nerc.ac.uk/collection/L22/current/TOOL0358/">
<dc:identifier>SDN:L22::TOOL0358</dc:identifier>
<skos:notation>SDN:L22::TOOL0358</skos:notation>
<skos:prefLabel xml:lang="en">Bolt Associates Inc. PAR air gun</skos:prefLabel>
<skos:altLabel>Bolt PAR air gun</skos:altLabel>
<skos:definition xml:lang="en">A towed chamber that rapidly released a single bubble of highly compressed air on command to generate an acoustic shock wave plus sonic oscillations as the bubble collapsed. These were used as energy sources for seafloor seismic surveys from the mid-60s until superseded by the Bolt Long-Life air gun in 1992. Bolt Associates Inc. are now known as Bolt Technology Corporation.</skos:definition>
<owl:versionInfo>2</owl:versionInfo>
<dc:date>2010-11-18 12:39:41.0</dc:date>
<skos:note xml:lang="en">accepted</skos:note>
<owl:deprecated>false</owl:deprecated>
<skos:related rdf:resource="http://vocab.nerc.ac.uk/collection/L05/current/154/"/>
<skos:related rdf:resource="http://vocab.nerc.ac.uk/collection/L05/current/153/"/>
<skos:related rdf:resource="http://vocab.nerc.ac.uk/collection/L05/current/375/"/>
<skos:related rdf:resource="http://vocab.nerc.ac.uk/collection/L05/current/362/"/>
<skos:broader rdf:resource="http://vocab.nerc.ac.uk/collection/L05/current/SNAG/"/>
<void:inDataset rdf:resource="http://vocab.nerc.ac.uk/.well-known/void"/>
</skos:Concept>
</skos:member>
<skos:member>
<skos:Concept rdf:about="http://vocab.nerc.ac.uk/collection/L22/current/TOOL0357/">
<dc:identifier>SDN:L22::TOOL0357</dc:identifier>
<skos:notation>SDN:L22::TOOL0357</skos:notation>
<skos:prefLabel xml:lang="en">Bolt Technology Corporation 1500-LL air gun</skos:prefLabel>
<skos:altLabel>Bolt 1500-LL air gun</skos:altLabel>
<skos:definition xml:lang="en">A towed chamber that rapidly releases a single bubble of highly compressed air on command to generate an acoustic shock wave plus sonic oscillations as the bubble collapses. It is used a an energy source for seafloor seismic surveys. The 1500-LL is designed for chamber volumes ranging from 40 to 1500 cubic inches and has a maximum operating pressure of 2000 psi. Multiple guns can be configured in a cluster to increase energy output.</skos:definition>
<owl:versionInfo>1</owl:versionInfo>
<dc:date>2010-11-18 12:37:16.0</dc:date>
<skos:note xml:lang="en">accepted</skos:note>
<owl:deprecated>false</owl:deprecated>
<skos:related rdf:resource="http://vocab.nerc.ac.uk/collection/L05/current/362/"/>
<skos:related rdf:resource="http://vocab.nerc.ac.uk/collection/L05/current/154/"/>
<skos:related rdf:resource="http://vocab.nerc.ac.uk/collection/L05/current/153/"/>
<skos:related rdf:resource="http://vocab.nerc.ac.uk/collection/L05/current/375/"/>
<skos:broader rdf:resource="http://vocab.nerc.ac.uk/collection/L05/current/SNAG/"/>
<void:inDataset rdf:resource="http://vocab.nerc.ac.uk/.well-known/void"/>
</skos:Concept>
</skos:member>
<skos:member>
<skos:Concept rdf:about="http://vocab.nerc.ac.uk/collection/L22/current/TOOL0356/">
<dc:identifier>SDN:L22::TOOL0356</dc:identifier>
<skos:notation>SDN:L22::TOOL0356</skos:notation>
<skos:prefLabel xml:lang="en">Bolt Technology Corporation 1900-LLXT air gun</skos:prefLabel>
<skos:altLabel>Bolt 1900-LLXT air gun</skos:altLabel>
<skos:definition xml:lang="en">A towed chamber that rapidly releases a single bubble of highly compressed air on command to generate an acoustic shock wave plus sonic oscillations as the bubble collapses. It is used a an energy source for seafloor seismic surveys and is suited to both shallow and deep water work. The 1900-LLXT is designed for chamber volumes ranging from 10 to 380 cubic inches and has been tested at an operating pressure of 3000 psi.</skos:definition>
<owl:versionInfo>1</owl:versionInfo>
<dc:date>2010-11-18 12:37:16.0</dc:date>
<skos:note xml:lang="en">accepted</skos:note>
<owl:deprecated>false</owl:deprecated>
<skos:related rdf:resource="http://vocab.nerc.ac.uk/collection/L05/current/154/"/>
<skos:related rdf:resource="http://vocab.nerc.ac.uk/collection/L05/current/153/"/>
<skos:related rdf:resource="http://vocab.nerc.ac.uk/collection/L05/current/362/"/>
<skos:related rdf:resource="http://vocab.nerc.ac.uk/collection/L05/current/375/"/>
<skos:broader rdf:resource="http://vocab.nerc.ac.uk/collection/L05/current/SNAG/"/>
<void:inDataset rdf:resource="http://vocab.nerc.ac.uk/.well-known/void"/>
</skos:Concept>
</skos:member>
<skos:member>
<skos:Concept rdf:about="http://vocab.nerc.ac.uk/collection/L22/current/TOOL0355/">
<dc:identifier>SDN:L22::TOOL0355</dc:identifier>
<skos:notation>SDN:L22::TOOL0355</skos:notation>
<skos:prefLabel xml:lang="en">Bolt Technology Corporation 2800-LLX air gun</skos:prefLabel>
<skos:altLabel>Bolt 2800-LLX air gun</skos:altLabel>
<skos:definition xml:lang="en">A towed chamber that rapidly releases a single bubble of highly compressed air on command to generate an acoustic shock wave plus sonic oscillations as the bubble collapses. It is used a an energy source for seafloor seismic surveys and is suited to shallow water work. The L2800-LLX is designed for chamber volumes ranging from 5 to 120 cubic inches and has a maximum operating pressure of 2000 psi. It can be configured in 2-3 gun clusters to increase energy output.</skos:definition>
<owl:versionInfo>1</owl:versionInfo>
<dc:date>2010-11-18 12:37:16.0</dc:date>
<skos:note xml:lang="en">accepted</skos:note>
<owl:deprecated>false</owl:deprecated>
<skos:related rdf:resource="http://vocab.nerc.ac.uk/collection/L05/current/154/"/>
<skos:related rdf:resource="http://vocab.nerc.ac.uk/collection/L05/current/375/"/>
<skos:related rdf:resource="http://vocab.nerc.ac.uk/collection/L05/current/362/"/>
<skos:related rdf:resource="http://vocab.nerc.ac.uk/collection/L05/current/153/"/>
<skos:broader rdf:resource="http://vocab.nerc.ac.uk/collection/L05/current/SNAG/"/>
<void:inDataset rdf:resource="http://vocab.nerc.ac.uk/.well-known/void"/>
</skos:Concept>
</skos:member>
<skos:member>
<skos:Concept rdf:about="http://vocab.nerc.ac.uk/collection/L22/current/TOOL0353/">
<dc:identifier>SDN:L22::TOOL0353</dc:identifier>
<skos:notation>SDN:L22::TOOL0353</skos:notation>
<skos:prefLabel xml:lang="en">Bolt Technology Corporation Long-Life air gun</skos:prefLabel>
<skos:altLabel>Bolt Long-Life air gun</skos:altLabel>
<skos:definition xml:lang="en">A family of air guns with maximum bubble sizes from 125 to 2000 cubic inches. Air guns comprise a towed chamber that rapidly release a single bubble of highly compressed air on command to generate an acoustic shock wave plus sonic oscillations as the bubble collapses. This family has been used as energy sources for seafloor seismic surveys since their introduction in 1992.</skos:definition>
<owl:versionInfo>2</owl:versionInfo>
<dc:date>2010-11-18 12:39:41.0</dc:date>
<skos:note xml:lang="en">accepted</skos:note>
<owl:deprecated>false</owl:deprecated>
<skos:related rdf:resource="http://vocab.nerc.ac.uk/collection/L05/current/153/"/>
<skos:related rdf:resource="http://vocab.nerc.ac.uk/collection/L05/current/154/"/>
<skos:related rdf:resource="http://vocab.nerc.ac.uk/collection/L05/current/375/"/>
<skos:related rdf:resource="http://vocab.nerc.ac.uk/collection/L05/current/362/"/>
<skos:broader rdf:resource="http://vocab.nerc.ac.uk/collection/L05/current/SNAG/"/>
<void:inDataset rdf:resource="http://vocab.nerc.ac.uk/.well-known/void"/>
</skos:Concept>
</skos:member>
<skos:member>
<skos:Concept rdf:about="http://vocab.nerc.ac.uk/collection/L22/current/NETT0009/">
<dc:identifier>SDN:L22::NETT0009</dc:identifier>
<skos:notation>SDN:L22::NETT0009</skos:notation>
<skos:prefLabel xml:lang="en">Bongo-style vertical closing net  - Brown (1975)</skos:prefLabel>
<skos:altLabel>Bongo-style net</skos:altLabel>
<skos:definition xml:lang="en">An open pair of 50 cm diameter circular net hoops were mounted on each end of a 150 cm wide cross-strut which was attached to a towing cable.  Nets were attached to the bottom of the hoops and their cod-ends were attached to a spreader bar which was also attached to the wire. The nets were lowered to a maximum depth to haul and then during the haul back to the surface, a messenger was used to close the nets either by releasing the hoops so that they turned 90 degrees or by releasing the nets which fell back and were pursed by throttling lines attached to the cross-strut. A non-opening/closing variant of this net is known as the CalVET net [Wiebe and Benfield 2003 Plate 10 A].</skos:definition>
<owl:versionInfo>1</owl:versionInfo>
<dc:date>2011-10-21 14:18:49.0</dc:date>
<skos:note xml:lang="en">accepted</skos:note>
<owl:deprecated>false</owl:deprecated>
<skos:broader rdf:resource="http://vocab.nerc.ac.uk/collection/L05/current/22/"/>
<void:inDataset rdf:resource="http://vocab.nerc.ac.uk/.well-known/void"/>
</skos:Concept>
</skos:member>
<skos:member>
<skos:Concept rdf:about="http://vocab.nerc.ac.uk/collection/L22/current/NETT0012/">
<dc:identifier>SDN:L22::NETT0012</dc:identifier>
<skos:notation>SDN:L22::NETT0012</skos:notation>
<skos:prefLabel xml:lang="en">Booby-II neuston net - Bieri and Newbury (1966)</skos:prefLabel>
<skos:altLabel>Booby-II net</skos:altLabel>
<skos:definition xml:lang="en">Construction is a wooden frame 63 cm wide x 16.5 cm tall x 121 cm long with a pair of Otter board fins extending down 58.5 cm below the top.  Styrofoam plastic used for floatation.  Inside the wooden frame is a metal framework to support a 63 cm x 20 cm rectangular net 100 cm long (number 54 nylon grit gauze). Towed at 1 to 3 kts from the bow of a vessel with bridle attached to the forward side of the frame so that it rides out away from the vessel [Wiebe and Benfield 2003 Plate 20 B].</skos:definition>
<owl:versionInfo>1</owl:versionInfo>
<dc:date>2011-10-21 14:18:49.0</dc:date>
<skos:note xml:lang="en">accepted</skos:note>
<owl:deprecated>false</owl:deprecated>
<skos:broader rdf:resource="http://vocab.nerc.ac.uk/collection/L05/current/69/"/>
<void:inDataset rdf:resource="http://vocab.nerc.ac.uk/.well-known/void"/>
</skos:Concept>
</skos:member>
<skos:member>
<skos:Concept rdf:about="http://vocab.nerc.ac.uk/collection/L22/current/NETT0014/">
<dc:identifier>SDN:L22::NETT0014</dc:identifier>
<skos:notation>SDN:L22::NETT0014</skos:notation>
<skos:prefLabel xml:lang="en">Bottom plankton sampler - Macer (1867)</skos:prefLabel>
<skos:altLabel>Macer BPS</skos:altLabel>
<skos:definition xml:lang="en">Approximately 30 cm x 20 cm mouth opening. Net dimensions or mesh used are not given [Wiebe and Benfield 2003 Plate 23 B].</skos:definition>
<owl:versionInfo>1</owl:versionInfo>
<dc:date>2011-10-21 14:18:49.0</dc:date>
<skos:note xml:lang="en">accepted</skos:note>
<owl:deprecated>false</owl:deprecated>
<skos:broader rdf:resource="http://vocab.nerc.ac.uk/collection/L05/current/388/"/>
<skos:broader rdf:resource="http://vocab.nerc.ac.uk/collection/L05/current/22/"/>
<skos:broader rdf:resource="http://vocab.nerc.ac.uk/collection/L05/current/24/"/>
<void:inDataset rdf:resource="http://vocab.nerc.ac.uk/.well-known/void"/>
</skos:Concept>
</skos:member>
<skos:member>
<skos:Concept rdf:about="http://vocab.nerc.ac.uk/collection/L22/current/NETT0013/">
<dc:identifier>SDN:L22::NETT0013</dc:identifier>
<skos:notation>SDN:L22::NETT0013</skos:notation>
<skos:prefLabel xml:lang="en">Bottom plankton sampler - Omori (1969)</skos:prefLabel>
<skos:altLabel>Omori BPS</skos:altLabel>
<skos:definition xml:lang="en">A 70 x 70 cm rectangular mouth opening net is attached to a sled made of iron (75 cm wide x 90 cm long x 25 cm tall) with a plastic runner on the bottom. The net of 2.0 mm mesh is 350 cm long. A finer mesh netting (330 microns) was used to line the posterior 150 cm to retain smaller zooplankton.  The system is equipped with a messenger operated closing mechanism and a flow meter.</skos:definition>
<owl:versionInfo>1</owl:versionInfo>
<dc:date>2011-10-21 14:18:49.0</dc:date>
<skos:note xml:lang="en">accepted</skos:note>
<owl:deprecated>false</owl:deprecated>
<skos:broader rdf:resource="http://vocab.nerc.ac.uk/collection/L05/current/24/"/>
<skos:broader rdf:resource="http://vocab.nerc.ac.uk/collection/L05/current/22/"/>
<skos:broader rdf:resource="http://vocab.nerc.ac.uk/collection/L05/current/388/"/>
<void:inDataset rdf:resource="http://vocab.nerc.ac.uk/.well-known/void"/>
</skos:Concept>
</skos:member>
<skos:member>
<skos:Concept rdf:about="http://vocab.nerc.ac.uk/collection/L22/current/NETT0015/">
<dc:identifier>SDN:L22::NETT0015</dc:identifier>
<skos:notation>SDN:L22::NETT0015</skos:notation>
<skos:prefLabel xml:lang="en">Bottom skimmer - Frolander and Pratt (1962)</skos:prefLabel>
<skos:altLabel>Bottom skimmer</skos:altLabel>
<skos:definition xml:lang="en">A double runner sled 46 cm wide x 23 cm tall x 132 cm long with a roller on the forward lower cross strut, sheet lead attached to the bottom near the front, and a pair of metal float balls snap-hooked to the top to keep sled right-side-up. Inside was mounted a Clarke-Bumpus cylinder and net (63.5 cm length). Towed at speeds of 1-2 knots [Wiebe and Benfield 2003 Plate 23 C].</skos:definition>
<owl:versionInfo>1</owl:versionInfo>
<dc:date>2011-10-21 14:18:49.0</dc:date>
<skos:note xml:lang="en">accepted</skos:note>
<owl:deprecated>false</owl:deprecated>
<skos:broader rdf:resource="http://vocab.nerc.ac.uk/collection/L05/current/22/"/>
<skos:broader rdf:resource="http://vocab.nerc.ac.uk/collection/L05/current/24/"/>
<skos:broader rdf:resource="http://vocab.nerc.ac.uk/collection/L05/current/388/"/>
<void:inDataset rdf:resource="http://vocab.nerc.ac.uk/.well-known/void"/>
</skos:Concept>
</skos:member>
<skos:member>
<skos:Concept rdf:about="http://vocab.nerc.ac.uk/collection/L22/current/TOOL0472/">
<dc:identifier>SDN:L22::TOOL0472</dc:identifier>
<skos:notation>SDN:L22::TOOL0472</skos:notation>
<skos:prefLabel xml:lang="en">Bowers and Connelly Mega Corer</skos:prefLabel>
<skos:altLabel>Bowers and Connelly Mega Corer</skos:altLabel>
<skos:definition xml:lang="en">A sediment corer which collects relatively undisturbed sea-floor sediment samples including an intact sediment-water interface and overlying supernatant water. The Mega Corer holds 12 tubes, each 600 mm in length, allowing collection of sediment cores up to 400 mm long. It has a hydrostatic damping system which is used to slow down the penetration rate and to remove the typical bow wave. Corer deployment rates are in the region of 1 metre per second on the descent, and at any speed on retrieval as the samples are sealed top and bottom. The core tubing can be manufactured from acrylic, poly carbonate or stainless steel. The instrument was designed by Bowers and Connelly and is now manufactured by OSIL.</skos:definition>
<owl:versionInfo>1</owl:versionInfo>
<dc:date>2012-02-21 16:06:42.0</dc:date>
<skos:note xml:lang="en">accepted</skos:note>
<owl:deprecated>false</owl:deprecated>
<skos:broader rdf:resource="http://vocab.nerc.ac.uk/collection/L05/current/51/"/>
<void:inDataset rdf:resource="http://vocab.nerc.ac.uk/.well-known/void"/>
</skos:Concept>
</skos:member>
<skos:member>
<skos:Concept rdf:about="http://vocab.nerc.ac.uk/collection/L22/current/TOOL0011/">
<dc:identifier>SDN:L22::TOOL0011</dc:identifier>
<skos:notation>SDN:L22::TOOL0011</skos:notation>
<skos:prefLabel xml:lang="en">Bubbler tide gauge</skos:prefLabel>
<skos:altLabel>Bubbler</skos:altLabel>
<skos:definition xml:lang="en">The full tide bubbler system normally consists of two independent measuring systems. The pressure points are mounted approx 1m below Admiralty Chart Datum (ACD) so that negative surges may be recorded and are similar in appearance to an inverted bucket with a copper nozzle mounted on the side. This nozzle is the actual measuring point. A low flow of dry air (normally 7ml/min) is fed down an air tube to the top of the pressure point. When the air pressure in the air line equals the pressure exerted by the column of water above it, then the excess air is released as bubbles through the copper nozzle. This means that the pressure in the air line is proportional to the weight of the water column.</skos:definition>
<owl:versionInfo>1</owl:versionInfo>
<dc:date>2008-11-28 07:54:28.0</dc:date>
<skos:note xml:lang="en">accepted</skos:note>
<owl:deprecated>false</owl:deprecated>
<skos:broader rdf:resource="http://vocab.nerc.ac.uk/collection/L05/current/111/"/>
<void:inDataset rdf:resource="http://vocab.nerc.ac.uk/.well-known/void"/>
</skos:Concept>
</skos:member>
<skos:member>
<skos:Concept rdf:about="http://vocab.nerc.ac.uk/collection/L22/current/TOOL0536/">
<dc:identifier>SDN:L22::TOOL0536</dc:identifier>
<skos:notation>SDN:L22::TOOL0536</skos:notation>
<skos:prefLabel xml:lang="en">Bucket</skos:prefLabel>
<skos:altLabel>Bucket</skos:altLabel>
<skos:definition xml:lang="en">Typically a watertight, vertical cylinder or truncated cone, with an open top and a flat bottom. Usually attached to a semicircular handle.</skos:definition>
<owl:versionInfo>1</owl:versionInfo>
<dc:date>2012-09-25 16:03:31.0</dc:date>
<skos:note xml:lang="en">accepted</skos:note>
<owl:deprecated>false</owl:deprecated>
<skos:broader rdf:resource="http://vocab.nerc.ac.uk/collection/L05/current/30/"/>
<void:inDataset rdf:resource="http://vocab.nerc.ac.uk/.well-known/void"/>
</skos:Concept>
</skos:member>
<skos:member>
<skos:Concept rdf:about="http://vocab.nerc.ac.uk/collection/L22/current/TOOL0614/">
<dc:identifier>SDN:L22::TOOL0614</dc:identifier>
<skos:notation>SDN:L22::TOOL0614</skos:notation>
<skos:prefLabel xml:lang="en">Burkard Scientific SFA 2000 colorimetric AA-II segmented flow analyser</skos:prefLabel>
<skos:altLabel>Burkard SFA 2000</skos:altLabel>
<skos:definition xml:lang="en">A colorimetric segmented flow nutrient AA-II analyser. The standard high sensitivity colorimetric and UV detectors use filter technology and flow through cells with a range of path lengths from 3-50mm.</skos:definition>
<owl:versionInfo>1</owl:versionInfo>
<dc:date>2013-04-23 11:31:40.0</dc:date>
<skos:note xml:lang="en">accepted</skos:note>
<owl:deprecated>false</owl:deprecated>
<skos:broader rdf:resource="http://vocab.nerc.ac.uk/collection/L05/current/LAB20/"/>
<skos:broader rdf:resource="http://vocab.nerc.ac.uk/collection/L05/current/LAB03/"/>
<skos:broader rdf:resource="http://vocab.nerc.ac.uk/collection/L05/current/LAB04/"/>
<void:inDataset rdf:resource="http://vocab.nerc.ac.uk/.well-known/void"/>
</skos:Concept>
</skos:member>
<skos:member>
<skos:Concept rdf:about="http://vocab.nerc.ac.uk/collection/L22/current/TOOL0349/">
<dc:identifier>SDN:L22::TOOL0349</dc:identifier>
<skos:notation>SDN:L22::TOOL0349</skos:notation>
<skos:prefLabel xml:lang="en">C&amp;C Technologies C-Nav3050 satellite positioning system receiver</skos:prefLabel>
<skos:altLabel>C&amp;C Tech. C-Nav3050 receiver</skos:altLabel>
<skos:definition xml:lang="en">A 66-channel "all-in-view" parallel tracking combined GPS/GNSS/L-band receiver providing high accuracy positional information worldwide between 72N and 72S. The C-Nav3050 tracks GPS, GLONASS, Galileo, C-Nav and other SBAS signals, producing positional fixes with a horizontal accuracy of &lt;10cm and a vertical accuracy of &lt;15cm. The instrument has a range of user-programmable output rates (1, 5, 10, 25, 50 and 100 Hz).</skos:definition>
<owl:versionInfo>1</owl:versionInfo>
<dc:date>2010-09-06 12:45:22.0</dc:date>
<skos:note xml:lang="en">accepted</skos:note>
<owl:deprecated>false</owl:deprecated>
<skos:broader rdf:resource="http://vocab.nerc.ac.uk/collection/L05/current/POS04/"/>
<void:inDataset rdf:resource="http://vocab.nerc.ac.uk/.well-known/void"/>
</skos:Concept>
</skos:member>
<skos:member>
<skos:Concept rdf:about="http://vocab.nerc.ac.uk/collection/L22/current/TOOL0652/">
<dc:identifier>SDN:L22::TOOL0652</dc:identifier>
<skos:notation>SDN:L22::TOOL0652</skos:notation>
<skos:prefLabel xml:lang="en">CEFAS 4m survey beam trawl</skos:prefLabel>
<skos:altLabel>CEFAS 4m beam trawl</skos:altLabel>
<skos:definition xml:lang="en">This is the standard net used by the CEFAS fisheries laboratory for beam trawl surveys in UK coastal waters. The net is held open by a 4m (measured inside the end plates) metal beam with a chain mat attached to the beam to increase seabed disturbance. 75mm cod ends were optionally fitted with 40mm liners. Post-1991 80mm (post-1991) cod ends were always fitted with 40mm liners.</skos:definition>
<owl:versionInfo>1</owl:versionInfo>
<dc:date>2013-11-19 10:00:04.0</dc:date>
<skos:note xml:lang="en">accepted</skos:note>
<owl:deprecated>false</owl:deprecated>
<skos:broader rdf:resource="http://vocab.nerc.ac.uk/collection/L05/current/62/"/>
<void:inDataset rdf:resource="http://vocab.nerc.ac.uk/.well-known/void"/>
</skos:Concept>
</skos:member>
<skos:member>
<skos:Concept rdf:about="http://vocab.nerc.ac.uk/collection/L22/current/TOOL0631/">
<dc:identifier>SDN:L22::TOOL0631</dc:identifier>
<skos:notation>SDN:L22::TOOL0631</skos:notation>
<skos:prefLabel xml:lang="en">CHN elemental analyser</skos:prefLabel>
<skos:altLabel>CHN analyser</skos:altLabel>
<skos:definition xml:lang="en">A laboratory instrument that primarily determines total carbon, hydrogen and nitrogen in a sample but may also measure total sulphur and oxygen. Flash combustion is used to convert all organic and inorganic substances into combustion products. The resulting combustion gases pass through a reduction furnace and are then swept into the chromatographic column by a carrier gas where they are separated and detected.</skos:definition>
<owl:versionInfo>1</owl:versionInfo>
<dc:date>2013-07-29 16:29:24.0</dc:date>
<skos:note xml:lang="en">accepted</skos:note>
<owl:deprecated>false</owl:deprecated>
<skos:broader rdf:resource="http://vocab.nerc.ac.uk/collection/L05/current/LAB01/"/>
<void:inDataset rdf:resource="http://vocab.nerc.ac.uk/.well-known/void"/>
</skos:Concept>
</skos:member>
<skos:member>
<skos:Concept rdf:about="http://vocab.nerc.ac.uk/collection/L22/current/TOOL0663/">
<dc:identifier>SDN:L22::TOOL0663</dc:identifier>
<skos:notation>SDN:L22::TOOL0663</skos:notation>
<skos:prefLabel xml:lang="en">CMST-DSTO underwater sound recorder</skos:prefLabel>
<skos:altLabel>CMST-DSTO USR</skos:altLabel>
<skos:definition xml:lang="en">Instrument that contains a hydrophone plus a data logger in a deep-water housing designed for long-term monitoring of underwater noise. It can be deployed for periods of up to two years. Sampling frequency and schedule (including burst recording) may be programmed. More information at http://cmst.curtin.edu.au/products/usr.cfm.</skos:definition>
<owl:versionInfo>1</owl:versionInfo>
<dc:date>2014-02-06 10:11:22.0</dc:date>
<skos:note xml:lang="en">accepted</skos:note>
<owl:deprecated>false</owl:deprecated>
<skos:broader rdf:resource="http://vocab.nerc.ac.uk/collection/L05/current/369/"/>
<void:inDataset rdf:resource="http://vocab.nerc.ac.uk/.well-known/void"/>
</skos:Concept>
</skos:member>
<skos:member>
<skos:Concept rdf:about="http://vocab.nerc.ac.uk/collection/L22/current/NETT0016/">
<dc:identifier>SDN:L22::NETT0016</dc:identifier>
<skos:notation>SDN:L22::NETT0016</skos:notation>
<skos:prefLabel xml:lang="en">CalCOFI net - Ahlstrom (1948)</skos:prefLabel>
<skos:altLabel>CalCOFI net</skos:altLabel>
<skos:definition xml:lang="en">A 100 cm diameter ring net about 5 m in length with No. 30 xxx grit gauze (a grade of silk bolting cloth). Netting changed to 505 micron Nitex mesh and then to 333 micron mesh [Wiebe and Benfield 2003 Plate 2 C].</skos:definition>
<owl:versionInfo>1</owl:versionInfo>
<dc:date>2011-10-21 14:18:49.0</dc:date>
<skos:note xml:lang="en">accepted</skos:note>
<owl:deprecated>false</owl:deprecated>
<skos:broader rdf:resource="http://vocab.nerc.ac.uk/collection/L05/current/22/"/>
<void:inDataset rdf:resource="http://vocab.nerc.ac.uk/.well-known/void"/>
</skos:Concept>
</skos:member>
<skos:member>
<skos:Concept rdf:about="http://vocab.nerc.ac.uk/collection/L22/current/TOOL0647/">
<dc:identifier>SDN:L22::TOOL0647</dc:identifier>
<skos:notation>SDN:L22::TOOL0647</skos:notation>
<skos:prefLabel xml:lang="en">Campbell Scientific 215 Temperature and Relative Humidity Probe</skos:prefLabel>
<skos:altLabel>CS215 Temperature and Relative Humidity Probe</skos:altLabel>
<skos:definition xml:lang="en">A meteorological sensor that uses the Sensirion SHT75 combined temperature and relative humidity element based on Sensiria combined temperature and humidity element called the Sensirion's CMOSens technology. This sensor comes pre-calibrated, is field-replacable and outputs an SDI-12 signal that can be measured by most Campbell Scientific dataloggers.</skos:definition>
<owl:versionInfo>1</owl:versionInfo>
<dc:date>2013-09-30 14:21:04.0</dc:date>
<skos:note xml:lang="en">accepted</skos:note>
<owl:deprecated>false</owl:deprecated>
<skos:broader rdf:resource="http://vocab.nerc.ac.uk/collection/L05/current/102/"/>
<void:inDataset rdf:resource="http://vocab.nerc.ac.uk/.well-known/void"/>
</skos:Concept>
</skos:member>
<skos:member>
<skos:Concept rdf:about="http://vocab.nerc.ac.uk/collection/L22/current/TOOL0646/">
<dc:identifier>SDN:L22::TOOL0646</dc:identifier>
<skos:notation>SDN:L22::TOOL0646</skos:notation>
<skos:prefLabel xml:lang="en">Campbell Scientific 50Y Temperature and Relative Humidity Probe</skos:prefLabel>
<skos:altLabel>CS 50Y Temperature and Relative Humidity Probe</skos:altLabel>
<skos:definition xml:lang="en">A meteorological probe that uses a 1000 ohm platinum resistance thermometer to measure temperature and a Vaisala (INTERCAP) capacitive humidity sensor to measure relative humidity. The instrument has a total operating range of -40 degC to +60 degC for temperature and a range of 0 to 100 percent for relative humidity.</skos:definition>
<owl:versionInfo>1</owl:versionInfo>
<dc:date>2013-09-30 14:19:16.0</dc:date>
<skos:note xml:lang="en">accepted</skos:note>
<owl:deprecated>false</owl:deprecated>
<skos:broader rdf:resource="http://vocab.nerc.ac.uk/collection/L05/current/102/"/>
<void:inDataset rdf:resource="http://vocab.nerc.ac.uk/.well-known/void"/>
</skos:Concept>
</skos:member>
<skos:member>
<skos:Concept rdf:about="http://vocab.nerc.ac.uk/collection/L22/current/TOOL0504/">
<dc:identifier>SDN:L22::TOOL0504</dc:identifier>
<skos:notation>SDN:L22::TOOL0504</skos:notation>
<skos:prefLabel xml:lang="en">Carboy</skos:prefLabel>
<skos:altLabel>Carboy</skos:altLabel>
<skos:definition xml:lang="en">A rigid container made of material such as glass or high density plastic with a typical capacity of 20 to 60 litres. A carboy is typically used to store or transport liquids.</skos:definition>
<owl:versionInfo>1</owl:versionInfo>
<dc:date>2012-06-21 16:09:48.0</dc:date>
<skos:note xml:lang="en">accepted</skos:note>
<owl:deprecated>false</owl:deprecated>
<skos:broader rdf:resource="http://vocab.nerc.ac.uk/collection/L05/current/30/"/>
<void:inDataset rdf:resource="http://vocab.nerc.ac.uk/.well-known/void"/>
</skos:Concept>
</skos:member>
<skos:member>
<skos:Concept rdf:about="http://vocab.nerc.ac.uk/collection/L22/current/TOOL0496/">
<dc:identifier>SDN:L22::TOOL0496</dc:identifier>
<skos:notation>SDN:L22::TOOL0496</skos:notation>
<skos:prefLabel xml:lang="en">Carlo Erba NC 2500 elemental analyser</skos:prefLabel>
<skos:altLabel>Carlo Erba NC 2500 EA</skos:altLabel>
<skos:definition xml:lang="en">A laboratory instrument that simultaneously determines total nitrogen, total hydrogen and total carbon in a solid sample. The sample is completely and instantaneously oxidised by flash combustion, which converts all organic and inorganic substances into combustion products.The resulting combustion gases pass through a reduction furnace and are swept into the chromatographic column by the helium carrier gas. The gases are separated in the column and quantified or they can be introduced into another instrument, such as an isotope ratio mass spectrometer, for further analysis. The instrument was originally manufactured by CE instruments (formerly Carlo Erba) and has since been replaced by Thermo Scientific (part of Thermo Fisher Scientific). This model is no longer in production.</skos:definition>
<owl:versionInfo>1</owl:versionInfo>
<dc:date>2012-05-21 15:03:55.0</dc:date>
<skos:note xml:lang="en">accepted</skos:note>
<owl:deprecated>false</owl:deprecated>
<skos:broader rdf:resource="http://vocab.nerc.ac.uk/collection/L05/current/LAB01/"/>
<void:inDataset rdf:resource="http://vocab.nerc.ac.uk/.well-known/void"/>
</skos:Concept>
</skos:member>
<skos:member>
<skos:Concept rdf:about="http://vocab.nerc.ac.uk/collection/L22/current/TOOL0470/">
<dc:identifier>SDN:L22::TOOL0470</dc:identifier>
<skos:notation>SDN:L22::TOOL0470</skos:notation>
<skos:prefLabel xml:lang="en">Carlo-Erba NA-1500 elemental analyser</skos:prefLabel>
<skos:altLabel>NA-1500 elemental analyser</skos:altLabel>
<skos:definition xml:lang="en">A laboratory instrument that simultaneously determines total nitrogen and total carbon from a wide range of organic and inorganic sediment samples. The sample is completely and instantaneously oxidised by flash combustion, which converts all organic and inorganic substances into combustion products. The resulting combustion gases pass through a reduction furnace and are swept into the chromatographic column by the carrier gas which is helium. The gases are separated in the column and detected by the thermal conductivity detector which gives an output signal proportional to the concentration of the individual components of the mixture. The instrument was originally manufactured by Carlo-Erba, which has since been replaced by Thermo Scientific (part of Thermo Fisher Scientific). This model is no longer in production.</skos:definition>
<owl:versionInfo>1</owl:versionInfo>
<dc:date>2012-02-21 16:06:42.0</dc:date>
<skos:note xml:lang="en">accepted</skos:note>
<owl:deprecated>false</owl:deprecated>
<skos:broader rdf:resource="http://vocab.nerc.ac.uk/collection/L05/current/LAB01/"/>
<void:inDataset rdf:resource="http://vocab.nerc.ac.uk/.well-known/void"/>
</skos:Concept>
</skos:member>
<skos:member>
<skos:Concept rdf:about="http://vocab.nerc.ac.uk/collection/L22/current/TOOL0622/">
<dc:identifier>SDN:L22::TOOL0622</dc:identifier>
<skos:notation>SDN:L22::TOOL0622</skos:notation>
<skos:prefLabel xml:lang="en">Cary Porter tide gauge</skos:prefLabel>
<skos:altLabel>Cary Porter tide gauge</skos:altLabel>
<skos:definition xml:lang="en">An analogue instrument that measured sea level by a float in a stilling well that was mechanically coupled to a pen recording on a rotating drum.</skos:definition>
<owl:versionInfo>1</owl:versionInfo>
<dc:date>2013-06-05 14:58:36.0</dc:date>
<skos:note xml:lang="en">accepted</skos:note>
<owl:deprecated>false</owl:deprecated>
<skos:broader rdf:resource="http://vocab.nerc.ac.uk/collection/L05/current/111/"/>
<void:inDataset rdf:resource="http://vocab.nerc.ac.uk/.well-known/void"/>
</skos:Concept>
</skos:member>
<skos:member>
<skos:Concept rdf:about="http://vocab.nerc.ac.uk/collection/L22/current/NETT0018/">
<dc:identifier>SDN:L22::NETT0018</dc:identifier>
<skos:notation>SDN:L22::NETT0018</skos:notation>
<skos:prefLabel xml:lang="en">Catcher II high-speed sampler</skos:prefLabel>
<skos:altLabel>Catcher II HSS</skos:altLabel>
<skos:definition xml:lang="en">A high-speed, opening-closing plankton sampler.</skos:definition>
<owl:versionInfo>1</owl:versionInfo>
<dc:date>2011-10-21 14:18:49.0</dc:date>
<skos:note xml:lang="en">accepted</skos:note>
<owl:deprecated>false</owl:deprecated>
<skos:broader rdf:resource="http://vocab.nerc.ac.uk/collection/L05/current/67/"/>
<skos:broader rdf:resource="http://vocab.nerc.ac.uk/collection/L05/current/388/"/>
<skos:broader rdf:resource="http://vocab.nerc.ac.uk/collection/L05/current/134/"/>
<void:inDataset rdf:resource="http://vocab.nerc.ac.uk/.well-known/void"/>
</skos:Concept>
</skos:member>
<skos:member>
<skos:Concept rdf:about="http://vocab.nerc.ac.uk/collection/L22/current/TOOL0469/">
<dc:identifier>SDN:L22::TOOL0469</dc:identifier>
<skos:notation>SDN:L22::TOOL0469</skos:notation>
<skos:prefLabel xml:lang="en">Challenger Oceanic Stand-alone Pump</skos:prefLabel>
<skos:altLabel>Challenger Oceanic SAP</skos:altLabel>
<skos:definition xml:lang="en">A submersible battery powered water pump that sucks water through various filters leaving the materials of interest on the filter for analysis. The SAP is deployed clamped to a hydrographic wire. Challenger Oceanic no longer exists.</skos:definition>
<owl:versionInfo>1</owl:versionInfo>
<dc:date>2012-02-21 16:06:42.0</dc:date>
<skos:note xml:lang="en">accepted</skos:note>
<owl:deprecated>false</owl:deprecated>
<skos:broader rdf:resource="http://vocab.nerc.ac.uk/collection/L05/current/84/"/>
<void:inDataset rdf:resource="http://vocab.nerc.ac.uk/.well-known/void"/>
</skos:Concept>
</skos:member>
<skos:member>
<skos:Concept rdf:about="http://vocab.nerc.ac.uk/collection/L22/current/TOOL0142/">
<dc:identifier>SDN:L22::TOOL0142</dc:identifier>
<skos:notation>SDN:L22::TOOL0142</skos:notation>
<skos:prefLabel xml:lang="en">Chelsea Instruments FASTtracka I Fast Repetition Rate Fluorometer</skos:prefLabel>
<skos:altLabel>CTG FASTtracka I FRRF</skos:altLabel>
<skos:definition xml:lang="en">An in-situ Fast Repetition Rate Fluorometer which can be deployed autonomously to depths upto 500m.</skos:definition>
<owl:versionInfo>1</owl:versionInfo>
<dc:date>2010-05-18 16:10:58.0</dc:date>
<skos:note xml:lang="en">accepted</skos:note>
<owl:deprecated>false</owl:deprecated>
<skos:broader rdf:resource="http://vocab.nerc.ac.uk/collection/L05/current/353/"/>
<void:inDataset rdf:resource="http://vocab.nerc.ac.uk/.well-known/void"/>
</skos:Concept>
</skos:member>
<skos:member>
<skos:Concept rdf:about="http://vocab.nerc.ac.uk/collection/L22/current/TOOL0143/">
<dc:identifier>SDN:L22::TOOL0143</dc:identifier>
<skos:notation>SDN:L22::TOOL0143</skos:notation>
<skos:prefLabel xml:lang="en">Chelsea Instruments FASTtracka II Fast Repetition Rate Fluorometer</skos:prefLabel>
<skos:altLabel>CTG FASTtracka II FRRF</skos:altLabel>
<skos:definition xml:lang="en">A Fast Repetition Rate Fluorometer incorporating significant improvements over the FASTtracka I. It may be deployed in-situ to depths up to 500m. Accessories include a dark chamber, a laboratory conversion module and a protective cage.</skos:definition>
<owl:versionInfo>1</owl:versionInfo>
<dc:date>2010-05-18 16:10:58.0</dc:date>
<skos:note xml:lang="en">accepted</skos:note>
<owl:deprecated>false</owl:deprecated>
<skos:broader rdf:resource="http://vocab.nerc.ac.uk/collection/L05/current/353/"/>
<void:inDataset rdf:resource="http://vocab.nerc.ac.uk/.well-known/void"/>
</skos:Concept>
</skos:member>
<skos:member>
<skos:Concept rdf:about="http://vocab.nerc.ac.uk/collection/L22/current/TOOL0118/">
<dc:identifier>SDN:L22::TOOL0118</dc:identifier>
<skos:notation>SDN:L22::TOOL0118</skos:notation>
<skos:prefLabel xml:lang="en">Chelsea Instruments MINITracka II fluorometer</skos:prefLabel>
<skos:altLabel>CTG MINITracka II</skos:altLabel>
<skos:definition xml:lang="en">In-situ miniature low-power fluorometer with good turbidity rejection and ability to operate at high levels of ambient light. Performance has a high degree of insensitivity to water temperature changes.A manifold is available for on-deck through flow applications.</skos:definition>
<owl:versionInfo>1</owl:versionInfo>
<dc:date>2010-05-18 16:10:58.0</dc:date>
<skos:note xml:lang="en">accepted</skos:note>
<owl:deprecated>false</owl:deprecated>
<skos:broader rdf:resource="http://vocab.nerc.ac.uk/collection/L05/current/113/"/>
<void:inDataset rdf:resource="http://vocab.nerc.ac.uk/.well-known/void"/>
</skos:Concept>
</skos:member>
<skos:member>
<skos:Concept rdf:about="http://vocab.nerc.ac.uk/collection/L22/current/TOOL0480/">
<dc:identifier>SDN:L22::TOOL0480</dc:identifier>
<skos:notation>SDN:L22::TOOL0480</skos:notation>
<skos:prefLabel xml:lang="en">Chelsea Technologies 4-pi Photosynthetically Active Radiation sensor HB 071</skos:prefLabel>
<skos:altLabel>CTG HB 071 4-pi PAR</skos:altLabel>
<skos:definition xml:lang="en">A submersible instrument designed to measure irradiance over the photosynthetically active radiation (PAR) spectral range. It includes two hemispherical sensors to provide a spherical field of view and uses a logarithmic amplification to provide light measurements over several orders of magnitude. It uses a photodiode with enhanced blue/green sensitivity which, when used in conjunction with blue-tint glass, produces a quantum response that is flat to +/- 3% over the range 450 to 700nm, and 8% at 400nm The instrument has a depth rating of 500m.</skos:definition>
<owl:versionInfo>1</owl:versionInfo>
<dc:date>2012-03-15 11:46:48.0</dc:date>
<skos:note xml:lang="en">accepted</skos:note>
<owl:deprecated>false</owl:deprecated>
<skos:broader rdf:resource="http://vocab.nerc.ac.uk/collection/L05/current/122/"/>
<void:inDataset rdf:resource="http://vocab.nerc.ac.uk/.well-known/void"/>
</skos:Concept>
</skos:member>
<skos:member>
<skos:Concept rdf:about="http://vocab.nerc.ac.uk/collection/L22/current/TOOL0662/">
<dc:identifier>SDN:L22::TOOL0662</dc:identifier>
<skos:notation>SDN:L22::TOOL0662</skos:notation>
<skos:prefLabel xml:lang="en">Chelsea Technologies GLOWtracka bioluminescence</skos:prefLabel>
<skos:altLabel>Chelsea Technologies GLOWtracka</skos:altLabel>
<skos:definition xml:lang="en">The GLOWtracka is designed to measure visible emissions from bioluminescent organisms in the marine environment. It can be moored, used in profiles, or deployed in towed vehicles. It's precision flow meter stimulates bioluminescent organisms and measures the light flashes as the organisms pass the photodiode. The sensor can be deployed to depths up to 1000 m and has an irradiance detectivity of 10 picowatt at 560 nm over z.f. -50 Hz (-3 db).</skos:definition>
<owl:versionInfo>2</owl:versionInfo>
<dc:date>2014-01-28 11:55:16.0</dc:date>
<skos:note xml:lang="en">accepted</skos:note>
<owl:deprecated>false</owl:deprecated>
<skos:broader rdf:resource="http://vocab.nerc.ac.uk/collection/L05/current/BLUMS/"/>
<void:inDataset rdf:resource="http://vocab.nerc.ac.uk/.well-known/void"/>
</skos:Concept>
</skos:member>
<skos:member>
<skos:Concept rdf:about="http://vocab.nerc.ac.uk/collection/L22/current/TOOL0050/">
<dc:identifier>SDN:L22::TOOL0050</dc:identifier>
<skos:notation>SDN:L22::TOOL0050</skos:notation>
<skos:prefLabel xml:lang="en">Chelsea Technologies Group 2-pi PAR irradiance sensor</skos:prefLabel>
<skos:altLabel>CTG 2-pi PAR</skos:altLabel>
<skos:definition xml:lang="en">A submersible irradiance sensor designed by Plymouth marine Laboratory and developed commercially by CTG. The collector is designed to measure the amount of light available for photosynthesis over a hemisphere. Sensors are often paired, one facing up the other down, to determine total PAR. Relative Spectral Sensitivity flat to + 3% from 450-700nm, down 8% of 400nm and 36% at 350nm. Casings on commercial instruments are rated to 1000m depth, but operationally deployed prototype instruments from PML were only rated to 500m.</skos:definition>
<owl:versionInfo>2</owl:versionInfo>
<dc:date>2010-11-18 12:39:41.0</dc:date>
<skos:note xml:lang="en">accepted</skos:note>
<owl:deprecated>false</owl:deprecated>
<skos:related rdf:resource="http://vocab.nerc.ac.uk/collection/P01/current/DWIRSXSD/"/>
<skos:related rdf:resource="http://vocab.nerc.ac.uk/collection/P01/current/LVLTPU01/"/>
<skos:related rdf:resource="http://vocab.nerc.ac.uk/collection/P01/current/IRRUPP01/"/>
<skos:related rdf:resource="http://vocab.nerc.ac.uk/collection/P01/current/LVLTPD01/"/>
<skos:related rdf:resource="http://vocab.nerc.ac.uk/collection/P01/current/IRRDPP01/"/>
<skos:broader rdf:resource="http://vocab.nerc.ac.uk/collection/L05/current/122/"/>
<void:inDataset rdf:resource="http://vocab.nerc.ac.uk/.well-known/void"/>
</skos:Concept>
</skos:member>
<skos:member>
<skos:Concept rdf:about="http://vocab.nerc.ac.uk/collection/L22/current/TOOL0425/">
<dc:identifier>SDN:L22::TOOL0425</dc:identifier>
<skos:notation>SDN:L22::TOOL0425</skos:notation>
<skos:prefLabel xml:lang="en">Chelsea Technologies Group Alphatracka II transmissometer</skos:prefLabel>
<skos:altLabel>CTG Alphatracka II</skos:altLabel>
<skos:definition xml:lang="en">A compact digitally controlled transmissometer similar to the CTG Alphatracka I but with smaller diameter titanium pressure housing. Versions available with optical path-lengths of 5 or 10 or 25 cm. Standard wavelength is 660 nm but optional wavelengths of 470 nm or 565 nm or 590 nm also available. Depth rated to 6000 m.</skos:definition>
<owl:versionInfo>1</owl:versionInfo>
<dc:date>2011-09-12 12:57:40.0</dc:date>
<skos:note xml:lang="en">accepted</skos:note>
<owl:deprecated>false</owl:deprecated>
<skos:broader rdf:resource="http://vocab.nerc.ac.uk/collection/L22/current/TOOL0065/"/>
<skos:broader rdf:resource="http://vocab.nerc.ac.uk/collection/L05/current/124/"/>
<void:inDataset rdf:resource="http://vocab.nerc.ac.uk/.well-known/void"/>
</skos:Concept>
</skos:member>
<skos:member>
<skos:Concept rdf:about="http://vocab.nerc.ac.uk/collection/L22/current/TOOL0065/">
<dc:identifier>SDN:L22::TOOL0065</dc:identifier>
<skos:notation>SDN:L22::TOOL0065</skos:notation>
<skos:prefLabel xml:lang="en">Chelsea Technologies Group Alphatracka transmissometer</skos:prefLabel>
<skos:altLabel>CTG Alphatracka transmissometer</skos:altLabel>
<skos:definition xml:lang="en">Dual beam, ratiometric digitally controlled transmissometer of titanium construction rated to 6000m. 5/10/25cm path lengths and 470/565/590/660nm wavelengths available.</skos:definition>
<owl:versionInfo>1</owl:versionInfo>
<dc:date>2009-11-30 11:56:35.0</dc:date>
<skos:note xml:lang="en">accepted</skos:note>
<owl:deprecated>false</owl:deprecated>
<skos:narrower rdf:resource="http://vocab.nerc.ac.uk/collection/L22/current/TOOL0425/"/>
<skos:broader rdf:resource="http://vocab.nerc.ac.uk/collection/L05/current/124/"/>
<void:inDataset rdf:resource="http://vocab.nerc.ac.uk/.well-known/void"/>
</skos:Concept>
</skos:member>
<skos:member>
<skos:Concept rdf:about="http://vocab.nerc.ac.uk/collection/L22/current/TOOL0043/">
<dc:identifier>SDN:L22::TOOL0043</dc:identifier>
<skos:notation>SDN:L22::TOOL0043</skos:notation>
<skos:prefLabel xml:lang="en">Chelsea Technologies Group Aqualog CTD</skos:prefLabel>
<skos:altLabel>CTG Aqualog CTD</skos:altLabel>
<skos:definition xml:lang="en">A self-contained unit comprising pressure, temperature and conductivity sensors, an optional dissolved oxygen sensor, a fluorometer and a data logger. The unit could be used in a variety of modes including vertical profiling, towed undulator and short-term moorings.</skos:definition>
<owl:versionInfo>2</owl:versionInfo>
<dc:date>2010-11-18 12:39:41.0</dc:date>
<skos:note xml:lang="en">accepted</skos:note>
<owl:deprecated>false</owl:deprecated>
<skos:broader rdf:resource="http://vocab.nerc.ac.uk/collection/L05/current/351/"/>
<skos:broader rdf:resource="http://vocab.nerc.ac.uk/collection/L05/current/130/"/>
<skos:broader rdf:resource="http://vocab.nerc.ac.uk/collection/L05/current/350/"/>
<skos:broader rdf:resource="http://vocab.nerc.ac.uk/collection/L05/current/134/"/>
<skos:broader rdf:resource="http://vocab.nerc.ac.uk/collection/L05/current/113/"/>
<void:inDataset rdf:resource="http://vocab.nerc.ac.uk/.well-known/void"/>
</skos:Concept>
</skos:member>
<skos:member>
<skos:Concept rdf:about="http://vocab.nerc.ac.uk/collection/L22/current/TOOL0048/">
<dc:identifier>SDN:L22::TOOL0048</dc:identifier>
<skos:notation>SDN:L22::TOOL0048</skos:notation>
<skos:prefLabel xml:lang="en">Chelsea Technologies Group Aquapack CTD</skos:prefLabel>
<skos:altLabel>CTG Aquapack CTD</skos:altLabel>
<skos:definition xml:lang="en">Single titanium housing containing temperature, conductivity, depth and fluorescence sensors. Also contains internal batteries and a data logger. Spare analogous channels are available to interface a range of additional externally mounted sensors such as PAR and dissolved oxygen. Has a depth rating of 200m.</skos:definition>
<owl:versionInfo>1</owl:versionInfo>
<dc:date>2009-11-30 11:56:35.0</dc:date>
<skos:note xml:lang="en">accepted</skos:note>
<owl:deprecated>false</owl:deprecated>
<skos:broader rdf:resource="http://vocab.nerc.ac.uk/collection/L05/current/113/"/>
<skos:broader rdf:resource="http://vocab.nerc.ac.uk/collection/L05/current/134/"/>
<skos:broader rdf:resource="http://vocab.nerc.ac.uk/collection/L05/current/130/"/>
<skos:broader rdf:resource="http://vocab.nerc.ac.uk/collection/L05/current/350/"/>
<void:inDataset rdf:resource="http://vocab.nerc.ac.uk/.well-known/void"/>
</skos:Concept>
</skos:member>
<skos:member>
<skos:Concept rdf:about="http://vocab.nerc.ac.uk/collection/L22/current/TOOL0424/">
<dc:identifier>SDN:L22::TOOL0424</dc:identifier>
<skos:notation>SDN:L22::TOOL0424</skos:notation>
<skos:prefLabel xml:lang="en">Chelsea Technologies Group Aquatracka III fluorometer</skos:prefLabel>
<skos:altLabel>CTG Aquatracka III</skos:altLabel>
<skos:definition xml:lang="en">A compact light-weight submersible fluorometer for detection of chlorophyll-a, dye tracing or turbidity with a 4-decade logarithmic output. It can sense chemical fluorescence or light scatter between 400-800nm and uses a pulsed xenon light source. Titanium casing rated to 6000m. Broadly similar to the Aquatracka II but with improved detection optics and internal enhancements.</skos:definition>
<owl:versionInfo>1</owl:versionInfo>
<dc:date>2011-09-12 12:57:40.0</dc:date>
<skos:note xml:lang="en">accepted</skos:note>
<owl:deprecated>false</owl:deprecated>
<skos:broader rdf:resource="http://vocab.nerc.ac.uk/collection/L05/current/113/"/>
<skos:broader rdf:resource="http://vocab.nerc.ac.uk/collection/L22/current/TOOL0049/"/>
<void:inDataset rdf:resource="http://vocab.nerc.ac.uk/.well-known/void"/>
</skos:Concept>
</skos:member>
<skos:member>
<skos:Concept rdf:about="http://vocab.nerc.ac.uk/collection/L22/current/TOOL0049/">
<dc:identifier>SDN:L22::TOOL0049</dc:identifier>
<skos:notation>SDN:L22::TOOL0049</skos:notation>
<skos:prefLabel xml:lang="en">Chelsea Technologies Group Aquatracka fluorometer</skos:prefLabel>
<skos:altLabel>CTG Aquatracka fluorometer</skos:altLabel>
<skos:definition xml:lang="en">A submersible fluorometer that may be configured for measurement of chlorophyll-a, tracer dye or set up as a nephelometer to measure turbidity. It is manufactured from titanium giving a depth rating of 6000m.</skos:definition>
<owl:versionInfo>4</owl:versionInfo>
<dc:date>2010-11-18 12:39:41.0</dc:date>
<skos:note xml:lang="en">accepted</skos:note>
<owl:deprecated>false</owl:deprecated>
<skos:narrower rdf:resource="http://vocab.nerc.ac.uk/collection/L22/current/TOOL0424/"/>
<skos:related rdf:resource="http://vocab.nerc.ac.uk/collection/P01/current/CPHLUW01/"/>
<skos:related rdf:resource="http://vocab.nerc.ac.uk/collection/P01/current/FVLTAQ01/"/>
<skos:related rdf:resource="http://vocab.nerc.ac.uk/collection/P01/current/CPHLPR01/"/>
<skos:related rdf:resource="http://vocab.nerc.ac.uk/collection/P01/current/NVLTAQ01/"/>
<skos:broader rdf:resource="http://vocab.nerc.ac.uk/collection/L05/current/113/"/>
<void:inDataset rdf:resource="http://vocab.nerc.ac.uk/.well-known/void"/>
</skos:Concept>
</skos:member>
<skos:member>
<skos:Concept rdf:about="http://vocab.nerc.ac.uk/collection/L22/current/TOOL0341/">
<dc:identifier>SDN:L22::TOOL0341</dc:identifier>
<skos:notation>SDN:L22::TOOL0341</skos:notation>
<skos:prefLabel xml:lang="en">Chelsea Technologies Group MINIpack CTD-F</skos:prefLabel>
<skos:altLabel>CTG MINIpack CTD-F</skos:altLabel>
<skos:definition xml:lang="en">A single titanium/acetyl housing containing temperature, conductivity, pressure and fluorescence sensors, a data logger and internal batteries. The fluorometer can be configured to measure a variety of pigments or turbidity and the sensor package has a depth rating of 600m. Data can be recorded internally or output in real time. Spare channels are available to interface up to 16 external sensors such as PAR and dissolved oxygen.</skos:definition>
<owl:versionInfo>1</owl:versionInfo>
<dc:date>2010-10-14 10:51:49.0</dc:date>
<skos:note xml:lang="en">accepted</skos:note>
<owl:deprecated>false</owl:deprecated>
<skos:broader rdf:resource="http://vocab.nerc.ac.uk/collection/L05/current/350/"/>
<skos:broader rdf:resource="http://vocab.nerc.ac.uk/collection/L05/current/134/"/>
<skos:broader rdf:resource="http://vocab.nerc.ac.uk/collection/L05/current/130/"/>
<skos:broader rdf:resource="http://vocab.nerc.ac.uk/collection/L05/current/113/"/>
<void:inDataset rdf:resource="http://vocab.nerc.ac.uk/.well-known/void"/>
</skos:Concept>
</skos:member>
<skos:member>
<skos:Concept rdf:about="http://vocab.nerc.ac.uk/collection/L22/current/TOOL0342/">
<dc:identifier>SDN:L22::TOOL0342</dc:identifier>
<skos:notation>SDN:L22::TOOL0342</skos:notation>
<skos:prefLabel xml:lang="en">ChemLab AA-II segmented continuous flow autoanalyser</skos:prefLabel>
<skos:altLabel>ChemLab AA-II</skos:altLabel>
<skos:definition xml:lang="en">A rapid flow analyser that may be used to measure nutrient concentrations in seawater. It is a continuous flow instrument consisting of a sampler, peristaltic pump, analytical cartridge, heating bath, colorimeter, data station, and printer.</skos:definition>
<owl:versionInfo>1</owl:versionInfo>
<dc:date>2010-09-06 12:45:22.0</dc:date>
<skos:note xml:lang="en">accepted</skos:note>
<owl:deprecated>false</owl:deprecated>
<skos:broader rdf:resource="http://vocab.nerc.ac.uk/collection/L05/current/LAB04/"/>
<skos:broader rdf:resource="http://vocab.nerc.ac.uk/collection/L05/current/LAB03/"/>
<void:inDataset rdf:resource="http://vocab.nerc.ac.uk/.well-known/void"/>
</skos:Concept>
</skos:member>
<skos:member>
<skos:Concept rdf:about="http://vocab.nerc.ac.uk/collection/L22/current/TOOL0206/">
<dc:identifier>SDN:L22::TOOL0206</dc:identifier>
<skos:notation>SDN:L22::TOOL0206</skos:notation>
<skos:prefLabel xml:lang="en">Chernikeeff Aquaprobe Mk5 electromagnetic log</skos:prefLabel>
<skos:altLabel>Chernikeeff Aquaprobe Mk5 em-log</skos:altLabel>
<skos:definition xml:lang="en">This is a military grade electromagnetic log system directly measuring speed relative to the water. It can be configured to provide single or dual axis speed and distance travelled measurement, using single or twin tranducers..</skos:definition>
<owl:versionInfo>1</owl:versionInfo>
<dc:date>2010-05-18 16:10:58.0</dc:date>
<skos:note xml:lang="en">accepted</skos:note>
<owl:deprecated>false</owl:deprecated>
<skos:broader rdf:resource="http://vocab.nerc.ac.uk/collection/L05/current/114/"/>
<void:inDataset rdf:resource="http://vocab.nerc.ac.uk/.well-known/void"/>
</skos:Concept>
</skos:member>
<skos:member>
<skos:Concept rdf:about="http://vocab.nerc.ac.uk/collection/L22/current/TOOL0371/">
<dc:identifier>SDN:L22::TOOL0371</dc:identifier>
<skos:notation>SDN:L22::TOOL0371</skos:notation>
<skos:prefLabel xml:lang="en">Christian Albrechts University of Kiel Multisonde CTD profiler</skos:prefLabel>
<skos:altLabel>CAU CTD Multisonde</skos:altLabel>
<skos:definition xml:lang="en">A conductivity-temperature-pressure profiler with a pressure rating of either 600dbar or 6000dbar and a pressure accuracy of +/- 0.01%. It was capable of operating over a temperature range of -2 to 40 degC with an accuracy of +/- 0.01 degC and a conductivity range of 5 to 55 mmho/cm with an accuracy of +/- 10 umho/cm. The instrument was developed in the 1970s by what was then the Institute for Applied Physics of Kiel University and was used by the then Institute for Marine Science, Kiel.</skos:definition>
<owl:versionInfo>1</owl:versionInfo>
<dc:date>2011-02-09 11:25:51.0</dc:date>
<skos:note xml:lang="en">accepted</skos:note>
<owl:deprecated>false</owl:deprecated>
<skos:related rdf:resource="http://vocab.nerc.ac.uk/collection/P01/current/SSALST01/"/>
<skos:related rdf:resource="http://vocab.nerc.ac.uk/collection/P01/current/PRESPR01/"/>
<skos:related rdf:resource="http://vocab.nerc.ac.uk/collection/P01/current/TEMPST01/"/>
<skos:broader rdf:resource="http://vocab.nerc.ac.uk/collection/L05/current/130/"/>
<skos:broader rdf:resource="http://vocab.nerc.ac.uk/collection/L05/current/134/"/>
<skos:broader rdf:resource="http://vocab.nerc.ac.uk/collection/L05/current/350/"/>
<void:inDataset rdf:resource="http://vocab.nerc.ac.uk/.well-known/void"/>
</skos:Concept>
</skos:member>
<skos:member>
<skos:Concept rdf:about="http://vocab.nerc.ac.uk/collection/L22/current/NETT0019/">
<dc:identifier>SDN:L22::NETT0019</dc:identifier>
<skos:notation>SDN:L22::NETT0019</skos:notation>
<skos:prefLabel xml:lang="en">Chun-Peterson net - Chun (1888, 1903)</skos:prefLabel>
<skos:altLabel>Chun-Peterson net</skos:altLabel>
<skos:definition xml:lang="en">A vertical net lowered closed with propellor-activated opening and closing.</skos:definition>
<owl:versionInfo>1</owl:versionInfo>
<dc:date>2011-10-21 14:18:49.0</dc:date>
<skos:note xml:lang="en">accepted</skos:note>
<owl:deprecated>false</owl:deprecated>
<skos:broader rdf:resource="http://vocab.nerc.ac.uk/collection/L05/current/22/"/>
<void:inDataset rdf:resource="http://vocab.nerc.ac.uk/.well-known/void"/>
</skos:Concept>
</skos:member>
<skos:member>
<skos:Concept rdf:about="http://vocab.nerc.ac.uk/collection/L22/current/NETT0020/">
<dc:identifier>SDN:L22::NETT0020</dc:identifier>
<skos:notation>SDN:L22::NETT0020</skos:notation>
<skos:prefLabel xml:lang="en">Clarke Jet Net high-speed plankton sampler - Clarke (1964)</skos:prefLabel>
<skos:altLabel>Clarke Jet Net HSS</skos:altLabel>
<skos:definition xml:lang="en">Construction is a 12 cm diameter mouth opening with an overall length of 125 cm. Uses nylon netting with 0.44 mm mesh. Towing speeds up to 10.5 knots [Wiebe and Benfield 2003 Plate 18 E].</skos:definition>
<owl:versionInfo>1</owl:versionInfo>
<dc:date>2011-10-21 14:18:49.0</dc:date>
<skos:note xml:lang="en">accepted</skos:note>
<owl:deprecated>false</owl:deprecated>
<skos:broader rdf:resource="http://vocab.nerc.ac.uk/collection/L05/current/67/"/>
<void:inDataset rdf:resource="http://vocab.nerc.ac.uk/.well-known/void"/>
</skos:Concept>
</skos:member>
<skos:member>
<skos:Concept rdf:about="http://vocab.nerc.ac.uk/collection/L22/current/NETT0021/">
<dc:identifier>SDN:L22::NETT0021</dc:identifier>
<skos:notation>SDN:L22::NETT0021</skos:notation>
<skos:prefLabel xml:lang="en">Clarke-Bumpus plankton sampler - Clarke and Bumpus (1939, 1950)</skos:prefLabel>
<skos:altLabel>Clarke-Bumpus plankton sampler</skos:altLabel>
<skos:definition xml:lang="en">Construction is a 12.7 cm diameter mouth opening with cylindrical tube 16.0 cm long. The tube is equipped with flat plate which pivots to open or close the flow through the tube and a flowmeter. A 61 cm long conical net is attached to the rear of the tube [Wiebe and Benfield 2003 Plate 8 A].</skos:definition>
<owl:versionInfo>1</owl:versionInfo>
<dc:date>2011-10-21 14:18:49.0</dc:date>
<skos:note xml:lang="en">accepted</skos:note>
<owl:deprecated>false</owl:deprecated>
<skos:broader rdf:resource="http://vocab.nerc.ac.uk/collection/L05/current/22/"/>
<skos:broader rdf:resource="http://vocab.nerc.ac.uk/collection/L05/current/388/"/>
<void:inDataset rdf:resource="http://vocab.nerc.ac.uk/.well-known/void"/>
</skos:Concept>
</skos:member>
<skos:member>
<skos:Concept rdf:about="http://vocab.nerc.ac.uk/collection/L22/current/TOOL0561/">
<dc:identifier>SDN:L22::TOOL0561</dc:identifier>
<skos:notation>SDN:L22::TOOL0561</skos:notation>
<skos:prefLabel xml:lang="en">Clean pumped sea water supply</skos:prefLabel>
<skos:altLabel>Clean pumped sea water supply</skos:altLabel>
<skos:definition xml:lang="en">The system comprises a precision echosounder (PES) fish attached to a clean, reinforced tube (typically composed of braided PVC). The fish is designed to be towed alongside a moving ship at a depth of 1-3m and water is drawn through the system by a clean pump. The tube usually leads to a clean laboratory on board the vessel, inside which samples are drawn for analysis. The system is typically used for continuous, underway, clean sampling (e.g., trace metal studies) of near-surface waters.</skos:definition>
<owl:versionInfo>2</owl:versionInfo>
<dc:date>2012-10-17 15:58:06.0</dc:date>
<skos:note xml:lang="en">accepted</skos:note>
<owl:deprecated>false</owl:deprecated>
<skos:broader rdf:resource="http://vocab.nerc.ac.uk/collection/L05/current/31/"/>
<void:inDataset rdf:resource="http://vocab.nerc.ac.uk/.well-known/void"/>
</skos:Concept>
</skos:member>
<skos:member>
<skos:Concept rdf:about="http://vocab.nerc.ac.uk/collection/L22/current/NETT0023/">
<dc:identifier>SDN:L22::NETT0023</dc:identifier>
<skos:notation>SDN:L22::NETT0023</skos:notation>
<skos:prefLabel xml:lang="en">Closing Net - Hart (1935)</skos:prefLabel>
<skos:altLabel>Hart net</skos:altLabel>
<skos:definition xml:lang="en">A rod of wood or pipe is outfitted with a combination wire clamp and closing release at the top and a pair of snap hooks at the bottom, one to secure the device to the wire and one to secure the bottom portion of the net. Attached to the rod is a net with a bridle which inserts into the release latch. Midway along the pipe is a second snap hook which is attached to the mid section of the net. Multiples of these units may be attached to the wire at various depth intervals as the wire is lowered vertically into the water.  Plankton collections are made as the nets are hauled up until a messenger hitting the release lets the bridle go, thus closing the net [Wiebe and Benfield 2003 Plate 5 B].</skos:definition>
<owl:versionInfo>1</owl:versionInfo>
<dc:date>2011-10-21 14:18:49.0</dc:date>
<skos:note xml:lang="en">accepted</skos:note>
<owl:deprecated>false</owl:deprecated>
<skos:broader rdf:resource="http://vocab.nerc.ac.uk/collection/L05/current/22/"/>
<void:inDataset rdf:resource="http://vocab.nerc.ac.uk/.well-known/void"/>
</skos:Concept>
</skos:member>
<skos:member>
<skos:Concept rdf:about="http://vocab.nerc.ac.uk/collection/L22/current/NETT0022/">
<dc:identifier>SDN:L22::NETT0022</dc:identifier>
<skos:notation>SDN:L22::NETT0022</skos:notation>
<skos:prefLabel xml:lang="en">Closing midwater trawl - Enzenhofer and Hume (1989)</skos:prefLabel>
<skos:altLabel>Enzhofer and Hume CMT</skos:altLabel>
<skos:definition xml:lang="en">Construction is a 300 cm x 700 cm rectangular mouth opening with net  1800 cm in length. The net is made from five sets of mesh with coarse mesh at the front and fine mesh at the back (600 cm of 10.2 cm mesh, 400 cm of 5.1 cm mesh, 300 cm of 1.9 cm mesh, 300 cm of 1.3 cm mesh and 200 cm of 0.3 cm mesh). There are two towing cables: one for the top spreader bar and one for the bottom. Each cable goes to separate winch. The net is lowered with tension on bottom spreader so that it is closed. Tension is then transferred to the top spreader to open the net. Tension again taken by lower spreader to close net [Wiebe and Benfield 2003 Plate 12 B].</skos:definition>
<owl:versionInfo>1</owl:versionInfo>
<dc:date>2011-10-21 14:18:49.0</dc:date>
<skos:note xml:lang="en">accepted</skos:note>
<owl:deprecated>false</owl:deprecated>
<skos:broader rdf:resource="http://vocab.nerc.ac.uk/collection/L05/current/23/"/>
<void:inDataset rdf:resource="http://vocab.nerc.ac.uk/.well-known/void"/>
</skos:Concept>
</skos:member>
<skos:member>
<skos:Concept rdf:about="http://vocab.nerc.ac.uk/collection/L22/current/NETT0006/">
<dc:identifier>SDN:L22::NETT0006</dc:identifier>
<skos:notation>SDN:L22::NETT0006</skos:notation>
<skos:prefLabel xml:lang="en">Closing net - Barnes (1953)</skos:prefLabel>
<skos:altLabel>Barnes net</skos:altLabel>
<skos:definition xml:lang="en">Construction is a hemispherical metal cowling mounted in front of a net ring with an opening sized so that a closing lid can be accommodated when the net is open. A Nansen messenger closing mechanism is used to release the spring loaded closing lid which pivots over the net mouth. No dimensions given for net size or mesh [Wiebe and Benfield 2003 Plate 8 C].</skos:definition>
<owl:versionInfo>1</owl:versionInfo>
<dc:date>2011-10-21 14:18:49.0</dc:date>
<skos:note xml:lang="en">accepted</skos:note>
<owl:deprecated>false</owl:deprecated>
<skos:broader rdf:resource="http://vocab.nerc.ac.uk/collection/L05/current/22/"/>
<void:inDataset rdf:resource="http://vocab.nerc.ac.uk/.well-known/void"/>
</skos:Concept>
</skos:member>
<skos:member>
<skos:Concept rdf:about="http://vocab.nerc.ac.uk/collection/L22/current/TOOL0302/">
<dc:identifier>SDN:L22::TOOL0302</dc:identifier>
<skos:notation>SDN:L22::TOOL0302</skos:notation>
<skos:prefLabel xml:lang="en">Coastal Leasing MacroTide water level recorder</skos:prefLabel>
<skos:altLabel>MacroTide WLR</skos:altLabel>
<skos:definition xml:lang="en">A sub-surface water level recorder designed for measurement of tidal signals and water temperature with an ICS Strain Gauge Pressure Sensor logged at 12-bit resolution and a YSI internal (or optionally external) thermistor. Pressure accuracy is 0.1% of measurement range. Temperature accuracy is 0.1C (resolution 0.02C).</skos:definition>
<owl:versionInfo>1</owl:versionInfo>
<dc:date>2010-05-18 16:10:58.0</dc:date>
<skos:note xml:lang="en">accepted</skos:note>
<owl:deprecated>false</owl:deprecated>
<skos:broader rdf:resource="http://vocab.nerc.ac.uk/collection/L05/current/111/"/>
<void:inDataset rdf:resource="http://vocab.nerc.ac.uk/.well-known/void"/>
</skos:Concept>
</skos:member>
<skos:member>
<skos:Concept rdf:about="http://vocab.nerc.ac.uk/collection/L22/current/TOOL0303/">
<dc:identifier>SDN:L22::TOOL0303</dc:identifier>
<skos:notation>SDN:L22::TOOL0303</skos:notation>
<skos:prefLabel xml:lang="en">Coastal Leasing MacroTide+ water level recorder</skos:prefLabel>
<skos:altLabel>MacroTide+ WLR</skos:altLabel>
<skos:definition xml:lang="en">A sub-surface water level recorder designed for measurement of tidal signals and water temperature with a Parascientific Digiquartz pressure sensor logged at 16-bit resolution and a YSI internal (or optionally external) thermistor. Pressure accuracy is 0.015% of measurement range. Temperature accuracy is 0.1C (resolution 0.02C).</skos:definition>
<owl:versionInfo>1</owl:versionInfo>
<dc:date>2010-05-18 16:10:58.0</dc:date>
<skos:note xml:lang="en">accepted</skos:note>
<owl:deprecated>false</owl:deprecated>
<skos:broader rdf:resource="http://vocab.nerc.ac.uk/collection/L05/current/111/"/>
<void:inDataset rdf:resource="http://vocab.nerc.ac.uk/.well-known/void"/>
</skos:Concept>
</skos:member>
<skos:member>
<skos:Concept rdf:about="http://vocab.nerc.ac.uk/collection/L22/current/NETT0024/">
<dc:identifier>SDN:L22::NETT0024</dc:identifier>
<skos:notation>SDN:L22::NETT0024</skos:notation>
<skos:prefLabel xml:lang="en">Cod-end sampler - Motoda (1953)</skos:prefLabel>
<skos:altLabel>Motoda cod-end sampler</skos:altLabel>
<skos:definition xml:lang="en">Construction is a 15.5 cm diameter mouth opening and 35.5 cm long body attached to 57 cm diameter net 200 cm long with bolting cloth 42.5 meshes per inch in upper 120 cm and 56.5 meshes per inch in lower 80 cm [Wiebe and Benfield 2003 Plate 25 A].</skos:definition>
<owl:versionInfo>1</owl:versionInfo>
<dc:date>2011-10-21 14:18:49.0</dc:date>
<skos:note xml:lang="en">accepted</skos:note>
<owl:deprecated>false</owl:deprecated>
<skos:broader rdf:resource="http://vocab.nerc.ac.uk/collection/L05/current/22/"/>
<void:inDataset rdf:resource="http://vocab.nerc.ac.uk/.well-known/void"/>
</skos:Concept>
</skos:member>
<skos:member>
<skos:Concept rdf:about="http://vocab.nerc.ac.uk/collection/L22/current/NETT0025/">
<dc:identifier>SDN:L22::NETT0025</dc:identifier>
<skos:notation>SDN:L22::NETT0025</skos:notation>
<skos:prefLabel xml:lang="en">Collapsible Rectangular Midwater Trawl 1+8 - Griffiths et al. (1980)</skos:prefLabel>
<skos:altLabel>Collapsible RMT 1+8</skos:altLabel>
<skos:definition xml:lang="en">The RMT 1+8 system described by Baker was modified to enable handling from smaller vessels without a crane using Kelly's eyes and chain rather than link wire.</skos:definition>
<owl:versionInfo>1</owl:versionInfo>
<dc:date>2011-10-21 14:18:49.0</dc:date>
<skos:note xml:lang="en">accepted</skos:note>
<owl:deprecated>false</owl:deprecated>
<skos:broader rdf:resource="http://vocab.nerc.ac.uk/collection/L05/current/388/"/>
<skos:broader rdf:resource="http://vocab.nerc.ac.uk/collection/L05/current/23/"/>
<skos:broader rdf:resource="http://vocab.nerc.ac.uk/collection/L05/current/134/"/>
<void:inDataset rdf:resource="http://vocab.nerc.ac.uk/.well-known/void"/>
</skos:Concept>
</skos:member>
<skos:member>
<skos:Concept rdf:about="http://vocab.nerc.ac.uk/collection/L22/current/TOOL0001/">
<dc:identifier>SDN:L22::TOOL0001</dc:identifier>
<skos:notation>SDN:L22::TOOL0001</skos:notation>
<skos:prefLabel xml:lang="en">Conductivity, temperature and depth package</skos:prefLabel>
<skos:altLabel>CTD</skos:altLabel>
<skos:definition xml:lang="en">A generic term for a set of co-located conductivity, temperature and pressure (proxy for depth) sensors.  The pressure sensor is generally used to ascertain the instrument Z co-ordinate in the water body, whilst the other sensors determine water temperature and salinity. Deployed on a range of platforms such as vertically lowered metal frames, towed fish, AUVs or moorings.</skos:definition>
<owl:versionInfo>1</owl:versionInfo>
<dc:date>2012-01-05 09:34:05.0</dc:date>
<skos:note xml:lang="en">accepted</skos:note>
<owl:deprecated>false</owl:deprecated>
<skos:related rdf:resource="http://vocab.nerc.ac.uk/collection/P01/current/TEMPST01/"/>
<skos:related rdf:resource="http://vocab.nerc.ac.uk/collection/P01/current/PSALPR01/"/>
<skos:related rdf:resource="http://vocab.nerc.ac.uk/collection/P01/current/PRESPR01/"/>
<skos:related rdf:resource="http://vocab.nerc.ac.uk/collection/L05/current/130/"/>
<skos:broader rdf:resource="http://vocab.nerc.ac.uk/collection/L05/current/134/"/>
<skos:broader rdf:resource="http://vocab.nerc.ac.uk/collection/L05/current/350/"/>
<void:inDataset rdf:resource="http://vocab.nerc.ac.uk/.well-known/void"/>
</skos:Concept>
</skos:member>
<skos:member>
<skos:Concept rdf:about="http://vocab.nerc.ac.uk/collection/L22/current/NETT0026/">
<dc:identifier>SDN:L22::NETT0026</dc:identifier>
<skos:notation>SDN:L22::NETT0026</skos:notation>
<skos:prefLabel xml:lang="en">Continuous Plankton Recorder - Hardy (1926, 1936); Glover (1962)</skos:prefLabel>
<skos:altLabel>CPR</skos:altLabel>
<skos:definition xml:lang="en">Construction is a 1.27 cm on side square mouth opening (originally 10.1 cm diameter) high-speed (12 to 17 knots) towed body collecting plankton on gauze (22.9 cm wide and 23.6 meshes per cm) rolls. The body is 50 cm wide x 50 cm tall x 100 cm long.  A propellor drives the rollers winding up the gauze.  The system is normally towed at 10 m depth at speeds up to 20 ktnos [Wiebe and Benfield 2003 Plate 19 A, B].</skos:definition>
<owl:versionInfo>1</owl:versionInfo>
<dc:date>2011-10-21 14:18:49.0</dc:date>
<skos:note xml:lang="en">accepted</skos:note>
<owl:deprecated>false</owl:deprecated>
<skos:broader rdf:resource="http://vocab.nerc.ac.uk/collection/L05/current/21/"/>
<void:inDataset rdf:resource="http://vocab.nerc.ac.uk/.well-known/void"/>
</skos:Concept>
</skos:member>
<skos:member>
<skos:Concept rdf:about="http://vocab.nerc.ac.uk/collection/L22/current/TOOL0571/">
<dc:identifier>SDN:L22::TOOL0571</dc:identifier>
<skos:notation>SDN:L22::TOOL0571</skos:notation>
<skos:prefLabel xml:lang="en">Copper pipe air sampler</skos:prefLabel>
<skos:altLabel>Copper pipe air sampler</skos:altLabel>
<skos:definition xml:lang="en">Copper tubing leading directly from the least contaminated part of a ship to an analytical instrument. Air is drawn through the pipe by the instrument.</skos:definition>
<owl:versionInfo>1</owl:versionInfo>
<dc:date>2012-11-15 09:32:51.0</dc:date>
<skos:note xml:lang="en">accepted</skos:note>
<owl:deprecated>false</owl:deprecated>
<skos:broader rdf:resource="http://vocab.nerc.ac.uk/collection/L05/current/58/"/>
<void:inDataset rdf:resource="http://vocab.nerc.ac.uk/.well-known/void"/>
</skos:Concept>
</skos:member>
<skos:member>
<skos:Concept rdf:about="http://vocab.nerc.ac.uk/collection/L22/current/TOOL0280/">
<dc:identifier>SDN:L22::TOOL0280</dc:identifier>
<skos:notation>SDN:L22::TOOL0280</skos:notation>
<skos:prefLabel xml:lang="en">Cup and vane anemometer</skos:prefLabel>
<skos:altLabel>Cup and vane anemometer</skos:altLabel>
<skos:definition xml:lang="en">A generic term for a device that measures windspeed by determining the speed of rotation of 3 cups mounted on horizontal arms with a central pivot and wind direction by determining the orientation of a separate pivot-mounted sail. The term is for use where the measurement principle is known, but details of the make and model number are not known.</skos:definition>
<owl:versionInfo>1</owl:versionInfo>
<dc:date>2010-05-18 16:10:58.0</dc:date>
<skos:note xml:lang="en">accepted</skos:note>
<owl:deprecated>false</owl:deprecated>
<skos:broader rdf:resource="http://vocab.nerc.ac.uk/collection/L05/current/101/"/>
<void:inDataset rdf:resource="http://vocab.nerc.ac.uk/.well-known/void"/>
</skos:Concept>
</skos:member>
<skos:member>
<skos:Concept rdf:about="http://vocab.nerc.ac.uk/collection/L22/current/TOOL0563/">
<dc:identifier>SDN:L22::TOOL0563</dc:identifier>
<skos:notation>SDN:L22::TOOL0563</skos:notation>
<skos:prefLabel xml:lang="en">Cyclonic separation sampler</skos:prefLabel>
<skos:altLabel>Cyclonic separation sampler</skos:altLabel>
<skos:definition xml:lang="en">A device designed to remove particulates from an air, gas or liquid stream through vortex separation. A high speed rotating flow is established within a vertical cylindrical or conical container, where the stream to be separated is fed in the top (wide) end, flows helically around the container to the bottom (narrow) end and then exits the cyclone in a straight stream through the centre and out the top. Instead of following the flow of the stream, the inertia of large (dense) particles causes them to hit the sides of the container and fall to the bottom, where they can be removed. The cyclone geometry and flow rate define a cut point, which is the size of the particle that will be removed from the stream with 50% efficiency. Larger particles will be removed with a greater efficiency and smaller particles with a lower efficiency. The sampler may be used in series with filters designed to collect different target particles.</skos:definition>
<owl:versionInfo>1</owl:versionInfo>
<dc:date>2012-10-15 14:57:16.0</dc:date>
<skos:note xml:lang="en">accepted</skos:note>
<owl:deprecated>false</owl:deprecated>
<skos:broader rdf:resource="http://vocab.nerc.ac.uk/collection/L05/current/58/"/>
<void:inDataset rdf:resource="http://vocab.nerc.ac.uk/.well-known/void"/>
</skos:Concept>
</skos:member>
<skos:member>
<skos:Concept rdf:about="http://vocab.nerc.ac.uk/collection/L22/current/TOOL0579/">
<dc:identifier>SDN:L22::TOOL0579</dc:identifier>
<skos:notation>SDN:L22::TOOL0579</skos:notation>
<skos:prefLabel xml:lang="en">D and A Instruments Optical Backscatter Sensor OBS-3</skos:prefLabel>
<skos:altLabel>D and A OBS-3</skos:altLabel>
<skos:definition xml:lang="en">Optical backscatter instrument measuring scattering in water between 140 - 160deg for a wavelength of 875nm. It has a turbidity range of 0-2000 FTU and a maximum working depth of 500m. This instrument was superseded by the OBS-3+ model in 2005. The D and A Instrument Company and its OBS product line were purchased by Campbell Scientific Inc who now has full responsibility for D and A Instruments.</skos:definition>
<owl:versionInfo>1</owl:versionInfo>
<dc:date>2012-12-18 15:09:37.0</dc:date>
<skos:note xml:lang="en">accepted</skos:note>
<owl:deprecated>false</owl:deprecated>
<skos:broader rdf:resource="http://vocab.nerc.ac.uk/collection/L05/current/123/"/>
<void:inDataset rdf:resource="http://vocab.nerc.ac.uk/.well-known/void"/>
</skos:Concept>
</skos:member>
<skos:member>
<skos:Concept rdf:about="http://vocab.nerc.ac.uk/collection/L22/current/NETT0028/">
<dc:identifier>SDN:L22::NETT0028</dc:identifier>
<skos:notation>SDN:L22::NETT0028</skos:notation>
<skos:prefLabel xml:lang="en">DBAD-MOCNESS - Wiebe (1994); Greene (1998)</skos:prefLabel>
<skos:altLabel>DBAD-MOCNESS</skos:altLabel>
<skos:definition xml:lang="en">A 1-m2 MOCNESS was equipped with a dual-beam echosounder and dual-axis training mechanism for the transducers.  An electro-optical cable was used data telemetry [Wiebe and Benfield 2003 Plate 40 E].</skos:definition>
<owl:versionInfo>1</owl:versionInfo>
<dc:date>2011-10-21 14:18:49.0</dc:date>
<skos:note xml:lang="en">accepted</skos:note>
<owl:deprecated>false</owl:deprecated>
<skos:broader rdf:resource="http://vocab.nerc.ac.uk/collection/L05/current/351/"/>
<skos:broader rdf:resource="http://vocab.nerc.ac.uk/collection/L05/current/183/"/>
<skos:broader rdf:resource="http://vocab.nerc.ac.uk/collection/L05/current/113/"/>
<skos:broader rdf:resource="http://vocab.nerc.ac.uk/collection/L05/current/134/"/>
<skos:broader rdf:resource="http://vocab.nerc.ac.uk/collection/L05/current/68/"/>
<skos:broader rdf:resource="http://vocab.nerc.ac.uk/collection/L05/current/124/"/>
<skos:broader rdf:resource="http://vocab.nerc.ac.uk/collection/L05/current/122/"/>
<skos:broader rdf:resource="http://vocab.nerc.ac.uk/collection/L05/current/23/"/>
<skos:broader rdf:resource="http://vocab.nerc.ac.uk/collection/L05/current/350/"/>
<void:inDataset rdf:resource="http://vocab.nerc.ac.uk/.well-known/void"/>
</skos:Concept>
</skos:member>
<skos:member>
<skos:Concept rdf:about="http://vocab.nerc.ac.uk/collection/L22/current/TOOL0553/">
<dc:identifier>SDN:L22::TOOL0553</dc:identifier>
<skos:notation>SDN:L22::TOOL0553</skos:notation>
<skos:prefLabel xml:lang="en">DGT Research Diffusive Gradients in Thin Films trace metal sampler</skos:prefLabel>
<skos:altLabel>DGT trace metal sampler</skos:altLabel>
<skos:definition xml:lang="en">A device designed to measure concentrations of dissolved metal species in water. It comprises a plastic casing that contains a Chelex resin impregnated in a hydrogel to accumulate metals. The resin layer is overlain by a diffusive layer of hydrogel and a filter. Ions diffuse through the filter and diffusive layer to reach the resin layer, thereby establishing a constant concentration gradient in the diffusive layer that allows the quantitative measurement of labile species in solution through laboratory analysis.</skos:definition>
<owl:versionInfo>3</owl:versionInfo>
<dc:date>2012-11-15 10:40:15.0</dc:date>
<skos:note xml:lang="en">accepted</skos:note>
<owl:deprecated>false</owl:deprecated>
<skos:broader rdf:resource="http://vocab.nerc.ac.uk/collection/L05/current/TFSAMP/"/>
<void:inDataset rdf:resource="http://vocab.nerc.ac.uk/.well-known/void"/>
</skos:Concept>
</skos:member>
<skos:member>
<skos:Concept rdf:about="http://vocab.nerc.ac.uk/collection/L22/current/TOOL0533/">
<dc:identifier>SDN:L22::TOOL0533</dc:identifier>
<skos:notation>SDN:L22::TOOL0533</skos:notation>
<skos:prefLabel xml:lang="en">DTU Nutech GM-25-5A beta Multicounter system</skos:prefLabel>
<skos:altLabel>DTU Nutech GM-25-5A</skos:altLabel>
<skos:definition xml:lang="en">A laboratory instrument designed to count beta particles emitted by a sample using the Geiger-Muller principle. A steady gas stream of argon (99%) and isobutene or propane (1%) becomes ionised due to beta particle emission from the sample, and the ionised gas particles are collected within a high voltage field, detected as an electric current pulse and recorded as a counting event. A guard counter allows the removal of the cosmic background radiation signal. The instrument is typically placed inside a lead shielding to reduce the ambient background radiation.</skos:definition>
<owl:versionInfo>1</owl:versionInfo>
<dc:date>2012-08-21 12:05:06.0</dc:date>
<skos:note xml:lang="en">accepted</skos:note>
<owl:deprecated>false</owl:deprecated>
<skos:broader rdf:resource="http://vocab.nerc.ac.uk/collection/L05/current/LAB39/"/>
<void:inDataset rdf:resource="http://vocab.nerc.ac.uk/.well-known/void"/>
</skos:Concept>
</skos:member>
<skos:member>
<skos:Concept rdf:about="http://vocab.nerc.ac.uk/collection/L22/current/TOOL0013/">
<dc:identifier>SDN:L22::TOOL0013</dc:identifier>
<skos:notation>SDN:L22::TOOL0013</skos:notation>
<skos:prefLabel xml:lang="en">Dataring pressure point transducer</skos:prefLabel>
<skos:altLabel>Pressure point</skos:altLabel>
<skos:definition xml:lang="en">The Dataring pressure point comprises differential transducers contained in a watertight housing. The reference port is vented to atmosphere via the power supply and signal cable tube, while the measuring port of the transducer is connected to a copper outlet nozzle on the top of the transducer housing. The copper nozzle, transducer measuring port and connecting tube are filled with oil so the pressure is transmitted to the crystal element via the oil, thus keeping the transducer components free from the effects of the saltwater.</skos:definition>
<owl:versionInfo>1</owl:versionInfo>
<dc:date>2008-11-28 07:54:41.0</dc:date>
<skos:note xml:lang="en">accepted</skos:note>
<owl:deprecated>false</owl:deprecated>
<skos:broader rdf:resource="http://vocab.nerc.ac.uk/collection/L05/current/111/"/>
<void:inDataset rdf:resource="http://vocab.nerc.ac.uk/.well-known/void"/>
</skos:Concept>
</skos:member>
<skos:member>
<skos:Concept rdf:about="http://vocab.nerc.ac.uk/collection/L22/current/TOOL0268/">
<dc:identifier>SDN:L22::TOOL0268</dc:identifier>
<skos:notation>SDN:L22::TOOL0268</skos:notation>
<skos:prefLabel xml:lang="en">Datawell directional waverider buoy</skos:prefLabel>
<skos:altLabel>Datawell waverider</skos:altLabel>
<skos:definition xml:lang="en">A directional waverider buoy comprising a heave-pitch-roll sensor, two accelerometers and a 3-axis fluxgate compass in a 90cm diameter spherical buoy that measures waves using a translational principle so that horizontal motions rather than wave slopes are measured making the measurement independent of buoy roll motions. A single point rubber cord vertical mooring ensures adequate symmetrical horizontal buoy response to resolve small motions at low frequencies. Data are transmitted to a shore based station and/or an Argos satellite. Three versions of the buoy designated MkI, MkII and MkIII have been produced with evolving internal electronics but fundamentally the same design. More information may be found at http://www.bodc.ac.uk/data/documents/nodb/65329/</skos:definition>
<owl:versionInfo>1</owl:versionInfo>
<dc:date>2010-05-18 16:10:58.0</dc:date>
<skos:note xml:lang="en">accepted</skos:note>
<owl:deprecated>false</owl:deprecated>
<skos:broader rdf:resource="http://vocab.nerc.ac.uk/collection/L05/current/110/"/>
<void:inDataset rdf:resource="http://vocab.nerc.ac.uk/.well-known/void"/>
</skos:Concept>
</skos:member>
<skos:member>
<skos:Concept rdf:about="http://vocab.nerc.ac.uk/collection/L22/current/TOOL0337/">
<dc:identifier>SDN:L22::TOOL0337</dc:identifier>
<skos:notation>SDN:L22::TOOL0337</skos:notation>
<skos:prefLabel xml:lang="en">Decca main chain navigation receiver</skos:prefLabel>
<skos:altLabel>Decca navigation</skos:altLabel>
<skos:definition xml:lang="en">A hyperbolic low-frequency (70 and 130 kHz) signal receiver that determined position based on the phase difference between signals transmitted by groups of a master plus three slave transmitters. Range depended on radio reception conditions but was typically 450km (day) to 750km (night). Accuracy ranged from 50m (day) or 200m (night) in ideal conditions down to 2km near the range limit. The system operated from the WWII until the UK transmitters were switched off at the end of March 2000.</skos:definition>
<owl:versionInfo>1</owl:versionInfo>
<dc:date>2010-09-06 12:45:22.0</dc:date>
<skos:note xml:lang="en">accepted</skos:note>
<owl:deprecated>false</owl:deprecated>
<skos:broader rdf:resource="http://vocab.nerc.ac.uk/collection/L05/current/POS01/"/>
<void:inDataset rdf:resource="http://vocab.nerc.ac.uk/.well-known/void"/>
</skos:Concept>
</skos:member>
<skos:member>
<skos:Concept rdf:about="http://vocab.nerc.ac.uk/collection/L22/current/NETT0034/">
<dc:identifier>SDN:L22::NETT0034</dc:identifier>
<skos:notation>SDN:L22::NETT0034</skos:notation>
<skos:prefLabel xml:lang="en">Deep Submergence Rescue Vehicle Alvin Net-1 - Grice and Huelsemann (1970)</skos:prefLabel>
<skos:altLabel>DSRV Alvin Net-1</skos:altLabel>
<skos:definition xml:lang="en">A pair of nets were mounted onto the front of DSRV Alvin for collecting planktobenthos at great depths. The mouth openings were D-shaped and hinged so that on descent and ascent of the submersible, the nets could be turned back away from the flow and would not filter. The Alvin arm was used by the pilot to open and close the net.  The nets had 0.233 mm mesh [Wiebe and Benfield 2003 Plate 23 D].</skos:definition>
<owl:versionInfo>1</owl:versionInfo>
<dc:date>2011-10-21 14:18:49.0</dc:date>
<skos:note xml:lang="en">accepted</skos:note>
<owl:deprecated>false</owl:deprecated>
<skos:broader rdf:resource="http://vocab.nerc.ac.uk/collection/L05/current/22/"/>
<void:inDataset rdf:resource="http://vocab.nerc.ac.uk/.well-known/void"/>
</skos:Concept>
</skos:member>
<skos:member>
<skos:Concept rdf:about="http://vocab.nerc.ac.uk/collection/L22/current/NETT0035/">
<dc:identifier>SDN:L22::NETT0035</dc:identifier>
<skos:notation>SDN:L22::NETT0035</skos:notation>
<skos:prefLabel xml:lang="en">Deep Submergence Rescue Vehicle Alvin Net-2 - Grice (1972)</skos:prefLabel>
<skos:altLabel>DSRV Alvin Net-2</skos:altLabel>
<skos:definition xml:lang="en">A pair of nets were attached to a pair of rectangular frames 61 cm wide x 31 cm tall which each had a metal door hinged at the top.  The Alvin arm was  used by the pilot to open and close the door.  The nets were positioned about 20 cm above the bottom. The nets had 0.239 mm mesh. Normal pushing speed was 1 knot [Wiebe and Benfield 2003 Plate 23 E].</skos:definition>
<owl:versionInfo>1</owl:versionInfo>
<dc:date>2011-10-21 14:18:49.0</dc:date>
<skos:note xml:lang="en">accepted</skos:note>
<owl:deprecated>false</owl:deprecated>
<skos:broader rdf:resource="http://vocab.nerc.ac.uk/collection/L05/current/22/"/>
<void:inDataset rdf:resource="http://vocab.nerc.ac.uk/.well-known/void"/>
</skos:Concept>
</skos:member>
<skos:member>
<skos:Concept rdf:about="http://vocab.nerc.ac.uk/collection/L22/current/NETT0030/">
<dc:identifier>SDN:L22::NETT0030</dc:identifier>
<skos:notation>SDN:L22::NETT0030</skos:notation>
<skos:prefLabel xml:lang="en">Deep-Tow net system - Wishner (1980)</skos:prefLabel>
<skos:altLabel>Wishner Deep-Tow net system</skos:altLabel>
<skos:definition xml:lang="en">Three rectangular mouth opening nets ~30 cm wide x 44 cm tall and 130 cm long mounted on a metal framework attached to the bottom of the Deep-Tow Instrument . The unobstructed nets were opened/closed by surface command transmitted via conducting cable to a release mechanism [Wiebe and Benfield 2003 Plate 24 A].</skos:definition>
<owl:versionInfo>1</owl:versionInfo>
<dc:date>2011-10-21 14:18:49.0</dc:date>
<skos:note xml:lang="en">accepted</skos:note>
<owl:deprecated>false</owl:deprecated>
<skos:broader rdf:resource="http://vocab.nerc.ac.uk/collection/L05/current/68/"/>
<skos:broader rdf:resource="http://vocab.nerc.ac.uk/collection/L05/current/22/"/>
<void:inDataset rdf:resource="http://vocab.nerc.ac.uk/.well-known/void"/>
</skos:Concept>
</skos:member>
<skos:member>
<skos:Concept rdf:about="http://vocab.nerc.ac.uk/collection/L22/current/TOOL0128/">
<dc:identifier>SDN:L22::TOOL0128</dc:identifier>
<skos:notation>SDN:L22::TOOL0128</skos:notation>
<skos:prefLabel xml:lang="en">Didcot/ELE DRP-5 PAR sensor</skos:prefLabel>
<skos:altLabel>DRP-5 PAR</skos:altLabel>
<skos:definition xml:lang="en">A sensor that measures the photon flux density of light in the 400-700nm waveband using a blue-enhanced silicon photocell. Cosine correction ensures that readings are obtained from widely varied angles of incidence.</skos:definition>
<owl:versionInfo>1</owl:versionInfo>
<dc:date>2010-05-18 16:10:58.0</dc:date>
<skos:note xml:lang="en">accepted</skos:note>
<owl:deprecated>false</owl:deprecated>
<skos:related rdf:resource="http://vocab.nerc.ac.uk/collection/P01/current/DWIRRXSD/"/>
<skos:broader rdf:resource="http://vocab.nerc.ac.uk/collection/L05/current/122/"/>
<void:inDataset rdf:resource="http://vocab.nerc.ac.uk/.well-known/void"/>
</skos:Concept>
</skos:member>
<skos:member>
<skos:Concept rdf:about="http://vocab.nerc.ac.uk/collection/L22/current/TOOL0659/">
<dc:identifier>SDN:L22::TOOL0659</dc:identifier>
<skos:notation>SDN:L22::TOOL0659</skos:notation>
<skos:prefLabel xml:lang="en">Dionex ICS-2500 ion chromatograph</skos:prefLabel>
<skos:altLabel>Dionex ICS-2500 IC</skos:altLabel>
<skos:definition xml:lang="en">A gas chromatograph that separates and analyses compounds that do not degrade or decompose in the gas phase. The instrument can be configured with a wide range of modules to build the optimum system for an application. The ICS-2500 features include component modularity, a variety of pump configurations, multiple detectors, full automation capability and System Wellness. The instrument was originally manufactured by Dionex Corporation which was bought by Thermo Scientific (part of Thermo Fisher Scientific). The ICS-2500 was introduced in 2005 and is no longer in production.</skos:definition>
<owl:versionInfo>1</owl:versionInfo>
<dc:date>2014-01-27 15:36:42.0</dc:date>
<skos:note xml:lang="en">accepted</skos:note>
<owl:deprecated>false</owl:deprecated>
<skos:broader rdf:resource="http://vocab.nerc.ac.uk/collection/L05/current/LAB15/"/>
<void:inDataset rdf:resource="http://vocab.nerc.ac.uk/.well-known/void"/>
</skos:Concept>
</skos:member>
<skos:member>
<skos:Concept rdf:about="http://vocab.nerc.ac.uk/collection/L22/current/NETT0108/">
<dc:identifier>SDN:L22::NETT0108</dc:identifier>
<skos:notation>SDN:L22::NETT0108</skos:notation>
<skos:prefLabel xml:lang="en">Discovery net N70 V net - Currie and Foxton (1956)</skos:prefLabel>
<skos:altLabel>Discovery net</skos:altLabel>
<skos:definition xml:lang="en">A version of the Nansen net with a 70 cm diameter mouth opening with 3 nearly cylindrical net sections and a final conical section. Section 1 with .63 cm mesh, section 2 canvas for closing rope, section 3 made of silk with 40 meshes per inch (15.7 meshes per 1 cm), and  section 4 made of silk with 74 meshes per inch (29.1 meshes per 1 cm)</skos:definition>
<owl:versionInfo>1</owl:versionInfo>
<dc:date>2011-10-21 14:18:49.0</dc:date>
<skos:note xml:lang="en">accepted</skos:note>
<owl:deprecated>false</owl:deprecated>
<skos:broader rdf:resource="http://vocab.nerc.ac.uk/collection/L05/current/22/"/>
<void:inDataset rdf:resource="http://vocab.nerc.ac.uk/.well-known/void"/>
</skos:Concept>
</skos:member>
<skos:member>
<skos:Concept rdf:about="http://vocab.nerc.ac.uk/collection/L22/current/NETT0029/">
<dc:identifier>SDN:L22::NETT0029</dc:identifier>
<skos:notation>SDN:L22::NETT0029</skos:notation>
<skos:prefLabel xml:lang="en">Discrete-depth plankton sampler - Aron et al. (1964)</skos:prefLabel>
<skos:altLabel>DDPS</skos:altLabel>
<skos:definition xml:lang="en">A cod-end sampler used with IKMT or a 1-m diameter net with underwater electronics to sample depth and temperature operated with single conductor cable. Mark III had 10 or 15 cm diameter opening and four catch chambers [Wiebe and Benfield 2003 Plate 26 B].</skos:definition>
<owl:versionInfo>1</owl:versionInfo>
<dc:date>2011-10-21 14:18:49.0</dc:date>
<skos:note xml:lang="en">accepted</skos:note>
<owl:deprecated>false</owl:deprecated>
<skos:broader rdf:resource="http://vocab.nerc.ac.uk/collection/L05/current/22/"/>
<skos:broader rdf:resource="http://vocab.nerc.ac.uk/collection/L05/current/134/"/>
<void:inDataset rdf:resource="http://vocab.nerc.ac.uk/.well-known/void"/>
</skos:Concept>
</skos:member>
<skos:member>
<skos:Concept rdf:about="http://vocab.nerc.ac.uk/collection/L22/current/NETT0031/">
<dc:identifier>SDN:L22::NETT0031</dc:identifier>
<skos:notation>SDN:L22::NETT0031</skos:notation>
<skos:prefLabel xml:lang="en">Diver tow net - Emery (1968)</skos:prefLabel>
<skos:altLabel>Emery diver tow net</skos:altLabel>
<skos:definition xml:lang="en">A 30 cm diameter ring net with 0.183 mm mesh towed by diver.</skos:definition>
<owl:versionInfo>1</owl:versionInfo>
<dc:date>2011-10-21 14:18:49.0</dc:date>
<skos:note xml:lang="en">accepted</skos:note>
<owl:deprecated>false</owl:deprecated>
<skos:broader rdf:resource="http://vocab.nerc.ac.uk/collection/L05/current/22/"/>
<void:inDataset rdf:resource="http://vocab.nerc.ac.uk/.well-known/void"/>
</skos:Concept>
</skos:member>
<skos:member>
<skos:Concept rdf:about="http://vocab.nerc.ac.uk/collection/L22/current/NETT0032/">
<dc:identifier>SDN:L22::NETT0032</dc:identifier>
<skos:notation>SDN:L22::NETT0032</skos:notation>
<skos:prefLabel xml:lang="en">Diver-pushed net - Porter (1973)</skos:prefLabel>
<skos:altLabel>Porter diver-pushed net</skos:altLabel>
<skos:definition xml:lang="en">A 50 cm diameter ring net 200 cm long with 0.12 mm mesh pushed by a diver.</skos:definition>
<owl:versionInfo>1</owl:versionInfo>
<dc:date>2011-10-21 14:18:49.0</dc:date>
<skos:note xml:lang="en">accepted</skos:note>
<owl:deprecated>false</owl:deprecated>
<skos:broader rdf:resource="http://vocab.nerc.ac.uk/collection/L05/current/22/"/>
<void:inDataset rdf:resource="http://vocab.nerc.ac.uk/.well-known/void"/>
</skos:Concept>
</skos:member>
<skos:member>
<skos:Concept rdf:about="http://vocab.nerc.ac.uk/collection/L22/current/NETT0033/">
<dc:identifier>SDN:L22::NETT0033</dc:identifier>
<skos:notation>SDN:L22::NETT0033</skos:notation>
<skos:prefLabel xml:lang="en">Double Longhurst-Hardy Plankton Recorder - Williams et al. (1983)</skos:prefLabel>
<skos:altLabel>Double LHPR</skos:altLabel>
<skos:definition xml:lang="en">A modified version of the LHPR . An unenclosed Lowestoft Sampler , 130 cm high x 92 cm wide x 357 cm long and with a 35.6 cm expanding to 76 cm diameter nose cone was used with a recorder box (with 0.28 mm nylon mesh gauze) attached to the cod-end of a main net. A second recorder box was attached to the end of 0.053 mm polyester mesh net. The mouth of this net was attached to a nose cone with 2.6 and 5.1 diameter  mouth openings expanding to 7.7 cm. System acoustically (IOS) telemeters depth, flow, and temperature.  System also carries a chlorophyll sensor with recorder system. Nose cones of both nets have doors that are shut when system deployed and can be opened remotely.  Designed to tow up to 6 knots [Wiebe and Benfield 2003 Plate 27 A].</skos:definition>
<owl:versionInfo>1</owl:versionInfo>
<dc:date>2011-10-21 14:18:49.0</dc:date>
<skos:note xml:lang="en">accepted</skos:note>
<owl:deprecated>false</owl:deprecated>
<skos:broader rdf:resource="http://vocab.nerc.ac.uk/collection/L05/current/134/"/>
<skos:broader rdf:resource="http://vocab.nerc.ac.uk/collection/L05/current/113/"/>
<skos:broader rdf:resource="http://vocab.nerc.ac.uk/collection/L05/current/388/"/>
<skos:broader rdf:resource="http://vocab.nerc.ac.uk/collection/L05/current/21/"/>
<void:inDataset rdf:resource="http://vocab.nerc.ac.uk/.well-known/void"/>
</skos:Concept>
</skos:member>
<skos:member>
<skos:Concept rdf:about="http://vocab.nerc.ac.uk/collection/L22/current/TOOL0066/">
<dc:identifier>SDN:L22::TOOL0066</dc:identifier>
<skos:notation>SDN:L22::TOOL0066</skos:notation>
<skos:prefLabel xml:lang="en">Dr.Haardt BackScat Fluorometer Model 1302</skos:prefLabel>
<skos:altLabel>BackScat 1302</skos:altLabel>
<skos:definition xml:lang="en">Backscatter fluorometer comprising three optical sensors integrated into one housing with a light source of 2 xenon flash tubes and filters for the detection of chlorophyll, yellow substance (gelbstoff) and Mie backscattering.</skos:definition>
<owl:versionInfo>1</owl:versionInfo>
<dc:date>2010-09-08 10:09:52.0</dc:date>
<skos:note xml:lang="en">accepted</skos:note>
<owl:deprecated>false</owl:deprecated>
<skos:broader rdf:resource="http://vocab.nerc.ac.uk/collection/L05/current/123/"/>
<skos:broader rdf:resource="http://vocab.nerc.ac.uk/collection/L05/current/113/"/>
<void:inDataset rdf:resource="http://vocab.nerc.ac.uk/.well-known/void"/>
</skos:Concept>
</skos:member>
<skos:member>
<skos:Concept rdf:about="http://vocab.nerc.ac.uk/collection/L22/current/TOOL0408/">
<dc:identifier>SDN:L22::TOOL0408</dc:identifier>
<skos:notation>SDN:L22::TOOL0408</skos:notation>
<skos:prefLabel xml:lang="en">Dr.Haardt BackScat I Fluorometer Model 1101</skos:prefLabel>
<skos:altLabel>BackScat I 1101</skos:altLabel>
<skos:definition xml:lang="en">Backscatter fluorometer with a xenon-flashlight source and filter for the detection of chlorophyll-a. The titanium housing has a maximum depth rating of 6000 m.</skos:definition>
<owl:versionInfo>1</owl:versionInfo>
<dc:date>2011-07-27 13:50:44.0</dc:date>
<skos:note xml:lang="en">accepted</skos:note>
<owl:deprecated>false</owl:deprecated>
<skos:broader rdf:resource="http://vocab.nerc.ac.uk/collection/L05/current/113/"/>
<skos:broader rdf:resource="http://vocab.nerc.ac.uk/collection/L05/current/123/"/>
<void:inDataset rdf:resource="http://vocab.nerc.ac.uk/.well-known/void"/>
</skos:Concept>
</skos:member>
<skos:member>
<skos:Concept rdf:about="http://vocab.nerc.ac.uk/collection/L22/current/TOOL0406/">
<dc:identifier>SDN:L22::TOOL0406</dc:identifier>
<skos:notation>SDN:L22::TOOL0406</skos:notation>
<skos:prefLabel xml:lang="en">Droplet Measurement Technologies Passive Cavity Aerosol Spectrometer Probe (PCASP) 100</skos:prefLabel>
<skos:altLabel>DMT PCASP 100</skos:altLabel>
<skos:definition xml:lang="en">The PCASP 100 is an optical particle counter that measures aerosol particle size distributions. It uses a 5 mW He-Ne passive cavity laser, directed onto the aerodynamically focussed air sample. Scattered light is collected at angles between 35 degrees and 120 degrees, and focussed onto a photodetector. Particle size is determined from the light scattering intensity using MIe scattering theory, assuming a spherical particle of refractive index 1.58. The instrument was developed by Particle Measuring Systems and was sold to Droplet Measurement Technologies.</skos:definition>
<owl:versionInfo>1</owl:versionInfo>
<dc:date>2011-07-27 13:50:44.0</dc:date>
<skos:note xml:lang="en">accepted</skos:note>
<owl:deprecated>false</owl:deprecated>
<skos:broader rdf:resource="http://vocab.nerc.ac.uk/collection/L05/current/386/"/>
<skos:broader rdf:resource="http://vocab.nerc.ac.uk/collection/L05/current/13/"/>
<skos:broader rdf:resource="http://vocab.nerc.ac.uk/collection/L05/current/58/"/>
<void:inDataset rdf:resource="http://vocab.nerc.ac.uk/.well-known/void"/>
</skos:Concept>
</skos:member>
<skos:member>
<skos:Concept rdf:about="http://vocab.nerc.ac.uk/collection/L22/current/TOOL0196/">
<dc:identifier>SDN:L22::TOOL0196</dc:identifier>
<skos:notation>SDN:L22::TOOL0196</skos:notation>
<skos:prefLabel xml:lang="en">Druck RPT 301 barometer</skos:prefLabel>
<skos:altLabel>Druck RPT 301 barometer</skos:altLabel>
<skos:definition xml:lang="en">A barometer based on silicon pressure sensor having a multi-layer construction. The resonator and pressure sensitive diaphragm micro-machined from one piece of silicon. The resonator is bonded to a second silicon wafer containing the drive and pick-up system under vacuum.</skos:definition>
<owl:versionInfo>1</owl:versionInfo>
<dc:date>2010-05-18 16:10:58.0</dc:date>
<skos:note xml:lang="en">accepted</skos:note>
<owl:deprecated>false</owl:deprecated>
<skos:broader rdf:resource="http://vocab.nerc.ac.uk/collection/L05/current/102/"/>
<void:inDataset rdf:resource="http://vocab.nerc.ac.uk/.well-known/void"/>
</skos:Concept>
</skos:member>
<skos:member>
<skos:Concept rdf:about="http://vocab.nerc.ac.uk/collection/L22/current/TOOL0437/">
<dc:identifier>SDN:L22::TOOL0437</dc:identifier>
<skos:notation>SDN:L22::TOOL0437</skos:notation>
<skos:prefLabel xml:lang="en">EcoMonitor PumpProbe Fluorometer</skos:prefLabel>
<skos:altLabel>EcoMonitor PProbe fluorometer</skos:altLabel>
<skos:definition xml:lang="en">A submersible double-flash pulse fluorometer for continuous, in situ measurement of chlorophyll fluorescence parameters. It contains two excitation channels and one emission channel. One of the excitation channels provides a weak, probe flash used for measuring the fluorescence yield of Photosystem II (PSII). The other excitation channel provides a pump flash which is used for closing the reaction centres of PSII. Both excitation signals are generated by xenon flash-lamps. The light from the flash-lamps is collected by condensers and by a set of bluegreen excitation filters. The emission signal is collected by the emission condenser and filtered by a red filter before striking the photodetector. The instrument operates over a chlorophyll-a concentration range of 0.03-50 ug/l and has a depth range of 200 m. The excitation wavelength range is 400-550 nm and the registration wavelength range is &gt;680 nm. The instrument was developed by the EcoMonitor Laboratory of the Moscow Institute of Engineering Physics and was used during the 1990s.</skos:definition>
<owl:versionInfo>1</owl:versionInfo>
<dc:date>2011-11-07 15:23:52.0</dc:date>
<skos:note xml:lang="en">accepted</skos:note>
<owl:deprecated>false</owl:deprecated>
<skos:broader rdf:resource="http://vocab.nerc.ac.uk/collection/L05/current/353/"/>
<void:inDataset rdf:resource="http://vocab.nerc.ac.uk/.well-known/void"/>
</skos:Concept>
</skos:member>
<skos:member>
<skos:Concept rdf:about="http://vocab.nerc.ac.uk/collection/L22/current/TOOL0544/">
<dc:identifier>SDN:L22::TOOL0544</dc:identifier>
<skos:notation>SDN:L22::TOOL0544</skos:notation>
<skos:prefLabel xml:lang="en">Electropolished air sample canister</skos:prefLabel>
<skos:altLabel>Electropolished canister</skos:altLabel>
<skos:definition xml:lang="en">Metal sampling container of unknown make and capacity that has been smoothed by electropolishing (also known as electrochemical or electrolytic polishing). Suitable for the collection of high pressure air samples.</skos:definition>
<owl:versionInfo>1</owl:versionInfo>
<dc:date>2012-09-26 16:33:22.0</dc:date>
<skos:note xml:lang="en">accepted</skos:note>
<owl:deprecated>false</owl:deprecated>
<skos:broader rdf:resource="http://vocab.nerc.ac.uk/collection/L05/current/11/"/>
<void:inDataset rdf:resource="http://vocab.nerc.ac.uk/.well-known/void"/>
</skos:Concept>
</skos:member>
<skos:member>
<skos:Concept rdf:about="http://vocab.nerc.ac.uk/collection/L22/current/TOOL0608/">
<dc:identifier>SDN:L22::TOOL0608</dc:identifier>
<skos:notation>SDN:L22::TOOL0608</skos:notation>
<skos:prefLabel xml:lang="en">Eliasson CBME80 infrared laser diode cloud ceilometer</skos:prefLabel>
<skos:altLabel>Eliasson CBME80 cloud ceilometer</skos:altLabel>
<skos:definition xml:lang="en">An infrared laser diode measuring the cloud base height or vertical visibility and cloud amount. The design is based on the LIDAR principle. The light emitting component is a low power diode laser with the output power limited to eye-safe level. Real time digitising technique is used in signal detection and the 80C186 microprocessor is used in signal processing.</skos:definition>
<owl:versionInfo>1</owl:versionInfo>
<dc:date>2013-03-22 16:42:24.0</dc:date>
<skos:note xml:lang="en">accepted</skos:note>
<owl:deprecated>false</owl:deprecated>
<skos:broader rdf:resource="http://vocab.nerc.ac.uk/collection/L05/current/ATRANS/"/>
<skos:broader rdf:resource="http://vocab.nerc.ac.uk/collection/L05/current/CCOV/"/>
<void:inDataset rdf:resource="http://vocab.nerc.ac.uk/.well-known/void"/>
</skos:Concept>
</skos:member>
<skos:member>
<skos:Concept rdf:about="http://vocab.nerc.ac.uk/collection/L22/current/TOOL0277/">
<dc:identifier>SDN:L22::TOOL0277</dc:identifier>
<skos:notation>SDN:L22::TOOL0277</skos:notation>
<skos:prefLabel xml:lang="en">Endeco model 1125 dissolved oxygen system</skos:prefLabel>
<skos:altLabel>Endeco 1125 DO</skos:altLabel>
<skos:definition xml:lang="en">A controller with up to four multiplexed Endeco type 1128 pulsed-electrode dissolved oxygen probes. Endeco are now a subsidiary of YSI.</skos:definition>
<owl:versionInfo>1</owl:versionInfo>
<dc:date>2010-05-18 16:10:58.0</dc:date>
<skos:note xml:lang="en">accepted</skos:note>
<owl:deprecated>false</owl:deprecated>
<skos:broader rdf:resource="http://vocab.nerc.ac.uk/collection/L05/current/351/"/>
<void:inDataset rdf:resource="http://vocab.nerc.ac.uk/.well-known/void"/>
</skos:Concept>
</skos:member>
<skos:member>
<skos:Concept rdf:about="http://vocab.nerc.ac.uk/collection/L22/current/NETT0036/">
<dc:identifier>SDN:L22::NETT0036</dc:identifier>
<skos:notation>SDN:L22::NETT0036</skos:notation>
<skos:prefLabel xml:lang="en">English umbrella net - Macaulay and Daly (1987)</skos:prefLabel>
<skos:altLabel>English umbrella net</skos:altLabel>
<skos:definition xml:lang="en">A rectangular net 200 cm on a side and 300 cm long made from 0.22 mm nylon mesh is designed to fit through a hole in an ice flow closed, and open once underneath. A messenger is used to close the mouth opening at a specific depth prior to retrieval though the ice [Wiebe and Benfield 2003 Plate 11 C].</skos:definition>
<owl:versionInfo>1</owl:versionInfo>
<dc:date>2011-10-21 14:18:49.0</dc:date>
<skos:note xml:lang="en">accepted</skos:note>
<owl:deprecated>false</owl:deprecated>
<skos:broader rdf:resource="http://vocab.nerc.ac.uk/collection/L05/current/22/"/>
<void:inDataset rdf:resource="http://vocab.nerc.ac.uk/.well-known/void"/>
</skos:Concept>
</skos:member>
<skos:member>
<skos:Concept rdf:about="http://vocab.nerc.ac.uk/collection/L22/current/NETT0038/">
<dc:identifier>SDN:L22::NETT0038</dc:identifier>
<skos:notation>SDN:L22::NETT0038</skos:notation>
<skos:prefLabel xml:lang="en">Enlarged Clarke-Bumpus sampler - Paquette et al. (1961)</skos:prefLabel>
<skos:altLabel>Paquette enlarged Clarke-Bumpus Sampler</skos:altLabel>
<skos:definition xml:lang="en">Construction is a 25.4 cm diameter mouth opening with cylindrical tube 12.7 cm long. The tube is equipped with flat plate which pivots to open or close the flow through the tube and a TSK flowmeter. A 107 cm long conical net is attached to the rear of the tube. (No mesh size given).</skos:definition>
<owl:versionInfo>1</owl:versionInfo>
<dc:date>2011-10-21 14:18:49.0</dc:date>
<skos:note xml:lang="en">accepted</skos:note>
<owl:deprecated>false</owl:deprecated>
<skos:broader rdf:resource="http://vocab.nerc.ac.uk/collection/L05/current/22/"/>
<skos:broader rdf:resource="http://vocab.nerc.ac.uk/collection/L05/current/388/"/>
<void:inDataset rdf:resource="http://vocab.nerc.ac.uk/.well-known/void"/>
</skos:Concept>
</skos:member>
<skos:member>
<skos:Concept rdf:about="http://vocab.nerc.ac.uk/collection/L22/current/NETT0037/">
<dc:identifier>SDN:L22::NETT0037</dc:identifier>
<skos:notation>SDN:L22::NETT0037</skos:notation>
<skos:prefLabel xml:lang="en">Enlarged Clarke-Bumpus sampler - Yentsch et al. (1962)</skos:prefLabel>
<skos:altLabel>Yentsch enlarged Clarke-Bumpus Sampler</skos:altLabel>
<skos:definition xml:lang="en">An enlarged (jumbo) version of the Clarke-Bumpus Sampler with a 30 cm diameter mouth opening and 183 cm long net [Wiebe and Benfield 2003 Plate 8 B]. A pressure potentiometer in a SS case and attached to a conducting cable described for determining the depth of the end of a net tow wire.</skos:definition>
<owl:versionInfo>1</owl:versionInfo>
<dc:date>2011-10-21 14:18:49.0</dc:date>
<skos:note xml:lang="en">accepted</skos:note>
<owl:deprecated>false</owl:deprecated>
<skos:broader rdf:resource="http://vocab.nerc.ac.uk/collection/L05/current/388/"/>
<skos:broader rdf:resource="http://vocab.nerc.ac.uk/collection/L05/current/22/"/>
<void:inDataset rdf:resource="http://vocab.nerc.ac.uk/.well-known/void"/>
</skos:Concept>
</skos:member>
<skos:member>
<skos:Concept rdf:about="http://vocab.nerc.ac.uk/collection/L22/current/TOOL0381/">
<dc:identifier>SDN:L22::TOOL0381</dc:identifier>
<skos:notation>SDN:L22::TOOL0381</skos:notation>
<skos:prefLabel xml:lang="en">EnviroTech LLC Aqua Monitor Smart Water Sampler</skos:prefLabel>
<skos:altLabel>Aqua Monitor Water Sampler</skos:altLabel>
<skos:definition xml:lang="en">A programmable water sampler that can collect up to 48 discrete water samples of up to 1000ml each and may be programmed for time series sampling or for operation in "slave" mode within a system. Samples are collected using a syringe mechanism and stored in gas impermeable bags within protective enclosures.The sampler can be deployed on moorings, towed-vehicle systems, ROV or AUV platforms, and can be used for applications such as phytoplankton, nutrients, salinity and suspended sediment measurements.</skos:definition>
<owl:versionInfo>1</owl:versionInfo>
<dc:date>2011-03-14 15:22:43.0</dc:date>
<skos:note xml:lang="en">accepted</skos:note>
<owl:deprecated>false</owl:deprecated>
<skos:broader rdf:resource="http://vocab.nerc.ac.uk/collection/L05/current/30/"/>
<void:inDataset rdf:resource="http://vocab.nerc.ac.uk/.well-known/void"/>
</skos:Concept>
</skos:member>
<skos:member>
<skos:Concept rdf:about="http://vocab.nerc.ac.uk/collection/L22/current/TOOL0170/">
<dc:identifier>SDN:L22::TOOL0170</dc:identifier>
<skos:notation>SDN:L22::TOOL0170</skos:notation>
<skos:prefLabel xml:lang="en">EnviroTech LLC NAS-2E Nutrient Analyser</skos:prefLabel>
<skos:altLabel>NAS-2E nutrient analyser</skos:altLabel>
<skos:definition xml:lang="en">In-situ nutrient analyser for high frequency time-series determination of nutrient concentrations in marine and fresh waters.</skos:definition>
<owl:versionInfo>1</owl:versionInfo>
<dc:date>2010-05-18 16:10:58.0</dc:date>
<skos:note xml:lang="en">accepted</skos:note>
<owl:deprecated>false</owl:deprecated>
<skos:broader rdf:resource="http://vocab.nerc.ac.uk/collection/L05/current/181/"/>
<void:inDataset rdf:resource="http://vocab.nerc.ac.uk/.well-known/void"/>
</skos:Concept>
</skos:member>
<skos:member>
<skos:Concept rdf:about="http://vocab.nerc.ac.uk/collection/L22/current/TOOL0380/">
<dc:identifier>SDN:L22::TOOL0380</dc:identifier>
<skos:notation>SDN:L22::TOOL0380</skos:notation>
<skos:prefLabel xml:lang="en">EnviroTech LLC NAS-3X Nutrient Analyser</skos:prefLabel>
<skos:altLabel>NAS-3X Nutrient Analyser</skos:altLabel>
<skos:definition xml:lang="en">In-situ nutrient analyzer for high-frequency time-series determination of nutrient concentrations in marine and fresh waters. It uses a pump and valve system to acquire and react individual water samples, and versions are available for the measurement of nitrate, phosphate, silicate and ammonia. The NAS-3X replaces the NAS-2E, providing higher precision and resolution measurements. The standard depth rating is 100m, although a 250m version is also available and deeper versions may be built on request.</skos:definition>
<owl:versionInfo>1</owl:versionInfo>
<dc:date>2011-03-14 15:22:43.0</dc:date>
<skos:note xml:lang="en">accepted</skos:note>
<owl:deprecated>false</owl:deprecated>
<skos:broader rdf:resource="http://vocab.nerc.ac.uk/collection/L05/current/181/"/>
<void:inDataset rdf:resource="http://vocab.nerc.ac.uk/.well-known/void"/>
</skos:Concept>
</skos:member>
<skos:member>
<skos:Concept rdf:about="http://vocab.nerc.ac.uk/collection/L22/current/NETT0039/">
<dc:identifier>SDN:L22::NETT0039</dc:identifier>
<skos:notation>SDN:L22::NETT0039</skos:notation>
<skos:prefLabel xml:lang="en">Epi-benthic plankton net - Russell (1928)</skos:prefLabel>
<skos:altLabel>Russell epi-benthic plankton net</skos:altLabel>
<skos:definition xml:lang="en">Construction is 122 cm wide x 30 cm tall rectangular mouth with a 240 cm length net made of stramin. The net is mounted in an Agassiz trawl frame [Wiebe and Benfield 2003 Plate 22 B].</skos:definition>
<owl:versionInfo>1</owl:versionInfo>
<dc:date>2011-10-21 14:18:49.0</dc:date>
<skos:note xml:lang="en">accepted</skos:note>
<owl:deprecated>false</owl:deprecated>
<skos:broader rdf:resource="http://vocab.nerc.ac.uk/collection/L05/current/22/"/>
<skos:broader rdf:resource="http://vocab.nerc.ac.uk/collection/L05/current/61/"/>
<void:inDataset rdf:resource="http://vocab.nerc.ac.uk/.well-known/void"/>
</skos:Concept>
</skos:member>
<skos:member>
<skos:Concept rdf:about="http://vocab.nerc.ac.uk/collection/L22/current/NETT0040/">
<dc:identifier>SDN:L22::NETT0040</dc:identifier>
<skos:notation>SDN:L22::NETT0040</skos:notation>
<skos:prefLabel xml:lang="en">Epi-benthic plankton sampler - Bossanyi (1951)</skos:prefLabel>
<skos:altLabel>Bossanyi epi-benthic plankton sampler</skos:altLabel>
<skos:definition xml:lang="en">Approximately 91 cm x 61 cm rectangular mouth with net about 213 cm long. Netting with 15.7 meshes per cm. Able of open/close mouth opening [Wiebe and Benfield 2003 Plate 22 C].</skos:definition>
<owl:versionInfo>1</owl:versionInfo>
<dc:date>2011-10-21 14:18:49.0</dc:date>
<skos:note xml:lang="en">accepted</skos:note>
<owl:deprecated>false</owl:deprecated>
<skos:broader rdf:resource="http://vocab.nerc.ac.uk/collection/L05/current/24/"/>
<skos:broader rdf:resource="http://vocab.nerc.ac.uk/collection/L05/current/22/"/>
<void:inDataset rdf:resource="http://vocab.nerc.ac.uk/.well-known/void"/>
</skos:Concept>
</skos:member>
<skos:member>
<skos:Concept rdf:about="http://vocab.nerc.ac.uk/collection/L22/current/NETT0041/">
<dc:identifier>SDN:L22::NETT0041</dc:identifier>
<skos:notation>SDN:L22::NETT0041</skos:notation>
<skos:prefLabel xml:lang="en">Epi-benthic plankton sampler - Clutter (1965)</skos:prefLabel>
<skos:altLabel>Clutter epi-benthic plankton sampler</skos:altLabel>
<skos:definition xml:lang="en">Construction is a 32cm x 32 cm rectangular mouth opening net attached to a metal box frame work which was 37 cm tall x 37 cm wide x 30 cm long. The net was about 30 cm long had 0.333 mm nylon mesh. The system was lowered to the seafloor where an anchor attached to the net frame by a spool of line became fixed. The net was towed at ~1.5 knots away from the anchor until the line was fully extended whereupon it triggered a choke rope closing the net. Distance covered by the sampler was about 10 m. A scaled up version with 70.1 cm x 70.1 cm mouth opening also described [Wiebe and Benfield 2003 Plate 23 A].</skos:definition>
<owl:versionInfo>1</owl:versionInfo>
<dc:date>2011-10-21 14:18:49.0</dc:date>
<skos:note xml:lang="en">accepted</skos:note>
<owl:deprecated>false</owl:deprecated>
<skos:broader rdf:resource="http://vocab.nerc.ac.uk/collection/L05/current/22/"/>
<skos:broader rdf:resource="http://vocab.nerc.ac.uk/collection/L05/current/24/"/>
<void:inDataset rdf:resource="http://vocab.nerc.ac.uk/.well-known/void"/>
</skos:Concept>
</skos:member>
<skos:member>
<skos:Concept rdf:about="http://vocab.nerc.ac.uk/collection/L22/current/TOOL0083/">
<dc:identifier>SDN:L22::TOOL0083</dc:identifier>
<skos:notation>SDN:L22::TOOL0083</skos:notation>
<skos:prefLabel xml:lang="en">Eppley Precision Infrared Radiometer Pyrgyometer</skos:prefLabel>
<skos:altLabel>Eppley PIR Pyrgyometer</skos:altLabel>
<skos:definition xml:lang="en">The Eppley Precision Infrared Radiometer (PIR) pyrgyometer measures longwave (infrared) radiation. It is housed in a weatherproof titanium canister that has been painted with a very flat black paint that absorbs radiation. A small glass dome at the top of the instrument is covered with an 'interference coating' which allows only infrared radiation to come through. Light levels are detected as temperature changes creating voltages in fine wire coil detectors.</skos:definition>
<owl:versionInfo>1</owl:versionInfo>
<dc:date>2009-11-30 11:56:35.0</dc:date>
<skos:note xml:lang="en">accepted</skos:note>
<owl:deprecated>false</owl:deprecated>
<skos:broader rdf:resource="http://vocab.nerc.ac.uk/collection/L05/current/122/"/>
<void:inDataset rdf:resource="http://vocab.nerc.ac.uk/.well-known/void"/>
</skos:Concept>
</skos:member>
<skos:member>
<skos:Concept rdf:about="http://vocab.nerc.ac.uk/collection/L22/current/TOOL0593/">
<dc:identifier>SDN:L22::TOOL0593</dc:identifier>
<skos:notation>SDN:L22::TOOL0593</skos:notation>
<skos:prefLabel xml:lang="en">Falmouth Scientific Instruments Excell thermosalinograph</skos:prefLabel>
<skos:altLabel>FSI Excell TSG</skos:altLabel>
<skos:definition xml:lang="en">The instrument comprises an FSI internal field conductivity sensor (NXIC cell) and two precision platinum resistance thermometers to provide salinity mounted in a urethane through-flow housing.  The temperature sensors are located at the inlet and outlet to provide an integrated temperature measurement across the conductivity sensor.  The salinity range is 2 to 42 PSU  and the accuracy id +- 0.03 PSU.  Sea temperature is measured by an independently-supplied remote PRT or thermistor located in the hull or seawater inlet.</skos:definition>
<owl:versionInfo>1</owl:versionInfo>
<dc:date>2013-01-23 09:30:18.0</dc:date>
<skos:note xml:lang="en">accepted</skos:note>
<owl:deprecated>false</owl:deprecated>
<skos:broader rdf:resource="http://vocab.nerc.ac.uk/collection/L05/current/133/"/>
<skos:broader rdf:resource="http://vocab.nerc.ac.uk/collection/L05/current/134/"/>
<skos:broader rdf:resource="http://vocab.nerc.ac.uk/collection/L05/current/350/"/>
<void:inDataset rdf:resource="http://vocab.nerc.ac.uk/.well-known/void"/>
</skos:Concept>
</skos:member>
<skos:member>
<skos:Concept rdf:about="http://vocab.nerc.ac.uk/collection/L22/current/TOOL0364/">
<dc:identifier>SDN:L22::TOOL0364</dc:identifier>
<skos:notation>SDN:L22::TOOL0364</skos:notation>
<skos:prefLabel xml:lang="en">Falmouth Scientific Instruments Integrated CTD Profiler</skos:prefLabel>
<skos:altLabel>FSI ICTD</skos:altLabel>
<skos:definition xml:lang="en">CTD profiler with a sampling frequency of 32Hz and a depth rating of 7000m. It is normally used in conjunction with a DT-2000 deck unit, although an internal memory can also be installed for self contained data logging. Parameters are measured to an accuracy of ±0.0002 S/m for conductivity, ±0.002°C for temperature and 0.01% for full scale pressure. The unit can support two additional primary temperature sensors and up to 8 auxiliary sensors.</skos:definition>
<owl:versionInfo>1</owl:versionInfo>
<dc:date>2011-01-28 12:46:19.0</dc:date>
<skos:note xml:lang="en">accepted</skos:note>
<owl:deprecated>false</owl:deprecated>
<skos:related rdf:resource="http://vocab.nerc.ac.uk/collection/P01/current/PRESPR01/"/>
<skos:related rdf:resource="http://vocab.nerc.ac.uk/collection/P01/current/PSALST01/"/>
<skos:related rdf:resource="http://vocab.nerc.ac.uk/collection/P01/current/TEMPST01/"/>
<skos:broader rdf:resource="http://vocab.nerc.ac.uk/collection/L05/current/130/"/>
<skos:broader rdf:resource="http://vocab.nerc.ac.uk/collection/L05/current/134/"/>
<skos:broader rdf:resource="http://vocab.nerc.ac.uk/collection/L05/current/350/"/>
<void:inDataset rdf:resource="http://vocab.nerc.ac.uk/.well-known/void"/>
</skos:Concept>
</skos:member>
<skos:member>
<skos:Concept rdf:about="http://vocab.nerc.ac.uk/collection/L22/current/TOOL0173/">
<dc:identifier>SDN:L22::TOOL0173</dc:identifier>
<skos:notation>SDN:L22::TOOL0173</skos:notation>
<skos:prefLabel xml:lang="en">Falmouth Scientific Instruments NXIC CTD</skos:prefLabel>
<skos:altLabel>FSI NXIC CTD</skos:altLabel>
<skos:definition xml:lang="en">A collection of sensors which are generally linked to a common data logger that samples at up to 15Hz. Parameters are measured to an accuracy of ±0.0002 S/m for conductivity, ±0.005°C for temperature and 0.08% for full scale pressure. Now marketed by Teledyne RD Instruments.</skos:definition>
<owl:versionInfo>1</owl:versionInfo>
<dc:date>2010-05-18 16:10:58.0</dc:date>
<skos:note xml:lang="en">accepted</skos:note>
<owl:deprecated>false</owl:deprecated>
<skos:related rdf:resource="http://vocab.nerc.ac.uk/collection/P01/current/PRESPR01/"/>
<skos:related rdf:resource="http://vocab.nerc.ac.uk/collection/P01/current/TEMPST01/"/>
<skos:related rdf:resource="http://vocab.nerc.ac.uk/collection/P01/current/PSALPR01/"/>
<skos:broader rdf:resource="http://vocab.nerc.ac.uk/collection/L05/current/350/"/>
<skos:broader rdf:resource="http://vocab.nerc.ac.uk/collection/L05/current/130/"/>
<skos:broader rdf:resource="http://vocab.nerc.ac.uk/collection/L05/current/134/"/>
<void:inDataset rdf:resource="http://vocab.nerc.ac.uk/.well-known/void"/>
</skos:Concept>
</skos:member>
<skos:member>
<skos:Concept rdf:about="http://vocab.nerc.ac.uk/collection/L22/current/TOOL0122/">
<dc:identifier>SDN:L22::TOOL0122</dc:identifier>
<skos:notation>SDN:L22::TOOL0122</skos:notation>
<skos:prefLabel xml:lang="en">Falmouth Scientific Instruments OEM conductivity-temperature sensor</skos:prefLabel>
<skos:altLabel>FSI OEM C-T module</skos:altLabel>
<skos:definition xml:lang="en">A high accuracy conductivity and temperature sensor that can be readily adapted to various user platforms. The interface electronics provide a DC voltage output proportional to conductivity or temperature. Conductivity is measured by a large inductively coupled sensor that is less affected by biofouling than wetted electrode sensors. Temperature is measured by a high grade Platiunum Resistence Thermometer (PRT) that provides linear temperature response and high stability. The electronics approach is very linear, eliminating the need for complex equations to convert outputs to physical units.</skos:definition>
<owl:versionInfo>1</owl:versionInfo>
<dc:date>2010-05-18 16:10:58.0</dc:date>
<skos:note xml:lang="en">accepted</skos:note>
<owl:deprecated>false</owl:deprecated>
<skos:broader rdf:resource="http://vocab.nerc.ac.uk/collection/L05/current/350/"/>
<skos:broader rdf:resource="http://vocab.nerc.ac.uk/collection/L05/current/134/"/>
<void:inDataset rdf:resource="http://vocab.nerc.ac.uk/.well-known/void"/>
</skos:Concept>
</skos:member>
<skos:member>
<skos:Concept rdf:about="http://vocab.nerc.ac.uk/collection/L22/current/TOOL0455/">
<dc:identifier>SDN:L22::TOOL0455</dc:identifier>
<skos:notation>SDN:L22::TOOL0455</skos:notation>
<skos:prefLabel xml:lang="en">Falmouth Scientific Instruments ocean conductivity module</skos:prefLabel>
<skos:altLabel>FSI OCM</skos:altLabel>
<skos:definition xml:lang="en">An inductively coupled conductivity sensor with a low-power micro-controller to collect, scale and transmit real-time data via RS-232 or RS-485. The sensor has an accuracy of +/- 0.0003 S/m and a resolution of 0.00001 S/m over the range 0-7.0 S/m. It has a response time of 50 ms at a flow rate of 1 m/s.</skos:definition>
<owl:versionInfo>1</owl:versionInfo>
<dc:date>2012-01-24 16:36:37.0</dc:date>
<skos:note xml:lang="en">accepted</skos:note>
<owl:deprecated>false</owl:deprecated>
<skos:broader rdf:resource="http://vocab.nerc.ac.uk/collection/L05/current/350/"/>
<void:inDataset rdf:resource="http://vocab.nerc.ac.uk/.well-known/void"/>
</skos:Concept>
</skos:member>
<skos:member>
<skos:Concept rdf:about="http://vocab.nerc.ac.uk/collection/L22/current/TOOL0123/">
<dc:identifier>SDN:L22::TOOL0123</dc:identifier>
<skos:notation>SDN:L22::TOOL0123</skos:notation>
<skos:prefLabel xml:lang="en">Falmouth Scientific Instruments ocean temperature module</skos:prefLabel>
<skos:altLabel>FSI OTM</skos:altLabel>
<skos:definition xml:lang="en">A standards-grade platinum resistance thermometer with a low-power micro-controller to collect, scale and transmit real-time data via RS-232 or RS-485</skos:definition>
<owl:versionInfo>1</owl:versionInfo>
<dc:date>2010-05-18 16:10:58.0</dc:date>
<skos:note xml:lang="en">accepted</skos:note>
<owl:deprecated>false</owl:deprecated>
<skos:broader rdf:resource="http://vocab.nerc.ac.uk/collection/L05/current/134/"/>
<void:inDataset rdf:resource="http://vocab.nerc.ac.uk/.well-known/void"/>
</skos:Concept>
</skos:member>
<skos:member>
<skos:Concept rdf:about="http://vocab.nerc.ac.uk/collection/L22/current/TOOL0428/">
<dc:identifier>SDN:L22::TOOL0428</dc:identifier>
<skos:notation>SDN:L22::TOOL0428</skos:notation>
<skos:prefLabel xml:lang="en">Fast Light Yo-yo (FLY II) microstructure profiler</skos:prefLabel>
<skos:altLabel>FLY II</skos:altLabel>
<skos:definition xml:lang="en">A free-falling instrument designed to measure temperature, salinity and turbulent shear from near surface to within 15cm of the seabed. The instrument includes airfoil shear probes (the shear sensing element comprises a piezo-ceramic bimorph beam which generates an electrical charge in response to cross-axial forces), slow and fast response thermistors, a conductivity cell, two tilt gauges and a pressure gauge. A probe guard mounted at the lower end of the instrument protects sensors from bottom sediments. Data are transmitted back to the ship in real time through a neutrally buoyant line. The FLY series of instruments was developed in the 1980s by the Institute of Ocean Sciences, British Columbia and others, and built by Sy-Tech Research Ltd of Sidney, British Columbia. The instrument is no longer in production.</skos:definition>
<owl:versionInfo>1</owl:versionInfo>
<dc:date>2011-11-02 11:37:25.0</dc:date>
<skos:note xml:lang="en">accepted</skos:note>
<owl:deprecated>false</owl:deprecated>
<skos:broader rdf:resource="http://vocab.nerc.ac.uk/collection/L05/current/350/"/>
<skos:broader rdf:resource="http://vocab.nerc.ac.uk/collection/L05/current/134/"/>
<skos:broader rdf:resource="http://vocab.nerc.ac.uk/collection/L05/current/184/"/>
<void:inDataset rdf:resource="http://vocab.nerc.ac.uk/.well-known/void"/>
</skos:Concept>
</skos:member>
<skos:member>
<skos:Concept rdf:about="http://vocab.nerc.ac.uk/collection/L22/current/TOOL0429/">
<dc:identifier>SDN:L22::TOOL0429</dc:identifier>
<skos:notation>SDN:L22::TOOL0429</skos:notation>
<skos:prefLabel xml:lang="en">Fast Light Yo-yo (FLY IV) microstructure profiler</skos:prefLabel>
<skos:altLabel>FLY IV</skos:altLabel>
<skos:definition xml:lang="en">A free-falling instrument designed to measure temperature, salinity and turbulent shear from near surface to within 15cm of the seabed. The instrument includes airfoil shear probes (the shear sensing element comprises a piezo-ceramic bimorph beam which generates an electrical charge in response to cross-axial forces), slow and fast response thermistors, a conductivity cell, two tilt gauges and a pressure gauge. A probe guard mounted at the lower end of the instrument protects sensors from bottom sediments. Data are transmitted back to the ship in real time through a neutrally buoyant line. The FLY series of instruments was developed in the 1980s by the Institute of Ocean Sciences, British Columbia and others, and built by Sy-Tech Research Ltd of Sidney, British Columbia. The FLY IV used the same sensors as the FLY II but incorporated more advanced electronics and software. Data transmission was achieved via the TELUS Mobility Network. The instrument is no longer in production.</skos:definition>
<owl:versionInfo>1</owl:versionInfo>
<dc:date>2011-11-02 11:37:25.0</dc:date>
<skos:note xml:lang="en">accepted</skos:note>
<owl:deprecated>false</owl:deprecated>
<skos:broader rdf:resource="http://vocab.nerc.ac.uk/collection/L05/current/350/"/>
<skos:broader rdf:resource="http://vocab.nerc.ac.uk/collection/L05/current/134/"/>
<skos:broader rdf:resource="http://vocab.nerc.ac.uk/collection/L05/current/184/"/>
<void:inDataset rdf:resource="http://vocab.nerc.ac.uk/.well-known/void"/>
</skos:Concept>
</skos:member>
<skos:member>
<skos:Concept rdf:about="http://vocab.nerc.ac.uk/collection/L22/current/NETT0137/">
<dc:identifier>SDN:L22::NETT0137</dc:identifier>
<skos:notation>SDN:L22::NETT0137</skos:notation>
<skos:prefLabel xml:lang="en">Fixed in-current plankton net - Johannes et al (1970)</skos:prefLabel>
<skos:altLabel>Johannes plankton net</skos:altLabel>
<skos:definition xml:lang="en">A pair of 50 cm diameter nets made from number 10 gauze were mounted side by side in a rectangular frame with an extender rod to support the net cod ends horizontally .  The nets and frame were attached 100 cm above the bottom to a wire extending from an anchor stand to a surface float. The nets were free to rotate so that they always faced into the flow [Wiebe and Benfield 2003 Plate 24 B].</skos:definition>
<owl:versionInfo>1</owl:versionInfo>
<dc:date>2011-10-21 14:18:49.0</dc:date>
<skos:note xml:lang="en">accepted</skos:note>
<owl:deprecated>false</owl:deprecated>
<skos:broader rdf:resource="http://vocab.nerc.ac.uk/collection/L05/current/22/"/>
<void:inDataset rdf:resource="http://vocab.nerc.ac.uk/.well-known/void"/>
</skos:Concept>
</skos:member>
<skos:member>
<skos:Concept rdf:about="http://vocab.nerc.ac.uk/collection/L22/current/TOOL0110/">
<dc:identifier>SDN:L22::TOOL0110</dc:identifier>
<skos:notation>SDN:L22::TOOL0110</skos:notation>
<skos:prefLabel xml:lang="en">Florida-Bahamas cable from 1990</skos:prefLabel>
<skos:altLabel>Florida-Bahamas cable 1990-</skos:altLabel>
<skos:definition xml:lang="en">Cabling installed on the seabed primarily to provide a telecommunication link between Florida and the Bahamas from 1990, but able to provide information on currents due to resistance variation. More information at http://www.bodc.ac.uk/data/documents/nodb/110741/.</skos:definition>
<owl:versionInfo>2</owl:versionInfo>
<dc:date>2010-11-18 12:39:41.0</dc:date>
<skos:note xml:lang="en">accepted</skos:note>
<owl:deprecated>false</owl:deprecated>
<skos:broader rdf:resource="http://vocab.nerc.ac.uk/collection/L05/current/380/"/>
<void:inDataset rdf:resource="http://vocab.nerc.ac.uk/.well-known/void"/>
</skos:Concept>
</skos:member>
<skos:member>
<skos:Concept rdf:about="http://vocab.nerc.ac.uk/collection/L22/current/TOOL0109/">
<dc:identifier>SDN:L22::TOOL0109</dc:identifier>
<skos:notation>SDN:L22::TOOL0109</skos:notation>
<skos:prefLabel xml:lang="en">Florida-Bahamas cable to 1990</skos:prefLabel>
<skos:altLabel>Florida-Bahamas cable -1990</skos:altLabel>
<skos:definition xml:lang="en">Cabling installed on the seabed primarily to provide a telecommunication link between Florida and the Bahamas until 1990 but able to provide information on currents due to resistance variation. More information at http://www.bodc.ac.uk/data/documents/nodb/110738/.</skos:definition>
<owl:versionInfo>2</owl:versionInfo>
<dc:date>2010-11-18 12:39:41.0</dc:date>
<skos:note xml:lang="en">accepted</skos:note>
<owl:deprecated>false</owl:deprecated>
<skos:broader rdf:resource="http://vocab.nerc.ac.uk/collection/L05/current/380/"/>
<void:inDataset rdf:resource="http://vocab.nerc.ac.uk/.well-known/void"/>
</skos:Concept>
</skos:member>
<skos:member>
<skos:Concept rdf:about="http://vocab.nerc.ac.uk/collection/L22/current/TOOL0483/">
<dc:identifier>SDN:L22::TOOL0483</dc:identifier>
<skos:notation>SDN:L22::TOOL0483</skos:notation>
<skos:prefLabel xml:lang="en">Flow injection chemiluminescence system with photon counting head</skos:prefLabel>
<skos:altLabel>FI-CL photon counting system</skos:altLabel>
<skos:definition xml:lang="en">An analytical system used to determine concentrations of chemical species in a sample based on the luminescence of the species of interest. The system typically comprises individual components typically including pumps, injection and autosampler valves, preconcentration columns and a photon counting head for chemiluminescence detection. The system is normally uniquely assembled for each analysis.</skos:definition>
<owl:versionInfo>1</owl:versionInfo>
<dc:date>2012-03-29 16:25:41.0</dc:date>
<skos:note xml:lang="en">accepted</skos:note>
<owl:deprecated>false</owl:deprecated>
<skos:broader rdf:resource="http://vocab.nerc.ac.uk/collection/L05/current/LAB34/"/>
<skos:broader rdf:resource="http://vocab.nerc.ac.uk/collection/L05/current/LAB36/"/>
<void:inDataset rdf:resource="http://vocab.nerc.ac.uk/.well-known/void"/>
</skos:Concept>
</skos:member>
<skos:member>
<skos:Concept rdf:about="http://vocab.nerc.ac.uk/collection/L22/current/TOOL0513/">
<dc:identifier>SDN:L22::TOOL0513</dc:identifier>
<skos:notation>SDN:L22::TOOL0513</skos:notation>
<skos:prefLabel xml:lang="en">Flow injection lumogallion system with fluorometer</skos:prefLabel>
<skos:altLabel>FIA fluorometer system</skos:altLabel>
<skos:definition xml:lang="en">An analytical system used to determine concentrations of chemical species in a sample based on the fluorescence from the reaction between lumogallion and the species of interest. The system typically comprises individual components typically including pumps, injection and autosampler valves, preconcentration columns and a fluorometer. The system is normally uniquely assembled for each analysis.</skos:definition>
<owl:versionInfo>1</owl:versionInfo>
<dc:date>2012-07-04 10:02:10.0</dc:date>
<skos:note xml:lang="en">accepted</skos:note>
<owl:deprecated>false</owl:deprecated>
<skos:broader rdf:resource="http://vocab.nerc.ac.uk/collection/L05/current/LAB36/"/>
<void:inDataset rdf:resource="http://vocab.nerc.ac.uk/.well-known/void"/>
</skos:Concept>
</skos:member>
<skos:member>
<skos:Concept rdf:about="http://vocab.nerc.ac.uk/collection/L22/current/TOOL0539/">
<dc:identifier>SDN:L22::TOOL0539</dc:identifier>
<skos:notation>SDN:L22::TOOL0539</skos:notation>
<skos:prefLabel xml:lang="en">Flygt pump</skos:prefLabel>
<skos:altLabel>Flygt pump</skos:altLabel>
<skos:definition xml:lang="en">Submersible electrical pump designed for continuous pumping of water. It incorporates an impeller, allowing large volumes of water to be pumped quickly. Flygt pumps were used by institutes such as the then Institute of Marine Environmental Research (now Plymouth Marine Laboratory) for oceanographic sampling in the 1970s. This allowed continuous monitoring of water properties as well as the collection of discrete samples from the pump outflow.</skos:definition>
<owl:versionInfo>2</owl:versionInfo>
<dc:date>2012-10-12 09:11:26.0</dc:date>
<skos:note xml:lang="en">accepted</skos:note>
<owl:deprecated>false</owl:deprecated>
<skos:broader rdf:resource="http://vocab.nerc.ac.uk/collection/L05/current/31/"/>
<void:inDataset rdf:resource="http://vocab.nerc.ac.uk/.well-known/void"/>
</skos:Concept>
</skos:member>
<skos:member>
<skos:Concept rdf:about="http://vocab.nerc.ac.uk/collection/L22/current/TOOL0628/">
<dc:identifier>SDN:L22::TOOL0628</dc:identifier>
<skos:notation>SDN:L22::TOOL0628</skos:notation>
<skos:prefLabel xml:lang="en">Focal Technologies Corporation optical plankton counter</skos:prefLabel>
<skos:altLabel>Focal Technologies OPC</skos:altLabel>
<skos:definition xml:lang="en">An in-situ instrument with a sampling tunnel that causes particles (presumed to be plankton) to pass through a collimated light beam that measures their effective spherical diameters. Counts are produced over the sampling interval (typically 30 seconds) of the number of particles in each of 128 equal size classes within a size range of 0-5500 microns. More information may be found in http://www.bodc.ac.uk/data/documents/nodb/104842/.</skos:definition>
<owl:versionInfo>1</owl:versionInfo>
<dc:date>2013-07-02 16:03:17.0</dc:date>
<skos:note xml:lang="en">accepted</skos:note>
<owl:deprecated>false</owl:deprecated>
<skos:broader rdf:resource="http://vocab.nerc.ac.uk/collection/L05/current/150/"/>
<void:inDataset rdf:resource="http://vocab.nerc.ac.uk/.well-known/void"/>
</skos:Concept>
</skos:member>
<skos:member>
<skos:Concept rdf:about="http://vocab.nerc.ac.uk/collection/L22/current/NETT0043/">
<dc:identifier>SDN:L22::NETT0043</dc:identifier>
<skos:notation>SDN:L22::NETT0043</skos:notation>
<skos:prefLabel xml:lang="en">Foxton two-chamber cod-end - Currie (1962) Foston (1963)</skos:prefLabel>
<skos:altLabel>Foxton two-chamber cod-end</skos:altLabel>
<skos:definition xml:lang="en">A modification to the IKMT to allow pressure actuated depth separated collections by a two-part cod end [Wiebe and Benfield 2003 Plate 25 D].</skos:definition>
<owl:versionInfo>1</owl:versionInfo>
<dc:date>2011-10-21 14:18:49.0</dc:date>
<skos:note xml:lang="en">accepted</skos:note>
<owl:deprecated>false</owl:deprecated>
<skos:broader rdf:resource="http://vocab.nerc.ac.uk/collection/L05/current/23/"/>
<void:inDataset rdf:resource="http://vocab.nerc.ac.uk/.well-known/void"/>
</skos:Concept>
</skos:member>
<skos:member>
<skos:Concept rdf:about="http://vocab.nerc.ac.uk/collection/L22/current/NETT0044/">
<dc:identifier>SDN:L22::NETT0044</dc:identifier>
<skos:notation>SDN:L22::NETT0044</skos:notation>
<skos:prefLabel xml:lang="en">Free-fall plankton net - Heron (1982)</skos:prefLabel>
<skos:altLabel>Heron free-fall plankton net</skos:altLabel>
<skos:definition xml:lang="en">A modified WP2 cylinder-cone closing net (mesh not specified) which is allowed to free-fall and then is strangled shut and retrieved.  [Wiebe and Benfield 2003 Plate 10C]</skos:definition>
<owl:versionInfo>1</owl:versionInfo>
<dc:date>2011-10-21 14:18:49.0</dc:date>
<skos:note xml:lang="en">accepted</skos:note>
<owl:deprecated>false</owl:deprecated>
<skos:broader rdf:resource="http://vocab.nerc.ac.uk/collection/L05/current/22/"/>
<void:inDataset rdf:resource="http://vocab.nerc.ac.uk/.well-known/void"/>
</skos:Concept>
</skos:member>
<skos:member>
<skos:Concept rdf:about="http://vocab.nerc.ac.uk/collection/L22/current/TOOL0508/">
<dc:identifier>SDN:L22::TOOL0508</dc:identifier>
<skos:notation>SDN:L22::TOOL0508</skos:notation>
<skos:prefLabel xml:lang="en">Friedinger bottle water sampler</skos:prefLabel>
<skos:altLabel>Friedinger bottle</skos:altLabel>
<skos:definition xml:lang="en">A free flushing sample bottle of 1-5 litre capacity comprising a glass, metal or plastic tube with a hinged lid at each end. The bottle is deployed on a wire with the lids held open. When the bottle reaches the target depth a weighted messenger is sent down the wire and releases the lids, sealing the sample in the bottle. The bottle was designed by H Friedinger (Lucerne, Switzerland) to collect water samples for plankton analysis.</skos:definition>
<owl:versionInfo>1</owl:versionInfo>
<dc:date>2012-06-22 15:36:10.0</dc:date>
<skos:note xml:lang="en">accepted</skos:note>
<owl:deprecated>false</owl:deprecated>
<skos:broader rdf:resource="http://vocab.nerc.ac.uk/collection/L05/current/30/"/>
<void:inDataset rdf:resource="http://vocab.nerc.ac.uk/.well-known/void"/>
</skos:Concept>
</skos:member>
<skos:member>
<skos:Concept rdf:about="http://vocab.nerc.ac.uk/collection/L22/current/TOOL0265/">
<dc:identifier>SDN:L22::TOOL0265</dc:identifier>
<skos:notation>SDN:L22::TOOL0265</skos:notation>
<skos:prefLabel xml:lang="en">Fugro Oceanor Wavescan buoy meteorological package</skos:prefLabel>
<skos:altLabel>Wavescan met package</skos:altLabel>
<skos:definition xml:lang="en">A meteorological tower with wind, air pressure and air temperature sensors mounted on top of a metocean waverider buoy with on-board data logging and telemetry capability. More information is given in https://www.bodc.ac.uk/data/documents/nodb/64211/</skos:definition>
<owl:versionInfo>1</owl:versionInfo>
<dc:date>2010-05-18 16:10:58.0</dc:date>
<skos:note xml:lang="en">accepted</skos:note>
<owl:deprecated>false</owl:deprecated>
<skos:broader rdf:resource="http://vocab.nerc.ac.uk/collection/L05/current/102/"/>
<skos:broader rdf:resource="http://vocab.nerc.ac.uk/collection/L05/current/110/"/>
<void:inDataset rdf:resource="http://vocab.nerc.ac.uk/.well-known/void"/>
</skos:Concept>
</skos:member>
<skos:member>
<skos:Concept rdf:about="http://vocab.nerc.ac.uk/collection/L22/current/TOOL0264/">
<dc:identifier>SDN:L22::TOOL0264</dc:identifier>
<skos:notation>SDN:L22::TOOL0264</skos:notation>
<skos:prefLabel xml:lang="en">Fugro Oceanor Wavescan buoy waverider</skos:prefLabel>
<skos:altLabel>Wavescan waverider</skos:altLabel>
<skos:definition xml:lang="en">A meteocean waverider buoy incorporating directional wave sensors with sophisticated on-board data reduction, data logging and telemetry capability. The buoy may also carry a meteorological tower and a sub-surface sensor package that are considered to be separate data production tools. More information is given in https://www.bodc.ac.uk/data/documents/nodb/64211/</skos:definition>
<owl:versionInfo>1</owl:versionInfo>
<dc:date>2010-05-18 16:10:58.0</dc:date>
<skos:note xml:lang="en">accepted</skos:note>
<owl:deprecated>false</owl:deprecated>
<skos:broader rdf:resource="http://vocab.nerc.ac.uk/collection/L05/current/110/"/>
<void:inDataset rdf:resource="http://vocab.nerc.ac.uk/.well-known/void"/>
</skos:Concept>
</skos:member>
<skos:member>
<skos:Concept rdf:about="http://vocab.nerc.ac.uk/collection/L22/current/TOOL0348/">
<dc:identifier>SDN:L22::TOOL0348</dc:identifier>
<skos:notation>SDN:L22::TOOL0348</skos:notation>
<skos:prefLabel xml:lang="en">Fugro SeaSTAR 9200-G2 Differential Navigation System receiver</skos:prefLabel>
<skos:altLabel>Fugro SeaSTAR 9200-G2</skos:altLabel>
<skos:definition xml:lang="en">A dual-frequency Differential Global Satellite Navigation System (DGSNS) receiver that incorporates both GPS and GLONASS reception capability. It also tracks the Fugro L-Band satellite broadcast of DGNSS corrections and, as backup, can receive these corrections via the internet. This functionality allows the instrument to provide positional information with a horizontal accuracy of 15cm and a vertical accuracy of 20cm.</skos:definition>
<owl:versionInfo>1</owl:versionInfo>
<dc:date>2010-09-06 12:45:22.0</dc:date>
<skos:note xml:lang="en">accepted</skos:note>
<owl:deprecated>false</owl:deprecated>
<skos:broader rdf:resource="http://vocab.nerc.ac.uk/collection/L05/current/POS04/"/>
<void:inDataset rdf:resource="http://vocab.nerc.ac.uk/.well-known/void"/>
</skos:Concept>
</skos:member>
<skos:member>
<skos:Concept rdf:about="http://vocab.nerc.ac.uk/collection/L22/current/TOOL0457/">
<dc:identifier>SDN:L22::TOOL0457</dc:identifier>
<skos:notation>SDN:L22::TOOL0457</skos:notation>
<skos:prefLabel xml:lang="en">Furuno GP32 Global Positioning System receiver</skos:prefLabel>
<skos:altLabel>Furuno GP32 GPS</skos:altLabel>
<skos:definition xml:lang="en">A 12-channel, all-in-view Global Positioning System (GPS) receiver. The unit also contains a Wide Area Augmentation System (WAAS) receiver, which applies correction data by means of geostationary satellites, thereby improving positional accuracy. It is Differential GPS (DGPS) ready, with a positional accuracy of 10 m in GPS mode, 5 m in DGPS mode and 3 m in WAAS mode.</skos:definition>
<owl:versionInfo>1</owl:versionInfo>
<dc:date>2012-02-07 12:32:54.0</dc:date>
<skos:note xml:lang="en">accepted</skos:note>
<owl:deprecated>false</owl:deprecated>
<skos:broader rdf:resource="http://vocab.nerc.ac.uk/collection/L05/current/POS03/"/>
<void:inDataset rdf:resource="http://vocab.nerc.ac.uk/.well-known/void"/>
</skos:Concept>
</skos:member>
<skos:member>
<skos:Concept rdf:about="http://vocab.nerc.ac.uk/collection/L22/current/TOOL0655/">
<dc:identifier>SDN:L22::TOOL0655</dc:identifier>
<skos:notation>SDN:L22::TOOL0655</skos:notation>
<skos:prefLabel xml:lang="en">GEOTEK Geoscan IV line scan camera</skos:prefLabel>
<skos:altLabel>Geotek Geoscan IV</skos:altLabel>
<skos:definition xml:lang="en">A 3 x 2048 pixel CCD, digital line-scan camera fitted with a standard Nikon lens mount which is used for imaging cores. Images can be collected at up to 400 lines per centimetre, resulting in a down-core resolution of 25 micron pixel.</skos:definition>
<owl:versionInfo>1</owl:versionInfo>
<dc:date>2013-12-02 12:24:49.0</dc:date>
<skos:note xml:lang="en">accepted</skos:note>
<owl:deprecated>false</owl:deprecated>
<skos:broader rdf:resource="http://vocab.nerc.ac.uk/collection/L05/current/LAB41/"/>
<void:inDataset rdf:resource="http://vocab.nerc.ac.uk/.well-known/void"/>
</skos:Concept>
</skos:member>
<skos:member>
<skos:Concept rdf:about="http://vocab.nerc.ac.uk/collection/L22/current/TOOL0654/">
<dc:identifier>SDN:L22::TOOL0654</dc:identifier>
<skos:notation>SDN:L22::TOOL0654</skos:notation>
<skos:prefLabel xml:lang="en">GEOTEK Multi-Sensor Core Logger XYZ</skos:prefLabel>
<skos:altLabel>Geotek MSCL-XYZ</skos:altLabel>
<skos:definition xml:lang="en">An automated, high-resolution, multi-sensor system used for non-destructive, geophysical measurements of sediment and rock cores. The XYZ system analyses along the length of multiple split core sections in sequential order, whilst maintaining distance to the core surface. The XYZ system comprises of a sensor arm, capable of mounting a line-scan camera to capture the colour of the core surface and multiple sensors to directly measure the core surface. Surface sensors which can be mounted on the system are a colour spectrophotometer, magnetic susceptibility sensor, x-ray fluorescence and natural gamma spectrometer. The system can analyse up to 9 x 1.55 m core sections (up to 15 cm dia.) with a linear precision of 0.02 mm.</skos:definition>
<owl:versionInfo>1</owl:versionInfo>
<dc:date>2013-12-02 12:24:49.0</dc:date>
<skos:note xml:lang="en">accepted</skos:note>
<owl:deprecated>false</owl:deprecated>
<skos:broader rdf:resource="http://vocab.nerc.ac.uk/collection/L05/current/LAB41/"/>
<skos:broader rdf:resource="http://vocab.nerc.ac.uk/collection/L05/current/LAB42/"/>
<skos:broader rdf:resource="http://vocab.nerc.ac.uk/collection/L05/current/LAB22/"/>
<skos:broader rdf:resource="http://vocab.nerc.ac.uk/collection/L05/current/LAB31/"/>
<skos:broader rdf:resource="http://vocab.nerc.ac.uk/collection/L05/current/LAB20/"/>
<skos:broader rdf:resource="http://vocab.nerc.ac.uk/collection/L05/current/LAB25/"/>
<void:inDataset rdf:resource="http://vocab.nerc.ac.uk/.well-known/void"/>
</skos:Concept>
</skos:member>
<skos:member>
<skos:Concept rdf:about="http://vocab.nerc.ac.uk/collection/L22/current/TOOL0299/">
<dc:identifier>SDN:L22::TOOL0299</dc:identifier>
<skos:notation>SDN:L22::TOOL0299</skos:notation>
<skos:prefLabel xml:lang="en">GRIMM 1.108 aerosol spectrometer</skos:prefLabel>
<skos:altLabel>GRIMM 1.108 aerosol spec</skos:altLabel>
<skos:definition xml:lang="en">An instrument that measures size-resolved aerosol abundances in the atmosphere. The ambient air sample is size-classified by a Differential Mobility Analyser, then counted by an Optical Particle Counter. The sample exits the OPC and is deposited on a PTFE filter. The filter may be removed for subsequent, bulk gravimetric or chemical analysis.</skos:definition>
<owl:versionInfo>3</owl:versionInfo>
<dc:date>2011-07-01 10:20:53.0</dc:date>
<skos:note xml:lang="en">accepted</skos:note>
<owl:deprecated>false</owl:deprecated>
<skos:broader rdf:resource="http://vocab.nerc.ac.uk/collection/L05/current/386/"/>
<void:inDataset rdf:resource="http://vocab.nerc.ac.uk/.well-known/void"/>
</skos:Concept>
</skos:member>
<skos:member>
<skos:Concept rdf:about="http://vocab.nerc.ac.uk/collection/L22/current/TOOL0298/">
<dc:identifier>SDN:L22::TOOL0298</dc:identifier>
<skos:notation>SDN:L22::TOOL0298</skos:notation>
<skos:prefLabel xml:lang="en">GRIMM 1.109 aerosol spectrometer</skos:prefLabel>
<skos:altLabel>GRIMM 1.109 aerosol spec</skos:altLabel>
<skos:definition xml:lang="en">A portable in-situ instrument that optically counts atmospheric particles in the size range 0.3um to 20um into 31 size classes.</skos:definition>
<owl:versionInfo>2</owl:versionInfo>
<dc:date>2011-07-01 10:20:55.0</dc:date>
<skos:note xml:lang="en">accepted</skos:note>
<owl:deprecated>false</owl:deprecated>
<skos:broader rdf:resource="http://vocab.nerc.ac.uk/collection/L05/current/386/"/>
<void:inDataset rdf:resource="http://vocab.nerc.ac.uk/.well-known/void"/>
</skos:Concept>
</skos:member>
<skos:member>
<skos:Concept rdf:about="http://vocab.nerc.ac.uk/collection/L22/current/TOOL0560/">
<dc:identifier>SDN:L22::TOOL0560</dc:identifier>
<skos:notation>SDN:L22::TOOL0560</skos:notation>
<skos:prefLabel xml:lang="en">GV Instruments IsoPrime Isotope Ratio Mass Spectrometer</skos:prefLabel>
<skos:altLabel>GV IsoPrime IRMS</skos:altLabel>
<skos:definition xml:lang="en">A laboratory benchtop isotope ratio mass spectrometer (IRMS), which operates in dual inlet or continuous flow modes. It forms part of the IsoPrime system which has a range of sample preparation and purification modules that can be coupled with the IsoPrime IRMS. The modules can analyse a range of samples (solids, liquids or gases) and each prepares the sample to be introduced into the IRMS as purified gases. The resultant prepared gases such as H2, CO2, CO, N2, SO2 or N2O are then ionised and analysed for their isotopic content by the IRMS. The instrument was originally manufactured GV instruments as part of the IsoPrime series, but this part of the business was sold to Isoprime Ltd (a group member of Elementar Analysensysteme GmbH) and this instrument has been superseded by more recent models.</skos:definition>
<owl:versionInfo>1</owl:versionInfo>
<dc:date>2012-10-04 12:03:09.0</dc:date>
<skos:note xml:lang="en">accepted</skos:note>
<owl:deprecated>false</owl:deprecated>
<skos:broader rdf:resource="http://vocab.nerc.ac.uk/collection/L05/current/LAB19/"/>
<skos:broader rdf:resource="http://vocab.nerc.ac.uk/collection/L05/current/LAB16/"/>
<void:inDataset rdf:resource="http://vocab.nerc.ac.uk/.well-known/void"/>
</skos:Concept>
</skos:member>
<skos:member>
<skos:Concept rdf:about="http://vocab.nerc.ac.uk/collection/L22/current/TOOL0559/">
<dc:identifier>SDN:L22::TOOL0559</dc:identifier>
<skos:notation>SDN:L22::TOOL0559</skos:notation>
<skos:prefLabel xml:lang="en">GV Instruments Trace Gas Preconcentrator</skos:prefLabel>
<skos:altLabel>GV Gas Preconcentrator</skos:altLabel>
<skos:definition xml:lang="en">A gas chromatograph used for the isotope characterisation of N2O, CO2 and CH4. Gas samples can be injected either manually, using dual-ended sample bottles with valves, or using the fully automated inlet system. Manual selection of the gas to be analysed (CH4, CO2 or N2O) dictates the route the sample will travel through the instrument. For CO2 and N2O analysis, a sample is diverted by a helium gas via the gas selector valves, through a sequence of chemical traps which purify the sample. The sample is then cryogenically frozen twice to concentrate the trace gas. The sample is then separated using the poraplot-Q gas chromatograph (GC) column, ready for analysis. During CH4 analysis, the sample is transported through additional stages including, the oxidation of CO to CO2 by a Sofnocat catalyst, combustion in the furnace and an additional cryogenic trap is used. The instrument is designed to be coupled with the IsoPrime stable isotope ratio mass spectrometer (IRMS). The Trace Gas preconcentrator was originally manufactured by GV Instruments, but part of the business was sold to Isoprime Ltd (a group member of Elementar Analysensysteme GmbH) in 2008, who now manufacturer the Trace Gas preconcentrator.</skos:definition>
<owl:versionInfo>1</owl:versionInfo>
<dc:date>2012-10-04 12:03:09.0</dc:date>
<skos:note xml:lang="en">accepted</skos:note>
<owl:deprecated>false</owl:deprecated>
<skos:broader rdf:resource="http://vocab.nerc.ac.uk/collection/L05/current/LAB02/"/>
<void:inDataset rdf:resource="http://vocab.nerc.ac.uk/.well-known/void"/>
</skos:Concept>
</skos:member>
<skos:member>
<skos:Concept rdf:about="http://vocab.nerc.ac.uk/collection/L22/current/TOOL0507/">
<dc:identifier>SDN:L22::TOOL0507</dc:identifier>
<skos:notation>SDN:L22::TOOL0507</skos:notation>
<skos:prefLabel xml:lang="en">Garrett Screen surface sampler</skos:prefLabel>
<skos:altLabel>Garrett Screen</skos:altLabel>
<skos:definition xml:lang="en">A hand-held Monel (nickel-copper alloy) mesh screen in a rigid frame designed to sample the surface film in oceanic waters. The screen is placed horizontally through the water surface then withdrawn from the water (still held horizontally) and drained into a sample bottle. It is used to sample chemical and biological species in the surface film. The Garrett Screen was developed in the 1960s by William Garrett of the US Naval Research Laboratory.</skos:definition>
<owl:versionInfo>1</owl:versionInfo>
<dc:date>2012-06-22 15:36:10.0</dc:date>
<skos:note xml:lang="en">accepted</skos:note>
<owl:deprecated>false</owl:deprecated>
<skos:broader rdf:resource="http://vocab.nerc.ac.uk/collection/L05/current/84/"/>
<void:inDataset rdf:resource="http://vocab.nerc.ac.uk/.well-known/void"/>
</skos:Concept>
</skos:member>
<skos:member>
<skos:Concept rdf:about="http://vocab.nerc.ac.uk/collection/L22/current/TOOL0231/">
<dc:identifier>SDN:L22::TOOL0231</dc:identifier>
<skos:notation>SDN:L22::TOOL0231</skos:notation>
<skos:prefLabel xml:lang="en">Gemini Tinytag plus TGP-0050 temperature recorder</skos:prefLabel>
<skos:altLabel>Tinytag TGP-0050 TR</skos:altLabel>
<skos:definition xml:lang="en">A data logger plus a 10k NTC thermistor internally mounted within a robust IP68 waterproof casing suitable for measuring atmospheric or shallow water temperatures. Temperatures in the range -30 to 50C can be measured and the logger may be used up to water depths of 15 metres. The instrument can store approximately 16000 data readings and be set up with measurement intervals between one second and ten days.</skos:definition>
<owl:versionInfo>1</owl:versionInfo>
<dc:date>2010-05-18 16:10:58.0</dc:date>
<skos:note xml:lang="en">accepted</skos:note>
<owl:deprecated>false</owl:deprecated>
<skos:broader rdf:resource="http://vocab.nerc.ac.uk/collection/L05/current/134/"/>
<skos:broader rdf:resource="http://vocab.nerc.ac.uk/collection/L05/current/102/"/>
<void:inDataset rdf:resource="http://vocab.nerc.ac.uk/.well-known/void"/>
</skos:Concept>
</skos:member>
<skos:member>
<skos:Concept rdf:about="http://vocab.nerc.ac.uk/collection/L22/current/TOOL0506/">
<dc:identifier>SDN:L22::TOOL0506</dc:identifier>
<skos:notation>SDN:L22::TOOL0506</skos:notation>
<skos:prefLabel xml:lang="en">General Oceanics GO-FLO water sampler</skos:prefLabel>
<skos:altLabel>GO-FLO bottle</skos:altLabel>
<skos:definition xml:lang="en">A plastic free-flushing water sampling bottle with a capacity of 1.7-100 litres. The tube is composed of PVC and has ball valves with Viton and silicone seals at each end joined by an external latex spring and nylon and Kevlar lanyards. It is closed when deployed then opens automatically (hydrostatic pressure activated) at approximately 10 m and flushes until closed. When the bottle reaches the desired depth the lanyards are released by a pressure-actuated switch, command signal or messenger weight and the caps are forced shut and sealed. Bottles may be deployed singly clamped to a wire or in groups on a rosette. A reversing thermometer assembly may be attached to the bottle. When extracting water from the bottle, inert gas can be injected into the bottle to force the sample out of the sampling valve. The GO-FLO sampler avoids sample contamination at the surface, internal spring contamination, loss of sample on deck (internal seals), and exchange of water from different depths.</skos:definition>
<owl:versionInfo>1</owl:versionInfo>
<dc:date>2012-06-21 16:09:48.0</dc:date>
<skos:note xml:lang="en">accepted</skos:note>
<owl:deprecated>false</owl:deprecated>
<skos:broader rdf:resource="http://vocab.nerc.ac.uk/collection/L05/current/30/"/>
<void:inDataset rdf:resource="http://vocab.nerc.ac.uk/.well-known/void"/>
</skos:Concept>
</skos:member>
<skos:member>
<skos:Concept rdf:about="http://vocab.nerc.ac.uk/collection/L22/current/TOOL0605/">
<dc:identifier>SDN:L22::TOOL0605</dc:identifier>
<skos:notation>SDN:L22::TOOL0605</skos:notation>
<skos:prefLabel xml:lang="en">Gill Instruments Intrinsically Safe WindObserver anemometer</skos:prefLabel>
<skos:altLabel>Gill IS WindObserver</skos:altLabel>
<skos:definition xml:lang="en">A 2-axis ultrasonic anemometer measuring horizontal wind speed and direction that is suitable for hazardous environments such as oil platforms.</skos:definition>
<owl:versionInfo>1</owl:versionInfo>
<dc:date>2013-03-22 16:30:34.0</dc:date>
<skos:note xml:lang="en">accepted</skos:note>
<owl:deprecated>false</owl:deprecated>
<skos:broader rdf:resource="http://vocab.nerc.ac.uk/collection/L05/current/101/"/>
<void:inDataset rdf:resource="http://vocab.nerc.ac.uk/.well-known/void"/>
</skos:Concept>
</skos:member>
<skos:member>
<skos:Concept rdf:about="http://vocab.nerc.ac.uk/collection/L22/current/TOOL0615/">
<dc:identifier>SDN:L22::TOOL0615</dc:identifier>
<skos:notation>SDN:L22::TOOL0615</skos:notation>
<skos:prefLabel xml:lang="en">Gill Instruments Ltd WindMaster pro ultrasonic anemometer</skos:prefLabel>
<skos:altLabel>WindMaster pro anemometer</skos:altLabel>
<skos:definition xml:lang="en">Three axis ultrasonic anemometer offers sonic temperature, speed of sound and wind vector outputs at 32 Hz. The instrument measures the time taken for an ultrasonic pulse of sound to travel from an upper transducer to the opposite lower transducer, and compares it with the time for a pulse to travel from lower to upper transducer. It has a stainless steel construction and will monitor either 0-60 m/s (0 - 134 mph) or 0-65 m/s (0-145 mph) wind speed depending upon the model. The units of wind speed, output rate, and formats are all user selectable. There are several optional analogue outputs and inputs depending on the model. Windspeed accuracy is 1.5 percent root mean squared (0 - 20 m/s) and wind direction accuracy is 2 degrees at less than 25 m/s.</skos:definition>
<owl:versionInfo>1</owl:versionInfo>
<dc:date>2013-04-23 11:31:52.0</dc:date>
<skos:note xml:lang="en">accepted</skos:note>
<owl:deprecated>false</owl:deprecated>
<skos:broader rdf:resource="http://vocab.nerc.ac.uk/collection/L05/current/101/"/>
<void:inDataset rdf:resource="http://vocab.nerc.ac.uk/.well-known/void"/>
</skos:Concept>
</skos:member>
<skos:member>
<skos:Concept rdf:about="http://vocab.nerc.ac.uk/collection/L22/current/TOOL0616/">
<dc:identifier>SDN:L22::TOOL0616</dc:identifier>
<skos:notation>SDN:L22::TOOL0616</skos:notation>
<skos:prefLabel xml:lang="en">Gill Instruments Ltd WindMaster ultrasonic anemometer</skos:prefLabel>
<skos:altLabel>WindMaster anemometer</skos:altLabel>
<skos:definition xml:lang="en">Three axis ultrasonic anemometer offers sonic temperature, speed of sound and wind vector outputs at 20 Hz (32 Hz option). The instrument measures the time taken for an ultrasonic pulse of sound to travel from an upper transducer to the opposite lower transducer, and compares it with the time for a pulse to travel from lower to upper transducer. It has an aluminium/carbon fibre construction and will monitor either 0-60 m/s (0 - 134 mph) or 0-45 m/s (0-100 mph) wind speed depending upon the model. The units of wind speed, output rate, and formats are all user selectable. There are several optional analogue outputs and inputs depending on the model. Windspeed accuracy is 1.5 percent root mean squared (0 - 20 m/s) and wind direction accuracy is 2 degrees at less than 25 m/s.</skos:definition>
<owl:versionInfo>1</owl:versionInfo>
<dc:date>2013-04-23 11:32:18.0</dc:date>
<skos:note xml:lang="en">accepted</skos:note>
<owl:deprecated>false</owl:deprecated>
<skos:broader rdf:resource="http://vocab.nerc.ac.uk/collection/L05/current/101/"/>
<void:inDataset rdf:resource="http://vocab.nerc.ac.uk/.well-known/void"/>
</skos:Concept>
</skos:member>
<skos:member>
<skos:Concept rdf:about="http://vocab.nerc.ac.uk/collection/L22/current/TOOL0197/">
<dc:identifier>SDN:L22::TOOL0197</dc:identifier>
<skos:notation>SDN:L22::TOOL0197</skos:notation>
<skos:prefLabel xml:lang="en">Gill Windsonic anemometer</skos:prefLabel>
<skos:altLabel>Gill Windsonic anemometer</skos:altLabel>
<skos:definition xml:lang="en">A 2-axis sonic anemometer measuring horizontal wind speed and direction that is suitable for land-based and marine environments. Available in four options, providing a number of different digital and analogue outputs.</skos:definition>
<owl:versionInfo>2</owl:versionInfo>
<dc:date>2010-11-18 12:39:41.0</dc:date>
<skos:note xml:lang="en">accepted</skos:note>
<owl:deprecated>false</owl:deprecated>
<skos:broader rdf:resource="http://vocab.nerc.ac.uk/collection/L05/current/101/"/>
<void:inDataset rdf:resource="http://vocab.nerc.ac.uk/.well-known/void"/>
</skos:Concept>
</skos:member>
<skos:member>
<skos:Concept rdf:about="http://vocab.nerc.ac.uk/collection/L22/current/NETT0045/">
<dc:identifier>SDN:L22::NETT0045</dc:identifier>
<skos:notation>SDN:L22::NETT0045</skos:notation>
<skos:prefLabel xml:lang="en">Gimbal-ring zooplankton sampler - Kozasa (1984)</skos:prefLabel>
<skos:altLabel>Kozasa zooplankton sampler</skos:altLabel>
<skos:definition xml:lang="en">Construction is a double-gimballed frame 100 cm tall x 65.5 cm wide supporting a ring net 30 cm in diameter. A bridle is attached to the top of the frame and a weight to the bottom so the net mouth is free of obstructions.   No description of net length or mesh size given.</skos:definition>
<owl:versionInfo>1</owl:versionInfo>
<dc:date>2011-10-21 14:18:49.0</dc:date>
<skos:note xml:lang="en">accepted</skos:note>
<owl:deprecated>false</owl:deprecated>
<skos:broader rdf:resource="http://vocab.nerc.ac.uk/collection/L05/current/22/"/>
<void:inDataset rdf:resource="http://vocab.nerc.ac.uk/.well-known/void"/>
</skos:Concept>
</skos:member>
<skos:member>
<skos:Concept rdf:about="http://vocab.nerc.ac.uk/collection/L22/current/TOOL0556/">
<dc:identifier>SDN:L22::TOOL0556</dc:identifier>
<skos:notation>SDN:L22::TOOL0556</skos:notation>
<skos:prefLabel xml:lang="en">Glass bottle and bung water sampler</skos:prefLabel>
<skos:altLabel>Glass bottle and bung</skos:altLabel>
<skos:definition xml:lang="en">Glass bottle of unknown capacity used for manual water sampling. The bottle was sealed with a bung attached to a rope. The system was used for near-surface sampling during the Marine and Freshwater Microbial Biodiversity project for sampling in Priest Pot.</skos:definition>
<owl:versionInfo>1</owl:versionInfo>
<dc:date>2012-09-28 14:08:54.0</dc:date>
<skos:note xml:lang="en">accepted</skos:note>
<owl:deprecated>false</owl:deprecated>
<skos:broader rdf:resource="http://vocab.nerc.ac.uk/collection/L05/current/30/"/>
<void:inDataset rdf:resource="http://vocab.nerc.ac.uk/.well-known/void"/>
</skos:Concept>
</skos:member>
<skos:member>
<skos:Concept rdf:about="http://vocab.nerc.ac.uk/collection/L22/current/TOOL0078/">
<dc:identifier>SDN:L22::TOOL0078</dc:identifier>
<skos:notation>SDN:L22::TOOL0078</skos:notation>
<skos:prefLabel xml:lang="en">Global Positioning Satellite System</skos:prefLabel>
<skos:altLabel>GPS</skos:altLabel>
<skos:definition xml:lang="en">A location system of unspecified make or model that determines location on the Earth's surface using the Global Positioning Satellite Network. Angular co-ordinates are given relative to WGS84 CRS. Other parameters such as platform velocity may be derived from this.</skos:definition>
<owl:versionInfo>1</owl:versionInfo>
<dc:date>2010-09-08 11:18:07.0</dc:date>
<skos:note xml:lang="en">accepted</skos:note>
<owl:deprecated>false</owl:deprecated>
<skos:related rdf:resource="http://vocab.nerc.ac.uk/collection/P01/current/ALATGP01/"/>
<skos:related rdf:resource="http://vocab.nerc.ac.uk/collection/P01/current/ALONGP01/"/>
<skos:related rdf:resource="http://vocab.nerc.ac.uk/collection/P01/current/APEWGP01/"/>
<skos:related rdf:resource="http://vocab.nerc.ac.uk/collection/P01/current/APNSGP01/"/>
<owl:sameAs rdf:resource="http://vocab.nerc.ac.uk/collection/L05/current/POS03/"/>
<void:inDataset rdf:resource="http://vocab.nerc.ac.uk/.well-known/void"/>
</skos:Concept>
</skos:member>
<skos:member>
<skos:Concept rdf:about="http://vocab.nerc.ac.uk/collection/L22/current/TOOL0382/">
<dc:identifier>SDN:L22::TOOL0382</dc:identifier>
<skos:notation>SDN:L22::TOOL0382</skos:notation>
<skos:prefLabel xml:lang="en">Grimm 5.403 Condensation Particle Counter</skos:prefLabel>
<skos:altLabel>Grimm CPC 5.403</skos:altLabel>
<skos:definition xml:lang="en">The GRIMM 5.403 Condensation Particle Counter is a portable nano particle counter. Sample air is saturated with butanol vapour and heated to 35 deg C, then cooled to 10 deg C. Particles act as condesation nuclei for the cooling butanol, forming droplets of around 10 um, which are counted by an optical particle counter.</skos:definition>
<owl:versionInfo>1</owl:versionInfo>
<dc:date>2011-03-14 15:22:43.0</dc:date>
<skos:note xml:lang="en">accepted</skos:note>
<owl:deprecated>false</owl:deprecated>
<skos:broader rdf:resource="http://vocab.nerc.ac.uk/collection/L05/current/386/"/>
<void:inDataset rdf:resource="http://vocab.nerc.ac.uk/.well-known/void"/>
</skos:Concept>
</skos:member>
<skos:member>
<skos:Concept rdf:about="http://vocab.nerc.ac.uk/collection/L22/current/TOOL0336/">
<dc:identifier>SDN:L22::TOOL0336</dc:identifier>
<skos:notation>SDN:L22::TOOL0336</skos:notation>
<skos:prefLabel xml:lang="en">Grundy Environmental 6620 thermosalinograph</skos:prefLabel>
<skos:altLabel>Grundy 6620 thermosalinograph</skos:altLabel>
<skos:definition xml:lang="en">An autoranging instrument taking inputs from a hull or inlet thermometer to give sea temperature plus co-located temperature and conductivity sensors to give salinity. In general use during the 1980s and 1990s.</skos:definition>
<owl:versionInfo>1</owl:versionInfo>
<dc:date>2010-09-06 12:45:22.0</dc:date>
<skos:note xml:lang="en">accepted</skos:note>
<owl:deprecated>false</owl:deprecated>
<skos:broader rdf:resource="http://vocab.nerc.ac.uk/collection/L05/current/133/"/>
<skos:broader rdf:resource="http://vocab.nerc.ac.uk/collection/L05/current/350/"/>
<skos:broader rdf:resource="http://vocab.nerc.ac.uk/collection/L05/current/134/"/>
<void:inDataset rdf:resource="http://vocab.nerc.ac.uk/.well-known/void"/>
</skos:Concept>
</skos:member>
<skos:member>
<skos:Concept rdf:about="http://vocab.nerc.ac.uk/collection/L22/current/TOOL0454/">
<dc:identifier>SDN:L22::TOOL0454</dc:identifier>
<skos:notation>SDN:L22::TOOL0454</skos:notation>
<skos:prefLabel xml:lang="en">Guildline 8400 bench salinometer</skos:prefLabel>
<skos:altLabel>8400 salinometer</skos:altLabel>
<skos:definition xml:lang="en">A laboratory instrument that determines salinity of a water sample by comparison of its electrical conductivity with a standard solution. The system employs a continuous flow system, where the sample is drawn into the unit under low air pressure. A high stability temperature control bath and heat exchanger maintain the sample at a precisely defined, user selected temperature during analysis. The instrument can operate over a salinity range of 0.005 to 42 with a resolution of &lt; 0.0002 and an accuracy of &lt; +/- 0.002. There are two models: 8400A and 8400B. The 8400A has an external interface as an optional extra.  The 8400B has improved stability over long periods and the external interface is fitted as standard.</skos:definition>
<owl:versionInfo>2</owl:versionInfo>
<dc:date>2013-01-25 12:33:29.0</dc:date>
<skos:note xml:lang="en">accepted</skos:note>
<owl:deprecated>false</owl:deprecated>
<skos:broader rdf:resource="http://vocab.nerc.ac.uk/collection/L05/current/LAB30/"/>
<void:inDataset rdf:resource="http://vocab.nerc.ac.uk/.well-known/void"/>
</skos:Concept>
</skos:member>
<skos:member>
<skos:Concept rdf:about="http://vocab.nerc.ac.uk/collection/L22/current/TOOL0032/">
<dc:identifier>SDN:L22::TOOL0032</dc:identifier>
<skos:notation>SDN:L22::TOOL0032</skos:notation>
<skos:prefLabel xml:lang="en">Guildline Model 8705 Digital CTD</skos:prefLabel>
<skos:altLabel>Guildline 8705 CTD</skos:altLabel>
<skos:definition xml:lang="en">A CTD unit designed for open ocean applications down to depths of 6000m. The probe was an anodised aluminium tube with a steel cage at one end protecting the temperature and conductivity sensors and a urethane cap at the other to protect the pressure sensor diaphragm. Conductivity cell was a Pyrex tube with four electrodes in an H configuration to allow free circulation of seawater. The thermometer was a fine copper wire enclosed in an oil-filled stainless steel capilliary. The pressure transducer was a 4-arm strain gauge bridge.</skos:definition>
<owl:versionInfo>1</owl:versionInfo>
<dc:date>2009-11-30 11:56:35.0</dc:date>
<skos:note xml:lang="en">accepted</skos:note>
<owl:deprecated>false</owl:deprecated>
<skos:related rdf:resource="http://vocab.nerc.ac.uk/collection/P01/current/PRESPR01/"/>
<skos:related rdf:resource="http://vocab.nerc.ac.uk/collection/P01/current/PSALST01/"/>
<skos:related rdf:resource="http://vocab.nerc.ac.uk/collection/P01/current/TEMPST01/"/>
<skos:broader rdf:resource="http://vocab.nerc.ac.uk/collection/L05/current/350/"/>
<void:inDataset rdf:resource="http://vocab.nerc.ac.uk/.well-known/void"/>
</skos:Concept>
</skos:member>
<skos:member>
<skos:Concept rdf:about="http://vocab.nerc.ac.uk/collection/L22/current/TOOL0034/">
<dc:identifier>SDN:L22::TOOL0034</dc:identifier>
<skos:notation>SDN:L22::TOOL0034</skos:notation>
<skos:prefLabel xml:lang="en">Guildline Model 8770 Digital CTD</skos:prefLabel>
<skos:altLabel>Guildline 8770 CTD</skos:altLabel>
<skos:definition xml:lang="en">CTD with conductivity electrode mounted in pyrex glass, copper resistance element in a stainless steel tube for temperature and a pressure sensor comprising a strain gauge element in a 4-arm resistance bridge network</skos:definition>
<owl:versionInfo>1</owl:versionInfo>
<dc:date>2009-11-30 11:56:35.0</dc:date>
<skos:note xml:lang="en">accepted</skos:note>
<owl:deprecated>false</owl:deprecated>
<skos:broader rdf:resource="http://vocab.nerc.ac.uk/collection/L05/current/130/"/>
<skos:broader rdf:resource="http://vocab.nerc.ac.uk/collection/L05/current/134/"/>
<void:inDataset rdf:resource="http://vocab.nerc.ac.uk/.well-known/void"/>
</skos:Concept>
</skos:member>
<skos:member>
<skos:Concept rdf:about="http://vocab.nerc.ac.uk/collection/L22/current/TOOL0242/">
<dc:identifier>SDN:L22::TOOL0242</dc:identifier>
<skos:notation>SDN:L22::TOOL0242</skos:notation>
<skos:prefLabel xml:lang="en">Guildline Portasal 8410 series salinometer</skos:prefLabel>
<skos:altLabel>Guildline 8410 salinometer</skos:altLabel>
<skos:definition xml:lang="en">A portable instrument for laboratory or field use that determines salinity of a water sample by comparison of its electrical conductivity with a standard solution. The system employs a continuous flow system, where the sample is drawn into the unit under low air pressure. A high stability temperature control bath and heat exchanger maintain the sample at a precisely defined, user selected temperature during analysis. The instrument can operate over a conductivity range of 0.004 to 76 mS/cm with a resolution of 0.0003 mS/cm (15 deg C and 35 PSU) or 0.0003 Equivalent PSU, and an accuracy of ± 0.003 Equivalent PSU (same set point temperature as standardization and within -2 deg C and +4 deg C of ambient). The series consists of 2 known models: 8410 and 8410A. The models have the same specifications although the 8410A has an RS232 interface. The reference number 8410N refers to an operational manual update only.</skos:definition>
<owl:versionInfo>3</owl:versionInfo>
<dc:date>2013-08-01 09:53:30.0</dc:date>
<skos:note xml:lang="en">accepted</skos:note>
<owl:deprecated>false</owl:deprecated>
<skos:broader rdf:resource="http://vocab.nerc.ac.uk/collection/L05/current/LAB30/"/>
<void:inDataset rdf:resource="http://vocab.nerc.ac.uk/.well-known/void"/>
</skos:Concept>
</skos:member>
<skos:member>
<skos:Concept rdf:about="http://vocab.nerc.ac.uk/collection/L22/current/NETT0046/">
<dc:identifier>SDN:L22::NETT0046</dc:identifier>
<skos:notation>SDN:L22::NETT0046</skos:notation>
<skos:prefLabel xml:lang="en">Gulf I high-speed sampler - Arnold (1952)</skos:prefLabel>
<skos:altLabel>Gulf I HSS</skos:altLabel>
<skos:definition xml:lang="en">A 7.6 cm diameter inside cylinder net 91 cm long of No. 10 screen (0.038 cm mesh).  Equipped with a flowmeter. Towed at ~ 9 knots [Wiebe and Benfield 2003 Plate 15 C].</skos:definition>
<owl:versionInfo>1</owl:versionInfo>
<dc:date>2011-10-21 14:18:49.0</dc:date>
<skos:note xml:lang="en">accepted</skos:note>
<owl:deprecated>false</owl:deprecated>
<skos:broader rdf:resource="http://vocab.nerc.ac.uk/collection/L05/current/67/"/>
<skos:broader rdf:resource="http://vocab.nerc.ac.uk/collection/L05/current/388/"/>
<void:inDataset rdf:resource="http://vocab.nerc.ac.uk/.well-known/void"/>
</skos:Concept>
</skos:member>
<skos:member>
<skos:Concept rdf:about="http://vocab.nerc.ac.uk/collection/L22/current/NETT0047/">
<dc:identifier>SDN:L22::NETT0047</dc:identifier>
<skos:notation>SDN:L22::NETT0047</skos:notation>
<skos:prefLabel xml:lang="en">Gulf II high-speed sampler - Collier (1957)</skos:prefLabel>
<skos:altLabel>Gulf II HSS</skos:altLabel>
<skos:definition xml:lang="en">A shipboard pump drew water from near the keel of the vessel which was delivered to a circular pan divided into 8 parts each with a filter to catch the plankton. The  sampling interval for a filter was 1 hour. Filters (#1 bolting silk) were replaced every 8 hours.  This system was developed as a substitute for the Continuous Plankton Recorder.</skos:definition>
<owl:versionInfo>1</owl:versionInfo>
<dc:date>2011-10-21 14:18:49.0</dc:date>
<skos:note xml:lang="en">accepted</skos:note>
<owl:deprecated>false</owl:deprecated>
<skos:broader rdf:resource="http://vocab.nerc.ac.uk/collection/L05/current/21/"/>
<void:inDataset rdf:resource="http://vocab.nerc.ac.uk/.well-known/void"/>
</skos:Concept>
</skos:member>
<skos:member>
<skos:Concept rdf:about="http://vocab.nerc.ac.uk/collection/L22/current/NETT0048/">
<dc:identifier>SDN:L22::NETT0048</dc:identifier>
<skos:notation>SDN:L22::NETT0048</skos:notation>
<skos:prefLabel xml:lang="en">Gulf III high-speed sampler - Gehringer (1952)</skos:prefLabel>
<skos:altLabel>Gulf III HSS</skos:altLabel>
<skos:definition xml:lang="en">Construction is a 40.7 cm diameter nose piece entrance into an 50.2 cm diameter cylinder 152 cm long made of 0.152 cm monel metal mesh. 49.5 cm diameter inside conical net 137 cm long of No. 10 screen (0.038 cm mesh ~ No. 1 silk).  Equipped with flowmeter. Towed at  5+ knots. Also used with 20.3 cm nose cone [Wiebe and Benfield 2003 Plate 15 D].</skos:definition>
<owl:versionInfo>1</owl:versionInfo>
<dc:date>2011-10-21 14:18:49.0</dc:date>
<skos:note xml:lang="en">accepted</skos:note>
<owl:deprecated>false</owl:deprecated>
<skos:broader rdf:resource="http://vocab.nerc.ac.uk/collection/L05/current/67/"/>
<skos:broader rdf:resource="http://vocab.nerc.ac.uk/collection/L05/current/388/"/>
<void:inDataset rdf:resource="http://vocab.nerc.ac.uk/.well-known/void"/>
</skos:Concept>
</skos:member>
<skos:member>
<skos:Concept rdf:about="http://vocab.nerc.ac.uk/collection/L22/current/NETT0050/">
<dc:identifier>SDN:L22::NETT0050</dc:identifier>
<skos:notation>SDN:L22::NETT0050</skos:notation>
<skos:prefLabel xml:lang="en">Gulf V high-speed sampler - Arnold (1959)</skos:prefLabel>
<skos:altLabel>Gulf V HSS</skos:altLabel>
<skos:definition xml:lang="en">A 41 cm diameter mouth opening with frame 130 cm long.  Conical Monel mesh net with 30 meshes per cm. An unencased and scaled down version of the Gulf III described by Gehringer   [Wiebe and Benfield 2003 Plate 16 A].</skos:definition>
<owl:versionInfo>1</owl:versionInfo>
<dc:date>2011-10-21 14:18:49.0</dc:date>
<skos:note xml:lang="en">accepted</skos:note>
<owl:deprecated>false</owl:deprecated>
<skos:broader rdf:resource="http://vocab.nerc.ac.uk/collection/L05/current/388/"/>
<skos:broader rdf:resource="http://vocab.nerc.ac.uk/collection/L05/current/67/"/>
<void:inDataset rdf:resource="http://vocab.nerc.ac.uk/.well-known/void"/>
</skos:Concept>
</skos:member>
<skos:member>
<skos:Concept rdf:about="http://vocab.nerc.ac.uk/collection/L22/current/NETT0051/">
<dc:identifier>SDN:L22::NETT0051</dc:identifier>
<skos:notation>SDN:L22::NETT0051</skos:notation>
<skos:prefLabel xml:lang="en">Gulf VII Pro-net and MAFF-Guildline high-speed samplers  - Nash et al. (1998)</skos:prefLabel>
<skos:altLabel>Gulf VII HSS</skos:altLabel>
<skos:definition xml:lang="en">An un-encased frame 275 cm long and 76 cm in diameter with a conical nose cone. (There are smaller and larger variants of the frame and nose cone). Standard mouth opening is 40 cm diameter. Pronet is a conical net with 0.28 mm nylon mesh is 230 cm long.   Both systems are equipped with a pressure, temperature, conductivity sensor, and flowmetering package for transmission to ship via conducting cable or logged internally. Other environmental sensors can be accommodated.  Data scanned/recorded twice per second.  Routinely towed at 5 knots and up to 7 knots [Wiebe and Benfield 2003 Plate 17 C].</skos:definition>
<owl:versionInfo>1</owl:versionInfo>
<dc:date>2011-10-21 14:18:49.0</dc:date>
<skos:note xml:lang="en">accepted</skos:note>
<owl:deprecated>false</owl:deprecated>
<skos:broader rdf:resource="http://vocab.nerc.ac.uk/collection/L05/current/134/"/>
<skos:broader rdf:resource="http://vocab.nerc.ac.uk/collection/L05/current/350/"/>
<skos:broader rdf:resource="http://vocab.nerc.ac.uk/collection/L05/current/388/"/>
<skos:broader rdf:resource="http://vocab.nerc.ac.uk/collection/L05/current/67/"/>
<void:inDataset rdf:resource="http://vocab.nerc.ac.uk/.well-known/void"/>
</skos:Concept>
</skos:member>
<skos:member>
<skos:Concept rdf:about="http://vocab.nerc.ac.uk/collection/L22/current/TOOL0079/">
<dc:identifier>SDN:L22::TOOL0079</dc:identifier>
<skos:notation>SDN:L22::TOOL0079</skos:notation>
<skos:prefLabel xml:lang="en">Gyrocompass</skos:prefLabel>
<skos:altLabel>Gyro</skos:altLabel>
<skos:definition xml:lang="en">A compass of unspecified make or model number that finds true north by using a fast-spinning wheel and friction forces to sense the rotation of the Earth.</skos:definition>
<owl:versionInfo>1</owl:versionInfo>
<dc:date>2010-09-08 11:20:45.0</dc:date>
<skos:note xml:lang="en">accepted</skos:note>
<owl:deprecated>false</owl:deprecated>
<skos:related rdf:resource="http://vocab.nerc.ac.uk/collection/P01/current/HEADCM01/"/>
<skos:broader rdf:resource="http://vocab.nerc.ac.uk/collection/L05/current/385/"/>
<void:inDataset rdf:resource="http://vocab.nerc.ac.uk/.well-known/void"/>
</skos:Concept>
</skos:member>
<skos:member>
<skos:Concept rdf:about="http://vocab.nerc.ac.uk/collection/L22/current/TOOL0141/">
<dc:identifier>SDN:L22::TOOL0141</dc:identifier>
<skos:notation>SDN:L22::TOOL0141</skos:notation>
<skos:prefLabel xml:lang="en">HOBI HydroScat-2 Optical Backscatter Fluorometer</skos:prefLabel>
<skos:altLabel>HS-2 OBS-fluorometer</skos:altLabel>
<skos:definition xml:lang="en">Instrument that measures optical backscatter at 2 wavelengths (420nm and 700nm as standard but can be customised) plus chlorophyll fluorescence. Casings available for 330m, 4000m or custom maximum depth working.</skos:definition>
<owl:versionInfo>1</owl:versionInfo>
<dc:date>2010-05-18 16:10:58.0</dc:date>
<skos:note xml:lang="en">accepted</skos:note>
<owl:deprecated>false</owl:deprecated>
<skos:broader rdf:resource="http://vocab.nerc.ac.uk/collection/L05/current/113/"/>
<skos:broader rdf:resource="http://vocab.nerc.ac.uk/collection/L05/current/123/"/>
<void:inDataset rdf:resource="http://vocab.nerc.ac.uk/.well-known/void"/>
</skos:Concept>
</skos:member>
<skos:member>
<skos:Concept rdf:about="http://vocab.nerc.ac.uk/collection/L22/current/NETT0064/">
<dc:identifier>SDN:L22::NETT0064</dc:identifier>
<skos:notation>SDN:L22::NETT0064</skos:notation>
<skos:prefLabel xml:lang="en">HOrizontal PLAnkton SAmpler  - Ruetzler et al. (1980)</skos:prefLabel>
<skos:altLabel>HOPLASA</skos:altLabel>
<skos:definition xml:lang="en">18.5 cm diameter x 40 cm long plexiglass cylinder houses a electric motor and propellor assembly and a flow meter. Attached to the back is a net 80 cm long made with 0.25 mm nylon mesh. The device which creates its own current flow through the net is intended for plankton collection on or near the bottom of coral reefs [Wiebe and Benfield 2003 Plate 24 C]</skos:definition>
<owl:versionInfo>1</owl:versionInfo>
<dc:date>2011-10-21 14:18:49.0</dc:date>
<skos:note xml:lang="en">accepted</skos:note>
<owl:deprecated>false</owl:deprecated>
<skos:broader rdf:resource="http://vocab.nerc.ac.uk/collection/L05/current/388/"/>
<skos:broader rdf:resource="http://vocab.nerc.ac.uk/collection/L05/current/22/"/>
<skos:broader rdf:resource="http://vocab.nerc.ac.uk/collection/L05/current/24/"/>
<void:inDataset rdf:resource="http://vocab.nerc.ac.uk/.well-known/void"/>
</skos:Concept>
</skos:member>
<skos:member>
<skos:Concept rdf:about="http://vocab.nerc.ac.uk/collection/L22/current/TOOL0603/">
<dc:identifier>SDN:L22::TOOL0603</dc:identifier>
<skos:notation>SDN:L22::TOOL0603</skos:notation>
<skos:prefLabel xml:lang="en">Helzel Messtechnik WERA HF Radar</skos:prefLabel>
<skos:altLabel>WERA HF Radar</skos:altLabel>
<skos:definition xml:lang="en">A shore based remote sensing HF radar system used for near real-time mapping of ocean surface currents, waves and wind direction using short radio wave radar. It is a long-range, high resolution monitoring sytem which can detect signals from ranges of more than 200 km.</skos:definition>
<owl:versionInfo>3</owl:versionInfo>
<dc:date>2013-03-13 16:11:10.0</dc:date>
<skos:note xml:lang="en">accepted</skos:note>
<owl:deprecated>false</owl:deprecated>
<skos:broader rdf:resource="http://vocab.nerc.ac.uk/collection/L05/current/110/"/>
<skos:broader rdf:resource="http://vocab.nerc.ac.uk/collection/L05/current/303/"/>
<skos:broader rdf:resource="http://vocab.nerc.ac.uk/collection/L05/current/305/"/>
<void:inDataset rdf:resource="http://vocab.nerc.ac.uk/.well-known/void"/>
</skos:Concept>
</skos:member>
<skos:member>
<skos:Concept rdf:about="http://vocab.nerc.ac.uk/collection/L22/current/NETT0054/">
<dc:identifier>SDN:L22::NETT0054</dc:identifier>
<skos:notation>SDN:L22::NETT0054</skos:notation>
<skos:prefLabel xml:lang="en">Hensen egg net - Hensen (1887); Jenkins (1901); Wimpenny (1937)</skos:prefLabel>
<skos:altLabel>Hensen egg net</skos:altLabel>
<skos:definition xml:lang="en">Construction is a 38 cm diameter mouth (40 cm long conical mouth piece); 100 cm diameter conical net mouth. 144 cm long net of No. 20 silk [Wiebe and Benfield 2003 Plate 1 A, B)</skos:definition>
<owl:versionInfo>1</owl:versionInfo>
<dc:date>2011-10-21 14:18:49.0</dc:date>
<skos:note xml:lang="en">accepted</skos:note>
<owl:deprecated>false</owl:deprecated>
<skos:broader rdf:resource="http://vocab.nerc.ac.uk/collection/L05/current/22/"/>
<void:inDataset rdf:resource="http://vocab.nerc.ac.uk/.well-known/void"/>
</skos:Concept>
</skos:member>
<skos:member>
<skos:Concept rdf:about="http://vocab.nerc.ac.uk/collection/L22/current/TOOL0558/">
<dc:identifier>SDN:L22::TOOL0558</dc:identifier>
<skos:notation>SDN:L22::TOOL0558</skos:notation>
<skos:prefLabel xml:lang="en">Hewlett Packard 5890 Series II Gas Chromatograph</skos:prefLabel>
<skos:altLabel>HP5890 II GC</skos:altLabel>
<skos:definition xml:lang="en">A gas chromatograph that separates and analyses compounds that do not degrade or decompose in the gas phase. The sample is dissolved in a solvent and vaporised in the instrument. A chemically inert gas, (e.g. helium or nitrogen) carries the vaporised analyte through a stationary phase which is coated inside the capillary column that is maintained at an elevated temperature. The analyte mixture separates on the stationary phase leading to chromatographic separation of the molecules. The HP 5890 Series II is completely customisable depending on the application, with choices of inlets, columns, detectors, sampling systems, flow and pressure control components. Optional detectors include Flame Ionization Detector (FID), Nitrogen-Phosphorus Detector (NPD), Electron Capture Detector (ECD), Thermal Conductivity Detector (TCD), Photoionisation Detector (PID), Flame Photometric Detector (FPD) and mass spectrometer. The instrument was originally manufactured by Hewlett Packard (HP), but part of this business was sold to Agilent Technologies in 1999. This model is no longer in production.</skos:definition>
<owl:versionInfo>1</owl:versionInfo>
<dc:date>2012-10-04 12:03:09.0</dc:date>
<skos:note xml:lang="en">accepted</skos:note>
<owl:deprecated>false</owl:deprecated>
<skos:broader rdf:resource="http://vocab.nerc.ac.uk/collection/L05/current/LAB02/"/>
<void:inDataset rdf:resource="http://vocab.nerc.ac.uk/.well-known/void"/>
</skos:Concept>
</skos:member>
<skos:member>
<skos:Concept rdf:about="http://vocab.nerc.ac.uk/collection/L22/current/TOOL0551/">
<dc:identifier>SDN:L22::TOOL0551</dc:identifier>
<skos:notation>SDN:L22::TOOL0551</skos:notation>
<skos:prefLabel xml:lang="en">High Volume Air Sampler</skos:prefLabel>
<skos:altLabel>HVAS</skos:altLabel>
<skos:definition xml:lang="en">An atmospheric sampler that pumps air through a series of filters and traps to collect samples for off-line analysis of aerosol and gas-phase constituents. Air samples are drawn into a sheltered housing, and through one or more aerosol filters, which collect samples of particulate material. Successive aerosol filters may have smaller pore sizes to collect size fractionated aerosol samples. The air may then be drawn through one or more gas-phase filters or traps, such as reagent-soaked filter papers, reagent-filled impingers, or resin (polymer) traps. Flow meters between the filter set and the pump determine the volume of air sampled.</skos:definition>
<owl:versionInfo>1</owl:versionInfo>
<dc:date>2012-09-26 16:33:22.0</dc:date>
<skos:note xml:lang="en">accepted</skos:note>
<owl:deprecated>false</owl:deprecated>
<skos:broader rdf:resource="http://vocab.nerc.ac.uk/collection/L05/current/13/"/>
<void:inDataset rdf:resource="http://vocab.nerc.ac.uk/.well-known/void"/>
</skos:Concept>
</skos:member>
<skos:member>
<skos:Concept rdf:about="http://vocab.nerc.ac.uk/collection/L22/current/NETT0067/">
<dc:identifier>SDN:L22::NETT0067</dc:identifier>
<skos:notation>SDN:L22::NETT0067</skos:notation>
<skos:prefLabel xml:lang="en">High speed-sampler - Monti (1910)</skos:prefLabel>
<skos:altLabel>Monti HSS</skos:altLabel>
<skos:definition xml:lang="en">A cylindrical tube modified from Zacharias with a 3-4 cm diameter mouth opening expanding to 10-12 cm diameter main body and a filtering cone leading to a stopcock at the rear.  Overall length 50 cm [Wiebe and Benfield 2003 Plate 13 C].</skos:definition>
<owl:versionInfo>1</owl:versionInfo>
<dc:date>2011-10-21 14:18:49.0</dc:date>
<skos:note xml:lang="en">accepted</skos:note>
<owl:deprecated>false</owl:deprecated>
<skos:broader rdf:resource="http://vocab.nerc.ac.uk/collection/L05/current/67/"/>
<void:inDataset rdf:resource="http://vocab.nerc.ac.uk/.well-known/void"/>
</skos:Concept>
</skos:member>
<skos:member>
<skos:Concept rdf:about="http://vocab.nerc.ac.uk/collection/L22/current/NETT0060/">
<dc:identifier>SDN:L22::NETT0060</dc:identifier>
<skos:notation>SDN:L22::NETT0060</skos:notation>
<skos:prefLabel xml:lang="en">High-Speed net model II - Cassie (1956)</skos:prefLabel>
<skos:altLabel>Cassie high-speed net model II</skos:altLabel>
<skos:definition xml:lang="en">Same as the model 1 (6cm diameter 6cm long brass cylinder with 180 cm net) except the system was shorter (90 cm) and the net made out of brass gauze with 16 meshes per cm and two metal rods (struts) connected the brass cylinder to the cod end bucket.</skos:definition>
<owl:versionInfo>1</owl:versionInfo>
<dc:date>2011-10-21 14:18:49.0</dc:date>
<skos:note xml:lang="en">accepted</skos:note>
<owl:deprecated>false</owl:deprecated>
<skos:broader rdf:resource="http://vocab.nerc.ac.uk/collection/L05/current/67/"/>
<void:inDataset rdf:resource="http://vocab.nerc.ac.uk/.well-known/void"/>
</skos:Concept>
</skos:member>
<skos:member>
<skos:Concept rdf:about="http://vocab.nerc.ac.uk/collection/L22/current/NETT0058/">
<dc:identifier>SDN:L22::NETT0058</dc:identifier>
<skos:notation>SDN:L22::NETT0058</skos:notation>
<skos:prefLabel xml:lang="en">High-speed metal plankton net - Fry (1937)</skos:prefLabel>
<skos:altLabel>Fry high-speed metal plankton net</skos:altLabel>
<skos:definition xml:lang="en">Construction comprises a 10.2 cm diameter mouth opening expanding to 25.4 cm followed by a mesh cone (15.7 meshes per cm) and a cod end. Overall length 152 cm. Towed with 3 part chain bridle at speeds up to 10 knots [Wiebe and Benfield 2003 Plate 14 C].</skos:definition>
<owl:versionInfo>1</owl:versionInfo>
<dc:date>2011-10-21 14:18:49.0</dc:date>
<skos:note xml:lang="en">accepted</skos:note>
<owl:deprecated>false</owl:deprecated>
<skos:broader rdf:resource="http://vocab.nerc.ac.uk/collection/L05/current/67/"/>
<void:inDataset rdf:resource="http://vocab.nerc.ac.uk/.well-known/void"/>
</skos:Concept>
</skos:member>
<skos:member>
<skos:Concept rdf:about="http://vocab.nerc.ac.uk/collection/L22/current/NETT0068/">
<dc:identifier>SDN:L22::NETT0068</dc:identifier>
<skos:notation>SDN:L22::NETT0068</skos:notation>
<skos:prefLabel xml:lang="en">High-speed multiple sampler - Porche (1978)</skos:prefLabel>
<skos:altLabel>Porche HSS</skos:altLabel>
<skos:definition xml:lang="en">Comprises 4 nets and one intake.  The nets rotate into the water flow position to collect a sample. Instrument reference is in French.</skos:definition>
<owl:versionInfo>1</owl:versionInfo>
<dc:date>2011-10-21 14:18:49.0</dc:date>
<skos:note xml:lang="en">accepted</skos:note>
<owl:deprecated>false</owl:deprecated>
<skos:broader rdf:resource="http://vocab.nerc.ac.uk/collection/L05/current/67/"/>
<void:inDataset rdf:resource="http://vocab.nerc.ac.uk/.well-known/void"/>
</skos:Concept>
</skos:member>
<skos:member>
<skos:Concept rdf:about="http://vocab.nerc.ac.uk/collection/L22/current/NETT0062/">
<dc:identifier>SDN:L22::NETT0062</dc:identifier>
<skos:notation>SDN:L22::NETT0062</skos:notation>
<skos:prefLabel xml:lang="en">High-speed net - Cassie (1956)</skos:prefLabel>
<skos:altLabel>Cassie high-speed net</skos:altLabel>
<skos:definition xml:lang="en">A combination of model 1, model 2 and model 3 nets  towed from the stern of the vessel at ~ 8 knots on a 40 m tow line.</skos:definition>
<owl:versionInfo>1</owl:versionInfo>
<dc:date>2011-10-21 14:18:49.0</dc:date>
<skos:note xml:lang="en">accepted</skos:note>
<owl:deprecated>false</owl:deprecated>
<skos:broader rdf:resource="http://vocab.nerc.ac.uk/collection/L05/current/67/"/>
<void:inDataset rdf:resource="http://vocab.nerc.ac.uk/.well-known/void"/>
</skos:Concept>
</skos:member>
<skos:member>
<skos:Concept rdf:about="http://vocab.nerc.ac.uk/collection/L22/current/NETT0059/">
<dc:identifier>SDN:L22::NETT0059</dc:identifier>
<skos:notation>SDN:L22::NETT0059</skos:notation>
<skos:prefLabel xml:lang="en">High-speed net model I - Cassie (1956)</skos:prefLabel>
<skos:altLabel>Cassie high-speed net model I</skos:altLabel>
<skos:definition xml:lang="en">A brass cylinder 6 cm diameter and 6 cm long with bridle attachment lugs that had a 180 cm bolting cloth net (16 or 30 meshes per cm) attached to the back [Wiebe and Benfield 2003 Plate 18 A ].</skos:definition>
<owl:versionInfo>1</owl:versionInfo>
<dc:date>2011-10-21 14:18:49.0</dc:date>
<skos:note xml:lang="en">accepted</skos:note>
<owl:deprecated>false</owl:deprecated>
<skos:broader rdf:resource="http://vocab.nerc.ac.uk/collection/L05/current/67/"/>
<void:inDataset rdf:resource="http://vocab.nerc.ac.uk/.well-known/void"/>
</skos:Concept>
</skos:member>
<skos:member>
<skos:Concept rdf:about="http://vocab.nerc.ac.uk/collection/L22/current/NETT0061/">
<dc:identifier>SDN:L22::NETT0061</dc:identifier>
<skos:notation>SDN:L22::NETT0061</skos:notation>
<skos:prefLabel xml:lang="en">High-speed net model III - Cassie (1956)</skos:prefLabel>
<skos:altLabel>Cassie high-speed net model III</skos:altLabel>
<skos:definition xml:lang="en">Same as model 2 (6cm diameter 6cm long brass cylinder with 90 cm net) except shorter again (60 cm) and four metal rods (struts) connected the brass cylinder to the cod end bucket.</skos:definition>
<owl:versionInfo>1</owl:versionInfo>
<dc:date>2011-10-21 14:18:49.0</dc:date>
<skos:note xml:lang="en">accepted</skos:note>
<owl:deprecated>false</owl:deprecated>
<skos:broader rdf:resource="http://vocab.nerc.ac.uk/collection/L05/current/67/"/>
<void:inDataset rdf:resource="http://vocab.nerc.ac.uk/.well-known/void"/>
</skos:Concept>
</skos:member>
<skos:member>
<skos:Concept rdf:about="http://vocab.nerc.ac.uk/collection/L22/current/NETT0056/">
<dc:identifier>SDN:L22::NETT0056</dc:identifier>
<skos:notation>SDN:L22::NETT0056</skos:notation>
<skos:prefLabel xml:lang="en">High-speed plankton sampler - Pierce (1937)</skos:prefLabel>
<skos:altLabel>Pierce HSS</skos:altLabel>
<skos:definition xml:lang="en">Construction comprises a 7 cm mouth opening of front cone which was 16.5 cm long.  17.8 cm diameter cylinder body which was 25.4 cm long. 7 cm conical coarse silk net 16.5 cm long with small jar cod end.</skos:definition>
<owl:versionInfo>1</owl:versionInfo>
<dc:date>2011-10-21 14:18:49.0</dc:date>
<skos:note xml:lang="en">accepted</skos:note>
<owl:deprecated>false</owl:deprecated>
<skos:broader rdf:resource="http://vocab.nerc.ac.uk/collection/L05/current/67/"/>
<void:inDataset rdf:resource="http://vocab.nerc.ac.uk/.well-known/void"/>
</skos:Concept>
</skos:member>
<skos:member>
<skos:Concept rdf:about="http://vocab.nerc.ac.uk/collection/L22/current/NETT0002/">
<dc:identifier>SDN:L22::NETT0002</dc:identifier>
<skos:notation>SDN:L22::NETT0002</skos:notation>
<skos:prefLabel xml:lang="en">High-speed sampler - Apstein (1906)</skos:prefLabel>
<skos:altLabel>Apstein HSS</skos:altLabel>
<skos:definition xml:lang="en">Construction is a cylindrical tube with ~2 cm diameter mouth opening expanding to 4 cm diameter in the main body with a filtering surface at the rear.  Overall length ~20 cm [Wiebe and Benfield 2003 Plate 13 A].</skos:definition>
<owl:versionInfo>1</owl:versionInfo>
<dc:date>2011-10-21 14:18:49.0</dc:date>
<skos:note xml:lang="en">accepted</skos:note>
<owl:deprecated>false</owl:deprecated>
<skos:broader rdf:resource="http://vocab.nerc.ac.uk/collection/L05/current/67/"/>
<void:inDataset rdf:resource="http://vocab.nerc.ac.uk/.well-known/void"/>
</skos:Concept>
</skos:member>
<skos:member>
<skos:Concept rdf:about="http://vocab.nerc.ac.uk/collection/L22/current/NETT0057/">
<dc:identifier>SDN:L22::NETT0057</dc:identifier>
<skos:notation>SDN:L22::NETT0057</skos:notation>
<skos:prefLabel xml:lang="en">High-speed sampler - Erdmann (1937)</skos:prefLabel>
<skos:altLabel>Erdmann HSS</skos:altLabel>
<skos:definition xml:lang="en">Construction comprises a ~4.5 cm diameter mouth expanding to 12 cm with overall length of 64 cm.  Has an opening/closing mechanism [Wiebe and Benfield 2003 Plate 14 D].</skos:definition>
<owl:versionInfo>1</owl:versionInfo>
<dc:date>2011-10-21 14:18:49.0</dc:date>
<skos:note xml:lang="en">accepted</skos:note>
<owl:deprecated>false</owl:deprecated>
<skos:broader rdf:resource="http://vocab.nerc.ac.uk/collection/L05/current/67/"/>
<void:inDataset rdf:resource="http://vocab.nerc.ac.uk/.well-known/void"/>
</skos:Concept>
</skos:member>
<skos:member>
<skos:Concept rdf:about="http://vocab.nerc.ac.uk/collection/L22/current/NETT0055/">
<dc:identifier>SDN:L22::NETT0055</dc:identifier>
<skos:notation>SDN:L22::NETT0055</skos:notation>
<skos:prefLabel xml:lang="en">High-speed sampler - Smith and Ahlstrom (1948)</skos:prefLabel>
<skos:altLabel>Smith HSS</skos:altLabel>
<skos:definition xml:lang="en">Construction comprises a 2.54 cm diameter mouth expanding to 5.08 cm (brass), cylindrical net 5.08 cm and 25.4 cm long made of No. 56xxx grit gauze, and a bucket. Towed at 9 knots.</skos:definition>
<owl:versionInfo>1</owl:versionInfo>
<dc:date>2011-10-21 14:18:49.0</dc:date>
<skos:note xml:lang="en">accepted</skos:note>
<owl:deprecated>false</owl:deprecated>
<skos:broader rdf:resource="http://vocab.nerc.ac.uk/collection/L05/current/67/"/>
<void:inDataset rdf:resource="http://vocab.nerc.ac.uk/.well-known/void"/>
</skos:Concept>
</skos:member>
<skos:member>
<skos:Concept rdf:about="http://vocab.nerc.ac.uk/collection/L22/current/NETT0066/">
<dc:identifier>SDN:L22::NETT0066</dc:identifier>
<skos:notation>SDN:L22::NETT0066</skos:notation>
<skos:prefLabel xml:lang="en">High-speed sampler - Zacharias (1907)</skos:prefLabel>
<skos:altLabel>Zacharias HSS</skos:altLabel>
<skos:definition xml:lang="en">A cylindrical tube similar to Apstein’s with ~3 cm diameter mouth opening expanding to 8 cm diameter main body with baffles for different towing speeds and a filtering surface at the rear. Overall length 42 cm [Wiebe and Benfield 2003 Plate 13 B].</skos:definition>
<owl:versionInfo>1</owl:versionInfo>
<dc:date>2011-10-21 14:18:49.0</dc:date>
<skos:note xml:lang="en">accepted</skos:note>
<owl:deprecated>false</owl:deprecated>
<skos:broader rdf:resource="http://vocab.nerc.ac.uk/collection/L05/current/67/"/>
<void:inDataset rdf:resource="http://vocab.nerc.ac.uk/.well-known/void"/>
</skos:Concept>
</skos:member>
<skos:member>
<skos:Concept rdf:about="http://vocab.nerc.ac.uk/collection/L22/current/NETT0065/">
<dc:identifier>SDN:L22::NETT0065</dc:identifier>
<skos:notation>SDN:L22::NETT0065</skos:notation>
<skos:prefLabel xml:lang="en">High-speed successive plankton sampler - Motoda (1953)</skos:prefLabel>
<skos:altLabel>Motoda HSS</skos:altLabel>
<skos:definition xml:lang="en">Body is 10 cm diameter and 100 cm in length. Tapered nose with two 2 cm openings. Body of cylinder has multiple sections 1.5 cm diameter x 18 cm long to store samples.  Equipped with depth/flowmeter. Collects samples at ~ 8 knots.</skos:definition>
<owl:versionInfo>1</owl:versionInfo>
<dc:date>2011-10-21 14:18:49.0</dc:date>
<skos:note xml:lang="en">accepted</skos:note>
<owl:deprecated>false</owl:deprecated>
<skos:broader rdf:resource="http://vocab.nerc.ac.uk/collection/L05/current/67/"/>
<void:inDataset rdf:resource="http://vocab.nerc.ac.uk/.well-known/void"/>
</skos:Concept>
</skos:member>
<skos:member>
<skos:Concept rdf:about="http://vocab.nerc.ac.uk/collection/L22/current/NETT0063/">
<dc:identifier>SDN:L22::NETT0063</dc:identifier>
<skos:notation>SDN:L22::NETT0063</skos:notation>
<skos:prefLabel xml:lang="en">High-speed tow net - Gauld and Beganal (1951)</skos:prefLabel>
<skos:altLabel>Gauld high-speed tow net</skos:altLabel>
<skos:definition xml:lang="en">A 46 cm diameter mouth opening with 15 cm long calico collar, 94 cm long silk net (10.2 meshes per cm), and 12 cm diameter x 17cm long sleeve with ring sewn in at end. The tail of the net is flipped inward and bridles attached to the ring are attached to the front of the net.  A three-part bridle tows the net at speeds up to 7 knots. Design taken from Sheard [Wiebe and Benfield 2003 Plate 15 A].</skos:definition>
<owl:versionInfo>1</owl:versionInfo>
<dc:date>2011-10-21 14:18:49.0</dc:date>
<skos:note xml:lang="en">accepted</skos:note>
<owl:deprecated>false</owl:deprecated>
<skos:broader rdf:resource="http://vocab.nerc.ac.uk/collection/L05/current/67/"/>
<void:inDataset rdf:resource="http://vocab.nerc.ac.uk/.well-known/void"/>
</skos:Concept>
</skos:member>
<skos:member>
<skos:Concept rdf:about="http://vocab.nerc.ac.uk/collection/L22/current/TOOL0243/">
<dc:identifier>SDN:L22::TOOL0243</dc:identifier>
<skos:notation>SDN:L22::TOOL0243</skos:notation>
<skos:prefLabel xml:lang="en">Hilger Spekker colorimeter</skos:prefLabel>
<skos:altLabel>Spekker colorimeter</skos:altLabel>
<skos:definition xml:lang="en">A photoelectric absorbsiometer developed in 1936 and manufactered by Adam Hilger Ltd, London. A light source with a photocell on each side provides a basic means of operation. The instrument is set up with a solution to be measured in the sample light beam and then balance the EMF of the photocells to zero on a galvanometer. It can be used to measure nutrient concentrations in seawater.</skos:definition>
<owl:versionInfo>2</owl:versionInfo>
<dc:date>2010-11-18 12:39:41.0</dc:date>
<skos:note xml:lang="en">accepted</skos:note>
<owl:deprecated>false</owl:deprecated>
<skos:broader rdf:resource="http://vocab.nerc.ac.uk/collection/L05/current/LAB03/"/>
<void:inDataset rdf:resource="http://vocab.nerc.ac.uk/.well-known/void"/>
</skos:Concept>
</skos:member>
<skos:member>
<skos:Concept rdf:about="http://vocab.nerc.ac.uk/collection/L22/current/TOOL0467/">
<dc:identifier>SDN:L22::TOOL0467</dc:identifier>
<skos:notation>SDN:L22::TOOL0467</skos:notation>
<skos:prefLabel xml:lang="en">Hitachi High-Technologies U-2000 UV-Visible spectrophotometer</skos:prefLabel>
<skos:altLabel>U-2000 spectrophotometer</skos:altLabel>
<skos:definition xml:lang="en">A laboratory instrument that measures the amount of light at discrete pre-determined wavelengths that is transmitted or emitted by a sample. This is a double beam instrument that operates over the spectral range 190-1100 nm with a 2 nm bandpass and an accuracy of 0.4 nm. The instrument uses a concave diffraction grating monochromator and a silicon photodiode detector. This model is no longer in production.</skos:definition>
<owl:versionInfo>1</owl:versionInfo>
<dc:date>2012-02-21 16:06:42.0</dc:date>
<skos:note xml:lang="en">accepted</skos:note>
<owl:deprecated>false</owl:deprecated>
<skos:broader rdf:resource="http://vocab.nerc.ac.uk/collection/L05/current/LAB20/"/>
<void:inDataset rdf:resource="http://vocab.nerc.ac.uk/.well-known/void"/>
</skos:Concept>
</skos:member>
<skos:member>
<skos:Concept rdf:about="http://vocab.nerc.ac.uk/collection/L22/current/TOOL0526/">
<dc:identifier>SDN:L22::TOOL0526</dc:identifier>
<skos:notation>SDN:L22::TOOL0526</skos:notation>
<skos:prefLabel xml:lang="en">Horiba U-22 multiparameter instrument</skos:prefLabel>
<skos:altLabel>Horiba U-22</skos:altLabel>
<skos:definition xml:lang="en">The Horiba U-22 multiparameter sensor is a submersible probe which allows simultaneous measurement of 10 water property parameters to depths of up to 100 metres. The measured parameters are pH, dissolved oxygen, conductivity, salinity, total dissolved solids, seawater specific gravity, temperature, turbidity, depth and oxidation reduction potential.</skos:definition>
<owl:versionInfo>1</owl:versionInfo>
<dc:date>2012-07-31 08:55:11.0</dc:date>
<skos:note xml:lang="en">accepted</skos:note>
<owl:deprecated>false</owl:deprecated>
<skos:broader rdf:resource="http://vocab.nerc.ac.uk/collection/L05/current/355/"/>
<skos:broader rdf:resource="http://vocab.nerc.ac.uk/collection/L05/current/351/"/>
<skos:broader rdf:resource="http://vocab.nerc.ac.uk/collection/L05/current/350/"/>
<skos:broader rdf:resource="http://vocab.nerc.ac.uk/collection/L05/current/356/"/>
<skos:broader rdf:resource="http://vocab.nerc.ac.uk/collection/L05/current/123/"/>
<skos:broader rdf:resource="http://vocab.nerc.ac.uk/collection/L05/current/134/"/>
<void:inDataset rdf:resource="http://vocab.nerc.ac.uk/.well-known/void"/>
</skos:Concept>
</skos:member>
<skos:member>
<skos:Concept rdf:about="http://vocab.nerc.ac.uk/collection/L22/current/NETT0069/">
<dc:identifier>SDN:L22::NETT0069</dc:identifier>
<skos:notation>SDN:L22::NETT0069</skos:notation>
<skos:prefLabel xml:lang="en">Horizontal ichthyoplankton tow-net system - Nester (1987)</skos:prefLabel>
<skos:altLabel>Nester ichthyoplankton system</skos:altLabel>
<skos:definition xml:lang="en">A 50 cm diameter circular net ring is mounted in a 53cm x 53 cm rectangular frame. The net is a cylinder-cone with 0.333 mm nylon mesh.  The tow bridle is attached to a spreader bar to keep the net opening clear of the bridle and depressor attached to bottom of frame.  It has two flowmeters: one inside the net and one outside. Usually towed at 3 knots.  Mainly for catching larval fish.  Similar to the Blackburn and Keith system. It has no opening/closing mechanism.</skos:definition>
<owl:versionInfo>1</owl:versionInfo>
<dc:date>2011-10-21 14:18:49.0</dc:date>
<skos:note xml:lang="en">accepted</skos:note>
<owl:deprecated>false</owl:deprecated>
<skos:broader rdf:resource="http://vocab.nerc.ac.uk/collection/L05/current/388/"/>
<skos:broader rdf:resource="http://vocab.nerc.ac.uk/collection/L05/current/22/"/>
<void:inDataset rdf:resource="http://vocab.nerc.ac.uk/.well-known/void"/>
</skos:Concept>
</skos:member>
<skos:member>
<skos:Concept rdf:about="http://vocab.nerc.ac.uk/collection/L22/current/NETT0129/">
<dc:identifier>SDN:L22::NETT0129</dc:identifier>
<skos:notation>SDN:L22::NETT0129</skos:notation>
<skos:prefLabel xml:lang="en">Horizontal opening-closing net - Bigelow (1913)</skos:prefLabel>
<skos:altLabel>Bigelow opening-closing net</skos:altLabel>
<skos:definition xml:lang="en">A hinged ring to which a net with 75 cm diameter mouth was attached. System sent down with ring closed and opened with a messenger. A second messenger released the ring and a draw-string closed the net off.</skos:definition>
<owl:versionInfo>1</owl:versionInfo>
<dc:date>2011-10-21 14:18:49.0</dc:date>
<skos:note xml:lang="en">accepted</skos:note>
<owl:deprecated>false</owl:deprecated>
<skos:broader rdf:resource="http://vocab.nerc.ac.uk/collection/L05/current/22/"/>
<void:inDataset rdf:resource="http://vocab.nerc.ac.uk/.well-known/void"/>
</skos:Concept>
</skos:member>
<skos:member>
<skos:Concept rdf:about="http://vocab.nerc.ac.uk/collection/L22/current/NETT0130/">
<dc:identifier>SDN:L22::NETT0130</dc:identifier>
<skos:notation>SDN:L22::NETT0130</skos:notation>
<skos:prefLabel xml:lang="en">Horizontal opening-closing plankton net - Slack (1955)</skos:prefLabel>
<skos:altLabel>Slack opening-closing net</skos:altLabel>
<skos:definition xml:lang="en">Has a 14.0 cm diameter mouth opening with framework 25.4 cm long. Has an internal flowmeter.</skos:definition>
<owl:versionInfo>1</owl:versionInfo>
<dc:date>2011-10-21 14:18:49.0</dc:date>
<skos:note xml:lang="en">accepted</skos:note>
<owl:deprecated>false</owl:deprecated>
<skos:broader rdf:resource="http://vocab.nerc.ac.uk/collection/L05/current/388/"/>
<skos:broader rdf:resource="http://vocab.nerc.ac.uk/collection/L05/current/22/"/>
<void:inDataset rdf:resource="http://vocab.nerc.ac.uk/.well-known/void"/>
</skos:Concept>
</skos:member>
<skos:member>
<skos:Concept rdf:about="http://vocab.nerc.ac.uk/collection/L22/current/NETT0153/">
<dc:identifier>SDN:L22::NETT0153</dc:identifier>
<skos:notation>SDN:L22::NETT0153</skos:notation>
<skos:prefLabel xml:lang="en">Horizontal self-closing net - Kofoid (1911, 1911, 1912)</skos:prefLabel>
<skos:altLabel>Kofoid self-closing net</skos:altLabel>
<skos:definition xml:lang="en">Has a 37 cm net diameter. Conical silk bolting cloth net (nos. 12 to 20) about 200 cm long.  Two hinged jaws in the mouth of the net swing forward and downward. Each is activated by a messenger to open then close the net mouth. Used at the end to a cable for horizontal/oblique towing [Wiebe and Benfield 2003 Plate 5D].</skos:definition>
<owl:versionInfo>1</owl:versionInfo>
<dc:date>2011-10-21 14:18:49.0</dc:date>
<skos:note xml:lang="en">accepted</skos:note>
<owl:deprecated>false</owl:deprecated>
<skos:broader rdf:resource="http://vocab.nerc.ac.uk/collection/L05/current/22/"/>
<void:inDataset rdf:resource="http://vocab.nerc.ac.uk/.well-known/void"/>
</skos:Concept>
</skos:member>
<skos:member>
<skos:Concept rdf:about="http://vocab.nerc.ac.uk/collection/L22/current/TOOL0527/">
<dc:identifier>SDN:L22::TOOL0527</dc:identifier>
<skos:notation>SDN:L22::TOOL0527</skos:notation>
<skos:prefLabel xml:lang="en">Howaldtswerke-Deutsche Werft Bathysonde CTD profiler</skos:prefLabel>
<skos:altLabel>HDW Bathysonde</skos:altLabel>
<skos:definition xml:lang="en">A conductivity-temperature-pressure profiler with a pressure rating of either 800dbar or 6000dbar, a pressure precision of +/- 0.25% of total range and a resolution of 1dbar or better. It had temperature precision of +/- 0.01 degC and a resolution of 0.01 degC. The conductivity range was 0 to 80 mmho/cm, with a precision of +/- 1.5 permil of total range and a resolution of 0.01 mmho/cm. The instrument was developed in the 1970s and was used by the then Institute for Marine Science, Kiel.</skos:definition>
<owl:versionInfo>3</owl:versionInfo>
<dc:date>2012-08-16 13:02:49.0</dc:date>
<skos:note xml:lang="en">accepted</skos:note>
<owl:deprecated>false</owl:deprecated>
<skos:broader rdf:resource="http://vocab.nerc.ac.uk/collection/L05/current/130/"/>
<skos:broader rdf:resource="http://vocab.nerc.ac.uk/collection/L05/current/134/"/>
<skos:broader rdf:resource="http://vocab.nerc.ac.uk/collection/L05/current/350/"/>
<void:inDataset rdf:resource="http://vocab.nerc.ac.uk/.well-known/void"/>
</skos:Concept>
</skos:member>
<skos:member>
<skos:Concept rdf:about="http://vocab.nerc.ac.uk/collection/L22/current/TOOL0228/">
<dc:identifier>SDN:L22::TOOL0228</dc:identifier>
<skos:notation>SDN:L22::TOOL0228</skos:notation>
<skos:prefLabel xml:lang="en">Hugrun Seamon Mini temperature recorder</skos:prefLabel>
<skos:altLabel>Hugrun Seamon Mini TR</skos:altLabel>
<skos:definition xml:lang="en">A small underwater temperature sensor and data logger manufactured by Hugrun (subsequently Star-Oddi) and no longer manufactured under that name.</skos:definition>
<owl:versionInfo>1</owl:versionInfo>
<dc:date>2010-05-18 16:10:58.0</dc:date>
<skos:note xml:lang="en">accepted</skos:note>
<owl:deprecated>false</owl:deprecated>
<skos:broader rdf:resource="http://vocab.nerc.ac.uk/collection/L05/current/134/"/>
<void:inDataset rdf:resource="http://vocab.nerc.ac.uk/.well-known/void"/>
</skos:Concept>
</skos:member>
<skos:member>
<skos:Concept rdf:about="http://vocab.nerc.ac.uk/collection/L22/current/TOOL0613/">
<dc:identifier>SDN:L22::TOOL0613</dc:identifier>
<skos:notation>SDN:L22::TOOL0613</skos:notation>
<skos:prefLabel xml:lang="en">Hydrolab DataSonde 3 Water Quality Multiple Probe Logger</skos:prefLabel>
<skos:altLabel>Hydrolab DS3</skos:altLabel>
<skos:definition xml:lang="en">The DS3 multiparameter DataSonde is a multiprobe logger which allows simultaneous measurement of water quality parameters. The measured/calculated parameters are surface elevation, dissolved oxygen (0-20 mg/L) and oxygen saturation, conductivity, salinity (0-70 PSU), temperature (-5 to 50 degC), turbidity, depth (0-100 m), pH and oxidation/reduction potential.</skos:definition>
<owl:versionInfo>1</owl:versionInfo>
<dc:date>2013-04-16 10:43:05.0</dc:date>
<skos:note xml:lang="en">accepted</skos:note>
<owl:deprecated>false</owl:deprecated>
<skos:broader rdf:resource="http://vocab.nerc.ac.uk/collection/L05/current/351/"/>
<skos:broader rdf:resource="http://vocab.nerc.ac.uk/collection/L05/current/355/"/>
<skos:broader rdf:resource="http://vocab.nerc.ac.uk/collection/L05/current/356/"/>
<skos:broader rdf:resource="http://vocab.nerc.ac.uk/collection/L05/current/134/"/>
<skos:broader rdf:resource="http://vocab.nerc.ac.uk/collection/L05/current/350/"/>
<skos:broader rdf:resource="http://vocab.nerc.ac.uk/collection/L05/current/111/"/>
<skos:broader rdf:resource="http://vocab.nerc.ac.uk/collection/L05/current/123/"/>
<void:inDataset rdf:resource="http://vocab.nerc.ac.uk/.well-known/void"/>
</skos:Concept>
</skos:member>
<skos:member>
<skos:Concept rdf:about="http://vocab.nerc.ac.uk/collection/L22/current/TOOL0354/">
<dc:identifier>SDN:L22::TOOL0354</dc:identifier>
<skos:notation>SDN:L22::TOOL0354</skos:notation>
<skos:prefLabel xml:lang="en">Hydrophone</skos:prefLabel>
<skos:altLabel>Hydrophone</skos:altLabel>
<skos:definition xml:lang="en">A generic term for an acoustic intensity sensor (microphone) with an acoustic impedence matched to the density of water to optimise sonic detection under water.</skos:definition>
<owl:versionInfo>1</owl:versionInfo>
<dc:date>2010-11-18 12:37:16.0</dc:date>
<skos:note xml:lang="en">accepted</skos:note>
<owl:deprecated>false</owl:deprecated>
<skos:narrower rdf:resource="http://vocab.nerc.ac.uk/collection/L22/current/TOOL0360/"/>
<skos:related rdf:resource="http://vocab.nerc.ac.uk/collection/L05/current/371/"/>
<skos:related rdf:resource="http://vocab.nerc.ac.uk/collection/L05/current/372/"/>
<skos:related rdf:resource="http://vocab.nerc.ac.uk/collection/L05/current/373/"/>
<skos:related rdf:resource="http://vocab.nerc.ac.uk/collection/L05/current/374/"/>
<skos:related rdf:resource="http://vocab.nerc.ac.uk/collection/L05/current/375/"/>
<skos:related rdf:resource="http://vocab.nerc.ac.uk/collection/L05/current/366/"/>
<skos:related rdf:resource="http://vocab.nerc.ac.uk/collection/L05/current/153/"/>
<skos:related rdf:resource="http://vocab.nerc.ac.uk/collection/L05/current/154/"/>
<skos:related rdf:resource="http://vocab.nerc.ac.uk/collection/L05/current/362/"/>
<skos:related rdf:resource="http://vocab.nerc.ac.uk/collection/L05/current/365/"/>
<skos:related rdf:resource="http://vocab.nerc.ac.uk/collection/L05/current/364/"/>
<skos:related rdf:resource="http://vocab.nerc.ac.uk/collection/L05/current/363/"/>
<owl:sameAs rdf:resource="http://vocab.nerc.ac.uk/collection/L05/current/369/"/>
<void:inDataset rdf:resource="http://vocab.nerc.ac.uk/.well-known/void"/>
</skos:Concept>
</skos:member>
<skos:member>
<skos:Concept rdf:about="http://vocab.nerc.ac.uk/collection/L22/current/TOOL0282/">
<dc:identifier>SDN:L22::TOOL0282</dc:identifier>
<skos:notation>SDN:L22::TOOL0282</skos:notation>
<skos:prefLabel xml:lang="en">Hygrometer</skos:prefLabel>
<skos:altLabel>Hygrometer</skos:altLabel>
<skos:definition xml:lang="en">A generic term for a device that measures atmospheric humidity. The term is for use where details of the make, model number and measurement principle are not known.</skos:definition>
<owl:versionInfo>1</owl:versionInfo>
<dc:date>2010-05-18 16:10:58.0</dc:date>
<skos:note xml:lang="en">accepted</skos:note>
<owl:deprecated>false</owl:deprecated>
<skos:broader rdf:resource="http://vocab.nerc.ac.uk/collection/L05/current/102/"/>
<void:inDataset rdf:resource="http://vocab.nerc.ac.uk/.well-known/void"/>
</skos:Concept>
</skos:member>
<skos:member>
<skos:Concept rdf:about="http://vocab.nerc.ac.uk/collection/L22/current/NETT0070/">
<dc:identifier>SDN:L22::NETT0070</dc:identifier>
<skos:notation>SDN:L22::NETT0070</skos:notation>
<skos:prefLabel xml:lang="en">ICITA plankton net - Jossi (1966)</skos:prefLabel>
<skos:altLabel>ICITA net</skos:altLabel>
<skos:definition xml:lang="en">A 100 cm diameter mouth opening with a conical net with a short (18cm) section of canvas and a 330 cm length section of 0.281 mm Nitex nylon mesh. Used with a flowmeter.  The standard net used during the International Cooperative Investigations of the Tropical Atlantic [Wiebe and Benfield 2003 Plate 2 B].</skos:definition>
<owl:versionInfo>1</owl:versionInfo>
<dc:date>2011-10-21 14:18:49.0</dc:date>
<skos:note xml:lang="en">accepted</skos:note>
<owl:deprecated>false</owl:deprecated>
<skos:broader rdf:resource="http://vocab.nerc.ac.uk/collection/L05/current/22/"/>
<skos:broader rdf:resource="http://vocab.nerc.ac.uk/collection/L05/current/388/"/>
<void:inDataset rdf:resource="http://vocab.nerc.ac.uk/.well-known/void"/>
</skos:Concept>
</skos:member>
<skos:member>
<skos:Concept rdf:about="http://vocab.nerc.ac.uk/collection/L22/current/TOOL0562/">
<dc:identifier>SDN:L22::TOOL0562</dc:identifier>
<skos:notation>SDN:L22::TOOL0562</skos:notation>
<skos:prefLabel xml:lang="en">IFM Kiel clean pumped sea water supply</skos:prefLabel>
<skos:altLabel>IFM clean pumped sea water supply</skos:altLabel>
<skos:definition xml:lang="en">A system designed for continuous, underway, clean sampling of near-surface waters. A hollow stainless steel shaft holding a high density polyethylene (HDPE) tube is submerged beneath a vessel through a hole in the hull. The inlet head is located 1.7 m below the keel and features a sieve-like Teflon cap. Water is pumped from the inlet through a serial ball-valve panel from which it can be directed to different sampling facilities. Flow is maintained by chemically inert double membrane pump driven by compressed air. HDPE tubing is used throughout the system and the valves are composed of polypropylene and Teflon, thereby ensuring that the sampled water remains clean and suitable for trace metal analyses. The system was developed by what was then the Institut fur Meereskunde at Kiel University.</skos:definition>
<owl:versionInfo>1</owl:versionInfo>
<dc:date>2012-10-15 14:57:16.0</dc:date>
<skos:note xml:lang="en">accepted</skos:note>
<owl:deprecated>false</owl:deprecated>
<skos:broader rdf:resource="http://vocab.nerc.ac.uk/collection/L05/current/31/"/>
<void:inDataset rdf:resource="http://vocab.nerc.ac.uk/.well-known/void"/>
</skos:Concept>
</skos:member>
<skos:member>
<skos:Concept rdf:about="http://vocab.nerc.ac.uk/collection/L22/current/TOOL0304/">
<dc:identifier>SDN:L22::TOOL0304</dc:identifier>
<skos:notation>SDN:L22::TOOL0304</skos:notation>
<skos:prefLabel xml:lang="en">IXSEA Photonic Inertial Navigation System</skos:prefLabel>
<skos:altLabel>IXSEA PHINS</skos:altLabel>
<skos:definition xml:lang="en">PHINS, or PHotonic Inertial Navigation System (INS) that outputs position, heading, pitch, roll, heave, depth and velocity. The PHINS uses a high accuracy inertial measurement unit and produces positional data with an accuracy ranging from metres to cm, depending on the specific instrumentation setup. INS drift performance is known to be inadequate without a velocity input from an ADCP.</skos:definition>
<owl:versionInfo>1</owl:versionInfo>
<dc:date>2010-05-18 16:10:58.0</dc:date>
<skos:note xml:lang="en">accepted</skos:note>
<owl:deprecated>false</owl:deprecated>
<skos:broader rdf:resource="http://vocab.nerc.ac.uk/collection/L05/current/POS19/"/>
<void:inDataset rdf:resource="http://vocab.nerc.ac.uk/.well-known/void"/>
</skos:Concept>
</skos:member>
<skos:member>
<skos:Concept rdf:about="http://vocab.nerc.ac.uk/collection/L22/current/TOOL0213/">
<dc:identifier>SDN:L22::TOOL0213</dc:identifier>
<skos:notation>SDN:L22::TOOL0213</skos:notation>
<skos:prefLabel xml:lang="en">Idronaut Ocean Seven 320 CTD</skos:prefLabel>
<skos:altLabel>Idronaut Ocean Seven 320 CTD</skos:altLabel>
<skos:definition xml:lang="en">A fast response, multi-parameter conductivity, temperature and depth probe. It can be fitted with an additional (redundant) pair of conductivity and temperature sensors allowing the precision and quality of the data to be checked.</skos:definition>
<owl:versionInfo>1</owl:versionInfo>
<dc:date>2010-05-18 16:10:58.0</dc:date>
<skos:note xml:lang="en">accepted</skos:note>
<owl:deprecated>false</owl:deprecated>
<skos:broader rdf:resource="http://vocab.nerc.ac.uk/collection/L05/current/130/"/>
<skos:broader rdf:resource="http://vocab.nerc.ac.uk/collection/L05/current/350/"/>
<skos:broader rdf:resource="http://vocab.nerc.ac.uk/collection/L05/current/134/"/>
<void:inDataset rdf:resource="http://vocab.nerc.ac.uk/.well-known/void"/>
</skos:Concept>
</skos:member>
<skos:member>
<skos:Concept rdf:about="http://vocab.nerc.ac.uk/collection/L22/current/NETT0075/">
<dc:identifier>SDN:L22::NETT0075</dc:identifier>
<skos:notation>SDN:L22::NETT0075</skos:notation>
<skos:prefLabel xml:lang="en">Indian Ocean standard net - Currie (1963)</skos:prefLabel>
<skos:altLabel>IOS net</skos:altLabel>
<skos:definition xml:lang="en">Net has a 113 cm diameter mouth with 3 cylinder sections 70 cm (12.5 mm mesh), 30 cm (sail cloth, and 100 cm (0.330 mm nylon mesh) and a conical section 300 cm (0.333 mm mesh). No closing mechanism is used in standard haul. Flowmeter use is recommended.  It was based on the Discovery N 100 net.  Used during the UK NIO Indian Ocean Expedition of the 1960s [Wiebe and Benfield 2003 Plate 1 G].</skos:definition>
<owl:versionInfo>1</owl:versionInfo>
<dc:date>2011-10-21 14:18:49.0</dc:date>
<skos:note xml:lang="en">accepted</skos:note>
<owl:deprecated>false</owl:deprecated>
<skos:broader rdf:resource="http://vocab.nerc.ac.uk/collection/L05/current/22/"/>
<void:inDataset rdf:resource="http://vocab.nerc.ac.uk/.well-known/void"/>
</skos:Concept>
</skos:member>
<skos:member>
<skos:Concept rdf:about="http://vocab.nerc.ac.uk/collection/L22/current/TOOL0359/">
<dc:identifier>SDN:L22::TOOL0359</dc:identifier>
<skos:notation>SDN:L22::TOOL0359</skos:notation>
<skos:prefLabel xml:lang="en">Institut Francais du Petrole Flexotir seismic source</skos:prefLabel>
<skos:altLabel>IFP Flexotir source</skos:altLabel>
<skos:definition xml:lang="en">A seismic source whereby small charges (50-150g) are propelled through a rubber hose by water under pressure into an empty, perforated sphere where they are detonated. The holes in the sphere allow the water repelled by the explosion to flow in and out, thus dissipating some of the energy in the bubble effect. Flexotir was commonly used as an energy source for seafloor seismic surveys during the 1970s.</skos:definition>
<owl:versionInfo>1</owl:versionInfo>
<dc:date>2010-11-24 09:31:30.0</dc:date>
<skos:note xml:lang="en">accepted</skos:note>
<owl:deprecated>false</owl:deprecated>
<skos:broader rdf:resource="http://vocab.nerc.ac.uk/collection/L05/current/FLXT/"/>
<void:inDataset rdf:resource="http://vocab.nerc.ac.uk/.well-known/void"/>
</skos:Concept>
</skos:member>
<skos:member>
<skos:Concept rdf:about="http://vocab.nerc.ac.uk/collection/L22/current/TOOL0360/">
<dc:identifier>SDN:L22::TOOL0360</dc:identifier>
<skos:notation>SDN:L22::TOOL0360</skos:notation>
<skos:prefLabel xml:lang="en">Institut Francais du Petrole Geomecanique hydrophone array</skos:prefLabel>
<skos:altLabel>IFP Geomecanique hydrophones</skos:altLabel>
<skos:definition xml:lang="en">A collection of underwater microphones mounted in cable designed to be towed behind a ship.</skos:definition>
<owl:versionInfo>1</owl:versionInfo>
<dc:date>2010-11-24 09:31:30.0</dc:date>
<skos:note xml:lang="en">accepted</skos:note>
<owl:deprecated>false</owl:deprecated>
<skos:related rdf:resource="http://vocab.nerc.ac.uk/collection/L05/current/364/"/>
<skos:related rdf:resource="http://vocab.nerc.ac.uk/collection/L05/current/374/"/>
<skos:related rdf:resource="http://vocab.nerc.ac.uk/collection/L05/current/373/"/>
<skos:related rdf:resource="http://vocab.nerc.ac.uk/collection/L05/current/153/"/>
<skos:related rdf:resource="http://vocab.nerc.ac.uk/collection/L05/current/154/"/>
<skos:related rdf:resource="http://vocab.nerc.ac.uk/collection/L05/current/362/"/>
<skos:related rdf:resource="http://vocab.nerc.ac.uk/collection/L05/current/363/"/>
<skos:related rdf:resource="http://vocab.nerc.ac.uk/collection/L05/current/375/"/>
<skos:related rdf:resource="http://vocab.nerc.ac.uk/collection/L05/current/365/"/>
<skos:related rdf:resource="http://vocab.nerc.ac.uk/collection/L05/current/366/"/>
<skos:related rdf:resource="http://vocab.nerc.ac.uk/collection/L05/current/371/"/>
<skos:related rdf:resource="http://vocab.nerc.ac.uk/collection/L05/current/372/"/>
<skos:broader rdf:resource="http://vocab.nerc.ac.uk/collection/L22/current/TOOL0354/"/>
<skos:broader rdf:resource="http://vocab.nerc.ac.uk/collection/L05/current/369/"/>
<void:inDataset rdf:resource="http://vocab.nerc.ac.uk/.well-known/void"/>
</skos:Concept>
</skos:member>
<skos:member>
<skos:Concept rdf:about="http://vocab.nerc.ac.uk/collection/L22/current/TOOL0594/">
<dc:identifier>SDN:L22::TOOL0594</dc:identifier>
<skos:notation>SDN:L22::TOOL0594</skos:notation>
<skos:prefLabel xml:lang="en">Institute of Oceanographic Sciences MkII bottom pressure recorder</skos:prefLabel>
<skos:altLabel>IOS MkII BPR</skos:altLabel>
<skos:definition xml:lang="en">The instrument comprised a strain gauge, vibrating wire or quartz pressure sensor and a temperature sensor in a self-contained housing connected to release and senor electronics, a data logger and battery pack located in an aluminium sphere. The logger was able to sample at intervals between 1.875 and 60 minutes with the inputs sampled continuously to give data values integrated over virtually the whole sampling interval.</skos:definition>
<owl:versionInfo>1</owl:versionInfo>
<dc:date>2013-01-23 09:58:33.0</dc:date>
<skos:note xml:lang="en">accepted</skos:note>
<owl:deprecated>false</owl:deprecated>
<skos:broader rdf:resource="http://vocab.nerc.ac.uk/collection/L05/current/111/"/>
<void:inDataset rdf:resource="http://vocab.nerc.ac.uk/.well-known/void"/>
</skos:Concept>
</skos:member>
<skos:member>
<skos:Concept rdf:about="http://vocab.nerc.ac.uk/collection/L22/current/TOOL0227/">
<dc:identifier>SDN:L22::TOOL0227</dc:identifier>
<skos:notation>SDN:L22::TOOL0227</skos:notation>
<skos:prefLabel xml:lang="en">Institute of Oceanographic Sciences MkIII bottom pressure recorder</skos:prefLabel>
<skos:altLabel>IOS MkIII BPR</skos:altLabel>
<skos:definition xml:lang="en">A deep water (300-5000m) seafloor pressure gauge designed and built by IOS Bidston (now Proudman Oceanographic Laboratory) with two pressure transducers and PRT sea temperature sensors coupled to a 12-channel commercial data logger in a spherical pressure housing.</skos:definition>
<owl:versionInfo>1</owl:versionInfo>
<dc:date>2010-05-18 16:10:58.0</dc:date>
<skos:note xml:lang="en">accepted</skos:note>
<owl:deprecated>false</owl:deprecated>
<skos:broader rdf:resource="http://vocab.nerc.ac.uk/collection/L05/current/111/"/>
<void:inDataset rdf:resource="http://vocab.nerc.ac.uk/.well-known/void"/>
</skos:Concept>
</skos:member>
<skos:member>
<skos:Concept rdf:about="http://vocab.nerc.ac.uk/collection/L22/current/TOOL0226/">
<dc:identifier>SDN:L22::TOOL0226</dc:identifier>
<skos:notation>SDN:L22::TOOL0226</skos:notation>
<skos:prefLabel xml:lang="en">Institute of Oceanographic Sciences MkIV bottom pressure recorder</skos:prefLabel>
<skos:altLabel>IOS MkIV BPR</skos:altLabel>
<skos:definition xml:lang="en">A deep water (300-5000m) seafloor pressure gauge designed and built by IOS Bidston (now Proudman Oceanographic Laboratory) with an internal casette tape data logger recording Bell and Howell strain gauges and/or Digiquartz pressure sensors.</skos:definition>
<owl:versionInfo>1</owl:versionInfo>
<dc:date>2010-05-18 16:10:58.0</dc:date>
<skos:note xml:lang="en">accepted</skos:note>
<owl:deprecated>false</owl:deprecated>
<skos:broader rdf:resource="http://vocab.nerc.ac.uk/collection/L05/current/111/"/>
<void:inDataset rdf:resource="http://vocab.nerc.ac.uk/.well-known/void"/>
</skos:Concept>
</skos:member>
<skos:member>
<skos:Concept rdf:about="http://vocab.nerc.ac.uk/collection/L22/current/TOOL0080/">
<dc:identifier>SDN:L22::TOOL0080</dc:identifier>
<skos:notation>SDN:L22::TOOL0080</skos:notation>
<skos:prefLabel xml:lang="en">Institute of Oceanographic Sciences psychrometer</skos:prefLabel>
<skos:altLabel>IOS psychrometer</skos:altLabel>
<skos:definition xml:lang="en">A psychrometer designed by Institute of Oceanographic Sciences (now National Oceanography Centre) to measure wet and dry bulb atmospheric temperature. The instrument consisted of two similar thermometers that were mounted side by side. The dry bulb has its bulb exposed to the air; the wet bulb was wrapped in an absorbent material (muslin), which was immersed in water and served as a wick.</skos:definition>
<owl:versionInfo>1</owl:versionInfo>
<dc:date>2009-11-30 11:56:35.0</dc:date>
<skos:note xml:lang="en">accepted</skos:note>
<owl:deprecated>false</owl:deprecated>
<skos:broader rdf:resource="http://vocab.nerc.ac.uk/collection/L05/current/102/"/>
<void:inDataset rdf:resource="http://vocab.nerc.ac.uk/.well-known/void"/>
</skos:Concept>
</skos:member>
<skos:member>
<skos:Concept rdf:about="http://vocab.nerc.ac.uk/collection/L22/current/TOOL0612/">
<dc:identifier>SDN:L22::TOOL0612</dc:identifier>
<skos:notation>SDN:L22::TOOL0612</skos:notation>
<skos:prefLabel xml:lang="en">Institute of Oceanographic Sciences shipborne wave recorder</skos:prefLabel>
<skos:altLabel>IOS SBWR</skos:altLabel>
<skos:definition xml:lang="en">A vessel-mounted wave recorder comprising a pair of heave transducers (accelerometers), a pair of pressure transducers, a signal processing unit and a data recorder. One heave transducer (measures long-period waves) and one pressure transducer (measures short-period waves) are mounted together on each side of the vessel close to the centre of pitch and 1-3m below the water-line to reduce the influence of pitch and roll. Waves of up to 30m height and 25 seconds period can be measured; the lower detectable limit depends on the installation depth of the pressure units. More information may be found in http://www.bodc.ac.uk/data/documents/nodb/45603/.</skos:definition>
<owl:versionInfo>1</owl:versionInfo>
<dc:date>2013-04-11 16:07:16.0</dc:date>
<skos:note xml:lang="en">accepted</skos:note>
<owl:deprecated>false</owl:deprecated>
<skos:broader rdf:resource="http://vocab.nerc.ac.uk/collection/L05/current/110/"/>
<void:inDataset rdf:resource="http://vocab.nerc.ac.uk/.well-known/void"/>
</skos:Concept>
</skos:member>
<skos:member>
<skos:Concept rdf:about="http://vocab.nerc.ac.uk/collection/L22/current/NETT0074/">
<dc:identifier>SDN:L22::NETT0074</dc:identifier>
<skos:notation>SDN:L22::NETT0074</skos:notation>
<skos:prefLabel xml:lang="en">International Council for the Exploration of the Seas standard net - Ostenfeld and Jespersen  (1924)</skos:prefLabel>
<skos:altLabel>ICES standard net</skos:altLabel>
<skos:definition xml:lang="en">Net has 50 cm diameter mouth with 60 cm cylindrical portion of 1 cm mesh,  200 cm conical section of silk (No. 25 or No 3).  This net is used for both vertical and horizontal closing tows (based on the Nansen net). A unique way to avoid ship motion described using two davits and a counter balancing weight [Wiebe and Benfield 2003 Plate 1 D].</skos:definition>
<owl:versionInfo>1</owl:versionInfo>
<dc:date>2011-10-21 14:18:49.0</dc:date>
<skos:note xml:lang="en">accepted</skos:note>
<owl:deprecated>false</owl:deprecated>
<skos:broader rdf:resource="http://vocab.nerc.ac.uk/collection/L05/current/22/"/>
<void:inDataset rdf:resource="http://vocab.nerc.ac.uk/.well-known/void"/>
</skos:Concept>
</skos:member>
<skos:member>
<skos:Concept rdf:about="http://vocab.nerc.ac.uk/collection/L22/current/TOOL0154/">
<dc:identifier>SDN:L22::TOOL0154</dc:identifier>
<skos:notation>SDN:L22::TOOL0154</skos:notation>
<skos:prefLabel xml:lang="en">Interocean S4 current meter</skos:prefLabel>
<skos:altLabel>S4 CM</skos:altLabel>
<skos:definition xml:lang="en">Basic elecromagnetic current meter with two pairs of internal electrodes and a flux-gate compass with integral data logger</skos:definition>
<owl:versionInfo>1</owl:versionInfo>
<dc:date>2010-05-18 16:10:58.0</dc:date>
<skos:note xml:lang="en">accepted</skos:note>
<owl:deprecated>false</owl:deprecated>
<skos:broader rdf:resource="http://vocab.nerc.ac.uk/collection/L05/current/114/"/>
<void:inDataset rdf:resource="http://vocab.nerc.ac.uk/.well-known/void"/>
</skos:Concept>
</skos:member>
<skos:member>
<skos:Concept rdf:about="http://vocab.nerc.ac.uk/collection/L22/current/TOOL0156/">
<dc:identifier>SDN:L22::TOOL0156</dc:identifier>
<skos:notation>SDN:L22::TOOL0156</skos:notation>
<skos:prefLabel xml:lang="en">Interocean S4A current meter</skos:prefLabel>
<skos:altLabel>S4A CM</skos:altLabel>
<skos:definition xml:lang="en">Advanced elecromagnetic current meter with two pairs of internal electrodes and a flux-gate compass with high capacity integral data logger. Includes adaptive current sampling as standard.</skos:definition>
<owl:versionInfo>1</owl:versionInfo>
<dc:date>2010-05-18 16:10:58.0</dc:date>
<skos:note xml:lang="en">accepted</skos:note>
<owl:deprecated>false</owl:deprecated>
<skos:broader rdf:resource="http://vocab.nerc.ac.uk/collection/L05/current/114/"/>
<void:inDataset rdf:resource="http://vocab.nerc.ac.uk/.well-known/void"/>
</skos:Concept>
</skos:member>
<skos:member>
<skos:Concept rdf:about="http://vocab.nerc.ac.uk/collection/L22/current/TOOL0153/">
<dc:identifier>SDN:L22::TOOL0153</dc:identifier>
<skos:notation>SDN:L22::TOOL0153</skos:notation>
<skos:prefLabel xml:lang="en">Interocean S4AD current meter</skos:prefLabel>
<skos:altLabel>S4AD CM</skos:altLabel>
<skos:definition xml:lang="en">A current meter is designed to directly measure the true magnitude and direction current motion in any water environment using two pairs of titanium electrodes located symmetrically on the equator of the sensor. An internal flux-gate compass provides heading information, used to reference current direction to magnetic North or, for fixed installations, the instrument may be operated in an X-Y orthogonal mode whereby the current vector can be referenced to a landform or structure. It can be deployed upto depths of 6000m. Further information may be found on the BODC document server at URL http://www.bodc.ac.uk/data/documents/nodb/40555/. The "A" designation indicates advanced current measurement with adaptive sampling as standard. The "D" indicates a pressure-hardened casing.</skos:definition>
<owl:versionInfo>1</owl:versionInfo>
<dc:date>2010-05-18 16:10:58.0</dc:date>
<skos:note xml:lang="en">accepted</skos:note>
<owl:deprecated>false</owl:deprecated>
<skos:broader rdf:resource="http://vocab.nerc.ac.uk/collection/L05/current/114/"/>
<void:inDataset rdf:resource="http://vocab.nerc.ac.uk/.well-known/void"/>
</skos:Concept>
</skos:member>
<skos:member>
<skos:Concept rdf:about="http://vocab.nerc.ac.uk/collection/L22/current/TOOL0157/">
<dc:identifier>SDN:L22::TOOL0157</dc:identifier>
<skos:notation>SDN:L22::TOOL0157</skos:notation>
<skos:prefLabel xml:lang="en">Interocean S4DW current meter directional wave monitor</skos:prefLabel>
<skos:altLabel>S4DW CM/wave</skos:altLabel>
<skos:definition xml:lang="en">Instrument combines electromagnetic current sensors and a high precision pressure sensor to measure wave orbital current components,directional wave spectra and tides. Incorporates programmable burst mode sampling and a very high capacity data logger.</skos:definition>
<owl:versionInfo>1</owl:versionInfo>
<dc:date>2010-05-18 16:10:58.0</dc:date>
<skos:note xml:lang="en">accepted</skos:note>
<owl:deprecated>false</owl:deprecated>
<skos:broader rdf:resource="http://vocab.nerc.ac.uk/collection/L05/current/110/"/>
<void:inDataset rdf:resource="http://vocab.nerc.ac.uk/.well-known/void"/>
</skos:Concept>
</skos:member>
<skos:member>
<skos:Concept rdf:about="http://vocab.nerc.ac.uk/collection/L22/current/TOOL0155/">
<dc:identifier>SDN:L22::TOOL0155</dc:identifier>
<skos:notation>SDN:L22::TOOL0155</skos:notation>
<skos:prefLabel xml:lang="en">Interocean S4R current meter</skos:prefLabel>
<skos:altLabel>S4R CM</skos:altLabel>
<skos:definition xml:lang="en">Basic elecromagnetic current meter with two pairs of internal electrodes and a flux-gate compass with no integral data logger. Designed for real-time monitoring applications.</skos:definition>
<owl:versionInfo>1</owl:versionInfo>
<dc:date>2010-05-18 16:10:58.0</dc:date>
<skos:note xml:lang="en">accepted</skos:note>
<owl:deprecated>false</owl:deprecated>
<skos:broader rdf:resource="http://vocab.nerc.ac.uk/collection/L05/current/114/"/>
<void:inDataset rdf:resource="http://vocab.nerc.ac.uk/.well-known/void"/>
</skos:Concept>
</skos:member>
<skos:member>
<skos:Concept rdf:about="http://vocab.nerc.ac.uk/collection/L22/current/NETT0076/">
<dc:identifier>SDN:L22::NETT0076</dc:identifier>
<skos:notation>SDN:L22::NETT0076</skos:notation>
<skos:prefLabel xml:lang="en">Isaacs high-speed sampler - Ahlstrom (1958)</skos:prefLabel>
<skos:altLabel>Isaacs HSS</skos:altLabel>
<skos:definition xml:lang="en">Construction comprises a 2.5 cm mouth opening expanding to a diameter of 7.6 cm; overall length of 130 cm. The plankton filter is a cylinder of Monel metal mesh (23 mesh per cm) ~5.2 cm in diameter and 36 cm long.  System equipped with a flowmeter and depth sensor (from bathythermograph) and a recording unit utilizing clear 35 mm acetate film.  Can be towed up 10 knots. Can be put anywhere on cable and multiple units can be towed simultaneously [Wiebe and Benfield 2003 Plate 15 B]</skos:definition>
<owl:versionInfo>1</owl:versionInfo>
<dc:date>2011-10-21 14:18:49.0</dc:date>
<skos:note xml:lang="en">accepted</skos:note>
<owl:deprecated>false</owl:deprecated>
<skos:broader rdf:resource="http://vocab.nerc.ac.uk/collection/L05/current/388/"/>
<skos:broader rdf:resource="http://vocab.nerc.ac.uk/collection/L05/current/67/"/>
<void:inDataset rdf:resource="http://vocab.nerc.ac.uk/.well-known/void"/>
</skos:Concept>
</skos:member>
<skos:member>
<skos:Concept rdf:about="http://vocab.nerc.ac.uk/collection/L22/current/NETT0071/">
<dc:identifier>SDN:L22::NETT0071</dc:identifier>
<skos:notation>SDN:L22::NETT0071</skos:notation>
<skos:prefLabel xml:lang="en">Isaacs-Kidd Midwater Trawl  - Isaacs and Kidd (1953)</skos:prefLabel>
<skos:altLabel>IKMT</skos:altLabel>
<skos:definition xml:lang="en">A trawl with a pentagonal mouth opening and a dihedral depressor vane as part of the mouth opening. The original IKMTs were 10 foot (304 cm), and 15 foot (457 cm) at the mouth. The 10 foot IKMT net was 31 feet (9.45 m) in length [Wiebe and Benfield 2003 Plate 3 D].</skos:definition>
<owl:versionInfo>1</owl:versionInfo>
<dc:date>2011-10-21 14:18:49.0</dc:date>
<skos:note xml:lang="en">accepted</skos:note>
<owl:deprecated>false</owl:deprecated>
<skos:broader rdf:resource="http://vocab.nerc.ac.uk/collection/L05/current/23/"/>
<void:inDataset rdf:resource="http://vocab.nerc.ac.uk/.well-known/void"/>
</skos:Concept>
</skos:member>
<skos:member>
<skos:Concept rdf:about="http://vocab.nerc.ac.uk/collection/L22/current/NETT0078/">
<dc:identifier>SDN:L22::NETT0078</dc:identifier>
<skos:notation>SDN:L22::NETT0078</skos:notation>
<skos:prefLabel xml:lang="en">Juday net - Juday (1916)</skos:prefLabel>
<skos:altLabel>Juday net</skos:altLabel>
<skos:definition xml:lang="en">Net has a 25 cm diameter mouth opening with 33 cm long canvas cone expanding to 30 cm diameter, followed by a conical net 70 cm long made of No 20 silk bolting cloth [Wiebe and Benfield 2003 Plate 1 C]. A closing net with simple messenger release is also described: this has a 12 cm diameter mouth opening with 40 cm long canvas cone expanding to 17 cm, followed by a 47 cm long conical net with the same mesh.</skos:definition>
<owl:versionInfo>1</owl:versionInfo>
<dc:date>2011-10-21 14:18:49.0</dc:date>
<skos:note xml:lang="en">accepted</skos:note>
<owl:deprecated>false</owl:deprecated>
<skos:broader rdf:resource="http://vocab.nerc.ac.uk/collection/L05/current/22/"/>
<void:inDataset rdf:resource="http://vocab.nerc.ac.uk/.well-known/void"/>
</skos:Concept>
</skos:member>
<skos:member>
<skos:Concept rdf:about="http://vocab.nerc.ac.uk/collection/L22/current/TOOL0082/">
<dc:identifier>SDN:L22::TOOL0082</dc:identifier>
<skos:notation>SDN:L22::TOOL0082</skos:notation>
<skos:prefLabel xml:lang="en">Kipp and Zonen CM11 pyranometer</skos:prefLabel>
<skos:altLabel>K&amp;Z CM11 pyranometer</skos:altLabel>
<skos:definition xml:lang="en">A pyranometer that measures solar irradiance with a spectral response from 310-2800 nm. It is housed in a weatherproof titanium canister that has been painted with a very flat black paint that absorbs radiation. A small glass dome at the top of the instrument is allows light to enter the sensor. Light levels are detected as temperature changes creating voltages in fine wire coil detectors.</skos:definition>
<owl:versionInfo>2</owl:versionInfo>
<dc:date>2011-08-01 09:23:53.0</dc:date>
<skos:note xml:lang="en">accepted</skos:note>
<owl:deprecated>false</owl:deprecated>
<skos:broader rdf:resource="http://vocab.nerc.ac.uk/collection/L05/current/122/"/>
<void:inDataset rdf:resource="http://vocab.nerc.ac.uk/.well-known/void"/>
</skos:Concept>
</skos:member>
<skos:member>
<skos:Concept rdf:about="http://vocab.nerc.ac.uk/collection/L22/current/TOOL0410/">
<dc:identifier>SDN:L22::TOOL0410</dc:identifier>
<skos:notation>SDN:L22::TOOL0410</skos:notation>
<skos:prefLabel xml:lang="en">Kipp and Zonen CM6B pyranometer</skos:prefLabel>
<skos:altLabel>K&amp;Z CM6B pyranometer</skos:altLabel>
<skos:definition xml:lang="en">A pyranometer that measures solar irradiance with a spectral range of 305-2800 nm. The robust sensor requires no power and provides all weather performance. It has a response time of 18 seconds, a maximum irradiance of 2000 W/m^2 and an expected daily accuracy of +/- 5%.</skos:definition>
<owl:versionInfo>1</owl:versionInfo>
<dc:date>2011-08-01 09:25:01.0</dc:date>
<skos:note xml:lang="en">accepted</skos:note>
<owl:deprecated>false</owl:deprecated>
<skos:related rdf:resource="http://vocab.nerc.ac.uk/collection/P01/current/CSLRZZ01/"/>
<skos:broader rdf:resource="http://vocab.nerc.ac.uk/collection/L05/current/122/"/>
<void:inDataset rdf:resource="http://vocab.nerc.ac.uk/.well-known/void"/>
</skos:Concept>
</skos:member>
<skos:member>
<skos:Concept rdf:about="http://vocab.nerc.ac.uk/collection/L22/current/TOOL0395/">
<dc:identifier>SDN:L22::TOOL0395</dc:identifier>
<skos:notation>SDN:L22::TOOL0395</skos:notation>
<skos:prefLabel xml:lang="en">Kipp and Zonen PAR LITE radiometer</skos:prefLabel>
<skos:altLabel>K&amp;Z PAR LITE radiometer</skos:altLabel>
<skos:definition xml:lang="en">A non-submersible PAR sensor with a spectral range of 400-700 nm. Its sensitivity is proportional to the cosine of the angle of incidence of the incoming radiation. It can measure irradiance over the range 0-10,000 umol/m^2/sec and can operate at temperatures between -30 and 70 degC.</skos:definition>
<owl:versionInfo>1</owl:versionInfo>
<dc:date>2011-04-14 09:29:16.0</dc:date>
<skos:note xml:lang="en">accepted</skos:note>
<owl:deprecated>false</owl:deprecated>
<skos:broader rdf:resource="http://vocab.nerc.ac.uk/collection/L05/current/122/"/>
<void:inDataset rdf:resource="http://vocab.nerc.ac.uk/.well-known/void"/>
</skos:Concept>
</skos:member>
<skos:member>
<skos:Concept rdf:about="http://vocab.nerc.ac.uk/collection/L22/current/TOOL0530/">
<dc:identifier>SDN:L22::TOOL0530</dc:identifier>
<skos:notation>SDN:L22::TOOL0530</skos:notation>
<skos:prefLabel xml:lang="en">Kipp and Zonen PSQ1 PAR Quantum Sensor</skos:prefLabel>
<skos:altLabel>Kipp and Zonen PSQ1</skos:altLabel>
<skos:definition xml:lang="en">A non-submersible PAR sensor incorporating a diffuser with an excellent directional (cosine) response and a silicon photodiode detector. It can be used in field research or permanent applications. It has a spectral range of 400 to 700 nm and a sensitivity of 4 to 10 mV/umol/m^2/s.</skos:definition>
<owl:versionInfo>1</owl:versionInfo>
<dc:date>2012-08-16 11:26:51.0</dc:date>
<skos:note xml:lang="en">accepted</skos:note>
<owl:deprecated>false</owl:deprecated>
<skos:broader rdf:resource="http://vocab.nerc.ac.uk/collection/L05/current/122/"/>
<void:inDataset rdf:resource="http://vocab.nerc.ac.uk/.well-known/void"/>
</skos:Concept>
</skos:member>
<skos:member>
<skos:Concept rdf:about="http://vocab.nerc.ac.uk/collection/L22/current/TOOL0396/">
<dc:identifier>SDN:L22::TOOL0396</dc:identifier>
<skos:notation>SDN:L22::TOOL0396</skos:notation>
<skos:prefLabel xml:lang="en">Kipp and Zonen SP LITE pyranometer</skos:prefLabel>
<skos:altLabel>K&amp;Z SP LITE pyranometer</skos:altLabel>
<skos:definition xml:lang="en">A silicon pyranometer with a spectral range of 400-1100 nm. Its sensitivity is proportional to the cosine of the angle of incidence of the incoming radiation. It can measure irradiance over the range 0-2,000 W/m^2 and can operate at temperatures between -30 and 70 degC.</skos:definition>
<owl:versionInfo>1</owl:versionInfo>
<dc:date>2011-04-14 09:29:16.0</dc:date>
<skos:note xml:lang="en">accepted</skos:note>
<owl:deprecated>false</owl:deprecated>
<skos:broader rdf:resource="http://vocab.nerc.ac.uk/collection/L05/current/122/"/>
<void:inDataset rdf:resource="http://vocab.nerc.ac.uk/.well-known/void"/>
</skos:Concept>
</skos:member>
<skos:member>
<skos:Concept rdf:about="http://vocab.nerc.ac.uk/collection/L22/current/TOOL0529/">
<dc:identifier>SDN:L22::TOOL0529</dc:identifier>
<skos:notation>SDN:L22::TOOL0529</skos:notation>
<skos:prefLabel xml:lang="en">Kipp and Zonen SP LITE2 pyranometer</skos:prefLabel>
<skos:altLabel>Kipp and Zonen SP LITE2</skos:altLabel>
<skos:definition xml:lang="en">A silicon pyranometer with a spectral range of 400-1100 nm. Its sensitivity is proportional to the cosine of the angle of incidence of the incoming radiation. It has a sensitivity of 60 to 100 uV/W/m^2 and can operate at temperatures between -30 and 70 degC. The instrument supersedes the original SP Lite and has an improved response time of &lt;500ns compared with &lt;1s for the older model.</skos:definition>
<owl:versionInfo>1</owl:versionInfo>
<dc:date>2012-08-15 15:00:32.0</dc:date>
<skos:note xml:lang="en">accepted</skos:note>
<owl:deprecated>false</owl:deprecated>
<skos:broader rdf:resource="http://vocab.nerc.ac.uk/collection/L05/current/122/"/>
<void:inDataset rdf:resource="http://vocab.nerc.ac.uk/.well-known/void"/>
</skos:Concept>
</skos:member>
<skos:member>
<skos:Concept rdf:about="http://vocab.nerc.ac.uk/collection/L22/current/NETT0080/">
<dc:identifier>SDN:L22::NETT0080</dc:identifier>
<skos:notation>SDN:L22::NETT0080</skos:notation>
<skos:prefLabel xml:lang="en">Kitahara - Nakai (1962)</skos:prefLabel>
<skos:altLabel>Kitahara</skos:altLabel>
<skos:definition xml:lang="en">Net has a 24 cm diameter mouth opening for head piece and 45 cm diameter conical net 80 cm long. A Hensen style net (KT)</skos:definition>
<owl:versionInfo>1</owl:versionInfo>
<dc:date>2011-10-21 14:18:49.0</dc:date>
<skos:note xml:lang="en">accepted</skos:note>
<owl:deprecated>false</owl:deprecated>
<skos:broader rdf:resource="http://vocab.nerc.ac.uk/collection/L05/current/22/"/>
<void:inDataset rdf:resource="http://vocab.nerc.ac.uk/.well-known/void"/>
</skos:Concept>
</skos:member>
<skos:member>
<skos:Concept rdf:about="http://vocab.nerc.ac.uk/collection/L22/current/TOOL0505/">
<dc:identifier>SDN:L22::TOOL0505</dc:identifier>
<skos:notation>SDN:L22::TOOL0505</skos:notation>
<skos:prefLabel xml:lang="en">Knudsen reversing water bottle</skos:prefLabel>
<skos:altLabel>Knudsen bottle</skos:altLabel>
<skos:definition xml:lang="en">A frameless reversing water bottle with reversing thermometers that is used to collect water samples. The bottom of the bottle is clamped to a wire and the top of the bottle is held to the wire by a catch. It has independent hinged lids at each end which are held open against an internal spring when the bottle is deployed. Once the bottle has reached the target depth a messenger is dropped down the wire and hits the catch. The lids close and the bottle falls through 180deg, pivoting on the bottom clamp. This action reversed the thermometers, which are housed in a frame attached to the bottle.</skos:definition>
<owl:versionInfo>1</owl:versionInfo>
<dc:date>2012-06-21 16:09:48.0</dc:date>
<skos:note xml:lang="en">accepted</skos:note>
<owl:deprecated>false</owl:deprecated>
<skos:broader rdf:resource="http://vocab.nerc.ac.uk/collection/L05/current/30/"/>
<void:inDataset rdf:resource="http://vocab.nerc.ac.uk/.well-known/void"/>
</skos:Concept>
</skos:member>
<skos:member>
<skos:Concept rdf:about="http://vocab.nerc.ac.uk/collection/L22/current/TOOL0319/">
<dc:identifier>SDN:L22::TOOL0319</dc:identifier>
<skos:notation>SDN:L22::TOOL0319</skos:notation>
<skos:prefLabel xml:lang="en">Kongsberg (Simrad) EA600 Echosounder</skos:prefLabel>
<skos:altLabel>EA600 echosounder</skos:altLabel>
<skos:definition xml:lang="en">The EA600 single beam echosounder operates up to four high power transceivers simultaneously. Available frequencies span from 12 to 710 kHz with a variable power output of up to 2 kW and a 160 dB dynamic range. The EA600 replaced the EA500 in 2000.</skos:definition>
<owl:versionInfo>1</owl:versionInfo>
<dc:date>2010-09-06 12:45:22.0</dc:date>
<skos:note xml:lang="en">accepted</skos:note>
<owl:deprecated>false</owl:deprecated>
<skos:broader rdf:resource="http://vocab.nerc.ac.uk/collection/L05/current/156/"/>
<void:inDataset rdf:resource="http://vocab.nerc.ac.uk/.well-known/void"/>
</skos:Concept>
</skos:member>
<skos:member>
<skos:Concept rdf:about="http://vocab.nerc.ac.uk/collection/L22/current/TOOL0384/">
<dc:identifier>SDN:L22::TOOL0384</dc:identifier>
<skos:notation>SDN:L22::TOOL0384</skos:notation>
<skos:prefLabel xml:lang="en">Kongsberg (Simrad) EM 1002 multibeam echosounder</skos:prefLabel>
<skos:altLabel>EM 1002 echosounder</skos:altLabel>
<skos:definition xml:lang="en">A 95 kHz multibeam echosounder designed for use in water depths of up to 1000 m. The transducer array includes 111  beams with a 2 deg beam width. Across-track coverage is up to 1500 m and angular coverage is adjustable up to 190 deg. The instrument has pulse lengths of 0.2, 0.7 and 2 ms and a depth resolution of 1, 4 or 8 cm.</skos:definition>
<owl:versionInfo>1</owl:versionInfo>
<dc:date>2011-04-01 15:53:35.0</dc:date>
<skos:note xml:lang="en">accepted</skos:note>
<owl:deprecated>false</owl:deprecated>
<skos:broader rdf:resource="http://vocab.nerc.ac.uk/collection/L05/current/157/"/>
<void:inDataset rdf:resource="http://vocab.nerc.ac.uk/.well-known/void"/>
</skos:Concept>
</skos:member>
<skos:member>
<skos:Concept rdf:about="http://vocab.nerc.ac.uk/collection/L22/current/TOOL0385/">
<dc:identifier>SDN:L22::TOOL0385</dc:identifier>
<skos:notation>SDN:L22::TOOL0385</skos:notation>
<skos:prefLabel xml:lang="en">Kongsberg (Simrad) EM 1002S multibeam echosounder</skos:prefLabel>
<skos:altLabel>EM 1002S echosounder</skos:altLabel>
<skos:definition xml:lang="en">A 95 kHz multibeam echosounder, this is the shallow-water version of the EM 1002. The transducer array includes 111 beams with a 2 deg beam width. Across-track coverage is limited to approximately 1000 m and angular coverage is adjustable up to 190 deg. The instrument has a single pulse length of 0.2 ms.</skos:definition>
<owl:versionInfo>1</owl:versionInfo>
<dc:date>2011-04-01 15:53:35.0</dc:date>
<skos:note xml:lang="en">accepted</skos:note>
<owl:deprecated>false</owl:deprecated>
<skos:broader rdf:resource="http://vocab.nerc.ac.uk/collection/L05/current/157/"/>
<void:inDataset rdf:resource="http://vocab.nerc.ac.uk/.well-known/void"/>
</skos:Concept>
</skos:member>
<skos:member>
<skos:Concept rdf:about="http://vocab.nerc.ac.uk/collection/L22/current/TOOL0386/">
<dc:identifier>SDN:L22::TOOL0386</dc:identifier>
<skos:notation>SDN:L22::TOOL0386</skos:notation>
<skos:prefLabel xml:lang="en">Kongsberg (Simrad) EM 120 multibeam echosounder</skos:prefLabel>
<skos:altLabel>EM 120 echosounder</skos:altLabel>
<skos:definition xml:lang="en">A low frequency (12 kHz) multibeam echosounder with full ocean depth capability. The transducer array includes 191 beams with angular coverage adjustable up to 150 deg and a swath width of up to 5.5 times water depth. The instrument has pulse lengths of 2, 5 and 15 ms and a depth resolution of 10 to 40 cm.</skos:definition>
<owl:versionInfo>1</owl:versionInfo>
<dc:date>2011-04-08 07:51:17.0</dc:date>
<skos:note xml:lang="en">accepted</skos:note>
<owl:deprecated>false</owl:deprecated>
<skos:related rdf:resource="http://vocab.nerc.ac.uk/collection/P01/current/MBANSWCB/"/>
<skos:broader rdf:resource="http://vocab.nerc.ac.uk/collection/L05/current/157/"/>
<void:inDataset rdf:resource="http://vocab.nerc.ac.uk/.well-known/void"/>
</skos:Concept>
</skos:member>
<skos:member>
<skos:Concept rdf:about="http://vocab.nerc.ac.uk/collection/L22/current/TOOL0492/">
<dc:identifier>SDN:L22::TOOL0492</dc:identifier>
<skos:notation>SDN:L22::TOOL0492</skos:notation>
<skos:prefLabel xml:lang="en">Kongsberg EM 122 multibeam echosounder</skos:prefLabel>
<skos:altLabel>Kongsberg EM 122</skos:altLabel>
<skos:definition xml:lang="en">A multibeam 12 kHz echsounder designed for high resolution seabed mapping. It uses both Continuous Wave (CW) and Frequency Modulated (FM) sweep pulses with pulse compression on reception in order to increase the maximum used swath width. This system has up to 288 beams/432 soundings per swath with pointing angles which are automatically adjusted according to achievable coverage or operator defined limits. The transducers are modular linear arrays in a Mills cross configuration with separate units for transmit and receive. It has a depth range of 20 to 11000 m and a depth resolution of 1 cm.</skos:definition>
<owl:versionInfo>1</owl:versionInfo>
<dc:date>2012-05-21 10:02:44.0</dc:date>
<skos:note xml:lang="en">accepted</skos:note>
<owl:deprecated>false</owl:deprecated>
<skos:broader rdf:resource="http://vocab.nerc.ac.uk/collection/L05/current/157/"/>
<void:inDataset rdf:resource="http://vocab.nerc.ac.uk/.well-known/void"/>
</skos:Concept>
</skos:member>
<skos:member>
<skos:Concept rdf:about="http://vocab.nerc.ac.uk/collection/L22/current/TOOL0623/">
<dc:identifier>SDN:L22::TOOL0623</dc:identifier>
<skos:notation>SDN:L22::TOOL0623</skos:notation>
<skos:prefLabel xml:lang="en">Kongsberg Seatex Differential Positioning Sensor 116</skos:prefLabel>
<skos:altLabel>Kongsberg Seatex DPS 116</skos:altLabel>
<skos:definition xml:lang="en">A 14-channel, all-in-view, L1 GPS receiver which primarily utilises the free, WAAS, EGNOS and MSAS Satellite Based Augmentation Systems (SBAS) for differential corrections (DGPS). It is also capable of simultaneous DGPS from a wide variety of other reference stations (Multiref), resulting in improved accuracy. Positional accuracy is &lt; 1.5 m, 95% CEP (SBAS service) and &lt; 1 m, 95% CEP (Multiref). Output rate is 1 Hz.</skos:definition>
<owl:versionInfo>1</owl:versionInfo>
<dc:date>2013-06-10 15:51:02.0</dc:date>
<skos:note xml:lang="en">accepted</skos:note>
<owl:deprecated>false</owl:deprecated>
<skos:broader rdf:resource="http://vocab.nerc.ac.uk/collection/L05/current/POS04/"/>
<void:inDataset rdf:resource="http://vocab.nerc.ac.uk/.well-known/void"/>
</skos:Concept>
</skos:member>
<skos:member>
<skos:Concept rdf:about="http://vocab.nerc.ac.uk/collection/L22/current/TOOL0456/">
<dc:identifier>SDN:L22::TOOL0456</dc:identifier>
<skos:notation>SDN:L22::TOOL0456</skos:notation>
<skos:prefLabel xml:lang="en">Kongsberg Seatex Seapath 200 Global Positioning System receiver and Gyrocompass</skos:prefLabel>
<skos:altLabel>Seapath 200 GPS</skos:altLabel>
<skos:definition xml:lang="en">Sensor-based inertial navigation and Differential Global Positioning System (DGPS) receiver unit, providing heading, attitude and position. Motion data are provided by the Inertial Measurements Unit (IMU), which contains linear accelerometers and Bosch Coriolis force angular rate gyros (CFG). The unit contains two fixed baseline GPS carrier-phase receivers and is equipped to utilise up to six different DGPS reference stations for position and velocity measurements. This model is no longer in production.</skos:definition>
<owl:versionInfo>1</owl:versionInfo>
<dc:date>2012-02-07 12:32:54.0</dc:date>
<skos:note xml:lang="en">accepted</skos:note>
<owl:deprecated>false</owl:deprecated>
<skos:broader rdf:resource="http://vocab.nerc.ac.uk/collection/L05/current/385/"/>
<skos:broader rdf:resource="http://vocab.nerc.ac.uk/collection/L05/current/POS04/"/>
<void:inDataset rdf:resource="http://vocab.nerc.ac.uk/.well-known/void"/>
</skos:Concept>
</skos:member>
<skos:member>
<skos:Concept rdf:about="http://vocab.nerc.ac.uk/collection/L22/current/TOOL0491/">
<dc:identifier>SDN:L22::TOOL0491</dc:identifier>
<skos:notation>SDN:L22::TOOL0491</skos:notation>
<skos:prefLabel xml:lang="en">Kongsberg Seatex Seapath 320+ Precise Heading, Attitude and Positioning Sensor</skos:prefLabel>
<skos:altLabel>Kongsberg Seapath 230+ GPS</skos:altLabel>
<skos:definition xml:lang="en">A navigational system including two Global Navigation Satellite System (GNSS) receivers and a MRU 5+ inertial sensor. The inertial sensor employs linear accelerometers and unique microelectromechanical systems (MEMS)-type angular rate gyros to provide 0.01 RMS pitch and roll accuracy. The GNSS receivers can use multiple satellite constellations (GPS, GLONASS and Galileo, when available) to provide accurate heading and position data. This model has a position accuracy of 1 m inifferential GPS (DGPS), GLONASS and satellite-based augmentation system (SBAS) modes, and an accuracy of 0.2 m with real-time kinematic (RTK) corrections.</skos:definition>
<owl:versionInfo>1</owl:versionInfo>
<dc:date>2012-05-21 10:02:44.0</dc:date>
<skos:note xml:lang="en">accepted</skos:note>
<owl:deprecated>false</owl:deprecated>
<skos:broader rdf:resource="http://vocab.nerc.ac.uk/collection/L05/current/POS19/"/>
<skos:broader rdf:resource="http://vocab.nerc.ac.uk/collection/L05/current/POS02/"/>
<skos:broader rdf:resource="http://vocab.nerc.ac.uk/collection/L05/current/POS04/"/>
<void:inDataset rdf:resource="http://vocab.nerc.ac.uk/.well-known/void"/>
</skos:Concept>
</skos:member>
<skos:member>
<skos:Concept rdf:about="http://vocab.nerc.ac.uk/collection/L22/current/TOOL0657/">
<dc:identifier>SDN:L22::TOOL0657</dc:identifier>
<skos:notation>SDN:L22::TOOL0657</skos:notation>
<skos:prefLabel xml:lang="en">Konica Minolta CM-2600d Spectrophotometer</skos:prefLabel>
<skos:altLabel>Konica Minolta CM-2600d</skos:altLabel>
<skos:definition xml:lang="en">A portable, sphere type spectrophotometer which measures reflectance over the 360 nm - 740 nm wavelength range (at 10 nm half-bandwidths). It comprises a d/8 (diffused illumination, 8-degree viewing angle) iluminating/viewing system. It is equipped with two interchangeable measurement apertures (MAV: 8mm dia., SAV: 3mm dia.). The operating range is 0 to 175 % reflectance (0.01 % resolution). Spectral reflectance repeatability is within 0.1 % S.D. (0.2 % S.D. between 360 nm - 380 nm).</skos:definition>
<owl:versionInfo>2</owl:versionInfo>
<dc:date>2013-12-06 10:33:01.0</dc:date>
<skos:note xml:lang="en">accepted</skos:note>
<owl:deprecated>false</owl:deprecated>
<skos:broader rdf:resource="http://vocab.nerc.ac.uk/collection/L05/current/LAB20/"/>
<void:inDataset rdf:resource="http://vocab.nerc.ac.uk/.well-known/void"/>
</skos:Concept>
</skos:member>
<skos:member>
<skos:Concept rdf:about="http://vocab.nerc.ac.uk/collection/L22/current/TOOL0601/">
<dc:identifier>SDN:L22::TOOL0601</dc:identifier>
<skos:notation>SDN:L22::TOOL0601</skos:notation>
<skos:prefLabel xml:lang="en">LAIPAC GD30L MMC Global Positioning System logger</skos:prefLabel>
<skos:altLabel>LAIPAC GD30L GPS</skos:altLabel>
<skos:definition xml:lang="en">A high performance Global Positioning System (GPS) recorder and vehicle tracking system for passive tracking applications. The maximum sampling interval selectable is 3 seconds, with a minimum sampling interval of 30 minutes. The recorded data includes date, time, longitude, latitude, speed, trajectory, and number of tracking satellites.</skos:definition>
<owl:versionInfo>1</owl:versionInfo>
<dc:date>2013-02-27 15:52:20.0</dc:date>
<skos:note xml:lang="en">accepted</skos:note>
<owl:deprecated>false</owl:deprecated>
<skos:broader rdf:resource="http://vocab.nerc.ac.uk/collection/L05/current/POS03/"/>
<void:inDataset rdf:resource="http://vocab.nerc.ac.uk/.well-known/void"/>
</skos:Concept>
</skos:member>
<skos:member>
<skos:Concept rdf:about="http://vocab.nerc.ac.uk/collection/L22/current/TOOL0085/">
<dc:identifier>SDN:L22::TOOL0085</dc:identifier>
<skos:notation>SDN:L22::TOOL0085</skos:notation>
<skos:prefLabel xml:lang="en">LI-COR 7500 infrared gas analyser</skos:prefLabel>
<skos:altLabel>LI-COR 7500 IR gas analyzer</skos:altLabel>
<skos:definition xml:lang="en">A non-dispersive infrared gas analyzer that measures carbon dioxide and water vapour concentrations in the atmosphere. The power received from the infrared source is measured at three wavelengths: one at a wavelength that is absorbed by carbon dioxide, another at a wavelength that is absorbed by water, and the third at a non-absorbing reference wavelength. The absorbance of each gas is calculated and converted to molar fraction using density, pressure and temperature data.</skos:definition>
<owl:versionInfo>2</owl:versionInfo>
<dc:date>2011-07-01 10:21:24.0</dc:date>
<skos:note xml:lang="en">accepted</skos:note>
<owl:deprecated>false</owl:deprecated>
<skos:broader rdf:resource="http://vocab.nerc.ac.uk/collection/L05/current/382/"/>
<void:inDataset rdf:resource="http://vocab.nerc.ac.uk/.well-known/void"/>
</skos:Concept>
</skos:member>
<skos:member>
<skos:Concept rdf:about="http://vocab.nerc.ac.uk/collection/L22/current/TOOL0432/">
<dc:identifier>SDN:L22::TOOL0432</dc:identifier>
<skos:notation>SDN:L22::TOOL0432</skos:notation>
<skos:prefLabel xml:lang="en">LI-COR LI-1800UW Underwater Spectroradiometer</skos:prefLabel>
<skos:altLabel>LI-1800UW radiometer</skos:altLabel>
<skos:definition xml:lang="en">A cosine-collector underwater radiometer with a spectral range of 100-850nm and a depth rating of 200m. Scan speed ranges from 20-45nm per second at intervals of 1, 2, 5 or 10nm. The instrument combines a holographic rating monochromator, and order sorting filter wheel and a silicon detector, and all operations are controlled by an internal microcomputer. Spectral data are automatically corrected for the wavelength-dependent immersion effect. Scanning can be initiated from the surface or the insturment can be programmed for autonomous operation, so it is useful for both real time profiling and time series monitoring applications. Although the LI-1800UW is designed for underwater measurements, it is also calibrated for use as a terrestrial spectro-radiometer and can be used in air with the standard 1800 cosine collector or with any of the optical receptors available for the LI-1800 Portable Spectroradiometer.</skos:definition>
<owl:versionInfo>1</owl:versionInfo>
<dc:date>2011-11-02 11:37:25.0</dc:date>
<skos:note xml:lang="en">accepted</skos:note>
<owl:deprecated>false</owl:deprecated>
<skos:broader rdf:resource="http://vocab.nerc.ac.uk/collection/L05/current/122/"/>
<void:inDataset rdf:resource="http://vocab.nerc.ac.uk/.well-known/void"/>
</skos:Concept>
</skos:member>
<skos:member>
<skos:Concept rdf:about="http://vocab.nerc.ac.uk/collection/L22/current/TOOL0193/">
<dc:identifier>SDN:L22::TOOL0193</dc:identifier>
<skos:notation>SDN:L22::TOOL0193</skos:notation>
<skos:prefLabel xml:lang="en">LI-COR LI-190 PAR sensor</skos:prefLabel>
<skos:altLabel>LI-190 PAR</skos:altLabel>
<skos:definition xml:lang="en">A non-submersible cosine-corrected PAR sensor sensitive wavelengths from 400-700nm with sharp cut-off due to an interference filter. It may be used as a reference sensor for LI-192 and LI-193 Underwater Quantum Sensor.</skos:definition>
<owl:versionInfo>1</owl:versionInfo>
<dc:date>2010-05-18 16:10:58.0</dc:date>
<skos:note xml:lang="en">accepted</skos:note>
<owl:deprecated>false</owl:deprecated>
<skos:broader rdf:resource="http://vocab.nerc.ac.uk/collection/L05/current/122/"/>
<void:inDataset rdf:resource="http://vocab.nerc.ac.uk/.well-known/void"/>
</skos:Concept>
</skos:member>
<skos:member>
<skos:Concept rdf:about="http://vocab.nerc.ac.uk/collection/L22/current/TOOL0120/">
<dc:identifier>SDN:L22::TOOL0120</dc:identifier>
<skos:notation>SDN:L22::TOOL0120</skos:notation>
<skos:prefLabel xml:lang="en">LI-COR LI-192 PAR sensor</skos:prefLabel>
<skos:altLabel>LI-192 PAR</skos:altLabel>
<skos:definition xml:lang="en">An underwater or atmospheric quantum sensor with cosine correction that can operate down to 560m. Fitted with a blue-enhanced silicon photovoltaic detector.</skos:definition>
<owl:versionInfo>1</owl:versionInfo>
<dc:date>2010-05-18 16:10:58.0</dc:date>
<skos:note xml:lang="en">accepted</skos:note>
<owl:deprecated>false</owl:deprecated>
<skos:broader rdf:resource="http://vocab.nerc.ac.uk/collection/L05/current/122/"/>
<void:inDataset rdf:resource="http://vocab.nerc.ac.uk/.well-known/void"/>
</skos:Concept>
</skos:member>
<skos:member>
<skos:Concept rdf:about="http://vocab.nerc.ac.uk/collection/L22/current/TOOL0458/">
<dc:identifier>SDN:L22::TOOL0458</dc:identifier>
<skos:notation>SDN:L22::TOOL0458</skos:notation>
<skos:prefLabel xml:lang="en">LI-COR LI-193 Spherical Quantum PAR sensor</skos:prefLabel>
<skos:altLabel>LI-193 PAR</skos:altLabel>
<skos:definition xml:lang="en">An underwater spherical quantum sensor which measures photon flux from all directions (termed quantum scalar irradiance). The sensor can operate down to 350 m and is fitted with a blue-enhanced silicon photovoltaic detector. Two versions of the instrument are available (193SA and 193SB). These use different connector types for the underwater cable.</skos:definition>
<owl:versionInfo>1</owl:versionInfo>
<dc:date>2012-02-16 10:05:14.0</dc:date>
<skos:note xml:lang="en">accepted</skos:note>
<owl:deprecated>false</owl:deprecated>
<skos:broader rdf:resource="http://vocab.nerc.ac.uk/collection/L05/current/122/"/>
<void:inDataset rdf:resource="http://vocab.nerc.ac.uk/.well-known/void"/>
</skos:Concept>
</skos:member>
<skos:member>
<skos:Concept rdf:about="http://vocab.nerc.ac.uk/collection/L22/current/TOOL0547/">
<dc:identifier>SDN:L22::TOOL0547</dc:identifier>
<skos:notation>SDN:L22::TOOL0547</skos:notation>
<skos:prefLabel xml:lang="en">Lancaster University syringe water sampler</skos:prefLabel>
<skos:altLabel>Lancs Uni syringe sampler</skos:altLabel>
<skos:definition xml:lang="en">A water sample collection system comprising a peristaltic pump attached to a syringe, allowing near-surface samples to be gathered without introducing oxygen (a closed system).</skos:definition>
<owl:versionInfo>1</owl:versionInfo>
<dc:date>2012-09-26 16:33:22.0</dc:date>
<skos:note xml:lang="en">accepted</skos:note>
<owl:deprecated>false</owl:deprecated>
<skos:broader rdf:resource="http://vocab.nerc.ac.uk/collection/L05/current/30/"/>
<void:inDataset rdf:resource="http://vocab.nerc.ac.uk/.well-known/void"/>
</skos:Concept>
</skos:member>
<skos:member>
<skos:Concept rdf:about="http://vocab.nerc.ac.uk/collection/L22/current/NETT0084/">
<dc:identifier>SDN:L22::NETT0084</dc:identifier>
<skos:notation>SDN:L22::NETT0084</skos:notation>
<skos:prefLabel xml:lang="en">Large Opening-closing High-speed Sampling System - Dunn et al. (1989, 1993)</skos:prefLabel>
<skos:altLabel>LOCHNESS</skos:altLabel>
<skos:definition xml:lang="en">Rectangular net design similar to BIONESS.  Uses an acoustic telemetry system to monitor depth, battery voltage, flow, and net function and to control the opening and closing of the nets. An underwater data logger is also present to log depth, conductivity, temperature and other parameters. LOCHNESS carries 5 nets with 224 cm x 224 cm mouth opening (5-m2) x 1400 cm long.  Tow speeds up to 6 knots [Wiebe and Benfield 2003 Plate 31 D, E].</skos:definition>
<owl:versionInfo>1</owl:versionInfo>
<dc:date>2011-10-21 14:18:49.0</dc:date>
<skos:note xml:lang="en">accepted</skos:note>
<owl:deprecated>false</owl:deprecated>
<skos:broader rdf:resource="http://vocab.nerc.ac.uk/collection/L05/current/134/"/>
<skos:broader rdf:resource="http://vocab.nerc.ac.uk/collection/L05/current/23/"/>
<skos:broader rdf:resource="http://vocab.nerc.ac.uk/collection/L05/current/68/"/>
<skos:broader rdf:resource="http://vocab.nerc.ac.uk/collection/L05/current/67/"/>
<skos:broader rdf:resource="http://vocab.nerc.ac.uk/collection/L05/current/388/"/>
<skos:broader rdf:resource="http://vocab.nerc.ac.uk/collection/L05/current/350/"/>
<void:inDataset rdf:resource="http://vocab.nerc.ac.uk/.well-known/void"/>
</skos:Concept>
</skos:member>
<skos:member>
<skos:Concept rdf:about="http://vocab.nerc.ac.uk/collection/L22/current/TOOL0509/">
<dc:identifier>SDN:L22::TOOL0509</dc:identifier>
<skos:notation>SDN:L22::TOOL0509</skos:notation>
<skos:prefLabel xml:lang="en">Lasentec Partec 100 focused beam reflectance measurement particle sizer</skos:prefLabel>
<skos:altLabel>Partec 100 FBRM</skos:altLabel>
<skos:definition xml:lang="en">An in situ particle sizer that uses the principal of focused beam reflectance measurement (FBRM) to measure particle sizes in the range 2-1000 um in a liquid. The probe tip includes an optic filter, beam splitter, laser beam and sapphire window, through which laser light is passed into the liquid. The light is diffracted by particles suspended in the liquid and the FBRM measures the chord length distribution (CLD), which is a function of the number, size and shape of the particles. Typically, many thousands of chords are measured per second, providing a robust measurement sensitive to the change in the size or number of particles. The instrument can be deployed on a hydrographic wire and lowered to the required depth, where is is held steady while a particle spectrum is collected. The instrument was developed by Lasentec (also known as Lasentech), which has since been taken over by Mettler Toledo. The Partec 100 is no longer in production.</skos:definition>
<owl:versionInfo>1</owl:versionInfo>
<dc:date>2012-06-22 15:36:10.0</dc:date>
<skos:note xml:lang="en">accepted</skos:note>
<owl:deprecated>false</owl:deprecated>
<skos:broader rdf:resource="http://vocab.nerc.ac.uk/collection/L05/current/123/"/>
<skos:broader rdf:resource="http://vocab.nerc.ac.uk/collection/L05/current/150/"/>
<void:inDataset rdf:resource="http://vocab.nerc.ac.uk/.well-known/void"/>
</skos:Concept>
</skos:member>
<skos:member>
<skos:Concept rdf:about="http://vocab.nerc.ac.uk/collection/L22/current/TOOL0010/">
<dc:identifier>SDN:L22::TOOL0010</dc:identifier>
<skos:notation>SDN:L22::TOOL0010</skos:notation>
<skos:prefLabel xml:lang="en">Lea float tide gauge</skos:prefLabel>
<skos:altLabel>Lea gauge</skos:altLabel>
<skos:definition xml:lang="en">The Lea gauge is a vertically mounted chart recording gauge which measures the sea level by means of a float in a stilling well. The float is connected to the large drum in the lower centre of the picture and the counter weight connected to the smaller drum on its right. This difference in drum size means the counter weight does not enter the seawater on every tide. The disadvantage is that the counter weight has to be proportionally heavier to counter balance the float. The pen arm is moved up and down the chart by means of a chain loop linked to a worm gear on the drum axle.</skos:definition>
<owl:versionInfo>1</owl:versionInfo>
<dc:date>2009-11-30 11:27:51.0</dc:date>
<skos:note xml:lang="en">accepted</skos:note>
<owl:deprecated>false</owl:deprecated>
<skos:broader rdf:resource="http://vocab.nerc.ac.uk/collection/L05/current/111/"/>
<void:inDataset rdf:resource="http://vocab.nerc.ac.uk/.well-known/void"/>
</skos:Concept>
</skos:member>
<skos:member>
<skos:Concept rdf:about="http://vocab.nerc.ac.uk/collection/L22/current/TOOL0427/">
<dc:identifier>SDN:L22::TOOL0427</dc:identifier>
<skos:notation>SDN:L22::TOOL0427</skos:notation>
<skos:prefLabel xml:lang="en">Lever Action Niskin Bottle</skos:prefLabel>
<skos:altLabel>Levered Niskin Bottle</skos:altLabel>
<skos:definition xml:lang="en">A plastic free-flushing water sampling bottle with a capacity of 1.7-12 litres. It has caps with rubber seals at each end and is deployed with the caps held open by externally mounted stainless steel springs. Unlike the standard Niskin design, this bottle does not feature an internal lanyard, and is thus recommended for applications where a completely clear sample chamber is critical. When the bottle reaches the desired depth it is closed by messenger when serially attached to hydrocable or by remote command when attached to sampling rosette.</skos:definition>
<owl:versionInfo>1</owl:versionInfo>
<dc:date>2011-10-17 12:44:36.0</dc:date>
<skos:note xml:lang="en">accepted</skos:note>
<owl:deprecated>false</owl:deprecated>
<skos:broader rdf:resource="http://vocab.nerc.ac.uk/collection/L05/current/30/"/>
<void:inDataset rdf:resource="http://vocab.nerc.ac.uk/.well-known/void"/>
</skos:Concept>
</skos:member>
<skos:member>
<skos:Concept rdf:about="http://vocab.nerc.ac.uk/collection/L22/current/TOOL0493/">
<dc:identifier>SDN:L22::TOOL0493</dc:identifier>
<skos:notation>SDN:L22::TOOL0493</skos:notation>
<skos:prefLabel xml:lang="en">Litre Meter LMSPFA.05 flow meter</skos:prefLabel>
<skos:altLabel>Litre Meter LMSPFA.05 flow meter</skos:altLabel>
<skos:definition xml:lang="en">Pelton Wheel flow meter designed to monitor water flow rates for pumped systems such as ships' continuous seawater supplies. The flow meter is designed to measure low flow rates in the range 0.006 to 0.1 l/min. Water flows through an inlet and is directed onto a rotor, whose rotation rate is directly proportional to the flow rate.</skos:definition>
<owl:versionInfo>1</owl:versionInfo>
<dc:date>2012-05-21 10:02:44.0</dc:date>
<skos:note xml:lang="en">accepted</skos:note>
<owl:deprecated>false</owl:deprecated>
<skos:broader rdf:resource="http://vocab.nerc.ac.uk/collection/L05/current/388/"/>
<void:inDataset rdf:resource="http://vocab.nerc.ac.uk/.well-known/void"/>
</skos:Concept>
</skos:member>
<skos:member>
<skos:Concept rdf:about="http://vocab.nerc.ac.uk/collection/L22/current/TOOL0400/">
<dc:identifier>SDN:L22::TOOL0400</dc:identifier>
<skos:notation>SDN:L22::TOOL0400</skos:notation>
<skos:prefLabel xml:lang="en">Litre Meter flow meter</skos:prefLabel>
<skos:altLabel>Litre Meter flow meter</skos:altLabel>
<skos:definition xml:lang="en">A flow meter of unspecified model used to monitor water flow rates for pumped systems such as ships' continuous seawater supplies.</skos:definition>
<owl:versionInfo>1</owl:versionInfo>
<dc:date>2011-05-16 09:44:34.0</dc:date>
<skos:note xml:lang="en">accepted</skos:note>
<owl:deprecated>false</owl:deprecated>
<skos:broader rdf:resource="http://vocab.nerc.ac.uk/collection/L05/current/388/"/>
<void:inDataset rdf:resource="http://vocab.nerc.ac.uk/.well-known/void"/>
</skos:Concept>
</skos:member>
<skos:member>
<skos:Concept rdf:about="http://vocab.nerc.ac.uk/collection/L22/current/TOOL0435/">
<dc:identifier>SDN:L22::TOOL0435</dc:identifier>
<skos:notation>SDN:L22::TOOL0435</skos:notation>
<skos:prefLabel xml:lang="en">Lockheed Martin Sippican T-4 XBT probe</skos:prefLabel>
<skos:altLabel>Sippican T-4 XBT</skos:altLabel>
<skos:definition xml:lang="en">An expendable free-fall temperature probe that provides a profile of measured temperature against depth calculated from a fall-rate model. The T-4 XBT Probe can be used within a maximum depth of 460m, may be deployed at a ship speed of up to 30 knots and has a vertical resolution of 65cm.</skos:definition>
<owl:versionInfo>1</owl:versionInfo>
<dc:date>2011-11-02 11:37:25.0</dc:date>
<skos:note xml:lang="en">accepted</skos:note>
<owl:deprecated>false</owl:deprecated>
<skos:broader rdf:resource="http://vocab.nerc.ac.uk/collection/L05/current/134/"/>
<skos:broader rdf:resource="http://vocab.nerc.ac.uk/collection/L05/current/132/"/>
<void:inDataset rdf:resource="http://vocab.nerc.ac.uk/.well-known/void"/>
</skos:Concept>
</skos:member>
<skos:member>
<skos:Concept rdf:about="http://vocab.nerc.ac.uk/collection/L22/current/TOOL0262/">
<dc:identifier>SDN:L22::TOOL0262</dc:identifier>
<skos:notation>SDN:L22::TOOL0262</skos:notation>
<skos:prefLabel xml:lang="en">Lockheed Martin Sippican T-5 XBT probe</skos:prefLabel>
<skos:altLabel>Sippican T-5 XBT</skos:altLabel>
<skos:definition xml:lang="en">An expendable free-fall temperature probe that provides a profile of measured temperature against depth calculated from a fall-rate model. The T-5 XBT Probe can be used within a maximum depth of 1830m, may be deployed at a ship speed of up to 6 knots and has a vertical resolution of 65cm.</skos:definition>
<owl:versionInfo>1</owl:versionInfo>
<dc:date>2010-05-18 16:10:58.0</dc:date>
<skos:note xml:lang="en">accepted</skos:note>
<owl:deprecated>false</owl:deprecated>
<skos:broader rdf:resource="http://vocab.nerc.ac.uk/collection/L05/current/132/"/>
<skos:broader rdf:resource="http://vocab.nerc.ac.uk/collection/L05/current/134/"/>
<void:inDataset rdf:resource="http://vocab.nerc.ac.uk/.well-known/void"/>
</skos:Concept>
</skos:member>
<skos:member>
<skos:Concept rdf:about="http://vocab.nerc.ac.uk/collection/L22/current/TOOL0263/">
<dc:identifier>SDN:L22::TOOL0263</dc:identifier>
<skos:notation>SDN:L22::TOOL0263</skos:notation>
<skos:prefLabel xml:lang="en">Lockheed Martin Sippican T-7 XBT probe</skos:prefLabel>
<skos:altLabel>Sippican T-7 XBT</skos:altLabel>
<skos:definition xml:lang="en">An expendable free-fall temperature probe that provides a profile of measured temperature against depth calculated from a fall-rate model. The T-7 XBT Probe can be used within a maximum depth of 760m, may be deployed at a ship speed of up to 15 knots and has a vertical resolution of 65cm.</skos:definition>
<owl:versionInfo>1</owl:versionInfo>
<dc:date>2010-05-18 16:10:58.0</dc:date>
<skos:note xml:lang="en">accepted</skos:note>
<owl:deprecated>false</owl:deprecated>
<skos:broader rdf:resource="http://vocab.nerc.ac.uk/collection/L05/current/134/"/>
<skos:broader rdf:resource="http://vocab.nerc.ac.uk/collection/L05/current/132/"/>
<void:inDataset rdf:resource="http://vocab.nerc.ac.uk/.well-known/void"/>
</skos:Concept>
</skos:member>
<skos:member>
<skos:Concept rdf:about="http://vocab.nerc.ac.uk/collection/L22/current/TOOL0591/">
<dc:identifier>SDN:L22::TOOL0591</dc:identifier>
<skos:notation>SDN:L22::TOOL0591</skos:notation>
<skos:prefLabel xml:lang="en">Lockheed Martin Sippican XCTD-1 probe</skos:prefLabel>
<skos:altLabel>Sippican XCTD-1</skos:altLabel>
<skos:definition xml:lang="en">An expendable free-fall CTD profiling system which provides a profile of measured temperature and conductivity against depth calculated using a fall-rate model. This instrument can be used within a maximum depth of 1000 m and may be deployed with a ship speed of up to 12 knots.</skos:definition>
<owl:versionInfo>1</owl:versionInfo>
<dc:date>2013-01-18 15:13:47.0</dc:date>
<skos:note xml:lang="en">accepted</skos:note>
<owl:deprecated>false</owl:deprecated>
<skos:broader rdf:resource="http://vocab.nerc.ac.uk/collection/L05/current/350/"/>
<skos:broader rdf:resource="http://vocab.nerc.ac.uk/collection/L05/current/134/"/>
<skos:broader rdf:resource="http://vocab.nerc.ac.uk/collection/L05/current/354/"/>
<void:inDataset rdf:resource="http://vocab.nerc.ac.uk/.well-known/void"/>
</skos:Concept>
</skos:member>
<skos:member>
<skos:Concept rdf:about="http://vocab.nerc.ac.uk/collection/L22/current/TOOL0592/">
<dc:identifier>SDN:L22::TOOL0592</dc:identifier>
<skos:notation>SDN:L22::TOOL0592</skos:notation>
<skos:prefLabel xml:lang="en">Lockheed Martin Sippican XCTD-2 probe</skos:prefLabel>
<skos:altLabel>Sippican XCTD-2</skos:altLabel>
<skos:definition xml:lang="en">An expendable free-fall CTD profiling system which provides a profile of measured temperature and conductivity against depth calculated using a fall-rate model. This instrument can be used within a maximum depth of 1850 m and may be deployed with a  ship speed of up to 3.5 knots.</skos:definition>
<owl:versionInfo>1</owl:versionInfo>
<dc:date>2013-01-18 15:13:47.0</dc:date>
<skos:note xml:lang="en">accepted</skos:note>
<owl:deprecated>false</owl:deprecated>
<skos:broader rdf:resource="http://vocab.nerc.ac.uk/collection/L05/current/350/"/>
<skos:broader rdf:resource="http://vocab.nerc.ac.uk/collection/L05/current/134/"/>
<skos:broader rdf:resource="http://vocab.nerc.ac.uk/collection/L05/current/354/"/>
<void:inDataset rdf:resource="http://vocab.nerc.ac.uk/.well-known/void"/>
</skos:Concept>
</skos:member>
<skos:member>
<skos:Concept rdf:about="http://vocab.nerc.ac.uk/collection/L22/current/NETT0082/">
<dc:identifier>SDN:L22::NETT0082</dc:identifier>
<skos:notation>SDN:L22::NETT0082</skos:notation>
<skos:prefLabel xml:lang="en">Longhurst-Hardy Plankton recorder - Longhurst et al (1966)</skos:prefLabel>
<skos:altLabel>LHPR</skos:altLabel>
<skos:definition xml:lang="en">A 50 cm diameter net mounted in a towing frame. Attached to the cod end of the net was a plankton recorder box with two rolls of gauze that were spooled onto a single spool after cutting across a tunnel through which water and plankton flowed out of the back of the net. The take-up spool with the plankton sandwiched between the two strips of gauze was advanced in discrete steps (15 seconds to 60 seconds) by an electronics package on the tow frame. Data on pressure and temperature and flow counts were logged on an internal recorder in the pressure case.  Normally towed at 1.5 to 2.5 knots and collected ~ 100 samples [Wiebe and Benfield 2003 Plate 26 C].</skos:definition>
<owl:versionInfo>1</owl:versionInfo>
<dc:date>2011-10-21 14:18:49.0</dc:date>
<skos:note xml:lang="en">accepted</skos:note>
<owl:deprecated>false</owl:deprecated>
<skos:broader rdf:resource="http://vocab.nerc.ac.uk/collection/L05/current/134/"/>
<skos:broader rdf:resource="http://vocab.nerc.ac.uk/collection/L05/current/21/"/>
<skos:broader rdf:resource="http://vocab.nerc.ac.uk/collection/L05/current/388/"/>
<void:inDataset rdf:resource="http://vocab.nerc.ac.uk/.well-known/void"/>
</skos:Concept>
</skos:member>
<skos:member>
<skos:Concept rdf:about="http://vocab.nerc.ac.uk/collection/L22/current/NETT0085/">
<dc:identifier>SDN:L22::NETT0085</dc:identifier>
<skos:notation>SDN:L22::NETT0085</skos:notation>
<skos:prefLabel xml:lang="en">Lowestoft frame trawl - Walker and Davies (1986)</skos:prefLabel>
<skos:altLabel>Lowestoft frame trawl</skos:altLabel>
<skos:definition xml:lang="en">A 142 cm x 142 cm rectangular mouth opening trawl with a rigid mouth frame and  nets 747.5 cm long of 5.0 cm mesh. Uses a TSK flowmeter converted to a digital counter unit and conducting cable to power  depth and temperature sensors.  Data recorded on a surface chart recorder.  Normally towed at 3 knots.  A 100 cm x 100 cm mouth opening trawl with a net length of 475 cm also described.  Mainly for small pelagic fish capture.  Not opening/closing [Wiebe and Benfield 2003 Plate 4 F].</skos:definition>
<owl:versionInfo>1</owl:versionInfo>
<dc:date>2011-10-21 14:18:49.0</dc:date>
<skos:note xml:lang="en">accepted</skos:note>
<owl:deprecated>false</owl:deprecated>
<skos:broader rdf:resource="http://vocab.nerc.ac.uk/collection/L05/current/23/"/>
<skos:broader rdf:resource="http://vocab.nerc.ac.uk/collection/L05/current/388/"/>
<skos:broader rdf:resource="http://vocab.nerc.ac.uk/collection/L05/current/134/"/>
<void:inDataset rdf:resource="http://vocab.nerc.ac.uk/.well-known/void"/>
</skos:Concept>
</skos:member>
<skos:member>
<skos:Concept rdf:about="http://vocab.nerc.ac.uk/collection/L22/current/NETT0086/">
<dc:identifier>SDN:L22::NETT0086</dc:identifier>
<skos:notation>SDN:L22::NETT0086</skos:notation>
<skos:prefLabel xml:lang="en">Lowestoft multiple high-speed plankton sampler - Beverton and Tungate (1967)</skos:prefLabel>
<skos:altLabel>Lowestoft HSS</skos:altLabel>
<skos:definition xml:lang="en">Construction comprises a 30.5 to  48.5 cm diameter nose cone aperture with 76.6 cm diameter body and 244 cm in length (a modified Gulf III sampler).  Conical netting of nylon mesh of 0.270, 0.305, or 0.420 mm or Monel metal mesh of 0.270, 0.42, 0.560 mm.  Has two auxiliary samplers with nose cones of 5 to 9 cm diameter and main body 16.5 cm diameter (0.061 - 0.270 cm mesh). An additional phytoplankton or water sampler has an aperture of 0.1 cm and a body diameter of 11.5 cm. Flowmeter mounted in nose cone [Wiebe and Benfield 2003 Plate 17 A].</skos:definition>
<owl:versionInfo>1</owl:versionInfo>
<dc:date>2011-10-21 14:18:49.0</dc:date>
<skos:note xml:lang="en">accepted</skos:note>
<owl:deprecated>false</owl:deprecated>
<skos:broader rdf:resource="http://vocab.nerc.ac.uk/collection/L05/current/388/"/>
<skos:broader rdf:resource="http://vocab.nerc.ac.uk/collection/L05/current/67/"/>
<void:inDataset rdf:resource="http://vocab.nerc.ac.uk/.well-known/void"/>
</skos:Concept>
</skos:member>
<skos:member>
<skos:Concept rdf:about="http://vocab.nerc.ac.uk/collection/L22/current/NETT0087/">
<dc:identifier>SDN:L22::NETT0087</dc:identifier>
<skos:notation>SDN:L22::NETT0087</skos:notation>
<skos:prefLabel xml:lang="en">MAFF-Guildline high-speed samplers - Milligan and Riches (1983)</skos:prefLabel>
<skos:altLabel>MAFF-Guildline HSS</skos:altLabel>
<skos:definition xml:lang="en">A modified Lowestoft Sampler -itself a modified Gulf III sampler - which has a 40 cm diameter conical nose cone aperture with 76.6 cm diameter body 275 cm long.  A second system has a 20 cm diameter nose cone aperture with a 53.3 cm diameter body that is 275 cm long. These systems have a Guildline CTD sensor unit with oxygen, pH, and digital flowmeter as additional probes with telemetry through a conducting cable. (MAFF stands for Ministry of Agriculture, Fisheries, and Food, now known as CEFAS)</skos:definition>
<owl:versionInfo>1</owl:versionInfo>
<dc:date>2011-10-21 14:18:49.0</dc:date>
<skos:note xml:lang="en">accepted</skos:note>
<owl:deprecated>false</owl:deprecated>
<skos:broader rdf:resource="http://vocab.nerc.ac.uk/collection/L05/current/130/"/>
<skos:broader rdf:resource="http://vocab.nerc.ac.uk/collection/L05/current/350/"/>
<skos:broader rdf:resource="http://vocab.nerc.ac.uk/collection/L05/current/134/"/>
<skos:broader rdf:resource="http://vocab.nerc.ac.uk/collection/L05/current/67/"/>
<skos:broader rdf:resource="http://vocab.nerc.ac.uk/collection/L05/current/351/"/>
<skos:broader rdf:resource="http://vocab.nerc.ac.uk/collection/L05/current/355/"/>
<skos:broader rdf:resource="http://vocab.nerc.ac.uk/collection/L05/current/388/"/>
<void:inDataset rdf:resource="http://vocab.nerc.ac.uk/.well-known/void"/>
</skos:Concept>
</skos:member>
<skos:member>
<skos:Concept rdf:about="http://vocab.nerc.ac.uk/collection/L22/current/NETT0089/">
<dc:identifier>SDN:L22::NETT0089</dc:identifier>
<skos:notation>SDN:L22::NETT0089</skos:notation>
<skos:prefLabel xml:lang="en">MARMAP Bongo net - Posgay and Marak (1980)</skos:prefLabel>
<skos:altLabel>MARMAP Bongo net</skos:altLabel>
<skos:definition xml:lang="en">A non-opening/closing descendant of the McGowan-Brown Bongo net. A pair of circular hoops (61 cm in diameter and 30 cm long) are joined by a central yoke which is clamped to the towing cable.   The nets are 61 cm in diameter and have cylindrical section 147 cm long and a conical section 153 cm long. Mesh sizes from 0.1 to 0.5 mm have been used, but normally 0.333 mm is used.  A flowmeter is  present in each hoop [Wiebe and Benfield 2003 Plate 2 D, E].</skos:definition>
<owl:versionInfo>1</owl:versionInfo>
<dc:date>2011-10-21 14:18:49.0</dc:date>
<skos:note xml:lang="en">accepted</skos:note>
<owl:deprecated>false</owl:deprecated>
<skos:broader rdf:resource="http://vocab.nerc.ac.uk/collection/L05/current/388/"/>
<skos:broader rdf:resource="http://vocab.nerc.ac.uk/collection/L05/current/22/"/>
<void:inDataset rdf:resource="http://vocab.nerc.ac.uk/.well-known/void"/>
</skos:Concept>
</skos:member>
<skos:member>
<skos:Concept rdf:about="http://vocab.nerc.ac.uk/collection/L22/current/NETT0097/">
<dc:identifier>SDN:L22::NETT0097</dc:identifier>
<skos:notation>SDN:L22::NETT0097</skos:notation>
<skos:prefLabel xml:lang="en">MOCNESS modified Tucker trawl - Wiebe et al (1976, 1985)</skos:prefLabel>
<skos:altLabel>MOCNESS</skos:altLabel>
<skos:definition xml:lang="en">Has a 100 cm x 141 cm rigid mouth opening  with nine 0.333 mm nylon mesh nets 6 meters long. System powered electrically on conducting wire and originally controlled from surface deck unit and now computer controlled.  Sensors include pressure, temperature, conductivity, fluorometer, transmissometer, oxygen, and light. Versions include systems with 1/4, 1, 2, 4, 10 and 20 m2 mouth openings all using the same release mechanisms, sensors, and compute logging and controls [Wiebe and Benfield 2003 Plates 28 D; 29 A-D].</skos:definition>
<owl:versionInfo>1</owl:versionInfo>
<dc:date>2011-10-21 14:18:49.0</dc:date>
<skos:note xml:lang="en">accepted</skos:note>
<owl:deprecated>false</owl:deprecated>
<skos:broader rdf:resource="http://vocab.nerc.ac.uk/collection/L05/current/350/"/>
<skos:broader rdf:resource="http://vocab.nerc.ac.uk/collection/L05/current/68/"/>
<skos:broader rdf:resource="http://vocab.nerc.ac.uk/collection/L05/current/122/"/>
<skos:broader rdf:resource="http://vocab.nerc.ac.uk/collection/L05/current/134/"/>
<skos:broader rdf:resource="http://vocab.nerc.ac.uk/collection/L05/current/351/"/>
<skos:broader rdf:resource="http://vocab.nerc.ac.uk/collection/L05/current/124/"/>
<skos:broader rdf:resource="http://vocab.nerc.ac.uk/collection/L05/current/113/"/>
<skos:broader rdf:resource="http://vocab.nerc.ac.uk/collection/L05/current/23/"/>
<void:inDataset rdf:resource="http://vocab.nerc.ac.uk/.well-known/void"/>
</skos:Concept>
</skos:member>
<skos:member>
<skos:Concept rdf:about="http://vocab.nerc.ac.uk/collection/L22/current/NETT0100/">
<dc:identifier>SDN:L22::NETT0100</dc:identifier>
<skos:notation>SDN:L22::NETT0100</skos:notation>
<skos:prefLabel xml:lang="en">MTD horizontal net - Motoda (1971)</skos:prefLabel>
<skos:altLabel>MTD horizontal net</skos:altLabel>
<skos:definition xml:lang="en">Comprises a 56 cm diameter cylinder (80 cm length and cone (110 cm length) net mounted on wire with a triangular framework so that up to 10 can be towed simultaneously. Has a closing system that inverts the forward portion of the net and draws mid-net section tight. A flowmeter can provide approximate volumes filtered. Mesh size not given [Wiebe and Benfield 2003 Plate 8 D].</skos:definition>
<owl:versionInfo>1</owl:versionInfo>
<dc:date>2011-10-21 14:18:49.0</dc:date>
<skos:note xml:lang="en">accepted</skos:note>
<owl:deprecated>false</owl:deprecated>
<skos:broader rdf:resource="http://vocab.nerc.ac.uk/collection/L05/current/22/"/>
<void:inDataset rdf:resource="http://vocab.nerc.ac.uk/.well-known/void"/>
</skos:Concept>
</skos:member>
<skos:member>
<skos:Concept rdf:about="http://vocab.nerc.ac.uk/collection/L22/current/TOOL0333/">
<dc:identifier>SDN:L22::TOOL0333</dc:identifier>
<skos:notation>SDN:L22::TOOL0333</skos:notation>
<skos:prefLabel xml:lang="en">Magee Scientific AE1 Aethalometer</skos:prefLabel>
<skos:altLabel>Magee AE1 Aethalometer</skos:altLabel>
<skos:definition xml:lang="en">The Magee Scientific AE1 Aethalometer determines concentration of light absorbing aerosol particles from measurements of light transmission through a sample. Air is filtered through a quartz fibre filter tape that traps particulate matter. Measurements are taken at user-specified time intervals ranging from one second to several minutes and the instrument outputs a voltage that is indicative of the amount of light absorbed by the sample.</skos:definition>
<owl:versionInfo>1</owl:versionInfo>
<dc:date>2010-09-06 12:45:22.0</dc:date>
<skos:note xml:lang="en">accepted</skos:note>
<owl:deprecated>false</owl:deprecated>
<skos:broader rdf:resource="http://vocab.nerc.ac.uk/collection/L05/current/387/"/>
<void:inDataset rdf:resource="http://vocab.nerc.ac.uk/.well-known/void"/>
</skos:Concept>
</skos:member>
<skos:member>
<skos:Concept rdf:about="http://vocab.nerc.ac.uk/collection/L22/current/TOOL0300/">
<dc:identifier>SDN:L22::TOOL0300</dc:identifier>
<skos:notation>SDN:L22::TOOL0300</skos:notation>
<skos:prefLabel xml:lang="en">Manchester Centre for Atmospheric Science Differential Mobility Particle Sizer</skos:prefLabel>
<skos:altLabel>Manchester CAS DMPS</skos:altLabel>
<skos:definition xml:lang="en">An in-situ instrument that gives size-resolved aerosol particle counts in the range 3.4 nm to 830 nm. The instrument comprises an ultrafine and a standard differential mobility analyser, and an ultrafine and a standard optical particle counter. It is a research mode instrument developed by the University of Manchester Centre for Atmospheric Science that is not in commercial production.</skos:definition>
<owl:versionInfo>1</owl:versionInfo>
<dc:date>2010-05-18 16:10:58.0</dc:date>
<skos:note xml:lang="en">accepted</skos:note>
<owl:deprecated>false</owl:deprecated>
<skos:broader rdf:resource="http://vocab.nerc.ac.uk/collection/L05/current/386/"/>
<void:inDataset rdf:resource="http://vocab.nerc.ac.uk/.well-known/void"/>
</skos:Concept>
</skos:member>
<skos:member>
<skos:Concept rdf:about="http://vocab.nerc.ac.uk/collection/L22/current/TOOL0352/">
<dc:identifier>SDN:L22::TOOL0352</dc:identifier>
<skos:notation>SDN:L22::TOOL0352</skos:notation>
<skos:prefLabel xml:lang="en">Manchester Centre for Atmospheric Science Hygroscopic Tandem Differential Mobility Analyser</skos:prefLabel>
<skos:altLabel>Manchester CAS HTDMA</skos:altLabel>
<skos:definition xml:lang="en">The Hygroscopic Tandem Differential Mobility Analyser (HTDMA) measures the changes in aerosol size distribution in response to a change in relative humidity. It uses two Differential Mobility Analysers (DMAs), operated in series. The incoming air sample is dried to &lt;10% relative humidity, and the first DMA selects a monodisperse distribution of a chosen size. The monodisperse subsample is humidified, and the second DMA, coupled to a particle counter, measures the size distribution of the humidified sample.</skos:definition>
<owl:versionInfo>1</owl:versionInfo>
<dc:date>2010-10-01 10:54:41.0</dc:date>
<skos:note xml:lang="en">accepted</skos:note>
<owl:deprecated>false</owl:deprecated>
<skos:broader rdf:resource="http://vocab.nerc.ac.uk/collection/L05/current/386/"/>
<void:inDataset rdf:resource="http://vocab.nerc.ac.uk/.well-known/void"/>
</skos:Concept>
</skos:member>
<skos:member>
<skos:Concept rdf:about="http://vocab.nerc.ac.uk/collection/L22/current/NETT0088/">
<dc:identifier>SDN:L22::NETT0088</dc:identifier>
<skos:notation>SDN:L22::NETT0088</skos:notation>
<skos:prefLabel xml:lang="en">Manta net - Brown and Cheng (1981)</skos:prefLabel>
<skos:altLabel>Manta net</skos:altLabel>
<skos:definition xml:lang="en">A rectangular framework 100 cm wide by 20 cm tall with a pair of wings that ride the sea surface and a pair of paravanes to guide the net away from the ship. Attached to the frame was a Bongo Net (240 cm circumference) with 505 um mesh.  A 100 kg weight was used to hold the asymmetrical bridle down below the surface so that the mouth opening was relatively free of towing lines. Equipped with a flow meter [Wiebe and Benfield 2003 Plate 21 A].</skos:definition>
<owl:versionInfo>1</owl:versionInfo>
<dc:date>2011-10-21 14:18:49.0</dc:date>
<skos:note xml:lang="en">accepted</skos:note>
<owl:deprecated>false</owl:deprecated>
<skos:broader rdf:resource="http://vocab.nerc.ac.uk/collection/L05/current/22/"/>
<skos:broader rdf:resource="http://vocab.nerc.ac.uk/collection/L05/current/388/"/>
<void:inDataset rdf:resource="http://vocab.nerc.ac.uk/.well-known/void"/>
</skos:Concept>
</skos:member>
<skos:member>
<skos:Concept rdf:about="http://vocab.nerc.ac.uk/collection/L22/current/TOOL0067/">
<dc:identifier>SDN:L22::TOOL0067</dc:identifier>
<skos:notation>SDN:L22::TOOL0067</skos:notation>
<skos:prefLabel xml:lang="en">Marcel Kruse PAR Spectrometer</skos:prefLabel>
<skos:altLabel>Marcel Kruse PAR Spectrometer</skos:altLabel>
<skos:definition xml:lang="en">Self-contained spectral radiometer manufactured by Ingenieurburo Marcel Kruse. It has a cosine diffusor and records radiation in the range of 400-700nm using a diode array. Depending on light intensities integration time ranges between 15ms to 16s for one spectrum. Storage capacity is 90 spectra.</skos:definition>
<owl:versionInfo>1</owl:versionInfo>
<dc:date>2009-11-30 11:56:35.0</dc:date>
<skos:note xml:lang="en">accepted</skos:note>
<owl:deprecated>false</owl:deprecated>
<skos:broader rdf:resource="http://vocab.nerc.ac.uk/collection/L05/current/122/"/>
<void:inDataset rdf:resource="http://vocab.nerc.ac.uk/.well-known/void"/>
</skos:Concept>
</skos:member>
<skos:member>
<skos:Concept rdf:about="http://vocab.nerc.ac.uk/collection/L22/current/TOOL0481/">
<dc:identifier>SDN:L22::TOOL0481</dc:identifier>
<skos:notation>SDN:L22::TOOL0481</skos:notation>
<skos:prefLabel xml:lang="en">Marianda VINDTA 3C total inorganic carbon and titration alkalinity analyser</skos:prefLabel>
<skos:altLabel>VINDTA 3C TIC and TA analyser</skos:altLabel>
<skos:definition xml:lang="en">The Versatile INstrument for the Determination of Total inorganic carbon and titration Alkalinity (VINDTA) 3C is a laboratory alkalinity titration system combined with an extraction unit for coulometric titration, which simultaneously determines the alkalinity and dissolved inorganic carbon content of a sample. The sample transport is performed with peristaltic pumps and acid is added to the sample using a membrane pump. No pressurizing system is required and only one gas supply (nitrogen or dry and CO2-free air) is necessary. The system uses a Metrohm Titrino 719S, an ORION-Ross pH electrode and a Metrohm reference electrode. The burette, the pipette and the analysis cell have a water jacket around them. Precision is typically ± 1 umol/kg for TA and/or DIC in open ocean water.</skos:definition>
<owl:versionInfo>1</owl:versionInfo>
<dc:date>2012-03-19 13:44:14.0</dc:date>
<skos:note xml:lang="en">accepted</skos:note>
<owl:deprecated>false</owl:deprecated>
<skos:broader rdf:resource="http://vocab.nerc.ac.uk/collection/L05/current/LAB12/"/>
<void:inDataset rdf:resource="http://vocab.nerc.ac.uk/.well-known/void"/>
</skos:Concept>
</skos:member>
<skos:member>
<skos:Concept rdf:about="http://vocab.nerc.ac.uk/collection/L22/current/TOOL0045/">
<dc:identifier>SDN:L22::TOOL0045</dc:identifier>
<skos:notation>SDN:L22::TOOL0045</skos:notation>
<skos:prefLabel xml:lang="en">Marine Electronics 3D Sand Ripple Profiling Logging Sonar</skos:prefLabel>
<skos:altLabel>Mar Elec 3D SRPLS</skos:altLabel>
<skos:definition xml:lang="en">A dual axis mechanically scanning sonar unit with a built in hard disk drive and associated controlling computer, powered by an external battery pack but is self-contained. The sonar has an oil-filled hemi-spherical plastic "boot" providing protection for its acoustic transducer which operates with a narrow conical beam pattern. Typically the sonar is mounted vertically, looking down at the sea-bed, and captures a sequence of profiles of the sea-bed over a pre-programmed sector and range. The sonar gathers a single swath of data in the horizontal plane and then rotates the transducer through a pre-programmed angle around the vertical axis and repeats the process until a circular area underneath the sonar has been scanned in a sequence of radial spokes. The raw data represents the signal amplitude of the envelope of the returned echoes. A suite of sensors to measure conductivity, temperature, depth, pitch and roll are also mounted on the instrument.</skos:definition>
<owl:versionInfo>1</owl:versionInfo>
<dc:date>2009-11-30 11:56:35.0</dc:date>
<skos:note xml:lang="en">accepted</skos:note>
<owl:deprecated>false</owl:deprecated>
<skos:broader rdf:resource="http://vocab.nerc.ac.uk/collection/L05/current/152/"/>
<void:inDataset rdf:resource="http://vocab.nerc.ac.uk/.well-known/void"/>
</skos:Concept>
</skos:member>
<skos:member>
<skos:Concept rdf:about="http://vocab.nerc.ac.uk/collection/L22/current/TOOL0046/">
<dc:identifier>SDN:L22::TOOL0046</dc:identifier>
<skos:notation>SDN:L22::TOOL0046</skos:notation>
<skos:prefLabel xml:lang="en">Marine Electronics Sand Ripple Profiling Sonar</skos:prefLabel>
<skos:altLabel>Mar Elec SRPS</skos:altLabel>
<skos:definition xml:lang="en">A single axis mechanically scanning sonar unit. The sonar has an oil-filled plastic "boot" providing protection for its acoustic transducer which operates with a narrow conical beam pattern.Typically the sonar is mounted vertically, looking down at the sea-bed, and captures a sequence of profiles of the sea-bed over a pre-programmed sector and range. The sonar gathers a single swath of data in the horizontal plane and then rotates the transducer through a pre-programmed angle around the vertical axis and repeats the process until a circular area underneath the sonar has been scanned in a sequence of radial spokes.</skos:definition>
<owl:versionInfo>1</owl:versionInfo>
<dc:date>2009-11-30 11:56:35.0</dc:date>
<skos:note xml:lang="en">accepted</skos:note>
<owl:deprecated>false</owl:deprecated>
<skos:broader rdf:resource="http://vocab.nerc.ac.uk/collection/L05/current/152/"/>
<void:inDataset rdf:resource="http://vocab.nerc.ac.uk/.well-known/void"/>
</skos:Concept>
</skos:member>
<skos:member>
<skos:Concept rdf:about="http://vocab.nerc.ac.uk/collection/L22/current/TOOL0474/">
<dc:identifier>SDN:L22::TOOL0474</dc:identifier>
<skos:notation>SDN:L22::TOOL0474</skos:notation>
<skos:prefLabel xml:lang="en">Marine Magnetics SeaSPY Marine Magnetometer</skos:prefLabel>
<skos:altLabel>SeaSPY magnetometer</skos:altLabel>
<skos:definition xml:lang="en">A marine magnetometer that measures the ambient magnetic field using a specialised branch of nuclear Magnetic Resonance technology applied to hydrogen nuclei. It uses an Overhauser sensor that allows omnidirectional data collection regardless of the direction of the ambient magnetic field. The sensor is accurate to 0.1 nT with a resolution of 0.01 nT. The magnetometer and associated electronics are held in a fibreglass towfish and the SeaSPY is available in three depth ratings: 1000 m, 3000 m and 6000 m. Optional extras include a pressure sensor, altimeter, transponder and side scan integration.</skos:definition>
<owl:versionInfo>1</owl:versionInfo>
<dc:date>2012-02-22 13:39:43.0</dc:date>
<skos:note xml:lang="en">accepted</skos:note>
<owl:deprecated>false</owl:deprecated>
<skos:broader rdf:resource="http://vocab.nerc.ac.uk/collection/L05/current/159/"/>
<void:inDataset rdf:resource="http://vocab.nerc.ac.uk/.well-known/void"/>
</skos:Concept>
</skos:member>
<skos:member>
<skos:Concept rdf:about="http://vocab.nerc.ac.uk/collection/L22/current/NETT0171/">
<dc:identifier>SDN:L22::NETT0171</dc:identifier>
<skos:notation>SDN:L22::NETT0171</skos:notation>
<skos:prefLabel xml:lang="en">Marine Scotland Opening Closing Environmental Acoustic Net MKI</skos:prefLabel>
<skos:altLabel>OCEAN MKI</skos:altLabel>
<skos:definition xml:lang="en">An oceanographic sampler designed to be towed behind a vessel. The sampler includes 4 nets which are controlled by acoustic signals from the towing ship. The system can be fitted with live codend buckets or codend bags. This version of the sampler has been supserseded.</skos:definition>
<owl:versionInfo>1</owl:versionInfo>
<dc:date>2012-09-25 14:08:12.0</dc:date>
<skos:note xml:lang="en">accepted</skos:note>
<owl:deprecated>false</owl:deprecated>
<skos:broader rdf:resource="http://vocab.nerc.ac.uk/collection/L05/current/22/"/>
<void:inDataset rdf:resource="http://vocab.nerc.ac.uk/.well-known/void"/>
</skos:Concept>
</skos:member>
<skos:member>
<skos:Concept rdf:about="http://vocab.nerc.ac.uk/collection/L22/current/NETT0172/">
<dc:identifier>SDN:L22::NETT0172</dc:identifier>
<skos:notation>SDN:L22::NETT0172</skos:notation>
<skos:prefLabel xml:lang="en">Marine Scotland Opening Closing Environmental Acoustic Net MKII</skos:prefLabel>
<skos:altLabel>OCEAN MKII</skos:altLabel>
<skos:definition xml:lang="en">An oceanographic sampler designed to be towed behind a vessel at a rate of 2-4 knots. The sampler includes 7 nets with mouth openings of 10cm internal and 160cms long. The nets are mounted in a removable stainless steel frame, which fits into the main stainless steel sampler frame, and can be changed to suit sampling requirements. The system can be fitted with live codend buckets or codend bags of similar mesh to the sampling nets. The system is pre-programmed using a computer which allocates depths where the sampler will activate.The operator can elect to sample down and up through the water column or only on the down leg or up leg. The  main nose cone contains a Marine Scotland titanium flowmeter whose measurements are recorded on a data logger. The system also contains a motor that controls the opening and closing of nets. The system also normally carries 7 water sampling bottles, an optical plankton counter and an SBE911 CTD fitted with transmissometer and fluorometer. The sampler is rated to 1000 m and can carry up to 250kg of other instrumentation.</skos:definition>
<owl:versionInfo>1</owl:versionInfo>
<dc:date>2012-09-25 14:08:12.0</dc:date>
<skos:note xml:lang="en">accepted</skos:note>
<owl:deprecated>false</owl:deprecated>
<skos:broader rdf:resource="http://vocab.nerc.ac.uk/collection/L05/current/388/"/>
<skos:broader rdf:resource="http://vocab.nerc.ac.uk/collection/L05/current/22/"/>
<void:inDataset rdf:resource="http://vocab.nerc.ac.uk/.well-known/void"/>
</skos:Concept>
</skos:member>
<skos:member>
<skos:Concept rdf:about="http://vocab.nerc.ac.uk/collection/L22/current/TOOL0535/">
<dc:identifier>SDN:L22::TOOL0535</dc:identifier>
<skos:notation>SDN:L22::TOOL0535</skos:notation>
<skos:prefLabel xml:lang="en">Marine Scotland Opening Closing Environmental Acoustic Net water bottle</skos:prefLabel>
<skos:altLabel>OCEAN water sample bottle</skos:altLabel>
<skos:definition xml:lang="en">A custom made water sampling bottle designed to fit on the OCEAN sampler. The bottle comprises a free-flooding tube with a capacity of 0.5 litres. The bottle closes when a net sample is collected. Bottle firing is pre-programmed using a computer prior to deployment of the sampler.</skos:definition>
<owl:versionInfo>1</owl:versionInfo>
<dc:date>2012-09-25 14:01:15.0</dc:date>
<skos:note xml:lang="en">accepted</skos:note>
<owl:deprecated>false</owl:deprecated>
<skos:broader rdf:resource="http://vocab.nerc.ac.uk/collection/L05/current/30/"/>
<void:inDataset rdf:resource="http://vocab.nerc.ac.uk/.well-known/void"/>
</skos:Concept>
</skos:member>
<skos:member>
<skos:Concept rdf:about="http://vocab.nerc.ac.uk/collection/L22/current/TOOL0057/">
<dc:identifier>SDN:L22::TOOL0057</dc:identifier>
<skos:notation>SDN:L22::TOOL0057</skos:notation>
<skos:prefLabel xml:lang="en">Marsh McBirney 585 OEM electromagnetic flowmeter</skos:prefLabel>
<skos:altLabel>Marsh McBirney 585 EMCM</skos:altLabel>
<skos:definition xml:lang="en">A rugged solid-state electromagnetic current sensor designed to measure horizontal currents with minimal interference from vertical flow. Manufactured between 1976 and 1992 by Marsh McBirney, now part of Hashflow. The OEM 585 was a dual-axis unit with a 4-inch sensor able to measure currents up to 3 ms-1 with 2% accuracy and a resolution of 0.0018 ms-1. It was supplied as a sensor plus associated electronic unit rather than packaged into a self-contained current meter.</skos:definition>
<owl:versionInfo>1</owl:versionInfo>
<dc:date>2012-11-20 14:50:06.0</dc:date>
<skos:note xml:lang="en">accepted</skos:note>
<owl:deprecated>false</owl:deprecated>
<skos:broader rdf:resource="http://vocab.nerc.ac.uk/collection/L05/current/114/"/>
<void:inDataset rdf:resource="http://vocab.nerc.ac.uk/.well-known/void"/>
</skos:Concept>
</skos:member>
<skos:member>
<skos:Concept rdf:about="http://vocab.nerc.ac.uk/collection/L22/current/NETT0090/">
<dc:identifier>SDN:L22::NETT0090</dc:identifier>
<skos:notation>SDN:L22::NETT0090</skos:notation>
<skos:prefLabel xml:lang="en">Maruchi conical nets - Nakai (1962)</skos:prefLabel>
<skos:altLabel>Maruchi nets</skos:altLabel>
<skos:definition xml:lang="en">Construction comprises a 130 cm diameter mouth opening with 450 cm long net. There were a series of variants MCA-MCE.</skos:definition>
<owl:versionInfo>1</owl:versionInfo>
<dc:date>2011-10-21 14:18:49.0</dc:date>
<skos:note xml:lang="en">accepted</skos:note>
<owl:deprecated>false</owl:deprecated>
<skos:broader rdf:resource="http://vocab.nerc.ac.uk/collection/L05/current/22/"/>
<void:inDataset rdf:resource="http://vocab.nerc.ac.uk/.well-known/void"/>
</skos:Concept>
</skos:member>
<skos:member>
<skos:Concept rdf:about="http://vocab.nerc.ac.uk/collection/L22/current/NETT0091/">
<dc:identifier>SDN:L22::NETT0091</dc:identifier>
<skos:notation>SDN:L22::NETT0091</skos:notation>
<skos:prefLabel xml:lang="en">Marudai - Nakai (1962)</skos:prefLabel>
<skos:altLabel>Marudai</skos:altLabel>
<skos:definition xml:lang="en">Construction comprises a 250 cm diameter mouth opening with 800 cm long net.  A series of variants designed to sample megaplankton and nekton (MDA, MDB, PMD)</skos:definition>
<owl:versionInfo>1</owl:versionInfo>
<dc:date>2011-10-21 14:18:49.0</dc:date>
<skos:note xml:lang="en">accepted</skos:note>
<owl:deprecated>false</owl:deprecated>
<skos:broader rdf:resource="http://vocab.nerc.ac.uk/collection/L05/current/22/"/>
<void:inDataset rdf:resource="http://vocab.nerc.ac.uk/.well-known/void"/>
</skos:Concept>
</skos:member>
<skos:member>
<skos:Concept rdf:about="http://vocab.nerc.ac.uk/collection/L22/current/NETT0092/">
<dc:identifier>SDN:L22::NETT0092</dc:identifier>
<skos:notation>SDN:L22::NETT0092</skos:notation>
<skos:prefLabel xml:lang="en">Marunaka - Nakai (1962)</skos:prefLabel>
<skos:altLabel>Marunaka</skos:altLabel>
<skos:definition xml:lang="en">Has a 60 cm diameter mouth opening  cylinder/cone design. Cylinder coarse mesh (3.3 cm) 33 cm long.  Conical portion silk net 150 cm long. Can accommodate flowmeter. Sometimes rigged as Nansen closing net. Variants listed as MNA, MNB.</skos:definition>
<owl:versionInfo>1</owl:versionInfo>
<dc:date>2011-10-21 14:18:49.0</dc:date>
<skos:note xml:lang="en">accepted</skos:note>
<owl:deprecated>false</owl:deprecated>
<skos:broader rdf:resource="http://vocab.nerc.ac.uk/collection/L05/current/22/"/>
<void:inDataset rdf:resource="http://vocab.nerc.ac.uk/.well-known/void"/>
</skos:Concept>
</skos:member>
<skos:member>
<skos:Concept rdf:about="http://vocab.nerc.ac.uk/collection/L22/current/NETT0093/">
<dc:identifier>SDN:L22::NETT0093</dc:identifier>
<skos:notation>SDN:L22::NETT0093</skos:notation>
<skos:prefLabel xml:lang="en">Marutoku - Nakai (1962)</skos:prefLabel>
<skos:altLabel>Marutoku</skos:altLabel>
<skos:definition xml:lang="en">Has a 45 cm diameter mouth opening with cylinder/cone design - similar to International Standard Net (MTA) - sometimes rigged as Nansen closing net. Cylinder coarse mesh; conical section 80cm silk mesh netting.  MTB- similar to above, but with flowmeter [Wiebe and Benfield 2003 Plate 3 A, B].</skos:definition>
<owl:versionInfo>1</owl:versionInfo>
<dc:date>2011-10-21 14:18:49.0</dc:date>
<skos:note xml:lang="en">accepted</skos:note>
<owl:deprecated>false</owl:deprecated>
<skos:broader rdf:resource="http://vocab.nerc.ac.uk/collection/L05/current/388/"/>
<skos:broader rdf:resource="http://vocab.nerc.ac.uk/collection/L05/current/22/"/>
<void:inDataset rdf:resource="http://vocab.nerc.ac.uk/.well-known/void"/>
</skos:Concept>
</skos:member>
<skos:member>
<skos:Concept rdf:about="http://vocab.nerc.ac.uk/collection/L22/current/NETT0042/">
<dc:identifier>SDN:L22::NETT0042</dc:identifier>
<skos:notation>SDN:L22::NETT0042</skos:notation>
<skos:prefLabel xml:lang="en">Mechanically opening-closing epi-benthic plankton sled - Wickstead (1953)</skos:prefLabel>
<skos:altLabel>Wickstead epi-benthic sled</skos:altLabel>
<skos:definition xml:lang="en">Construction is a 61 cm x 30 cm rectangular mouth opening : length of net or mesh size not given [Wiebe and Benfield 2003 Plate 22 D].</skos:definition>
<owl:versionInfo>1</owl:versionInfo>
<dc:date>2011-10-21 14:18:49.0</dc:date>
<skos:note xml:lang="en">accepted</skos:note>
<owl:deprecated>false</owl:deprecated>
<skos:broader rdf:resource="http://vocab.nerc.ac.uk/collection/L05/current/24/"/>
<skos:broader rdf:resource="http://vocab.nerc.ac.uk/collection/L05/current/22/"/>
<void:inDataset rdf:resource="http://vocab.nerc.ac.uk/.well-known/void"/>
</skos:Concept>
</skos:member>
<skos:member>
<skos:Concept rdf:about="http://vocab.nerc.ac.uk/collection/L22/current/TOOL0438/">
<dc:identifier>SDN:L22::TOOL0438</dc:identifier>
<skos:notation>SDN:L22::TOOL0438</skos:notation>
<skos:prefLabel xml:lang="en">Meerestechnik Elektronik or MICSOS microstructure profiler</skos:prefLabel>
<skos:altLabel>MST/MICSOS microstructure profiler</skos:altLabel>
<skos:definition xml:lang="en">A free sinking or rising multi-parameter probe equipped with high resolution temperature and current shear sensors for microstructure observations and precision CTD sensors for standard hydrography. The shear is measured by an aero-foil-shaped shear probe with an overall time constant of 4 ms. The high resolution temperature probe works with a Negative Temperature Coefficient (NTC) sensor which has an overall time constant of about 10 ms.The sampling rates of the sensors are about 1 kHz. An internal vibration sensor compensates for vibrations of the profiler itself. The data are transmitted via a fast link to a computer on the mother ship. The descent rate of the profiler can be adjusted to the surrounding water density by removable weights. The CTD sensors are a piezo-resistive pressure sensor, Platinum resistance thermometer and 7-Pole conductivity cell. The profiler was developed in the framework of the MICSOS project and is often called the 'MICSOS profiler'. The MST System consists of the profiler, a neutrally-buoyant cable for data transmission, a data and power supply interface, and a logger. Only 3 MST profilers were ever built. Meerestechnik Elektronik no longer exists but the instrument is supported by ISW Wassermesstechnik.</skos:definition>
<owl:versionInfo>1</owl:versionInfo>
<dc:date>2011-11-07 15:23:52.0</dc:date>
<skos:note xml:lang="en">accepted</skos:note>
<owl:deprecated>false</owl:deprecated>
<skos:broader rdf:resource="http://vocab.nerc.ac.uk/collection/L05/current/350/"/>
<skos:broader rdf:resource="http://vocab.nerc.ac.uk/collection/L05/current/384/"/>
<skos:broader rdf:resource="http://vocab.nerc.ac.uk/collection/L05/current/134/"/>
<void:inDataset rdf:resource="http://vocab.nerc.ac.uk/.well-known/void"/>
</skos:Concept>
</skos:member>
<skos:member>
<skos:Concept rdf:about="http://vocab.nerc.ac.uk/collection/L22/current/TOOL0149/">
<dc:identifier>SDN:L22::TOOL0149</dc:identifier>
<skos:notation>SDN:L22::TOOL0149</skos:notation>
<skos:prefLabel xml:lang="en">Meerestechnik OTS-1200 CTD</skos:prefLabel>
<skos:altLabel>OTS-1200 CTD</skos:altLabel>
<skos:definition xml:lang="en">An integral unit comprising pressure, temperature and conductivity sensors.</skos:definition>
<owl:versionInfo>1</owl:versionInfo>
<dc:date>2010-05-18 16:10:58.0</dc:date>
<skos:note xml:lang="en">accepted</skos:note>
<owl:deprecated>false</owl:deprecated>
<skos:related rdf:resource="http://vocab.nerc.ac.uk/collection/P01/current/POTMCV01/"/>
<skos:related rdf:resource="http://vocab.nerc.ac.uk/collection/P01/current/PSALST01/"/>
<skos:related rdf:resource="http://vocab.nerc.ac.uk/collection/P01/current/TEMPST01/"/>
<skos:related rdf:resource="http://vocab.nerc.ac.uk/collection/P01/current/PRESPR01/"/>
<skos:related rdf:resource="http://vocab.nerc.ac.uk/collection/P01/current/SIGTPR01/"/>
<skos:broader rdf:resource="http://vocab.nerc.ac.uk/collection/L05/current/130/"/>
<skos:broader rdf:resource="http://vocab.nerc.ac.uk/collection/L05/current/134/"/>
<skos:broader rdf:resource="http://vocab.nerc.ac.uk/collection/L05/current/350/"/>
<void:inDataset rdf:resource="http://vocab.nerc.ac.uk/.well-known/void"/>
</skos:Concept>
</skos:member>
<skos:member>
<skos:Concept rdf:about="http://vocab.nerc.ac.uk/collection/L22/current/TOOL0238/">
<dc:identifier>SDN:L22::TOOL0238</dc:identifier>
<skos:notation>SDN:L22::TOOL0238</skos:notation>
<skos:prefLabel xml:lang="en">Mercury reversing thermometer</skos:prefLabel>
<skos:altLabel>Hg RTM</skos:altLabel>
<skos:definition xml:lang="en">A generic term for a mercury-in-glass thermometer that freezes the temperature reading when turned upside-down.</skos:definition>
<owl:versionInfo>1</owl:versionInfo>
<dc:date>2010-05-18 16:10:58.0</dc:date>
<skos:note xml:lang="en">accepted</skos:note>
<owl:deprecated>false</owl:deprecated>
<skos:broader rdf:resource="http://vocab.nerc.ac.uk/collection/L05/current/134/"/>
<void:inDataset rdf:resource="http://vocab.nerc.ac.uk/.well-known/void"/>
</skos:Concept>
</skos:member>
<skos:member>
<skos:Concept rdf:about="http://vocab.nerc.ac.uk/collection/L22/current/NETT0159/">
<dc:identifier>SDN:L22::NETT0159</dc:identifier>
<skos:notation>SDN:L22::NETT0159</skos:notation>
<skos:prefLabel xml:lang="en">Messenger-operated Tucker Trawl - Hopkins et al. (1973)</skos:prefLabel>
<skos:altLabel>Hopkins modified Tucker Trawl</skos:altLabel>
<skos:definition xml:lang="en">A 180 cm x 180 cm rectangular mouth opening Tucker trawl with a double messenger activated release mechanism made by General Oceanics. Net is made from 1.1 cm mesh for first 500 cm and 0.33 mm nylon mesh for last 2 meters.  Flow measured with a TSK flowmeter and a time-depth recorder is used to log net trajectory.  Also used with trawl with 180 cm x 360 cm mouth opening. Tow speeds generally are between 2and 2.5 knots [Wiebe and Benfield 2003 Plate 6 C].</skos:definition>
<owl:versionInfo>1</owl:versionInfo>
<dc:date>2011-10-21 14:18:49.0</dc:date>
<skos:note xml:lang="en">accepted</skos:note>
<owl:deprecated>false</owl:deprecated>
<skos:broader rdf:resource="http://vocab.nerc.ac.uk/collection/L05/current/23/"/>
<skos:broader rdf:resource="http://vocab.nerc.ac.uk/collection/L05/current/388/"/>
<void:inDataset rdf:resource="http://vocab.nerc.ac.uk/.well-known/void"/>
</skos:Concept>
</skos:member>
<skos:member>
<skos:Concept rdf:about="http://vocab.nerc.ac.uk/collection/L22/current/NETT0160/">
<dc:identifier>SDN:L22::NETT0160</dc:identifier>
<skos:notation>SDN:L22::NETT0160</skos:notation>
<skos:prefLabel xml:lang="en">Messenger-operated Tucker Trawl - Sameoto and Jaroszynski (1976)</skos:prefLabel>
<skos:altLabel>Sameoto modified Tucker Trawl</skos:altLabel>
<skos:definition xml:lang="en">A 100 cm x 100 cm and a 400 cm x 400 cm rectangular mouth opening Tucker trawl with a double messenger activated release mechanism. Net is made from coarse mesh.  Flow measured with a digital flowmeter.  A depressor plate is mounted on bottom net bar.  Tow speeds generally are between 2 and 4 knots [Wiebe and Benfield 2003 Plate 6 D].</skos:definition>
<owl:versionInfo>1</owl:versionInfo>
<dc:date>2011-10-21 14:18:49.0</dc:date>
<skos:note xml:lang="en">accepted</skos:note>
<owl:deprecated>false</owl:deprecated>
<skos:broader rdf:resource="http://vocab.nerc.ac.uk/collection/L05/current/388/"/>
<skos:broader rdf:resource="http://vocab.nerc.ac.uk/collection/L05/current/23/"/>
<void:inDataset rdf:resource="http://vocab.nerc.ac.uk/.well-known/void"/>
</skos:Concept>
</skos:member>
<skos:member>
<skos:Concept rdf:about="http://vocab.nerc.ac.uk/collection/L22/current/TOOL0515/">
<dc:identifier>SDN:L22::TOOL0515</dc:identifier>
<skos:notation>SDN:L22::TOOL0515</skos:notation>
<skos:prefLabel xml:lang="en">Metrohm 663 VA Stand mercury electrode</skos:prefLabel>
<skos:altLabel>Metrohm 663 VA</skos:altLabel>
<skos:definition xml:lang="en">The Metrohm 663 VA stand forms the wet chemical part of a polarographic and voltammetric analytical system. It features a mercury electrode, an Ag/AgCl reference electrode and a glassy carbon counter electrode. The size of the mercury drop and the stirrer speed are set manually on the VA Stand. The VA Stand can be operated in Dropping Mercury Electrode (DME), Hanging Mercury Drop Electrode (HMDE) and Static Mercury Drop Electrode (SMDE) modes. The VA Stand can be controlled by a potentiostat in conjunction with the Metrohm IME663 interface.</skos:definition>
<owl:versionInfo>1</owl:versionInfo>
<dc:date>2012-07-04 10:02:10.0</dc:date>
<skos:note xml:lang="en">accepted</skos:note>
<owl:deprecated>false</owl:deprecated>
<skos:broader rdf:resource="http://vocab.nerc.ac.uk/collection/L05/current/LAB35/"/>
<void:inDataset rdf:resource="http://vocab.nerc.ac.uk/.well-known/void"/>
</skos:Concept>
</skos:member>
<skos:member>
<skos:Concept rdf:about="http://vocab.nerc.ac.uk/collection/L22/current/TOOL0633/">
<dc:identifier>SDN:L22::TOOL0633</dc:identifier>
<skos:notation>SDN:L22::TOOL0633</skos:notation>
<skos:prefLabel xml:lang="en">Metrohm 716 DMS Titrino</skos:prefLabel>
<skos:altLabel>Metrohm 716</skos:altLabel>
<skos:definition xml:lang="en">A titrator used for dynamic and monotonic titrations. The instrument consists of an exchange unit, a magnetic stirer, and a live display. It measures pH in the range -20 to 20, voltage in the range -2000 to 2000 mV, and current in the range -200 to 200 uA. Temperature is measured by either Pt1000 or Pt100 in the range -150 to 450 degC.</skos:definition>
<owl:versionInfo>1</owl:versionInfo>
<dc:date>2013-07-31 14:01:26.0</dc:date>
<skos:note xml:lang="en">accepted</skos:note>
<owl:deprecated>false</owl:deprecated>
<skos:broader rdf:resource="http://vocab.nerc.ac.uk/collection/L05/current/LAB12/"/>
<void:inDataset rdf:resource="http://vocab.nerc.ac.uk/.well-known/void"/>
</skos:Concept>
</skos:member>
<skos:member>
<skos:Concept rdf:about="http://vocab.nerc.ac.uk/collection/L22/current/TOOL0572/">
<dc:identifier>SDN:L22::TOOL0572</dc:identifier>
<skos:notation>SDN:L22::TOOL0572</skos:notation>
<skos:prefLabel xml:lang="en">Metrohm 765 Dosimat Burette</skos:prefLabel>
<skos:altLabel>Metrohm 765 Dosimat</skos:altLabel>
<skos:definition xml:lang="en">A dispensing instrument for titrating and dosing operations in the laboratory. The instrument includes the following functions: automatic preparation of standard solutions; pipetting, diluting and dispensing; calculation of results. Dispensing rates of between 0.001 mL/min and 150 mL/min can be selected alongside pippetting volumes of between 0.001 mL/min and 150 mL/min. The 765 Dosimat is an upgrade of the 776 model, with additional features including automatic dosing test; tandem dispensing with a second Dosimat; data connection for a balance, computer or printer; remote control; and optional analogue output.</skos:definition>
<owl:versionInfo>1</owl:versionInfo>
<dc:date>2012-11-19 17:07:42.0</dc:date>
<skos:note xml:lang="en">accepted</skos:note>
<owl:deprecated>false</owl:deprecated>
<skos:broader rdf:resource="http://vocab.nerc.ac.uk/collection/L05/current/LAB40/"/>
<void:inDataset rdf:resource="http://vocab.nerc.ac.uk/.well-known/void"/>
</skos:Concept>
</skos:member>
<skos:member>
<skos:Concept rdf:about="http://vocab.nerc.ac.uk/collection/L22/current/TOOL0595/">
<dc:identifier>SDN:L22::TOOL0595</dc:identifier>
<skos:notation>SDN:L22::TOOL0595</skos:notation>
<skos:prefLabel xml:lang="en">Metrohm 794 Basic Titrino Titrator</skos:prefLabel>
<skos:altLabel>Metrohm 794 Basic Titrino</skos:altLabel>
<skos:definition xml:lang="en">A titrator used for dynamic and monotonic titrations. The instrument consists of an exchange unit, a magnetic or propellor stirrer, a small display and remote control. The instrument measures pH in the range -20 to 20 (resolution 0.01), voltage in the range -2000 to 2000 mV (resolution 1 mV), current in the range -200 to 200 uA (resolution 1 uA), and temperature in the range -150 to 450 degC (resolution 1 degC).</skos:definition>
<owl:versionInfo>1</owl:versionInfo>
<dc:date>2013-01-25 11:59:48.0</dc:date>
<skos:note xml:lang="en">accepted</skos:note>
<owl:deprecated>false</owl:deprecated>
<skos:broader rdf:resource="http://vocab.nerc.ac.uk/collection/L05/current/LAB12/"/>
<void:inDataset rdf:resource="http://vocab.nerc.ac.uk/.well-known/void"/>
</skos:Concept>
</skos:member>
<skos:member>
<skos:Concept rdf:about="http://vocab.nerc.ac.uk/collection/L22/current/TOOL0568/">
<dc:identifier>SDN:L22::TOOL0568</dc:identifier>
<skos:notation>SDN:L22::TOOL0568</skos:notation>
<skos:prefLabel xml:lang="en">Metrohm 848 Titrino Plus Titrator</skos:prefLabel>
<skos:altLabel>Metrohm 848 Titrino Plus</skos:altLabel>
<skos:definition xml:lang="en">A titrator used for dynamic and monotonic titrations. The instrument consists of an exchange unit, a magnetic or propellor stirrer, and a large, live display. It measures pH in the range -13 to 20 (resolution 0.001), voltage in the range -1200 to 1200 mV (resolution 0.1 mV), and current in the range -120 to 120 uA (resolution 1 uA). Teperature is measured by either Pt1000 (range -150 to 250 degC, resolution 0.1 degC, accuracy +/- 0.2 degC), or NTC (range -5 to 250 degC, resolution 0.1 degC, accuracy +/- 0.6 degC).</skos:definition>
<owl:versionInfo>2</owl:versionInfo>
<dc:date>2013-01-25 11:58:57.0</dc:date>
<skos:note xml:lang="en">accepted</skos:note>
<owl:deprecated>false</owl:deprecated>
<skos:broader rdf:resource="http://vocab.nerc.ac.uk/collection/L05/current/LAB12/"/>
<void:inDataset rdf:resource="http://vocab.nerc.ac.uk/.well-known/void"/>
</skos:Concept>
</skos:member>
<skos:member>
<skos:Concept rdf:about="http://vocab.nerc.ac.uk/collection/L22/current/TOOL0514/">
<dc:identifier>SDN:L22::TOOL0514</dc:identifier>
<skos:notation>SDN:L22::TOOL0514</skos:notation>
<skos:prefLabel xml:lang="en">Metrohm microAutolab type 2 potentiostat/galvanostat</skos:prefLabel>
<skos:altLabel>Metrohm microAutolab 2</skos:altLabel>
<skos:definition xml:lang="en">A computer-controlled compact potentiostat/galvanostat for electrochemical research and electroanalysis. It has a potentiostat bandwidth of 500 kHz, an input impedance of &gt;100 GOhm and features an analog integrator. The instrument can supply a maximum current of 80 mA with an accuracy of 0.2% and a resolution of 0.0003%. Potential accuracy is 0.2% and potential resolution is 3 uV.  The instrument can perform almost all elelctrochemical techniques including voltammetry, fuel cell, battery, biosensors, electroplating, coatings and corrosion. It has an external USB interface and is controlled by NOVA software.</skos:definition>
<owl:versionInfo>1</owl:versionInfo>
<dc:date>2012-07-04 10:02:10.0</dc:date>
<skos:note xml:lang="en">accepted</skos:note>
<owl:deprecated>false</owl:deprecated>
<skos:broader rdf:resource="http://vocab.nerc.ac.uk/collection/L05/current/LAB35/"/>
<void:inDataset rdf:resource="http://vocab.nerc.ac.uk/.well-known/void"/>
</skos:Concept>
</skos:member>
<skos:member>
<skos:Concept rdf:about="http://vocab.nerc.ac.uk/collection/L22/current/TOOL0471/">
<dc:identifier>SDN:L22::TOOL0471</dc:identifier>
<skos:notation>SDN:L22::TOOL0471</skos:notation>
<skos:prefLabel xml:lang="en">Mettler AE240 dual range analytical balance</skos:prefLabel>
<skos:altLabel>AE240 analytical balance</skos:altLabel>
<skos:definition xml:lang="en">A laboratory instrument used to measure sample mass over the range 0-40 g or 0-200 g. The 40 g range has a readability of 0.01 mg, a reproducibility standard deviation of 0.02 mg and a typical stabilisation time of 8 sec, while the 200 g range has a readability of 0.1 mg, reproducibility standard devation of 0.1 mg and typical stabilisation time of 5 sec. This model is no longer in production.</skos:definition>
<owl:versionInfo>1</owl:versionInfo>
<dc:date>2012-02-21 16:06:42.0</dc:date>
<skos:note xml:lang="en">accepted</skos:note>
<owl:deprecated>false</owl:deprecated>
<skos:broader rdf:resource="http://vocab.nerc.ac.uk/collection/L05/current/LAB13/"/>
<void:inDataset rdf:resource="http://vocab.nerc.ac.uk/.well-known/void"/>
</skos:Concept>
</skos:member>
<skos:member>
<skos:Concept rdf:about="http://vocab.nerc.ac.uk/collection/L22/current/NETT0094/">
<dc:identifier>SDN:L22::NETT0094</dc:identifier>
<skos:notation>SDN:L22::NETT0094</skos:notation>
<skos:prefLabel xml:lang="en">Micronketon net - Blackburn and Keith (1962)</skos:prefLabel>
<skos:altLabel>Blackburn micronketon net</skos:altLabel>
<skos:definition xml:lang="en">A 152 cm x 152 cm rectangular mouth opening net attached to metal tube frame with Isaacs depressors attached to bottom corners. Net was 579 cm long made of 5.5 x 2.5 mm rectangular nylon mesh. Towed at speeds of 5 knots. A bathythermograph attached to the top frame member provide a temperature-depth trace for a tow. Not ordinarily used with a flowmeter [Wiebe and Benfield 2003 Plate 4 C, D].</skos:definition>
<owl:versionInfo>1</owl:versionInfo>
<dc:date>2011-10-21 14:18:49.0</dc:date>
<skos:note xml:lang="en">accepted</skos:note>
<owl:deprecated>false</owl:deprecated>
<skos:broader rdf:resource="http://vocab.nerc.ac.uk/collection/L05/current/134/"/>
<skos:broader rdf:resource="http://vocab.nerc.ac.uk/collection/L05/current/22/"/>
<void:inDataset rdf:resource="http://vocab.nerc.ac.uk/.well-known/void"/>
</skos:Concept>
</skos:member>
<skos:member>
<skos:Concept rdf:about="http://vocab.nerc.ac.uk/collection/L22/current/TOOL0012/">
<dc:identifier>SDN:L22::TOOL0012</dc:identifier>
<skos:notation>SDN:L22::TOOL0012</skos:notation>
<skos:prefLabel xml:lang="en">Mid-tide bubbler tide gauge</skos:prefLabel>
<skos:altLabel>Mid-tide bubbler</skos:altLabel>
<skos:definition xml:lang="en">The operation of the mid tide bubbler is similar to that of the full tide system, except that the measuring point is mounted at the mid tide height. This means that the pressure point is only immersed for half of the tidal cycle. The reason for this is that when the measuring point is exposed it can be accurately levelled into the geodetic network. Once this is accomplished the full tide pressure points can be fitted to match the tidal curve produced by the mid tide pressure point, thereby connecting them to the geodetic network.</skos:definition>
<owl:versionInfo>1</owl:versionInfo>
<dc:date>2009-11-30 11:27:51.0</dc:date>
<skos:note xml:lang="en">accepted</skos:note>
<owl:deprecated>false</owl:deprecated>
<skos:broader rdf:resource="http://vocab.nerc.ac.uk/collection/L05/current/111/"/>
<void:inDataset rdf:resource="http://vocab.nerc.ac.uk/.well-known/void"/>
</skos:Concept>
</skos:member>
<skos:member>
<skos:Concept rdf:about="http://vocab.nerc.ac.uk/collection/L22/current/NETT0095/">
<dc:identifier>SDN:L22::NETT0095</dc:identifier>
<skos:notation>SDN:L22::NETT0095</skos:notation>
<skos:prefLabel xml:lang="en">Midwater net - Fowler (1898)</skos:prefLabel>
<skos:altLabel>Fowler midwater net</skos:altLabel>
<skos:definition xml:lang="en">A 11.4 cm x 11.4 cm rectangular net mouth frame which was hinged at the central axis.  It was equipped with a silk net ( 9.8 or 15.7 meshes per cm) which was enclosed by a similar net made from mosquito netting. This net was sent down closed, opened by a messenger and closed by a second one.  Designed for vertical towing.</skos:definition>
<owl:versionInfo>1</owl:versionInfo>
<dc:date>2011-10-21 14:18:49.0</dc:date>
<skos:note xml:lang="en">accepted</skos:note>
<owl:deprecated>false</owl:deprecated>
<skos:broader rdf:resource="http://vocab.nerc.ac.uk/collection/L05/current/22/"/>
<void:inDataset rdf:resource="http://vocab.nerc.ac.uk/.well-known/void"/>
</skos:Concept>
</skos:member>
<skos:member>
<skos:Concept rdf:about="http://vocab.nerc.ac.uk/collection/L22/current/NETT0096/">
<dc:identifier>SDN:L22::NETT0096</dc:identifier>
<skos:notation>SDN:L22::NETT0096</skos:notation>
<skos:prefLabel xml:lang="en">Midwater neuston trawl - Zaitsev (1970)</skos:prefLabel>
<skos:altLabel>Zaitsev MNT</skos:altLabel>
<skos:definition xml:lang="en">Construction is an elliptical metal frame 100 cm wide x 50 cm tall with a net 400 cm long made of netting with Nos. 21-23 meshes. Two plastic foam floats (25 cm x 12 cm x 8 cm) are attached to each side of the net frame. The net is towed in a circle at about 4 knots.</skos:definition>
<owl:versionInfo>1</owl:versionInfo>
<dc:date>2011-10-21 14:18:49.0</dc:date>
<skos:note xml:lang="en">accepted</skos:note>
<owl:deprecated>false</owl:deprecated>
<skos:broader rdf:resource="http://vocab.nerc.ac.uk/collection/L05/current/69/"/>
<void:inDataset rdf:resource="http://vocab.nerc.ac.uk/.well-known/void"/>
</skos:Concept>
</skos:member>
<skos:member>
<skos:Concept rdf:about="http://vocab.nerc.ac.uk/collection/L22/current/NETT0115/">
<dc:identifier>SDN:L22::NETT0115</dc:identifier>
<skos:notation>SDN:L22::NETT0115</skos:notation>
<skos:prefLabel xml:lang="en">Mini-neuston net - Schram et al. (1981)</skos:prefLabel>
<skos:altLabel>Schram neuston net</skos:altLabel>
<skos:definition xml:lang="en">Neuston sampling system with three nets having a 60x20 cm rectangular mouth and 250 cm long.</skos:definition>
<owl:versionInfo>1</owl:versionInfo>
<dc:date>2011-10-21 14:18:49.0</dc:date>
<skos:note xml:lang="en">accepted</skos:note>
<owl:deprecated>false</owl:deprecated>
<skos:broader rdf:resource="http://vocab.nerc.ac.uk/collection/L05/current/69/"/>
<void:inDataset rdf:resource="http://vocab.nerc.ac.uk/.well-known/void"/>
</skos:Concept>
</skos:member>
<skos:member>
<skos:Concept rdf:about="http://vocab.nerc.ac.uk/collection/L22/current/NETT0136/">
<dc:identifier>SDN:L22::NETT0136</dc:identifier>
<skos:notation>SDN:L22::NETT0136</skos:notation>
<skos:prefLabel xml:lang="en">Miniature Plankton Indicator  - Henderson et al. (1936); Glover (1953)</skos:prefLabel>
<skos:altLabel>Henderson MPI</skos:altLabel>
<skos:definition xml:lang="en">This indicator had a body length of 33 cm, a diameter of 3.8 cm, an aperture diameter of 1.27 cm, a filter disc of 2.54 cm in diameter and was towed at about 2 knots [Wiebe and Benfield 2003 Plate 13 F].</skos:definition>
<owl:versionInfo>1</owl:versionInfo>
<dc:date>2011-10-21 14:18:49.0</dc:date>
<skos:note xml:lang="en">accepted</skos:note>
<owl:deprecated>false</owl:deprecated>
<skos:broader rdf:resource="http://vocab.nerc.ac.uk/collection/L05/current/22/"/>
<void:inDataset rdf:resource="http://vocab.nerc.ac.uk/.well-known/void"/>
</skos:Concept>
</skos:member>
<skos:member>
<skos:Concept rdf:about="http://vocab.nerc.ac.uk/collection/L22/current/NETT0027/">
<dc:identifier>SDN:L22::NETT0027</dc:identifier>
<skos:notation>SDN:L22::NETT0027</skos:notation>
<skos:prefLabel xml:lang="en">Modified David neuston net - Hempel and Weikert (1972)</skos:prefLabel>
<skos:altLabel>Modified David neuston net</skos:altLabel>
<skos:definition xml:lang="en">A pair of vertically stacked nets with 30 cm x 15 cm rectangular mouth opening and 0.3 or 0.5 mm mesh [Wiebe and Benfield 2003 Plate 21 B].</skos:definition>
<owl:versionInfo>1</owl:versionInfo>
<dc:date>2011-10-21 14:18:49.0</dc:date>
<skos:note xml:lang="en">accepted</skos:note>
<owl:deprecated>false</owl:deprecated>
<skos:broader rdf:resource="http://vocab.nerc.ac.uk/collection/L05/current/69/"/>
<void:inDataset rdf:resource="http://vocab.nerc.ac.uk/.well-known/void"/>
</skos:Concept>
</skos:member>
<skos:member>
<skos:Concept rdf:about="http://vocab.nerc.ac.uk/collection/L22/current/NETT0052/">
<dc:identifier>SDN:L22::NETT0052</dc:identifier>
<skos:notation>SDN:L22::NETT0052</skos:notation>
<skos:prefLabel xml:lang="en">Modified Gulf III high-speed sampler - Hempel (1960)</skos:prefLabel>
<skos:altLabel>Hempel modified Gulf III HSS (HAI)</skos:altLabel>
<skos:definition xml:lang="en">Construction comprises an entrance of 18 cm diameter and a net mesh of 0.4mm. Towed at 6 knots.</skos:definition>
<owl:versionInfo>1</owl:versionInfo>
<dc:date>2011-10-21 14:18:49.0</dc:date>
<skos:note xml:lang="en">accepted</skos:note>
<owl:deprecated>false</owl:deprecated>
<skos:broader rdf:resource="http://vocab.nerc.ac.uk/collection/L05/current/67/"/>
<void:inDataset rdf:resource="http://vocab.nerc.ac.uk/.well-known/void"/>
</skos:Concept>
</skos:member>
<skos:member>
<skos:Concept rdf:about="http://vocab.nerc.ac.uk/collection/L22/current/NETT0049/">
<dc:identifier>SDN:L22::NETT0049</dc:identifier>
<skos:notation>SDN:L22::NETT0049</skos:notation>
<skos:prefLabel xml:lang="en">Modified Gulf V high-speed sampler - Lockwood (1974)</skos:prefLabel>
<skos:altLabel>Lockwood modified Gulf V HSS</skos:altLabel>
<skos:definition xml:lang="en">Construction is a 50 cm diameter mouth opening x 213 cm long with a nose cone; netting 24.6 mesh per cm; Two flowmeters.  based on Beverton and Tungate sampler. Towed at about 3 knots [Wiebe and Benfield 2003 Plate 17 B].</skos:definition>
<owl:versionInfo>1</owl:versionInfo>
<dc:date>2011-10-21 14:18:49.0</dc:date>
<skos:note xml:lang="en">accepted</skos:note>
<owl:deprecated>false</owl:deprecated>
<skos:broader rdf:resource="http://vocab.nerc.ac.uk/collection/L05/current/67/"/>
<skos:broader rdf:resource="http://vocab.nerc.ac.uk/collection/L05/current/388/"/>
<void:inDataset rdf:resource="http://vocab.nerc.ac.uk/.well-known/void"/>
</skos:Concept>
</skos:member>
<skos:member>
<skos:Concept rdf:about="http://vocab.nerc.ac.uk/collection/L22/current/NETT0072/">
<dc:identifier>SDN:L22::NETT0072</dc:identifier>
<skos:notation>SDN:L22::NETT0072</skos:notation>
<skos:prefLabel xml:lang="en">Modified Isaacs-Kidd Midwater Trawl with MPS cod-end - Pearcy and Hubbard (1964)</skos:prefLabel>
<skos:altLabel>Pearcy modified IKMT</skos:altLabel>
<skos:definition xml:lang="en">A 1.8 m IKMT fitted with a scaled down version of the Be MPS with 3 nets attached to the back of the trawl.  A pressure-release system controls the opening/closing of the cod-end nets [Wiebe and Benfield 2003 Plate 26 B].</skos:definition>
<owl:versionInfo>1</owl:versionInfo>
<dc:date>2011-10-21 14:18:49.0</dc:date>
<skos:note xml:lang="en">accepted</skos:note>
<owl:deprecated>false</owl:deprecated>
<skos:broader rdf:resource="http://vocab.nerc.ac.uk/collection/L05/current/68/"/>
<skos:broader rdf:resource="http://vocab.nerc.ac.uk/collection/L05/current/23/"/>
<void:inDataset rdf:resource="http://vocab.nerc.ac.uk/.well-known/void"/>
</skos:Concept>
</skos:member>
<skos:member>
<skos:Concept rdf:about="http://vocab.nerc.ac.uk/collection/L22/current/NETT0079/">
<dc:identifier>SDN:L22::NETT0079</dc:identifier>
<skos:notation>SDN:L22::NETT0079</skos:notation>
<skos:prefLabel xml:lang="en">Modified Juday net  - Clayton and Pavlou (1978)</skos:prefLabel>
<skos:altLabel>Clayton modified Juday net.</skos:altLabel>
<skos:definition xml:lang="en">A net designed to avoid surface contamination of the sample. Construction is a 75 cm diameter cylinder (120 cm length) and cone (290 cm length), net (Nitex mesh size not given) with a cylinder skirt 380 cm long to enclose the net mesh.  The net ring and netting are enclosed in nylon utility cloth and tied with a release line that is pulled free after the net is underwater.  A messenger used to close net [Wiebe and Benfield 2003 Plate 7 B, C].</skos:definition>
<owl:versionInfo>1</owl:versionInfo>
<dc:date>2011-10-21 14:18:49.0</dc:date>
<skos:note xml:lang="en">accepted</skos:note>
<owl:deprecated>false</owl:deprecated>
<skos:broader rdf:resource="http://vocab.nerc.ac.uk/collection/L05/current/22/"/>
<void:inDataset rdf:resource="http://vocab.nerc.ac.uk/.well-known/void"/>
</skos:Concept>
</skos:member>
<skos:member>
<skos:Concept rdf:about="http://vocab.nerc.ac.uk/collection/L22/current/NETT0077/">
<dc:identifier>SDN:L22::NETT0077</dc:identifier>
<skos:notation>SDN:L22::NETT0077</skos:notation>
<skos:prefLabel xml:lang="en">Modified Juday net - Aksnes and Magnesen (1983)</skos:prefLabel>
<skos:altLabel>Aksnes modified Juday net</skos:altLabel>
<skos:definition xml:lang="en">A pair of Juday nets with 40 cm diameter mouth openings were mounted on a frame 50 cm apart. Mesh of nets 0.18 mm. Designed to be towed vertically.</skos:definition>
<owl:versionInfo>1</owl:versionInfo>
<dc:date>2011-10-21 14:18:49.0</dc:date>
<skos:note xml:lang="en">accepted</skos:note>
<owl:deprecated>false</owl:deprecated>
<skos:broader rdf:resource="http://vocab.nerc.ac.uk/collection/L05/current/22/"/>
<void:inDataset rdf:resource="http://vocab.nerc.ac.uk/.well-known/void"/>
</skos:Concept>
</skos:member>
<skos:member>
<skos:Concept rdf:about="http://vocab.nerc.ac.uk/collection/L22/current/NETT0083/">
<dc:identifier>SDN:L22::NETT0083</dc:identifier>
<skos:notation>SDN:L22::NETT0083</skos:notation>
<skos:prefLabel xml:lang="en">Modified Longhurt-Hardy Plankton Recorder - Haury et al. (1976)</skos:prefLabel>
<skos:altLabel>Haury modified LHPR</skos:altLabel>
<skos:definition xml:lang="en">Three lengths  (230, 300, 370 cm) of  70 cm diameter net were mounted in a towing frame.  The modified recorder box had a mesh area to mouth opening ratio of 2.9 as opposed to &lt; 1.0 for previous designs and the orientation of the gauze across the recorder box tunnels was horizontal instead of vertical. The modified design reduced or eliminated many of the problems observed in earlier designs.  Data on pressure and temperature and flow counts were logged on an internal recorder in the pressure case.  Normally towed at 1.5 to 2.5 knots and collected ~ 100 samples [Wiebe and Benfield 2003 Plate 26 E].</skos:definition>
<owl:versionInfo>1</owl:versionInfo>
<dc:date>2011-10-21 14:18:49.0</dc:date>
<skos:note xml:lang="en">accepted</skos:note>
<owl:deprecated>false</owl:deprecated>
<skos:broader rdf:resource="http://vocab.nerc.ac.uk/collection/L05/current/134/"/>
<skos:broader rdf:resource="http://vocab.nerc.ac.uk/collection/L05/current/21/"/>
<skos:broader rdf:resource="http://vocab.nerc.ac.uk/collection/L05/current/388/"/>
<void:inDataset rdf:resource="http://vocab.nerc.ac.uk/.well-known/void"/>
</skos:Concept>
</skos:member>
<skos:member>
<skos:Concept rdf:about="http://vocab.nerc.ac.uk/collection/L22/current/NETT0098/">
<dc:identifier>SDN:L22::NETT0098</dc:identifier>
<skos:notation>SDN:L22::NETT0098</skos:notation>
<skos:prefLabel xml:lang="en">Modified Multiple Plankton Sampler - Weikert and John (1981)</skos:prefLabel>
<skos:altLabel>Weikert modified MPS</skos:altLabel>
<skos:definition xml:lang="en">A modified version of the Be MPS net with a rectangular sampler box 50 cm x 50 cm on a side and 60 cm deep equipped with 5 nets (0.3 mm mesh) each 250 cm long.  Nets are opened and closed electronically through conducting cable and pressure is monitored. No flowmeter used [Wiebe and Benfield 2003 Plate 31 A, B].</skos:definition>
<owl:versionInfo>1</owl:versionInfo>
<dc:date>2011-10-21 14:18:49.0</dc:date>
<skos:note xml:lang="en">accepted</skos:note>
<owl:deprecated>false</owl:deprecated>
<skos:broader rdf:resource="http://vocab.nerc.ac.uk/collection/L05/current/68/"/>
<skos:broader rdf:resource="http://vocab.nerc.ac.uk/collection/L05/current/22/"/>
<void:inDataset rdf:resource="http://vocab.nerc.ac.uk/.well-known/void"/>
</skos:Concept>
</skos:member>
<skos:member>
<skos:Concept rdf:about="http://vocab.nerc.ac.uk/collection/L22/current/NETT0107/">
<dc:identifier>SDN:L22::NETT0107</dc:identifier>
<skos:notation>SDN:L22::NETT0107</skos:notation>
<skos:prefLabel xml:lang="en">Modified N70 net - Currie ans Foston (1957)</skos:prefLabel>
<skos:altLabel>Currie modified N70</skos:altLabel>
<skos:definition xml:lang="en">A modified version of the Nansen net with a large depth-flowmeter mounted mid-way down the middle of the cylinder portion of the net.</skos:definition>
<owl:versionInfo>1</owl:versionInfo>
<dc:date>2011-10-21 14:18:49.0</dc:date>
<skos:note xml:lang="en">accepted</skos:note>
<owl:deprecated>false</owl:deprecated>
<skos:broader rdf:resource="http://vocab.nerc.ac.uk/collection/L05/current/22/"/>
<skos:broader rdf:resource="http://vocab.nerc.ac.uk/collection/L05/current/388/"/>
<void:inDataset rdf:resource="http://vocab.nerc.ac.uk/.well-known/void"/>
</skos:Concept>
</skos:member>
<skos:member>
<skos:Concept rdf:about="http://vocab.nerc.ac.uk/collection/L22/current/NETT0123/">
<dc:identifier>SDN:L22::NETT0123</dc:identifier>
<skos:notation>SDN:L22::NETT0123</skos:notation>
<skos:prefLabel xml:lang="en">Modified North Pacific standard net - Motoda (1994)</skos:prefLabel>
<skos:altLabel>Motoda modified NorPac net</skos:altLabel>
<skos:definition xml:lang="en">Has a 45 cm diameter circular mouth opening with cylinder 65 cm and 130 cm cone mesh (0.35 mm). Equipped with a flowmeter. Also there is a description of a self-closing cod end box which has two net bags to collect the catch. The net is sent down vertically and when towed horizontally, a counter balance weight opens one net bag. When the net is brought to the surface vertically, the weight shifts closing the one and opening the other net bag [Wiebe and Benfield 2003 Plate 25 B].</skos:definition>
<owl:versionInfo>1</owl:versionInfo>
<dc:date>2011-10-21 14:18:49.0</dc:date>
<skos:note xml:lang="en">accepted</skos:note>
<owl:deprecated>false</owl:deprecated>
<skos:broader rdf:resource="http://vocab.nerc.ac.uk/collection/L05/current/388/"/>
<skos:broader rdf:resource="http://vocab.nerc.ac.uk/collection/L05/current/22/"/>
<void:inDataset rdf:resource="http://vocab.nerc.ac.uk/.well-known/void"/>
</skos:Concept>
</skos:member>
<skos:member>
<skos:Concept rdf:about="http://vocab.nerc.ac.uk/collection/L22/current/NETT0120/">
<dc:identifier>SDN:L22::NETT0120</dc:identifier>
<skos:notation>SDN:L22::NETT0120</skos:notation>
<skos:prefLabel xml:lang="en">Modified Rectangular Midwater Trawl 1+8 - Dimmler and Klindt (1990)</skos:prefLabel>
<skos:altLabel>Dimmler modified RMT 1+8</skos:altLabel>
<skos:definition xml:lang="en">RMT fitted with modified electronics comprising a PC-controlled unit with an underwater electronics unit connected by conducting cable. Nets are opened and closed by command at the surface. Sensors include pressure, temperature, conductivity, tilt-angle of net mouth, flow from two flowmeters and data acquisition rate is 4 times per second.  Data processing and display occurs in realtime.</skos:definition>
<owl:versionInfo>1</owl:versionInfo>
<dc:date>2011-10-21 14:18:49.0</dc:date>
<skos:note xml:lang="en">accepted</skos:note>
<owl:deprecated>false</owl:deprecated>
<skos:broader rdf:resource="http://vocab.nerc.ac.uk/collection/L05/current/350/"/>
<skos:broader rdf:resource="http://vocab.nerc.ac.uk/collection/L05/current/68/"/>
<skos:broader rdf:resource="http://vocab.nerc.ac.uk/collection/L05/current/134/"/>
<skos:broader rdf:resource="http://vocab.nerc.ac.uk/collection/L05/current/385/"/>
<skos:broader rdf:resource="http://vocab.nerc.ac.uk/collection/L05/current/23/"/>
<skos:broader rdf:resource="http://vocab.nerc.ac.uk/collection/L05/current/388/"/>
<void:inDataset rdf:resource="http://vocab.nerc.ac.uk/.well-known/void"/>
</skos:Concept>
</skos:member>
<skos:member>
<skos:Concept rdf:about="http://vocab.nerc.ac.uk/collection/L22/current/NETT0081/">
<dc:identifier>SDN:L22::NETT0081</dc:identifier>
<skos:notation>SDN:L22::NETT0081</skos:notation>
<skos:prefLabel xml:lang="en">Modified large Longhurt-Hardy Plankton Recorder - Bone (1986)</skos:prefLabel>
<skos:altLabel>Bone modified LHPR</skos:altLabel>
<skos:definition xml:lang="en">A modified version of the LHPR . A tubular frame 185 cm high x 125 cm wide x 640 cm long and with a 81 cm expanding to 100 cm diameter nose cone was used with a recorder box (with 1.55 mm nylon mesh gauze) attached to the cod-end of a conical net 300 cm long with same mesh.  The mouth of the recorder box is equipped with an opening/closing unit which shunts water flowing through the net to the open sea when closed and into the recorder when open. System acoustically (IOS) telemeters depth, flow, and temperature and controls recorder box opening/closing unit.  Underwater electronics records temperature, depth, flow, and controls gauze advance. Designed to tow up to 4 knots [Wiebe and Benfield 2003 Plate 27 B].</skos:definition>
<owl:versionInfo>1</owl:versionInfo>
<dc:date>2011-10-21 14:18:49.0</dc:date>
<skos:note xml:lang="en">accepted</skos:note>
<owl:deprecated>false</owl:deprecated>
<skos:broader rdf:resource="http://vocab.nerc.ac.uk/collection/L05/current/21/"/>
<skos:broader rdf:resource="http://vocab.nerc.ac.uk/collection/L05/current/388/"/>
<skos:broader rdf:resource="http://vocab.nerc.ac.uk/collection/L05/current/134/"/>
<void:inDataset rdf:resource="http://vocab.nerc.ac.uk/.well-known/void"/>
</skos:Concept>
</skos:member>
<skos:member>
<skos:Concept rdf:about="http://vocab.nerc.ac.uk/collection/L22/current/NETT0010/">
<dc:identifier>SDN:L22::NETT0010</dc:identifier>
<skos:notation>SDN:L22::NETT0010</skos:notation>
<skos:prefLabel xml:lang="en">Modified opening-closing Bongo net - Sameoto and Jaroszynski (1976)</skos:prefLabel>
<skos:altLabel>Modified Bongo opening-closing net</skos:altLabel>
<skos:definition xml:lang="en">A 75 cm diameter reinforced ring held to the wire by the same method as the Octagon Net. The net had a double messenger release mechanism with the first messenger releasing a dacron cloth door blocking the net mouth and the second one releasing the net.</skos:definition>
<owl:versionInfo>1</owl:versionInfo>
<dc:date>2011-10-21 14:18:49.0</dc:date>
<skos:note xml:lang="en">accepted</skos:note>
<owl:deprecated>false</owl:deprecated>
<skos:broader rdf:resource="http://vocab.nerc.ac.uk/collection/L05/current/22/"/>
<void:inDataset rdf:resource="http://vocab.nerc.ac.uk/.well-known/void"/>
</skos:Concept>
</skos:member>
<skos:member>
<skos:Concept rdf:about="http://vocab.nerc.ac.uk/collection/L22/current/NETT0073/">
<dc:identifier>SDN:L22::NETT0073</dc:identifier>
<skos:notation>SDN:L22::NETT0073</skos:notation>
<skos:prefLabel xml:lang="en">Modified opening-closing Isaacs-Kidd Midwater Trawl - Brown (1975)</skos:prefLabel>
<skos:altLabel>Brown modified IKMT</skos:altLabel>
<skos:definition xml:lang="en">An IKMT was outfitted with a flap of material that extended from the net mouth to the back end of the net and a 3-stage cod end.  At the start of a haul the flap was down and animals collect in stage 1 of the cod end. A timer released the flap which rode to the top of the net and animals collected in the stage II cod end.  A second timer release caused the stage II cod end to be pursed and it was replaced with the stage III cod end.</skos:definition>
<owl:versionInfo>1</owl:versionInfo>
<dc:date>2011-10-21 14:18:49.0</dc:date>
<skos:note xml:lang="en">accepted</skos:note>
<owl:deprecated>false</owl:deprecated>
<skos:broader rdf:resource="http://vocab.nerc.ac.uk/collection/L05/current/68/"/>
<skos:broader rdf:resource="http://vocab.nerc.ac.uk/collection/L05/current/23/"/>
<void:inDataset rdf:resource="http://vocab.nerc.ac.uk/.well-known/void"/>
</skos:Concept>
</skos:member>
<skos:member>
<skos:Concept rdf:about="http://vocab.nerc.ac.uk/collection/L22/current/NETT0053/">
<dc:identifier>SDN:L22::NETT0053</dc:identifier>
<skos:notation>SDN:L22::NETT0053</skos:notation>
<skos:prefLabel xml:lang="en">Modified small Hardy Plankton Sampler - Miller (1961)</skos:prefLabel>
<skos:altLabel>Miller modified Hardy Plankton Sampler</skos:altLabel>
<skos:definition xml:lang="en">This is a small high-speed sampler (modified from that described by Glover) with 10.1cm diameter aperture opening on a body tube 14 cm internal diameter and a 61cm overall length. Attached to the back of the tube is a 91 cm long nylon net of three meshes (0.947 mm, 0.526 mm, and 0.264 mm). Multiple units used on the towing wire at speeds of 7 to 8 knots with a multiplane kit otter depressor on bottom of wire [Wiebe and Benfield 2003 Plate 14 B].</skos:definition>
<owl:versionInfo>1</owl:versionInfo>
<dc:date>2011-10-21 14:18:49.0</dc:date>
<skos:note xml:lang="en">accepted</skos:note>
<owl:deprecated>false</owl:deprecated>
<skos:broader rdf:resource="http://vocab.nerc.ac.uk/collection/L05/current/67/"/>
<void:inDataset rdf:resource="http://vocab.nerc.ac.uk/.well-known/void"/>
</skos:Concept>
</skos:member>
<skos:member>
<skos:Concept rdf:about="http://vocab.nerc.ac.uk/collection/L22/current/TOOL0606/">
<dc:identifier>SDN:L22::TOOL0606</dc:identifier>
<skos:notation>SDN:L22::TOOL0606</skos:notation>
<skos:prefLabel xml:lang="en">Muir Matheson OMC-150 Combined Wind Speed and Direction Sensor</skos:prefLabel>
<skos:altLabel>Muir Matheson OMC-150</skos:altLabel>
<skos:definition xml:lang="en">A cup and vane anemometer measuring horizontal wind speed and direction that is suitable for hazardous environments.</skos:definition>
<owl:versionInfo>1</owl:versionInfo>
<dc:date>2013-03-22 16:34:21.0</dc:date>
<skos:note xml:lang="en">accepted</skos:note>
<owl:deprecated>false</owl:deprecated>
<skos:broader rdf:resource="http://vocab.nerc.ac.uk/collection/L05/current/101/"/>
<void:inDataset rdf:resource="http://vocab.nerc.ac.uk/.well-known/void"/>
</skos:Concept>
</skos:member>
<skos:member>
<skos:Concept rdf:about="http://vocab.nerc.ac.uk/collection/L22/current/NETT0099/">
<dc:identifier>SDN:L22::NETT0099</dc:identifier>
<skos:notation>SDN:L22::NETT0099</skos:notation>
<skos:prefLabel xml:lang="en">Multiple Plankton Sampler - Be et al. (1959); Be (1962)</skos:prefLabel>
<skos:altLabel>MPS</skos:altLabel>
<skos:definition xml:lang="en">Construction is a 50 cm x 50 cm opening with nets of 0.2 mm mesh 300 cm long ( 50 cm nylon cloth collar; 240 cm netting, 10 cm nylon cloth for cod-end attachment). First described as a vertically towed system using messengers to open and close three nets.  A depth-flowmeter readings continuous recorded on smoked glass cylinder.  Then modified to do horizontal or oblique towing using a pressure actuated device to open and close nets a preselected depths (MPS 0-100, 100-250 m, and 250-500 m; BPS 500-1000 m). Also built with 100 cm x 100 cm mouth opening. Sometimes referred to as the Bathypelagic Plankton Sampler [Wiebe and Benfield 2003 Plate 9 A, B, C].</skos:definition>
<owl:versionInfo>1</owl:versionInfo>
<dc:date>2011-10-21 14:18:49.0</dc:date>
<skos:note xml:lang="en">accepted</skos:note>
<owl:deprecated>false</owl:deprecated>
<skos:broader rdf:resource="http://vocab.nerc.ac.uk/collection/L05/current/22/"/>
<skos:broader rdf:resource="http://vocab.nerc.ac.uk/collection/L05/current/68/"/>
<skos:broader rdf:resource="http://vocab.nerc.ac.uk/collection/L05/current/388/"/>
<void:inDataset rdf:resource="http://vocab.nerc.ac.uk/.well-known/void"/>
</skos:Concept>
</skos:member>
<skos:member>
<skos:Concept rdf:about="http://vocab.nerc.ac.uk/collection/L22/current/NETT0101/">
<dc:identifier>SDN:L22::NETT0101</dc:identifier>
<skos:notation>SDN:L22::NETT0101</skos:notation>
<skos:prefLabel xml:lang="en">Multiple Plankton Sampler based on MOCNESS and NIO nets - Sameoto et al. (1977)</skos:prefLabel>
<skos:altLabel>Sameto MPS</skos:altLabel>
<skos:definition xml:lang="en">A 100 cm x 100 cm mouth opening with 10 nets (0.243 mm mesh ).  Net length not given.  Non-rigid mouth opening with net bars similar in design to MOCNESS that slide down cables.  A depressor is mounted below the bottom net bar.  System powered electrically on conducting wire and controlled from surface deck unit. Data logging included depth, roll, pitch, and temperature. A non-telemetering flowmeter was mounted in each net [Wiebe and Benfield 2003 Plate 30 A].</skos:definition>
<owl:versionInfo>1</owl:versionInfo>
<dc:date>2011-10-21 14:18:49.0</dc:date>
<skos:note xml:lang="en">accepted</skos:note>
<owl:deprecated>false</owl:deprecated>
<skos:broader rdf:resource="http://vocab.nerc.ac.uk/collection/L05/current/134/"/>
<skos:broader rdf:resource="http://vocab.nerc.ac.uk/collection/L05/current/388/"/>
<skos:broader rdf:resource="http://vocab.nerc.ac.uk/collection/L05/current/385/"/>
<skos:broader rdf:resource="http://vocab.nerc.ac.uk/collection/L05/current/23/"/>
<skos:broader rdf:resource="http://vocab.nerc.ac.uk/collection/L05/current/68/"/>
<void:inDataset rdf:resource="http://vocab.nerc.ac.uk/.well-known/void"/>
</skos:Concept>
</skos:member>
<skos:member>
<skos:Concept rdf:about="http://vocab.nerc.ac.uk/collection/L22/current/NETT0148/">
<dc:identifier>SDN:L22::NETT0148</dc:identifier>
<skos:notation>SDN:L22::NETT0148</skos:notation>
<skos:prefLabel xml:lang="en">Multiple Rectangular Midwater Trawl 1+8 - Roe and Shale (1979)</skos:prefLabel>
<skos:altLabel>Roe modified RMT 1+8</skos:altLabel>
<skos:definition xml:lang="en">A combination multiple plankton and nekton collecting system with three 1-m2 and three 8-m2 with pair of nets opened and closed by acoustic command.  Also transmitted acoustically are depth and flow. A modification of system described by Baker et al., 1973. [Wiebe and Benfield 2003 Plate 28 B]</skos:definition>
<owl:versionInfo>1</owl:versionInfo>
<dc:date>2011-10-21 14:18:49.0</dc:date>
<skos:note xml:lang="en">accepted</skos:note>
<owl:deprecated>false</owl:deprecated>
<skos:broader rdf:resource="http://vocab.nerc.ac.uk/collection/L05/current/388/"/>
<skos:broader rdf:resource="http://vocab.nerc.ac.uk/collection/L05/current/23/"/>
<skos:broader rdf:resource="http://vocab.nerc.ac.uk/collection/L05/current/68/"/>
<void:inDataset rdf:resource="http://vocab.nerc.ac.uk/.well-known/void"/>
</skos:Concept>
</skos:member>
<skos:member>
<skos:Concept rdf:about="http://vocab.nerc.ac.uk/collection/L22/current/NETT0158/">
<dc:identifier>SDN:L22::NETT0158</dc:identifier>
<skos:notation>SDN:L22::NETT0158</skos:notation>
<skos:prefLabel xml:lang="en">Multiple-net Tucker Trawl - Frost and McCrone (1974)</skos:prefLabel>
<skos:altLabel>Frost modified Tucker Trawl</skos:altLabel>
<skos:definition xml:lang="en">A 100 cm x 141 cm rectangular flexible mouth opening  with 0.33 mm nylon mesh nets 6 meters long. Originally with 5 nets and increased to 9 nets.  (Also a 200 cm x 282 cm mouth opening trawl with 5 nets of 6.35 mm stretch mesh). System powered electrically on conducting wire and controlled from surface. Monitored depth, angle, and flowmeter revolutions [Wiebe and Benfield 2003 Plate 28 A].</skos:definition>
<owl:versionInfo>1</owl:versionInfo>
<dc:date>2011-10-21 14:18:49.0</dc:date>
<skos:note xml:lang="en">accepted</skos:note>
<owl:deprecated>false</owl:deprecated>
<skos:broader rdf:resource="http://vocab.nerc.ac.uk/collection/L05/current/68/"/>
<skos:broader rdf:resource="http://vocab.nerc.ac.uk/collection/L05/current/385/"/>
<skos:broader rdf:resource="http://vocab.nerc.ac.uk/collection/L05/current/388/"/>
<skos:broader rdf:resource="http://vocab.nerc.ac.uk/collection/L05/current/23/"/>
<void:inDataset rdf:resource="http://vocab.nerc.ac.uk/.well-known/void"/>
</skos:Concept>
</skos:member>
<skos:member>
<skos:Concept rdf:about="http://vocab.nerc.ac.uk/collection/L22/current/TOOL0607/">
<dc:identifier>SDN:L22::TOOL0607</dc:identifier>
<skos:notation>SDN:L22::TOOL0607</skos:notation>
<skos:prefLabel xml:lang="en">Munro SO/8 cup and vane anemometer</skos:prefLabel>
<skos:altLabel>Munro SO/8 anemometer</skos:altLabel>
<skos:definition xml:lang="en">A cup and vane anemometer measuring horizontal wind speed and direction.</skos:definition>
<owl:versionInfo>1</owl:versionInfo>
<dc:date>2013-03-22 16:36:45.0</dc:date>
<skos:note xml:lang="en">accepted</skos:note>
<owl:deprecated>false</owl:deprecated>
<skos:broader rdf:resource="http://vocab.nerc.ac.uk/collection/L05/current/101/"/>
<void:inDataset rdf:resource="http://vocab.nerc.ac.uk/.well-known/void"/>
</skos:Concept>
</skos:member>
<skos:member>
<skos:Concept rdf:about="http://vocab.nerc.ac.uk/collection/L22/current/TOOL0014/">
<dc:identifier>SDN:L22::TOOL0014</dc:identifier>
<skos:notation>SDN:L22::TOOL0014</skos:notation>
<skos:prefLabel xml:lang="en">Munro tide gauge</skos:prefLabel>
<skos:altLabel>Munro gauge</skos:altLabel>
<skos:definition xml:lang="en">The Munro gauge measures sea level by means of a float in a stilling well. The float is about 45cm in diameter - the large diameter reduces inevitable errors in buoyancy due to friction of the gearing and small changes in the length of float wire. This wire is coiled round a drum on the end of the gauge and another drum contains a counter balance wire. The drum is geared to a slotted tape attached to a pen carriage which traces the tide curve on the chart during the rise and fall of the tide. A precision potentiometer is attached to the gauge to provide an input to the data logger.</skos:definition>
<owl:versionInfo>1</owl:versionInfo>
<dc:date>2008-11-28 07:54:52.0</dc:date>
<skos:note xml:lang="en">accepted</skos:note>
<owl:deprecated>false</owl:deprecated>
<skos:broader rdf:resource="http://vocab.nerc.ac.uk/collection/L05/current/111/"/>
<void:inDataset rdf:resource="http://vocab.nerc.ac.uk/.well-known/void"/>
</skos:Concept>
</skos:member>
<skos:member>
<skos:Concept rdf:about="http://vocab.nerc.ac.uk/collection/L22/current/NETT0124/">
<dc:identifier>SDN:L22::NETT0124</dc:identifier>
<skos:notation>SDN:L22::NETT0124</skos:notation>
<skos:prefLabel xml:lang="en">N-series (N50, N70, N100, N200, N450) nets - Kemp et al. (1929); Marr (1938)</skos:prefLabel>
<skos:altLabel>N-series nets</skos:altLabel>
<skos:definition xml:lang="en">Cylinder-cone nets of varying sizes that were used in conjunction and towed either vertically, horizontally or obliquely depending upon size. All could be closed. N50 and N70  were similar in size and mesh to Hjort net [Wiebe and Benfield 2003 Plate 1 E].  Grouping term for N50, N70, N100, N200 and N450 nets.</skos:definition>
<owl:versionInfo>1</owl:versionInfo>
<dc:date>2011-10-21 14:18:49.0</dc:date>
<skos:note xml:lang="en">accepted</skos:note>
<owl:deprecated>false</owl:deprecated>
<skos:broader rdf:resource="http://vocab.nerc.ac.uk/collection/L05/current/22/"/>
<void:inDataset rdf:resource="http://vocab.nerc.ac.uk/.well-known/void"/>
</skos:Concept>
</skos:member>
<skos:member>
<skos:Concept rdf:about="http://vocab.nerc.ac.uk/collection/L22/current/NETT0102/">
<dc:identifier>SDN:L22::NETT0102</dc:identifier>
<skos:notation>SDN:L22::NETT0102</skos:notation>
<skos:prefLabel xml:lang="en">N100 - Kemp et al. (1929); Marr (1938)</skos:prefLabel>
<skos:altLabel>N100</skos:altLabel>
<skos:definition xml:lang="en">Cylinder-cone net structure. The cylinder is 100 cm diameter  by 107 cm long with a 1.27 cm mesh. The cone has two sections one 107 cm long with 4 mm mesh, and the other 213 cm long with 5.9 meshes per cm or stramin.</skos:definition>
<owl:versionInfo>1</owl:versionInfo>
<dc:date>2011-10-21 14:18:49.0</dc:date>
<skos:note xml:lang="en">accepted</skos:note>
<owl:deprecated>false</owl:deprecated>
<skos:broader rdf:resource="http://vocab.nerc.ac.uk/collection/L05/current/22/"/>
<void:inDataset rdf:resource="http://vocab.nerc.ac.uk/.well-known/void"/>
</skos:Concept>
</skos:member>
<skos:member>
<skos:Concept rdf:about="http://vocab.nerc.ac.uk/collection/L22/current/NETT0103/">
<dc:identifier>SDN:L22::NETT0103</dc:identifier>
<skos:notation>SDN:L22::NETT0103</skos:notation>
<skos:prefLabel xml:lang="en">N200 - Kemp et al. (1929); Marr (1938)</skos:prefLabel>
<skos:altLabel>N200</skos:altLabel>
<skos:definition xml:lang="en">Cylinder-cone net structure. The cylinder is 200 cm diameter by 213 cm long with a 2.54 cm mesh 213 cm long. The cone has two sections one 198 cm long with 7 mm mesh, and the other 396 cm long with 4 mm mesh.</skos:definition>
<owl:versionInfo>1</owl:versionInfo>
<dc:date>2011-10-21 14:18:49.0</dc:date>
<skos:note xml:lang="en">accepted</skos:note>
<owl:deprecated>false</owl:deprecated>
<skos:broader rdf:resource="http://vocab.nerc.ac.uk/collection/L05/current/22/"/>
<void:inDataset rdf:resource="http://vocab.nerc.ac.uk/.well-known/void"/>
</skos:Concept>
</skos:member>
<skos:member>
<skos:Concept rdf:about="http://vocab.nerc.ac.uk/collection/L22/current/NETT0104/">
<dc:identifier>SDN:L22::NETT0104</dc:identifier>
<skos:notation>SDN:L22::NETT0104</skos:notation>
<skos:prefLabel xml:lang="en">N450 - Kemp et al. (1929); Marr (1938)</skos:prefLabel>
<skos:altLabel>N450</skos:altLabel>
<skos:definition xml:lang="en">Cylinder-cone net structure with four sections. The cylinder is 450cm diameter by 457 cm long with a 3.8 cm mesh. The cone is  1371 cm long with three equal length sections with 1.27 cm mesh, 0.7 cm mesh, and 0.7 cm mesh with 0.4 cm mesh liner respectively. Used either as open net or with a messenger device that closed the net about half way back to the cod end while still allowing the net ring to tow normally.  Depth recording instrument used on the net.</skos:definition>
<owl:versionInfo>1</owl:versionInfo>
<dc:date>2011-10-21 14:18:49.0</dc:date>
<skos:note xml:lang="en">accepted</skos:note>
<owl:deprecated>false</owl:deprecated>
<skos:broader rdf:resource="http://vocab.nerc.ac.uk/collection/L05/current/22/"/>
<void:inDataset rdf:resource="http://vocab.nerc.ac.uk/.well-known/void"/>
</skos:Concept>
</skos:member>
<skos:member>
<skos:Concept rdf:about="http://vocab.nerc.ac.uk/collection/L22/current/NETT0105/">
<dc:identifier>SDN:L22::NETT0105</dc:identifier>
<skos:notation>SDN:L22::NETT0105</skos:notation>
<skos:prefLabel xml:lang="en">N50 - Kemp et al. (1929); Marr (1938)</skos:prefLabel>
<skos:altLabel>N50</skos:altLabel>
<skos:definition xml:lang="en">Cylinder-cone net structure. The cylinder is 50 cm diameter by 66 cm long made of canvas. The cone is 65 cm long made of silk netting of 78 meshes /cm.</skos:definition>
<owl:versionInfo>1</owl:versionInfo>
<dc:date>2011-10-21 14:18:49.0</dc:date>
<skos:note xml:lang="en">accepted</skos:note>
<owl:deprecated>false</owl:deprecated>
<skos:broader rdf:resource="http://vocab.nerc.ac.uk/collection/L05/current/22/"/>
<void:inDataset rdf:resource="http://vocab.nerc.ac.uk/.well-known/void"/>
</skos:Concept>
</skos:member>
<skos:member>
<skos:Concept rdf:about="http://vocab.nerc.ac.uk/collection/L22/current/NETT0106/">
<dc:identifier>SDN:L22::NETT0106</dc:identifier>
<skos:notation>SDN:L22::NETT0106</skos:notation>
<skos:prefLabel xml:lang="en">N70 - Kemp et al. (1929)</skos:prefLabel>
<skos:altLabel>N70</skos:altLabel>
<skos:definition xml:lang="en">Cylinder-cone net structure. The cylinder is 70 cm diameter by 53 cm long with  0.64 cm mesh.  The cone has two sections: one 96.5 cm long with 15.74 threads per cm, and the other 134.6 cm long with 29.1 threads per cm.</skos:definition>
<owl:versionInfo>1</owl:versionInfo>
<dc:date>2011-10-21 14:18:49.0</dc:date>
<skos:note xml:lang="en">accepted</skos:note>
<owl:deprecated>false</owl:deprecated>
<skos:broader rdf:resource="http://vocab.nerc.ac.uk/collection/L05/current/22/"/>
<void:inDataset rdf:resource="http://vocab.nerc.ac.uk/.well-known/void"/>
</skos:Concept>
</skos:member>
<skos:member>
<skos:Concept rdf:about="http://vocab.nerc.ac.uk/collection/L22/current/TOOL0584/">
<dc:identifier>SDN:L22::TOOL0584</dc:identifier>
<skos:notation>SDN:L22::TOOL0584</skos:notation>
<skos:prefLabel xml:lang="en">NBA DNC-2 recording current meter</skos:prefLabel>
<skos:altLabel>NBA DNC-2 RCM</skos:altLabel>
<skos:definition xml:lang="en">A self-logging instrument measuring current speed with an impeller directly coupled to an electronic reed switch counter and current direction with a digital magnetic compass with 7-bit optical encoder. Accuracy quoted as +/- 2 per cent for speed and +/- 3 degrees for direction. Further information may be found in http://www.bodc.ac.uk/data/documents/nodb/508/ . Manufacturer went into liquidation in November 2012.</skos:definition>
<owl:versionInfo>1</owl:versionInfo>
<dc:date>2013-01-10 09:56:58.0</dc:date>
<skos:note xml:lang="en">accepted</skos:note>
<owl:deprecated>false</owl:deprecated>
<skos:broader rdf:resource="http://vocab.nerc.ac.uk/collection/L05/current/114/"/>
<void:inDataset rdf:resource="http://vocab.nerc.ac.uk/.well-known/void"/>
</skos:Concept>
</skos:member>
<skos:member>
<skos:Concept rdf:about="http://vocab.nerc.ac.uk/collection/L22/current/TOOL0585/">
<dc:identifier>SDN:L22::TOOL0585</dc:identifier>
<skos:notation>SDN:L22::TOOL0585</skos:notation>
<skos:prefLabel xml:lang="en">NBA DNC-2B recording current meter</skos:prefLabel>
<skos:altLabel>NBA DNC-2B RCM</skos:altLabel>
<skos:definition xml:lang="en">A self-logging instrument measuring current speed with an impeller directly coupled to an electronic reed switch counter and current direction with a digital magnetic compass with 7-bit optical encoder. Provision is included for two optional sensors each mesuring temperature, pressure or conductivity.  Accuracy quoted as +/- 2 per cent for speed, +/- 3 degrees for direction, +/- 0.25C for temperature, +/- 1 per cent for pressure and +/- 4 per cent for conductivity. Further information may be found in http://www.bodc.ac.uk/data/documents/nodb/508/ . Manufacturer went into liquidation in November 2012.</skos:definition>
<owl:versionInfo>2</owl:versionInfo>
<dc:date>2013-01-10 10:12:44.0</dc:date>
<skos:note xml:lang="en">accepted</skos:note>
<owl:deprecated>false</owl:deprecated>
<skos:broader rdf:resource="http://vocab.nerc.ac.uk/collection/L05/current/114/"/>
<void:inDataset rdf:resource="http://vocab.nerc.ac.uk/.well-known/void"/>
</skos:Concept>
</skos:member>
<skos:member>
<skos:Concept rdf:about="http://vocab.nerc.ac.uk/collection/L22/current/TOOL0586/">
<dc:identifier>SDN:L22::TOOL0586</dc:identifier>
<skos:notation>SDN:L22::TOOL0586</skos:notation>
<skos:prefLabel xml:lang="en">NBA DNC-2M recording current meter</skos:prefLabel>
<skos:altLabel>NBA DNC-2M RCM</skos:altLabel>
<skos:definition xml:lang="en">A self-logging instrument measuring current speed with an impeller directly coupled to an electronic reed switch counter and current direction with a digital magnetic compass with 8-bit optical encoder. Provision is included for three optional sensors each mesuring temperature, pressure or conductivity.  Accuracy quoted as +/- 2 per cent for speed, +/- 5 degrees for direction, +/- 0.2C for temperature, +/- 0.5 per cent for pressure and +/- 2mmho/cm for conductivity. Further information may be found in http://www.bodc.ac.uk/data/documents/nodb/50504/ . Manufacturer went into liquidation in November 2012.</skos:definition>
<owl:versionInfo>1</owl:versionInfo>
<dc:date>2013-01-10 10:16:08.0</dc:date>
<skos:note xml:lang="en">accepted</skos:note>
<owl:deprecated>false</owl:deprecated>
<skos:broader rdf:resource="http://vocab.nerc.ac.uk/collection/L05/current/114/"/>
<void:inDataset rdf:resource="http://vocab.nerc.ac.uk/.well-known/void"/>
</skos:Concept>
</skos:member>
<skos:member>
<skos:Concept rdf:about="http://vocab.nerc.ac.uk/collection/L22/current/TOOL0583/">
<dc:identifier>SDN:L22::TOOL0583</dc:identifier>
<skos:notation>SDN:L22::TOOL0583</skos:notation>
<skos:prefLabel xml:lang="en">NBA DNC-3 direct reading current meter</skos:prefLabel>
<skos:altLabel>NBA DNC-3 DRCM</skos:altLabel>
<skos:definition xml:lang="en">A direct-reading instrument measuring current speed with an impeller directly coupled to an optical sensor and current direction with a precision double-mounted compass. Accuracy quoted as +/- 0.05 m/s for speed and +/- 10 degrees for direction. Instrument providied continuous readings of instantaneous speed and direction to either analogue/digital gauges or an independent data logger. Manufacturer went into liquidation in November 2012.</skos:definition>
<owl:versionInfo>1</owl:versionInfo>
<dc:date>2013-01-10 09:41:46.0</dc:date>
<skos:note xml:lang="en">accepted</skos:note>
<owl:deprecated>false</owl:deprecated>
<skos:broader rdf:resource="http://vocab.nerc.ac.uk/collection/L05/current/114/"/>
<void:inDataset rdf:resource="http://vocab.nerc.ac.uk/.well-known/void"/>
</skos:Concept>
</skos:member>
<skos:member>
<skos:Concept rdf:about="http://vocab.nerc.ac.uk/collection/L22/current/TOOL0503/">
<dc:identifier>SDN:L22::TOOL0503</dc:identifier>
<skos:notation>SDN:L22::TOOL0503</skos:notation>
<skos:prefLabel xml:lang="en">NIOZ PRISTINE ultraclean water sampler</skos:prefLabel>
<skos:altLabel>PRISTINE sampler</skos:altLabel>
<skos:definition xml:lang="en">Ultraclean water sampler developed by the Royal Netherlands Institute For Sea Research (NIOZ) for the GEOTRACES Program. Individual sample bottles have a capacity of 27 litres and include butterfly valves that ensure bottles are closed when passing through the ocean surface and reopen subsurface. Teflon valves for subsampling at the base of bottles ensure drainage of settling particulates. Samplers are deployed with a Kevlar hydrowire cable with internal signal cables. A single bottle may be used (e.g. during small boat work) or an array of bottles may be mounted on a frame for shipboard CTD work. Trip mechanisms range from a weighted messenger to trip wires or hydraulics for rosette sampling.</skos:definition>
<owl:versionInfo>1</owl:versionInfo>
<dc:date>2012-06-21 16:09:48.0</dc:date>
<skos:note xml:lang="en">accepted</skos:note>
<owl:deprecated>false</owl:deprecated>
<skos:broader rdf:resource="http://vocab.nerc.ac.uk/collection/L05/current/30/"/>
<void:inDataset rdf:resource="http://vocab.nerc.ac.uk/.well-known/void"/>
</skos:Concept>
</skos:member>
<skos:member>
<skos:Concept rdf:about="http://vocab.nerc.ac.uk/collection/L22/current/NETT0121/">
<dc:identifier>SDN:L22::NETT0121</dc:identifier>
<skos:notation>SDN:L22::NETT0121</skos:notation>
<skos:prefLabel xml:lang="en">NIPR-I sampler - Fukuchi et al. (1979)</skos:prefLabel>
<skos:altLabel>NIPR-I sampler</skos:altLabel>
<skos:definition xml:lang="en">A cylinder (24 cm x 57.5 cm) contains a motor driven propellor and a flow meter.  Water is pushed into a net (20 cm diameter x 50 cm length with 100 ?m mesh attached to the rear end of the cylinder.. The system is used to sample under sea ice to depth of 10 m.</skos:definition>
<owl:versionInfo>1</owl:versionInfo>
<dc:date>2011-10-21 14:18:49.0</dc:date>
<skos:note xml:lang="en">accepted</skos:note>
<owl:deprecated>false</owl:deprecated>
<skos:broader rdf:resource="http://vocab.nerc.ac.uk/collection/L05/current/388/"/>
<skos:broader rdf:resource="http://vocab.nerc.ac.uk/collection/L05/current/22/"/>
<void:inDataset rdf:resource="http://vocab.nerc.ac.uk/.well-known/void"/>
</skos:Concept>
</skos:member>
<skos:member>
<skos:Concept rdf:about="http://vocab.nerc.ac.uk/collection/L22/current/TOOL0233/">
<dc:identifier>SDN:L22::TOOL0233</dc:identifier>
<skos:notation>SDN:L22::TOOL0233</skos:notation>
<skos:prefLabel xml:lang="en">NKE SP2T temperature and depth recorder</skos:prefLabel>
<skos:altLabel>NKE SP2T TDR</skos:altLabel>
<skos:definition xml:lang="en">A family of small self-contained temperature and depth recorders with either internal or external (fast response) temperature sensors. A range of casing options give operating depths of between 10m and 4000m (operating depth specified as model number suffix). Temperature accuracy is 0.05C in range 0-20C and 0.1C outside this range. Depth accuracy is 0.3% full scale and resolution is 0.3% full scale. Wireless (inductive or radio) data connections are available.</skos:definition>
<owl:versionInfo>1</owl:versionInfo>
<dc:date>2010-05-18 16:10:58.0</dc:date>
<skos:note xml:lang="en">accepted</skos:note>
<owl:deprecated>false</owl:deprecated>
<skos:broader rdf:resource="http://vocab.nerc.ac.uk/collection/L05/current/134/"/>
<void:inDataset rdf:resource="http://vocab.nerc.ac.uk/.well-known/void"/>
</skos:Concept>
</skos:member>
<skos:member>
<skos:Concept rdf:about="http://vocab.nerc.ac.uk/collection/L22/current/NETT0109/">
<dc:identifier>SDN:L22::NETT0109</dc:identifier>
<skos:notation>SDN:L22::NETT0109</skos:notation>
<skos:prefLabel xml:lang="en">Nackthai net - Nellen and Hempel (1969)</skos:prefLabel>
<skos:altLabel>Nackthai net</skos:altLabel>
<skos:definition xml:lang="en">A modified Gulf V sampler with a 20 cm diameter nose cone aperture expanding to 38 cm diameter over length of 53 cm. Attached to back of cone is a net 120 cm long.  Frame work in which net supported 45 cm x 45 cm x 190 cm long. Overall length 143 cm. A comparison was made between the Hai and the Nackthai samplers which showed the Nackthai filtered more water and caught significantly more plankton and fish a result attributed to its non-encased net [Wiebe and Benfield 2003 Plate 16 E].</skos:definition>
<owl:versionInfo>1</owl:versionInfo>
<dc:date>2011-10-21 14:18:49.0</dc:date>
<skos:note xml:lang="en">accepted</skos:note>
<owl:deprecated>false</owl:deprecated>
<skos:broader rdf:resource="http://vocab.nerc.ac.uk/collection/L05/current/67/"/>
<void:inDataset rdf:resource="http://vocab.nerc.ac.uk/.well-known/void"/>
</skos:Concept>
</skos:member>
<skos:member>
<skos:Concept rdf:about="http://vocab.nerc.ac.uk/collection/L22/current/TOOL0248/">
<dc:identifier>SDN:L22::TOOL0248</dc:identifier>
<skos:notation>SDN:L22::TOOL0248</skos:notation>
<skos:prefLabel xml:lang="en">Nansen-Petterson water bottle</skos:prefLabel>
<skos:altLabel>Nansen bottle</skos:altLabel>
<skos:definition xml:lang="en">Metal or plastic insulated bottles with an approximate capacity of 1-2 litres designed for deployment on a cable, sealed by with a spring-loaded valve when triggered by dropping a weight down the cable. It was designed to recover an uncontaminated sample from depth within 0.01C of its in-situ temperature. The design is an improvement by Petterson in collaboration with Nansen on an original design by Nansen. Both designs are commonly known as Nansen bottles.</skos:definition>
<owl:versionInfo>2</owl:versionInfo>
<dc:date>2010-11-18 12:39:41.0</dc:date>
<skos:note xml:lang="en">accepted</skos:note>
<owl:deprecated>false</owl:deprecated>
<skos:broader rdf:resource="http://vocab.nerc.ac.uk/collection/L05/current/30/"/>
<void:inDataset rdf:resource="http://vocab.nerc.ac.uk/.well-known/void"/>
</skos:Concept>
</skos:member>
<skos:member>
<skos:Concept rdf:about="http://vocab.nerc.ac.uk/collection/L22/current/TOOL0236/">
<dc:identifier>SDN:L22::TOOL0236</dc:identifier>
<skos:notation>SDN:L22::TOOL0236</skos:notation>
<skos:prefLabel xml:lang="en">National Institute of Oceanography plastic reversing water bottle</skos:prefLabel>
<skos:altLabel>NIO bottle</skos:altLabel>
<skos:definition xml:lang="en">A 1.35 litre plastic water bottle designed by the National Institute of Oceanography. It is deployed clamped to a cable and triggered by a weight sliding down the cable. When triggered the bottle rotates through 180 degrees which simultaneously closes the valves and fires any reversing thermometers mounted on the bottle.</skos:definition>
<owl:versionInfo>2</owl:versionInfo>
<dc:date>2010-11-18 12:39:41.0</dc:date>
<skos:note xml:lang="en">accepted</skos:note>
<owl:deprecated>false</owl:deprecated>
<skos:broader rdf:resource="http://vocab.nerc.ac.uk/collection/L05/current/30/"/>
<void:inDataset rdf:resource="http://vocab.nerc.ac.uk/.well-known/void"/>
</skos:Concept>
</skos:member>
<skos:member>
<skos:Concept rdf:about="http://vocab.nerc.ac.uk/collection/L22/current/TOOL0540/">
<dc:identifier>SDN:L22::TOOL0540</dc:identifier>
<skos:notation>SDN:L22::TOOL0540</skos:notation>
<skos:prefLabel xml:lang="en">National Institute of Oceanography water sampling bottle</skos:prefLabel>
<skos:altLabel>NIO bottle</skos:altLabel>
<skos:definition xml:lang="en">A plastic free-flushing water sampling bottle designed for oceanographic sampling. It has valves at each end, which are held open on deployment. When the bottle reaches the desired depth the valves are released and sealed. A reversing thermometer may be mounted on the bottle. The bottle inverts on closure, triggering the thermometer. A sampling spigot is positioned at the base of the bottle. The bottle was designed in the 1970s by Francis E. Pierce, Dennis I. Gaunt, and Richard Dobson at what was  then the National Institute of Oceanography, UK (a predecessor of the National Oceanography Centre).</skos:definition>
<owl:versionInfo>1</owl:versionInfo>
<dc:date>2012-09-25 16:03:31.0</dc:date>
<skos:note xml:lang="en">accepted</skos:note>
<owl:deprecated>false</owl:deprecated>
<skos:broader rdf:resource="http://vocab.nerc.ac.uk/collection/L05/current/30/"/>
<void:inDataset rdf:resource="http://vocab.nerc.ac.uk/.well-known/void"/>
</skos:Concept>
</skos:member>
<skos:member>
<skos:Concept rdf:about="http://vocab.nerc.ac.uk/collection/L22/current/TOOL0405/">
<dc:identifier>SDN:L22::TOOL0405</dc:identifier>
<skos:notation>SDN:L22::TOOL0405</skos:notation>
<skos:prefLabel xml:lang="en">National Marine Facilities Microelectrode Oxygen Sensor</skos:prefLabel>
<skos:altLabel>NMF Microelectrode DO</skos:altLabel>
<skos:definition xml:lang="en">A non-membrane dissolved oxygen sensor for marine applications. The sensor uses a platinum microelectrode and a counter electrode (thus far composed of copper). A measurement potential is applied to the microelectrode relative to a counter electrode, reducing the dissolved oxygen in the water and generating a current through the microelectrode proportional to the number of oxygen molecules at that electrode. The sensor was first used in 2000 and development is ongoing. Early versions of the instrument applied the measurement potential for up to 30 seconds, with sampling starting approximately one second after the potential was applied. The sensor response to oxygen remained almost constant for a given concentration and data could be sampled at frequencies exceeding 1 Hz. To reduce noise generated by sensitivity to flow fluctuations a mesoporous layer was used to increase the surface area of the microelectrode, but this proved unstable and was replaced by a stop-flow system which pumped water in to a very small chamber, with measurements being taken while the water was still. This significantly improved results but the sensor was still affected by small convection currents. The current version of the sensor only applies the measurement potential for a few 10s of milliseconds and data are collected at approximately 1 Hz in an attempt to minimise the effects of convection currents. The latest development is a very small sensor head containing an array of microelectrodes (currently an array of five) that work together. The counter electrode consists of silver or silver chloride. This is currently undergoing trials and is yet to be deployed on a CTD profiler.</skos:definition>
<owl:versionInfo>1</owl:versionInfo>
<dc:date>2011-07-27 13:50:44.0</dc:date>
<skos:note xml:lang="en">accepted</skos:note>
<owl:deprecated>false</owl:deprecated>
<skos:broader rdf:resource="http://vocab.nerc.ac.uk/collection/L05/current/351/"/>
<void:inDataset rdf:resource="http://vocab.nerc.ac.uk/.well-known/void"/>
</skos:Concept>
</skos:member>
<skos:member>
<skos:Concept rdf:about="http://vocab.nerc.ac.uk/collection/L22/current/TOOL0370/">
<dc:identifier>SDN:L22::TOOL0370</dc:identifier>
<skos:notation>SDN:L22::TOOL0370</skos:notation>
<skos:prefLabel xml:lang="en">National Oceanography Centre Nitrate Sensor SUV6</skos:prefLabel>
<skos:altLabel>NOC Nitrate Sensor SUV6</skos:altLabel>
<skos:definition xml:lang="en">An in situ UV absorption spectrophotometer that measures nitrate concentrations in the ocean. The sensor is rated to either 500 m or 6000 m. It uses a Xenon flash lamp as a light source and has a path length of either 70 mm or 200 mm, permitting nitrate detection up to 400 uM or 100 uM, respectively. The minimum nitrate detection limit is 0.2 uM and accuracy is +/- 0.2 uM. Nitrate concentrations are determined from the ratio of the absorption at 220 nm and 280 nm. The sensor was developed by NOC in association with Valeport Ltd.</skos:definition>
<owl:versionInfo>1</owl:versionInfo>
<dc:date>2011-02-09 11:25:51.0</dc:date>
<skos:note xml:lang="en">accepted</skos:note>
<owl:deprecated>false</owl:deprecated>
<skos:broader rdf:resource="http://vocab.nerc.ac.uk/collection/L05/current/181/"/>
<void:inDataset rdf:resource="http://vocab.nerc.ac.uk/.well-known/void"/>
</skos:Concept>
</skos:member>
<skos:member>
<skos:Concept rdf:about="http://vocab.nerc.ac.uk/collection/L22/current/TOOL0555/">
<dc:identifier>SDN:L22::TOOL0555</dc:identifier>
<skos:notation>SDN:L22::TOOL0555</skos:notation>
<skos:prefLabel xml:lang="en">National Oceanography Centre torpedo towfish water sampler</skos:prefLabel>
<skos:altLabel>NOC torpedo towfish</skos:altLabel>
<skos:definition xml:lang="en">An epoxy resin-coated steel torpedo-shaped object designed to be towed alongside a moving ship at speeds of 1-12 knots. A teflon-lined tube runs through the centre of the fish and is connected to a pump on board the ship. Stabilising fins at the rear of the fish ensure that the sampling hose points forwards and that the fish maintains a roughly constant depth. The system is typically used for continuous, underway, clean sampling (e.g., trace metal studies) of near-surface waters.</skos:definition>
<owl:versionInfo>1</owl:versionInfo>
<dc:date>2012-09-28 14:08:54.0</dc:date>
<skos:note xml:lang="en">accepted</skos:note>
<owl:deprecated>false</owl:deprecated>
<skos:broader rdf:resource="http://vocab.nerc.ac.uk/collection/L05/current/31/"/>
<void:inDataset rdf:resource="http://vocab.nerc.ac.uk/.well-known/void"/>
</skos:Concept>
</skos:member>
<skos:member>
<skos:Concept rdf:about="http://vocab.nerc.ac.uk/collection/L22/current/TOOL0144/">
<dc:identifier>SDN:L22::TOOL0144</dc:identifier>
<skos:notation>SDN:L22::TOOL0144</skos:notation>
<skos:prefLabel xml:lang="en">Neil Brown MK2 conductivity temperature and depth system</skos:prefLabel>
<skos:altLabel>Neil Brown MK2 CTD</skos:altLabel>
<skos:definition xml:lang="en">An integral unit comprising pressure, temperature and conductivity sensors.</skos:definition>
<owl:versionInfo>1</owl:versionInfo>
<dc:date>2010-05-18 16:10:58.0</dc:date>
<skos:note xml:lang="en">accepted</skos:note>
<owl:deprecated>false</owl:deprecated>
<skos:related rdf:resource="http://vocab.nerc.ac.uk/collection/P01/current/PRESPR01/"/>
<skos:related rdf:resource="http://vocab.nerc.ac.uk/collection/P01/current/SIGTPR01/"/>
<skos:related rdf:resource="http://vocab.nerc.ac.uk/collection/P01/current/TEMPST01/"/>
<skos:related rdf:resource="http://vocab.nerc.ac.uk/collection/P01/current/PSALST01/"/>
<skos:related rdf:resource="http://vocab.nerc.ac.uk/collection/P01/current/POTMCV01/"/>
<skos:broader rdf:resource="http://vocab.nerc.ac.uk/collection/L05/current/134/"/>
<skos:broader rdf:resource="http://vocab.nerc.ac.uk/collection/L05/current/130/"/>
<skos:broader rdf:resource="http://vocab.nerc.ac.uk/collection/L05/current/350/"/>
<void:inDataset rdf:resource="http://vocab.nerc.ac.uk/.well-known/void"/>
</skos:Concept>
</skos:member>
<skos:member>
<skos:Concept rdf:about="http://vocab.nerc.ac.uk/collection/L22/current/TOOL0002/">
<dc:identifier>SDN:L22::TOOL0002</dc:identifier>
<skos:notation>SDN:L22::TOOL0002</skos:notation>
<skos:prefLabel xml:lang="en">Neil Brown MK3 CTD</skos:prefLabel>
<skos:altLabel>Neil Brown MK3 CTD</skos:altLabel>
<skos:definition xml:lang="en">The Neil Brown MK3 CTD consists of an integral unit containing pressure, temperature and conductivity sensors with an optional dissolved oxygen sensor in a pressure-hardened casing. The most widely used variant in the 1980s and 1990s was the MK3B. The MK3C fitted with an improved pressure sensor to reduce hysteresis was developed to meet the requirements of the WOCE project. The instrument is no longer in production, but is supported (repair and calibration) by General Oceanics.</skos:definition>
<owl:versionInfo>3</owl:versionInfo>
<dc:date>2010-11-18 12:39:41.0</dc:date>
<skos:note xml:lang="en">accepted</skos:note>
<owl:deprecated>false</owl:deprecated>
<skos:related rdf:resource="http://vocab.nerc.ac.uk/collection/P01/current/OXYSBB01/"/>
<skos:related rdf:resource="http://vocab.nerc.ac.uk/collection/P01/current/SIGTEQ01/"/>
<skos:related rdf:resource="http://vocab.nerc.ac.uk/collection/P01/current/CPHLPR01/"/>
<skos:related rdf:resource="http://vocab.nerc.ac.uk/collection/P01/current/CNDCPR01/"/>
<skos:related rdf:resource="http://vocab.nerc.ac.uk/collection/P01/current/DEPHPR01/"/>
<skos:related rdf:resource="http://vocab.nerc.ac.uk/collection/P01/current/PSALCC01/"/>
<skos:related rdf:resource="http://vocab.nerc.ac.uk/collection/P01/current/TEMPCC01/"/>
<skos:related rdf:resource="http://vocab.nerc.ac.uk/collection/P01/current/TEMPCU01/"/>
<skos:related rdf:resource="http://vocab.nerc.ac.uk/collection/P01/current/POTMCV01/"/>
<skos:related rdf:resource="http://vocab.nerc.ac.uk/collection/P01/current/PSALST01/"/>
<skos:related rdf:resource="http://vocab.nerc.ac.uk/collection/P01/current/CNDCST01/"/>
<skos:related rdf:resource="http://vocab.nerc.ac.uk/collection/P01/current/CNDCZZ01/"/>
<skos:related rdf:resource="http://vocab.nerc.ac.uk/collection/P01/current/PRESPR01/"/>
<skos:related rdf:resource="http://vocab.nerc.ac.uk/collection/P01/current/DOXYPR01/"/>
<skos:related rdf:resource="http://vocab.nerc.ac.uk/collection/P01/current/PSALPR01/"/>
<skos:related rdf:resource="http://vocab.nerc.ac.uk/collection/P01/current/TEMPST01/"/>
<skos:related rdf:resource="http://vocab.nerc.ac.uk/collection/P01/current/SSALPR01/"/>
<skos:related rdf:resource="http://vocab.nerc.ac.uk/collection/P01/current/SIGTPR01/"/>
<skos:related rdf:resource="http://vocab.nerc.ac.uk/collection/P01/current/SSALST01/"/>
<skos:broader rdf:resource="http://vocab.nerc.ac.uk/collection/L05/current/134/"/>
<skos:broader rdf:resource="http://vocab.nerc.ac.uk/collection/L05/current/130/"/>
<skos:broader rdf:resource="http://vocab.nerc.ac.uk/collection/L05/current/350/"/>
<skos:broader rdf:resource="http://vocab.nerc.ac.uk/collection/L05/current/351/"/>
<void:inDataset rdf:resource="http://vocab.nerc.ac.uk/.well-known/void"/>
</skos:Concept>
</skos:member>
<skos:member>
<skos:Concept rdf:about="http://vocab.nerc.ac.uk/collection/L22/current/TOOL0431/">
<dc:identifier>SDN:L22::TOOL0431</dc:identifier>
<skos:notation>SDN:L22::TOOL0431</skos:notation>
<skos:prefLabel xml:lang="en">Neil Brown MK5 conductivity temperature and depth system</skos:prefLabel>
<skos:altLabel>Neil Brown MK5 CTD</skos:altLabel>
<skos:definition xml:lang="en">The Neil Brown MK5 CTD consists of an integral unit containing pressure, temperature and conductivity sensors with an optional dissolved oxygen sensor in a pressure-hardened casing. It provides higher quality salinity data than previous versions of the instrument. It was developed in the 1970s by Neil Brown Instrument Systems, later EG&amp;G, and is no longer in production, but is supported (repair and calibration) by General Oceanics.</skos:definition>
<owl:versionInfo>1</owl:versionInfo>
<dc:date>2011-11-02 11:37:25.0</dc:date>
<skos:note xml:lang="en">accepted</skos:note>
<owl:deprecated>false</owl:deprecated>
<skos:broader rdf:resource="http://vocab.nerc.ac.uk/collection/L05/current/130/"/>
<skos:broader rdf:resource="http://vocab.nerc.ac.uk/collection/L05/current/134/"/>
<skos:broader rdf:resource="http://vocab.nerc.ac.uk/collection/L05/current/350/"/>
<void:inDataset rdf:resource="http://vocab.nerc.ac.uk/.well-known/void"/>
</skos:Concept>
</skos:member>
<skos:member>
<skos:Concept rdf:about="http://vocab.nerc.ac.uk/collection/L22/current/TOOL0033/">
<dc:identifier>SDN:L22::TOOL0033</dc:identifier>
<skos:notation>SDN:L22::TOOL0033</skos:notation>
<skos:prefLabel xml:lang="en">Neil Brown Smart CTD</skos:prefLabel>
<skos:altLabel>Neil Brown Smart CTD</skos:altLabel>
<skos:definition xml:lang="en">The Neil Brown Smart CTD consists of and integral unit containing pressure, temperature and conductivity sensors combined with an integral data logger</skos:definition>
<owl:versionInfo>2</owl:versionInfo>
<dc:date>2009-11-30 16:34:50.0</dc:date>
<skos:note xml:lang="en">accepted</skos:note>
<owl:deprecated>false</owl:deprecated>
<skos:broader rdf:resource="http://vocab.nerc.ac.uk/collection/L05/current/130/"/>
<skos:broader rdf:resource="http://vocab.nerc.ac.uk/collection/L05/current/134/"/>
<skos:broader rdf:resource="http://vocab.nerc.ac.uk/collection/L05/current/350/"/>
<void:inDataset rdf:resource="http://vocab.nerc.ac.uk/.well-known/void"/>
</skos:Concept>
</skos:member>
<skos:member>
<skos:Concept rdf:about="http://vocab.nerc.ac.uk/collection/L22/current/TOOL0552/">
<dc:identifier>SDN:L22::TOOL0552</dc:identifier>
<skos:notation>SDN:L22::TOOL0552</skos:notation>
<skos:prefLabel xml:lang="en">Nereides 300l sample bottle</skos:prefLabel>
<skos:altLabel>Nereides 300l bottle</skos:altLabel>
<skos:definition xml:lang="en">A 300 litre capacity sampling bottle designed for oceanographic sampling. The bottle was closed by a messenger. It was used during the OMEX project in the 1990s.</skos:definition>
<owl:versionInfo>1</owl:versionInfo>
<dc:date>2012-09-26 17:11:56.0</dc:date>
<skos:note xml:lang="en">accepted</skos:note>
<owl:deprecated>false</owl:deprecated>
<skos:broader rdf:resource="http://vocab.nerc.ac.uk/collection/L05/current/30/"/>
<void:inDataset rdf:resource="http://vocab.nerc.ac.uk/.well-known/void"/>
</skos:Concept>
</skos:member>
<skos:member>
<skos:Concept rdf:about="http://vocab.nerc.ac.uk/collection/L22/current/NETT0113/">
<dc:identifier>SDN:L22::NETT0113</dc:identifier>
<skos:notation>SDN:L22::NETT0113</skos:notation>
<skos:prefLabel xml:lang="en">Neuston net - David (1965)</skos:prefLabel>
<skos:altLabel>David neuston net</skos:altLabel>
<skos:definition xml:lang="en">Has a 30 cm x 15 cm rectangular mouth opening with a net 365 cm in length (21.3 meshes to cm). Normally towed at 5-6 knots [Wiebe and Benfield 2003 Plate 20 D].</skos:definition>
<owl:versionInfo>1</owl:versionInfo>
<dc:date>2011-10-21 14:18:49.0</dc:date>
<skos:note xml:lang="en">accepted</skos:note>
<owl:deprecated>false</owl:deprecated>
<skos:broader rdf:resource="http://vocab.nerc.ac.uk/collection/L05/current/69/"/>
<void:inDataset rdf:resource="http://vocab.nerc.ac.uk/.well-known/void"/>
</skos:Concept>
</skos:member>
<skos:member>
<skos:Concept rdf:about="http://vocab.nerc.ac.uk/collection/L22/current/NETT0111/">
<dc:identifier>SDN:L22::NETT0111</dc:identifier>
<skos:notation>SDN:L22::NETT0111</skos:notation>
<skos:prefLabel xml:lang="en">Neuston net - Ellertsen (1977)</skos:prefLabel>
<skos:altLabel>Ellertsen neuston net</skos:altLabel>
<skos:definition xml:lang="en">Six stacked nets two with 10 cm tall x 25 cm wide rectangular mouth opening and four with 20 cm tall x 25 cm wide mouths. Nets 100 cm long made of 0.2 mm nylon mesh. Pontoons made of fiberglass covered Styrofoam 10 x 15 x 100 cm. A flowmeter can be used [Wiebe and Benfield 2003 Plate 21 C].</skos:definition>
<owl:versionInfo>1</owl:versionInfo>
<dc:date>2011-10-21 14:18:49.0</dc:date>
<skos:note xml:lang="en">accepted</skos:note>
<owl:deprecated>false</owl:deprecated>
<skos:broader rdf:resource="http://vocab.nerc.ac.uk/collection/L05/current/69/"/>
<void:inDataset rdf:resource="http://vocab.nerc.ac.uk/.well-known/void"/>
</skos:Concept>
</skos:member>
<skos:member>
<skos:Concept rdf:about="http://vocab.nerc.ac.uk/collection/L22/current/NETT0110/">
<dc:identifier>SDN:L22::NETT0110</dc:identifier>
<skos:notation>SDN:L22::NETT0110</skos:notation>
<skos:prefLabel xml:lang="en">Neuston net - Lippincott and Thomas (1983)</skos:prefLabel>
<skos:altLabel>Lippincott neuston net</skos:altLabel>
<skos:definition xml:lang="en">Has a 128 cm wide x 30 cm tall rectangular mouth opening with 260 cm long net with 0.351 mm nylon mesh. A TSK flowmeter is mounted in the lower portion of the net mouth. Lobster buoy floats provide buoyancy.</skos:definition>
<owl:versionInfo>1</owl:versionInfo>
<dc:date>2011-10-21 14:18:49.0</dc:date>
<skos:note xml:lang="en">accepted</skos:note>
<owl:deprecated>false</owl:deprecated>
<skos:broader rdf:resource="http://vocab.nerc.ac.uk/collection/L05/current/388/"/>
<skos:broader rdf:resource="http://vocab.nerc.ac.uk/collection/L05/current/69/"/>
<void:inDataset rdf:resource="http://vocab.nerc.ac.uk/.well-known/void"/>
</skos:Concept>
</skos:member>
<skos:member>
<skos:Concept rdf:about="http://vocab.nerc.ac.uk/collection/L22/current/NETT0112/">
<dc:identifier>SDN:L22::NETT0112</dc:identifier>
<skos:notation>SDN:L22::NETT0112</skos:notation>
<skos:prefLabel xml:lang="en">Neuston net - Sconfietti and Cantonati (1990)</skos:prefLabel>
<skos:altLabel>Sconfietti neuston net</skos:altLabel>
<skos:definition xml:lang="en">A 40 cm diameter net (60 cm long) is attached at the front and rear to a polyurethane float by rods extending down below the float with the top of net about 12 cm below the surface.  [Wiebe and Benfield 2003 Plate 20 F]</skos:definition>
<owl:versionInfo>1</owl:versionInfo>
<dc:date>2011-10-21 14:18:49.0</dc:date>
<skos:note xml:lang="en">accepted</skos:note>
<owl:deprecated>false</owl:deprecated>
<skos:broader rdf:resource="http://vocab.nerc.ac.uk/collection/L05/current/69/"/>
<void:inDataset rdf:resource="http://vocab.nerc.ac.uk/.well-known/void"/>
</skos:Concept>
</skos:member>
<skos:member>
<skos:Concept rdf:about="http://vocab.nerc.ac.uk/collection/L22/current/NETT0116/">
<dc:identifier>SDN:L22::NETT0116</dc:identifier>
<skos:notation>SDN:L22::NETT0116</skos:notation>
<skos:prefLabel xml:lang="en">Neuston net - Willis (1963)</skos:prefLabel>
<skos:altLabel>Willis neuston net</skos:altLabel>
<skos:definition xml:lang="en">Has a 17.8 cm x 3.8 cm rectangular mouth opening of net 67.3 cm long (netting nylon with 78.7 meshes/cm).  Normally towed while ship drifting at 1 knot [Wiebe and Benfield 2003 Plate 20 C].</skos:definition>
<owl:versionInfo>1</owl:versionInfo>
<dc:date>2011-10-21 14:18:49.0</dc:date>
<skos:note xml:lang="en">accepted</skos:note>
<owl:deprecated>false</owl:deprecated>
<skos:broader rdf:resource="http://vocab.nerc.ac.uk/collection/L05/current/69/"/>
<void:inDataset rdf:resource="http://vocab.nerc.ac.uk/.well-known/void"/>
</skos:Concept>
</skos:member>
<skos:member>
<skos:Concept rdf:about="http://vocab.nerc.ac.uk/collection/L22/current/NETT0114/">
<dc:identifier>SDN:L22::NETT0114</dc:identifier>
<skos:notation>SDN:L22::NETT0114</skos:notation>
<skos:prefLabel xml:lang="en">Neuston net - Zaitsev (1959, 1970)</skos:prefLabel>
<skos:altLabel>Zaitsev neuston net</skos:altLabel>
<skos:definition xml:lang="en">Has a 60cm x 20 cm rectangular mouth aperture with a net 250 cm long with plastic foam floats 20 cm x 10 cm x 4 cm attached to sides of metal net frame.  Used from drifting or anchored vessel [Wiebe and Benfield 2003 Plate 20 A].</skos:definition>
<owl:versionInfo>1</owl:versionInfo>
<dc:date>2011-10-21 14:18:49.0</dc:date>
<skos:note xml:lang="en">accepted</skos:note>
<owl:deprecated>false</owl:deprecated>
<skos:broader rdf:resource="http://vocab.nerc.ac.uk/collection/L05/current/69/"/>
<void:inDataset rdf:resource="http://vocab.nerc.ac.uk/.well-known/void"/>
</skos:Concept>
</skos:member>
<skos:member>
<skos:Concept rdf:about="http://vocab.nerc.ac.uk/collection/L22/current/NETT0117/">
<dc:identifier>SDN:L22::NETT0117</dc:identifier>
<skos:notation>SDN:L22::NETT0117</skos:notation>
<skos:prefLabel xml:lang="en">Neuston sampler - Danielssen and Tveite (1968)</skos:prefLabel>
<skos:altLabel>Danielssen neuston Sampler</skos:altLabel>
<skos:definition xml:lang="en">A framework supports five rectangular nets with mesh sizes ranging from 0.150 to 0.500 mm. A flowmeter is used.</skos:definition>
<owl:versionInfo>1</owl:versionInfo>
<dc:date>2011-10-21 14:18:49.0</dc:date>
<skos:note xml:lang="en">accepted</skos:note>
<owl:deprecated>false</owl:deprecated>
<skos:broader rdf:resource="http://vocab.nerc.ac.uk/collection/L05/current/388/"/>
<skos:broader rdf:resource="http://vocab.nerc.ac.uk/collection/L05/current/69/"/>
<void:inDataset rdf:resource="http://vocab.nerc.ac.uk/.well-known/void"/>
</skos:Concept>
</skos:member>
<skos:member>
<skos:Concept rdf:about="http://vocab.nerc.ac.uk/collection/L22/current/NETT0118/">
<dc:identifier>SDN:L22::NETT0118</dc:identifier>
<skos:notation>SDN:L22::NETT0118</skos:notation>
<skos:prefLabel xml:lang="en">Neuston sampler - Sameoto and Jaroszynski (1969)</skos:prefLabel>
<skos:altLabel>Sameoto neuston sampler</skos:altLabel>
<skos:definition xml:lang="en">Has a 102 cm x 102 cm square mouth opening aluminum box frame 152 cm long equipped with foam floatation on top, a pair of fins on the side, and a fin on the bottom.  Attached to the back is a net 104 cm x 104 cm at the mouth and 927 cm long made from 0.308 mm nylon mesh. A two-part towing bridle was attached to one side and the sampler kited out away from the side of the vessel beyond the ships wake. Towing speeds 8 to 11 knots [Wiebe and Benfield 2003 Plate 20 E].</skos:definition>
<owl:versionInfo>1</owl:versionInfo>
<dc:date>2011-10-21 14:18:49.0</dc:date>
<skos:note xml:lang="en">accepted</skos:note>
<owl:deprecated>false</owl:deprecated>
<skos:broader rdf:resource="http://vocab.nerc.ac.uk/collection/L05/current/69/"/>
<void:inDataset rdf:resource="http://vocab.nerc.ac.uk/.well-known/void"/>
</skos:Concept>
</skos:member>
<skos:member>
<skos:Concept rdf:about="http://vocab.nerc.ac.uk/collection/L22/current/NETT0119/">
<dc:identifier>SDN:L22::NETT0119</dc:identifier>
<skos:notation>SDN:L22::NETT0119</skos:notation>
<skos:prefLabel xml:lang="en">Neuston sampler - Schram et al. (1981)</skos:prefLabel>
<skos:altLabel>Schram neuston Sampler</skos:altLabel>
<skos:definition xml:lang="en">A framework supports five 50 cm x 20 cm mouth opening rectangular nets each 125 cm long with mesh sizes ranging from 0.150 to 0.500 mm. Frame equipped with a flowmeter is used [Wiebe and Benfield 2003 Plate 21 D].</skos:definition>
<owl:versionInfo>1</owl:versionInfo>
<dc:date>2011-10-21 14:18:49.0</dc:date>
<skos:note xml:lang="en">accepted</skos:note>
<owl:deprecated>false</owl:deprecated>
<skos:broader rdf:resource="http://vocab.nerc.ac.uk/collection/L05/current/388/"/>
<skos:broader rdf:resource="http://vocab.nerc.ac.uk/collection/L05/current/69/"/>
<void:inDataset rdf:resource="http://vocab.nerc.ac.uk/.well-known/void"/>
</skos:Concept>
</skos:member>
<skos:member>
<skos:Concept rdf:about="http://vocab.nerc.ac.uk/collection/L22/current/TOOL0610/">
<dc:identifier>SDN:L22::TOOL0610</dc:identifier>
<skos:notation>SDN:L22::TOOL0610</skos:notation>
<skos:prefLabel xml:lang="en">Neyrpic bubbler pressure gauge</skos:prefLabel>
<skos:altLabel>Neyrpic bubbler</skos:altLabel>
<skos:definition xml:lang="en">An early tide gauge comprising a seabed-mounted gas outlet and a manometer to measure the compressed gas pressure necessary to force gas through this outlet. The manometer comprised a stainless steel float in a tube that was connected through pulleys to a clockwork chart recorder. Chart advance speed was 2.5, 5, 10 or 20 mm/hour (10 mm/hour was generally used for tidal measurements) and pressure ranges corresponding to depth scales of 0-3m, 0-6m, 0-9m, 0-12m or 0-18m were available. More information may be found in http://www.bodc.ac.uk/data/documents/nodb/27190/</skos:definition>
<owl:versionInfo>2</owl:versionInfo>
<dc:date>2013-04-10 16:41:24.0</dc:date>
<skos:note xml:lang="en">accepted</skos:note>
<owl:deprecated>false</owl:deprecated>
<skos:broader rdf:resource="http://vocab.nerc.ac.uk/collection/L05/current/111/"/>
<void:inDataset rdf:resource="http://vocab.nerc.ac.uk/.well-known/void"/>
</skos:Concept>
</skos:member>
<skos:member>
<skos:Concept rdf:about="http://vocab.nerc.ac.uk/collection/L22/current/TOOL0412/">
<dc:identifier>SDN:L22::TOOL0412</dc:identifier>
<skos:notation>SDN:L22::TOOL0412</skos:notation>
<skos:prefLabel xml:lang="en">Niskin bottle</skos:prefLabel>
<skos:altLabel>Niskin bottle</skos:altLabel>
<skos:definition xml:lang="en">A plastic free-flushing water sampling bottle with a capacity of 1.7-30 litres. It has caps with rubber seals at each end joined by a plastic-coated metal spring or elastic cord running through the interior of the bottle. It is deployed with the caps held open against the spring by plastic lanyards. When the bottle reaches the desired depth the lanyards are released by a pressure-actuated switch, command signal or messenger weight and the caps are forced shut and sealed. Bottles may be deployed singly clamped to a wire or in groups of up to 48 on a rosette. Reversing thermometers may be attached to a spring-loaded disk that rotates through 180 degrees on bottle closure.</skos:definition>
<owl:versionInfo>2</owl:versionInfo>
<dc:date>2012-06-22 13:43:26.0</dc:date>
<skos:note xml:lang="en">accepted</skos:note>
<owl:deprecated>false</owl:deprecated>
<skos:broader rdf:resource="http://vocab.nerc.ac.uk/collection/L05/current/30/"/>
<void:inDataset rdf:resource="http://vocab.nerc.ac.uk/.well-known/void"/>
</skos:Concept>
</skos:member>
<skos:member>
<skos:Concept rdf:about="http://vocab.nerc.ac.uk/collection/L22/current/TOOL0413/">
<dc:identifier>SDN:L22::TOOL0413</dc:identifier>
<skos:notation>SDN:L22::TOOL0413</skos:notation>
<skos:prefLabel xml:lang="en">Non-toxic sea water supply</skos:prefLabel>
<skos:altLabel>Non-toxic supply</skos:altLabel>
<skos:definition xml:lang="en">A source of uncontaminated near-surface (commonly 3 to 7 m) seawater pumped continuously to shipboard laboratories on research vessels. There is typically a temperature sensor near the intake (known as the hull temperature) to provide measurements that are as close as possible to the ambient water temperature. The flow from the supply is typically directed through continuously logged sensors such as a thermosalinograph and a fluorometer. Water samples are often collected from the non-toxic supply. The system is also referred to as the underway supply.</skos:definition>
<owl:versionInfo>1</owl:versionInfo>
<dc:date>2011-08-05 09:08:32.0</dc:date>
<skos:note xml:lang="en">accepted</skos:note>
<owl:deprecated>false</owl:deprecated>
<skos:broader rdf:resource="http://vocab.nerc.ac.uk/collection/L05/current/31/"/>
<void:inDataset rdf:resource="http://vocab.nerc.ac.uk/.well-known/void"/>
</skos:Concept>
</skos:member>
<skos:member>
<skos:Concept rdf:about="http://vocab.nerc.ac.uk/collection/L22/current/TOOL0477/">
<dc:identifier>SDN:L22::TOOL0477</dc:identifier>
<skos:notation>SDN:L22::TOOL0477</skos:notation>
<skos:prefLabel xml:lang="en">Nortek Aquadopp 3000 3D Doppler current meter</skos:prefLabel>
<skos:altLabel>Nortek Aquadopp 3000</skos:altLabel>
<skos:definition xml:lang="en">The Nortek Aquadopp 3000 is a single-depth doppler current meter designed for deployment in intermediate water depths down to 3000 m. It is suitable for use on moorings or fixed structures. It features higher power and an increased signal-to-noise ratio compared with the standard (300 m depth rated) Aquadopp so that it can provide accurate current measurements in water with low concentrations of suspended particulate matter. Current velocity is derived from the Doppler shift measured by two or three 2MHz acoustic beams. It comes with compass, tilt, pressure and temperature sensors. Data are stored on an internal data logger. It can be run in 'diagnostic' mode when set to collect data at 1 Hz frequency in user specified intervals, which allows studies of mooring motion and the performance of other current meters to be conducted.</skos:definition>
<owl:versionInfo>1</owl:versionInfo>
<dc:date>2012-03-06 15:57:11.0</dc:date>
<skos:note xml:lang="en">accepted</skos:note>
<owl:deprecated>false</owl:deprecated>
<skos:broader rdf:resource="http://vocab.nerc.ac.uk/collection/L05/current/134/"/>
<skos:broader rdf:resource="http://vocab.nerc.ac.uk/collection/L05/current/114/"/>
<skos:broader rdf:resource="http://vocab.nerc.ac.uk/collection/L22/current/TOOL0089/"/>
<void:inDataset rdf:resource="http://vocab.nerc.ac.uk/.well-known/void"/>
</skos:Concept>
</skos:member>
<skos:member>
<skos:Concept rdf:about="http://vocab.nerc.ac.uk/collection/L22/current/TOOL0089/">
<dc:identifier>SDN:L22::TOOL0089</dc:identifier>
<skos:notation>SDN:L22::TOOL0089</skos:notation>
<skos:prefLabel xml:lang="en">Nortek Aquadopp 3D doppler current meter</skos:prefLabel>
<skos:altLabel>Nortek Aquadopp</skos:altLabel>
<skos:definition xml:lang="en">The Aquadopp is a single-depth doppler current meter designed both for real time data collection and self contained deployments logging internally. It comes with compass, tilt, pressure and temperature sensors. It can also be configured to measure surface wave height, period and direction concurrently. It has the unique feature of being run in 'diagnostic' mode when set to collect data at 1 Hz frequency in user specified intervals. This allows studies of mooring motion and the performance of other current meters to be conducted. It can be set in various configurations with titanium housings for deployment at greater depths.</skos:definition>
<owl:versionInfo>1</owl:versionInfo>
<dc:date>2009-11-30 11:56:35.0</dc:date>
<skos:note xml:lang="en">accepted</skos:note>
<owl:deprecated>false</owl:deprecated>
<skos:narrower rdf:resource="http://vocab.nerc.ac.uk/collection/L22/current/TOOL0476/"/>
<skos:narrower rdf:resource="http://vocab.nerc.ac.uk/collection/L22/current/TOOL0477/"/>
<skos:broader rdf:resource="http://vocab.nerc.ac.uk/collection/L05/current/134/"/>
<skos:broader rdf:resource="http://vocab.nerc.ac.uk/collection/L05/current/114/"/>
<void:inDataset rdf:resource="http://vocab.nerc.ac.uk/.well-known/void"/>
</skos:Concept>
</skos:member>
<skos:member>
<skos:Concept rdf:about="http://vocab.nerc.ac.uk/collection/L22/current/TOOL0392/">
<dc:identifier>SDN:L22::TOOL0392</dc:identifier>
<skos:notation>SDN:L22::TOOL0392</skos:notation>
<skos:prefLabel xml:lang="en">Nortek Aquadopp 400 kHz Doppler current profiler</skos:prefLabel>
<skos:altLabel>Aquadopp 400 kHz profiler</skos:altLabel>
<skos:definition xml:lang="en">A self-contained 400 kHz Doppler current profiler designed for deployment on the seabed, moorings, buoys or fixed structures. The instrument uses 3 beams to measure water velocities over a range of +/-10 m/s and has a standard depth rating of 100 m. Depth cell size ranges from 2-8 m, with a maximum of 128 cells.</skos:definition>
<owl:versionInfo>1</owl:versionInfo>
<dc:date>2011-04-14 09:29:16.0</dc:date>
<skos:note xml:lang="en">accepted</skos:note>
<owl:deprecated>false</owl:deprecated>
<skos:broader rdf:resource="http://vocab.nerc.ac.uk/collection/L05/current/115/"/>
<void:inDataset rdf:resource="http://vocab.nerc.ac.uk/.well-known/void"/>
</skos:Concept>
</skos:member>
<skos:member>
<skos:Concept rdf:about="http://vocab.nerc.ac.uk/collection/L22/current/TOOL0476/">
<dc:identifier>SDN:L22::TOOL0476</dc:identifier>
<skos:notation>SDN:L22::TOOL0476</skos:notation>
<skos:prefLabel xml:lang="en">Nortek Aquadopp 6000 3D Doppler current meter</skos:prefLabel>
<skos:altLabel>Nortek Aquadopp 6000</skos:altLabel>
<skos:definition xml:lang="en">The Nortek Aquadopp 6000 is a single-depth doppler current meter designed for deployment on deep water moorings, although it is also suitable for attachment to fixed structures. It features higher power and an increased signal-to-noise ratio compared with the standard (300 m depth rated) Aquadopp so that it can provide accurate current measurements in water with low concentrations of suspended particulate matter. Current velocity is derived from the Doppler shift measured by two or three 2MHz acoustic beams. It comes with compass, tilt, pressure and temperature sensors. It has a titanium casing rated to 6000 m and data are stored on an internal logger. It can be run in 'diagnostic' mode when set to collect data at 1 Hz frequency in user specified intervals, which allows studies of mooring motion and the performance of other current meters to be conducted.</skos:definition>
<owl:versionInfo>1</owl:versionInfo>
<dc:date>2012-03-06 15:57:11.0</dc:date>
<skos:note xml:lang="en">accepted</skos:note>
<owl:deprecated>false</owl:deprecated>
<skos:broader rdf:resource="http://vocab.nerc.ac.uk/collection/L05/current/114/"/>
<skos:broader rdf:resource="http://vocab.nerc.ac.uk/collection/L22/current/TOOL0089/"/>
<skos:broader rdf:resource="http://vocab.nerc.ac.uk/collection/L05/current/134/"/>
<void:inDataset rdf:resource="http://vocab.nerc.ac.uk/.well-known/void"/>
</skos:Concept>
</skos:member>
<skos:member>
<skos:Concept rdf:about="http://vocab.nerc.ac.uk/collection/L22/current/NETT0122/">
<dc:identifier>SDN:L22::NETT0122</dc:identifier>
<skos:notation>SDN:L22::NETT0122</skos:notation>
<skos:prefLabel xml:lang="en">North Pacific standard net  - Motoda (1957)</skos:prefLabel>
<skos:altLabel>NorPac net</skos:altLabel>
<skos:definition xml:lang="en">Has a 45 cm mouth diameter with a conical net length of 180 cm (mesh 0.33 mm - GG54) [Wiebe and Benfield 2003 Plate 1 F].</skos:definition>
<owl:versionInfo>1</owl:versionInfo>
<dc:date>2011-10-21 14:18:49.0</dc:date>
<skos:note xml:lang="en">accepted</skos:note>
<owl:deprecated>false</owl:deprecated>
<skos:broader rdf:resource="http://vocab.nerc.ac.uk/collection/L05/current/22/"/>
<void:inDataset rdf:resource="http://vocab.nerc.ac.uk/.well-known/void"/>
</skos:Concept>
</skos:member>
<skos:member>
<skos:Concept rdf:about="http://vocab.nerc.ac.uk/collection/L22/current/TOOL0516/">
<dc:identifier>SDN:L22::TOOL0516</dc:identifier>
<skos:notation>SDN:L22::TOOL0516</skos:notation>
<skos:prefLabel xml:lang="en">Nu Instruments Plasma 1700 High Resolution Multi Collector inductively coupled plasma mass spectrometer</skos:prefLabel>
<skos:altLabel>Nu Plasma 1700 MC-ICP-MS</skos:altLabel>
<skos:definition xml:lang="en">The Nu Plasma 1700 High Resolution Multi Collector inductively coupled plasma mass spectrometer (MC-ICP-MS) is designed for high resolution isotope ratio measurements. The instrument features a high dispersion and large geometry to provide a high mass resolution of 700 to 3000 m/Dm (10% valley convention) whilst still maintaining flat top peaks for high precision measurements with minimal loss in sensitivity. The instrument has a mass dispersion of 17% at zoom magnification 1 and is equipped with 16 Faraday cups: ten incorporated in a fixed central array and three each to the low and high mass side as well as three secondary electron multipliers, of which one is equipped with an abundance sensitivity filter. Independent computer controlled adjustable slits positioned in front of all detectors, allow movement in width and central position providing perfect alignment of the peaks of interest.</skos:definition>
<owl:versionInfo>1</owl:versionInfo>
<dc:date>2012-07-04 10:02:10.0</dc:date>
<skos:note xml:lang="en">accepted</skos:note>
<owl:deprecated>false</owl:deprecated>
<skos:broader rdf:resource="http://vocab.nerc.ac.uk/collection/L05/current/LAB15/"/>
<void:inDataset rdf:resource="http://vocab.nerc.ac.uk/.well-known/void"/>
</skos:Concept>
</skos:member>
<skos:member>
<skos:Concept rdf:about="http://vocab.nerc.ac.uk/collection/L22/current/TOOL0522/">
<dc:identifier>SDN:L22::TOOL0522</dc:identifier>
<skos:notation>SDN:L22::TOOL0522</skos:notation>
<skos:prefLabel xml:lang="en">Nu Instruments Plasma I (HR) Multi-Collector Inductively Coupled Plasma Mass Spectrometer</skos:prefLabel>
<skos:altLabel>Nu Plasma I MC-ICP-MS</skos:altLabel>
<skos:definition xml:lang="en">A double focusing multi-collector inductively coupled plasma mass spectrometer (MC-ICP-MS) featuring unique variable dispersion optics. The instrument includes: a double focusing system, vacuum system, zoom optics, Faraday detector system, multiplier detector system, water cooling and computer systems. Twelve Faraday detectors are fitted to the instrument as standard and up to three ion-counting multiplier channels can be specified for the standard collector housing. Deflection with a magnet and second electrostatic anaylser compensates for any energy spread of the ion beam.</skos:definition>
<owl:versionInfo>1</owl:versionInfo>
<dc:date>2012-07-05 15:53:41.0</dc:date>
<skos:note xml:lang="en">accepted</skos:note>
<owl:deprecated>false</owl:deprecated>
<skos:broader rdf:resource="http://vocab.nerc.ac.uk/collection/L05/current/LAB15/"/>
<void:inDataset rdf:resource="http://vocab.nerc.ac.uk/.well-known/void"/>
</skos:Concept>
</skos:member>
<skos:member>
<skos:Concept rdf:about="http://vocab.nerc.ac.uk/collection/L22/current/NETT0131/">
<dc:identifier>SDN:L22::NETT0131</dc:identifier>
<skos:notation>SDN:L22::NETT0131</skos:notation>
<skos:prefLabel xml:lang="en">ORI nets - Omori (1965)</skos:prefLabel>
<skos:altLabel>ORI nets</skos:altLabel>
<skos:definition xml:lang="en">Generic term for 160 cm cylinder-cone nets equipped for a Motoda double releasing mechanism.</skos:definition>
<owl:versionInfo>1</owl:versionInfo>
<dc:date>2011-10-21 14:18:49.0</dc:date>
<skos:note xml:lang="en">accepted</skos:note>
<owl:deprecated>false</owl:deprecated>
<skos:broader rdf:resource="http://vocab.nerc.ac.uk/collection/L05/current/22/"/>
<void:inDataset rdf:resource="http://vocab.nerc.ac.uk/.well-known/void"/>
</skos:Concept>
</skos:member>
<skos:member>
<skos:Concept rdf:about="http://vocab.nerc.ac.uk/collection/L22/current/NETT0132/">
<dc:identifier>SDN:L22::NETT0132</dc:identifier>
<skos:notation>SDN:L22::NETT0132</skos:notation>
<skos:prefLabel xml:lang="en">ORI-200 - Omori (1965)</skos:prefLabel>
<skos:altLabel>ORI-200 net</skos:altLabel>
<skos:definition xml:lang="en">Has a 160 cm diameter mouth opening with 2x70 cm long cylinder sections plus 2 conical sections 450 cm. All 1.97 mm mesh. Equipped for a Motoda double releasing mechanism.</skos:definition>
<owl:versionInfo>1</owl:versionInfo>
<dc:date>2011-10-21 14:18:49.0</dc:date>
<skos:note xml:lang="en">accepted</skos:note>
<owl:deprecated>false</owl:deprecated>
<skos:broader rdf:resource="http://vocab.nerc.ac.uk/collection/L05/current/22/"/>
<void:inDataset rdf:resource="http://vocab.nerc.ac.uk/.well-known/void"/>
</skos:Concept>
</skos:member>
<skos:member>
<skos:Concept rdf:about="http://vocab.nerc.ac.uk/collection/L22/current/NETT0169/">
<dc:identifier>SDN:L22::NETT0169</dc:identifier>
<skos:notation>SDN:L22::NETT0169</skos:notation>
<skos:prefLabel xml:lang="en">ORI-33 - Omori (1965)</skos:prefLabel>
<skos:altLabel>ORI-33 net</skos:altLabel>
<skos:definition xml:lang="en">Has a 160 cm diameter mouth opening with 2x70 cm long cylinder sections plus 2 conical sections 450 cm. All GG 54 silk netting. Equipped for a Motoda double releasing mechanism.</skos:definition>
<owl:versionInfo>1</owl:versionInfo>
<dc:date>2011-10-21 14:18:49.0</dc:date>
<skos:note xml:lang="en">accepted</skos:note>
<owl:deprecated>false</owl:deprecated>
<skos:broader rdf:resource="http://vocab.nerc.ac.uk/collection/L05/current/22/"/>
<void:inDataset rdf:resource="http://vocab.nerc.ac.uk/.well-known/void"/>
</skos:Concept>
</skos:member>
<skos:member>
<skos:Concept rdf:about="http://vocab.nerc.ac.uk/collection/L22/current/NETT0133/">
<dc:identifier>SDN:L22::NETT0133</dc:identifier>
<skos:notation>SDN:L22::NETT0133</skos:notation>
<skos:prefLabel xml:lang="en">ORI-C - Omori (1965)</skos:prefLabel>
<skos:altLabel>ORI-C net</skos:altLabel>
<skos:definition xml:lang="en">Has a 160 cm diameter mouth opening with 2x70 cm long cylinder sections made of 1.97 mm mesh and sail cloth plus 2 conical sections 450 cm (1.97 mm mesh) and 150 cm (.33 mm mesh). Equipped for a Motoda double releasing mechanism.</skos:definition>
<owl:versionInfo>1</owl:versionInfo>
<dc:date>2011-10-21 14:18:49.0</dc:date>
<skos:note xml:lang="en">accepted</skos:note>
<owl:deprecated>false</owl:deprecated>
<skos:broader rdf:resource="http://vocab.nerc.ac.uk/collection/L05/current/22/"/>
<void:inDataset rdf:resource="http://vocab.nerc.ac.uk/.well-known/void"/>
</skos:Concept>
</skos:member>
<skos:member>
<skos:Concept rdf:about="http://vocab.nerc.ac.uk/collection/L22/current/TOOL0660/">
<dc:identifier>SDN:L22::TOOL0660</dc:identifier>
<skos:notation>SDN:L22::TOOL0660</skos:notation>
<skos:prefLabel xml:lang="en">OSIL Marine Snow Catcher</skos:prefLabel>
<skos:altLabel>OSIL MSC</skos:altLabel>
<skos:definition xml:lang="en">The Marine Snow Catcher is a large volume water bottle designed to collect Marine Snow particles. The water transport through the device during the descent is controlled through two large diameter terminal apertures constructed to reduce turbulence. The device is usually rested upright after recovery to allow the marine particles to sink to the bottom, after which, the overlying water is slowly drained off via a tap. The bottom section of the water bottle is detachable allowing recovery of the marine snow.</skos:definition>
<owl:versionInfo>2</owl:versionInfo>
<dc:date>2014-01-28 11:01:06.0</dc:date>
<skos:note xml:lang="en">accepted</skos:note>
<owl:deprecated>false</owl:deprecated>
<skos:broader rdf:resource="http://vocab.nerc.ac.uk/collection/L05/current/30/"/>
<void:inDataset rdf:resource="http://vocab.nerc.ac.uk/.well-known/void"/>
</skos:Concept>
</skos:member>
<skos:member>
<skos:Concept rdf:about="http://vocab.nerc.ac.uk/collection/L22/current/NETT0134/">
<dc:identifier>SDN:L22::NETT0134</dc:identifier>
<skos:notation>SDN:L22::NETT0134</skos:notation>
<skos:prefLabel xml:lang="en">Ocean Research Institute Vertical Muliple Plankton Sampler - Terazaki (1991)</skos:prefLabel>
<skos:altLabel>ORI-VMPS</skos:altLabel>
<skos:definition xml:lang="en">Has a 100 cm x 100 cm rectangular mouth opening multiple net system that can be equipped with 4 to 10 nets 510 cm long with 0.33 mm nylon mesh.  Nets are opened/closed by surface commands down transmitted via conduction cable to an underwater unit [Wiebe and Benfield 2003 Plate 31 C].</skos:definition>
<owl:versionInfo>1</owl:versionInfo>
<dc:date>2011-10-21 14:18:49.0</dc:date>
<skos:note xml:lang="en">accepted</skos:note>
<owl:deprecated>false</owl:deprecated>
<skos:broader rdf:resource="http://vocab.nerc.ac.uk/collection/L05/current/22/"/>
<skos:broader rdf:resource="http://vocab.nerc.ac.uk/collection/L05/current/68/"/>
<void:inDataset rdf:resource="http://vocab.nerc.ac.uk/.well-known/void"/>
</skos:Concept>
</skos:member>
<skos:member>
<skos:Concept rdf:about="http://vocab.nerc.ac.uk/collection/L22/current/TOOL0276/">
<dc:identifier>SDN:L22::TOOL0276</dc:identifier>
<skos:notation>SDN:L22::TOOL0276</skos:notation>
<skos:prefLabel xml:lang="en">OceanData TSG103 thermosalinograph</skos:prefLabel>
<skos:altLabel>TSG103 thermosalinograph</skos:altLabel>
<skos:definition xml:lang="en">An autoranging instrument taking inputs from a hull or inlet thermometer to give sea temperature plus co-located temperature and conductivity sensors to give salinity. In general use during the 1980s and 1990s</skos:definition>
<owl:versionInfo>1</owl:versionInfo>
<dc:date>2010-05-18 16:10:58.0</dc:date>
<skos:note xml:lang="en">accepted</skos:note>
<owl:deprecated>false</owl:deprecated>
<skos:related rdf:resource="http://vocab.nerc.ac.uk/collection/P01/current/TEMPSG01/"/>
<skos:related rdf:resource="http://vocab.nerc.ac.uk/collection/P01/current/PSALSG01/"/>
<skos:broader rdf:resource="http://vocab.nerc.ac.uk/collection/L05/current/350/"/>
<skos:broader rdf:resource="http://vocab.nerc.ac.uk/collection/L05/current/133/"/>
<skos:broader rdf:resource="http://vocab.nerc.ac.uk/collection/L05/current/134/"/>
<void:inDataset rdf:resource="http://vocab.nerc.ac.uk/.well-known/void"/>
</skos:Concept>
</skos:member>
<skos:member>
<skos:Concept rdf:about="http://vocab.nerc.ac.uk/collection/L22/current/NETT0125/">
<dc:identifier>SDN:L22::NETT0125</dc:identifier>
<skos:notation>SDN:L22::NETT0125</skos:notation>
<skos:prefLabel xml:lang="en">Octagon net - Sameoto and Jaroszynski (1976)</skos:prefLabel>
<skos:altLabel>Sameoto octagon net</skos:altLabel>
<skos:definition xml:lang="en">Has a 75 cm diameter iron channel octagon mouth opening which was attached to the towing wire with stainless steel snap swivels and held from sliding down by a stop on the wire. Used with a net made of 1 mm nylon mesh and towed at speeds up to 7 knots [Wiebe and Benfield 2003 Plate 3 C].</skos:definition>
<owl:versionInfo>1</owl:versionInfo>
<dc:date>2011-10-21 14:18:49.0</dc:date>
<skos:note xml:lang="en">accepted</skos:note>
<owl:deprecated>false</owl:deprecated>
<skos:broader rdf:resource="http://vocab.nerc.ac.uk/collection/L05/current/22/"/>
<skos:broader rdf:resource="http://vocab.nerc.ac.uk/collection/L05/current/67/"/>
<void:inDataset rdf:resource="http://vocab.nerc.ac.uk/.well-known/void"/>
</skos:Concept>
</skos:member>
<skos:member>
<skos:Concept rdf:about="http://vocab.nerc.ac.uk/collection/L22/current/TOOL0575/">
<dc:identifier>SDN:L22::TOOL0575</dc:identifier>
<skos:notation>SDN:L22::TOOL0575</skos:notation>
<skos:prefLabel xml:lang="en">Olympus BH2 series system microscope</skos:prefLabel>
<skos:altLabel>Olympus BH2</skos:altLabel>
<skos:definition xml:lang="en">A polarized light microscope that uses Koehler illumination for high performance microscopic techniques. The instrument utilises a coarse stage adjustment and coaxial focusing. A camera can be attached for use in photo micrography. The Olympus BH2 series includes many microscopes such as the BHS and BHT models. An optional attachment (BH2-RFC) converts microscopes in this series into fluorescence microscopes.</skos:definition>
<owl:versionInfo>2</owl:versionInfo>
<dc:date>2012-12-18 15:30:23.0</dc:date>
<skos:note xml:lang="en">accepted</skos:note>
<owl:deprecated>false</owl:deprecated>
<skos:broader rdf:resource="http://vocab.nerc.ac.uk/collection/L05/current/LAB06/"/>
<skos:broader rdf:resource="http://vocab.nerc.ac.uk/collection/L05/current/LAB05/"/>
<void:inDataset rdf:resource="http://vocab.nerc.ac.uk/.well-known/void"/>
</skos:Concept>
</skos:member>
<skos:member>
<skos:Concept rdf:about="http://vocab.nerc.ac.uk/collection/L22/current/TOOL0182/">
<dc:identifier>SDN:L22::TOOL0182</dc:identifier>
<skos:notation>SDN:L22::TOOL0182</skos:notation>
<skos:prefLabel xml:lang="en">Omni Tinytalk TK-0040 temperature recorder</skos:prefLabel>
<skos:altLabel>Tinytalk TK-0040 TR</skos:altLabel>
<skos:definition xml:lang="en">A miniature temperature logger with a user programmed time interval. This model has an encapsulated thermistor with a range of -30 to 50C at a resolution of 0.25C and an accuracy of +-0.2C. It is housed in a splashproof metal 35mm film cannister.</skos:definition>
<owl:versionInfo>1</owl:versionInfo>
<dc:date>2010-05-18 16:10:58.0</dc:date>
<skos:note xml:lang="en">accepted</skos:note>
<owl:deprecated>false</owl:deprecated>
<skos:broader rdf:resource="http://vocab.nerc.ac.uk/collection/L05/current/134/"/>
<void:inDataset rdf:resource="http://vocab.nerc.ac.uk/.well-known/void"/>
</skos:Concept>
</skos:member>
<skos:member>
<skos:Concept rdf:about="http://vocab.nerc.ac.uk/collection/L22/current/NETT0011/">
<dc:identifier>SDN:L22::NETT0011</dc:identifier>
<skos:notation>SDN:L22::NETT0011</skos:notation>
<skos:prefLabel xml:lang="en">Opening-closing Bongo net - McGowan and Brown (1966)</skos:prefLabel>
<skos:altLabel>Bongo opening-closing net</skos:altLabel>
<skos:definition xml:lang="en">A pair of circular hoops (70 cm diameter  joined by a central axial which was clamped to a cable. A dacron cloth door covered each mouth opening which when released by a messenger, folded into the net mouth.  The nets were 71 cm in diameter, had a non-filtering collar section 84 cm long and a conical net 420 cm long with 0.505 mm mesh.  A flowmeter was present and after a set number of revolutions, caused the nets to be released from the hoops; choke ropes closed them [Wiebe and Benfield 2003 Plate 9 D].</skos:definition>
<owl:versionInfo>1</owl:versionInfo>
<dc:date>2011-10-21 14:18:49.0</dc:date>
<skos:note xml:lang="en">accepted</skos:note>
<owl:deprecated>false</owl:deprecated>
<skos:broader rdf:resource="http://vocab.nerc.ac.uk/collection/L05/current/388/"/>
<skos:broader rdf:resource="http://vocab.nerc.ac.uk/collection/L05/current/22/"/>
<void:inDataset rdf:resource="http://vocab.nerc.ac.uk/.well-known/void"/>
</skos:Concept>
</skos:member>
<skos:member>
<skos:Concept rdf:about="http://vocab.nerc.ac.uk/collection/L22/current/NETT0162/">
<dc:identifier>SDN:L22::NETT0162</dc:identifier>
<skos:notation>SDN:L22::NETT0162</skos:notation>
<skos:prefLabel xml:lang="en">Opening-closing Tucker Trawl  - Davis and Barham (1969)</skos:prefLabel>
<skos:altLabel>Davis modified Tucker Trawl</skos:altLabel>
<skos:definition xml:lang="en">Modification used timing clocks to open and close the Tucker trawl mouth.  Net design modified from that described by Tucker so that first 500 cm of the net mesh was 1.1 cm Marlon netting and last 200 cm was 0.33 mm nylon mesh.  A depth-telemetering pinger used to monitor net depth during tow and a depth-time recorder used to make alternate record [Wiebe and Benfield 2003 Plate 9 E].</skos:definition>
<owl:versionInfo>1</owl:versionInfo>
<dc:date>2011-10-21 14:18:49.0</dc:date>
<skos:note xml:lang="en">accepted</skos:note>
<owl:deprecated>false</owl:deprecated>
<skos:broader rdf:resource="http://vocab.nerc.ac.uk/collection/L05/current/23/"/>
<void:inDataset rdf:resource="http://vocab.nerc.ac.uk/.well-known/void"/>
</skos:Concept>
</skos:member>
<skos:member>
<skos:Concept rdf:about="http://vocab.nerc.ac.uk/collection/L22/current/NETT0126/">
<dc:identifier>SDN:L22::NETT0126</dc:identifier>
<skos:notation>SDN:L22::NETT0126</skos:notation>
<skos:prefLabel xml:lang="en">Opening-closing mechanism for plankton nets - Bourdillon et al. (1978)</skos:prefLabel>
<skos:altLabel>Bourdillon mechanism</skos:altLabel>
<skos:definition xml:lang="en">A double messenger system to allow a ring net to be sent down closed, opened at depth, and then closed again by a second messenger [Wiebe and Benfield 2003 Plate 7 A]</skos:definition>
<owl:versionInfo>1</owl:versionInfo>
<dc:date>2011-10-21 14:18:49.0</dc:date>
<skos:note xml:lang="en">accepted</skos:note>
<owl:deprecated>false</owl:deprecated>
<skos:broader rdf:resource="http://vocab.nerc.ac.uk/collection/L05/current/22/"/>
<void:inDataset rdf:resource="http://vocab.nerc.ac.uk/.well-known/void"/>
</skos:Concept>
</skos:member>
<skos:member>
<skos:Concept rdf:about="http://vocab.nerc.ac.uk/collection/L22/current/NETT0127/">
<dc:identifier>SDN:L22::NETT0127</dc:identifier>
<skos:notation>SDN:L22::NETT0127</skos:notation>
<skos:prefLabel xml:lang="en">Opening-closing net - Hoyle (1889)</skos:prefLabel>
<skos:altLabel>Hoyle opening-closing net</skos:altLabel>
<skos:definition xml:lang="en">A 61 cm diameter conical net (muslin or silk). No other dimensions given. Proposed electrical activation to open/close net [Wiebe and Benfield 2003 Plate 5 C].</skos:definition>
<owl:versionInfo>1</owl:versionInfo>
<dc:date>2011-10-21 14:18:49.0</dc:date>
<skos:note xml:lang="en">accepted</skos:note>
<owl:deprecated>false</owl:deprecated>
<skos:broader rdf:resource="http://vocab.nerc.ac.uk/collection/L05/current/22/"/>
<void:inDataset rdf:resource="http://vocab.nerc.ac.uk/.well-known/void"/>
</skos:Concept>
</skos:member>
<skos:member>
<skos:Concept rdf:about="http://vocab.nerc.ac.uk/collection/L22/current/NETT0128/">
<dc:identifier>SDN:L22::NETT0128</dc:identifier>
<skos:notation>SDN:L22::NETT0128</skos:notation>
<skos:prefLabel xml:lang="en">Opening-closing net system  - Leavitt (1935, 1938)</skos:prefLabel>
<skos:altLabel>Leavitt opening-closing net</skos:altLabel>
<skos:definition xml:lang="en">100, 150, and 200 cm diameter nets made of scrim, silk, and stramin respectively. Net dimensions not given [Wiebe and Benfield 2003 Plate 6 A].</skos:definition>
<owl:versionInfo>1</owl:versionInfo>
<dc:date>2011-10-21 14:18:49.0</dc:date>
<skos:note xml:lang="en">accepted</skos:note>
<owl:deprecated>false</owl:deprecated>
<skos:broader rdf:resource="http://vocab.nerc.ac.uk/collection/L05/current/22/"/>
<void:inDataset rdf:resource="http://vocab.nerc.ac.uk/.well-known/void"/>
</skos:Concept>
</skos:member>
<skos:member>
<skos:Concept rdf:about="http://vocab.nerc.ac.uk/collection/L22/current/TOOL0097/">
<dc:identifier>SDN:L22::TOOL0097</dc:identifier>
<skos:notation>SDN:L22::TOOL0097</skos:notation>
<skos:prefLabel xml:lang="en">Ott chart float tide gauge</skos:prefLabel>
<skos:altLabel>Ott chart float gauge</skos:altLabel>
<skos:definition xml:lang="en">Mechanical tide gauge with a float installed in a stilling well connected by wire through a set of pulleys that transmit the movement of the float to a continuous pen recorder.</skos:definition>
<owl:versionInfo>1</owl:versionInfo>
<dc:date>2009-04-28 11:30:37.0</dc:date>
<skos:note xml:lang="en">accepted</skos:note>
<owl:deprecated>false</owl:deprecated>
<skos:broader rdf:resource="http://vocab.nerc.ac.uk/collection/L05/current/111/"/>
<void:inDataset rdf:resource="http://vocab.nerc.ac.uk/.well-known/void"/>
</skos:Concept>
</skos:member>
<skos:member>
<skos:Concept rdf:about="http://vocab.nerc.ac.uk/collection/L22/current/TOOL0099/">
<dc:identifier>SDN:L22::TOOL0099</dc:identifier>
<skos:notation>SDN:L22::TOOL0099</skos:notation>
<skos:prefLabel xml:lang="en">Ott magnetic float tide gauge</skos:prefLabel>
<skos:altLabel>Ott magnetic float gauge</skos:altLabel>
<skos:definition xml:lang="en">Mechanical tide gauge with a float installed in a stilling well and a magnetic encoder that converts linear movement of the wire connected to the float into a digital value.</skos:definition>
<owl:versionInfo>1</owl:versionInfo>
<dc:date>2009-04-28 11:30:37.0</dc:date>
<skos:note xml:lang="en">accepted</skos:note>
<owl:deprecated>false</owl:deprecated>
<skos:broader rdf:resource="http://vocab.nerc.ac.uk/collection/L05/current/111/"/>
<void:inDataset rdf:resource="http://vocab.nerc.ac.uk/.well-known/void"/>
</skos:Concept>
</skos:member>
<skos:member>
<skos:Concept rdf:about="http://vocab.nerc.ac.uk/collection/L22/current/TOOL0098/">
<dc:identifier>SDN:L22::TOOL0098</dc:identifier>
<skos:notation>SDN:L22::TOOL0098</skos:notation>
<skos:prefLabel xml:lang="en">Ott optical float tide gauge</skos:prefLabel>
<skos:altLabel>Ott optical float gauge</skos:altLabel>
<skos:definition xml:lang="en">Mechanical tide gauge with a float installed in a stilling well and an optical encoder that converts linear movement of the wire connected to the float into a digital value.</skos:definition>
<owl:versionInfo>1</owl:versionInfo>
<dc:date>2009-04-28 11:30:37.0</dc:date>
<skos:note xml:lang="en">accepted</skos:note>
<owl:deprecated>false</owl:deprecated>
<skos:broader rdf:resource="http://vocab.nerc.ac.uk/collection/L05/current/111/"/>
<void:inDataset rdf:resource="http://vocab.nerc.ac.uk/.well-known/void"/>
</skos:Concept>
</skos:member>
<skos:member>
<skos:Concept rdf:about="http://vocab.nerc.ac.uk/collection/L22/current/TOOL0016/">
<dc:identifier>SDN:L22::TOOL0016</dc:identifier>
<skos:notation>SDN:L22::TOOL0016</skos:notation>
<skos:prefLabel xml:lang="en">Ott pneumatic tide gauge</skos:prefLabel>
<skos:altLabel>Ott gauge</skos:altLabel>
<skos:definition xml:lang="en">The Ott pneumatic gauge derives its measuring signal from the pressure produced in a bubbler system. The pressure is applied to one end of a pivoted beam. On the other side of the pivot is a weight which is moved up and down the beam by an electric motor in order to counter balance the pressure signal. At the far end of the beam are electrical contacts which operate the motor in the correct sense when the beam moves out of balance.   The motor is also geared to a double helix shaft with the pen arm attached. The position of the pen is therefore proportional to the applied air pressure.</skos:definition>
<owl:versionInfo>1</owl:versionInfo>
<dc:date>2009-11-30 11:27:51.0</dc:date>
<skos:note xml:lang="en">accepted</skos:note>
<owl:deprecated>false</owl:deprecated>
<skos:broader rdf:resource="http://vocab.nerc.ac.uk/collection/L05/current/111/"/>
<void:inDataset rdf:resource="http://vocab.nerc.ac.uk/.well-known/void"/>
</skos:Concept>
</skos:member>
<skos:member>
<skos:Concept rdf:about="http://vocab.nerc.ac.uk/collection/L22/current/NETT0145/">
<dc:identifier>SDN:L22::NETT0145</dc:identifier>
<skos:notation>SDN:L22::NETT0145</skos:notation>
<skos:prefLabel xml:lang="en">PNS neuston net - Zaitsev (1961, 1970)</skos:prefLabel>
<skos:altLabel>Zaitsev PNS</skos:altLabel>
<skos:definition xml:lang="en">A five-stage sampling frame with a height of 100 cm and width of 60 cm in which five 60cm x 20 cm rectangular mouth aperture nets are stacked. Nets and frame flotation similar to that described by Zaitsev . Used from drifting or anchored vessel.</skos:definition>
<owl:versionInfo>1</owl:versionInfo>
<dc:date>2011-10-21 14:18:49.0</dc:date>
<skos:note xml:lang="en">accepted</skos:note>
<owl:deprecated>false</owl:deprecated>
<skos:broader rdf:resource="http://vocab.nerc.ac.uk/collection/L05/current/69/"/>
<void:inDataset rdf:resource="http://vocab.nerc.ac.uk/.well-known/void"/>
</skos:Concept>
</skos:member>
<skos:member>
<skos:Concept rdf:about="http://vocab.nerc.ac.uk/collection/L22/current/TOOL0420/">
<dc:identifier>SDN:L22::TOOL0420</dc:identifier>
<skos:notation>SDN:L22::TOOL0420</skos:notation>
<skos:prefLabel xml:lang="en">Pall AcroPak 200 filter cartridge</skos:prefLabel>
<skos:altLabel>Pall AcroPak 200</skos:altLabel>
<skos:definition xml:lang="en">A filter cartridge designed for small- to medium-volume sterile filtration. It incorporates a Supor [hydrophilic polyethersulfone (PES)] membrane, which allows high flow rates and throughputs (up to 20 litres), and is ideal for solutions where low protein binding is required. Pore sizes range from 0.2 to 0.8 um and the effective filtration area is 200 cm^2. A built-in prefilter extends filter life when particulate-laden solutions, such as serum-containing media, are processed. The filter is manufactured without the use of adhesives to minimize extractables, sterilized by gamma irradiation and individually packaged.</skos:definition>
<owl:versionInfo>1</owl:versionInfo>
<dc:date>2011-09-03 16:28:15.0</dc:date>
<skos:note xml:lang="en">accepted</skos:note>
<owl:deprecated>false</owl:deprecated>
<skos:broader rdf:resource="http://vocab.nerc.ac.uk/collection/L05/current/84/"/>
<void:inDataset rdf:resource="http://vocab.nerc.ac.uk/.well-known/void"/>
</skos:Concept>
</skos:member>
<skos:member>
<skos:Concept rdf:about="http://vocab.nerc.ac.uk/collection/L22/current/NETT0135/">
<dc:identifier>SDN:L22::NETT0135</dc:identifier>
<skos:notation>SDN:L22::NETT0135</skos:notation>
<skos:prefLabel xml:lang="en">Parachute net - Wheeler (1941)</skos:prefLabel>
<skos:altLabel>Parachute net</skos:altLabel>
<skos:definition xml:lang="en">This has a 275 cm diameter parachute opening tapering over a distance of 350 cm to a 100 cm diameter mosquito netting net.  Free fall to bottom with concrete weights, released by salt block dissolution, and floated backwards to surface with gasoline float [Wiebe and Benfield 2003 Plate 11 B].</skos:definition>
<owl:versionInfo>1</owl:versionInfo>
<dc:date>2011-10-21 14:18:49.0</dc:date>
<skos:note xml:lang="en">accepted</skos:note>
<owl:deprecated>false</owl:deprecated>
<skos:broader rdf:resource="http://vocab.nerc.ac.uk/collection/L05/current/22/"/>
<void:inDataset rdf:resource="http://vocab.nerc.ac.uk/.well-known/void"/>
</skos:Concept>
</skos:member>
<skos:member>
<skos:Concept rdf:about="http://vocab.nerc.ac.uk/collection/L22/current/TOOL0403/">
<dc:identifier>SDN:L22::TOOL0403</dc:identifier>
<skos:notation>SDN:L22::TOOL0403</skos:notation>
<skos:prefLabel xml:lang="en">Paroscientific 410K Pressure Transducer</skos:prefLabel>
<skos:altLabel>Paroscientific 410K</skos:altLabel>
<skos:definition xml:lang="en">An absolute pressure transducer with a Digiquartz pressure sensor and precision thermometer. Operates over a temperature range of 0-125 degC and a pressure range of 0-10000 psia with a typical accuracy of 0.01% and a resolution of 0.0001%.</skos:definition>
<owl:versionInfo>2</owl:versionInfo>
<dc:date>2012-01-24 10:08:14.0</dc:date>
<skos:note xml:lang="en">accepted</skos:note>
<owl:deprecated>false</owl:deprecated>
<skos:related rdf:resource="http://vocab.nerc.ac.uk/collection/P01/current/PRESPR01/"/>
<skos:broader rdf:resource="http://vocab.nerc.ac.uk/collection/L05/current/111/"/>
<skos:broader rdf:resource="http://vocab.nerc.ac.uk/collection/L05/current/134/"/>
<void:inDataset rdf:resource="http://vocab.nerc.ac.uk/.well-known/void"/>
</skos:Concept>
</skos:member>
<skos:member>
<skos:Concept rdf:about="http://vocab.nerc.ac.uk/collection/L22/current/TOOL0475/">
<dc:identifier>SDN:L22::TOOL0475</dc:identifier>
<skos:notation>SDN:L22::TOOL0475</skos:notation>
<skos:prefLabel xml:lang="en">Paroscientific 415K Pressure Transducer</skos:prefLabel>
<skos:altLabel>Paroscientific 415K</skos:altLabel>
<skos:definition xml:lang="en">An absolute pressure transducer with a Digiquartz pressure sensor and precision thermometer. Operates over a temperature range of 0-50 degC and a pressure range of 0-15000 psia with a typical accuracy of 0.01% and a resolution of 0.0001%.</skos:definition>
<owl:versionInfo>1</owl:versionInfo>
<dc:date>2012-02-29 16:34:45.0</dc:date>
<skos:note xml:lang="en">accepted</skos:note>
<owl:deprecated>false</owl:deprecated>
<skos:broader rdf:resource="http://vocab.nerc.ac.uk/collection/L05/current/111/"/>
<skos:broader rdf:resource="http://vocab.nerc.ac.uk/collection/L05/current/134/"/>
<void:inDataset rdf:resource="http://vocab.nerc.ac.uk/.well-known/void"/>
</skos:Concept>
</skos:member>
<skos:member>
<skos:Concept rdf:about="http://vocab.nerc.ac.uk/collection/L22/current/TOOL0534/">
<dc:identifier>SDN:L22::TOOL0534</dc:identifier>
<skos:notation>SDN:L22::TOOL0534</skos:notation>
<skos:prefLabel xml:lang="en">Perkin-Elmer Model 204 Fluorescence Spectrophotometer</skos:prefLabel>
<skos:altLabel>Perkin-Elmer 204 spectrophotometer</skos:altLabel>
<skos:definition xml:lang="en">An automatic recording that measures the fluorescence of a sample using a Xenon lamp with full UV/visible range capability. It incorporates two monochromators, and automatic scanning of each over the 200 to 780 nm wavelength range permits the recording of excitation or emission spectra. The instrument can take up to four samples at a time.</skos:definition>
<owl:versionInfo>1</owl:versionInfo>
<dc:date>2012-08-22 13:43:43.0</dc:date>
<skos:note xml:lang="en">accepted</skos:note>
<owl:deprecated>false</owl:deprecated>
<skos:broader rdf:resource="http://vocab.nerc.ac.uk/collection/L05/current/LAB20/"/>
<void:inDataset rdf:resource="http://vocab.nerc.ac.uk/.well-known/void"/>
</skos:Concept>
</skos:member>
<skos:member>
<skos:Concept rdf:about="http://vocab.nerc.ac.uk/collection/L22/current/TOOL0468/">
<dc:identifier>SDN:L22::TOOL0468</dc:identifier>
<skos:notation>SDN:L22::TOOL0468</skos:notation>
<skos:prefLabel xml:lang="en">PerkinElmer AAnalyst 800 Atomic Absorption Spectrometer</skos:prefLabel>
<skos:altLabel>PerkinElmer AA 800 spectrometer</skos:altLabel>
<skos:definition xml:lang="en">A fully-integrated benchtop atomic absorption spectrometer that determines the elemental composition of a sample through the amount of light energy absorbed at specific wavelengths in the range 190-900 nm. The instrument contains an 8-lamp holder with built-in power supplies for hollow cathode and electrodeless discharge lamps, allowing automatic lamp selection. The instrument uses a real-time double-beam optical system (single-beam for Zeeman furnace operation) and includes both a flame and a Transversely Heated Graphite Atomizer furnace for atomisation of the sample. The specific wavelength of light to be measured is isolated by a monochromator and absorption is measured by a solid-state detector, with a built-in low-noise CMOS charge amplifier array. The burner is equipped with a high-strength inert mixing chamber and includes an adjustable nebulizer and an all-titanium, 10-cm, single-slot burner head. The instrument has a modulated 0.8 Tesla magnetic field oriented longitudinally to the optical path and a built-in continuum source double-beam background correction for flame operation. There is also a furnace autosampler which contains a removable sample tray.</skos:definition>
<owl:versionInfo>1</owl:versionInfo>
<dc:date>2012-02-21 16:06:42.0</dc:date>
<skos:note xml:lang="en">accepted</skos:note>
<owl:deprecated>false</owl:deprecated>
<skos:broader rdf:resource="http://vocab.nerc.ac.uk/collection/L05/current/LAB10/"/>
<void:inDataset rdf:resource="http://vocab.nerc.ac.uk/.well-known/void"/>
</skos:Concept>
</skos:member>
<skos:member>
<skos:Concept rdf:about="http://vocab.nerc.ac.uk/collection/L22/current/TOOL0485/">
<dc:identifier>SDN:L22::TOOL0485</dc:identifier>
<skos:notation>SDN:L22::TOOL0485</skos:notation>
<skos:prefLabel xml:lang="en">PerkinElmer AS 93plus autosampler</skos:prefLabel>
<skos:altLabel>PerkinElmer AS 93plus autosampler</skos:altLabel>
<skos:definition xml:lang="en">A laboratory random-access autosampler which is a computer-controlled, multi-purpose sampling system for flame and flow-injection atomic absorption, ICP-OES and ICP-MS. The instrument automates standard and sample introductions via software commands. Random-access programming gives broad flexibility in the placement of samples and standards. The sample probe, including the sample transport capillary tubing is made of acid and solvent-resistant materials. The AS 93plus model is compatible with commonly used sample trays from other manufacturers.  The instrument includes an integrated power supply and control electronics, and also has automatic rinsing.</skos:definition>
<owl:versionInfo>1</owl:versionInfo>
<dc:date>2012-03-29 16:25:41.0</dc:date>
<skos:note xml:lang="en">accepted</skos:note>
<owl:deprecated>false</owl:deprecated>
<skos:broader rdf:resource="http://vocab.nerc.ac.uk/collection/L05/current/LAB33/"/>
<void:inDataset rdf:resource="http://vocab.nerc.ac.uk/.well-known/void"/>
</skos:Concept>
</skos:member>
<skos:member>
<skos:Concept rdf:about="http://vocab.nerc.ac.uk/collection/L22/current/TOOL0484/">
<dc:identifier>SDN:L22::TOOL0484</dc:identifier>
<skos:notation>SDN:L22::TOOL0484</skos:notation>
<skos:prefLabel xml:lang="en">PerkinElmer Optima 4300 DV inductively coupled plasma optical emission spectrometer</skos:prefLabel>
<skos:altLabel>PerkinElmer 4300 DV ICP-OES</skos:altLabel>
<skos:definition xml:lang="en">An optical emission spectrometer (OES) that determines elemental composition of a sample through the amount of light emitted from atoms or ions at specific wavelengths. The atomization source is an inductively coupled plasma (ICP) which is maintained by the interaction of Radio Frequency (RF) energy, generated by a solid-state RF generator, a horizontally mounted quartz torch and ionized argon gas. Standards and samples are acquired with the aid of an autosampler. The sample solution is injected as an aerosol into the plasma via a nebuliser and spray chamber using the integral peristaltic pump. Light from the plasma and the various atomic emissions therein pass through duel view (DV) windows into the thermally stabilised, argon-purged optical compartment housing an Echelle polychromator to separate the light into its component wavelengths. The polychromator comprises diffraction gratings, mirrors, lenses and visible and ultra-violet detector sets, each comprising arrays of segmented-array charge-coupled device (SCD) detectors and allows simultaneous quantification of atomic emissions in the plasma.</skos:definition>
<owl:versionInfo>1</owl:versionInfo>
<dc:date>2012-03-29 16:25:41.0</dc:date>
<skos:note xml:lang="en">accepted</skos:note>
<owl:deprecated>false</owl:deprecated>
<skos:broader rdf:resource="http://vocab.nerc.ac.uk/collection/L05/current/LAB14/"/>
<void:inDataset rdf:resource="http://vocab.nerc.ac.uk/.well-known/void"/>
</skos:Concept>
</skos:member>
<skos:member>
<skos:Concept rdf:about="http://vocab.nerc.ac.uk/collection/L22/current/TOOL0518/">
<dc:identifier>SDN:L22::TOOL0518</dc:identifier>
<skos:notation>SDN:L22::TOOL0518</skos:notation>
<skos:prefLabel xml:lang="en">PerkinElmer Tri-Carb 3110TR low activity liquid scintillation analyzer</skos:prefLabel>
<skos:altLabel>Tri-Carb 3110TR liquid scintillation</skos:altLabel>
<skos:definition xml:lang="en">A benchtop liquid scintillation analyser for detecting small amounts of alpha, beta and gamma radioactivity. It features a Multichannel Analyzer with an effective resolution of 1/10 keV and an extended dynamic quench range. Sample capacity is either 408 standard 20 mL vials, or 720 small 4 or 7 mL vials. The instrument includes a barium-133 low energy external standard source centered under the sample vial which eliminates the effects of volume variations. It has an energy range of 0-2000 keV and an operating ambient temperature range of 15-35 degC.</skos:definition>
<owl:versionInfo>1</owl:versionInfo>
<dc:date>2012-07-04 10:02:10.0</dc:date>
<skos:note xml:lang="en">accepted</skos:note>
<owl:deprecated>false</owl:deprecated>
<skos:broader rdf:resource="http://vocab.nerc.ac.uk/collection/L05/current/LAB21/"/>
<void:inDataset rdf:resource="http://vocab.nerc.ac.uk/.well-known/void"/>
</skos:Concept>
</skos:member>
<skos:member>
<skos:Concept rdf:about="http://vocab.nerc.ac.uk/collection/L22/current/TOOL0525/">
<dc:identifier>SDN:L22::TOOL0525</dc:identifier>
<skos:notation>SDN:L22::TOOL0525</skos:notation>
<skos:prefLabel xml:lang="en">Picarro L1102-i Isotopic Water Liquid Analyzer</skos:prefLabel>
<skos:altLabel>Picarro L1102-i Water Analyzer</skos:altLabel>
<skos:definition xml:lang="en">A portable analyser designed for laboratories or field based isotope analysis. It uses Cavity Ring-Down Spectroscopy (CRDS) to measure the spectral signature of the molecule of interest. The instrument includes a closed-loop temperature and pressure control. The L1102-i can be used for analysis of liquid water only. It has a typical precision of 0.1 per mil for d18O and 0.5 per mil for dD.</skos:definition>
<owl:versionInfo>1</owl:versionInfo>
<dc:date>2012-07-25 09:19:33.0</dc:date>
<skos:note xml:lang="en">accepted</skos:note>
<owl:deprecated>false</owl:deprecated>
<skos:broader rdf:resource="http://vocab.nerc.ac.uk/collection/L05/current/LAB38/"/>
<void:inDataset rdf:resource="http://vocab.nerc.ac.uk/.well-known/void"/>
</skos:Concept>
</skos:member>
<skos:member>
<skos:Concept rdf:about="http://vocab.nerc.ac.uk/collection/L22/current/TOOL0517/">
<dc:identifier>SDN:L22::TOOL0517</dc:identifier>
<skos:notation>SDN:L22::TOOL0517</skos:notation>
<skos:prefLabel xml:lang="en">Picarro L2130-I deltaD/delta18O Isotopic Water Analyzer</skos:prefLabel>
<skos:altLabel>Picarro L2130-I Water Analyzer</skos:altLabel>
<skos:definition xml:lang="en">A portable analyser designed for laboratories or field based isotope analysis. It uses Cavity Ring-Down Spectroscopy (CRDS) to measure the spectral signature of the molecule of interest. The instrument includes a closed-loop temperature and pressure control. The L2130-i can be used in all aspects of the water cycle: water vapor, liquid water, or water trapped in solids. It has a typical precision of 0.25 per mil for d18O and 1.20 per mil for dD in solid samples. Corresponding typical values for liquid samples are 0.011 per mil for d18O and 0.038 per mil for dD.</skos:definition>
<owl:versionInfo>1</owl:versionInfo>
<dc:date>2012-07-04 10:02:10.0</dc:date>
<skos:note xml:lang="en">accepted</skos:note>
<owl:deprecated>false</owl:deprecated>
<skos:broader rdf:resource="http://vocab.nerc.ac.uk/collection/L05/current/LAB38/"/>
<void:inDataset rdf:resource="http://vocab.nerc.ac.uk/.well-known/void"/>
</skos:Concept>
</skos:member>
<skos:member>
<skos:Concept rdf:about="http://vocab.nerc.ac.uk/collection/L22/current/NETT0173/">
<dc:identifier>SDN:L22::NETT0173</dc:identifier>
<skos:notation>SDN:L22::NETT0173</skos:notation>
<skos:prefLabel xml:lang="en">Plankton pump sampler</skos:prefLabel>
<skos:altLabel>Plankton pump sampler</skos:altLabel>
<skos:definition xml:lang="en">An in situ pump and net system for collecting plankton samples. Water is pumped at approximately 1.2 m^3 per minute through a mesh, and samples are collected in the net cod end. The device was used on research cruises in the late 1990s.</skos:definition>
<owl:versionInfo>1</owl:versionInfo>
<dc:date>2012-10-12 14:13:09.0</dc:date>
<skos:note xml:lang="en">accepted</skos:note>
<owl:deprecated>false</owl:deprecated>
<skos:broader rdf:resource="http://vocab.nerc.ac.uk/collection/L05/current/22/"/>
<void:inDataset rdf:resource="http://vocab.nerc.ac.uk/.well-known/void"/>
</skos:Concept>
</skos:member>
<skos:member>
<skos:Concept rdf:about="http://vocab.nerc.ac.uk/collection/L22/current/NETT0138/">
<dc:identifier>SDN:L22::NETT0138</dc:identifier>
<skos:notation>SDN:L22::NETT0138</skos:notation>
<skos:prefLabel xml:lang="en">Plankton purse seine  - Murphy and Clutter (1972)</skos:prefLabel>
<skos:altLabel>Murphy plankton purse seine</skos:altLabel>
<skos:definition xml:lang="en">A miniature purse seine 3048 cm long x 640 cm tall with netting of 0.333 mm nylon mesh [Wiebe and Benfield 2003 Plate 12 C].</skos:definition>
<owl:versionInfo>1</owl:versionInfo>
<dc:date>2011-10-21 14:18:49.0</dc:date>
<skos:note xml:lang="en">accepted</skos:note>
<owl:deprecated>false</owl:deprecated>
<skos:broader rdf:resource="http://vocab.nerc.ac.uk/collection/L05/current/22/"/>
<void:inDataset rdf:resource="http://vocab.nerc.ac.uk/.well-known/void"/>
</skos:Concept>
</skos:member>
<skos:member>
<skos:Concept rdf:about="http://vocab.nerc.ac.uk/collection/L22/current/NETT0140/">
<dc:identifier>SDN:L22::NETT0140</dc:identifier>
<skos:notation>SDN:L22::NETT0140</skos:notation>
<skos:prefLabel xml:lang="en">Plankton-Bar - Tonolli (1951)</skos:prefLabel>
<skos:altLabel>Plankton-Bar</skos:altLabel>
<skos:definition xml:lang="en">A device for continuously sampling plankton from several depths simultaneously using a combination of ~18 cm diameter nets with 38 meshes per cm and a pumping system.  Five nets with equidistant spacing on a towing wire were normally used [Wiebe and Benfield 2003 Plate 11 D].</skos:definition>
<owl:versionInfo>1</owl:versionInfo>
<dc:date>2011-10-21 14:18:49.0</dc:date>
<skos:note xml:lang="en">accepted</skos:note>
<owl:deprecated>false</owl:deprecated>
<skos:broader rdf:resource="http://vocab.nerc.ac.uk/collection/L05/current/22/"/>
<void:inDataset rdf:resource="http://vocab.nerc.ac.uk/.well-known/void"/>
</skos:Concept>
</skos:member>
<skos:member>
<skos:Concept rdf:about="http://vocab.nerc.ac.uk/collection/L22/current/NETT0141/">
<dc:identifier>SDN:L22::NETT0141</dc:identifier>
<skos:notation>SDN:L22::NETT0141</skos:notation>
<skos:prefLabel xml:lang="en">Planktonbenthos dredge - Beauchamp (1932)</skos:prefLabel>
<skos:altLabel>Beauchamp planktonbenthos dredge</skos:altLabel>
<skos:definition xml:lang="en">A simple pair of U-shaped runners were connected by two cross struts which supported a net which collected animals living  just above the bottom. No opening/closing mechanism was present.</skos:definition>
<owl:versionInfo>1</owl:versionInfo>
<dc:date>2011-10-21 14:18:49.0</dc:date>
<skos:note xml:lang="en">accepted</skos:note>
<owl:deprecated>false</owl:deprecated>
<skos:broader rdf:resource="http://vocab.nerc.ac.uk/collection/L05/current/22/"/>
<skos:broader rdf:resource="http://vocab.nerc.ac.uk/collection/L05/current/24/"/>
<void:inDataset rdf:resource="http://vocab.nerc.ac.uk/.well-known/void"/>
</skos:Concept>
</skos:member>
<skos:member>
<skos:Concept rdf:about="http://vocab.nerc.ac.uk/collection/L22/current/NETT0142/">
<dc:identifier>SDN:L22::NETT0142</dc:identifier>
<skos:notation>SDN:L22::NETT0142</skos:notation>
<skos:prefLabel xml:lang="en">Planktonbenthos sampler - Hensen (1895)</skos:prefLabel>
<skos:altLabel>Hensen planktonbenthos sampler</skos:altLabel>
<skos:definition xml:lang="en">An eight wheeled carriage-like sled with a net mounted in between the third and fourth pairs of wheels. [Wiebe and Benfield 2003 Plate 22 A]</skos:definition>
<owl:versionInfo>1</owl:versionInfo>
<dc:date>2011-10-21 14:18:49.0</dc:date>
<skos:note xml:lang="en">accepted</skos:note>
<owl:deprecated>false</owl:deprecated>
<skos:broader rdf:resource="http://vocab.nerc.ac.uk/collection/L05/current/24/"/>
<skos:broader rdf:resource="http://vocab.nerc.ac.uk/collection/L05/current/22/"/>
<void:inDataset rdf:resource="http://vocab.nerc.ac.uk/.well-known/void"/>
</skos:Concept>
</skos:member>
<skos:member>
<skos:Concept rdf:about="http://vocab.nerc.ac.uk/collection/L22/current/TOOL0009/">
<dc:identifier>SDN:L22::TOOL0009</dc:identifier>
<skos:notation>SDN:L22::TOOL0009</skos:notation>
<skos:prefLabel xml:lang="en">Plessey 9400 CTD</skos:prefLabel>
<skos:altLabel>Plessey 9400</skos:altLabel>
<skos:definition xml:lang="en">The Plessey 9400 CTD system combines a Plessey 6500 inductive conductivity sensor, a Plessey 4500 platinum resistance temperature sensor and Plessey 4600 bonded strain gauge pressure sensor.</skos:definition>
<owl:versionInfo>1</owl:versionInfo>
<dc:date>2009-11-30 11:27:51.0</dc:date>
<skos:note xml:lang="en">accepted</skos:note>
<owl:deprecated>false</owl:deprecated>
<skos:related rdf:resource="http://vocab.nerc.ac.uk/collection/P01/current/DEPHPR01/"/>
<skos:related rdf:resource="http://vocab.nerc.ac.uk/collection/P01/current/TEMPST01/"/>
<skos:related rdf:resource="http://vocab.nerc.ac.uk/collection/P01/current/PSALPR01/"/>
<skos:broader rdf:resource="http://vocab.nerc.ac.uk/collection/L05/current/130/"/>
<skos:broader rdf:resource="http://vocab.nerc.ac.uk/collection/L05/current/134/"/>
<skos:broader rdf:resource="http://vocab.nerc.ac.uk/collection/L05/current/350/"/>
<void:inDataset rdf:resource="http://vocab.nerc.ac.uk/.well-known/void"/>
</skos:Concept>
</skos:member>
<skos:member>
<skos:Concept rdf:about="http://vocab.nerc.ac.uk/collection/L22/current/TOOL0241/">
<dc:identifier>SDN:L22::TOOL0241</dc:identifier>
<skos:notation>SDN:L22::TOOL0241</skos:notation>
<skos:prefLabel xml:lang="en">Plessey Environmenal Systems 6230N bench salinometer</skos:prefLabel>
<skos:altLabel>Plessey 6230N salinometer</skos:altLabel>
<skos:definition xml:lang="en">A laboratory instrument that determines salinity of a water sample by comparison of its electrical conductivity with a standard solution.</skos:definition>
<owl:versionInfo>1</owl:versionInfo>
<dc:date>2010-05-18 16:10:58.0</dc:date>
<skos:note xml:lang="en">accepted</skos:note>
<owl:deprecated>false</owl:deprecated>
<skos:broader rdf:resource="http://vocab.nerc.ac.uk/collection/L05/current/LAB30/"/>
<void:inDataset rdf:resource="http://vocab.nerc.ac.uk/.well-known/void"/>
</skos:Concept>
</skos:member>
<skos:member>
<skos:Concept rdf:about="http://vocab.nerc.ac.uk/collection/L22/current/TOOL0577/">
<dc:identifier>SDN:L22::TOOL0577</dc:identifier>
<skos:notation>SDN:L22::TOOL0577</skos:notation>
<skos:prefLabel xml:lang="en">Plessey recording current meter model 9021</skos:prefLabel>
<skos:altLabel>Plessey 9021</skos:altLabel>
<skos:definition xml:lang="en">An axial flow impeller current meter designed to operate at depths to 2000 m (6000 m optional), and in temperatures from -5 to 40 degC. Forward currents rotate the impeller clockwise, and reverse currents rotate it anticlockwise (starting speed 1.5 cm/s; speed range 2.5 to 500 cm/s; accuracy greater of 2 cm/s or 2 percent). A counter is magnetically coupled to the impeller, and records net current speed over the sample period. A vane with horizontal stabiliser fins aligns the impeller with the current flow (minimum current velocity for alignment 3 cm/s). Current direction is measured by magnetic compass (360 degree range; accuracy 3 degrees; resolution 1.4 degrees; tolerated tilt rangeis -1 degrees to 4 degrees, or up to 40 degrees if gimballed). A solid state crystal clock measures time (accuracy better than 2 sec/day). Optional sensors include platinum resistance thermometer (range -2 to 35 degC; accuracy 0.1 degC; 99 percent response time 15 sec), pressure sensor (accuracy 0.5 percent of full scale; response time 10 msec), conductivity sensor and sample counter.</skos:definition>
<owl:versionInfo>1</owl:versionInfo>
<dc:date>2012-12-18 15:09:37.0</dc:date>
<skos:note xml:lang="en">accepted</skos:note>
<owl:deprecated>false</owl:deprecated>
<skos:broader rdf:resource="http://vocab.nerc.ac.uk/collection/L05/current/114/"/>
<void:inDataset rdf:resource="http://vocab.nerc.ac.uk/.well-known/void"/>
</skos:Concept>
</skos:member>
<skos:member>
<skos:Concept rdf:about="http://vocab.nerc.ac.uk/collection/L22/current/TOOL0578/">
<dc:identifier>SDN:L22::TOOL0578</dc:identifier>
<skos:notation>SDN:L22::TOOL0578</skos:notation>
<skos:prefLabel xml:lang="en">Plessey recording current meter model M021</skos:prefLabel>
<skos:altLabel>Plessey M021</skos:altLabel>
<skos:definition xml:lang="en">An axial flow impeller current meter designed to operate at depths to 1000 m, and in temperatures from -4 to 35 degC. Forward currents rotate the impeller clockwise, and reverse currents rotate it anticlockwise (starting speed 2 cm/s; speed range 5 to 250 cm/s; accuracy greater of 3 cm/s or 3 percent). A counter is magnetically coupled to the impeller, and records net current speed over the sample period. A vane with horizontal stabiliser fins aligns the impeller with the current flow. Current direction is measured by magnetic compass (tolerated tilt range is 15 degrees in both pitch and roll axes). Pre-1972 instruments were equipped with a battery-driven clock (accuracy better than 10 sec/day), whereas post-1972 instruments used a solid state crystal clock (accuracy 2 sec/day).</skos:definition>
<owl:versionInfo>1</owl:versionInfo>
<dc:date>2012-12-18 15:09:37.0</dc:date>
<skos:note xml:lang="en">accepted</skos:note>
<owl:deprecated>false</owl:deprecated>
<skos:broader rdf:resource="http://vocab.nerc.ac.uk/collection/L05/current/114/"/>
<void:inDataset rdf:resource="http://vocab.nerc.ac.uk/.well-known/void"/>
</skos:Concept>
</skos:member>
<skos:member>
<skos:Concept rdf:about="http://vocab.nerc.ac.uk/collection/L22/current/TOOL0574/">
<dc:identifier>SDN:L22::TOOL0574</dc:identifier>
<skos:notation>SDN:L22::TOOL0574</skos:notation>
<skos:prefLabel xml:lang="en">Plessey underwater radiometer</skos:prefLabel>
<skos:altLabel>Plessey underwater radiometer</skos:altLabel>
<skos:definition xml:lang="en">A submersible cosine collector radiometer designed to measure downwelling radiation. The collector is designed to measure the amount of light over a hemisphere. The instrument was commonly used in the 1980s.</skos:definition>
<owl:versionInfo>1</owl:versionInfo>
<dc:date>2012-12-06 14:06:57.0</dc:date>
<skos:note xml:lang="en">accepted</skos:note>
<owl:deprecated>false</owl:deprecated>
<skos:related rdf:resource="http://vocab.nerc.ac.uk/collection/P01/current/DWIRPP01/"/>
<skos:broader rdf:resource="http://vocab.nerc.ac.uk/collection/L05/current/122/"/>
<void:inDataset rdf:resource="http://vocab.nerc.ac.uk/.well-known/void"/>
</skos:Concept>
</skos:member>
<skos:member>
<skos:Concept rdf:about="http://vocab.nerc.ac.uk/collection/L22/current/NETT0143/">
<dc:identifier>SDN:L22::NETT0143</dc:identifier>
<skos:notation>SDN:L22::NETT0143</skos:notation>
<skos:prefLabel xml:lang="en">Plummet net - Hovekamp ; Daly [personal communication to Wiebe and Benfield]</skos:prefLabel>
<skos:altLabel>Hovekamp-Daly plummet net</skos:altLabel>
<skos:definition xml:lang="en">Construction has a 100 cm diameter mouth with a lead weighted net ring and net with 0.571 mm mesh. For downward collecting, the net was lowered by the cod-end to a pre-determined depth and a messenger used to release the cod-end attachment and draw tight a choke collar near the mouth of the net [Wiebe and Benfield 2003 Plate 9 D].</skos:definition>
<owl:versionInfo>1</owl:versionInfo>
<dc:date>2011-10-21 14:18:49.0</dc:date>
<skos:note xml:lang="en">accepted</skos:note>
<owl:deprecated>false</owl:deprecated>
<skos:broader rdf:resource="http://vocab.nerc.ac.uk/collection/L05/current/22/"/>
<void:inDataset rdf:resource="http://vocab.nerc.ac.uk/.well-known/void"/>
</skos:Concept>
</skos:member>
<skos:member>
<skos:Concept rdf:about="http://vocab.nerc.ac.uk/collection/L22/current/NETT0144/">
<dc:identifier>SDN:L22::NETT0144</dc:identifier>
<skos:notation>SDN:L22::NETT0144</skos:notation>
<skos:prefLabel xml:lang="en">Plummet net type II - Hovekamp (1989) and Daly [personal communication to Wiebe and Benfield]</skos:prefLabel>
<skos:altLabel>Hovekamp-Daly plummet net type II</skos:altLabel>
<skos:definition xml:lang="en">A downward-fishing, vertical, closing plummet net with a 1-m2 rectangular mouth opening with a net that is attached to two bars that run along a pair of net bar glides along parallel sides.  A double messenger system is used to opened the net as it falls to depth and to close it as it reaches the bottom of the haul.  The net ~ 180 cm in length has been used with a variety of mesh sizes; 0.163 mm, 0.560 mm, and 1600 mm Nitex.  According to Daly [personal communication], the first messenger releases a bridle attached to the opening net bar under tension from a shock cord.  The second messenger releases two bridles, one attached to the back of the net frame and the other attached to the closing net bar.  The net frame assumes a vertical position, allowing the second net bar to fall, closing the net, and retrieval is begun.</skos:definition>
<owl:versionInfo>1</owl:versionInfo>
<dc:date>2011-10-21 14:18:49.0</dc:date>
<skos:note xml:lang="en">accepted</skos:note>
<owl:deprecated>false</owl:deprecated>
<skos:broader rdf:resource="http://vocab.nerc.ac.uk/collection/L05/current/22/"/>
<void:inDataset rdf:resource="http://vocab.nerc.ac.uk/.well-known/void"/>
</skos:Concept>
</skos:member>
<skos:member>
<skos:Concept rdf:about="http://vocab.nerc.ac.uk/collection/L22/current/TOOL0450/">
<dc:identifier>SDN:L22::TOOL0450</dc:identifier>
<skos:notation>SDN:L22::TOOL0450</skos:notation>
<skos:prefLabel xml:lang="en">Plymouth Marine Laboratory Aiken CTD</skos:prefLabel>
<skos:altLabel>PML Aiken CTD</skos:altLabel>
<skos:definition xml:lang="en">A conductivity-temperature-depth package developed at Plymouth Marine Laboratory by J. Aiken. The unit had a depth rating of 200 m and data were logged internally on a miniature digital tape recorder. The package was originally developed for use on an Undulating Oceanographic Recorder but was also used to collect standard CTD profiles.</skos:definition>
<owl:versionInfo>1</owl:versionInfo>
<dc:date>2012-01-05 09:34:05.0</dc:date>
<skos:note xml:lang="en">accepted</skos:note>
<owl:deprecated>false</owl:deprecated>
<skos:broader rdf:resource="http://vocab.nerc.ac.uk/collection/L05/current/134/"/>
<skos:broader rdf:resource="http://vocab.nerc.ac.uk/collection/L05/current/130/"/>
<skos:broader rdf:resource="http://vocab.nerc.ac.uk/collection/L05/current/350/"/>
<void:inDataset rdf:resource="http://vocab.nerc.ac.uk/.well-known/void"/>
</skos:Concept>
</skos:member>
<skos:member>
<skos:Concept rdf:about="http://vocab.nerc.ac.uk/collection/L22/current/TOOL0546/">
<dc:identifier>SDN:L22::TOOL0546</dc:identifier>
<skos:notation>SDN:L22::TOOL0546</skos:notation>
<skos:prefLabel xml:lang="en">Plymouth Marine Laboratory Interfacial Sampler</skos:prefLabel>
<skos:altLabel>PML Interfacial Sampler</skos:altLabel>
<skos:definition xml:lang="en">A sampler comprising a frame fitted with 10 horizontal syringe-type 4 litre water bottles. An electronic control cylinder, mounted in the top of the frame, is programmed to release the bottle pistons once the frame has settled on the seabed and disturbed sediment has had time to disperse. The release of the piston draws in a sample and, at completion of the piston stroke, a mechanism is triggered to close the bottle inlet.</skos:definition>
<owl:versionInfo>1</owl:versionInfo>
<dc:date>2012-09-26 16:33:22.0</dc:date>
<skos:note xml:lang="en">accepted</skos:note>
<owl:deprecated>false</owl:deprecated>
<skos:broader rdf:resource="http://vocab.nerc.ac.uk/collection/L05/current/30/"/>
<void:inDataset rdf:resource="http://vocab.nerc.ac.uk/.well-known/void"/>
</skos:Concept>
</skos:member>
<skos:member>
<skos:Concept rdf:about="http://vocab.nerc.ac.uk/collection/L22/current/TOOL0548/">
<dc:identifier>SDN:L22::TOOL0548</dc:identifier>
<skos:notation>SDN:L22::TOOL0548</skos:notation>
<skos:prefLabel xml:lang="en">Plymouth Marine Laboratory Near-Surface Sampling Device</skos:prefLabel>
<skos:altLabel>PML NSSD</skos:altLabel>
<skos:definition xml:lang="en">A water sample collection system comprising a flotation ring supporting a central vertical spar that carries a 8 sampling bottles, of which the upper 5 are vertically spaced at 20 cm intervals and the lower 3 at approximately 30 cm intervals. The spar also carries an array of thermistors spaced at logarithmic intervals between a few mm below the surface to approximately 2 m depth. Atop the spar is a control system which continuously logs the thermistor data. The device is deployed from a vessel and allowed to drift away on a tether with a conductive core. Thermistor data are transmitted up the cable to a host computer on board the ship, while the control system allows for the remote firing of the sampling bottles by the host computer.</skos:definition>
<owl:versionInfo>1</owl:versionInfo>
<dc:date>2012-09-26 16:33:22.0</dc:date>
<skos:note xml:lang="en">accepted</skos:note>
<owl:deprecated>false</owl:deprecated>
<skos:broader rdf:resource="http://vocab.nerc.ac.uk/collection/L05/current/30/"/>
<void:inDataset rdf:resource="http://vocab.nerc.ac.uk/.well-known/void"/>
</skos:Concept>
</skos:member>
<skos:member>
<skos:Concept rdf:about="http://vocab.nerc.ac.uk/collection/L22/current/TOOL0542/">
<dc:identifier>SDN:L22::TOOL0542</dc:identifier>
<skos:notation>SDN:L22::TOOL0542</skos:notation>
<skos:prefLabel xml:lang="en">Polypropylene 10L surface sample bottle</skos:prefLabel>
<skos:altLabel>Polypropylene 10L bottle</skos:altLabel>
<skos:definition xml:lang="en">Polypropylene plastic bottle with 10 litre capacity used for surface sampling from small boats during OMEX and LOIS RACS projects in the 1990s.</skos:definition>
<owl:versionInfo>1</owl:versionInfo>
<dc:date>2012-09-26 16:33:22.0</dc:date>
<skos:note xml:lang="en">accepted</skos:note>
<owl:deprecated>false</owl:deprecated>
<skos:broader rdf:resource="http://vocab.nerc.ac.uk/collection/L05/current/30/"/>
<void:inDataset rdf:resource="http://vocab.nerc.ac.uk/.well-known/void"/>
</skos:Concept>
</skos:member>
<skos:member>
<skos:Concept rdf:about="http://vocab.nerc.ac.uk/collection/L22/current/TOOL0473/">
<dc:identifier>SDN:L22::TOOL0473</dc:identifier>
<skos:notation>SDN:L22::TOOL0473</skos:notation>
<skos:prefLabel xml:lang="en">Precision Measurement Engineering SCAMP microstructure profiler</skos:prefLabel>
<skos:altLabel>SCAMP microstructure profiler</skos:altLabel>
<skos:definition xml:lang="en">A self contained, autonomous microstructure profiler designed to measure extremely small scale (order 1 mm) fluctuations of electrical conductivity, temperature, and chlorophyll concentration in aquatic environments. It has a maximum depth rating of 100 m, a travel rate of 10 cm/s and a sampling rate of 100 Hz. The instrument is powered by internal batteries that allow it to operate continuously for at least 4 hours. The fast conductivity channel uses a PME 4-electrode conductivity microsensor while the standard conductivity channel uses a PME 4-electrode ceramic sensor. The instrument has two available fast temperature channels, each using a Thermometrics FP07 thermistor, and includes a Keller PSI PAA-10 pressure sensor. Two gradient channels are used to store d/dt computations. These data can be used to infer the levels of dissipation of turbulent kinetic energy, in-situ fluxes of heat and salt, and the microstructure behavior of these parameters. The chlorophyll fluorometer consists of a high intense blue LED and a 455 nm interface filter that illuminates a small water sample. Chlorophyll fluorescence is observed through a 685 nm interference filter by a photo diode detector. A Li-Cor LI-192SA PAR sensor can also be attached to the SCAMP. Data are stored on an internal data logger.</skos:definition>
<owl:versionInfo>1</owl:versionInfo>
<dc:date>2012-02-21 16:06:42.0</dc:date>
<skos:note xml:lang="en">accepted</skos:note>
<owl:deprecated>false</owl:deprecated>
<skos:broader rdf:resource="http://vocab.nerc.ac.uk/collection/L05/current/113/"/>
<skos:broader rdf:resource="http://vocab.nerc.ac.uk/collection/L05/current/134/"/>
<skos:broader rdf:resource="http://vocab.nerc.ac.uk/collection/L05/current/184/"/>
<skos:broader rdf:resource="http://vocab.nerc.ac.uk/collection/L05/current/350/"/>
<void:inDataset rdf:resource="http://vocab.nerc.ac.uk/.well-known/void"/>
</skos:Concept>
</skos:member>
<skos:member>
<skos:Concept rdf:about="http://vocab.nerc.ac.uk/collection/L22/current/TOOL0600/">
<dc:identifier>SDN:L22::TOOL0600</dc:identifier>
<skos:notation>SDN:L22::TOOL0600</skos:notation>
<skos:prefLabel xml:lang="en">Proudman Oceanographic Laboratory 1MHz ADCP</skos:prefLabel>
<skos:altLabel>POL 1MHz ADCP</skos:altLabel>
<skos:definition xml:lang="en">An ADCP with a range of 30 m, designed to measure currents in up to 24 bins. Data from bins in the shallowest 15 percent of the depth range (ie: closest to the transducer) and in the deepest 10 percent (furthest from the transducer) are unreliable due to interference. The instrument uses two orthogonal beams and a built-in compass to resolve northward and eastward components of current.</skos:definition>
<owl:versionInfo>1</owl:versionInfo>
<dc:date>2013-02-07 15:46:44.0</dc:date>
<skos:note xml:lang="en">accepted</skos:note>
<owl:deprecated>false</owl:deprecated>
<skos:broader rdf:resource="http://vocab.nerc.ac.uk/collection/L05/current/115/"/>
<void:inDataset rdf:resource="http://vocab.nerc.ac.uk/.well-known/void"/>
</skos:Concept>
</skos:member>
<skos:member>
<skos:Concept rdf:about="http://vocab.nerc.ac.uk/collection/L22/current/TOOL0599/">
<dc:identifier>SDN:L22::TOOL0599</dc:identifier>
<skos:notation>SDN:L22::TOOL0599</skos:notation>
<skos:prefLabel xml:lang="en">Proudman Oceanographic Laboratory 250kHz ADCP</skos:prefLabel>
<skos:altLabel>POL 250kHz ADCP</skos:altLabel>
<skos:definition xml:lang="en">An ADCP with a range of 100 m, designed to measure currents in up to 24 bins. Data from bins in the shallowest 25 percent of the depth range (ie: closest to the transducer) and in the deepest 10 percent (furthest from the transducer) are unreliable due to interference. The instrument uses two orthogonal beams and a built-in compass to resolve northward and eastward components of current.</skos:definition>
<owl:versionInfo>1</owl:versionInfo>
<dc:date>2013-02-07 15:47:04.0</dc:date>
<skos:note xml:lang="en">accepted</skos:note>
<owl:deprecated>false</owl:deprecated>
<skos:broader rdf:resource="http://vocab.nerc.ac.uk/collection/L05/current/115/"/>
<void:inDataset rdf:resource="http://vocab.nerc.ac.uk/.well-known/void"/>
</skos:Concept>
</skos:member>
<skos:member>
<skos:Concept rdf:about="http://vocab.nerc.ac.uk/collection/L22/current/TOOL0598/">
<dc:identifier>SDN:L22::TOOL0598</dc:identifier>
<skos:notation>SDN:L22::TOOL0598</skos:notation>
<skos:prefLabel xml:lang="en">Proudman Oceanographic Laboratory 75kHz ADCP</skos:prefLabel>
<skos:altLabel>POL 75kHz ADCP</skos:altLabel>
<skos:definition xml:lang="en">An ADCP designed to use low-frequency sound (actually 79-80 kHz) for optimum performance in water depths between 500 and 1000 m. The instrument was originally built with two orthogonal beams, but following the initial, 2-week deployment, it was modified to include a third beam.</skos:definition>
<owl:versionInfo>1</owl:versionInfo>
<dc:date>2013-02-07 15:46:03.0</dc:date>
<skos:note xml:lang="en">accepted</skos:note>
<owl:deprecated>false</owl:deprecated>
<skos:broader rdf:resource="http://vocab.nerc.ac.uk/collection/L05/current/115/"/>
<void:inDataset rdf:resource="http://vocab.nerc.ac.uk/.well-known/void"/>
</skos:Concept>
</skos:member>
<skos:member>
<skos:Concept rdf:about="http://vocab.nerc.ac.uk/collection/L22/current/NETT0146/">
<dc:identifier>SDN:L22::NETT0146</dc:identifier>
<skos:notation>SDN:L22::NETT0146</skos:notation>
<skos:prefLabel xml:lang="en">Pumped multiple sample collection system - Yamazi (1960)</skos:prefLabel>
<skos:altLabel>Yamazi pumped sampling system</skos:altLabel>
<skos:definition xml:lang="en">A submersible pump mounted in a circular frame work. Flow from the pump is directed to a flat disc to which 16 to 24 small net cod ends are attached. A ratchet mechanisms rotates the disk and enables the changing of the nets into the path of the flow. System has temperature and light sensors.</skos:definition>
<owl:versionInfo>1</owl:versionInfo>
<dc:date>2011-10-21 14:18:49.0</dc:date>
<skos:note xml:lang="en">accepted</skos:note>
<owl:deprecated>false</owl:deprecated>
<skos:broader rdf:resource="http://vocab.nerc.ac.uk/collection/L05/current/122/"/>
<skos:broader rdf:resource="http://vocab.nerc.ac.uk/collection/L05/current/21/"/>
<skos:broader rdf:resource="http://vocab.nerc.ac.uk/collection/L05/current/134/"/>
<void:inDataset rdf:resource="http://vocab.nerc.ac.uk/.well-known/void"/>
</skos:Concept>
</skos:member>
<skos:member>
<skos:Concept rdf:about="http://vocab.nerc.ac.uk/collection/L22/current/TOOL0557/">
<dc:identifier>SDN:L22::TOOL0557</dc:identifier>
<skos:notation>SDN:L22::TOOL0557</skos:notation>
<skos:prefLabel xml:lang="en">RAPID ISOMAP-UK manual water sampler</skos:prefLabel>
<skos:altLabel>ISOMAP-UK manual sampler</skos:altLabel>
<skos:definition xml:lang="en">Manual water sample collection system used during the RAPID ISOMAP-UK project. It comprises a sample container attached to the end of an extendable pole marked with target depths. The container is fitted with a sealing plug attached to a long cord. Samples are obtained by lowering the pole (or just the container for surface samples) vertically into the water. At the required depth the cord is pulled, thereby removing the plug and filling the container. After 30 seconds the container is brought slowly to the surface and the sample transfered to a storage bottle.</skos:definition>
<owl:versionInfo>2</owl:versionInfo>
<dc:date>2012-10-04 11:59:23.0</dc:date>
<skos:note xml:lang="en">accepted</skos:note>
<owl:deprecated>false</owl:deprecated>
<skos:broader rdf:resource="http://vocab.nerc.ac.uk/collection/L05/current/30/"/>
<void:inDataset rdf:resource="http://vocab.nerc.ac.uk/.well-known/void"/>
</skos:Concept>
</skos:member>
<skos:member>
<skos:Concept rdf:about="http://vocab.nerc.ac.uk/collection/L22/current/TOOL0169/">
<dc:identifier>SDN:L22::TOOL0169</dc:identifier>
<skos:notation>SDN:L22::TOOL0169</skos:notation>
<skos:prefLabel xml:lang="en">RBR DR-1050 depth recorder</skos:prefLabel>
<skos:altLabel>RBR DR-1050 depth recorder</skos:altLabel>
<skos:definition xml:lang="en">The DR-1050 is a pressure recorder with possible ranges of 10, 20, 50, 100, 200, 500, 740, 1000, 2000, 4000, 6000 and 10000 dbar; an accuracy of 0.05% full scale; a resolution of &lt;0.001% full scale; and a time constant of &lt;10 msec.</skos:definition>
<owl:versionInfo>1</owl:versionInfo>
<dc:date>2010-05-18 16:10:58.0</dc:date>
<skos:note xml:lang="en">accepted</skos:note>
<owl:deprecated>false</owl:deprecated>
<skos:broader rdf:resource="http://vocab.nerc.ac.uk/collection/L05/current/111/"/>
<void:inDataset rdf:resource="http://vocab.nerc.ac.uk/.well-known/void"/>
</skos:Concept>
</skos:member>
<skos:member>
<skos:Concept rdf:about="http://vocab.nerc.ac.uk/collection/L22/current/TOOL0054/">
<dc:identifier>SDN:L22::TOOL0054</dc:identifier>
<skos:notation>SDN:L22::TOOL0054</skos:notation>
<skos:prefLabel xml:lang="en">RBR TDR-2050 underwater temperature logger</skos:prefLabel>
<skos:altLabel>RBR TDR-2050</skos:altLabel>
<skos:definition xml:lang="en">The TDR-2050 is a small (235mm x 38mm OD), self-contained, submersible temperature and depth recorder (sensors and data logger). It can be deployed for a period of up to three years and can collect more than 1,200,000 sets of samples. Data can be retained in memory for 20 years (even without batteries). Available in two casings, plastic and titanium, with depth ratings of 740m and 6600m respectively. The temperature channel of the TDR-2050 is calibrated to an accuracy of ± 0.002°C (ITS-90) over the range -5 to +35°C.  Typical drift has been measured to be 0.002°C per year. The thermistor may be external (&lt;3sec time constant) or internal (&lt;20sec time constant). A fast thermistor probe (0.095sec) is also available. The depth channel is calibrated to an accuracy of 0.05%fs  Ranges from 10m to 6,600m are available.</skos:definition>
<owl:versionInfo>1</owl:versionInfo>
<dc:date>2009-11-30 11:56:35.0</dc:date>
<skos:note xml:lang="en">accepted</skos:note>
<owl:deprecated>false</owl:deprecated>
<skos:broader rdf:resource="http://vocab.nerc.ac.uk/collection/L05/current/134/"/>
<void:inDataset rdf:resource="http://vocab.nerc.ac.uk/.well-known/void"/>
</skos:Concept>
</skos:member>
<skos:member>
<skos:Concept rdf:about="http://vocab.nerc.ac.uk/collection/L22/current/TOOL0387/">
<dc:identifier>SDN:L22::TOOL0387</dc:identifier>
<skos:notation>SDN:L22::TOOL0387</skos:notation>
<skos:prefLabel xml:lang="en">RBR TGR-1050P submersible tide gauge</skos:prefLabel>
<skos:altLabel>RBR TGR-1050P</skos:altLabel>
<skos:definition xml:lang="en">A pressure recorder designed to measure tides. Possible ranges are 10, 20 50 and 100 dbar, with an accuracy of ± 0.05% full scale, resolution of &lt;0.001% full scale and a time constant of &lt;10 msec. Pressure data are sampled at 4Hz. The sample period and the length of the averaging burst are fully programmable. It has a built-in averaging function to eliminate wave action.</skos:definition>
<owl:versionInfo>1</owl:versionInfo>
<dc:date>2011-04-08 07:51:17.0</dc:date>
<skos:note xml:lang="en">accepted</skos:note>
<owl:deprecated>false</owl:deprecated>
<skos:broader rdf:resource="http://vocab.nerc.ac.uk/collection/L05/current/111/"/>
<void:inDataset rdf:resource="http://vocab.nerc.ac.uk/.well-known/void"/>
</skos:Concept>
</skos:member>
<skos:member>
<skos:Concept rdf:about="http://vocab.nerc.ac.uk/collection/L22/current/TOOL0055/">
<dc:identifier>SDN:L22::TOOL0055</dc:identifier>
<skos:notation>SDN:L22::TOOL0055</skos:notation>
<skos:prefLabel xml:lang="en">RBR TR-1050 underwater temperature logger</skos:prefLabel>
<skos:altLabel>RBR TR-1050</skos:altLabel>
<skos:definition xml:lang="en">The TR-1050 is a small (230mm x 38mm OD), self-contained, submersible temperature recorder with a calibration to ±0.002ºC.  Typical calibration drift of 0.002ºC per year has been measured. It can be deployed for a period of up to three years and can collect more than 2,400,000 samples. Data are retained in memory for 20 years (even without batteries). It has a measurement range of -5ºC to +35ºC in its standard calibration but can be configured to measure wider ranges. The logger can be fitted with different thermistors to operate to as low as -40ºC or up to +50ºC.</skos:definition>
<owl:versionInfo>1</owl:versionInfo>
<dc:date>2009-11-30 11:56:35.0</dc:date>
<skos:note xml:lang="en">accepted</skos:note>
<owl:deprecated>false</owl:deprecated>
<skos:broader rdf:resource="http://vocab.nerc.ac.uk/collection/L05/current/134/"/>
<void:inDataset rdf:resource="http://vocab.nerc.ac.uk/.well-known/void"/>
</skos:Concept>
</skos:member>
<skos:member>
<skos:Concept rdf:about="http://vocab.nerc.ac.uk/collection/L22/current/TOOL0053/">
<dc:identifier>SDN:L22::TOOL0053</dc:identifier>
<skos:notation>SDN:L22::TOOL0053</skos:notation>
<skos:prefLabel xml:lang="en">RBR XR-420 CTD Marine</skos:prefLabel>
<skos:altLabel>RBR XR-420 CTD</skos:altLabel>
<skos:definition xml:lang="en">A small autonomous data logger designed to monitor conductivity, temperature and depth. Conductivity (accuracy ± 0.003 mS/cm) is measured using a 3-coil closed loop feedback inductive cell for superior temperature compensation. The thermistor (Themometrics) used to record temperature (accuracy ± 0.002°C) is aged and hermetically sealed in the tip of a shock resistant solid glass rod. Pressure (accuracy 0.05% full scale) sensors use reliable semiconductor technology and 316 stainless steel housing developed for long-term stability in harsh environments.</skos:definition>
<owl:versionInfo>2</owl:versionInfo>
<dc:date>2010-11-18 12:39:41.0</dc:date>
<skos:note xml:lang="en">accepted</skos:note>
<owl:deprecated>false</owl:deprecated>
<skos:broader rdf:resource="http://vocab.nerc.ac.uk/collection/L05/current/350/"/>
<skos:broader rdf:resource="http://vocab.nerc.ac.uk/collection/L05/current/134/"/>
<void:inDataset rdf:resource="http://vocab.nerc.ac.uk/.well-known/void"/>
</skos:Concept>
</skos:member>
<skos:member>
<skos:Concept rdf:about="http://vocab.nerc.ac.uk/collection/L22/current/TOOL0273/">
<dc:identifier>SDN:L22::TOOL0273</dc:identifier>
<skos:notation>SDN:L22::TOOL0273</skos:notation>
<skos:prefLabel xml:lang="en">RD200A echosounder</skos:prefLabel>
<skos:altLabel>RD200A echosounder</skos:altLabel>
<skos:definition xml:lang="en">A single-beam navigational echo sounder optimised for measurements of water depth below keel in water depths less than 100m.</skos:definition>
<owl:versionInfo>1</owl:versionInfo>
<dc:date>2010-05-18 16:10:58.0</dc:date>
<skos:note xml:lang="en">accepted</skos:note>
<owl:deprecated>false</owl:deprecated>
<skos:broader rdf:resource="http://vocab.nerc.ac.uk/collection/L05/current/156/"/>
<void:inDataset rdf:resource="http://vocab.nerc.ac.uk/.well-known/void"/>
</skos:Concept>
</skos:member>
<skos:member>
<skos:Concept rdf:about="http://vocab.nerc.ac.uk/collection/L22/current/TOOL0361/">
<dc:identifier>SDN:L22::TOOL0361</dc:identifier>
<skos:notation>SDN:L22::TOOL0361</skos:notation>
<skos:prefLabel xml:lang="en">RS Aqua WaveRadar Rex wave and sea level sensor</skos:prefLabel>
<skos:altLabel>RS Aqua WaveRadar Rex</skos:altLabel>
<skos:definition xml:lang="en">Microwave radar measuring the distance between instrument and water surface. It uses a 9.7-10.3GHz linear sweep pulse to measure distances over the range 3-65 metres with an accuracy of +- 6mm for a range of less than 50 metres or +-12mm for longer ranges.</skos:definition>
<owl:versionInfo>1</owl:versionInfo>
<dc:date>2010-11-24 09:31:30.0</dc:date>
<skos:note xml:lang="en">accepted</skos:note>
<owl:deprecated>false</owl:deprecated>
<skos:broader rdf:resource="http://vocab.nerc.ac.uk/collection/L05/current/111/"/>
<skos:broader rdf:resource="http://vocab.nerc.ac.uk/collection/L05/current/110/"/>
<void:inDataset rdf:resource="http://vocab.nerc.ac.uk/.well-known/void"/>
</skos:Concept>
</skos:member>
<skos:member>
<skos:Concept rdf:about="http://vocab.nerc.ac.uk/collection/L22/current/TOOL0331/">
<dc:identifier>SDN:L22::TOOL0331</dc:identifier>
<skos:notation>SDN:L22::TOOL0331</skos:notation>
<skos:prefLabel xml:lang="en">Radar Water Level Recorder</skos:prefLabel>
<skos:altLabel>Radar Water Level Recorder</skos:altLabel>
<skos:definition xml:lang="en">A generic term for radar water level recorders (also known as wavemeters) that measure the distance between the instrument and the water surface. They can be used to measure ocean waves or sea level (depending on sampling frequency) and have been employed on structures such as oil platforms.</skos:definition>
<owl:versionInfo>1</owl:versionInfo>
<dc:date>2010-09-06 12:45:22.0</dc:date>
<skos:note xml:lang="en">accepted</skos:note>
<owl:deprecated>false</owl:deprecated>
<skos:broader rdf:resource="http://vocab.nerc.ac.uk/collection/L05/current/111/"/>
<skos:broader rdf:resource="http://vocab.nerc.ac.uk/collection/L05/current/110/"/>
<void:inDataset rdf:resource="http://vocab.nerc.ac.uk/.well-known/void"/>
</skos:Concept>
</skos:member>
<skos:member>
<skos:Concept rdf:about="http://vocab.nerc.ac.uk/collection/L22/current/NETT0147/">
<dc:identifier>SDN:L22::NETT0147</dc:identifier>
<skos:notation>SDN:L22::NETT0147</skos:notation>
<skos:prefLabel xml:lang="en">Reeve net - Reeve (1981)</skos:prefLabel>
<skos:altLabel>Reeve Net</skos:altLabel>
<skos:definition xml:lang="en">A very large acrylic cylindrical cod end (30 litres) attached to a simple ring net or a paired net system (with 75 cm diameter nets) to collect fragile gelatinous animals (with 17-litre cod ends). Also describes a pressure activated mechanism to enable the nets to float up the wire to the surface without being affected by the motion of the vessel [Wiebe and Benfield 2003 Plate 3 E, F].</skos:definition>
<owl:versionInfo>1</owl:versionInfo>
<dc:date>2011-10-21 14:18:49.0</dc:date>
<skos:note xml:lang="en">accepted</skos:note>
<owl:deprecated>false</owl:deprecated>
<skos:broader rdf:resource="http://vocab.nerc.ac.uk/collection/L05/current/22/"/>
<void:inDataset rdf:resource="http://vocab.nerc.ac.uk/.well-known/void"/>
</skos:Concept>
</skos:member>
<skos:member>
<skos:Concept rdf:about="http://vocab.nerc.ac.uk/collection/L22/current/TOOL0641/">
<dc:identifier>SDN:L22::TOOL0641</dc:identifier>
<skos:notation>SDN:L22::TOOL0641</skos:notation>
<skos:prefLabel xml:lang="en">Rockland Scientific FP07-38 microstructure thermistor</skos:prefLabel>
<skos:altLabel>FP07-38 microstructure thermistor</skos:altLabel>
<skos:definition xml:lang="en">A fast-response temperature sensor for oceanographic applications. The sensing tip is a microbead thermistor (manufactured by GE Thermometics), mounted on a 9.525 mm diameter stainless steel string which can be attached to ocean microstructure instruments. The instrument has a frequency response of approximately 23 Hz and a response time of 0.007 s. The sensor operates over the range -2 to +32 degC and has a resolution of 0.0001 degC.</skos:definition>
<owl:versionInfo>1</owl:versionInfo>
<dc:date>2013-09-24 15:43:26.0</dc:date>
<skos:note xml:lang="en">accepted</skos:note>
<owl:deprecated>false</owl:deprecated>
<skos:broader rdf:resource="http://vocab.nerc.ac.uk/collection/L05/current/184/"/>
<skos:broader rdf:resource="http://vocab.nerc.ac.uk/collection/L05/current/134/"/>
<void:inDataset rdf:resource="http://vocab.nerc.ac.uk/.well-known/void"/>
</skos:Concept>
</skos:member>
<skos:member>
<skos:Concept rdf:about="http://vocab.nerc.ac.uk/collection/L22/current/TOOL0643/">
<dc:identifier>SDN:L22::TOOL0643</dc:identifier>
<skos:notation>SDN:L22::TOOL0643</skos:notation>
<skos:prefLabel xml:lang="en">Rockland Scientific Geo-electro magnetic current meter (GEMCM)</skos:prefLabel>
<skos:altLabel>Rockland Scientific GEMCM</skos:altLabel>
<skos:definition xml:lang="en">A geo-electromagnetic current meter based upon Stanford et al. (1978). The instrument measures the variations of horizontal velocity between the sea surface and bottom, based on the measurement of electric currents generated by the motion of the seawater through the Earth's magnetic field. The GEMCM supports a completely isolated measurement of the battery voltage in an instrument system and 2-component signals from a geo-electro-magnetic current meter. The instrument carries a 3-axis magnetometer that can be used as a compass. All outputs are digital and connect to the serial instrument bus.</skos:definition>
<owl:versionInfo>1</owl:versionInfo>
<dc:date>2013-09-24 15:48:09.0</dc:date>
<skos:note xml:lang="en">accepted</skos:note>
<owl:deprecated>false</owl:deprecated>
<skos:broader rdf:resource="http://vocab.nerc.ac.uk/collection/L05/current/384/"/>
<void:inDataset rdf:resource="http://vocab.nerc.ac.uk/.well-known/void"/>
</skos:Concept>
</skos:member>
<skos:member>
<skos:Concept rdf:about="http://vocab.nerc.ac.uk/collection/L22/current/TOOL0642/">
<dc:identifier>SDN:L22::TOOL0642</dc:identifier>
<skos:notation>SDN:L22::TOOL0642</skos:notation>
<skos:prefLabel xml:lang="en">Rockland Scientific SPM-38 velocity shear probe</skos:prefLabel>
<skos:altLabel>SPM-38 velocity shear probe</skos:altLabel>
<skos:definition xml:lang="en">A velocity shear probe measuring microstructure velocity fluctuations in oceans and lakes. The instrument measures a single spatial component of turbulent velocity fluctuations, in a direction perpendicular to the probes main axis. The sensing head is based upon the design by Osborn (1974) and the sensing element consists of a parabolic, flexible rubber tip. The oncoming flow produces a hydrodynamic lift force proportional to the fluctuating cross-stream velocity component u. A piezo-ceramic beam embedded in the rubber tip translates the lift force into an electric signal that is proportional to u. The length of the sensing tip (10 mm) determines the maximum wavenumber resolution of the sensor which is approximately 48 cycles per meter. The measurements can be corrected to include wavenumbers up to 150 cpm. The sensor operates over the range 0 to 10 s^-1, has a sensitivity of 0.04 to 0.09 V m s^-2 and resolution of approximately 10 to 4 s.</skos:definition>
<owl:versionInfo>1</owl:versionInfo>
<dc:date>2013-09-24 15:45:14.0</dc:date>
<skos:note xml:lang="en">accepted</skos:note>
<owl:deprecated>false</owl:deprecated>
<skos:broader rdf:resource="http://vocab.nerc.ac.uk/collection/L05/current/384/"/>
<void:inDataset rdf:resource="http://vocab.nerc.ac.uk/.well-known/void"/>
</skos:Concept>
</skos:member>
<skos:member>
<skos:Concept rdf:about="http://vocab.nerc.ac.uk/collection/L22/current/TOOL0639/">
<dc:identifier>SDN:L22::TOOL0639</dc:identifier>
<skos:notation>SDN:L22::TOOL0639</skos:notation>
<skos:prefLabel xml:lang="en">Rockland Scientific Vertical Microstructure Profiler (VMP) 5500</skos:prefLabel>
<skos:altLabel>VMP 5500</skos:altLabel>
<skos:definition xml:lang="en">A full ocean-depth untethered vertical microstructure turbulence profiler for the measurement of dissipation-scale turbulence along with fine-scale temperature and conductivity for up to 5500 m depth. The instrument is fitted with pressure, temperature (SBE-3F) and conductivity (SBE-4C) sensors, three acceleration sensors, a PC104 computer data acquisition and communication system, anti-aliasing filters and a standard suite of microstructure sensors which includes two SPM-38-5 velocity shear probes, two FP07-38-5 fast thermistors and an optional microstructure conductivity probe (SBE7). The instrument has an aluminium frame with syntactic foam attached for flotation. Data is collected on the downcast and after reaching a pre-defined depth the profiler releases ballast weights so that the instrument becomes positively buoyant. The VMP 5500 has a strobe light and a radio beacon and can also be fitted with an Argos transmitter for locating purposes. The instrument was replaced by the VMP 6000 in 2010.</skos:definition>
<owl:versionInfo>1</owl:versionInfo>
<dc:date>2013-09-24 14:37:47.0</dc:date>
<skos:note xml:lang="en">accepted</skos:note>
<owl:deprecated>false</owl:deprecated>
<skos:broader rdf:resource="http://vocab.nerc.ac.uk/collection/L05/current/384/"/>
<skos:broader rdf:resource="http://vocab.nerc.ac.uk/collection/L05/current/184/"/>
<void:inDataset rdf:resource="http://vocab.nerc.ac.uk/.well-known/void"/>
</skos:Concept>
</skos:member>
<skos:member>
<skos:Concept rdf:about="http://vocab.nerc.ac.uk/collection/L22/current/TOOL0576/">
<dc:identifier>SDN:L22::TOOL0576</dc:identifier>
<skos:notation>SDN:L22::TOOL0576</skos:notation>
<skos:prefLabel xml:lang="en">Rockland Scientific Vertical Microstructure Profiler VMP 500</skos:prefLabel>
<skos:altLabel>VMP 500</skos:altLabel>
<skos:definition xml:lang="en">A vertical microstructure turbulence profiler for the measurement of dissipation-scale turbulence in oceans and lakes up to 500 m depth. It is equipped with microstructure velocity probes (shear probes), high-resolution temperature sensors (fast thermistors), pressure sensor and three-axis high accuracy accelerometers. The instrument includes a bottom landing guard and a deck unit for data communication. Optional extras include high-accuracy CTD sensors either a SBE7-38 microstructure conductivity sensor or SBE-3F/SBE-4C temperature and conductivity sensors. The VMP 500 is suitable for deployment from small vessels and can be powered by a 12 V car battery (using an inverter).</skos:definition>
<owl:versionInfo>1</owl:versionInfo>
<dc:date>2012-12-18 15:09:37.0</dc:date>
<skos:note xml:lang="en">accepted</skos:note>
<owl:deprecated>false</owl:deprecated>
<skos:broader rdf:resource="http://vocab.nerc.ac.uk/collection/L05/current/384/"/>
<void:inDataset rdf:resource="http://vocab.nerc.ac.uk/.well-known/void"/>
</skos:Concept>
</skos:member>
<skos:member>
<skos:Concept rdf:about="http://vocab.nerc.ac.uk/collection/L22/current/NETT0157/">
<dc:identifier>SDN:L22::NETT0157</dc:identifier>
<skos:notation>SDN:L22::NETT0157</skos:notation>
<skos:prefLabel xml:lang="en">Rosette-Controlled Tucker Trawl system - Burd and Thompson (1993)</skos:prefLabel>
<skos:altLabel>Burd modified Tucker Trawl</skos:altLabel>
<skos:definition xml:lang="en">A 100 cm x 140 cm rectangular mouth opening frame frame with 7 nets made with 0.33 mm mesh. A rosette release mechanism was used to open and close nets by commands from the ship via conducting cable. The frame carried pressure, temperature, conductivity, transmissometer sensors.  Flow past the frame was measured with an ADCP [Wiebe and Benfield 2003 Plate 30 B].</skos:definition>
<owl:versionInfo>1</owl:versionInfo>
<dc:date>2011-10-21 14:18:49.0</dc:date>
<skos:note xml:lang="en">accepted</skos:note>
<owl:deprecated>false</owl:deprecated>
<skos:broader rdf:resource="http://vocab.nerc.ac.uk/collection/L05/current/134/"/>
<skos:broader rdf:resource="http://vocab.nerc.ac.uk/collection/L05/current/23/"/>
<skos:broader rdf:resource="http://vocab.nerc.ac.uk/collection/L05/current/124/"/>
<skos:broader rdf:resource="http://vocab.nerc.ac.uk/collection/L05/current/350/"/>
<skos:broader rdf:resource="http://vocab.nerc.ac.uk/collection/L05/current/68/"/>
<void:inDataset rdf:resource="http://vocab.nerc.ac.uk/.well-known/void"/>
</skos:Concept>
</skos:member>
<skos:member>
<skos:Concept rdf:about="http://vocab.nerc.ac.uk/collection/L22/current/TOOL0494/">
<dc:identifier>SDN:L22::TOOL0494</dc:identifier>
<skos:notation>SDN:L22::TOOL0494</skos:notation>
<skos:prefLabel xml:lang="en">Rotronic Hygromet MP102H temperature and humidity probe</skos:prefLabel>
<skos:altLabel>Rotronic MP102H</skos:altLabel>
<skos:definition xml:lang="en">Meteorological probe with a Hygro Clip HC2-S3 plug-in sensor that measures humidity and temperature. This model has a range of 0 to 100% in humidity, with an accuracy of 0.8%, and a temperature range of -40 to 80 degC, with an accuracy of 0.1 degC. It can be equipped with a signal conditioned Pt100 temperature probe. Model MP102H produces a voltage output as opposed to the current output produced by the similar MP402H.</skos:definition>
<owl:versionInfo>1</owl:versionInfo>
<dc:date>2012-05-21 10:02:44.0</dc:date>
<skos:note xml:lang="en">accepted</skos:note>
<owl:deprecated>false</owl:deprecated>
<skos:broader rdf:resource="http://vocab.nerc.ac.uk/collection/L05/current/102/"/>
<skos:broader rdf:resource="http://vocab.nerc.ac.uk/collection/L22/current/TOOL0618/"/>
<void:inDataset rdf:resource="http://vocab.nerc.ac.uk/.well-known/void"/>
</skos:Concept>
</skos:member>
<skos:member>
<skos:Concept rdf:about="http://vocab.nerc.ac.uk/collection/L22/current/TOOL0495/">
<dc:identifier>SDN:L22::TOOL0495</dc:identifier>
<skos:notation>SDN:L22::TOOL0495</skos:notation>
<skos:prefLabel xml:lang="en">Rotronic Hygromet MP402H temperature and humidity probe</skos:prefLabel>
<skos:altLabel>Rotronic MP402H</skos:altLabel>
<skos:definition xml:lang="en">Meteorological probe with a Hygro Clip HC2-S3 plug-in sensor that measures humidity and temperature. This model has a range of 0 to 100% in humidity, with an accuracy of 0.8%, and a temperature range of -40 to 80 degC, with an accuracy of 0.1 degC. It can be equipped with a signal conditioned Pt100 temperature probe. Model MP402H produces a current output as opposed to the voltage output produced by the similar MP102H.</skos:definition>
<owl:versionInfo>1</owl:versionInfo>
<dc:date>2012-05-21 10:02:44.0</dc:date>
<skos:note xml:lang="en">accepted</skos:note>
<owl:deprecated>false</owl:deprecated>
<skos:broader rdf:resource="http://vocab.nerc.ac.uk/collection/L05/current/102/"/>
<skos:broader rdf:resource="http://vocab.nerc.ac.uk/collection/L22/current/TOOL0618/"/>
<void:inDataset rdf:resource="http://vocab.nerc.ac.uk/.well-known/void"/>
</skos:Concept>
</skos:member>
<skos:member>
<skos:Concept rdf:about="http://vocab.nerc.ac.uk/collection/L22/current/TOOL0618/">
<dc:identifier>SDN:L22::TOOL0618</dc:identifier>
<skos:notation>SDN:L22::TOOL0618</skos:notation>
<skos:prefLabel xml:lang="en">Rotronic Instruments Hygromet (MP1xxH) humidity and temperature probe series</skos:prefLabel>
<skos:altLabel>Rotronic Hygromet series</skos:altLabel>
<skos:definition xml:lang="en">An analogue atmospheric humidity and temperature probe. The instrument operates within 0-100 percent relative humidity, with an accuracy of +/-0.8 percent. The temperature range varies between -50 to 80 degC and has an accuracy of +/- 0.1 degC.</skos:definition>
<owl:versionInfo>1</owl:versionInfo>
<dc:date>2013-04-23 12:30:40.0</dc:date>
<skos:note xml:lang="en">accepted</skos:note>
<owl:deprecated>false</owl:deprecated>
<skos:narrower rdf:resource="http://vocab.nerc.ac.uk/collection/L22/current/TOOL0495/"/>
<skos:narrower rdf:resource="http://vocab.nerc.ac.uk/collection/L22/current/TOOL0494/"/>
<skos:broader rdf:resource="http://vocab.nerc.ac.uk/collection/L05/current/102/"/>
<void:inDataset rdf:resource="http://vocab.nerc.ac.uk/.well-known/void"/>
</skos:Concept>
</skos:member>
<skos:member>
<skos:Concept rdf:about="http://vocab.nerc.ac.uk/collection/L22/current/TOOL0399/">
<dc:identifier>SDN:L22::TOOL0399</dc:identifier>
<skos:notation>SDN:L22::TOOL0399</skos:notation>
<skos:prefLabel xml:lang="en">Rotronic Instruments MP103A humidity and temperature probe</skos:prefLabel>
<skos:altLabel>Rotronic MP103A</skos:altLabel>
<skos:definition xml:lang="en">An analogue, linear response atmospheric humidity and temperature probe. The instrument operates over ranges of 0-100% relative humidity (0 to 1 volts), with an accuracy of +/-1%, and -40 to 60 degC (-0.4 to 0.6 volts), with an accuracy of +/-0.3 degC.</skos:definition>
<owl:versionInfo>1</owl:versionInfo>
<dc:date>2011-04-14 09:29:16.0</dc:date>
<skos:note xml:lang="en">accepted</skos:note>
<owl:deprecated>false</owl:deprecated>
<skos:broader rdf:resource="http://vocab.nerc.ac.uk/collection/L22/current/TOOL0617/"/>
<skos:broader rdf:resource="http://vocab.nerc.ac.uk/collection/L05/current/102/"/>
<void:inDataset rdf:resource="http://vocab.nerc.ac.uk/.well-known/void"/>
</skos:Concept>
</skos:member>
<skos:member>
<skos:Concept rdf:about="http://vocab.nerc.ac.uk/collection/L22/current/TOOL0617/">
<dc:identifier>SDN:L22::TOOL0617</dc:identifier>
<skos:notation>SDN:L22::TOOL0617</skos:notation>
<skos:prefLabel xml:lang="en">Rotronic Instruments MP1xxA humidity and temperature probe series</skos:prefLabel>
<skos:altLabel>Rotronic MP100 series</skos:altLabel>
<skos:definition xml:lang="en">An analogue, linear response atmospheric humidity and temperature probe. The instrument operates within 0-100 percent relative humidity (0 to 1 volts), with an accuracy of +/-1 percent. The temperature range varies between -40 to 60 degC (-0.4 to 0.6 volts) depending on the specific model and has an accuracy of +/-0.3 degC.</skos:definition>
<owl:versionInfo>1</owl:versionInfo>
<dc:date>2013-04-23 12:30:38.0</dc:date>
<skos:note xml:lang="en">accepted</skos:note>
<owl:deprecated>false</owl:deprecated>
<skos:narrower rdf:resource="http://vocab.nerc.ac.uk/collection/L22/current/TOOL0399/"/>
<skos:broader rdf:resource="http://vocab.nerc.ac.uk/collection/L05/current/102/"/>
<void:inDataset rdf:resource="http://vocab.nerc.ac.uk/.well-known/void"/>
</skos:Concept>
</skos:member>
<skos:member>
<skos:Concept rdf:about="http://vocab.nerc.ac.uk/collection/L22/current/TOOL0200/">
<dc:identifier>SDN:L22::TOOL0200</dc:identifier>
<skos:notation>SDN:L22::TOOL0200</skos:notation>
<skos:prefLabel xml:lang="en">Ruthern Instruments marine pH monitor</skos:prefLabel>
<skos:altLabel>Ruthern pH monitor</skos:altLabel>
<skos:definition xml:lang="en">A pH monitor that may be included in either a portable or bulkhead-mounted system. It consists of a highly reproducible free-diffusion liquid junction which reduces the usual liquid junction potential error encountered with electrode systems. A capillary liquid junction is formed between the reference reservior (containing the silver/silver chloride electrode) and the pH cell (containing the pH electrode and the sample to be analysed). Capable of extreme accuracy and long term stability, giving a precision of +/- 0.01 pH unit across the salinity range 1 to 40 ppt combined with temperature precision to 0.02 deg C.</skos:definition>
<owl:versionInfo>1</owl:versionInfo>
<dc:date>2010-05-18 16:10:58.0</dc:date>
<skos:note xml:lang="en">accepted</skos:note>
<owl:deprecated>false</owl:deprecated>
<skos:broader rdf:resource="http://vocab.nerc.ac.uk/collection/L05/current/355/"/>
<void:inDataset rdf:resource="http://vocab.nerc.ac.uk/.well-known/void"/>
</skos:Concept>
</skos:member>
<skos:member>
<skos:Concept rdf:about="http://vocab.nerc.ac.uk/collection/L22/current/TOOL0180/">
<dc:identifier>SDN:L22::TOOL0180</dc:identifier>
<skos:notation>SDN:L22::TOOL0180</skos:notation>
<skos:prefLabel xml:lang="en">SAIV SD-204 CTD</skos:prefLabel>
<skos:altLabel>SAIV SD-204 CTD</skos:altLabel>
<skos:definition xml:lang="en">A CTD that measures, calculates and records sea water conductivity, salinity, temperature, depth (pressure),  sound velocity and water density. Three optional sensors can be added, for example: dissolved oxygen, fluorescence and turbidity. For optional sensors with several sensitivies, the SD204 has an autorange capability. The instrument is equipped with a mooring bar with a shackle at each end. Data are recorded in physical units and simultaneously transmitted via an RS232 I/O watertight connector for on-line use.</skos:definition>
<owl:versionInfo>1</owl:versionInfo>
<dc:date>2010-05-18 16:10:58.0</dc:date>
<skos:note xml:lang="en">accepted</skos:note>
<owl:deprecated>false</owl:deprecated>
<skos:broader rdf:resource="http://vocab.nerc.ac.uk/collection/L05/current/130/"/>
<skos:broader rdf:resource="http://vocab.nerc.ac.uk/collection/L05/current/350/"/>
<skos:broader rdf:resource="http://vocab.nerc.ac.uk/collection/L05/current/134/"/>
<void:inDataset rdf:resource="http://vocab.nerc.ac.uk/.well-known/void"/>
</skos:Concept>
</skos:member>
<skos:member>
<skos:Concept rdf:about="http://vocab.nerc.ac.uk/collection/L22/current/TOOL0511/">
<dc:identifier>SDN:L22::TOOL0511</dc:identifier>
<skos:notation>SDN:L22::TOOL0511</skos:notation>
<skos:prefLabel xml:lang="en">SEAL Analytical QuAAtro Autoanalyser</skos:prefLabel>
<skos:altLabel>QuAAtro SFA</skos:altLabel>
<skos:definition xml:lang="en">A microflow Segmented Flow Analysis (SFA) system, ideal for water and seawater analysis. It comprises a sampler, a peristaltic pump which simultaneously pumps samples, reagents and air bubbles (to segment the flow) through the system, a chemistry manifold and a high resolution digital photometer that allows detection of a variety of substances at low concentrations. The unit also includes AACE data acquisition software. High temperature heating baths, distillation and dialyzers are available for methods that require them.</skos:definition>
<owl:versionInfo>2</owl:versionInfo>
<dc:date>2012-07-10 09:07:46.0</dc:date>
<skos:note xml:lang="en">accepted</skos:note>
<owl:deprecated>false</owl:deprecated>
<skos:broader rdf:resource="http://vocab.nerc.ac.uk/collection/L05/current/LAB20/"/>
<skos:broader rdf:resource="http://vocab.nerc.ac.uk/collection/L05/current/LAB04/"/>
<void:inDataset rdf:resource="http://vocab.nerc.ac.uk/.well-known/void"/>
</skos:Concept>
</skos:member>
<skos:member>
<skos:Concept rdf:about="http://vocab.nerc.ac.uk/collection/L22/current/TOOL0094/">
<dc:identifier>SDN:L22::TOOL0094</dc:identifier>
<skos:notation>SDN:L22::TOOL0094</skos:notation>
<skos:prefLabel xml:lang="en">SEBAPULS 20 radar water level recorder</skos:prefLabel>
<skos:altLabel>SEBAPULS 20 radar WLR</skos:altLabel>
<skos:definition xml:lang="en">Pulse microwave radar measuring the distance between instrument and surface water. This model is able to measure distances up to 20m with an accuracy of plus or minus 5mm.</skos:definition>
<owl:versionInfo>2</owl:versionInfo>
<dc:date>2010-11-18 12:39:41.0</dc:date>
<skos:note xml:lang="en">accepted</skos:note>
<owl:deprecated>false</owl:deprecated>
<skos:broader rdf:resource="http://vocab.nerc.ac.uk/collection/L05/current/111/"/>
<void:inDataset rdf:resource="http://vocab.nerc.ac.uk/.well-known/void"/>
</skos:Concept>
</skos:member>
<skos:member>
<skos:Concept rdf:about="http://vocab.nerc.ac.uk/collection/L22/current/TOOL0095/">
<dc:identifier>SDN:L22::TOOL0095</dc:identifier>
<skos:notation>SDN:L22::TOOL0095</skos:notation>
<skos:prefLabel xml:lang="en">SEBAPULS 30 radar water level recorder</skos:prefLabel>
<skos:altLabel>SEBAPULS 30 radar WLR</skos:altLabel>
<skos:definition xml:lang="en">Pulse microwave radar measuring the distance between instrument and surface water. This model is able to measure distances up to 30m with an accuracy of plus or minus 3mm.</skos:definition>
<owl:versionInfo>2</owl:versionInfo>
<dc:date>2010-11-18 12:39:41.0</dc:date>
<skos:note xml:lang="en">accepted</skos:note>
<owl:deprecated>false</owl:deprecated>
<skos:broader rdf:resource="http://vocab.nerc.ac.uk/collection/L05/current/111/"/>
<void:inDataset rdf:resource="http://vocab.nerc.ac.uk/.well-known/void"/>
</skos:Concept>
</skos:member>
<skos:member>
<skos:Concept rdf:about="http://vocab.nerc.ac.uk/collection/L22/current/TOOL0096/">
<dc:identifier>SDN:L22::TOOL0096</dc:identifier>
<skos:notation>SDN:L22::TOOL0096</skos:notation>
<skos:prefLabel xml:lang="en">SEBAPULS 70 radar water level recorder</skos:prefLabel>
<skos:altLabel>SEBAPULS 70 radar WLR</skos:altLabel>
<skos:definition xml:lang="en">Pulse microwave radar measuring the distance between instrument and surface water. This model is able to measure distances up to 70m with an accuracy of plus or minus 15mm.</skos:definition>
<owl:versionInfo>2</owl:versionInfo>
<dc:date>2010-11-18 12:39:41.0</dc:date>
<skos:note xml:lang="en">accepted</skos:note>
<owl:deprecated>false</owl:deprecated>
<skos:broader rdf:resource="http://vocab.nerc.ac.uk/collection/L05/current/111/"/>
<void:inDataset rdf:resource="http://vocab.nerc.ac.uk/.well-known/void"/>
</skos:Concept>
</skos:member>
<skos:member>
<skos:Concept rdf:about="http://vocab.nerc.ac.uk/collection/L22/current/TOOL0630/">
<dc:identifier>SDN:L22::TOOL0630</dc:identifier>
<skos:notation>SDN:L22::TOOL0630</skos:notation>
<skos:prefLabel xml:lang="en">SIS Dissolved Oxygen Analyser</skos:prefLabel>
<skos:altLabel>SIS DOA</skos:altLabel>
<skos:definition xml:lang="en">A PC-controlled instrument for determining dissolved oxygen using the Winkler (1888) titration method. The system consists of a transportable box containing a motor burette, an alternating light photometer and a stand with stirrer for the sample flask. The titration endpoint is determined by eye. The photometer is connected to a PC by an interface cable via an RS 232 serial link.</skos:definition>
<owl:versionInfo>2</owl:versionInfo>
<dc:date>2013-07-29 16:31:23.0</dc:date>
<skos:note xml:lang="en">accepted</skos:note>
<owl:deprecated>false</owl:deprecated>
<skos:broader rdf:resource="http://vocab.nerc.ac.uk/collection/L05/current/LAB12/"/>
<void:inDataset rdf:resource="http://vocab.nerc.ac.uk/.well-known/void"/>
</skos:Concept>
</skos:member>
<skos:member>
<skos:Concept rdf:about="http://vocab.nerc.ac.uk/collection/L22/current/TOOL0446/">
<dc:identifier>SDN:L22::TOOL0446</dc:identifier>
<skos:notation>SDN:L22::TOOL0446</skos:notation>
<skos:prefLabel xml:lang="en">SMRU Ltd CTD-Satellite Relay Data Logger 9000</skos:prefLabel>
<skos:altLabel>SMRU Ltd CTD-SDRL 9000</skos:altLabel>
<skos:definition xml:lang="en">CTD sensor package combined with a 401 MHz RF unit and antenna suitable for transmission of conductivity, temperature and pressure data via the Argos satellite system. The unit contains an internal battery and a microprocessor that logs data and schedules the transfer of data. The package is designed for attachment to marine mammals and has an operational temperature range of -20 to +50 degC and a depth range of up to 2000 m. Auxiliary sensors may be attached. It is built and calibrated at Valeport Ltd, while SMRU Ltd, the commercial arm of the Sea Mammal Research Unit of the University of St Andrews, is responsible for its distribution, and for streaming and processing the data.</skos:definition>
<owl:versionInfo>1</owl:versionInfo>
<dc:date>2011-11-24 11:44:57.0</dc:date>
<skos:note xml:lang="en">accepted</skos:note>
<owl:deprecated>false</owl:deprecated>
<skos:broader rdf:resource="http://vocab.nerc.ac.uk/collection/L05/current/POS17/"/>
<skos:broader rdf:resource="http://vocab.nerc.ac.uk/collection/L05/current/350/"/>
<skos:broader rdf:resource="http://vocab.nerc.ac.uk/collection/L05/current/134/"/>
<skos:broader rdf:resource="http://vocab.nerc.ac.uk/collection/L05/current/130/"/>
<void:inDataset rdf:resource="http://vocab.nerc.ac.uk/.well-known/void"/>
</skos:Concept>
</skos:member>
<skos:member>
<skos:Concept rdf:about="http://vocab.nerc.ac.uk/collection/L22/current/TOOL0497/">
<dc:identifier>SDN:L22::TOOL0497</dc:identifier>
<skos:notation>SDN:L22::TOOL0497</skos:notation>
<skos:prefLabel xml:lang="en">SPX Bran+Luebbe colorimetric Autoanalyser 3</skos:prefLabel>
<skos:altLabel>Bran+Luebbe Autoanalyser 3</skos:altLabel>
<skos:definition xml:lang="en">A colorimetric autoanalyser (AA) that may be used to measure nutrient concentrations in seawater. It is an air-segmented, continuous flow instrument comprising a sampler, a peristaltic pump which simultaneously pumps samples, reagents and air bubbles through the system, an analytical cartridge and a colorimeter. Additional modules for functions such as dialysis, distillation and heating can be added to the system, depending on user requirements.</skos:definition>
<owl:versionInfo>1</owl:versionInfo>
<dc:date>2012-05-23 10:01:58.0</dc:date>
<skos:note xml:lang="en">accepted</skos:note>
<owl:deprecated>false</owl:deprecated>
<skos:related rdf:resource="http://vocab.nerc.ac.uk/collection/P01/current/PHOSAATX/"/>
<skos:related rdf:resource="http://vocab.nerc.ac.uk/collection/P01/current/AMONAATX/"/>
<skos:related rdf:resource="http://vocab.nerc.ac.uk/collection/P01/current/NTRIAATX/"/>
<skos:related rdf:resource="http://vocab.nerc.ac.uk/collection/P01/current/NTRZAATX/"/>
<skos:related rdf:resource="http://vocab.nerc.ac.uk/collection/P01/current/PHOSLWTX/"/>
<skos:related rdf:resource="http://vocab.nerc.ac.uk/collection/P01/current/NTRILWTX/"/>
<skos:related rdf:resource="http://vocab.nerc.ac.uk/collection/P01/current/NTRZLWTX/"/>
<skos:related rdf:resource="http://vocab.nerc.ac.uk/collection/P01/current/SLCAAATX/"/>
<skos:broader rdf:resource="http://vocab.nerc.ac.uk/collection/L05/current/LAB04/"/>
<skos:broader rdf:resource="http://vocab.nerc.ac.uk/collection/L05/current/LAB03/"/>
<void:inDataset rdf:resource="http://vocab.nerc.ac.uk/.well-known/void"/>
</skos:Concept>
</skos:member>
<skos:member>
<skos:Concept rdf:about="http://vocab.nerc.ac.uk/collection/L22/current/TOOL0135/">
<dc:identifier>SDN:L22::TOOL0135</dc:identifier>
<skos:notation>SDN:L22::TOOL0135</skos:notation>
<skos:prefLabel xml:lang="en">Satlantic ISUS V2 Nitrate Sensor</skos:prefLabel>
<skos:altLabel>ISUS V2 NO3 sensor</skos:altLabel>
<skos:definition xml:lang="en">An in-situ UV absorption sensor which calculates nitrate concentration from the seawater spectrum. It has a 1cm path length and 200-400 nm wavelength range. It is depth rated to 1000 m.</skos:definition>
<owl:versionInfo>2</owl:versionInfo>
<dc:date>2012-08-09 13:03:05.0</dc:date>
<skos:note xml:lang="en">accepted</skos:note>
<owl:deprecated>false</owl:deprecated>
<skos:broader rdf:resource="http://vocab.nerc.ac.uk/collection/L05/current/181/"/>
<void:inDataset rdf:resource="http://vocab.nerc.ac.uk/.well-known/void"/>
</skos:Concept>
</skos:member>
<skos:member>
<skos:Concept rdf:about="http://vocab.nerc.ac.uk/collection/L22/current/TOOL0528/">
<dc:identifier>SDN:L22::TOOL0528</dc:identifier>
<skos:notation>SDN:L22::TOOL0528</skos:notation>
<skos:prefLabel xml:lang="en">Satlantic ISUS V3 Nitrate Sensor</skos:prefLabel>
<skos:altLabel>ISUS V3 NO3 sensor</skos:altLabel>
<skos:definition xml:lang="en">An active optical instrument with an internal UV light source and spectrometer used to measure in-situ dissolved nitrate. It is a chemical-free method that allows real-time and continuous nitrate concentration measurements in a variety of environments. It uses a Deuterium lamp as a light source and has a 1cm path length and 200-400 nm wavelength range. It has a depth rating of 1000 m and a detection range of  0.5 to 2000 uM *(0.007 to 28 mg/l-N)  and accuracy of +/- 0.2 uM (0.028 mg/l) or ± 10% of reading, whichever is greater. The V3 has USB data transfer ability and window based software.</skos:definition>
<owl:versionInfo>1</owl:versionInfo>
<dc:date>2012-08-09 12:59:50.0</dc:date>
<skos:note xml:lang="en">accepted</skos:note>
<owl:deprecated>false</owl:deprecated>
<skos:broader rdf:resource="http://vocab.nerc.ac.uk/collection/L05/current/181/"/>
<void:inDataset rdf:resource="http://vocab.nerc.ac.uk/.well-known/void"/>
</skos:Concept>
</skos:member>
<skos:member>
<skos:Concept rdf:about="http://vocab.nerc.ac.uk/collection/L22/current/TOOL0398/">
<dc:identifier>SDN:L22::TOOL0398</dc:identifier>
<skos:notation>SDN:L22::TOOL0398</skos:notation>
<skos:prefLabel xml:lang="en">Satlantic Micro Surface Acquisition System (MicroSAS) radiometer</skos:prefLabel>
<skos:altLabel>MicroSAS radiometer</skos:altLabel>
<skos:definition xml:lang="en">A remote sensing system for above-water measurement of ocean colour over the spectral range 300-865 nm. The system includes two radiance sensors for measurement of the sea surface signal and surface glint, and one irradiance sensor for downwelling irradiance. The irradiance sensor response is proportional to the cosine of the angle of incidence of the incoming radiation, while each radiance sensor has a 3.3 deg field of view.</skos:definition>
<owl:versionInfo>1</owl:versionInfo>
<dc:date>2011-04-14 09:29:16.0</dc:date>
<skos:note xml:lang="en">accepted</skos:note>
<owl:deprecated>false</owl:deprecated>
<skos:broader rdf:resource="http://vocab.nerc.ac.uk/collection/L05/current/122/"/>
<void:inDataset rdf:resource="http://vocab.nerc.ac.uk/.well-known/void"/>
</skos:Concept>
</skos:member>
<skos:member>
<skos:Concept rdf:about="http://vocab.nerc.ac.uk/collection/L22/current/TOOL0625/">
<dc:identifier>SDN:L22::TOOL0625</dc:identifier>
<skos:notation>SDN:L22::TOOL0625</skos:notation>
<skos:prefLabel xml:lang="en">Satlantic OCR-504 multispectral radiometer</skos:prefLabel>
<skos:altLabel>Satlantic OCR-504</skos:altLabel>
<skos:definition xml:lang="en">A cosine-response, submersible radiometer designed for multiwavelength measurements of irradiance and radiance for in-water or in-air use. The standard instrument comes with 4 customer defined channels that measures wavelengths in the bandwidth from 400 to 700 nm. UV wavelengths of 305, 325, 340 and 380 nm are available. The radiometer has a depth rating of 350 m, a sampling rate of 7 to 24 Hz and a spectral bandwidth of 10 or 20 nm. The instrument can be mounted on real-time profilers, moored and autonomous deepwater buoys and autonomous underwater vehicles.</skos:definition>
<owl:versionInfo>1</owl:versionInfo>
<dc:date>2013-06-11 16:08:07.0</dc:date>
<skos:note xml:lang="en">accepted</skos:note>
<owl:deprecated>false</owl:deprecated>
<skos:broader rdf:resource="http://vocab.nerc.ac.uk/collection/L05/current/122/"/>
<void:inDataset rdf:resource="http://vocab.nerc.ac.uk/.well-known/void"/>
</skos:Concept>
</skos:member>
<skos:member>
<skos:Concept rdf:about="http://vocab.nerc.ac.uk/collection/L22/current/TOOL0442/">
<dc:identifier>SDN:L22::TOOL0442</dc:identifier>
<skos:notation>SDN:L22::TOOL0442</skos:notation>
<skos:prefLabel xml:lang="en">Satlantic OCR-507 multispectral radiometer</skos:prefLabel>
<skos:altLabel>Satlantic OCR-507</skos:altLabel>
<skos:definition xml:lang="en">A cosine-response, submersible radiometer designed for multiwavelength measurements of irradiance and radiance for in-water or in-air use. The standard instrument comes with 7 customer defined channels that measure wavelengths in the bandwidth from 400 to 700 nm. UV wavelengths of 305, 325, 340 and 380 nm are available. The radiometer has a depth rating of 350 m, a sampling rate of 7 to 24 Hz and a spectral bandwidth of 10 or 20 nm. The instrument can be mounted on real-time profilers, moored and autonomous deepwater buoys and autonomous underwater vehicles.</skos:definition>
<owl:versionInfo>3</owl:versionInfo>
<dc:date>2013-06-11 16:05:54.0</dc:date>
<skos:note xml:lang="en">accepted</skos:note>
<owl:deprecated>false</owl:deprecated>
<skos:broader rdf:resource="http://vocab.nerc.ac.uk/collection/L05/current/122/"/>
<void:inDataset rdf:resource="http://vocab.nerc.ac.uk/.well-known/void"/>
</skos:Concept>
</skos:member>
<skos:member>
<skos:Concept rdf:about="http://vocab.nerc.ac.uk/collection/L22/current/TOOL0489/">
<dc:identifier>SDN:L22::TOOL0489</dc:identifier>
<skos:notation>SDN:L22::TOOL0489</skos:notation>
<skos:prefLabel xml:lang="en">Satlantic Submersible Ultraviolet Nitrate Analyser</skos:prefLabel>
<skos:altLabel>Satlantic SUNA NO3 analyser</skos:altLabel>
<skos:definition xml:lang="en">The Submersible Ultraviolet Nitrate Analyser (SUNA) uses ultraviolet absorption spectroscopy to measure in-situ dissolved nitrate. It is a chemical-free method that allows real-time and continuous nitrate concentration measurements in a variety of environments. It has a 1 cm path length, 190 - 370 nm wavelength range and a depth rating of 100 m.</skos:definition>
<owl:versionInfo>1</owl:versionInfo>
<dc:date>2012-04-17 13:56:38.0</dc:date>
<skos:note xml:lang="en">accepted</skos:note>
<owl:deprecated>false</owl:deprecated>
<skos:broader rdf:resource="http://vocab.nerc.ac.uk/collection/L05/current/181/"/>
<void:inDataset rdf:resource="http://vocab.nerc.ac.uk/.well-known/void"/>
</skos:Concept>
</skos:member>
<skos:member>
<skos:Concept rdf:about="http://vocab.nerc.ac.uk/collection/L22/current/NETT0151/">
<dc:identifier>SDN:L22::NETT0151</dc:identifier>
<skos:notation>SDN:L22::NETT0151</skos:notation>
<skos:prefLabel xml:lang="en">Scotia closing plankton net - Bruce (1904)</skos:prefLabel>
<skos:altLabel>Scotia net</skos:altLabel>
<skos:definition xml:lang="en">Essentially like the Nansen net (construction has a 35 to 100 cm net diameter 50 cm cylindrical portion of canvas; 150 cm long conical section of silk).</skos:definition>
<owl:versionInfo>1</owl:versionInfo>
<dc:date>2011-10-21 14:18:49.0</dc:date>
<skos:note xml:lang="en">accepted</skos:note>
<owl:deprecated>false</owl:deprecated>
<skos:broader rdf:resource="http://vocab.nerc.ac.uk/collection/L05/current/22/"/>
<void:inDataset rdf:resource="http://vocab.nerc.ac.uk/.well-known/void"/>
</skos:Concept>
</skos:member>
<skos:member>
<skos:Concept rdf:about="http://vocab.nerc.ac.uk/collection/L22/current/NETT0152/">
<dc:identifier>SDN:L22::NETT0152</dc:identifier>
<skos:notation>SDN:L22::NETT0152</skos:notation>
<skos:prefLabel xml:lang="en">Scripps-Narragansett high-speed multiple plankton sampler - Fish and Snodgrass (1962)</skos:prefLabel>
<skos:altLabel>Scripps-Narragansett HSS</skos:altLabel>
<skos:definition xml:lang="en">A 50 cm diameter mouth opening Gulf III sampler with a circular disk holding five cod-end metal mesh buckets.  The disk is rotated to open and close the buckets by electrical commands from the surface transmitted on a double conductor towing cable. Net depth, flowmeter readings, filtered volume are recorded [Wiebe and Benfield 2003 Plate 16 B].</skos:definition>
<owl:versionInfo>1</owl:versionInfo>
<dc:date>2011-10-21 14:18:49.0</dc:date>
<skos:note xml:lang="en">accepted</skos:note>
<owl:deprecated>false</owl:deprecated>
<skos:broader rdf:resource="http://vocab.nerc.ac.uk/collection/L05/current/67/"/>
<skos:broader rdf:resource="http://vocab.nerc.ac.uk/collection/L05/current/388/"/>
<void:inDataset rdf:resource="http://vocab.nerc.ac.uk/.well-known/void"/>
</skos:Concept>
</skos:member>
<skos:member>
<skos:Concept rdf:about="http://vocab.nerc.ac.uk/collection/L22/current/TOOL0453/">
<dc:identifier>SDN:L22::TOOL0453</dc:identifier>
<skos:notation>SDN:L22::TOOL0453</skos:notation>
<skos:prefLabel xml:lang="en">Sea and Sun Technology Microstructure Profiler MSS 90</skos:prefLabel>
<skos:altLabel>MSS 90 microstructure profiler</skos:altLabel>
<skos:definition xml:lang="en">A profiler that measures micro-structure water stratification and small scale turbulence in the water column in marine and limnic environments. It can be used for free sinking or rising measurements. Its sinking or rising velocity can be adjusted by a combination of weights and buoyancy elements. It has a depth rating of approx. 500 m, samples at 1024Hz and is equipped with high resolution micro-structure and turbulence sensors (temperature, current shear) and standard CTD sensors (temperature, conductivity, pressure). All microstructure channels have a response time of &lt;12ms. The unit controls vibrations and tilt internally, and additional sensors, such as oxygen and optical scattering, can be attached.</skos:definition>
<owl:versionInfo>1</owl:versionInfo>
<dc:date>2012-01-24 16:36:37.0</dc:date>
<skos:note xml:lang="en">accepted</skos:note>
<owl:deprecated>false</owl:deprecated>
<skos:broader rdf:resource="http://vocab.nerc.ac.uk/collection/L05/current/134/"/>
<skos:broader rdf:resource="http://vocab.nerc.ac.uk/collection/L05/current/384/"/>
<skos:broader rdf:resource="http://vocab.nerc.ac.uk/collection/L05/current/350/"/>
<void:inDataset rdf:resource="http://vocab.nerc.ac.uk/.well-known/void"/>
</skos:Concept>
</skos:member>
<skos:member>
<skos:Concept rdf:about="http://vocab.nerc.ac.uk/collection/L22/current/TOOL0439/">
<dc:identifier>SDN:L22::TOOL0439</dc:identifier>
<skos:notation>SDN:L22::TOOL0439</skos:notation>
<skos:prefLabel xml:lang="en">Sea and Sun Technology and ISW Wassermesstechnik microstructure profiler</skos:prefLabel>
<skos:altLabel>MSS microstructure profiler</skos:altLabel>
<skos:definition xml:lang="en">The MSS Profiler is designed for simultaneous microstructure and precision measurements of physical parameters in marine water. The instrument includes a microstructure shear sensor, two microstructure temperature sensors, three standard CTD sensors for precision measurements and a sensor to measure the horizontal profiler acceleration. The microstructure sensors are placed at the tip of a slim shaft, about 150 mm in front of the CTD sensors. The shear and horizontal acceleration sensors use a piezoceramic bending beam while the microstructure temperature sensors are resistance thermistors. The CTD sensors are a piezo-resistive pressure sensor, Platinum resistance thermometer and 7-Pole conductivity cell. The MSS was developed jointly in the 1990s by Sea &amp; Sun Technology and ISW Wassermesstechnik. Sea &amp; Sun Technology now support a series of MSS profilers.</skos:definition>
<owl:versionInfo>1</owl:versionInfo>
<dc:date>2011-11-07 15:23:52.0</dc:date>
<skos:note xml:lang="en">accepted</skos:note>
<owl:deprecated>false</owl:deprecated>
<skos:broader rdf:resource="http://vocab.nerc.ac.uk/collection/L05/current/134/"/>
<skos:broader rdf:resource="http://vocab.nerc.ac.uk/collection/L05/current/350/"/>
<skos:broader rdf:resource="http://vocab.nerc.ac.uk/collection/L05/current/384/"/>
<void:inDataset rdf:resource="http://vocab.nerc.ac.uk/.well-known/void"/>
</skos:Concept>
</skos:member>
<skos:member>
<skos:Concept rdf:about="http://vocab.nerc.ac.uk/collection/L22/current/TOOL0039/">
<dc:identifier>SDN:L22::TOOL0039</dc:identifier>
<skos:notation>SDN:L22::TOOL0039</skos:notation>
<skos:prefLabel xml:lang="en">Sea-Bird SBE 13 Dissolved Oxygen Sensor</skos:prefLabel>
<skos:altLabel>SBE 13 DO</skos:altLabel>
<skos:definition xml:lang="en">Dissolved oxygen sensor with either a Beckmann (SBE 13B) or YSI polarographic element (SBE 13Y limited to 2000m depth). Designed to interface with the SBE 9 and 9plus CTD underwater units. An optional plenum to connect into the pumped plumbing system was available but usage with the membrane exposed was possible. Replaced by the SBE 43 in 2001.</skos:definition>
<owl:versionInfo>2</owl:versionInfo>
<dc:date>2010-11-18 12:39:41.0</dc:date>
<skos:note xml:lang="en">accepted</skos:note>
<owl:deprecated>false</owl:deprecated>
<skos:related rdf:resource="http://vocab.nerc.ac.uk/collection/P01/current/OXYSBB01/"/>
<skos:related rdf:resource="http://vocab.nerc.ac.uk/collection/P01/current/DOXYPR01/"/>
<skos:broader rdf:resource="http://vocab.nerc.ac.uk/collection/L05/current/351/"/>
<void:inDataset rdf:resource="http://vocab.nerc.ac.uk/.well-known/void"/>
</skos:Concept>
</skos:member>
<skos:member>
<skos:Concept rdf:about="http://vocab.nerc.ac.uk/collection/L22/current/TOOL0023/">
<dc:identifier>SDN:L22::TOOL0023</dc:identifier>
<skos:notation>SDN:L22::TOOL0023</skos:notation>
<skos:prefLabel xml:lang="en">Sea-Bird SBE 16 SEACAT C-T Recorder</skos:prefLabel>
<skos:altLabel>SBE 16 SEACAT</skos:altLabel>
<skos:definition xml:lang="en">The SBE 16 SEACAT is a conductivity and temperature recorder with an optional pressure sensor designed for depolyment on moorings. Further information may be found on the BODC document server at URL http://www.bodc.ac.uk/data/documents/nodb/117180/. Replaced by the SBE 16plus range in 2001.</skos:definition>
<owl:versionInfo>1</owl:versionInfo>
<dc:date>2009-11-30 11:27:51.0</dc:date>
<skos:note xml:lang="en">accepted</skos:note>
<owl:deprecated>false</owl:deprecated>
<skos:broader rdf:resource="http://vocab.nerc.ac.uk/collection/L05/current/134/"/>
<skos:broader rdf:resource="http://vocab.nerc.ac.uk/collection/L05/current/350/"/>
<void:inDataset rdf:resource="http://vocab.nerc.ac.uk/.well-known/void"/>
</skos:Concept>
</skos:member>
<skos:member>
<skos:Concept rdf:about="http://vocab.nerc.ac.uk/collection/L22/current/TOOL0100/">
<dc:identifier>SDN:L22::TOOL0100</dc:identifier>
<skos:notation>SDN:L22::TOOL0100</skos:notation>
<skos:prefLabel xml:lang="en">Sea-Bird SBE 16Plus SEACAT C-T Recorder</skos:prefLabel>
<skos:altLabel>SBE 16+ SEACAT</skos:altLabel>
<skos:definition xml:lang="en">The SBE 16plus is a high accuracy conductivity and temperature recorder (pressure optional) with RS232 or RS485 interfaces. It is designed for moorings and other long-duration, fixed-site deployments. The SBE 16plus has 6 amplified A/D input channels and conditioned power of 500 ma is avaliable for auxiliary sensors, dissolved oxygen, turbidity, fluorescence, PAR etc. Further information may be found on the BODC document server at URL: http://www.bodc.ac.uk/data/documents/nodb/153217/ (RS485) or http://www.bodc.ac.uk/data/documents/nodb/158981/ (RS232).</skos:definition>
<owl:versionInfo>1</owl:versionInfo>
<dc:date>2010-05-18 16:10:58.0</dc:date>
<skos:note xml:lang="en">accepted</skos:note>
<owl:deprecated>false</owl:deprecated>
<skos:broader rdf:resource="http://vocab.nerc.ac.uk/collection/L05/current/350/"/>
<skos:broader rdf:resource="http://vocab.nerc.ac.uk/collection/L05/current/134/"/>
<void:inDataset rdf:resource="http://vocab.nerc.ac.uk/.well-known/void"/>
</skos:Concept>
</skos:member>
<skos:member>
<skos:Concept rdf:about="http://vocab.nerc.ac.uk/collection/L22/current/TOOL0069/">
<dc:identifier>SDN:L22::TOOL0069</dc:identifier>
<skos:notation>SDN:L22::TOOL0069</skos:notation>
<skos:prefLabel xml:lang="en">Sea-Bird SBE 18 pH Sensor</skos:prefLabel>
<skos:altLabel>SBE 18 pH</skos:altLabel>
<skos:definition xml:lang="en">A pH sensor using a pressure-balanced glass-electrode Ag_AgCl-reference pH probe to provide in-situ measurements at depths up to 1200m. The replaceable pH probe is permanently sealed and is supplied with a soaker bottle attachment that prevents the reference electrode from drying out during storage.</skos:definition>
<owl:versionInfo>1</owl:versionInfo>
<dc:date>2009-11-30 11:56:35.0</dc:date>
<skos:note xml:lang="en">accepted</skos:note>
<owl:deprecated>false</owl:deprecated>
<skos:broader rdf:resource="http://vocab.nerc.ac.uk/collection/L05/current/355/"/>
<void:inDataset rdf:resource="http://vocab.nerc.ac.uk/.well-known/void"/>
</skos:Concept>
</skos:member>
<skos:member>
<skos:Concept rdf:about="http://vocab.nerc.ac.uk/collection/L22/current/TOOL0042/">
<dc:identifier>SDN:L22::TOOL0042</dc:identifier>
<skos:notation>SDN:L22::TOOL0042</skos:notation>
<skos:prefLabel xml:lang="en">Sea-Bird SBE 19 SEACAT CTD</skos:prefLabel>
<skos:altLabel>SBE 19 SEACAT</skos:altLabel>
<skos:definition xml:lang="en">A self-contained battery powered CTD with precision semiconductor strain gauge pressure sensor. Water was supplied to the conductivity sensor by a pump. Housing was plastic (up to 600m depth), aluminium (up to 6800m depth) or titanium (up to 10500m depth). Optional oxygen, pH, fluorescence, PAR, light transmission and turbidity sensors could be fitted. Primarily designed for profiling applications but may be used on a short (less than 2 weeks) duration mooring. Replaced by the SBE19plus model in 2001.</skos:definition>
<owl:versionInfo>2</owl:versionInfo>
<dc:date>2010-11-18 12:39:41.0</dc:date>
<skos:note xml:lang="en">accepted</skos:note>
<owl:deprecated>false</owl:deprecated>
<skos:related rdf:resource="http://vocab.nerc.ac.uk/collection/P01/current/SIGTPR01/"/>
<skos:related rdf:resource="http://vocab.nerc.ac.uk/collection/P01/current/PSALPR01/"/>
<skos:related rdf:resource="http://vocab.nerc.ac.uk/collection/P01/current/SIGTEQ01/"/>
<skos:related rdf:resource="http://vocab.nerc.ac.uk/collection/P01/current/TEMPST01/"/>
<skos:related rdf:resource="http://vocab.nerc.ac.uk/collection/P01/current/CNDCST01/"/>
<skos:related rdf:resource="http://vocab.nerc.ac.uk/collection/P01/current/PSALST01/"/>
<skos:related rdf:resource="http://vocab.nerc.ac.uk/collection/P01/current/POTMCV01/"/>
<skos:related rdf:resource="http://vocab.nerc.ac.uk/collection/P01/current/PRESPR01/"/>
<skos:broader rdf:resource="http://vocab.nerc.ac.uk/collection/L05/current/134/"/>
<skos:broader rdf:resource="http://vocab.nerc.ac.uk/collection/L05/current/130/"/>
<skos:broader rdf:resource="http://vocab.nerc.ac.uk/collection/L05/current/350/"/>
<void:inDataset rdf:resource="http://vocab.nerc.ac.uk/.well-known/void"/>
</skos:Concept>
</skos:member>
<skos:member>
<skos:Concept rdf:about="http://vocab.nerc.ac.uk/collection/L22/current/TOOL0047/">
<dc:identifier>SDN:L22::TOOL0047</dc:identifier>
<skos:notation>SDN:L22::TOOL0047</skos:notation>
<skos:prefLabel xml:lang="en">Sea-Bird SBE 19plus SEACAT CTD</skos:prefLabel>
<skos:altLabel>SBE 19+ SEACAT</skos:altLabel>
<skos:definition xml:lang="en">Self contained self powered CTD profiler. Measures conductivity, temperature and pressure in both profiling (samples at 4 scans/sec) and moored (sample rates of once every 5 seconds to once every 9 hours) mode. Available in plastic or titanium housing with depth ranges of 600m and 7000m respectively. Minature submersible pump provides water to conductivity cell.</skos:definition>
<owl:versionInfo>4</owl:versionInfo>
<dc:date>2010-11-18 12:39:41.0</dc:date>
<skos:note xml:lang="en">accepted</skos:note>
<owl:deprecated>false</owl:deprecated>
<skos:broader rdf:resource="http://vocab.nerc.ac.uk/collection/L05/current/130/"/>
<skos:broader rdf:resource="http://vocab.nerc.ac.uk/collection/L05/current/134/"/>
<skos:broader rdf:resource="http://vocab.nerc.ac.uk/collection/L05/current/350/"/>
<void:inDataset rdf:resource="http://vocab.nerc.ac.uk/.well-known/void"/>
</skos:Concept>
</skos:member>
<skos:member>
<skos:Concept rdf:about="http://vocab.nerc.ac.uk/collection/L22/current/TOOL0040/">
<dc:identifier>SDN:L22::TOOL0040</dc:identifier>
<skos:notation>SDN:L22::TOOL0040</skos:notation>
<skos:prefLabel xml:lang="en">Sea-Bird SBE 25 Sealogger CTD</skos:prefLabel>
<skos:altLabel>SBE 25 Sealogger</skos:altLabel>
<skos:definition xml:lang="en">A compact self-contained CTD comprising a conductivity sensor plumbed into a pumped water supply and separate pressure and temperature sensor modules. The whole unit is mounted in a stainless steel cage with a battery pack, data logger and memory. A dissolved oxygen sensor may be plumbed into the pumped water supply and other sensor modules such as fluorometers and transmissometers may be mounted in the cage and interfaced to the data logger. The instrument may also be used with external power and data logging through an RS-232 interface.</skos:definition>
<owl:versionInfo>2</owl:versionInfo>
<dc:date>2010-11-18 12:39:41.0</dc:date>
<skos:note xml:lang="en">accepted</skos:note>
<owl:deprecated>false</owl:deprecated>
<skos:related rdf:resource="http://vocab.nerc.ac.uk/collection/P01/current/CNDCST01/"/>
<skos:related rdf:resource="http://vocab.nerc.ac.uk/collection/P01/current/PRESPR01/"/>
<skos:related rdf:resource="http://vocab.nerc.ac.uk/collection/P01/current/PSALST01/"/>
<skos:related rdf:resource="http://vocab.nerc.ac.uk/collection/P01/current/OXYSBB01/"/>
<skos:related rdf:resource="http://vocab.nerc.ac.uk/collection/P01/current/TEMPST01/"/>
<skos:related rdf:resource="http://vocab.nerc.ac.uk/collection/P01/current/SIGTPR01/"/>
<skos:related rdf:resource="http://vocab.nerc.ac.uk/collection/P01/current/POTMCV01/"/>
<skos:related rdf:resource="http://vocab.nerc.ac.uk/collection/P01/current/DOXYPR01/"/>
<skos:related rdf:resource="http://vocab.nerc.ac.uk/collection/P01/current/SIGTEQ01/"/>
<skos:broader rdf:resource="http://vocab.nerc.ac.uk/collection/L05/current/130/"/>
<skos:broader rdf:resource="http://vocab.nerc.ac.uk/collection/L05/current/350/"/>
<skos:broader rdf:resource="http://vocab.nerc.ac.uk/collection/L05/current/134/"/>
<void:inDataset rdf:resource="http://vocab.nerc.ac.uk/.well-known/void"/>
</skos:Concept>
</skos:member>
<skos:member>
<skos:Concept rdf:about="http://vocab.nerc.ac.uk/collection/L22/current/TOOL0024/">
<dc:identifier>SDN:L22::TOOL0024</dc:identifier>
<skos:notation>SDN:L22::TOOL0024</skos:notation>
<skos:prefLabel xml:lang="en">Sea-Bird SBE 26 SEAGAUGE Wave and Tide Recorder</skos:prefLabel>
<skos:altLabel>SBE 26 SEAGAUGE</skos:altLabel>
<skos:definition xml:lang="en">The SBE 26 SEAGAUGE is a water level recorder with a Digiquartz pressure sensor, accurate clock, precision thermometer and optional conductivity sensor. Pressure data are integrated to give sea level or are burst recorded at rates up to 4 Hz to measure characterise waves. Further information may be found on the BODC document server at URL http://www.bodc.ac.uk/data/documents/nodb/82441/.</skos:definition>
<owl:versionInfo>1</owl:versionInfo>
<dc:date>2009-11-30 11:27:51.0</dc:date>
<skos:note xml:lang="en">accepted</skos:note>
<owl:deprecated>false</owl:deprecated>
<skos:broader rdf:resource="http://vocab.nerc.ac.uk/collection/L05/current/111/"/>
<skos:broader rdf:resource="http://vocab.nerc.ac.uk/collection/L05/current/110/"/>
<void:inDataset rdf:resource="http://vocab.nerc.ac.uk/.well-known/void"/>
</skos:Concept>
</skos:member>
<skos:member>
<skos:Concept rdf:about="http://vocab.nerc.ac.uk/collection/L22/current/TOOL0022/">
<dc:identifier>SDN:L22::TOOL0022</dc:identifier>
<skos:notation>SDN:L22::TOOL0022</skos:notation>
<skos:prefLabel xml:lang="en">Sea-Bird SBE 37-IM MicroCAT C-T Sensor</skos:prefLabel>
<skos:altLabel>SBE 37-IM MicroCAT</skos:altLabel>
<skos:definition xml:lang="en">The SBE 37 MicroCAT is a high accuracy conductivity and temperature recorder with an optional pressure sensor designed for depolyment on moorings. The IM model has an inductive modem for real-time data transmission plus internal flash memory data storage. Further information may be found on the BODC document server at URL http://www.bodc.ac.uk/data/documents/nodb/113079/.</skos:definition>
<owl:versionInfo>2</owl:versionInfo>
<dc:date>2010-11-18 12:39:41.0</dc:date>
<skos:note xml:lang="en">accepted</skos:note>
<owl:deprecated>false</owl:deprecated>
<skos:broader rdf:resource="http://vocab.nerc.ac.uk/collection/L05/current/350/"/>
<skos:broader rdf:resource="http://vocab.nerc.ac.uk/collection/L05/current/134/"/>
<void:inDataset rdf:resource="http://vocab.nerc.ac.uk/.well-known/void"/>
</skos:Concept>
</skos:member>
<skos:member>
<skos:Concept rdf:about="http://vocab.nerc.ac.uk/collection/L22/current/TOOL0019/">
<dc:identifier>SDN:L22::TOOL0019</dc:identifier>
<skos:notation>SDN:L22::TOOL0019</skos:notation>
<skos:prefLabel xml:lang="en">Sea-Bird SBE 37-IMP MicroCAT C-T Sensor</skos:prefLabel>
<skos:altLabel>SBE 37-IMP MicroCAT</skos:altLabel>
<skos:definition xml:lang="en">The SBE 37 MicroCAT is a high accuracy conductivity and temperature recorder with an optional pressure sensor designed for depolyment on moorings. The IMP model has an inductive modem for real-time data transmission plus internal flash memory data storage with an internal pump to improve conductivity response and protection against fouling.</skos:definition>
<owl:versionInfo>2</owl:versionInfo>
<dc:date>2010-11-18 12:39:41.0</dc:date>
<skos:note xml:lang="en">accepted</skos:note>
<owl:deprecated>false</owl:deprecated>
<skos:broader rdf:resource="http://vocab.nerc.ac.uk/collection/L05/current/350/"/>
<skos:broader rdf:resource="http://vocab.nerc.ac.uk/collection/L05/current/134/"/>
<void:inDataset rdf:resource="http://vocab.nerc.ac.uk/.well-known/void"/>
</skos:Concept>
</skos:member>
<skos:member>
<skos:Concept rdf:about="http://vocab.nerc.ac.uk/collection/L22/current/TOOL0021/">
<dc:identifier>SDN:L22::TOOL0021</dc:identifier>
<skos:notation>SDN:L22::TOOL0021</skos:notation>
<skos:prefLabel xml:lang="en">Sea-Bird SBE 37-SI MicroCAT C-T Sensor</skos:prefLabel>
<skos:altLabel>SBE 37-SI MicroCAT</skos:altLabel>
<skos:definition xml:lang="en">The SBE 37 MicroCAT is a high accuracy conductivity and temperature recorder with an optional pressure sensor designed for depolyment on moorings. The SI model has a serial interface.</skos:definition>
<owl:versionInfo>2</owl:versionInfo>
<dc:date>2010-11-18 12:39:41.0</dc:date>
<skos:note xml:lang="en">accepted</skos:note>
<owl:deprecated>false</owl:deprecated>
<skos:broader rdf:resource="http://vocab.nerc.ac.uk/collection/L05/current/350/"/>
<skos:broader rdf:resource="http://vocab.nerc.ac.uk/collection/L05/current/134/"/>
<void:inDataset rdf:resource="http://vocab.nerc.ac.uk/.well-known/void"/>
</skos:Concept>
</skos:member>
<skos:member>
<skos:Concept rdf:about="http://vocab.nerc.ac.uk/collection/L22/current/TOOL0020/">
<dc:identifier>SDN:L22::TOOL0020</dc:identifier>
<skos:notation>SDN:L22::TOOL0020</skos:notation>
<skos:prefLabel xml:lang="en">Sea-Bird SBE 37-SIP MicroCAT C-T Sensor</skos:prefLabel>
<skos:altLabel>SBE 37-SIP MicroCAT</skos:altLabel>
<skos:definition xml:lang="en">The SBE 37 MicroCAT is a high accuracy conductivity and temperature recorder with an optional pressure sensor designed for depolyment on moorings. The SIP model has a serial interface with an internal pump to improve conductivity response and protection against fouling.</skos:definition>
<owl:versionInfo>2</owl:versionInfo>
<dc:date>2010-11-18 12:39:41.0</dc:date>
<skos:note xml:lang="en">accepted</skos:note>
<owl:deprecated>false</owl:deprecated>
<skos:broader rdf:resource="http://vocab.nerc.ac.uk/collection/L05/current/350/"/>
<skos:broader rdf:resource="http://vocab.nerc.ac.uk/collection/L05/current/134/"/>
<void:inDataset rdf:resource="http://vocab.nerc.ac.uk/.well-known/void"/>
</skos:Concept>
</skos:member>
<skos:member>
<skos:Concept rdf:about="http://vocab.nerc.ac.uk/collection/L22/current/TOOL0017/">
<dc:identifier>SDN:L22::TOOL0017</dc:identifier>
<skos:notation>SDN:L22::TOOL0017</skos:notation>
<skos:prefLabel xml:lang="en">Sea-Bird SBE 37-SM MicroCAT C-T Sensor</skos:prefLabel>
<skos:altLabel>SBE 37-SM MicroCAT</skos:altLabel>
<skos:definition xml:lang="en">The SBE 37 MicroCAT is a high accuracy conductivity and temperature recorder with an optional pressure sensor designed for depolyment on moorings. The SM model has a serial interface plus internal flash memory data storage. Further information may be found on the BODC document server at URL http://www.bodc.ac.uk/data/documents/nodb/108613/.</skos:definition>
<owl:versionInfo>2</owl:versionInfo>
<dc:date>2010-11-18 12:39:41.0</dc:date>
<skos:note xml:lang="en">accepted</skos:note>
<owl:deprecated>false</owl:deprecated>
<skos:broader rdf:resource="http://vocab.nerc.ac.uk/collection/L05/current/134/"/>
<skos:broader rdf:resource="http://vocab.nerc.ac.uk/collection/L05/current/350/"/>
<void:inDataset rdf:resource="http://vocab.nerc.ac.uk/.well-known/void"/>
</skos:Concept>
</skos:member>
<skos:member>
<skos:Concept rdf:about="http://vocab.nerc.ac.uk/collection/L22/current/TOOL0018/">
<dc:identifier>SDN:L22::TOOL0018</dc:identifier>
<skos:notation>SDN:L22::TOOL0018</skos:notation>
<skos:prefLabel xml:lang="en">Sea-Bird SBE 37-SMP MicroCAT C-T Sensor</skos:prefLabel>
<skos:altLabel>SBE 37-SMP MicroCAT</skos:altLabel>
<skos:definition xml:lang="en">The SBE 37 MicroCAT is a high accuracy conductivity and temperature recorder with an optional pressure sensor designed for depolyment on moorings. The SMP model has a serial interface plus internal flash memory data storage with an internal pump to improve conductivity response and protection against fouling.</skos:definition>
<owl:versionInfo>2</owl:versionInfo>
<dc:date>2010-11-18 12:39:41.0</dc:date>
<skos:note xml:lang="en">accepted</skos:note>
<owl:deprecated>false</owl:deprecated>
<skos:related rdf:resource="http://vocab.nerc.ac.uk/collection/P01/current/CNDCPR01/"/>
<skos:related rdf:resource="http://vocab.nerc.ac.uk/collection/P01/current/PSALPR01/"/>
<skos:related rdf:resource="http://vocab.nerc.ac.uk/collection/P01/current/TEMPPR01/"/>
<skos:broader rdf:resource="http://vocab.nerc.ac.uk/collection/L05/current/134/"/>
<skos:broader rdf:resource="http://vocab.nerc.ac.uk/collection/L05/current/350/"/>
<void:inDataset rdf:resource="http://vocab.nerc.ac.uk/.well-known/void"/>
</skos:Concept>
</skos:member>
<skos:member>
<skos:Concept rdf:about="http://vocab.nerc.ac.uk/collection/L22/current/TOOL0634/">
<dc:identifier>SDN:L22::TOOL0634</dc:identifier>
<skos:notation>SDN:L22::TOOL0634</skos:notation>
<skos:prefLabel xml:lang="en">Sea-Bird SBE 37-SMP-IDO MicroCAT C-T-DO</skos:prefLabel>
<skos:altLabel>SBE 37-SMP-IDO MicroCAT</skos:altLabel>
<skos:definition xml:lang="en">The SBE 37 MicroCAT is a high accuracy conductivity and temperature recorder with an optional pressure sensor and a membrane-type Integrated Dissolved Oxygen sensor (IDO) designed for deployment on moorings. The SMP IDO model has an internal pump to improve conductivity and oxygen response as well as protection against fouling.</skos:definition>
<owl:versionInfo>1</owl:versionInfo>
<dc:date>2013-08-07 13:36:55.0</dc:date>
<skos:note xml:lang="en">accepted</skos:note>
<owl:deprecated>false</owl:deprecated>
<skos:broader rdf:resource="http://vocab.nerc.ac.uk/collection/L05/current/134/"/>
<skos:broader rdf:resource="http://vocab.nerc.ac.uk/collection/L05/current/351/"/>
<skos:broader rdf:resource="http://vocab.nerc.ac.uk/collection/L05/current/350/"/>
<void:inDataset rdf:resource="http://vocab.nerc.ac.uk/.well-known/void"/>
</skos:Concept>
</skos:member>
<skos:member>
<skos:Concept rdf:about="http://vocab.nerc.ac.uk/collection/L22/current/TOOL0266/">
<dc:identifier>SDN:L22::TOOL0266</dc:identifier>
<skos:notation>SDN:L22::TOOL0266</skos:notation>
<skos:prefLabel xml:lang="en">Sea-Bird SBE 39 temperature recorder</skos:prefLabel>
<skos:altLabel>SBE 39 TR</skos:altLabel>
<skos:definition xml:lang="en">A high-accuracy temperature recorder (pressure optional) with internal battery and non-volatile memory for deployment at depths up to 10500 meters. It is intended for moorings or other long-term, fixed-site applications, as well as shorter-term deployments on nets, towed vehicles or ROVs. Calibration coefficients stored in EEPROM allow the SBE 39 to transmit data in engineering units. The SBE 39 thermistor has a long history of exceptional accuracy and stability (typical drift is less than 0.002C per year). The SBE 39 communicates directly with a computer via a standard RA-232 interface. For more information see http://www.bodc.ac.uk/data/documents/nodb/108627/</skos:definition>
<owl:versionInfo>1</owl:versionInfo>
<dc:date>2010-05-18 16:10:58.0</dc:date>
<skos:note xml:lang="en">accepted</skos:note>
<owl:deprecated>false</owl:deprecated>
<skos:broader rdf:resource="http://vocab.nerc.ac.uk/collection/L05/current/134/"/>
<void:inDataset rdf:resource="http://vocab.nerc.ac.uk/.well-known/void"/>
</skos:Concept>
</skos:member>
<skos:member>
<skos:Concept rdf:about="http://vocab.nerc.ac.uk/collection/L22/current/TOOL0640/">
<dc:identifier>SDN:L22::TOOL0640</dc:identifier>
<skos:notation>SDN:L22::TOOL0640</skos:notation>
<skos:prefLabel xml:lang="en">Sea-Bird SBE 3F temperature sensor</skos:prefLabel>
<skos:altLabel>SBE 3F temperature sensor</skos:altLabel>
<skos:definition xml:lang="en">Water temperature sensor primarily designed for use on the SBE 25 and 25plus Sealogger CTD systems but can be used as a component in custom oceanographic profiling systems or high-accuracy temperature-monitoring applications. The sensor operates over the range -5 to +35 degC and has an initial accuracy of +/-0.001 degC. The sensor has a depth rating of 6800 m (aluminum housing) or 10500 m (titanium housing). The SBE 3F is an enhanced version of the SBE 3 temperature sensor.</skos:definition>
<owl:versionInfo>1</owl:versionInfo>
<dc:date>2013-09-24 14:39:34.0</dc:date>
<skos:note xml:lang="en">accepted</skos:note>
<owl:deprecated>false</owl:deprecated>
<skos:broader rdf:resource="http://vocab.nerc.ac.uk/collection/L05/current/134/"/>
<void:inDataset rdf:resource="http://vocab.nerc.ac.uk/.well-known/void"/>
</skos:Concept>
</skos:member>
<skos:member>
<skos:Concept rdf:about="http://vocab.nerc.ac.uk/collection/L22/current/TOOL0036/">
<dc:identifier>SDN:L22::TOOL0036</dc:identifier>
<skos:notation>SDN:L22::TOOL0036</skos:notation>
<skos:prefLabel xml:lang="en">Sea-Bird SBE 43 Dissolved Oxygen Sensor</skos:prefLabel>
<skos:altLabel>SBE 43 DO</skos:altLabel>
<skos:definition xml:lang="en">High performance through-flow Clark polarographic membrane sensor designed to be plumbed in to a Sea-Bird underwater unit pumped water supply on a profiling CTD package. Designed specifically to give rapid temperature response and minimal pressure hysteresis. Signal output is voltage based to interface to a CTD deck unit.</skos:definition>
<owl:versionInfo>1</owl:versionInfo>
<dc:date>2009-11-30 11:56:35.0</dc:date>
<skos:note xml:lang="en">accepted</skos:note>
<owl:deprecated>false</owl:deprecated>
<skos:broader rdf:resource="http://vocab.nerc.ac.uk/collection/L05/current/351/"/>
<void:inDataset rdf:resource="http://vocab.nerc.ac.uk/.well-known/void"/>
</skos:Concept>
</skos:member>
<skos:member>
<skos:Concept rdf:about="http://vocab.nerc.ac.uk/collection/L22/current/TOOL0037/">
<dc:identifier>SDN:L22::TOOL0037</dc:identifier>
<skos:notation>SDN:L22::TOOL0037</skos:notation>
<skos:prefLabel xml:lang="en">Sea-Bird SBE 43F Dissolved Oxygen Sensor</skos:prefLabel>
<skos:altLabel>SBE 43F DO</skos:altLabel>
<skos:definition xml:lang="en">High performance through-flow Clark polarographic membrane sensor designed to be interfaced to an SBE 52-MP profiling moored CTD or integrated into OEM moorings. Designed specifically to give rapid temperature response and minimal pressure hysteresis. Signal output is frequency based.</skos:definition>
<owl:versionInfo>1</owl:versionInfo>
<dc:date>2009-11-30 11:56:35.0</dc:date>
<skos:note xml:lang="en">accepted</skos:note>
<owl:deprecated>false</owl:deprecated>
<skos:broader rdf:resource="http://vocab.nerc.ac.uk/collection/L05/current/351/"/>
<void:inDataset rdf:resource="http://vocab.nerc.ac.uk/.well-known/void"/>
</skos:Concept>
</skos:member>
<skos:member>
<skos:Concept rdf:about="http://vocab.nerc.ac.uk/collection/L22/current/TOOL0025/">
<dc:identifier>SDN:L22::TOOL0025</dc:identifier>
<skos:notation>SDN:L22::TOOL0025</skos:notation>
<skos:prefLabel xml:lang="en">Sea-Bird SBE 53 BPR Bottom Pressure Recorder</skos:prefLabel>
<skos:altLabel>SBE 53 BPR</skos:altLabel>
<skos:definition xml:lang="en">The SBE 53 BPR is a water level recorder with a Digiquartz pressure sensor, precision thermometer and optional conductivity sensor. Pressure data are integrated to give sea level free from wave interference at frequencies of a minute to an hour.</skos:definition>
<owl:versionInfo>1</owl:versionInfo>
<dc:date>2009-11-30 11:27:51.0</dc:date>
<skos:note xml:lang="en">accepted</skos:note>
<owl:deprecated>false</owl:deprecated>
<skos:related rdf:resource="http://vocab.nerc.ac.uk/collection/P01/current/PRSTPS01/"/>
<skos:related rdf:resource="http://vocab.nerc.ac.uk/collection/P01/current/TEMPPR01/"/>
<skos:related rdf:resource="http://vocab.nerc.ac.uk/collection/P01/current/PRSTRS01/"/>
<skos:related rdf:resource="http://vocab.nerc.ac.uk/collection/P01/current/PRSTDR01/"/>
<skos:broader rdf:resource="http://vocab.nerc.ac.uk/collection/L05/current/111/"/>
<skos:broader rdf:resource="http://vocab.nerc.ac.uk/collection/L05/current/134/"/>
<void:inDataset rdf:resource="http://vocab.nerc.ac.uk/.well-known/void"/>
</skos:Concept>
</skos:member>
<skos:member>
<skos:Concept rdf:about="http://vocab.nerc.ac.uk/collection/L22/current/TOOL0644/">
<dc:identifier>SDN:L22::TOOL0644</dc:identifier>
<skos:notation>SDN:L22::TOOL0644</skos:notation>
<skos:prefLabel xml:lang="en">Sea-Bird SBE 7 microstructure conductivity sensor</skos:prefLabel>
<skos:altLabel>SBE 7 microstructure conductivity sensor</skos:altLabel>
<skos:definition xml:lang="en">Microstructure conductivity sensor designed for use on marine profiling applications to characterise small scale ocean conductivity features. The sensor is primarily used for the determination of conductivity gradients but it is configured to respond to absolute conductivity as well. The SBE 7 has an accuracy typically within 0.005 S m^-1 over periods of several hours and has a high speed micro-scale resolution of 3 dbar at 100 cycles ^-1 (-3 dbar at 1000 Hz). The sensor has aluminium housing and a depth rating of 6800 m.</skos:definition>
<owl:versionInfo>1</owl:versionInfo>
<dc:date>2013-09-24 15:49:25.0</dc:date>
<skos:note xml:lang="en">accepted</skos:note>
<owl:deprecated>false</owl:deprecated>
<skos:broader rdf:resource="http://vocab.nerc.ac.uk/collection/L05/current/350/"/>
<skos:broader rdf:resource="http://vocab.nerc.ac.uk/collection/L05/current/184/"/>
<void:inDataset rdf:resource="http://vocab.nerc.ac.uk/.well-known/void"/>
</skos:Concept>
</skos:member>
<skos:member>
<skos:Concept rdf:about="http://vocab.nerc.ac.uk/collection/L22/current/TOOL0035/">
<dc:identifier>SDN:L22::TOOL0035</dc:identifier>
<skos:notation>SDN:L22::TOOL0035</skos:notation>
<skos:prefLabel xml:lang="en">Sea-Bird SBE 911 CTD</skos:prefLabel>
<skos:altLabel>SBE 911 CTD</skos:altLabel>
<skos:definition xml:lang="en">High precision and accuracy CTD made up from a Sea-Bird SBE 9 underwater unit and a SBE 11 deck unit. The underwater unit comprises protective cage (usually with a rosette) holding a pressure unit and temperature/conductivity unit. The latter is connected to a pump-fed plastic tubing circuit that may include other sensors. All plumbed and non-plumbed instruments (e.g. transmissometers and light meters) on the package are logged by the SBE 11. The unit was replaced by the SBE 911plus in 1997.</skos:definition>
<owl:versionInfo>6</owl:versionInfo>
<dc:date>2010-11-18 12:42:13.0</dc:date>
<skos:note xml:lang="en">accepted</skos:note>
<owl:deprecated>false</owl:deprecated>
<skos:related rdf:resource="http://vocab.nerc.ac.uk/collection/P01/current/SIGTPR01/"/>
<skos:related rdf:resource="http://vocab.nerc.ac.uk/collection/P01/current/POTMCV01/"/>
<skos:related rdf:resource="http://vocab.nerc.ac.uk/collection/P01/current/PRESPR01/"/>
<skos:related rdf:resource="http://vocab.nerc.ac.uk/collection/P01/current/PSALST01/"/>
<skos:related rdf:resource="http://vocab.nerc.ac.uk/collection/P01/current/TEMPST01/"/>
<skos:related rdf:resource="http://vocab.nerc.ac.uk/collection/P01/current/DOXYPR01/"/>
<skos:broader rdf:resource="http://vocab.nerc.ac.uk/collection/L05/current/350/"/>
<skos:broader rdf:resource="http://vocab.nerc.ac.uk/collection/L05/current/130/"/>
<skos:broader rdf:resource="http://vocab.nerc.ac.uk/collection/L05/current/134/"/>
<void:inDataset rdf:resource="http://vocab.nerc.ac.uk/.well-known/void"/>
</skos:Concept>
</skos:member>
<skos:member>
<skos:Concept rdf:about="http://vocab.nerc.ac.uk/collection/L22/current/TOOL0058/">
<dc:identifier>SDN:L22::TOOL0058</dc:identifier>
<skos:notation>SDN:L22::TOOL0058</skos:notation>
<skos:prefLabel xml:lang="en">Sea-Bird SBE 911plus CTD</skos:prefLabel>
<skos:altLabel>SBE 911+ CTD</skos:altLabel>
<skos:definition xml:lang="en">High precision and accuracy CTD comprising an SBE 9plus underwater unit (SBE 3 temperature and SBE 4 conductivity sensors) and an SBE 11plus deck unit. Sensors may be connected to a pump-fed plastic tubing circuit (usually temperature, salinity and oxygen) or stand-alone. All instruments (8 channels available) on the package are logged by the SBE 11. The unit is the production off the shelf version of the SBE 911 (each 911 was custom built to individual specification).</skos:definition>
<owl:versionInfo>3</owl:versionInfo>
<dc:date>2013-03-13 15:55:10.0</dc:date>
<skos:note xml:lang="en">accepted</skos:note>
<owl:deprecated>false</owl:deprecated>
<skos:related rdf:resource="http://vocab.nerc.ac.uk/collection/P01/current/DEPHPR01/"/>
<skos:related rdf:resource="http://vocab.nerc.ac.uk/collection/P01/current/PSALCC01/"/>
<skos:related rdf:resource="http://vocab.nerc.ac.uk/collection/P01/current/SIGTEQ01/"/>
<skos:related rdf:resource="http://vocab.nerc.ac.uk/collection/P01/current/TEMPCU01/"/>
<skos:related rdf:resource="http://vocab.nerc.ac.uk/collection/P01/current/TEMPCC01/"/>
<skos:related rdf:resource="http://vocab.nerc.ac.uk/collection/P01/current/TEMPST01/"/>
<skos:related rdf:resource="http://vocab.nerc.ac.uk/collection/P01/current/PRESPR01/"/>
<skos:related rdf:resource="http://vocab.nerc.ac.uk/collection/P01/current/POTMCV01/"/>
<skos:related rdf:resource="http://vocab.nerc.ac.uk/collection/P01/current/DOXYPR01/"/>
<skos:related rdf:resource="http://vocab.nerc.ac.uk/collection/P01/current/OXYSBB01/"/>
<skos:related rdf:resource="http://vocab.nerc.ac.uk/collection/P01/current/SIGTPR01/"/>
<skos:related rdf:resource="http://vocab.nerc.ac.uk/collection/P01/current/PSALPR01/"/>
<skos:related rdf:resource="http://vocab.nerc.ac.uk/collection/P01/current/PSALST01/"/>
<skos:related rdf:resource="http://vocab.nerc.ac.uk/collection/P01/current/CNDCST01/"/>
<skos:broader rdf:resource="http://vocab.nerc.ac.uk/collection/L05/current/130/"/>
<skos:broader rdf:resource="http://vocab.nerc.ac.uk/collection/L05/current/350/"/>
<skos:broader rdf:resource="http://vocab.nerc.ac.uk/collection/L05/current/134/"/>
<void:inDataset rdf:resource="http://vocab.nerc.ac.uk/.well-known/void"/>
</skos:Concept>
</skos:member>
<skos:member>
<skos:Concept rdf:about="http://vocab.nerc.ac.uk/collection/L22/current/TOOL0409/">
<dc:identifier>SDN:L22::TOOL0409</dc:identifier>
<skos:notation>SDN:L22::TOOL0409</skos:notation>
<skos:prefLabel xml:lang="en">Sea-Bird SBE 917 CTD</skos:prefLabel>
<skos:altLabel>SBE 917 CTD</skos:altLabel>
<skos:definition xml:lang="en">High precision and accuracy CTD comprising an SBE 9 underwater unit (SBE 3 temperature and SBE 4 conductivity sensors) and an SBE 17 SEARAM data logger. Sensors may be connected to a pump-fed plastic tubing circuit (usually temperature, salinity and oxygen) or stand-alone. All instruments (8 channels available) on the package are logged by the SBE 17, which provides battery power, has memory for CTD data recording, and provides autonomous carousel water sampler control.</skos:definition>
<owl:versionInfo>1</owl:versionInfo>
<dc:date>2011-07-27 13:50:44.0</dc:date>
<skos:note xml:lang="en">accepted</skos:note>
<owl:deprecated>false</owl:deprecated>
<skos:broader rdf:resource="http://vocab.nerc.ac.uk/collection/L05/current/350/"/>
<skos:broader rdf:resource="http://vocab.nerc.ac.uk/collection/L05/current/130/"/>
<skos:broader rdf:resource="http://vocab.nerc.ac.uk/collection/L05/current/134/"/>
<void:inDataset rdf:resource="http://vocab.nerc.ac.uk/.well-known/void"/>
</skos:Concept>
</skos:member>
<skos:member>
<skos:Concept rdf:about="http://vocab.nerc.ac.uk/collection/L22/current/TOOL0214/">
<dc:identifier>SDN:L22::TOOL0214</dc:identifier>
<skos:notation>SDN:L22::TOOL0214</skos:notation>
<skos:prefLabel xml:lang="en">Sea-Bird SBE 917plus CTD</skos:prefLabel>
<skos:altLabel>SBE 917+ CTD</skos:altLabel>
<skos:definition xml:lang="en">High precision and accuracy CTD comprising an SBE 9plus underwater unit (SBE 3 temperature and SBE 4 conductivity sensors) and an SBE 17plus SEARAM data logger. Sensors may be connected to a pump-fed plastic tubing circuit (usually temperature, salinity and oxygen) or stand-alone. All instruments (8 channels available) on the package are logged by the SBE 17+, which provides battery power, has memory for CTD data recording, and provides autonomous carousel water sampler control.</skos:definition>
<owl:versionInfo>3</owl:versionInfo>
<dc:date>2013-03-13 15:55:10.0</dc:date>
<skos:note xml:lang="en">accepted</skos:note>
<owl:deprecated>false</owl:deprecated>
<skos:broader rdf:resource="http://vocab.nerc.ac.uk/collection/L05/current/134/"/>
<skos:broader rdf:resource="http://vocab.nerc.ac.uk/collection/L05/current/130/"/>
<skos:broader rdf:resource="http://vocab.nerc.ac.uk/collection/L05/current/350/"/>
<void:inDataset rdf:resource="http://vocab.nerc.ac.uk/.well-known/void"/>
</skos:Concept>
</skos:member>
<skos:member>
<skos:Concept rdf:about="http://vocab.nerc.ac.uk/collection/L22/current/TOOL0318/">
<dc:identifier>SDN:L22::TOOL0318</dc:identifier>
<skos:notation>SDN:L22::TOOL0318</skos:notation>
<skos:prefLabel xml:lang="en">Sea-Bird SBE35 thermometer</skos:prefLabel>
<skos:altLabel>SBE 35</skos:altLabel>
<skos:definition xml:lang="en">An oceanographic thermometer with a measurement range of -5 to +35 deg C; an initial accuracy of 0.001 deg C; and a resolution of 0.000025 deg C. The sensor is an ultra-stable aged thermistor with a drift rate of less than 0.001deg C per year. It can be used both in fixed point cells and at depths up to 6800 metres in combination with an SBE water sampling carousel.</skos:definition>
<owl:versionInfo>3</owl:versionInfo>
<dc:date>2013-03-13 15:55:10.0</dc:date>
<skos:note xml:lang="en">accepted</skos:note>
<owl:deprecated>false</owl:deprecated>
<skos:broader rdf:resource="http://vocab.nerc.ac.uk/collection/L05/current/134/"/>
<void:inDataset rdf:resource="http://vocab.nerc.ac.uk/.well-known/void"/>
</skos:Concept>
</skos:member>
<skos:member>
<skos:Concept rdf:about="http://vocab.nerc.ac.uk/collection/L22/current/TOOL0191/">
<dc:identifier>SDN:L22::TOOL0191</dc:identifier>
<skos:notation>SDN:L22::TOOL0191</skos:notation>
<skos:prefLabel xml:lang="en">Sea-Bird SBE38 thermometer</skos:prefLabel>
<skos:altLabel>SBE 38 TS</skos:altLabel>
<skos:definition xml:lang="en">An oceanographic thermometer with a measurement range of -5 to +35C; absolute accuracy better than 0.001C and resolution of approximately 0.00025C. The sensor is an ultra-stable aged thermistor with a drift rate of less than 0.002C per year. The reference resistor is a hermetically sealed VISHAY. It may be fitted in a 10,500m titanium pressure housing.</skos:definition>
<owl:versionInfo>2</owl:versionInfo>
<dc:date>2013-03-13 15:55:10.0</dc:date>
<skos:note xml:lang="en">accepted</skos:note>
<owl:deprecated>false</owl:deprecated>
<skos:broader rdf:resource="http://vocab.nerc.ac.uk/collection/L05/current/134/"/>
<void:inDataset rdf:resource="http://vocab.nerc.ac.uk/.well-known/void"/>
</skos:Concept>
</skos:member>
<skos:member>
<skos:Concept rdf:about="http://vocab.nerc.ac.uk/collection/L22/current/TOOL0416/">
<dc:identifier>SDN:L22::TOOL0416</dc:identifier>
<skos:notation>SDN:L22::TOOL0416</skos:notation>
<skos:prefLabel xml:lang="en">Sea-Bird SBE3plus (SBE 3P) temperature sensor</skos:prefLabel>
<skos:altLabel>SBE 3P temperature sensor</skos:altLabel>
<skos:definition xml:lang="en">Water temperature sensor designed for use on the SBE 9plus CTD system. The sensor operates over the range -5 to +35 °C, a resolution of 0.0003 °C at 24 Hz and an initial accuracy of ± 0.001 °C. The typical sampling rate is 24 Hz, and the sensor has a depth rating of 6800 meters (aluminum housing) or 10500 meters (titanium housing).</skos:definition>
<owl:versionInfo>2</owl:versionInfo>
<dc:date>2013-03-13 15:55:10.0</dc:date>
<skos:note xml:lang="en">accepted</skos:note>
<owl:deprecated>false</owl:deprecated>
<skos:related rdf:resource="http://vocab.nerc.ac.uk/collection/P01/current/TEMPCU01/"/>
<skos:related rdf:resource="http://vocab.nerc.ac.uk/collection/P01/current/TEMPCC01/"/>
<skos:broader rdf:resource="http://vocab.nerc.ac.uk/collection/L05/current/134/"/>
<void:inDataset rdf:resource="http://vocab.nerc.ac.uk/.well-known/void"/>
</skos:Concept>
</skos:member>
<skos:member>
<skos:Concept rdf:about="http://vocab.nerc.ac.uk/collection/L22/current/TOOL0190/">
<dc:identifier>SDN:L22::TOOL0190</dc:identifier>
<skos:notation>SDN:L22::TOOL0190</skos:notation>
<skos:prefLabel xml:lang="en">Sea-Bird SBE45 MicroTSG thermosalinograph</skos:prefLabel>
<skos:altLabel>SBE 45 MicroTSG</skos:altLabel>
<skos:definition xml:lang="en">A small externally powered, high-accuracy instrument, designed for shipboard determination of sea surface (pumped-water) conductivity and temperature. It is constructed of plastic and titanium to ensure long life with minimum maintenance. It may optionally be interfaced to an external SBE 38 hull temperature sensor.</skos:definition>
<owl:versionInfo>2</owl:versionInfo>
<dc:date>2013-03-13 15:55:10.0</dc:date>
<skos:note xml:lang="en">accepted</skos:note>
<owl:deprecated>false</owl:deprecated>
<skos:broader rdf:resource="http://vocab.nerc.ac.uk/collection/L05/current/133/"/>
<skos:broader rdf:resource="http://vocab.nerc.ac.uk/collection/L05/current/350/"/>
<skos:broader rdf:resource="http://vocab.nerc.ac.uk/collection/L05/current/134/"/>
<void:inDataset rdf:resource="http://vocab.nerc.ac.uk/.well-known/void"/>
</skos:Concept>
</skos:member>
<skos:member>
<skos:Concept rdf:about="http://vocab.nerc.ac.uk/collection/L22/current/TOOL0417/">
<dc:identifier>SDN:L22::TOOL0417</dc:identifier>
<skos:notation>SDN:L22::TOOL0417</skos:notation>
<skos:prefLabel xml:lang="en">Sea-Bird SBE4C conductivity sensor</skos:prefLabel>
<skos:altLabel>SBE 4C conductivity sensor</skos:altLabel>
<skos:definition xml:lang="en">Water conductivity sensor designed for use on the SBE 9plus or SBE 25 CTD system. The sensor operates over the range 0 to 7 S/m, with a resolution of 0.00004 S/m at 24 Hz and an initial accuracy of 0.0003 S/m. The typical sampling rate is 24 Hz, and the sensor has a depth rating of 3400 meters or 6800 meters (aluminum housing), or 10500 meters (titanium housing).</skos:definition>
<owl:versionInfo>5</owl:versionInfo>
<dc:date>2013-10-11 13:38:02.0</dc:date>
<skos:note xml:lang="en">accepted</skos:note>
<owl:deprecated>false</owl:deprecated>
<skos:related rdf:resource="http://vocab.nerc.ac.uk/collection/P01/current/CNDCST01/"/>
<skos:related rdf:resource="http://vocab.nerc.ac.uk/collection/P01/current/PSALCC01/"/>
<skos:broader rdf:resource="http://vocab.nerc.ac.uk/collection/L05/current/350/"/>
<void:inDataset rdf:resource="http://vocab.nerc.ac.uk/.well-known/void"/>
</skos:Concept>
</skos:member>
<skos:member>
<skos:Concept rdf:about="http://vocab.nerc.ac.uk/collection/L22/current/TOOL0637/">
<dc:identifier>SDN:L22::TOOL0637</dc:identifier>
<skos:notation>SDN:L22::TOOL0637</skos:notation>
<skos:prefLabel xml:lang="en">SeaTech 57S fluorometer</skos:prefLabel>
<skos:altLabel>SeaTech 57S fluorometer</skos:altLabel>
<skos:definition xml:lang="en">A linear-response submersible chlorophyll-a fluorometer fitted to CTD packages in the early 1990s.</skos:definition>
<owl:versionInfo>2</owl:versionInfo>
<dc:date>2013-08-22 15:37:19.0</dc:date>
<skos:note xml:lang="en">accepted</skos:note>
<owl:deprecated>false</owl:deprecated>
<skos:related rdf:resource="http://vocab.nerc.ac.uk/collection/P01/current/CPHLPR01/"/>
<skos:broader rdf:resource="http://vocab.nerc.ac.uk/collection/L05/current/113/"/>
<void:inDataset rdf:resource="http://vocab.nerc.ac.uk/.well-known/void"/>
</skos:Concept>
</skos:member>
<skos:member>
<skos:Concept rdf:about="http://vocab.nerc.ac.uk/collection/L22/current/TOOL0426/">
<dc:identifier>SDN:L22::TOOL0426</dc:identifier>
<skos:notation>SDN:L22::TOOL0426</skos:notation>
<skos:prefLabel xml:lang="en">SeaTech Light Back-Scattering Sensor</skos:prefLabel>
<skos:altLabel>SeaTech LBSS</skos:altLabel>
<skos:definition xml:lang="en">The instrument projects light into the sample volume using two modulated 880 nm Light Emitting Diodes. Light back-scattered from the suspended particles inthe water column is measured with a solar-blind silicon detector. A light stop between the light source and the light detector prevents the measurement of direct transmitted light so that only back-scattered light from suspended particles in water are measured. The instrument is no longer manufactured and no source of support is known.</skos:definition>
<owl:versionInfo>1</owl:versionInfo>
<dc:date>2011-09-26 11:52:17.0</dc:date>
<skos:note xml:lang="en">accepted</skos:note>
<owl:deprecated>false</owl:deprecated>
<skos:broader rdf:resource="http://vocab.nerc.ac.uk/collection/L05/current/123/"/>
<void:inDataset rdf:resource="http://vocab.nerc.ac.uk/.well-known/void"/>
</skos:Concept>
</skos:member>
<skos:member>
<skos:Concept rdf:about="http://vocab.nerc.ac.uk/collection/L22/current/TOOL0187/">
<dc:identifier>SDN:L22::TOOL0187</dc:identifier>
<skos:notation>SDN:L22::TOOL0187</skos:notation>
<skos:prefLabel xml:lang="en">SeaTech S131 fluorometer</skos:prefLabel>
<skos:altLabel>SeaTech S131 fluorometer</skos:altLabel>
<skos:definition xml:lang="en">A chlorophyll-a fluorometer with six internally selectable ranges, permitting measurement of chlorophyll-a permitting measurement of chlorophyll-a concentrations from approximately 0.015ug/l to 1000ug/l.</skos:definition>
<owl:versionInfo>1</owl:versionInfo>
<dc:date>2010-05-18 16:10:58.0</dc:date>
<skos:note xml:lang="en">accepted</skos:note>
<owl:deprecated>false</owl:deprecated>
<skos:related rdf:resource="http://vocab.nerc.ac.uk/collection/P01/current/FVLTWS01/"/>
<skos:related rdf:resource="http://vocab.nerc.ac.uk/collection/P01/current/CPHLPR01/"/>
<skos:broader rdf:resource="http://vocab.nerc.ac.uk/collection/L05/current/113/"/>
<void:inDataset rdf:resource="http://vocab.nerc.ac.uk/.well-known/void"/>
</skos:Concept>
</skos:member>
<skos:member>
<skos:Concept rdf:about="http://vocab.nerc.ac.uk/collection/L22/current/TOOL0003/">
<dc:identifier>SDN:L22::TOOL0003</dc:identifier>
<skos:notation>SDN:L22::TOOL0003</skos:notation>
<skos:prefLabel xml:lang="en">SeaTech transmissometer</skos:prefLabel>
<skos:altLabel>SeaTech transmissometer</skos:altLabel>
<skos:definition xml:lang="en">SeaTech manufactured a range of transmissometers to measure optical attenuance, usually (but not exclusively) at red (660nm) light wavelengths. Path lengths varied from 5cm for use in turbid waters to 1m for use in the clear deep ocean. The instruments are no longer manufactured and no source of support is known.</skos:definition>
<owl:versionInfo>2</owl:versionInfo>
<dc:date>2010-11-18 12:39:41.0</dc:date>
<skos:note xml:lang="en">accepted</skos:note>
<owl:deprecated>false</owl:deprecated>
<skos:related rdf:resource="http://vocab.nerc.ac.uk/collection/P01/current/OSEDTR01/"/>
<skos:related rdf:resource="http://vocab.nerc.ac.uk/collection/P01/current/ATTNZR02/"/>
<skos:related rdf:resource="http://vocab.nerc.ac.uk/collection/P01/current/NVLTST01/"/>
<skos:related rdf:resource="http://vocab.nerc.ac.uk/collection/P01/current/TVLTZZ01/"/>
<skos:related rdf:resource="http://vocab.nerc.ac.uk/collection/P01/current/TVLTZR01/"/>
<skos:related rdf:resource="http://vocab.nerc.ac.uk/collection/P01/current/PPOPPR01/"/>
<skos:related rdf:resource="http://vocab.nerc.ac.uk/collection/P01/current/ATTNMR01/"/>
<skos:related rdf:resource="http://vocab.nerc.ac.uk/collection/P01/current/TSEDTR01/"/>
<skos:related rdf:resource="http://vocab.nerc.ac.uk/collection/P01/current/POATCV01/"/>
<skos:related rdf:resource="http://vocab.nerc.ac.uk/collection/P01/current/ATTNZR01/"/>
<skos:related rdf:resource="http://vocab.nerc.ac.uk/collection/P01/current/POPTDR01/"/>
<skos:related rdf:resource="http://vocab.nerc.ac.uk/collection/P01/current/POPTPR01/"/>
<skos:related rdf:resource="http://vocab.nerc.ac.uk/collection/P01/current/ISEDTR01/"/>
<skos:broader rdf:resource="http://vocab.nerc.ac.uk/collection/L05/current/124/"/>
<void:inDataset rdf:resource="http://vocab.nerc.ac.uk/.well-known/void"/>
</skos:Concept>
</skos:member>
<skos:member>
<skos:Concept rdf:about="http://vocab.nerc.ac.uk/collection/L22/current/TOOL0664/">
<dc:identifier>SDN:L22::TOOL0664</dc:identifier>
<skos:notation>SDN:L22::TOOL0664</skos:notation>
<skos:prefLabel xml:lang="en">Seapoint Fluorescein Fluorometer</skos:prefLabel>
<skos:altLabel>Seapoint SFF</skos:altLabel>
<skos:definition xml:lang="en">A low power fluorometer for in-situ measurements of fluorescein dye, at concentrations as low as 0.02 ug/L, and at depths to 6000 metres. May be used open in-situ, or with a pump through sample volume. Output voltage is proportional to fluorescein concentration.</skos:definition>
<owl:versionInfo>1</owl:versionInfo>
<dc:date>2014-02-14 10:44:00.0</dc:date>
<skos:note xml:lang="en">accepted</skos:note>
<owl:deprecated>false</owl:deprecated>
<skos:broader rdf:resource="http://vocab.nerc.ac.uk/collection/L05/current/113/"/>
<void:inDataset rdf:resource="http://vocab.nerc.ac.uk/.well-known/void"/>
</skos:Concept>
</skos:member>
<skos:member>
<skos:Concept rdf:about="http://vocab.nerc.ac.uk/collection/L22/current/TOOL0104/">
<dc:identifier>SDN:L22::TOOL0104</dc:identifier>
<skos:notation>SDN:L22::TOOL0104</skos:notation>
<skos:prefLabel xml:lang="en">Seapoint Turbidity Meter</skos:prefLabel>
<skos:altLabel>Seapoint Turbidity Meter</skos:altLabel>
<skos:definition xml:lang="en">A turbidity meter that detects light scattered by particles suspended in water and generates an output voltage proportional to the SPM concentration. Range is selected by two digital lines which can be hard wired or microprocessor controlled, thereby choosing the appropriate range and resolution for measurement of extremely clean to very turbid waters. The offset voltage is within 1 mV of zero and requires no adjustment across gains. The optical design confines the sensing volume to within 5 cm of the sensor allowing near-bottom measurements and minimizing errant reflections in restricted spaces. Further information may be found on the BODC document server at URL: http://www.bodc.ac.uk/data/documents/nodb/119173/</skos:definition>
<owl:versionInfo>1</owl:versionInfo>
<dc:date>2010-05-18 16:10:58.0</dc:date>
<skos:note xml:lang="en">accepted</skos:note>
<owl:deprecated>false</owl:deprecated>
<skos:broader rdf:resource="http://vocab.nerc.ac.uk/collection/L05/current/123/"/>
<void:inDataset rdf:resource="http://vocab.nerc.ac.uk/.well-known/void"/>
</skos:Concept>
</skos:member>
<skos:member>
<skos:Concept rdf:about="http://vocab.nerc.ac.uk/collection/L22/current/TOOL0119/">
<dc:identifier>SDN:L22::TOOL0119</dc:identifier>
<skos:notation>SDN:L22::TOOL0119</skos:notation>
<skos:prefLabel xml:lang="en">Seapoint chlorophyll fluorometer</skos:prefLabel>
<skos:altLabel>Seapoint SCF</skos:altLabel>
<skos:definition xml:lang="en">A high-performance, low power fluorometer for in-situ measurements of chlorophyll-a able to operate at depths of up to 6000 metres. May be used open in-situ or with a pump through sample volume. Internal circuitry gives an output voltage that is proportional to chlorophyll-a concentration.</skos:definition>
<owl:versionInfo>1</owl:versionInfo>
<dc:date>2010-05-18 16:10:58.0</dc:date>
<skos:note xml:lang="en">accepted</skos:note>
<owl:deprecated>false</owl:deprecated>
<skos:related rdf:resource="http://vocab.nerc.ac.uk/collection/P01/current/FVLTWS01/"/>
<skos:related rdf:resource="http://vocab.nerc.ac.uk/collection/P01/current/CPHLPR01/"/>
<skos:broader rdf:resource="http://vocab.nerc.ac.uk/collection/L05/current/113/"/>
<void:inDataset rdf:resource="http://vocab.nerc.ac.uk/.well-known/void"/>
</skos:Concept>
</skos:member>
<skos:member>
<skos:Concept rdf:about="http://vocab.nerc.ac.uk/collection/L22/current/TOOL0430/">
<dc:identifier>SDN:L22::TOOL0430</dc:identifier>
<skos:notation>SDN:L22::TOOL0430</skos:notation>
<skos:prefLabel xml:lang="en">Secchi disk</skos:prefLabel>
<skos:altLabel>Secchi disk</skos:altLabel>
<skos:definition xml:lang="en">A circular disk, typically 20cm in diameter, used to measure water transparency. For marine applications, the disk is usually entirely white, while for limnological studies it is common to use one with alternating black and white quadrants. The reasons for this may be historical rather thah theoretical. A black Secchi disk has recently been developed for use in shallow rivers and streams. The disk is lowered slowly into the water on a pole or line until it can no longer be seen by the observer. The depth of disappearance provides an estimate of the transparency of the water, although any reading is affected by the observer's eyesight and ambient light conditions.</skos:definition>
<owl:versionInfo>1</owl:versionInfo>
<dc:date>2011-11-02 11:37:25.0</dc:date>
<skos:note xml:lang="en">accepted</skos:note>
<owl:deprecated>false</owl:deprecated>
<skos:broader rdf:resource="http://vocab.nerc.ac.uk/collection/L05/current/124/"/>
<void:inDataset rdf:resource="http://vocab.nerc.ac.uk/.well-known/void"/>
</skos:Concept>
</skos:member>
<skos:member>
<skos:Concept rdf:about="http://vocab.nerc.ac.uk/collection/L22/current/TOOL0596/">
<dc:identifier>SDN:L22::TOOL0596</dc:identifier>
<skos:notation>SDN:L22::TOOL0596</skos:notation>
<skos:prefLabel xml:lang="en">Sediment Transport and Boundary Layer Equipment Mark II</skos:prefLabel>
<skos:altLabel>STABLE2</skos:altLabel>
<skos:definition xml:lang="en">A pop-up benthic lander with four Savonius rotor current sensors between 0.2 and 2 metres above the bed, a current vane and compass for current direction, a digiquartz pressure sensor and a data logger with an integral temperature sensor. Further information may be found in http://www.bodc.ac.uk/data/documents/nodb/68616/</skos:definition>
<owl:versionInfo>1</owl:versionInfo>
<dc:date>2013-01-31 15:12:27.0</dc:date>
<skos:note xml:lang="en">accepted</skos:note>
<owl:deprecated>false</owl:deprecated>
<skos:broader rdf:resource="http://vocab.nerc.ac.uk/collection/L05/current/115/"/>
<skos:broader rdf:resource="http://vocab.nerc.ac.uk/collection/L05/current/134/"/>
<skos:broader rdf:resource="http://vocab.nerc.ac.uk/collection/L05/current/111/"/>
<void:inDataset rdf:resource="http://vocab.nerc.ac.uk/.well-known/void"/>
</skos:Concept>
</skos:member>
<skos:member>
<skos:Concept rdf:about="http://vocab.nerc.ac.uk/collection/L22/current/TOOL0044/">
<dc:identifier>SDN:L22::TOOL0044</dc:identifier>
<skos:notation>SDN:L22::TOOL0044</skos:notation>
<skos:prefLabel xml:lang="en">Sequoia Laser In-Situ Sediment Size Transmissometer</skos:prefLabel>
<skos:altLabel>LISST</skos:altLabel>
<skos:definition xml:lang="en">A self-contained unit which measures the scattering of LASER light at a number of angles. This primary measurement is mathematically inverted to give a grain size distribution, and also scaled to obtain the volume scattering function. The size distribution is presented as concentration in each of the grain-size class bins. Optical transmission, water depth and temperature are recorded as supporting measurements.</skos:definition>
<owl:versionInfo>1</owl:versionInfo>
<dc:date>2009-11-30 11:56:35.0</dc:date>
<skos:note xml:lang="en">accepted</skos:note>
<owl:deprecated>false</owl:deprecated>
<skos:broader rdf:resource="http://vocab.nerc.ac.uk/collection/L05/current/124/"/>
<skos:broader rdf:resource="http://vocab.nerc.ac.uk/collection/L05/current/134/"/>
<skos:broader rdf:resource="http://vocab.nerc.ac.uk/collection/L05/current/150/"/>
<void:inDataset rdf:resource="http://vocab.nerc.ac.uk/.well-known/void"/>
</skos:Concept>
</skos:member>
<skos:member>
<skos:Concept rdf:about="http://vocab.nerc.ac.uk/collection/L22/current/TOOL0441/">
<dc:identifier>SDN:L22::TOOL0441</dc:identifier>
<skos:notation>SDN:L22::TOOL0441</skos:notation>
<skos:prefLabel xml:lang="en">Sequoia Laser In-Situ Sediment Size Transmissometer model 100-B</skos:prefLabel>
<skos:altLabel>LISST 100-B</skos:altLabel>
<skos:definition xml:lang="en">A self-contained unit which measures the scattering of LASER light at a number of angles. This primary measurement is mathematically inverted to give a grain size distribution, and also scaled to obtain the volume scattering function. The size distribution is presented as concentration in each of the grain-size class bins. The instrument has an optical path length of 5cm as standard (2.5cm optional) and measures particles over the size range 1.2 - 250um in 32 log-spaced size classes. The standard maximum sampling speed is 4 size distributions per second and the instrument has a depth rating of 300m. Optical transmission, water depth and temperature are recorded as supporting measurements.</skos:definition>
<owl:versionInfo>1</owl:versionInfo>
<dc:date>2011-11-16 08:14:57.0</dc:date>
<skos:note xml:lang="en">accepted</skos:note>
<owl:deprecated>false</owl:deprecated>
<skos:broader rdf:resource="http://vocab.nerc.ac.uk/collection/L05/current/134/"/>
<skos:broader rdf:resource="http://vocab.nerc.ac.uk/collection/L05/current/124/"/>
<skos:broader rdf:resource="http://vocab.nerc.ac.uk/collection/L05/current/150/"/>
<void:inDataset rdf:resource="http://vocab.nerc.ac.uk/.well-known/void"/>
</skos:Concept>
</skos:member>
<skos:member>
<skos:Concept rdf:about="http://vocab.nerc.ac.uk/collection/L22/current/TOOL0222/">
<dc:identifier>SDN:L22::TOOL0222</dc:identifier>
<skos:notation>SDN:L22::TOOL0222</skos:notation>
<skos:prefLabel xml:lang="en">Setra CS100 barometer</skos:prefLabel>
<skos:altLabel>CS100 barometer</skos:altLabel>
<skos:definition xml:lang="en">A barometer based on a capacitive pressure transducer measuring pressure in the 600 to 1100 mB range. Accuracy is +-0.5 mB at 20C and +-1 mB over the range 0-40C. Marketed by Campbell Scientific.</skos:definition>
<owl:versionInfo>1</owl:versionInfo>
<dc:date>2010-05-18 16:10:58.0</dc:date>
<skos:note xml:lang="en">accepted</skos:note>
<owl:deprecated>false</owl:deprecated>
<skos:broader rdf:resource="http://vocab.nerc.ac.uk/collection/L05/current/102/"/>
<void:inDataset rdf:resource="http://vocab.nerc.ac.uk/.well-known/void"/>
</skos:Concept>
</skos:member>
<skos:member>
<skos:Concept rdf:about="http://vocab.nerc.ac.uk/collection/L22/current/TOOL0239/">
<dc:identifier>SDN:L22::TOOL0239</dc:identifier>
<skos:notation>SDN:L22::TOOL0239</skos:notation>
<skos:prefLabel xml:lang="en">SiS RTM 4002 X digital reversing thermometer</skos:prefLabel>
<skos:altLabel>SiS RTM 4002 X</skos:altLabel>
<skos:definition xml:lang="en">A second-generation digital thermometer that collects a burst of temperature readings when inverted. It has a range of -2C to 40C, a resolution of 0.0001C below 10C (0.001C above 10C) and an accuracy of 0.003C. A glass-titanium housing with double o-ring seals of similar physical dimensions to an Hg-in-glass instrument gives an operating depth of 10000m.</skos:definition>
<owl:versionInfo>1</owl:versionInfo>
<dc:date>2010-05-18 16:10:58.0</dc:date>
<skos:note xml:lang="en">accepted</skos:note>
<owl:deprecated>false</owl:deprecated>
<skos:broader rdf:resource="http://vocab.nerc.ac.uk/collection/L05/current/134/"/>
<void:inDataset rdf:resource="http://vocab.nerc.ac.uk/.well-known/void"/>
</skos:Concept>
</skos:member>
<skos:member>
<skos:Concept rdf:about="http://vocab.nerc.ac.uk/collection/L22/current/TOOL0130/">
<dc:identifier>SDN:L22::TOOL0130</dc:identifier>
<skos:notation>SDN:L22::TOOL0130</skos:notation>
<skos:prefLabel xml:lang="en">Simrad EA500 echosounder</skos:prefLabel>
<skos:altLabel>EA500 echosounder</skos:altLabel>
<skos:definition xml:lang="en">A single-beam, single-frequency (12kHz) deep water echosounder, with a maximum power of 2kW, 160dB dynamic range and Transducer 12-16-60 (16 degree circular, 60 degree passive beams). It was introduced in June 1989 and and replaced by the EA 600 in 2000.</skos:definition>
<owl:versionInfo>1</owl:versionInfo>
<dc:date>2010-05-18 16:10:58.0</dc:date>
<skos:note xml:lang="en">accepted</skos:note>
<owl:deprecated>false</owl:deprecated>
<skos:related rdf:resource="http://vocab.nerc.ac.uk/collection/P01/current/MBANCT01/"/>
<skos:broader rdf:resource="http://vocab.nerc.ac.uk/collection/L05/current/156/"/>
<void:inDataset rdf:resource="http://vocab.nerc.ac.uk/.well-known/void"/>
</skos:Concept>
</skos:member>
<skos:member>
<skos:Concept rdf:about="http://vocab.nerc.ac.uk/collection/L22/current/TOOL0198/">
<dc:identifier>SDN:L22::TOOL0198</dc:identifier>
<skos:notation>SDN:L22::TOOL0198</skos:notation>
<skos:prefLabel xml:lang="en">Simrad EK-60 echosounder</skos:prefLabel>
<skos:altLabel>Simrad EK-60 echosounder</skos:altLabel>
<skos:definition xml:lang="en">A split-beam scientific echosounder primarily designed for fisheries research. It can operate seven frequencies simultaneously ranging from 18 to 710 kHz. Real time echo integration and target strength analysis in an unlimited number of layers is provided as well as storage of raw data for replay or analysis in one of several post-processing software packages such as Simrad's BI60.</skos:definition>
<owl:versionInfo>1</owl:versionInfo>
<dc:date>2010-05-18 16:10:58.0</dc:date>
<skos:note xml:lang="en">accepted</skos:note>
<owl:deprecated>false</owl:deprecated>
<skos:broader rdf:resource="http://vocab.nerc.ac.uk/collection/L05/current/FFES/"/>
<void:inDataset rdf:resource="http://vocab.nerc.ac.uk/.well-known/void"/>
</skos:Concept>
</skos:member>
<skos:member>
<skos:Concept rdf:about="http://vocab.nerc.ac.uk/collection/L22/current/TOOL0131/">
<dc:identifier>SDN:L22::TOOL0131</dc:identifier>
<skos:notation>SDN:L22::TOOL0131</skos:notation>
<skos:prefLabel xml:lang="en">Simrad EM12 S-120 multibeam echosounder</skos:prefLabel>
<skos:altLabel>EM12 S-120 echosounder</skos:altLabel>
<skos:definition xml:lang="en">A low frequency (13 kHz) multibeam echo sounder with full ocean depth capability. The angular coverage is 120 degrees with a swath width of 3.5 times depth. It was introduced in 1989 replaced by the EM120 in 2000.</skos:definition>
<owl:versionInfo>1</owl:versionInfo>
<dc:date>2010-05-18 16:10:58.0</dc:date>
<skos:note xml:lang="en">accepted</skos:note>
<owl:deprecated>false</owl:deprecated>
<skos:broader rdf:resource="http://vocab.nerc.ac.uk/collection/L05/current/157/"/>
<void:inDataset rdf:resource="http://vocab.nerc.ac.uk/.well-known/void"/>
</skos:Concept>
</skos:member>
<skos:member>
<skos:Concept rdf:about="http://vocab.nerc.ac.uk/collection/L22/current/TOOL0394/">
<dc:identifier>SDN:L22::TOOL0394</dc:identifier>
<skos:notation>SDN:L22::TOOL0394</skos:notation>
<skos:prefLabel xml:lang="en">Simrad EM12D multibeam echosounder</skos:prefLabel>
<skos:altLabel>EM12D echosounder</skos:altLabel>
<skos:definition xml:lang="en">A low frequency (13 kHz) multibeam echo sounder with a depth capability of approximately 2000 m. The EM12D is a dual version of the EM12S, with 162 beams instead of the 81 used by the EM12S. The angular coverage is variable from 98 deg, with a swath width of 2.3 times depth,  to 150 deg, with a swath width of 7.4 times depth. The EM12 series of echosounders was replaced by the EM120 in 2000.</skos:definition>
<owl:versionInfo>1</owl:versionInfo>
<dc:date>2011-04-14 09:29:16.0</dc:date>
<skos:note xml:lang="en">accepted</skos:note>
<owl:deprecated>false</owl:deprecated>
<skos:broader rdf:resource="http://vocab.nerc.ac.uk/collection/L05/current/157/"/>
<void:inDataset rdf:resource="http://vocab.nerc.ac.uk/.well-known/void"/>
</skos:Concept>
</skos:member>
<skos:member>
<skos:Concept rdf:about="http://vocab.nerc.ac.uk/collection/L22/current/TOOL0245/">
<dc:identifier>SDN:L22::TOOL0245</dc:identifier>
<skos:notation>SDN:L22::TOOL0245</skos:notation>
<skos:prefLabel xml:lang="en">Skalar SAN+ System colorimetric autoanalyser</skos:prefLabel>
<skos:altLabel>Skalar SAN+ AA</skos:altLabel>
<skos:definition xml:lang="en">A continuous flow analyser designed for laboratory use capable of simultaneous determination of up to 16 analystical measurements on a sample. It may be used to measure nutrient concentrations in seawater. The instrument is also known as the Skalar SAN++.</skos:definition>
<owl:versionInfo>4</owl:versionInfo>
<dc:date>2012-11-06 15:30:27.0</dc:date>
<skos:note xml:lang="en">accepted</skos:note>
<owl:deprecated>false</owl:deprecated>
<skos:broader rdf:resource="http://vocab.nerc.ac.uk/collection/L05/current/LAB03/"/>
<skos:broader rdf:resource="http://vocab.nerc.ac.uk/collection/L05/current/LAB04/"/>
<void:inDataset rdf:resource="http://vocab.nerc.ac.uk/.well-known/void"/>
</skos:Concept>
</skos:member>
<skos:member>
<skos:Concept rdf:about="http://vocab.nerc.ac.uk/collection/L22/current/TOOL0479/">
<dc:identifier>SDN:L22::TOOL0479</dc:identifier>
<skos:notation>SDN:L22::TOOL0479</skos:notation>
<skos:prefLabel xml:lang="en">Skye High Output Silicon Cell Pyranometer Sensor SKL 2650</skos:prefLabel>
<skos:altLabel>Skye SKL 2650 Pyranometer</skos:altLabel>
<skos:definition xml:lang="en">A cosine corrected silicon cell pyranometer designed for measurement of solar irradiance in outdoor locations. It operates over the range 350-1100 nm and provides excellent linearity, with a maximum of 1% deviation up to levels beyond 3000 W/m^2. The sensor is calibrated against precision reference thermopile pyranometers in natural light conditions.</skos:definition>
<owl:versionInfo>1</owl:versionInfo>
<dc:date>2012-03-15 11:46:48.0</dc:date>
<skos:note xml:lang="en">accepted</skos:note>
<owl:deprecated>false</owl:deprecated>
<skos:broader rdf:resource="http://vocab.nerc.ac.uk/collection/L05/current/122/"/>
<void:inDataset rdf:resource="http://vocab.nerc.ac.uk/.well-known/void"/>
</skos:Concept>
</skos:member>
<skos:member>
<skos:Concept rdf:about="http://vocab.nerc.ac.uk/collection/L22/current/TOOL0411/">
<dc:identifier>SDN:L22::TOOL0411</dc:identifier>
<skos:notation>SDN:L22::TOOL0411</skos:notation>
<skos:prefLabel xml:lang="en">Skye Instruments SKE510 PAR energy sensor</skos:prefLabel>
<skos:altLabel>Skye SKE510 PAR sensor</skos:altLabel>
<skos:definition xml:lang="en">A PAR energy sensor suitable for atmospheric or very shallow water applications (it is fully waterproof and guaranteed submersible to 4 m depth). It has a cosine-corrected head and a square spectral response over the range 400-700 nm. The instrument uses an optical glass filter and a blue-enhanced planar diffused silicon detector to measure PAR energy from 0-5000 W/m^2. It has a response time of 10 ns and a typical absolute calibration error of &lt;3%.</skos:definition>
<owl:versionInfo>1</owl:versionInfo>
<dc:date>2011-08-01 09:25:01.0</dc:date>
<skos:note xml:lang="en">accepted</skos:note>
<owl:deprecated>false</owl:deprecated>
<skos:broader rdf:resource="http://vocab.nerc.ac.uk/collection/L05/current/122/"/>
<void:inDataset rdf:resource="http://vocab.nerc.ac.uk/.well-known/void"/>
</skos:Concept>
</skos:member>
<skos:member>
<skos:Concept rdf:about="http://vocab.nerc.ac.uk/collection/L22/current/TOOL0194/">
<dc:identifier>SDN:L22::TOOL0194</dc:identifier>
<skos:notation>SDN:L22::TOOL0194</skos:notation>
<skos:prefLabel xml:lang="en">Skye Instruments SKS1110 pyranometer</skos:prefLabel>
<skos:altLabel>Skye SKS1110 pyranometer</skos:altLabel>
<skos:definition xml:lang="en">A silicon cell pyranometer for measurement of sunlight in outdoor locations with sensors are calibrated against precision reference thermopile pyranometers in natural light conditions.</skos:definition>
<owl:versionInfo>1</owl:versionInfo>
<dc:date>2010-05-18 16:10:58.0</dc:date>
<skos:note xml:lang="en">accepted</skos:note>
<owl:deprecated>false</owl:deprecated>
<skos:broader rdf:resource="http://vocab.nerc.ac.uk/collection/L05/current/122/"/>
<void:inDataset rdf:resource="http://vocab.nerc.ac.uk/.well-known/void"/>
</skos:Concept>
</skos:member>
<skos:member>
<skos:Concept rdf:about="http://vocab.nerc.ac.uk/collection/L22/current/TOOL0645/">
<dc:identifier>SDN:L22::TOOL0645</dc:identifier>
<skos:notation>SDN:L22::TOOL0645</skos:notation>
<skos:prefLabel xml:lang="en">Skye SKP215 Quantum Sensor</skos:prefLabel>
<skos:altLabel>SKP215 Quantum Sensor</skos:altLabel>
<skos:definition xml:lang="en">A meteorological radiometer with a blue-enhanced silicon photocell and a cosine corrected head that measures Photosynthetically Active Radiation (PAR) between 400 and 700 nm.</skos:definition>
<owl:versionInfo>1</owl:versionInfo>
<dc:date>2013-09-30 14:17:19.0</dc:date>
<skos:note xml:lang="en">accepted</skos:note>
<owl:deprecated>false</owl:deprecated>
<skos:broader rdf:resource="http://vocab.nerc.ac.uk/collection/L05/current/122/"/>
<void:inDataset rdf:resource="http://vocab.nerc.ac.uk/.well-known/void"/>
</skos:Concept>
</skos:member>
<skos:member>
<skos:Concept rdf:about="http://vocab.nerc.ac.uk/collection/L22/current/NETT0139/">
<dc:identifier>SDN:L22::NETT0139</dc:identifier>
<skos:notation>SDN:L22::NETT0139</skos:notation>
<skos:prefLabel xml:lang="en">Small plankton sampler - Glover (1953)</skos:prefLabel>
<skos:altLabel>Glover plankton sampler</skos:altLabel>
<skos:definition xml:lang="en">This is a small high-speed sampler (similar to the Hardy Standard Plankton Indicator and the Miniature Plankton Indicator) with a 1.9 cm diameter aperture opening, 3.2 cm diameter internal net and 8.9 cm long, and a 30.5 cm overall length [Wiebe and Benfield 2003 Plate 14 A].</skos:definition>
<owl:versionInfo>1</owl:versionInfo>
<dc:date>2011-10-21 14:18:49.0</dc:date>
<skos:note xml:lang="en">accepted</skos:note>
<owl:deprecated>false</owl:deprecated>
<skos:broader rdf:resource="http://vocab.nerc.ac.uk/collection/L05/current/67/"/>
<void:inDataset rdf:resource="http://vocab.nerc.ac.uk/.well-known/void"/>
</skos:Concept>
</skos:member>
<skos:member>
<skos:Concept rdf:about="http://vocab.nerc.ac.uk/collection/L22/current/TOOL0092/">
<dc:identifier>SDN:L22::TOOL0092</dc:identifier>
<skos:notation>SDN:L22::TOOL0092</skos:notation>
<skos:prefLabel xml:lang="en">SonTek ADVOcean/Hydra acoustic doppler velocimeter</skos:prefLabel>
<skos:altLabel>SonTek ADVOcean/Hydra</skos:altLabel>
<skos:definition xml:lang="en">The ADVOcean uses acoustic Doppler technology to measure 3D flow in a small sampling volume located at a fixed distance (18cm) from the probe. The velocity range is programmable from +/- 5 to +/- 500 cm/s. Data can be acquired at sampling rates up to 25 Hz. The ADVOcean consists of two elements: acoustic sensor probe and processer. The Hydra label is used when additional optional sensors and interfaces for non-current parameters are included. The acoustic probe calibration can only change if the system is physically damaged.</skos:definition>
<owl:versionInfo>3</owl:versionInfo>
<dc:date>2010-07-20 16:32:34.0</dc:date>
<skos:note xml:lang="en">accepted</skos:note>
<owl:deprecated>false</owl:deprecated>
<skos:broader rdf:resource="http://vocab.nerc.ac.uk/collection/L05/current/384/"/>
<void:inDataset rdf:resource="http://vocab.nerc.ac.uk/.well-known/void"/>
</skos:Concept>
</skos:member>
<skos:member>
<skos:Concept rdf:about="http://vocab.nerc.ac.uk/collection/L22/current/TOOL0090/">
<dc:identifier>SDN:L22::TOOL0090</dc:identifier>
<skos:notation>SDN:L22::TOOL0090</skos:notation>
<skos:prefLabel xml:lang="en">SonTek Argonaut moored 3D doppler current meter</skos:prefLabel>
<skos:altLabel>SonTek Argonaut-MD</skos:altLabel>
<skos:definition xml:lang="en">The Argonaut-MD is a single-point doppler 3D vector averaging current meter designed for mooring deploymen for up to 2 years. It does not require calibration, has no moving parts, no threshold velocity and can be fitted with optional pressure and temperature sensors, Sea-Bird SeaCAT CTD or an inductive modem. It uses a fixed measurement volume centered 1.25 m from the instrument for 3 MHz systems (2.0 m for 1.5 MHz systems) and is housed in a single Deltrin or Titanium canister with internal memory and batteries. It can be clamped to the mooring line or mounted within a mooring cage.</skos:definition>
<owl:versionInfo>1</owl:versionInfo>
<dc:date>2009-11-30 11:56:35.0</dc:date>
<skos:note xml:lang="en">accepted</skos:note>
<owl:deprecated>false</owl:deprecated>
<skos:broader rdf:resource="http://vocab.nerc.ac.uk/collection/L05/current/114/"/>
<void:inDataset rdf:resource="http://vocab.nerc.ac.uk/.well-known/void"/>
</skos:Concept>
</skos:member>
<skos:member>
<skos:Concept rdf:about="http://vocab.nerc.ac.uk/collection/L22/current/TOOL0404/">
<dc:identifier>SDN:L22::TOOL0404</dc:identifier>
<skos:notation>SDN:L22::TOOL0404</skos:notation>
<skos:prefLabel xml:lang="en">Sonic Gill R3-100 Research sonic anemometer</skos:prefLabel>
<skos:altLabel>Gill R3-100 anemometer</skos:altLabel>
<skos:definition xml:lang="en">Triaxial sonic anemometer with symmetrical head (vertical configuration with 3-fold rotational symmetry) and a data output rate of 100Hz. The sensor head incorporates three pairs of transducers orientated orthogonally across the measurement region. Each transducer in a pair alternately transmits and receives ultrasound pulses to and from its partner. By measuring the travel time of the pulse in both directions, the velocity component of the air flow along the line of each transducer pair is determined. A mathematical transformation converts the three wind vectors into U, V, W resultants.</skos:definition>
<owl:versionInfo>1</owl:versionInfo>
<dc:date>2011-07-01 10:22:02.0</dc:date>
<skos:note xml:lang="en">accepted</skos:note>
<owl:deprecated>false</owl:deprecated>
<skos:broader rdf:resource="http://vocab.nerc.ac.uk/collection/L05/current/101/"/>
<void:inDataset rdf:resource="http://vocab.nerc.ac.uk/.well-known/void"/>
</skos:Concept>
</skos:member>
<skos:member>
<skos:Concept rdf:about="http://vocab.nerc.ac.uk/collection/L22/current/TOOL0084/">
<dc:identifier>SDN:L22::TOOL0084</dc:identifier>
<skos:notation>SDN:L22::TOOL0084</skos:notation>
<skos:prefLabel xml:lang="en">Sonic Gill R3A-100 Research sonic anemometer</skos:prefLabel>
<skos:altLabel>Gill R3A-100 anemometer</skos:altLabel>
<skos:definition xml:lang="en">Triaxial sonic anemometer with asymmetric head and a data output rate of 100Hz. The sensor head of the anemometer consists of three pairs of transducers orientated at different angles across the measurement region. Each pair of transducers act alternately as transmitters and receivers, sending pulses of ultrasound between them. By measuring the time of flight of the pulse in both directions, the velocity component of the air flow along the line of the transducer pair can be determined. This measurement is carried out for each of the three transducer pairs in turn. A mathematical transformation is then performed, to convert the resulting three wind vectors into U,V,W format.</skos:definition>
<owl:versionInfo>2</owl:versionInfo>
<dc:date>2011-07-01 10:14:11.0</dc:date>
<skos:note xml:lang="en">accepted</skos:note>
<owl:deprecated>false</owl:deprecated>
<skos:related rdf:resource="http://vocab.nerc.ac.uk/collection/P01/current/EWSKSS01/"/>
<skos:related rdf:resource="http://vocab.nerc.ac.uk/collection/P01/current/EWDASS01/"/>
<skos:related rdf:resource="http://vocab.nerc.ac.uk/collection/P01/current/ESZKSA01/"/>
<skos:broader rdf:resource="http://vocab.nerc.ac.uk/collection/L05/current/101/"/>
<void:inDataset rdf:resource="http://vocab.nerc.ac.uk/.well-known/void"/>
</skos:Concept>
</skos:member>
<skos:member>
<skos:Concept rdf:about="http://vocab.nerc.ac.uk/collection/L22/current/TOOL0661/">
<dc:identifier>SDN:L22::TOOL0661</dc:identifier>
<skos:notation>SDN:L22::TOOL0661</skos:notation>
<skos:prefLabel xml:lang="en">Sperry Marine MK-37 Model E Gyrocompass</skos:prefLabel>
<skos:altLabel>Sperry Marine MK-37 Gyrocompass</skos:altLabel>
<skos:definition xml:lang="en">Instrument that contains a controlled gyroscope which seeks and aligns itself with the meridian and points to true north. It uses the properties of the gyroscope in combination with the rotation of the earth and the effect of gravity. The effects of varying speed and latitude are compensated for by the use of manually operated controls.</skos:definition>
<owl:versionInfo>1</owl:versionInfo>
<dc:date>2014-01-28 11:29:55.0</dc:date>
<skos:note xml:lang="en">accepted</skos:note>
<owl:deprecated>false</owl:deprecated>
<skos:broader rdf:resource="http://vocab.nerc.ac.uk/collection/L05/current/385/"/>
<void:inDataset rdf:resource="http://vocab.nerc.ac.uk/.well-known/void"/>
</skos:Concept>
</skos:member>
<skos:member>
<skos:Concept rdf:about="http://vocab.nerc.ac.uk/collection/L22/current/TOOL0624/">
<dc:identifier>SDN:L22::TOOL0624</dc:identifier>
<skos:notation>SDN:L22::TOOL0624</skos:notation>
<skos:prefLabel xml:lang="en">Sperry Marine NAVIGAT X MK 2 digital gyrocompass system</skos:prefLabel>
<skos:altLabel>Sperry NAVIGAT X MK 2 gyrocompass</skos:altLabel>
<skos:definition xml:lang="en">A digital gyrocompass system which runs on a 24-volt power supply with two independent DC inputs. It can drive up to four analogue repeaters and provides five additional serial data outputs and one six-steps/degree output. Heading accuracy is &lt; 0.1° secant latitude (static), &lt; 0.4° secant latitude (dynamic) and &lt; 0.1° secant latitude (settle point error)</skos:definition>
<owl:versionInfo>1</owl:versionInfo>
<dc:date>2013-06-10 16:36:53.0</dc:date>
<skos:note xml:lang="en">accepted</skos:note>
<owl:deprecated>false</owl:deprecated>
<skos:broader rdf:resource="http://vocab.nerc.ac.uk/collection/L05/current/385/"/>
<void:inDataset rdf:resource="http://vocab.nerc.ac.uk/.well-known/void"/>
</skos:Concept>
</skos:member>
<skos:member>
<skos:Concept rdf:about="http://vocab.nerc.ac.uk/collection/L22/current/TOOL0545/">
<dc:identifier>SDN:L22::TOOL0545</dc:identifier>
<skos:notation>SDN:L22::TOOL0545</skos:notation>
<skos:prefLabel xml:lang="en">Stainless steel air sample canister</skos:prefLabel>
<skos:altLabel>Stainless steel canister</skos:altLabel>
<skos:definition xml:lang="en">Stainless steel sampling container suitable for the collection of high pressure air samples. The container has a capacity of several litres.</skos:definition>
<owl:versionInfo>1</owl:versionInfo>
<dc:date>2012-09-26 16:33:22.0</dc:date>
<skos:note xml:lang="en">accepted</skos:note>
<owl:deprecated>false</owl:deprecated>
<skos:broader rdf:resource="http://vocab.nerc.ac.uk/collection/L05/current/11/"/>
<void:inDataset rdf:resource="http://vocab.nerc.ac.uk/.well-known/void"/>
</skos:Concept>
</skos:member>
<skos:member>
<skos:Concept rdf:about="http://vocab.nerc.ac.uk/collection/L22/current/TOOL0500/">
<dc:identifier>SDN:L22::TOOL0500</dc:identifier>
<skos:notation>SDN:L22::TOOL0500</skos:notation>
<skos:prefLabel xml:lang="en">Stand-alone pump</skos:prefLabel>
<skos:altLabel>SAP</skos:altLabel>
<skos:definition xml:lang="en">A submersible battery powered water pump that sucks water through various filters leaving the materials of interest on the filter for analysis. SAPs are deployed clamped to a hydrographic wire and may be used to sample at depths of up to 6000 m. A SAP can pump thousands of litres of water over a few hours.</skos:definition>
<owl:versionInfo>1</owl:versionInfo>
<dc:date>2012-06-21 16:09:48.0</dc:date>
<skos:note xml:lang="en">accepted</skos:note>
<owl:deprecated>false</owl:deprecated>
<skos:broader rdf:resource="http://vocab.nerc.ac.uk/collection/L05/current/84/"/>
<void:inDataset rdf:resource="http://vocab.nerc.ac.uk/.well-known/void"/>
</skos:Concept>
</skos:member>
<skos:member>
<skos:Concept rdf:about="http://vocab.nerc.ac.uk/collection/L22/current/NETT0154/">
<dc:identifier>SDN:L22::NETT0154</dc:identifier>
<skos:notation>SDN:L22::NETT0154</skos:notation>
<skos:prefLabel xml:lang="en">Standard Plankton Indicator high-speed sampler - Hardy (1926, 1936); Glover (1953)</skos:prefLabel>
<skos:altLabel>Standard Plankton Indicator HSS</skos:altLabel>
<skos:definition xml:lang="en">Originally had a 10.1 cm diameter mouth opening expanding to 17.8 cm diameter main body. Overall length 91.4 cm.  In modified form with 3.8 cm diameter aperture opening, 7.6 cm diameter filter disc, 56 cm overall length, and with depressor and stabilizing fins.  Normal towing speed 8 knots [Wiebe and Benfield 2003 Plate 13 D,E].</skos:definition>
<owl:versionInfo>1</owl:versionInfo>
<dc:date>2011-10-21 14:18:49.0</dc:date>
<skos:note xml:lang="en">accepted</skos:note>
<owl:deprecated>false</owl:deprecated>
<skos:broader rdf:resource="http://vocab.nerc.ac.uk/collection/L05/current/67/"/>
<void:inDataset rdf:resource="http://vocab.nerc.ac.uk/.well-known/void"/>
</skos:Concept>
</skos:member>
<skos:member>
<skos:Concept rdf:about="http://vocab.nerc.ac.uk/collection/L22/current/TOOL0183/">
<dc:identifier>SDN:L22::TOOL0183</dc:identifier>
<skos:notation>SDN:L22::TOOL0183</skos:notation>
<skos:prefLabel xml:lang="en">Star-Oddi DST CTD</skos:prefLabel>
<skos:altLabel>Star-Oddi DST CTD</skos:altLabel>
<skos:definition xml:lang="en">A miniature self-contained CTD primarily designed for mounting on fish, birds or marine mammals. Salinity resolution is 0.02 PSU and accuracy +-0.75 PSU. Temperature resolution is 0.032C and accuracy +-0.1C.</skos:definition>
<owl:versionInfo>1</owl:versionInfo>
<dc:date>2010-05-18 16:10:58.0</dc:date>
<skos:note xml:lang="en">accepted</skos:note>
<owl:deprecated>false</owl:deprecated>
<skos:broader rdf:resource="http://vocab.nerc.ac.uk/collection/L05/current/134/"/>
<skos:broader rdf:resource="http://vocab.nerc.ac.uk/collection/L05/current/130/"/>
<skos:broader rdf:resource="http://vocab.nerc.ac.uk/collection/L05/current/350/"/>
<void:inDataset rdf:resource="http://vocab.nerc.ac.uk/.well-known/void"/>
</skos:Concept>
</skos:member>
<skos:member>
<skos:Concept rdf:about="http://vocab.nerc.ac.uk/collection/L22/current/TOOL0490/">
<dc:identifier>SDN:L22::TOOL0490</dc:identifier>
<skos:notation>SDN:L22::TOOL0490</skos:notation>
<skos:prefLabel xml:lang="en">Star-Oddi DST Pitch and Roll Recorder</skos:prefLabel>
<skos:altLabel>Star-Oddi DST Pitch and Roll</skos:altLabel>
<skos:definition xml:lang="en">A miniature underwater data logger which measures temperature, pressure and pitch and roll (tilt angle) relative to the earth gravity. It has a range of depth ratings from 30 m to 3000 m and a temperature range of -1 degC to 40 degC with an accuracy of +/- 0.1 degC and a resolution of 0.032 degC. The tilt range is 160 deg (+/- 80 deg) with an accuracy of +/- 5deg and a resolution of 0.3 deg.</skos:definition>
<owl:versionInfo>1</owl:versionInfo>
<dc:date>2012-04-30 10:32:27.0</dc:date>
<skos:note xml:lang="en">accepted</skos:note>
<owl:deprecated>false</owl:deprecated>
<skos:broader rdf:resource="http://vocab.nerc.ac.uk/collection/L05/current/385/"/>
<skos:broader rdf:resource="http://vocab.nerc.ac.uk/collection/L05/current/134/"/>
<void:inDataset rdf:resource="http://vocab.nerc.ac.uk/.well-known/void"/>
</skos:Concept>
</skos:member>
<skos:member>
<skos:Concept rdf:about="http://vocab.nerc.ac.uk/collection/L22/current/TOOL0580/">
<dc:identifier>SDN:L22::TOOL0580</dc:identifier>
<skos:notation>SDN:L22::TOOL0580</skos:notation>
<skos:prefLabel xml:lang="en">Star-Oddi DST centi-T Temperature Recorder</skos:prefLabel>
<skos:altLabel>Star-Oddi centi-T</skos:altLabel>
<skos:definition xml:lang="en">A miniature underwater temperature recorder with a temperature resolution of 0.032 degC and an accuracy of +/- 0.1 degC over a range of -1 degC to 40 degC. It has a memory capacity of 174,000 measurements in total; 261,819 bytes/ temperature 1.5 bytes. A memory extension option of 786,099 bytes is available with a data retention of 25 years.</skos:definition>
<owl:versionInfo>1</owl:versionInfo>
<dc:date>2012-12-20 15:48:57.0</dc:date>
<skos:note xml:lang="en">accepted</skos:note>
<owl:deprecated>false</owl:deprecated>
<skos:broader rdf:resource="http://vocab.nerc.ac.uk/collection/L05/current/134/"/>
<void:inDataset rdf:resource="http://vocab.nerc.ac.uk/.well-known/void"/>
</skos:Concept>
</skos:member>
<skos:member>
<skos:Concept rdf:about="http://vocab.nerc.ac.uk/collection/L22/current/TOOL0383/">
<dc:identifier>SDN:L22::TOOL0383</dc:identifier>
<skos:notation>SDN:L22::TOOL0383</skos:notation>
<skos:prefLabel xml:lang="en">Star-Oddi DST centi-TD Temperature and Depth Recorder</skos:prefLabel>
<skos:altLabel>Star-Oddi centi-TD</skos:altLabel>
<skos:definition xml:lang="en">A miniature underwater temperature-pressure recorder with a range of depth ratings from 30 m to 3000 m. Temperature resolution is 0.032C, with an accuracy of ±0.1C over a range -2C to 40C. Depth resolution is 0.03% of selected range, with an accuracy of ±0.4% of selected range for 30 m to 270 m range and ±0.6% of selected range for 800 m to 3000 m range. See https://www.bodc.ac.uk/data/documents/nodb/223482/ for further details.</skos:definition>
<owl:versionInfo>1</owl:versionInfo>
<dc:date>2011-03-23 20:28:03.0</dc:date>
<skos:note xml:lang="en">accepted</skos:note>
<owl:deprecated>false</owl:deprecated>
<skos:broader rdf:resource="http://vocab.nerc.ac.uk/collection/L05/current/134/"/>
<void:inDataset rdf:resource="http://vocab.nerc.ac.uk/.well-known/void"/>
</skos:Concept>
</skos:member>
<skos:member>
<skos:Concept rdf:about="http://vocab.nerc.ac.uk/collection/L22/current/TOOL0267/">
<dc:identifier>SDN:L22::TOOL0267</dc:identifier>
<skos:notation>SDN:L22::TOOL0267</skos:notation>
<skos:prefLabel xml:lang="en">Star-Oddi Starmon mini temperature recorder</skos:prefLabel>
<skos:altLabel>Starmon mini TR</skos:altLabel>
<skos:definition xml:lang="en">An underwater temperature recorder in either a plastic (400m) or titanium (11000m) casing.  Temperature average resolution is 0.013C and accuracy is +-0.05C over a range -2C to 40C: clock accuray better than 1 minute per month. Temperature equilibration: 63% 18 seconds (plastic case) or 6 seconds (titanium case); 100% 3 minutes (plastic case) or 1 minute (titanium case).</skos:definition>
<owl:versionInfo>1</owl:versionInfo>
<dc:date>2010-05-18 16:10:58.0</dc:date>
<skos:note xml:lang="en">accepted</skos:note>
<owl:deprecated>false</owl:deprecated>
<skos:broader rdf:resource="http://vocab.nerc.ac.uk/collection/L05/current/134/"/>
<void:inDataset rdf:resource="http://vocab.nerc.ac.uk/.well-known/void"/>
</skos:Concept>
</skos:member>
<skos:member>
<skos:Concept rdf:about="http://vocab.nerc.ac.uk/collection/L22/current/TOOL0620/">
<dc:identifier>SDN:L22::TOOL0620</dc:identifier>
<skos:notation>SDN:L22::TOOL0620</skos:notation>
<skos:prefLabel xml:lang="en">Steedman Science and Engineering CM01 Acoustic Current Meter</skos:prefLabel>
<skos:altLabel>Steedman CM01 ACM</skos:altLabel>
<skos:definition xml:lang="en">A recording current meter fitted with two orthogonal acoustic transducers and a flux-gate compass. The water velocity is measured using an acoustic phase shift technique and the resulting current vectors are averaged over a user-specified interval. Further information may be found in http://www.bodc.ac.uk/data/documents/nodb/148626/.</skos:definition>
<owl:versionInfo>1</owl:versionInfo>
<dc:date>2013-05-09 16:22:25.0</dc:date>
<skos:note xml:lang="en">accepted</skos:note>
<owl:deprecated>false</owl:deprecated>
<skos:broader rdf:resource="http://vocab.nerc.ac.uk/collection/L05/current/114/"/>
<skos:broader rdf:resource="http://vocab.nerc.ac.uk/collection/L05/current/134/"/>
<void:inDataset rdf:resource="http://vocab.nerc.ac.uk/.well-known/void"/>
</skos:Concept>
</skos:member>
<skos:member>
<skos:Concept rdf:about="http://vocab.nerc.ac.uk/collection/L22/current/NETT0155/">
<dc:identifier>SDN:L22::NETT0155</dc:identifier>
<skos:notation>SDN:L22::NETT0155</skos:notation>
<skos:prefLabel xml:lang="en">Streamer Plankton sampler - Ishida (1963, 1964)</skos:prefLabel>
<skos:altLabel>Ishida streamer sampler</skos:altLabel>
<skos:definition xml:lang="en">A 45 cm diameter mouth opening with a closing door and a metal cylinder 45 cm long to which is attached a net of 5 meters length.  The sampler sinks with closing door open flushing the net. When halted attached line lifted, the door closes and end of net is closed capturing a 600 litre sample [Wiebe and Benfield 2003 Plate 10 E].</skos:definition>
<owl:versionInfo>1</owl:versionInfo>
<dc:date>2011-10-21 14:18:49.0</dc:date>
<skos:note xml:lang="en">accepted</skos:note>
<owl:deprecated>false</owl:deprecated>
<skos:broader rdf:resource="http://vocab.nerc.ac.uk/collection/L05/current/22/"/>
<void:inDataset rdf:resource="http://vocab.nerc.ac.uk/.well-known/void"/>
</skos:Concept>
</skos:member>
<skos:member>
<skos:Concept rdf:about="http://vocab.nerc.ac.uk/collection/L22/current/TOOL0611/">
<dc:identifier>SDN:L22::TOOL0611</dc:identifier>
<skos:notation>SDN:L22::TOOL0611</skos:notation>
<skos:prefLabel xml:lang="en">Suber SLS21 vector-averaging current meter</skos:prefLabel>
<skos:altLabel>Suber SLS21 VACM</skos:altLabel>
<skos:definition xml:lang="en">A current meter fitted with a Savonius rotor magnetically coupled to a reed switch counter, a vane on tungsten carbide bearings magnetically coupled to a compass and solid-state crystal clock. Current vectors were continuously measured and then averaged after a specified time interval (generally 10 minutes) by an on-board minicomputer to produce the logged data values. Accuracy was 2 per cent for speed, 4 degrees for direction and 2 seconds per day for the clock. Casings were available for operating depths of 1000m, 3000m and 6000m.More information may be found in http://www.bodc.ac.uk/data/documents/nodb/19202/</skos:definition>
<owl:versionInfo>1</owl:versionInfo>
<dc:date>2013-04-10 17:01:43.0</dc:date>
<skos:note xml:lang="en">accepted</skos:note>
<owl:deprecated>false</owl:deprecated>
<skos:broader rdf:resource="http://vocab.nerc.ac.uk/collection/L05/current/114/"/>
<void:inDataset rdf:resource="http://vocab.nerc.ac.uk/.well-known/void"/>
</skos:Concept>
</skos:member>
<skos:member>
<skos:Concept rdf:about="http://vocab.nerc.ac.uk/collection/L22/current/TOOL0139/">
<dc:identifier>SDN:L22::TOOL0139</dc:identifier>
<skos:notation>SDN:L22::TOOL0139</skos:notation>
<skos:prefLabel xml:lang="en">Sunburst Submersible Autonomous Moored Instrument Carbon Dioxide Sensor</skos:prefLabel>
<skos:altLabel>Sunburst SAMI-CO2</skos:altLabel>
<skos:definition xml:lang="en">A reagent based CO2 sensor for measuring partial pressure of carbon dioxide (pCO2) in-situ in water over a range of approximately 0-2000 micro-atmospheres with a precision of approximately 1 microatmosphere at 360 microatmospheres. Maximum deployment depth is approximately 100 metres for SAMI-CO2-100 (PVC housing) and 1500 metres for SAMI-CO2-1500 (aluminium housing).</skos:definition>
<owl:versionInfo>1</owl:versionInfo>
<dc:date>2010-05-18 16:10:58.0</dc:date>
<skos:note xml:lang="en">accepted</skos:note>
<owl:deprecated>false</owl:deprecated>
<skos:broader rdf:resource="http://vocab.nerc.ac.uk/collection/L05/current/351/"/>
<void:inDataset rdf:resource="http://vocab.nerc.ac.uk/.well-known/void"/>
</skos:Concept>
</skos:member>
<skos:member>
<skos:Concept rdf:about="http://vocab.nerc.ac.uk/collection/L22/current/NETT0156/">
<dc:identifier>SDN:L22::NETT0156</dc:identifier>
<skos:notation>SDN:L22::NETT0156</skos:notation>
<skos:prefLabel xml:lang="en">Surface plankton push net - Miller (1973)</skos:prefLabel>
<skos:altLabel>Miller neuston net</skos:altLabel>
<skos:definition xml:lang="en">A pair of rectangular nets (0.505 mm nylon mesh)each 60 cm x 60 cm mouth opening and ~420 cm long are positioned side by side in a framework that is mounted in front of a small catamaran boat that pushes the frame through the water at ~ 2.6 knots.  Samples are removed from the nets through a well in the catamaran floor. Flow is measured with a TSK flowmeter modified to electronically record flow counts [Wiebe and Benfield 2003 Plate 21 E].</skos:definition>
<owl:versionInfo>1</owl:versionInfo>
<dc:date>2011-10-21 14:18:49.0</dc:date>
<skos:note xml:lang="en">accepted</skos:note>
<owl:deprecated>false</owl:deprecated>
<skos:broader rdf:resource="http://vocab.nerc.ac.uk/collection/L05/current/69/"/>
<skos:broader rdf:resource="http://vocab.nerc.ac.uk/collection/L05/current/388/"/>
<void:inDataset rdf:resource="http://vocab.nerc.ac.uk/.well-known/void"/>
</skos:Concept>
</skos:member>
<skos:member>
<skos:Concept rdf:about="http://vocab.nerc.ac.uk/collection/L22/current/TOOL0086/">
<dc:identifier>SDN:L22::TOOL0086</dc:identifier>
<skos:notation>SDN:L22::TOOL0086</skos:notation>
<skos:prefLabel xml:lang="en">Systron Donner MotionPak accelerometer</skos:prefLabel>
<skos:altLabel>SD MotionPak accelerometer</skos:altLabel>
<skos:definition xml:lang="en">The Systron Donner Inertial MotionPak is a solid-state MEMS six Degree-of-Freedom inertial sensing system used for measuring angular rates and linear accelerations in instrumentation and control applications. These multi-axis packages allow a pre-combined solution, minimizing the customer burden of sensor integration. The multi-axis sensor assemblies sense roll, pitch and yaw inputs simultaneously on a moving platform.</skos:definition>
<owl:versionInfo>1</owl:versionInfo>
<dc:date>2009-11-30 11:56:35.0</dc:date>
<skos:note xml:lang="en">accepted</skos:note>
<owl:deprecated>false</owl:deprecated>
<skos:broader rdf:resource="http://vocab.nerc.ac.uk/collection/L05/current/385/"/>
<void:inDataset rdf:resource="http://vocab.nerc.ac.uk/.well-known/void"/>
</skos:Concept>
</skos:member>
<skos:member>
<skos:Concept rdf:about="http://vocab.nerc.ac.uk/collection/L22/current/TOOL0422/">
<dc:identifier>SDN:L22::TOOL0422</dc:identifier>
<skos:notation>SDN:L22::TOOL0422</skos:notation>
<skos:prefLabel xml:lang="en">TSI 3321 Aerodynamic Particle Sizer</skos:prefLabel>
<skos:altLabel>TSI 3321 APS</skos:altLabel>
<skos:definition xml:lang="en">The TSI 3321 Aerodynamic Particle Sizer (APS) measures the size distribution and concentration of aerosol particles in the diameter range 0.5 - 20 um. The aerosol sample is accelerated toward the detection area, where it crosses two slightly overlapping laser beams. The rate of acceleration is determined by the particle size. Larger particles accelerate more slowly due to their greater inertia. Light scattered by each particle is focussed onto a photodiode. The use of twin lasers results in a two-crested signal. The peak-to-peak time-of-flight is used to determine the particle velocity, and thus its aerodynamic size. The amplitude of the signal may be used to provide an alternative measure of particle size through light-scattering techniques.</skos:definition>
<owl:versionInfo>1</owl:versionInfo>
<dc:date>2011-09-06 17:41:15.0</dc:date>
<skos:note xml:lang="en">accepted</skos:note>
<owl:deprecated>false</owl:deprecated>
<skos:broader rdf:resource="http://vocab.nerc.ac.uk/collection/L05/current/386/"/>
<void:inDataset rdf:resource="http://vocab.nerc.ac.uk/.well-known/void"/>
</skos:Concept>
</skos:member>
<skos:member>
<skos:Concept rdf:about="http://vocab.nerc.ac.uk/collection/L22/current/TOOL0419/">
<dc:identifier>SDN:L22::TOOL0419</dc:identifier>
<skos:notation>SDN:L22::TOOL0419</skos:notation>
<skos:prefLabel xml:lang="en">TSI 3800 Aerosol Time-of-Flight Mass Spectrometer</skos:prefLabel>
<skos:altLabel>TSI 3800 ATOFMS</skos:altLabel>
<skos:definition xml:lang="en">The TSI 3800 Aerosol Time-of-Flight Mass Spectrometer (ATOFMS) provides size and chemical characterisation of aerosol particles in the size range 0.1-3.0 um. Air is pumped through the system in real time and particles are counted and timed as they pass each of two lasers in the sizing chamber. The particle size is determined from the particle's velocity through the sizing chamber. The particle is subjected to ultraviolet desorption and ionisation in the mass spectrometer chamber. Positive and negative ions are identified by separate detectors, based on their time of flight through the mass spectrometer chamber.</skos:definition>
<owl:versionInfo>1</owl:versionInfo>
<dc:date>2011-09-03 16:28:15.0</dc:date>
<skos:note xml:lang="en">accepted</skos:note>
<owl:deprecated>false</owl:deprecated>
<skos:broader rdf:resource="http://vocab.nerc.ac.uk/collection/L05/current/386/"/>
<void:inDataset rdf:resource="http://vocab.nerc.ac.uk/.well-known/void"/>
</skos:Concept>
</skos:member>
<skos:member>
<skos:Concept rdf:about="http://vocab.nerc.ac.uk/collection/L22/current/TOOL0423/">
<dc:identifier>SDN:L22::TOOL0423</dc:identifier>
<skos:notation>SDN:L22::TOOL0423</skos:notation>
<skos:prefLabel xml:lang="en">TSI 3936 Scanning Mobility Particle Sizer</skos:prefLabel>
<skos:altLabel>TSI 3936 SMPS</skos:altLabel>
<skos:definition xml:lang="en">A differential mobility analyser that measures the size distribution and concentration of aerosol particles. It includes a cylindrical detection chamber with a variable-voltage collection rod running centrally along its length. The aerosol sample is introduced to the axial laminar flow of the chamber, where particles are deflected toward the collection rod by its electric field. Only particles within a narrow range of sizes, and thus a narrow range of mobilities, have the necessary trajectory to exit to the particle counter. The instrument is programmed to scan through a range of voltages, thereby varying the size of particles to be counted. The SMPS can scan through its full diameter range, 0.0025 um - 1 um, in 16 seconds. The scanning period can be increased to improve resolution at low concentrations. At its highest resolution, the SMPS can distinguish particle counts in 167 size bins.</skos:definition>
<owl:versionInfo>1</owl:versionInfo>
<dc:date>2011-09-06 17:41:15.0</dc:date>
<skos:note xml:lang="en">accepted</skos:note>
<owl:deprecated>false</owl:deprecated>
<skos:broader rdf:resource="http://vocab.nerc.ac.uk/collection/L05/current/386/"/>
<void:inDataset rdf:resource="http://vocab.nerc.ac.uk/.well-known/void"/>
</skos:Concept>
</skos:member>
<skos:member>
<skos:Concept rdf:about="http://vocab.nerc.ac.uk/collection/L22/current/TOOL0093/">
<dc:identifier>SDN:L22::TOOL0093</dc:identifier>
<skos:notation>SDN:L22::TOOL0093</skos:notation>
<skos:prefLabel xml:lang="en">TSS HRP-2-25 compact motion sensor</skos:prefLabel>
<skos:altLabel>TSS HRP-2-25 CMS</skos:altLabel>
<skos:definition xml:lang="en">The TSS Compact Motion Sensor is designed to meet the motion measurement requirements of a oceanographic instruments and platforms from single-beam echo-sounders to dynamic positioning systems. The CMS can be used to measure heave, pitch and roll of a vessel. For more information see http://www.bodc.ac.uk/data/documents/nodb/147645/</skos:definition>
<owl:versionInfo>1</owl:versionInfo>
<dc:date>2010-09-06 17:01:34.0</dc:date>
<skos:note xml:lang="en">accepted</skos:note>
<owl:deprecated>false</owl:deprecated>
<skos:broader rdf:resource="http://vocab.nerc.ac.uk/collection/L05/current/385/"/>
<void:inDataset rdf:resource="http://vocab.nerc.ac.uk/.well-known/void"/>
</skos:Concept>
</skos:member>
<skos:member>
<skos:Concept rdf:about="http://vocab.nerc.ac.uk/collection/L22/current/TOOL0538/">
<dc:identifier>SDN:L22::TOOL0538</dc:identifier>
<skos:notation>SDN:L22::TOOL0538</skos:notation>
<skos:prefLabel xml:lang="en">Technicap NOEX bottle</skos:prefLabel>
<skos:altLabel>NOEX bottle</skos:altLabel>
<skos:definition xml:lang="en">Water bottle designed for oceanographic sampling. The bottle comprises a plastic tube with caps at each end and is deployed with the caps held open, then closed at the target depth. Multiple bottles can be deployed on a CTD frame rosette. Bottle capacity is variable, but normally several litres. The bottle was developed by Technicap in the 1990s but has been superseded by more recent models. There is no known source of support available for this sampler.</skos:definition>
<owl:versionInfo>1</owl:versionInfo>
<dc:date>2012-09-25 16:03:31.0</dc:date>
<skos:note xml:lang="en">accepted</skos:note>
<owl:deprecated>false</owl:deprecated>
<skos:broader rdf:resource="http://vocab.nerc.ac.uk/collection/L05/current/30/"/>
<void:inDataset rdf:resource="http://vocab.nerc.ac.uk/.well-known/void"/>
</skos:Concept>
</skos:member>
<skos:member>
<skos:Concept rdf:about="http://vocab.nerc.ac.uk/collection/L22/current/TOOL0291/">
<dc:identifier>SDN:L22::TOOL0291</dc:identifier>
<skos:notation>SDN:L22::TOOL0291</skos:notation>
<skos:prefLabel xml:lang="en">Technicon AutoAnalyzer II colorimetric autoanalyser</skos:prefLabel>
<skos:altLabel>Technicon AAII AA</skos:altLabel>
<skos:definition xml:lang="en">A rapid flow analyser that may be used to measure nutrient concentrations in seawater. It is a continuous segmented flow instrument consisting of a sampler, peristaltic pump, analytical cartridge, heating bath, and colorimeter.</skos:definition>
<owl:versionInfo>2</owl:versionInfo>
<dc:date>2010-11-18 12:39:41.0</dc:date>
<skos:note xml:lang="en">accepted</skos:note>
<owl:deprecated>false</owl:deprecated>
<skos:related rdf:resource="http://vocab.nerc.ac.uk/collection/P01/current/PHOSAATX/"/>
<skos:related rdf:resource="http://vocab.nerc.ac.uk/collection/P01/current/NTRIAATX/"/>
<skos:related rdf:resource="http://vocab.nerc.ac.uk/collection/P01/current/NTRZAATX/"/>
<skos:related rdf:resource="http://vocab.nerc.ac.uk/collection/P01/current/AMONAATX/"/>
<skos:related rdf:resource="http://vocab.nerc.ac.uk/collection/P01/current/SLCAAATX/"/>
<skos:broader rdf:resource="http://vocab.nerc.ac.uk/collection/L05/current/LAB03/"/>
<skos:broader rdf:resource="http://vocab.nerc.ac.uk/collection/L05/current/LAB04/"/>
<owl:sameAs rdf:resource="http://onto.nerc.ac.uk/CAST/121"/>
<void:inDataset rdf:resource="http://vocab.nerc.ac.uk/.well-known/void"/>
</skos:Concept>
</skos:member>
<skos:member>
<skos:Concept rdf:about="http://vocab.nerc.ac.uk/collection/L22/current/TOOL0520/">
<dc:identifier>SDN:L22::TOOL0520</dc:identifier>
<skos:notation>SDN:L22::TOOL0520</skos:notation>
<skos:prefLabel xml:lang="en">Technicon TrAAcs 800 colorimetric autoanalyser</skos:prefLabel>
<skos:altLabel>TrAAcs 800 autoanalyser</skos:altLabel>
<skos:definition xml:lang="en">The TrAAcs system is a continuous flow wet chemistry analyser that determines analyte concentrations using a colorimeter to detect changes in colour produced by the presence of the analytes. It may be used to measure nutrient concentrations in seawater. The instrument is no longer in production and Technicon no longer exists. However, the instrument is supported (parts, servicing and consumables) by SEAL Analytical.</skos:definition>
<owl:versionInfo>1</owl:versionInfo>
<dc:date>2012-07-04 10:02:10.0</dc:date>
<skos:note xml:lang="en">accepted</skos:note>
<owl:deprecated>false</owl:deprecated>
<skos:broader rdf:resource="http://vocab.nerc.ac.uk/collection/L05/current/LAB04/"/>
<skos:broader rdf:resource="http://vocab.nerc.ac.uk/collection/L05/current/LAB03/"/>
<void:inDataset rdf:resource="http://vocab.nerc.ac.uk/.well-known/void"/>
</skos:Concept>
</skos:member>
<skos:member>
<skos:Concept rdf:about="http://vocab.nerc.ac.uk/collection/L22/current/TOOL0588/">
<dc:identifier>SDN:L22::TOOL0588</dc:identifier>
<skos:notation>SDN:L22::TOOL0588</skos:notation>
<skos:prefLabel xml:lang="en">Tedlar atmospheric sampling bag</skos:prefLabel>
<skos:altLabel>Tedlar bag</skos:altLabel>
<skos:definition xml:lang="en">A generic term for atmospheric sampling bags manufactured from Tedlar (DuPont trade name for the chemically inert plastic polyvinyl fluoride) film, fitted with a polypropylene or stainless steel valve and available with capacities ranging from 1-100 litres.  Samples are taken by either pumping air into the bag or evacuating the bag and opening the valve at the sampling site. Filled bags are connected directly to measuring equipment for analysis. Bags are available from several manufactureres and suppliers</skos:definition>
<owl:versionInfo>1</owl:versionInfo>
<dc:date>2013-01-15 15:43:48.0</dc:date>
<skos:note xml:lang="en">accepted</skos:note>
<owl:deprecated>false</owl:deprecated>
<skos:broader rdf:resource="http://vocab.nerc.ac.uk/collection/L05/current/11/"/>
<void:inDataset rdf:resource="http://vocab.nerc.ac.uk/.well-known/void"/>
</skos:Concept>
</skos:member>
<skos:member>
<skos:Concept rdf:about="http://vocab.nerc.ac.uk/collection/L22/current/TOOL0573/">
<dc:identifier>SDN:L22::TOOL0573</dc:identifier>
<skos:notation>SDN:L22::TOOL0573</skos:notation>
<skos:prefLabel xml:lang="en">Teflon PFA manifold air sampler</skos:prefLabel>
<skos:altLabel>Teflon PFA manifold air sampler</skos:altLabel>
<skos:definition xml:lang="en">Teflon PFA manifold leading directly from the least contaminated part of a ship to a clean metal bellows pump. Air is drawn through the tube by the pump at a flow rate of 30 litres/min and a subsample is fed into an analytical instrument.</skos:definition>
<owl:versionInfo>1</owl:versionInfo>
<dc:date>2012-11-28 14:15:26.0</dc:date>
<skos:note xml:lang="en">accepted</skos:note>
<owl:deprecated>false</owl:deprecated>
<skos:broader rdf:resource="http://vocab.nerc.ac.uk/collection/L05/current/58/"/>
<void:inDataset rdf:resource="http://vocab.nerc.ac.uk/.well-known/void"/>
</skos:Concept>
</skos:member>
<skos:member>
<skos:Concept rdf:about="http://vocab.nerc.ac.uk/collection/L22/current/TOOL0418/">
<dc:identifier>SDN:L22::TOOL0418</dc:identifier>
<skos:notation>SDN:L22::TOOL0418</skos:notation>
<skos:prefLabel xml:lang="en">Teflon-coated Niskin bottle</skos:prefLabel>
<skos:altLabel>Teflon-coated Niskin</skos:altLabel>
<skos:definition xml:lang="en">A teflon-coated free-flushing water sampling bottle with a capacity of 1.7-30 litres. It has caps with rubber seals at each end joined by a latex cord running through the interior of the bottle. It is deployed with the caps held open against the latex cord by plastic lanyards. When the bottle reaches the desired depth the lanyards are released by a pressure-actuated switch, command signal or messenger weight and the caps are forced shut and sealed. Bottles may be deployed singly clamped to a wire or in groups of up to 48 on a rosette. Reversing thermometers may be attached to a spring-loaded disk that rotates through 180 degrees on bottle closure. These bottles are specifically designed to minimise metal contamination when sampling trace metals.</skos:definition>
<owl:versionInfo>2</owl:versionInfo>
<dc:date>2012-06-22 13:49:29.0</dc:date>
<skos:note xml:lang="en">accepted</skos:note>
<owl:deprecated>false</owl:deprecated>
<skos:broader rdf:resource="http://vocab.nerc.ac.uk/collection/L05/current/30/"/>
<void:inDataset rdf:resource="http://vocab.nerc.ac.uk/.well-known/void"/>
</skos:Concept>
</skos:member>
<skos:member>
<skos:Concept rdf:about="http://vocab.nerc.ac.uk/collection/L22/current/TOOL0062/">
<dc:identifier>SDN:L22::TOOL0062</dc:identifier>
<skos:notation>SDN:L22::TOOL0062</skos:notation>
<skos:prefLabel xml:lang="en">Teledyne RDI 150kHz Narrowband Vessel-Mounted ADCP</skos:prefLabel>
<skos:altLabel>RDI 150kHz VM-ADCP</skos:altLabel>
<skos:definition xml:lang="en">The Teledyne RDI Narrowband Vessel-Mounted Acoustic Doppler Current Profiler is a long-range 3D current profiling ADCP designed for continuous current profiling from a moving ship. It has 150kHz narrowband signal processing and a patented 4 beam design.</skos:definition>
<owl:versionInfo>2</owl:versionInfo>
<dc:date>2010-05-05 13:47:14.0</dc:date>
<skos:note xml:lang="en">accepted</skos:note>
<owl:deprecated>false</owl:deprecated>
<skos:broader rdf:resource="http://mmisw.org/ont/trdi/models/VesselMount"/>
<skos:broader rdf:resource="http://vocab.nerc.ac.uk/collection/L05/current/115/"/>
<void:inDataset rdf:resource="http://vocab.nerc.ac.uk/.well-known/void"/>
</skos:Concept>
</skos:member>
<skos:member>
<skos:Concept rdf:about="http://vocab.nerc.ac.uk/collection/L22/current/TOOL0158/">
<dc:identifier>SDN:L22::TOOL0158</dc:identifier>
<skos:notation>SDN:L22::TOOL0158</skos:notation>
<skos:prefLabel xml:lang="en">Teledyne RDI 300kHz Narrowband Vessel-Mounted ADCP</skos:prefLabel>
<skos:altLabel>RDI 300kHz VM-ADCP</skos:altLabel>
<skos:definition xml:lang="en">The 300 kHz Teledyne RDI Narrowband Vessel-Mounted Acoustic Doppler Current Profiler is a 4-beam medium range ADCP designed for vessel mounting.</skos:definition>
<owl:versionInfo>1</owl:versionInfo>
<dc:date>2010-05-18 16:10:58.0</dc:date>
<skos:note xml:lang="en">accepted</skos:note>
<owl:deprecated>false</owl:deprecated>
<skos:broader rdf:resource="http://vocab.nerc.ac.uk/collection/L05/current/115/"/>
<skos:broader rdf:resource="http://mmisw.org/ont/trdi/models/VesselMount"/>
<void:inDataset rdf:resource="http://vocab.nerc.ac.uk/.well-known/void"/>
</skos:Concept>
</skos:member>
<skos:member>
<skos:Concept rdf:about="http://vocab.nerc.ac.uk/collection/L22/current/TOOL0061/">
<dc:identifier>SDN:L22::TOOL0061</dc:identifier>
<skos:notation>SDN:L22::TOOL0061</skos:notation>
<skos:prefLabel xml:lang="en">Teledyne RDI 300kHz Workhorse Monitor direct-reading ADCP</skos:prefLabel>
<skos:altLabel>RDI Workhorse-300 DR-ADCP</skos:altLabel>
<skos:definition xml:lang="en">A direct reading acoustic doppler current profiler (ADCP) with a standard depth rating of 200m with a 6000m-rated case available as an option. 300kHz Broadband signal processing gives high data resolution and a four-beam solution gives an independent error velocity measurement. It operates effectively between temperatures of -5°C and 45°C and has a velocity accuracy of 0.5% of the water velocity ±0.5cm/s.</skos:definition>
<owl:versionInfo>1</owl:versionInfo>
<dc:date>2009-11-30 11:56:35.0</dc:date>
<skos:note xml:lang="en">accepted</skos:note>
<owl:deprecated>false</owl:deprecated>
<skos:broader rdf:resource="http://vocab.nerc.ac.uk/collection/L05/current/115/"/>
<skos:broader rdf:resource="http://mmisw.org/ont/trdi/models/WorkhorseADCP"/>
<void:inDataset rdf:resource="http://vocab.nerc.ac.uk/.well-known/void"/>
</skos:Concept>
</skos:member>
<skos:member>
<skos:Concept rdf:about="http://vocab.nerc.ac.uk/collection/L22/current/TOOL0351/">
<dc:identifier>SDN:L22::TOOL0351</dc:identifier>
<skos:notation>SDN:L22::TOOL0351</skos:notation>
<skos:prefLabel xml:lang="en">Teledyne RDI 75kHz Ocean Observer narrowband ADCP</skos:prefLabel>
<skos:altLabel>RDI 75kHz narrowband Ocean Observer</skos:altLabel>
<skos:definition xml:lang="en">An acoustic doppler current profiler (ADCP) designed for deployment from oil platforms. It has a 75kHz narrowband signal and a standard depth rating of 100m. It can operate in long range or high precision modes with between 1 and 128 depth cells, typically 8m or 16m in size. The maximum measurement range is 700m, which decreases with decreasing bin size and the use of high precision mode. The instrument operates effectively between temperatures of -5 to 45 C and has a velocity accuracy of +/- 0.5cm per second or +/- 1% over the range +/- 7m per second. It includes a temperature sensor, a tilt meter and a fluxgate compass as standard.</skos:definition>
<owl:versionInfo>1</owl:versionInfo>
<dc:date>2010-09-06 12:45:22.0</dc:date>
<skos:note xml:lang="en">accepted</skos:note>
<owl:deprecated>false</owl:deprecated>
<skos:broader rdf:resource="http://mmisw.org/ont/trdi/models/OceanObserver"/>
<skos:broader rdf:resource="http://vocab.nerc.ac.uk/collection/L05/current/115/"/>
<void:inDataset rdf:resource="http://vocab.nerc.ac.uk/.well-known/void"/>
</skos:Concept>
</skos:member>
<skos:member>
<skos:Concept rdf:about="http://vocab.nerc.ac.uk/collection/L22/current/TOOL0445/">
<dc:identifier>SDN:L22::TOOL0445</dc:identifier>
<skos:notation>SDN:L22::TOOL0445</skos:notation>
<skos:prefLabel xml:lang="en">Teledyne RDI Broadband 150kHz ADCP</skos:prefLabel>
<skos:altLabel>RDI 150kHz BB ADCP</skos:altLabel>
<skos:definition xml:lang="en">The RDI Broadband ADCP is designed for mooring deployment and has an operating frequency of 150 kHz. The instrument uses Doppler-technology to achieve accurate and non-intrusive measurements and it can come with pressure and temperature sensors. It can be used in real time measurement situations or can log to an internal recorder powered by internal batteries.</skos:definition>
<owl:versionInfo>1</owl:versionInfo>
<dc:date>2011-11-24 11:44:57.0</dc:date>
<skos:note xml:lang="en">accepted</skos:note>
<owl:deprecated>false</owl:deprecated>
<skos:broader rdf:resource="http://vocab.nerc.ac.uk/collection/L05/current/115/"/>
<skos:broader rdf:resource="http://mmisw.org/ont/trdi/models/WorkhorseADCP"/>
<void:inDataset rdf:resource="http://vocab.nerc.ac.uk/.well-known/void"/>
</skos:Concept>
</skos:member>
<skos:member>
<skos:Concept rdf:about="http://vocab.nerc.ac.uk/collection/L22/current/TOOL0602/">
<dc:identifier>SDN:L22::TOOL0602</dc:identifier>
<skos:notation>SDN:L22::TOOL0602</skos:notation>
<skos:prefLabel xml:lang="en">Teledyne RDI Citadel TS-N Thermosalinograph</skos:prefLabel>
<skos:altLabel>RDI Citadel TS-N TSG</skos:altLabel>
<skos:definition xml:lang="en">A compact, low-maintenance system that uses Teledyne RDI's NXIC (Nonexternal-Field Inductive Conductivity) sensor and an aged thermistor in a through-flow housing. The system is designed for mounting on ships or gliders down to 500m. Parameters are measured to an accuracy of ±0.001 S/m for conductivity, ±0.005°C for temperature and ±0.015 PSU for salinity. Prior to 2009 this instrument was manufactured by Falmouth Scientific (FSI).</skos:definition>
<owl:versionInfo>1</owl:versionInfo>
<dc:date>2013-02-28 10:03:55.0</dc:date>
<skos:note xml:lang="en">accepted</skos:note>
<owl:deprecated>false</owl:deprecated>
<skos:broader rdf:resource="http://vocab.nerc.ac.uk/collection/L05/current/134/"/>
<skos:broader rdf:resource="http://vocab.nerc.ac.uk/collection/L05/current/133/"/>
<skos:broader rdf:resource="http://vocab.nerc.ac.uk/collection/L05/current/350/"/>
<void:inDataset rdf:resource="http://vocab.nerc.ac.uk/.well-known/void"/>
</skos:Concept>
</skos:member>
<skos:member>
<skos:Concept rdf:about="http://vocab.nerc.ac.uk/collection/L22/current/TOOL0091/">
<dc:identifier>SDN:L22::TOOL0091</dc:identifier>
<skos:notation>SDN:L22::TOOL0091</skos:notation>
<skos:prefLabel xml:lang="en">Teledyne RDI Narrowband 150kHz ADCP</skos:prefLabel>
<skos:altLabel>RDI 150kHz ADCP</skos:altLabel>
<skos:definition xml:lang="en">A narrowband ADCP designed for mooring deployment operating at 150 kHz with a measurement range of 300m in the water column. The instrument uses Doppler-technology to achieve accurate and non-intrusive measurements and it can come with pressure and temperature sensors. It can be used in real time measurement situations or can log to an internal recorder powered by internal batteries.</skos:definition>
<owl:versionInfo>1</owl:versionInfo>
<dc:date>2010-09-07 10:10:46.0</dc:date>
<skos:note xml:lang="en">accepted</skos:note>
<owl:deprecated>false</owl:deprecated>
<skos:broader rdf:resource="http://vocab.nerc.ac.uk/collection/L05/current/115/"/>
<void:inDataset rdf:resource="http://vocab.nerc.ac.uk/.well-known/void"/>
</skos:Concept>
</skos:member>
<skos:member>
<skos:Concept rdf:about="http://vocab.nerc.ac.uk/collection/L22/current/TOOL0363/">
<dc:identifier>SDN:L22::TOOL0363</dc:identifier>
<skos:notation>SDN:L22::TOOL0363</skos:notation>
<skos:prefLabel xml:lang="en">Teledyne RDI Ocean Surveyor 150kHz vessel-mounted ADCP</skos:prefLabel>
<skos:altLabel>RDI OS 150kHz VM-ADCP</skos:altLabel>
<skos:definition xml:lang="en">The Teledyne RDI 150kHz Ocean Surveyor vessel-mounted acoustic Doppler current profiler is designed for continuous current profiling from a moving ship. This ADCP provides a vertical cell resolution of 4 or 8 m, a maximum range of 200-400 m, precision of 9-30 cm/s, velocity range of -5 to 9 m/s, velocity accuracy of +/-0.5 cm/s and a maximum ping rate of 1.5. It can be used in either narrowband or broadband mode.</skos:definition>
<owl:versionInfo>1</owl:versionInfo>
<dc:date>2010-12-14 15:31:03.0</dc:date>
<skos:note xml:lang="en">accepted</skos:note>
<owl:deprecated>false</owl:deprecated>
<skos:related rdf:resource="http://vocab.nerc.ac.uk/collection/P01/current/LCEWAS01/"/>
<skos:related rdf:resource="http://vocab.nerc.ac.uk/collection/P01/current/DBINAA01/"/>
<skos:related rdf:resource="http://vocab.nerc.ac.uk/collection/P01/current/LCNSAS01/"/>
<skos:broader rdf:resource="http://mmisw.org/ont/trdi/models/OceanSurveyor"/>
<skos:broader rdf:resource="http://vocab.nerc.ac.uk/collection/L05/current/115/"/>
<void:inDataset rdf:resource="http://vocab.nerc.ac.uk/.well-known/void"/>
</skos:Concept>
</skos:member>
<skos:member>
<skos:Concept rdf:about="http://vocab.nerc.ac.uk/collection/L22/current/TOOL0362/">
<dc:identifier>SDN:L22::TOOL0362</dc:identifier>
<skos:notation>SDN:L22::TOOL0362</skos:notation>
<skos:prefLabel xml:lang="en">Teledyne RDI Ocean Surveyor 75kHz vessel-mounted ADCP</skos:prefLabel>
<skos:altLabel>RDI OS 75kHz VM-ADCP</skos:altLabel>
<skos:definition xml:lang="en">The Teledyne RDI 75kHz Ocean Surveyor vessel-mounted acoustic Doppler current profiler is designed for continuous current profiling from a moving ship. This ADCP provides a vertical cell resolution of 8 or 16 m, a maximum range of 310-700 m, precision of 9-30 cm/s, velocity range of -5 to 9 m/s, velocity accuracy of +/-0.5 cm/s and a maximum ping rate of 0.7. It can be used in either narrowband or broadband mode.</skos:definition>
<owl:versionInfo>1</owl:versionInfo>
<dc:date>2010-12-14 15:31:03.0</dc:date>
<skos:note xml:lang="en">accepted</skos:note>
<owl:deprecated>false</owl:deprecated>
<skos:related rdf:resource="http://vocab.nerc.ac.uk/collection/P01/current/DBINAA01/"/>
<skos:related rdf:resource="http://vocab.nerc.ac.uk/collection/P01/current/LCEWAS01/"/>
<skos:related rdf:resource="http://vocab.nerc.ac.uk/collection/P01/current/LCNSAS01/"/>
<skos:broader rdf:resource="http://vocab.nerc.ac.uk/collection/L05/current/115/"/>
<skos:broader rdf:resource="http://mmisw.org/ont/trdi/models/OceanSurveyor"/>
<void:inDataset rdf:resource="http://vocab.nerc.ac.uk/.well-known/void"/>
</skos:Concept>
</skos:member>
<skos:member>
<skos:Concept rdf:about="http://vocab.nerc.ac.uk/collection/L22/current/TOOL0056/">
<dc:identifier>SDN:L22::TOOL0056</dc:identifier>
<skos:notation>SDN:L22::TOOL0056</skos:notation>
<skos:prefLabel xml:lang="en">Teledyne RDI Workhorse Long-Ranger ADCP</skos:prefLabel>
<skos:altLabel>RDI Workhorse Long-Ranger ADCP</skos:altLabel>
<skos:definition xml:lang="en">The Teledyne RDI Workhorse Long-Ranger acoustic doppler current profiler is a long-range and long-term self contained ADCP. It has a patented broadband signal (75 kHz) and a standard depth rating of 1500m. It operates effectively between temperatures of -5°C and 45°C and has a velocity accuracy of ±1%; ±5 mm per s</skos:definition>
<owl:versionInfo>2</owl:versionInfo>
<dc:date>2010-11-18 12:39:41.0</dc:date>
<skos:note xml:lang="en">accepted</skos:note>
<owl:deprecated>false</owl:deprecated>
<skos:broader rdf:resource="http://vocab.nerc.ac.uk/collection/L05/current/115/"/>
<owl:sameAs rdf:resource="http://mmisw.org/ont/trdi/models/LongRanger"/>
<void:inDataset rdf:resource="http://vocab.nerc.ac.uk/.well-known/void"/>
</skos:Concept>
</skos:member>
<skos:member>
<skos:Concept rdf:about="http://vocab.nerc.ac.uk/collection/L22/current/TOOL0373/">
<dc:identifier>SDN:L22::TOOL0373</dc:identifier>
<skos:notation>SDN:L22::TOOL0373</skos:notation>
<skos:prefLabel xml:lang="en">Teledyne RDI Workhorse Navigator 150 kHz Doppler Velocity Log</skos:prefLabel>
<skos:altLabel>RDI Workhorse Navigator 150kHz DVL</skos:altLabel>
<skos:definition xml:lang="en">A Doppler velocity log (DVL) measuring bottom track and water track velocities, altitude, heading, tilt, temperature and echo intensity. 150kHz Broadband signal processing gives high data resolution and a four-beam solution gives an independent error velocity measurement as an indicator of data quality. It has a bottom track range of 400m and velocity accuracy for both bottom and water track modes is 0.4% of the velocity, ±0.2cm/s. The instrument operates effectively over a temperature range of -5°C to 45°C and with a tilt of up to ±15 deg.</skos:definition>
<owl:versionInfo>1</owl:versionInfo>
<dc:date>2011-02-28 16:20:23.0</dc:date>
<skos:note xml:lang="en">accepted</skos:note>
<owl:deprecated>false</owl:deprecated>
<skos:broader rdf:resource="http://vocab.nerc.ac.uk/collection/L05/current/385/"/>
<skos:broader rdf:resource="http://vocab.nerc.ac.uk/collection/L05/current/134/"/>
<skos:broader rdf:resource="http://vocab.nerc.ac.uk/collection/L05/current/379/"/>
<void:inDataset rdf:resource="http://vocab.nerc.ac.uk/.well-known/void"/>
</skos:Concept>
</skos:member>
<skos:member>
<skos:Concept rdf:about="http://vocab.nerc.ac.uk/collection/L22/current/TOOL0372/">
<dc:identifier>SDN:L22::TOOL0372</dc:identifier>
<skos:notation>SDN:L22::TOOL0372</skos:notation>
<skos:prefLabel xml:lang="en">Teledyne RDI Workhorse Navigator 150 kHz Doppler Velocity Log and current profiler</skos:prefLabel>
<skos:altLabel>Autosub RDI Workhorse Navigator 150kHz DVL CP</skos:altLabel>
<skos:definition xml:lang="en">A Doppler velocity log (DVL) measuring bottom track and water track velocities, altitude, heading, tilt, temperature, echo intensity and current velocities. 150kHz Broadband signal processing gives high data resolution and a four-beam solution gives an independent error velocity measurement as an indicator of data quality. It has a bottom track range of 400m and velocity accuracy for both bottom and water track modes is 0.4% of the velocity, ±0.2cm/s. The instrument operates effectively over a temperature range of -5°C to 45°C and with a tilt of up to ±15 deg.</skos:definition>
<owl:versionInfo>1</owl:versionInfo>
<dc:date>2011-02-28 16:21:14.0</dc:date>
<skos:note xml:lang="en">accepted</skos:note>
<owl:deprecated>false</owl:deprecated>
<skos:broader rdf:resource="http://vocab.nerc.ac.uk/collection/L05/current/115/"/>
<skos:broader rdf:resource="http://vocab.nerc.ac.uk/collection/L05/current/134/"/>
<skos:broader rdf:resource="http://vocab.nerc.ac.uk/collection/L05/current/385/"/>
<skos:broader rdf:resource="http://vocab.nerc.ac.uk/collection/L05/current/379/"/>
<void:inDataset rdf:resource="http://vocab.nerc.ac.uk/.well-known/void"/>
</skos:Concept>
</skos:member>
<skos:member>
<skos:Concept rdf:about="http://vocab.nerc.ac.uk/collection/L22/current/TOOL0374/">
<dc:identifier>SDN:L22::TOOL0374</dc:identifier>
<skos:notation>SDN:L22::TOOL0374</skos:notation>
<skos:prefLabel xml:lang="en">Teledyne RDI Workhorse Navigator 150 kHz Doppler Velocity Log and pressure sensor</skos:prefLabel>
<skos:altLabel>RDI Workhorse Navigator 150kHz DVL PS</skos:altLabel>
<skos:definition xml:lang="en">A Doppler velocity log (DVL) measuring bottom track and water track velocities, altitude, heading, tilt, temperature, echo intensity and pressure. 150kHz Broadband signal processing gives high data resolution and a four-beam solution gives an independent error velocity measurement as an indicator of data quality. It has a bottom track range of 400m and velocity accuracy for both bottom and water track modes is 0.4% of the velocity, ±0.2cm/s. The instrument operates effectively over a temperature range of -5°C to 45°C and with a tilt of up to ±15 deg.</skos:definition>
<owl:versionInfo>1</owl:versionInfo>
<dc:date>2011-02-28 16:20:23.0</dc:date>
<skos:note xml:lang="en">accepted</skos:note>
<owl:deprecated>false</owl:deprecated>
<skos:broader rdf:resource="http://vocab.nerc.ac.uk/collection/L05/current/379/"/>
<skos:broader rdf:resource="http://vocab.nerc.ac.uk/collection/L05/current/385/"/>
<skos:broader rdf:resource="http://vocab.nerc.ac.uk/collection/L05/current/134/"/>
<void:inDataset rdf:resource="http://vocab.nerc.ac.uk/.well-known/void"/>
</skos:Concept>
</skos:member>
<skos:member>
<skos:Concept rdf:about="http://vocab.nerc.ac.uk/collection/L22/current/TOOL0375/">
<dc:identifier>SDN:L22::TOOL0375</dc:identifier>
<skos:notation>SDN:L22::TOOL0375</skos:notation>
<skos:prefLabel xml:lang="en">Teledyne RDI Workhorse Navigator 150 kHz Doppler Velocity Log, current profiler and pressure sensor</skos:prefLabel>
<skos:altLabel>RDI Workhorse Navigator 150kHz DVL CP PS</skos:altLabel>
<skos:definition xml:lang="en">A Doppler velocity log (DVL) measuring bottom track and water track velocities, altitude, heading, tilt, temperature, echo intensity, pressure and current velocities. 150kHz Broadband signal processing gives high data resolution and a four-beam solution gives an independent error velocity measurement as an indicator of data quality. It has a bottom track range of 400m and velocity accuracy for both bottom and water track modes is 0.4% of the velocity, ±0.2cm/s. The instrument operates effectively over a temperature range of -5°C to 45°C and with a tilt of up to ±15 deg.</skos:definition>
<owl:versionInfo>1</owl:versionInfo>
<dc:date>2011-02-28 16:20:23.0</dc:date>
<skos:note xml:lang="en">accepted</skos:note>
<owl:deprecated>false</owl:deprecated>
<skos:broader rdf:resource="http://vocab.nerc.ac.uk/collection/L05/current/379/"/>
<skos:broader rdf:resource="http://vocab.nerc.ac.uk/collection/L05/current/385/"/>
<skos:broader rdf:resource="http://vocab.nerc.ac.uk/collection/L05/current/115/"/>
<skos:broader rdf:resource="http://vocab.nerc.ac.uk/collection/L05/current/134/"/>
<void:inDataset rdf:resource="http://vocab.nerc.ac.uk/.well-known/void"/>
</skos:Concept>
</skos:member>
<skos:member>
<skos:Concept rdf:about="http://vocab.nerc.ac.uk/collection/L22/current/TOOL0377/">
<dc:identifier>SDN:L22::TOOL0377</dc:identifier>
<skos:notation>SDN:L22::TOOL0377</skos:notation>
<skos:prefLabel xml:lang="en">Teledyne RDI Workhorse Navigator 300 kHz Doppler Velocity Log</skos:prefLabel>
<skos:altLabel>RDI Workhorse Navigator 300kHz DVL</skos:altLabel>
<skos:definition xml:lang="en">A Doppler velocity log (DVL) measuring bottom track and water track velocities, altitude, heading, tilt, temperature and echo intensity. 300kHz Broadband signal processing gives high data resolution and a four-beam solution gives an independent error velocity measurement as an indicator of data quality. It has a bottom track range of 200m and velocity accuracy for both bottom and water track modes is 0.4% of the velocity, ±0.2cm/s. The instrument operates effectively over a temperature range of -5°C to 45°C and with a tilt of up to ±15 deg.</skos:definition>
<owl:versionInfo>1</owl:versionInfo>
<dc:date>2011-02-28 16:20:23.0</dc:date>
<skos:note xml:lang="en">accepted</skos:note>
<owl:deprecated>false</owl:deprecated>
<skos:broader rdf:resource="http://vocab.nerc.ac.uk/collection/L05/current/385/"/>
<skos:broader rdf:resource="http://vocab.nerc.ac.uk/collection/L05/current/134/"/>
<skos:broader rdf:resource="http://vocab.nerc.ac.uk/collection/L05/current/379/"/>
<void:inDataset rdf:resource="http://vocab.nerc.ac.uk/.well-known/void"/>
</skos:Concept>
</skos:member>
<skos:member>
<skos:Concept rdf:about="http://vocab.nerc.ac.uk/collection/L22/current/TOOL0376/">
<dc:identifier>SDN:L22::TOOL0376</dc:identifier>
<skos:notation>SDN:L22::TOOL0376</skos:notation>
<skos:prefLabel xml:lang="en">Teledyne RDI Workhorse Navigator 300 kHz Doppler Velocity Log and current profiler</skos:prefLabel>
<skos:altLabel>RDI Workhorse Navigator 300kHz DVL CP</skos:altLabel>
<skos:definition xml:lang="en">A Doppler velocity log (DVL) measuring bottom track and water track velocities, altitude, heading, tilt, temperature, echo intensity and current velocities. 300kHz Broadband signal processing gives high data resolution and a four-beam solution gives an independent error velocity measurement as an indicator of data quality. It has a bottom track range of 200m and velocity accuracy for both bottom and water track modes is 0.4% of the velocity, ±0.2cm/s. The instrument operates effectively over a temperature range of -5°C to 45°C and with a tilt of up to ±15 deg.</skos:definition>
<owl:versionInfo>1</owl:versionInfo>
<dc:date>2011-02-28 16:20:23.0</dc:date>
<skos:note xml:lang="en">accepted</skos:note>
<owl:deprecated>false</owl:deprecated>
<skos:broader rdf:resource="http://vocab.nerc.ac.uk/collection/L05/current/385/"/>
<skos:broader rdf:resource="http://vocab.nerc.ac.uk/collection/L05/current/379/"/>
<skos:broader rdf:resource="http://vocab.nerc.ac.uk/collection/L05/current/115/"/>
<skos:broader rdf:resource="http://vocab.nerc.ac.uk/collection/L05/current/134/"/>
<void:inDataset rdf:resource="http://vocab.nerc.ac.uk/.well-known/void"/>
</skos:Concept>
</skos:member>
<skos:member>
<skos:Concept rdf:about="http://vocab.nerc.ac.uk/collection/L22/current/TOOL0379/">
<dc:identifier>SDN:L22::TOOL0379</dc:identifier>
<skos:notation>SDN:L22::TOOL0379</skos:notation>
<skos:prefLabel xml:lang="en">Teledyne RDI Workhorse Navigator 300 kHz Doppler Velocity Log and pressure sensor</skos:prefLabel>
<skos:altLabel>RDI Workhorse Navigator 300kHz DVL PS</skos:altLabel>
<skos:definition xml:lang="en">A Doppler velocity log (DVL) measuring bottom track and water track velocities, altitude, heading, tilt, temperature, echo intensity and pressure. 300kHz Broadband signal processing gives high data resolution and a four-beam solution gives an independent error velocity measurement as an indicator of data quality. It has a bottom track range of 200m and velocity accuracy for both bottom and water track modes is 0.4% of the velocity, ±0.2cm/s. The instrument operates effectively over a temperature range of -5°C to 45°C and with a tilt of up to ±15 deg.</skos:definition>
<owl:versionInfo>1</owl:versionInfo>
<dc:date>2011-02-28 16:20:23.0</dc:date>
<skos:note xml:lang="en">accepted</skos:note>
<owl:deprecated>false</owl:deprecated>
<skos:broader rdf:resource="http://vocab.nerc.ac.uk/collection/L05/current/379/"/>
<skos:broader rdf:resource="http://vocab.nerc.ac.uk/collection/L05/current/385/"/>
<skos:broader rdf:resource="http://vocab.nerc.ac.uk/collection/L05/current/134/"/>
<void:inDataset rdf:resource="http://vocab.nerc.ac.uk/.well-known/void"/>
</skos:Concept>
</skos:member>
<skos:member>
<skos:Concept rdf:about="http://vocab.nerc.ac.uk/collection/L22/current/TOOL0378/">
<dc:identifier>SDN:L22::TOOL0378</dc:identifier>
<skos:notation>SDN:L22::TOOL0378</skos:notation>
<skos:prefLabel xml:lang="en">Teledyne RDI Workhorse Navigator 300 kHz Doppler Velocity Log, current profiler and pressure sensor</skos:prefLabel>
<skos:altLabel>RDI Workhorse Navigator 300kHz DVL CP PS</skos:altLabel>
<skos:definition xml:lang="en">A Doppler velocity log (DVL) measuring bottom track and water track velocities, altitude, heading, tilt, temperature, echo intensity, pressure and current velocities. 300kHz Broadband signal processing gives high data resolution and a four-beam solution gives an independent error velocity measurement as an indicator of data quality. It has a bottom track range of 200m and velocity accuracy for both bottom and water track modes is 0.4% of the velocity, ±0.2cm/s. The instrument operates effectively over a temperature range of -5°C to 45°C and with a tilt of up to ±15 deg.</skos:definition>
<owl:versionInfo>1</owl:versionInfo>
<dc:date>2011-02-28 16:20:23.0</dc:date>
<skos:note xml:lang="en">accepted</skos:note>
<owl:deprecated>false</owl:deprecated>
<skos:broader rdf:resource="http://vocab.nerc.ac.uk/collection/L05/current/115/"/>
<skos:broader rdf:resource="http://vocab.nerc.ac.uk/collection/L05/current/385/"/>
<skos:broader rdf:resource="http://vocab.nerc.ac.uk/collection/L05/current/134/"/>
<skos:broader rdf:resource="http://vocab.nerc.ac.uk/collection/L05/current/379/"/>
<void:inDataset rdf:resource="http://vocab.nerc.ac.uk/.well-known/void"/>
</skos:Concept>
</skos:member>
<skos:member>
<skos:Concept rdf:about="http://vocab.nerc.ac.uk/collection/L22/current/TOOL0293/">
<dc:identifier>SDN:L22::TOOL0293</dc:identifier>
<skos:notation>SDN:L22::TOOL0293</skos:notation>
<skos:prefLabel xml:lang="en">Teledyne RDI Workhorse Sentinel-1200 ADCP</skos:prefLabel>
<skos:altLabel>RDI Workhorse Sentinel-1200 ADCP</skos:altLabel>
<skos:definition xml:lang="en">An ADCP designed for self-contained use on moorings or vessel mounting. It has a patented 1200 kHz broadband signal and a standard depth rating of 200 metres. It operates effectively between temperatures of -5 to 45 C and a range of up to 20m with a depth cell size of 2m.Velocity accuracy is +/- 0.3% or 0.3 cm/sec.</skos:definition>
<owl:versionInfo>2</owl:versionInfo>
<dc:date>2013-08-22 12:43:30.0</dc:date>
<skos:note xml:lang="en">accepted</skos:note>
<owl:deprecated>false</owl:deprecated>
<skos:broader rdf:resource="http://vocab.nerc.ac.uk/collection/L05/current/115/"/>
<skos:broader rdf:resource="http://mmisw.org/ont/trdi/models/Sentinel"/>
<void:inDataset rdf:resource="http://vocab.nerc.ac.uk/.well-known/void"/>
</skos:Concept>
</skos:member>
<skos:member>
<skos:Concept rdf:about="http://vocab.nerc.ac.uk/collection/L22/current/TOOL0295/">
<dc:identifier>SDN:L22::TOOL0295</dc:identifier>
<skos:notation>SDN:L22::TOOL0295</skos:notation>
<skos:prefLabel xml:lang="en">Teledyne RDI Workhorse Sentinel-300 ADCP</skos:prefLabel>
<skos:altLabel>RDI Workhorse Sentinel-300 ADCP</skos:altLabel>
<skos:definition xml:lang="en">An ADCP designed for self-contained use on moorings or vessel mounting. It has a patented 300 kHz broadband signal and a standard depth rating of 200 metres. It operates effectively between temperatures of -5 to 45 C and a range of up to 165m with a depth cell size of 8m.Velocity accuracy is +/- 0.5% or 0.5 cm/sec.</skos:definition>
<owl:versionInfo>2</owl:versionInfo>
<dc:date>2013-08-22 12:43:47.0</dc:date>
<skos:note xml:lang="en">accepted</skos:note>
<owl:deprecated>false</owl:deprecated>
<skos:broader rdf:resource="http://vocab.nerc.ac.uk/collection/L05/current/115/"/>
<skos:broader rdf:resource="http://mmisw.org/ont/trdi/models/Sentinel"/>
<void:inDataset rdf:resource="http://vocab.nerc.ac.uk/.well-known/void"/>
</skos:Concept>
</skos:member>
<skos:member>
<skos:Concept rdf:about="http://vocab.nerc.ac.uk/collection/L22/current/TOOL0294/">
<dc:identifier>SDN:L22::TOOL0294</dc:identifier>
<skos:notation>SDN:L22::TOOL0294</skos:notation>
<skos:prefLabel xml:lang="en">Teledyne RDI Workhorse Sentinel-600 ADCP</skos:prefLabel>
<skos:altLabel>RDI Workhorse Sentinel-600 ADCP</skos:altLabel>
<skos:definition xml:lang="en">An ADCP designed for self-contained use on moorings or vessel mounting. It has a patented 600 kHz broadband signal and a standard depth rating of 200 metres. It operates effectively between temperatures of -5 to 45 C and a range of up to 70m with a depth cell size of 4m.Velocity accuracy is +/- 0.3% or 0.3 cm/sec.</skos:definition>
<owl:versionInfo>2</owl:versionInfo>
<dc:date>2013-08-22 12:43:39.0</dc:date>
<skos:note xml:lang="en">accepted</skos:note>
<owl:deprecated>false</owl:deprecated>
<skos:broader rdf:resource="http://mmisw.org/ont/trdi/models/Sentinel"/>
<skos:broader rdf:resource="http://vocab.nerc.ac.uk/collection/L05/current/115/"/>
<void:inDataset rdf:resource="http://vocab.nerc.ac.uk/.well-known/void"/>
</skos:Concept>
</skos:member>
<skos:member>
<skos:Concept rdf:about="http://vocab.nerc.ac.uk/collection/L22/current/TOOL0636/">
<dc:identifier>SDN:L22::TOOL0636</dc:identifier>
<skos:notation>SDN:L22::TOOL0636</skos:notation>
<skos:prefLabel xml:lang="en">Teledyne RDI Workhorse Waves Array</skos:prefLabel>
<skos:altLabel>RDI Workhorse Waves Array</skos:altLabel>
<skos:definition xml:lang="en">An optional upgrade package that may be fitted to RDI Workhorse Sentinel, Monitor, H-ADCP or Express ADCP that measures multi-directional wave parameters derived from acoustic measurements of wave orbital velocities. The process is fully described in https://www.bodc.ac.uk/data/documents/nodb/pdf/waveprimer.pdf.</skos:definition>
<owl:versionInfo>1</owl:versionInfo>
<dc:date>2013-08-22 12:53:42.0</dc:date>
<skos:note xml:lang="en">accepted</skos:note>
<owl:deprecated>false</owl:deprecated>
<skos:broader rdf:resource="http://vocab.nerc.ac.uk/collection/L05/current/110/"/>
<void:inDataset rdf:resource="http://vocab.nerc.ac.uk/.well-known/void"/>
</skos:Concept>
</skos:member>
<skos:member>
<skos:Concept rdf:about="http://vocab.nerc.ac.uk/collection/L22/current/TOOL0621/">
<dc:identifier>SDN:L22::TOOL0621</dc:identifier>
<skos:notation>SDN:L22::TOOL0621</skos:notation>
<skos:prefLabel xml:lang="en">Teleost Pressure Recorder</skos:prefLabel>
<skos:altLabel>Teleost BPR</skos:altLabel>
<skos:definition xml:lang="en">A pressure recorder developed by the Institute of Oceanographic Sciences Bidston Laboratory in the late 1970s to measure sea level at offshore locations. It comprised a Bell and Howell strain gauge or a Digiquartz pressure transducer with an optional platinum resistance thermometer. Data were logged by an adapted Aanderaa current meter logger. More information is available at http://www.bodc.ac.uk/data/documents/nodb/27840/.</skos:definition>
<owl:versionInfo>1</owl:versionInfo>
<dc:date>2013-06-04 16:11:11.0</dc:date>
<skos:note xml:lang="en">accepted</skos:note>
<owl:deprecated>false</owl:deprecated>
<skos:broader rdf:resource="http://vocab.nerc.ac.uk/collection/L05/current/111/"/>
<skos:broader rdf:resource="http://vocab.nerc.ac.uk/collection/L05/current/134/"/>
<void:inDataset rdf:resource="http://vocab.nerc.ac.uk/.well-known/void"/>
</skos:Concept>
</skos:member>
<skos:member>
<skos:Concept rdf:about="http://vocab.nerc.ac.uk/collection/L22/current/TOOL0221/">
<dc:identifier>SDN:L22::TOOL0221</dc:identifier>
<skos:notation>SDN:L22::TOOL0221</skos:notation>
<skos:prefLabel xml:lang="en">Texas Electronics TE525 rain gauge</skos:prefLabel>
<skos:altLabel>TE525 rain gauge</skos:altLabel>
<skos:definition xml:lang="en">A tipping bucket rain gauge with a 6 inch collector and levelling screw adjustment. The sensor output has a switch closure for each bucket tip. It has a resolution of 0.01 inches and accuracy of between 1 and 5% depending on rainfall rate (more accurate for lighter rainfall). Marketed by Campbell Scientific.</skos:definition>
<owl:versionInfo>1</owl:versionInfo>
<dc:date>2010-05-18 16:10:58.0</dc:date>
<skos:note xml:lang="en">accepted</skos:note>
<owl:deprecated>false</owl:deprecated>
<skos:broader rdf:resource="http://vocab.nerc.ac.uk/collection/L05/current/381/"/>
<void:inDataset rdf:resource="http://vocab.nerc.ac.uk/.well-known/void"/>
</skos:Concept>
</skos:member>
<skos:member>
<skos:Concept rdf:about="http://vocab.nerc.ac.uk/collection/L22/current/NETT0149/">
<dc:identifier>SDN:L22::NETT0149</dc:identifier>
<skos:notation>SDN:L22::NETT0149</skos:notation>
<skos:prefLabel xml:lang="en">The National Institute of Oceanography Rectangular Midwater Trawl combination net 1+8  - Baker et al. (1973)</skos:prefLabel>
<skos:altLabel>RMT 1+8</skos:altLabel>
<skos:definition xml:lang="en">A combination 100 cm x 141 cm rectangular flexible  mouth opening net and one with a 283 cm x 400 cm mouth opening, one above the other on the same towing framework. The 8-m2 as described by Clarke . The 1-m2 was 423 cm long and had 0.32 mm nylon mesh. Data telemetry improved to include temperature and flow. Descriptions of scaled up versions of the RMT 8 to  25-m2 and  90-m2 mouth openings provided [Wiebe and Benfield 2003 Plate 28 A].</skos:definition>
<owl:versionInfo>2</owl:versionInfo>
<dc:date>2012-06-21 13:49:01.0</dc:date>
<skos:note xml:lang="en">accepted</skos:note>
<owl:deprecated>false</owl:deprecated>
<skos:broader rdf:resource="http://vocab.nerc.ac.uk/collection/L05/current/134/"/>
<skos:broader rdf:resource="http://vocab.nerc.ac.uk/collection/L05/current/68/"/>
<skos:broader rdf:resource="http://vocab.nerc.ac.uk/collection/L05/current/23/"/>
<skos:broader rdf:resource="http://vocab.nerc.ac.uk/collection/L05/current/388/"/>
<void:inDataset rdf:resource="http://vocab.nerc.ac.uk/.well-known/void"/>
</skos:Concept>
</skos:member>
<skos:member>
<skos:Concept rdf:about="http://vocab.nerc.ac.uk/collection/L22/current/TOOL0296/">
<dc:identifier>SDN:L22::TOOL0296</dc:identifier>
<skos:notation>SDN:L22::TOOL0296</skos:notation>
<skos:prefLabel xml:lang="en">Thermo Scientific 5012 Multi Angle Absorption Photometer</skos:prefLabel>
<skos:altLabel>Thermo 5012 MAAP</skos:altLabel>
<skos:definition xml:lang="en">An in-situ instrument that determines atmospheric aerosol light absorption from coincident measurements of light scattering and transmission of continuous samples collected on a GF10 filter tape. The detection limit is 0.05ug m-3 for data averaged over 10 minutes.</skos:definition>
<owl:versionInfo>1</owl:versionInfo>
<dc:date>2010-05-18 16:10:58.0</dc:date>
<skos:note xml:lang="en">accepted</skos:note>
<owl:deprecated>false</owl:deprecated>
<skos:broader rdf:resource="http://vocab.nerc.ac.uk/collection/L05/current/ATRANS/"/>
<void:inDataset rdf:resource="http://vocab.nerc.ac.uk/.well-known/void"/>
</skos:Concept>
</skos:member>
<skos:member>
<skos:Concept rdf:about="http://vocab.nerc.ac.uk/collection/L22/current/TOOL0565/">
<dc:identifier>SDN:L22::TOOL0565</dc:identifier>
<skos:notation>SDN:L22::TOOL0565</skos:notation>
<skos:prefLabel xml:lang="en">Thermo VG PQ ExCell Inductively Coupled Plasma Mass Spectrometer</skos:prefLabel>
<skos:altLabel>Thermo VG PQ ExCell ICP-MS</skos:altLabel>
<skos:definition xml:lang="en">A quadrupole-based inductively coupled plasma mass spectrometer (ICP-MS) designed for the determination of trace elements in a range of sample types. The instrument comprises a sample introduction system including a peristaltic pump, a peltier cooled pnuematic nebulisation system, a one-piece quartz torch, mass flow controllers and a solid-state RF generator. There is an interface of two cones which sample the ions created in the plasma and provide an ion skimming function. Cylindrical electrodes are then used to extract and focus ions from the interface into the mass spectrometer. The instrument includes a vacuum pumping system, argon backfill system and an autorange standard detector system. There is a high efficiency ion guide and chicane deflector coupled to an off-axis quadrupole mass analyser known as the Infinity Lens System which reduces background noise. The ICP-MS is fully automated and is operated using PlasmaLab software. Optional extras include collision cell technology, choice of detectors, 4th gas supply with mass flow controller, organic matrix sample option, S-Option interface technology and a range of sampling accessories. This model was released in 1999 and was replaced by the XSERIES in 2001.</skos:definition>
<owl:versionInfo>1</owl:versionInfo>
<dc:date>2012-10-22 13:48:32.0</dc:date>
<skos:note xml:lang="en">accepted</skos:note>
<owl:deprecated>false</owl:deprecated>
<skos:broader rdf:resource="http://vocab.nerc.ac.uk/collection/L05/current/LAB15/"/>
<void:inDataset rdf:resource="http://vocab.nerc.ac.uk/.well-known/void"/>
</skos:Concept>
</skos:member>
<skos:member>
<skos:Concept rdf:about="http://vocab.nerc.ac.uk/collection/L22/current/TOOL0486/">
<dc:identifier>SDN:L22::TOOL0486</dc:identifier>
<skos:notation>SDN:L22::TOOL0486</skos:notation>
<skos:prefLabel xml:lang="en">ThermoFinnigan AS3000 Autosampler</skos:prefLabel>
<skos:altLabel>ThermoF AS3000 autosampler</skos:altLabel>
<skos:definition xml:lang="en">A laboratory autosampler for automatic routine sampling and complete sample preparation. The instrument includes a sample tray, injector and column oven, all of which are precisely temperature-controlled. It features a 120 vial capacity with random vial access and multiple injection modes to maximise sampling flexibility. Unique sample withdrawal and automatic flush procedures minimise cross contamination between samples, typically less than 0.01% with a 400 uL flush volume. RSD precision is better than 0.5%. The instrument was designed for use with the SpectraSYSTEM HPLC. The instrument was originally manufactured by Thermo Finnigan, which was replaced by Thermo Electron and later Thermo Scientific (part of Thermo Fisher Scientific).</skos:definition>
<owl:versionInfo>1</owl:versionInfo>
<dc:date>2012-03-29 16:25:41.0</dc:date>
<skos:note xml:lang="en">accepted</skos:note>
<owl:deprecated>false</owl:deprecated>
<skos:broader rdf:resource="http://vocab.nerc.ac.uk/collection/L05/current/LAB33/"/>
<skos:broader rdf:resource="http://vocab.nerc.ac.uk/collection/L22/current/TOOL0487/"/>
<void:inDataset rdf:resource="http://vocab.nerc.ac.uk/.well-known/void"/>
</skos:Concept>
</skos:member>
<skos:member>
<skos:Concept rdf:about="http://vocab.nerc.ac.uk/collection/L22/current/TOOL0532/">
<dc:identifier>SDN:L22::TOOL0532</dc:identifier>
<skos:notation>SDN:L22::TOOL0532</skos:notation>
<skos:prefLabel xml:lang="en">ThermoFinnigan EA 1112 Flash Elemental Analyser</skos:prefLabel>
<skos:altLabel>ThermoF EA 1112</skos:altLabel>
<skos:definition xml:lang="en">A laboratory instrument used to determine total carbon, hydrogen, nitrogen, sulphur and oxygen in a sample. The sample is completely and instantaneously oxidised by flash combustion, which converts all organic and inorganic substances into combustion products. The resulting combustion gases pass through a reduction furnace and are swept into the chromatographic column by the helium carrier gas. The gases are separated in the column and detected by the thermal conductivity detector which gives an output signal proportional to the concentration of the individual components of the mixture. ThermoFinnigan is part of Thermo Fisher Scientific.</skos:definition>
<owl:versionInfo>1</owl:versionInfo>
<dc:date>2012-08-21 12:05:06.0</dc:date>
<skos:note xml:lang="en">accepted</skos:note>
<owl:deprecated>false</owl:deprecated>
<skos:broader rdf:resource="http://vocab.nerc.ac.uk/collection/L05/current/LAB01/"/>
<void:inDataset rdf:resource="http://vocab.nerc.ac.uk/.well-known/void"/>
</skos:Concept>
</skos:member>
<skos:member>
<skos:Concept rdf:about="http://vocab.nerc.ac.uk/collection/L22/current/TOOL0462/">
<dc:identifier>SDN:L22::TOOL0462</dc:identifier>
<skos:notation>SDN:L22::TOOL0462</skos:notation>
<skos:prefLabel xml:lang="en">ThermoFinnigan Neptune inductively coupled plasma mass spectrometer</skos:prefLabel>
<skos:altLabel>Neptune ICP-MS</skos:altLabel>
<skos:definition xml:lang="en">A laboratory high mass resolution inductively coupled plasma mass spectrometer (ICP-MS) designed for elemental and isotopic analysis. The instrument is based on a multicollector platform, comprising eight moveable collector supports and one fixed center channel equipped with a Faraday cup and, optionally, an ion counter with or without a retardation lens. The Faraday cup is connected to a current amplifier, whose signal is digitized by a high linearity voltage to frequency converter. The instrument was originally manufactured by Thermo Finnigan, which has since been replaced by Thermo Scientific (part of Thermo Fisher Scientific). This model is no longer in production.</skos:definition>
<owl:versionInfo>1</owl:versionInfo>
<dc:date>2012-02-16 10:05:14.0</dc:date>
<skos:note xml:lang="en">accepted</skos:note>
<owl:deprecated>false</owl:deprecated>
<skos:broader rdf:resource="http://vocab.nerc.ac.uk/collection/L05/current/LAB15/"/>
<void:inDataset rdf:resource="http://vocab.nerc.ac.uk/.well-known/void"/>
</skos:Concept>
</skos:member>
<skos:member>
<skos:Concept rdf:about="http://vocab.nerc.ac.uk/collection/L22/current/TOOL0487/">
<dc:identifier>SDN:L22::TOOL0487</dc:identifier>
<skos:notation>SDN:L22::TOOL0487</skos:notation>
<skos:prefLabel xml:lang="en">ThermoFinnigan SpectraSYSTEM High Performance Liquid Chromatograph</skos:prefLabel>
<skos:altLabel>ThermoF Spectra HPLC</skos:altLabel>
<skos:definition xml:lang="en">The SpectraSYSTEM is designed for automated sample preparation and HPLC analysis. It comprises a series of modules, including a range of degassers, pumps, autosamplers and detectors. The solvent is delivered by a pump featuring a real-time pressure feedback and automatic solvent compressibility system optimized to provide accurate and precise pump flows, regardless of solvent composition. SpectraSYSTEM pumps are designed for flow rates of 10 uL to 10 mL/min (flow rate precision &lt; 0.2% RSD) and feature excellent gradient accuracy and linearity. The SpectraSYSTEM includes an autosampler with a 120 vial capacityThe SpectraSYSTEM can be fitted with a variety of detectors, including UV/Visible (deuterium and tungsten lamps), photodiode array (deuterium and tungsten-halogen lamps) and fluorescence (pulsed xenon lamps) spectrometers. The instrument was originally manufactured by Thermo Finnigan, which was replaced by Thermo Electron and later Thermo Scientific (part of Thermo Fisher Scientific).</skos:definition>
<owl:versionInfo>1</owl:versionInfo>
<dc:date>2012-03-29 16:25:41.0</dc:date>
<skos:note xml:lang="en">accepted</skos:note>
<owl:deprecated>false</owl:deprecated>
<skos:narrower rdf:resource="http://vocab.nerc.ac.uk/collection/L22/current/TOOL0488/"/>
<skos:narrower rdf:resource="http://vocab.nerc.ac.uk/collection/L22/current/TOOL0486/"/>
<skos:broader rdf:resource="http://vocab.nerc.ac.uk/collection/L05/current/LAB33/"/>
<skos:broader rdf:resource="http://vocab.nerc.ac.uk/collection/L05/current/LAB20/"/>
<skos:broader rdf:resource="http://vocab.nerc.ac.uk/collection/L05/current/LAB11/"/>
<void:inDataset rdf:resource="http://vocab.nerc.ac.uk/.well-known/void"/>
</skos:Concept>
</skos:member>
<skos:member>
<skos:Concept rdf:about="http://vocab.nerc.ac.uk/collection/L22/current/TOOL0488/">
<dc:identifier>SDN:L22::TOOL0488</dc:identifier>
<skos:notation>SDN:L22::TOOL0488</skos:notation>
<skos:prefLabel xml:lang="en">ThermoFinnigan UV6000LP photodiode array detector</skos:prefLabel>
<skos:altLabel>ThermoF UV6000LP detector</skos:altLabel>
<skos:definition xml:lang="en">A UV/Visible programmable detector designed for spectroscopic applications. It uses a linear array of discrete photodiodes and allows a range of wavelengths to be detected simultaneously. A LightPipe flowcell produces higher signal-to-noise ratio than standard flowcells, while deuterium and tungsten-halogen lamps increase light level across the full spectral range from 190-800 nm. Noise is lower than 6 uAU/cm of pathlength and a unique fiber-optic bundle creates a high resolution image with minimal light loss. The instrument was designed for use with the SpectraSYSTEM HPLC. The instrument was originally manufactured by Thermo Finnigan, which was replaced by Thermo Electron and later Thermo Scientific (part of Thermo Fisher Scientific).</skos:definition>
<owl:versionInfo>2</owl:versionInfo>
<dc:date>2012-05-21 12:01:02.0</dc:date>
<skos:note xml:lang="en">accepted</skos:note>
<owl:deprecated>false</owl:deprecated>
<skos:broader rdf:resource="http://vocab.nerc.ac.uk/collection/L22/current/TOOL0487/"/>
<skos:broader rdf:resource="http://vocab.nerc.ac.uk/collection/L05/current/LAB20/"/>
<void:inDataset rdf:resource="http://vocab.nerc.ac.uk/.well-known/void"/>
</skos:Concept>
</skos:member>
<skos:member>
<skos:Concept rdf:about="http://vocab.nerc.ac.uk/collection/L22/current/TOOL0581/">
<dc:identifier>SDN:L22::TOOL0581</dc:identifier>
<skos:notation>SDN:L22::TOOL0581</skos:notation>
<skos:prefLabel xml:lang="en">ThermoQuest Finnigan Trace Mass Spectrometer</skos:prefLabel>
<skos:altLabel>ThermoQ Finnigan Trace MS</skos:altLabel>
<skos:definition xml:lang="en">The ThermoQuest Finnigan Trace Mass Spectrometer (MS) is an analytical laboratory instrument that identifies and quantifies chemical compounds. An ion source converts the sample molecules into ions using Electron Ionization (EI) or Chemical Ionization (CI+ and CI-), which then pass into the quadrupole mass analyser which separates the ions, the detector then measures their mass-to-charge ratio and intensity. Pure samples may also be injected directly into the MS. The instrument is not suited to dealing with mixtures of compounds, therefore it is usually coupled with a gas chromatograph (typically a ThermoQuest Trace 2000 GC) which separates the compounds first. The Finnigan Trace MS was originally manufactured by ThermoQuest which has since been replaced by Thermo Scientific (part of Thermo Fisher Scientific). This model is no longer in production.</skos:definition>
<owl:versionInfo>1</owl:versionInfo>
<dc:date>2013-01-08 11:52:24.0</dc:date>
<skos:note xml:lang="en">accepted</skos:note>
<owl:deprecated>false</owl:deprecated>
<skos:broader rdf:resource="http://vocab.nerc.ac.uk/collection/L05/current/LAB16/"/>
<void:inDataset rdf:resource="http://vocab.nerc.ac.uk/.well-known/void"/>
</skos:Concept>
</skos:member>
<skos:member>
<skos:Concept rdf:about="http://vocab.nerc.ac.uk/collection/L22/current/TOOL0466/">
<dc:identifier>SDN:L22::TOOL0466</dc:identifier>
<skos:notation>SDN:L22::TOOL0466</skos:notation>
<skos:prefLabel xml:lang="en">ThermoQuest TSQ 7000 Mass Spectrometer</skos:prefLabel>
<skos:altLabel>ThermoQ TSQ 7000 Mass Spectrometer</skos:altLabel>
<skos:definition xml:lang="en">A laboratory instrument which identifies and quantifies the compounds present in a sample based on mass measurements. It is a triple quadrupole mass spectrometer designed for use with an electro-spray ionisation source. It is usually coupled with a ThermoQuest gas chromatograph, which separates the chemical species. The instrument was originally manufactured by ThermoQuest, which has since been replaced by Thermo Scientific (part of Thermo Fisher Scientific). This model is no longer in production.</skos:definition>
<owl:versionInfo>1</owl:versionInfo>
<dc:date>2012-02-21 16:06:42.0</dc:date>
<skos:note xml:lang="en">accepted</skos:note>
<owl:deprecated>false</owl:deprecated>
<skos:broader rdf:resource="http://vocab.nerc.ac.uk/collection/L05/current/LAB16/"/>
<void:inDataset rdf:resource="http://vocab.nerc.ac.uk/.well-known/void"/>
</skos:Concept>
</skos:member>
<skos:member>
<skos:Concept rdf:about="http://vocab.nerc.ac.uk/collection/L22/current/TOOL0465/">
<dc:identifier>SDN:L22::TOOL0465</dc:identifier>
<skos:notation>SDN:L22::TOOL0465</skos:notation>
<skos:prefLabel xml:lang="en">ThermoQuest Trace 2000 Gas Chromatograph</skos:prefLabel>
<skos:altLabel>ThermoQ T-2000 Gas Chromatograph</skos:altLabel>
<skos:definition xml:lang="en">A gas chromatograph that separates mixtures of chemical species on the basis of their relative affinities for a mobile gaseous phase and a stationary liquid phase. The instrument includes a split/splitless injector, capillary or wide bore columns and a detector. Possible detector types are flame ionisation, flame photometric, photo-ionisation and photo-multiplier. It is usually coupled with a ThermoQuest mass spectrometer, which identifies and quantifies the compounds. The instrument was originally manufactured by ThermoQuest which has since been replaced by Thermo Scientific (part of Thermo Fisher Scientific). This model is no longer in production.</skos:definition>
<owl:versionInfo>2</owl:versionInfo>
<dc:date>2012-12-20 16:00:07.0</dc:date>
<skos:note xml:lang="en">accepted</skos:note>
<owl:deprecated>false</owl:deprecated>
<skos:broader rdf:resource="http://vocab.nerc.ac.uk/collection/L05/current/LAB02/"/>
<void:inDataset rdf:resource="http://vocab.nerc.ac.uk/.well-known/void"/>
</skos:Concept>
</skos:member>
<skos:member>
<skos:Concept rdf:about="http://vocab.nerc.ac.uk/collection/L22/current/TOOL0543/">
<dc:identifier>SDN:L22::TOOL0543</dc:identifier>
<skos:notation>SDN:L22::TOOL0543</skos:notation>
<skos:prefLabel xml:lang="en">Transparent sample bottle</skos:prefLabel>
<skos:altLabel>Transparent sample bottle</skos:altLabel>
<skos:definition xml:lang="en">Sampling bottle of unknown material that posseses the physical property of allowing the transmission of light with little or no intereference.</skos:definition>
<owl:versionInfo>1</owl:versionInfo>
<dc:date>2012-09-26 16:33:22.0</dc:date>
<skos:note xml:lang="en">accepted</skos:note>
<owl:deprecated>false</owl:deprecated>
<skos:broader rdf:resource="http://vocab.nerc.ac.uk/collection/L05/current/30/"/>
<void:inDataset rdf:resource="http://vocab.nerc.ac.uk/.well-known/void"/>
</skos:Concept>
</skos:member>
<skos:member>
<skos:Concept rdf:about="http://vocab.nerc.ac.uk/collection/L22/current/TOOL0313/">
<dc:identifier>SDN:L22::TOOL0313</dc:identifier>
<skos:notation>SDN:L22::TOOL0313</skos:notation>
<skos:prefLabel xml:lang="en">Trimble 4000AX Global Positioning System receiver</skos:prefLabel>
<skos:altLabel>Trimble 4000AX GPS</skos:altLabel>
<skos:definition xml:lang="en">A GPS receiver in use on research vessels in the 1990s. Sampling rate reported in cruise report literature as approximately 1 second</skos:definition>
<owl:versionInfo>1</owl:versionInfo>
<dc:date>2010-09-06 12:45:22.0</dc:date>
<skos:note xml:lang="en">accepted</skos:note>
<owl:deprecated>false</owl:deprecated>
<skos:broader rdf:resource="http://vocab.nerc.ac.uk/collection/L05/current/POS03/"/>
<void:inDataset rdf:resource="http://vocab.nerc.ac.uk/.well-known/void"/>
</skos:Concept>
</skos:member>
<skos:member>
<skos:Concept rdf:about="http://vocab.nerc.ac.uk/collection/L22/current/TOOL0391/">
<dc:identifier>SDN:L22::TOOL0391</dc:identifier>
<skos:notation>SDN:L22::TOOL0391</skos:notation>
<skos:prefLabel xml:lang="en">Trimble 4000DL Global Positioning System receiver</skos:prefLabel>
<skos:altLabel>Trimble 4000DL GPS</skos:altLabel>
<skos:definition xml:lang="en">A differential GPS receiver used on research vessels during the 1990s and early 2000s. Cruise literature reports that this instrument used an 8-channel receiver. Maximum sampling rate is recorded as approximately 1 Hz.</skos:definition>
<owl:versionInfo>1</owl:versionInfo>
<dc:date>2011-04-14 09:29:16.0</dc:date>
<skos:note xml:lang="en">accepted</skos:note>
<owl:deprecated>false</owl:deprecated>
<skos:broader rdf:resource="http://vocab.nerc.ac.uk/collection/L05/current/POS04/"/>
<void:inDataset rdf:resource="http://vocab.nerc.ac.uk/.well-known/void"/>
</skos:Concept>
</skos:member>
<skos:member>
<skos:Concept rdf:about="http://vocab.nerc.ac.uk/collection/L22/current/TOOL0482/">
<dc:identifier>SDN:L22::TOOL0482</dc:identifier>
<skos:notation>SDN:L22::TOOL0482</skos:notation>
<skos:prefLabel xml:lang="en">Trimble Applanix POSMV global positioning system</skos:prefLabel>
<skos:altLabel>Applanix POSMV GPS</skos:altLabel>
<skos:definition xml:lang="en">The Position and Orientation Systems for Marine Vessels (POSMV) is a real time kinematic (RTK) and differential global positioning system (DGPS) receiver for marine navigation. It includes an inertial system that provides platform attitude information. The instrument provides accurate location, heading, velocity, attitude, heave, acceleration and angular rate measurements.</skos:definition>
<owl:versionInfo>1</owl:versionInfo>
<dc:date>2012-03-19 13:44:14.0</dc:date>
<skos:note xml:lang="en">accepted</skos:note>
<owl:deprecated>false</owl:deprecated>
<skos:related rdf:resource="http://vocab.nerc.ac.uk/collection/P01/current/ALATGP01/"/>
<skos:related rdf:resource="http://vocab.nerc.ac.uk/collection/P01/current/ALATPM01/"/>
<skos:related rdf:resource="http://vocab.nerc.ac.uk/collection/P01/current/ALONPM01/"/>
<skos:related rdf:resource="http://vocab.nerc.ac.uk/collection/P01/current/ALONGP01/"/>
<skos:broader rdf:resource="http://vocab.nerc.ac.uk/collection/L05/current/POS19/"/>
<skos:broader rdf:resource="http://vocab.nerc.ac.uk/collection/L05/current/POS04/"/>
<skos:broader rdf:resource="http://vocab.nerc.ac.uk/collection/L05/current/POS25/"/>
<void:inDataset rdf:resource="http://vocab.nerc.ac.uk/.well-known/void"/>
</skos:Concept>
</skos:member>
<skos:member>
<skos:Concept rdf:about="http://vocab.nerc.ac.uk/collection/L22/current/TOOL0199/">
<dc:identifier>SDN:L22::TOOL0199</dc:identifier>
<skos:notation>SDN:L22::TOOL0199</skos:notation>
<skos:prefLabel xml:lang="en">Trimble NT300D Global Positioning System receiver</skos:prefLabel>
<skos:altLabel>Trimble NT300D GPS</skos:altLabel>
<skos:definition xml:lang="en">A high-performance, sub-meter position GPS receiver for marine applications. It combines a state-of-the-art, 12-channel GPS receiver and a high-performance dual-channel transmitter. It was discontinued in 2009.</skos:definition>
<owl:versionInfo>1</owl:versionInfo>
<dc:date>2010-05-18 16:10:58.0</dc:date>
<skos:note xml:lang="en">accepted</skos:note>
<owl:deprecated>false</owl:deprecated>
<skos:broader rdf:resource="http://vocab.nerc.ac.uk/collection/L05/current/POS03/"/>
<void:inDataset rdf:resource="http://vocab.nerc.ac.uk/.well-known/void"/>
</skos:Concept>
</skos:member>
<skos:member>
<skos:Concept rdf:about="http://vocab.nerc.ac.uk/collection/L22/current/TOOL0059/">
<dc:identifier>SDN:L22::TOOL0059</dc:identifier>
<skos:notation>SDN:L22::TOOL0059</skos:notation>
<skos:prefLabel xml:lang="en">Tritech PA-200 Altimeter</skos:prefLabel>
<skos:altLabel>TPA200 Altimeter</skos:altLabel>
<skos:definition xml:lang="en">Digital precision altimeter with 200kHz signal giving highly accurate height off seabed and subsea distance measurements. Operates effectively between -10°C and 40°C at heights up to 100m above the seabed. Standard depth rating 4000m.</skos:definition>
<owl:versionInfo>1</owl:versionInfo>
<dc:date>2009-11-30 11:56:35.0</dc:date>
<skos:note xml:lang="en">accepted</skos:note>
<owl:deprecated>false</owl:deprecated>
<skos:broader rdf:resource="http://vocab.nerc.ac.uk/collection/L05/current/379/"/>
<void:inDataset rdf:resource="http://vocab.nerc.ac.uk/.well-known/void"/>
</skos:Concept>
</skos:member>
<skos:member>
<skos:Concept rdf:about="http://vocab.nerc.ac.uk/collection/L22/current/NETT0161/">
<dc:identifier>SDN:L22::NETT0161</dc:identifier>
<skos:notation>SDN:L22::NETT0161</skos:notation>
<skos:prefLabel xml:lang="en">Tucker Trawl - Tucker (1951)</skos:prefLabel>
<skos:altLabel>Tucker Trawl</skos:altLabel>
<skos:definition xml:lang="en">Has a  183 cm x 183 cm flexible rectangular net mouth. 914 cm long net with 1.8 cm streched mesh for first 457 cm and 1.3 cm mesh for last 457 cm. 152 cm of coarse plankton or muslin netting lined the end of the net. System equipped with mechanical time/depth recorder [Wiebe and Benfield 2003 Plate 4 A, B].</skos:definition>
<owl:versionInfo>1</owl:versionInfo>
<dc:date>2011-10-21 14:18:49.0</dc:date>
<skos:note xml:lang="en">accepted</skos:note>
<owl:deprecated>false</owl:deprecated>
<skos:broader rdf:resource="http://vocab.nerc.ac.uk/collection/L05/current/23/"/>
<void:inDataset rdf:resource="http://vocab.nerc.ac.uk/.well-known/void"/>
</skos:Concept>
</skos:member>
<skos:member>
<skos:Concept rdf:about="http://vocab.nerc.ac.uk/collection/L22/current/NETT0150/">
<dc:identifier>SDN:L22::NETT0150</dc:identifier>
<skos:notation>SDN:L22::NETT0150</skos:notation>
<skos:prefLabel xml:lang="en">Tucker-style opening-closing Rectangular Midwater Trawl 8 - Clarke (1969)</skos:prefLabel>
<skos:altLabel>RMT 8</skos:altLabel>
<skos:definition xml:lang="en">A 283 cm x 400 cm rectangular flexible mouth opening with 5 mm mesh net 1188 cm long. Net mouth is opened and closed acoustically. Pinger used to determine depth.</skos:definition>
<owl:versionInfo>1</owl:versionInfo>
<dc:date>2011-10-21 14:18:49.0</dc:date>
<skos:note xml:lang="en">accepted</skos:note>
<owl:deprecated>false</owl:deprecated>
<skos:broader rdf:resource="http://vocab.nerc.ac.uk/collection/L05/current/23/"/>
<void:inDataset rdf:resource="http://vocab.nerc.ac.uk/.well-known/void"/>
</skos:Concept>
</skos:member>
<skos:member>
<skos:Concept rdf:about="http://vocab.nerc.ac.uk/collection/L22/current/TOOL0393/">
<dc:identifier>SDN:L22::TOOL0393</dc:identifier>
<skos:notation>SDN:L22::TOOL0393</skos:notation>
<skos:prefLabel xml:lang="en">Turner 10-AU chlorophyll field fluorometer</skos:prefLabel>
<skos:altLabel>10-AU chlorophyll fluorometer</skos:altLabel>
<skos:definition xml:lang="en">A field fluorometer designed for continuous-flow monitoring or discrete sample analyses of chlorophyll-a. It has a minimum detection limit of 0.025 ug/L extracted chlorophyll-a over the range  0-250 ug/L and can operate over a temperature range of 0-55 degC.</skos:definition>
<owl:versionInfo>1</owl:versionInfo>
<dc:date>2011-04-14 09:29:16.0</dc:date>
<skos:note xml:lang="en">accepted</skos:note>
<owl:deprecated>false</owl:deprecated>
<skos:broader rdf:resource="http://vocab.nerc.ac.uk/collection/L05/current/113/"/>
<void:inDataset rdf:resource="http://vocab.nerc.ac.uk/.well-known/void"/>
</skos:Concept>
</skos:member>
<skos:member>
<skos:Concept rdf:about="http://vocab.nerc.ac.uk/collection/L22/current/TOOL0510/">
<dc:identifier>SDN:L22::TOOL0510</dc:identifier>
<skos:notation>SDN:L22::TOOL0510</skos:notation>
<skos:prefLabel xml:lang="en">Turner Designs 700 Laboratory Fluorometer</skos:prefLabel>
<skos:altLabel>TD-700 Lab Fluorometer</skos:altLabel>
<skos:definition xml:lang="en">A benchtop fluorometer designed to detect fluorescence over the UV to red range. It uses a Quartz Halogen Lamp or a Low Pressure Mercury Vapour Lamp to excite the species of interest and fluorescence is detected by a photomultiplier tube with a range of 300-650 nm. A red-sensitive tube with a detection range of 185-870 nm is also available. The instrument can measure concentrations of a variety of compounds, including chlorophyll-a and fluorescent dyes, and is thus suitable for a range of applications, including chlorophyll, water quality monitoring and fluorescent tracer studies. Samples can be averaged by the instrument to improve accuracy, and it can read and subtract a blank measurement from the data, further improving the accuracy. Data can be output as concentrations or raw fluorescence measurements.</skos:definition>
<owl:versionInfo>1</owl:versionInfo>
<dc:date>2012-06-28 09:49:48.0</dc:date>
<skos:note xml:lang="en">accepted</skos:note>
<owl:deprecated>false</owl:deprecated>
<skos:broader rdf:resource="http://vocab.nerc.ac.uk/collection/L05/current/LAB23/"/>
<void:inDataset rdf:resource="http://vocab.nerc.ac.uk/.well-known/void"/>
</skos:Concept>
</skos:member>
<skos:member>
<skos:Concept rdf:about="http://vocab.nerc.ac.uk/collection/L22/current/TOOL0365/">
<dc:identifier>SDN:L22::TOOL0365</dc:identifier>
<skos:notation>SDN:L22::TOOL0365</skos:notation>
<skos:prefLabel xml:lang="en">Turner Designs Cyclops-7 chlorophyll fluorometer</skos:prefLabel>
<skos:altLabel>Cyclops-7 chlorophyll fluorometer</skos:altLabel>
<skos:definition xml:lang="en">A high performance, in-situ fluorometer with 470 nm excitation filter and 685 nm emission filter which detects chlorophyll-a. It has a minimum detection limit of 0.025 ug/L and a dynamic range of 0-500 ug/L. The instrument can be used at depths of up to 600 m and in water temperatures of -2 to 50 degC.</skos:definition>
<owl:versionInfo>1</owl:versionInfo>
<dc:date>2011-01-28 12:46:19.0</dc:date>
<skos:note xml:lang="en">accepted</skos:note>
<owl:deprecated>false</owl:deprecated>
<skos:broader rdf:resource="http://vocab.nerc.ac.uk/collection/L05/current/113/"/>
<void:inDataset rdf:resource="http://vocab.nerc.ac.uk/.well-known/void"/>
</skos:Concept>
</skos:member>
<skos:member>
<skos:Concept rdf:about="http://vocab.nerc.ac.uk/collection/L22/current/TOOL0368/">
<dc:identifier>SDN:L22::TOOL0368</dc:identifier>
<skos:notation>SDN:L22::TOOL0368</skos:notation>
<skos:prefLabel xml:lang="en">Turner Designs Cyclops-7 coloured dissolved organic matter fluorometer</skos:prefLabel>
<skos:altLabel>Cyclops-7 CDOM fluorometer</skos:altLabel>
<skos:definition xml:lang="en">A high performance, in-situ fluorometer with 365 nm excitation filter and 470 nm emission filter which detects coloured dissolved organic matter (CDOM). Tests with quinine sulphate have shown the instrument to have a minimum detection limit of 0.4 ppb and a dynamic range of 0-2500 ppb. The instrument can be used at depths of up to 600 m and in water temperatures of -2 to 50 degC.</skos:definition>
<owl:versionInfo>1</owl:versionInfo>
<dc:date>2011-01-28 12:46:19.0</dc:date>
<skos:note xml:lang="en">accepted</skos:note>
<owl:deprecated>false</owl:deprecated>
<skos:broader rdf:resource="http://vocab.nerc.ac.uk/collection/L05/current/113/"/>
<void:inDataset rdf:resource="http://vocab.nerc.ac.uk/.well-known/void"/>
</skos:Concept>
</skos:member>
<skos:member>
<skos:Concept rdf:about="http://vocab.nerc.ac.uk/collection/L22/current/TOOL0367/">
<dc:identifier>SDN:L22::TOOL0367</dc:identifier>
<skos:notation>SDN:L22::TOOL0367</skos:notation>
<skos:prefLabel xml:lang="en">Turner Designs Cyclops-7 phycocyanin cyanobacteria fluorometer</skos:prefLabel>
<skos:altLabel>Cyclops-7 phycocyanin fluorometer</skos:altLabel>
<skos:definition xml:lang="en">A high performance, in-situ fluorometer with 600 nm excitation filter and 640 nm emission filter which detects Phycocyanin cyanobacteria. It has a minimum detection limit of 150 cells/mL and a dynamic range of 0-150,000 cells/mL. The instrument can be used at depths of up to 600 m and in water temperatures of -2 to 50 degC.</skos:definition>
<owl:versionInfo>1</owl:versionInfo>
<dc:date>2011-01-28 12:46:19.0</dc:date>
<skos:note xml:lang="en">accepted</skos:note>
<owl:deprecated>false</owl:deprecated>
<skos:broader rdf:resource="http://vocab.nerc.ac.uk/collection/L05/current/113/"/>
<void:inDataset rdf:resource="http://vocab.nerc.ac.uk/.well-known/void"/>
</skos:Concept>
</skos:member>
<skos:member>
<skos:Concept rdf:about="http://vocab.nerc.ac.uk/collection/L22/current/TOOL0366/">
<dc:identifier>SDN:L22::TOOL0366</dc:identifier>
<skos:notation>SDN:L22::TOOL0366</skos:notation>
<skos:prefLabel xml:lang="en">Turner Designs Cyclops-7 phycoerythrin cyanobacteria fluorometer</skos:prefLabel>
<skos:altLabel>Cyclops-7 phycoerythrin fluorometer</skos:altLabel>
<skos:definition xml:lang="en">A high performance, in-situ fluorometer with 544 nm excitation filter and 577 nm emission filter which detects Phycoerythrin cyanobacteria. It has a minimum detection limit of 150 cells/mL and a dynamic range of 0-150,000 cells/mL. The instrument can be used at depths of up to 600 m and in water temperatures of -2 to 50 degC.</skos:definition>
<owl:versionInfo>1</owl:versionInfo>
<dc:date>2011-01-28 12:46:19.0</dc:date>
<skos:note xml:lang="en">accepted</skos:note>
<owl:deprecated>false</owl:deprecated>
<skos:broader rdf:resource="http://vocab.nerc.ac.uk/collection/L05/current/113/"/>
<void:inDataset rdf:resource="http://vocab.nerc.ac.uk/.well-known/void"/>
</skos:Concept>
</skos:member>
<skos:member>
<skos:Concept rdf:about="http://vocab.nerc.ac.uk/collection/L22/current/TOOL0189/">
<dc:identifier>SDN:L22::TOOL0189</dc:identifier>
<skos:notation>SDN:L22::TOOL0189</skos:notation>
<skos:prefLabel xml:lang="en">Turner Designs SCUFA II Submersible Fluorometer</skos:prefLabel>
<skos:altLabel>SCUFA II fluorometer</skos:altLabel>
<skos:definition xml:lang="en">An accurate, versatile submersible fluorometer for chlorophyll and dye tracking applications. It is capable of operation in a wide range of concentrations and environmental conditions. Output options include chlorophyll-a, cyanobacteria, Rhodamine WT, fluorescin. A turbidity sensor may also be incorporated and logged as a parallel channel. From 1 December 2008, Turner Designs have discontinued all SCUFA Submersible Fluorometer applications. Supported until end 2013</skos:definition>
<owl:versionInfo>1</owl:versionInfo>
<dc:date>2010-05-18 16:10:58.0</dc:date>
<skos:note xml:lang="en">accepted</skos:note>
<owl:deprecated>false</owl:deprecated>
<skos:broader rdf:resource="http://vocab.nerc.ac.uk/collection/L05/current/113/"/>
<void:inDataset rdf:resource="http://vocab.nerc.ac.uk/.well-known/void"/>
</skos:Concept>
</skos:member>
<skos:member>
<skos:Concept rdf:about="http://vocab.nerc.ac.uk/collection/L22/current/TOOL0459/">
<dc:identifier>SDN:L22::TOOL0459</dc:identifier>
<skos:notation>SDN:L22::TOOL0459</skos:notation>
<skos:prefLabel xml:lang="en">Turner Designs Trilogy fluorometer with non-acidified module NA-046</skos:prefLabel>
<skos:altLabel>Turner Trilogy NA-046</skos:altLabel>
<skos:definition xml:lang="en">A compact laboratory instrument for making fluorescence, absorbance and turbidity measurements using the appropriate snap-in Application Module. The NA-046 Application Module allows measurement of chlorophyll-a in non-acidified samples and has the capability to set up calibrations based on chlorophyll-a standards.</skos:definition>
<owl:versionInfo>1</owl:versionInfo>
<dc:date>2012-02-16 10:05:14.0</dc:date>
<skos:note xml:lang="en">accepted</skos:note>
<owl:deprecated>false</owl:deprecated>
<skos:broader rdf:resource="http://vocab.nerc.ac.uk/collection/L05/current/LAB23/"/>
<void:inDataset rdf:resource="http://vocab.nerc.ac.uk/.well-known/void"/>
</skos:Concept>
</skos:member>
<skos:member>
<skos:Concept rdf:about="http://vocab.nerc.ac.uk/collection/L22/current/NETT0163/">
<dc:identifier>SDN:L22::NETT0163</dc:identifier>
<skos:notation>SDN:L22::NETT0163</skos:notation>
<skos:prefLabel xml:lang="en">Umbrella net - Rakusa-Suszczewski (1972)</skos:prefLabel>
<skos:altLabel>Umbrella net</skos:altLabel>
<skos:definition xml:lang="en">A pair of nets attached to an umbrella-like support.  The system was deployed down a 12 cm ice hole and expanded below the undersurface of the ice. A circular motion caused the nets to scrap the undersurface of the ice and collect organisms in the water just below it. There was no flow meter or a description of the net specifications.</skos:definition>
<owl:versionInfo>1</owl:versionInfo>
<dc:date>2011-10-21 14:18:49.0</dc:date>
<skos:note xml:lang="en">accepted</skos:note>
<owl:deprecated>false</owl:deprecated>
<skos:broader rdf:resource="http://vocab.nerc.ac.uk/collection/L05/current/22/"/>
<void:inDataset rdf:resource="http://vocab.nerc.ac.uk/.well-known/void"/>
</skos:Concept>
</skos:member>
<skos:member>
<skos:Concept rdf:about="http://vocab.nerc.ac.uk/collection/L22/current/TOOL0448/">
<dc:identifier>SDN:L22::TOOL0448</dc:identifier>
<skos:notation>SDN:L22::TOOL0448</skos:notation>
<skos:prefLabel xml:lang="en">Uncles STD profiler</skos:prefLabel>
<skos:altLabel>Uncles STD</skos:altLabel>
<skos:definition xml:lang="en">A direct-reading salinity-temperature-depth profiler including a conductivity cell and thermistor. An analogue readout provides low accuracy and precision measurements. The unit was home-built by R.J. Uncles from the Plymouth Marine Laboratory to measure water characteristics in estuarine environments. It was used from the late 1970s to the 1990s.</skos:definition>
<owl:versionInfo>1</owl:versionInfo>
<dc:date>2012-01-05 09:34:05.0</dc:date>
<skos:note xml:lang="en">accepted</skos:note>
<owl:deprecated>false</owl:deprecated>
<skos:broader rdf:resource="http://vocab.nerc.ac.uk/collection/L05/current/134/"/>
<skos:broader rdf:resource="http://vocab.nerc.ac.uk/collection/L05/current/350/"/>
<skos:broader rdf:resource="http://vocab.nerc.ac.uk/collection/L05/current/130/"/>
<void:inDataset rdf:resource="http://vocab.nerc.ac.uk/.well-known/void"/>
</skos:Concept>
</skos:member>
<skos:member>
<skos:Concept rdf:about="http://vocab.nerc.ac.uk/collection/L22/current/TOOL0449/">
<dc:identifier>SDN:L22::TOOL0449</dc:identifier>
<skos:notation>SDN:L22::TOOL0449</skos:notation>
<skos:prefLabel xml:lang="en">Uncles direct reading current meter</skos:prefLabel>
<skos:altLabel>Uncles DRCM</skos:altLabel>
<skos:definition xml:lang="en">A version of the Valeport Braystoke impeller flow meter adapted by R.J. Uncles from the Plymouth Marine Laboratory to measure current in estuarine environments. An analogue readout provided low accuracy and precision measurements. The instrument was used from the late 1970s to the 1990s.</skos:definition>
<owl:versionInfo>1</owl:versionInfo>
<dc:date>2012-01-05 09:34:05.0</dc:date>
<skos:note xml:lang="en">accepted</skos:note>
<owl:deprecated>false</owl:deprecated>
<skos:broader rdf:resource="http://vocab.nerc.ac.uk/collection/L05/current/114/"/>
<void:inDataset rdf:resource="http://vocab.nerc.ac.uk/.well-known/void"/>
</skos:Concept>
</skos:member>
<skos:member>
<skos:Concept rdf:about="http://vocab.nerc.ac.uk/collection/L22/current/TOOL0074/">
<dc:identifier>SDN:L22::TOOL0074</dc:identifier>
<skos:notation>SDN:L22::TOOL0074</skos:notation>
<skos:prefLabel xml:lang="en">Underwater PAR radiometer</skos:prefLabel>
<skos:altLabel>Underwater PAR</skos:altLabel>
<skos:definition xml:lang="en">Underwater PAR radiometer of unknown type. Assumed to have a spectral response of 400-700nm. Could have any type of collector (flat plate cosine collector, spherical or hemispherical).</skos:definition>
<owl:versionInfo>1</owl:versionInfo>
<dc:date>2010-09-08 10:12:41.0</dc:date>
<skos:note xml:lang="en">accepted</skos:note>
<owl:deprecated>false</owl:deprecated>
<skos:broader rdf:resource="http://vocab.nerc.ac.uk/collection/L05/current/122/"/>
<void:inDataset rdf:resource="http://vocab.nerc.ac.uk/.well-known/void"/>
</skos:Concept>
</skos:member>
<skos:member>
<skos:Concept rdf:about="http://vocab.nerc.ac.uk/collection/L22/current/TOOL0246/">
<dc:identifier>SDN:L22::TOOL0246</dc:identifier>
<skos:notation>SDN:L22::TOOL0246</skos:notation>
<skos:prefLabel xml:lang="en">Unicam SP500 spectrophotometer</skos:prefLabel>
<skos:altLabel>SP500 spectrophotometer</skos:altLabel>
<skos:definition xml:lang="en">A laboratory instrument that measures the amount of light at discrete pre-determined wavelengths that is transmitted or emitted by a sample.</skos:definition>
<owl:versionInfo>1</owl:versionInfo>
<dc:date>2010-05-18 16:10:58.0</dc:date>
<skos:note xml:lang="en">accepted</skos:note>
<owl:deprecated>false</owl:deprecated>
<skos:broader rdf:resource="http://vocab.nerc.ac.uk/collection/L05/current/LAB20/"/>
<void:inDataset rdf:resource="http://vocab.nerc.ac.uk/.well-known/void"/>
</skos:Concept>
</skos:member>
<skos:member>
<skos:Concept rdf:about="http://vocab.nerc.ac.uk/collection/L22/current/TOOL0461/">
<dc:identifier>SDN:L22::TOOL0461</dc:identifier>
<skos:notation>SDN:L22::TOOL0461</skos:notation>
<skos:prefLabel xml:lang="en">Unisense oxygen microsensor</skos:prefLabel>
<skos:altLabel>Unisense oxygen microsensor</skos:altLabel>
<skos:definition xml:lang="en">A miniaturized Clark-type dissolved oxygen instrument, including glass micro-sensors with minute tips (diameters ranging from 1 to 800 um). A gold sensing cathode is polarized against an internal reference and, driven by external partial pressure, oxygen from the environment penetrates through the sensor tip membrane and is reduced at the sensing cathode surface. A picoammeter converts the resulting reduction current to a signal. The sensor also includes a polarized guard cathode, which scavenges oxygen in the electrolyte, thus minimizing zero-current and pre-polarization time.</skos:definition>
<owl:versionInfo>1</owl:versionInfo>
<dc:date>2012-02-16 10:05:14.0</dc:date>
<skos:note xml:lang="en">accepted</skos:note>
<owl:deprecated>false</owl:deprecated>
<skos:broader rdf:resource="http://vocab.nerc.ac.uk/collection/L05/current/351/"/>
<void:inDataset rdf:resource="http://vocab.nerc.ac.uk/.well-known/void"/>
</skos:Concept>
</skos:member>
<skos:member>
<skos:Concept rdf:about="http://vocab.nerc.ac.uk/collection/L22/current/TOOL0550/">
<dc:identifier>SDN:L22::TOOL0550</dc:identifier>
<skos:notation>SDN:L22::TOOL0550</skos:notation>
<skos:prefLabel xml:lang="en">University of East Anglia Low Volume Air Sampler</skos:prefLabel>
<skos:altLabel>UEA LVAS</skos:altLabel>
<skos:definition xml:lang="en">An atmospheric sampler that pumps air through a series of filters to collect samples for off-line analysis of aerosol and gas-phase constituents. Air samples are drawn into a sheltered housing, and through a PTFE filter, which collect samples of particulate material. The air is then drawn through a pair of oxalic acid-impregnated paper filters, which trap gas-phase components. The pump is chosen to produce a flow rate of approximately 50 litres per minute. Inline flow meters between the filter set and the pump determine the volume of air sampled.</skos:definition>
<owl:versionInfo>1</owl:versionInfo>
<dc:date>2012-09-26 16:33:22.0</dc:date>
<skos:note xml:lang="en">accepted</skos:note>
<owl:deprecated>false</owl:deprecated>
<skos:broader rdf:resource="http://vocab.nerc.ac.uk/collection/L05/current/13/"/>
<void:inDataset rdf:resource="http://vocab.nerc.ac.uk/.well-known/void"/>
</skos:Concept>
</skos:member>
<skos:member>
<skos:Concept rdf:about="http://vocab.nerc.ac.uk/collection/L22/current/TOOL0541/">
<dc:identifier>SDN:L22::TOOL0541</dc:identifier>
<skos:notation>SDN:L22::TOOL0541</skos:notation>
<skos:prefLabel xml:lang="en">University of East Anglia rainwater sampler</skos:prefLabel>
<skos:altLabel>UEA rainwater sampler</skos:altLabel>
<skos:definition xml:lang="en">A rainwater sampler comprising a 40 cm diameter polypropylene plastic funnel feeding into a low density polyethylene (LDPE) bottle.</skos:definition>
<owl:versionInfo>1</owl:versionInfo>
<dc:date>2012-09-26 16:33:22.0</dc:date>
<skos:note xml:lang="en">accepted</skos:note>
<owl:deprecated>false</owl:deprecated>
<skos:broader rdf:resource="http://vocab.nerc.ac.uk/collection/L05/current/14/"/>
<void:inDataset rdf:resource="http://vocab.nerc.ac.uk/.well-known/void"/>
</skos:Concept>
</skos:member>
<skos:member>
<skos:Concept rdf:about="http://vocab.nerc.ac.uk/collection/L22/current/TOOL0340/">
<dc:identifier>SDN:L22::TOOL0340</dc:identifier>
<skos:notation>SDN:L22::TOOL0340</skos:notation>
<skos:prefLabel xml:lang="en">University of Leeds Volatile Aerosol Concentration and Composition instrument</skos:prefLabel>
<skos:altLabel>VACC</skos:altLabel>
<skos:definition xml:lang="en">The Volatile Aerosol Concentration and Composition instrument (VACC) indicates the size-resolved chemical composition of an aerosol sample. Air is drawn in through a quartz tube heating element, programmed to cycle over temperatures between 40 and 900 degrees C. Particles are sized by a hybrid optical particle counter. Temperature dependent changes in size spectra are characteristic of the chemical composition of the aerosol particles.</skos:definition>
<owl:versionInfo>1</owl:versionInfo>
<dc:date>2010-09-06 12:45:22.0</dc:date>
<skos:note xml:lang="en">accepted</skos:note>
<owl:deprecated>false</owl:deprecated>
<skos:broader rdf:resource="http://vocab.nerc.ac.uk/collection/L05/current/386/"/>
<void:inDataset rdf:resource="http://vocab.nerc.ac.uk/.well-known/void"/>
</skos:Concept>
</skos:member>
<skos:member>
<skos:Concept rdf:about="http://vocab.nerc.ac.uk/collection/L22/current/TOOL0436/">
<dc:identifier>SDN:L22::TOOL0436</dc:identifier>
<skos:notation>SDN:L22::TOOL0436</skos:notation>
<skos:prefLabel xml:lang="en">University of Leeds compact Fluorescence Assay by Gas Expansion instrument</skos:prefLabel>
<skos:altLabel>Leeds University FAGE</skos:altLabel>
<skos:definition xml:lang="en">The compact Fluorescence Assay by Gas Expansion (FAGE) instrument is used in ship and aircraft deployments to measure hydroxyl radicals (OH) and iodine monoxide radicals (IO). It uses low pressure Laser Induced Fluorescence (LIF). The laser, tuned to 308 nm for OH or to 445 nm for IO, is directed through the ambient air sample. The resulting fluorescence is filtered and focussed onto a photomultiplier tube, and analysed by photon counting. The signal is calibrated using known standards of OH and IO.</skos:definition>
<owl:versionInfo>1</owl:versionInfo>
<dc:date>2011-11-07 15:23:52.0</dc:date>
<skos:note xml:lang="en">accepted</skos:note>
<owl:deprecated>false</owl:deprecated>
<skos:broader rdf:resource="http://vocab.nerc.ac.uk/collection/L05/current/382/"/>
<void:inDataset rdf:resource="http://vocab.nerc.ac.uk/.well-known/void"/>
</skos:Concept>
</skos:member>
<skos:member>
<skos:Concept rdf:about="http://vocab.nerc.ac.uk/collection/L22/current/TOOL0278/">
<dc:identifier>SDN:L22::TOOL0278</dc:identifier>
<skos:notation>SDN:L22::TOOL0278</skos:notation>
<skos:prefLabel xml:lang="en">University of Liverpool cathodic stripping voltammetry metal analyser</skos:prefLabel>
<skos:altLabel>Liverpool CSV metals</skos:altLabel>
<skos:definition xml:lang="en">A research mode continuous flow metal analyser developed and deployed by Liverpool University Earth and Ocean Sciences department. It is based on cathodic stripping voltammetry with a mercury cathode and the capability for continuous UV light digestion if required.</skos:definition>
<owl:versionInfo>1</owl:versionInfo>
<dc:date>2010-05-18 16:10:58.0</dc:date>
<skos:note xml:lang="en">accepted</skos:note>
<owl:deprecated>false</owl:deprecated>
<skos:broader rdf:resource="http://vocab.nerc.ac.uk/collection/L05/current/383/"/>
<void:inDataset rdf:resource="http://vocab.nerc.ac.uk/.well-known/void"/>
</skos:Concept>
</skos:member>
<skos:member>
<skos:Concept rdf:about="http://vocab.nerc.ac.uk/collection/L22/current/TOOL0554/">
<dc:identifier>SDN:L22::TOOL0554</dc:identifier>
<skos:notation>SDN:L22::TOOL0554</skos:notation>
<skos:prefLabel xml:lang="en">University of Manchester 4-stage Compact Cascade Impactor</skos:prefLabel>
<skos:altLabel>UMA 4-stage CCI</skos:altLabel>
<skos:definition xml:lang="en">An aerosol sampler modelled on the Harvard Compact Cascade Impactor. Sample air is accelerated through an orifice towards a collector plate, which deflects the airflow around it. Particles too large to follow the streamlines impact on the plate. The air stream, now with the largest particles removed, proceeds to the subsequent impactor stages, each tuned to collect successively smaller particles. The four stages collect particles in the following size categories: greater than 9.9 um; 5.3-9.9 um; 1.0-5.3 um; 0.16-1.0 um.</skos:definition>
<owl:versionInfo>1</owl:versionInfo>
<dc:date>2012-09-28 09:56:09.0</dc:date>
<skos:note xml:lang="en">accepted</skos:note>
<owl:deprecated>false</owl:deprecated>
<skos:broader rdf:resource="http://vocab.nerc.ac.uk/collection/L05/current/13/"/>
<void:inDataset rdf:resource="http://vocab.nerc.ac.uk/.well-known/void"/>
</skos:Concept>
</skos:member>
<skos:member>
<skos:Concept rdf:about="http://vocab.nerc.ac.uk/collection/L22/current/TOOL0651/">
<dc:identifier>SDN:L22::TOOL0651</dc:identifier>
<skos:notation>SDN:L22::TOOL0651</skos:notation>
<skos:prefLabel xml:lang="en">Unknown beam trawl</skos:prefLabel>
<skos:altLabel>Beam trawl</skos:altLabel>
<skos:definition xml:lang="en">A net that is held open by a solid wooden or metal beam, attached to plates at the ends that act as runners over the seabed. The beam can vary in length from 2-12m. A chain mat may be fitted to the beam to increase seabed disturbance. The net is towed on the seabed and the resulting disturbance causes fish and shellfish to swim up and get caught in the net.</skos:definition>
<owl:versionInfo>2</owl:versionInfo>
<dc:date>2013-11-19 09:51:15.0</dc:date>
<skos:note xml:lang="en">accepted</skos:note>
<owl:deprecated>false</owl:deprecated>
<skos:broader rdf:resource="http://vocab.nerc.ac.uk/collection/L05/current/62/"/>
<void:inDataset rdf:resource="http://vocab.nerc.ac.uk/.well-known/void"/>
</skos:Concept>
</skos:member>
<skos:member>
<skos:Concept rdf:about="http://vocab.nerc.ac.uk/collection/L22/current/TOOL0145/">
<dc:identifier>SDN:L22::TOOL0145</dc:identifier>
<skos:notation>SDN:L22::TOOL0145</skos:notation>
<skos:prefLabel xml:lang="en">Unknown chlorophyll fluorometer</skos:prefLabel>
<skos:altLabel>Unknown fluorometer</skos:altLabel>
<skos:definition xml:lang="en">An in-situ instrument that transmits pulses of UV light into a region of the surrounding water body and records the amount of red light generated as a result by chlorophyll fluorescence.</skos:definition>
<owl:versionInfo>1</owl:versionInfo>
<dc:date>2010-05-18 16:10:58.0</dc:date>
<skos:note xml:lang="en">accepted</skos:note>
<owl:deprecated>false</owl:deprecated>
<skos:related rdf:resource="http://vocab.nerc.ac.uk/collection/P01/current/CPHLPS01/"/>
<skos:related rdf:resource="http://vocab.nerc.ac.uk/collection/P01/current/FVLTZZ01/"/>
<skos:related rdf:resource="http://vocab.nerc.ac.uk/collection/P01/current/CPHLPR01/"/>
<skos:broader rdf:resource="http://vocab.nerc.ac.uk/collection/L05/current/113/"/>
<void:inDataset rdf:resource="http://vocab.nerc.ac.uk/.well-known/void"/>
</skos:Concept>
</skos:member>
<skos:member>
<skos:Concept rdf:about="http://vocab.nerc.ac.uk/collection/L22/current/TOOL0650/">
<dc:identifier>SDN:L22::TOOL0650</dc:identifier>
<skos:notation>SDN:L22::TOOL0650</skos:notation>
<skos:prefLabel xml:lang="en">Unknown high-performance liquid chromatograph</skos:prefLabel>
<skos:altLabel>Unknown HPLC</skos:altLabel>
<skos:definition xml:lang="en">A high-performance liquid chromatograph that separates and analyses compounds present in a liquid sample. Separation results from the difference in the relative distribution ratios of the solutes between a solid stationary phase packed into a column and a liquid mobile phase. The separated compound bands which elute from the column are then measured using a detector. HPLC forces the mobile phase under high pressures which is distinguished from traditional liquid chromatography which relies on the force of gravity. The HPLC also has better separation of the components due to the smaller particle size of the column packing material. HPLC instruments usually consist of a reservoir of mobile phase, a pump, an injector, a separation column and a detector.</skos:definition>
<owl:versionInfo>1</owl:versionInfo>
<dc:date>2013-11-12 13:16:41.0</dc:date>
<skos:note xml:lang="en">accepted</skos:note>
<owl:deprecated>false</owl:deprecated>
<skos:broader rdf:resource="http://vocab.nerc.ac.uk/collection/L05/current/LAB11/"/>
<void:inDataset rdf:resource="http://vocab.nerc.ac.uk/.well-known/void"/>
</skos:Concept>
</skos:member>
<skos:member>
<skos:Concept rdf:about="http://vocab.nerc.ac.uk/collection/L22/current/TOOL0148/">
<dc:identifier>SDN:L22::TOOL0148</dc:identifier>
<skos:notation>SDN:L22::TOOL0148</skos:notation>
<skos:prefLabel xml:lang="en">Unknown transmissometer</skos:prefLabel>
<skos:altLabel>Unknown transmissometer</skos:altLabel>
<skos:definition xml:lang="en">An in-situ instrument that transmits monochromatic light through a region of the surrounding water body and records how much is received by a sensor a fixed distance away.</skos:definition>
<owl:versionInfo>1</owl:versionInfo>
<dc:date>2010-05-18 16:10:58.0</dc:date>
<skos:note xml:lang="en">accepted</skos:note>
<owl:deprecated>false</owl:deprecated>
<skos:related rdf:resource="http://vocab.nerc.ac.uk/collection/P01/current/ATTNZR01/"/>
<skos:related rdf:resource="http://vocab.nerc.ac.uk/collection/P01/current/POATCV01/"/>
<skos:broader rdf:resource="http://vocab.nerc.ac.uk/collection/L05/current/124/"/>
<void:inDataset rdf:resource="http://vocab.nerc.ac.uk/.well-known/void"/>
</skos:Concept>
</skos:member>
<skos:member>
<skos:Concept rdf:about="http://vocab.nerc.ac.uk/collection/L22/current/TOOL0567/">
<dc:identifier>SDN:L22::TOOL0567</dc:identifier>
<skos:notation>SDN:L22::TOOL0567</skos:notation>
<skos:prefLabel xml:lang="en">VG IsoPrep 18 water equilibration device</skos:prefLabel>
<skos:altLabel>VG IsoPrep 18</skos:altLabel>
<skos:definition xml:lang="en">A laboratory instrument which prepares water samples for isotopic analysis using a H2O-CO2 equilibration system. The instrument requires 3 ml of water for one measurement to be made. The IsoPrep 18 is usually coupled with an Isotope-Ratio Mass Spectrometer (IRMS) where the prepared gases are then ionised and analysed for their isotopic content.</skos:definition>
<owl:versionInfo>1</owl:versionInfo>
<dc:date>2012-10-22 13:48:32.0</dc:date>
<skos:note xml:lang="en">accepted</skos:note>
<owl:deprecated>false</owl:deprecated>
<skos:broader rdf:resource="http://vocab.nerc.ac.uk/collection/L05/current/EQUIL/"/>
<void:inDataset rdf:resource="http://vocab.nerc.ac.uk/.well-known/void"/>
</skos:Concept>
</skos:member>
<skos:member>
<skos:Concept rdf:about="http://vocab.nerc.ac.uk/collection/L22/current/TOOL0566/">
<dc:identifier>SDN:L22::TOOL0566</dc:identifier>
<skos:notation>SDN:L22::TOOL0566</skos:notation>
<skos:prefLabel xml:lang="en">VG SIRA 10 Isotope-Ratio Mass Spectrometer</skos:prefLabel>
<skos:altLabel>VG SIRA 10 IRMS</skos:altLabel>
<skos:definition xml:lang="en">An Isotope-Ratio Mass Spectrometer (IRMS) which operates in dual inlet flow mode for the measurement of the isotope ratios d13C/12C, d18O/16O and d34S/32S. It is used to determine the d13C/12C of carbon in different materials (organic matter, dissolved carbon in water), d13C/12C and d18O/16O in carbonates, d18O/16O and d34S/32S in sulphates and d34S/32S in sulphides. The natural sample is processed first (e.g. combustion, acid attack, or purification) in order to obtain a directly analysable gas. The prepared gases (CO2 or SO2) are then ionised and analysed for their isotopic content by the IRMS. This model is no longer in production.</skos:definition>
<owl:versionInfo>1</owl:versionInfo>
<dc:date>2012-10-22 13:48:32.0</dc:date>
<skos:note xml:lang="en">accepted</skos:note>
<owl:deprecated>false</owl:deprecated>
<skos:broader rdf:resource="http://vocab.nerc.ac.uk/collection/L05/current/LAB16/"/>
<void:inDataset rdf:resource="http://vocab.nerc.ac.uk/.well-known/void"/>
</skos:Concept>
</skos:member>
<skos:member>
<skos:Concept rdf:about="http://vocab.nerc.ac.uk/collection/L22/current/TOOL0619/">
<dc:identifier>SDN:L22::TOOL0619</dc:identifier>
<skos:notation>SDN:L22::TOOL0619</skos:notation>
<skos:prefLabel xml:lang="en">VIZ 1223 Radiosonde</skos:prefLabel>
<skos:altLabel>VIZ 1223 Radiosonde</skos:altLabel>
<skos:definition xml:lang="en">An instrument package in common use in the 1970s and 1980s comprising a rod thermistor (for air temperature measurements), a carbon hygristor (for humidity measurements) and an aneroid pressure sensor with a radio data transmitter. The package was attached to a balloon filled with hydrogen or helium and released to measure an atmospheric profile on the ascent and, if fitted with a parachute, the descent. The radio retransmitted LORAN-C signals allowing the balloon to be tracked giving measurements of winds.</skos:definition>
<owl:versionInfo>1</owl:versionInfo>
<dc:date>2013-05-09 14:54:45.0</dc:date>
<skos:note xml:lang="en">accepted</skos:note>
<owl:deprecated>false</owl:deprecated>
<skos:broader rdf:resource="http://vocab.nerc.ac.uk/collection/L05/current/103/"/>
<void:inDataset rdf:resource="http://vocab.nerc.ac.uk/.well-known/void"/>
</skos:Concept>
</skos:member>
<skos:member>
<skos:Concept rdf:about="http://vocab.nerc.ac.uk/collection/L22/current/TOOL0229/">
<dc:identifier>SDN:L22::TOOL0229</dc:identifier>
<skos:notation>SDN:L22::TOOL0229</skos:notation>
<skos:prefLabel xml:lang="en">Vaisala GM70 atmospheric carbon dioxide analyser</skos:prefLabel>
<skos:altLabel>Vaisala GM70 CO2 analyser</skos:altLabel>
<skos:definition xml:lang="en">An instrument designed for the measurement of atmospheric carbon dioxide incorporating a probe that connects to a pump aspirator. The probe contains a CARBOCAP sensor comprising three major components - a light source, a Fabry-Perot interferometer and an IR detector. The interferometer allows light of two wavelengths to pass through to the detector - the wavelength at which carbon dioxide absorbs light and a nearby non-absorbing wavelength for comparison purposes. The probe is used in conjunction with a MI70 meter which promotes easy transfer of data to a PC.</skos:definition>
<owl:versionInfo>2</owl:versionInfo>
<dc:date>2010-11-18 12:39:41.0</dc:date>
<skos:note xml:lang="en">accepted</skos:note>
<owl:deprecated>false</owl:deprecated>
<skos:broader rdf:resource="http://vocab.nerc.ac.uk/collection/L05/current/382/"/>
<void:inDataset rdf:resource="http://vocab.nerc.ac.uk/.well-known/void"/>
</skos:Concept>
</skos:member>
<skos:member>
<skos:Concept rdf:about="http://vocab.nerc.ac.uk/collection/L22/current/TOOL0081/">
<dc:identifier>SDN:L22::TOOL0081</dc:identifier>
<skos:notation>SDN:L22::TOOL0081</skos:notation>
<skos:prefLabel xml:lang="en">Vaisala HMP temperature and humidity sensor</skos:prefLabel>
<skos:altLabel>Vaisala HMP probe</skos:altLabel>
<skos:definition xml:lang="en">A family of sensors and instruments (sensors plus integral displays or loggers) for the measurement of air temperature and relative humidity. All are based on a probe containing a patent (HUMICAP) capacitive thin film polymer humidity sensor and a Pt100 platinum resistance thermometer. The probes are available with a wide range of packaging, cabling and interface options all of which have designations of the form HMPnn such as HMP45 and HMP75. Vaisala sensors are incorporated into weather stations and marketed by Campbell Scientific.</skos:definition>
<owl:versionInfo>2</owl:versionInfo>
<dc:date>2009-12-10 11:27:25.0</dc:date>
<skos:note xml:lang="en">accepted</skos:note>
<owl:deprecated>false</owl:deprecated>
<skos:related rdf:resource="http://vocab.nerc.ac.uk/collection/P01/current/CDTASS01/"/>
<skos:related rdf:resource="http://vocab.nerc.ac.uk/collection/P01/current/CRELSS01/"/>
<skos:broader rdf:resource="http://vocab.nerc.ac.uk/collection/L05/current/102/"/>
<void:inDataset rdf:resource="http://vocab.nerc.ac.uk/.well-known/void"/>
</skos:Concept>
</skos:member>
<skos:member>
<skos:Concept rdf:about="http://vocab.nerc.ac.uk/collection/L22/current/TOOL0397/">
<dc:identifier>SDN:L22::TOOL0397</dc:identifier>
<skos:notation>SDN:L22::TOOL0397</skos:notation>
<skos:prefLabel xml:lang="en">Vaisala PTB 210 digital barometer</skos:prefLabel>
<skos:altLabel>PTB 210 barometer</skos:altLabel>
<skos:definition xml:lang="en">Digital barometer using a silicon capacitive absolute pressure sensor. The instrument can operate over a pressure range of 50 to 1100 hPa and a temperature range of -40 to 60 degC. Two basic configurations are available: serial output for 500-1100 hPa and 50-1100 hPa, and analog output with different scalings between 500 and 1100 hPa. It is designed for a variety of applications, such as weather stations, data buoys and ships.</skos:definition>
<owl:versionInfo>1</owl:versionInfo>
<dc:date>2011-04-14 09:29:16.0</dc:date>
<skos:note xml:lang="en">accepted</skos:note>
<owl:deprecated>false</owl:deprecated>
<skos:broader rdf:resource="http://vocab.nerc.ac.uk/collection/L05/current/102/"/>
<void:inDataset rdf:resource="http://vocab.nerc.ac.uk/.well-known/void"/>
</skos:Concept>
</skos:member>
<skos:member>
<skos:Concept rdf:about="http://vocab.nerc.ac.uk/collection/L22/current/TOOL0125/">
<dc:identifier>SDN:L22::TOOL0125</dc:identifier>
<skos:notation>SDN:L22::TOOL0125</skos:notation>
<skos:prefLabel xml:lang="en">Vaisala PTB100 barometric pressure sensor</skos:prefLabel>
<skos:altLabel>Vaisala PTB100 barometer</skos:altLabel>
<skos:definition xml:lang="en">A series of analogue barometers using the BAROCAP silicon capacitive absolute pressure sensor developed by Vaisala able to operate over a wide temperature range. The series has low power consumption, selectable external on/off control, practical output voltage ranges and three or four wire connection capability.</skos:definition>
<owl:versionInfo>1</owl:versionInfo>
<dc:date>2010-05-18 16:10:58.0</dc:date>
<skos:note xml:lang="en">accepted</skos:note>
<owl:deprecated>false</owl:deprecated>
<skos:related rdf:resource="http://vocab.nerc.ac.uk/collection/P01/current/CAPHZZ01/"/>
<skos:broader rdf:resource="http://vocab.nerc.ac.uk/collection/L05/current/102/"/>
<void:inDataset rdf:resource="http://vocab.nerc.ac.uk/.well-known/void"/>
</skos:Concept>
</skos:member>
<skos:member>
<skos:Concept rdf:about="http://vocab.nerc.ac.uk/collection/L22/current/TOOL0126/">
<dc:identifier>SDN:L22::TOOL0126</dc:identifier>
<skos:notation>SDN:L22::TOOL0126</skos:notation>
<skos:prefLabel xml:lang="en">Vaisala WAA151 cup anemometer</skos:prefLabel>
<skos:altLabel>Vaisala WAA151 anemometer</skos:altLabel>
<skos:definition xml:lang="en">Three lightweight, conical cups mounted on the cup wheel providing linearity with windspeeds up to 75m/s. Rotation speed is measured by a disk attached to the shaft cutting an infrared light beam 14 times per revolution producing pulses counted by a phototransistor. The output rate is directly proportional to wind speed.</skos:definition>
<owl:versionInfo>1</owl:versionInfo>
<dc:date>2010-05-18 16:10:58.0</dc:date>
<skos:note xml:lang="en">accepted</skos:note>
<owl:deprecated>false</owl:deprecated>
<skos:related rdf:resource="http://vocab.nerc.ac.uk/collection/P01/current/EWSKSS01/"/>
<skos:broader rdf:resource="http://vocab.nerc.ac.uk/collection/L05/current/101/"/>
<void:inDataset rdf:resource="http://vocab.nerc.ac.uk/.well-known/void"/>
</skos:Concept>
</skos:member>
<skos:member>
<skos:Concept rdf:about="http://vocab.nerc.ac.uk/collection/L22/current/TOOL0127/">
<dc:identifier>SDN:L22::TOOL0127</dc:identifier>
<skos:notation>SDN:L22::TOOL0127</skos:notation>
<skos:prefLabel xml:lang="en">Vaisala WAV151 wind vane</skos:prefLabel>
<skos:altLabel>Vaisala WAV151 vane</skos:altLabel>
<skos:definition xml:lang="en">A counter-balanced, low-threshold, optoelectic wind-vane. Infrared LEDs and phototransistors are mounted on six orbits on each side of a 6-bit GRAY-coded disc. Turning the vane causes the disc to change the code received by the phototransistors.</skos:definition>
<owl:versionInfo>1</owl:versionInfo>
<dc:date>2010-05-18 16:10:58.0</dc:date>
<skos:note xml:lang="en">accepted</skos:note>
<owl:deprecated>false</owl:deprecated>
<skos:related rdf:resource="http://vocab.nerc.ac.uk/collection/P01/current/EWDASS01/"/>
<skos:broader rdf:resource="http://vocab.nerc.ac.uk/collection/L05/current/101/"/>
<void:inDataset rdf:resource="http://vocab.nerc.ac.uk/.well-known/void"/>
</skos:Concept>
</skos:member>
<skos:member>
<skos:Concept rdf:about="http://vocab.nerc.ac.uk/collection/L22/current/TOOL0587/">
<dc:identifier>SDN:L22::TOOL0587</dc:identifier>
<skos:notation>SDN:L22::TOOL0587</skos:notation>
<skos:prefLabel xml:lang="en">Valeport 308 recording current meter</skos:prefLabel>
<skos:altLabel>Valeport 308 RCM</skos:altLabel>
<skos:definition xml:lang="en">A self-recording instrument with speed and direction sensors as standard and optional conductivity, temperature and pressure sensors. Speed is measured by a neutrally-buoyant styrene impeller mounted in a jewelled main thrust bearing and PTFE radial guides. Two magnets are fitted to the impeller and a reed switch fitted inside the pressure housing counts the rotations of the impeller.  Direction is sensed using a Valeport two axis, gimballed flux-gate compass.  Temperature is sensed by a Valeport platinum resistance thermometer (PRT) or thermistor, depending on the response and specification required.  Conductivity is sensed by Valeport Inductive coils and pressure by a strain-gauge transducer.   Sensor accuracy is 1.5% for speed, +/- 0.25 degrees for direction, +/-0.02C for PRT temperature, +/-0.1C for thermistor temperature, +/-0.003mS/cm for conductivity and 0.1% to 0.005% full-scale for pressure depending on sensor range.    The vector average is based on a 5 second period during which impeller counts are measured and a single compass reading is made. An average period can be any multiple of 5 seconds up to a maximum of 30 minutes. For the optional parameters, the sample is taken at the end of the sample period and averaged over the averaging period. Further information may be found in http://www.bodc.ac.uk/data/documents/nodb/49777/ .</skos:definition>
<owl:versionInfo>1</owl:versionInfo>
<dc:date>2013-01-14 09:34:23.0</dc:date>
<skos:note xml:lang="en">accepted</skos:note>
<owl:deprecated>false</owl:deprecated>
<skos:broader rdf:resource="http://vocab.nerc.ac.uk/collection/L05/current/114/"/>
<void:inDataset rdf:resource="http://vocab.nerc.ac.uk/.well-known/void"/>
</skos:Concept>
</skos:member>
<skos:member>
<skos:Concept rdf:about="http://vocab.nerc.ac.uk/collection/L22/current/TOOL0320/">
<dc:identifier>SDN:L22::TOOL0320</dc:identifier>
<skos:notation>SDN:L22::TOOL0320</skos:notation>
<skos:prefLabel xml:lang="en">Valeport 740 tide gauge</skos:prefLabel>
<skos:altLabel>Valeport 740</skos:altLabel>
<skos:definition xml:lang="en">The Valeport 740 tide gauge is a strain gauge sensor with a resolution of 1 mm. A user-selectable sampling regime allows up to 2 years’ autonomous operation, whilst the optional radio transmission package extends the capabilities for real time operations.</skos:definition>
<owl:versionInfo>2</owl:versionInfo>
<dc:date>2012-05-11 10:25:05.0</dc:date>
<skos:note xml:lang="en">accepted</skos:note>
<owl:deprecated>false</owl:deprecated>
<skos:broader rdf:resource="http://vocab.nerc.ac.uk/collection/L05/current/111/"/>
<void:inDataset rdf:resource="http://vocab.nerc.ac.uk/.well-known/void"/>
</skos:Concept>
</skos:member>
<skos:member>
<skos:Concept rdf:about="http://vocab.nerc.ac.uk/collection/L22/current/TOOL0638/">
<dc:identifier>SDN:L22::TOOL0638</dc:identifier>
<skos:notation>SDN:L22::TOOL0638</skos:notation>
<skos:prefLabel xml:lang="en">Valeport BFM 208 current meter</skos:prefLabel>
<skos:altLabel>Valeport 208 CM</skos:altLabel>
<skos:definition xml:lang="en">A current meter with styrene impeller current sensor and relatively low resolution (6-bit) compass. In self-recording mode the compass and rotor count were read every 5 seconds and summed over the required sampling interval. A 5-second data stream including corrected vector data was output via a connector to facilitate use as a direct reading instrument. Further information may be found in http://www.bodc.ac.uk/data/documents/nodb/95303/ .</skos:definition>
<owl:versionInfo>2</owl:versionInfo>
<dc:date>2013-08-29 15:54:12.0</dc:date>
<skos:note xml:lang="en">accepted</skos:note>
<owl:deprecated>false</owl:deprecated>
<skos:broader rdf:resource="http://vocab.nerc.ac.uk/collection/L05/current/114/"/>
<void:inDataset rdf:resource="http://vocab.nerc.ac.uk/.well-known/void"/>
</skos:Concept>
</skos:member>
<skos:member>
<skos:Concept rdf:about="http://vocab.nerc.ac.uk/collection/L22/current/TOOL0232/">
<dc:identifier>SDN:L22::TOOL0232</dc:identifier>
<skos:notation>SDN:L22::TOOL0232</skos:notation>
<skos:prefLabel xml:lang="en">Valeport CTD 600</skos:prefLabel>
<skos:altLabel>Valeport CTD 600</skos:altLabel>
<skos:definition xml:lang="en">A CTD that samples on either time or depth increments based sampling with direct-reading or self-logging modes. Depth rating is 1500m. Available with either a platinum resistance thermometer (accuracy temperature 0.02C, salinity 0.07 PSU) or thermistor (accuracy temperature 0.1C, salinity 0.15 PSU) temperature sensors and inductive coil conductivity sensors. Both types have a resolution of 0.002C for temperature and 0.003 PSU for salinity.</skos:definition>
<owl:versionInfo>2</owl:versionInfo>
<dc:date>2010-11-18 12:39:41.0</dc:date>
<skos:note xml:lang="en">accepted</skos:note>
<owl:deprecated>false</owl:deprecated>
<skos:related rdf:resource="http://vocab.nerc.ac.uk/collection/P01/current/PRESPR01/"/>
<skos:related rdf:resource="http://vocab.nerc.ac.uk/collection/P01/current/PSALST01/"/>
<skos:related rdf:resource="http://vocab.nerc.ac.uk/collection/P01/current/TEMPST01/"/>
<skos:related rdf:resource="http://vocab.nerc.ac.uk/collection/P01/current/CNDCST01/"/>
<skos:broader rdf:resource="http://vocab.nerc.ac.uk/collection/L05/current/130/"/>
<skos:broader rdf:resource="http://vocab.nerc.ac.uk/collection/L05/current/350/"/>
<skos:broader rdf:resource="http://vocab.nerc.ac.uk/collection/L05/current/134/"/>
<void:inDataset rdf:resource="http://vocab.nerc.ac.uk/.well-known/void"/>
</skos:Concept>
</skos:member>
<skos:member>
<skos:Concept rdf:about="http://vocab.nerc.ac.uk/collection/L22/current/TOOL0407/">
<dc:identifier>SDN:L22::TOOL0407</dc:identifier>
<skos:notation>SDN:L22::TOOL0407</skos:notation>
<skos:prefLabel xml:lang="en">Valeport CTD 604</skos:prefLabel>
<skos:altLabel>Valeport CTD 604</skos:altLabel>
<skos:definition xml:lang="en">A CTD that samples on either time or depth increments based sampling with direct-reading or self-logging modes. Standard depth rating is 3000m, with 1000m and 2000m versions available for shallower work. The instrument is available with either a fast- or slow-response platinum resistance thermometer for profiling or mooring operations, respectively. Temperature accuracy is 0.02C and resolution is 0.002C over a range of -5 to +35C. The inductive coil conductivity sensors are accurate to 0.05 mS/cm with a resolution of 0.0003 mS/cm over the range 0.1 to 60 mS/cm, while the strain gauge pressure sensor has an accuracy of 0.1% full scale and a resolution of 0.005% full scale.</skos:definition>
<owl:versionInfo>1</owl:versionInfo>
<dc:date>2011-07-27 13:50:44.0</dc:date>
<skos:note xml:lang="en">accepted</skos:note>
<owl:deprecated>false</owl:deprecated>
<skos:broader rdf:resource="http://vocab.nerc.ac.uk/collection/L05/current/350/"/>
<skos:broader rdf:resource="http://vocab.nerc.ac.uk/collection/L05/current/134/"/>
<skos:broader rdf:resource="http://vocab.nerc.ac.uk/collection/L05/current/130/"/>
<void:inDataset rdf:resource="http://vocab.nerc.ac.uk/.well-known/void"/>
</skos:Concept>
</skos:member>
<skos:member>
<skos:Concept rdf:about="http://vocab.nerc.ac.uk/collection/L22/current/TOOL0531/">
<dc:identifier>SDN:L22::TOOL0531</dc:identifier>
<skos:notation>SDN:L22::TOOL0531</skos:notation>
<skos:prefLabel xml:lang="en">Valeport MIDAS Sound Velocity Probe</skos:prefLabel>
<skos:altLabel>Valeport MIDAS SVP</skos:altLabel>
<skos:definition xml:lang="en">This instrument comprises a time of flight sound speed sensor, pressure transducer and platinum resistance temperature sensor. It is suitable for rapid profiling down to 6000 metres depth. It can be operated in continuous, burst, trip/profile, conditional or delayed mode. The instrument was formerly known as Model 650 Mk2.</skos:definition>
<owl:versionInfo>1</owl:versionInfo>
<dc:date>2012-08-16 11:26:51.0</dc:date>
<skos:note xml:lang="en">accepted</skos:note>
<owl:deprecated>false</owl:deprecated>
<skos:broader rdf:resource="http://vocab.nerc.ac.uk/collection/L05/current/185/"/>
<skos:broader rdf:resource="http://vocab.nerc.ac.uk/collection/L05/current/134/"/>
<void:inDataset rdf:resource="http://vocab.nerc.ac.uk/.well-known/void"/>
</skos:Concept>
</skos:member>
<skos:member>
<skos:Concept rdf:about="http://vocab.nerc.ac.uk/collection/L22/current/TOOL0502/">
<dc:identifier>SDN:L22::TOOL0502</dc:identifier>
<skos:notation>SDN:L22::TOOL0502</skos:notation>
<skos:prefLabel xml:lang="en">Van Dorn water sampler</skos:prefLabel>
<skos:altLabel>Van Dorn water sampler</skos:altLabel>
<skos:definition xml:lang="en">A free-flushing water sample bottle comprising a cylinder (polycarbonate, acrylic or PVC) with a stopper at each end. The bottle is closed by means of a messenger from the surface releasing the tension on a latex band and thus pulling the two stoppers firmly into place. A thermometer can be mounted inside the bottle. One or more bottles can be lowered on a line to allow sampling at a single or multiple depth levels. Van Dorn samplers are suitable for for physical (temperature), chemical and biological sampling in shallow to very deep water. Bottles are typically lowered vertically through the water column although a horizontal version is available for sampling near the seabed or at thermoclines or chemoclines. Because of the lack of metal parts the bottles are suitable for trace metal sampling, although the blue polyurethane seal used in the Alpha version may leach mercury. The Beta version uses white ASA plastic seals that do not leach mercury but are less durable.</skos:definition>
<owl:versionInfo>1</owl:versionInfo>
<dc:date>2012-06-21 16:09:48.0</dc:date>
<skos:note xml:lang="en">accepted</skos:note>
<owl:deprecated>false</owl:deprecated>
<skos:broader rdf:resource="http://vocab.nerc.ac.uk/collection/L05/current/30/"/>
<void:inDataset rdf:resource="http://vocab.nerc.ac.uk/.well-known/void"/>
</skos:Concept>
</skos:member>
<skos:member>
<skos:Concept rdf:about="http://vocab.nerc.ac.uk/collection/L22/current/TOOL0653/">
<dc:identifier>SDN:L22::TOOL0653</dc:identifier>
<skos:notation>SDN:L22::TOOL0653</skos:notation>
<skos:prefLabel xml:lang="en">Van Veen grab</skos:prefLabel>
<skos:altLabel>Van Veen grab</skos:altLabel>
<skos:definition xml:lang="en">A simple clam-shell sediment grab penetrating approximately 20cm with a typical sampling area of 0.1m2 (but grab sizes can vary). On descent two levers with buckets at their ends are spread like open scissors that unlock on hitting the seabed. When pulled upwards the two buckets close and grab a sample. This is subject to more disturbance than by Craib or box corers.</skos:definition>
<owl:versionInfo>2</owl:versionInfo>
<dc:date>2013-11-26 08:11:24.0</dc:date>
<skos:note xml:lang="en">accepted</skos:note>
<owl:deprecated>false</owl:deprecated>
<skos:broader rdf:resource="http://vocab.nerc.ac.uk/collection/L05/current/50/"/>
<void:inDataset rdf:resource="http://vocab.nerc.ac.uk/.well-known/void"/>
</skos:Concept>
</skos:member>
<skos:member>
<skos:Concept rdf:about="http://vocab.nerc.ac.uk/collection/L22/current/TOOL0444/">
<dc:identifier>SDN:L22::TOOL0444</dc:identifier>
<skos:notation>SDN:L22::TOOL0444</skos:notation>
<skos:prefLabel xml:lang="en">Varian 3300 Gas Chromatograph</skos:prefLabel>
<skos:altLabel>Varian 3300 Gas Chromatograph</skos:altLabel>
<skos:definition xml:lang="en">A gas chromatograph that separates and analyses gas mixtures in water or air. The instrument includes an injector, autosampler, capillary column and one or more detectors. The column oven accepts packed or fused silica capillary columns, while the instrument accommodates a range of standard and capillary injectors, including split/splitless, capillary septum-equipped programmable, large bore capillary, large bore capillary flash, packed column and packed flash types. Possible detector types are flame ionisation, thermionic sensitive, electron capture, flame photometric, thermal conductivity, electrolytic conductivity and photo-ionisation. Optional carrier gas and oxygen filters may also be incorporated into the instrument. The equipment is controlled by a built-in microcomputer and can perform electron-impact, chemical ionisation, and negative ion analysis. The instrument was originally manufactured by Varian, Inc., which was bought by Agilent Technologies in 2010.</skos:definition>
<owl:versionInfo>1</owl:versionInfo>
<dc:date>2011-11-16 08:14:57.0</dc:date>
<skos:note xml:lang="en">accepted</skos:note>
<owl:deprecated>false</owl:deprecated>
<skos:broader rdf:resource="http://vocab.nerc.ac.uk/collection/L05/current/LAB02/"/>
<void:inDataset rdf:resource="http://vocab.nerc.ac.uk/.well-known/void"/>
</skos:Concept>
</skos:member>
<skos:member>
<skos:Concept rdf:about="http://vocab.nerc.ac.uk/collection/L22/current/TOOL0421/">
<dc:identifier>SDN:L22::TOOL0421</dc:identifier>
<skos:notation>SDN:L22::TOOL0421</skos:notation>
<skos:prefLabel xml:lang="en">Varian 820-MS  inductively coupled plasma mass spectrometer</skos:prefLabel>
<skos:altLabel>Varian 820-MS ICPMS</skos:altLabel>
<skos:definition xml:lang="en">A compact, floor-mounted inductively coupled plasma mass spectrometer (ICP-MS) featuring 90 deg reflecting ion optics systems for gigahertz sensitivity (1000 Mc/s/mg/L) and low background and interferences. The instrument comprises a sample introduction system (spraychamber, nebuliser and peristaltic pump), solid state 27 MHz RF generator and Turner Interlaced Coils. Plasma positioning, the triple stage vacuum system (which is fully contained within the instrument), all plasma gas flows, the mass analyzer and the Discrete Dynode Electron Multiplier (DDEM) detector are fully controlled by a PC. The DDEM detector provides nine decades of dynamic range in an all-digital pulse design. The Varian 820-MS system also features a unique Collision Reaction Interface (CRI) providing fast, flexible, interference-free analysis using simple collision and reaction gases. The instrument was originally manufactured by Varian, Inc., which was bought by Agilent Technologies in 2010.</skos:definition>
<owl:versionInfo>1</owl:versionInfo>
<dc:date>2011-09-03 16:28:15.0</dc:date>
<skos:note xml:lang="en">accepted</skos:note>
<owl:deprecated>false</owl:deprecated>
<skos:broader rdf:resource="http://vocab.nerc.ac.uk/collection/L05/current/LAB15/"/>
<void:inDataset rdf:resource="http://vocab.nerc.ac.uk/.well-known/void"/>
</skos:Concept>
</skos:member>
<skos:member>
<skos:Concept rdf:about="http://vocab.nerc.ac.uk/collection/L22/current/TOOL0523/">
<dc:identifier>SDN:L22::TOOL0523</dc:identifier>
<skos:notation>SDN:L22::TOOL0523</skos:notation>
<skos:prefLabel xml:lang="en">Varian Cary 50 UV-Vis Spectrophotometer</skos:prefLabel>
<skos:altLabel>Cary 50 UV-Vis Spectrophotometer</skos:altLabel>
<skos:definition xml:lang="en">A laboratory instrument that measures the amount of light at discrete pre-determined wavelengths that is transmitted or emitted by a sample. The instrument uses a dual beam, Czerny-Turner monochromator with a 190–1100 nm wavelength range and approximately 1.5 nm fixed spectral bandwidth. It uses a full spectrum Xe pulse lamp single source and dual Si diode detectors. The instrument has scan rates of up to 24000 nm/min and a maximum measurement rate of 80 data points per s. It also has room light immunity. It was manufactured by Varian (now part of Agilent Technologies).</skos:definition>
<owl:versionInfo>1</owl:versionInfo>
<dc:date>2012-07-09 09:48:34.0</dc:date>
<skos:note xml:lang="en">accepted</skos:note>
<owl:deprecated>false</owl:deprecated>
<skos:broader rdf:resource="http://vocab.nerc.ac.uk/collection/L05/current/LAB20/"/>
<void:inDataset rdf:resource="http://vocab.nerc.ac.uk/.well-known/void"/>
</skos:Concept>
</skos:member>
<skos:member>
<skos:Concept rdf:about="http://vocab.nerc.ac.uk/collection/L22/current/TOOL0582/">
<dc:identifier>SDN:L22::TOOL0582</dc:identifier>
<skos:notation>SDN:L22::TOOL0582</skos:notation>
<skos:prefLabel xml:lang="en">Vector Instruments H301 psychrometer</skos:prefLabel>
<skos:altLabel>VI H301 psychrometer</skos:altLabel>
<skos:definition xml:lang="en">A precision instrument for the measurement of air temperature and humidity by the wet and dry bulb method.  A pair of 100 Ohm 4-terminal platinum resistance elements were enclosed in a double-walled enclosure with an optional radiation shield to minimise thermal radiation errors.  The wet bulb element was enclosed by a wick leading to a 500 ml water reservoir (sufficient for 7 days) in a fan-driven airflow.  Accuracy was quoted by the manufacturer as 0.2C with a response time of 50 seconds.  The instrument was discontinued in 2010.</skos:definition>
<owl:versionInfo>1</owl:versionInfo>
<dc:date>2013-01-09 13:07:22.0</dc:date>
<skos:note xml:lang="en">accepted</skos:note>
<owl:deprecated>false</owl:deprecated>
<skos:related rdf:resource="http://vocab.nerc.ac.uk/collection/P01/current/CDTASS01/"/>
<skos:related rdf:resource="http://vocab.nerc.ac.uk/collection/P01/current/CWETSS01/"/>
<skos:broader rdf:resource="http://vocab.nerc.ac.uk/collection/L05/current/102/"/>
<void:inDataset rdf:resource="http://vocab.nerc.ac.uk/.well-known/void"/>
</skos:Concept>
</skos:member>
<skos:member>
<skos:Concept rdf:about="http://vocab.nerc.ac.uk/collection/L22/current/TOOL0105/">
<dc:identifier>SDN:L22::TOOL0105</dc:identifier>
<skos:notation>SDN:L22::TOOL0105</skos:notation>
<skos:prefLabel xml:lang="en">Vemco Minilog12 temperature recorder</skos:prefLabel>
<skos:altLabel>Minilog12-TR</skos:altLabel>
<skos:definition xml:lang="en">A miniature data logger that records temperature at a user programmed time interval. 12-bit version gives a resolution of 0.015C and an accuracy of +-0.1C. It is housed in a waterproof cylinder and the temperature sensor is mounted on a protruding stainless steel probe. Further information may be found on the BODC document server at URL: http://www.bodc.ac.uk/data/documents/nodb/108661/</skos:definition>
<owl:versionInfo>2</owl:versionInfo>
<dc:date>2014-02-14 10:13:29.0</dc:date>
<skos:note xml:lang="en">accepted</skos:note>
<owl:deprecated>false</owl:deprecated>
<skos:broader rdf:resource="http://vocab.nerc.ac.uk/collection/L05/current/134/"/>
<void:inDataset rdf:resource="http://vocab.nerc.ac.uk/.well-known/void"/>
</skos:Concept>
</skos:member>
<skos:member>
<skos:Concept rdf:about="http://vocab.nerc.ac.uk/collection/L22/current/TOOL0665/">
<dc:identifier>SDN:L22::TOOL0665</dc:identifier>
<skos:notation>SDN:L22::TOOL0665</skos:notation>
<skos:prefLabel xml:lang="en">Vemco Minilog12 temperature-pressure recorder</skos:prefLabel>
<skos:altLabel>Minilog12-TDR</skos:altLabel>
<skos:definition xml:lang="en">A miniature data logger that records temperature and depth at a user programmed time interval. 12-bit version gives a resolution of 0.015 degC and an accuracy of +/-0.1 degC. It is housed in a waterproof cylinder and the temperature sensor is mounted on a protruding stainless steel probe.</skos:definition>
<owl:versionInfo>1</owl:versionInfo>
<dc:date>2014-02-14 10:45:27.0</dc:date>
<skos:note xml:lang="en">accepted</skos:note>
<owl:deprecated>false</owl:deprecated>
<skos:broader rdf:resource="http://vocab.nerc.ac.uk/collection/L05/current/134/"/>
<void:inDataset rdf:resource="http://vocab.nerc.ac.uk/.well-known/void"/>
</skos:Concept>
</skos:member>
<skos:member>
<skos:Concept rdf:about="http://vocab.nerc.ac.uk/collection/L22/current/TOOL0181/">
<dc:identifier>SDN:L22::TOOL0181</dc:identifier>
<skos:notation>SDN:L22::TOOL0181</skos:notation>
<skos:prefLabel xml:lang="en">Vemco Minilog8 temperature recorder</skos:prefLabel>
<skos:altLabel>Minilog8-TR</skos:altLabel>
<skos:definition xml:lang="en">A miniature data logger that records temperature at a user programmed time interval. 8-bit version gives a resolution of 0.1C and an accuracy of between +-0.2C to +-0.3C depending on range specified. It is housed in a waterproof cylinder and the temperature sensor is mounted on a protruding stainless steel probe.</skos:definition>
<owl:versionInfo>2</owl:versionInfo>
<dc:date>2014-02-14 10:14:38.0</dc:date>
<skos:note xml:lang="en">accepted</skos:note>
<owl:deprecated>false</owl:deprecated>
<skos:broader rdf:resource="http://vocab.nerc.ac.uk/collection/L05/current/134/"/>
<void:inDataset rdf:resource="http://vocab.nerc.ac.uk/.well-known/void"/>
</skos:Concept>
</skos:member>
<skos:member>
<skos:Concept rdf:about="http://vocab.nerc.ac.uk/collection/L22/current/NETT0164/">
<dc:identifier>SDN:L22::NETT0164</dc:identifier>
<skos:notation>SDN:L22::NETT0164</skos:notation>
<skos:prefLabel xml:lang="en">Vertical and horizontal closing nets with flow meter - Nansen (1915)</skos:prefLabel>
<skos:altLabel>Nansen net system</skos:altLabel>
<skos:definition xml:lang="en">Construction has a 35 to 100 cm net diameter (but up to 300 cm for Murray and Hjort Expedition of 1910); 50 cm cylindrical portion of canvas; 150 cm long conical section of silk (no size given) [Wiebe and Benfield 2003 Plate 5 A].</skos:definition>
<owl:versionInfo>1</owl:versionInfo>
<dc:date>2011-10-21 14:18:49.0</dc:date>
<skos:note xml:lang="en">accepted</skos:note>
<owl:deprecated>false</owl:deprecated>
<skos:broader rdf:resource="http://vocab.nerc.ac.uk/collection/L05/current/22/"/>
<void:inDataset rdf:resource="http://vocab.nerc.ac.uk/.well-known/void"/>
</skos:Concept>
</skos:member>
<skos:member>
<skos:Concept rdf:about="http://vocab.nerc.ac.uk/collection/L22/current/NETT0165/">
<dc:identifier>SDN:L22::NETT0165</dc:identifier>
<skos:notation>SDN:L22::NETT0165</skos:notation>
<skos:prefLabel xml:lang="en">Vertical high-speed plankton net - Jaschnov (1961)</skos:prefLabel>
<skos:altLabel>VHSS</skos:altLabel>
<skos:definition xml:lang="en">Rectangular mouth opening. Closed like a Juday net. Used No. 38 silk. Speeds up to 2.8 m/sec (5+ knots)</skos:definition>
<owl:versionInfo>1</owl:versionInfo>
<dc:date>2011-10-21 14:18:49.0</dc:date>
<skos:note xml:lang="en">accepted</skos:note>
<owl:deprecated>false</owl:deprecated>
<skos:broader rdf:resource="http://vocab.nerc.ac.uk/collection/L05/current/67/"/>
<void:inDataset rdf:resource="http://vocab.nerc.ac.uk/.well-known/void"/>
</skos:Concept>
</skos:member>
<skos:member>
<skos:Concept rdf:about="http://vocab.nerc.ac.uk/collection/L22/current/TOOL0160/">
<dc:identifier>SDN:L22::TOOL0160</dc:identifier>
<skos:notation>SDN:L22::TOOL0160</skos:notation>
<skos:prefLabel xml:lang="en">WETLabs C-Star transmissometer</skos:prefLabel>
<skos:altLabel>WetLabs transmissometer</skos:altLabel>
<skos:definition xml:lang="en">An underwater optical beam transmissometer capable of free-space measurements or mounting in a flow tube with a pump for underway or moored applications. It is available in 370, 470, 530 and 660 nm wavelengths with a path length of 10 or 25 cm.</skos:definition>
<owl:versionInfo>1</owl:versionInfo>
<dc:date>2010-05-18 16:10:58.0</dc:date>
<skos:note xml:lang="en">accepted</skos:note>
<owl:deprecated>false</owl:deprecated>
<skos:related rdf:resource="http://vocab.nerc.ac.uk/collection/P01/current/ATTNZS01/"/>
<skos:broader rdf:resource="http://vocab.nerc.ac.uk/collection/L05/current/124/"/>
<void:inDataset rdf:resource="http://vocab.nerc.ac.uk/.well-known/void"/>
</skos:Concept>
</skos:member>
<skos:member>
<skos:Concept rdf:about="http://vocab.nerc.ac.uk/collection/L22/current/TOOL0060/">
<dc:identifier>SDN:L22::TOOL0060</dc:identifier>
<skos:notation>SDN:L22::TOOL0060</skos:notation>
<skos:prefLabel xml:lang="en">WETLabs ECO BB(RT)D Scattering Meter</skos:prefLabel>
<skos:altLabel>WL BB(RT)D OBS</skos:altLabel>
<skos:definition xml:lang="en">Single angle optical backscattering meter, measures scattering at 117 degrees. Provides analog or RS-232 serial output with 4000-count range. The housing is constructed from titanium and has a 6000m depth rating, operating effectively between temperatures of 0°C and 30°C.</skos:definition>
<owl:versionInfo>1</owl:versionInfo>
<dc:date>2009-11-30 11:56:35.0</dc:date>
<skos:note xml:lang="en">accepted</skos:note>
<owl:deprecated>false</owl:deprecated>
<skos:broader rdf:resource="http://vocab.nerc.ac.uk/collection/L05/current/123/"/>
<void:inDataset rdf:resource="http://vocab.nerc.ac.uk/.well-known/void"/>
</skos:Concept>
</skos:member>
<skos:member>
<skos:Concept rdf:about="http://vocab.nerc.ac.uk/collection/L22/current/TOOL0172/">
<dc:identifier>SDN:L22::TOOL0172</dc:identifier>
<skos:notation>SDN:L22::TOOL0172</skos:notation>
<skos:prefLabel xml:lang="en">WETLabs ECO FL fluorometer</skos:prefLabel>
<skos:altLabel>WETLabs ECO FL fluorometer</skos:altLabel>
<skos:definition xml:lang="en">An open flat-face fluorometer that can be used to measure relative chlorophyll, CDOM, uranine, phycocyanin, or phycoerythrin concentrations by directly measuring the amount of fluorescence emission in a sample volume of water.</skos:definition>
<owl:versionInfo>1</owl:versionInfo>
<dc:date>2010-05-18 16:10:58.0</dc:date>
<skos:note xml:lang="en">accepted</skos:note>
<owl:deprecated>false</owl:deprecated>
<skos:broader rdf:resource="http://vocab.nerc.ac.uk/collection/L05/current/113/"/>
<void:inDataset rdf:resource="http://vocab.nerc.ac.uk/.well-known/void"/>
</skos:Concept>
</skos:member>
<skos:member>
<skos:Concept rdf:about="http://vocab.nerc.ac.uk/collection/L22/current/TOOL0215/">
<dc:identifier>SDN:L22::TOOL0215</dc:identifier>
<skos:notation>SDN:L22::TOOL0215</skos:notation>
<skos:prefLabel xml:lang="en">WETLabs ECO-FLNTU combined fluorometer and turbidity sensor</skos:prefLabel>
<skos:altLabel>WETLabs fluorometer and turbidity sensor</skos:altLabel>
<skos:definition xml:lang="en">The ECO-FLNTU combines the ECO fluorometer with an optical scattering measurement at 700nm for simultaneous determination of turbidity. The fluorometer can typically measure phytoplankton concentrations in the range 0.01-50 ug/l, with a sensitivity of 0.01 ug/l. The turbidity sensor can measure within the range 0.01-25 NTU, with a sensitivity of 0.01 NTU. The instrument is stable over a temperature range of 0-20 degC and is rated to a depth of 600 m as standard, with the option of a 'deep' instrument rated to 6000m.</skos:definition>
<owl:versionInfo>2</owl:versionInfo>
<dc:date>2010-11-18 12:39:41.0</dc:date>
<skos:note xml:lang="en">accepted</skos:note>
<owl:deprecated>false</owl:deprecated>
<skos:broader rdf:resource="http://vocab.nerc.ac.uk/collection/L05/current/113/"/>
<skos:broader rdf:resource="http://vocab.nerc.ac.uk/collection/L05/current/123/"/>
<void:inDataset rdf:resource="http://vocab.nerc.ac.uk/.well-known/void"/>
</skos:Concept>
</skos:member>
<skos:member>
<skos:Concept rdf:about="http://vocab.nerc.ac.uk/collection/L22/current/TOOL0452/">
<dc:identifier>SDN:L22::TOOL0452</dc:identifier>
<skos:notation>SDN:L22::TOOL0452</skos:notation>
<skos:prefLabel xml:lang="en">WETLabs ECO-NTU(RT)D turbidity sensor</skos:prefLabel>
<skos:altLabel>WETLabs ECO-NTU(RT)D turbidity</skos:altLabel>
<skos:definition xml:lang="en">The ECO-NTU(RT)D uses optical scattering to measure turbidity over the range 0.02-125 NTU (nephelometric turbidity units), with a sensitivity of 0.02 NTU. The instrument is stable over a temperature range of 0-30 degC and is rated to a depth of 6000 m. This unit has an analog and RS-232 serial output, and operates continuously when power is supplied. Optional temperature and pressure sensors may be included.</skos:definition>
<owl:versionInfo>1</owl:versionInfo>
<dc:date>2012-01-10 13:45:04.0</dc:date>
<skos:note xml:lang="en">accepted</skos:note>
<owl:deprecated>false</owl:deprecated>
<skos:broader rdf:resource="http://vocab.nerc.ac.uk/collection/L05/current/123/"/>
<void:inDataset rdf:resource="http://vocab.nerc.ac.uk/.well-known/void"/>
</skos:Concept>
</skos:member>
<skos:member>
<skos:Concept rdf:about="http://vocab.nerc.ac.uk/collection/L22/current/TOOL0401/">
<dc:identifier>SDN:L22::TOOL0401</dc:identifier>
<skos:notation>SDN:L22::TOOL0401</skos:notation>
<skos:prefLabel xml:lang="en">WETLabs ECO-VSF Optical Backscatter Meter</skos:prefLabel>
<skos:altLabel>WETLabs ECO-VSF</skos:altLabel>
<skos:definition xml:lang="en">A three-angle optical backscatter meter, measuring scattering in water at 100, 125 and 150 deg for a wavelength of 470, 532 or 660 nm. It provides RS-232 serial output with 4000-count range, has a standard depth rating of 600 m and operates over the temperature range 0-30 degC. Optional extras include pressure and temperature sensors, internal data logging, internal batteries, anti-fouling capabilities and user-programmable sampling strategy.</skos:definition>
<owl:versionInfo>1</owl:versionInfo>
<dc:date>2011-06-13 15:07:47.0</dc:date>
<skos:note xml:lang="en">accepted</skos:note>
<owl:deprecated>false</owl:deprecated>
<skos:broader rdf:resource="http://vocab.nerc.ac.uk/collection/L05/current/123/"/>
<void:inDataset rdf:resource="http://vocab.nerc.ac.uk/.well-known/void"/>
</skos:Concept>
</skos:member>
<skos:member>
<skos:Concept rdf:about="http://vocab.nerc.ac.uk/collection/L22/current/TOOL0075/">
<dc:identifier>SDN:L22::TOOL0075</dc:identifier>
<skos:notation>SDN:L22::TOOL0075</skos:notation>
<skos:prefLabel xml:lang="en">WETLabs WETStar fluorometer</skos:prefLabel>
<skos:altLabel>WETStar fluorometer</skos:altLabel>
<skos:definition xml:lang="en">Submersible fluorometer designed for through-flow or pumped CTD applications manufactured by WetLabs and which can be configured for various types of fluorescence. The probe has a temperature range of 0-30°C and a depth rating of 600m.</skos:definition>
<owl:versionInfo>1</owl:versionInfo>
<dc:date>2009-11-30 11:56:35.0</dc:date>
<skos:note xml:lang="en">accepted</skos:note>
<owl:deprecated>false</owl:deprecated>
<skos:broader rdf:resource="http://vocab.nerc.ac.uk/collection/L05/current/113/"/>
<void:inDataset rdf:resource="http://vocab.nerc.ac.uk/.well-known/void"/>
</skos:Concept>
</skos:member>
<skos:member>
<skos:Concept rdf:about="http://vocab.nerc.ac.uk/collection/L22/current/TOOL0114/">
<dc:identifier>SDN:L22::TOOL0114</dc:identifier>
<skos:notation>SDN:L22::TOOL0114</skos:notation>
<skos:prefLabel xml:lang="en">WETLabs ac-3 Absorption and Attenuation meter</skos:prefLabel>
<skos:altLabel>WETLabs AC3</skos:altLabel>
<skos:definition xml:lang="en">Spectral transmittance and spectral absorption sensor measuring over three wavelengths (650, 676 and 715 nm). Available in 25 cm and also 10 cm pathlengths.</skos:definition>
<owl:versionInfo>3</owl:versionInfo>
<dc:date>2012-11-13 09:23:51.0</dc:date>
<skos:note xml:lang="en">accepted</skos:note>
<owl:deprecated>false</owl:deprecated>
<skos:broader rdf:resource="http://vocab.nerc.ac.uk/collection/L05/current/124/"/>
<void:inDataset rdf:resource="http://vocab.nerc.ac.uk/.well-known/void"/>
</skos:Concept>
</skos:member>
<skos:member>
<skos:Concept rdf:about="http://vocab.nerc.ac.uk/collection/L22/current/TOOL0402/">
<dc:identifier>SDN:L22::TOOL0402</dc:identifier>
<skos:notation>SDN:L22::TOOL0402</skos:notation>
<skos:prefLabel xml:lang="en">WETLabs ac-9 Absorption and Attenuation meter</skos:prefLabel>
<skos:altLabel>WETLabs ac-9</skos:altLabel>
<skos:definition xml:lang="en">Flow-through absorption and attenuation meter that measures absorption and attenuation coefficients in water over the spectral range 412-715 nm with an accuracy of +/- 0.01 m^-1. It has a standard path length of 25 cm (10 cm optional), a depth rating of either 500 ar 5000 m (with an optional pressure sensor), and operates over a temperature range of 0-30 degC.</skos:definition>
<owl:versionInfo>2</owl:versionInfo>
<dc:date>2012-11-13 09:24:06.0</dc:date>
<skos:note xml:lang="en">accepted</skos:note>
<owl:deprecated>false</owl:deprecated>
<skos:broader rdf:resource="http://vocab.nerc.ac.uk/collection/L05/current/124/"/>
<void:inDataset rdf:resource="http://vocab.nerc.ac.uk/.well-known/void"/>
</skos:Concept>
</skos:member>
<skos:member>
<skos:Concept rdf:about="http://vocab.nerc.ac.uk/collection/L22/current/TOOL0570/">
<dc:identifier>SDN:L22::TOOL0570</dc:identifier>
<skos:notation>SDN:L22::TOOL0570</skos:notation>
<skos:prefLabel xml:lang="en">WETLabs ac-9 plus Absorption and Attenuation meter</skos:prefLabel>
<skos:altLabel>WETLabs ac-9plus</skos:altLabel>
<skos:definition xml:lang="en">WETLabs ac-9 Plus is a flow-through absorption and attenuation meter that measures the absorption and attenuation coefficients of the water body over the spectral range 410-715 nm with an accuracy of +/- 0.01 m-1. It can be used with a pathlength of either 10 or 25 cm, a depth rating of 500 m and operates over a temperature range of 0 - 30 deg C. The ac-9 Plus is based on the earlier ac-9 model, but with the added capability of integrating data from ancillary sensors.</skos:definition>
<owl:versionInfo>1</owl:versionInfo>
<dc:date>2012-11-13 09:13:56.0</dc:date>
<skos:note xml:lang="en">accepted</skos:note>
<owl:deprecated>false</owl:deprecated>
<skos:broader rdf:resource="http://vocab.nerc.ac.uk/collection/L05/current/124/"/>
<void:inDataset rdf:resource="http://vocab.nerc.ac.uk/.well-known/void"/>
</skos:Concept>
</skos:member>
<skos:member>
<skos:Concept rdf:about="http://vocab.nerc.ac.uk/collection/L22/current/NETT0168/">
<dc:identifier>SDN:L22::NETT0168</dc:identifier>
<skos:notation>SDN:L22::NETT0168</skos:notation>
<skos:prefLabel xml:lang="en">WP2 net - Fraser (1966); UNESCO Working Party 2 (1968)</skos:prefLabel>
<skos:altLabel>WP2 net</skos:altLabel>
<skos:definition xml:lang="en">The net has a 57 cm diameter mouth opening (0.25 m2) cylinder (95 cm length)/cone (166 cm length) net made with nylon mesh (0.2 mm).  A flowmeter is mounted offset in the mouth. Designed for vertical hauls. A recommended standard net for collecting 0.2 mm to ~ 10 mm zooplankton [Wiebe and Benfield 2003 Plate 2 A].</skos:definition>
<owl:versionInfo>1</owl:versionInfo>
<dc:date>2011-10-21 14:18:49.0</dc:date>
<skos:note xml:lang="en">accepted</skos:note>
<owl:deprecated>false</owl:deprecated>
<skos:broader rdf:resource="http://vocab.nerc.ac.uk/collection/L05/current/22/"/>
<skos:broader rdf:resource="http://vocab.nerc.ac.uk/collection/L05/current/388/"/>
<void:inDataset rdf:resource="http://vocab.nerc.ac.uk/.well-known/void"/>
</skos:Concept>
</skos:member>
<skos:member>
<skos:Concept rdf:about="http://vocab.nerc.ac.uk/collection/L22/current/NETT0170/">
<dc:identifier>SDN:L22::NETT0170</dc:identifier>
<skos:notation>SDN:L22::NETT0170</skos:notation>
<skos:prefLabel xml:lang="en">WP3 net - UNESCO Working Party 3 (1968)</skos:prefLabel>
<skos:altLabel>WP3 net</skos:altLabel>
<skos:definition xml:lang="en">A non-closing net with a 1.13 m diameter mouth opening (1 m^2). The cylinder is 57 cm long and the cone is 200 cm long. It uses 1 mm nylon mesh as standard, although others may be used (e.g. 300 um).  The cod-end is a non-filtering canvas cylinder 12 cm in diameter by 12 cm in length. A flowmeter is mounted offset in the mouth.</skos:definition>
<owl:versionInfo>1</owl:versionInfo>
<dc:date>2011-12-05 11:41:22.0</dc:date>
<skos:note xml:lang="en">accepted</skos:note>
<owl:deprecated>false</owl:deprecated>
<skos:broader rdf:resource="http://vocab.nerc.ac.uk/collection/L05/current/22/"/>
<skos:broader rdf:resource="http://vocab.nerc.ac.uk/collection/L05/current/388/"/>
<void:inDataset rdf:resource="http://vocab.nerc.ac.uk/.well-known/void"/>
</skos:Concept>
</skos:member>
<skos:member>
<skos:Concept rdf:about="http://vocab.nerc.ac.uk/collection/L22/current/TOOL0235/">
<dc:identifier>SDN:L22::TOOL0235</dc:identifier>
<skos:notation>SDN:L22::TOOL0235</skos:notation>
<skos:prefLabel xml:lang="en">Water bottle</skos:prefLabel>
<skos:altLabel>Bottle</skos:altLabel>
<skos:definition xml:lang="en">A generic term for a device for the collection of a water sample from a pre-determined depth in a water body. The device is positioned at the desired depth where it is closed and sealed by some form of command from the surface.</skos:definition>
<owl:versionInfo>1</owl:versionInfo>
<dc:date>2010-05-18 16:10:58.0</dc:date>
<skos:note xml:lang="en">accepted</skos:note>
<owl:deprecated>false</owl:deprecated>
<skos:broader rdf:resource="http://vocab.nerc.ac.uk/collection/L05/current/30/"/>
<void:inDataset rdf:resource="http://vocab.nerc.ac.uk/.well-known/void"/>
</skos:Concept>
</skos:member>
<skos:member>
<skos:Concept rdf:about="http://vocab.nerc.ac.uk/collection/L22/current/TOOL0237/">
<dc:identifier>SDN:L22::TOOL0237</dc:identifier>
<skos:notation>SDN:L22::TOOL0237</skos:notation>
<skos:prefLabel xml:lang="en">Waterproof thermometer</skos:prefLabel>
<skos:altLabel>Thermometer</skos:altLabel>
<skos:definition xml:lang="en">A generic term for a temperature sensor capable of being immersed in water primarily intended to measure water body temperature but could also be used to determine temperature of other matrices.</skos:definition>
<owl:versionInfo>1</owl:versionInfo>
<dc:date>2010-05-18 16:10:58.0</dc:date>
<skos:note xml:lang="en">accepted</skos:note>
<owl:deprecated>false</owl:deprecated>
<skos:broader rdf:resource="http://vocab.nerc.ac.uk/collection/L05/current/134/"/>
<void:inDataset rdf:resource="http://vocab.nerc.ac.uk/.well-known/void"/>
</skos:Concept>
</skos:member>
<skos:member>
<skos:Concept rdf:about="http://vocab.nerc.ac.uk/collection/L22/current/TOOL0015/">
<dc:identifier>SDN:L22::TOOL0015</dc:identifier>
<skos:notation>SDN:L22::TOOL0015</skos:notation>
<skos:prefLabel xml:lang="en">Wellhead tide gauge</skos:prefLabel>
<skos:altLabel>Wellhead gauge</skos:altLabel>
<skos:definition xml:lang="en">The Wellhead gauge measures the sea level by means of a float in a stilling well. The float is usually of a smaller diameter than that used on a Munro gauge (about 45cm diameter), and has a counterweight attached to a smaller diameter pulley than that of the float so it is not immersed in the sea when the float rises. The Wellhead unit does not produce a chart but does give a readout of the height. It is interfaced to the data logger via a precision potentiometer.</skos:definition>
<owl:versionInfo>1</owl:versionInfo>
<dc:date>2009-11-30 11:27:51.0</dc:date>
<skos:note xml:lang="en">accepted</skos:note>
<owl:deprecated>false</owl:deprecated>
<skos:broader rdf:resource="http://vocab.nerc.ac.uk/collection/L05/current/111/"/>
<void:inDataset rdf:resource="http://vocab.nerc.ac.uk/.well-known/void"/>
</skos:Concept>
</skos:member>
<skos:member>
<skos:Concept rdf:about="http://vocab.nerc.ac.uk/collection/L22/current/TOOL0512/">
<dc:identifier>SDN:L22::TOOL0512</dc:identifier>
<skos:notation>SDN:L22::TOOL0512</skos:notation>
<skos:prefLabel xml:lang="en">WestCo Scientific Instruments SmartChem 200 Discrete Analyzer</skos:prefLabel>
<skos:altLabel>SmartChem 200 Discrete Analyzer</skos:altLabel>
<skos:definition xml:lang="en">A laboratory instrument designed for discrete sample analysis. A manual arm collects sample and reagents and dispenses them in a cuvette. The cuvette resides in a heated carousel wheel where the chemical reaction is allowed to proceed to the development of a colored product. The optical density of the reaction product is then measured. It may be used to measure nutrient concentrations in seawater. WestCo Scientific Instruments is a subsidiary of Unity Scientific.</skos:definition>
<owl:versionInfo>1</owl:versionInfo>
<dc:date>2012-07-04 10:02:10.0</dc:date>
<skos:note xml:lang="en">accepted</skos:note>
<owl:deprecated>false</owl:deprecated>
<skos:broader rdf:resource="http://vocab.nerc.ac.uk/collection/L05/current/LAB04/"/>
<void:inDataset rdf:resource="http://vocab.nerc.ac.uk/.well-known/void"/>
</skos:Concept>
</skos:member>
<skos:member>
<skos:Concept rdf:about="http://vocab.nerc.ac.uk/collection/L22/current/TOOL0537/">
<dc:identifier>SDN:L22::TOOL0537</dc:identifier>
<skos:notation>SDN:L22::TOOL0537</skos:notation>
<skos:prefLabel xml:lang="en">Winchester bottle</skos:prefLabel>
<skos:altLabel>Winchester bottle</skos:altLabel>
<skos:definition xml:lang="en">A strong, heavy bottle typically made of brown glass (to filter out UV light) but may also be made of plastics. A range of capacities is available. Also known as a Boston round bottle.</skos:definition>
<owl:versionInfo>1</owl:versionInfo>
<dc:date>2012-09-25 16:03:31.0</dc:date>
<skos:note xml:lang="en">accepted</skos:note>
<owl:deprecated>false</owl:deprecated>
<skos:broader rdf:resource="http://vocab.nerc.ac.uk/collection/L05/current/30/"/>
<void:inDataset rdf:resource="http://vocab.nerc.ac.uk/.well-known/void"/>
</skos:Concept>
</skos:member>
<skos:member>
<skos:Concept rdf:about="http://vocab.nerc.ac.uk/collection/L22/current/NETT0166/">
<dc:identifier>SDN:L22::NETT0166</dc:identifier>
<skos:notation>SDN:L22::NETT0166</skos:notation>
<skos:prefLabel xml:lang="en">Wishner Deep-Tow net system adapted for use on Alvin - Kim and Mullineaux (1998)</skos:prefLabel>
<skos:altLabel>Kim modified Deep-Tow net system</skos:altLabel>
<skos:definition xml:lang="en">Three rectangular mouth opening nets ~30 cm wide x 44 cm tall and 130 cm long mounted on a metal framework attached to the front instrument basket of DSRV Alvin. Sequential opening and closing of the nets done by the pilot using the manipulator arm.</skos:definition>
<owl:versionInfo>1</owl:versionInfo>
<dc:date>2011-10-21 14:18:49.0</dc:date>
<skos:note xml:lang="en">accepted</skos:note>
<owl:deprecated>false</owl:deprecated>
<skos:broader rdf:resource="http://vocab.nerc.ac.uk/collection/L05/current/22/"/>
<skos:broader rdf:resource="http://vocab.nerc.ac.uk/collection/L05/current/68/"/>
<void:inDataset rdf:resource="http://vocab.nerc.ac.uk/.well-known/void"/>
</skos:Concept>
</skos:member>
<skos:member>
<skos:Concept rdf:about="http://vocab.nerc.ac.uk/collection/L22/current/NETT0167/">
<dc:identifier>SDN:L22::NETT0167</dc:identifier>
<skos:notation>SDN:L22::NETT0167</skos:notation>
<skos:prefLabel xml:lang="en">Wollaston pop-down net - Buchanan-Wollaston (1911)</skos:prefLabel>
<skos:altLabel>Wollaston net</skos:altLabel>
<skos:definition xml:lang="en">A 55 cm net opening diameter 34 cm long made of canvas; 25 cm diameter conical section 68 cm long made of silk netting (no size given).  [Wiebe and Benfield 2003 Plate 10 B].</skos:definition>
<owl:versionInfo>1</owl:versionInfo>
<dc:date>2011-10-21 14:18:49.0</dc:date>
<skos:note xml:lang="en">accepted</skos:note>
<owl:deprecated>false</owl:deprecated>
<skos:broader rdf:resource="http://vocab.nerc.ac.uk/collection/L05/current/22/"/>
<void:inDataset rdf:resource="http://vocab.nerc.ac.uk/.well-known/void"/>
</skos:Concept>
</skos:member>
<skos:member>
<skos:Concept rdf:about="http://vocab.nerc.ac.uk/collection/L22/current/TOOL0604/">
<dc:identifier>SDN:L22::TOOL0604</dc:identifier>
<skos:notation>SDN:L22::TOOL0604</skos:notation>
<skos:prefLabel xml:lang="en">World Precision Instruments Liquid Waveguide Capillary Cell</skos:prefLabel>
<skos:altLabel>WPI LWCC</skos:altLabel>
<skos:definition xml:lang="en">Liquid Waveguide Capillary Cells (LWCC) are fiber optic cells that combine an increased optical pathlength (50–500 cm) with small sample volumes (125–1250 mL). They can be connected via optical fibers to a spectrophotometer with fiber optic capabilities. Ultra-sensitive absorbance measurements can be performed in the ultraviolet (UV), visible (VIS) and near-infrared (NIR) to detect low sample concentrations in a laboratory or process control environment.</skos:definition>
<owl:versionInfo>1</owl:versionInfo>
<dc:date>2013-03-14 11:39:02.0</dc:date>
<skos:note xml:lang="en">accepted</skos:note>
<owl:deprecated>false</owl:deprecated>
<skos:related rdf:resource="http://vocab.nerc.ac.uk/collection/P01/current/NTRZLWTX/"/>
<skos:related rdf:resource="http://vocab.nerc.ac.uk/collection/P01/current/AMONNATX/"/>
<skos:related rdf:resource="http://vocab.nerc.ac.uk/collection/P01/current/PHOSLWTX/"/>
<skos:related rdf:resource="http://vocab.nerc.ac.uk/collection/P01/current/NTRILWTX/"/>
<skos:broader rdf:resource="http://vocab.nerc.ac.uk/collection/L05/current/LAB20/"/>
<void:inDataset rdf:resource="http://vocab.nerc.ac.uk/.well-known/void"/>
</skos:Concept>
</skos:member>
<skos:member>
<skos:Concept rdf:about="http://vocab.nerc.ac.uk/collection/L22/current/TOOL0460/">
<dc:identifier>SDN:L22::TOOL0460</dc:identifier>
<skos:notation>SDN:L22::TOOL0460</skos:notation>
<skos:prefLabel xml:lang="en">World Precision Instruments UltraPath Ultraviolet spectrophotometer</skos:prefLabel>
<skos:altLabel>UPUV spectrophotometer</skos:altLabel>
<skos:definition xml:lang="en">A high performance spectrophotometer that measures absorbance of UV light over the range 250-730 nm with a resolution of 5 nm. It is designed to detect low absorbing substances in solution. The instrument uses a deuterium/tungsten light source with a user-selectable optical path length of 2, 10, 50 or 500 cm. The UltraPath system typically includes a Tidas I spectrometer module, a fibre optic light source, fibre optic cables and a Peri-Star Pro peristaltic pump. A sample is drawn into the sample cell by the peristaltic pump and absorbance of the solution at the selected path length is measured. Individual samples are separated by air bubbles, thereby minimizing cross-contamination.</skos:definition>
<owl:versionInfo>1</owl:versionInfo>
<dc:date>2012-02-16 10:05:14.0</dc:date>
<skos:note xml:lang="en">accepted</skos:note>
<owl:deprecated>false</owl:deprecated>
<skos:broader rdf:resource="http://vocab.nerc.ac.uk/collection/L05/current/LAB20/"/>
<void:inDataset rdf:resource="http://vocab.nerc.ac.uk/.well-known/void"/>
</skos:Concept>
</skos:member>
<skos:member>
<skos:Concept rdf:about="http://vocab.nerc.ac.uk/collection/L22/current/TOOL0549/">
<dc:identifier>SDN:L22::TOOL0549</dc:identifier>
<skos:notation>SDN:L22::TOOL0549</skos:notation>
<skos:prefLabel xml:lang="en">YSI Model 57 Dissolved Oxygen Meter</skos:prefLabel>
<skos:altLabel>YSI Dissolved oxygen 57</skos:altLabel>
<skos:definition xml:lang="en">A field instrument designed for measurement of dissolved oxygen and temperature in water. It comprises a submersible probe and a battery-powered meter. The probe incorporates Clark-type membrane covered polarographic sensors with built in thermistors for temperature measurement and compensation. Available oxygen measurement ranges are 0-5, 0-10 and 0-20 mg/l, with an accuracy of +/- 1% of full scale at calibration temperature or 0.1 mg/l, whichever is larger. The temperature range is -5 to 45 degC, with an accuracy of +/- 0.5 degC.</skos:definition>
<owl:versionInfo>2</owl:versionInfo>
<dc:date>2012-11-15 12:23:13.0</dc:date>
<skos:note xml:lang="en">accepted</skos:note>
<owl:deprecated>false</owl:deprecated>
<skos:broader rdf:resource="http://vocab.nerc.ac.uk/collection/L05/current/351/"/>
<skos:broader rdf:resource="http://vocab.nerc.ac.uk/collection/L05/current/134/"/>
<void:inDataset rdf:resource="http://vocab.nerc.ac.uk/.well-known/void"/>
</skos:Concept>
</skos:member>
<skos:member>
<skos:Concept rdf:about="http://vocab.nerc.ac.uk/collection/L22/current/TOOL0220/">
<dc:identifier>SDN:L22::TOOL0220</dc:identifier>
<skos:notation>SDN:L22::TOOL0220</skos:notation>
<skos:prefLabel xml:lang="en">Young 05305 Wind Monitor-AQ anemometer</skos:prefLabel>
<skos:altLabel>Young 05305 anemometer</skos:altLabel>
<skos:definition xml:lang="en">An anemometer with a lightweight, carbon fibre thermoplastic (CFT), helicoid propeller wind sensor designed for air quality applications. The wind direction sensor is a lightweight, balanced vane. The instrument body is UV stabilized plastic with stainless steel and anodized aluminum fittings. The instrument mounts on standard 1 inch pipe. Winspeed accuracy is +-0.2m/s and wind direction accuracy is 3 degrees.</skos:definition>
<owl:versionInfo>1</owl:versionInfo>
<dc:date>2010-05-18 16:10:58.0</dc:date>
<skos:note xml:lang="en">accepted</skos:note>
<owl:deprecated>false</owl:deprecated>
<skos:broader rdf:resource="http://vocab.nerc.ac.uk/collection/L05/current/101/"/>
<void:inDataset rdf:resource="http://vocab.nerc.ac.uk/.well-known/void"/>
</skos:Concept>
</skos:member>
<skos:member>
<skos:Concept rdf:about="http://vocab.nerc.ac.uk/collection/L22/current/TOOL0648/">
<dc:identifier>SDN:L22::TOOL0648</dc:identifier>
<skos:notation>SDN:L22::TOOL0648</skos:notation>
<skos:prefLabel xml:lang="en">Young 522 series Tipping Bucket Raingauge</skos:prefLabel>
<skos:altLabel>522 series Tipping Bucket Raingauge</skos:altLabel>
<skos:definition xml:lang="en">A series comprising two tipping bucket raingauges, the 52202 (heated) and 52203 (unheated). They both have a catchment area of 200 cm2 and a resolution of 0.1 mm per tip. The accuracy is 2 percent up to 25 mm/hour, 3 percent up to 50 mm/hour. This instrument is marketed by Campbell Scientific.</skos:definition>
<owl:versionInfo>1</owl:versionInfo>
<dc:date>2013-09-30 14:23:03.0</dc:date>
<skos:note xml:lang="en">accepted</skos:note>
<owl:deprecated>false</owl:deprecated>
<skos:broader rdf:resource="http://vocab.nerc.ac.uk/collection/L05/current/14/"/>
<void:inDataset rdf:resource="http://vocab.nerc.ac.uk/.well-known/void"/>
</skos:Concept>
</skos:member>
<skos:member>
<skos:Concept rdf:about="http://vocab.nerc.ac.uk/collection/L22/current/TOOL0260/">
<dc:identifier>SDN:L22::TOOL0260</dc:identifier>
<skos:notation>SDN:L22::TOOL0260</skos:notation>
<skos:prefLabel xml:lang="en">Young MA05103 Wind Monitor anemometer</skos:prefLabel>
<skos:altLabel>Young MA05103 anemometer</skos:altLabel>
<skos:definition xml:lang="en">An anemometer with a four blade helicoid propeller and lightweight direction vane. Vane angle is sensed by a precision potentiometer. The instrument body is UV stabilized plastic with stainless steel and anodized aluminum fittings. The instrument mounts on standard 1 inch pipe. Windspeed accuracy is +-0.3m/s and wind direction accuracy is 3 degrees..</skos:definition>
<owl:versionInfo>1</owl:versionInfo>
<dc:date>2010-05-18 16:10:58.0</dc:date>
<skos:note xml:lang="en">accepted</skos:note>
<owl:deprecated>false</owl:deprecated>
<skos:broader rdf:resource="http://vocab.nerc.ac.uk/collection/L05/current/101/"/>
<void:inDataset rdf:resource="http://vocab.nerc.ac.uk/.well-known/void"/>
</skos:Concept>
</skos:member>
<skos:member>
<skos:Concept rdf:about="http://vocab.nerc.ac.uk/collection/L22/current/TOOL0195/">
<dc:identifier>SDN:L22::TOOL0195</dc:identifier>
<skos:notation>SDN:L22::TOOL0195</skos:notation>
<skos:prefLabel xml:lang="en">Young MA05106 Wind Monitor anemometer</skos:prefLabel>
<skos:altLabel>Young MA05106 anemometer</skos:altLabel>
<skos:definition xml:lang="en">A lightweight anemometer with a helicoid propellor speed sensor attached to a vane. The instrument is designed to withstand the marine environment.</skos:definition>
<owl:versionInfo>1</owl:versionInfo>
<dc:date>2010-05-18 16:10:58.0</dc:date>
<skos:note xml:lang="en">accepted</skos:note>
<owl:deprecated>false</owl:deprecated>
<skos:broader rdf:resource="http://vocab.nerc.ac.uk/collection/L05/current/101/"/>
<void:inDataset rdf:resource="http://vocab.nerc.ac.uk/.well-known/void"/>
</skos:Concept>
</skos:member>
<skos:member>
<skos:Concept rdf:about="http://vocab.nerc.ac.uk/collection/L22/current/TOOL0451/">
<dc:identifier>SDN:L22::TOOL0451</dc:identifier>
<skos:notation>SDN:L22::TOOL0451</skos:notation>
<skos:prefLabel xml:lang="en">Zullig Hydropolytester profiler</skos:prefLabel>
<skos:altLabel>Zullig Hydropolytester profiler</skos:altLabel>
<skos:definition xml:lang="en">Profiling package for measurement of water properties. The unit includes pressure, temperature, conductivity, pH, dissolved oxygen and optical backscatter sensors. The system is no longer in production and no source of support is known.</skos:definition>
<owl:versionInfo>1</owl:versionInfo>
<dc:date>2012-01-10 13:45:04.0</dc:date>
<skos:note xml:lang="en">accepted</skos:note>
<owl:deprecated>false</owl:deprecated>
<skos:related rdf:resource="http://vocab.nerc.ac.uk/collection/P01/current/SIGTPR01/"/>
<skos:related rdf:resource="http://vocab.nerc.ac.uk/collection/P01/current/PSALST01/"/>
<skos:related rdf:resource="http://vocab.nerc.ac.uk/collection/P01/current/TEMPST01/"/>
<skos:related rdf:resource="http://vocab.nerc.ac.uk/collection/P01/current/PRESPR01/"/>
<skos:related rdf:resource="http://vocab.nerc.ac.uk/collection/P01/current/POTMCV01/"/>
<skos:broader rdf:resource="http://vocab.nerc.ac.uk/collection/L05/current/130/"/>
<skos:broader rdf:resource="http://vocab.nerc.ac.uk/collection/L05/current/134/"/>
<skos:broader rdf:resource="http://vocab.nerc.ac.uk/collection/L05/current/351/"/>
<skos:broader rdf:resource="http://vocab.nerc.ac.uk/collection/L05/current/350/"/>
<skos:broader rdf:resource="http://vocab.nerc.ac.uk/collection/L05/current/123/"/>
<skos:broader rdf:resource="http://vocab.nerc.ac.uk/collection/L05/current/355/"/>
<void:inDataset rdf:resource="http://vocab.nerc.ac.uk/.well-known/void"/>
</skos:Concept>
</skos:member>
<skos:member>
<skos:Concept rdf:about="http://vocab.nerc.ac.uk/collection/L22/current/TOOL0269/">
<dc:identifier>SDN:L22::TOOL0269</dc:identifier>
<skos:notation>SDN:L22::TOOL0269</skos:notation>
<skos:prefLabel xml:lang="en">anemometer</skos:prefLabel>
<skos:altLabel>anemometer</skos:altLabel>
<skos:definition xml:lang="en">A generic term for a mechanical device for measuring wind speed and direction designed for use where no information on instrument make, model or measurement principle are obtainable.</skos:definition>
<owl:versionInfo>1</owl:versionInfo>
<dc:date>2010-05-18 16:10:58.0</dc:date>
<skos:note xml:lang="en">accepted</skos:note>
<owl:deprecated>false</owl:deprecated>
<skos:broader rdf:resource="http://vocab.nerc.ac.uk/collection/L05/current/101/"/>
<void:inDataset rdf:resource="http://vocab.nerc.ac.uk/.well-known/void"/>
</skos:Concept>
</skos:member>
<skos:member>
<skos:Concept rdf:about="http://vocab.nerc.ac.uk/collection/L22/current/TOOLZZZ/">
<dc:identifier>SDN:L22::TOOLZZZ</dc:identifier>
<skos:notation>SDN:L22::TOOLZZZ</skos:notation>
<skos:prefLabel xml:lang="en">unknown</skos:prefLabel>
<skos:altLabel>unknown</skos:altLabel>
<skos:definition xml:lang="en">The correct value is not known to, and not computable by, the creator of this information. However, a correct value probably exists.</skos:definition>
<owl:versionInfo>1</owl:versionInfo>
<dc:date>2009-11-26 12:14:36.0</dc:date>
<skos:note xml:lang="en">accepted</skos:note>
<owl:deprecated>false</owl:deprecated>
<owl:sameAs rdf:resource="http://vocab.nerc.ac.uk/collection/L05/current/999/"/>
<void:inDataset rdf:resource="http://vocab.nerc.ac.uk/.well-known/void"/>
</skos:Concept>
</skos:member>
</skos:Collection>
</rdf:RDF>
